@prefix adms:  <http://www.w3.org/ns/adms#> .
@prefix dc:    <http://purl.org/dc/elements/1.1/> .
@prefix comm:  <http://vocab.resc.info/communication#> .
@prefix rdfs:  <http://www.w3.org/2000/01/rdf-schema#> .
@prefix foaf:  <http://xmlns.com/foaf/0.1/> .
@prefix owl:   <http://www.w3.org/2002/07/owl#> .
@prefix xsd:   <http://www.w3.org/2001/XMLSchema#> .
@prefix rdf:   <http://www.w3.org/1999/02/22-rdf-syntax-ns#> .
@prefix vann:  <http://purl.org/vocab/vann/> .
@prefix dcterms: <http://purl.org/dc/terms/> .

comm:DispatchMessage  a  owl:Class , rdfs:Class ;
        rdfs:comment     "Resources of this class describe messages sent by a dispatch to individual units" ;
        rdfs:label       "DispatchMessage" ;
        rdfs:subClassOf  rdfs:Class .

comm:pagerMessage  a  rdf:Property ;
        rdfs:comment  "This property contains the full message as send through pager networks" ;
        rdfs:label    "The message send to pagers" .

comm:Unit  a             owl:Class , rdfs:Class ;
        rdfs:comment     "A Unit which can be send to a incident" ;
        rdfs:label       "Unit" ;
        rdfs:subClassOf  rdfs:Resource .

comm:rdf  a                 adms:AssetDistribution ;
        dcterms:FileFormat  <http://vocab.resc.info/communication> ;
        adms:status         <http://purl.org/adms/status/Completed> .

<http://vocab.resc.info/communication>
        a                              owl:Ontology , adms:Asset ;
        dc:creator                     comm:bart ;
        dcterms:created                "2014-05-05"^^xsd:date ;
        dcterms:description            "This vocabulary is intended to describe all the aspects which are needed to communicate incident related information for fire department services" ;
        dcterms:isPartOf               <http://vocab.resc.info> ;
        dcterms:modified               "2014-09-12"^^xsd:date ;
        dcterms:title                  "Vocabulary related to incident communication" ;
        dcterms:type                   <http://purl.org/adms/assettype/Ontology> ;
        vann:preferredNamespacePrefix  "comm" ;
        vann:preferredNamespaceUri     "http://vocab.resc.info/communication#" ;
        adms:status                    <http://purl.org/adms/status/UnderDevelopment> ;
        foaf:homepage                  <http://vocab.resc.info/communication.html> .

comm:incidentLocation
        a             rdf:Property ;
        rdfs:comment  "The location in geo format where incident is reported" ;
        rdfs:domain   comm:DispatchMessage ;
        rdfs:label    "Location" .

comm:classificationType
        a             owl:DatatypeProperty , rdf:Property ;
        rdfs:comment  "The type of classification" ;
        rdfs:domain   comm:Classification ;
        rdfs:label    "Type" ;
        rdfs:range    rdfs:Literal .

comm:Classification  a   owl:Class , rdfs:Class ;
        rdfs:comment     "The classification of the incident" ;
        rdfs:label       "Classification" ;
        rdfs:subClassOf  rdfs:Class .

comm:bart  a       foaf:Person ;
        foaf:nick  "bart" .

comm:unit  a          rdf:Property ;
        rdfs:comment  "Unit sent to the incident" ;
        rdfs:domain   comm:DispatchMessage ;
        rdfs:label    "Unit" ;
        rdfs:range    comm:Unit .

comm:incidentAddress  a  rdf:Property ;
        rdfs:comment  "The address where the incident was reported" ;
        rdfs:domain   comm:DispatchMessage ;
        rdfs:label    "Incident address" .

comm:dispatchedTo  a  rdf:Property ;
        rdfs:comment  "the adress on the P2000 pager network where the message was sent to" ;
        rdfs:domain   comm:DispatchMessage ;
        rdfs:label    "Dispatched to" .

comm:ttl  a                 adms:AssetDistribution ;
        dcterms:FileFormat  <http://vocab.resc.info/communication> ;
        adms:status         <http://purl.org/adms/status/Completed> .
