@prefix dc: <http://purl.org/dc/elements/1.1/> .
@prefix onto: <http://www.ontotext.com/> .
@prefix result: <http://purl.org/ontology/rdf-result/> .
@prefix news: <http://www.bbc.co.uk/ontologies/news/> .
@prefix tagging: <http://www.bbc.co.uk/ontologies/tagging/> .
@prefix cms: <http://www.bbc.co.uk/ontologies/cms/> .
@prefix sport: <http://www.bbc.co.uk/ontologies/sport/> .
@prefix biz: <http://www.bbc.co.uk/ontologies/business/> .
@prefix bbc: <http://www.bbc.co.uk/ontologies/bbc/> .
@prefix dcterms: <http://purl.org/dc/terms/> .
@prefix provenance: <http://www.bbc.co.uk/ontologies/provenance/> .
@prefix rdfs: <http://www.w3.org/2000/01/rdf-schema#> .
@prefix pol: <http://www.bbc.co.uk/ontologies/politics/> .
@prefix owl: <http://www.w3.org/2002/07/owl#> .
@prefix xsd: <http://www.w3.org/2001/XMLSchema#> .
@prefix rdf: <http://www.w3.org/1999/02/22-rdf-syntax-ns#> .
@prefix core: <http://www.bbc.co.uk/ontologies/coreconcepts/> .
@prefix sesame: <http://www.openrdf.org/schema/sesame#> .
@prefix fn: <http://www.w3.org/2005/xpath-functions#> .
@prefix cwork: <http://www.bbc.co.uk/ontologies/creativework/> .
@prefix nsl: <http://purl.org/ontology/storyline/> .

sport:division a rdf:Property .

sport:subDisciplineOf a owl:TransitiveProperty .

<http://www.bbc.co.uk/ontologies/sport> a owl:Ontology .

sport:CompetesForRole a owl:Class .

sport:MedalCompetition a owl:Class .

sport:RoundType a owl:Class .

sport:Session a owl:Class .

sport:Competition a owl:Class .

sport:RecurringCompetition a owl:Class .

sport:CompetitiveSportingOrganisation a owl:Class .

sport:SportingOrganisation a owl:Class .

sport:SportsDiscipline a owl:Class .

sport:DivisionalCompetition a owl:Class .

sport:EventGender a owl:Class .

sport:GroupCompetition a owl:Class .

sport:MultiRoundCompetition a owl:Class .

sport:KnockoutCompetition a owl:Class .

sport:LeagueCompetition a owl:Class .

sport:Match a owl:Class .

sport:UnitCompetition a owl:Class .

sport:MultiStageCompetition a owl:Class .

sport:Person a owl:Class .

sport:Round a owl:Class .

sport:CompetitiveSportingGroup a owl:Class .

sport:CompetitionType a owl:Class .

sport:MultiDisciplineRecurringCompetition a owl:Class .

sport:Home a owl:Class .

sport:Venue a owl:Class .

sport:MultiDisciplineCompetition a owl:Class .

sport:GoverningBody a owl:Class .

<http://www.bbc.co.uk/things/event-gender/womens> a sport:EventGender .

<http://www.bbc.co.uk/things/event-gender/mens> a sport:EventGender .

<http://www.bbc.co.uk/things/event-gender/mixed> a sport:EventGender .

<http://www.bbc.co.uk/things/competition-types/domestic-league> a sport:CompetitionType .

<http://www.bbc.co.uk/things/competition-types/domestic-cup> a sport:CompetitionType .

<http://www.bbc.co.uk/things/competition-types/european-cup> a sport:CompetitionType .

<http://www.bbc.co.uk/things/competition-types/international> a sport:CompetitionType .

<http://www.bbc.co.uk/things/competition-types/domestic-league-womens> a sport:CompetitionType .

<http://www.bbc.co.uk/things/competition-types/domestic-cup-womens> a sport:CompetitionType .

<http://www.bbc.co.uk/things/competition-types/domestic> a sport:CompetitionType .

<http://www.bbc.co.uk/things/competition-types/club-league> a sport:CompetitionType .

<http://www.bbc.co.uk/things/competition-types/club-cup> a sport:CompetitionType .

<http://www.bbc.co.uk/things/competition-types/international-groupcup> a sport:CompetitionType .

<http://www.bbc.co.uk/things/competition-types/international-cup-womens> a sport:CompetitionType .

<http://www.bbc.co.uk/things/competition-types/international-group-womens> a sport:CompetitionType .

<http://www.bbc.co.uk/things/competition-types/international-cup> a sport:CompetitionType .

<http://www.bbc.co.uk/things/competition-types/international-group> a sport:CompetitionType .

<http://www.bbc.co.uk/things/competition-types/club-groupcup> a sport:CompetitionType .

<http://www.bbc.co.uk/things/competition-types/club-groupcup-womens> a sport:CompetitionType .

<http://www.bbc.co.uk/things/competition-types/international-groupcup-womens> a sport:CompetitionType .

sport:awayCompetitor a owl:ObjectProperty .

sport:firstRound a owl:ObjectProperty .

sport:firstStage a owl:ObjectProperty .

sport:isGroupOf a owl:ObjectProperty .

sport:isCompetitiveSportingOrganisationOf a owl:ObjectProperty .

sport:homeCompetitor a owl:ObjectProperty .

sport:lastRound a owl:ObjectProperty .

sport:lastStage a owl:ObjectProperty .

sport:nextRound a owl:ObjectProperty .

sport:nextStage a owl:ObjectProperty .

sport:prevRound a owl:ObjectProperty .

sport:prevStage a owl:ObjectProperty .

sport:hasSession a owl:ObjectProperty .

sport:roundType a owl:ObjectProperty .

sport:competesIn a owl:ObjectProperty .

sport:hasRound a owl:ObjectProperty .

sport:hasStage a owl:ObjectProperty .

sport:flagImage a owl:ObjectProperty .

sport:hasGroup a owl:ObjectProperty .

sport:hasMatch a owl:ObjectProperty .

sport:hasUnitCompetition a owl:ObjectProperty .

sport:discipline a owl:ObjectProperty .

sport:subDiscipline a owl:ObjectProperty .

sport:eventGender a owl:ObjectProperty .

sport:competitionType a owl:ObjectProperty .

sport:hasDivision a owl:ObjectProperty .

sport:promotesTo a owl:ObjectProperty .

sport:relegatesTo a owl:ObjectProperty .

sport:recurringCompetition a owl:ObjectProperty .

sport:hasHome a owl:ObjectProperty .

sport:subDisciplineOf a owl:ObjectProperty .

sport:firstUnitCompetition a owl:ObjectProperty .

sport:isRoundOf a owl:ObjectProperty .

sport:prevUnitCompetition a owl:ObjectProperty .

sport:hasCompetitor a owl:ObjectProperty .

sport:prevSession a owl:ObjectProperty .

sport:lastUnitCompetition a owl:ObjectProperty .

sport:nextUnitCompetition a owl:ObjectProperty .

sport:isSessionOf a owl:ObjectProperty .

sport:hasCompetedFor a owl:ObjectProperty .

sport:nextSession a owl:ObjectProperty .

sport:lastSession a owl:ObjectProperty .

sport:firstSession a owl:ObjectProperty .

sport:isMatchOf a owl:ObjectProperty .

sport:isStageOf a owl:ObjectProperty .

sport:dateOfBirth a owl:AnnotationProperty , owl:DatatypeProperty .

sport:roundNumber a owl:DatatypeProperty .

<http://www.bbc.co.uk/ontologies/sport> a provenance:Ontology .

sport:lastSession rdfs:subPropertyOf sport:hasSession .

sport:firstSession rdfs:subPropertyOf sport:hasSession .

sport:competesIn rdfs:subPropertyOf <http://purl.org/NET/c4dm/event.owl#agent_in> .

sport:firstRound rdfs:subPropertyOf sport:hasRound .

sport:lastRound rdfs:subPropertyOf sport:hasRound .

sport:firstStage rdfs:subPropertyOf sport:hasStage .

sport:lastStage rdfs:subPropertyOf sport:hasStage .

sport:hasMatch rdfs:subPropertyOf sport:hasUnitCompetition .

sport:firstUnitCompetition rdfs:subPropertyOf sport:hasUnitCompetition .

sport:lastUnitCompetition rdfs:subPropertyOf sport:hasUnitCompetition .

sport:homeCompetitor rdfs:subPropertyOf sport:hasCompetitor .

sport:Person rdfs:subClassOf <http://xmlns.com/foaf/0.1/Person> .

sport:SportingOrganisation rdfs:subClassOf <http://xmlns.com/foaf/0.1/Organization> .

sport:CompetitiveSportingGroup rdfs:subClassOf <http://xmlns.com/foaf/0.1/Group> .

sport:Competition rdfs:subClassOf <http://purl.org/NET/c4dm/event.owl#Event> .

sport:MedalCompetition rdfs:subClassOf sport:Competition .

sport:Session rdfs:subClassOf sport:Competition .

sport:DivisionalCompetition rdfs:subClassOf sport:Competition .

sport:MultiRoundCompetition rdfs:subClassOf sport:Competition .

sport:UnitCompetition rdfs:subClassOf sport:Competition .

sport:MultiStageCompetition rdfs:subClassOf sport:Competition .

sport:Round rdfs:subClassOf sport:Competition .

sport:MultiDisciplineCompetition rdfs:subClassOf sport:Competition .

sport:CompetitiveSportingOrganisation rdfs:subClassOf sport:SportingOrganisation .

sport:GoverningBody rdfs:subClassOf sport:SportingOrganisation .

sport:GroupCompetition rdfs:subClassOf sport:MultiRoundCompetition .

sport:KnockoutCompetition rdfs:subClassOf sport:MultiRoundCompetition .

sport:LeagueCompetition rdfs:subClassOf sport:MultiRoundCompetition .

sport:Match rdfs:subClassOf sport:UnitCompetition .

sport:Person rdfs:subClassOf core:Person .

sport:prevSession rdfs:domain sport:Session .

sport:isSessionOf rdfs:domain sport:Session .

sport:nextSession rdfs:domain sport:Session .

sport:competesIn rdfs:domain <http://xmlns.com/foaf/0.1/Agent> .

sport:hasCompetedFor rdfs:domain <http://xmlns.com/foaf/0.1/Agent> .

sport:nextStage rdfs:domain sport:Competition .

sport:prevStage rdfs:domain sport:Competition .

sport:hasSession rdfs:domain sport:Competition .

sport:eventGender rdfs:domain sport:Competition .

sport:competitionType rdfs:domain sport:Competition .

sport:promotesTo rdfs:domain sport:Competition .

sport:relegatesTo rdfs:domain sport:Competition .

sport:recurringCompetition rdfs:domain sport:Competition .

sport:firstUnitCompetition rdfs:domain sport:Competition .

sport:hasCompetitor rdfs:domain sport:Competition .

sport:lastUnitCompetition rdfs:domain sport:Competition .

sport:lastSession rdfs:domain sport:Competition .

sport:firstSession rdfs:domain sport:Competition .

sport:isStageOf rdfs:domain sport:Competition .

sport:hasHome rdfs:domain sport:CompetitiveSportingOrganisation .

sport:subDiscipline rdfs:domain sport:SportsDiscipline .

sport:subDisciplineOf rdfs:domain sport:SportsDiscipline .

sport:division rdfs:domain sport:DivisionalCompetition .

sport:hasDivision rdfs:domain sport:DivisionalCompetition .

sport:isGroupOf rdfs:domain sport:GroupCompetition .

sport:firstRound rdfs:domain sport:MultiRoundCompetition .

sport:lastRound rdfs:domain sport:MultiRoundCompetition .

sport:hasRound rdfs:domain sport:MultiRoundCompetition .

sport:hasGroup rdfs:domain sport:LeagueCompetition .

sport:awayCompetitor rdfs:domain sport:Match .

sport:homeCompetitor rdfs:domain sport:Match .

sport:isMatchOf rdfs:domain sport:Match .

sport:prevUnitCompetition rdfs:domain sport:UnitCompetition .

sport:nextUnitCompetition rdfs:domain sport:UnitCompetition .

sport:firstStage rdfs:domain sport:MultiStageCompetition .

sport:lastStage rdfs:domain sport:MultiStageCompetition .

sport:hasStage rdfs:domain sport:MultiStageCompetition .

sport:dateOfBirth rdfs:domain sport:Person .

sport:nextRound rdfs:domain sport:Round .

sport:prevRound rdfs:domain sport:Round .

sport:roundType rdfs:domain sport:Round .

sport:hasMatch rdfs:domain sport:Round .

sport:hasUnitCompetition rdfs:domain sport:Round .

sport:roundNumber rdfs:domain sport:Round .

sport:isRoundOf rdfs:domain sport:Round .

sport:isCompetitiveSportingOrganisationOf rdfs:domain sport:CompetitiveSportingGroup .

sport:flagImage rdfs:domain sport:CompetitiveSportingGroup .

sport:roundType rdfs:range sport:RoundType .

sport:hasSession rdfs:range sport:Session .

sport:prevSession rdfs:range sport:Session .

sport:nextSession rdfs:range sport:Session .

sport:lastSession rdfs:range sport:Session .

sport:firstSession rdfs:range sport:Session .

sport:awayCompetitor rdfs:range <http://xmlns.com/foaf/0.1/Agent> .

sport:homeCompetitor rdfs:range <http://xmlns.com/foaf/0.1/Agent> .

sport:hasCompetitor rdfs:range <http://xmlns.com/foaf/0.1/Agent> .

sport:division rdfs:range sport:Competition .

sport:firstStage rdfs:range sport:Competition .

sport:lastStage rdfs:range sport:Competition .

sport:nextStage rdfs:range sport:Competition .

sport:prevStage rdfs:range sport:Competition .

sport:competesIn rdfs:range sport:Competition .

sport:hasStage rdfs:range sport:Competition .

sport:hasDivision rdfs:range sport:Competition .

sport:promotesTo rdfs:range sport:Competition .

sport:relegatesTo rdfs:range sport:Competition .

sport:isSessionOf rdfs:range sport:Competition .

sport:recurringCompetition rdfs:range sport:RecurringCompetition .

sport:isCompetitiveSportingOrganisationOf rdfs:range sport:CompetitiveSportingOrganisation .

sport:hasCompetedFor rdfs:range sport:SportingOrganisation .

sport:discipline rdfs:range sport:SportsDiscipline .

sport:subDiscipline rdfs:range sport:SportsDiscipline .

sport:subDisciplineOf rdfs:range sport:SportsDiscipline .

sport:eventGender rdfs:range sport:EventGender .

sport:hasGroup rdfs:range sport:GroupCompetition .

sport:isRoundOf rdfs:range sport:MultiRoundCompetition .

sport:isGroupOf rdfs:range sport:LeagueCompetition .

sport:hasMatch rdfs:range sport:Match .

sport:hasUnitCompetition rdfs:range sport:UnitCompetition .

sport:firstUnitCompetition rdfs:range sport:UnitCompetition .

sport:prevUnitCompetition rdfs:range sport:UnitCompetition .

sport:lastUnitCompetition rdfs:range sport:UnitCompetition .

sport:nextUnitCompetition rdfs:range sport:UnitCompetition .

sport:isStageOf rdfs:range sport:MultiStageCompetition .

sport:firstRound rdfs:range sport:Round .

sport:lastRound rdfs:range sport:Round .

sport:nextRound rdfs:range sport:Round .

sport:prevRound rdfs:range sport:Round .

sport:hasRound rdfs:range sport:Round .

sport:isMatchOf rdfs:range sport:Round .

sport:competitionType rdfs:range sport:CompetitionType .

sport:roundNumber rdfs:range xsd:int .

sport:dateOfBirth rdfs:range xsd:date .

sport:flagImage rdfs:range <http://www.bbc.co.uk/ontologies/asset/FlagImage> .

sport:hasHome rdfs:range sport:Home .

sport:hasGroup owl:inverseOf sport:isGroupOf .

sport:isSessionOf owl:inverseOf sport:hasSession .

sport:isRoundOf owl:inverseOf sport:hasRound .

sport:isStageOf owl:inverseOf sport:hasStage .

sport:isMatchOf owl:inverseOf sport:hasMatch .

sport:relegatesTo owl:inverseOf sport:promotesTo .

sport:promotesTo owl:inverseOf sport:relegatesTo .

sport:hasStage rdfs:comment "Relates a multi-stage competition to a stage that it contains."@en-gb .

sport:isCompetitiveSportingOrganisationOf rdfs:comment "Relates a competitive sporting organisation to a competitive sporting group."@en-gb .

sport:Session rdfs:comment "A sub-division of a competition, that must be broken up due to the duration of that competition, occurring for example in snooker or cricket."@en-gb .

sport:hasSession rdfs:comment "Relates a competition to a session within that competition."@en-gb .

sport:DivisionalCompetition rdfs:comment "A Divisional Competition is a competition that is divided into a number of competitions. London 2012 is an example of a Divisional Competition."@en-gb .

sport:roundType rdfs:comment "Relates a round, to an enumerated round type."@en-gb .

sport:eventGender rdfs:comment "Relates a competition to a gender class instance."@en-gb .

sport:MultiStageCompetition rdfs:comment "A Multi-stage Competition is a competition that is organised as a set of stages. An example is the Football World Cup."@en-gb .

sport:SportingOrganisation rdfs:comment "An organisation involved in Sport, for example the UK Government Department for Culture, Media and Sport."@en-gb .

sport:hasUnitCompetition rdfs:comment "Relates a round to a unit competition in that round."@en-gb .

sport:Round rdfs:comment "A round is one or more competitions that is part of a Multi-Round Competition. Examples include the first round of Wimbledon and the final round of the FA Cup."@en-gb .

sport:LeagueCompetition rdfs:comment "A League Competition is a hierarchy of competitions or competition within such a hierarchy."@en-gb .

sport:awayCompetitor rdfs:comment "Relates a match to one competitor, by definition or designation not the home competitor."@en-gb .

sport:competesIn rdfs:comment "Relates a competitor, team or other agent to a competition."@en-gb .

sport:hasGroup rdfs:comment "Relates a league competition to a corresponding group competition."@en-gb .

sport:CompetitiveSportingOrganisation rdfs:comment "A sporting organisation that participates in competitive sporting events. For example Manchester United or Team GB at the Olympics."@en-gb .

sport:Person rdfs:comment "An athlete or other person with typically a participating role in a CompetitiveSportingOrganisation."@en-gb .

sport:GroupCompetition rdfs:comment "An organisation as a collection of leagues used to select the top N competitors from each league."@en-gb .

sport:promotesTo rdfs:comment "Relates a competition to the next competition in a heirarchy that teams are promoted to. For example the nPower Championship promotes to the Premier League."@en-gb .

sport:CompetitionType rdfs:comment "Enumerated competition types, for example: domestic, international."@en-gb .

sport:prevRound rdfs:comment "Relates a Round in a multi-round competition to its previous round."@en-gb .

sport:lastStage rdfs:comment "Relates a stage in a multi-stage competition to its last stage."@en-gb .

sport:MedalCompetition rdfs:comment "A competition that results in the awarding of a medal to the winner or runner up in that competition."@en-gb .

sport:SportsDiscipline rdfs:comment "The type of discipline a sporting event involves. Rugby League is a discipline as it has a different set of rules from Rugby Union."@en-gb .

sport:isGroupOf rdfs:comment "Relates a group competition to its corresponding League competition."@en-gb .

sport:nextStage rdfs:comment "Relates a stage in a multi-stage competition to its next stage."@en-gb .

sport:dateOfBirth rdfs:comment "Implemented because foaf has no notion of date of birth."@en-gb .

sport:hasMatch rdfs:comment "Relates a round to a match."@en-gb .

sport:prevStage rdfs:comment "Relates a stage in a multi-stage competition to its previous stage."@en-gb .

sport:CompetitiveSportingGroup rdfs:comment "The group of people that are available to compete in a particular competition. Two groups with the same members are not necessarily the same group."@en-gb .

sport:MultiRoundCompetition rdfs:comment "A Competition organised as a sequence of rounds, for example the Premier League or group stage of the World Cup."@en-gb .

sport:EventGender rdfs:comment "Enumerated type, typically Male, Female or Mixed."@en-gb .

sport:hasRound rdfs:comment "Relates a multi-round competition to a round in that competition."@en-gb .

sport:KnockoutCompetition rdfs:comment "A competition or stage of competition that progresses through rounds of individual fixtures whereby one team is eliminated as a result of each fixture."@en-gb .

sport:firstRound rdfs:comment "Relates a multi-round competition to the first round in that competition."@en-gb .

sport:Match rdfs:comment "The smallest unit of sporting competition."@en-gb .

sport:firstStage rdfs:comment "Relates a multi-stage competition to its first stage in that competition."@en-gb .

sport:nextRound rdfs:comment "Relates a round in a multi-round competition to its next round."@en-gb .

sport:homeCompetitor rdfs:comment "Relates a match to one competitor, by definition or designation not the away competitor."@en-gb .

sport:Competition rdfs:comment "A competitive sporting event that usually appears as an occurrence of a recurring competition, for example the recurring English Football Premier League has a seasonal competition occurrence during 2012/13"@en-gb .

sport:UnitCompetition rdfs:comment "A unit competition is the unit of competition defined by a competition discipline rules. Examples include a 100m race or Football match."@en-gb .

sport:lastRound rdfs:comment "Relates a multi-round competition to the last round in that competition."@en-gb .

sport:RecurringCompetition rdfs:comment "A recurring sports competition such as the Rugby Super League."@en-gb .

sport:RoundType rdfs:comment "Enumerated round types, for example: preliminary, qualifying or final."@en-gb .

sport:discipline rdfs:comment "Relates something to a sporting discipline, for example a person to athletics."@en-gb .

sport:subDisciplineOf rdfs:comment "Relates a discipline with a parent discipline, for example rhythmic gymnastics with gymnastics."@en-gb .

sport:MultiDisciplineCompetition rdfs:comment "A competition that incorporates a number of different sports, such as the Olympics."@en-gb .

sport:Home rdfs:comment "The home ground, stadium or location of a Competitive Sporting Organisation."@en-gb .

sport:recurringCompetition rdfs:comment "Relates a competition to the recurring instance of that competition, for example the 2012/13 Premier League to the Premier League."@en-gb .

sport:CompetesForRole rdfs:comment "legacy Class, used for associating an athlete with the national team they competed for during the olympics" .

<http://www.bbc.co.uk/ontologies/sport> rdfs:comment "The Sport Ontology is a simple lightweight ontology for publishing data about competitive sports events."^^xsd:string .

sport:competitionType rdfs:comment "Relates something, typically a competition, to an enumerated competition type."@en-gb .

sport:firstUnitCompetition rdfs:comment "Relates a multi-round competition to its first unit competition."@en-gb .

sport:isRoundOf rdfs:comment "Relates a round to its corresponding multi-round competition."@en-gb .

sport:prevUnitCompetition rdfs:comment "Relates a multi-round competition to its previous unit competition."@en-gb .

sport:relegatesTo rdfs:comment "Relates a competition to the previous competition in a heirarchy that teams are relegated to. For example the  Premier League relegates to the nPower Championship."@en-gb .

sport:division rdfs:comment "Division relates a DivisionalCompetition to a competition which is a division of that DivisionalCompetition. Used for the olympics"^^xsd:string .

sport:Venue rdfs:comment "The location of a sporting event. May be a stadium, track, lake etc."@en-gb .

sport:GoverningBody rdfs:comment "The Governing Body for a sport, such as The Football Association."@en-gb .

sport:hasCompetitor rdfs:comment "Relates a competition to a competitor in that competition."@en-gb .

sport:prevSession rdfs:comment "Relates a session to its previous session."@en-gb .

sport:flagImage rdfs:comment "Legacy property used to associate a team with the country flag it represented during the olympics" .

sport:lastUnitCompetition rdfs:comment "Relates a competition to its last unit competition."@en-gb .

sport:MultiDisciplineRecurringCompetition rdfs:comment "A recurring sports competition the covers many sports, such as the Summer Olympics."@en-gb .

sport:hasDivision rdfs:comment "Relates a divisional competition to a division in that competition."@en-gb .

sport:subDiscipline rdfs:comment "Relates a discipline with a child discipline, for example gymnastics with rhythmic gymnastics."@en-gb .

sport:nextUnitCompetition rdfs:comment "Relates a multi-round competition to its next unit competition."@en-gb .

sport:isSessionOf rdfs:comment "Relates a session to a competition."@en-gb .

sport:hasHome rdfs:comment "Relates a Competitive Sporting Organisation to its home ground, stadium or location."@en-gb .

sport:hasCompetedFor rdfs:comment "Associates an agent with sporting organisations non-temporally."@en-gb .

sport:roundNumber rdfs:comment "Indicates the sequential number of a round."@en-gb .

sport:nextSession rdfs:comment "Relates a session to its next session."@en-gb .

sport:lastSession rdfs:comment "Relates a competition to the last session of a series of sessions."@en-gb .

sport:firstSession rdfs:comment "Relates a competition to the first session of a series of sessions."@en-gb .

sport:isMatchOf rdfs:comment "Relates a match to a round."@en-gb .

sport:isStageOf rdfs:comment "Relates a stage to a multi-stage competition."@en-gb .

sport:Competition rdfs:label "Competition"@en-gb .

sport:Person rdfs:label "Person"@en-gb .

sport:dateOfBirth rdfs:label "dateOfBirth"@en-gb .

sport:hasStage rdfs:label "hasStage"@en-gb .

sport:isCompetitiveSportingOrganisationOf rdfs:label "isCompetitiveSportingOrganisationOf"@en-gb .

sport:Session rdfs:label "Session"@en-gb .

sport:hasSession rdfs:label "hasSession"@en-gb .

sport:DivisionalCompetition rdfs:label "DivisionalCompetition"@en-gb .

sport:roundType rdfs:label "roundType"@en-gb .

sport:eventGender rdfs:label "eventGender"@en-gb .

sport:MultiStageCompetition rdfs:label "MultiStageCompetition"@en-gb .

sport:SportingOrganisation rdfs:label "SportingOrganisation"@en-gb .

<http://www.bbc.co.uk/ontologies/sport> rdfs:label "Sport Ontology"^^xsd:string .

sport:hasUnitCompetition rdfs:label "hasUnitCompetition"@en-gb .

sport:Round rdfs:label "Round"@en-gb .

sport:LeagueCompetition rdfs:label "LeagueCompetition"@en-gb .

sport:competitionType rdfs:label "competitionType"@en-gb .

sport:awayCompetitor rdfs:label "awayCompetitor"@en-gb .

sport:competesIn rdfs:label "competesIn"@en-gb .

sport:hasGroup rdfs:label "hasGroup"@en-gb .

sport:CompetitiveSportingOrganisation rdfs:label "CompetitiveSportingOrganisation"@en-gb .

sport:GroupCompetition rdfs:label "GroupCompetition"@en-gb .

sport:promotesTo rdfs:label "promotesTo"@en-gb .

sport:CompetitionType rdfs:label "CompetitionType"@en-gb .

sport:prevRound rdfs:label "prevRound"@en-gb .

sport:lastStage rdfs:label "lastStage"@en-gb .

sport:MedalCompetition rdfs:label "MedalCompetition"@en-gb .

sport:SportsDiscipline rdfs:label "SportsDiscipline"@en-gb .

sport:isGroupOf rdfs:label "isGroupOf"@en-gb .

sport:nextStage rdfs:label "nextStage"@en-gb .

sport:hasMatch rdfs:label "hasMatch"@en-gb .

sport:prevStage rdfs:label "prevStage"@en-gb .

sport:CompetitiveSportingGroup rdfs:label "CompetitiveSportingGroup"@en-gb .

sport:MultiRoundCompetition rdfs:label "MultiRoundCompetition"@en-gb .

sport:EventGender rdfs:label "EventGender"@en-gb .

sport:hasRound rdfs:label "hasRound"@en-gb .

sport:KnockoutCompetition rdfs:label "KnockoutCompetition"@en-gb .

sport:subDiscipline rdfs:label "subDiscipline"@en-gb .

sport:firstRound rdfs:label "firstRound"@en-gb .

sport:Match rdfs:label "Match"@en-gb .

sport:firstStage rdfs:label "firstStage"@en-gb .

sport:nextRound rdfs:label "nextRound"@en-gb .

sport:homeCompetitor rdfs:label "homeCompetitor"@en-gb .

sport:UnitCompetition rdfs:label "UnitCompetition"@en-gb .

sport:lastRound rdfs:label "lastRound"@en-gb .

sport:RecurringCompetition rdfs:label "RecurringCompetition"@en-gb .

sport:RoundType rdfs:label "RoundType"@en-gb .

sport:discipline rdfs:label "discipline"@en-gb .

sport:subDisciplineOf rdfs:label "subDisciplineOf"@en-gb .

sport:MultiDisciplineCompetition rdfs:label "MultiDisciplineCompetition"@en-gb .

sport:Home rdfs:label "Home"@en-gb .

sport:recurringCompetition rdfs:label "recurringCompetition"@en-gb .

sport:CompetesForRole rdfs:label "CompetesForRole"^^xsd:string .

sport:firstUnitCompetition rdfs:label "firstUnitCompetition"@en-gb .

sport:isRoundOf rdfs:label "isRoundOf"@en-gb .

sport:prevUnitCompetition rdfs:label "prevUnitCompetition"@en-gb .

sport:relegatesTo rdfs:label "relegatesTo"@en-gb .

sport:Venue rdfs:label "Venue"@en-gb .

sport:GoverningBody rdfs:label "GoverningBody"@en-gb .

sport:hasCompetitor rdfs:label "hasCompetitor"@en-gb .

sport:prevSession rdfs:label "prevSession"@en-gb .

sport:lastUnitCompetition rdfs:label "lastUnitCompetition"@en-gb .

sport:MultiDisciplineRecurringCompetition rdfs:label "MultiDisciplineRecurringCompetition"@en-gb .

sport:hasDivision rdfs:label "hasDivision"@en-gb .

sport:nextUnitCompetition rdfs:label "nextUnitCompetition"@en-gb .

sport:isSessionOf rdfs:label "isSessionOf"@en-gb .

sport:hasHome rdfs:label "hasHome"@en-gb .

sport:hasCompetedFor rdfs:label "hasCompetedFor"@en-gb .

sport:roundNumber rdfs:label "roundNumber"@en-gb .

sport:nextSession rdfs:label "nextSession"@en-gb .

sport:lastSession rdfs:label "lastSession"@en-gb .

sport:firstSession rdfs:label "firstSession"@en-gb .

sport:isMatchOf rdfs:label "isMatchOf"@en-gb .

sport:isStageOf rdfs:label "isStageOf"@en-gb .

sport:MedalCompetition rdfs:isDefinedBy <http://www.bbc.co.uk/ontologies/sport> .

sport:RoundType rdfs:isDefinedBy <http://www.bbc.co.uk/ontologies/sport> .

sport:Session rdfs:isDefinedBy <http://www.bbc.co.uk/ontologies/sport> .

sport:awayCompetitor rdfs:isDefinedBy <http://www.bbc.co.uk/ontologies/sport> .

sport:firstRound rdfs:isDefinedBy <http://www.bbc.co.uk/ontologies/sport> .

sport:firstStage rdfs:isDefinedBy <http://www.bbc.co.uk/ontologies/sport> .

sport:isGroupOf rdfs:isDefinedBy <http://www.bbc.co.uk/ontologies/sport> .

sport:isCompetitiveSportingOrganisationOf rdfs:isDefinedBy <http://www.bbc.co.uk/ontologies/sport> .

sport:homeCompetitor rdfs:isDefinedBy <http://www.bbc.co.uk/ontologies/sport> .

sport:lastRound rdfs:isDefinedBy <http://www.bbc.co.uk/ontologies/sport> .

sport:lastStage rdfs:isDefinedBy <http://www.bbc.co.uk/ontologies/sport> .

sport:nextRound rdfs:isDefinedBy <http://www.bbc.co.uk/ontologies/sport> .

sport:nextStage rdfs:isDefinedBy <http://www.bbc.co.uk/ontologies/sport> .

sport:prevRound rdfs:isDefinedBy <http://www.bbc.co.uk/ontologies/sport> .

sport:prevStage rdfs:isDefinedBy <http://www.bbc.co.uk/ontologies/sport> .

sport:Competition rdfs:isDefinedBy <http://www.bbc.co.uk/ontologies/sport> .

sport:RecurringCompetition rdfs:isDefinedBy <http://www.bbc.co.uk/ontologies/sport> .

sport:CompetitiveSportingOrganisation rdfs:isDefinedBy <http://www.bbc.co.uk/ontologies/sport> .

sport:SportingOrganisation rdfs:isDefinedBy <http://www.bbc.co.uk/ontologies/sport> .

sport:SportsDiscipline rdfs:isDefinedBy <http://www.bbc.co.uk/ontologies/sport> .

sport:DivisionalCompetition rdfs:isDefinedBy <http://www.bbc.co.uk/ontologies/sport> .

sport:EventGender rdfs:isDefinedBy <http://www.bbc.co.uk/ontologies/sport> .

sport:GroupCompetition rdfs:isDefinedBy <http://www.bbc.co.uk/ontologies/sport> .

sport:MultiRoundCompetition rdfs:isDefinedBy <http://www.bbc.co.uk/ontologies/sport> .

sport:KnockoutCompetition rdfs:isDefinedBy <http://www.bbc.co.uk/ontologies/sport> .

sport:LeagueCompetition rdfs:isDefinedBy <http://www.bbc.co.uk/ontologies/sport> .

sport:Match rdfs:isDefinedBy <http://www.bbc.co.uk/ontologies/sport> .

sport:UnitCompetition rdfs:isDefinedBy <http://www.bbc.co.uk/ontologies/sport> .

sport:MultiStageCompetition rdfs:isDefinedBy <http://www.bbc.co.uk/ontologies/sport> .

sport:Person rdfs:isDefinedBy <http://www.bbc.co.uk/ontologies/sport> .

sport:Round rdfs:isDefinedBy <http://www.bbc.co.uk/ontologies/sport> .

sport:CompetitiveSportingGroup rdfs:isDefinedBy <http://www.bbc.co.uk/ontologies/sport> .

sport:CompetitionType rdfs:isDefinedBy <http://www.bbc.co.uk/ontologies/sport> .

sport:hasSession rdfs:isDefinedBy <http://www.bbc.co.uk/ontologies/sport> .

sport:roundType rdfs:isDefinedBy <http://www.bbc.co.uk/ontologies/sport> .

sport:dateOfBirth rdfs:isDefinedBy <http://www.bbc.co.uk/ontologies/sport> .

sport:competesIn rdfs:isDefinedBy <http://www.bbc.co.uk/ontologies/sport> .

sport:hasRound rdfs:isDefinedBy <http://www.bbc.co.uk/ontologies/sport> .

sport:hasStage rdfs:isDefinedBy <http://www.bbc.co.uk/ontologies/sport> .

sport:hasGroup rdfs:isDefinedBy <http://www.bbc.co.uk/ontologies/sport> .

sport:hasMatch rdfs:isDefinedBy <http://www.bbc.co.uk/ontologies/sport> .

sport:hasUnitCompetition rdfs:isDefinedBy <http://www.bbc.co.uk/ontologies/sport> .

sport:discipline rdfs:isDefinedBy <http://www.bbc.co.uk/ontologies/sport> .

sport:subDiscipline rdfs:isDefinedBy <http://www.bbc.co.uk/ontologies/sport> .

sport:eventGender rdfs:isDefinedBy <http://www.bbc.co.uk/ontologies/sport> .

sport:competitionType rdfs:isDefinedBy <http://www.bbc.co.uk/ontologies/sport> .

sport:MultiDisciplineRecurringCompetition rdfs:isDefinedBy <http://www.bbc.co.uk/ontologies/sport> .

sport:hasDivision rdfs:isDefinedBy <http://www.bbc.co.uk/ontologies/sport> .

sport:recurringCompetition rdfs:isDefinedBy <http://www.bbc.co.uk/ontologies/sport> .

sport:roundNumber rdfs:isDefinedBy <http://www.bbc.co.uk/ontologies/sport> .

sport:Home rdfs:isDefinedBy <http://www.bbc.co.uk/ontologies/sport> .

sport:Venue rdfs:isDefinedBy <http://www.bbc.co.uk/ontologies/sport> .

sport:hasHome rdfs:isDefinedBy <http://www.bbc.co.uk/ontologies/sport> .

sport:subDisciplineOf rdfs:isDefinedBy <http://www.bbc.co.uk/ontologies/sport> .

sport:MultiDisciplineCompetition rdfs:isDefinedBy <http://www.bbc.co.uk/ontologies/sport> .

sport:firstUnitCompetition rdfs:isDefinedBy <http://www.bbc.co.uk/ontologies/sport> .

sport:isRoundOf rdfs:isDefinedBy <http://www.bbc.co.uk/ontologies/sport> .

sport:prevUnitCompetition rdfs:isDefinedBy <http://www.bbc.co.uk/ontologies/sport> .

sport:GoverningBody rdfs:isDefinedBy <http://www.bbc.co.uk/ontologies/sport> .

sport:hasCompetitor rdfs:isDefinedBy <http://www.bbc.co.uk/ontologies/sport> .

sport:prevSession rdfs:isDefinedBy <http://www.bbc.co.uk/ontologies/sport> .

sport:lastUnitCompetition rdfs:isDefinedBy <http://www.bbc.co.uk/ontologies/sport> .

sport:nextUnitCompetition rdfs:isDefinedBy <http://www.bbc.co.uk/ontologies/sport> .

sport:isSessionOf rdfs:isDefinedBy <http://www.bbc.co.uk/ontologies/sport> .

sport:hasCompetedFor rdfs:isDefinedBy <http://www.bbc.co.uk/ontologies/sport> .

sport:nextSession rdfs:isDefinedBy <http://www.bbc.co.uk/ontologies/sport> .

sport:lastSession rdfs:isDefinedBy <http://www.bbc.co.uk/ontologies/sport> .

sport:firstSession rdfs:isDefinedBy <http://www.bbc.co.uk/ontologies/sport> .

sport:isMatchOf rdfs:isDefinedBy <http://www.bbc.co.uk/ontologies/sport> .

sport:isStageOf rdfs:isDefinedBy <http://www.bbc.co.uk/ontologies/sport> .

sport:division rdfs:seeAlso sport:hasDivisionList .

sport:isMatchOf <http://proton.semanticweb.org/2005/04/protons#transitiveOver> sport:isGroupOf , sport:isRoundOf , sport:isStageOf .

<http://www.bbc.co.uk/ontologies/sport> <http://xmlns.com/foaf/0.1/maker> <http://uk.linkedin.com/in/paulwilton> , <http://www.linkedin.com/in/tfgrahame> , <http://uk.linkedin.com/pub/jem-rayfield/27/b19/757> , <http://www.blockslabpillar.com> , <http://uk.linkedin.com/pub/stuart-williams/8/684/351> , <http://uk.linkedin.com/in/brianwmcbride> ;
	dcterms:license <http://bbcarchdev.github.io/licences/dps/1.0#id> ;
	owl:versionInfo "2.10"^^xsd:string ;
	owl:imports <http://purl.org/NET/c4dm/event.owl> , <http://xmlns.com/foaf/0.1/> , <http://proton.semanticweb.org/2005/04/protons> , <http://www.bbc.co.uk/ontologies/provenance> , <http://www.bbc.co.uk/ontologies/coreconcepts> , <http://www.bbc.co.uk/ontologies/asset/> ;
	provenance:canonicalLocation "https://repo.dev.bbc.co.uk/services/linked-data/ontologies/domain/sport/sport-2.10.ttl"^^xsd:string ;
	provenance:changeReason "Corrected Labels"@en-gb ;
	provenance:provided "2014-02-20T09:09:41+00:00"^^xsd:dateTime ;
	provenance:provider <mailto:clynt.pinfold@bbc.co.uk> ;
	provenance:version "2.10"^^xsd:double ;
	owl:versionIRI <http://www.bbc.co.uk/ontologies/sport/2.10> ;
	provenance:slug "sport"^^xsd:string ;
	provenance:public "true"^^xsd:boolean .

sport:division owl:deprecated "true"^^xsd:boolean .

sport:CompetesForRole owl:deprecated "true"^^xsd:boolean .

sport:flagImage owl:deprecated "true"^^xsd:boolean .
