@prefix rdfs:  <http://www.w3.org/2000/01/rdf-schema#> .
@prefix foaf:  <http://xmlns.com/foaf/0.1/> .
@prefix dct:   <http://purl.org/dc/terms/> .
@prefix owl:   <http://www.w3.org/2002/07/owl#> .
@prefix xsd:   <http://www.w3.org/2001/XMLSchema#> .
@prefix rdf:   <http://www.w3.org/1999/02/22-rdf-syntax-ns#> .
@prefix mdi:   <https://w3id.org/multidimensional-interface/ontology#> .
@prefix void:  <http://rdfs.org/ns/void#> .
@prefix vann:  <http://purl.org/vocab/vann/> .
@prefix hydra: <https://www.w3.org/ns/hydra/core#> .

mdi:RangeGate  a          rdfs:Class ;
        rdfs:comment      "A Linked Data interface through which Range Fragments can be selected by interval. This interface selects all Range Fragments whose interval overlap with the Range Gateâ€™s interval."@en ;
        rdfs:isDefinedBy  mdi: ;
        rdfs:label        "RangeGate"@en ;
        rdfs:subClassOf   hydra:PagedCollection .

<https://w3id.org/multidimensional-interface/ontology>
        a                              owl:Ontology ;
        rdfs:comment                   "An RDF vocabulary to describe and facilitate the usage of a Multidimensional Interface."@en ;
        rdfs:label                     "RDF vocabulary to describe a Multidimensional Interface."@en ;
        dct:creator                    [ foaf:mbox  "Ruben.Taelman@UGent.be" ;
                                         foaf:name  "Ruben Taelman"
                                       ] ;
        dct:issued                     "2016-06-28"^^xsd:date ;
        dct:modified                   "2016-06-28"^^xsd:date ;
        dct:title                      "The vocabulary for describing Multidimensional Interfaces"@en ;
        vann:preferredNamespacePrefix  "mid" ;
        vann:preferredNamespaceUri     "https://w3id.org/multidimensional-interface/ontology#" .

mdi:hasRangeGate  a       rdf:Property ;
        rdfs:comment      "A link to the Range Gate of a Multidimensional Index of a datasource."@en ;
        rdfs:domain       void:Dataset ;
        rdfs:isDefinedBy  mdi: ;
        rdfs:label        "has range gate"@en ;
        rdfs:range        mdi:RangeGate .

mdi:final  a              rdf:Property ;
        rdfs:comment      "The upper bound of an interval, excluding this value."@en ;
        rdfs:isDefinedBy  mdi: ;
        rdfs:label        "interval final"@en ;
        rdfs:range        xsd:numeric .

mdi:initial  a            rdf:Property ;
        rdfs:comment      "The lower bound of an interval, including this value."@en ;
        rdfs:isDefinedBy  mdi: ;
        rdfs:label        "interval initial"@en ;
        rdfs:range        xsd:numeric .

mdi:RangeFragment  a      rdfs:Class ;
        rdfs:comment      "A Linked Data Fragment that has an interval as selector, which apply to dimensional resources at one of its n dimensions."@en ;
        rdfs:isDefinedBy  mdi: ;
        rdfs:label        "RangeFragment"@en ;
        rdfs:subClassOf   hydra:PagedCollection .
