@prefix rdfs:  <http://www.w3.org/2000/01/rdf-schema#> .
@prefix ns1:   <http://www.w3.org/2003/06/sw-vocab-status/ns#> .
@prefix foaf:  <http://xmlns.com/foaf/0.1/> .
@prefix ns0:   <http://purl.org/vocab/vann/> .
@prefix owl:   <http://www.w3.org/2002/07/owl#> .
@prefix dc11:  <http://purl.org/dc/elements/1.1/> .
@prefix rdf:   <http://www.w3.org/1999/02/22-rdf-syntax-ns#> .
@prefix cc:    <http://creativecommons.org/ns#> .

<http://ns.inria.fr/ludo/v1/gamemodel#GameRecord>
        a                 owl:Class ;
        rdfs:comment      "A game record is a log of game players achievements in the game"@en ;
        rdfs:isDefinedBy  <http://ns.inria.fr/ludo/v1/gamemodel#> ;
        rdfs:label        "Game Record"@en ;
        rdfs:subClassOf   owl:Thing ;
        ns1:term_status   "stable" .

<http://ns.inria.fr/ludo/v1/gamemodel#VirtualCamera>
        a                 owl:Class ;
        rdfs:comment      "Viewport to the game world"@en ;
        rdfs:isDefinedBy  <http://ns.inria.fr/ludo/v1/gamemodel#> ;
        rdfs:label        "Virtual Camera"@en ;
        rdfs:subClassOf   owl:Thing ;
        ns1:term_status   "stable" .

<http://ns.inria.fr/ludo/v1/gamemodel#hasActingCoordination>
        a                 owl:DatatypeProperty ;
        rdfs:comment      "The coordination of a game object can involve appear (for generation and re- spawning of game object), animating an action, playing a sound, moving towards a checkpoint, interacting with another game object or a composition of these."@en ;
        rdfs:domain       <http://ns.inria.fr/ludo/v1/gamemodel#GameActingScript> ;
        rdfs:isDefinedBy  <http://ns.inria.fr/ludo/v1/gamemodel#> ;
        rdfs:label        "Has Game Acting Coordination"@en ;
        rdfs:range        <http://www.w3.org/2001/XMLSchema#string> ;
        ns1:term_status   "stable" .

<http://ns.inria.fr/ludo/v1/gamemodel#DecidingCondition>
        a                 owl:Class ;
        rdfs:comment      "Deciding Condition"@en ;
        rdfs:isDefinedBy  <http://ns.inria.fr/ludo/v1/gamemodel#> ;
        rdfs:label        "Deciding Condition"@en ;
        rdfs:subClassOf   <http://ns.inria.fr/ludo/v1/gamemodel#Intelligence> ;
        ns1:term_status   "stable" .

<http://ns.inria.fr/ludo/v1/gamemodel#hasGameActingScript>
        a                 owl:ObjectProperty ;
        rdfs:comment      "Game Acting Script"@en ;
        rdfs:domain       <http://ns.inria.fr/ludo/v1/gamemodel#GameAct> ;
        rdfs:isDefinedBy  <http://ns.inria.fr/ludo/v1/gamemodel#> ;
        rdfs:label        "Game Acting Script"@en ;
        rdfs:range        <http://ns.inria.fr/ludo/v1/gamemodel#GameActingScript> ;
        ns1:term_status   "stable" .

<http://ns.inria.fr/ludo/v1/gamemodel#DifficultyIndicator>
        a                 owl:Class ;
        rdfs:comment      "A value associated to the difficulty of the game scenario"@en ;
        rdfs:isDefinedBy  <http://ns.inria.fr/ludo/v1/gamemodel#> ;
        rdfs:label        "Difficulty Indicator"@en ;
        rdfs:subClassOf   owl:Thing ;
        ns1:term_status   "stable" .

<http://ns.inria.fr/ludo/v1/gamemodel#hasAction>
        a                 owl:ObjectProperty ;
        rdfs:comment      "Has action"@en ;
        rdfs:domain       <http://ns.inria.fr/ludo/v1/gamemodel#GameObject> ;
        rdfs:isDefinedBy  <http://ns.inria.fr/ludo/v1/gamemodel#> ;
        rdfs:label        "Has action"@en ;
        rdfs:range        <http://ns.inria.fr/ludo/v1/gamemodel#Action> ;
        ns1:term_status   "stable" .

<http://ns.inria.fr/ludo/v1/gamemodel#>
        a                             owl:Ontology ;
        rdfs:comment                  "Given the increasing amount of structured data published on the Web, many possibilities are open for creating new types of games that use resources from the Web of Data. In particular, if we consider the subcategory of Serious Games in which the object of the game is to educate the user through the interactive discovery of real-life concepts (associated to Semantic Web resources), the inclusion of a semantic representation of the user profile and his contextual information becomes an important element to recommend the user more accurate concepts. Ludo is an ontology that allows the creation of Serious Games with those characteristics."@en ;
        cc:license                    <http://creativecommons.org/licenses/by/3.0/> ;
        dc11:creator                  <http://www.oscarrodriguez.me> , <https://plus.google.com/106595696646939943813> ;
        dc11:issued                   "2016-02-01"^^<http://www.w3.org/2001/XMLSchema#date> ;
        dc11:modified                 "2016-08-09"^^<http://www.w3.org/2001/XMLSchema#date> ;
        dc11:publisher                <http://dbpedia.org/resource/National_Institute_for_Research_in_Computer_Science_and_Control> ;
        ns0:preferredNamespacePrefix  "gamemodel" ;
        ns0:preferredNamespaceUri     "http://ns.inria.fr/ludo/v1/gamemodel#"^^<http://www.w3.org/2001/XMLSchema#string> ;
        owl:versionInfo               0.1 .

<http://ns.inria.fr/ludo/v1/gamemodel#GameEnvironment>
        a                 owl:Class ;
        rdfs:comment      "Represents the composition of the virtual world by populating the virtual space with game objects."@en ;
        rdfs:isDefinedBy  <http://ns.inria.fr/ludo/v1/gamemodel#> ;
        rdfs:label        "Game Environment"@en ;
        rdfs:subClassOf   owl:Thing ;
        ns1:term_status   "stable" .

<http://ns.inria.fr/ludo/v1/gamemodel#hasVirtualCameraPosition>
        a                 owl:DatatypeProperty ;
        rdfs:comment      "Position of the virtual camera in the game world"@en ;
        rdfs:domain       <http://ns.inria.fr/ludo/v1/gamemodel#VirtualCamera> ;
        rdfs:isDefinedBy  <http://ns.inria.fr/ludo/v1/gamemodel#> ;
        rdfs:label        "Has Virtual Camera Position"@en ;
        rdfs:range        <http://www.w3.org/2001/XMLSchema#string> ;
        ns1:term_status   "stable" .

<http://ns.inria.fr/ludo/v1/gamemodel#Force>
        a                 owl:Class ;
        rdfs:comment      "A motion is subject to a force"@en ;
        rdfs:isDefinedBy  <http://ns.inria.fr/ludo/v1/gamemodel#> ;
        rdfs:label        "Force"@en ;
        rdfs:subClassOf   owl:Thing ;
        ns1:term_status   "stable" .

<http://ns.inria.fr/ludo/v1/gamemodel#GameScoringRule>
        a                 owl:Class ;
        rdfs:comment      "Only applies to game player and it defines what to be awarded to the game player when a scoring condition is met."@en ;
        rdfs:isDefinedBy  <http://ns.inria.fr/ludo/v1/gamemodel#> ;
        rdfs:label        "Game Scoring Rule"@en ;
        rdfs:subClassOf   <http://ns.inria.fr/ludo/v1/gamemodel#GameRule> ;
        ns1:term_status   "stable" .

<http://ns.inria.fr/ludo/v1/gamemodel#hasGameStructure>
        a                 owl:ObjectProperty ;
        rdfs:comment      "Has Game Structure"@en ;
        rdfs:domain       <http://ns.inria.fr/ludo/v1/gamemodel#SeriousGame> ;
        rdfs:isDefinedBy  <http://ns.inria.fr/ludo/v1/gamemodel#> ;
        rdfs:label        "Has Game Structure"@en ;
        rdfs:range        <http://ns.inria.fr/ludo/v1/gamemodel#GameStructure> ;
        ns1:term_status   "stable" .

<http://ns.inria.fr/ludo/v1/gamemodel#hasMotion>
        a                 owl:ObjectProperty ;
        rdfs:comment      "Has Motion"@en ;
        rdfs:domain       <http://ns.inria.fr/ludo/v1/gamemodel#Action> ;
        rdfs:isDefinedBy  <http://ns.inria.fr/ludo/v1/gamemodel#> ;
        rdfs:label        "Has Motion"@en ;
        rdfs:range        <http://ns.inria.fr/ludo/v1/gamemodel#Motion> ;
        ns1:term_status   "stable" .

<http://ns.inria.fr/ludo/v1/gamemodel#Mass>
        a                 owl:Class ;
        rdfs:comment      "The mass that affects the motion of the game object"@en ;
        rdfs:isDefinedBy  <http://ns.inria.fr/ludo/v1/gamemodel#> ;
        rdfs:label        "Mass"@en ;
        rdfs:subClassOf   <http://ns.inria.fr/ludo/v1/gamemodel#ObjectAttribute> ;
        ns1:term_status   "stable" .

<http://ns.inria.fr/ludo/v1/gamemodel#Training-basedStructure>
        a                 owl:Class ;
        rdfs:comment      "Training-based Structure"@en ;
        rdfs:isDefinedBy  <http://ns.inria.fr/ludo/v1/gamemodel#> ;
        rdfs:label        "Training-based Structure"@en ;
        rdfs:subClassOf   <http://ns.inria.fr/ludo/v1/gamemodel#GameStructure> ;
        ns1:term_status   "stable" .

<http://ns.inria.fr/ludo/v1/gamemodel#hasSoringRuleOutcome>
        a                 owl:DatatypeProperty ;
        rdfs:comment      "The outcome of an Scoring Rule"@en ;
        rdfs:domain       <http://ns.inria.fr/ludo/v1/gamemodel#GameScoringRule> ;
        rdfs:isDefinedBy  <http://ns.inria.fr/ludo/v1/gamemodel#> ;
        rdfs:label        "Scoring Rule Outcome"@en ;
        rdfs:range        <http://www.w3.org/2001/XMLSchema#string> ;
        ns1:term_status   "stable" .

<https://plus.google.com/106595696646939943813>
        a       foaf:Person .

<http://ns.inria.fr/ludo/v1/gamemodel#Inventory>
        a                 owl:Class ;
        rdfs:comment      "Inventory presents the idea where player can own a number of game objects in the game as part of the game play. An inventory can be a collection of weapons in a shooter game or a collection of magic spell and potions in a role-playing game. In games such as Resident Evil 5 (www.residentevil.com), a game player can hold 9 items in the inventory at any one time."@en ;
        rdfs:isDefinedBy  <http://ns.inria.fr/ludo/v1/gamemodel#> ;
        rdfs:label        "Inventory"@en ;
        rdfs:subClassOf   owl:Thing ;
        ns1:term_status   "stable" .

<http://ns.inria.fr/ludo/v1/gamemodel#hasMass>
        a                 owl:DatatypeProperty ;
        rdfs:comment      "The amount of matter of an object in Kilograms."@en ;
        rdfs:domain       <http://ns.inria.fr/ludo/v1/gamemodel#Mass> ;
        rdfs:isDefinedBy  <http://ns.inria.fr/ludo/v1/gamemodel#> ;
        rdfs:label        "Mass"@en ;
        rdfs:range        <http://www.w3.org/2001/XMLSchema#float> ;
        ns1:term_status   "stable" .

<http://ns.inria.fr/ludo/v1/gamemodel#hasGameObject>
        a                 owl:ObjectProperty ;
        rdfs:comment      "This property applies for a Game Environment, a Serious Game and an Inventory"@en ;
        rdfs:isDefinedBy  <http://ns.inria.fr/ludo/v1/gamemodel#> ;
        rdfs:label        "Has Game Object"@en ;
        rdfs:range        <http://ns.inria.fr/ludo/v1/gamemodel#GameObject> ;
        ns1:term_status   "stable" .

<http://ns.inria.fr/ludo/v1/gamemodel#hasObjectVitalityValue>
        a                 owl:DatatypeProperty ;
        rdfs:comment      "Object Vitality Value"@en ;
        rdfs:domain       <http://ns.inria.fr/ludo/v1/gamemodel#ObjectVitality> ;
        rdfs:isDefinedBy  <http://ns.inria.fr/ludo/v1/gamemodel#> ;
        rdfs:label        "Object Vitality Value"@en ;
        rdfs:range        <http://www.w3.org/2001/XMLSchema#integer> ;
        ns1:term_status   "stable" .

<http://ns.inria.fr/ludo/v1/gamemodel#hasInteractionCondition>
        a                 owl:DatatypeProperty ;
        rdfs:comment      "It refers to the state of actor or the state of the game world"@en ;
        rdfs:domain       <http://ns.inria.fr/ludo/v1/gamemodel#GameInteractionRule> ;
        rdfs:isDefinedBy  <http://ns.inria.fr/ludo/v1/gamemodel#> ;
        rdfs:label        "Interaction Condition"@en ;
        rdfs:range        <http://www.w3.org/2001/XMLSchema#string> ;
        ns1:term_status   "stable" .

<http://ns.inria.fr/ludo/v1/gamemodel#Animation>
        a                 owl:Class ;
        rdfs:comment      "An animation defines the virtual performance of a game object without reference of the position of the game object as a whole."@en ;
        rdfs:isDefinedBy  <http://ns.inria.fr/ludo/v1/gamemodel#> ;
        rdfs:label        "Animation"@en ;
        rdfs:subClassOf   owl:Thing ;
        ns1:term_status   "stable" .

<http://ns.inria.fr/ludo/v1/gamemodel#GameEvent>
        a                 owl:Class ;
        rdfs:comment      "Is the happening associated to a game scenario. A game event is composed of a set of game act and an event trigger which initiate the game event."@en ;
        rdfs:isDefinedBy  <http://ns.inria.fr/ludo/v1/gamemodel#> ;
        rdfs:label        "Game Event"@en ;
        rdfs:subClassOf   owl:Thing ;
        ns1:term_status   "stable" .

<http://ns.inria.fr/ludo/v1/gamemodel#hasGameTheme>
        a                 owl:ObjectProperty ;
        rdfs:comment      "Has Game Theme"@en ;
        rdfs:domain       <http://ns.inria.fr/ludo/v1/gamemodel#SeriousGame> ;
        rdfs:isDefinedBy  <http://ns.inria.fr/ludo/v1/gamemodel#> ;
        rdfs:label        "Has Game Theme"@en ;
        rdfs:range        <http://ns.inria.fr/ludo/v1/gamemodel#GameTheme> ;
        ns1:term_status   "stable" .

<http://ns.inria.fr/ludo/v1/gamemodel#Button>
        a                 owl:Class ;
        rdfs:comment      "Button"@en ;
        rdfs:isDefinedBy  <http://ns.inria.fr/ludo/v1/gamemodel#> ;
        rdfs:label        "Button"@en ;
        rdfs:subClassOf   owl:Thing , <http://ns.inria.fr/ludo/v1/gamemodel#GUIComponent> ;
        ns1:term_status   "stable" .

<http://ns.inria.fr/ludo/v1/gamemodel#hasAppearance>
        a                 owl:ObjectProperty ;
        rdfs:comment      "Has appearance"@en ;
        rdfs:domain       <http://ns.inria.fr/ludo/v1/gamemodel#GameObject> ;
        rdfs:isDefinedBy  <http://ns.inria.fr/ludo/v1/gamemodel#> ;
        rdfs:label        "Has appearance"@en ;
        rdfs:range        <http://ns.inria.fr/ludo/v1/gamemodel#Appearance> ;
        ns1:term_status   "stable" .

<http://ns.inria.fr/ludo/v1/gamemodel#hasGamePhysics>
        a                 owl:DatatypeProperty ;
        rdfs:comment      "Has Game Physics"@en ;
        rdfs:isDefinedBy  <http://ns.inria.fr/ludo/v1/gamemodel#> ;
        rdfs:label        "Has Game Physics"@en ;
        rdfs:range        <http://www.w3.org/2001/XMLSchema#string> ;
        ns1:term_status   "stable" .

[ a            owl:AllDisjointClasses ;
  owl:members  ( <http://ns.inria.fr/ludo/v1/gamemodel#GameAttribute> <http://ns.inria.fr/ludo/v1/gamemodel#GameControl> <http://ns.inria.fr/ludo/v1/gamemodel#GameRecord> )
] .

<http://ns.inria.fr/ludo/v1/gamemodel#Scenario-basedStructure>
        a                 owl:Class ;
        rdfs:comment      "Scenario-based Structure"@en ;
        rdfs:isDefinedBy  <http://ns.inria.fr/ludo/v1/gamemodel#> ;
        rdfs:label        "Scenario-based Structure"@en ;
        rdfs:subClassOf   <http://ns.inria.fr/ludo/v1/gamemodel#GameStructure> ;
        ns1:term_status   "stable" .

<http://ns.inria.fr/ludo/v1/gamemodel#GameAttribute>
        a                 owl:Class ;
        rdfs:comment      "Data properties that represent a game objects vitality, physical being, cognitive state and ownership."@en ;
        rdfs:isDefinedBy  <http://ns.inria.fr/ludo/v1/gamemodel#> ;
        rdfs:label        "Game Attribute"@en ;
        rdfs:subClassOf   owl:Thing ;
        ns1:term_status   "stable" .

<http://ns.inria.fr/ludo/v1/gamemodel#PedagogicEventIndicator>
        a                 owl:Class ;
        rdfs:comment      "Each game section is associated with one or more pedagogic events from the Gagnes nine events of instructions"@en ;
        rdfs:isDefinedBy  <http://ns.inria.fr/ludo/v1/gamemodel#> ;
        rdfs:label        "Pedagogic Event Indicator"@en ;
        rdfs:subClassOf   owl:Thing ;
        ns1:term_status   "stable" .

<http://ns.inria.fr/ludo/v1/gamemodel#Learn>
        a                 owl:Class ;
        rdfs:comment      "Learn"@en ;
        rdfs:isDefinedBy  <http://ns.inria.fr/ludo/v1/gamemodel#> ;
        rdfs:label        "Learn"@en ;
        rdfs:subClassOf   owl:Thing ;
        ns1:term_status   "stable" .

<http://ns.inria.fr/ludo/v1/gamemodel#GameControl>
        a                 owl:Class ;
        rdfs:comment      "Provides game player the channel to control game objects"@en ;
        rdfs:isDefinedBy  <http://ns.inria.fr/ludo/v1/gamemodel#> ;
        rdfs:label        "Game Control"@en ;
        rdfs:subClassOf   owl:Thing ;
        ns1:term_status   "stable" .

<http://ns.inria.fr/ludo/v1/gamemodel#GameInteractionRule>
        a                 owl:Class ;
        rdfs:comment      "It dictates the outcome of the interaction from two game objects."@en ;
        rdfs:isDefinedBy  <http://ns.inria.fr/ludo/v1/gamemodel#> ;
        rdfs:label        "Game Interaction Rule"@en ;
        rdfs:subClassOf   <http://ns.inria.fr/ludo/v1/gamemodel#GameRule> ;
        owl:disjointWith  <http://ns.inria.fr/ludo/v1/gamemodel#GameScoringRule> ;
        ns1:term_status   "stable" .

[ a            owl:AllDisjointClasses ;
  owl:members  ( <http://ns.inria.fr/ludo/v1/gamemodel#Animation> <http://ns.inria.fr/ludo/v1/gamemodel#Motion> <http://ns.inria.fr/ludo/v1/gamemodel#Sound> <http://ns.inria.fr/ludo/v1/gamemodel#VitalUpdate> )
] .

[ a            owl:AllDisjointClasses ;
  owl:members  ( <http://ns.inria.fr/ludo/v1/gamemodel#Graphic> <http://ns.inria.fr/ludo/v1/gamemodel#Sound> <http://ns.inria.fr/ludo/v1/gamemodel#Video> <http://ns.inria.fr/ludo/v1/gamemodel#hasText> )
] .

<http://ns.inria.fr/ludo/v1/gamemodel#Intelligence>
        a                 owl:Class ;
        rdfs:comment      "Provides game object the ability to decide, navigate and even learn."@en ;
        rdfs:isDefinedBy  <http://ns.inria.fr/ludo/v1/gamemodel#> ;
        rdfs:label        "Intelligence"@en ;
        rdfs:subClassOf   owl:Thing ;
        ns1:term_status   "stable" .

<http://ns.inria.fr/ludo/v1/gamemodel#GameScenario>
        a                 owl:Class ;
        rdfs:comment      "A description of a situation which require game player to overcome a number of challenges in order to achieve the defined objectives. It is also commonly termed as game level in gaming jargon."@en ;
        rdfs:isDefinedBy  <http://ns.inria.fr/ludo/v1/gamemodel#> ;
        rdfs:label        "Game Scenario"@en ;
        rdfs:subClassOf   owl:Thing ;
        ns1:term_status   "stable" .

<http://ns.inria.fr/ludo/v1/gamemodel#GameContext>
        a                 owl:Class ;
        rdfs:comment      "Describes the type of game content presented to game players in a game presentation or game simulation."@en ;
        rdfs:isDefinedBy  <http://ns.inria.fr/ludo/v1/gamemodel#> ;
        rdfs:label        "Game Context"@en ;
        rdfs:subClassOf   owl:Thing ;
        ns1:term_status   "stable" .

<http://ns.inria.fr/ludo/v1/gamemodel#GameInteractionRuleOutcome>
        a                 owl:Class ;
        rdfs:comment      "Outcome of an Interaction Rule"@en ;
        rdfs:isDefinedBy  <http://ns.inria.fr/ludo/v1/gamemodel#> ;
        rdfs:label        "Interaction Rule Outcome"@en ;
        rdfs:subClassOf   owl:Thing ;
        ns1:term_status   "stable" .

foaf:Person  a  owl:Class .

<http://rdfs.org/ns/void#Dataset>
        a       owl:Class .

[ a            owl:AllDisjointClasses ;
  owl:members  ( <http://ns.inria.fr/ludo/v1/gamemodel#GameEvent> <http://ns.inria.fr/ludo/v1/gamemodel#GameObject> <http://ns.inria.fr/ludo/v1/gamemodel#GameObjective> <http://ns.inria.fr/ludo/v1/gamemodel#GamePlayer> <http://ns.inria.fr/ludo/v1/gamemodel#GamePresentation> <http://ns.inria.fr/ludo/v1/gamemodel#GameRule> <http://ns.inria.fr/ludo/v1/gamemodel#GameScenario> <http://ns.inria.fr/ludo/v1/gamemodel#GameSimulation> <http://ns.inria.fr/ludo/v1/gamemodel#GameStructure> <http://ns.inria.fr/ludo/v1/gamemodel#GameTheme> )
] .

<http://ns.inria.fr/ludo/v1/gamemodel#GameKnowledgeBase>
        a                owl:Class ;
        rdfs:comment     "A Knowledge Base to be used by the game."@en ;
        rdfs:label       "Game Knowledge Base"@en ;
        rdfs:subClassOf  <http://rdfs.org/ns/void#Dataset> .

<http://ns.inria.fr/ludo/v1/gamemodel#hasGameDimension>
        a                 owl:DatatypeProperty ;
        rdfs:comment      "The game dimension refers to the virtual space of which the game simulation takes place. It can either be 2D or 3D."@en ;
        rdfs:domain       <http://ns.inria.fr/ludo/v1/gamemodel#GameDimension> ;
        rdfs:isDefinedBy  <http://ns.inria.fr/ludo/v1/gamemodel#> ;
        rdfs:label        "Has Game Dimension"@en ;
        rdfs:range        <http://www.w3.org/2001/XMLSchema#string> ;
        ns1:term_status   "stable" .

<http://ns.inria.fr/ludo/v1/gamemodel#GamePresentation>
        a                 owl:Class ;
        rdfs:comment      "A virtual canvas that holds media components and GUI components to form a game menu, a game notification or a cut-scene to present information about the game and allow them to navigate through the game structure"@en ;
        rdfs:isDefinedBy  <http://ns.inria.fr/ludo/v1/gamemodel#> ;
        rdfs:label        "Game Presentation"@en ;
        rdfs:subClassOf   <http://ns.inria.fr/ludo/v1/gamemodel#GameContext> ;
        ns1:term_status   "stable" .

<http://ns.inria.fr/ludo/v1/gamemodel#VitalUpdate>
        a                 owl:Class ;
        rdfs:comment      "Revises the value of vitals for a game object as a measure that takes into account the cost of an action inflicted to the object or the cost of performing an action."@en ;
        rdfs:isDefinedBy  <http://ns.inria.fr/ludo/v1/gamemodel#> ;
        rdfs:label        "Vital Update"@en ;
        rdfs:subClassOf   owl:Thing ;
        ns1:term_status   "stable" .

<http://ns.inria.fr/ludo/v1/gamemodel#hasConstraint>
        a                 owl:ObjectProperty ;
        rdfs:comment      "Has constraint"@en ;
        rdfs:domain       <http://ns.inria.fr/ludo/v1/gamemodel#Motion> ;
        rdfs:isDefinedBy  <http://ns.inria.fr/ludo/v1/gamemodel#> ;
        rdfs:label        "Has constraint"@en ;
        rdfs:range        <http://ns.inria.fr/ludo/v1/gamemodel#Constraint> ;
        ns1:term_status   "stable" .

<http://ns.inria.fr/ludo/v1/gamemodel#hasObjectVitality>
        a                 owl:DatatypeProperty ;
        rdfs:comment      "Vitality of an object such as life or interrelated attributes such as health, energy, strength, social and etc."@en ;
        rdfs:domain       <http://ns.inria.fr/ludo/v1/gamemodel#ObjectVitality> ;
        rdfs:isDefinedBy  <http://ns.inria.fr/ludo/v1/gamemodel#> ;
        rdfs:label        "Has Object Vitality"@en ;
        rdfs:range        <http://www.w3.org/2001/XMLSchema#string> ;
        ns1:term_status   "stable" .

<http://ns.inria.fr/ludo/v1/gamemodel#hasArtRequirement>
        a                 owl:ObjectProperty ;
        rdfs:comment      "Has art requirement"@en ;
        rdfs:domain       <http://ns.inria.fr/ludo/v1/gamemodel#GameTheme> ;
        rdfs:isDefinedBy  <http://ns.inria.fr/ludo/v1/gamemodel#> ;
        rdfs:label        "Has art requirement"@en ;
        rdfs:range        <http://ns.inria.fr/ludo/v1/gamemodel#ArtRequirement> ;
        ns1:term_status   "stable" .

<http://ns.inria.fr/ludo/v1/gamemodel#GameSimulation>
        a                 owl:Class ;
        rdfs:comment      "Represents the simulation of a game scenario and is governed by a set of rules that define the interactivity, physical and temporal properties of the virtual world. It has game rules, game dimension, game tempo and game physics."@en ;
        rdfs:isDefinedBy  <http://ns.inria.fr/ludo/v1/gamemodel#> ;
        rdfs:label        "Game Simulation"@en ;
        rdfs:subClassOf   <http://ns.inria.fr/ludo/v1/gamemodel#GameContext> ;
        ns1:term_status   "stable" .

<http://ns.inria.fr/ludo/v1/gamemodel#hasInteractionRuleOutcomeOperation>
        a                 owl:DatatypeProperty ;
        rdfs:comment      "Rewarding the player with any game object can mean give (add) or take away (subtract) an item or increase (add) or decrease (subtract) in the value of an attribute to provide the game player the advantage to succeed in the game."@en ;
        rdfs:domain       <http://ns.inria.fr/ludo/v1/gamemodel#GameInteractionRuleOutcome> ;
        rdfs:isDefinedBy  <http://ns.inria.fr/ludo/v1/gamemodel#> ;
        rdfs:label        "Interaction Rule Outcome Operation"@en ;
        rdfs:range        <http://www.w3.org/2001/XMLSchema#string> ;
        ns1:term_status   "stable" .

<http://ns.inria.fr/ludo/v1/gamemodel#hasIntelligences>
        a                 owl:ObjectProperty ;
        rdfs:comment      "Has Intelligences"@en ;
        rdfs:domain       <http://ns.inria.fr/ludo/v1/gamemodel#GameObject> ;
        rdfs:isDefinedBy  <http://ns.inria.fr/ludo/v1/gamemodel#> ;
        rdfs:label        "Has Intelligences"@en ;
        rdfs:range        <http://ns.inria.fr/ludo/v1/gamemodel#Intelligence> ;
        ns1:term_status   "stable" .

<http://ns.inria.fr/ludo/v1/gamemodel#GameObject>
        a                 owl:Class ;
        rdfs:comment      "Represents virtual things that populate the game world and can be designed to have a combination of abilities such as decision making, moving, acting and responding to surroundings and game players input simulating their existence in the game world."@en ;
        rdfs:isDefinedBy  <http://ns.inria.fr/ludo/v1/gamemodel#> ;
        rdfs:label        "Game Object"@en ;
        rdfs:subClassOf   owl:Thing ;
        ns1:term_status   "stable" .

<http://ns.inria.fr/ludo/v1/gamemodel#Navigate>
        a                 owl:Class ;
        rdfs:comment      "Navigate"@en ;
        rdfs:isDefinedBy  <http://ns.inria.fr/ludo/v1/gamemodel#> ;
        rdfs:label        "Navigate"@en ;
        rdfs:subClassOf   owl:Thing ;
        ns1:term_status   "stable" .

<http://ns.inria.fr/ludo/v1/gamemodel#EventTrigger>
        a                 owl:Class ;
        rdfs:comment      "Event triggers are used to invoke the transition between game sections and activate the game events within a game scenario"@en ;
        rdfs:isDefinedBy  <http://ns.inria.fr/ludo/v1/gamemodel#> ;
        rdfs:label        "Event Trigger"@en ;
        rdfs:subClassOf   owl:Thing ;
        ns1:term_status   "stable" .

<http://ns.inria.fr/ludo/v1/gamemodel#hasGoalCondition>
        a                 owl:ObjectProperty ;
        rdfs:comment      "Has Goal Condition"@en ;
        rdfs:domain       <http://ns.inria.fr/ludo/v1/gamemodel#GameObjective> ;
        rdfs:isDefinedBy  <http://ns.inria.fr/ludo/v1/gamemodel#> ;
        rdfs:label        "Has Goal Condition"@en ;
        rdfs:range        <http://ns.inria.fr/ludo/v1/gamemodel#GoalCondition> ;
        ns1:term_status   "stable" .

<http://ns.inria.fr/ludo/v1/gamemodel#ArtRequirement>
        a                 owl:Class ;
        rdfs:comment      "Art requirements related the game through expressive written text"@en ;
        rdfs:isDefinedBy  <http://ns.inria.fr/ludo/v1/gamemodel#> ;
        rdfs:label        "Art Requirement"@en ;
        rdfs:subClassOf   owl:Thing ;
        ns1:term_status   "stable" .

<http://ns.inria.fr/ludo/v1/gamemodel#SoidityState>
        a                owl:Class ;
        rdfs:comment     "The solidity state defines if a game object is solid, whereas the mass affects the motion of the game object."@en ;
        rdfs:label       "Solidity State"@en ;
        rdfs:subClassOf  <http://ns.inria.fr/ludo/v1/gamemodel#ObjectsAttribute> ;
        ns1:term_status  "stable" .

<http://ns.inria.fr/ludo/v1/gamemodel#Appearance>
        a                 owl:Class ;
        rdfs:comment      "The visual appearance of a game object"@en ;
        rdfs:isDefinedBy  <http://ns.inria.fr/ludo/v1/gamemodel#> ;
        rdfs:label        "Appearance"@en ;
        rdfs:subClassOf   owl:Thing ;
        ns1:term_status   "stable" .

<http://ns.inria.fr/ludo/v1/gamemodel#GameTheme>
        a                 owl:Class ;
        rdfs:comment      "Describes most of the art requirements related the game through expressive written text."@en ;
        rdfs:isDefinedBy  <http://ns.inria.fr/ludo/v1/gamemodel#> ;
        rdfs:label        "Game Theme"@en ;
        rdfs:subClassOf   owl:Thing ;
        ns1:term_status   "stable" .

<http://ns.inria.fr/ludo/v1/gamemodel#hasInventory>
        a                 owl:ObjectProperty ;
        rdfs:comment      "Has Inventory"@en ;
        rdfs:domain       <http://ns.inria.fr/ludo/v1/gamemodel#GamePlayer> ;
        rdfs:isDefinedBy  <http://ns.inria.fr/ludo/v1/gamemodel#> ;
        rdfs:label        "Has Inventory"@en ;
        rdfs:range        <http://ns.inria.fr/ludo/v1/gamemodel#Inventory> ;
        ns1:term_status   "stable" .

<http://ns.inria.fr/ludo/v1/gamemodel#InventoryState>
        a                 owl:Class ;
        rdfs:comment      "The inventory is defined to hold a limited supply of consumable for a game object."@en ;
        rdfs:isDefinedBy  <http://ns.inria.fr/ludo/v1/gamemodel#> ;
        rdfs:label        "Inventory State"@en ;
        rdfs:subClassOf   <http://ns.inria.fr/ludo/v1/gamemodel#ObjectAttribute> ;
        ns1:term_status   "stable" .

<http://ns.inria.fr/ludo/v1/gamemodel#hasEventTriggerClass>
        a                         owl:DatatypeProperty ;
        rdfs:comment              "Event triggers are used to invoke the transition between game sections and activate the game events within a game scenario. They can be classified into four distinct classes, namely: Input trigger detects user input via hardware interface or graphical user interface (GUI); Time trigger is essentially a countdown timer with an interval value with frequency of once, to repeat infinitely or to repeat finitely; Proximity trigger like input trigger has a hotspot that detects the collision of a specified game object, a class of game object or a group of game objects from different classes; Game mechanics trigger is associated to a range of game application related of events such media event, game event and simulation event. Each event trigger is associated with a command that specify the transition between game sections or activation of a game event."@en ;
        rdfs:domain               <http://ns.inria.fr/ludo/v1/gamemodel#EventTrigger> ;
        rdfs:isDefinedBy          <http://ns.inria.fr/ludo/v1/gamemodel#> ;
        rdfs:label                "Has Event Trigger Class"@en ;
        rdfs:range                <http://www.w3.org/2001/XMLSchema#string> ;
        owl:propertyDisjointWith  <http://ns.inria.fr/ludo/v1/gamemodel#hasEventTriggerCommand> ;
        ns1:term_status           "stable" .

<http://ns.inria.fr/ludo/v1/gamemodel#ObjectsAttribute>
        a                 owl:Class ;
        rdfs:comment      "Objects attribute"@en ;
        rdfs:isDefinedBy  <http://ns.inria.fr/ludo/v1/gamemodel#> ;
        rdfs:label        "Objects attribute"@en ;
        rdfs:subClassOf   owl:Thing ;
        ns1:term_status   "stable" .

<http://ns.inria.fr/ludo/v1/gamemodel#hasGameObjective>
        a                 owl:ObjectProperty ;
        rdfs:comment      "This property relates with a Game Objective. Can be used for Game Scenario and Inventory objects."@en ;
        rdfs:isDefinedBy  <http://ns.inria.fr/ludo/v1/gamemodel#> ;
        rdfs:label        "Has Game Objective"@en ;
        rdfs:range        <http://ns.inria.fr/ludo/v1/gamemodel#GameObjective> ;
        ns1:term_status   "stable" .

<http://ns.inria.fr/ludo/v1/gamemodel#hasURI>
        a                 owl:ObjectProperty ;
        rdfs:comment      "Uniform Resource Identifier"@en ;
        rdfs:isDefinedBy  <http://ns.inria.fr/ludo/v1/gamemodel#> ;
        rdfs:label        "URI"@en ;
        ns1:term_status   "stable" .

<http://ns.inria.fr/ludo/v1/gamemodel#hasInputEvent>
        a                 owl:ObjectProperty ;
        rdfs:comment      "Has Input Event"@en ;
        rdfs:domain       <http://ns.inria.fr/ludo/v1/gamemodel#GameControl> ;
        rdfs:isDefinedBy  <http://ns.inria.fr/ludo/v1/gamemodel#> ;
        rdfs:label        "Has Input Event"@en ;
        rdfs:range        <http://ns.inria.fr/ludo/v1/gamemodel#InputEvent> ;
        ns1:term_status   "stable" .

<http://ns.inria.fr/ludo/v1/gamemodel#hasArea>
        a                 owl:ObjectProperty ;
        rdfs:comment      "Relates an Area with any component to be represented graphically on the game screen, sucha as GUI components and Media components"@en ;
        rdfs:isDefinedBy  <http://ns.inria.fr/ludo/v1/gamemodel#> ;
        rdfs:label        "Has area"@en ;
        rdfs:range        <http://ns.inria.fr/ludo/v1/gamemodel#Area> ;
        ns1:term_status   "stable" .

[ a            owl:AllDisjointClasses ;
  owl:members  ( <http://ns.inria.fr/ludo/v1/gamemodel#CompleteGameStructure> <http://ns.inria.fr/ludo/v1/gamemodel#Presentation-basedStructure> <http://ns.inria.fr/ludo/v1/gamemodel#Scenario-basedStructure> <http://ns.inria.fr/ludo/v1/gamemodel#Training-basedStructure> )
] .

<http://ns.inria.fr/ludo/v1/gamemodel#hasGameKnowledgeBase>
        a                 owl:ObjectProperty ;
        rdfs:comment      "Has Game Knowledge-Base"@en ;
        rdfs:domain       <http://ns.inria.fr/ludo/v1/gamemodel#SeriousGame> ;
        rdfs:isDefinedBy  <http://ns.inria.fr/ludo/v1/gamemodel#> ;
        rdfs:label        "Has Game Knowledge-Base"@en ;
        rdfs:range        <http://ns.inria.fr/ludo/v1/gamemodel#GameKnowledgeBase> ;
        ns1:term_status   "stable" .

<http://ns.inria.fr/ludo/v1/gamemodel#GameActingScript>
        a                 owl:Class ;
        rdfs:comment      "Is composed by one or more acting coordination that instruct how a specific game object act in a defined sequence."@en ;
        rdfs:isDefinedBy  <http://ns.inria.fr/ludo/v1/gamemodel#> ;
        rdfs:label        "Game Acting Script"@en ;
        rdfs:subClassOf   owl:Thing ;
        ns1:term_status   "stable" .

[ a            owl:AllDisjointClasses ;
  owl:members  ( <http://ns.inria.fr/ludo/v1/gamemodel#InventoryState> <http://ns.inria.fr/ludo/v1/gamemodel#Mass> <http://ns.inria.fr/ludo/v1/gamemodel#SoidityState> )
] .

<http://ns.inria.fr/ludo/v1/gamemodel#hasGameAct>
        a                 owl:ObjectProperty ;
        rdfs:comment      "Has Game Act"@en ;
        rdfs:domain       <http://ns.inria.fr/ludo/v1/gamemodel#GameEvent> ;
        rdfs:isDefinedBy  <http://ns.inria.fr/ludo/v1/gamemodel#> ;
        rdfs:label        "Has Game Act"@en ;
        rdfs:range        <http://ns.inria.fr/ludo/v1/gamemodel#GameAct> ;
        ns1:term_status   "stable" .

<http://ns.inria.fr/ludo/v1/gamemodel#GameObjective>
        a                 owl:Class ;
        rdfs:comment      "Represents the goal associated to a game scenario"@en ;
        rdfs:isDefinedBy  <http://ns.inria.fr/ludo/v1/gamemodel#> ;
        rdfs:label        "Game Objective"@en ;
        rdfs:subClassOf   owl:Thing ;
        ns1:term_status   "stable" .

<http://ns.inria.fr/ludo/v1/gamemodel#hasGameActObject>
        a                 owl:ObjectProperty ;
        rdfs:comment      "Has Game Act Object"@en ;
        rdfs:domain       <http://ns.inria.fr/ludo/v1/gamemodel#GameAct> ;
        rdfs:isDefinedBy  <http://ns.inria.fr/ludo/v1/gamemodel#> ;
        rdfs:label        "Has Game Act Object"@en ;
        rdfs:range        <http://ns.inria.fr/ludo/v1/gamemodel#GameObject> ;
        ns1:term_status   "stable" .

<http://ns.inria.fr/ludo/v1/gamemodel#hasMatter>
        a                 owl:DatatypeProperty ;
        rdfs:comment      "Each game rule is paired with an outcome which has a matter and an operation to add or subtract a value from the matter. Matter in the context of game refers to an item, an attribute or permission."@en ;
        rdfs:domain       <http://ns.inria.fr/ludo/v1/gamemodel#GameInteractionRuleOutcome> ;
        rdfs:isDefinedBy  <http://ns.inria.fr/ludo/v1/gamemodel#> ;
        rdfs:label        "Interaction Rule Outcome Matter"@en ;
        rdfs:range        <http://www.w3.org/2001/XMLSchema#string> ;
        ns1:term_status   "stable" .

<http://ns.inria.fr/ludo/v1/gamemodel#Action>
        a                 owl:Class ;
        rdfs:comment      "The action of a game object, it consists of motion, animation, sound and vital updates."@en ;
        rdfs:isDefinedBy  <http://ns.inria.fr/ludo/v1/gamemodel#> ;
        rdfs:label        "Action"@en ;
        rdfs:subClassOf   owl:Thing ;
        ns1:term_status   "stable" .

<http://ns.inria.fr/ludo/v1/gamemodel#CompleteGameStructure>
        a                 owl:Class ;
        rdfs:comment      "Complete Game Structure"@en ;
        rdfs:isDefinedBy  <http://ns.inria.fr/ludo/v1/gamemodel#> ;
        rdfs:label        "Complete Game Structure"@en ;
        rdfs:subClassOf   <http://ns.inria.fr/ludo/v1/gamemodel#GameStructure> ;
        ns1:term_status   "stable" .

<http://ns.inria.fr/ludo/v1/gamemodel#hasAnimationType>
        a                 owl:DatatypeProperty ;
        rdfs:comment      "Defines the animation type, either 2D or 3D"@en ;
        rdfs:domain       <http://ns.inria.fr/ludo/v1/gamemodel#Animation> ;
        rdfs:isDefinedBy  <http://ns.inria.fr/ludo/v1/gamemodel#> ;
        rdfs:label        "Has Animation Type"@en ;
        rdfs:range        <http://www.w3.org/2001/XMLSchema#string> ;
        ns1:term_status   "stable" .

<http://ns.inria.fr/ludo/v1/gamemodel#hasSound>
        a                 owl:ObjectProperty ;
        rdfs:comment      "Has Sound"@en ;
        rdfs:domain       <http://ns.inria.fr/ludo/v1/gamemodel#Action> ;
        rdfs:isDefinedBy  <http://ns.inria.fr/ludo/v1/gamemodel#> ;
        rdfs:label        "Has Sound"@en ;
        rdfs:range        <http://ns.inria.fr/ludo/v1/gamemodel#Sound> ;
        ns1:term_status   "stable" .

<http://ns.inria.fr/ludo/v1/gamemodel#Constraint>
        a                 owl:Class ;
        rdfs:comment      "External forces"@en ;
        rdfs:isDefinedBy  <http://ns.inria.fr/ludo/v1/gamemodel#> ;
        rdfs:label        "Constraint"@en ;
        rdfs:subClassOf   owl:Thing ;
        ns1:term_status   "stable" .

<http://ns.inria.fr/ludo/v1/gamemodel#Motion>
        a                 owl:Class ;
        rdfs:comment      "Motion refers to the actual translation of game object position in the game world. A motion is subject to a force and also constraints (external force)."@en ;
        rdfs:isDefinedBy  <http://ns.inria.fr/ludo/v1/gamemodel#> ;
        rdfs:label        "Motion"@en ;
        rdfs:subClassOf   owl:Thing ;
        ns1:term_status   "stable" .

<http://ns.inria.fr/ludo/v1/gamemodel#GameStructure>
        a                 owl:Class ;
        rdfs:comment      "Describes the architecture and flow of the game. It segments game into game sections. A game section is composed of a game context, pedagogic event indicator and event trigger."@en ;
        rdfs:isDefinedBy  <http://ns.inria.fr/ludo/v1/gamemodel#> ;
        rdfs:label        "Game Structure"@en ;
        rdfs:subClassOf   owl:Thing ;
        ns1:term_status   "stable" .

<http://ns.inria.fr/ludo/v1/gamemodel#hasPedagogicEventIndicator>
        a                 owl:ObjectProperty , owl:FunctionalProperty ;
        rdfs:comment      "Has Pedagogic Event Indicator"@en ;
        rdfs:domain       <http://ns.inria.fr/ludo/v1/gamemodel#GameStructure> ;
        rdfs:isDefinedBy  <http://ns.inria.fr/ludo/v1/gamemodel#> ;
        rdfs:label        "Has Pedagogic Event Indicator"@en ;
        rdfs:range        <http://ns.inria.fr/ludo/v1/gamemodel#PedagogicEventIndicator> ;
        ns1:term_status   "stable" .

[ a            owl:AllDisjointClasses ;
  owl:members  ( <http://ns.inria.fr/ludo/v1/gamemodel#DecidingCondition> <http://ns.inria.fr/ludo/v1/gamemodel#Learn> <http://ns.inria.fr/ludo/v1/gamemodel#Navigate> )
] .

<http://ns.inria.fr/ludo/v1/gamemodel#hasGameResult>
        a                 owl:ObjectProperty ;
        rdfs:comment      "Has Game Result"@en ;
        rdfs:domain       <http://ns.inria.fr/ludo/v1/gamemodel#GameRecord> ;
        rdfs:isDefinedBy  <http://ns.inria.fr/ludo/v1/gamemodel#> ;
        rdfs:label        "Has Game Result"@en ;
        rdfs:range        <http://ns.inria.fr/ludo/v1/gamemodel#GameResult> ;
        ns1:term_status   "stable" .

<http://ns.inria.fr/ludo/v1/gamemodel#hasGameScenario>
        a                 owl:ObjectProperty ;
        rdfs:comment      "Has Game Scenario"@en ;
        rdfs:domain       <http://ns.inria.fr/ludo/v1/gamemodel#GameSimulation> ;
        rdfs:isDefinedBy  <http://ns.inria.fr/ludo/v1/gamemodel#> ;
        rdfs:label        "Has Game Scenario"@en ;
        rdfs:range        <http://ns.inria.fr/ludo/v1/gamemodel#GameScenario> ;
        ns1:term_status   "stable" .

<http://ns.inria.fr/ludo/v1/gamemodel#hasGameTempo>
        a                 owl:ObjectProperty ;
        rdfs:comment      "Has Game Tempo"@en ;
        rdfs:domain       <http://ns.inria.fr/ludo/v1/gamemodel#GameSimulation> ;
        rdfs:isDefinedBy  <http://ns.inria.fr/ludo/v1/gamemodel#> ;
        rdfs:label        "Has Game Tempo"@en ;
        rdfs:range        <http://ns.inria.fr/ludo/v1/gamemodel#GameTempo> ;
        ns1:term_status   "stable" .

<http://ns.inria.fr/ludo/v1/gamemodel#hasPedagogicEvent>
        a                 owl:DatatypeProperty ;
        rdfs:comment      "Associates each game section with one or more pedagogic events from the Gagne's nine events of instructions. These events ordered in sequence are (1) gaining attention, (2) informing learning objectives, (3) recalling prior learning, (4) presenting learning content, (5) providing learning guidance, (6) eliciting performance, (7) provide feedback, (8) assess performance and, (9) enhance retention and transfer."@en ;
        rdfs:domain       <http://ns.inria.fr/ludo/v1/gamemodel#PedagogicEventIndicator> ;
        rdfs:isDefinedBy  <http://ns.inria.fr/ludo/v1/gamemodel#> ;
        rdfs:label        "Pedagogic Event"@en ;
        rdfs:range        <http://www.w3.org/2001/XMLSchema#string> ;
        ns1:term_status   "stable" .

<http://ns.inria.fr/ludo/v1/gamemodel#hasInventoryQuantity>
        a                 owl:DatatypeProperty ;
        rdfs:comment      "Has inventory quantity"@en ;
        rdfs:domain       <http://ns.inria.fr/ludo/v1/gamemodel#InventoryState> ;
        rdfs:isDefinedBy  <http://ns.inria.fr/ludo/v1/gamemodel#> ;
        rdfs:label        "Has inventory quantity"@en ;
        rdfs:range        <http://www.w3.org/2001/XMLSchema#integer> ;
        ns1:term_status   "stable" .

<http://ns.inria.fr/ludo/v1/gamemodel#SeriousGame>
        a                 owl:Class ;
        rdfs:comment      "Serious Game"@en ;
        rdfs:isDefinedBy  <http://ns.inria.fr/ludo/v1/gamemodel#> ;
        rdfs:label        "Serious Game"@en ;
        rdfs:subClassOf   owl:Thing ;
        ns1:term_status   "stable" .

<http://ns.inria.fr/ludo/v1/gamemodel#hasDifficultyIndicatorValue>
        a                 owl:DatatypeProperty ;
        rdfs:comment      "Has difficulty indicator value"@en ;
        rdfs:domain       <http://ns.inria.fr/ludo/v1/gamemodel#DifficultyIndicator> ;
        rdfs:isDefinedBy  <http://ns.inria.fr/ludo/v1/gamemodel#> ;
        rdfs:label        "Difficulty"@en ;
        rdfs:range        <http://www.w3.org/2001/XMLSchema#integer> ;
        ns1:term_status   "stable" .

<http://ns.inria.fr/ludo/v1/gamemodel#hasText>
        a                 owl:DatatypeProperty ;
        rdfs:comment      "Has text"@en ;
        rdfs:isDefinedBy  <http://ns.inria.fr/ludo/v1/gamemodel#> ;
        rdfs:label        "Has text"@en ;
        rdfs:range        <http://www.w3.org/2001/XMLSchema#string> ;
        ns1:term_status   "stable" .

<http://ns.inria.fr/ludo/v1/gamemodel#hasInteractionRuleOutcome>
        a                 owl:ObjectProperty ;
        rdfs:comment      "Interaction Rule Outcome"@en ;
        rdfs:domain       <http://ns.inria.fr/ludo/v1/gamemodel#GameInteractionRule> ;
        rdfs:isDefinedBy  <http://ns.inria.fr/ludo/v1/gamemodel#> ;
        rdfs:label        "Interaction Rule Outcome"@en ;
        rdfs:range        <http://ns.inria.fr/ludo/v1/gamemodel#GameInteractionRuleOutcome> ;
        ns1:term_status   "stable" .

<http://ns.inria.fr/ludo/v1/gamemodel#RawResult>
        a                 owl:Class ;
        rdfs:comment      "Raw result"@en ;
        rdfs:isDefinedBy  <http://ns.inria.fr/ludo/v1/gamemodel#> ;
        rdfs:label        "Raw result"@en ;
        rdfs:subClassOf   <http://ns.inria.fr/ludo/v1/gamemodel#GameResult> ;
        ns1:term_status   "stable" .

<http://ns.inria.fr/ludo/v1/gamemodel#hasGamePlayer>
        a                 owl:ObjectProperty ;
        rdfs:comment      "Has Game Player"@en ;
        rdfs:domain       <http://ns.inria.fr/ludo/v1/gamemodel#SeriousGame> ;
        rdfs:isDefinedBy  <http://ns.inria.fr/ludo/v1/gamemodel#> ;
        rdfs:label        "Has Game Player"@en ;
        rdfs:range        <http://ns.inria.fr/ludo/v1/gamemodel#GamePlayer> ;
        ns1:term_status   "stable" .

<http://ns.inria.fr/ludo/v1/gamemodel#hasEventTrigger>
        a                 owl:ObjectProperty ;
        rdfs:comment      "The property to relate a Game Structure or a Game Event with an Event Trigger"@en ;
        rdfs:isDefinedBy  <http://ns.inria.fr/ludo/v1/gamemodel#> ;
        rdfs:label        "Has event trigger"@en ;
        rdfs:range        <http://ns.inria.fr/ludo/v1/gamemodel#EventTrigger> ;
        ns1:term_status   "stable" .

<http://ns.inria.fr/ludo/v1/gamemodel>
        a       owl:Ontology .

<http://ns.inria.fr/ludo/v1/gamemodel#GamePhysics>
        a                 owl:Class ;
        rdfs:comment      "Defines the physicality of the game world. It encompasses the collision world and environment forces."@en ;
        rdfs:isDefinedBy  <http://ns.inria.fr/ludo/v1/gamemodel#> ;
        rdfs:label        "Game Physics"@en ;
        rdfs:subClassOf   owl:Thing ;
        ns1:term_status   "stable" .

<http://ns.inria.fr/ludo/v1/gamemodel#hasInteractionRuleSubject>
        a                 owl:ObjectProperty ;
        rdfs:comment      "Interaction Rule Subject"@en ;
        rdfs:domain       <http://ns.inria.fr/ludo/v1/gamemodel#GameInteractionRule> ;
        rdfs:isDefinedBy  <http://ns.inria.fr/ludo/v1/gamemodel#> ;
        rdfs:label        "Interaction Rule Subject"@en ;
        rdfs:range        <http://ns.inria.fr/ludo/v1/gamemodel#GameObject> ;
        ns1:term_status   "stable" .

<http://ns.inria.fr/ludo/v1/gamemodel#hasDifficultyIndicator>
        a                 owl:ObjectProperty ;
        rdfs:comment      "Has difficulty indicator"@en ;
        rdfs:domain       <http://ns.inria.fr/ludo/v1/gamemodel#GameScenario> ;
        rdfs:isDefinedBy  <http://ns.inria.fr/ludo/v1/gamemodel#> ;
        rdfs:label        "Has difficulty indicator"@en ;
        rdfs:range        <http://ns.inria.fr/ludo/v1/gamemodel#DifficultyIndicator> ;
        ns1:term_status   "stable" .

<http://ns.inria.fr/ludo/v1/gamemodel#hasInteractionRuleActor>
        a                 owl:ObjectProperty ;
        rdfs:comment      "Interaction Rule Actor"@en ;
        rdfs:domain       <http://ns.inria.fr/ludo/v1/gamemodel#GameInteractionRule> ;
        rdfs:isDefinedBy  <http://ns.inria.fr/ludo/v1/gamemodel#> ;
        rdfs:label        "Interaction Rule Actor"@en ;
        rdfs:range        <http://ns.inria.fr/ludo/v1/gamemodel#GameObject> ;
        ns1:term_status   "stable" .

<http://ns.inria.fr/ludo/v1/gamemodel#hasNormalForce>
        a                 owl:DatatypeProperty ;
        rdfs:comment      "The normal force"@en ;
        rdfs:domain       <http://ns.inria.fr/ludo/v1/gamemodel#Force> ;
        rdfs:isDefinedBy  <http://ns.inria.fr/ludo/v1/gamemodel#> ;
        rdfs:label        "Normal force"@en ;
        rdfs:range        <http://www.w3.org/2001/XMLSchema#float> ;
        ns1:term_status   "stable" .

<http://ns.inria.fr/ludo/v1/gamemodel#hasGameAttribute>
        a                 owl:ObjectProperty ;
        rdfs:comment      "Has Game Attribute"@en ;
        rdfs:isDefinedBy  <http://ns.inria.fr/ludo/v1/gamemodel#> ;
        rdfs:label        "Has Game Attribute"@en ;
        ns1:term_status   "stable" .

<http://ns.inria.fr/ludo/v1/gamemodel#hasGameRule>
        a                 owl:ObjectProperty ;
        rdfs:comment      "This property relates a Game Simulation with a Game Rule"@en ;
        rdfs:domain       <http://ns.inria.fr/ludo/v1/gamemodel#GameSimulation> ;
        rdfs:isDefinedBy  <http://ns.inria.fr/ludo/v1/gamemodel#> ;
        rdfs:label        "Has Game Rule"@en ;
        rdfs:range        <http://ns.inria.fr/ludo/v1/gamemodel#GameRule> ;
        ns1:term_status   "stable" .

<http://ns.inria.fr/ludo/v1/gamemodel#ObjectImage>
        a                 owl:Class ;
        rdfs:comment      "The object image is represented using one or more image components"@en ;
        rdfs:isDefinedBy  <http://ns.inria.fr/ludo/v1/gamemodel#> ;
        rdfs:label        "Object Image"@en ;
        rdfs:subClassOf   <http://ns.inria.fr/ludo/v1/gamemodel#Appearance> ;
        ns1:term_status   "stable" .

<http://ns.inria.fr/ludo/v1/gamemodel#hasTempoScale>
        a                 owl:DatatypeProperty ;
        rdfs:comment      "The tempo scale at which the time is passing. This can be used for slow motion effects. When timeScale is 1.0 the time is passing as fast as realtime. When timeScale is 0.5 the time is passing 2x slower than realtime. When timeScale is set to zero the game is basically paused if all your functions are frame rate independent.y. Based on: http://docs.unity3d.com/ScriptReference/Time-timeScale.html"@en ;
        rdfs:domain       <http://ns.inria.fr/ludo/v1/gamemodel#GameTempo> ;
        rdfs:isDefinedBy  <http://ns.inria.fr/ludo/v1/gamemodel#> ;
        rdfs:label        "Game tempo scale"@en ;
        rdfs:range        <http://www.w3.org/2001/XMLSchema#double> ;
        ns1:term_status   "stable" .

<http://ns.inria.fr/ludo/v1/gamemodel#ObjectAttribute>
        a                 owl:Class ;
        rdfs:comment      "Data properties that represent a game objects vitality, physical being, cognitive state and ownership"@en ;
        rdfs:isDefinedBy  <http://ns.inria.fr/ludo/v1/gamemodel#> ;
        rdfs:label        "Object Atrribute"@en ;
        rdfs:subClassOf   owl:Thing ;
        ns1:term_status   "stable" .

<http://ns.inria.fr/ludo/v1/gamemodel#hasEventTriggerCommand>
        a                 owl:DatatypeProperty ;
        rdfs:comment      "Has Event trigger command"@en ;
        rdfs:domain       <http://ns.inria.fr/ludo/v1/gamemodel#EventTrigger> ;
        rdfs:isDefinedBy  <http://ns.inria.fr/ludo/v1/gamemodel#> ;
        rdfs:label        "Has Event trigger command"@en ;
        rdfs:range        <http://www.w3.org/2001/XMLSchema#string> ;
        ns1:term_status   "stable" .

<http://ns.inria.fr/ludo/v1/gamemodel#hasGameRecord>
        a                 owl:ObjectProperty ;
        rdfs:comment      "Has Game Record"@en ;
        rdfs:domain       <http://ns.inria.fr/ludo/v1/gamemodel#GamePlayer> ;
        rdfs:isDefinedBy  <http://ns.inria.fr/ludo/v1/gamemodel#> ;
        rdfs:label        "Has Game Record"@en ;
        rdfs:range        <http://ns.inria.fr/ludo/v1/gamemodel#GameRecord> ;
        ns1:term_status   "stable" .

<http://ns.inria.fr/ludo/v1/gamemodel#hasGameControl>
        a                 owl:ObjectProperty ;
        rdfs:comment      "Has Game Control"@en ;
        rdfs:domain       <http://ns.inria.fr/ludo/v1/gamemodel#GamePlayer> ;
        rdfs:isDefinedBy  <http://ns.inria.fr/ludo/v1/gamemodel#> ;
        rdfs:label        "Has Game Control"@en ;
        rdfs:range        <http://ns.inria.fr/ludo/v1/gamemodel#GameControl> ;
        ns1:term_status   "stable" .

<http://dbpedia.org/resource/National_Institute_for_Research_in_Computer_Science_and_Control>
        a       foaf:Organization .

<http://ns.inria.fr/ludo/v1/gamemodel#GameAct>
        a                 owl:Class ;
        rdfs:comment      "The performance of a game object in a game event. It consists of a game object and a game acting script that describe how the game object should move, animate, sound and interact with other game object in a game scenario."@en ;
        rdfs:isDefinedBy  <http://ns.inria.fr/ludo/v1/gamemodel#> ;
        rdfs:label        "Game Act"@en ;
        rdfs:subClassOf   owl:Thing ;
        ns1:term_status   "stable" .

[ a            owl:AllDisjointClasses ;
  owl:members  ( <http://ns.inria.fr/ludo/v1/gamemodel#Action> <http://ns.inria.fr/ludo/v1/gamemodel#Appearance> <http://ns.inria.fr/ludo/v1/gamemodel#Intelligence> )
] .

<http://ns.inria.fr/ludo/v1/gamemodel#hasGoalConditionDescription>
        a                 owl:DatatypeProperty ;
        rdfs:comment      "The description of the goal condition"@en ;
        rdfs:domain       <http://ns.inria.fr/ludo/v1/gamemodel#GoalCondition> ;
        rdfs:isDefinedBy  <http://ns.inria.fr/ludo/v1/gamemodel#> ;
        rdfs:label        "Goal Condition description"@en ;
        rdfs:range        rdfs:Literal ;
        ns1:term_status   "stable" .

<http://www.oscarrodriguez.me>
        a       foaf:Person .

<http://ns.inria.fr/ludo/v1/gamemodel#hasGameContext>
        a                 owl:ObjectProperty ;
        rdfs:comment      "Has Game Context"@en ;
        rdfs:domain       <http://ns.inria.fr/ludo/v1/gamemodel#GameStructure> ;
        rdfs:isDefinedBy  <http://ns.inria.fr/ludo/v1/gamemodel#> ;
        rdfs:label        "Has Game Context"@en ;
        rdfs:range        <http://ns.inria.fr/ludo/v1/gamemodel#GameContext> ;
        ns1:term_status   "stable" .

<http://ns.inria.fr/ludo/v1/gamemodel#GameControlInterface>
        a                 owl:Class ;
        rdfs:comment      "Game Control Interface"@en ;
        rdfs:isDefinedBy  <http://ns.inria.fr/ludo/v1/gamemodel#> ;
        rdfs:label        "Game Control Interface"@en ;
        rdfs:subClassOf   owl:Thing ;
        owl:disjointWith  <http://ns.inria.fr/ludo/v1/gamemodel#InputEvent> ;
        ns1:term_status   "stable" .

<http://ns.inria.fr/ludo/v1/gamemodel#ObjectVitality>
        a                 owl:Class ;
        rdfs:comment      "Vitality of an object such as life or interrelated attributes such as health, energy, strength, social and etc."@en ;
        rdfs:isDefinedBy  <http://ns.inria.fr/ludo/v1/gamemodel#> ;
        rdfs:label        "Object Vitality"@en ;
        rdfs:subClassOf   <http://ns.inria.fr/ludo/v1/gamemodel#ObjectAttribute> ;
        ns1:term_status   "stable" .

<http://ns.inria.fr/ludo/v1/gamemodel#GameResult>
        a                 owl:Class ;
        rdfs:comment      "Game Result"@en ;
        rdfs:isDefinedBy  <http://ns.inria.fr/ludo/v1/gamemodel#> ;
        rdfs:label        "Game Result"@en ;
        rdfs:subClassOf   owl:Thing ;
        ns1:term_status   "stable" .

<http://ns.inria.fr/ludo/v1/gamemodel#GameRule>
        a                 owl:Class ;
        rdfs:comment      "States the relationship between game objects and game world, and the effect of an interaction. It can either be a Game Scoring Rule or Game Interaction Rule."@en ;
        rdfs:isDefinedBy  <http://ns.inria.fr/ludo/v1/gamemodel#> ;
        rdfs:label        "Game Rule"@en ;
        rdfs:subClassOf   owl:Thing ;
        ns1:term_status   "stable" .

<http://ns.inria.fr/ludo/v1/gamemodel#GameDimension>
        a                 owl:Class ;
        rdfs:comment      "Represents the virtual space in which the game simulation takes place in 2D or 3D."@en ;
        rdfs:isDefinedBy  <http://ns.inria.fr/ludo/v1/gamemodel#> ;
        rdfs:label        "Game Dimension"@en ;
        rdfs:subClassOf   owl:Thing ;
        ns1:term_status   "stable" .

[ a            owl:AllDisjointClasses ;
  owl:members  ( <http://ns.inria.fr/ludo/v1/gamemodel#GameDimension> <http://ns.inria.fr/ludo/v1/gamemodel#GamePhysics> <http://ns.inria.fr/ludo/v1/gamemodel#GameTempo> )
] .

<http://ns.inria.fr/ludo/v1/gamemodel#hasVitalUpdate>
        a                 owl:DatatypeProperty ;
        rdfs:comment      "Has Vital Update"@en ;
        rdfs:domain       <http://ns.inria.fr/ludo/v1/gamemodel#Action> ;
        rdfs:isDefinedBy  <http://ns.inria.fr/ludo/v1/gamemodel#> ;
        rdfs:label        "Has Vital Update"@en ;
        rdfs:range        <http://www.w3.org/2001/XMLSchema#double> ;
        ns1:term_status   "stable" .

<http://ns.inria.fr/ludo/v1/gamemodel#hasScoringCondition>
        a                 owl:DatatypeProperty ;
        rdfs:comment      "Every game scoring rule has a scoring condition which has no direct relation with interaction. It can be derived from the state of a game object (e.g. enemy is dead or fire is extinguished), the input statistics (e.g. accuracy is above 80%), the time (e.g. respond is less than 5 seconds or level completed in less than 5 minutes), or the game objective (e.g. objective 1, 2 and 5 are met)."@en ;
        rdfs:domain       <http://ns.inria.fr/ludo/v1/gamemodel#GameScoringRule> ;
        rdfs:isDefinedBy  <http://ns.inria.fr/ludo/v1/gamemodel#> ;
        rdfs:label        "Scoring Condition"@en ;
        rdfs:range        <http://www.w3.org/2001/XMLSchema#string> ;
        ns1:term_status   "stable" .

<http://ns.inria.fr/ludo/v1/gamemodel#GameTempo>
        a                 owl:Class ;
        rdfs:comment      "Represents the realtion between the pace of the time in a game and the time in the real world."@en ;
        rdfs:isDefinedBy  <http://ns.inria.fr/ludo/v1/gamemodel#> ;
        rdfs:label        "Game Tempo"@en ;
        rdfs:subClassOf   owl:Thing ;
        ns1:term_status   "stable" .

<http://ns.inria.fr/ludo/v1/gamemodel#hasGameEnvironment>
        a                 owl:ObjectProperty ;
        rdfs:comment      "Has Game Environment"@en ;
        rdfs:domain       <http://ns.inria.fr/ludo/v1/gamemodel#GameScenario> ;
        rdfs:isDefinedBy  <http://ns.inria.fr/ludo/v1/gamemodel#> ;
        rdfs:label        "Has Game Environment"@en ;
        rdfs:range        <http://ns.inria.fr/ludo/v1/gamemodel#GameEnvironment> ;
        ns1:term_status   "stable" .

<http://ns.inria.fr/ludo/v1/gamemodel#Presentation-basedStructure>
        a                 owl:Class ;
        rdfs:comment      "Presentation-based Structure"@en ;
        rdfs:isDefinedBy  <http://ns.inria.fr/ludo/v1/gamemodel#> ;
        rdfs:label        "Presentation-based Structure"@en ;
        rdfs:subClassOf   <http://ns.inria.fr/ludo/v1/gamemodel#GameStructure> ;
        ns1:term_status   "stable" .

<http://ns.inria.fr/ludo/v1/gamemodel#isSolid>
        a                 owl:DatatypeProperty ;
        rdfs:comment      "Solidity"@en ;
        rdfs:domain       <http://ns.inria.fr/ludo/v1/gamemodel#SoidityState> ;
        rdfs:isDefinedBy  <http://ns.inria.fr/ludo/v1/gamemodel#> ;
        rdfs:label        "Solidity"@en ;
        rdfs:range        <http://www.w3.org/2001/XMLSchema#boolean> ;
        ns1:term_status   "stable" .

<http://ns.inria.fr/ludo/v1/gamemodel#GoalCondition>
        a                 owl:Class ;
        rdfs:comment      "The goal condition checks a track-able value against a constant value defined by the game designer to determine if the game objective has been met or not. The game objective is marked as achieve once the goal condition has been satisfied."@en ;
        rdfs:isDefinedBy  <http://ns.inria.fr/ludo/v1/gamemodel#> ;
        rdfs:label        "Goal Condition"@en ;
        rdfs:subClassOf   owl:Thing ;
        ns1:term_status   "stable" .

<http://ns.inria.fr/ludo/v1/gamemodel#hasHardwareInterface>
        a                 owl:DatatypeProperty ;
        rdfs:comment      "Examples of hardware interface include keyboard, mouse, gamepad, joystick, motionsensor, camera and microphone."@en ;
        rdfs:domain       <http://ns.inria.fr/ludo/v1/gamemodel#GameControlInterface> ;
        rdfs:isDefinedBy  <http://ns.inria.fr/ludo/v1/gamemodel#> ;
        rdfs:label        "Has hardware Interface"@en ;
        rdfs:range        <http://www.w3.org/2001/XMLSchema#string> ;
        ns1:term_status   "stable" .

<http://ns.inria.fr/ludo/v1/gamemodel#hasForce>
        a                 owl:ObjectProperty ;
        rdfs:comment      "Has force"@en ;
        rdfs:domain       <http://ns.inria.fr/ludo/v1/gamemodel#Motion> ;
        rdfs:isDefinedBy  <http://ns.inria.fr/ludo/v1/gamemodel#> ;
        rdfs:label        "Has force"@en ;
        rdfs:range        <http://ns.inria.fr/ludo/v1/gamemodel#Force> ;
        ns1:term_status   "stable" .

<http://ns.inria.fr/ludo/v1/gamemodel#Vital>
        a                 owl:Class ;
        rdfs:comment      "Game designers can choose to represent the game object using a single vital definition such as life or further elaborate the vitality of a game object into interrelated attributes such as health, energy, strength, social and etc. "@en ;
        rdfs:isDefinedBy  <http://ns.inria.fr/ludo/v1/gamemodel#> ;
        rdfs:label        "Vital"@en ;
        rdfs:subClassOf   <http://ns.inria.fr/ludo/v1/gamemodel#GameAttribute> ;
        ns1:term_status   "stable" .

<http://ns.inria.fr/ludo/v1/gamemodel#hasAnimation>
        a                 owl:ObjectProperty ;
        rdfs:comment      "Has animation"@en ;
        rdfs:domain       <http://ns.inria.fr/ludo/v1/gamemodel#Action> ;
        rdfs:isDefinedBy  <http://ns.inria.fr/ludo/v1/gamemodel#> ;
        rdfs:label        "Has animation"@en ;
        rdfs:range        <http://ns.inria.fr/ludo/v1/gamemodel#Animation> ;
        ns1:term_status   "stable" .

<http://ns.inria.fr/ludo/v1/gamemodel#hasFrontEndDisplay>
        a                 owl:ObjectProperty ;
        rdfs:comment      "Has front end display"@en ;
        rdfs:domain       <http://ns.inria.fr/ludo/v1/gamemodel#GameSimulation> ;
        rdfs:isDefinedBy  <http://ns.inria.fr/ludo/v1/gamemodel#> ;
        rdfs:label        "Has front end display"@en ;
        rdfs:range        <http://ns.inria.fr/ludo/v1/gamepresentation#FrontEndDisplay> ;
        ns1:term_status   "stable" .

<http://ns.inria.fr/ludo/v1/gamemodel#hasGameEvent>
        a                 owl:ObjectProperty ;
        rdfs:comment      "Has Game Event"@en ;
        rdfs:domain       <http://ns.inria.fr/ludo/v1/gamemodel#GameScenario> ;
        rdfs:isDefinedBy  <http://ns.inria.fr/ludo/v1/gamemodel#> ;
        rdfs:label        "Has Game Event"@en ;
        rdfs:range        <http://ns.inria.fr/ludo/v1/gamemodel#GameEvent> ;
        ns1:term_status   "stable" .

<http://ns.inria.fr/ludo/v1/gamemodel#GamePlayer>
        a                 owl:Class ;
        rdfs:comment      "The user of the game application who provides inputs to the game system as part of the gaming activity."@en ;
        rdfs:isDefinedBy  <http://ns.inria.fr/ludo/v1/gamemodel#> ;
        rdfs:label        "Game Player"@en ;
        rdfs:subClassOf   foaf:Person ;
        ns1:term_status   "stable" .

<http://ns.inria.fr/ludo/v1/gamemodel#Checkbox>
        a                 owl:Class ;
        rdfs:comment      "Checkbox"@en ;
        rdfs:isDefinedBy  <http://ns.inria.fr/ludo/v1/gamemodel#> ;
        rdfs:label        "Checkbox"@en ;
        rdfs:subClassOf   owl:Thing , <http://ns.inria.fr/ludo/v1/gamemodel#GUIComponent> ;
        ns1:term_status   "stable" .

<http://ns.inria.fr/ludo/v1/gamemodel#hasGameControlInterface>
        a             owl:ObjectProperty ;
        rdfs:comment  "Has Game Control Interface"@en ;
        rdfs:domain   <http://ns.inria.fr/ludo/v1/gamemodel#GameControl> ;
        rdfs:label    "Has Game Control Interface"@en ;
        rdfs:range    <http://ns.inria.fr/ludo/v1/gamemodel#GameControlInterface> .

<http://ns.inria.fr/ludo/v1/gamemodel#Score>
        a                 owl:Class ;
        rdfs:comment      "Score"@en ;
        rdfs:isDefinedBy  <http://ns.inria.fr/ludo/v1/gamemodel#> ;
        rdfs:label        "Score"@en ;
        rdfs:subClassOf   <http://ns.inria.fr/ludo/v1/gamemodel#GameAttribute> ;
        owl:disjointWith  <http://ns.inria.fr/ludo/v1/gamemodel#Vital> ;
        ns1:term_status   "stable" .

<http://ns.inria.fr/ludo/v1/gamemodel#hasVirtualCamera>
        a                 owl:ObjectProperty ;
        rdfs:comment      "Has Virtual Camera"@en ;
        rdfs:domain       <http://ns.inria.fr/ludo/v1/gamemodel#GameScenario> ;
        rdfs:isDefinedBy  <http://ns.inria.fr/ludo/v1/gamemodel#> ;
        rdfs:label        "Has Virtual Camera"@en ;
        rdfs:range        <http://ns.inria.fr/ludo/v1/gamemodel#VirtualCamera> ;
        ns1:term_status   "stable" .

<http://ns.inria.fr/ludo/v1/gamemodel#ComputedResult>
        a                 owl:Class ;
        rdfs:comment      "Computed result"@en ;
        rdfs:isDefinedBy  <http://ns.inria.fr/ludo/v1/gamemodel#> ;
        rdfs:label        "Computed result"@en ;
        rdfs:subClassOf   <http://ns.inria.fr/ludo/v1/gamemodel#GameResult> ;
        owl:disjointWith  <http://ns.inria.fr/ludo/v1/gamemodel#RawResult> ;
        ns1:term_status   "stable" .

<http://ns.inria.fr/ludo/v1/gamemodel#hasGameDimention>
        a                 owl:ObjectProperty ;
        rdfs:comment      "Has Game Dimention"@en ;
        rdfs:domain       <http://ns.inria.fr/ludo/v1/gamemodel#GameSimulation> ;
        rdfs:isDefinedBy  <http://ns.inria.fr/ludo/v1/gamemodel#> ;
        rdfs:label        "Has Game Dimention"@en ;
        rdfs:range        <http://ns.inria.fr/ludo/v1/gamemodel#GameDimension> ;
        ns1:term_status   "stable" .
