@prefix owl: <http://www.w3.org/2002/07/owl#> .
@prefix dc: <http://purl.org/dc/terms/> .
@prefix xsd: <http://www.w3.org/2001/XMLSchema#> .
@prefix ns0: <http://purl.org/vocab/vann/> .
@prefix cc: <http://creativecommons.org/ns#> .
@prefix rdfs: <http://www.w3.org/2000/01/rdf-schema#> .
@prefix foaf: <http://xmlns.com/foaf/0.1/> .

<http://data.ign.fr/def/ignf>
  a owl:Ontology, <http://purl.org/vocommons/voaf#Vocabulary> ;
  dc:description "Codes pour la description de systÃƒÂ¨mes de coordonnÃƒÂ©es de rÃƒÂ©fÃƒÂ©rence conforme ISO TC/211. Les traductions franÃƒÂ§aises des termes et leurs dÃƒÂ©finitions sont pour la plupart issues du glossaire multilingue ISO/TC 211 disponible ici: http://www.isotc211.org/Terminology.htm"@fr, "Codes for describing coordinates reference systems consistently with ISO TC/211. French translations of terms and definitions are mainly taken from the multilingual glossary of ISO/TC 211 available online: http://www.isotc211.org/Terminology.htm"@en ;
  dc:title "Ontologie des systÃƒÂ¨mes de coordonnÃƒÂ©es de rÃƒÂ©fÃƒÂ©rence"@fr, "Ontology of coordinates reference systems"@en ;
  dc:creator <http://recherche.ign.fr/labos/cogit/cv.php?prenom=Nathalie&nom=Abadie>, <http://www.eurecom.fr/~atemezin/> ;
  dc:contributor <http://www.eurecom.fr/~troncy/> ;
  dc:issued "2013-06-11"^^xsd:date ;
  dc:modified "2014-04-09"^^xsd:date, "2015-05-05"^^xsd:date ;
  dc:publisher <http://fr.dbpedia.org/resource/Institut_national_de_l%27information_g%C3%A9ographique_et_foresti%C3%A8re> ;
  dc:rights "Copyright 2014, IGN" ;
  ns0:preferredNamespacePrefix "ignf" ;
  ns0:preferredNamespaceUri <http://data.ign.fr/def/ignf#> ;
  cc:license <http://www.data.gouv.fr/Licence-Ouverte-Open-Licence>, <http://creativecommons.org/licenses/by/2.0/>, <http://opendatacommons.org/licenses/by/> ;
  rdfs:seeAlso <http://librairies.ignf.fr/geoportail/resources/IGNF.xml> ;
  owl:priorVersion <http://data.ign.fr/def/ignf/20140409.ttl> ;
  owl:versionInfo "Version 2.0 - 2015-05-05" .

<http://www.eurecom.fr/~atemezin/> a foaf:Person .
<http://www.eurecom.fr/~troncy/> a foaf:Person .
<http://recherche.ign.fr/labos/cogit/cv.php?prenom=Nathalie&nom=Abadie> a foaf:Person .
<http://data.ign.fr/def/ignf#CRS>
  a owl:Class ;
  rdfs:label "Coordinate reference system (CRS)"@en, "SystÃƒÂ¨me de coordonnÃƒÂ©es de rÃƒÂ©fÃƒÂ©rence"@fr ;
  rdfs:comment "MÃƒÂ©tadonnÃƒÂ©es permettant de prÃƒÂ©ciser, selon la dimension spatiale des coordonnÃƒÂ©es 1D, 2D ou 3D, les ÃƒÂ©lÃƒÂ©ments de dÃƒÂ©finition associÃƒÂ©s au jeu de coordonnÃƒÂ©es: le systÃƒÂ¨me de rÃƒÂ©fÃƒÂ©rence terrestre, l'ellipsoÃƒÂ¯de gÃƒÂ©odÃƒÂ©sique, le mÃƒÂ©ridien origine, le type de coordonnÃƒÂ©es (cartÃƒÂ©siennes gÃƒÂ©ocentriques, planes, gÃƒÂ©ographiques,...), les unitÃƒÂ©s dans lesquelles sont exprimÃƒÂ©es les coordonnÃƒÂ©es, la projection cartographique, le rÃƒÂ©fÃƒÂ©rentiel altimÃƒÂ©trique(http://geodesie.ign.fr/index.php?page=glossaire). Cf. ISO 19111:2007:2007-07, partie 8.2, tableau 4 et annexe B.1."@fr, "Depending on the spatial dimension of coordinates (1D, 2D, 3D), this piece of metadata is used for specifying the elements of definition associated to a given set of coordinates: its datum, its ellipsoid, its prime meridian, the type of coordinates (geocentric, geographic, projected,...), the coordinates units of measure, when appropriate the cartographic projection used, the vertical coordinate reference system. Definition translated from: http://geodesie.ign.fr/index.php?page=glossaire. Cf. ISO 19111:2007:2007-07, part 8.2, table 4 and annex B.1."@en ;
  rdfs:subClassOf [
    a owl:Restriction ;
    owl:someValuesFrom <http://data.ign.fr/def/ignf#Extent> ;
    owl:onProperty <http://data.ign.fr/def/ignf#domainOfValidity>
  ] ;
  rdfs:isDefinedBy <http://data.ign.fr/def/ignf> ;
  owl:disjointWith <http://data.ign.fr/def/ignf#CoordinateSystem> .

<http://data.ign.fr/def/ignf#CoordinateSystem>
  a owl:Class ;
  rdfs:label "Coordinate system"@en, "SystÃƒÂ¨me de coordonnÃƒÂ©es"@fr ;
  rdfs:comment "Ensemble d'axes couvrant un espace de coordonnÃƒÂ©es, et de rÃƒÂ¨gles mathÃƒÂ©matiques permettant l'affectation de coordonnÃƒÂ©es Ãƒ  un point. Cf. ISO 19111:2007:2007-07, partie 9.2, tableau 17 et annexe B.2."@fr, "Set of axes that spans a given coordinate space and of mathematical rules for specifying how coordinates are to be assigned to points. Cf. ISO 19111:2007:2007-07, part 9.2, table 17 and annex B.2."@en ;
  rdfs:subClassOf [
    a owl:Restriction ;
    owl:onClass <http://data.ign.fr/def/ignf#CoordinateSystemAxis> ;
    owl:onProperty <http://data.ign.fr/def/ignf#axis> ;
    owl:minCardinality "1"^^xsd:nonNegativeInteger
  ] ;
  rdfs:isDefinedBy <http://data.ign.fr/def/ignf> .

<http://data.ign.fr/def/ignf#SingleCRS>
  a owl:Class ;
  rdfs:label "Single coordinate reference system"@en, "SystÃƒÂ¨me de coordonnÃƒÂ©es de rÃƒÂ©fÃƒÂ©rence simple"@fr ;
  rdfs:comment "SystÃƒÂ¨me de coordonnÃƒÂ©es de rÃƒÂ©fÃƒÂ©rence composÃƒÂ© d'un systÃƒÂ¨me de coordonnÃƒÂ©es et d'un rÃƒÂ©fÃƒÂ©rentiel. Cf. ISO 19111:2007:2007-07 tableau 5."@fr, "Coordinate reference system consisting of one coordinate system and one datum. Cf. ISO 19111:2007:2007-07, table 5."@en ;
  rdfs:subClassOf <http://data.ign.fr/def/ignf#CRS>, [
    a owl:Class ;
    owl:intersectionOf (
     _:genid5
     _:genid7
   )
  ] ;
  rdfs:isDefinedBy <http://data.ign.fr/def/ignf> .

<http://data.ign.fr/def/ignf#GeodeticCRS>
  a owl:Class, rdfs:Class ;
  rdfs:label "Geodetic coordinate reference system"@en, "SystÃƒÂ¨me de coordonnÃƒÂ©es de rÃƒÂ©fÃƒÂ©rence geodÃƒÂ©sique"@fr ;
  rdfs:comment "SystÃƒÂ¨me de coordonnÃƒÂ©es de rÃƒÂ©fÃƒÂ©rence associÃƒÂ© Ãƒ  un rÃƒÂ©fÃƒÂ©rentiel gÃƒÂ©odÃƒÂ©sique. Cf. ISO 19111:2007:2007-07, partie 8.2.2.a, tableau 10 et annexe B.1.2.1.a."@fr, "Coordinate reference system associated with a geodetic datum. Cf. ISO 19111:2007:2007-07, part 8.2.2.a, table 10 and annex B.1.2.1.a."@en ;
  rdfs:subClassOf <http://data.ign.fr/def/ignf#SingleCRS>, [
    a owl:Restriction ;
    owl:allValuesFrom <http://data.ign.fr/def/ignf#GeodeticDatum> ;
    owl:onProperty <http://data.ign.fr/def/ignf#datum>
  ] ;
  rdfs:isDefinedBy <http://data.ign.fr/def/ignf> .

<http://data.ign.fr/def/ignf#ProjectedCRS>
  a owl:Class, rdfs:Class ;
  rdfs:label "Projected coordinate reference system"@en, "SystÃƒÂ¨me de coordonnÃƒÂ©es de rÃƒÂ©fÃƒÂ©rence projetÃƒÂ©"@fr ;
  rdfs:comment "SystÃƒÂ¨me de coordonnÃƒÂ©es de rÃƒÂ©fÃƒÂ©rence dÃƒÂ©rivÃƒÂ© par projection cartographique d'un systÃƒÂ¨me de coordonnÃƒÂ©es de rÃƒÂ©fÃƒÂ©rence bidimentionnel. Cf. ISO 19111:2007:2007-07, partie 8.2.3.b, tableau 11 et annexe B.1.2.3."@fr, "Coordinate reference system derived from a two-dimensional geodetic coordinate reference system by applying a map projection. Cf. ISO 19111:2007:2007-07, part 8.2.3.b, table 11 and annex B.1.2.3."@en ;
  rdfs:subClassOf <http://data.ign.fr/def/ignf#SingleCRS>, [
    a owl:Restriction ;
    owl:allValuesFrom <http://data.ign.fr/def/ignf#GeodeticCRS> ;
    owl:onProperty <http://data.ign.fr/def/ignf#baseCRS>
  ] ;
  rdfs:isDefinedBy <http://data.ign.fr/def/ignf> .

<http://data.ign.fr/def/ignf#CompoundCRS>
  a owl:Class, rdfs:Class ;
  rdfs:label "Compound coordinate reference system"@en, "SystÃƒÂ¨me de coordonnÃƒÂ©es de rÃƒÂ©fÃƒÂ©rence combinÃƒÂ©"@fr ;
  rdfs:comment "SystÃƒÂ¨me de coordonnÃƒÂ©es de rÃƒÂ©fÃƒÂ©rence utilisant au moins deux systÃƒÂ¨mes de coordonnÃƒÂ©es de rÃƒÂ©fÃƒÂ©rence simples indÃƒÂ©pendants. Cf. ISO 19111:2007:2007-07, parties 8.2.3.c, 8.2.4, tableau 6 et annexe B.1.2.4."@fr, "Coordinate reference system using at least two independent single coordinate reference systems. Cf. ISO 19111:2007:2007-07, parts 8.2.3.c, 8.2.4, table 6 and annex B.1.2.4."@en ;
  rdfs:subClassOf <http://data.ign.fr/def/ignf#CRS>, [
    a owl:Restriction ;
    owl:onClass <http://data.ign.fr/def/ignf#SingleCRS> ;
    owl:onProperty <http://data.ign.fr/def/ignf#includesSingleCRS> ;
    owl:minCardinality "2"^^xsd:nonNegativeInteger
  ] ;
  rdfs:isDefinedBy <http://data.ign.fr/def/ignf> ;
  owl:disjointWith <http://data.ign.fr/def/ignf#GeodeticCRS> .

<http://data.ign.fr/def/ignf#VerticalCRS>
  a owl:Class, rdfs:Class ;
  rdfs:label "Vertical coordinate reference system"@en, "SystÃƒÂ¨me de coordonnÃƒÂ©es de rÃƒÂ©fÃƒÂ©rence vertical"@fr ;
  rdfs:comment "SystÃƒÂ¨me de coordonnÃƒÂ©es de rÃƒÂ©fÃƒÂ©rence Ãƒ  une dimension, associÃƒÂ© Ãƒ  un rÃƒÂ©fÃƒÂ©rentiel vertical, et utilisÃƒÂ© pour enregistrer des hauteurs ou des profondeurs. Les hauteurs ellipsoÃƒÂ¯dales ne sont pas enregistrÃƒÂ©es Ãƒ  l'aide d'un systÃƒÂ¨me de coordonnÃƒÂ©es de rÃƒÂ©fÃƒÂ©rence vertical, mais au sein d'un tuple de coordonnÃƒÂ©es 3D dÃƒÂ©fini dans un systÃƒÂ¨me de coordonnÃƒÂ©es de rÃƒÂ©fÃƒÂ©rence gÃƒÂ©odÃƒÂ©sique 3D. Cf. ISO 19111:2007:2007-07, parties 8.2.2.b, tableau 14 et annexe B.1.2.1.b."@fr, "One-dimensional coordinate reference system associated with a vertical datum and used for recording heights or depths.Ellipsoidal heights are not captured in a vertical coordinate reference system but as part of a 3D coordinates tuple defined in a geodetic 3D coordinate reference system. Cf. ISO 19111:2007:2007-07, parts 8.2.2.b, table 14 and annex B.1.2.1.b."@en ;
  rdfs:subClassOf <http://data.ign.fr/def/ignf#SingleCRS>, [
    a owl:Class ;
    owl:intersectionOf (
     _:genid13
     _:genid15
   )
  ] ;
  rdfs:isDefinedBy <http://data.ign.fr/def/ignf> .

<http://data.ign.fr/def/ignf#Extent>
  a owl:Class, rdfs:Class ;
  rdfs:label "Extent"@en, "Ãƒâ€°tendue"@fr ;
  rdfs:comment "Zone gÃƒÂ©ographique ou intervalle de temps dans lequel la rÃƒÂ©fÃƒÂ©rence est valide. Cf. ISO 19115-1:2014:2014-04, partie 6.6.1 et tableau B.15 ligne 335."@fr, "Geographic area or time interval in which the referring object is valid. Cf. ISO 19115-1:2014:2014-04, part 6.6.1 and table B.15 line 335."@en ;
  rdfs:isDefinedBy <http://data.ign.fr/def/ignf> .

<http://data.ign.fr/def/ignf#Datum>
  a owl:Class, rdfs:Class ;
  rdfs:label "Datum"@en, "RÃƒÂ©fÃƒÂ©rentiel"@fr ;
  rdfs:comment "ParamÃƒÂ¨tre ou ensemble de paramÃƒÂ¨tres dÃƒÂ©finissant la position de l'origine, l'ÃƒÂ©chelle et l'orientation d'un systÃƒÂ¨me de coordonnÃƒÂ©es. Cf. ISO 19111:2007:2007-07, partie 10.1, tableau 33 et annexe B.3."@fr, "Parameter or set of parameters that define the position of the origin, the scale and the orientation of a coordinate system. Cf. ISO 19111:2007:2007-07, part 10.1, table 33 and annex B.3."@en ;
  rdfs:isDefinedBy <http://data.ign.fr/def/ignf> .

<http://data.ign.fr/def/ignf#GeodeticDatum>
  a owl:Class, rdfs:Class ;
  rdfs:label "Geodetic datum"@en, "RÃƒÂ©fÃƒÂ©rentiel gÃƒÂ©odÃƒÂ©sique"@fr ;
  rdfs:comment "RÃƒÂ©fÃƒÂ©rentiel dÃƒÂ©crivant la relation entre un systÃƒÂ¨me de coordonnÃƒÂ©es Ãƒ  deux ou trois dimensions et la Terre. Cf. ISO 19111:2007:2007-07, partie 10.2, tableau 34 et annexe B.3.2."@fr, "Datum describing the relation of a two- or three-dimensional coordinate system to the Earth. Cf. ISO 19111:2007:2007-07, part 10.2, table 34 and annex B.3.2."@en ;
  rdfs:subClassOf <http://data.ign.fr/def/ignf#Datum>, [
    a owl:Class ;
    owl:intersectionOf (
     _:genid18
     _:genid20
   )
  ] ;
  rdfs:isDefinedBy <http://data.ign.fr/def/ignf> .

<http://data.ign.fr/def/ignf#VerticalDatum>
  a owl:Class, rdfs:Class ;
  rdfs:label "Vertical datum"@en, "RÃƒÂ©fÃƒÂ©rentiel vertical"@fr ;
  rdfs:comment "RÃƒÂ©fÃƒÂ©rentiel dÃƒÂ©crivant la relation entre les hauteurs ou les profondeurs relatives Ãƒ  la gravitÃƒÂ© et la Terre. Cf. ISO 19111:2007:2007-07, tableau 41 et annexe B.3.3."@fr, "Datum describing the relation of gravity-related heights or depths to the Earth. Cf. ISO 19111:2007:2007-07, table 41 and annex B.3.3."@en ;
  rdfs:subClassOf <http://data.ign.fr/def/ignf#Datum> ;
  rdfs:isDefinedBy <http://data.ign.fr/def/ignf> .

<http://data.ign.fr/def/ignf#VerticalCS>
  a owl:Class, rdfs:Class ;
  rdfs:label "Vertical coordinate system"@en, "SystÃƒÂ¨me de coordonnÃƒÂ©es vertical"@fr ;
  rdfs:comment "SystÃƒÂ¨me de coordonnÃƒÂ©es Ãƒ  une dimension utilisÃƒÂ© pour les mesures de hauteur ou de profondeur relatives Ãƒ  la gravitÃƒÂ©. Cf. ISO 19111:2007:2007-07, tableaux 15 et 25."@fr, "One-dimensional coordinate system used for gravity related height or depth measurements. Cf. ISO 19111:2007:2007-07, tables 15 and 25."@en ;
  rdfs:subClassOf <http://data.ign.fr/def/ignf#CoordinateSystem> ;
  rdfs:isDefinedBy <http://data.ign.fr/def/ignf> ;
  owl:disjointWith <http://data.ign.fr/def/ignf#VerticalCRS> .

<http://data.ign.fr/def/ignf#CartesianCS>
  a owl:Class, rdfs:Class ;
  rdfs:label "Cartesian coordinate system"@en, "SystÃƒÂ¨me cartÃƒÂ©sien de coordonnÃƒÂ©es"@fr ;
  rdfs:comment "SystÃƒÂ¨me de coordonnÃƒÂ©es donnant la position des points relativement Ãƒ  n axes perpendiculaires deux Ãƒ  deux. Cf. ISO 19111:2007:2007-07, tableaux 15 et 18."@fr, "Coordinate system which gives the position of points relative to n mutually perpendicular axes. Cf. ISO 19111:2007:2007-07, tables 15 and 18."@en ;
  rdfs:subClassOf <http://data.ign.fr/def/ignf#CoordinateSystem> ;
  rdfs:isDefinedBy <http://data.ign.fr/def/ignf> ;
  owl:disjointWith <http://data.ign.fr/def/ignf#GeodeticCRS> .

<http://data.ign.fr/def/ignf#EllipsoidalCS>
  a owl:Class, rdfs:Class ;
  rdfs:label "Ellipsoidal coordinate system"@en, "SystÃƒÂ¨me de coordonnÃƒÂ©es ellipsoÃƒÂ¯dal"@fr ;
  rdfs:comment "SystÃƒÂ¨me de coordonnÃƒÂ©es dans lequel la position est spÃƒÂ©cifiÃƒÂ©e par la latitude gÃƒÂ©odÃƒÂ©sique, la longitude gÃƒÂ©odÃƒÂ©sique et (dans le cas tridimensionnel) la hauteur ellipsoÃƒÂ¯dale. Cf. ISO 19111:2007:2007-07, tableaux 15 et 20."@fr, "Coordinate system which gives the position is specified by geodetic latitude, geodetic longitude and (in the three-dimensional case) ellipsoidal height. Cf. ISO 19111:2007:2007-07, tables 15 and 20."@en ;
  rdfs:subClassOf <http://data.ign.fr/def/ignf#CoordinateSystem> ;
  rdfs:isDefinedBy <http://data.ign.fr/def/ignf> ;
  owl:disjointWith <http://data.ign.fr/def/ignf#GeodeticCRS> .

<http://data.ign.fr/def/ignf#CoordinateSystemAxis>
  a owl:Class, rdfs:Class ;
  rdfs:label "Axis"@en, "Axe"@fr ;
  rdfs:comment "Axe par rapport auquel une coordonnÃƒÂ©e d'un point est spÃƒÂ©cifiÃƒÂ©e dans un systÃƒÂ¨me de coordonnÃƒÂ©es. Cf. ISO 19111:2007:2007-07, partie 9.3, tableau 27 et annexe B.2.2."@fr, "Axis composing a coordinate system and used to specify one given coordinate in a coordinate tuple describing the position of a point. Cf. ISO 19111:2007:2007-07, part 9.3, table 27 and annex B.2.2."@en ;
  rdfs:isDefinedBy <http://data.ign.fr/def/ignf> .

<http://data.ign.fr/def/ignf#Ellipsoid>
  a owl:Class, rdfs:Class ;
  rdfs:label "Ellipsoid"@en, "EllipsoÃƒÂ¯de"@fr ;
  rdfs:comment "Surface de rÃƒÂ©volution engendrÃƒÂ©e par une ellipse tournant autour de son petit axe, dÃƒÂ©finie par le rayon ÃƒÂ©quatorial et un paramÃƒÂ¨tre d'aplatissement, et sensiblement gÃƒÂ©ocentrique. Note : Il s'agit d'un modÃƒÂ¨le mathÃƒÂ©matique du gÃƒÂ©oÃƒÂ¯de, c'est-Ãƒ -dire de la Terre dÃƒÂ©barrassÃƒÂ©e de son relief. Il existe de nombreux ellipsoÃƒÂ¯des gÃƒÂ©odÃƒÂ©siques. Cf. ISO 19111:2007:2007-07, partie 10.2.2, tableau 36 et annexe B.3.2.3."@fr, "Surface formed by the rotation of an ellipse about its minor axis, defined by a semi-major axis and a flattening parameter and fairly geocentric. NB : It is a mathematical model of the geoid, i.e. the Earth without its relief. Many geodetic ellipsoids exist. Cf. ISO 19111:2007:2007-07, part 10.2.2, table 36 and annex B.3.2.3."@en ;
  rdfs:subClassOf [
    a owl:Class ;
    owl:intersectionOf (
     _:genid23
     _:genid25
   )
  ] ;
  rdfs:isDefinedBy <http://data.ign.fr/def/ignf> .

<http://data.ign.fr/def/ignf#PrimeMeridian>
  a owl:Class, rdfs:Class ;
  rdfs:label "Prime meridian"@en, "MÃƒÂ©ridien origine"@fr ;
  rdfs:comment "MÃƒÂ©ridien Ãƒ  partir duquel les longitudes d'autres mÃƒÂ©ridiens sont mesurÃƒÂ©es. Cf. ISO 19111:2007:2007-07, partie 10.2.1, tableau 35 et annexe B.3.2.2."@fr, "Meridian from which the longitudes of other meridians are quantified. Cf. ISO 19111:2007:2007-07, part 10.2.1, table 35 and annex B.3.2.2."@en ;
  rdfs:isDefinedBy <http://data.ign.fr/def/ignf> ;
  owl:disjointWith <http://data.ign.fr/def/ignf#Ellipsoid> .

<http://data.ign.fr/def/ignf#GeographicBoundingBox>
  a owl:Class, rdfs:Class ;
  rdfs:label "Geographic bounding box"@en, "Cadre englobant gÃƒÂ©ographique"@fr ;
  rdfs:comment "Cadre dÃƒÂ©limitant une zone d'intÃƒÂ©rÃƒÂªt. Cf. ISO 19115-1:2014:2014-04, partie 6.6.1 et tableau B.15.1 ligne 344."@fr, "Box bounding an area of interest. Cf. ISO 19115-1:2014:2014-04, part 6.6.1 and table B.15.1 line 344."@en ;
  rdfs:subClassOf [
    a owl:Class ;
    owl:intersectionOf (
     _:genid34
     _:genid36
     _:genid38
     _:genid40
   )
  ] ;
  rdfs:isDefinedBy <http://data.ign.fr/def/ignf> .

<http://data.ign.fr/def/ignf#CoordinateOperation>
  a owl:Class, rdfs:Class ;
  rdfs:label "Coordinate operation"@en, "OpÃƒÂ©ration sur les coordonnÃƒÂ©es"@fr ;
  rdfs:comment "OpÃƒÂ©ration mathÃƒÂ©matique sur des coordonnÃƒÂ©es, basÃƒÂ©e sur une relation 1:1, qui change ces coordonnÃƒÂ©es d'une systÃƒÂ¨me de coordonnÃƒÂ©es de rÃƒÂ©fÃƒÂ©rence Ãƒ  un autre. Cf. ISO 19111:2007:2007-07, partie 11.1, tableau 42 et annexe B.4."@fr, "Mathematical operation on coordinates, based on one-to-one relationship, that changes coordinates from one coordinate reference system to another. Cf. ISO 19111:2007:2007-07, part 11.1, table 42 and annex B.4."@en ;
  rdfs:isDefinedBy <http://data.ign.fr/def/ignf> .

<http://data.ign.fr/def/ignf#SingleOperation>
  a owl:Class, rdfs:Class ;
  rdfs:label "Single coordinate operation"@en, "OpÃƒÂ©ration simple sur les coordonnÃƒÂ©es"@fr ;
  rdfs:comment "OpÃƒÂ©ration non concatÃƒÂ©nÃƒÂ©e sur des coordonnÃƒÂ©es. Cf. ISO 19111:2007:2007-07, tableau 43."@fr, "A non concatenated coordinate operation. Cf. ISO 19111:2007:2007-07, table 43."@en ;
  rdfs:subClassOf <http://data.ign.fr/def/ignf#CoordinateOperation> ;
  rdfs:isDefinedBy <http://data.ign.fr/def/ignf> .

<http://data.ign.fr/def/ignf#Transformation>
  a owl:Class, rdfs:Class ;
  rdfs:label "Transformation"@en, "Transformation"@fr ;
  rdfs:comment "OpÃƒÂ©ration sur les coordonnÃƒÂ©es dans laquelle les deux systÃƒÂ¨mes de coordonnÃƒÂ©es de rÃƒÂ©fÃƒÂ©rence sont basÃƒÂ©s sur des rÃƒÂ©fÃƒÂ©rentiels distincts. Cf. ISO 19111:2007:2007-07, tableau 44."@fr, "Coordinate operation in which the two coordinate reference systems are based on different datums. Cf. ISO 19111:2007:2007-07, table 44."@en ;
  rdfs:subClassOf <http://data.ign.fr/def/ignf#SingleOperation> ;
  rdfs:isDefinedBy <http://data.ign.fr/def/ignf> .

<http://data.ign.fr/def/ignf#Conversion>
  a owl:Class, rdfs:Class ;
  rdfs:label "Conversion"@en, "Conversion"@fr ;
  rdfs:comment "OpÃƒÂ©ration sur les coordonnÃƒÂ©es dans laquelle les deux systÃƒÂ¨mes de coordonnÃƒÂ©es de rÃƒÂ©fÃƒÂ©rence sont basÃƒÂ©s sur le mÃƒÂªme rÃƒÂ©fÃƒÂ©rentiel (ex: projection cartographique). Cf. ISO 19111:2007:2007-07, tableau 45 et annexe B.4.2."@fr, "Coordinate operation in which both coordinate reference systems are based on the same datum. Cf. ISO 19111:2007:2007-07, table 45 and annex B.4.2."@en ;
  rdfs:subClassOf <http://data.ign.fr/def/ignf#SingleOperation> ;
  rdfs:isDefinedBy <http://data.ign.fr/def/ignf> .

<http://data.ign.fr/def/ignf#OperationMethod>
  a owl:Class, rdfs:Class ;
  rdfs:label "Operation method"@en, "MÃƒÂ©thode"@fr ;
  rdfs:comment "MÃƒÂ©thode utilisÃƒÂ©e pour faire une opÃƒÂ©ration sur des coordonnÃƒÂ©es. Cf. ISO 19111:2007:2007-07, tableau 48 et annexe B.4.5."@fr, "The method (algorithm or procedure) used to perform the coordinate operation. Cf. ISO 19111:2007:2007-07, table 48 and annex B.4.5."@en ;
  rdfs:isDefinedBy <http://data.ign.fr/def/ignf> .

<http://data.ign.fr/def/ignf#OperationParameter>
  a owl:Class, rdfs:Class ;
  rdfs:label "Operation parameter"@en, "ParamÃƒÂ¨tre"@fr ;
  rdfs:comment "ParamÃƒÂ¨tre utilisÃƒÂ© par une mÃƒÂ©thode pour faire une opÃƒÂ©ration sur des coordonnÃƒÂ©es. Cf. ISO 19111:2007:2007-07, tableau 52 et annexe B.4.5."@fr, "Parameter used by a method to perform some coordinate operation. Cf. ISO 19111:2007:2007-07, table 52 and annex B.4.5."@en ;
  rdfs:isDefinedBy <http://data.ign.fr/def/ignf> .

<http://data.ign.fr/def/ignf#OperationParameterValue>
  a owl:Class, rdfs:Class ;
  rdfs:label "Operation parameter value"@en, "Valeur de paramÃƒÂ¨tre"@fr ;
  rdfs:comment "Valeur d'un paramÃƒÂ¨tre utilisÃƒÂ© par une mÃƒÂ©thode pour faire une opÃƒÂ©ration sur des coordonnÃƒÂ©es. Cf. ISO 19111:2007:2007-07, tableau 55."@fr, "Value of a parameter used by a method to perform some coordinate operation. Cf. ISO 19111:2007:2007-07, table 55."@en ;
  rdfs:isDefinedBy <http://data.ign.fr/def/ignf> .

<http://data.ign.fr/def/ignf#domainOfValidity>
  a owl:ObjectProperty ;
  rdfs:label "domain of validity"@en, "domaine de validitÃƒÂ©"@fr ;
  rdfs:comment "Zone ou intervalle de temps dans lequel l'objet de rÃƒÂ©fÃƒÂ©rence est valide. Cf. ISO 19111:2007:2007-07, tableaux 4, 33 et 42, attribut domainOfValidity."@fr, "Geographic area or time interval in which the referring object is valid. Cf. ISO 19111:2007:2007-07, tables 4, 33 and 42, attribute domainOfValidity."@en ;
  rdfs:range <http://data.ign.fr/def/ignf#Extent> ;
  rdfs:isDefinedBy <http://data.ign.fr/def/ignf> .

<http://data.ign.fr/def/ignf#includesSingleCRS>
  a owl:ObjectProperty ;
  rdfs:label "includes a single coordinate reference system"@en, "inclut un simple systÃƒÂ¨me de coordonnÃƒÂ©es de rÃƒÂ©fÃƒÂ©rence"@fr ;
  rdfs:comment "DÃƒÂ©signe les systÃƒÂ¨mes de coordonnÃƒÂ©es de rÃƒÂ©fÃƒÂ©rence simples qui composent un systÃƒÂ¨me de coordonnÃƒÂ©es de rÃƒÂ©fÃƒÂ©rence composÃƒÂ©. Cf. ISO 19111:2007:2007-07, tableau 6, rÃƒÂ´le d'association componentReferenceSystem."@fr, "Indicates the single coordinate reference systems used by a compound coordinate reference system. Cf. ISO 19111:2007:2007-07, table 6, association role componentReferenceSystem."@en ;
  rdfs:domain <http://data.ign.fr/def/ignf#CompoundCRS> ;
  rdfs:range <http://data.ign.fr/def/ignf#SingleCRS> ;
  rdfs:isDefinedBy <http://data.ign.fr/def/ignf> .

<http://data.ign.fr/def/ignf#baseCRS>
  a owl:ObjectProperty ;
  rdfs:label "base coordinate reference system"@en, "systÃƒÂ¨me de coordonnÃƒÂ©es de rÃƒÂ©fÃƒÂ©rence de base"@fr ;
  rdfs:comment "DÃƒÂ©signe le systÃƒÂ¨me de coordonnÃƒÂ©es de rÃƒÂ©fÃƒÂ©rence gÃƒÂ©odÃƒÂ©sique sur lequel repose un systÃƒÂ¨me de coordonnÃƒÂ©es de rÃƒÂ©fÃƒÂ©rence projetÃƒÂ©. Cf. ISO 19111:2007:2007-07, tableau 11, rÃƒÂ´le d'association baseCRS."@fr, "The geodetic coordinate reference system on which a projected coordinate reference system is based. Cf. ISO 19111:2007:2007-07, table 11, association role baseCRS."@en ;
  rdfs:domain <http://data.ign.fr/def/ignf#ProjectedCRS> ;
  rdfs:range <http://data.ign.fr/def/ignf#GeodeticCRS> ;
  rdfs:isDefinedBy <http://data.ign.fr/def/ignf> .

<http://data.ign.fr/def/ignf#coordinateSystem>
  a owl:ObjectProperty ;
  rdfs:label "uses coordinate system"@en, "utilise le systÃƒÂ¨me de coordonnÃƒÂ©es"@fr ;
  rdfs:comment "DÃƒÂ©signe le systÃƒÂ¨me de coordonnÃƒÂ©es utilisÃƒÂ© par un systÃƒÂ¨me de coordonnÃƒÂ©es de rÃƒÂ©fÃƒÂ©rence. Cf. ISO 19111:2007:2007-07, tableau 5, association nommÃƒÂ©e CoordinateSystem."@fr, "The coordinate system used by a coordinate reference system. Cf. ISO 19111:2007:2007-07, table 5, named association CoordinateSystem."@en ;
  rdfs:domain <http://data.ign.fr/def/ignf#SingleCRS> ;
  rdfs:range <http://data.ign.fr/def/ignf#CoordinateSystem> ;
  rdfs:isDefinedBy <http://data.ign.fr/def/ignf> .

<http://data.ign.fr/def/ignf#ellipsoidalCS>
  a owl:ObjectProperty ;
  rdfs:label "uses ellipsoidal coordinate system"@en, "utilise le systÃƒÂ¨me de coordonnÃƒÂ©es ellipsoÃƒÂ¯dal"@fr ;
  rdfs:comment "DÃƒÂ©signe le systÃƒÂ¨me de coordonnÃƒÂ©es ellipsoÃƒÂ¯dal utilisÃƒÂ© par un systÃƒÂ¨me de coordonnÃƒÂ©es de rÃƒÂ©fÃƒÂ©rence gÃƒÂ©odÃƒÂ©sique. Cf. ISO 19111:2007:2007-07, tableau 10, association nommÃƒÂ©e CoordinateSystem."@fr, "The ellipsoidal coordinate system used by a geodetic coordinate reference system. Cf. ISO 19111:2007:2007-07, table 10, named association CoordinateSystem."@en ;
  rdfs:subPropertyOf <http://data.ign.fr/def/ignf#coordinateSystem> ;
  rdfs:domain <http://data.ign.fr/def/ignf#GeodeticCRS> ;
  rdfs:range <http://data.ign.fr/def/ignf#EllipsoidalCS> ;
  rdfs:isDefinedBy <http://data.ign.fr/def/ignf> .

<http://data.ign.fr/def/ignf#cartesianCS>
  a owl:ObjectProperty ;
  rdfs:label "uses cartesian coordinate system"@en, "utilise le systÃƒÂ¨me de coordonnÃƒÂ©es cartesien"@fr ;
  rdfs:comment "DÃƒÂ©signe le systÃƒÂ¨me de coordonnÃƒÂ©es cartÃƒÂ©sien utilisÃƒÂ© par un systÃƒÂ¨me de coordonnÃƒÂ©es de rÃƒÂ©fÃƒÂ©rence gÃƒÂ©odÃƒÂ©sique ou projetÃƒÂ©. Cf. ISO 19111:2007:2007-07, tableaux 10 et 11, association nommÃƒÂ©e CoordinateSystem."@fr, "The cartesian coordinate system used by some geodetic or projected coordinate reference system. Cf. ISO 19111:2007:2007-07, tables 10 et 11, association roles coordinateSystem."@en ;
  rdfs:subPropertyOf <http://data.ign.fr/def/ignf#coordinateSystem> ;
  rdfs:domain [
    a owl:Class ;
    owl:unionOf (
     <http://data.ign.fr/def/ignf#GeodeticCRS>
     <http://data.ign.fr/def/ignf#ProjectedCRS>
   )
  ] ;
  rdfs:range <http://data.ign.fr/def/ignf#CartesianCS> ;
  rdfs:isDefinedBy <http://data.ign.fr/def/ignf> .

<http://data.ign.fr/def/ignf#verticalCS>
  a owl:ObjectProperty ;
  rdfs:label "uses vertical coordinate system"@en, "utilise le systÃƒÂ¨me vertical de coordonnÃƒÂ©es"@fr ;
  rdfs:comment "DÃƒÂ©signe le systÃƒÂ¨me de coordonnÃƒÂ©es vertical utilisÃƒÂ© par un systÃƒÂ¨me de coordonnÃƒÂ©es de rÃƒÂ©fÃƒÂ©rence vertical. Cf. ISO 19111:2007:2007-07, tableau 14, association nommÃƒÂ©e CoordinateSystem."@fr, "The vertical coordinate system used by a vertical coordinate reference system. Cf. ISO 19111:2007:2007-07, table 14, named association CoordinateSystem."@en ;
  rdfs:subPropertyOf <http://data.ign.fr/def/ignf#coordinateSystem> ;
  rdfs:domain <http://data.ign.fr/def/ignf#VerticalCRS> ;
  rdfs:range <http://data.ign.fr/def/ignf#VerticalCS> ;
  rdfs:isDefinedBy <http://data.ign.fr/def/ignf> .

<http://data.ign.fr/def/ignf#datum>
  a owl:ObjectProperty ;
  rdfs:label "uses datum"@en, "utilise le rÃƒÂ©fÃƒÂ©rentiel"@fr ;
  rdfs:comment "DÃƒÂ©signe le rÃƒÂ©fÃƒÂ©rentiel utilisÃƒÂ© par un systÃƒÂ¨me de coordonnÃƒÂ©es de rÃƒÂ©fÃƒÂ©rence simple. Cf. ISO 19111:2007:2007-07, tableau 5, association nommÃƒÂ©e DefiningDatum."@fr, "The datum used by a single coordinate reference system. Cf. ISO 19111:2007:2007-07, table 5, named association DefiningDatum."@en ;
  rdfs:domain <http://data.ign.fr/def/ignf#SingleCRS> ;
  rdfs:range <http://data.ign.fr/def/ignf#Datum> ;
  rdfs:isDefinedBy <http://data.ign.fr/def/ignf> .

<http://data.ign.fr/def/ignf#geodeticDatum>
  a owl:ObjectProperty ;
  rdfs:label "uses geodetic datum"@en, "utilise le rÃƒÂ©fÃƒÂ©rentiel gÃƒÂ©odÃƒÂ©sique"@fr ;
  rdfs:comment "DÃƒÂ©signe le rÃƒÂ©fÃƒÂ©rentiel gÃƒÂ©odÃƒÂ©sique utilisÃƒÂ© par un systÃƒÂ¨me de coordonnÃƒÂ©es de rÃƒÂ©fÃƒÂ©rence gÃƒÂ©odÃƒÂ©sique. Cf. ISO 19111:2007:2007-07, tableau 10, association nommÃƒÂ©e DefiningDatum."@fr, "The geodetic datum used by a geodetic coordinate reference system. Cf. ISO 19111:2007:2007-07, table 10, named association DefiningDatum."@en ;
  rdfs:subPropertyOf <http://data.ign.fr/def/ignf#datum> ;
  rdfs:domain <http://data.ign.fr/def/ignf#GeodeticCRS> ;
  rdfs:range <http://data.ign.fr/def/ignf#GeodeticDatum> ;
  rdfs:isDefinedBy <http://data.ign.fr/def/ignf> .

<http://data.ign.fr/def/ignf#verticalDatum>
  a owl:ObjectProperty ;
  rdfs:label "uses vertical datum"@en, "utilise le rÃƒÂ©fÃƒÂ©rentiel vertical"@fr ;
  rdfs:comment "DÃƒÂ©signe le rÃƒÂ©fÃƒÂ©rentiel vertical utilisÃƒÂ© par un systÃƒÂ¨me de coordonnÃƒÂ©es de rÃƒÂ©fÃƒÂ©rence vertical. Cf. ISO 19111:2007:2007-07, tableau 14, association nommÃƒÂ©e DefiningDatum."@fr, "The vertical datum used by a vertical coordinate reference system. Cf. ISO 19111:2007:2007-07, table 14, named association DefiningDatum."@en ;
  rdfs:subPropertyOf <http://data.ign.fr/def/ignf#datum> ;
  rdfs:domain <http://data.ign.fr/def/ignf#VerticalCRS> ;
  rdfs:range <http://data.ign.fr/def/ignf#VerticalDatum> ;
  rdfs:isDefinedBy <http://data.ign.fr/def/ignf> .

<http://data.ign.fr/def/ignf#axis>
  a owl:ObjectProperty ;
  rdfs:label "uses axis"@en, "utilise l'axe"@fr ;
  rdfs:comment "DÃƒÂ©signe un axe utilisÃƒÂ© par un systÃƒÂ¨me de coordonnÃƒÂ©es ellipsoÃƒÂ¯dal ou cartÃƒÂ©sien. Cf. ISO 19111:2007:2007-07, tableau 17, rÃƒÂ´le d'association axis."@fr, "An axis used by some ellipsoidal or cartesian coordinate system. Cf. ISO 19111:2007:2007-07, table 17, association role axis."@en ;
  rdfs:domain <http://data.ign.fr/def/ignf#CoordinateSystem> ;
  rdfs:range <http://data.ign.fr/def/ignf#CoordinateSystemAxis> ;
  rdfs:isDefinedBy <http://data.ign.fr/def/ignf> .

<http://data.ign.fr/def/ignf#primeMeridian>
  a owl:ObjectProperty ;
  rdfs:label "uses prime meridian"@en, "utilise le mÃƒÂ©ridien origine"@fr ;
  rdfs:comment "DÃƒÂ©signe le mÃƒÂ©ridien origine d'un rÃƒÂ©fÃƒÂ©rentiel gÃƒÂ©odÃƒÂ©sique. Cf. ISO 19111:2007:2007-07, tableau 34, rÃƒÂ´le d'association primeMeridian."@fr, "The prime meridian used by a geodetic datum. Cf. ISO 19111:2007:2007-07, table 34, association role primeMeridian."@en ;
  rdfs:domain <http://data.ign.fr/def/ignf#GeodeticDatum> ;
  rdfs:range <http://data.ign.fr/def/ignf#PrimeMeridian> ;
  rdfs:isDefinedBy <http://data.ign.fr/def/ignf> .

<http://data.ign.fr/def/ignf#ellipsoid>
  a owl:ObjectProperty ;
  rdfs:label "uses ellipsoid"@en, "utilise l'ellipsoÃƒÂ¯de"@fr ;
  rdfs:comment "DÃƒÂ©signe l'ellipsoÃƒÂ¯de utilisÃƒÂ© par un rÃƒÂ©fÃƒÂ©rentiel gÃƒÂ©odÃƒÂ©sique. Cf. ISO 19111:2007:2007-07, tableau 34, rÃƒÂ´le d'association ellipsoid."@fr, "The ellipsoid used by a geodetic datum. Cf. ISO 19111:2007:2007-07, table 34, association role ellipsoid."@en ;
  rdfs:domain <http://data.ign.fr/def/ignf#GeodeticDatum> ;
  rdfs:range <http://data.ign.fr/def/ignf#Ellipsoid> ;
  rdfs:isDefinedBy <http://data.ign.fr/def/ignf> .

<http://data.ign.fr/def/ignf#geographicElement>
  a owl:ObjectProperty ;
  rdfs:label "geographic element"@en, "ÃƒÂ©lÃƒÂ©ment gÃƒÂ©ographique"@fr ;
  rdfs:comment "DÃƒÂ©signe le cadre englobant gÃƒÂ©ographique d'une rÃƒÂ©gion de validitÃƒÂ©. Cf. ISO 19115-1:2014:2014-04, partie 6.6.1 et tableau B.15 ligne 337."@fr, "The geographic bounding box used for defining a domain of validity. Cf. ISO 19115-1:2014:2014-04, part 6.6.1 and table B.15 line 337."@en ;
  rdfs:domain <http://data.ign.fr/def/ignf#Extent> ;
  rdfs:range <http://data.ign.fr/def/ignf#GeographicBoundingBox> ;
  rdfs:isDefinedBy <http://data.ign.fr/def/ignf> .

<http://data.ign.fr/def/ignf#semiMajorAxis>
  a owl:ObjectProperty ;
  rdfs:label "semi major axis"@en, "demi grand axe"@fr ;
  rdfs:comment "DÃƒÂ©signe la longueur du demi grand axe d'un ellipsoÃƒÂ¯de. Cf. ISO 19111:2007:2007-07, tableau 36, attribut longueur du demi-grand axe."@fr, "Indicates the length of the semi major axis of an ellipsoid. Cf. ISO 19111:2007:2007-07, table 36, attribute length of semi-major axis."@en ;
  rdfs:domain <http://data.ign.fr/def/ignf#Ellipsoid> ;
  rdfs:range [
    a owl:Class ;
    owl:intersectionOf (
     <http://qudt.org/schema/qudt#QuantityValue>
     _:genid47
   )
  ] ;
  rdfs:isDefinedBy <http://data.ign.fr/def/ignf> .

<http://data.ign.fr/def/ignf#semiMinorAxis>
  a owl:ObjectProperty ;
  rdfs:label "semi minor axis"@en, "demi petit axe"@fr ;
  rdfs:comment "DÃƒÂ©signe la longueur du demi petit axe d'un ellipsoÃƒÂ¯de. Cf. ISO 19111:2007:2007-07, tableau 37, attribut longueur du demi-petit axe."@fr, "Indicates the length of the semi minor axis of an ellipsoid. Cf. ISO 19111:2007:2007-07, table 37, attribute length of semi-minor axis."@en ;
  rdfs:domain <http://data.ign.fr/def/ignf#Ellipsoid> ;
  rdfs:range [
    a owl:Class ;
    owl:intersectionOf (
     <http://qudt.org/schema/qudt#QuantityValue>
     _:genid51
   )
  ] ;
  rdfs:isDefinedBy <http://data.ign.fr/def/ignf> .

<http://data.ign.fr/def/ignf#inverseFlattening>
  a owl:ObjectProperty ;
  rdfs:label "inverse flattening"@en, "aplatissement inverse"@fr ;
  rdfs:comment "DÃƒÂ©signe la valeur d'aplatissement inverse d'un ellipsoÃƒÂ¯de, exprimÃƒÂ©e sous la forme d'un nombre ou d'un ratio (pourcentage, parties par million, etc.). Cf. ISO 19111:2007:2007-07, tableau 37, attribut aplatissement inverse."@fr, "Indicates the inverse flattening value of an ellipsoid, expressed as a number or a ratio (percentage rate, parts per million, etc.). Cf. ISO 19111:2007:2007-07, table 37, attribute inverse flattening"@en ;
  rdfs:domain <http://data.ign.fr/def/ignf#Ellipsoid> ;
  rdfs:range [
    a owl:Class ;
    owl:intersectionOf (
     <http://qudt.org/schema/qudt#QuantityValue>
     _:genid55
   )
  ] ;
  rdfs:isDefinedBy <http://data.ign.fr/def/ignf> .

<http://data.ign.fr/def/ignf#greenwichLongitude>
  a owl:ObjectProperty ;
  rdfs:label "greenwich longitude"@en, "longitude par rapport Ãƒ  Greenwich"@fr ;
  rdfs:comment "DÃƒÂ©signe la longitude par rapport au mÃƒÂ©ridien de Greenwich. Cf. ISO 19111:2007:2007-07, tableau 35, attribut longitude du mÃƒÂ©ridien d'origine."@fr, "Indicates the longitude from Greenwich meridian. Cf. ISO 19111:2007:2007-07, table 35, attribute prime meridian Greenwich longitude."@en ;
  rdfs:domain <http://data.ign.fr/def/ignf#PrimeMeridian> ;
  rdfs:range [
    a owl:Class ;
    owl:intersectionOf (
     <http://qudt.org/schema/qudt#QuantityValue>
     _:genid59
   )
  ] ;
  rdfs:isDefinedBy <http://data.ign.fr/def/ignf> .

<http://data.ign.fr/def/ignf#usesMethod>
  a owl:ObjectProperty ;
  rdfs:label "uses method"@en, "utilise la mÃƒÂ©thode"@fr ;
  rdfs:comment "DÃƒÂ©signe la mÃƒÂ©thode utilisÃƒÂ©e par une opÃƒÂ©ration sur des coordonnÃƒÂ©es. Cf. ISO 19111:2007:2007-07, tableau 43, rÃƒÂ´le d'association method."@fr, "The method used by an operation on coordinates. Cf. ISO 19111:2007:2007-07, table 43, association role method."@en ;
  rdfs:domain <http://data.ign.fr/def/ignf#CoordinateOperation> ;
  rdfs:range <http://data.ign.fr/def/ignf#OperationMethod> ;
  rdfs:isDefinedBy <http://data.ign.fr/def/ignf> .

<http://data.ign.fr/def/ignf#usesValue>
  a owl:ObjectProperty ;
  rdfs:label "uses value"@en, "utilise la valeur"@fr ;
  rdfs:comment "DÃƒÂ©signe une valeur utilisÃƒÂ©e par une opÃƒÂ©ration sur des coordonnÃƒÂ©es. Cf. ISO 19111:2007:2007-07, tableau 43, rÃƒÂ´le d'association parameterValue."@fr, "A value used by an operation on coordinates. Cf. ISO 19111:2007:2007-07, table 43, association role parameterValue."@en ;
  rdfs:domain <http://data.ign.fr/def/ignf#CoordinateOperation> ;
  rdfs:range <http://data.ign.fr/def/ignf#OperationParameterValue> ;
  rdfs:isDefinedBy <http://data.ign.fr/def/ignf> .

<http://data.ign.fr/def/ignf#usesParameter>
  a owl:ObjectProperty ;
  rdfs:label "uses parameter"@en, "utilise le paramÃƒÂ¨tre"@fr ;
  rdfs:comment "DÃƒÂ©signe un paramÃƒÂ¨tre utilisÃƒÂ© par une mÃƒÂ©thode pour faire une opÃƒÂ©ration sur des coordonnÃƒÂ©es. Cf. ISO 19111:2007:2007-07, tableau 48, rÃƒÂ´le d'association parameter."@fr, "A parameter used by a method to perform an operation on coordinates. Cf. ISO 19111:2007:2007-07, table 48, association role parameter."@en ;
  rdfs:domain <http://data.ign.fr/def/ignf#OperationMethod> ;
  rdfs:range <http://data.ign.fr/def/ignf#OperationParameter> ;
  rdfs:isDefinedBy <http://data.ign.fr/def/ignf> .

<http://data.ign.fr/def/ignf#parameter>
  a owl:ObjectProperty ;
  rdfs:label "parameter"@en, "paramÃƒÂ¨tre"@fr ;
  rdfs:comment "DÃƒÂ©signe le paramÃƒÂ¨tre auquel est associÃƒÂ©e une valeur. Cf. ISO 19111:2007:2007-07, tableau 55, rÃƒÂ´le d'association parameter."@fr, "The parameter associated to a given value. Cf. ISO 19111:2007:2007-07, table 55, association role parameter."@en ;
  rdfs:domain <http://data.ign.fr/def/ignf#OperationParameterValue> ;
  rdfs:range <http://data.ign.fr/def/ignf#OperationParameter> ;
  rdfs:isDefinedBy <http://data.ign.fr/def/ignf> .

<http://data.ign.fr/def/ignf#sourceCRS>
  a owl:ObjectProperty ;
  rdfs:label "source coordinate reference system"@en, "systÃƒÂ¨me de coordonnÃƒÂ©es de rÃƒÂ©fÃƒÂ©rence source"@fr ;
  rdfs:comment "DÃƒÂ©signe le systÃƒÂ¨me de coordonnÃƒÂ©es de rÃƒÂ©fÃƒÂ©rence des donnÃƒÂ©es en entrÃƒÂ©e d'une opÃƒÂ©ration. Cf. ISO 19111:2007:2007-07, tableau 42, association nommÃƒÂ©e Source."@fr, "The coordinate reference system associated to the data used as input of a given operation. Cf. ISO 19111:2007:2007-07, table 42, named association Source."@en ;
  rdfs:domain <http://data.ign.fr/def/ignf#CoordinateOperation> ;
  rdfs:range <http://data.ign.fr/def/ignf#CRS> ;
  rdfs:isDefinedBy <http://data.ign.fr/def/ignf> .

<http://data.ign.fr/def/ignf#targetCRS>
  a owl:ObjectProperty ;
  rdfs:label "target coordinate reference system"@en, "systÃƒÂ¨me de coordonnÃƒÂ©es de rÃƒÂ©fÃƒÂ©rence cible"@fr ;
  rdfs:comment "DÃƒÂ©signe le systÃƒÂ¨me de coordonnÃƒÂ©es de rÃƒÂ©fÃƒÂ©rence des donnÃƒÂ©es en sortie d'une opÃƒÂ©ration. Cf. ISO 19111:2007:2007-07, tableau 42, association nommÃƒÂ©e Target."@fr, "The coordinate reference system associated to the data obtained as output of a given operation. Cf. ISO 19111:2007:2007-07, table 42, named association Target."@en ;
  rdfs:domain <http://data.ign.fr/def/ignf#CoordinateOperation> ;
  rdfs:range <http://data.ign.fr/def/ignf#CRS> ;
  rdfs:isDefinedBy <http://data.ign.fr/def/ignf> .

<http://data.ign.fr/def/ignf#conversion>
  a owl:ObjectProperty ;
  rdfs:label "defined by conversion"@en, "dÃƒÂ©fini par conversion"@fr ;
  rdfs:comment "DÃƒÂ©signe la conversion utilisÃƒÂ©e pour dÃƒÂ©finir un systÃƒÂ¨me de coordonnÃƒÂ©es de rÃƒÂ©fÃƒÂ©rence projetÃƒÂ©. Cf. ISO 19111:2007:2007-07, tableau 7, association nommÃƒÂ©e Definition."@fr, "The conversion used to define a projected coordinate reference system. Cf. ISO 19111:2007:2007-07, table 7, named association Definition."@en ;
  rdfs:domain <http://data.ign.fr/def/ignf#ProjectedCRS> ;
  rdfs:range <http://data.ign.fr/def/ignf#Conversion> ;
  rdfs:isDefinedBy <http://data.ign.fr/def/ignf> .

<http://data.ign.fr/def/ignf#westBoundLongitude>
  a owl:DatatypeProperty ;
  rdfs:domain <http://data.ign.fr/def/ignf#GeographicBoundingBox> ;
  rdfs:label "west bound longitude"@en, "longitude ouest minimale"@fr ;
  rdfs:comment "DÃƒÂ©signe la longitude ouest minimale du cadre englobant. Cf. ISO 19115-1:2014:2014-04, partie 6.6.1 et tableau B.15.1 ligne 345."@fr, "Indicates the west bound longitude of a bounding box. Cf. ISO 19115-1:2014:2014-04, part 6.6.1 and table B.15.1 line 345."@en ;
  rdfs:range xsd:double ;
  rdfs:isDefinedBy <http://data.ign.fr/def/ignf> .

<http://data.ign.fr/def/ignf#eastBoundLongitude>
  a owl:DatatypeProperty ;
  rdfs:domain <http://data.ign.fr/def/ignf#GeographicBoundingBox> ;
  rdfs:label "east bound longitude"@en, "longitude est maximale"@fr ;
  rdfs:comment "DÃƒÂ©signe la longitude est maximale du cadre englobant. Cf. ISO 19115-1:2014:2014-04, partie 6.6.1 et tableau B.15.1 ligne 346."@fr, "Indicates the east bound longitude of a bounding box. Cf. ISO 19115-1:2014:2014-04, part 6.6.1 and table B.15.1 line 346."@en ;
  rdfs:range xsd:double ;
  rdfs:isDefinedBy <http://data.ign.fr/def/ignf> .

<http://data.ign.fr/def/ignf#southBoundLatitude>
  a owl:DatatypeProperty ;
  rdfs:domain <http://data.ign.fr/def/ignf#GeographicBoundingBox> ;
  rdfs:label "south bound latitude"@en, "latitude sud minimale"@fr ;
  rdfs:comment "DÃƒÂ©signe la latitude sud minimale du cadre englobant. Cf. ISO 19115-1:2014:2014-04, partie 6.6.1 et tableau B.15.1 ligne 347."@fr, "Indicates the south bound latitude of a bounding box. Cf. ISO 19115-1:2014:2014-04, part 6.6.1 and table B.15.1 line 347."@en ;
  rdfs:range xsd:double ;
  rdfs:isDefinedBy <http://data.ign.fr/def/ignf> .

<http://data.ign.fr/def/ignf#northBoundLatitude>
  a owl:DatatypeProperty ;
  rdfs:domain <http://data.ign.fr/def/ignf#GeographicBoundingBox> ;
  rdfs:label "north bound longitude"@en, "latitude nord maximale"@fr ;
  rdfs:comment "DÃƒÂ©signe la latitude nord maximale du cadre englobant. Cf. ISO 19115-1:2014:2014-04, partie 6.6.1 et tableau B.15.1 ligne 348."@fr, "Indicates the north bound longitude of a bounding box. Cf. ISO 19115-1:2014:2014-04, part 6.6.1 and table B.15.1 line 348."@en ;
  rdfs:range xsd:double ;
  rdfs:isDefinedBy <http://data.ign.fr/def/ignf> .

<http://data.ign.fr/def/ignf#scope>
  a owl:DatatypeProperty ;
  rdfs:label "scope"@en, "portÃƒÂ©e"@fr ;
  rdfs:comment "DÃƒÂ©signe la portÃƒÂ©e de la rÃƒÂ©fÃƒÂ©rence. Cf. ISO 19111:2007:2007-07, tableaux 4, 33 et 42, attribut scope."@fr, "The scope of the referring object. Cf. ISO 19111:2007:2007-07, tables 4, 33 et 42, attribute scope."@en ;
  rdfs:range xsd:string ;
  rdfs:isDefinedBy <http://data.ign.fr/def/ignf> .

<http://data.ign.fr/def/ignf#codeSpace>
  a owl:DatatypeProperty ;
  rdfs:label "code space"@en, "espace de codage"@fr ;
  rdfs:comment "DÃƒÂ©signe la rÃƒÂ¨gle ou l'autoritÃƒÂ© dont rÃƒÂ©sulte la valeur de la rÃƒÂ©fÃƒÂ©rence."@fr, "Rule or authority for a code, name, term or category."@en ;
  rdfs:range xsd:string ;
  rdfs:isDefinedBy <http://data.ign.fr/def/ignf> .

<http://data.ign.fr/def/ignf#axisAbbrev>
  a owl:DatatypeProperty ;
  rdfs:label "axis abbreviation"@en, "abrÃƒÂ©viation utilisÃƒÂ©e pour dÃƒÂ©signer l'axe"@fr ;
  rdfs:comment "DÃƒÂ©signe l'abrÃƒÂ©viation utilisÃƒÂ©e pour dÃƒÂ©signer l'axe. Cf. ISO 19111:2007:2007-07, tableau 27, attribut abrÃƒÂ©viation de l'axe du systÃƒÂ¨me de coordonnÃƒÂ©es."@fr, "The abbreviation used to identify an axis. Cf. ISO 19111:2007:2007-07, table 27, attribute coordinate system axis abbreviation."@en ;
  rdfs:domain <http://data.ign.fr/def/ignf#CoordinateSystemAxis> ;
  rdfs:range xsd:string ;
  rdfs:isDefinedBy <http://data.ign.fr/def/ignf> .

<http://data.ign.fr/def/ignf#axisDirection>
  a owl:DatatypeProperty ;
  rdfs:label "axis direction"@en, "direction de l'axe"@fr ;
  rdfs:comment "DÃƒÂ©signe la direction de l'axe. Cf. ISO 19111:2007:2007-07, tableau 27, attribut direction de l'axe du systÃƒÂ¨me de coordonnÃƒÂ©es."@fr, "The direction of an axis. Cf. ISO 19111:2007:2007-07, table 27, attribute coordinate system axis direction."@en ;
  rdfs:domain <http://data.ign.fr/def/ignf#CoordinateSystemAxis> ;
  rdfs:range xsd:string ;
  rdfs:isDefinedBy <http://data.ign.fr/def/ignf> .

<http://data.ign.fr/def/ignf#isSphere>
  a owl:DatatypeProperty ;
  rdfs:label "is sphere"@en, "est une sphÃƒÂ¨re"@fr ;
  rdfs:comment "Indique si l'ellipsoÃƒÂ¯de est une sphÃƒÂ¨re. Cf. ISO 19111:2007:2007-07, tableau 37, attribut indicateur ellipsoÃƒÂ¯de=sphÃƒÂ¨re."@fr, "Indicates whether the ellipsoid is a sphere. Cf. ISO 19111:2007:2007-07, table 37, attribute ellipsoid=sphere indicator."@en ;
  rdfs:domain <http://data.ign.fr/def/ignf#Ellipsoid> ;
  rdfs:range xsd:boolean ;
  rdfs:isDefinedBy <http://data.ign.fr/def/ignf> .

<http://data.ign.fr/def/ignf#epsgID>
  a owl:DatatypeProperty ;
  rdfs:label "espg identifier"@en, "identifiant epsg"@fr ;
  rdfs:comment "Indique l'identifiant EPSG de la ressource."@fr, "The EPSG identifier of the resource."@en ;
  rdfs:range xsd:string ;
  rdfs:isDefinedBy <http://data.ign.fr/def/ignf> .

<http://data.ign.fr/def/ignf#operationVersion>
  a owl:DatatypeProperty ;
  rdfs:label "operation version"@en, "version de l'opÃƒÂ©ration"@fr ;
  rdfs:comment "Indique la version d'une opÃƒÂ©ration appliquÃƒÂ©e sur des coordonnÃƒÂ©es. Cf. ISO 19111:2007:2007-07, tableau 42, attribut version de l'opÃƒÂ©ration sur les coordonnÃƒÂ©es."@fr, "The version of an operation performed on coordinates. Cf. ISO 19111:2007:2007-07, table 42, attribute coordinate operation version."@en ;
  rdfs:domain <http://data.ign.fr/def/ignf#CoordinateOperation> ;
  rdfs:range xsd:string ;
  rdfs:isDefinedBy <http://data.ign.fr/def/ignf> .

<http://data.ign.fr/def/ignf#methodFormula>
  a owl:DatatypeProperty ;
  rdfs:label "method formula"@en, "formule de la mÃƒÂ©thode"@fr ;
  rdfs:comment "Indique la formule utilisÃƒÂ©e par une mÃƒÂ©thode pour faire opÃƒÂ©ration sur des coordonnÃƒÂ©es. Cf. ISO 19111:2007:2007-07, tableau 48, attribut rÃƒÂ©fÃƒÂ©rence de formule de la mÃƒÂ©thode d'opÃƒÂ©ration sur les coordonnÃƒÂ©es."@fr, "The formula used by a method to perform an operation on coordinates. Cf. ISO 19111:2007:2007-07, table 48, attribute coordinate operation method formula reference."@en ;
  rdfs:domain <http://data.ign.fr/def/ignf#OperationMethod> ;
  rdfs:range xsd:string ;
  rdfs:isDefinedBy <http://data.ign.fr/def/ignf> .

<http://data.ign.fr/def/ignf#sourceDimension>
  a owl:DatatypeProperty ;
  rdfs:label "source coordinate reference system dimension"@en, "dimension du systÃƒÂ¨me de coordonnÃƒÂ©es de rÃƒÂ©fÃƒÂ©rence source"@fr ;
  rdfs:comment "Indique la dimension du systÃƒÂ¨me de coordonnÃƒÂ©es de rÃƒÂ©fÃƒÂ©rence des donnÃƒÂ©es en entrÃƒÂ©e d'une opÃƒÂ©ration. Cf. ISO 19111:2007:2007-07, tableau 48, attribut dimension du systÃƒÂ¨me de coordonnÃƒÂ©es de rÃƒÂ©fÃƒÂ©rence source."@fr, "The dimension of the coordinate reference system associated with the data used as input of an operation. Cf. ISO 19111:2007:2007-07, table 48, attribute dimension of source CRS."@en ;
  rdfs:domain <http://data.ign.fr/def/ignf#OperationMethod> ;
  rdfs:range xsd:integer ;
  rdfs:isDefinedBy <http://data.ign.fr/def/ignf> .

<http://data.ign.fr/def/ignf#targetDimension>
  a owl:DatatypeProperty ;
  rdfs:label "target coordinate reference system dimension"@en, "dimension du systÃƒÂ¨me de coordonnÃƒÂ©es de rÃƒÂ©fÃƒÂ©rence cible"@fr ;
  rdfs:comment "Indique la dimension du systÃƒÂ¨me de coordonnÃƒÂ©es de rÃƒÂ©fÃƒÂ©rence des donnÃƒÂ©es en sortie d'une opÃƒÂ©ration. Cf. ISO 19111:2007:2007-07, tableau 48, attribut dimension du systÃƒÂ¨me de coordonnÃƒÂ©es de rÃƒÂ©fÃƒÂ©rence cible."@fr, "The dimension of the coordinate reference system associated with the data obtained as output of an operation. Cf. ISO 19111:2007:2007-07, table 48, attribute dimension of target CRS."@en ;
  rdfs:domain <http://data.ign.fr/def/ignf#OperationMethod> ;
  rdfs:range xsd:integer ;
  rdfs:isDefinedBy <http://data.ign.fr/def/ignf> .

_:genid5
  a owl:Restriction ;
  owl:onClass <http://data.ign.fr/def/ignf#Datum> ;
  owl:onProperty <http://data.ign.fr/def/ignf#datum> ;
  owl:qualifiedCardinality "1"^^xsd:nonNegativeInteger .

_:genid7
  a owl:Restriction ;
  owl:onClass <http://data.ign.fr/def/ignf#CoordinateSystem> ;
  owl:onProperty <http://data.ign.fr/def/ignf#coordinateSystem> ;
  owl:qualifiedCardinality "1"^^xsd:nonNegativeInteger .

_:genid13
  a owl:Restriction ;
  owl:allValuesFrom <http://data.ign.fr/def/ignf#VerticalDatum> ;
  owl:onProperty <http://data.ign.fr/def/ignf#datum> .

_:genid15
  a owl:Restriction ;
  owl:allValuesFrom <http://data.ign.fr/def/ignf#VerticalCS> ;
  owl:onProperty <http://data.ign.fr/def/ignf#coordinateSystem> .

_:genid18
  a owl:Restriction ;
  owl:onClass <http://data.ign.fr/def/ignf#Ellipsoid> ;
  owl:onProperty <http://data.ign.fr/def/ignf#ellipsoid> ;
  owl:qualifiedCardinality "1"^^xsd:nonNegativeInteger .

_:genid20
  a owl:Restriction ;
  owl:onClass <http://data.ign.fr/def/ignf#PrimeMeridian> ;
  owl:onProperty <http://data.ign.fr/def/ignf#primeMeridian> ;
  owl:qualifiedCardinality "1"^^xsd:nonNegativeInteger .

_:genid23
  a owl:Restriction ;
  owl:onClass <http://qudt.org/schema/qudt#QuantityValue> ;
  owl:onProperty <http://data.ign.fr/def/ignf#semiMajorAxis> ;
  owl:qualifiedCardinality "1"^^xsd:nonNegativeInteger .

_:genid25
  a owl:Class ;
  owl:unionOf (
   _:genid27
   _:genid29
   _:genid31
 ) .

_:genid27
  a owl:Restriction ;
  owl:onClass <http://qudt.org/schema/qudt#QuantityValue> ;
  owl:onProperty <http://data.ign.fr/def/ignf#semiMinorAxis> ;
  owl:qualifiedCardinality "1"^^xsd:nonNegativeInteger .

_:genid29
  a owl:Restriction ;
  owl:onClass <http://qudt.org/schema/qudt#QuantityValue> ;
  owl:onProperty <http://data.ign.fr/def/ignf#inverseFlattening> ;
  owl:qualifiedCardinality "1"^^xsd:nonNegativeInteger .

_:genid31
  a owl:Restriction ;
  owl:onDataRange xsd:boolean ;
  owl:onProperty <http://data.ign.fr/def/ignf#isSphere> ;
  owl:qualifiedCardinality "1"^^xsd:nonNegativeInteger .

_:genid34
  a owl:Restriction ;
  owl:onDataRange xsd:double ;
  owl:onProperty <http://data.ign.fr/def/ignf#westBoundLongitude> ;
  owl:qualifiedCardinality "1"^^xsd:nonNegativeInteger .

_:genid36
  a owl:Restriction ;
  owl:onDataRange xsd:double ;
  owl:onProperty <http://data.ign.fr/def/ignf#eastBoundLongitude> ;
  owl:qualifiedCardinality "1"^^xsd:nonNegativeInteger .

_:genid38
  a owl:Restriction ;
  owl:onDataRange xsd:double ;
  owl:onProperty <http://data.ign.fr/def/ignf#southBoundLatitude> ;
  owl:qualifiedCardinality "1"^^xsd:nonNegativeInteger .

_:genid40
  a owl:Restriction ;
  owl:onDataRange xsd:double ;
  owl:onProperty <http://data.ign.fr/def/ignf#northBoundLatitude> ;
  owl:qualifiedCardinality "1"^^xsd:nonNegativeInteger .

_:genid47
  a owl:Restriction ;
  owl:allValuesFrom <http://qudt.org/schema/qudt#LengthUnit> ;
  owl:onProperty <http://qudt.org/schema/qudt#unit> .

_:genid51
  a owl:Restriction ;
  owl:allValuesFrom <http://qudt.org/schema/qudt#LengthUnit> ;
  owl:onProperty <http://qudt.org/schema/qudt#unit> .

_:genid55
  a owl:Restriction ;
  owl:allValuesFrom <http://qudt.org/schema/qudt#CountingUnit> ;
  owl:onProperty <http://qudt.org/schema/qudt#unit> .

_:genid59
  a owl:Restriction ;
  owl:allValuesFrom <http://qudt.org/schema/qudt#AngleUnit> ;
  owl:onProperty <http://qudt.org/schema/qudt#unit> .
