@prefix :      <http://www.opmw.org/ontology/> .
@prefix dc:    <http://purl.org/dc/elements/1.1/> .
@prefix rdfs:  <http://www.w3.org/2000/01/rdf-schema#> .
@prefix ns:    <http://purl.org/net/opmv/ns#> .
@prefix owl2xml: <http://www.w3.org/2006/12/owl2-xml#> .
@prefix foaf:  <http://xmlns.com/foaf/0.1/> .
@prefix terms: <http://purl.org/dc/terms/> .
@prefix owl:   <http://www.w3.org/2002/07/owl#> .
@prefix xsd:   <http://www.w3.org/2001/XMLSchema#> .
@prefix vann:  <http://purl.org/vocab/vann/> .
@prefix rdf:   <http://www.w3.org/1999/02/22-rdf-syntax-ns#> .
@prefix opmo:  <http://openprovenance.org/model/opmo#> .

:hasFileName  a       owl:FunctionalProperty , owl:DatatypeProperty ;
        rdfs:comment  "Property used to link an execution artifact to its file name (independently of its URI).\n\nExample:\n@prefix opmw: <http://www.opmw.org/ontology/> .\n@prefix opmv: <http://purl.org/net/opmv/ns#> .\n\n<http://www.opmw.org/export/resource/WorkflowExecutionArtifact/DCF49186981194248009E24BAD6A6412>\n      a opmv:Artifact, opmw:WorkflowExecutionArtifact.\n      opmw:hasFileName \"NTMParams_SMN_2010_03_14Z\"^^xsd:string."@en ;
        rdfs:domain   :WorkflowExecutionArtifact ;
        rdfs:label    "has File Name"@en ;
        rdfs:range    xsd:string .

:isStepOfTemplate  a        owl:ObjectProperty ;
        rdfs:comment        "Property used to dessignate which workflow Steps (or Workflow Template Processes) belong to a workflow template.\n\nExample:\n@prefix opmw: <http://www.opmw.org/ontology/> .\n\n<http://www.opmw.org/export/resource/WorkflowTemplateProcess/AQUAFLOW_EDM_CALCULATEHOURLYAVERAGES>\n     a opmw:WorkflowTemplateProcess;\n     opmw:isStepOfTemplate <http://www.opmw.org/export/resource/WorkflowTemplate/AQUAFLOW_EDM>." ;
        rdfs:domain         :WorkflowTemplateProcess ;
        rdfs:label          "is Step of Template" ;
        rdfs:range          :WorkflowTemplate ;
        rdfs:subPropertyOf  <http://purl.org/net/p-plan#isStepOfPlan> .

:WorkflowExecutionProcess
        a                owl:Class ;
        rdfs:comment     "A workflow execution process represents the execution of a step in workflow template. The execution process also describes the specific method used to acomplish the task described in the proces template.\n\nExample:\n@prefix rdfs: <http://www.w3.org/2000/01/rdf-schema#> .\n@prefix opmw: <http://www.opmw.org/ontology/> .\n@prefix opmv: <http://purl.org/net/opmv/ns#> .\n@prefix opmo: <http://openprovenance.org/model/opmo#> .\n\n<http://www.opmw.org/export/resource/WorkflowExecutionProcess/CONVERTTOSTANDARDFORMAT133553>\n      a      opmw:/WorkflowExecutionProcess , opmv:Process ;\n      rdfs:label \"Execution process ConvertToStandardFormat\" ;\n      opmo:account              <http://www.opmw.org/export/resource/WorkflowExecutionAccount/ACCOUNT1335533097598> ;\n      opmv:used              <http://www.opmw.org/export/resource/WorkflowExecutionArtifact/6C7CF277338D9590EE18534D4D78924F> ;\n      opmv:wasControlledBy               <http://www.opmw.org/export/resource/Agent/ADMIN> ;\n      opmw:hasWorkflowTemplateProcess              <http://www.opmw.org/export/resource/WorkflowTemplateProcess/AQUAFLOW_EDM_CONVERTTOSTANDARDFORMAT> ."@en ;
        rdfs:label       "Workflow Execution Process"@en ;
        rdfs:subClassOf  <http://www.w3.org/ns/prov#Activity> , ns:Process .

:isParameterOfTemplate
        a                   owl:ObjectProperty ;
        rdfs:comment        "Property used to dessignate which workflow Parameter Variables belong to a workflow template.\n\nExample:\n@prefix opmw: <http://www.opmw.org/ontology/> .\n\n<http://www.opmw.org/export/resource/ParameterVariable/AQUAFLOW_EDM_DATE>\n     a opmw:ParameterVariable;\n     opmw:isParameterOfTemplate <http://www.opmw.org/export/resource/WorkflowTemplate/AQUAFLOW_EDM>." ;
        rdfs:domain         :ParameterVariable ;
        rdfs:label          "is Parameter of Template" ;
        rdfs:range          :WorkflowTemplate ;
        rdfs:subPropertyOf  <http://purl.org/net/p-plan#isVariableOfPlan> .

ns:Artifact  a  owl:Class .

:uses   a                   owl:ObjectProperty ;
        rdfs:comment        "Property that binds a workflow template process to the workflow template artifact that generates it.\n\nExample:\n@prefix opmw: <http://www.opmw.org/ontology/> .\n\n<http://www.opmw.org/export/resource/WorkflowTemplateProcess/AQUAFLOW_EDM_REAERATIONEDM>\n     a opmw:WorkflowTemplateProcess;\n     opmw:uses <http://www.opmw.org/export/resource/DataVariable/PARAMETERSFILE>."@en ;
        rdfs:domain         :WorkflowTemplateProcess ;
        rdfs:label          "uses"@en ;
        rdfs:range          :WorkflowTemplateArtifact ;
        rdfs:subPropertyOf  <http://purl.org/net/p-plan#hasInputVar> .

:WorkflowTemplate  a     owl:Class ;
        rdfs:comment     "A workflow template represents the design of the workflow. In such design, the different steps and inputs don't have to be bound to a specific tool or dataset. It is a generic view of the workflow, which is instantiated in each execution.\n \nExample:\n@prefix dc:  <http://purl.org/dc/terms/> .\n@prefix opmw: <http://www.opmw.org/ontology/> .\n<http://www.opmw.org/export/resource/WorkflowTemplate/AQUAFLOW_NTM>\n     a opmw:WorkflowTemplate;\n     rdfs:label \"AquaFlow_NTM\" ;\n     dc.contributor\n              <http://www.opmw.org/export/resource/Agent/WATER> ;\n     dc:modified\n              \"2011-06-08T09:57:12-07:00\"^^xsd:dateTime ;\n     opmw:hasVersion \"2\"^^xsd:int ."@en ;
        rdfs:label       "Workflow Template"@en ;
        rdfs:subClassOf  <http://www.w3.org/ns/prov#Plan> , owl:Thing , <http://purl.org/net/p-plan#Plan> .

:       a                              owl:Ontology ;
        rdfs:comment                   "OPMW is an OPMV, PROV and P-plan extension to model the executions and definitions of scientific workflows." ;
        dc:title                       "The OPMW ontology"@en ;
        terms:created                  "2011-09-27"^^xsd:date ;
        terms:creator                  "http://delicias.dia.fi.upm.es/members/DGarijo/#me"^^xsd:anyURI , "http://www.isi.edu/~gil/"^^xsd:anyURI ;
        terms:description              "OPMW is an OPMV, PROV and P-plan extension to model the executions and definitions of scientific workflows."@en ;
        terms:license                  "http://creativecommons.org/licenses/by-nc-sa/2.0/" ;
        terms:modified                 "2014-12-22"^^xsd:date ;
        vann:preferredNamespacePrefix  "opmw" ;
        vann:preferredNamespaceUri     "http://www.opmw.org/ontology/" ;
        owl:imports                    <http://purl.org/net/p-plan#> , <http://openprovenance.org/model/opmo-20101012.owl> , <http://www.w3.org/ns/prov-o-20130430> ;
        owl:versionInfo                3.1 ;
        foaf:homepage                  "http://www.opmw.org/" .

:DataVariable  a         owl:Class ;
        rdfs:comment     "A Data variable is a workflow template artifact that represents a variable in the workflow specification.\n\nExample:\n@prefix rdfs: <http://www.w3.org/2000/01/rdf-schema#> .\n@prefix opmw: <http://www.opmw.org/ontology/> .\n\n<http://www.opmw.org/export/resource/DataVariable/AQUAFLOW_NTM_SUM_CORRDO>\n      a      opmw:WorkflowTemplateArtifact , opmw:DataVariable ;\n      rdfs:label \"Data variable Sum_CorrDO\" ;\n      opmw:hasDimensionality \"0\"^^xsd:int ;\n      opmw:isGeneratedBy              <http://www.opmw.org/export/resource/WorkflowTemplateProcess/AQUAFLOW_NTM_CREATEPLOTS> ;\n      opmw:template              <http://www.opmw.org/export/resource/WorkflowTemplate/AQUAFLOW_NTM> ." ;
        rdfs:label       "Data Variable"@en ;
        rdfs:subClassOf  :WorkflowTemplateArtifact .

:isConcrete  a        owl:FunctionalProperty , owl:DatatypeProperty ;
        rdfs:comment  "Property that specifies whether a component is abstract or not."@en ;
        rdfs:label    "is Concrete"@en ;
        rdfs:range    xsd:boolean .

:versionNumber  a     owl:FunctionalProperty , owl:DatatypeProperty ;
        rdfs:comment  "Property used to annotate a resource with it version number.\n\nExample:\n@prefix rdfs: <http://www.w3.org/2000/01/rdf-schema#> .\n@prefix xsd:  <http://www.w3.org/2001/XMLSchema#> .\n@prefix owl:  <http://www.w3.org/2002/07/owl#> .\n@prefix opmw: <http://www.opmw.org/ontology/> .\n@prefix opmv: <http://purl.org/net/opmv/ns#> .\n@prefix opmo: <http://openprovenance.org/model/opmo#> .\n\n<http://www.opmw.org/export/resource/WorkflowTemplate/AQUAFLOW_NTM>\n     a opmw:WorkflowTemplate;\n     opmw:versionNumber \"2\"^^xsd:int."@en ;
        rdfs:label    "version Number"@en ;
        rdfs:range    xsd:int .

:hasOriginalLogFile  a  owl:FunctionalProperty , owl:DatatypeProperty ;
        rdfs:comment  "Property used to link an execution account or a workflow execution process to the correspondent log file produced by the enacting workflow engine.\n\n\nExample:\n@prefix opmw: <http://www.opmw.org/ontology/> .\n@prefix opmo: <http://openprovenance.org/model/opmo#> .\n\n<http://www.opmw.org/export/resource/WorkflowExecutionAccount/ACCOUNT1335506667949>\n     a opmw:WorkflowExecutionAccount,opmo:Account;\n     opmw:hasOriginalLogFile \"http://wind.isi.edu/marbles/assets/components/workflow_portal/users/1/Water/runs/run_148.ttl\"^^sxd:anyURI."@en ;
        rdfs:domain   [ a            owl:Class ;
                        owl:unionOf  ( :WorkflowExecutionAccount :WorkflowExecutionProcess )
                      ] ;
        rdfs:label    "has Original Log File"@en ;
        rdfs:range    xsd:anyURI .

:hasNativeSystemTemplate
        a             owl:FunctionalProperty , owl:DatatypeProperty ;
        rdfs:comment  "Property used to link a workflow template to its native template (encoded in the syntax of the workflow system where it was designed: scufl, owl, etc.).\n\nExample:\n@prefix opmw: <http://www.opmw.org/ontology/> .\n\n<http://www.opmw.org/export/resource/WorkflowTemplate/AQUAFLOW_NTM>\n     a opmw:WorkflowTemplate;\n     opmw:hasNativeSystemTemplate \"http://wind.isi.edu/marbles/assets/components/workflow_portal/users/1/Water/ontology/Water/AquaFlow_NTM.owl\"xsd:anyURI."@en ;
        rdfs:domain   :WorkflowTemplate ;
        rdfs:label    "has Native System Template"@en ;
        rdfs:range    xsd:anyURI .

:correspondsToTemplateProcess
        a                   owl:FunctionalProperty , owl:ObjectProperty ;
        rdfs:comment        "Property that binds a workflow execution process  to its correspondant process template.\n\nExample:\n@prefix opmw: <http://www.opmw.org/ontology/> .\n@prefix opmv: <http://purl.org/net/opmv/ns#> .\n\n<http://www.opmw.org/export/resource/WorkflowExecutionProcess/REAERATIONEDM133549210450086>\n     a opmv:Process, opmw:WorkflowExecutionProcess;\n     opmw:correspondsToTemplateProcess <http://www.opmw.org/export/resource/WorkflowTemplateProcess/AQUAFLOW_EDM_REAERATIONEDM>. "@en ;
        rdfs:domain         :WorkflowExecutionProcess ;
        rdfs:label          "corresponds to Template Process"@en ;
        rdfs:range          :WorkflowTemplateProcess ;
        rdfs:subPropertyOf  owl:topObjectProperty , <http://purl.org/net/p-plan#correspondsToStep> .

:WorkflowTemplateProcess
        a                owl:Class ;
        rdfs:comment     "A workflow process template is an abstraction of the workflow execution process step that aims to describe the method followed by the scientist instead of its specific instantiation.\n\nExample:\n@prefix opmw: <http://www.opmw.org/ontology/> .\n@prefix water: <http://www.isi.edu/ac/Water/library.owl#> .\n\n<http://www.opmw.org/export/resource/WorkflowTemplateProcess/AQUAFLOW_NTM_CALCULATEHOURLYAVERAGES>\n      a opmw:ProcessTemplate, water:CalculateHourlyAverages;\n      opmw:template <http://www.opmw.org/export/resource/WorkflowTemplate/AQUAFLOW_NTM>;\n      opmw:uses <http://www.opmw.org/export/resource/DataVariable/AQUAFLOW_NTM_FILTEREDDATA>.\n      "@en ;
        rdfs:label       "Workflow Template Process"@en ;
        rdfs:subClassOf  owl:Thing , <http://purl.org/net/p-plan#Step> .

:isVariableOfTemplate
        a                   owl:ObjectProperty ;
        rdfs:comment        "Property used to dessignate which workflow Data Variables belong to a workflow template.\n\nExample:\n@prefix opmw: <http://www.opmw.org/ontology/> .\n\n<http://www.opmw.org/export/page/resource/DataVariable/AQUAFLOW_EDM_HOURLYDATA>\n     a opmw:DataVariable;\n     opmw:isVariableOfTemplate <http://www.opmw.org/export/resource/WorkflowTemplate/AQUAFLOW_EDM>." ;
        rdfs:domain         :DataVariable ;
        rdfs:label          "is Variable of Template" ;
        rdfs:range          :WorkflowTemplate ;
        rdfs:subPropertyOf  <http://purl.org/net/p-plan#isVariableOfPlan> .

:createdInWorkflowSystem
        a             owl:FunctionalProperty , owl:DatatypeProperty ;
        rdfs:comment  "This data property binds a workflow template to the tool used for its design and creation. The tool is represented by its URL.\n\nExample:\n@prefix opmw: <http://www.opmw.org/ontology/> .\n\n<http://www.opmw.org/export/resource/WorkflowTemplate/AQUAFLOW_EDM>\n         a opmw:WorkflowTemplate;\n         opmw:createdInWorkflowSystem \"http://wings.isi.edu\"^^xsd:anyURI."@en ;
        rdfs:domain   :WorkflowTemplate ;
        rdfs:label    "created in Workflow System"@en ;
        rdfs:range    xsd:anyURI .

:hasTemplateDiagram  a  owl:DatatypeProperty ;
        rdfs:comment  "Property used to link a workflow template to its graphical representation.\n\nExample:\n@prefix opmw: <http://www.opmw.org/ontology/> .\n\n<http://www.opmw.org/export/resource/WorkflowTemplate/AQUAFLOW_NTM>\n     a opmw:WorkflowTemplate;\n     opmw:hasTemplateDiagram \"http://wind.isi.edu/marbles/assets/components/workflow_portal/users/1/Water/runs/run_148.png\"xsd:anyURI."@en ;
        rdfs:domain   :WorkflowTemplate ;
        rdfs:label    "has Template Diagram"@en ;
        rdfs:range    xsd:anyURI .

:hasLocation  a       owl:DatatypeProperty ;
        rdfs:comment  "Property used to link an execution artifact to the physical location of its file in the server.\n\nExample\n@prefix opmw: <http://www.opmw.org/ontology/> .\n@prefix opmv: <http://purl.org/net/opmv/ns#> .\n\n<http://www.opmw.org/export/resource/WorkflowExecutionArtifact/DCF49186981194248009E24BAD6A6412>\n      a opmv:Artifact, opmw:WorkflowExecutionArtifact.\n      opmw:hasLocation \"http://www.opmw.org/datasets/resource/1/148/NTMParams_SMN_2010_03_14Z\"^^xsd:anyURI."@en ;
        rdfs:domain   :WorkflowExecutionArtifact ;
        rdfs:label    "has Location"@en ;
        rdfs:range    xsd:anyURI .

:hasSize  a           owl:FunctionalProperty , owl:DatatypeProperty ;
        rdfs:comment  "Property used to annotate a workflow execution artifact with the size in bytes of its file.\n\nExample\n@prefix opmw: <http://www.opmw.org/ontology/> .\n@prefix opmv: <http://purl.org/net/opmv/ns#> .\n\n<http://www.opmw.org/export/resource/WorkflowExecutionArtifact/DCF49186981194248009E24BAD6A6412>\n      a opmv:Artifact, opmw:WorkflowExecutionArtifact.\n      opmw:hasLocation \"68\"^^xsd:int."@en ;
        rdfs:domain   :WorkflowExecutionArtifact ;
        rdfs:label    "has Size"@en ;
        rdfs:range    xsd:int .

:ParameterVariable  a    owl:Class ;
        rdfs:comment     "An parameter variable represents a description of an input parameter of a process. Parameter variables can only be used by process.\n\nExample:\n@prefix rdfs: <http://www.w3.org/2000/01/rdf-schema#> .\n@prefix opmw: <http://www.opmw.org/ontology/> .\n\n<http://www.opmw.org/export/resource/ParameterVariable/AQUAFLOW_NTM_LATITUDE>\n      a      opmw:/WorkflowTemplateArtifact , opmw:ParameterVariable ;\n      rdfs:label \"Parameter variable Latitude\" ;\n      opmw:template              <http://www.opmw.org/export/resource/WorkflowTemplate/AQUAFLOW_NTM> ."@en ;
        rdfs:label       "Parameter Variable"@en ;
        rdfs:subClassOf  :WorkflowTemplateArtifact .

:hasDocumentation  a  owl:DatatypeProperty ;
        rdfs:comment  "Property that binds a workflow template to its documentation.\n\nExample:\n@prefix opmw: <http://www.opmw.org/ontology/> .\n<http://www.opmw.org/export/resource/WorkflowTemplate/AQUAFLOW_NTM>\n      a opmw:WorkflowTemplate;\n      opmw:hasDocumentation \"A copy of the documentation related to this template \"^^xsd:string."@en ;
        rdfs:domain   :WorkflowTemplate ;
        rdfs:label    "has Documentation"@en ;
        rdfs:range    [ a            rdfs:Datatype ;
                        owl:unionOf  ( xsd:anyURI xsd:string )
                      ] .

:WorkflowTemplateArtifact
        a                owl:Class ;
        rdfs:comment     "A workflow template artifact is part of a workflow template. It explains what kind of artifact is used or generated by the process template, along with possible restrictions that it may have.\n\nThere are two different types of workflow template artifacts: data variables and parameter variables."@en ;
        rdfs:label       "Workflow Template Artifact"@en ;
        rdfs:subClassOf  owl:Thing , <http://purl.org/net/p-plan#Variable> .

:hasStatus  a         owl:FunctionalProperty , owl:DatatypeProperty ;
        rdfs:comment  "Property used to state whether an ececution account was successful or not.\n\nExample:\n@prefix opmw: <http://www.opmw.org/ontology/> .\n@prefix opmo: <http://openprovenance.org/model/opmo#> .\n\n<http://www.opmw.org/export/resource/WorkflowExecutionAccount/ACCOUNT1335506667949>\n      a opmo:Account, opmw:ExecutionAccount;\n      opmw:hasStatus \"SUCCESS\"^^xsd.string."@en ;
        rdfs:domain   :WorkflowExecutionAccount ;
        rdfs:label    "has Status"@en ;
        rdfs:range    xsd:string .

:correspondsToTemplateArtifact
        a                   owl:FunctionalProperty , owl:ObjectProperty ;
        rdfs:comment        "Property that binds a workflow execution artifact to its correspondant workflow template artifact.\n\nExample:\n@prefix opmw: <http://www.opmw.org/ontology/> .\n@prefix opmv: <http://purl.org/net/opmv/ns#> .\n\n<http://www.opmw.org/export/resource/WorkflowExecutionArtifact/DEPTH1.2150836> \n       a opmv:Artifact, opmw:WorkflowExecutionArtifact;\n       opmw:correspondsToTemplateArtifact <http://www.opmw.org/export/resource/ParameterVariable/AQUAFLOW_EDM_DEPTH>."@en ;
        rdfs:domain         :WorkflowExecutionArtifact ;
        rdfs:label          "corresponds to Template Artifact"@en ;
        rdfs:range          :WorkflowTemplateArtifact ;
        rdfs:subPropertyOf  owl:topObjectProperty , <http://purl.org/net/p-plan#correspondsToVariable> .

:correspondsToTemplate
        a                   owl:FunctionalProperty , owl:ObjectProperty ;
        rdfs:comment        "Property that binds an execution account to the template of the whole workflow. The template contains the plan for the workflow.\n\nExample:\n@prefix opmw: <http://www.opmw.org/ontology/> .\n@prefix opmo: <http://openprovenance.org/model/opmo#> .\n\n<http://www.opmw.org/export/resource/WorkflowExecutionProcess/acc1>\n     a opmo:Account, opmw:workflowExecutionAccount;\n     opmw:correspondsToTemplate <http://www.opmw.org/export/resource/WorkflowTemplate/AQUAFLOW_EDM>."@en ;
        rdfs:domain         :WorkflowExecutionAccount ;
        rdfs:label          "corresponds to Template"@en ;
        rdfs:range          :WorkflowTemplate ;
        rdfs:subPropertyOf  <http://www.w3.org/ns/prov#wasDerivedFrom> , owl:topObjectProperty , ns:wasDerivedFrom .

:overallEndTime  a    owl:FunctionalProperty , owl:DatatypeProperty ;
        rdfs:comment  "Property which states that none of the activities contained in the account finished executing after the End Time.\n\nExample:\n@prefix opmw: <http://www.opmw.org/ontology/> .\n@prefix opmo: <http://openprovenance.org/model/opmo#> .\n\n<http://www.opmw.org/export/resource/WorkflowExecutionAccount/ACCOUNT1335506667949>\n     a opmw:WorkflowExecutionAccount,opmo:Account;\n     opmw:overallEndTime \"2012-04-25T10:28:55-07:00\"^^xsd:dateTime."@en ;
        rdfs:domain   :WorkflowExecutionAccount ;
        rdfs:label    "overall End Time"@en ;
        rdfs:range    xsd:dateTime .

:hasExecutableComponent
        a                   owl:FunctionalProperty , owl:ObjectProperty ;
        rdfs:comment        "Property that binds a workflow execution process to the specific component (code, scripts, etc.) used in the execution.\n\nExample:\n@prefix opmw: <http://www.opmw.org/ontology/> .\n@prefix opmv: <http://purl.org/net/opmv/ns#> .\n\n<http://www.opmw.org/export/resource/WorkflowExecutionProcess/REAERATIONEDM133549210450086>\n     a opmv:Process, opmw:WorkflowExecutionProcess;\n     opmw:hasExecutableComponent <http://www.opmw.org/export/resource/ReaerationEDM/COMPONENTREAERATIONEDM>."@en ;
        rdfs:domain         :WorkflowExecutionProcess ;
        rdfs:label          "has Executable Component"@en ;
        rdfs:subPropertyOf  <http://www.w3.org/ns/prov#used> , owl:topObjectProperty , ns:used .

:overallStartTime  a  owl:FunctionalProperty , owl:DatatypeProperty ;
        rdfs:comment  "Property which states that none of the activities in the current account started executing before the start time.\n\nExample:\n@prefix opmw: <http://www.opmw.org/ontology/> .\n@prefix opmo: <http://openprovenance.org/model/opmo#> .\n\n<http://www.opmw.org/export/resource/WorkflowExecutionAccount/ACCOUNT1335506667949>\n     a opmw:WorkflowExecutionAccount,opmo:Account;\n     opmw:overallStartTime \"2012-04-25T10:28:07-07:00\"^^xsd:dateTime."@en ;
        rdfs:domain   :WorkflowExecutionAccount ;
        rdfs:label    "overall Start Time"@en ;
        rdfs:range    xsd:dateTime .

ns:Process  a   owl:Class .

:hasExecutionDiagram  a  owl:FunctionalProperty , owl:DatatypeProperty ;
        rdfs:comment  "Property that links an execution account to its diagram. The diagram shows how the template has been instantiated with different components.\n\nExample:\n@prefix opmw: <http://www.opmw.org/ontology/> .\n@prefix opmo: <http://openprovenance.org/model/opmo#> .\n\n<http://www.opmw.org/export/resource/WorkflowExecutionAccount/ACCOUNT1335506667949>\n     a opmw:WorkflowExecutionAccount,opmo:Account;\n     opmw:hasExecutionDiagram \"http://wind.isi.edu/marbles/assets/components/workflow_portal/users/1/Water/runs/run_148.png\"^^sxd:anyURI."@en ;
        rdfs:domain   :WorkflowExecutionAccount ;
        rdfs:label    "has Execution Diagram"@en ;
        rdfs:range    xsd:anyURI .

:hasValue  a          owl:FunctionalProperty , owl:DatatypeProperty ;
        rdfs:comment  "Property used to state the value of the artifact (in case of being a parameter).\n\nExample:\n@prefix opmw: <http://www.opmw.org/ontology/> .\n@prefix opmv: <http://purl.org/net/opmv/ns#> .\n\n<http://www.opmw.org/export/resource/WorkflowExecutionArtifact/DEPTH0.61959237>\n     a opmv:Artifact, opmw:WorkflowExecutionArtifact;\n     opmw:hasValue \"0.61959237\"^^xsd:string."@en ;
        rdfs:domain   :WorkflowExecutionArtifact ;
        rdfs:label    "has Value"@en ;
        rdfs:range    xsd:string .

:isGeneratedBy  a           owl:ObjectProperty ;
        rdfs:comment        "Property that binds a workflow template artifact to the workflow template process that generates it.\n\nExample:\n@prefix opmw: <http://www.opmw.org/ontology/> .\n\n<http://www.opmw.org/export/resource/DataVariable/AQUAFLOW_EDM_REAERATIONPARAMS>\n     a opmw:DataVariable, opmw:WorkflowTemplateArtifact;\n     opmw:isGeneratedBy <http://www.opmw.org/export/resource/WorkflowTemplateProcess/AQUAFLOW_EDM_REAERATIONEDM>.\n\n"@en ;
        rdfs:domain         :WorkflowTemplateArtifact ;
        rdfs:label          "is Generated By"@en ;
        rdfs:range          :WorkflowTemplateProcess ;
        rdfs:subPropertyOf  <http://purl.org/net/p-plan#isOutputVarOf> .

:WorkflowExecutionArtifact
        a                owl:Class ;
        rdfs:comment     "A workflow execution artifact represents a resource used or generated in the execution of a workflow.\n\nExample:\n@prefix rdfs: <http://www.w3.org/2000/01/rdf-schema#> .\n@prefix opmw: <http://www.opmw.org/ontology/> .\n@prefix opmv: <http://purl.org/net/opmv/ns#> .\n@prefix opmo: <http://openprovenance.org/model/opmo#> .\n\n<http://www.opmw.org/export/resource/WorkflowExecutionArtifact/25F1016C12EBE301EE7AADBC0B085C45>\n      a       opmw:WorkflowExecutionArtifact , opmv:Artifact;\n      rdfs:label \"Execution artifact with id: 25f1016c12ebe301ee7aadbc0b085c45\" ;\n      opmo:account              <http://www.opmw.org/export/resource/WorkflowExecutionAccount/ACCOUNT1335533097598> ;\n      opmv:wasGeneratedBy     <http://www.opmw.org/export/resource/WorkflowExecutionProcess/p1> ;\n      opmw:hasLocation     \"http://wings.isi.edu/opmexport/resource/1/144/Formatted_SMN_2010_03_10Z\"^^xsd:anyURI ;\n      opmw:hasSize \"8618\"^^xsd:int ;\n      opmw:hasWorkflowTemplateArtifact              <http://www.opmw.org/export/resource/DataVariable/AQUAFLOW_EDM_FORMATTEDDATA>."@en ;
        rdfs:label       "Workflow Execution Artifact"@en ;
        rdfs:subClassOf  <http://www.w3.org/ns/prov#Entity> , ns:Artifact .

:WorkflowExecutionAccount
        a                owl:Class ;
        rdfs:comment     "A workflow execution account represents the execution from the perspective of the system.\n\nExample:\n@prefix rdfs: <http://www.w3.org/2000/01/rdf-schema#> .\n@prefix opmw: <http://www.opmw.org/ontology/> .\n@prefix opmo: <http://openprovenance.org/model/opmo#> .\n\n<http://www.opmw.org/export/resource/WorkflowExecutionAccount/ACCOUNT1335533097598>\n      a       opmo:Account , opmw:WorkflowExecutionAccount> ;\n      rdfs:label \"Execution account created on 1335533097598\" ;\n      opmw:executedInWorkflowSystem\n              <http://www.opmw.org/export/resource/Agent/SHELL> ;\n     opmw:hasEndTime\n              \"2012-04-25T07:17:48-07:00\"^^xsd:dateTime ;\n      opmw:hasExecutionDiagram \"http://wind.isi.edu/marbles/assets/components/workflow_portal/users/1/Water/runs/run_144.png\"^^xsd:anyURI ;\n      opmw:hasStartTime               \"2012-04-25T07:17:05-07:00\"^^xsd:dateTime ;\n      opmw:hasStatus \"SUCCESS\" ;"@en ;
        rdfs:label       "Workflow Execution Account"@en ;
        rdfs:subClassOf  <http://www.w3.org/ns/prov#Bundle> , opmo:Account .

opmo:OPMGraph  a  owl:Class .

opmo:Account  a  owl:Class .

:executedInWorkflowSystem
        a                   owl:FunctionalProperty , owl:ObjectProperty ;
        rdfs:comment        "Property to bind an execution account to the system where it was executed (which could be different from the one used for designing its workflow template).\n\nExample:\n@prefix opmw: <http://www.opmw.org/ontology/> .\n@prefix opmo: <http://openprovenance.org/model/opmo#> .\n\n<http://www.opmw.org/export/resource/WorkflowExecutionAccount/acc1>\n      a opmo:Account, opmw:executionAccount;\n      opmw:executedInWorkflowSystem <http://www.opmw.org/export/resource/Agent/SHELL>.\n\n<http://www.opmw.org/export/resource/Agent/SHELL> \n     a opmw:Agent."@en ;
        rdfs:domain         :WorkflowExecutionAccount ;
        rdfs:label          "executed in Workflow System"@en ;
        rdfs:range          ns:Agent ;
        rdfs:subPropertyOf  <http://www.w3.org/ns/prov#wasAttributedTo> .

:hasDimensionality  a  owl:FunctionalProperty , owl:DatatypeProperty ;
        rdfs:comment  "Property that represents the dimensionality of the artifact: 0 is a single file, 1 for a collection, etc.\n\nExample:\n@prefix opmw: <http://www.opmw.org/ontology/> .\n\n<http://www.opmw.org/export/resource/DataVariable/AQUAFLOW_NTM_DAILYDATA>\n     a opmw:DataVariable, opmw:WorkflowTemplateArtifact;\n     opmw:hasDimensionality \"1\"^^xsd:int.\n"@en ;
        rdfs:domain   :WorkflowTemplateArtifact ;
        rdfs:label    "has Dimensionality"@en ;
        rdfs:range    xsd:int .
