@prefix rdfs:  <http://www.w3.org/2000/01/rdf-schema#> .
@prefix ns1:   <http://www.w3.org/2003/06/sw-vocab-status/ns#> .
@prefix foaf:  <http://xmlns.com/foaf/0.1/> .
@prefix ns0:   <http://purl.org/vocab/vann/> .
@prefix owl:   <http://www.w3.org/2002/07/owl#> .
@prefix dc11:  <http://purl.org/dc/elements/1.1/> .
@prefix rdf:   <http://www.w3.org/1999/02/22-rdf-syntax-ns#> .
@prefix cc:    <http://creativecommons.org/ns#> .

<http://ns.inria.fr/ludo/v1/virtualcontext#VirtualLocation>
        a                 owl:Class ;
        rdfs:comment      "Represents the relation between a real life location and a location inside the game"@en ;
        rdfs:isDefinedBy  <http://ns.inria.fr/ludo/v1/virtualcontext#> ;
        rdfs:label        "Virtual location"@en ;
        rdfs:subClassOf   owl:Thing ;
        ns1:term_status   "stable" .

<http://www.oscarrodriguez.me>
        a       foaf:Person .

<http://ns.inria.fr/ludo/v1/virtualcontext#hasPOICategory>
        a                 owl:DatatypeProperty ;
        rdfs:comment      "The category of the POI"@en ;
        rdfs:domain       <http://ns.inria.fr/ludo/v1/virtualcontext#POI> ;
        rdfs:isDefinedBy  <http://ns.inria.fr/ludo/v1/virtualcontext#> ;
        rdfs:label        "Has POI category"@en ;
        rdfs:range        <http://www.w3.org/2001/XMLSchema#string> ;
        ns1:term_status   "stable" .

<http://ns.inria.fr/ludo/v1/virtualcontext#hasCurrentPOI>
        a                 owl:ObjectProperty ;
        rdfs:comment      "Given the current virtual location of a GamePlayer, it defines the corresponding POI in real life"@en ;
        rdfs:domain       foaf:Person ;
        rdfs:isDefinedBy  <http://ns.inria.fr/ludo/v1/virtualcontext#> ;
        rdfs:label        "Has current POI"@en ;
        rdfs:range        <http://ns.inria.fr/ludo/v1/virtualcontext#POI> ;
        ns1:term_status   "stable" .

<http://ns.inria.fr/ludo/v1/virtualcontext#hasCurrentGameLevel>
        a                 owl:ObjectProperty ;
        rdfs:comment      "The current level of the game in which the Gameplayer is"@en ;
        rdfs:domain       foaf:Person ;
        rdfs:isDefinedBy  <http://ns.inria.fr/ludo/v1/virtualcontext#> ;
        rdfs:label        "Has current game level"@en ;
        rdfs:range        <http://ns.inria.fr/ludo/v1/virtualcontext#GameLevel> ;
        ns1:term_status   "stable" .

<http://dbpedia.org/resource/National_Institute_for_Research_in_Computer_Science_and_Control>
        a       foaf:Organization .

<http://ns.inria.fr/ludo/v1/virtualcontext#GameLevel>
        a                 owl:Class ;
        rdfs:comment      "Represents the current (latest) game level in which the player is in the serious game"@en ;
        rdfs:isDefinedBy  <http://ns.inria.fr/ludo/v1/virtualcontext#> ;
        rdfs:label        "Game level"@en ;
        rdfs:subClassOf   owl:Thing ;
        ns1:term_status   "stable" .

<http://ns.inria.fr/ludo/v1/virtualcontext#hasGameLevelLabel>
        a                 owl:DatatypeProperty ;
        rdfs:comment      "The label of the game level"@en ;
        rdfs:domain       <http://ns.inria.fr/ludo/v1/virtualcontext#GameLevel> ;
        rdfs:isDefinedBy  <http://ns.inria.fr/ludo/v1/virtualcontext#> ;
        rdfs:label        "Has game level label"@en ;
        rdfs:range        <http://www.w3.org/2001/XMLSchema#string> ;
        ns1:term_status   "stable" .

<http://ns.inria.fr/ludo/v1/virtualcontext#hasDistance>
        a                 owl:ObjectProperty ;
        rdfs:comment      "Nearby player distance"@en ;
        rdfs:domain       foaf:Person ;
        rdfs:isDefinedBy  <http://ns.inria.fr/ludo/v1/virtualcontext#> ;
        rdfs:label        "Has distance"@en ;
        rdfs:range        <http://ns.inria.fr/ludo/v1/virtualcontext#NearbyPlayer> ;
        ns1:term_status   "stable" .

<https://plus.google.com/106595696646939943813>
        a       foaf:Person .

<http://ns.inria.fr/ludo/v1/virtualcontext#POI>
        a                 owl:Class ;
        rdfs:comment      "Point of interest"@en ;
        rdfs:isDefinedBy  <http://ns.inria.fr/ludo/v1/virtualcontext#> ;
        rdfs:label        "POI"@en ;
        rdfs:subClassOf   <http://www.w3.org/2003/01/geo/wgs84_pos#SpatialThing> , owl:Thing ;
        ns1:term_status   "stable" .

<http://ns.inria.fr/ludo/v1/virtualcontext#hasPOILabel>
        a                 owl:DatatypeProperty ;
        rdfs:comment      "A label with the name of the POI"@en ;
        rdfs:domain       <http://ns.inria.fr/ludo/v1/virtualcontext#POI> ;
        rdfs:isDefinedBy  <http://ns.inria.fr/ludo/v1/virtualcontext#> ;
        rdfs:label        "Has POI label"@en ;
        rdfs:range        <http://www.w3.org/2001/XMLSchema#string> ;
        ns1:term_status   "stable" .

<http://ns.inria.fr/ludo/v1/virtualcontext#VirtualActivity>
        a                 owl:Class ;
        rdfs:comment      "Represents the virtual activity that the player is performing inside the game. Such as learning, exploring."@en ;
        rdfs:isDefinedBy  <http://ns.inria.fr/ludo/v1/virtualcontext#> ;
        rdfs:label        "Virtual activity"@en ;
        rdfs:subClassOf   owl:Thing ;
        ns1:term_status   "stable" .

<http://ns.inria.fr/ludo/v1/virtualcontext#hasCurrentVirtualActivity>
        a                 owl:ObjectProperty ;
        rdfs:comment      "The currrent VirtualAcitivity of a GamePlayer"@en ;
        rdfs:domain       foaf:Person ;
        rdfs:isDefinedBy  <http://ns.inria.fr/ludo/v1/virtualcontext#> ;
        rdfs:label        "Has currrent VirtualAcitivity"@en ;
        rdfs:range        <http://ns.inria.fr/ludo/v1/virtualcontext#VirtualActivity> ;
        ns1:term_status   "stable" .

<http://ns.inria.fr/ludo/v1/virtualcontext#hasVirtualActivityLabel>
        a                 owl:DatatypeProperty ;
        rdfs:comment      "Virtual Activity"@en ;
        rdfs:domain       <http://ns.inria.fr/ludo/v1/virtualcontext#VirtualActivity> ;
        rdfs:isDefinedBy  <http://ns.inria.fr/ludo/v1/virtualcontext#> ;
        rdfs:label        "Virtual Activity"@en ;
        rdfs:range        <http://www.w3.org/2001/XMLSchema#string> ;
        ns1:term_status   "stable" .

<http://ns.inria.fr/ludo/v1/virtualcontext#>
        a                             owl:Ontology ;
        rdfs:comment                  "Given the increasing amount of structured data published on the Web, many possibilities are open for creating new types of games that use resources from the Web of Data. In particular, if we consider the subcategory of Serious Games in which the object of the game is to educate the user through the interactive discovery of real-life concepts (associated to Semantic Web resources), the inclusion of a semantic representation of the user profile and his contextual information becomes an important element to recommend the user more accurate concepts. Ludo is an ontology that allows the creation of Serious Games with those characteristics."@en ;
        cc:license                    <http://creativecommons.org/licenses/by/3.0/> ;
        dc11:creator                  <http://www.oscarrodriguez.me> , <https://plus.google.com/106595696646939943813> ;
        dc11:description              "This vocabulary is a component of Ludo. It was created to describe and represent the virtual context of a game player in a serious game."@en ;
        dc11:issued                   "2016-02-01"^^<http://www.w3.org/2001/XMLSchema#date> ;
        dc11:modified                 "2016-08-09"^^<http://www.w3.org/2001/XMLSchema#date> ;
        dc11:publisher                <http://dbpedia.org/resource/National_Institute_for_Research_in_Computer_Science_and_Control> ;
        dc11:rights                   "This ontology is distributed under a Creative Commons Attribution License - http://creativecommons.org/licenses/by/3.0 ."@en ;
        dc11:title                    "Ludo - Virtual Context"@en ;
        ns0:preferredNamespacePrefix  "virtualcontext" ;
        ns0:preferredNamespaceUri     "http://ns.inria.fr/ludo/v1/virtualcontext#"^^<http://www.w3.org/2001/XMLSchema#string> ;
        owl:imports                   foaf: ;
        owl:versionInfo               0.1 .

<http://ns.inria.fr/ludo/v1/virtualcontext>
        a       owl:Ontology .

<http://ns.inria.fr/ludo/v1/virtualcontext#nearbyPlayerDistance>
        a                 owl:DatatypeProperty ;
        rdfs:comment      "Nearby Player Distance in meters"@en ;
        rdfs:domain       <http://ns.inria.fr/ludo/v1/virtualcontext#NearbyPlayer> ;
        rdfs:isDefinedBy  <http://ns.inria.fr/ludo/v1/virtualcontext#> ;
        rdfs:label        "Nearby Player Distance"@en ;
        rdfs:range        <http://www.w3.org/2001/XMLSchema#decimal> ;
        ns1:term_status   "stable" .

<http://ns.inria.fr/ludo/v1/virtualcontext#NearbyPlayer>
        a                 owl:Class ;
        rdfs:comment      "It represents the realation of proximity between two players"@en ;
        rdfs:isDefinedBy  <http://ns.inria.fr/ludo/v1/virtualcontext#> ;
        rdfs:label        "Nearby Player"@en ;
        rdfs:subClassOf   owl:Thing ;
        ns1:term_status   "stable" .

<http://ns.inria.fr/ludo/v1/virtualcontext#hasGameLevelNumber>
        a                 owl:DatatypeProperty ;
        rdfs:comment      "The numeric label of the game level"@en ;
        rdfs:domain       <http://ns.inria.fr/ludo/v1/virtualcontext#GameLevel> ;
        rdfs:isDefinedBy  <http://ns.inria.fr/ludo/v1/virtualcontext#> ;
        rdfs:label        "Has game level number"@en ;
        rdfs:range        <http://www.w3.org/2001/XMLSchema#nonNegativeInteger> ;
        ns1:term_status   "stable" .
