@prefix :      <http://promsns.org/def/do#> .
@prefix rdfs:  <http://www.w3.org/2000/01/rdf-schema#> .
@prefix owl:   <http://www.w3.org/2002/07/owl#> .
@prefix xsd:   <http://www.w3.org/2001/XMLSchema#> .
@prefix rdf:   <http://www.w3.org/1999/02/22-rdf-syntax-ns#> .
@prefix xml:   <http://www.w3.org/XML/1998/namespace> .
@prefix dcterms: <http://purl.org/dc/terms/> .

:Question  a             owl:Class ;
        rdfs:comment     "A recorded question"@en ;
        rdfs:label       "Question"@en ;
        rdfs:subClassOf  <http://www.w3.org/ns/prov#Entity> .

:DecisionMaking  a        owl:Class ;
        rdfs:comment      "A temporal event in which decision processes are undertaken, such as initiating sub-questions for the question to be answered, consideration of options etc."@en ;
        rdfs:label        "Decision Making"@en ;
        rdfs:subClassOf   <http://www.w3.org/ns/prov#Activity> ;
        owl:disjointWith  :OptionSelection .

<http://promsns.org/def/decprov>
        a                    owl:Ontology ;
        rdfs:comment         "This ontology is for modelling decisions and thus the causes for actions or the use or generation of things. It allows for a better understanding of *why* something might have taken place, have been used or produced than the more generic [PROV ontology](https://www.w3.org/TR/prov-o/), on which it is mainly based, does.  \n\n                                  The specialised decision modelling elements of this ontology have been derived from the [W3C Decisions and Decision-Making Incubator Group](https://www.w3.org/2005/Incubator/decision/)'s Decision Ontology (DO) which can be found at <https://github.com/nicholascar/decision-o>. Many DO classes have been aligned with the PROV-O since it is widely recognised that analysing the elements of decisions *post hoc* is an exercise in provenance.\n\n                                  Unlike the original DO, this ontology cannot be used for *normative* scenarios: it is only capable of recording decisions that have already been made (so-called *data-driven* use in the DO). This is because PROV does not have a templating system which can indicate what *should* occur in future scenarios.\n\n                                  This ontology introduces only one new element for decision modelling over that which was present in the DO: an Agent which allows agency in decision making to be recorded."@en ;
        rdfs:label           "Decision Provenance ontology (DecPROV)"^^xsd:string ;
        rdfs:seeAlso         "The GitHub repository containing addition documentation: http://github.com/nicholascar/decprov-ont/"@en ;
        dcterms:created      "2017-06-28"^^xsd:date ;
        dcterms:creator      "Nicholas Car"^^xsd:string ;
        dcterms:creator      <http://orcid.org/0000-0002-8742-7730> ;
        dcterms:description  "This ontology is a reduced-in-scope version of the [W3C Decisions and Decision-Making Incubator Group](https://www.w3.org/2005/Incubator/decision/)'s Decision Ontology (DO) which can be found at <https://github.com/nicholascar/decision-o>. It has been re-worked to align entirely with the W3C's [PROV ontology](https://www.w3.org/TR/prov-o/) since it is widely recognised that analysing the elements of decisions *post hoc* is an exercise in provenance.\n\nUnlike the original DO, this ontology cannot be used for *normative* scenarios: it is only capable of recording decisions that have already been made (so-called *data-driven* use in the DO). This is because PROV, to which this ontology is completely mapped, does not have a templating system which can indicate what *should* occur in future scenarios.\n\nThis ontology introduces only one new element for decision modelling over that which was present in the DO: an Agent which allows agency in decision making to be recorded."@en ;
        dcterms:modified     "2017-09-01"@en ;
        owl:imports          <http://www.w3.org/ns/prov-o> ;
        owl:priorVersion     "1.0"^^xsd:string ;
        owl:versionIRI       <http://promsns.org/def/decprov> ;
        owl:versionInfo      "1.1"^^xsd:string .

:DecisionMaker  a  <http://www.w3.org/ns/prov#Role> , owl:NamedIndividual .

:Requirement  a          owl:Class ;
        rdfs:comment     "Requirements require something from an OptionSelection Activity. They indicate their requirement with a set (a class) of objects. They are then satisified by the presense of an onject within that class. Multiple Requirements can be intersected to require very specific OptionSelection outcomes."@en ;
        rdfs:label       "Requirement"@en ;
        rdfs:subClassOf  <http://www.w3.org/ns/prov#Entity> .

:Answer  a                owl:Class ;
        rdfs:comment      "A recorded answer to a Question"@en ;
        rdfs:label        "Answer"@en ;
        rdfs:subClassOf   <http://www.w3.org/ns/prov#Entity> ;
        rdfs:subClassOf   [ a                   owl:Restriction ;
                            owl:onProperty      <http://www.w3.org/ns/prov#wasInfluencedBy> ;
                            owl:someValuesFrom  :Question
                          ] ;
        rdfs:subClassOf   [ a                   owl:Restriction ;
                            owl:onProperty      <http://www.w3.org/ns/prov#wasGeneratedBy> ;
                            owl:someValuesFrom  :OptionSelection
                          ] ;
        owl:disjointWith  :Question .

:OptionSelection  a      owl:Class ;
        rdfs:comment     "Option Selection is a process (prov:Activity) through which a decision-making Agent selects something.\n\nAt least two Option Selection Activities, possibly more, must be run in parrallel by an Agent and at least one must yield an outcome in order for a Question to be answered."@en ;
        rdfs:label       "Wyb√≥r opcji"@pl , "OptionSelection"@en ;
        rdfs:seeAlso     :Decision_making ;
        rdfs:subClassOf  <http://www.w3.org/ns/prov#Activity> ;
        rdfs:subClassOf  [ a                   owl:Restriction ;
                           owl:onProperty      <http://www.w3.org/ns/prov#wasStartedBy> ;
                           owl:someValuesFrom  :Question
                         ] .
