@prefix prv: <http://purl.org/net/provenance/ns#> .
@prefix : <http://www.w3.org/1999/xhtml> .
@prefix rdfs: <http://www.w3.org/2000/01/rdf-schema#> .
@prefix wot: <http://xmlns.com/wot/0.1/> .
@prefix foaf: <http://xmlns.com/foaf/0.1/> .
@prefix owl: <http://www.w3.org/2002/07/owl#> .
@prefix xsd: <http://www.w3.org/2001/XMLSchema#> .
@prefix rdf: <http://www.w3.org/1999/02/22-rdf-syntax-ns#> .
@prefix xhv: <http://www.w3.org/1999/xhtml/vocab#> .
@prefix dcterms: <http://purl.org/dc/terms/> .

prv:accessedService a owl:ObjectProperty ;
	rdfs:comment "This property refers to the service that provided the Web representation during the execution of a data access."@en ;
	rdfs:domain prv:DataAccess .

prv:DataAccess a owl:Class ;
	rdfs:comment "DataAccess is a class that represents the completed execution of accessing a data item on the Web."@en ;
	rdfs:label "Data Access"@en ;
	rdfs:isDefinedBy <http://purl.org/net/provenance/ns> ;
	owl:disjointWith prv:DataCreation .

prv:DataCreation a owl:Class ;
	rdfs:comment "DataCreation is a class that represents the completed creation of a data item."@en ;
	rdfs:label "Data Creation"@en ;
	rdfs:isDefinedBy <http://purl.org/net/provenance/ns> ;
	owl:disjointWith prv:DataAccess ;
	rdfs:subClassOf prv:Execution .

prv:Execution a owl:Class ;
	rdfs:comment "Execution is a general class that represents completed executions of actions or processes. An execution is usually performed by an actor (see the class <a xmlns=\"http://www.w3.org/1999/xhtml\" href=\"#Actor\" xml:lang=\"en\">Actor</a>) and an execution, in most cases, yielded an artifact (see the class <a xmlns=\"http://www.w3.org/1999/xhtml\" href=\"#Artifact\" xml:lang=\"en\">Artifact</a>)."^^rdf:XMLLiteral ;
	owl:disjointWith prv:Artifact .

prv:Artifact a owl:Class ;
	rdfs:comment "Artifact is a general class that represents artifacts which can be used during the execution (see the class <a xmlns=\"http://www.w3.org/1999/xhtml\" href=\"#Execution\" xml:lang=\"en\">Execution</a>) of an action or a process and which can also be the result of such an execution."^^rdf:XMLLiteral ;
	owl:disjointWith prv:Execution , prv:Actor ;
	rdfs:label "Artifact"@en ;
	rdfs:isDefinedBy <http://purl.org/net/provenance/ns> .

prv:Execution owl:disjointWith prv:Actor .

prv:Actor a owl:Class ;
	owl:equivalentClass foaf:Agent ;
	rdfs:comment "Actor is a general class that represents actors which usually performed the execution (see the class <a xmlns=\"http://www.w3.org/1999/xhtml\" href=\"#Execution\" xml:lang=\"en\">Execution</a>) of an action or a process."^^rdf:XMLLiteral ;
	rdfs:label "Actor"@en ;
	rdfs:isDefinedBy <http://purl.org/net/provenance/ns> .

prv:Execution rdfs:label "Execution"@en ;
	rdfs:isDefinedBy <http://purl.org/net/provenance/ns> .

prv:DataAccess rdfs:subClassOf prv:Execution .

prv:accessedService rdfs:label "accessed"@en ;
	rdfs:isDefinedBy <http://purl.org/net/provenance/ns> ;
	rdfs:range prv:DataProvidingService .

prv:DataProvidingService a owl:Class ;
	rdfs:comment "DataProvidingService is a class that represents a non-human actor - usually a Web service or a server - that processes data access requests and actually sends the requested Web representations (i.e. <a xmlns=\"http://www.w3.org/1999/xhtml\" href=\"#Representation\" xml:lang=\"en\">prv:Representation</a>) over the Web."^^rdf:XMLLiteral ;
	rdfs:label "Data Providing Service"@en ;
	rdfs:isDefinedBy <http://purl.org/net/provenance/ns> ;
	rdfs:subClassOf prv:NonHumanActor .

prv:NonHumanActor a owl:Class ;
	rdfs:comment "NonHumanActor is a general class that represents actors who are not social beings."@en ;
	rdfs:label "Non-Human Actor"@en ;
	rdfs:isDefinedBy <http://purl.org/net/provenance/ns> ;
	owl:disjointWith prv:HumanActor .

prv:HumanActor a owl:Class ;
	rdfs:comment "HumanActor is a general class that represents actors who are social beings such as persons, organizations, companies."@en ;
	rdfs:label "Human Actor"@en ;
	rdfs:isDefinedBy <http://purl.org/net/provenance/ns> ;
	owl:disjointWith prv:Artifact , prv:Execution , prv:NonHumanActor ;
	rdfs:subClassOf prv:Actor .

prv:NonHumanActor rdfs:subClassOf prv:Actor .

prv:accessedService rdfs:subPropertyOf prv:involvedActor .

prv:involvedActor a owl:ObjectProperty ;
	rdfs:comment "This is an abstract property that refers to an actor involved in an execution."@en ;
	rdfs:domain prv:Execution ;
	rdfs:label "involved"@en ;
	rdfs:isDefinedBy <http://purl.org/net/provenance/ns> ;
	rdfs:range prv:Actor .

prv:usedGuideline a owl:ObjectProperty ;
	rdfs:comment "This property refers to a creation guideline which guided the execution of a data creation. Examples for creation guidelines are transformation rules, mapping definitions, entailment rules, and database queries. Notice, all creation guidelines have provenance; we strongly encourage to describe this provenance as well, at least as far as available information permits."@en ;
	rdfs:domain prv:DataCreation ;
	rdfs:label "guided by"@en ;
	rdfs:isDefinedBy <http://purl.org/net/provenance/ns> ;
	rdfs:range prv:CreationGuideline .

prv:CreationGuideline a owl:Class ;
	rdfs:comment "CreationGuideline is a class that represents a guideline used to guide the execution of a data creation. Examples for creation guidelines are transformation rules, mapping definitions, entailment rules, and database queries."@en ;
	rdfs:label "Creation Guideline"@en ;
	rdfs:isDefinedBy <http://purl.org/net/provenance/ns> ;
	rdfs:subClassOf prv:DataItem .

prv:DataItem a owl:Class ;
	rdfs:comment "DataItem is a general class that represents data items of any kind."@en ;
	rdfs:label "Data Item"@en ;
	rdfs:isDefinedBy <http://purl.org/net/provenance/ns> ;
	owl:disjointWith prv:Representation .

prv:Representation a owl:Class ;
	rdfs:comment "Representation is a general concept that represents a Web representation of an information resource such as a data item. Such a Web representation was used during the retrieval of a data item from the Web."@en ;
	rdfs:label "Web Representation"@en ;
	rdfs:isDefinedBy <http://purl.org/net/provenance/ns> ;
	owl:disjointWith prv:DataItem ;
	rdfs:subClassOf prv:Artifact , <http://www.ontologydesignpatterns.org/ont/web/irw.owl#WebRepresentation> .

<http://www.ontologydesignpatterns.org/ont/web/irw.owl#WebRepresentation> a owl:Class .

prv:Representation rdfs:subClassOf <http://sw.nokia.com/WebArch-1/Representation> .

<http://sw.nokia.com/WebArch-1/Representation> a owl:Class .

prv:DataItem rdfs:subClassOf prv:Artifact , <http://www.ontologydesignpatterns.org/ont/web/irw.owl#InformationResource> .

<http://www.ontologydesignpatterns.org/ont/web/irw.owl#InformationResource> a owl:Class .

prv:usedGuideline rdfs:subPropertyOf prv:usedData .

prv:usedData a owl:ObjectProperty ;
	rdfs:comment "This property refers to a source data item that has been used during the creation of a data item. Examples for source data are the content of a document used for machine learning, the statements in a knowledge base used to entail a new statement, and the entries in a database used to answer a query. Notice, all source data has provenance; we strongly encourage to describe this provenance as well, at least as far as available information permits."@en ;
	rdfs:domain prv:DataCreation ;
	rdfs:label "used"@en ;
	rdfs:isDefinedBy <http://purl.org/net/provenance/ns> ;
	rdfs:range prv:DataItem ;
	rdfs:subPropertyOf prv:employedArtifact .

prv:employedArtifact a owl:ObjectProperty ;
	rdfs:comment "This is an abstract property that refers to an artifact which was used during an execution."@en ;
	rdfs:domain prv:Execution ;
	rdfs:label "used"@en ;
	rdfs:isDefinedBy <http://purl.org/net/provenance/ns> ;
	rdfs:range prv:Artifact .

dcterms:created a owl:DatatypeProperty .

foaf:Organization a owl:Class ;
	rdfs:subClassOf prv:HumanActor .

<http://trdf.sourceforge.net/provenance/ns-20091007.html> a foaf:Document ;
	dcterms:title "Provenance Vocabulary Core Ontology Specification"@en ;
	rdfs:label "Document that defines the core ontology of the Provenance Vocabulary"@en ;
	xhv:alternate <http://trdf.sourceforge.net/provenance/ns.rdf> ;
	dcterms:description "This documents specifies the classes and properties introduced by the Provenance Vocabulary Core Ontology."@en ;
	dcterms:conformsTo <http://www.w3.org/TR/rdfa-syntax> .

<http://www.w3.org/TR/rdfa-syntax> a owl:Thing .

<http://trdf.sourceforge.net/provenance/ns-20091007.html> foaf:primaryTopic <http://purl.org/net/provenance/ns#> .

<http://purl.org/net/provenance/ns#> a prv:DataItem ;
	dcterms:title "Provenance Vocabulary Core Ontology namespace"@en ;
	prv:createdBy _:node183fu7k97x1 .

_:node183fu7k97x1 a prv:DataCreation ;
	prv:performedBy <http://www.informatik.hu-berlin.de/~hartig/foaf.rdf#olaf> .

<http://www.informatik.hu-berlin.de/~hartig/foaf.rdf#olaf> a foaf:Person ;
	foaf:name "Olaf Hartig"@en ;
	foaf:homepage <http://olafhartig.de/> .

<http://olafhartig.de/> a foaf:Document .

_:node183fu7k97x1 prv:performedBy <http://users.ox.ac.uk/~zool0770/foaf.rdf#me> .

<http://users.ox.ac.uk/~zool0770/foaf.rdf#me> a foaf:Person ;
	foaf:name "Jun Zhao"@en ;
	foaf:homepage <http://users.ox.ac.uk/~zool0770/> .

<http://users.ox.ac.uk/~zool0770/> a foaf:Document .

_:node183fu7k97x1 prv:performedAt "2009-10-07T12:00:00Z"^^xsd:dateTime .

<http://purl.org/net/provenance/ns#> dcterms:creator <http://www.informatik.hu-berlin.de/~hartig/foaf.rdf#olaf> , <http://users.ox.ac.uk/~zool0770/foaf.rdf#me> ;
	a owl:Ontology ;
	dcterms:created "2009-10-07T12:00:00Z"^^xsd:dateTime ;
	dcterms:description "The Provenance Vocabulary provides classes and properties to describe the provenance of data from the Web. Hence, this vocabulary enables providers of Web data to publish provenance-related metadata about their data. The Provenance Vocabulary Core Ontology provides the main classes and properties required to describe provenance of data on the Web. Notice, this vocabulary is not designed to describe provenance of other kinds of content such as documents."@en .

<http://trdf.sourceforge.net/provenance/ns-20091007.html> xhv:license <http://creativecommons.org/licenses/by/1.0/> .

<http://creativecommons.org/licenses/by/1.0/> a owl:Thing .

wot:assurance a owl:ObjectProperty .

foaf:name a owl:DatatypeProperty .

prv:operatedBy a owl:ObjectProperty ;
	rdfs:comment "This property refers to a human actor who was operating a non-human actor. For instance, a service provider operates a data providing service (see class <a xmlns=\"http://www.w3.org/1999/xhtml\" href=\"#DataProvidingService\" xml:lang=\"en\">prv:DataProvidingService</a>). Another example is a human actor who operates a non-human data creating actor."^^rdf:XMLLiteral ;
	rdfs:domain prv:NonHumanActor ;
	rdfs:label "operated by"@en ;
	rdfs:isDefinedBy <http://purl.org/net/provenance/ns> ;
	rdfs:range prv:HumanActor .

<http://purl.org/net/provenance/ns.rdf> a foaf:Document .

<http://trdf.sourceforge.net/provenance/ns.html> a foaf:Document ;
	wot:assurance <http://trdf.sourceforge.net/provenance/ns.html.sig> .

<http://trdf.sourceforge.net/provenance/ns.html.sig> a wot:Endorsement ;
	dcterms:title "Detached signature"@en ;
	wot:endorser <http://www.informatik.hu-berlin.de/~hartig/foaf.rdf#pubkey> .

<http://www.informatik.hu-berlin.de/~hartig/foaf.rdf#pubkey> a wot:PubKey .

wot:endorser a owl:ObjectProperty .

dcterms:creator a owl:ObjectProperty .

prv:performedAt a owl:DatatypeProperty ;
	rdfs:comment "This property refers to the time an execution has been performed at."@en ;
	rdfs:domain prv:Execution ;
	rdfs:label "executed at"@en ;
	rdfs:isDefinedBy <http://purl.org/net/provenance/ns> ;
	rdfs:range xsd:dateTime .

dcterms:conformsTo a owl:ObjectProperty .

foaf:Group a owl:Class ;
	rdfs:subClassOf prv:HumanActor .

<http://sw.nokia.com/WebArch-1/Service> a owl:Class ;
	rdfs:subClassOf prv:DataProvidingService .

prv:createdBy a owl:ObjectProperty ;
	rdfs:comment "This property refers to the creation of a data item."@en ;
	rdfs:domain prv:DataItem ;
	rdfs:label "created by"@en ;
	rdfs:isDefinedBy <http://purl.org/net/provenance/ns> ;
	rdfs:range prv:DataCreation ;
	rdfs:subPropertyOf prv:yieldedBy .

prv:yieldedBy a owl:ObjectProperty ;
	rdfs:comment "This is an abstract property that refers to the execution by which an artifact was yielded."@en ;
	rdfs:domain prv:Artifact ;
	rdfs:label "yielded by"@en ;
	rdfs:isDefinedBy <http://purl.org/net/provenance/ns> ;
	rdfs:range prv:Execution .

prv:usedBy a owl:ObjectProperty ;
	rdfs:comment "This property refers to a data publisher who used a data providing services."@en ;
	rdfs:domain prv:DataProvidingService ;
	rdfs:label "used by"@en ;
	rdfs:isDefinedBy <http://purl.org/net/provenance/ns> ;
	rdfs:range prv:DataPublisher .

prv:DataPublisher a owl:Class ;
	rdfs:comment "DataPublisher is a class that represents entities such as persons, groups, or organizations who use a data providing service (see class <a xmlns=\"http://www.w3.org/1999/xhtml\" href=\"#DataProvidingService\" xml:lang=\"en\">prv:DataProvidingService</a>) to publish data on the Web."^^rdf:XMLLiteral ;
	rdfs:label "Data Publisher"@en ;
	rdfs:isDefinedBy <http://purl.org/net/provenance/ns> ;
	rdfs:subClassOf prv:HumanActor .

<http://sw.nokia.com/WebArch-1/Server> a owl:Class ;
	rdfs:subClassOf prv:DataProvidingService .

prv:retrievedBy a owl:ObjectProperty ;
	rdfs:comment "This property refers to the data access by which a Web representation of a data item has been retrieved from the Web."@en ;
	rdfs:domain prv:Representation ;
	rdfs:label "retrieved by"@en ;
	rdfs:isDefinedBy <http://purl.org/net/provenance/ns> ;
	rdfs:range prv:DataAccess ;
	rdfs:subPropertyOf prv:yieldedBy .

prv:containedBy a owl:ObjectProperty ;
	rdfs:comment "This property refers to an artifact that contained a data item. This artifact can either be a Web representation of the data item (see class <a xmlns=\"http://www.w3.org/1999/xhtml\" href=\"#Representation\" xml:lang=\"en\">prv:Representation</a>) or it can be another data item of a larger granularity (e.g. an RDF statement is usually contained in an RDF graph)."^^rdf:XMLLiteral ;
	rdfs:domain prv:DataItem ;
	rdfs:label "contained in"@en ;
	rdfs:isDefinedBy <http://purl.org/net/provenance/ns> ;
	rdfs:range prv:Artifact .

foaf:homepage a owl:ObjectProperty .

prv:Document a owl:DeprecatedClass ;
	owl:equivalentClass prv:Representation ;
	rdfs:comment "This class is deprecated and will be removed from the Provenance Vocabulary shortly. Use <a xmlns=\"http://www.w3.org/1999/xhtml\" href=\"#Representation\" xml:lang=\"en\">prv:Representation</a> instead. prv:Document was deprecated because its name caused confusion; the name made people assume this class represents information resources which is not the case; in fact, it represents a Web representation of an information resource."^^rdf:XMLLiteral ;
	rdfs:label "Web Representation"@en ;
	rdfs:isDefinedBy <http://purl.org/net/provenance/ns> .

prv:performedBy a owl:ObjectProperty ;
	rdfs:comment "This property refers to an actor that/who performed an execution."@en ;
	rdfs:domain prv:Execution ;
	rdfs:label "performed by"@en ;
	rdfs:isDefinedBy <http://purl.org/net/provenance/ns> ;
	rdfs:range prv:Actor ;
	rdfs:subPropertyOf prv:involvedActor .

<http://www.ontologydesignpatterns.org/ont/web/irw.owl#WebServer> a owl:Class ;
	rdfs:subClassOf prv:DataProvidingService .

xhv:alternate a owl:ObjectProperty .

foaf:primaryTopic a owl:ObjectProperty .

dcterms:description a owl:DatatypeProperty .

dcterms:title a owl:DatatypeProperty .

prv:precededBy a owl:ObjectProperty ;
	rdfs:comment "This property refers to an immediately preceding version of a data item; hence, the new version (i.e. the subject) has been created using the old version (i.e. the object). We strongly encourage to also describe this creation of the new version explicitly."@en ;
	rdfs:domain prv:DataItem ;
	rdfs:label "immediately preceded by"@en ;
	rdfs:isDefinedBy <http://purl.org/net/provenance/ns> ;
	rdfs:range prv:DataItem ;
	rdfs:subPropertyOf dcterms:replaces .

dcterms:replaces a owl:ObjectProperty .

xhv:license a owl:ObjectProperty .

wot:Endorsement a owl:Class .

wot:PubKey a owl:Class .

foaf:Agent a owl:Class .

foaf:Document a owl:Class .

foaf:Person a owl:Class ;
	rdfs:subClassOf prv:HumanActor .

<http://purl.org/net/provenance/ns#> prv:createdBy _:node183fu7k97x2 .

_:node183fu7k97x2 a prv:DataCreation ;
	prv:performedBy <http://www.informatik.hu-berlin.de/~hartig/foaf.rdf#olaf> , <http://users.ox.ac.uk/~zool0770/foaf.rdf#me> ;
	prv:performedAt "2009-10-07T12:00:00Z"^^xsd:dateTime .

<http://purl.org/net/provenance/ns#> prv:createdBy _:node183fu7k97x3 .

_:node183fu7k97x3 a prv:DataCreation ;
	prv:performedBy <http://www.informatik.hu-berlin.de/~hartig/foaf.rdf#olaf> , <http://users.ox.ac.uk/~zool0770/foaf.rdf#me> ;
	prv:performedAt "2009-10-07T12:00:00Z"^^xsd:dateTime .

<http://purl.org/net/provenance/ns#> prv:createdBy _:node183fu7k97x4 .

_:node183fu7k97x4 a prv:DataCreation ;
	prv:performedBy <http://www.informatik.hu-berlin.de/~hartig/foaf.rdf#olaf> , <http://users.ox.ac.uk/~zool0770/foaf.rdf#me> ;
	prv:performedAt "2009-10-07T12:00:00Z"^^xsd:dateTime .
