@prefix dc: <http://purl.org/dc/elements/1.1/> .
@prefix frbr: <http://purl.org/vocab/frbr/core#> .
@prefix vs: <http://www.w3.org/2003/06/sw-vocab-status/ns#> .
@prefix pbo: <http://purl.org/ontology/pbo/core#> .
@prefix dcterms: <http://purl.org/dc/terms/> .
@prefix rdfs: <http://www.w3.org/2000/01/rdf-schema#> .
@prefix co: <http://purl.org/ontology/co/core#> .
@prefix time: <http://www.w3.org/2006/time#> .
@prefix olo: <http://purl.org/ontology/olo/core#> .
@prefix bibo: <http://purl.org/ontology/bibo/> .
@prefix xsd: <http://www.w3.org/2001/XMLSchema#> .
@prefix owl: <http://www.w3.org/2002/07/owl#> .
@prefix rdf: <http://www.w3.org/1999/02/22-rdf-syntax-ns#> .
@prefix sim: <http://purl.org/ontology/similarity/> .

<http://purl.org/ontology/pbo/core#> a owl:Ontology ;
	dc:creator <http://foaf.me/zazi#me> , <http://kurtisrandom.com/foaf.rdf#kurtjx> ;
	dc:date "2010-09-13T18:31:52+01:00"^^xsd:dateTime ;
	dc:description """The Play Back Ontology specification provides basic concepts and properties 
for describing concepts that are related to the play back domain, e.g. an playlist, play back count and skip counter 
on/ for the Semantic Web. This document contains a RDF description of the Play Back Ontology."""@en ;
	dc:title "The Play Back Ontology"@en ;
	owl:imports <http://purl.org/NET/c4dm/event.owl> , <http://purl.org/dc/elements/1.1/> , <http://purl.org/ontology/bibo/> , <http://purl.org/ontology/co/core> , <http://purl.org/ontology/olo/core> , <http://purl.org/ontology/similarity/> , <http://purl.org/vocab/frbr/core> , <http://www.w3.org/2003/06/sw-vocab-status/ns> ;
	owl:versionInfo "0.6"^^xsd:decimal .

pbo:FixedPlaylist a owl:Class ;
	rdfs:comment """A (sub) playlist of a fixed length and a fixed order. This concept should be used to express static relations, 
e.g. \"those three music tracks must always be played in a row\"."""@en ;
	rdfs:isDefinedBy <http://purl.org/ontology/pbo/core#> ;
	rdfs:label "Fixed Playlist"@en ;
	rdfs:subClassOf pbo:Playlist ;
	vs:term_status "testing"@en .

pbo:MediaActionCounter a owl:Class ;
	rdfs:comment "A media action counter. Media actions are for example play back or skip events."^^xsd:string ;
	rdfs:isDefinedBy <http://purl.org/ontology/pbo/core#> ;
	rdfs:label "Media Action Counter"@en ;
	rdfs:subClassOf co:Counter ;
	vs:term_status "unstable"@en .

pbo:PlayBackCounter a owl:Class ;
	rdfs:comment "A play back counter, e.g. to count the playback of a media object."^^xsd:string ;
	rdfs:isDefinedBy <http://purl.org/ontology/pbo/core#> ;
	rdfs:label "Play Back Counter"@en ;
	rdfs:subClassOf pbo:MediaActionCounter ;
	vs:term_status "unstable"@en .

pbo:Playlist a owl:Class ;
	rdfs:comment "A playlist of specific media items, e.g. music tracks, videos or slides."@en ;
	rdfs:isDefinedBy <http://purl.org/ontology/pbo/core#> ;
	rdfs:label "Playlist"@en ;
	rdfs:subClassOf bibo:Document , olo:OrderedList ;
	vs:term_status "unstable"@en .

pbo:PlaylistSlot a owl:Class ;
	rdfs:comment """A playlist slot. It could contain e.g. a music track, a video or a slide, and maybe related with some 
additional properties. However, it could maybe also included a \"sub\" playlist, e.g. to keep a fixed sequence of some tracks."""@en ;
	rdfs:isDefinedBy <http://purl.org/ontology/pbo/core#> ;
	rdfs:label "Playlist Slot"@en ;
	rdfs:subClassOf olo:Slot , _:node17168lv1hx12 .

_:node17168lv1hx12 a owl:Restriction ;
	owl:minCardinality "1"^^xsd:nonNegativeInteger ;
	owl:onProperty pbo:playlist_item .

pbo:PlaylistSlot vs:term_status "testing"@en .

pbo:SkipCounter a owl:Class ;
	rdfs:comment "A skip counter, e.g. to count skip events of a media object."^^xsd:string ;
	rdfs:isDefinedBy <http://purl.org/ontology/pbo/core#> ;
	rdfs:label "Skip Counter"^^xsd:string ;
	rdfs:subClassOf pbo:MediaActionCounter ;
	vs:term_status "unstable"^^xsd:string .

pbo:SkipEvent a owl:Class ;
	rdfs:comment "A specific skip event of something."^^xsd:string ;
	rdfs:isDefinedBy <http://purl.org/ontology/pbo/core#> ;
	rdfs:label "Skip Event"^^xsd:string ;
	rdfs:subClassOf co:ScrobbleEvent ;
	vs:term_status "testing"^^xsd:string .

pbo:media_object a owl:ObjectProperty ;
	rdfs:comment "Associates a media object to its related counter."@en ;
	rdfs:domain pbo:MediaActionCounter ;
	rdfs:isDefinedBy <http://purl.org/ontology/pbo/core#> ;
	rdfs:label "has media object"@en ;
	rdfs:range _:node17168lv1hx13 .

_:node17168lv1hx13 a owl:Class ;
	owl:unionOf _:node17168lv1hx14 .

_:node17168lv1hx14 rdf:first bibo:Document ;
	rdf:rest _:node17168lv1hx15 .

_:node17168lv1hx15 rdf:first frbr:Endeavour ;
	rdf:rest rdf:nil .

pbo:media_object rdfs:subPropertyOf co:object ;
	vs:term_status "unstable"@en .

pbo:media_scrobble_object a owl:ObjectProperty ;
	rdfs:comment "A media specific scrobble object, e.g. a music track or a video."@en ;
	rdfs:isDefinedBy <http://purl.org/ontology/pbo/core#> ;
	rdfs:label "has media scrobble object"@en ;
	rdfs:range _:node17168lv1hx16 .

_:node17168lv1hx16 a owl:Class ;
	owl:unionOf _:node17168lv1hx17 .

_:node17168lv1hx17 rdf:first bibo:Document ;
	rdf:rest _:node17168lv1hx18 .

_:node17168lv1hx18 rdf:first frbr:Endeavour ;
	rdf:rest rdf:nil .

pbo:media_scrobble_object rdfs:subPropertyOf co:scrobble_object ;
	vs:term_status "testing"@en .

pbo:playlist a owl:ObjectProperty ;
	rdfs:comment "Associates a playlist to something."@en ;
	rdfs:domain owl:Thing ;
	rdfs:isDefinedBy <http://purl.org/ontology/pbo/core#> ;
	rdfs:label "has playlist"@en ;
	rdfs:range pbo:Playlist ;
	vs:term_status "testing"@en .

pbo:playlist_item a owl:ObjectProperty ;
	rdfs:comment """A specific playlist item, e.g. a music track, video or slides. The range types of this property must be 
based on bibo:Document or frbr:Endeavour (to keep it somehow media based)."""@en ;
	rdfs:domain pbo:PlaylistSlot ;
	rdfs:isDefinedBy <http://purl.org/ontology/pbo/core#> ;
	rdfs:label "has playlist item"@en ;
	rdfs:range _:node17168lv1hx19 .

_:node17168lv1hx19 a owl:Class ;
	owl:unionOf _:node17168lv1hx20 .

_:node17168lv1hx20 rdf:first bibo:Document ;
	rdf:rest _:node17168lv1hx21 .

_:node17168lv1hx21 rdf:first frbr:Endeavour ;
	rdf:rest rdf:nil .

pbo:playlist_item rdfs:subPropertyOf olo:item ;
	owl:inverseOf _:node17168lv1hx22 .

_:node17168lv1hx22 a owl:ObjectProperty ;
	rdfs:label "is playlist item of"@en .

pbo:playlist_item vs:term_status "unstable"@en .

pbo:playlist_slot a owl:ObjectProperty ;
	rdfs:comment "A specific slot in a playlist."@en ;
	rdfs:domain pbo:Playlist ;
	rdfs:label "has playlist slot"@en ;
	rdfs:range pbo:PlaylistSlot ;
	rdfs:subPropertyOf olo:slot ;
	vs:term_status "testing"@en .

pbo:skip_time a owl:ObjectProperty ;
	rdfs:comment "The moment, when someone skipped the media object, e.g. an instant of a timeline of an audio signal."^^xsd:string ;
	rdfs:domain pbo:SkipEvent ;
	rdfs:isDefinedBy <http://purl.org/ontology/pbo/core#> ;
	rdfs:label "has skip time"^^xsd:string ;
	rdfs:subPropertyOf <http://purl.org/NET/c4dm/event.owl#time> ;
	vs:term_status "testing"^^xsd:string .

pbo:transition a owl:ObjectProperty ;
	rdfs:comment "This relation directs to a description of a transition between two neighbouring playlist slots, e.g. two successive music tracks in a dj mix."@en ;
	rdfs:domain pbo:PlaylistSlot ;
	rdfs:isDefinedBy <http://purl.org/ontology/pbo/core#> ;
	rdfs:label "has transition"@en ;
	rdfs:subPropertyOf sim:association ;
	vs:term_status "testing"@en .
