@prefix :      <http://lod.taxonconcept.org/ontology/txn.owl#> .
@prefix usda_plants: <http://lod.taxonconcept.org/ontology/usda_plants.owl#> .
@prefix dwc_terms: <http://rs.tdwg.org/dwc/terms/index.htm#> .
@prefix gs_void: <http://lod.geospecies.org/ontology/void#> .
@prefix vann:  <http://purl.org/vocab/vann/> .
@prefix vs:    <http://www.w3.org/2003/06/sw-vocab-status/ns#> .
@prefix dcterms: <http://purl.org/dc/terms/> .
@prefix rdfs:  <http://www.w3.org/2000/01/rdf-schema#> .
@prefix owl2xml: <http://www.w3.org/2006/12/owl2-xml#> .
@prefix event: <http://purl.org/NET/c4dm/event.owl#> .
@prefix rdf:   <http://www.w3.org/1999/02/22-rdf-syntax-ns#> .
@prefix taxon: <http://purl.org/biodiversity/taxon/> .
@prefix dc:    <http://purl.org/dc/elements/1.1/> .
@prefix ia_mdb_void: <http://ia_mdb.geospecies.org/ontology/void#> .
@prefix biol:  <http://purl.org/NET/biol/ns#> .
@prefix wgs84_pos: <http://www.w3.org/2003/01/geo/wgs84_pos#> .
@prefix foaf:  <http://xmlns.com/foaf/0.1/> .
@prefix wo:    <http://purl.org/ontology/wo/> .
@prefix void:  <http://rdfs.org/ns/void#> .
@prefix txn_void: <http://lod.taxonconcept.org/ontology/void#> .
@prefix gn:    <http://www.geonames.org/ontology#> .
@prefix voaf:  <http://labs.mondeca.com/vocab/voaf#> .
@prefix uniprot_resource: <http://bio2rdf.org/uniprot_resource:> .
@prefix txn_people: <http://lod.taxonconcept.org/ontology/people.owl#> .
@prefix dwc_area: <http://lod.taxonconcept.org/ontology/dwc_area.owl#> .
@prefix bibo:  <http://purl.org/ontology/bibo/> .
@prefix xsd:   <http://www.w3.org/2001/XMLSchema#> .
@prefix owl:   <http://www.w3.org/2002/07/owl#> .
@prefix core:  <http://purl.uniprot.org/core/> .
@prefix doap:  <http://usefulinc.com/ns/doap#> .
@prefix skos:  <http://www.w3.org/2004/02/skos/core#> .
@prefix cc:    <http://creativecommons.org/ns#> .

:Sex_hermaphrodite  a        owl:NamedIndividual , :Sex , owl:Class ;
        rdfs:isDefinedBy     <http://lod.taxonconcept.org/ontology/txn.owl> ;
        rdfs:label           "hermaphrodite"@en ;
        dcterms:description  "one organism having both male and female sexual characteristics and organs; at birth an unambiguous assignment of male or female cannot be made"@en ;
        vs:term_status       "testing" .

:occurrenceHasIndividual
        a                 owl:ObjectProperty ;
        rdfs:comment      "Links an occurrence to an individual" ;
        rdfs:domain       :Occurrence ;
        rdfs:isDefinedBy  <http://lod.taxonconcept.org/ontology/txn.owl> ;
        rdfs:label        "occurrenceHasIndividual" ;
        vs:term_status    "testing" .

:botanyAuthorName  a        owl:DatatypeProperty ;
        rdfs:isDefinedBy    <http://lod.taxonconcept.org/ontology/txn.owl> ;
        rdfs:label          "botany author abbreviation" ;
        rdfs:subPropertyOf  foaf:nick ;
        vs:term_status      "testing" .

uniprot_resource:Taxon
        a       owl:Class .

:samplingProtocol  a      owl:ObjectProperty ;
        rdfs:comment      "Links an Occurrence to a standard vocabulary of sampling protocols as URI's" ;
        rdfs:domain       :Occurrence ;
        rdfs:isDefinedBy  <http://lod.taxonconcept.org/ontology/txn.owl> ;
        rdfs:label        "samplingProtocol" ;
        vs:term_status    "testing" .

:RankSubgenus  a          :TaxonRank , owl:NamedIndividual , owl:Class ;
        rdfs:isDefinedBy  <http://lod.taxonconcept.org/ontology/txn.owl> ;
        rdfs:label        "Rank Subgenus" ;
        vs:term_status    "testing" ;
        skos:broader      :RankGenus ;
        skos:narrower     :RankSpecies .

:RankSubclass  a          :TaxonRank , owl:NamedIndividual , owl:Class ;
        rdfs:isDefinedBy  <http://lod.taxonconcept.org/ontology/txn.owl> ;
        rdfs:label        "Rank Subclass" ;
        vs:term_status    "testing" ;
        skos:broader      :RankClass ;
        skos:narrower     :RankInfraclass .

:SpeciesImageTag  a       owl:Class ;
        rdfs:comment      "A tag like entity that can be used to indicate that an image is associated with a specific species concept. Instances of SpeciesImageTag take the form of the species concept URI with the fragment of #Image rather than #Species." ;
        rdfs:isDefinedBy  <http://lod.taxonconcept.org/ontology/txn.owl> ;
        rdfs:label        "SpeciesImageTag" ;
        vs:term_status    "testing" .

:hasAcceptedName  a         owl:DatatypeProperty ;
        rdfs:isDefinedBy    <http://lod.taxonconcept.org/ontology/txn.owl> ;
        rdfs:label          "hasAcceptedName" ;
        rdfs:subPropertyOf  skos:prefLabel ;
        vs:term_status      "deprecated" .

:hasDLPage  a               owl:ObjectProperty ;
        rdfs:comment        "The range is a page on the DiscoverLife.org site." ;
        rdfs:isDefinedBy    <http://lod.taxonconcept.org/ontology/txn.owl> ;
        rdfs:label          "hasDLPage" ;
        rdfs:range          bibo:Webpage ;
        rdfs:subPropertyOf  foaf:page ;
        vs:term_status      "testing" .

:hasDiscoverLifePage  a     owl:ObjectProperty ;
        rdfs:comment        "The range is a page on the http://www.discoverlife.org/ site." , "The range is a page on the Discover Life Web site." ;
        rdfs:isDefinedBy    <http://lod.taxonconcept.org/ontology/txn.owl> ;
        rdfs:label          "hasDiscoverLifePage" ;
        rdfs:range          bibo:Webpage ;
        rdfs:subPropertyOf  foaf:page ;
        vs:term_status      "testing" .

<http://dbpedia.org/property/classis>
        a       owl:DatatypeProperty .

:continent  a             owl:DatatypeProperty ;
        rdfs:isDefinedBy  <http://lod.taxonconcept.org/ontology/txn.owl> ;
        rdfs:label        "continent" ;
        vs:term_status    "testing" .

:radius  a                owl:DatatypeProperty ;
        rdfs:comment      "The radius in meters from a particular latitude, longitude point from within which a thing was observed or collected." ;
        rdfs:domain       :Area ;
        rdfs:isDefinedBy  <http://lod.taxonconcept.org/ontology/txn.owl> ;
        rdfs:label        "radius" .

:MarineHabitat  a            owl:Class ;
        rdfs:isDefinedBy     <http://lod.taxonconcept.org/ontology/txn.owl> ;
        rdfs:label           "FreshwaterHabitat" ;
        rdfs:subClassOf      :Habitat ;
        owl:equivalentClass  wo:MarineHabitat ;
        vs:term_status       "testing" .

:countryCode  a           owl:DatatypeProperty ;
        rdfs:isDefinedBy  <http://lod.taxonconcept.org/ontology/txn.owl> ;
        rdfs:label        "countryCode" ;
        vs:term_status    "testing" .

:isWikispeciesArticleOf
        a                 owl:ObjectProperty ;
        rdfs:domain       bibo:Webpage ;
        rdfs:isDefinedBy  <http://lod.taxonconcept.org/ontology/txn.owl> ;
        rdfs:label        "isWikispeciesArticleOf" ;
        owl:inverseOf     :hasWikispeciesArticle ;
        vs:term_status    "testing" .

:Status_Testing  a        owl:NamedIndividual , skos:Concept ;
        rdfs:isDefinedBy  <http://lod.taxonconcept.org/ontology/txn.owl> ;
        rdfs:label        "Status_Testing" ;
        vs:term_status    "testing" .

:hasGBIFPage  a             owl:ObjectProperty ;
        rdfs:comment        "A page at GBIF.org"@en ;
        rdfs:isDefinedBy    <http://lod.taxonconcept.org/ontology/txn.owl> ;
        rdfs:label          "hasGBIFPage" ;
        rdfs:range          bibo:Webpage ;
        rdfs:subPropertyOf  foaf:page ;
        vs:term_status      "testing" .

:TDWG2010_BioBlitz_Project
        a                 owl:NamedIndividual , foaf:Project ;
        rdfs:isDefinedBy  <http://lod.taxonconcept.org/ontology/txn.owl> ;
        rdfs:label        "TDWG2010 BioBlitz Project" ;
        vs:term_status    "testing" .

dcterms:description  a  owl:DatatypeProperty .

:Identification  a        owl:Class ;
        rdfs:comment      "An identification action. The identification of a specimen." ;
        rdfs:isDefinedBy  <http://lod.taxonconcept.org/ontology/txn.owl> ;
        rdfs:label        "Identification" ;
        rdfs:subClassOf   event:Event ;
        vs:term_status    "testing" .

:RankDivision  a          :TaxonRank , owl:NamedIndividual , owl:Class ;
        rdfs:isDefinedBy  <http://lod.taxonconcept.org/ontology/txn.owl> ;
        rdfs:label        "Rank Division" ;
        vs:term_status    "testing" .

<http://dbpedia.org/property/phylum>
        a       owl:DatatypeProperty .

:hasImage  a                    owl:ObjectProperty ;
        rdfs:comment            "Superproperty of all the links to images" ;
        rdfs:isDefinedBy        <http://lod.taxonconcept.org/ontology/txn.owl> ;
        rdfs:label              "hasImage" ;
        owl:equivalentProperty  foaf:depiction ;
        vs:term_status          "testing" .

:canonicalFormID_Of  a      owl:ObjectProperty ;
        rdfs:comment        "The URI ID for the scientific name with authorship form of the name i.e. Puma concolor Linnaeus 1758, for name to name mapping" ;
        rdfs:domain         :TaxonNameID ;
        rdfs:isDefinedBy    <http://lod.taxonconcept.org/ontology/taxon.owl> ;
        rdfs:label          "canonicalFormID Of" ;
        rdfs:range          :TaxonNameID ;
        rdfs:subPropertyOf  :relatedTaxonNameID .

<http://dbpedia.org/property/familia>
        a       owl:DatatypeProperty .

core:Taxon  a   owl:Class .

biol:order  a   owl:DatatypeProperty .

:TaxonOntology  a         owl:Class ;
        rdfs:isDefinedBy  <http://lod.taxonconcept.org/ontology/txn.owl> ;
        rdfs:label        "TaxonOntology" ;
        vs:term_status    "testing" .

:hasWikipediaMap  a         owl:ObjectProperty ;
        rdfs:isDefinedBy    <http://lod.taxonconcept.org/ontology/txn.owl> ;
        rdfs:label          "hasWikipediaMap" ;
        rdfs:range          :MapImage ;
        rdfs:subPropertyOf  :hasMapImage ;
        vs:term_status      "testing" .

:identificationMethod
        a                 owl:ObjectProperty ;
        rdfs:comment      "Method used to identify the individual, as a URI" ;
        rdfs:domain       :Identification ;
        rdfs:isDefinedBy  <http://lod.taxonconcept.org/ontology/txn.owl> ;
        rdfs:label        "identificationMethod" ;
        vs:term_status    "testing" .

:RankSpecies  a           :TaxonRank , owl:NamedIndividual , owl:Class ;
        rdfs:isDefinedBy  <http://lod.taxonconcept.org/ontology/txn.owl> ;
        rdfs:label        "Rank Species" ;
        vs:term_status    "testing" ;
        skos:broader      :RankSubgenus ;
        skos:narrower     :RankSubpecies .

:RankParvorder  a         :TaxonRank , owl:NamedIndividual , owl:Class ;
        rdfs:isDefinedBy  <http://lod.taxonconcept.org/ontology/txn.owl> ;
        rdfs:label        "Rank Parvorder" ;
        vs:term_status    "testing" ;
        skos:broader      :RankInfraorder ;
        skos:narrower     :RankSuperfamily .

:occurrenceInStateProvince
        a                 owl:ObjectProperty ;
        rdfs:comment      "Links an Occurrence to Geonames StateProvince URI" ;
        rdfs:domain       :Occurrence ;
        rdfs:isDefinedBy  <http://lod.taxonconcept.org/ontology/txn.owl> ;
        rdfs:label        "occurrenceInStateProvince" ;
        rdfs:range        gn:Feature ;
        vs:term_status    "testing" .

foaf:workInfoHomepage
        a       owl:ObjectProperty .

:taxonNameID  a           owl:ObjectProperty ;
        rdfs:comment      "The URI to the Taxon Name String" ;
        rdfs:isDefinedBy  <http://lod.taxonconcept.org/ontology/txn.owl> ;
        rdfs:label        "taxonNameID" ;
        rdfs:range        :TaxonNameID ;
        vs:term_status    "testing" .

dcterms:hasPart  a  owl:ObjectProperty .

:inPhylum  a              owl:ObjectProperty ;
        rdfs:isDefinedBy  <http://lod.taxonconcept.org/ontology/txn.owl> ;
        rdfs:label        "inPhylum" ;
        vs:term_status    "testing" .

:identificationHasLabelImage
        a                   owl:ObjectProperty ;
        rdfs:comment        "The image of the identification label on a specimen" ;
        rdfs:domain         :Identification ;
        rdfs:isDefinedBy    <http://lod.taxonconcept.org/ontology/txn.owl> ;
        rdfs:label          "identificationHasLabelImage" ;
        rdfs:range          :Image ;
        rdfs:subPropertyOf  :hasImage ;
        vs:term_status      "testing" .

:habitat  a                     owl:ObjectProperty ;
        rdfs:comment            "associates a taxon with a habitat in which it may typically be found" ;
        rdfs:isDefinedBy        <http://lod.taxonconcept.org/ontology/txn.owl> ;
        rdfs:label              "habitat" ;
        owl:equivalentProperty  wo:habitat ;
        vs:term_status          "testing" .

<http://dbpedia.org/property/genus>
        a       owl:DatatypeProperty .

:Area   a                 owl:Class ;
        rdfs:isDefinedBy  <http://lod.taxonconcept.org/ontology/txn.owl> ;
        rdfs:label        "Area" ;
        rdfs:subClassOf   wgs84_pos:SpatialThing ;
        vs:term_status    "testing" .

:originalName  a            owl:DatatypeProperty ;
        rdfs:isDefinedBy    <http://lod.taxonconcept.org/ontology/txn.owl> ;
        rdfs:label          "originalName" ;
        rdfs:subPropertyOf  skos:altLabel ;
        vs:term_status      "testing" .

:hasBioimagesPage  a        owl:ObjectProperty ;
        rdfs:comment        "The range is a page on the Bioimages site." ;
        rdfs:isDefinedBy    <http://lod.taxonconcept.org/ontology/txn.owl> ;
        rdfs:label          "hasBioimagesPage" ;
        rdfs:range          bibo:Webpage ;
        rdfs:subPropertyOf  foaf:page ;
        vs:term_status      "testing" .

:individualHasPreviousIdentificationAssertion
        a                 owl:ObjectProperty ;
        rdfs:comment      "Links an individual to the most appropriate identification. Zero to many" ;
        rdfs:domain       :SpeciesIndividual ;
        rdfs:isDefinedBy  <http://lod.taxonconcept.org/ontology/txn.owl> ;
        rdfs:label        "individualHasPreviousIdentificationAssertion" ;
        vs:term_status    "testing" .

:inCoLKingdom  a          owl:ObjectProperty ;
        rdfs:comment      "Links a species concept to a Catalog of Life Kingdom in an ontology" ;
        rdfs:isDefinedBy  <http://lod.taxonconcept.org/ontology/txn.owl> ;
        rdfs:label        "inCoLKingdom" ;
        vs:term_status    "testing" .

skos:broader  a  owl:ObjectProperty .

:heterochresonymID  a       owl:ObjectProperty ;
        rdfs:comment        "The URI to the Heterochresonym Name String" ;
        rdfs:isDefinedBy    <http://lod.taxonconcept.org/ontology/txn.owl> ;
        rdfs:label          "heterochresonymID" ;
        rdfs:range          :TaxonNameID ;
        rdfs:subPropertyOf  :synonymID ;
        vs:term_status      "testing" .

:institutionCode  a       owl:DatatypeProperty ;
        rdfs:isDefinedBy  <http://lod.taxonconcept.org/ontology/txn.owl> ;
        rdfs:label        "institutionCode" ;
        vs:term_status    "testing" .

dwc_area:radius  a  owl:DatatypeProperty .

skos:ConceptScheme  a  owl:Class .

:taxonRank  a             owl:DatatypeProperty ;
        rdfs:isDefinedBy  <http://lod.taxonconcept.org/ontology/txn.owl> ;
        rdfs:label        "taxonRank" ;
        vs:term_status    "testing" .

dwc_terms:acceptedNameUsageID
        a       owl:ObjectProperty .

:inFamily  a              owl:ObjectProperty ;
        rdfs:isDefinedBy  <http://lod.taxonconcept.org/ontology/txn.owl> ;
        rdfs:label        "inFamily" ;
        vs:term_status    "testing" .

:RankInfraorder  a        :TaxonRank , owl:NamedIndividual , owl:Class ;
        rdfs:isDefinedBy  <http://lod.taxonconcept.org/ontology/txn.owl> ;
        rdfs:label        "Rank Infraorder" ;
        vs:term_status    "testing" ;
        skos:broader      :RankSuborder ;
        skos:narrower     :RankParvorder .

:hasGBIFMap  a              owl:ObjectProperty ;
        rdfs:isDefinedBy    <http://lod.taxonconcept.org/ontology/txn.owl> ;
        rdfs:label          "hasGBIFmap" ;
        rdfs:range          :MapImage ;
        rdfs:subPropertyOf  :hasMapImage ;
        vs:term_status      "testing" .

:infraspecificEpithet
        a                   owl:DatatypeProperty ;
        rdfs:isDefinedBy    <http://lod.taxonconcept.org/ontology/txn.owl> ;
        rdfs:label          "infraspecificEpithet" ;
        rdfs:subPropertyOf  :scientificName ;
        vs:term_status      "testing" .

:speciesConcepthasVaritypeSpecimen
        a                 owl:ObjectProperty ;
        rdfs:comment      "Links a species concept to a varitype specimen" ;
        rdfs:isDefinedBy  <http://lod.taxonconcept.org/ontology/txn.owl> ;
        rdfs:label        "speciesConcepthasVaritypeSpecimen" ;
        owl:inverseOf     :varitypeSpecimenHasSpeciesConcept ;
        vs:term_status    "testing" .

:RankSubspecificAggregate
        a                 :TaxonRank , owl:NamedIndividual , owl:Class ;
        rdfs:isDefinedBy  <http://lod.taxonconcept.org/ontology/txn.owl> ;
        rdfs:label        "Rank SubspecificAggregate" ;
        vs:term_status    "testing" ;
        skos:broader      :RankSpecies .

:RankSubkingdom  a        :TaxonRank , owl:NamedIndividual , owl:Class ;
        rdfs:isDefinedBy  <http://lod.taxonconcept.org/ontology/txn.owl> ;
        rdfs:label        "Rank Subkingdom" ;
        vs:term_status    "testing" ;
        skos:broader      :RankKingdom ;
        skos:narrower     :RankInfrakingdom .

:hasCollector  a          owl:ObjectProperty ;
        rdfs:comment      "The occurrence observer or specimen collector, hasCollector?" ;
        rdfs:domain       :Occurrence ;
        rdfs:isDefinedBy  <http://lod.taxonconcept.org/ontology/txn.owl> ;
        rdfs:label        "hasCollector" ;
        rdfs:range        foaf:Person ;
        vs:term_status    "testing" .

:areaInStateProvince  a   owl:ObjectProperty ;
        rdfs:comment      "Links an Area to Geonames State/Province URI" ;
        rdfs:isDefinedBy  <http://lod.taxonconcept.org/ontology/txn.owl> ;
        rdfs:label        "areaInStateProvince" ;
        vs:term_status    "testing" .

:identificationReference
        a                 owl:ObjectProperty ;
        rdfs:comment      "Links an identification to the URI for the reference used." ;
        rdfs:isDefinedBy  <http://lod.taxonconcept.org/ontology/txn.owl> ;
        rdfs:label        "identificationReference" ;
        vs:term_status    "testing" .

:scientificName  a          owl:DatatypeProperty ;
        rdfs:isDefinedBy    <http://lod.taxonconcept.org/ontology/txn.owl> ;
        rdfs:label          "scientificName" ;
        rdfs:subPropertyOf  taxon:scientificName ;
        vs:term_status      "testing" .

dwc_area:Area  a  owl:Class .

:uniprotKingdom  a        owl:ObjectProperty ;
        rdfs:isDefinedBy  <http://lod.taxonconcept.org/ontology/taxon.owl> ;
        rdfs:label        "uniprotKingdom"@en ;
        rdfs:range        core:Taxon .

biol:commonName  a  owl:DatatypeProperty .

:stateProvince  a         owl:DatatypeProperty ;
        rdfs:isDefinedBy  <http://lod.taxonconcept.org/ontology/txn.owl> ;
        rdfs:label        "stateProvince" ;
        vs:term_status    "testing" .

:originalNameID_Of  a       owl:ObjectProperty ;
        rdfs:domain         :TaxonNameID ;
        rdfs:isDefinedBy    <http://lod.taxonconcept.org/ontology/txn.owl> ;
        rdfs:label          "originalNameID_Of" ;
        rdfs:subPropertyOf  :taxonNameID_Of ;
        owl:inverseOf       :originalNameID ;
        vs:term_status      "testing" .

:specificEpithet  a         owl:DatatypeProperty ;
        rdfs:isDefinedBy    <http://lod.taxonconcept.org/ontology/txn.owl> ;
        rdfs:label          "Specific epithet" ;
        rdfs:subPropertyOf  :scientificName ;
        vs:term_status      "testing" .

:descYearOf  a            owl:ObjectProperty ;
        rdfs:domain       :Year ;
        rdfs:isDefinedBy  <http://lod.taxonconcept.org/ontology/txn.owl> ;
        rdfs:label        "descYearOf" ;
        owl:inverseOf     :descYear ;
        vs:term_status    "testing" .

event:Event  a  owl:Class .

:inSuborder  a            owl:ObjectProperty ;
        rdfs:isDefinedBy  <http://lod.taxonconcept.org/ontology/txn.owl> ;
        rdfs:label        "inSuborder" ;
        vs:term_status    "testing" .

:phylum  a                  owl:DatatypeProperty ;
        rdfs:isDefinedBy    <http://lod.taxonconcept.org/ontology/txn.owl> ;
        rdfs:label          "phylum" ;
        rdfs:subPropertyOf  :scientificName ;
        vs:term_status      "testing" .

:behavioralNote  a        owl:DatatypeProperty ;
        rdfs:isDefinedBy  <http://lod.taxonconcept.org/ontology/txn.owl> ;
        rdfs:label        "behavioralNote" ;
        vs:term_status    "testing" .

:inCoLPhylum  a           owl:ObjectProperty ;
        rdfs:comment      "Links a species concept to a Catalog of Life Phylum in an ontology" ;
        rdfs:isDefinedBy  <http://lod.taxonconcept.org/ontology/txn.owl> ;
        rdfs:label        "inCoLPhylum" ;
        vs:term_status    "testing" .

dcterms:creator  a  owl:AnnotationProperty .

:firstAuthorID  a         owl:ObjectProperty ;
        rdfs:comment      "The URI to the First Author" ;
        rdfs:domain       :TaxonNameID ;
        rdfs:isDefinedBy  <http://lod.taxonconcept.org/ontology/txn.owl> ;
        rdfs:label        "firstAuthorID" ;
        rdfs:range        :Taxonomist ;
        vs:term_status    "testing" .

:trinomial  a               owl:DatatypeProperty ;
        rdfs:isDefinedBy    <http://lod.taxonconcept.org/ontology/txn.owl> ;
        rdfs:label          "trinomial" ;
        rdfs:subPropertyOf  taxon:trinomial ;
        vs:term_status      "testing" .

:hasEOLPage  a              owl:ObjectProperty ;
        rdfs:comment        "The range is a page on the Encyclopedia of Life site." ;
        rdfs:isDefinedBy    <http://lod.taxonconcept.org/ontology/txn.owl> ;
        rdfs:label          "hasEOLPage" ;
        rdfs:range          bibo:Webpage ;
        rdfs:subPropertyOf  foaf:page ;
        vs:term_status      "testing" .

:Year   a                 owl:Class ;
        rdfs:comment      "Class for the Concept Year"@en ;
        rdfs:isDefinedBy  <http://lod.taxonconcept.org/ontology/txn.owl> ;
        rdfs:label        "Year"@en ;
        rdfs:subClassOf   <http://www.w3.org/2006/time#DateTimeDescription> ;
        vs:term_status    "testing" .

:relatedTaxonNameID  a    owl:ObjectProperty ;
        rdfs:comment      "The URI to the Taxon Name String" ;
        rdfs:domain       :TaxonNameID ;
        rdfs:isDefinedBy  <http://lod.taxonconcept.org/ontology/txn.owl> ;
        rdfs:label        "relatedTaxonNameID" ;
        rdfs:range        :TaxonNameID ;
        vs:term_status    "testing" .

:RankFamily  a            :TaxonRank , owl:NamedIndividual , owl:Class ;
        rdfs:isDefinedBy  <http://lod.taxonconcept.org/ontology/txn.owl> ;
        rdfs:label        "Rank Family" ;
        vs:term_status    "testing" ;
        skos:broader      :RankSuperfamily ;
        skos:narrower     :RankSubfamily .

foaf:page  a    owl:ObjectProperty .

dc:title  a     owl:AnnotationProperty .

:conceptStatus  a         owl:ObjectProperty ;
        rdfs:comment      "The Links to the Status of the TaxonConcept" ;
        rdfs:isDefinedBy  <http://lod.taxonconcept.org/ontology/txn.owl> ;
        rdfs:label        "conceptStatus" ;
        vs:term_status    "testing" .

<http://www.w3.org/2006/time#DateTimeDescription>
        a       owl:Class .

taxon:commonName  a  owl:DatatypeProperty .

:MonomialNameID  a        owl:Class ;
        rdfs:isDefinedBy  <http://lod.taxonconcept.org/ontology/txn.owl> ;
        rdfs:label        "MonomialNameID" ;
        rdfs:subClassOf   :ScientificNameID ;
        vs:term_status    "testing" .

:hasNCBI  a               owl:DatatypeProperty ;
        rdfs:comment      "The NCBI Taxonomy ID" ;
        rdfs:isDefinedBy  <http://lod.taxonconcept.org/ontology/txn.owl> ;
        rdfs:label        "hasNCBI" ;
        vs:term_status    "testing" .

:hasMapImage  a             owl:ObjectProperty ;
        rdfs:isDefinedBy    <http://lod.taxonconcept.org/ontology/txn.owl> ;
        rdfs:label          "hasMapImage" ;
        rdfs:range          :MapImage ;
        rdfs:subPropertyOf  foaf:depiction ;
        vs:term_status      "testing" .

:RankDomain  a            :TaxonRank , owl:NamedIndividual , owl:Class ;
        rdfs:isDefinedBy  <http://lod.taxonconcept.org/ontology/txn.owl> ;
        rdfs:label        "Rank Domain" ;
        vs:term_status    "testing" ;
        skos:narrower     :RankSubdomain .

:basisOfRecord  a         owl:ObjectProperty ;
        rdfs:comment      "Assumed to be equivalent to TDWG Basis of Record" ;
        rdfs:isDefinedBy  <http://lod.taxonconcept.org/ontology/txn.owl> ;
        rdfs:label        "basisOfRecord" ;
        vs:term_status    "testing" .

:isBioimagesPageOf  a     owl:ObjectProperty ;
        rdfs:domain       bibo:Webpage ;
        rdfs:isDefinedBy  <http://lod.taxonconcept.org/ontology/txn.owl> ;
        rdfs:label        "isBioimagesPageOf" ;
        owl:inverseOf     :hasBioimagesPage ;
        vs:term_status    "testing" .

:acceptedName  a            owl:DatatypeProperty ;
        rdfs:isDefinedBy    <http://lod.taxonconcept.org/ontology/txn.owl> ;
        rdfs:label          "acceptedName" ;
        rdfs:subPropertyOf  skos:prefLabel ;
        vs:term_status      "testing" .

:SpeciesConcept  a        owl:Class ;
        rdfs:isDefinedBy  <http://lod.taxonconcept.org/ontology/txn.owl> ;
        rdfs:label        "SpeciesConcept" ;
        rdfs:subClassOf   :TaxonConcept ;
        vs:term_status    "testing" .

<http://dbpedia.org/property/trinomial>
        a       owl:DatatypeProperty .

dcterms:title  a  owl:DatatypeProperty , owl:AnnotationProperty .

:areaInCounty  a          owl:ObjectProperty ;
        rdfs:comment      "Links an Area to Geonames County URI" ;
        rdfs:isDefinedBy  <http://lod.taxonconcept.org/ontology/txn.owl> ;
        rdfs:label        "areaInCounty" ;
        vs:term_status    "testing" .

skos:Concept  a  owl:Class .

vs:term_status  a  owl:AnnotationProperty .

:speciesConceptHasOcccurrence
        a                 owl:ObjectProperty ;
        rdfs:comment      "Links a species to an occurrence. Should be speciesConcept?" ;
        rdfs:domain       :SpeciesConcept ;
        rdfs:isDefinedBy  <http://lod.taxonconcept.org/ontology/txn.owl> ;
        rdfs:label        "speciesConceptHasOcccurrence" ;
        vs:term_status    "testing" .

:hasCitation  a             owl:ObjectProperty ;
        rdfs:comment        "The range is a uniprot pubmed uri for example http://purl.uniprot.org/pubmed/1083304 " ;
        rdfs:isDefinedBy    <http://lod.taxonconcept.org/ontology/txn.owl> ;
        rdfs:label          "hasCitation" ;
        rdfs:range          core:Citation ;
        rdfs:subPropertyOf  foaf:page ;
        vs:term_status      "testing" .

:isUnknownAboutIn  a      owl:ObjectProperty ;
        rdfs:comment      "Links a species concept to a Geonames URI where the relationship is unknown" ;
        rdfs:isDefinedBy  <http://lod.taxonconcept.org/ontology/txn.owl> ;
        rdfs:label        "isUnknownAboutIn" ;
        vs:term_status    "testing" .

skos:prefLabel  a  owl:DatatypeProperty .

:inCoLClass  a            owl:ObjectProperty ;
        rdfs:comment      "Links a species concept to a Catalog of Life Class in an ontology" ;
        rdfs:isDefinedBy  <http://lod.taxonconcept.org/ontology/txn.owl> ;
        rdfs:label        "inCoLClass" ;
        vs:term_status    "testing" .

:occurrenceInCounty  a    owl:ObjectProperty ;
        rdfs:comment      "Links an Occurrence to Geonames County URI" ;
        rdfs:domain       :Occurrence ;
        rdfs:isDefinedBy  <http://lod.taxonconcept.org/ontology/txn.owl> ;
        rdfs:label        "occurrenceInCounty" ;
        rdfs:range        gn:Feature ;
        vs:term_status    "testing" .

:taxonNameGroupID  a      owl:ObjectProperty ;
        rdfs:comment      "The URI to the Taxon Name Group String" ;
        rdfs:isDefinedBy  <http://lod.taxonconcept.org/ontology/txn.owl> ;
        rdfs:label        "taxonNameGroupID" ;
        vs:term_status    "testing" .

owl:versionInfo  a  owl:AnnotationProperty .

:hasEtypePage  a            owl:ObjectProperty ;
        rdfs:isDefinedBy    <http://lod.taxonconcept.org/ontology/txn.owl> ;
        rdfs:label          "hasEtypePage" ;
        rdfs:range          bibo:Webpage ;
        rdfs:subPropertyOf  foaf:page ;
        vs:term_status      "testing" .

:georeferenceVerificationStatus
        a                 owl:ObjectProperty ;
        rdfs:comment      "Was this location verified, controlled choices URI" ;
        rdfs:isDefinedBy  <http://lod.taxonconcept.org/ontology/txn.owl> ;
        rdfs:label        "georeferenceVerificationStatus" ;
        vs:term_status    "testing" .

<http://dbpedia.org/property/regnum>
        a       owl:DatatypeProperty .

dcterms:partOf  a  owl:ObjectProperty .

:kingdom  a                 owl:DatatypeProperty ;
        rdfs:isDefinedBy    <http://lod.taxonconcept.org/ontology/txn.owl> ;
        rdfs:label          "kingdom" ;
        rdfs:subPropertyOf  :scientificName ;
        vs:term_status      "testing" .

:hasSpeciesConceptID  a   owl:DatatypeProperty ;
        rdfs:comment      "This is for a string urn type identifier" ;
        rdfs:domain       :SpeciesConcept ;
        rdfs:isDefinedBy  <http://lod.taxonconcept.org/ontology/txn.owl> ;
        rdfs:label        "hasSpeciesConceptID" ;
        vs:term_status    "testing" .

<http://dbpedia.org/property/species>
        a       owl:DatatypeProperty .

:Sex_male  a                 owl:NamedIndividual , :Sex , owl:Class ;
        rdfs:isDefinedBy     <http://lod.taxonconcept.org/ontology/txn.owl> ;
        rdfs:label           "male"@en ;
        dcterms:description  "Male (♂) refers to the sex of an organism, or part of an organism, which produces small mobile gametes, called spermatozoa."@en ;
        vs:term_status       "testing" .

:occurrenceHasArea  a     owl:ObjectProperty ;
        rdfs:comment      "Links an occurrence to an area" ;
        rdfs:domain       :Occurrence ;
        rdfs:isDefinedBy  <http://lod.taxonconcept.org/ontology/txn.owl> ;
        rdfs:label        "occurrenceHasArea" ;
        rdfs:range        :Area ;
        vs:term_status    "testing" .

:RankOrder  a             :TaxonRank , owl:NamedIndividual , owl:Class ;
        rdfs:isDefinedBy  <http://lod.taxonconcept.org/ontology/txn.owl> ;
        rdfs:label        "Rank Order" ;
        vs:term_status    "testing" ;
        skos:broader      :RankSuperorder ;
        skos:narrower     :RankSuborder .

taxon:DataObject  a  owl:Class .

:GenusNameID  a           owl:Class ;
        rdfs:isDefinedBy  <http://lod.taxonconcept.org/ontology/txn.owl> ;
        rdfs:label        "GenusNameID" ;
        rdfs:subClassOf   :MonomialNameID ;
        vs:term_status    "testing" .

:RankSubdivision  a       :TaxonRank , owl:NamedIndividual , owl:Class ;
        rdfs:isDefinedBy  <http://lod.taxonconcept.org/ontology/txn.owl> ;
        rdfs:label        "Rank Subdivision" ;
        vs:term_status    "testing" .

wo:Habitat  a   owl:Class .

dwc_terms:vernacularName
        a       owl:DatatypeProperty .

wgs84_pos:SpatialThing
        a       owl:Class .

rdfs:isDefinedBy  a  owl:AnnotationProperty .

:Occurrence  a            owl:Class ;
        rdfs:isDefinedBy  <http://lod.taxonconcept.org/ontology/txn.owl> ;
        rdfs:label        "Occurrence" ;
        rdfs:subClassOf   event:Event ;
        vs:term_status    "testing" .

:areaHasOccurrence  a     owl:ObjectProperty ;
        rdfs:comment      "Links an Area to an Occurrence" ;
        rdfs:isDefinedBy  <http://lod.taxonconcept.org/ontology/txn.owl> ;
        rdfs:label        "areaHasOccurrence" ;
        vs:term_status    "testing" .

:descYear  a              owl:ObjectProperty ;
        rdfs:comment      "This is the year of the description" ;
        rdfs:isDefinedBy  <http://lod.taxonconcept.org/ontology/txn.owl> ;
        rdfs:label        "descYear" ;
        rdfs:range        :Year ;
        vs:term_status    "testing" .

skos:hiddenLabel  a  owl:DatatypeProperty .

:inInfraclass  a          owl:ObjectProperty ;
        rdfs:isDefinedBy  <http://lod.taxonconcept.org/ontology/txn.owl> ;
        rdfs:label        "inInfraclass" ;
        vs:term_status    "testing" .

:SpeciesModel  a          owl:Class ;
        rdfs:isDefinedBy  <http://lod.taxonconcept.org/ontology/txn.owl> ;
        rdfs:label        "SpeciesModel" ;
        vs:term_status    "testing" .

core:Citation  a  owl:Class .

:isBugGuidePageOf  a      owl:ObjectProperty ;
        rdfs:domain       bibo:Webpage ;
        rdfs:isDefinedBy  <http://lod.taxonconcept.org/ontology/txn.owl> ;
        rdfs:label        "isBugGuidePageOf" ;
        owl:inverseOf     :hasBugGuidePage ;
        vs:term_status    "testing" .

:hasEbird  a              owl:DatatypeProperty ;
        rdfs:comment      "eBird Species Code" ;
        rdfs:isDefinedBy  <http://lod.taxonconcept.org/ontology/txn.owl> ;
        rdfs:label        "hasEbird" ;
        vs:term_status    "testing" .

:homotypicNameID  a         owl:ObjectProperty ;
        rdfs:comment        "The URI to the HomotypicName Name String" ;
        rdfs:isDefinedBy    <http://lod.taxonconcept.org/ontology/txn.owl> ;
        rdfs:label          "homotypicNameID" ;
        rdfs:range          :TaxonNameID ;
        rdfs:subPropertyOf  :synonymID ;
        vs:term_status      "testing" .

:uniprotOrder  a          owl:ObjectProperty ;
        rdfs:isDefinedBy  <http://lod.taxonconcept.org/ontology/taxon.owl> ;
        rdfs:label        "uniprotOrder"@en ;
        rdfs:range        core:Taxon .

:ScientificNameID  a      owl:Class ;
        rdfs:isDefinedBy  <http://lod.taxonconcept.org/ontology/txn.owl> ;
        rdfs:label        "ScientificNameID" ;
        rdfs:subClassOf   :TaxonNameID ;
        vs:term_status    "testing" .

:inDBpediaClade  a        owl:ObjectProperty ;
        rdfs:comment      "Links a species concept to a clade in the DBpedia ontology" ;
        rdfs:isDefinedBy  <http://lod.taxonconcept.org/ontology/txn.owl> ;
        rdfs:label        "inDBpediaClade" ;
        vs:term_status    "testing" .

:individualHasOccurrence
        a                 owl:ObjectProperty ;
        rdfs:comment      "Links an individual to an Occurrence, correct" ;
        rdfs:domain       :SpeciesIndividual ;
        rdfs:isDefinedBy  <http://lod.taxonconcept.org/ontology/txn.owl> ;
        rdfs:label        "individualHasOccurrence" ;
        vs:term_status    "testing" .

owl:Thing  a    owl:Class .

:TrinomialNameID  a       owl:Class ;
        rdfs:isDefinedBy  <http://lod.taxonconcept.org/ontology/txn.owl> ;
        rdfs:label        "TrinomialNameID" ;
        rdfs:subClassOf   :ScientificNameID ;
        vs:term_status    "testing" .

biol:class  a   owl:DatatypeProperty .

:Taxonomist  a            owl:Class ;
        rdfs:comment      "Class for a Taxonomist a subclass of dbpedia-owl:Scientist"@en ;
        rdfs:isDefinedBy  <http://lod.taxonconcept.org/ontology/txn.owl> ;
        rdfs:label        "Taxonomist"@en ;
        rdfs:subClassOf   :Scientist ;
        vs:term_status    "testing" .

biol:genus  a   owl:DatatypeProperty .

:occurrenceHasLabelImage
        a                   owl:ObjectProperty ;
        rdfs:comment        "The image of the occurrence label on a specimen" ;
        rdfs:domain         :Occurrence ;
        rdfs:isDefinedBy    <http://lod.taxonconcept.org/ontology/txn.owl> ;
        rdfs:label          "occurrenceHasLabelImage" ;
        rdfs:range          :Image ;
        rdfs:subPropertyOf  :hasImage ;
        vs:term_status      "testing" .

:FamilyNameID  a          owl:Class ;
        rdfs:isDefinedBy  <http://lod.taxonconcept.org/ontology/txn.owl> ;
        rdfs:label        "FamilyNameID" ;
        rdfs:subClassOf   :MonomialNameID ;
        vs:term_status    "testing" .

biol:kingdom  a  owl:DatatypeProperty .

:hasWildObsPage  a          owl:ObjectProperty ;
        rdfs:isDefinedBy    <http://lod.taxonconcept.org/ontology/txn.owl> ;
        rdfs:label          "hasWildObsPage" ;
        rdfs:range          bibo:Webpage ;
        rdfs:subPropertyOf  foaf:page ;
        vs:term_status      "testing" .

:hasITIS  a               owl:DatatypeProperty ;
        rdfs:comment      "The ITIS ID" ;
        rdfs:isDefinedBy  <http://lod.taxonconcept.org/ontology/txn.owl> ;
        rdfs:label        "hasITIS" ;
        vs:term_status    "testing" .

dwc_terms:originalNameUsageID
        a       owl:ObjectProperty .

:individualHasCurrrentIdentificationAssertion
        a                 owl:ObjectProperty ;
        rdfs:comment      "Links an individual to the most appropriate identification. Should be one." ;
        rdfs:domain       :SpeciesIndividual ;
        rdfs:isDefinedBy  <http://lod.taxonconcept.org/ontology/txn.owl> ;
        rdfs:label        "individualHasCurrrentIdentificationAssertion" ;
        vs:term_status    "testing" .

<http://www.uniprot.org/core/scientificName>
        a       owl:DatatypeProperty .

:RankVariety  a           :TaxonRank , owl:NamedIndividual , owl:Class ;
        rdfs:isDefinedBy  <http://lod.taxonconcept.org/ontology/txn.owl> ;
        rdfs:label        "Rank Variety" ;
        vs:term_status    "testing" ;
        skos:broader      :RankSpecies .

:Sex    a                 owl:Class ;
        rdfs:isDefinedBy  <http://lod.taxonconcept.org/ontology/txn.owl> ;
        rdfs:label        "Sex" ;
        vs:term_status    "testing" .

:inClass  a               owl:ObjectProperty ;
        rdfs:isDefinedBy  <http://lod.taxonconcept.org/ontology/txn.owl> ;
        rdfs:label        "inClass" ;
        vs:term_status    "testing" .

:inGenus  a               owl:ObjectProperty ;
        rdfs:isDefinedBy  <http://lod.taxonconcept.org/ontology/txn.owl> ;
        rdfs:label        "inGenus" ;
        vs:term_status    "testing" .

:SpeciesIndividual  a     owl:Class ;
        rdfs:isDefinedBy  <http://lod.taxonconcept.org/ontology/txn.owl> ;
        rdfs:label        "SpeciesIndividual" ;
        vs:term_status    "testing" .

<http://www.w3.org/2006/time#after>
        a       owl:ObjectProperty .

<http://dbpedia.org/property/binomial>
        a       owl:DatatypeProperty .

:RankSuperphylum  a       :TaxonRank , owl:NamedIndividual , owl:Class ;
        rdfs:isDefinedBy  <http://lod.taxonconcept.org/ontology/txn.owl> ;
        rdfs:label        "Rank Superphylum" ;
        vs:term_status    "testing" ;
        skos:broader      :RankInfrakingdom ;
        skos:narrower     :RankPhylum .

:RankSubpecies  a         :TaxonRank , owl:NamedIndividual , owl:Class ;
        rdfs:isDefinedBy  <http://lod.taxonconcept.org/ontology/txn.owl> ;
        rdfs:label        "Rank Subpecies" ;
        vs:term_status    "testing" ;
        skos:broader      :RankSpecies .

bibo:Collection  a  owl:Class .

rdfs:comment  a  owl:AnnotationProperty .

:individualHasObservedArea
        a                 owl:ObjectProperty ;
        rdfs:comment      "Links an individual to an Area" ;
        rdfs:domain       :SpeciesIndividual ;
        rdfs:isDefinedBy  <http://lod.taxonconcept.org/ontology/txn.owl> ;
        rdfs:label        "individualHasObservedArea" ;
        rdfs:range        :Area ;
        vs:term_status    "testing" .

wo:MarineHabitat  a  owl:Class .

:individualHasSpeciesConcept
        a                 owl:ObjectProperty ;
        rdfs:comment      "Links an individual a Species Concept" ;
        rdfs:domain       :SpeciesIndividual ;
        rdfs:isDefinedBy  <http://lod.taxonconcept.org/ontology/txn.owl> ;
        rdfs:label        "individualHasSpeciesConcept" ;
        vs:term_status    "testing" .

:RankInfraclass  a        :TaxonRank , owl:NamedIndividual , owl:Class ;
        rdfs:isDefinedBy  <http://lod.taxonconcept.org/ontology/txn.owl> ;
        rdfs:label        "Rank Infraclass" ;
        vs:term_status    "testing" ;
        skos:broader      :RankSubclass ;
        skos:narrower     :RankSuperorder .

:hasBBCPage  a              owl:ObjectProperty ;
        rdfs:comment        "The range is a page on the BBC site." ;
        rdfs:isDefinedBy    <http://lod.taxonconcept.org/ontology/txn.owl> ;
        rdfs:label          "hasBBCPage" ;
        rdfs:range          bibo:Webpage ;
        rdfs:subPropertyOf  foaf:page ;
        vs:term_status      "testing" .

:yearDescribed  a         owl:DatatypeProperty ;
        rdfs:comment      "The year that the species was originally described" ;
        rdfs:isDefinedBy  <http://lod.taxonconcept.org/ontology/txn.owl> ;
        rdfs:label        "yearDescribed" ;
        vs:term_status    "testing" .

biol:authority  a  owl:DatatypeProperty .

:RankSuperkingdom  a      :TaxonRank , owl:NamedIndividual , owl:Class ;
        rdfs:isDefinedBy  <http://lod.taxonconcept.org/ontology/txn.owl> ;
        rdfs:label        "Rank Superkingdom" ;
        vs:term_status    "testing" ;
        skos:broader      :RankSubdomain ;
        skos:narrower     :RankKingdom .

:ScientificCollectorPerson
        a                 owl:Class ;
        rdfs:comment      "Someone who has collected a scientific sample or specimen." ;
        rdfs:isDefinedBy  <http://lod.taxonconcept.org/ontology/txn.owl> ;
        rdfs:label        "ScientificCollectorPerson" ;
        rdfs:subClassOf   :Scientist ;
        vs:term_status    "testing" .

:acceptedTaxonNameID_Of
        a                   owl:ObjectProperty ;
        rdfs:domain         :TaxonNameID ;
        rdfs:isDefinedBy    <http://lod.taxonconcept.org/ontology/txn.owl> ;
        rdfs:label          "acceptedTaxonNameID_Of" ;
        rdfs:subPropertyOf  :taxonNameID_Of ;
        owl:inverseOf       :acceptedNameID ;
        vs:term_status      "testing" .

:TaxonNameGroupID  a      owl:Class ;
        rdfs:isDefinedBy  <http://lod.taxonconcept.org/ontology/txn.owl> ;
        rdfs:label        "TaxonNameGroupID" ;
        vs:term_status    "testing" .

:order  a                       owl:DatatypeProperty ;
        rdfs:isDefinedBy        <http://lod.taxonconcept.org/ontology/txn.owl> ;
        rdfs:label              "order" ;
        rdfs:subPropertyOf      :scientificName ;
        owl:equivalentProperty  biol:order ;
        vs:term_status          "testing" .

rdfs:seeAlso  a  owl:AnnotationProperty .

:localityText  a          owl:DatatypeProperty ;
        rdfs:isDefinedBy  <http://lod.taxonconcept.org/ontology/txn.owl> ;
        rdfs:label        "localityText" ;
        vs:term_status    "testing" .

taxon:binomial  a  owl:DatatypeProperty .

:MapImage  a              owl:Class ;
        rdfs:isDefinedBy  <http://lod.taxonconcept.org/ontology/txn.owl> ;
        rdfs:label        "MapImage" ;
        rdfs:subClassOf   :Image ;
        vs:term_status    "testing" .

:OpenCycTaxon  a          owl:Class ;
        rdfs:isDefinedBy  <http://lod.taxonconcept.org/ontology/txn.owl> ;
        rdfs:label        "OpenCycTaxon" ;
        vs:term_status    "testing" .

:startDate  a             owl:DatatypeProperty ;
        rdfs:isDefinedBy  <http://lod.taxonconcept.org/ontology/txn.owl> ;
        rdfs:label        "startDate" ;
        vs:term_status    "testing" .

:pubYearOf  a             owl:ObjectProperty ;
        rdfs:comment      "The year that document was pub" ;
        rdfs:domain       :Year ;
        rdfs:isDefinedBy  <http://lod.taxonconcept.org/ontology/txn.owl> ;
        rdfs:label        "pubYearOf"@en ;
        rdfs:range        bibo:Document ;
        owl:inverseOf     :yearPub ;
        vs:term_status    "testing" .

:commonName  a              owl:DatatypeProperty ;
        rdfs:isDefinedBy    <http://lod.taxonconcept.org/ontology/txn.owl> ;
        rdfs:label          "commonName" ;
        rdfs:subPropertyOf  taxon:commonName ;
        vs:term_status      "testing" .

biol:division  a  owl:DatatypeProperty .

:family  a                  owl:DatatypeProperty ;
        rdfs:isDefinedBy    <http://lod.taxonconcept.org/ontology/txn.owl> ;
        rdfs:label          "family" ;
        rdfs:subPropertyOf  :scientificName ;
        vs:term_status      "testing" .

:RankSubphylum  a         :TaxonRank , owl:NamedIndividual , owl:Class ;
        rdfs:isDefinedBy  <http://lod.taxonconcept.org/ontology/txn.owl> ;
        rdfs:label        "Rank Subphylum" ;
        vs:term_status    "testing" ;
        skos:broader      :RankPhylum ;
        skos:narrower     :RankSuperclass .

:OccurrenceSpecimenTag
        a                 owl:Class ;
        rdfs:isDefinedBy  <http://lod.taxonconcept.org/ontology/txn.owl> ;
        vs:term_status    "testing" .

:RankInfrakingdom  a      :TaxonRank , owl:NamedIndividual , owl:Class ;
        rdfs:isDefinedBy  <http://lod.taxonconcept.org/ontology/txn.owl> ;
        rdfs:label        "Rank Infrakingdom" ;
        vs:term_status    "testing" ;
        skos:broader      :RankSubkingdom ;
        skos:narrower     :RankSuperphylum .

:occurrenceInContinent
        a                 owl:ObjectProperty ;
        rdfs:comment      "Links an Occurrence to Geonames Continent URI" ;
        rdfs:domain       :Occurrence ;
        rdfs:isDefinedBy  <http://lod.taxonconcept.org/ontology/txn.owl> ;
        rdfs:label        "occurrenceInContinent" ;
        rdfs:range        gn:Feature ;
        vs:term_status    "testing" .

:yearPub  a               owl:ObjectProperty ;
        rdfs:comment      "The year that document was pub" ;
        rdfs:domain       bibo:Document ;
        rdfs:isDefinedBy  <http://lod.taxonconcept.org/ontology/txn.owl> ;
        rdfs:label        "yearPub"@en ;
        rdfs:range        :Year ;
        vs:term_status    "testing" .

:typeSpecimenHasSod  a    owl:ObjectProperty ;
        rdfs:comment      "Links specimen to an original species description" ;
        rdfs:isDefinedBy  <http://lod.taxonconcept.org/ontology/txn.owl> ;
        rdfs:label        "typeSpecimenHasSod" ;
        vs:term_status    "testing" .

:inCoLFamily  a           owl:ObjectProperty ;
        rdfs:comment      "Links a species concept to a Catalog of Life Family in an ontology" ;
        rdfs:isDefinedBy  <http://lod.taxonconcept.org/ontology/txn.owl> ;
        rdfs:label        "inCoLFamily" ;
        vs:term_status    "testing" .

:inSubclass  a            owl:ObjectProperty ;
        rdfs:isDefinedBy  <http://lod.taxonconcept.org/ontology/txn.owl> ;
        rdfs:label        "inSubclass" ;
        vs:term_status    "testing" .

:georeferenceProtocol
        a                 owl:ObjectProperty ;
        rdfs:comment      "The method used to determine the latitude, longitude as a URI" ;
        rdfs:isDefinedBy  <http://lod.taxonconcept.org/ontology/txn.owl> ;
        rdfs:label        "georeferenceProtocol" ;
        vs:term_status    "testing" .

:uniprotPhylum  a         owl:ObjectProperty ;
        rdfs:isDefinedBy  <http://lod.taxonconcept.org/ontology/taxon.owl> ;
        rdfs:label        "uniprotPhylum"@en ;
        rdfs:range        core:Taxon .

foaf:workplaceHomepage
        a       owl:ObjectProperty .

:featureContainsArea  a     owl:ObjectProperty ;
        rdfs:comment        "This is used to link a geonames feature to a geo area. For example geo:44.86528100,-87.23147800;u=10" ;
        rdfs:domain         gn:Feature ;
        rdfs:isDefinedBy    <http://lod.taxonconcept.org/ontology/txn.owl> ;
        rdfs:label          "featureContainsArea" ;
        rdfs:range          :Area ;
        rdfs:subPropertyOf  dcterms:hasPart ;
        owl:inverseOf       :areaWithInFeature ;
        vs:term_status      "testing" .

:county  a                owl:DatatypeProperty ;
        rdfs:isDefinedBy  <http://lod.taxonconcept.org/ontology/txn.owl> ;
        rdfs:label        "county" ;
        vs:term_status    "testing" .

:orthochresonymID  a        owl:ObjectProperty ;
        rdfs:comment        "The URI to the Orthochresonym Name String" ;
        rdfs:isDefinedBy    <http://lod.taxonconcept.org/ontology/txn.owl> ;
        rdfs:label          "orthochresonymID" ;
        rdfs:range          :TaxonNameID ;
        rdfs:subPropertyOf  :synonymID ;
        vs:term_status      "testing" .

:scientificNameAuthorship
        a                       owl:DatatypeProperty ;
        rdfs:comment            "The author and year of the species description publication i.e (Baker, 1899)" ;
        rdfs:isDefinedBy        <http://lod.taxonconcept.org/ontology/txn.owl> ;
        rdfs:label              "scientificNameAuthorship" ;
        owl:equivalentProperty  biol:authority ;
        vs:term_status          "testing" .

wo:habitat  a   owl:ObjectProperty .

gn:Feature  a   owl:Class .

:RankSubfamily  a         :TaxonRank , owl:NamedIndividual , owl:Class ;
        rdfs:isDefinedBy  <http://lod.taxonconcept.org/ontology/txn.owl> ;
        rdfs:label        "Rank Subfamily" ;
        vs:term_status    "testing" ;
        skos:broader      :RankFamily ;
        skos:narrower     :RankTribe .

<http://www.w3.org/2006/time#before>
        a       owl:ObjectProperty .

:RankSuperclass  a        :TaxonRank , owl:NamedIndividual , owl:Class ;
        rdfs:isDefinedBy  <http://lod.taxonconcept.org/ontology/txn.owl> ;
        rdfs:label        "Rank Superclass" ;
        vs:term_status    "testing" ;
        skos:broader      :RankSubphylum ;
        skos:narrower     :RankClass .

biol:rank  a    owl:DatatypeProperty .

foaf:Image  a   owl:Class .

:BinomialNameID  a        owl:Class ;
        rdfs:isDefinedBy  <http://lod.taxonconcept.org/ontology/txn.owl> ;
        rdfs:label        "BinomialNameID" ;
        rdfs:subClassOf   :ScientificNameID ;
        vs:term_status    "testing" .

foaf:Person  a  owl:Class .

:speciesConceptBasedOn
        a                 owl:ObjectProperty ;
        rdfs:comment      "This describes the theoretical models behind the species concept. All species concepts are at least based on an Objective Model. In addition the may also be based on a Biological Species Model and or a Phylogenetic Species Model. A species concept could be based on all three of these. This is to reflect that there are several criteria used to support a species concept. It also allows one to create a species concept for the domestic cat that is separate from its wild relative. If one followed a strict phylogentic species model, than the domestic cat would be considered to be a subclass of the species Felis sylvestris. This would result in observations or references about the domestic cat being interpreted as observations or references of the African Wildcat Felis sylvestris." ;
        rdfs:domain       :SpeciesConcept ;
        rdfs:isDefinedBy  <http://lod.taxonconcept.org/ontology/txn.owl> ;
        rdfs:label        "speciesConceptBasedOn" ;
        vs:term_status    "testing" .

:occurrenceHasSpeciesConcept
        a                 owl:ObjectProperty ;
        rdfs:comment      "Links an occurrence to a species concept" ;
        rdfs:domain       :Occurrence ;
        rdfs:isDefinedBy  <http://lod.taxonconcept.org/ontology/txn.owl> ;
        rdfs:label        "occurrenceHasSpeciesConcept" ;
        rdfs:range        :SpeciesConcept ;
        vs:term_status    "testing" .

:RankSubdomain  a         :TaxonRank , owl:NamedIndividual , owl:Class ;
        rdfs:isDefinedBy  <http://lod.taxonconcept.org/ontology/txn.owl> ;
        rdfs:label        "Rank Subdomain" ;
        vs:term_status    "testing" ;
        skos:broader      :RankDomain ;
        skos:narrower     :RankSuperkingdom .

:CommonNameID  a          owl:Class ;
        rdfs:isDefinedBy  <http://lod.taxonconcept.org/ontology/txn.owl> ;
        rdfs:label        "CommonNameID" ;
        rdfs:subClassOf   :TaxonNameID ;
        vs:term_status    "testing" .

:altAcceptedNameID  a       owl:ObjectProperty ;
        rdfs:comment        "The URI to an Alternative Accepted Name String" ;
        rdfs:isDefinedBy    <http://lod.taxonconcept.org/ontology/txn.owl> ;
        rdfs:label          "altAcceptedNameID" ;
        rdfs:range          :TaxonNameID ;
        rdfs:subPropertyOf  :taxonNameID ;
        vs:term_status      "testing" .

:taxonNameID_Of  a        owl:ObjectProperty ;
        rdfs:comment      "The URI to the Taxon Name String" ;
        rdfs:domain       :TaxonNameID ;
        rdfs:isDefinedBy  <http://lod.taxonconcept.org/ontology/txn.owl> ;
        rdfs:label        "taxonNameID_Of" ;
        vs:term_status    "testing" .

:DataObject  a            owl:Class ;
        rdfs:isDefinedBy  <http://lod.taxonconcept.org/ontology/txn.owl> ;
        rdfs:label        "DataObject"@en ;
        rdfs:subClassOf   taxon:DataObject .

:Scientist  a                owl:Class ;
        rdfs:comment         "Class for Scientist a foaf:Person"@en ;
        rdfs:isDefinedBy     <http://lod.taxonconcept.org/ontology/txn.owl> ;
        rdfs:label           "Scientist"@en ;
        rdfs:subClassOf      foaf:Person ;
        owl:equivalentClass  <http://dbpedia.org/ontology/Scientist> ;
        vs:term_status       "testing" .

foaf:depicts  a  owl:ObjectProperty .

taxon:TaxonNameID  a  owl:Class .

<http://www.w3.org/2006/time#year>
        a       owl:DatatypeProperty .

:Sex_female  a               owl:NamedIndividual , :Sex , owl:Class ;
        rdfs:isDefinedBy     <http://lod.taxonconcept.org/ontology/txn.owl> ;
        rdfs:label           "female"@en ;
        dcterms:description  "Female (♀) is the sex of an organism, or a part of an organism, which produces mobile ova (egg cells)."@en ;
        vs:term_status       "testing" .

:SurrogateNameID  a       owl:Class ;
        rdfs:isDefinedBy  <http://lod.taxonconcept.org/ontology/txn.owl> ;
        rdfs:label        "SurrogateNameID" ;
        rdfs:subClassOf   :TaxonNameID ;
        vs:term_status    "testing" .

:ScientificAuthorPerson
        a                 owl:Class ;
        rdfs:comment      "Someone who has authored a scientific article." ;
        rdfs:isDefinedBy  <http://lod.taxonconcept.org/ontology/txn.owl> ;
        rdfs:label        "ScientificAuthorPerson" ;
        rdfs:subClassOf   :Scientist ;
        vs:term_status    "testing" .

taxon:authority  a  owl:DatatypeProperty .

:locationName  a          owl:DatatypeProperty ;
        rdfs:isDefinedBy  <http://lod.taxonconcept.org/ontology/txn.owl> ;
        rdfs:label        "locationName" ;
        vs:term_status    "testing" .

foaf:name  a    owl:DatatypeProperty .

:hasEUNISPage  a            owl:ObjectProperty ;
        rdfs:isDefinedBy    <http://lod.taxonconcept.org/ontology/txn.owl> ;
        rdfs:label          "hasEUNISPage" ;
        rdfs:range          bibo:Webpage ;
        rdfs:subPropertyOf  foaf:page ;
        vs:term_status      "testing" .

wo:FreshwaterHabitat  a  owl:Class .

<http://dbpedia.org/property/ordo>
        a       owl:DatatypeProperty .

dwc_terms:acceptedNameUsage
        a       owl:DatatypeProperty .

rdfs:label  a   owl:AnnotationProperty .

:identificationOfIndividual
        a                 owl:ObjectProperty ;
        rdfs:comment      "Links an identification to an individual" ;
        rdfs:domain       :Identification ;
        rdfs:isDefinedBy  <http://lod.taxonconcept.org/ontology/txn.owl> ;
        rdfs:label        "identificationOfIndividual" ;
        vs:term_status    "testing" .

:canonicalFormID  a         owl:ObjectProperty ;
        rdfs:comment        "The URI ID for the canonical form of the name i.e. Puma concolor or Felidae, for name to name mapping" ;
        rdfs:domain         :TaxonNameID ;
        rdfs:isDefinedBy    <http://lod.taxonconcept.org/ontology/taxon.owl> ;
        rdfs:label          "canonicalFormID" ;
        rdfs:range          :TaxonNameID ;
        rdfs:subPropertyOf  :relatedTaxonNameID .

biol:species  a  owl:DatatypeProperty .

:hasEOL  a                owl:DatatypeProperty ;
        rdfs:comment      "The Encyclopedia of Life Integer ID" ;
        rdfs:isDefinedBy  <http://lod.taxonconcept.org/ontology/txn.owl> ;
        rdfs:label        "hasEOL" ;
        vs:term_status    "testing" .

:ncbiGenus  a             owl:ObjectProperty ;
        rdfs:comment      "Links to the most appropriate NCBI Genus" ;
        rdfs:isDefinedBy  <http://lod.taxonconcept.org/ontology/txn.owl> ;
        rdfs:label        "NCBI Genus" ;
        vs:term_status    "testing" .

:RankKingdom  a           :TaxonRank , owl:NamedIndividual , owl:Class ;
        rdfs:isDefinedBy  <http://lod.taxonconcept.org/ontology/txn.owl> ;
        rdfs:label        "Rank Kingdom" ;
        vs:term_status    "testing" ;
        skos:broader      :RankSuperkingdom ;
        skos:narrower     :RankSubkingdom .

:taxonNameGroupID_Of  a   owl:ObjectProperty ;
        rdfs:isDefinedBy  <http://lod.taxonconcept.org/ontology/txn.owl> ;
        rdfs:label        "taxonNameGroupID_Of" ;
        owl:inverseOf     :taxonNameGroupID ;
        vs:term_status    "testing" .

:altAcceptedNameID_Of
        a                   owl:ObjectProperty ;
        rdfs:comment        "The URI to an Alternative Accepted Name String" ;
        rdfs:domain         :TaxonNameID ;
        rdfs:isDefinedBy    <http://lod.taxonconcept.org/ontology/txn.owl> ;
        rdfs:label          "altAcceptedNameID_Of" ;
        rdfs:subPropertyOf  :taxonNameID_Of ;
        owl:inverseOf       :originalNameID ;
        vs:term_status      "testing" .

:areaHasIndividual  a     owl:ObjectProperty ;
        rdfs:comment      "Links an Area to an Individual" ;
        rdfs:isDefinedBy  <http://lod.taxonconcept.org/ontology/txn.owl> ;
        rdfs:label        "areaHasIndividual" ;
        vs:term_status    "testing" .

foaf:nick  a    owl:DatatypeProperty .

:uniprotSpecies  a        owl:ObjectProperty ;
        rdfs:isDefinedBy  <http://lod.taxonconcept.org/ontology/taxon.owl> ;
        rdfs:label        "uniprotSpecies"@en ;
        rdfs:range        core:Taxon .

<http://lod.taxonconcept.org/ontology/txn.owl>
        a                              voaf:Vocabulary , owl:Ontology ;
        rdfs:comment                   "Version 0.976 Added additional GenusNameID, SubfamilyNameID and FamilyNameID for NLP project"@en ;
        rdfs:label                     "TaxonConcept Ontology"@en ;
        rdfs:seeAlso                   <http://purl.org/NET/biol/ns> , bibo: , <http://labs.mondeca.com/dataset/lov/details/vocabulary_txn.html> , <http://lod.taxonconcept.org/ontology/void.rdf> , <http://lod.taxonconcept.org/ontology/doc/index.html> , <http://vocab.deri.ie/void> , <http://www.w3.org/TR/skos-reference/skos-owl1-dl.rdf> , foaf: ;
        dcterms:creator                txn_people:Peter_J_DeVries ;
        dcterms:description            "Version 0.976 This is an ontology for dealing with data related to species including observations, specimens, images etc. Traditionally species have been identified by the combination of a genus and specific epithet, for example Puma concolor. However these names change frequently as new information moves a given species into a different genus etc. Most of the time the species concept itself is unchanged. This leads a lot of confusion and difficulty connecting data relating to a given species concept together. This ontology and the related TaxonConcept data set avoids this by minting identifiers that are tied to a specific species concept which can have several names and classifications. The RDF descriptions of each species concept provides some guide as to what is the best species concept for a given specimen or observation, and links together data sets containing additional information about that concept. Since some of these related data sets entail specific names or classifications they are loosely linked using skos:closeMatch etc. Depending on your particular needs, you might want to merge these in your own knowledge base as sameAs or simply merge those properties that you think are appropriate."@en ;
        dcterms:modified               "2013-05-19" ;
        dcterms:publisher              :TaxonConcept_Knowledge_Base_Project ;
        dcterms:title                  "TaxonConcept Ontology"@en ;
        vann:preferredNamespacePrefix  "txn" ;
        vann:preferredNamespaceUri     "http://lod.taxonconcept.org/ontology/txn.owl#" ;
        owl:versionInfo                0.976 .

:surrogateName  a           owl:DatatypeProperty ;
        rdfs:isDefinedBy    <http://lod.taxonconcept.org/ontology/txn.owl> ;
        rdfs:label          "surrogateName" ;
        rdfs:subPropertyOf  skos:altLabel ;
        vs:term_status      "testing" .

:hasBOLDPage  a             owl:ObjectProperty ;
        rdfs:comment        "A page at boldsystems.org"@en ;
        rdfs:isDefinedBy    <http://lod.taxonconcept.org/ontology/txn.owl> ;
        rdfs:label          "hasBOLDPage" ;
        rdfs:range          bibo:Webpage ;
        rdfs:subPropertyOf  foaf:page ;
        vs:term_status      "testing" .

dcterms:issued  a  owl:DatatypeProperty , owl:AnnotationProperty .

:Sex_unknowable  a        owl:NamedIndividual , :Sex , owl:Class ;
        rdfs:isDefinedBy  <http://lod.taxonconcept.org/ontology/txn.owl> ;
        rdfs:label        "Sex Unknowable" ;
        vs:term_status    "testing" .

[ a                    owl:AllDifferent ;
  owl:distinctMembers  ( :Sex_female :Sex_hermaphrodite :Sex_male :Sex_undetermined :Sex_unknowable )
] .

biol:phylum  a  owl:DatatypeProperty .

dc:date  a      owl:AnnotationProperty .

:Habitat  a                  owl:Class ;
        rdfs:isDefinedBy     <http://lod.taxonconcept.org/ontology/txn.owl> ;
        rdfs:label           "Habitat" ;
        owl:equivalentClass  wo:Habitat ;
        vs:term_status       "testing" .

:zoologyAuthorName  a       owl:DatatypeProperty ;
        rdfs:isDefinedBy    <http://lod.taxonconcept.org/ontology/txn.owl> ;
        rdfs:label          "zoology author abbreviation" ;
        rdfs:subPropertyOf  foaf:nick ;
        vs:term_status      "testing" .

:OccurrenceTaxonTag  a    owl:Class ;
        rdfs:isDefinedBy  <http://lod.taxonconcept.org/ontology/txn.owl> ;
        vs:term_status    "testing" .

:thumbnail  a               owl:ObjectProperty ;
        rdfs:isDefinedBy    <http://lod.taxonconcept.org/ontology/txn.owl> ;
        rdfs:label          "thumbnail" ;
        rdfs:range          :Image ;
        rdfs:subPropertyOf  foaf:depiction ;
        vs:term_status      "testing" .

:identificationDate  a    owl:DatatypeProperty ;
        rdfs:isDefinedBy  <http://lod.taxonconcept.org/ontology/txn.owl> ;
        rdfs:label        "identificationDate" ;
        vs:term_status    "testing" .

wo:TerrestrialHabitat
        a       owl:Class .

:binomial  a                owl:DatatypeProperty ;
        rdfs:isDefinedBy    <http://lod.taxonconcept.org/ontology/txn.owl> ;
        rdfs:label          "binomial" ;
        rdfs:subPropertyOf  taxon:binomial ;
        vs:term_status      "testing" .

:catalogCode  a           owl:DatatypeProperty ;
        rdfs:isDefinedBy  <http://lod.taxonconcept.org/ontology/txn.owl> ;
        rdfs:label        "catalogCode" ;
        vs:term_status    "testing" .

:RankSuborder  a          :TaxonRank , owl:NamedIndividual , owl:Class ;
        rdfs:isDefinedBy  <http://lod.taxonconcept.org/ontology/txn.owl> ;
        rdfs:label        "Rank Suborder" ;
        vs:term_status    "testing" ;
        skos:broader      :RankOrder ;
        skos:narrower     :RankInfraorder .

dwc_terms:originalNameUsage
        a       owl:DatatypeProperty .

:sodHasTypeSpecimen  a    owl:ObjectProperty ;
        rdfs:comment      "Links an original description to a species type specimen" ;
        rdfs:isDefinedBy  <http://lod.taxonconcept.org/ontology/txn.owl> ;
        rdfs:label        "sodHasTypeSpecimen" ;
        owl:inverseOf     :typeSpecimenHasSod ;
        vs:term_status    "testing" .

:nameYear  a              owl:ObjectProperty ;
        rdfs:comment      "The year that a name was published" ;
        rdfs:domain       :TaxonNameID ;
        rdfs:isDefinedBy  <http://lod.taxonconcept.org/ontology/txn.owl> ;
        rdfs:label        "nameYear"@en ;
        rdfs:range        :Year ;
        vs:term_status    "testing" .

:yearDied  a              owl:ObjectProperty ;
        rdfs:domain       foaf:Person ;
        rdfs:isDefinedBy  <http://lod.taxonconcept.org/ontology/txn.owl> ;
        rdfs:label        "yearDied" ;
        rdfs:range        :Year ;
        vs:term_status    "testing" .

:RankSuperdivision  a     :TaxonRank , owl:NamedIndividual , owl:Class ;
        rdfs:isDefinedBy  <http://lod.taxonconcept.org/ontology/txn.owl> ;
        rdfs:label        "Rank Superdivision" ;
        vs:term_status    "testing" .

:Status_Preliminary  a    owl:NamedIndividual , skos:Concept ;
        rdfs:isDefinedBy  <http://lod.taxonconcept.org/ontology/txn.owl> ;
        rdfs:label        "Status_Preliminary" ;
        vs:term_status    "testing" .

skos:altLabel  a  owl:DatatypeProperty .

:RankSuperfamily  a       :TaxonRank , owl:NamedIndividual , owl:Class ;
        rdfs:isDefinedBy  <http://lod.taxonconcept.org/ontology/txn.owl> ;
        rdfs:label        "Rank Superfamily" ;
        vs:term_status    "testing" ;
        skos:broader      :RankParvorder ;
        skos:narrower     :RankFamily .

:hasBugGuidePage  a         owl:ObjectProperty ;
        rdfs:isDefinedBy    <http://lod.taxonconcept.org/ontology/txn.owl> ;
        rdfs:label          "hasBugGuidePage" ;
        rdfs:range          bibo:Webpage ;
        rdfs:subPropertyOf  foaf:page ;
        vs:term_status      "testing" .

:Sex_undetermined  a      owl:NamedIndividual , :Sex , owl:Class ;
        rdfs:isDefinedBy  <http://lod.taxonconcept.org/ontology/txn.owl> ;
        rdfs:label        "Sex Undetermined" ;
        vs:term_status    "testing" .

skos:narrower  a  owl:ObjectProperty .

:speciesConceptHasObservedArea
        a                 owl:ObjectProperty ;
        rdfs:comment      "Links a species to an area. Should be speciesConcept?" ;
        rdfs:domain       :SpeciesConcept ;
        rdfs:isDefinedBy  <http://lod.taxonconcept.org/ontology/txn.owl> ;
        rdfs:label        "speciesConceptHasObservedArea" ;
        rdfs:range        :Area ;
        vs:term_status    "testing" .

:SubfamilyNameID  a       owl:Class ;
        rdfs:isDefinedBy  <http://lod.taxonconcept.org/ontology/txn.owl> ;
        rdfs:label        "SubfamilyNameID" ;
        rdfs:subClassOf   :MonomialNameID ;
        vs:term_status    "testing" .

:hasADWPage  a              owl:ObjectProperty ;
        rdfs:comment        "The range is a page on the Animal Diversity Web site." ;
        rdfs:isDefinedBy    <http://lod.taxonconcept.org/ontology/txn.owl> ;
        rdfs:label          "hasADWPage" ;
        rdfs:range          bibo:Webpage ;
        rdfs:subPropertyOf  foaf:page ;
        vs:term_status      "testing" .

:SpeciesIndividualTag
        a                 owl:Class ;
        rdfs:comment      "A tag like entity that can be used to indicate that an individual organism is an associated with a particular species concept. Instances of SpeciesIndividualTag take the form of the species concept URI with the fragment of #Individual rather than #Species." ;
        rdfs:isDefinedBy  <http://lod.taxonconcept.org/ontology/txn.owl> ;
        rdfs:label        "SpeciesIndividualTag" .

foaf:schoolHomepage  a  owl:ObjectProperty .

:scientificNameWithAuthor
        a                   owl:DatatypeProperty ;
        rdfs:isDefinedBy    <http://lod.taxonconcept.org/ontology/txn.owl> ;
        rdfs:label          "scientificNameWithAuthor" ;
        rdfs:subPropertyOf  skos:prefLabel ;
        vs:term_status      "testing" .

:inSubfamily  a           owl:ObjectProperty ;
        rdfs:isDefinedBy  <http://lod.taxonconcept.org/ontology/txn.owl> ;
        rdfs:label        "inSubfamily" ;
        vs:term_status    "testing" .

:inSuperfamily  a         owl:ObjectProperty ;
        rdfs:isDefinedBy  <http://lod.taxonconcept.org/ontology/txn.owl> ;
        rdfs:label        "inSuperfamily" ;
        vs:term_status    "testing" .

:TaxonRank  a             owl:Class ;
        rdfs:isDefinedBy  <http://lod.taxonconcept.org/ontology/txn.owl> ;
        rdfs:label        "TaxonRank" ;
        vs:term_status    "testing" .

wgs84_pos:Point  a  owl:Class .

foaf:Organization  a  owl:Class .

:varitypeSpecimenHasSpeciesConcept
        a                 owl:ObjectProperty ;
        rdfs:comment      "Links a varitype specimen to a  species concept" ;
        rdfs:isDefinedBy  <http://lod.taxonconcept.org/ontology/txn.owl> ;
        rdfs:label        "varitypeSpecimenHasSpeciesConcept" ;
        vs:term_status    "testing" .

:ScientificNameWithAuthorID
        a                 owl:Class ;
        rdfs:isDefinedBy  <http://lod.taxonconcept.org/ontology/txn.owl> ;
        rdfs:label        "ScientificNameWithAuthorID" ;
        rdfs:subClassOf   :TaxonNameID ;
        vs:term_status    "testing" .

bibo:Webpage  a  owl:Class .

:occurrenceInFeature  a   owl:ObjectProperty ;
        rdfs:domain       :Occurrence ;
        rdfs:isDefinedBy  <http://lod.taxonconcept.org/ontology/txn.owl> ;
        rdfs:label        "occurrenceInFeature" ;
        rdfs:range        gn:Feature ;
        vs:term_status    "testing" .

:inKingdom  a             owl:ObjectProperty ;
        rdfs:isDefinedBy  <http://lod.taxonconcept.org/ontology/txn.owl> ;
        rdfs:label        "inKingdom" ;
        vs:term_status    "testing" .

:Gallery  a               owl:Class ;
        rdfs:isDefinedBy  <http://lod.taxonconcept.org/ontology/txn.owl> ;
        rdfs:label        "Gallery" ;
        vs:term_status    "testing" .

taxon:Taxon  a  owl:Class .

:class  a                       owl:DatatypeProperty ;
        rdfs:isDefinedBy        <http://lod.taxonconcept.org/ontology/txn.owl> ;
        rdfs:label              "class" ;
        rdfs:subPropertyOf      :scientificName ;
        owl:equivalentProperty  biol:class ;
        vs:term_status          "testing" .

:hybrid  a                owl:DatatypeProperty ;
        rdfs:isDefinedBy  <http://lod.taxonconcept.org/ontology/txn.owl> ;
        rdfs:label        "hybrid" ;
        vs:term_status    "testing" .

:genus  a                   owl:DatatypeProperty ;
        rdfs:isDefinedBy    <http://lod.taxonconcept.org/ontology/txn.owl> ;
        rdfs:label          "genus" ;
        rdfs:subPropertyOf  :scientificName ;
        vs:term_status      "testing" .

:synonymName  a             owl:DatatypeProperty ;
        rdfs:isDefinedBy    <http://lod.taxonconcept.org/ontology/txn.owl> ;
        rdfs:label          "synonymName" ;
        rdfs:subPropertyOf  skos:hiddenLabel ;
        vs:term_status      "testing" .

:FreshwaterHabitat  a        owl:Class ;
        rdfs:isDefinedBy     <http://lod.taxonconcept.org/ontology/txn.owl> ;
        rdfs:label           "FreshwaterHabitat" ;
        rdfs:subClassOf      :Habitat ;
        owl:equivalentClass  wo:FreshwaterHabitat ;
        vs:term_status       "testing" .

:hasGBIF  a               owl:DatatypeProperty ;
        rdfs:comment      "The Global Biodiversity Information Facility integer ID" ;
        rdfs:isDefinedBy  <http://lod.taxonconcept.org/ontology/txn.owl> ;
        rdfs:label        "hasGBIF" ;
        vs:term_status    "testing" .

:isTaxonNameID_Of  a  owl:ObjectProperty .

:identifiedBy  a          owl:ObjectProperty ;
        rdfs:comment      "Links an identification to the URI a human that made the identification as URI" ;
        rdfs:domain       :Identification ;
        rdfs:isDefinedBy  <http://lod.taxonconcept.org/ontology/txn.owl> ;
        rdfs:label        "identifiedBy" ;
        rdfs:range        foaf:Person ;
        vs:term_status    "testing" .

:Image  a                    owl:Class ;
        rdfs:isDefinedBy     <http://lod.taxonconcept.org/ontology/txn.owl> ;
        rdfs:label           "Image" ;
        owl:equivalentClass  foaf:Image ;
        vs:term_status       "testing" .

:heterotypicNameID  a       owl:ObjectProperty ;
        rdfs:comment        "The URI to the HeterotypicName Name String" ;
        rdfs:isDefinedBy    <http://lod.taxonconcept.org/ontology/txn.owl> ;
        rdfs:label          "heterotypicNameID" ;
        rdfs:range          :TaxonNameID ;
        rdfs:subPropertyOf  :synonymID ;
        vs:term_status      "testing" .

:uniprotFamily  a         owl:ObjectProperty ;
        rdfs:isDefinedBy  <http://lod.taxonconcept.org/ontology/taxon.owl> ;
        rdfs:label        "uniprotFamily"@en ;
        rdfs:range        core:Taxon .

:hasBOLD  a               owl:DatatypeProperty ;
        rdfs:comment      "The Barcode of Life Integer ID" ;
        rdfs:isDefinedBy  <http://lod.taxonconcept.org/ontology/txn.owl> ;
        rdfs:label        "hasBOLD" ;
        vs:term_status    "testing" .

:Specimen  a              owl:Class ;
        rdfs:comment      "A organismal specimen that is related to a specific organism, parts of an individual organism, or a collection of these from several organisms. It should be used for the smallest entity in a specimen database. Ideally there should be at least one specimen per individual organism. Specimens consisting of multiple individuals or multiple species often complicate analysis. If one photo contains multiple entities, document these as separate specimens all linked to the same photo." ;
        rdfs:isDefinedBy  <http://lod.taxonconcept.org/ontology/txn.owl> ;
        rdfs:label        "Specimen" ;
        vs:term_status    "testing" .

:identificationHasSpeciesConcept
        a                 owl:ObjectProperty ;
        rdfs:comment      "The link between an Identification and Species Concept, redundant with identifiedAs" ;
        rdfs:isDefinedBy  <http://lod.taxonconcept.org/ontology/txn.owl> ;
        rdfs:label        "identificationHasSpeciesConcept" ;
        vs:term_status    "testing" .

skos:closeMatch  a  owl:ObjectProperty .

:collectionCode  a        owl:DatatypeProperty ;
        rdfs:isDefinedBy  <http://lod.taxonconcept.org/ontology/txn.owl> ;
        rdfs:label        "collectionCode" ;
        vs:term_status    "testing" .

:TaxonConcept_Knowledge_Base_Project
        a                 owl:NamedIndividual , foaf:Project , foaf:Organization ;
        rdfs:isDefinedBy  <http://lod.taxonconcept.org/ontology/txn.owl> ;
        rdfs:label        "TaxonConcept_Knowledge_Base_Project" ;
        vs:term_status    "testing" .

voaf:Vocabulary  a  owl:Class .

:areaHasObservedSpeciesConcept
        a                 owl:ObjectProperty ;
        rdfs:comment      "Links an Area to a Species Concept" ;
        rdfs:isDefinedBy  <http://lod.taxonconcept.org/ontology/txn.owl> ;
        rdfs:label        "areaHasObservedSpeciesConcept" ;
        vs:term_status    "testing" .

dcterms:spatial  a  owl:ObjectProperty .

dcterms:publisher  a  owl:ObjectProperty .

:hasExpectationOf  a      owl:ObjectProperty ;
        rdfs:comment      "This is to link between a geographical area and a taxon-like entity. The doman and range are left blank so this can be used with different kinds of geographic vocabularies and different kinds of taxon concept vocabularies. It should not be used to indicate that a location has the expectation of a specific individual specimen, but to indicate that the location has an expectation of a specific class of organisms. For instance, it would be used to indicate that a geographic location has an expectation of a particular species. The use should approximate assertions similar to what one might find in a state or country checklist." ;
        rdfs:isDefinedBy  <http://lod.taxonconcept.org/ontology/txn.owl> ;
        rdfs:label        "hasExpectationOf" ;
        vs:term_status    "testing" .

:SpeciesOriginalDescription
        a                 owl:Class ;
        rdfs:isDefinedBy  <http://lod.taxonconcept.org/ontology/txn.owl> ;
        rdfs:label        "SpeciesOriginalDescription" ;
        vs:term_status    "testing" .

:lastAuthorID  a          owl:ObjectProperty ;
        rdfs:comment      "The URI to the Last Author" ;
        rdfs:domain       :TaxonNameID ;
        rdfs:isDefinedBy  <http://lod.taxonconcept.org/ontology/txn.owl> ;
        rdfs:label        "lastAuthorID" ;
        rdfs:range        :Taxonomist ;
        vs:term_status    "testing" .

:thumbnailOf  a             owl:ObjectProperty ;
        rdfs:domain         :Image ;
        rdfs:isDefinedBy    <http://lod.taxonconcept.org/ontology/txn.owl> ;
        rdfs:label          "thumbnailOf" ;
        rdfs:subPropertyOf  foaf:depicts ;
        vs:term_status      "testing" .

:TerrestrialHabitat  a       owl:Class ;
        rdfs:isDefinedBy     <http://lod.taxonconcept.org/ontology/txn.owl> ;
        rdfs:label           "TerrestrialHabitat" ;
        rdfs:subClassOf      :Habitat ;
        owl:equivalentClass  wo:TerrestrialHabitat ;
        vs:term_status       "testing" .

:isExpectedIn  a          owl:ObjectProperty ;
        rdfs:comment      "This is to link between a taxon-like entity and a geographical area. The doman and range are left blank so this can be used with different kinds of geographic vocabularies and different kinds of taxon concept vocabularies. It should not be used to indicate that a particular individual organism is expecten in a geographical area, but to indicate that the species etc. is expected in a particular geographical area. For instance, it would be used to indicate that a species is expected in a particular state or province. The use should approximate assertions similar to what one might find in a state or country checklist." ;
        rdfs:isDefinedBy  <http://lod.taxonconcept.org/ontology/txn.owl> ;
        rdfs:label        "isExpectedIn" ;
        owl:inverseOf     :hasExpectationOf ;
        vs:term_status    "testing" .

:authority  a                   owl:DatatypeProperty ;
        rdfs:comment            "The author and year of the species description publication i.e (Baker, 1899)" ;
        rdfs:isDefinedBy        <http://lod.taxonconcept.org/ontology/txn.owl> ;
        rdfs:label              "authority" ;
        owl:equivalentProperty  biol:authority ;
        vs:term_status          "testing" .

<http://dbpedia.org/ontology/Scientist>
        a       owl:Class .

:inOrder  a               owl:ObjectProperty ;
        rdfs:isDefinedBy  <http://lod.taxonconcept.org/ontology/txn.owl> ;
        rdfs:label        "inOrder" ;
        vs:term_status    "testing" .

:individualhasImage  a      owl:ObjectProperty ;
        rdfs:comment        "Intended to link an individual to a image. Should be subproperty of foaf:depiction" ;
        rdfs:domain         :SpeciesIndividual ;
        rdfs:isDefinedBy    <http://lod.taxonconcept.org/ontology/txn.owl> ;
        rdfs:label          "individualhasImage" ;
        rdfs:subPropertyOf  :hasImage ;
        vs:term_status      "testing" .

owl:topDataProperty  a  owl:DatatypeProperty .

:ScientificIdentifierPerson
        a                 owl:Class ;
        rdfs:comment      "Someone who has identified a specimen." ;
        rdfs:isDefinedBy  <http://lod.taxonconcept.org/ontology/txn.owl> ;
        rdfs:label        "ScientificIdentifierPerson" ;
        rdfs:subClassOf   :Scientist ;
        vs:term_status    "testing" .

foaf:Project  a  owl:Class .

:individualStatus  a      owl:ObjectProperty ;
        rdfs:comment      "Links from an individual to a controlled vocabulary of URI's for the current status of that individual" ;
        rdfs:domain       :SpeciesIndividual ;
        rdfs:isDefinedBy  <http://lod.taxonconcept.org/ontology/txn.owl> ;
        rdfs:label        "individualStatus" ;
        vs:term_status    "testing" .

:acceptedNameID  a          owl:ObjectProperty ;
        rdfs:comment        "The URI to the Accepted Name String, should only be one." ;
        rdfs:isDefinedBy    <http://lod.taxonconcept.org/ontology/txn.owl> ;
        rdfs:label          "acceptedNameID" ;
        rdfs:range          :TaxonNameID ;
        rdfs:subPropertyOf  :taxonNameID ;
        vs:term_status      "testing" .

:RankTribe  a             :TaxonRank , owl:NamedIndividual , owl:Class ;
        rdfs:isDefinedBy  <http://lod.taxonconcept.org/ontology/txn.owl> ;
        rdfs:label        "Rank Tribe" ;
        vs:term_status    "testing" ;
        skos:broader      :RankSubfamily ;
        skos:narrower     :RankGenus .

:endDate  a               owl:DatatypeProperty ;
        rdfs:isDefinedBy  <http://lod.taxonconcept.org/ontology/txn.owl> ;
        rdfs:label        "endDate" ;
        vs:term_status    "testing" .

:country  a               owl:DatatypeProperty ;
        rdfs:isDefinedBy  <http://lod.taxonconcept.org/ontology/txn.owl> ;
        rdfs:label        "country" ;
        vs:term_status    "testing" .

:inSuperorder  a          owl:ObjectProperty ;
        rdfs:isDefinedBy  <http://lod.taxonconcept.org/ontology/txn.owl> ;
        rdfs:label        "inSuperorder" ;
        vs:term_status    "testing" .

:RankClass  a             :TaxonRank , owl:NamedIndividual , owl:Class ;
        rdfs:isDefinedBy  <http://lod.taxonconcept.org/ontology/txn.owl> ;
        rdfs:label        "Rank Class" ;
        vs:term_status    "testing" ;
        skos:broader      :RankSuperclass ;
        skos:narrower     :RankSubclass .

:TaxonConcept_Scheme  a   owl:NamedIndividual , skos:Concept ;
        rdfs:isDefinedBy  <http://lod.taxonconcept.org/ontology/txn.owl> ;
        rdfs:label        "TaxonConcept_Scheme" ;
        vs:term_status    "testing" .

:RankGenus  a             :TaxonRank , owl:NamedIndividual , owl:Class ;
        rdfs:isDefinedBy  <http://lod.taxonconcept.org/ontology/txn.owl> ;
        rdfs:label        "Rank Genus" ;
        vs:term_status    "testing" ;
        skos:broader      :RankTribe ;
        skos:narrower     :RankSubgenus .

:hasOriginalName  a         owl:DatatypeProperty ;
        rdfs:isDefinedBy    <http://lod.taxonconcept.org/ontology/txn.owl> ;
        rdfs:label          "hasOriginalName" ;
        rdfs:subPropertyOf  skos:altLabel ;
        vs:term_status      "deprecated" .

:nameYearOf  a            owl:ObjectProperty ;
        rdfs:comment      "Inverse of The year that a name was published" ;
        rdfs:domain       :Year ;
        rdfs:isDefinedBy  <http://lod.taxonconcept.org/ontology/txn.owl> ;
        rdfs:label        "nameYear"@en ;
        rdfs:range        :TaxonNameID ;
        owl:inverseOf     :nameYear ;
        vs:term_status    "testing" .

:hasWikipediaArticle  a     owl:ObjectProperty ;
        rdfs:isDefinedBy    <http://lod.taxonconcept.org/ontology/txn.owl> ;
        rdfs:label          "hasWikipediaArticle" ;
        rdfs:range          bibo:Webpage ;
        rdfs:subPropertyOf  foaf:page ;
        vs:term_status      "testing" .

bibo:Document  a  owl:Class .

:isWikipediaArticleOf
        a                 owl:ObjectProperty ;
        rdfs:domain       bibo:Webpage ;
        rdfs:isDefinedBy  <http://lod.taxonconcept.org/ontology/txn.owl> ;
        rdfs:label        "isWikipediaArticleOf" ;
        owl:inverseOf     :hasWikipediaArticle ;
        vs:term_status    "testing" .

:SpeciesTaxonomyNCBI  a   owl:Class ;
        rdfs:comment      "A tag like entity for the NCBI Taxonomic Classification." ;
        rdfs:isDefinedBy  <http://lod.taxonconcept.org/ontology/txn.owl> ;
        rdfs:label        "SpeciesTaxonomyNCBI" ;
        vs:term_status    "testing" .

:identificationNote  a    owl:DatatypeProperty ;
        rdfs:isDefinedBy  <http://lod.taxonconcept.org/ontology/txn.owl> ;
        rdfs:label        "identificationNote" ;
        vs:term_status    "testing" .

:hasITISPage  a             owl:ObjectProperty ;
        rdfs:comment        "The range is a page on the ITIS.gov site." ;
        rdfs:isDefinedBy    <http://lod.taxonconcept.org/ontology/txn.owl> ;
        rdfs:label          "hasITISPage" ;
        rdfs:range          bibo:Webpage ;
        rdfs:subPropertyOf  foaf:page ;
        vs:term_status      "testing" .

foaf:publications  a  owl:ObjectProperty .

:ScientificDataCuratorPerson
        a                 owl:Class ;
        rdfs:comment      "Someone who has curated or entered data into a scientific data set." ;
        rdfs:isDefinedBy  <http://lod.taxonconcept.org/ontology/txn.owl> ;
        rdfs:label        "ScientificDataCuratorPerson" ;
        rdfs:subClassOf   :Scientist ;
        vs:term_status    "testing" .

:TaxonNameID  a           owl:Class ;
        rdfs:isDefinedBy  <http://lod.taxonconcept.org/ontology/txn.owl> ;
        rdfs:label        "TaxonNameID" ;
        rdfs:subClassOf   taxon:TaxonNameID .

:uniprotClass  a          owl:ObjectProperty ;
        rdfs:isDefinedBy  <http://lod.taxonconcept.org/ontology/taxon.owl> ;
        rdfs:label        "uniprotClass"@en ;
        rdfs:range        core:Taxon .

:uniprotGenus  a          owl:ObjectProperty ;
        rdfs:isDefinedBy  <http://lod.taxonconcept.org/ontology/taxon.owl> ;
        rdfs:label        "uniprotGenus"@en ;
        rdfs:range        core:Taxon .

:originalNameID  a          owl:ObjectProperty ;
        rdfs:comment        "The URI to the Original Name String" ;
        rdfs:isDefinedBy    <http://lod.taxonconcept.org/ontology/txn.owl> ;
        rdfs:label          "originalNameID" ;
        rdfs:range          :TaxonNameID ;
        rdfs:subPropertyOf  :taxonNameID ;
        vs:term_status      "testing" .

:hasWikispeciesArticle
        a                   owl:ObjectProperty ;
        rdfs:isDefinedBy    <http://lod.taxonconcept.org/ontology/txn.owl> ;
        rdfs:label          "hasWikispeciesArticle" ;
        rdfs:range          bibo:Webpage ;
        rdfs:subPropertyOf  foaf:page ;
        vs:term_status      "testing" .

vann:preferredNamespaceUri
        a       owl:AnnotationProperty .

dc:description  a  owl:AnnotationProperty .

taxon:trinomial  a  owl:DatatypeProperty .

:RankPhylum  a            :TaxonRank , owl:NamedIndividual , owl:Class ;
        rdfs:isDefinedBy  <http://lod.taxonconcept.org/ontology/txn.owl> ;
        rdfs:label        "Rank Phylum" ;
        vs:term_status    "testing" ;
        skos:broader      :RankSuperphylum ;
        skos:narrower     :RankSubphylum .

:isEOLPageOf  a           owl:ObjectProperty ;
        rdfs:comment      "The range is a page on the Encyclopedia of Life site." ;
        rdfs:domain       bibo:Webpage ;
        rdfs:isDefinedBy  <http://lod.taxonconcept.org/ontology/txn.owl> ;
        rdfs:label        "isEOLPageOf" ;
        vs:term_status    "testing" .

biol:family  a  owl:DatatypeProperty .

foaf:depiction  a  owl:ObjectProperty .

:hasUSDAPlantsPage  a       owl:ObjectProperty ;
        rdfs:isDefinedBy    <http://lod.taxonconcept.org/ontology/txn.owl> ;
        rdfs:label          "hasUSDAPlantsPage" ;
        rdfs:range          bibo:Webpage ;
        rdfs:subPropertyOf  foaf:page ;
        vs:term_status      "testing" .

:synonymID  a               owl:ObjectProperty ;
        rdfs:comment        "The URI to a synonymID of the TaxonNameID" ;
        rdfs:isDefinedBy    <http://lod.taxonconcept.org/ontology/txn.owl> ;
        rdfs:label          "synonymID" ;
        rdfs:range          :TaxonNameID ;
        rdfs:subPropertyOf  :relatedTaxonNameID ;
        vs:term_status      "testing" .

:TaxonConcept  a          owl:Class ;
        rdfs:comment      "A particular taxonomic concept. Currently only species concepts are implemented, however theoretically there could be additional subclasses of GenusConcepts, FamilyConcepts etc. A SubspeciesConcept and lower are considered to be subclasses of SpeciesConcepts, but one persons subspecies is often anothers species. My current thinking is to represent individuals and observations of subspecies as individuals and observations of the larger species concept. It has yet to be implemented but I am considering recording these as observations and individuals of a given species \"in the form of\" their subspecies indentifier or name." ;
        rdfs:isDefinedBy  <http://lod.taxonconcept.org/ontology/txn.owl> ;
        rdfs:label        "TaxonConcept" ;
        vs:term_status    "testing" .

:ncbiSpecies  a           owl:ObjectProperty ;
        rdfs:comment      "Links to the most appropriate NCBI Species" ;
        rdfs:isDefinedBy  <http://lod.taxonconcept.org/ontology/txn.owl> ;
        rdfs:label        "NCBI Species" ;
        vs:term_status    "testing" .

<http://dbpedia.org/property/synonym>
        a       owl:DatatypeProperty .

:hasUnknownExpectationOf
        a                 owl:ObjectProperty ;
        rdfs:comment      "This is to link between a geographical area and a taxon-like entity. Where the association is not known. The doman and range are left blank so this can be used with different kinds of geographic vocabularies and different kinds of taxon concept vocabularies. It should not be used to indicate that a location has the expectation of a specific individual specimen, but to indicate that the location has an expectation of a specific class of organisms. For instance, it would be used to indicate that a geographic location has an expectation of a particular species. The use should approximate assertions similar to what one might find in a state or country checklist." ;
        rdfs:isDefinedBy  <http://lod.taxonconcept.org/ontology/txn.owl> ;
        rdfs:label        "hasUnknownExpectationOf" ;
        owl:inverseOf     :isUnknownAboutIn ;
        vs:term_status    "testing" .

:inCoLOrder  a            owl:ObjectProperty ;
        rdfs:comment      "Links a species concept to a Catalog of Life Order in an ontology" ;
        rdfs:isDefinedBy  <http://lod.taxonconcept.org/ontology/txn.owl> ;
        rdfs:label        "inCoLOrder" ;
        vs:term_status    "testing" .

:identificationHasOcccurrence
        a                 owl:ObjectProperty ;
        rdfs:comment      "The link between an Identification and an Occurrence" ;
        rdfs:domain       :Identification ;
        rdfs:isDefinedBy  <http://lod.taxonconcept.org/ontology/txn.owl> ;
        rdfs:label        "identificationHasOcccurrence" ;
        vs:term_status    "testing" .

:RankSuperorder  a        :TaxonRank , owl:NamedIndividual , owl:Class ;
        rdfs:isDefinedBy  <http://lod.taxonconcept.org/ontology/txn.owl> ;
        rdfs:label        "Rank Superorder" ;
        vs:term_status    "testing" ;
        skos:broader      :RankInfraclass ;
        skos:narrower     :RankOrder .

dcterms:modified  a  owl:DatatypeProperty .

:yearBorn  a              owl:ObjectProperty ;
        rdfs:domain       foaf:Person ;
        rdfs:isDefinedBy  <http://lod.taxonconcept.org/ontology/txn.owl> ;
        rdfs:label        "yearBorn" ;
        rdfs:range        :Year ;
        vs:term_status    "testing" .

taxon:scientificName  a  owl:DatatypeProperty .

txn_people:Peter_J_DeVries
        a       foaf:Person .

:areaWithInFeature  a       owl:ObjectProperty ;
        rdfs:comment        "This is used to connect geo areas to geoname features" ;
        rdfs:domain         :Area ;
        rdfs:isDefinedBy    <http://lod.taxonconcept.org/ontology/txn.owl> ;
        rdfs:label          "areaWithInFeature" ;
        rdfs:range          gn:Feature ;
        rdfs:subPropertyOf  dcterms:partOf ;
        vs:term_status      "testing" .

vann:preferredNamespacePrefix
        a       owl:AnnotationProperty .
