@prefix rdfs:  <http://www.w3.org/2000/01/rdf-schema#> .
@prefix dcat:  <http://www.w3.org/ns/dcat#> .
@prefix foaf:  <http://xmlns.com/foaf/0.1/> .
@prefix dct:   <http://purl.org/dc/terms/> .
@prefix owl:   <http://www.w3.org/2002/07/owl#> .
@prefix xsd:   <http://www.w3.org/2001/XMLSchema#> .
@prefix rdf:   <http://www.w3.org/1999/02/22-rdf-syntax-ns#> .
@prefix vann:  <http://purl.org/vocab/vann/> .
@prefix st:    <http://semweb.mmlab.be/ns/stoptimes#> .
@prefix skos:  <http://www.w3.org/2004/02/skos/core#> .

st:nextStopTime  a    rdf:Property ;
        rdfs:comment  "The next stop time on this vehicle's trajectory."@en ;
        rdfs:domain   st:StopTime ;
        rdfs:label    "Next Stop Time"@en ;
        rdfs:range    st:StopTime .

st:avgStopTimes  a    rdf:Property ;
        rdfs:comment  "The average st:StopTimes per day"@en ;
        rdfs:label    "Average Stop Times"@en ;
        rdfs:range    xsd:double .

st:Ontology  a                         owl:Ontology ;
        rdfs:comment                   "This ontology provides the predicates necessary to describe an arrival of a transit vehicle and its departure at a certain Stop."@en ;
        rdfs:label                     "The Stop Times ontology"@en ;
        dct:creator                    <http://pieter.pm/#me> ;
        vann:preferredNamespacePrefix  "st" ;
        vann:preferredNamespaceUri     "http://semweb.mmlab.be/ns/stoptimes#" .

st:Arrival  a         rdfs:Class ;
        rdfs:comment  "A location and a time where a vehicle stops for the purpose of unloading people or things"@en ;
        rdfs:label    "Arrival"@en .

st:Departure  a       rdfs:Class ;
        rdfs:comment  "A location and a departure time where a vehicle departs where people or things can be loaded"@en ;
        rdfs:label    "Arrival"@en .

st:departureDelay  a  rdf:Property ;
        rdfs:comment  "The time in seconds in which the st:departureTime differs from the scheduled departure time"@en ;
        rdfs:label    "Departure Delay"@en ;
        rdfs:range    xsd:duration .

st:arrivalDelay  a    rdf:Property ;
        rdfs:comment  "The time in seconds in which the st:arrivalTime differs from the scheduled arrival time"@en ;
        rdfs:label    "Arrival Delay"@en ;
        rdfs:range    xsd:duration .

st:StopTime  a        rdfs:Class ;
        rdfs:comment  "A location and a time where a vehicle stops for the purpose of loading and/or unloading people or things"@en ;
        rdfs:label    "Stop Time"@en .

<http://pieter.pm/#me>
        foaf:mbox  "Pieter.Colpaert@UGent.be" ;
        foaf:name  "Pieter Colpaert" .

<http://semweb.mmlab.be/ns/stoptimes>
        a                  foaf:Document ;
        dct:hasFormat      <https://raw.githubusercontent.com/OpenTransport/StopTimes/master/stoptimes.ttl> ;
        dct:issued         "2014-10-31"^^xsd:date ;
        dct:license        <http://creativecommons.org/licenses/by/3.0/> ;
        dct:modified       "2015-09-04"^^xsd:date ;
        dct:rights         "Copyright 2014, 2015 - Open Transport contributors" ;
        foaf:primaryTopic  st:Ontology .
