@prefix dc: <http://purl.org/dc/elements/1.1/> .
@prefix prov: <http://www.w3.org/ns/prov#> .
@prefix foaf: <http://xmlns.com/foaf/0.1/> .
@prefix qb: <http://purl.org/linked-data/cube#> .
@prefix org: <http://www.w3.org/ns/org#> .
@prefix dcterms: <http://purl.org/dc/terms/> .
@prefix xkos: <http://purl.org/linked-data/xkos#> .
@prefix adms: <http://www.w3.org/ns/adms#> .
@prefix rdfs: <http://www.w3.org/2000/01/rdf-schema#> .
@prefix dcat: <http://www.w3.org/ns/dcat#> .
@prefix disco: <http://rdf-vocabulary.ddialliance.org/discovery#> .
@prefix xsd: <http://www.w3.org/2001/XMLSchema#> .
@prefix owl: <http://www.w3.org/2002/07/owl#> .
@prefix rdf: <http://www.w3.org/1999/02/22-rdf-syntax-ns#> .
@prefix skos: <http://www.w3.org/2004/02/skos/core#> .

<http://rdf-vocabulary.ddialliance.org/discovery> a owl:Ontology ;
	dc:title "DDI discovery model ontology"@en , "Ontologie pour le modèle DDI discovery"@fr , "DDI-Entdeckungsontologie"@de ;
	rdfs:comment "This ontology is based on the Data Documentation Initiative model, especially the elements useful for data discovery"@en ;
	dc:contributor "Thomas Bosch" , "Franck Cotton" , "Richard Cyganiak" , "Arofan Gregory" , "Larry Hoyle" , "Benedikt Kämpgen" , "Olof Olsson" , "Heiko Paulheim" , "Dan Smith" , "Wendy Thomas" , "Johanna Vompras" , "Joachim Wackerow" , "Benjamin Zapilko" ;
	dc:creator "Franck Cotton" ;
	owl:versionInfo "Version 0.6 - 2013-07-05" .

disco:AnalysisUnit a rdfs:Class , owl:Class ;
	rdfs:label "analysis unit"@en , "Analyseeinheit"@de ;
	rdfs:comment "The process collecting data is focusing on the analysis of a particular type of subject. If, for example, the adult population of Finland is being studied, the AnalysisUnit would be individuals or persons."@en ;
	rdfs:isDefinedBy <http://rdf-vocabulary.ddialliance.org/discovery> ;
	rdfs:subClassOf skos:Concept .

disco:VariableDefinition a rdfs:Class , owl:Class ;
	rdfs:label "Data element"@en , "Élément de donnée"@fr ;
	rdfs:comment "VariableDefinitions encompasse study-independent, re-usable parts of variables like occupation classification."@en ;
	rdfs:isDefinedBy <http://rdf-vocabulary.ddialliance.org/discovery> .

disco:DataFile a rdfs:Class , owl:Class ;
	rdfs:label "Data file"@en , "Fichier de données"@fr ;
	rdfs:comment "The class DataFile, which is also a dcterms:Dataset, represents all the data files containing the microdata datasets."@en ;
	rdfs:subClassOf dcat:Distribution ;
	rdfs:isDefinedBy <http://rdf-vocabulary.ddialliance.org/discovery> .

disco:DescriptiveStatistics a rdfs:Class , owl:Class ;
	rdfs:label "Descriptive statistics"@en , "Statistique descriptive"@fr ;
	rdfs:comment "SummaryStatistics pointing to variables and CategoryStatistics pointing to categories and codes are both DescriptiveStatistics."@en ;
	rdfs:isDefinedBy <http://rdf-vocabulary.ddialliance.org/discovery> .

disco:SummaryStatistics a rdfs:Class , owl:Class ;
	rdfs:label "Summary statistics"@en ;
	rdfs:comment "For SummaryStatistics, maximum values, minimum values, and standard deviations can be defined."@en ;
	rdfs:subClassOf disco:DescriptiveStatistics ;
	rdfs:isDefinedBy <http://rdf-vocabulary.ddialliance.org/discovery> .

disco:CategoryStatistics a rdfs:Class , owl:Class ;
	rdfs:label "Category statistics"@en ;
	rdfs:comment "For CategoryStatistics, frequencies, percentages, and weighted percentages can be defined."@en ;
	rdfs:subClassOf disco:DescriptiveStatistics ;
	rdfs:isDefinedBy <http://rdf-vocabulary.ddialliance.org/discovery> .

disco:Instrument a rdfs:Class , owl:Class ;
	rdfs:label "The data for the study are collected by an Instrument. The purpose of an Instrument, i.e. an interview, a questionnaire or another entity used as a means of data collection, is in the case of a survey to record the flow of a questionnaire, its use of questions, and additional component parts. A questionnaire contains a flow of questions. "@en , "Instrument de collecte"@fr ;
	rdfs:comment "The data for the study are collected by an Instrument. The purpose of an Instrument, i.e. an interview, a questionnaire or another entity used as a means of data collection, is in the case of a survey to record the flow of a questionnaire, its use of questions, and additional component parts. A questionnaire contains a flow of questions. "@en ;
	rdfs:isDefinedBy <http://rdf-vocabulary.ddialliance.org/discovery> .

disco:LogicalDataSet a rdfs:Class , owl:Class ;
	rdfs:label "LogicalDataSet"@en , "Ensemble de données"@fr ;
	rdfs:comment "Each study has a set of logical metadata associated with the processing of data, at the time of collection or later during cleaning, and re-coding. LogicalDataSet represents the microdata dataset."@en ;
	rdfs:subClassOf dcat:Dataset ;
	rdfs:isDefinedBy <http://rdf-vocabulary.ddialliance.org/discovery> .

disco:Question a rdfs:Class , owl:Class ;
	rdfs:label "Question"@en , "Question"@fr ;
	rdfs:comment "A Question is designed to get information upon a subject, or sequence of subjects, from a respondent."@en ;
	rdfs:isDefinedBy <http://rdf-vocabulary.ddialliance.org/discovery> .

disco:Questionnaire a rdfs:Class , owl:Class ;
	rdfs:label "Questionnaire"@en , "Fragebogen"@de ;
	rdfs:comment "A questionnaire contains a flow of questions. "@en ;
	rdfs:isDefinedBy <http://rdf-vocabulary.ddialliance.org/discovery> ;
	rdfs:subClassOf disco:Instrument .

disco:Study a rdfs:Class , owl:Class ;
	rdfs:label "Study"@en , "Étude"@fr ;
	rdfs:comment "A Study represents the process by which a data set was generated or collected."@en ;
	rdfs:isDefinedBy <http://rdf-vocabulary.ddialliance.org/discovery> .

disco:StudyGroup a rdfs:Class , owl:Class ;
	rdfs:label "Study Group"@en , "Studiengruppe"@de ;
	rdfs:comment "In some cases, where data collection is cyclic or on-going, data sets may be released as a StudyGroup, where each cycle or wave of the data collection activity produces one or more data sets. This is typical for longitudinal studies, panel studies, and other types of series (to use the DDI term). In this case, a number of Study objects would be collected into a single StudyGroup."@en ;
	rdfs:isDefinedBy <http://rdf-vocabulary.ddialliance.org/discovery> .

disco:Variable a rdfs:Class , owl:Class ;
	rdfs:label "Variable"@en , "Variable"@fr ;
	rdfs:comment "Variables provide a definition of the column in a rectangular data file. Variable is a characteristic of a unit being observed. A variable might be the answer of a question, have an administrative source, or be derived from other variables."@en ;
	rdfs:isDefinedBy <http://rdf-vocabulary.ddialliance.org/discovery> .

disco:Universe a rdfs:Class , owl:Class ;
	rdfs:label "Universe"@en , "Univers"@fr ;
	rdfs:comment "A Universe is the total membership or population of a defined class of people, objects or events."@en ;
	rdfs:isDefinedBy <http://rdf-vocabulary.ddialliance.org/discovery> ;
	rdfs:subClassOf skos:Concept .

disco:caseQuantity a rdf:Property , owl:DatatypeProperty ;
	rdfs:label "number of cases"@en , "nombre d'observations"@fr ;
	rdfs:comment "case quantity of a DataFile."@en ;
	rdfs:domain disco:DataFile ;
	rdfs:range xsd:nonNegativeInteger ;
	rdfs:isDefinedBy <http://rdf-vocabulary.ddialliance.org/discovery> .

disco:frequency a rdf:Property , owl:DatatypeProperty ;
	rdfs:label "frequency"@en , "fréquence"@fr ;
	rdfs:comment "frequency"@en ;
	rdfs:domain disco:CategoryStatistics ;
	rdfs:range xsd:nonNegativeInteger ;
	rdfs:isDefinedBy <http://rdf-vocabulary.ddialliance.org/discovery> .

disco:isPublic a rdf:Property , owl:DatatypeProperty ;
	rdfs:label "is public"@en , "ist öffentlich"@de ;
	rdfs:domain disco:LogicalDataSet ;
	rdfs:comment "The value true indicates that the dataset can be accessed (usually downloaded) by anyone."@en ;
	rdfs:range xsd:boolean ;
	rdfs:isDefinedBy <http://rdf-vocabulary.ddialliance.org/discovery> .

disco:isValid a rdf:Property , owl:DatatypeProperty ;
	rdfs:label "is valid"@en ;
	rdfs:domain skos:Concept ;
	rdfs:comment "Indicates if the code (represented by skos:Concept) is valid or missing."@en ;
	rdfs:range xsd:boolean ;
	rdfs:isDefinedBy <http://rdf-vocabulary.ddialliance.org/discovery> .

disco:questionText a rdf:Property , owl:DatatypeProperty ;
	rdfs:label "question text"@en , "Fragetext"@de ;
	rdfs:comment "question text"@en ;
	rdfs:domain disco:Question ;
	rdfs:range rdf:langString ;
	rdfs:isDefinedBy <http://rdf-vocabulary.ddialliance.org/discovery> .

disco:percentage a rdf:Property , owl:DatatypeProperty ;
	rdfs:label "percentage"@en , "pourcentage"@fr ;
	rdfs:comment "percentage"@en .

_:node1857e284cx57 rdf:first disco:SummaryStatistics ;
	rdf:rest _:node1857e284cx58 .

_:node1857e284cx58 rdf:first disco:CategoryStatistics ;
	rdf:rest rdf:nil .

_:node1857e284cx59 owl:unionOf _:node1857e284cx57 .

disco:percentage rdfs:domain _:node1857e284cx59 ;
	rdfs:range xsd:decimal ;
	rdfs:isDefinedBy <http://rdf-vocabulary.ddialliance.org/discovery> .

disco:computationBase a rdf:Property , owl:DatatypeProperty ;
	rdfs:label "computation base"@en , "pourcentage"@fr ;
	rdfs:comment "computation base"@en .

_:node1857e284cx60 rdf:first disco:SummaryStatistics ;
	rdf:rest _:node1857e284cx61 .

_:node1857e284cx61 rdf:first disco:CategoryStatistics ;
	rdf:rest rdf:nil .

_:node1857e284cx62 owl:unionOf _:node1857e284cx60 .

disco:computationBase rdfs:domain _:node1857e284cx62 ;
	rdfs:range rdf:langString ;
	rdfs:isDefinedBy <http://rdf-vocabulary.ddialliance.org/discovery> .

disco:cumulativePercentage a rdf:Property , owl:DatatypeProperty ;
	rdfs:label "cumulative percentage"@en ;
	rdfs:comment "cumulative percentage"@en ;
	rdfs:domain disco:CategoryStatistics ;
	rdfs:range xsd:decimal ;
	rdfs:isDefinedBy <http://rdf-vocabulary.ddialliance.org/discovery> .

disco:purpose a rdf:Property , owl:DatatypeProperty ;
	rdfs:label "purpose"@en , "Grund"@de ;
	rdfs:comment "The purpose of a Study of a StudyGroup."@en .

_:node1857e284cx63 rdf:first disco:Study ;
	rdf:rest _:node1857e284cx64 .

_:node1857e284cx64 rdf:first disco:StudyGroup ;
	rdf:rest rdf:nil .

_:node1857e284cx65 owl:unionOf _:node1857e284cx63 .

disco:purpose rdfs:domain _:node1857e284cx65 ;
	rdfs:range rdf:langString ;
	rdfs:isDefinedBy <http://rdf-vocabulary.ddialliance.org/discovery> .

disco:subtitle a rdf:Property , owl:DatatypeProperty ;
	rdfs:label "subtitle"@en , "Untertitel"@de ;
	rdfs:comment "The sub-title of a Study of a StudyGroup."@en .

_:node1857e284cx66 rdf:first disco:Study ;
	rdf:rest _:node1857e284cx67 .

_:node1857e284cx67 rdf:first disco:StudyGroup ;
	rdf:rest rdf:nil .

_:node1857e284cx68 owl:unionOf _:node1857e284cx66 .

disco:subtitle rdfs:domain _:node1857e284cx68 ;
	rdfs:range rdf:langString ;
	rdfs:isDefinedBy <http://rdf-vocabulary.ddialliance.org/discovery> .

disco:standardDeviation a rdf:Property , owl:DatatypeProperty ;
	rdfs:label "standard deviation"@en ;
	rdfs:comment "standard deviation"@en ;
	rdfs:domain disco:SummaryStatistics ;
	rdfs:range xsd:decimal ;
	rdfs:isDefinedBy <http://rdf-vocabulary.ddialliance.org/discovery> .

disco:numberOfCases a rdf:Property , owl:DatatypeProperty ;
	rdfs:label "number of cases"@en ;
	rdfs:comment "number of cases"@en ;
	rdfs:domain disco:SummaryStatistics ;
	rdfs:range xsd:nonNegativeInteger ;
	rdfs:isDefinedBy <http://rdf-vocabulary.ddialliance.org/discovery> .

disco:maximum a rdf:Property , owl:DatatypeProperty ;
	rdfs:label "maximum"@en ;
	rdfs:comment "maximum"@en ;
	rdfs:domain disco:SummaryStatistics ;
	rdfs:range xsd:decimal ;
	rdfs:isDefinedBy <http://rdf-vocabulary.ddialliance.org/discovery> .

disco:mean a rdf:Property , owl:DatatypeProperty ;
	rdfs:label "mean"@en ;
	rdfs:comment "mean"@en ;
	rdfs:domain disco:SummaryStatistics ;
	rdfs:range xsd:decimal ;
	rdfs:isDefinedBy <http://rdf-vocabulary.ddialliance.org/discovery> .

disco:median a rdf:Property , owl:DatatypeProperty ;
	rdfs:label "median"@en ;
	rdfs:comment "median"@en ;
	rdfs:domain disco:SummaryStatistics ;
	rdfs:range xsd:decimal ;
	rdfs:isDefinedBy <http://rdf-vocabulary.ddialliance.org/discovery> .

disco:minimum a rdf:Property , owl:DatatypeProperty ;
	rdfs:label "minimum"@en ;
	rdfs:comment "minimum"@en ;
	rdfs:domain disco:SummaryStatistics ;
	rdfs:range xsd:decimal ;
	rdfs:isDefinedBy <http://rdf-vocabulary.ddialliance.org/discovery> .

disco:mode a rdf:Property , owl:DatatypeProperty ;
	rdfs:label "mode"@en ;
	rdfs:comment "mode"@en ;
	rdfs:domain disco:SummaryStatistics ;
	rdfs:range xsd:decimal ;
	rdfs:isDefinedBy <http://rdf-vocabulary.ddialliance.org/discovery> .

disco:startDate a rdf:Property , owl:DatatypeProperty ;
	rdfs:label "Start Date"@en ;
	rdfs:comment "start date"@en ;
	rdfs:domain dcterms:PeriodOfTime ;
	rdfs:range xsd:date ;
	rdfs:isDefinedBy <http://rdf-vocabulary.ddialliance.org/discovery> .

disco:endDate a rdf:Property , owl:DatatypeProperty ;
	rdfs:label "End Date"@en ;
	rdfs:comment "end date"@en ;
	rdfs:domain dcterms:PeriodOfTime ;
	rdfs:range xsd:date ;
	rdfs:isDefinedBy <http://rdf-vocabulary.ddialliance.org/discovery> .

disco:analysisUnit a rdf:Property , owl:ObjectProperty ;
	rdfs:label "analysis unit"@en , "Analyseeinheit"@de ;
	rdfs:comment "analysis unit of a Study, a StudyGroup, or a Variable."@en .

_:node1857e284cx69 rdf:first owl:unionOf ;
	rdf:rest _:node1857e284cx70 .

_:node1857e284cx71 rdf:first disco:Study ;
	rdf:rest _:node1857e284cx72 .

_:node1857e284cx72 rdf:first disco:StudyGroup ;
	rdf:rest rdf:nil .

_:node1857e284cx70 rdf:first _:node1857e284cx71 ;
	rdf:rest _:node1857e284cx73 .

_:node1857e284cx73 rdf:first disco:Variable ;
	rdf:rest rdf:nil .

_:node1857e284cx74 owl:unionOf _:node1857e284cx69 .

disco:analysisUnit rdfs:domain _:node1857e284cx74 ;
	rdfs:range disco:AnalysisUnit ;
	rdfs:isDefinedBy <http://rdf-vocabulary.ddialliance.org/discovery> .

disco:basedOn a rdf:Property , owl:ObjectProperty ;
	rdfs:label "based on"@en , "utilise l'élément de donnée"@fr ;
	rdfs:comment "points to the VariableDefinition the Variable is based on."@en ;
	rdfs:domain disco:Variable ;
	rdfs:range disco:VariableDefinition ;
	rdfs:isDefinedBy <http://rdf-vocabulary.ddialliance.org/discovery> .

disco:collectionMode a rdf:Property , owl:ObjectProperty ;
	rdfs:label "collection mode"@en , "Datenerfassungsmodus"@de ;
	rdfs:comment "mode of collection of a Questionnaire"@en ;
	rdfs:domain disco:Questionnaire ;
	rdfs:range skos:Concept ;
	rdfs:isDefinedBy <http://rdf-vocabulary.ddialliance.org/discovery> .

disco:containsVariable a rdf:Property , owl:ObjectProperty ;
	rdfs:label "contains variable"@en , "contient la variable"@fr ;
	rdfs:comment "points to Variable contained in the LogicalDataSet"@en ;
	rdfs:domain disco:LogicalDataSet ;
	rdfs:range disco:Variable ;
	rdfs:isDefinedBy <http://rdf-vocabulary.ddialliance.org/discovery> .

disco:concept a rdf:Property , owl:ObjectProperty ;
	rdfs:label "concept"@en , "a pour concept"@fr ;
	rdfs:comment "points to the DDI concept of a VariableDefinition, a Variable, or a Question"@en .

_:node1857e284cx75 rdf:first disco:VariableDefinition ;
	rdf:rest _:node1857e284cx76 .

_:node1857e284cx76 rdf:first disco:Question ;
	rdf:rest _:node1857e284cx77 .

_:node1857e284cx77 rdf:first disco:Variable ;
	rdf:rest rdf:nil .

_:node1857e284cx78 owl:unionOf _:node1857e284cx75 .

disco:concept rdfs:domain _:node1857e284cx78 ;
	rdfs:range skos:Concept ;
	rdfs:isDefinedBy <http://rdf-vocabulary.ddialliance.org/discovery> .

disco:aggregation a rdf:Property , owl:ObjectProperty ;
	rdfs:label "aggregation"@en ;
	rdfs:comment "points to the aggregated data set of a microdata data set."@en ;
	rdfs:domain disco:LogicalDataSet ;
	rdfs:range qb:DataSet ;
	rdfs:isDefinedBy <http://rdf-vocabulary.ddialliance.org/discovery> .

disco:dataFile a rdf:Property , owl:ObjectProperty ;
	rdfs:label "data file"@en , "a pour fichier de données"@fr ;
	rdfs:comment "points to the DataFile of a Study or a LogicalDataSet."@en .

_:node1857e284cx79 rdf:first disco:Study ;
	rdf:rest _:node1857e284cx80 .

_:node1857e284cx80 rdf:first disco:LogicalDataSet ;
	rdf:rest rdf:nil .

_:node1857e284cx81 owl:unionOf _:node1857e284cx79 .

disco:dataFile rdfs:domain _:node1857e284cx81 ;
	rdfs:range disco:DataFile ;
	rdfs:isDefinedBy <http://rdf-vocabulary.ddialliance.org/discovery> .

disco:ddifile a rdf:Property , owl:ObjectProperty ;
	rdfs:label "DDI file"@en , "DDI-Datei"@de ;
	rdfs:comment "points from a Study or a StudyGroup to the original DDI file which is a foaf:Document."@en .

_:node1857e284cx82 rdf:first disco:Study ;
	rdf:rest _:node1857e284cx83 .

_:node1857e284cx83 rdf:first disco:StudyGroup ;
	rdf:rest rdf:nil .

_:node1857e284cx84 owl:unionOf _:node1857e284cx82 .

disco:ddifile rdfs:domain _:node1857e284cx84 ;
	rdfs:range foaf:Document ;
	rdfs:isDefinedBy <http://rdf-vocabulary.ddialliance.org/discovery> .

disco:externalDocumentation a rdf:Property , owl:ObjectProperty ;
	rdfs:label "external documentation"@en , "externe Dokumentation"@de ;
	rdfs:comment "points from an Instrument to a foaf:Document which is the external documentation of the Instrument."@en ;
	rdfs:domain disco:Instrument ;
	rdfs:range foaf:Document ;
	rdfs:isDefinedBy <http://rdf-vocabulary.ddialliance.org/discovery> .

disco:fundedBy a rdf:Property , owl:ObjectProperty ;
	rdfs:label "funded by"@en ;
	rdfs:comment "points from a Study or a StudyGroup to the funding foaf:Agent which is either a foaf:Person or a org:Organization."@en .

_:node1857e284cx85 rdf:first disco:Study ;
	rdf:rest _:node1857e284cx86 .

_:node1857e284cx86 rdf:first disco:StudyGroup ;
	rdf:rest rdf:nil .

_:node1857e284cx87 owl:unionOf _:node1857e284cx85 .

disco:fundedBy rdfs:domain _:node1857e284cx87 ;
	rdfs:range foaf:Agent ;
	rdfs:subPropertyOf dcterms:contributor ;
	rdfs:isDefinedBy <http://rdf-vocabulary.ddialliance.org/discovery> .

disco:inGroup a rdf:Property , owl:ObjectProperty ;
	rdfs:label "in group"@en ;
	rdfs:comment "points from a Study to the StudyGroup which contains the Study."@en ;
	rdfs:domain disco:Study ;
	rdfs:range disco:StudyGroup ;
	rdfs:isDefinedBy <http://rdf-vocabulary.ddialliance.org/discovery> .

disco:inputVariable a rdf:Property , owl:ObjectProperty ;
	rdfs:label "input variable"@en , "variable en entrée"@fr ;
	rdfs:comment "Indicates the original Variable of an aggregated qb:DataSet."@en ;
	rdfs:domain qb:DataSet ;
	rdfs:range disco:Variable ;
	rdfs:isDefinedBy <http://rdf-vocabulary.ddialliance.org/discovery> .

disco:instrument a rdf:Property , owl:ObjectProperty ;
	rdfs:label "instrument"@en , "a comme instrument"@fr ;
	rdfs:comment "Indicates the Instrument of a Study or a LogicalDataSet."@en .

_:node1857e284cx88 rdf:first disco:Study ;
	rdf:rest _:node1857e284cx89 .

_:node1857e284cx89 rdf:first disco:LogicalDataSet ;
	rdf:rest rdf:nil .

_:node1857e284cx90 owl:unionOf _:node1857e284cx88 .

disco:instrument rdfs:domain _:node1857e284cx90 ;
	rdfs:range disco:Instrument ;
	rdfs:isDefinedBy <http://rdf-vocabulary.ddialliance.org/discovery> .

disco:kindOfData a rdf:Property , owl:ObjectProperty ;
	rdfs:label "kind of data"@en .

_:node1857e284cx91 rdf:first disco:Study ;
	rdf:rest _:node1857e284cx92 .

_:node1857e284cx92 rdf:first disco:StudyGroup ;
	rdf:rest rdf:nil .

_:node1857e284cx93 owl:unionOf _:node1857e284cx91 .

disco:kindOfData rdfs:domain _:node1857e284cx93 ;
	rdfs:range skos:Concept ;
	rdfs:comment "The general kind of data (e.g. geospatial, register, survey) collected in this study, given either as a skos:Concept, or as a blank node with attached free-text rdfs:label." ;
	rdfs:isDefinedBy <http://rdf-vocabulary.ddialliance.org/discovery> .

disco:product a rdf:Property , owl:ObjectProperty ;
	rdfs:label "product"@en , "Produkt"@de ;
	rdfs:comment "Indicates the LogicalDataSets of a Studies."@en ;
	rdfs:domain disco:Study ;
	rdfs:range qb:LogicalDataSet ;
	rdfs:isDefinedBy <http://rdf-vocabulary.ddialliance.org/discovery> .

disco:question a rdf:Property , owl:ObjectProperty ;
	rdfs:label "question"@en , "a comme question"@fr ;
	rdfs:comment "Indicates the Questions associated to Variables or contained in Questionnaires."@en .

_:node1857e284cx94 rdf:first disco:Variable ;
	rdf:rest _:node1857e284cx95 .

_:node1857e284cx95 rdf:first disco:Questionnaire ;
	rdf:rest rdf:nil .

_:node1857e284cx96 owl:unionOf _:node1857e284cx94 .

disco:question rdfs:domain _:node1857e284cx96 ;
	rdfs:range disco:Question ;
	rdfs:isDefinedBy <http://rdf-vocabulary.ddialliance.org/discovery> .

disco:representation a rdf:Property , owl:ObjectProperty ;
	rdfs:label "representation"@en , "a pour représentation"@fr ;
	rdfs:comment "VariableDefinitions and Variables can have a Representation whose individuals are either of the class rdfs:Datatype (to represent values) or skos:ConceptScheme (to represent code lists)."@en .

_:node1857e284cx97 rdf:first disco:VariableDefinition ;
	rdf:rest _:node1857e284cx98 .

_:node1857e284cx98 rdf:first disco:Variable ;
	rdf:rest rdf:nil .

_:node1857e284cx99 owl:unionOf _:node1857e284cx97 .

disco:representation rdfs:domain _:node1857e284cx99 .

_:node1857e284cx100 rdf:first skos:ConceptScheme ;
	rdf:rest _:node1857e284cx101 .

_:node1857e284cx101 rdf:first rdfs:Datatype ;
	rdf:rest rdf:nil .

_:node1857e284cx102 owl:unionOf _:node1857e284cx100 .

disco:representation rdfs:range _:node1857e284cx102 ;
	rdfs:isDefinedBy <http://rdf-vocabulary.ddialliance.org/discovery> .

disco:statisticsCategory a rdf:Property , owl:ObjectProperty ;
	rdfs:label "statistics category"@en , "a pour concept statistique"@fr ;
	rdfs:comment "Indicates the skos:Concept (representing codes and categories) of a specific CategoryStatistics individual."@en ;
	rdfs:domain disco:CategoryStatistics ;
	rdfs:range skos:Concept ;
	rdfs:isDefinedBy <http://rdf-vocabulary.ddialliance.org/discovery> .

disco:statisticsDataFile a rdf:Property , owl:ObjectProperty ;
	rdfs:label "statistics data file"@en , "a pour fichier statistique"@fr ;
	rdfs:comment "Indicates the DataFile of a specific DesciptiveStatistics individual."@en ;
	rdfs:domain disco:DescriptiveStatistics ;
	rdfs:range disco:DataFile ;
	rdfs:isDefinedBy <http://rdf-vocabulary.ddialliance.org/discovery> .

disco:statisticsVariable a rdf:Property , owl:ObjectProperty ;
	rdfs:label "statistics variable"@en , "a pour variable statistique"@fr ;
	rdfs:comment "Indicates the Variable of a specific SummaryStatistics individual."@en ;
	rdfs:domain disco:SummaryStatistics ;
	rdfs:range disco:Variable ;
	rdfs:isDefinedBy <http://rdf-vocabulary.ddialliance.org/discovery> .

disco:weightedBy a rdf:Property , owl:ObjectProperty ;
	rdfs:label "weighted by"@en , ""@fr ;
	rdfs:comment "SummaryStatistics or CategoryStatistics resources may be weighted by a specific Variable."@en .

_:node1857e284cx103 rdf:first disco:SummaryStatistics ;
	rdf:rest _:node1857e284cx104 .

_:node1857e284cx104 rdf:first disco:CategoryStatistics ;
	rdf:rest rdf:nil .

_:node1857e284cx105 owl:unionOf _:node1857e284cx103 .

disco:weightedBy rdfs:domain _:node1857e284cx105 ;
	rdfs:range disco:Variable ;
	rdfs:isDefinedBy <http://rdf-vocabulary.ddialliance.org/discovery> .

disco:universe a rdf:Property , owl:ObjectProperty ;
	rdfs:label "universe"@en , "a comme univers"@fr ;
	rdfs:comment "Indicates the Universe(s) of Studies, StudyGrous, VariableDefinitions, Variables, Questions, and LogicalDataSets."@en .

_:node1857e284cx106 rdf:first disco:Study ;
	rdf:rest _:node1857e284cx107 .

_:node1857e284cx107 rdf:first disco:StudyGroup ;
	rdf:rest _:node1857e284cx108 .

_:node1857e284cx108 rdf:first disco:VariableDefinition ;
	rdf:rest _:node1857e284cx109 .

_:node1857e284cx109 rdf:first disco:Variable ;
	rdf:rest _:node1857e284cx110 .

_:node1857e284cx110 rdf:first disco:Question ;
	rdf:rest _:node1857e284cx111 .

_:node1857e284cx111 rdf:first disco:LogicalDataSet ;
	rdf:rest rdf:nil .

_:node1857e284cx112 owl:unionOf _:node1857e284cx106 .

disco:universe rdfs:domain _:node1857e284cx112 ;
	rdfs:range disco:Universe ;
	rdfs:isDefinedBy <http://rdf-vocabulary.ddialliance.org/discovery> .

disco:variable a rdf:Property , owl:ObjectProperty ;
	rdfs:label "variable"@en , "Variable"@de ;
	rdfs:comment "Indicates the Variable of a Study."@en ;
	rdfs:domain disco:Study ;
	rdfs:range disco:Variable ;
	rdfs:isDefinedBy <http://rdf-vocabulary.ddialliance.org/discovery> .
