@prefix ns1:   <http://purl.org/net/hifm/ontology#> .
@prefix rdfs:  <http://www.w3.org/2000/01/rdf-schema#> .
@prefix owl:   <http://www.w3.org/2002/07/owl#> .
@prefix xsd:   <http://www.w3.org/2001/XMLSchema#> .
@prefix rdf:   <http://www.w3.org/1999/02/22-rdf-syntax-ns#> .
@prefix ns5:   <http://purl.org/dc/terms/> .
@prefix ns6:   <http://purl.org/vocab/vann/> .
@prefix ns7:   <http://creativecommons.org/ns#> .

ns1:strength  a       owl:DatatypeProperty ;
        rdfs:comment  "This property represents the strength of the drug, in milligrams." ;
        rdfs:domain   ns1:Drug ;
        rdfs:range    xsd:string .

ns1:Drug  a           owl:Class ;
        rdfs:comment  "This class represents a brand-name drug." .

ns1:refPriceWithVAT  a  owl:DatatypeProperty ;
        rdfs:comment  "This property represents the referent value of the medicine in macedonian denars (MKD), with VAT calculated" ;
        rdfs:domain   ns1:Drug ;
        rdfs:range    xsd:float .

ns1:packaging  a      owl:DatatypeProperty ;
        rdfs:comment  "This property represents the number of units per drug package." ;
        rdfs:domain   ns1:Drug ;
        rdfs:range    xsd:nonNegativeInteger .

ns1:refPriceNoVAT  a  owl:DatatypeProperty ;
        rdfs:comment  "This property represents the referent price of the medicine in macedonian denars (MKD), with NO VAT calculated" ;
        rdfs:domain   ns1:Drug ;
        rdfs:range    xsd:float .

ns1:notes  a          owl:DatatypeProperty ;
        rdfs:comment  "This property represents additional notes related to a medicine." ;
        rdfs:domain   ns1:Drug ;
        rdfs:range    xsd:string .

ns1:id  a             owl:DatatypeProperty ;
        rdfs:comment  "This is the ID that the medicine has in the local system of the Health Insurance Fund of Macedonia" ;
        rdfs:domain   ns1:Drug ;
        rdfs:range    xsd:string .

ns1:similarTo  a      owl:ObjectProperty , owl:SymmetricProperty , owl:TransitiveProperty ;
        rdfs:comment  "This property represents a similarity that is known between two drugs." ;
        rdfs:domain   ns1:Drug ;
        rdfs:range    ns1:Drug .

ns1:    a                             owl:Ontology ;
        rdfs:comment                  "The HIFM Ontology." ;
        ns7:license                   <https://creativecommons.org/licenses/by/3.0/> ;
        ns5:contributor               <https://plus.google.com/+BojanNajdenov> ;
        ns5:creator                   <https://plus.google.com/+MilosJovanovik> ;
        ns5:description               "An ontology for describing brand-name drugs." ;
        ns5:issued                    "2014-04-01" ;
        ns5:modified                  "2016-08-28" ;
        ns5:publisher                 <http://finki.ukim.mk/> ;
        ns5:rights                    "Copyright 2014, Milos Jovanovik" ;
        ns5:title                     "HIFM Ontology" ;
        ns6:preferredNamespacePrefix  "hifm" ;
        ns6:preferredNamespaceUri     "http://purl.org/net/hifm/ontology#" ;
        owl:versionInfo               "1.1" .

ns1:dosageForm  a     owl:DatatypeProperty ;
        rdfs:comment  "This property represents the dosage form of the medicine." ;
        rdfs:domain   ns1:Drug ;
        rdfs:range    xsd:string .

ns1:manufacturer  a   owl:DatatypeProperty ;
        rdfs:comment  "This property represents a manufacturer of a drug." ;
        rdfs:domain   ns1:Drug ;
        rdfs:range    xsd:string .
