@prefix :      <http://vocab.sindice.net/> .
@prefix geo:   <http://www.w3.org/2003/01/geo/wgs84_pos#> .
@prefix foaf:  <http://xmlns.com/foaf/0.1/> .
@prefix vann:  <http://purl.org/vocab/vann/> .
@prefix vs:    <http://www.w3.org/2003/06/sw-vocab-status/ns#> .
@prefix rdfs:  <http://www.w3.org/2000/01/rdf-schema#> .
@prefix time:  <http://www.w3.org/2006/time#> .
@prefix bio:   <http://purl.org/vocab/bio/0.1/> .
@prefix dct:   <http://purl.org/dc/terms/> .
@prefix event: <http://purl.org/NET/c4dm/event.owl#> .
@prefix bibo:  <http://purl.org/ontology/bibo/> .
@prefix xsd:   <http://www.w3.org/2001/XMLSchema#> .
@prefix owl:   <http://www.w3.org/2002/07/owl#> .
@prefix rdf:   <http://www.w3.org/1999/02/22-rdf-syntax-ns#> .

bio:Birth  a              owl:Class ;
        rdfs:comment      "The event of a person entering into life."@en ;
        rdfs:isDefinedBy  bio: ;
        rdfs:label        "Birth"@en ;
        rdfs:subClassOf   bio:IndividualEvent .

<http://purl.org/gen/0.1#participant>
        a                   rdf:Property ;
        rdfs:comment        "Adapts bio:agent by having a range of foaf:Person rather than foaf:Agent."@en ;
        rdfs:domain         bio:Event ;
        rdfs:label          "participant"@en ;
        rdfs:range          foaf:Person ;
        rdfs:subPropertyOf  bio:agent ;
        owl:inverseOf       <http://purl.org/gen/0.1#lifeEvent> .

bio:Marriage  a           owl:Class ;
        rdfs:comment      "The event of creating uniting the participants into a new family unit, sometimes accompanied by a formal wedding ceremony. This is intended to cover a broad range of marriages including those given formal legal standing, common-law, or by convention. It is not restricted to marriages of two people of the opposite gender, but also includes polygamous and same-sex unions."@en ;
        rdfs:isDefinedBy  bio: ;
        rdfs:label        "Marriage"@en ;
        rdfs:subClassOf   bio:GroupEvent .

foaf:givenName  a         owl:DatatypeProperty , rdf:Property ;
        rdfs:comment      "The given name of some person." ;
        rdfs:isDefinedBy  foaf: ;
        rdfs:label        "Given name" .

<http://purl.org/gen/0.1#Microfilm>
        a                owl:Class ;
        rdfs:comment     "A microfilm reel"@en ;
        rdfs:label       "Microfilm"@en ;
        rdfs:subClassOf  <http://purl.org/gen/0.1#Microform> ;
        vs:term_status   "testing" .

<http://purl.org/gen/0.1#Place>
        a                owl:Class ;
        rdfs:comment     "A geolocated position"@en ;
        rdfs:label       "Place"@en ;
        rdfs:subClassOf  geo:SpatialThing ;
        vs:term_status   "testing" .

event:Event  a            owl:Class ;
        rdfs:comment      "\n\t\tAn arbitrary classification of a space/time region, by a \n\t\tcognitive agent. An event may have actively participating agents,\n\t\tpassive factors, products, and a location in space/time.\n\t\t" ;
        rdfs:isDefinedBy  <http://purl.org/NET/c4dm/event.owl> ;
        rdfs:label        "Event" .

<http://purl.org/gen/0.1#Microform>
        a                owl:Class ;
        rdfs:comment     "The general class of microform media, defined by Wikipedia as 'any forms, either films or paper,\n\t\tcontaining microreproductions of documents for transmission, storage, reading, and printing.'"@en ;
        rdfs:label       "Microform"@en ;
        rdfs:subClassOf  bibo:Document ;
        vs:term_status   "testing" .

<http://purl.org/gen/0.1#GraveInscription>
        a                owl:Class ;
        rdfs:comment     "A grave inscription, such as on a tomb or headstone."@en ;
        rdfs:label       "Grave Inscription"@en ;
        rdfs:subClassOf  <http://purl.org/gen/0.1#MonumentalInscription> ;
        vs:term_status   "testing" .

<http://purl.org/gen/0.1#birthParent>
        a                   rdf:Property ;
        rdfs:domain         bio:Birth ;
        rdfs:range          foaf:Person ;
        rdfs:subPropertyOf  bio:parent , <http://purl.org/gen/0.1#participant> .

<http://purl.org/gen/0.1#mother>
        a                   rdf:Property ;
        rdfs:comment        "A mother of a family."@en ;
        rdfs:domain         <http://purl.org/gen/0.1#Family> ;
        rdfs:label          "mother"@en ;
        rdfs:range          foaf:Person ;
        rdfs:subPropertyOf  <http://purl.org/gen/0.1#parent> .

<http://any23.org/tmp/>
        :date   "2012-01-26T19:01:48+00:00" ;
        :size   "272"^^xsd:int .

<http://purl.org/gen/0.1#birthMother>
        a                   rdf:Property ;
        rdfs:domain         bio:Birth ;
        rdfs:range          foaf:Person ;
        rdfs:subPropertyOf  <http://purl.org/gen/0.1#birthParent> .

<http://purl.org/gen/0.1#stepParent>
        a                   rdf:Property ;
        rdfs:comment        "A step-parent of a family."@en ;
        rdfs:domain         <http://purl.org/gen/0.1#Family> ;
        rdfs:label          "stepParent"@en ;
        rdfs:range          foaf:Person ;
        rdfs:subPropertyOf  <http://purl.org/gen/0.1#parent> .

<http://purl.org/gen/0.1#parent>
        a                   rdf:Property ;
        rdfs:comment        "A parent in a family."@en ;
        rdfs:domain         <http://purl.org/gen/0.1#Family> ;
        rdfs:label          "parent"@en ;
        rdfs:range          foaf:Person ;
        rdfs:subPropertyOf  <http://purl.org/gen/0.1#familyMember> .

foaf:familyName  a        owl:DatatypeProperty , rdf:Property ;
        rdfs:comment      "The family name of some person." ;
        rdfs:domain       foaf:Person ;
        rdfs:isDefinedBy  foaf: ;
        rdfs:label        "familyName" ;
        rdfs:range        rdfs:Literal .

bio:Divorce  a            owl:Class ;
        rdfs:comment      "The event of legally dissolving a marriage."@en ;
        rdfs:isDefinedBy  bio: ;
        rdfs:label        "Divorce"@en ;
        rdfs:subClassOf   bio:GroupEvent .

<http://purl.org/gen/0.1#Microfiche>
        a                owl:Class ;
        rdfs:comment     "'A microfiche is a flat film 105 x 148 mm in size, that is ISO A6.' (Wikipedia:Microform)"@en ;
        rdfs:label       "Microfiche"@en ;
        rdfs:subClassOf  <http://purl.org/gen/0.1#Microform> ;
        vs:term_status   "testing" .

<http://purl.org/gen/0.1#lifeEvent>
        a                   rdf:Property ;
        rdfs:comment        "The lifeEvent property is a slight variation on bio:event in which the domain is foaf:Person rather than foaf:Agent, since genealogy is about people."@en ;
        rdfs:domain         foaf:Person ;
        rdfs:label          "lifeEvent"@en ;
        rdfs:range          bio:Event ;
        rdfs:subPropertyOf  bio:event ;
        owl:inverseOf       <http://purl.org/gen/0.1#participant> .

<http://purl.org/gen/0.1#source>
        a               rdf:Property ;
        rdfs:comment    "A source justifying some assertion or claim of fact. The range is deliberately left as general as possible\n\t\t(owl:Thing) because of the unsettled state of bibliographic vocabularies. My recommendation is to use\n\t\tbibo:Document and its associated vocabulary, though frbr:Work seems reasonable, too. Surely there are\n\t\tmany other options---hopefully a clear standard emerges in the future."@en ;
        rdfs:domain     <http://purl.org/gen/0.1#Assertion> ;
        rdfs:label      "Source"@en ;
        rdfs:range      owl:Thing ;
        vs:term_status  "unstable" .

<http://purl.org/gen/0.1#stepMother>
        a                   rdf:Property ;
        rdfs:comment        "A step-mother of a family."@en ;
        rdfs:domain         <http://purl.org/gen/0.1#Family> ;
        rdfs:label          "stepMother"@en ;
        rdfs:range          foaf:Person ;
        rdfs:subPropertyOf  <http://purl.org/gen/0.1#stepParent> .

<http://purl.org/gen/0.1#child>
        a                   rdf:Property ;
        rdfs:comment        "A child in a family."@en ;
        rdfs:domain         <http://purl.org/gen/0.1#Family> ;
        rdfs:label          "child"@en ;
        rdfs:range          foaf:Person ;
        rdfs:subPropertyOf  <http://purl.org/gen/0.1#familyMember> .

bio:Burial  a             owl:Class ;
        rdfs:comment      "The event of interring the remains of a person's body into the ground."@en ;
        rdfs:isDefinedBy  bio: ;
        rdfs:label        "Burial"@en ;
        rdfs:subClassOf   bio:IndividualEvent .

<http://purl.org/gen/0.1#FamilyTree>
        a               owl:Class ;
        rdfs:comment    "This container class should be populated with individual people, families, or other records\n\t\tthat constitute a single 'family tree'. It is intended to help users in management of their\n\t\tgenealogical data."@en ;
        rdfs:label      "Family Tree"@en ;
        vs:term_status  "testing" .

bio:Baptism  a            owl:Class ;
        rdfs:comment      "The ceremonial event held to admit a person to membership of a Christian church."@en ;
        rdfs:isDefinedBy  bio: ;
        rdfs:label        "Baptism"@en ;
        rdfs:subClassOf   bio:IndividualEvent .

<http://purl.org/gen/0.1#Family>
        a                owl:Class ;
        rdfs:comment     "Though it is preferred to represent families by describing the relationships between its members\n\t\t(parent-child, husband-wife, etc.) this class can be used to represent a group of people who are\n\t\tconsidered to be a family unit."@en ;
        rdfs:label       "Family"@en ;
        rdfs:subClassOf  foaf:Group ;
        vs:term_status   "testing" .

<http://purl.org/gen/0.1#name>
        a               rdf:Property ;
        rdfs:comment    "A person's name."@en ;
        rdfs:domain     foaf:Person ;
        rdfs:label      "name"@en ;
        rdfs:range      <http://purl.org/gen/0.1#Name> ;
        vs:term_status  "testing" .

<http://purl.org/gen/0.1#birthFather>
        a                   rdf:Property ;
        rdfs:domain         bio:Birth ;
        rdfs:range          foaf:Person ;
        rdfs:subPropertyOf  <http://purl.org/gen/0.1#birthParent> .

<http://purl.org/gen/0.1#Name>
        a               owl:Class ;
        rdfs:comment    "A personal name. Names are a class of their own to facilitate associating multiple names with\n\t\tthe same individual, and to allow different types of names or ways of representing them."@en ;
        rdfs:label      "Name"@en ;
        vs:term_status  "testing" .

<http://purl.org/gen/0.1#death>
        a                   rdf:Property ;
        rdfs:comment        "Specifies a person's death event."@en ;
        rdfs:domain         foaf:Person ;
        rdfs:label          "death"@en ;
        rdfs:range          bio:Death ;
        rdfs:subPropertyOf  bio:death , <http://purl.org/gen/0.1#lifeEvent> .

<http://purl.org/gen/0.1#Time>
        a                owl:Class ;
        rdfs:comment     "A moment in time or a span of time"@en ;
        rdfs:label       "Time"@en ;
        rdfs:subClassOf  time:TemporalEntity ;
        vs:term_status   "testing" .

<http://purl.org/gen/0.1#birth>
        a                   rdf:Property ;
        rdfs:comment        "Specifies a person's birth event."@en ;
        rdfs:domain         foaf:Person ;
        rdfs:label          "birth"@en ;
        rdfs:range          bio:Birth ;
        rdfs:subPropertyOf  bio:event , <http://purl.org/gen/0.1#lifeEvent> ;
        owl:inverseOf       <http://purl.org/gen/0.1#newborn> .

<http://purl.org/gen/0.1#FoafName>
        a                owl:Class ;
        rdfs:comment     "A name class aiming for maximum compatibility with FOAF. Individuals in this class are intended\n\t\tto be described using foaf's name properties, namely foaf:name, foaf:givenName, and\n\t\tfoaf:familyName."@en ;
        rdfs:label       "FOAF Name"@en ;
        rdfs:subClassOf  <http://purl.org/gen/0.1#Name> ;
        vs:term_status   "testing" .

<http://purl.org/gen/0.1#stepFather>
        a                   rdf:Property ;
        rdfs:comment        "A step-father of a family."@en ;
        rdfs:domain         <http://purl.org/gen/0.1#Family> ;
        rdfs:label          "stepFather"@en ;
        rdfs:range          foaf:Person ;
        rdfs:subPropertyOf  <http://purl.org/gen/0.1#stepParent> .

foaf:name  a                owl:DatatypeProperty , rdf:Property ;
        rdfs:comment        "A name for some thing." ;
        rdfs:domain         owl:Thing ;
        rdfs:isDefinedBy    foaf: ;
        rdfs:label          "name" ;
        rdfs:range          rdfs:Literal ;
        rdfs:subPropertyOf  rdfs:label .

<http://purl.org/gen/0.1#father>
        a                   rdf:Property ;
        rdfs:comment        "A father of a family."@en ;
        rdfs:domain         <http://purl.org/gen/0.1#Family> ;
        rdfs:label          "father"@en ;
        rdfs:range          foaf:Person ;
        rdfs:subPropertyOf  <http://purl.org/gen/0.1#parent> .

<http://purl.org/gen/0.1#familyMember>
        a                   rdf:Property ;
        rdfs:comment        "Indicates a member of a Family" ;
        rdfs:domain         <http://purl.org/gen/0.1#Family> ;
        rdfs:label          "familyMember" ;
        rdfs:range          foaf:Person ;
        rdfs:subPropertyOf  foaf:member ;
        vs:term_status      "testing" .

<http://purl.org/gen/0.1#newborn>
        a                   rdf:Property ;
        rdfs:domain         bio:Birth ;
        rdfs:range          foaf:Person ;
        rdfs:subPropertyOf  bio:principal , <http://purl.org/gen/0.1#participant> ;
        owl:inverseOf       <http://purl.org/gen/0.1#birth> .

<http://purl.org/gen/0.1#MonumentalInscription>
        a                owl:Class ;
        rdfs:comment     "The general class of monumental inscriptions, defined by Wikipedia as 'an inscription, typically\n\t\tcarved in stone, on a grave marker, cenotaph, memorial plaque, church monument or other memorial.'"@en ;
        rdfs:label       "Monumental Inscription"@en ;
        rdfs:subClassOf  bibo:Document ;
        vs:term_status   "testing" .

bio:GroupEvent  a         owl:Class ;
        rdfs:comment      "A type of event that is principally about one or more agents and their partnership. Other agents may be involved but the event is most significant for the partner agent."@en ;
        rdfs:isDefinedBy  bio: ;
        rdfs:label        "Group Event"@en ;
        rdfs:subClassOf   bio:Event ;
        rdfs:subClassOf   [ a                   owl:Restriction ;
                            owl:minCardinality  "2"^^xsd:nonNegativeInteger ;
                            owl:onProperty      bio:partner
                          ] .

foaf:Person  a            owl:Class , rdfs:Class ;
        rdfs:comment      "A person." ;
        rdfs:isDefinedBy  foaf: ;
        rdfs:label        "Person" ;
        rdfs:subClassOf   foaf:Agent ;
        vs:term_status    "stable" .

<http://purl.org/gen/0.1#spouse>
        a                   rdf:Property ;
        rdfs:domain         bio:Marriage ;
        rdfs:range          foaf:Person ;
        rdfs:subPropertyOf  bio:partner , <http://purl.org/gen/0.1#participant> .

<http://purl.org/gen/0.1#subAssertion>
        a            rdf:Property ;
        rdfs:domain  <http://purl.org/gen/0.1#Assertion> ;
        rdfs:range   <http://purl.org/gen/0.1#Assertion> .

<http://purl.org/gen/0.1#Assertion>
        a                owl:Class ;
        rdfs:subClassOf  rdf:Statement .

bio:IndividualEvent  a    owl:Class ;
        rdfs:comment      "A type of event that is principally about a single person, group or organization. Other agents may be involved but the event is most significant for the principal agent."@en ;
        rdfs:isDefinedBy  bio: ;
        rdfs:label        "Individual Event"@en ;
        rdfs:subClassOf   bio:Event ;
        rdfs:subClassOf   [ a                owl:Restriction ;
                            owl:cardinality  "1"^^xsd:nonNegativeInteger ;
                            owl:onProperty   bio:principal
                          ] .

<http://purl.org/gen/0.1#>
        a                              owl:Ontology ;
        dct:abstract                   "A simple RDF vocabulary containing terms to facilitate the linking of genealogical data."@en ;
        dct:creator                    "Josh Hansen"@en ;
        dct:date                       "2012-01-26"^^xsd:date ;
        dct:issued                     "2012-01-26"^^xsd:date ;
        dct:rights                     "Copyright Â© 2012 FamilySearch"@en ;
        dct:title                      "Gen---A Vocabulary for Linked Genealogical Data"@en ;
        vann:preferredNamespacePrefix  "gen"@en ;
        vann:preferredNamespaceUri     "http://purl.org/gen/0.1#"@en .

<http://purl.org/gen/0.1#deceased>
        a                   rdf:Property ;
        rdfs:domain         bio:Death ;
        rdfs:range          foaf:Person ;
        rdfs:subPropertyOf  bio:principal , <http://purl.org/gen/0.1#participant> ;
        owl:inverseOf       <http://purl.org/gen/0.1#death> .

bio:Event  a              owl:Class ;
        rdfs:comment      "An event is an occurrence that brings about a change in the state of affairs for one or more people and/or other agents. Events are assumed to occur over a period of time and may not have precise start and end points."@en ;
        rdfs:isDefinedBy  bio: ;
        rdfs:label        "Event"@en .

bio:Death  a              owl:Class ;
        rdfs:comment      "The event of a person's life ending."@en ;
        rdfs:isDefinedBy  bio: ;
        rdfs:label        "Death"@en ;
        rdfs:subClassOf   bio:IndividualEvent .
