@prefix prv: <http://purl.org/ontology/prv/core#> .
@prefix dc: <http://purl.org/dc/elements/1.1/> .
@prefix rdfs: <http://www.w3.org/2000/01/rdf-schema#> .
@prefix foaf: <http://xmlns.com/foaf/0.1/> .
@prefix status: <http://www.w3.org/2003/06/sw-vocab-status/ns#> .
@prefix xsd: <http://www.w3.org/2001/XMLSchema#> .
@prefix owl: <http://www.w3.org/2002/07/owl#> .
@prefix vann: <http://purl.org/vocab/vann/> .
@prefix spin: <http://spinrdf.org/spin#> .
@prefix rdf: <http://www.w3.org/1999/02/22-rdf-syntax-ns#> .

<http://purl.org/ontology/prv/core#> a owl:Ontology ;
	dc:creator <http://foaf.me/zazi#me> , <http://mud.cz/foaf.rdf#ojirio> , <http://tobyinkster.co.uk/#i> , <http://richard.cyganiak.de/foaf.rdf#cygri> ;
	dc:date "2011-02-19T14:38:53+01:00"^^xsd:dateTime ;
	dc:description """A vocabulary for describing the ontology design pattern of property reification. That means the semantic relation of 
a \"shortcut relation\" (subject, predicate, object) with its detailed description of the relationship."""@en ;
	dc:title "Property Reification Vocabulary"@en ;
	vann:preferredNamespacePrefix "prv" ;
	vann:preferredNamespaceUri "http://purl.org/ontology/prv/core#" ;
	spin:imports <http://purl.org/ontology/prv/rules> ;
	owl:imports <http://xmlns.com/foaf/0.1/> , <http://purl.org/dc/elements/1.1/> , <http://www.w3.org/2003/06/sw-vocab-status/ns> , <http://purl.org/vocab/vann/> ;
	owl:versionInfo "0.11"^^xsd:decimal .

prv:PropertyReification a rdfs:Class ;
	rdfs:comment """The class, which describes the relations of a property reification. That means, its \"shortcut relation\", its 
reification class, and the properties that are relating to the subject and object of the \"shortcut relation\"."""@en ;
	rdfs:isDefinedBy <http://purl.org/ontology/prv/core#> ;
	rdfs:label "Property Reification"@en ;
	rdfs:subClassOf rdfs:Class ;
	status:term_status "testing"@en .

prv:object_property a rdf:Property ;
	rdfs:comment "Relates to the property of the reification class, which relates to the object of the \"shortcut relation\"."@en ;
	rdfs:domain prv:PropertyReification ;
	rdfs:isDefinedBy <http://purl.org/ontology/prv/core#> ;
	rdfs:label "has object property"@en ;
	rdfs:range rdf:Property ;
	status:term_status "testing"@en .

prv:reification_class a rdf:Property ;
	rdfs:comment """Relates to the reification class, which can be related to the object and subject property to be able to associate the 
object and subject of the \"shortcut relation\". The reification class should provide detailed descriptions of the relationship that is 
described in a simple form by the \"shortcut relation\"."""@en ;
	rdfs:domain prv:PropertyReification ;
	rdfs:isDefinedBy <http://purl.org/ontology/prv/core#> ;
	rdfs:label "has reification class"@en ;
	rdfs:range rdfs:Class ;
	status:term_status "testing"@en .

prv:reified a rdf:Property ;
	rdfs:comment "This property relates an statement identifier of a shortcut relation with an instance of a reification class. Although, this is at the moment not really applicable, because it requires a notation for statement identifier as optional fourth element of a tuple; that means, triple + statement identifier."@en ;
	rdfs:domain rdfs:Resource ;
	rdfs:isDefinedBy <http://purl.org/ontology/prv/core#> ;
	rdfs:label "reified"@en ;
	rdfs:range owl:Thing ;
	status:term_status "testing"@en .

prv:shortcut a rdf:Property ;
	rdfs:comment "Relates to the property of the \"shortcut relation\" (its predicate)."@en ;
	rdfs:domain prv:PropertyReification ;
	rdfs:isDefinedBy <http://purl.org/ontology/prv/core#> ;
	rdfs:label "has shortcut"@en ;
	rdfs:range rdf:Property ;
	status:term_status "testing"@en .

prv:shortcut_property a rdf:Property ;
	rdfs:comment """Relates to the property of the reification class,  which relates to the predicate of the \"shortcut relation\". So 
that the specific property reification can be \"verified\" (the property of the prv:shortcut relation and this one associated by the 
referred shortcut property should be equal)."""@en ;
	rdfs:domain prv:PropertyReification ;
	rdfs:isDefinedBy <http://purl.org/ontology/prv/core#> ;
	rdfs:label "has shortcut property"@en ;
	rdfs:range rdf:Property ;
	status:term_status "testing"@en .

prv:subject_property a rdf:Property ;
	rdfs:comment "Relates to the property of the reification class, which relates to the subject of the \"shortcut relation\"."@en ;
	rdfs:domain prv:PropertyReification ;
	rdfs:isDefinedBy <http://purl.org/ontology/prv/core#> ;
	rdfs:label "has subject property"@en ;
	rdfs:range rdf:Property ;
	status:term_status "testing"@en .
