@prefix owl: <http://www.w3.org/2002/07/owl#> .
@prefix rdfs: <http://www.w3.org/2000/01/rdf-schema#> .
@prefix xsd: <http://www.w3.org/2001/XMLSchema#> .
@prefix dc11: <http://purl.org/dc/elements/1.1/> .
@prefix dc: <http://purl.org/dc/terms/> .
@prefix ns0: <http://www.bbc.co.uk/ontologies/provenance/> .
@prefix foaf: <http://xmlns.com/foaf/0.1/> .
@prefix rdf: <http://www.w3.org/1999/02/22-rdf-syntax-ns#> .

<http://www.bbc.co.uk/ontologies/sport/subDisciplineOf>
  a owl:TransitiveProperty, owl:ObjectProperty ;
  rdfs:comment "Relates a discipline with a parent discipline, for example rhythmic gymnastics with gymnastics."@en-gb ;
  rdfs:domain <http://www.bbc.co.uk/ontologies/sport/SportsDiscipline> ;
  rdfs:isDefinedBy <http://www.bbc.co.uk/ontologies/sport> ;
  rdfs:label "subDisciplineOf"@en-gb ;
  rdfs:range <http://www.bbc.co.uk/ontologies/sport/SportsDiscipline> .

<http://www.bbc.co.uk/ontologies/sport/Home>
  a owl:Class ;
  rdfs:comment "The home ground, stadium or location of a Competitive Sporting Organisation."@en-gb ;
  rdfs:isDefinedBy <http://www.bbc.co.uk/ontologies/sport> ;
  rdfs:label "Home"@en-gb .

<http://www.bbc.co.uk/ontologies/sport/hasStage>
  a owl:ObjectProperty ;
  rdfs:comment "Relates a multi-stage competition to a stage that it contains."@en-gb ;
  rdfs:domain <http://www.bbc.co.uk/ontologies/sport/MultiStageCompetition> ;
  rdfs:isDefinedBy <http://www.bbc.co.uk/ontologies/sport> ;
  rdfs:label "hasStage"@en-gb ;
  rdfs:range <http://www.bbc.co.uk/ontologies/sport/Competition> .

<http://www.bbc.co.uk/things/competition-types/club-groupcup> a <http://www.bbc.co.uk/ontologies/sport/CompetitionType> .
<http://www.bbc.co.uk/ontologies/sport/roundType>
  a owl:ObjectProperty ;
  rdfs:comment "Relates a round to an enumerated round type."@en-gb ;
  rdfs:domain <http://www.bbc.co.uk/ontologies/sport/Round> ;
  rdfs:isDefinedBy <http://www.bbc.co.uk/ontologies/sport> ;
  rdfs:label "roundType"@en-gb ;
  rdfs:range <http://www.bbc.co.uk/ontologies/sport/RoundType> .

<http://www.bbc.co.uk/ontologies/sport/MultiStageCompetition>
  a owl:Class ;
  rdfs:comment "A Multi-stage Competition is a competition that is organised as a set of stages. An example is the Football World Cup."@en-gb ;
  rdfs:isDefinedBy <http://www.bbc.co.uk/ontologies/sport> ;
  rdfs:label "MultiStageCompetition"@en-gb ;
  rdfs:subClassOf <http://www.bbc.co.uk/ontologies/sport/Competition> .

<http://www.bbc.co.uk/ontologies/sport>
  a owl:Ontology, <http://www.bbc.co.uk/ontologies/provenance/Ontology> ;
  rdfs:comment "The Sport Ontology is a simple lightweight ontology for publishing data about competitive sports events."^^xsd:string ;
  rdfs:label "Sport Ontology"^^xsd:string ;
  dc11:creator <http://uk.linkedin.com/pub/jem-rayfield/27/b19/757>, <http://uk.linkedin.com/in/paulwilton>, <http://www.blockslabpillar.com>, <http://www.linkedin.com/in/tfgrahame>, <http://uk.linkedin.com/pub/stuart-williams/8/684/351>, <http://uk.linkedin.com/in/brianwmcbride> ;
  dc:license <http://creativecommons.org/licenses/by/4.0#id> ;
  ns0:canonicalLocation "https://repo.dev.bbc.co.uk/services/linked-data/ontologies/domain/sport/sport-2.13.ttl"^^xsd:string ;
  ns0:changeReason "Making sport:SportingOrganisation subClass core:Organisation. Refining some descriptions."@en-gb ;
  ns0:provided "2015-05-14T08:53:58+00:00"^^xsd:dateTime ;
  ns0:provider <mailto:tom.grahame@bbc.co.uk> ;
  ns0:public true ;
  ns0:slug "sport"^^xsd:string ;
  ns0:version "3.2"^^xsd:string ;
  owl:imports <http://www.bbc.co.uk/ontologies/coreconcepts>, foaf:, <http://www.bbc.co.uk/ontologies/asset/>, <http://purl.org/NET/c4dm/event.owl>, <http://www.bbc.co.uk/ontologies/provenance> ;
  owl:priorVersion <http://www.bbc.co.uk/ontologies/sport/3.1> ;
  owl:versionIRI <http://www.bbc.co.uk/ontologies/sport/3.2> ;
  owl:versionInfo "3.2"^^xsd:string .

<http://www.bbc.co.uk/things/competition-types/european-groupcup> a <http://www.bbc.co.uk/ontologies/sport/CompetitionType> .
<http://www.bbc.co.uk/ontologies/sport/Round>
  a owl:Class ;
  rdfs:comment "A round is one or more competitions that is part of a Multi-Round Competition. Examples include the first round of Wimbledon and the final round of the FA Cup."@en-gb ;
  rdfs:isDefinedBy <http://www.bbc.co.uk/ontologies/sport> ;
  rdfs:label "Round"@en-gb ;
  rdfs:subClassOf <http://www.bbc.co.uk/ontologies/sport/Competition> .

<http://www.bbc.co.uk/ontologies/sport/competesIn>
  a owl:ObjectProperty ;
  rdfs:comment "Relates a competitor, team or other agent to a competition."@en-gb ;
  rdfs:domain foaf:Agent ;
  rdfs:isDefinedBy <http://www.bbc.co.uk/ontologies/sport> ;
  rdfs:label "competesIn"@en-gb ;
  rdfs:range <http://www.bbc.co.uk/ontologies/sport/Competition> ;
  rdfs:subPropertyOf <http://purl.org/NET/c4dm/event.owl#agent_in> .

<http://www.bbc.co.uk/ontologies/sport/CompetitiveSportingOrganisation>
  a owl:Class ;
  rdfs:comment "A sporting organisation that participates in competitive sporting events. For example Manchester United or Team GB at the Olympics."@en-gb ;
  rdfs:isDefinedBy <http://www.bbc.co.uk/ontologies/sport> ;
  rdfs:label "CompetitiveSportingOrganisation"@en-gb ;
  rdfs:subClassOf <http://www.bbc.co.uk/ontologies/sport/SportingOrganisation> .

<http://www.bbc.co.uk/ontologies/sport/isRoundOf>
  a owl:ObjectProperty ;
  rdfs:comment "Relates a round to its corresponding multi-round competition."@en-gb ;
  rdfs:domain <http://www.bbc.co.uk/ontologies/sport/Round> ;
  rdfs:isDefinedBy <http://www.bbc.co.uk/ontologies/sport> ;
  rdfs:label "isRoundOf"@en-gb ;
  rdfs:range <http://www.bbc.co.uk/ontologies/sport/MultiRoundCompetition> ;
  owl:inverseOf <http://www.bbc.co.uk/ontologies/sport/hasRound> .

<http://www.bbc.co.uk/ontologies/sport/relegatesTo>
  a owl:ObjectProperty ;
  rdfs:comment "Relates a competition to the previous competition in a heirarchy that teams are relegated to. For example the  Premier League relegates to the nPower Championship."@en-gb ;
  rdfs:domain <http://www.bbc.co.uk/ontologies/sport/Competition> ;
  rdfs:isDefinedBy <http://www.bbc.co.uk/ontologies/sport> ;
  rdfs:label "relegatesTo"@en-gb ;
  rdfs:range <http://www.bbc.co.uk/ontologies/sport/Competition> ;
  owl:inverseOf <http://www.bbc.co.uk/ontologies/sport/promotesTo> .

<http://www.bbc.co.uk/ontologies/sport/Person>
  a owl:Class ;
  rdfs:comment "An athlete or other person with typically a participating role in a CompetitiveSportingOrganisation."@en-gb ;
  rdfs:isDefinedBy <http://www.bbc.co.uk/ontologies/sport> ;
  rdfs:label "Person"@en-gb ;
  rdfs:subClassOf foaf:Person, <http://www.bbc.co.uk/ontologies/coreconcepts/Person> .

<http://www.bbc.co.uk/ontologies/sport/GroupCompetition>
  a owl:Class ;
  rdfs:comment "An organisation as a collection of leagues used to select the top N competitors from each league."@en-gb ;
  rdfs:isDefinedBy <http://www.bbc.co.uk/ontologies/sport> ;
  rdfs:label "GroupCompetition"@en-gb ;
  rdfs:subClassOf <http://www.bbc.co.uk/ontologies/sport/MultiRoundCompetition> .

<http://www.bbc.co.uk/things/round-types/round-of-16> a <http://www.bbc.co.uk/ontologies/sport/RoundType> .
<http://www.bbc.co.uk/things/round-types/group> a <http://www.bbc.co.uk/ontologies/sport/RoundType> .
<http://www.bbc.co.uk/things/competition-types/domestic-groupcup-womens> a <http://www.bbc.co.uk/ontologies/sport/CompetitionType> .
<http://www.bbc.co.uk/ontologies/sport/CompetitionType>
  a owl:Class ;
  rdfs:comment "Enumerated competition types, for example: domestic, international."@en-gb ;
  rdfs:isDefinedBy <http://www.bbc.co.uk/ontologies/sport> ;
  rdfs:label "CompetitionType"@en-gb .

<http://www.bbc.co.uk/things/round-types/race> a <http://www.bbc.co.uk/ontologies/sport/RoundType> .
<http://www.bbc.co.uk/ontologies/sport/division>
  a rdf:Property ;
  rdfs:comment "Division relates a DivisionalCompetition to a competition which is a division of that DivisionalCompetition. Used for the olympics"^^xsd:string ;
  rdfs:domain <http://www.bbc.co.uk/ontologies/sport/DivisionalCompetition> ;
  rdfs:isDefinedBy <http://www.bbc.co.uk/ontologies/sport/2.0> ;
  rdfs:range <http://www.bbc.co.uk/ontologies/sport/Competition> ;
  rdfs:seeAlso <http://www.bbc.co.uk/ontologies/sport/hasDivisionList> ;
  owl:deprecated true .

<http://www.bbc.co.uk/ontologies/sport/Venue>
  a owl:Class ;
  rdfs:comment "The location of a sporting event. May be a stadium, track, lake etc."@en-gb ;
  rdfs:isDefinedBy <http://www.bbc.co.uk/ontologies/sport> ;
  rdfs:label "Venue"@en-gb .

<http://www.bbc.co.uk/things/competition-types/european-groupcup-womens> a <http://www.bbc.co.uk/ontologies/sport/CompetitionType> .
<http://www.bbc.co.uk/ontologies/sport/GoverningBody>
  a owl:Class ;
  rdfs:comment "The Governing Body for a sport, such as The Football Association."@en-gb ;
  rdfs:isDefinedBy <http://www.bbc.co.uk/ontologies/sport> ;
  rdfs:label "GoverningBody"@en-gb ;
  rdfs:subClassOf <http://www.bbc.co.uk/ontologies/sport/SportingOrganisation> .

<http://www.bbc.co.uk/things/competition-types/domestic-groupcup> a <http://www.bbc.co.uk/ontologies/sport/CompetitionType> .
<http://www.bbc.co.uk/things/round-types/round-of-32> a <http://www.bbc.co.uk/ontologies/sport/RoundType> .
<http://www.bbc.co.uk/ontologies/sport/MedalCompetition>
  a owl:Class ;
  rdfs:comment "A competition that results in the awarding of a medal to the winner or runner up in that competition."@en-gb ;
  rdfs:isDefinedBy <http://www.bbc.co.uk/ontologies/sport> ;
  rdfs:label "MedalCompetition"@en-gb ;
  rdfs:subClassOf <http://www.bbc.co.uk/ontologies/sport/Competition> .

<http://www.bbc.co.uk/ontologies/sport/hasCompetitor>
  a owl:ObjectProperty ;
  rdfs:comment "Relates a competition to a competitor in that competition."@en-gb ;
  rdfs:domain <http://www.bbc.co.uk/ontologies/sport/Competition> ;
  rdfs:isDefinedBy <http://www.bbc.co.uk/ontologies/sport> ;
  rdfs:label "hasCompetitor"@en-gb ;
  rdfs:range foaf:Agent .

<http://www.bbc.co.uk/ontologies/sport/isGroupOf>
  a owl:ObjectProperty ;
  rdfs:comment "Relates a group competition to its corresponding League competition."@en-gb ;
  rdfs:domain <http://www.bbc.co.uk/ontologies/sport/GroupCompetition> ;
  rdfs:isDefinedBy <http://www.bbc.co.uk/ontologies/sport> ;
  rdfs:label "isGroupOf"@en-gb ;
  rdfs:range <http://www.bbc.co.uk/ontologies/sport/LeagueCompetition> .

<http://www.bbc.co.uk/things/competition-types/domestic-league-womens> a <http://www.bbc.co.uk/ontologies/sport/CompetitionType> .
<http://www.bbc.co.uk/ontologies/sport/prevSession>
  a owl:ObjectProperty ;
  rdfs:comment "Relates a session to its previous session."@en-gb ;
  rdfs:domain <http://www.bbc.co.uk/ontologies/sport/Session> ;
  rdfs:isDefinedBy <http://www.bbc.co.uk/ontologies/sport> ;
  rdfs:label "prevSession"@en-gb ;
  rdfs:range <http://www.bbc.co.uk/ontologies/sport/Session> .

<http://www.bbc.co.uk/ontologies/sport/prevStage>
  a owl:ObjectProperty ;
  rdfs:comment "Relates a stage in a multi-stage competition to its previous stage."@en-gb ;
  rdfs:domain <http://www.bbc.co.uk/ontologies/sport/Competition> ;
  rdfs:isDefinedBy <http://www.bbc.co.uk/ontologies/sport> ;
  rdfs:label "prevStage"@en-gb ;
  rdfs:range <http://www.bbc.co.uk/ontologies/sport/Competition> .

<http://www.bbc.co.uk/things/round-types/semi-final> a <http://www.bbc.co.uk/ontologies/sport/RoundType> .
<http://www.bbc.co.uk/things/competition-types/club-groupcup-womens> a <http://www.bbc.co.uk/ontologies/sport/CompetitionType> .
<http://www.bbc.co.uk/ontologies/sport/flagImage>
  a owl:ObjectProperty ;
  rdfs:comment "Legacy property used to associate a team with the country flag it represented during the olympics" ;
  rdfs:domain <http://www.bbc.co.uk/ontologies/sport/CompetitiveSportingGroup> ;
  rdfs:isDefinedBy <http://www.bbc.co.uk/ontologies/sport/2.0> ;
  rdfs:range <http://www.bbc.co.uk/ontologies/asset/FlagImage> ;
  owl:deprecated true .

<http://www.bbc.co.uk/things/competition-types/international-groupcup> a <http://www.bbc.co.uk/ontologies/sport/CompetitionType> .
<http://www.bbc.co.uk/things/competition-types/domestic-league> a <http://www.bbc.co.uk/ontologies/sport/CompetitionType> .
<http://www.bbc.co.uk/ontologies/sport/CompetitiveSportingGroup>
  a owl:Class ;
  rdfs:comment "The group of people that are available to compete in a particular competition. Two groups with the same members are not necessarily the same group."@en-gb ;
  rdfs:isDefinedBy <http://www.bbc.co.uk/ontologies/sport> ;
  rdfs:label "CompetitiveSportingGroup"@en-gb ;
  rdfs:subClassOf foaf:Group .

<http://www.bbc.co.uk/ontologies/sport/lastUnitCompetition>
  a owl:ObjectProperty ;
  rdfs:comment "Relates a competition to its last unit competition."@en-gb ;
  rdfs:domain <http://www.bbc.co.uk/ontologies/sport/Competition> ;
  rdfs:isDefinedBy <http://www.bbc.co.uk/ontologies/sport> ;
  rdfs:label "lastUnitCompetition"@en-gb ;
  rdfs:range <http://www.bbc.co.uk/ontologies/sport/UnitCompetition> ;
  rdfs:subPropertyOf <http://www.bbc.co.uk/ontologies/sport/hasUnitCompetition> .

<http://www.bbc.co.uk/things/competition-types/international-cup-womens> a <http://www.bbc.co.uk/ontologies/sport/CompetitionType> .
<http://www.bbc.co.uk/ontologies/sport/hasRound>
  a owl:ObjectProperty ;
  rdfs:comment "Relates a multi-round competition to a round in that competition."@en-gb ;
  rdfs:domain <http://www.bbc.co.uk/ontologies/sport/MultiRoundCompetition> ;
  rdfs:isDefinedBy <http://www.bbc.co.uk/ontologies/sport> ;
  rdfs:label "hasRound"@en-gb ;
  rdfs:range <http://www.bbc.co.uk/ontologies/sport/Round> .

<http://www.bbc.co.uk/ontologies/sport/nextUnitCompetition>
  a owl:ObjectProperty ;
  rdfs:comment "Relates a unit competition to its next unit competition."@en-gb ;
  rdfs:domain <http://www.bbc.co.uk/ontologies/sport/UnitCompetition> ;
  rdfs:isDefinedBy <http://www.bbc.co.uk/ontologies/sport> ;
  rdfs:label "nextUnitCompetition"@en-gb ;
  rdfs:range <http://www.bbc.co.uk/ontologies/sport/UnitCompetition> .

<http://www.bbc.co.uk/ontologies/sport/Match>
  a owl:Class ;
  rdfs:comment "The smallest unit of sporting competition."@en-gb ;
  rdfs:isDefinedBy <http://www.bbc.co.uk/ontologies/sport> ;
  rdfs:label "Match"@en-gb ;
  rdfs:subClassOf <http://www.bbc.co.uk/ontologies/sport/UnitCompetition> .

<http://www.bbc.co.uk/ontologies/sport/firstStage>
  a owl:ObjectProperty ;
  rdfs:comment "Relates a multi-stage competition to its first stage in that competition."@en-gb ;
  rdfs:domain <http://www.bbc.co.uk/ontologies/sport/MultiStageCompetition> ;
  rdfs:isDefinedBy <http://www.bbc.co.uk/ontologies/sport> ;
  rdfs:label "firstStage"@en-gb ;
  rdfs:range <http://www.bbc.co.uk/ontologies/sport/Competition> ;
  rdfs:subPropertyOf <http://www.bbc.co.uk/ontologies/sport/hasStage> .

<http://www.bbc.co.uk/things/competition-types/domestic-cup> a <http://www.bbc.co.uk/ontologies/sport/CompetitionType> .
<http://www.bbc.co.uk/ontologies/sport/lastSession>
  a owl:ObjectProperty ;
  rdfs:comment "Relates a competition to the last session of a series of sessions."@en-gb ;
  rdfs:domain <http://www.bbc.co.uk/ontologies/sport/Competition> ;
  rdfs:isDefinedBy <http://www.bbc.co.uk/ontologies/sport> ;
  rdfs:label "lastSession"@en-gb ;
  rdfs:range <http://www.bbc.co.uk/ontologies/sport/Session> ;
  rdfs:subPropertyOf <http://www.bbc.co.uk/ontologies/sport/hasSession> .

<http://www.bbc.co.uk/things/event-gender/mixed> a <http://www.bbc.co.uk/ontologies/sport/EventGender> .
<http://www.bbc.co.uk/ontologies/sport/Competition>
  a owl:Class ;
  rdfs:comment "A competitive sporting event that usually appears as an occurrence of a recurring competition, for example the recurring English Football Premier League has a seasonal competition occurrence during 2012/13"@en-gb ;
  rdfs:isDefinedBy <http://www.bbc.co.uk/ontologies/sport> ;
  rdfs:label "Competition"@en-gb ;
  rdfs:subClassOf <http://purl.org/NET/c4dm/event.owl#Event> .

<http://www.bbc.co.uk/things/round-types/quarter-final> a <http://www.bbc.co.uk/ontologies/sport/RoundType> .
<http://www.bbc.co.uk/things/round-types/hosted> a <http://www.bbc.co.uk/ontologies/sport/RoundType> .
<http://www.bbc.co.uk/ontologies/sport/isMatchOf>
  a owl:ObjectProperty ;
  rdfs:comment "Relates a match to a round."@en-gb ;
  rdfs:domain <http://www.bbc.co.uk/ontologies/sport/Match> ;
  rdfs:isDefinedBy <http://www.bbc.co.uk/ontologies/sport> ;
  rdfs:label "isMatchOf"@en-gb ;
  rdfs:range <http://www.bbc.co.uk/ontologies/sport/Round> ;
  owl:inverseOf <http://www.bbc.co.uk/ontologies/sport/hasMatch> .

<http://www.bbc.co.uk/ontologies/sport/UnitCompetition>
  a owl:Class ;
  rdfs:comment "A unit competition is the unit of competition defined by a competition discipline rules. Examples include a 100m race or Football match."@en-gb ;
  rdfs:isDefinedBy <http://www.bbc.co.uk/ontologies/sport> ;
  rdfs:label "UnitCompetition"@en-gb ;
  rdfs:subClassOf <http://www.bbc.co.uk/ontologies/sport/Competition> .

<http://www.bbc.co.uk/ontologies/sport/CompetitiveSportingRole>
  a owl:Class ;
  rdfs:comment "General description of the participation of players, drivers, riders etc, in groups and organisations."@en-gb ;
  rdfs:isDefinedBy <http://www.bbc.co.uk/ontologies/sport> ;
  rdfs:label "CompetitiveSportingRole"@en-gb ;
  rdfs:subClassOf <http://purl.org/vocab/participation/schema#Role> .

<http://www.bbc.co.uk/ontologies/sport/lastRound>
  a owl:ObjectProperty ;
  rdfs:comment "Relates a multi-round competition to the last round in that competition."@en-gb ;
  rdfs:domain <http://www.bbc.co.uk/ontologies/sport/MultiRoundCompetition> ;
  rdfs:isDefinedBy <http://www.bbc.co.uk/ontologies/sport> ;
  rdfs:label "lastRound"@en-gb ;
  rdfs:range <http://www.bbc.co.uk/ontologies/sport/Round> ;
  rdfs:subPropertyOf <http://www.bbc.co.uk/ontologies/sport/hasRound> .

<http://www.bbc.co.uk/things/competition-types/european-cup> a <http://www.bbc.co.uk/ontologies/sport/CompetitionType> .
<http://www.bbc.co.uk/things/competition-types/international-group-womens> a <http://www.bbc.co.uk/ontologies/sport/CompetitionType> .
<http://www.bbc.co.uk/things/competition-types/club-league> a <http://www.bbc.co.uk/ontologies/sport/CompetitionType> .
<http://www.bbc.co.uk/things/round-types/final> a <http://www.bbc.co.uk/ontologies/sport/RoundType> .
<http://www.bbc.co.uk/things/competition-types/international-cup> a <http://www.bbc.co.uk/ontologies/sport/CompetitionType> .
<http://www.bbc.co.uk/ontologies/sport/MultiDisciplineCompetition>
  a owl:Class ;
  rdfs:comment "A competition that incorporates a number of different sports, such as the Olympics."@en-gb ;
  rdfs:isDefinedBy <http://www.bbc.co.uk/ontologies/sport> ;
  rdfs:label "MultiDisciplineCompetition"@en-gb ;
  rdfs:subClassOf <http://www.bbc.co.uk/ontologies/sport/Competition> .

<http://www.bbc.co.uk/things/competition-types/international> a <http://www.bbc.co.uk/ontologies/sport/CompetitionType> .
<http://www.bbc.co.uk/ontologies/sport/recurringCompetition>
  a owl:ObjectProperty ;
  rdfs:comment "Relates a competition to the recurring instance of that competition, for example the 2012/13 Premier League to the Premier League."@en-gb ;
  rdfs:domain <http://www.bbc.co.uk/ontologies/sport/Competition> ;
  rdfs:isDefinedBy <http://www.bbc.co.uk/ontologies/sport> ;
  rdfs:label "recurringCompetition"@en-gb ;
  rdfs:range <http://www.bbc.co.uk/ontologies/sport/RecurringCompetition> .

<http://www.bbc.co.uk/ontologies/sport/CompetesForRole>
  a owl:Class ;
  rdfs:comment "Legacy class, used for associating an athlete with the national team they competed for during the Summer Olympics. Deprecated due to improper naming."@en-gb ;
  rdfs:isDefinedBy <http://www.bbc.co.uk/ontologies/sport/2.0> ;
  rdfs:label "CompetesForRole"^^xsd:string ;
  owl:deprecated true .

<http://www.bbc.co.uk/ontologies/sport/isCompetitiveSportingOrganisationOf>
  a owl:ObjectProperty ;
  rdfs:comment "Relates a competitive sporting group to a competitive sporting organisation."@en-gb ;
  rdfs:domain <http://www.bbc.co.uk/ontologies/sport/CompetitiveSportingOrganisation> ;
  rdfs:isDefinedBy <http://www.bbc.co.uk/ontologies/sport> ;
  rdfs:label "isCompetitiveSportingOrganisationOf"@en-gb ;
  rdfs:range <http://www.bbc.co.uk/ontologies/sport/CompetitiveSportingGroup> .

<http://www.bbc.co.uk/ontologies/sport/Session>
  a owl:Class ;
  rdfs:comment "A sub-division of a competition, that must be broken up due to the duration of that competition, occurring for example in snooker or cricket."@en-gb ;
  rdfs:isDefinedBy <http://www.bbc.co.uk/ontologies/sport> ;
  rdfs:label "Session"@en-gb ;
  rdfs:subClassOf <http://www.bbc.co.uk/ontologies/sport/Competition> .

<http://www.bbc.co.uk/ontologies/sport/hasSession>
  a owl:ObjectProperty ;
  rdfs:comment "Relates a competition to a session within that competition."@en-gb ;
  rdfs:domain <http://www.bbc.co.uk/ontologies/sport/Competition> ;
  rdfs:isDefinedBy <http://www.bbc.co.uk/ontologies/sport> ;
  rdfs:label "hasSession"@en-gb ;
  rdfs:range <http://www.bbc.co.uk/ontologies/sport/Session> .

<http://www.bbc.co.uk/ontologies/sport/DivisionalCompetition>
  a owl:Class ;
  rdfs:comment "A Divisional Competition is a competition that is divided into a number of competitions. London 2012 is an example of a Divisional Competition."@en-gb ;
  rdfs:isDefinedBy <http://www.bbc.co.uk/ontologies/sport> ;
  rdfs:label "DivisionalCompetition"@en-gb ;
  rdfs:subClassOf <http://www.bbc.co.uk/ontologies/sport/Competition> .

<http://www.bbc.co.uk/ontologies/sport/eventGender>
  a owl:ObjectProperty ;
  rdfs:comment "Relates a competition to a gender class instance."@en-gb ;
  rdfs:domain <http://www.bbc.co.uk/ontologies/sport/Competition> ;
  rdfs:isDefinedBy <http://www.bbc.co.uk/ontologies/sport> ;
  rdfs:label "eventGender"@en-gb ;
  rdfs:range <http://www.bbc.co.uk/ontologies/sport/EventGender> .

<http://www.bbc.co.uk/things/competition-types/domestic> a <http://www.bbc.co.uk/ontologies/sport/CompetitionType> .
<http://www.bbc.co.uk/things/round-types/final-qualifying> a <http://www.bbc.co.uk/ontologies/sport/RoundType> .
<http://www.bbc.co.uk/ontologies/sport/SportingOrganisation>
  a owl:Class ;
  rdfs:comment "An organisation involved in Sport, for example a Football team or the UK Government Department for Culture, Media and Sport."@en-gb ;
  rdfs:isDefinedBy <http://www.bbc.co.uk/ontologies/sport> ;
  rdfs:label "SportingOrganisation"@en-gb ;
  rdfs:subClassOf foaf:Organization, <http://www.bbc.co.uk/ontologies/coreconcepts/Organisation> .

<http://www.bbc.co.uk/things/competition-types/club-cup> a <http://www.bbc.co.uk/ontologies/sport/CompetitionType> .
<http://www.bbc.co.uk/ontologies/sport/hasUnitCompetition>
  a owl:ObjectProperty ;
  rdfs:comment "Relates a round to a unit competition in that round."@en-gb ;
  rdfs:domain <http://www.bbc.co.uk/ontologies/sport/Round> ;
  rdfs:isDefinedBy <http://www.bbc.co.uk/ontologies/sport> ;
  rdfs:label "hasUnitCompetition"@en-gb ;
  rdfs:range <http://www.bbc.co.uk/ontologies/sport/UnitCompetition> .

<http://www.bbc.co.uk/things/round-types/qualifying> a <http://www.bbc.co.uk/ontologies/sport/RoundType> .
<http://www.bbc.co.uk/ontologies/sport/LeagueCompetition>
  a owl:Class ;
  rdfs:comment "A League Competition is a hierarchy of competitions or competition within such a hierarchy."@en-gb ;
  rdfs:isDefinedBy <http://www.bbc.co.uk/ontologies/sport> ;
  rdfs:label "LeagueCompetition"@en-gb ;
  rdfs:subClassOf <http://www.bbc.co.uk/ontologies/sport/MultiRoundCompetition> .

<http://www.bbc.co.uk/things/competition-types/domestic-cup-womens> a <http://www.bbc.co.uk/ontologies/sport/CompetitionType> .
<http://www.bbc.co.uk/ontologies/sport/competitionType>
  a owl:ObjectProperty ;
  rdfs:comment "Relates something, typically a competition, to an enumerated competition type."@en-gb ;
  rdfs:domain <http://www.bbc.co.uk/ontologies/sport/Competition> ;
  rdfs:isDefinedBy <http://www.bbc.co.uk/ontologies/sport> ;
  rdfs:label "competitionType"@en-gb ;
  rdfs:range <http://www.bbc.co.uk/ontologies/sport/CompetitionType> .

<http://www.bbc.co.uk/ontologies/sport/awayCompetitor>
  a owl:ObjectProperty ;
  rdfs:comment "Relates a match to one competitor, by definition or designation not the home competitor."@en-gb ;
  rdfs:domain <http://www.bbc.co.uk/ontologies/sport/Match> ;
  rdfs:isDefinedBy <http://www.bbc.co.uk/ontologies/sport> ;
  rdfs:label "awayCompetitor"@en-gb ;
  rdfs:range foaf:Agent .

<http://www.bbc.co.uk/ontologies/sport/hasGroup>
  a owl:ObjectProperty ;
  rdfs:comment "Relates a league competition to a corresponding group competition."@en-gb ;
  rdfs:domain <http://www.bbc.co.uk/ontologies/sport/LeagueCompetition> ;
  rdfs:isDefinedBy <http://www.bbc.co.uk/ontologies/sport> ;
  rdfs:label "hasGroup"@en-gb ;
  rdfs:range <http://www.bbc.co.uk/ontologies/sport/GroupCompetition> ;
  owl:inverseOf <http://www.bbc.co.uk/ontologies/sport/isGroupOf> .

<http://www.bbc.co.uk/things/event-gender/womens> a <http://www.bbc.co.uk/ontologies/sport/EventGender> .
<http://www.bbc.co.uk/ontologies/sport/firstUnitCompetition>
  a owl:ObjectProperty ;
  rdfs:comment "Relates a competition to its first unit competition."@en-gb ;
  rdfs:domain <http://www.bbc.co.uk/ontologies/sport/Competition> ;
  rdfs:isDefinedBy <http://www.bbc.co.uk/ontologies/sport> ;
  rdfs:label "firstUnitCompetition"@en-gb ;
  rdfs:range <http://www.bbc.co.uk/ontologies/sport/UnitCompetition> ;
  rdfs:subPropertyOf <http://www.bbc.co.uk/ontologies/sport/hasUnitCompetition> .

<http://www.bbc.co.uk/ontologies/sport/prevUnitCompetition>
  a owl:ObjectProperty ;
  rdfs:comment "Relates a multi-round competition to its previous unit competition."@en-gb ;
  rdfs:domain <http://www.bbc.co.uk/ontologies/sport/UnitCompetition> ;
  rdfs:isDefinedBy <http://www.bbc.co.uk/ontologies/sport> ;
  rdfs:label "prevUnitCompetition"@en-gb ;
  rdfs:range <http://www.bbc.co.uk/ontologies/sport/UnitCompetition> .

<http://www.bbc.co.uk/things/round-types/single-group> a <http://www.bbc.co.uk/ontologies/sport/RoundType> .
<http://www.bbc.co.uk/ontologies/sport/promotesTo>
  a owl:ObjectProperty ;
  rdfs:comment "Relates a competition to the next competition in a heirarchy that teams are promoted to. For example the nPower Championship promotes to the Premier League."@en-gb ;
  rdfs:domain <http://www.bbc.co.uk/ontologies/sport/Competition> ;
  rdfs:isDefinedBy <http://www.bbc.co.uk/ontologies/sport> ;
  rdfs:label "promotesTo"@en-gb ;
  rdfs:range <http://www.bbc.co.uk/ontologies/sport/Competition> ;
  owl:inverseOf <http://www.bbc.co.uk/ontologies/sport/relegatesTo> .

<http://www.bbc.co.uk/things/round-types/home-and-home> a <http://www.bbc.co.uk/ontologies/sport/RoundType> .
<http://www.bbc.co.uk/ontologies/sport/prevRound>
  a owl:ObjectProperty ;
  rdfs:comment "Relates a round in a multi-round competition to its previous round."@en-gb ;
  rdfs:domain <http://www.bbc.co.uk/ontologies/sport/Round> ;
  rdfs:isDefinedBy <http://www.bbc.co.uk/ontologies/sport> ;
  rdfs:label "prevRound"@en-gb ;
  rdfs:range <http://www.bbc.co.uk/ontologies/sport/Round> .

<http://www.bbc.co.uk/things/round-types/practice> a <http://www.bbc.co.uk/ontologies/sport/RoundType> .
<http://www.bbc.co.uk/ontologies/sport/lastStage>
  a owl:ObjectProperty ;
  rdfs:comment "Relates a stage in a multi-stage competition to its last stage."@en-gb ;
  rdfs:domain <http://www.bbc.co.uk/ontologies/sport/MultiStageCompetition> ;
  rdfs:isDefinedBy <http://www.bbc.co.uk/ontologies/sport> ;
  rdfs:label "lastStage"@en-gb ;
  rdfs:range <http://www.bbc.co.uk/ontologies/sport/Competition> ;
  rdfs:subPropertyOf <http://www.bbc.co.uk/ontologies/sport/hasStage> .

<http://www.bbc.co.uk/things/event-gender/mens> a <http://www.bbc.co.uk/ontologies/sport/EventGender> .
<http://www.bbc.co.uk/things/round-types/single> a <http://www.bbc.co.uk/ontologies/sport/RoundType> .
<http://www.bbc.co.uk/ontologies/sport/SportsDiscipline>
  a owl:Class ;
  rdfs:comment "The type of discipline a sporting event involves."@en-gb ;
  rdfs:isDefinedBy <http://www.bbc.co.uk/ontologies/sport> ;
  rdfs:label "SportsDiscipline"@en-gb .

<http://www.bbc.co.uk/ontologies/sport/nextStage>
  a owl:ObjectProperty ;
  rdfs:comment "Relates a stage in a multi-stage competition to its next stage."@en-gb ;
  rdfs:domain <http://www.bbc.co.uk/ontologies/sport/Competition> ;
  rdfs:isDefinedBy <http://www.bbc.co.uk/ontologies/sport> ;
  rdfs:label "nextStage"@en-gb ;
  rdfs:range <http://www.bbc.co.uk/ontologies/sport/Competition> .

<http://www.bbc.co.uk/things/round-types/play-off> a <http://www.bbc.co.uk/ontologies/sport/RoundType> .
<http://www.bbc.co.uk/ontologies/sport/dateOfBirth>
  a owl:AnnotationProperty, owl:DatatypeProperty ;
  rdfs:comment "Implemented because foaf has no notion of date of birth. Deprecated in favour of core:dateOfBirth."@en-gb ;
  rdfs:domain <http://www.bbc.co.uk/ontologies/sport/Person> ;
  rdfs:isDefinedBy <http://www.bbc.co.uk/ontologies/sport/2.11> ;
  rdfs:label "dateOfBirth"@en-gb ;
  rdfs:range xsd:date ;
  owl:deprecated true .

<http://www.bbc.co.uk/ontologies/sport/hasMatch>
  a owl:ObjectProperty ;
  rdfs:comment "Relates a round to a match."@en-gb ;
  rdfs:domain <http://www.bbc.co.uk/ontologies/sport/Round> ;
  rdfs:isDefinedBy <http://www.bbc.co.uk/ontologies/sport> ;
  rdfs:label "hasMatch"@en-gb ;
  rdfs:range <http://www.bbc.co.uk/ontologies/sport/Match> ;
  rdfs:subPropertyOf <http://www.bbc.co.uk/ontologies/sport/hasUnitCompetition> .

<http://www.bbc.co.uk/ontologies/sport/hasDivision>
  a owl:ObjectProperty ;
  rdfs:comment "Relates a divisional competition to a division in that competition."@en-gb ;
  rdfs:domain <http://www.bbc.co.uk/ontologies/sport/DivisionalCompetition> ;
  rdfs:isDefinedBy <http://www.bbc.co.uk/ontologies/sport> ;
  rdfs:label "hasDivision"@en-gb ;
  rdfs:range <http://www.bbc.co.uk/ontologies/sport/Competition> .

<http://www.bbc.co.uk/ontologies/sport/MultiDisciplineRecurringCompetition>
  a owl:Class ;
  rdfs:comment "A recurring sports competition the covers many sports, such as the Summer Olympics."@en-gb ;
  rdfs:isDefinedBy <http://www.bbc.co.uk/ontologies/sport> ;
  rdfs:label "MultiDisciplineRecurringCompetition"@en-gb .

<http://www.bbc.co.uk/ontologies/sport/MultiRoundCompetition>
  a owl:Class ;
  rdfs:comment "A Competition organised as a sequence of rounds, for example the Premier League or group stage of the World Cup."@en-gb ;
  rdfs:isDefinedBy <http://www.bbc.co.uk/ontologies/sport> ;
  rdfs:label "MultiRoundCompetition"@en-gb ;
  rdfs:subClassOf <http://www.bbc.co.uk/ontologies/sport/Competition> .

<http://www.bbc.co.uk/ontologies/sport/EventGender>
  a owl:Class ;
  rdfs:comment "Enumerated type, typically Male, Female or Mixed."@en-gb ;
  rdfs:isDefinedBy <http://www.bbc.co.uk/ontologies/sport> ;
  rdfs:label "EventGender"@en-gb .

<http://www.bbc.co.uk/ontologies/sport/KnockoutCompetition>
  a owl:Class ;
  rdfs:comment "A competition or stage of competition that progresses through rounds of individual fixtures whereby one team is eliminated as a result of each fixture."@en-gb ;
  rdfs:isDefinedBy <http://www.bbc.co.uk/ontologies/sport> ;
  rdfs:label "KnockoutCompetition"@en-gb ;
  rdfs:subClassOf <http://www.bbc.co.uk/ontologies/sport/MultiRoundCompetition> .

<http://www.bbc.co.uk/ontologies/sport/subDiscipline>
  a owl:ObjectProperty ;
  rdfs:comment "Relates a discipline with a child discipline, for example gymnastics with rhythmic gymnastics."@en-gb ;
  rdfs:domain <http://www.bbc.co.uk/ontologies/sport/SportsDiscipline> ;
  rdfs:isDefinedBy <http://www.bbc.co.uk/ontologies/sport> ;
  rdfs:label "subDiscipline"@en-gb ;
  rdfs:range <http://www.bbc.co.uk/ontologies/sport/SportsDiscipline> .

<http://www.bbc.co.uk/ontologies/sport/firstRound>
  a owl:ObjectProperty ;
  rdfs:comment "Relates a multi-round competition to the first round in that competition."@en-gb ;
  rdfs:domain <http://www.bbc.co.uk/ontologies/sport/MultiRoundCompetition> ;
  rdfs:isDefinedBy <http://www.bbc.co.uk/ontologies/sport> ;
  rdfs:label "firstRound"@en-gb ;
  rdfs:range <http://www.bbc.co.uk/ontologies/sport/Round> ;
  rdfs:subPropertyOf <http://www.bbc.co.uk/ontologies/sport/hasRound> .

<http://www.bbc.co.uk/ontologies/sport/isSessionOf>
  a owl:ObjectProperty ;
  rdfs:comment "Relates a session to a competition."@en-gb ;
  rdfs:domain <http://www.bbc.co.uk/ontologies/sport/Session> ;
  rdfs:isDefinedBy <http://www.bbc.co.uk/ontologies/sport> ;
  rdfs:label "isSessionOf"@en-gb ;
  rdfs:range <http://www.bbc.co.uk/ontologies/sport/Competition> ;
  owl:inverseOf <http://www.bbc.co.uk/ontologies/sport/hasSession> .

<http://www.bbc.co.uk/ontologies/sport/hasHome>
  a owl:ObjectProperty ;
  rdfs:comment "Relates a Competitive Sporting Organisation to its home ground, stadium or location."@en-gb ;
  rdfs:domain <http://www.bbc.co.uk/ontologies/sport/CompetitiveSportingOrganisation> ;
  rdfs:isDefinedBy <http://www.bbc.co.uk/ontologies/sport> ;
  rdfs:label "hasHome"@en-gb ;
  rdfs:range <http://www.bbc.co.uk/ontologies/sport/Home> .

<http://www.bbc.co.uk/ontologies/sport/nextRound>
  a owl:ObjectProperty ;
  rdfs:comment "Relates a round in a multi-round competition to its next round."@en-gb ;
  rdfs:domain <http://www.bbc.co.uk/ontologies/sport/Round> ;
  rdfs:isDefinedBy <http://www.bbc.co.uk/ontologies/sport> ;
  rdfs:label "nextRound"@en-gb ;
  rdfs:range <http://www.bbc.co.uk/ontologies/sport/Round> .

<http://www.bbc.co.uk/things/competition-types/international-group> a <http://www.bbc.co.uk/ontologies/sport/CompetitionType> .
<http://www.bbc.co.uk/ontologies/sport/hasCompetedFor>
  a owl:ObjectProperty ;
  rdfs:comment "Associates an agent with sporting organisations non-temporally."@en-gb ;
  rdfs:domain foaf:Agent ;
  rdfs:isDefinedBy <http://www.bbc.co.uk/ontologies/sport> ;
  rdfs:label "hasCompetedFor"@en-gb ;
  rdfs:range <http://www.bbc.co.uk/ontologies/sport/SportingOrganisation> .

<http://www.bbc.co.uk/ontologies/sport/homeCompetitor>
  a owl:ObjectProperty ;
  rdfs:comment "Relates a match to one competitor, by definition or designation not the away competitor."@en-gb ;
  rdfs:domain <http://www.bbc.co.uk/ontologies/sport/Match> ;
  rdfs:isDefinedBy <http://www.bbc.co.uk/ontologies/sport> ;
  rdfs:label "homeCompetitor"@en-gb ;
  rdfs:range foaf:Agent ;
  rdfs:subPropertyOf <http://www.bbc.co.uk/ontologies/sport/hasCompetitor> .

<http://www.bbc.co.uk/ontologies/sport/nextSession>
  a owl:ObjectProperty ;
  rdfs:comment "Relates a session to its next session."@en-gb ;
  rdfs:domain <http://www.bbc.co.uk/ontologies/sport/Session> ;
  rdfs:isDefinedBy <http://www.bbc.co.uk/ontologies/sport> ;
  rdfs:label "nextSession"@en-gb ;
  rdfs:range <http://www.bbc.co.uk/ontologies/sport/Session> .

<http://www.bbc.co.uk/ontologies/sport/roundNumber>
  a owl:DatatypeProperty ;
  rdfs:comment "Indicates the sequential number of a round."@en-gb ;
  rdfs:domain <http://www.bbc.co.uk/ontologies/sport/Round> ;
  rdfs:isDefinedBy <http://www.bbc.co.uk/ontologies/sport> ;
  rdfs:label "roundNumber"@en-gb ;
  rdfs:range xsd:int .

<http://www.bbc.co.uk/ontologies/sport/firstSession>
  a owl:ObjectProperty ;
  rdfs:comment "Relates a competition to the first session of a series of sessions."@en-gb ;
  rdfs:domain <http://www.bbc.co.uk/ontologies/sport/Competition> ;
  rdfs:isDefinedBy <http://www.bbc.co.uk/ontologies/sport> ;
  rdfs:label "firstSession"@en-gb ;
  rdfs:range <http://www.bbc.co.uk/ontologies/sport/Session> ;
  rdfs:subPropertyOf <http://www.bbc.co.uk/ontologies/sport/hasSession> .

<http://www.bbc.co.uk/things/competition-types/international-groupcup-womens> a <http://www.bbc.co.uk/ontologies/sport/CompetitionType> .
<http://www.bbc.co.uk/ontologies/sport/RecurringCompetition>
  a owl:Class ;
  rdfs:comment "A recurring sports competition such as the Rugby Super League."@en-gb ;
  rdfs:isDefinedBy <http://www.bbc.co.uk/ontologies/sport> ;
  rdfs:label "RecurringCompetition"@en-gb .

<http://www.bbc.co.uk/ontologies/sport/RoundType>
  a owl:Class ;
  rdfs:comment "Enumerated round types, for example: preliminary, qualifying or final."@en-gb ;
  rdfs:isDefinedBy <http://www.bbc.co.uk/ontologies/sport> ;
  rdfs:label "RoundType"@en-gb .

<http://www.bbc.co.uk/ontologies/sport/discipline>
  a owl:ObjectProperty ;
  rdfs:comment "Relates something to a sporting discipline, for example a person to athletics."@en-gb ;
  rdfs:isDefinedBy <http://www.bbc.co.uk/ontologies/sport> ;
  rdfs:label "discipline"@en-gb ;
  rdfs:range <http://www.bbc.co.uk/ontologies/sport/SportsDiscipline> .

<http://www.bbc.co.uk/ontologies/sport/isStageOf>
  a owl:ObjectProperty ;
  rdfs:comment "Relates a stage to a multi-stage competition."@en-gb ;
  rdfs:domain <http://www.bbc.co.uk/ontologies/sport/Competition> ;
  rdfs:isDefinedBy <http://www.bbc.co.uk/ontologies/sport> ;
  rdfs:label "isStageOf"@en-gb ;
  rdfs:range <http://www.bbc.co.uk/ontologies/sport/MultiStageCompetition> ;
  owl:inverseOf <http://www.bbc.co.uk/ontologies/sport/hasStage> .

<http://www.bbc.co.uk/things/round-types/single-elimination> a <http://www.bbc.co.uk/ontologies/sport/RoundType> .