@prefix owl: <http://www.w3.org/2002/07/owl#> .
@prefix rdfs: <http://www.w3.org/2000/01/rdf-schema#> .
@prefix cc: <http://creativecommons.org/ns#> .
@prefix dc: <http://purl.org/dc/terms/> .
@prefix xsd: <http://www.w3.org/2001/XMLSchema#> .
@prefix ns0: <http://purl.org/vocab/vann/> .
@prefix prov: <http://www.w3.org/ns/prov#> .
@prefix skos: <http://www.w3.org/2004/02/skos/core#> .

<http://purl.org/xapi/ontology#>
  a owl:Ontology ;
  rdfs:label "xAPI Controlled Vocabulary Ontology"@en ;
  cc:license <http://creativecommons.org/licenses/by/3.0/> ;
  dc:created "2015-04-27"^^xsd:date ;
  dc:modified "2015-08-13"^^xsd:date ;
  ns0:preferredNamespacePrefix "xapi" ;
  ns0:preferredNamespaceUri "http://purl.org/xapi/ontology#" ;
  rdfs:comment "This ontology contains a list of the classes and properties that can be used when for creating and publishing a controlled vocabulary dataset for xAPI communities of practice."@en ;
  prov:wasAttributedTo <https://www.w3.org/community/xapivocabulary> .

<http://purl.org/xapi/ontology#ActivityType>
  a owl:Class ;
  rdfs:label "ActivityType"@en ;
  rdfs:comment "The Activity Type is the identifier of the Activity Definition in an xAPI statement and when dereferenced can provide more information (metadata) about the activity type."@en ;
  rdfs:subClassOf skos:Concept .

<http://purl.org/xapi/ontology#Statement>
  a owl:Class ;
  rdfs:label "Statement"@en ;
  rdfs:comment "The class for xAPI Statements, mainly for use with Statements in vocabulary examples."@en ;
  rdfs:subClassOf skos:Concept .

<http://purl.org/xapi/ontology#Verb>
  a owl:Class ;
  rdfs:label "Verb"@en ;
  rdfs:comment "The Class for a Verb in a controlled vocabulary."@en ;
  rdfs:subClassOf skos:Concept .

<http://purl.org/xapi/ontology#closelyRelatedNaturalLanguageTerm>
  a owl:ObjectProperty ;
  rdfs:label "closelyRelatedNaturalLanguageTerm"@en ;
  rdfs:comment "A property used to connect the xAPI term to a specific sense, or meaning, in natural language that is very closely related. The sense will be identified with Wordnet, a carefully constructed ontology that aids in word sense disambiguation, which has been used with many different languages."@en ;
  rdfs:domain skos:Concept ;
  rdfs:range <http://wordnet-rdf.princeton.edu/ontology#Synset> ;
  rdfs:subPropertyOf skos:relatedMatch .

<http://purl.org/xapi/ontology#referenced>
  a owl:ObjectProperty ;
  rdfs:label "referenced"@en ;
  rdfs:comment "A property used to connects an xapi:Verb or other xAPI term not directly maintained by the vocabulary author to the skos:ConceptScheme that is the xAPI vocabulary referencing the term."@en ;
  rdfs:subPropertyOf skos:inScheme .

<http://purl.org/xapi/ontology#thirdPartyLabel>
  a owl:AnnotationProperty ;
  rdfs:label "thirdPartyLabel"@en ;
  rdfs:comment "A property used by people who did not create the original verb, but would like to offer an alternative label for it."@en ;
  rdfs:subPropertyOf skos:altLabel .