@prefix dc: <http://purl.org/dc/elements/1.1/> .
@prefix rdfs: <http://www.w3.org/2000/01/rdf-schema#> .
@prefix foaf: <http://xmlns.com/foaf/0.1/> .
@prefix status: <http://metadataregistry.org/uri/RegStatus/> .
@prefix reg: <http://metadataregistry.org/uri/profile/RegAp/> .
@prefix dct: <http://purl.org/dc/terms/> .
@prefix owl: <http://www.w3.org/2002/07/owl#> .
@prefix rdf: <http://www.w3.org/1999/02/22-rdf-syntax-ns#> .
@prefix skos: <http://www.w3.org/2004/02/skos/core#> .

status:1001 a skos:Concept ;
	skos:prefLabel "Published"@en .

status:1008 a skos:Concept ;
	skos:prefLabel "Deprecated"@en .

<http://rdaregistry.info/Elements/u/> dc:title "RDA Unconstrained properties"@en ;
	skos:note "Properties derived from RDA elements and relationship designators without specific or implicit restrictions to RDA entities."@en .

<http://rdaregistry.info/Elements/u/P60001> reg:name "respondentOf"@en ;
	reg:status status:1001 ;
	a rdf:Property ;
	rdfs:isDefinedBy <http://rdaregistry.info/Elements/u/> ;
	rdfs:label "is respondent of"@en ;
	rdfs:subPropertyOf <http://rdaregistry.info/Elements/u/P60672> ;
	owl:inverseOf <http://rdaregistry.info/Elements/u/P60045> ;
	owl:sameAs <http://rdaregistry.info/Elements/u/respondentOf> ;
	skos:definition "Relates a candidate for a degree who defends or opposes a thesis provided by the praeses in an academic disputation to the resource."@en .

<http://rdaregistry.info/Elements/u/P60002> reg:name "degreeGrantingInstitutionOf"@en ;
	reg:status status:1001 ;
	a rdf:Property ;
	rdfs:isDefinedBy <http://rdaregistry.info/Elements/u/> ;
	rdfs:label "is degree granting institution of"@en ;
	rdfs:subPropertyOf <http://rdaregistry.info/Elements/u/P60602> ;
	owl:inverseOf <http://rdaregistry.info/Elements/u/P60060> ;
	owl:sameAs <http://rdaregistry.info/Elements/u/degreeGrantingInstitutionOf> ;
	skos:definition "Relates a corporate body granting an academic degree to the resource."@en .

<http://rdaregistry.info/Elements/u/P60003> reg:name "hostInstitutionOf"@en ;
	reg:status status:1001 ;
	a rdf:Property ;
	rdfs:isDefinedBy <http://rdaregistry.info/Elements/u/> ;
	rdfs:label "is host institution of"@en ;
	rdfs:subPropertyOf <http://rdaregistry.info/Elements/u/P60602> ;
	owl:inverseOf <http://rdaregistry.info/Elements/u/P60061> ;
	owl:sameAs <http://rdaregistry.info/Elements/u/hostInstitutionOf> ;
	skos:definition "Relates a corporate body hosting the event, exhibit, conference, etc., which gave rise to a resource, but having little or no responsibility for the content of the resource to the resource."@en .

<http://rdaregistry.info/Elements/u/P60004> reg:name "productionCompanyOf"@en ;
	reg:status status:1001 ;
	a rdf:Property ;
	rdfs:isDefinedBy <http://rdaregistry.info/Elements/u/> ;
	rdfs:label "is production company of"@en ;
	rdfs:subPropertyOf <http://rdaregistry.info/Elements/u/P60602> ;
	owl:inverseOf <http://rdaregistry.info/Elements/u/P60062> ;
	owl:sameAs <http://rdaregistry.info/Elements/u/productionCompanyOf> ;
	skos:definition "Relates a corporate body that is responsible for financial, technical, and organizational management of a production for stage, screen, sound recording, television, webcast, etc. to the resource."@en .

<http://rdaregistry.info/Elements/u/P60005> reg:hasSubproperty <http://rdaregistry.info/Elements/a/P50044> ;
	reg:name "courtGovernedOf"@en ;
	reg:status status:1001 ;
	a rdf:Property ;
	rdfs:isDefinedBy <http://rdaregistry.info/Elements/u/> ;
	rdfs:label "is court governed of"@en ;
	rdfs:subPropertyOf <http://rdaregistry.info/Elements/u/P60602> ;
	owl:inverseOf <http://rdaregistry.info/Elements/u/P60065> ;
	owl:sameAs <http://rdaregistry.info/Elements/u/courtGovernedOf> ;
	skos:definition "Relates a court governed by court rules, regardless of their official nature (e.g., laws, administrative regulations) to the resource."@en .

<http://rdaregistry.info/Elements/u/P60006> reg:hasSubproperty <http://rdaregistry.info/Elements/a/P50045> ;
	reg:name "collectorOf"@en ;
	reg:status status:1001 ;
	a rdf:Property ;
	rdfs:isDefinedBy <http://rdaregistry.info/Elements/u/> ;
	rdfs:label "is collector of"@en ;
	rdfs:subPropertyOf <http://rdaregistry.info/Elements/u/P60604> ;
	owl:inverseOf <http://rdaregistry.info/Elements/u/P60066> ;
	owl:sameAs <http://rdaregistry.info/Elements/u/collectorOf> ;
	skos:definition "Relates a curator who brings together resources from various sources that are then arranged, described, and cataloged as a collection to the resource."@en .

<http://rdaregistry.info/Elements/u/P60007> reg:hasSubproperty <http://rdaregistry.info/Elements/a/P50046> ;
	reg:name "collectionRegistrarOf"@en ;
	reg:status status:1001 ;
	a rdf:Property ;
	rdfs:isDefinedBy <http://rdaregistry.info/Elements/u/> ;
	rdfs:label "is collection registrar of"@en ;
	rdfs:subPropertyOf <http://rdaregistry.info/Elements/u/P60604> ;
	owl:inverseOf <http://rdaregistry.info/Elements/u/P60067> ;
	owl:sameAs <http://rdaregistry.info/Elements/u/collectionRegistrarOf> ;
	skos:definition "Relates a curator who lists or inventories the items in an aggregate resource such as a collection of items or resources to the resource."@en .

<http://rdaregistry.info/Elements/u/P60008> reg:hasSubproperty <http://rdaregistry.info/Elements/a/P50047> ;
	reg:name "depositorOf"@en ;
	reg:status status:1001 ;
	a rdf:Property ;
	rdfs:isDefinedBy <http://rdaregistry.info/Elements/u/> ;
	rdfs:label "is depositor of"@en ;
	rdfs:subPropertyOf <http://rdaregistry.info/Elements/u/P60628> ;
	owl:inverseOf <http://rdaregistry.info/Elements/u/P60068> ;
	owl:sameAs <http://rdaregistry.info/Elements/u/depositorOf> ;
	skos:definition "Relates a current owner of a resource who deposited the resource into the custody of another person, family, or corporate body, while still retaining ownership to the resource."@en .

<http://rdaregistry.info/Elements/u/P60009> reg:hasSubproperty <http://rdaregistry.info/Elements/a/P50048> ;
	reg:name "filmDirectorOf"@en ;
	reg:status status:1001 ;
	a rdf:Property ;
	rdfs:isDefinedBy <http://rdaregistry.info/Elements/u/> ;
	rdfs:label "is film director of"@en ;
	rdfs:subPropertyOf <http://rdaregistry.info/Elements/u/P60673> ;
	owl:inverseOf <http://rdaregistry.info/Elements/u/P60084> ;
	owl:sameAs <http://rdaregistry.info/Elements/u/filmDirectorOf> ;
	skos:definition "Relates a director responsible for the general management and supervision of a filmed performance to the resource."@en .

<http://rdaregistry.info/Elements/u/P60010> reg:hasSubproperty <http://rdaregistry.info/Elements/a/P50049> ;
	reg:name "radioDirectorOf"@en ;
	reg:status status:1001 ;
	a rdf:Property ;
	rdfs:isDefinedBy <http://rdaregistry.info/Elements/u/> ;
	rdfs:label "is radio director of"@en ;
	rdfs:subPropertyOf <http://rdaregistry.info/Elements/u/P60673> ;
	owl:inverseOf <http://rdaregistry.info/Elements/u/P60085> ;
	owl:sameAs <http://rdaregistry.info/Elements/u/radioDirectorOf> ;
	skos:definition "Relates a director responsible for the general management and supervision of a radio program to the resource."@en .

<http://rdaregistry.info/Elements/u/P60011> reg:hasSubproperty <http://rdaregistry.info/Elements/a/P50050> ;
	reg:name "televisionDirectorOf"@en ;
	reg:status status:1001 ;
	a rdf:Property ;
	rdfs:isDefinedBy <http://rdaregistry.info/Elements/u/> ;
	rdfs:label "is television director of"@en ;
	rdfs:subPropertyOf <http://rdaregistry.info/Elements/u/P60673> ;
	owl:inverseOf <http://rdaregistry.info/Elements/u/P60086> ;
	owl:sameAs <http://rdaregistry.info/Elements/u/televisionDirectorOf> ;
	skos:definition "Relates a director responsible for the general management and supervision of a television program to the resource."@en .

<http://rdaregistry.info/Elements/u/P60012> reg:hasSubproperty <http://rdaregistry.info/Elements/a/P50066> ;
	reg:name "donorOf"@en ;
	reg:status status:1001 ;
	a rdf:Property ;
	rdfs:isDefinedBy <http://rdaregistry.info/Elements/u/> ;
	rdfs:label "is donor of"@en ;
	rdfs:subPropertyOf <http://rdaregistry.info/Elements/u/P60630> ;
	owl:inverseOf <http://rdaregistry.info/Elements/u/P60091> ;
	owl:sameAs <http://rdaregistry.info/Elements/u/donorOf> ;
	skos:definition "Relates a former owner of a resource who donated that resource to another owner to the resource."@en .

<http://rdaregistry.info/Elements/u/P60013> reg:hasSubproperty <http://rdaregistry.info/Elements/a/P50067> ;
	reg:name "sellerOf"@en ;
	reg:status status:1001 ;
	a rdf:Property ;
	rdfs:isDefinedBy <http://rdaregistry.info/Elements/u/> ;
	rdfs:label "is seller of"@en ;
	rdfs:subPropertyOf <http://rdaregistry.info/Elements/u/P60630> ;
	owl:inverseOf <http://rdaregistry.info/Elements/u/P60092> ;
	owl:sameAs <http://rdaregistry.info/Elements/u/sellerOf> ;
	skos:definition "Relates a former owner of a resource who sold that resource to another owner to the resource."@en .

<http://rdaregistry.info/Elements/u/P60014> reg:hasSubproperty <http://rdaregistry.info/Elements/a/P50068> ;
	reg:name "enactingJurisdictionOf"@en ;
	reg:status status:1001 ;
	a rdf:Property ;
	rdfs:isDefinedBy <http://rdaregistry.info/Elements/u/> ;
	rdfs:label "is enacting jurisdiction of"@en ;
	rdfs:subPropertyOf <http://rdaregistry.info/Elements/u/P60672> ;
	owl:inverseOf <http://rdaregistry.info/Elements/u/P60096> ;
	owl:sameAs <http://rdaregistry.info/Elements/u/enactingJurisdictionOf> ;
	skos:definition "Relates a jurisdiction enacting a law, regulation, constitution, court rule, etc. to the resource."@en .

<http://rdaregistry.info/Elements/u/P60015> reg:hasSubproperty <http://rdaregistry.info/Elements/a/P50069> ;
	reg:name "jurisdictionGovernedOf"@en ;
	reg:status status:1001 ;
	a rdf:Property ;
	rdfs:isDefinedBy <http://rdaregistry.info/Elements/u/> ;
	rdfs:label "is jurisdiction governed of"@en ;
	rdfs:subPropertyOf <http://rdaregistry.info/Elements/u/P60602> ;
	owl:inverseOf <http://rdaregistry.info/Elements/u/P60097> ;
	owl:sameAs <http://rdaregistry.info/Elements/u/jurisdictionGovernedOf> ;
	skos:definition "Relates a jurisdiction governed by a law, regulation, etc., that was enacted by another jurisdiction to the resource."@en .

<http://rdaregistry.info/Elements/u/P60016> reg:hasSubproperty <http://rdaregistry.info/Elements/a/P50070> ;
	reg:name "conductorOf"@en ;
	reg:status status:1001 ;
	a rdf:Property ;
	rdfs:isDefinedBy <http://rdaregistry.info/Elements/u/> ;
	rdfs:label "is conductor of"@en ;
	rdfs:subPropertyOf <http://rdaregistry.info/Elements/u/P60615> ;
	owl:inverseOf <http://rdaregistry.info/Elements/u/P60141> ;
	owl:sameAs <http://rdaregistry.info/Elements/u/conductorOf> ;
	skos:definition "Relates a performer contributing to a musical resource by leading a performing group (orchestra, chorus, opera, etc.) in a musical or dramatic presentation, etc. to the resource."@en .

<http://rdaregistry.info/Elements/u/P60017> reg:hasSubproperty <http://rdaregistry.info/Elements/a/P50071> , <http://rdaregistry.info/Elements/u/P60027> ;
	reg:name "actorOf"@en ;
	reg:status status:1001 ;
	a rdf:Property ;
	rdfs:isDefinedBy <http://rdaregistry.info/Elements/u/> ;
	rdfs:label "is actor of"@en ;
	rdfs:subPropertyOf <http://rdaregistry.info/Elements/u/P60615> ;
	owl:inverseOf <http://rdaregistry.info/Elements/u/P60142> ;
	owl:sameAs <http://rdaregistry.info/Elements/u/actorOf> ;
	skos:definition "Relates a performer contributing to a resource by acting as a cast member or player in a musical or dramatic presentation, etc. to the resource."@en .

<http://rdaregistry.info/Elements/u/P60018> reg:hasSubproperty <http://rdaregistry.info/Elements/a/P50072> ;
	reg:name "onScreenPresenterOf"@en ;
	reg:status status:1001 ;
	a rdf:Property ;
	rdfs:isDefinedBy <http://rdaregistry.info/Elements/u/> ;
	rdfs:label "is on-screen presenter of"@en ;
	rdfs:subPropertyOf <http://rdaregistry.info/Elements/u/P60615> ;
	owl:inverseOf <http://rdaregistry.info/Elements/u/P60143> ;
	owl:sameAs <http://rdaregistry.info/Elements/u/onScreenPresenterOf> ;
	skos:definition "Relates a performer contributing to a resource by appearing on screen to provide contextual or background information. an on-screen presenter may appear in nonfiction moving image materials or in introductions to fiction moving image materials to the resource."@en .

<http://rdaregistry.info/Elements/u/P60019> reg:hasSubproperty <http://rdaregistry.info/Elements/a/P50073> ;
	reg:name "dancerOf"@en ;
	reg:status status:1001 ;
	a rdf:Property ;
	rdfs:isDefinedBy <http://rdaregistry.info/Elements/u/> ;
	rdfs:label "is dancer of"@en ;
	rdfs:subPropertyOf <http://rdaregistry.info/Elements/u/P60615> ;
	owl:inverseOf <http://rdaregistry.info/Elements/u/P60144> ;
	owl:sameAs <http://rdaregistry.info/Elements/u/dancerOf> ;
	skos:definition "Relates a performer contributing to a resource by dancing in a musical, dramatic, etc., presentation to the resource."@en .

<http://rdaregistry.info/Elements/u/P60020> reg:hasSubproperty <http://rdaregistry.info/Elements/a/P50074> ;
	reg:name "teacherOf"@en ;
	reg:status status:1001 ;
	a rdf:Property ;
	rdfs:isDefinedBy <http://rdaregistry.info/Elements/u/> ;
	rdfs:label "is teacher of"@en ;
	rdfs:subPropertyOf <http://rdaregistry.info/Elements/u/P60615> ;
	owl:inverseOf <http://rdaregistry.info/Elements/u/P60145> ;
	owl:sameAs <http://rdaregistry.info/Elements/u/teacherOf> ;
	skos:definition "Relates a performer contributing to a resource by giving instruction or providing a demonstration to the resource."@en .

<http://rdaregistry.info/Elements/u/P60021> reg:hasSubproperty <http://rdaregistry.info/Elements/a/P50075> ;
	reg:name "hostOf"@en ;
	reg:status status:1001 ;
	a rdf:Property ;
	rdfs:isDefinedBy <http://rdaregistry.info/Elements/u/> ;
	rdfs:label "is host of"@en ;
	rdfs:subPropertyOf <http://rdaregistry.info/Elements/u/P60615> ;
	owl:inverseOf <http://rdaregistry.info/Elements/u/P60146> ;
	owl:sameAs <http://rdaregistry.info/Elements/u/hostOf> ;
	skos:definition "Relates a performer contributing to a resource by leading a program (often broadcast) that includes other guests, performers, etc. (e.g., talk show host) to the resource."@en .

<http://rdaregistry.info/Elements/u/P60022> reg:hasSubproperty <http://rdaregistry.info/Elements/a/P50076> ;
	reg:name "moderatorOf"@en ;
	reg:status status:1001 ;
	a rdf:Property ;
	rdfs:isDefinedBy <http://rdaregistry.info/Elements/u/> ;
	rdfs:label "is moderator of"@en ;
	rdfs:subPropertyOf <http://rdaregistry.info/Elements/u/P60615> ;
	owl:inverseOf <http://rdaregistry.info/Elements/u/P60147> ;
	owl:sameAs <http://rdaregistry.info/Elements/u/moderatorOf> ;
	skos:definition "Relates a performer contributing to a resource by leading a program (often broadcast) where topics are discussed, usually with participation of experts in fields related to the discussion to the resource."@en .

<http://rdaregistry.info/Elements/u/P60023> reg:hasSubproperty <http://rdaregistry.info/Elements/a/P50077> ;
	reg:name "puppeteerOf"@en ;
	reg:status status:1001 ;
	a rdf:Property ;
	rdfs:isDefinedBy <http://rdaregistry.info/Elements/u/> ;
	rdfs:label "is puppeteer of"@en ;
	rdfs:subPropertyOf <http://rdaregistry.info/Elements/u/P60615> ;
	owl:inverseOf <http://rdaregistry.info/Elements/u/P60148> ;
	owl:sameAs <http://rdaregistry.info/Elements/u/puppeteerOf> ;
	skos:definition "Relates a performer contributing to a resource by manipulating, controlling, or directing puppets or marionettes in a moving image production or a musical or dramatic presentation or entertainment to the resource."@en .

<http://rdaregistry.info/Elements/u/P60024> reg:hasSubproperty <http://rdaregistry.info/Elements/a/P50078> ;
	reg:name "panelistOf"@en ;
	reg:status status:1001 ;
	a rdf:Property ;
	rdfs:isDefinedBy <http://rdaregistry.info/Elements/u/> ;
	rdfs:label "is panelist of"@en ;
	rdfs:subPropertyOf <http://rdaregistry.info/Elements/u/P60615> ;
	owl:inverseOf <http://rdaregistry.info/Elements/u/P60149> ;
	owl:sameAs <http://rdaregistry.info/Elements/u/panelistOf> ;
	skos:definition "Relates a performer contributing to a resource by participating in a program (often broadcast) where topics are discussed, usually with participation of experts in fields related to the discussion to the resource."@en .

<http://rdaregistry.info/Elements/u/P60025> reg:hasSubproperty <http://rdaregistry.info/Elements/a/P50079> ;
	reg:name "instrumentalistOf"@en ;
	reg:status status:1001 ;
	a rdf:Property ;
	rdfs:isDefinedBy <http://rdaregistry.info/Elements/u/> ;
	rdfs:label "is instrumentalist of"@en ;
	rdfs:subPropertyOf <http://rdaregistry.info/Elements/u/P60615> ;
	owl:inverseOf <http://rdaregistry.info/Elements/u/P60150> ;
	owl:sameAs <http://rdaregistry.info/Elements/u/instrumentalistOf> ;
	skos:definition "Relates a performer contributing to a resource by playing a musical instrument to the resource."@en .

<http://rdaregistry.info/Elements/u/P60026> reg:hasSubproperty <http://rdaregistry.info/Elements/a/P50080> ;
	reg:name "commentatorOf"@en ;
	reg:status status:1001 ;
	a rdf:Property ;
	rdfs:isDefinedBy <http://rdaregistry.info/Elements/u/> ;
	rdfs:label "is commentator of"@en ;
	rdfs:subPropertyOf <http://rdaregistry.info/Elements/u/P60615> ;
	owl:inverseOf <http://rdaregistry.info/Elements/u/P60151> ;
	owl:sameAs <http://rdaregistry.info/Elements/u/commentatorOf> ;
	skos:definition "Relates a performer contributing to a resource by providing interpretation, analysis, or a discussion of the subject matter on a recording, film, or other audiovisual medium to the resource."@en .

<http://rdaregistry.info/Elements/u/P60027> reg:hasSubproperty <http://rdaregistry.info/Elements/a/P50217> ;
	reg:name "voiceActorOf"@en ;
	reg:status status:1001 ;
	a rdf:Property ;
	rdfs:isDefinedBy <http://rdaregistry.info/Elements/u/> ;
	rdfs:label "is voice actor of"@en ;
	rdfs:subPropertyOf <http://rdaregistry.info/Elements/u/P60017> ;
	owl:inverseOf <http://rdaregistry.info/Elements/u/P60152> ;
	owl:sameAs <http://rdaregistry.info/Elements/u/voiceActorOf> ;
	skos:definition "Relates a performer contributing to a resource by providing the voice for characters in radio and audio productions and for animated characters in moving image resources as well as by providing voice-overs in radio and television commercials, dubbed resources, etc. to the resource."@en .

<http://rdaregistry.info/Elements/u/P60028> reg:hasSubproperty <http://rdaregistry.info/Elements/a/P50081> ;
	reg:name "narratorOf"@en ;
	reg:status status:1001 ;
	a rdf:Property ;
	rdfs:isDefinedBy <http://rdaregistry.info/Elements/u/> ;
	rdfs:label "is narrator of"@en ;
	rdfs:subPropertyOf <http://rdaregistry.info/Elements/u/P60615> ;
	owl:inverseOf <http://rdaregistry.info/Elements/u/P60153> ;
	owl:sameAs <http://rdaregistry.info/Elements/u/narratorOf> ;
	skos:definition "Relates a performer contributing to a resource by reading or speaking in order to give an account of an act, occurrence, course of events, etc. to the resource."@en .

<http://rdaregistry.info/Elements/u/P60029> reg:hasSubproperty <http://rdaregistry.info/Elements/a/P50082> ;
	reg:name "storytellerOf"@en ;
	reg:status status:1001 ;
	a rdf:Property ;
	rdfs:isDefinedBy <http://rdaregistry.info/Elements/u/> ;
	rdfs:label "is storyteller of"@en ;
	rdfs:subPropertyOf <http://rdaregistry.info/Elements/u/P60615> ;
	owl:inverseOf <http://rdaregistry.info/Elements/u/P60154> ;
	owl:sameAs <http://rdaregistry.info/Elements/u/storytellerOf> ;
	skos:definition "Relates a performer contributing to a resource by relaying a creator’s original story with dramatic or theatrical interpretation to the resource."@en .

<http://rdaregistry.info/Elements/u/P60030> reg:hasSubproperty <http://rdaregistry.info/Elements/a/P50083> ;
	reg:name "speakerOf"@en ;
	reg:status status:1001 ;
	a rdf:Property ;
	rdfs:isDefinedBy <http://rdaregistry.info/Elements/u/> ;
	rdfs:label "is speaker of"@en ;
	rdfs:subPropertyOf <http://rdaregistry.info/Elements/u/P60615> ;
	owl:inverseOf <http://rdaregistry.info/Elements/u/P60155> ;
	owl:sameAs <http://rdaregistry.info/Elements/u/speakerOf> ;
	skos:definition "Relates a performer contributing to a resource by speaking words, such as a lecture, speech, etc. to the resource."@en .

<http://rdaregistry.info/Elements/u/P60031> reg:hasSubproperty <http://rdaregistry.info/Elements/a/P50084> ;
	reg:name "singerOf"@en ;
	reg:status status:1001 ;
	a rdf:Property ;
	rdfs:isDefinedBy <http://rdaregistry.info/Elements/u/> ;
	rdfs:label "is singer of"@en ;
	rdfs:subPropertyOf <http://rdaregistry.info/Elements/u/P60615> ;
	owl:inverseOf <http://rdaregistry.info/Elements/u/P60156> ;
	owl:sameAs <http://rdaregistry.info/Elements/u/singerOf> ;
	skos:definition "Relates a performer contributing to a resource by using his/her/their voice, with or without instrumental accompaniment, to produce music. a singer’s performance may or may not include actual words to the resource."@en .

<http://rdaregistry.info/Elements/u/P60032> reg:hasSubproperty <http://rdaregistry.info/Elements/a/P50086> ;
	reg:name "mediumOf"@en ;
	reg:status status:1001 ;
	a rdf:Property ;
	rdfs:isDefinedBy <http://rdaregistry.info/Elements/u/> ;
	rdfs:label "is medium of"@en ;
	rdfs:subPropertyOf <http://rdaregistry.info/Elements/u/P60602> ;
	owl:inverseOf <http://rdaregistry.info/Elements/u/P60157> ;
	owl:sameAs <http://rdaregistry.info/Elements/u/mediumOf> ;
	skos:definition "Relates a person held to be a channel of communication between the earthly world and a world of spirits to the resource."@en .

<http://rdaregistry.info/Elements/u/P60033> reg:hasSubproperty <http://rdaregistry.info/Elements/a/P50213> ;
	reg:name "filmProducerOf"@en ;
	reg:status status:1001 ;
	a rdf:Property ;
	rdfs:isDefinedBy <http://rdaregistry.info/Elements/u/> ;
	rdfs:label "is film producer of"@en ;
	rdfs:subPropertyOf <http://rdaregistry.info/Elements/u/P60668> ;
	owl:inverseOf <http://rdaregistry.info/Elements/u/P60169> ;
	owl:sameAs <http://rdaregistry.info/Elements/u/filmProducerOf> ;
	skos:definition "Relates a producer responsible for most of the business aspects of a film to the resource."@en .

<http://rdaregistry.info/Elements/u/P60034> reg:hasSubproperty <http://rdaregistry.info/Elements/a/P50214> ;
	reg:name "radioProducerOf"@en ;
	reg:status status:1001 ;
	a rdf:Property ;
	rdfs:isDefinedBy <http://rdaregistry.info/Elements/u/> ;
	rdfs:label "is radio producer of"@en ;
	rdfs:subPropertyOf <http://rdaregistry.info/Elements/u/P60668> ;
	owl:inverseOf <http://rdaregistry.info/Elements/u/P60170> ;
	owl:sameAs <http://rdaregistry.info/Elements/u/radioProducerOf> ;
	skos:definition "Relates a producer responsible for most of the business aspects of a radio program to the resource."@en .

<http://rdaregistry.info/Elements/u/P60035> reg:hasSubproperty <http://rdaregistry.info/Elements/a/P50215> ;
	reg:name "televisionProducerOf"@en ;
	reg:status status:1001 ;
	a rdf:Property ;
	rdfs:isDefinedBy <http://rdaregistry.info/Elements/u/> ;
	rdfs:label "is television producer of"@en ;
	rdfs:subPropertyOf <http://rdaregistry.info/Elements/u/P60668> ;
	owl:inverseOf <http://rdaregistry.info/Elements/u/P60171> ;
	owl:sameAs <http://rdaregistry.info/Elements/u/televisionProducerOf> ;
	skos:definition "Relates a producer responsible for most of the business aspects of a television program to the resource."@en .

<http://rdaregistry.info/Elements/u/P60036> reg:hasSubproperty <http://rdaregistry.info/Elements/a/P50105> ;
	reg:name "alternateIdentity"@en ;
	reg:status status:1001 ;
	a rdf:Property ;
	rdfs:isDefinedBy <http://rdaregistry.info/Elements/u/> ;
	rdfs:label "has alternate identity"@en ;
	owl:inverseOf <http://rdaregistry.info/Elements/u/P60037> ;
	owl:sameAs <http://rdaregistry.info/Elements/u/alternateIdentity> ;
	skos:definition "Relates a pseudonymous or other identity assumed by the agent to the agent."@en .

<http://rdaregistry.info/Elements/u/P60037> reg:hasSubproperty <http://rdaregistry.info/Elements/a/P50106> ;
	reg:name "realIdentity"@en ;
	reg:status status:1001 ;
	a rdf:Property ;
	rdfs:isDefinedBy <http://rdaregistry.info/Elements/u/> ;
	rdfs:label "has real identity"@en ;
	owl:inverseOf <http://rdaregistry.info/Elements/u/P60036> ;
	owl:sameAs <http://rdaregistry.info/Elements/u/realIdentity> ;
	skos:definition "Relates a real agent who assumes the alternate identity to the agent."@en .

<http://rdaregistry.info/Elements/u/P60045> reg:hasSubproperty <http://rdaregistry.info/Elements/w/P10001> ;
	reg:name "respondent"@en ;
	reg:status status:1001 ;
	a rdf:Property ;
	rdfs:isDefinedBy <http://rdaregistry.info/Elements/u/> ;
	rdfs:label "has respondent"@en ;
	rdfs:subPropertyOf <http://rdaregistry.info/Elements/u/P60447> ;
	owl:inverseOf <http://rdaregistry.info/Elements/u/P60001> ;
	owl:sameAs <http://rdaregistry.info/Elements/u/respondent> ;
	skos:closeMatch "http://id.loc.gov/vocabulary/relators/rsp"@en ;
	skos:definition "Relates a resource to a candidate for a degree who defends or opposes a thesis provided by the praeses in an academic disputation."@en .

<http://rdaregistry.info/Elements/u/P60046> reg:hasSubproperty <http://rdaregistry.info/Elements/a/P50093> ;
	reg:name "undifferentiatedNameIndicator"@en ;
	reg:status status:1001 ;
	a rdf:Property ;
	rdfs:isDefinedBy <http://rdaregistry.info/Elements/u/> ;
	rdfs:label "has undifferentiated name indicator"@en ;
	owl:sameAs <http://rdaregistry.info/Elements/u/undifferentiatedNameIndicator> ;
	skos:definition "Relates a resource to a categorization indicating that the core elements recorded are insufficient to differentiate between two or more agents with the same name."@en .

<http://rdaregistry.info/Elements/u/P60047> reg:hasSubproperty <http://rdaregistry.info/Elements/a/P50051> ;
	reg:name "typeOfAgent"@en ;
	reg:status status:1001 ;
	a rdf:Property ;
	rdfs:isDefinedBy <http://rdaregistry.info/Elements/u/> ;
	rdfs:label "has type of agent"@en ;
	owl:sameAs <http://rdaregistry.info/Elements/u/typeOfAgent> ;
	skos:definition "Relates a resource to a categorization or generic descriptor for the type of agent."@en .

<http://rdaregistry.info/Elements/u/P60048> reg:hasSubproperty <http://rdaregistry.info/Elements/m/P30001> ;
	reg:name "carrierType"@en ;
	reg:status status:1001 ;
	a rdf:Property ;
	rdfs:isDefinedBy <http://rdaregistry.info/Elements/u/> ;
	rdfs:label "has carrier type"@en ;
	owl:sameAs <http://rdaregistry.info/Elements/u/carrierType> ;
	skos:definition "Relates a resource to a categorization reflecting the format of the storage medium and housing of a carrier in combination with the type of intermediation device required to view, play, run, etc., the content of a resource."@en .

<http://rdaregistry.info/Elements/u/P60049> reg:hasSubproperty <http://rdaregistry.info/Elements/e/P20001> ;
	reg:name "contentType"@en ;
	reg:status status:1001 ;
	a rdf:Property ;
	rdfs:isDefinedBy <http://rdaregistry.info/Elements/u/> ;
	rdfs:label "has content type"@en ;
	owl:sameAs <http://rdaregistry.info/Elements/u/contentType> ;
	skos:definition "Relates a resource to a categorization reflecting the fundamental form of communication in which the content is expressed and the human sense through which it is intended to be perceived."@en .

<http://rdaregistry.info/Elements/u/P60050> reg:hasSubproperty <http://rdaregistry.info/Elements/m/P30002> ;
	reg:name "mediaType"@en ;
	reg:status status:1001 ;
	a rdf:Property ;
	rdfs:isDefinedBy <http://rdaregistry.info/Elements/u/> ;
	rdfs:label "has media type"@en ;
	owl:sameAs <http://rdaregistry.info/Elements/u/mediaType> ;
	skos:definition "Relates a resource to a categorization reflecting the general type of intermediation device required to view, play, run, etc., the content of a resource."@en .

<http://rdaregistry.info/Elements/u/P60051> reg:hasSubproperty <http://rdaregistry.info/Elements/m/P30003> ;
	reg:name "modeOfIssuance"@en ;
	reg:status status:1001 ;
	a rdf:Property ;
	rdfs:isDefinedBy <http://rdaregistry.info/Elements/u/> ;
	rdfs:label "has mode of issuance"@en ;
	owl:sameAs <http://rdaregistry.info/Elements/u/modeOfIssuance> ;
	skos:definition "Relates a resource to a categorization reflecting whether a resource is issued in one or more parts, the way it is updated, and its intended termination."@en .

<http://rdaregistry.info/Elements/u/P60052> reg:hasSubproperty <http://rdaregistry.info/Elements/e/P20002> , <http://rdaregistry.info/Elements/i/P40001> , <http://rdaregistry.info/Elements/m/P30004> , <http://rdaregistry.info/Elements/u/P60139> , <http://rdaregistry.info/Elements/u/P60140> , <http://rdaregistry.info/Elements/w/P10002> ;
	reg:name "identifierForTheResource"@en ;
	reg:status status:1001 ;
	a rdf:Property ;
	rdfs:isDefinedBy <http://rdaregistry.info/Elements/u/> ;
	rdfs:label "has identifier for the resource"@en ;
	owl:sameAs <http://rdaregistry.info/Elements/u/identifierForTheResource> ;
	skos:definition "Relates a resource to a character string associated with a resource that serves to differentiate that resource from other resources."@en .

<http://rdaregistry.info/Elements/u/P60053> reg:hasSubproperty <http://rdaregistry.info/Elements/a/P50052> , <http://rdaregistry.info/Elements/a/P50094> ;
	reg:name "identifierForTheAgent"@en ;
	reg:status status:1001 ;
	a rdf:Property ;
	rdfs:isDefinedBy <http://rdaregistry.info/Elements/u/> ;
	rdfs:label "has identifier for the agent"@en ;
	owl:sameAs <http://rdaregistry.info/Elements/u/identifierForTheAgent> ;
	skos:definition "Relates a resource to a character string uniquely associated with an agent, or with a surrogate for an agent (e.g., an authority record)."@en .

<http://rdaregistry.info/Elements/u/P60054> reg:hasSubproperty <http://rdaregistry.info/Elements/e/P20003> , <http://rdaregistry.info/Elements/w/P10003> ;
	reg:name "otherDistinguishingCharacteristicOfTheResource"@en ;
	reg:status status:1001 ;
	a rdf:Property ;
	rdfs:isDefinedBy <http://rdaregistry.info/Elements/u/> ;
	rdfs:label "has other distinguishing characteristic of the resource"@en ;
	owl:sameAs <http://rdaregistry.info/Elements/u/otherDistinguishingCharacteristicOfTheResource> ;
	skos:definition "Relates a resource to a characteristic other than content type, language of resource, date of resource, form of resource, or place of origin of the resource."@en .

<http://rdaregistry.info/Elements/u/P60055> reg:status status:1008 ;
	rdfs:isDefinedBy <http://rdaregistry.info/Elements/u/> .

<http://rdaregistry.info/Elements/u/P60056> reg:hasSubproperty <http://rdaregistry.info/Elements/u/P60055> ;
	reg:name "noteOnResourceSpecificCarrierCharacteristic"@en ;
	reg:status status:1001 ;
	a rdf:Property ;
	rdfs:isDefinedBy <http://rdaregistry.info/Elements/u/> ;
	rdfs:label "has note on resource-specific carrier characteristic"@en ;
	owl:sameAs <http://rdaregistry.info/Elements/u/itemSpecificCarrierCharacteristic> , <http://rdaregistry.info/Elements/u/noteOnResourceSpecificCarrierCharacteristic> ;
	skos:definition "Relates a resource to a note providing information about additional characteristics that are specific to the resource being described and are assumed not to apply to other resources exemplifying the same resource."@en .

<http://rdaregistry.info/Elements/u/P60057> reg:hasSubproperty <http://rdaregistry.info/Elements/m/P30005> ;
	reg:name "preferredCitation"@en ;
	reg:status status:1001 ;
	a rdf:Property ;
	rdfs:isDefinedBy <http://rdaregistry.info/Elements/u/> ;
	rdfs:label "has preferred citation"@en ;
	owl:sameAs <http://rdaregistry.info/Elements/u/preferredCitation> ;
	skos:definition "Relates a resource to a citation for a resource in the form preferred by a creator, publisher, custodian, indexing or abstracting service, etc."@en .

<http://rdaregistry.info/Elements/u/P60058> reg:hasSubproperty <http://rdaregistry.info/Elements/w/P10004> ;
	reg:name "formOfResource"@en ;
	reg:status status:1001 ;
	a rdf:Property ;
	rdfs:isDefinedBy <http://rdaregistry.info/Elements/u/> ;
	rdfs:label "has form of resource"@en ;
	owl:sameAs <http://rdaregistry.info/Elements/u/formOfResource> ;
	skos:definition "Relates a resource to a class or genre to which a resource belongs."@en .

<http://rdaregistry.info/Elements/u/P60059> reg:hasSubproperty <http://rdaregistry.info/Elements/m/P30006> ;
	reg:name "regionalEncoding"@en ;
	reg:status status:1001 ;
	a rdf:Property ;
	rdfs:isDefinedBy <http://rdaregistry.info/Elements/u/> ;
	rdfs:label "has regional encoding"@en ;
	rdfs:subPropertyOf <http://rdaregistry.info/Elements/u/P60350> ;
	owl:sameAs <http://rdaregistry.info/Elements/u/regionalEncoding> ;
	skos:definition "Relates a resource to a code identifying the region of the world for which a videodisc has been encoded and preventing the disc from being played on a player sold in a different region."@en .

<http://rdaregistry.info/Elements/u/P60060> reg:hasSubproperty <http://rdaregistry.info/Elements/w/P10006> ;
	reg:name "degreeGrantingInstitution"@en ;
	reg:status status:1001 ;
	a rdf:Property ;
	rdfs:isDefinedBy <http://rdaregistry.info/Elements/u/> ;
	rdfs:label "has degree granting institution"@en ;
	rdfs:subPropertyOf <http://rdaregistry.info/Elements/u/P60374> ;
	owl:inverseOf <http://rdaregistry.info/Elements/u/P60002> ;
	owl:sameAs <http://rdaregistry.info/Elements/u/degreeGrantingInstitution> ;
	skos:closeMatch "http://id.loc.gov/vocabulary/relators/dgg"@en ;
	skos:definition "Relates a resource to a corporate body granting an academic degree."@en .

<http://rdaregistry.info/Elements/u/P60061> reg:hasSubproperty <http://rdaregistry.info/Elements/w/P10007> ;
	reg:name "host institution"@en ;
	reg:status status:1001 ;
	a rdf:Property ;
	rdfs:isDefinedBy <http://rdaregistry.info/Elements/u/> ;
	rdfs:label "has host institution"@en ;
	rdfs:subPropertyOf <http://rdaregistry.info/Elements/u/P60374> ;
	owl:inverseOf <http://rdaregistry.info/Elements/u/P60003> ;
	owl:sameAs <http://rdaregistry.info/Elements/u/hostInstitution> ;
	skos:closeMatch "http://id.loc.gov/vocabulary/relators/his"@en ;
	skos:definition "Relates a resource to a corporate body hosting the event, exhibit, conference, etc., which gave rise to a resource, but having little or no responsibility for the content of the resource."@en .

<http://rdaregistry.info/Elements/u/P60062> reg:hasSubproperty <http://rdaregistry.info/Elements/w/P10008> ;
	reg:name "productionCompany"@en ;
	reg:status status:1001 ;
	a rdf:Property ;
	rdfs:isDefinedBy <http://rdaregistry.info/Elements/u/> ;
	rdfs:label "has production company"@en ;
	rdfs:subPropertyOf <http://rdaregistry.info/Elements/u/P60374> ;
	owl:inverseOf <http://rdaregistry.info/Elements/u/P60004> ;
	owl:sameAs <http://rdaregistry.info/Elements/u/productionCompany> ;
	skos:closeMatch "http://id.loc.gov/vocabulary/relators/prn"@en ;
	skos:definition "Relates a resource to a corporate body that is responsible for financial, technical, and organizational management of a production for stage, screen, sound recording, television, webcast, etc."@en .

<http://rdaregistry.info/Elements/u/P60064> reg:name "locationOfHeadquarters"@en ;
	reg:status status:1001 ;
	a rdf:Property ;
	rdfs:isDefinedBy <http://rdaregistry.info/Elements/u/> ;
	rdfs:label "has location of headquarters"@en ;
	rdfs:subPropertyOf <http://rdaregistry.info/Elements/u/P60325> ;
	owl:sameAs <http://rdaregistry.info/Elements/u/locationOfHeadquarters> ;
	skos:definition "Relates a resource to a country, state, province, etc., or local place in which an organization has its headquarters."@en .

<http://rdaregistry.info/Elements/u/P60065> reg:hasSubproperty <http://rdaregistry.info/Elements/w/P10011> ;
	reg:name "courtGoverned"@en ;
	reg:status status:1001 ;
	a rdf:Property ;
	rdfs:isDefinedBy <http://rdaregistry.info/Elements/u/> ;
	rdfs:label "has court governed"@en ;
	rdfs:subPropertyOf <http://rdaregistry.info/Elements/u/P60374> ;
	owl:inverseOf <http://rdaregistry.info/Elements/u/P60005> ;
	owl:sameAs <http://rdaregistry.info/Elements/u/courtGoverned> ;
	skos:closeMatch "http://id.loc.gov/vocabulary/relators/cou"@en ;
	skos:definition "Relates a resource to a court governed by court rules, regardless of their official nature (e.g., laws, administrative regulations)."@en .

<http://rdaregistry.info/Elements/u/P60066> reg:hasSubproperty <http://rdaregistry.info/Elements/i/P40004> ;
	reg:name "collector"@en ;
	reg:status status:1001 ;
	a rdf:Property ;
	rdfs:isDefinedBy <http://rdaregistry.info/Elements/u/> ;
	rdfs:label "has collector"@en ;
	rdfs:subPropertyOf <http://rdaregistry.info/Elements/u/P60376> ;
	owl:inverseOf <http://rdaregistry.info/Elements/u/P60006> ;
	owl:sameAs <http://rdaregistry.info/Elements/u/collector> ;
	skos:closeMatch "http://id.loc.gov/vocabulary/relators/col"@en ;
	skos:definition "Relates a resource to a curator who brings together resources from various sources that are then arranged, described, and cataloged as a collection."@en .

<http://rdaregistry.info/Elements/u/P60067> reg:hasSubproperty <http://rdaregistry.info/Elements/i/P40005> ;
	reg:name "collectionRegistrar"@en ;
	reg:status status:1001 ;
	a rdf:Property ;
	rdfs:isDefinedBy <http://rdaregistry.info/Elements/u/> ;
	rdfs:label "has collection registrar"@en ;
	rdfs:subPropertyOf <http://rdaregistry.info/Elements/u/P60376> ;
	owl:inverseOf <http://rdaregistry.info/Elements/u/P60007> ;
	owl:sameAs <http://rdaregistry.info/Elements/u/collectionRegistrar> ;
	skos:closeMatch "http://id.loc.gov/vocabulary/relators/cor"@en ;
	skos:definition "Relates a resource to a curator who lists or inventories the items in an aggregate resource such as a collection of items or resources."@en .

<http://rdaregistry.info/Elements/u/P60068> reg:hasSubproperty <http://rdaregistry.info/Elements/i/P40006> ;
	reg:name "depositor"@en ;
	reg:status status:1001 ;
	a rdf:Property ;
	rdfs:isDefinedBy <http://rdaregistry.info/Elements/u/> ;
	rdfs:label "has depositor"@en ;
	rdfs:subPropertyOf <http://rdaregistry.info/Elements/u/P60400> ;
	owl:inverseOf <http://rdaregistry.info/Elements/u/P60008> ;
	owl:sameAs <http://rdaregistry.info/Elements/u/depositor> ;
	skos:closeMatch "http://id.loc.gov/vocabulary/relators/dpt"@en ;
	skos:definition "Relates a resource to a current owner of a resource who deposited the resource into the custody of another person, family, or corporate body, while still retaining ownership."@en .

<http://rdaregistry.info/Elements/u/P60070> reg:hasSubproperty <http://rdaregistry.info/Elements/m/P30008> ;
	reg:name "dateOfDistribution"@en ;
	reg:status status:1001 ;
	a rdf:Property ;
	rdfs:isDefinedBy <http://rdaregistry.info/Elements/u/> ;
	rdfs:label "has date of distribution"@en ;
	owl:sameAs <http://rdaregistry.info/Elements/u/dateOfDistribution> ;
	skos:definition "Relates a resource to a date associated with the distribution of a resource in a published form."@en .

<http://rdaregistry.info/Elements/u/P60071> reg:hasSubproperty <http://rdaregistry.info/Elements/m/P30009> ;
	reg:name "dateOfProduction"@en ;
	reg:status status:1001 ;
	a rdf:Property ;
	rdfs:isDefinedBy <http://rdaregistry.info/Elements/u/> ;
	rdfs:label "has date of production"@en ;
	owl:sameAs <http://rdaregistry.info/Elements/u/dateOfProduction> ;
	skos:definition "Relates a resource to a date associated with the inscription, fabrication, construction, etc., of a resource in an unpublished form."@en .

<http://rdaregistry.info/Elements/u/P60072> reg:hasSubproperty <http://rdaregistry.info/Elements/m/P30010> ;
	reg:name "dateOfManufacture"@en ;
	reg:status status:1001 ;
	a rdf:Property ;
	rdfs:isDefinedBy <http://rdaregistry.info/Elements/u/> ;
	rdfs:label "has date of manufacture"@en ;
	owl:sameAs <http://rdaregistry.info/Elements/u/dateOfManufacture> ;
	skos:definition "Relates a resource to a date associated with the printing, duplicating, casting, etc., of a resource in a published form."@en .

<http://rdaregistry.info/Elements/u/P60073> reg:hasSubproperty <http://rdaregistry.info/Elements/m/P30011> ;
	reg:name "dateOfPublication"@en ;
	reg:status status:1001 ;
	a rdf:Property ;
	rdfs:isDefinedBy <http://rdaregistry.info/Elements/u/> ;
	rdfs:label "has date of publication"@en ;
	owl:sameAs <http://rdaregistry.info/Elements/u/dateOfPublication> ;
	skos:definition "Relates a resource to a date associated with the publication, release, or issuing of a resource."@en .

<http://rdaregistry.info/Elements/u/P60074> reg:hasSubproperty <http://rdaregistry.info/Elements/e/P20004> ;
	reg:name "dateOfCapture"@en ;
	reg:status status:1001 ;
	a rdf:Property ;
	rdfs:isDefinedBy <http://rdaregistry.info/Elements/u/> ;
	rdfs:label "has date of capture"@en ;
	owl:sameAs <http://rdaregistry.info/Elements/u/dateOfCapture> ;
	skos:definition "Relates a resource to a date or range of dates associated with the capture (i.e., recording, filming, etc.) of the content of a resource."@en .

<http://rdaregistry.info/Elements/u/P60075> reg:name "dateOfUsage"@en ;
	reg:status status:1001 ;
	a rdf:Property ;
	rdfs:isDefinedBy <http://rdaregistry.info/Elements/u/> ;
	rdfs:label "has date of usage"@en ;
	owl:sameAs <http://rdaregistry.info/Elements/u/dateOfUsage> ;
	skos:definition "Relates a resource to a date or range of dates associated with the use of the name designated as the preferred name for an agent."@en .

<http://rdaregistry.info/Elements/u/P60076> reg:hasSubproperty <http://rdaregistry.info/Elements/a/P50098> ;
	reg:name "periodOfActivityOfTheAgent"@en ;
	reg:status status:1001 ;
	a rdf:Property ;
	rdfs:isDefinedBy <http://rdaregistry.info/Elements/u/> ;
	rdfs:label "has period of activity of the agent"@en ;
	rdfs:subPropertyOf <http://rdaregistry.info/Elements/u/P60324> ;
	owl:sameAs <http://rdaregistry.info/Elements/u/periodOfActivityOfTheAgent> ;
	skos:definition "Relates a resource to a date or range of dates indicative of the period in which an agent was active in his or her primary field of endeavour."@en .

<http://rdaregistry.info/Elements/u/P60077> reg:hasSubproperty <http://rdaregistry.info/Elements/m/P30012> ;
	reg:name "parallelDesignationOfANamedRevisionOfAnEdition"@en ;
	reg:status status:1001 ;
	a rdf:Property ;
	rdfs:isDefinedBy <http://rdaregistry.info/Elements/u/> ;
	rdfs:label "has parallel designation of a named revision of an edition"@en ;
	owl:sameAs <http://rdaregistry.info/Elements/u/parallelDesignationOfANamedRevisionOfAnEdition> ;
	skos:definition "Relates a resource to a designation of a named revision of an edition in a language and/or script that differs from that recorded in the designation of a named revision of an edition element."@en .

<http://rdaregistry.info/Elements/u/P60078> reg:hasSubproperty <http://rdaregistry.info/Elements/m/P30013> ;
	reg:name "parallelDesignationOfEdition"@en ;
	reg:status status:1001 ;
	a rdf:Property ;
	rdfs:isDefinedBy <http://rdaregistry.info/Elements/u/> ;
	rdfs:label "has parallel designation of edition"@en ;
	owl:sameAs <http://rdaregistry.info/Elements/u/parallelDesignationOfEdition> ;
	skos:definition "Relates a resource to a designation of edition in a language and/or script that differs from that recorded in the designation of edition element."@en .

<http://rdaregistry.info/Elements/u/P60079> reg:name "numberOfAConferenceEtc"@en ;
	reg:status status:1001 ;
	a rdf:Property ;
	rdfs:isDefinedBy <http://rdaregistry.info/Elements/u/> ;
	rdfs:label "has number of a conference, etc."@en ;
	owl:sameAs <http://rdaregistry.info/Elements/u/numberOfAConferenceEtc> ;
	skos:definition "Relates a resource to a designation of the sequencing of a conference, etc., within a series of conferences, etc."@en .

<http://rdaregistry.info/Elements/u/P60080> reg:hasSubproperty <http://rdaregistry.info/Elements/w/P10012> ;
	reg:name "numberingOfPart"@en ;
	reg:status status:1001 ;
	a rdf:Property ;
	rdfs:isDefinedBy <http://rdaregistry.info/Elements/u/> ;
	rdfs:label "has numbering of part"@en ;
	owl:sameAs <http://rdaregistry.info/Elements/u/numberingOfPart> ;
	skos:definition "Relates a resource to a designation of the sequencing of a part or parts within a larger resource. numbering of part may include a numeral, a letter, any other character, or the combination of these with or without an accompanying caption (volume, number, etc.) and/or a chronological designation."@en .

<http://rdaregistry.info/Elements/u/P60081> reg:hasSubproperty <http://rdaregistry.info/Elements/m/P30014> ;
	reg:name "numberingWithinSeries"@en ;
	reg:status status:1001 ;
	a rdf:Property ;
	rdfs:isDefinedBy <http://rdaregistry.info/Elements/u/> ;
	rdfs:label "has numbering within series"@en ;
	owl:sameAs <http://rdaregistry.info/Elements/u/numberingWithinSeries> ;
	skos:definition "Relates a resource to a designation of the sequencing of a part or parts within a series. numbering within series may include a numeral, a letter, any other character, or the combination of these with or without an accompanying caption (volume, number, etc.) and/or a chronological designation."@en .

<http://rdaregistry.info/Elements/u/P60082> reg:hasSubproperty <http://rdaregistry.info/Elements/m/P30015> ;
	reg:name "numberingWithinSubseries"@en ;
	reg:status status:1001 ;
	a rdf:Property ;
	rdfs:isDefinedBy <http://rdaregistry.info/Elements/u/> ;
	rdfs:label "has numbering within subseries"@en ;
	owl:sameAs <http://rdaregistry.info/Elements/u/numberingWithinSubseries> ;
	skos:definition "Relates a resource to a designation of the sequencing of a part or parts within a subseries. numbering within subseries may include a numeral, a letter, any other character, or the combination of these with or without an accompanying caption (volume, number, etc.) and/or a chronological designation."@en .

<http://rdaregistry.info/Elements/u/P60083> reg:hasSubproperty <http://rdaregistry.info/Elements/m/P30016> ;
	reg:name "electronicReproduction"@en ;
	reg:status status:1001 ;
	a rdf:Property ;
	rdfs:isDefinedBy <http://rdaregistry.info/Elements/u/> ;
	rdfs:label "is electronic reproduction"@en ;
	rdfs:subPropertyOf <http://rdaregistry.info/Elements/u/P60272> ;
	owl:inverseOf <http://rdaregistry.info/Elements/u/P60469> ;
	owl:sameAs <http://rdaregistry.info/Elements/u/electronicReproduction> ;
	skos:definition "Relates a resource to a digital resource resulting from the reproduction of an analog resource."@en .

<http://rdaregistry.info/Elements/u/P60084> reg:hasSubproperty <http://rdaregistry.info/Elements/w/P10013> ;
	reg:name "filmDirector"@en ;
	reg:status status:1001 ;
	a rdf:Property ;
	rdfs:isDefinedBy <http://rdaregistry.info/Elements/u/> ;
	rdfs:label "has film director"@en ;
	rdfs:subPropertyOf <http://rdaregistry.info/Elements/u/P60449> ;
	owl:inverseOf <http://rdaregistry.info/Elements/u/P60009> ;
	owl:sameAs <http://rdaregistry.info/Elements/u/filmDirector> ;
	skos:closeMatch "http://id.loc.gov/vocabulary/relators/fmd"@en ;
	skos:definition "Relates a resource to a director responsible for the general management and supervision of a filmed performance."@en .

<http://rdaregistry.info/Elements/u/P60085> reg:hasSubproperty <http://rdaregistry.info/Elements/w/P10014> ;
	reg:name "radioDirector"@en ;
	reg:status status:1001 ;
	a rdf:Property ;
	rdfs:isDefinedBy <http://rdaregistry.info/Elements/u/> ;
	rdfs:label "has radio director"@en ;
	rdfs:subPropertyOf <http://rdaregistry.info/Elements/u/P60449> ;
	owl:inverseOf <http://rdaregistry.info/Elements/u/P60010> ;
	owl:sameAs <http://rdaregistry.info/Elements/u/radioDirector> ;
	skos:closeMatch "http://id.loc.gov/vocabulary/relators/rdd"@en ;
	skos:definition "Relates a resource to a director responsible for the general management and supervision of a radio program."@en .

<http://rdaregistry.info/Elements/u/P60086> reg:hasSubproperty <http://rdaregistry.info/Elements/w/P10015> ;
	reg:name "televisionDirector"@en ;
	reg:status status:1001 ;
	a rdf:Property ;
	rdfs:isDefinedBy <http://rdaregistry.info/Elements/u/> ;
	rdfs:label "has television director"@en ;
	rdfs:subPropertyOf <http://rdaregistry.info/Elements/u/P60449> ;
	owl:inverseOf <http://rdaregistry.info/Elements/u/P60011> ;
	owl:sameAs <http://rdaregistry.info/Elements/u/televisionDirector> ;
	skos:closeMatch "http://id.loc.gov/vocabulary/relators/tld"@en ;
	skos:definition "Relates a resource to a director responsible for the general management and supervision of a television program."@en .

<http://rdaregistry.info/Elements/u/P60087> reg:hasSubproperty <http://rdaregistry.info/Elements/m/P30017> ;
	reg:name "parallelDistributorsName"@en ;
	reg:status status:1001 ;
	a rdf:Property ;
	rdfs:isDefinedBy <http://rdaregistry.info/Elements/u/> ;
	rdfs:label "has parallel distributor's name"@en ;
	owl:sameAs <http://rdaregistry.info/Elements/u/parallelDistributorsName> ;
	skos:definition "Relates a resource to a distributor’s name in a language and/or script that differs from that recorded in the distributor’s name element."@en .

<http://rdaregistry.info/Elements/u/P60088> reg:hasSubproperty <http://rdaregistry.info/Elements/e/P20073> , <http://rdaregistry.info/Elements/w/P10016> ;
	reg:name "dramatizedAs"@en ;
	reg:status status:1001 ;
	a rdf:Property ;
	rdfs:isDefinedBy <http://rdaregistry.info/Elements/u/> ;
	rdfs:label "is dramatized as"@en ;
	rdfs:subPropertyOf <http://rdaregistry.info/Elements/u/P60260> ;
	owl:inverseOf <http://rdaregistry.info/Elements/u/P60225> ;
	owl:sameAs <http://rdaregistry.info/Elements/u/dramatizedAs> ;
	skos:definition "Relates a resource to a dramatic resource adapted from the source resource."@en .

<http://rdaregistry.info/Elements/u/P60089> reg:hasSubproperty <http://rdaregistry.info/Elements/a/P50100> ;
	reg:name "fieldOfActivity"@en ;
	reg:status status:1001 ;
	a rdf:Property ;
	rdfs:isDefinedBy <http://rdaregistry.info/Elements/u/> ;
	rdfs:label "has field of activity of the agent"@en ;
	owl:sameAs <http://rdaregistry.info/Elements/u/fieldOfActivity> ;
	skos:definition "Relates a resource to a field of endeavour, area of expertise, competence, responsibility, jurisdiction etc., in which an agent is engaged or was engaged."@en .

<http://rdaregistry.info/Elements/u/P60090> reg:hasSubproperty <http://rdaregistry.info/Elements/e/P20005> ;
	reg:name "award"@en ;
	reg:status status:1001 ;
	a rdf:Property ;
	rdfs:isDefinedBy <http://rdaregistry.info/Elements/u/> ;
	rdfs:label "has award"@en ;
	owl:sameAs <http://rdaregistry.info/Elements/u/award> ;
	skos:definition "Relates a resource to a formal recognition of excellence, etc., given by an award- or prize-granting body, for the content of a resource."@en .

<http://rdaregistry.info/Elements/u/P60091> reg:hasSubproperty <http://rdaregistry.info/Elements/i/P40007> ;
	reg:name "donor"@en ;
	reg:status status:1001 ;
	a rdf:Property ;
	rdfs:isDefinedBy <http://rdaregistry.info/Elements/u/> ;
	rdfs:label "has donor"@en ;
	rdfs:subPropertyOf <http://rdaregistry.info/Elements/u/P60401> ;
	owl:inverseOf <http://rdaregistry.info/Elements/u/P60012> ;
	owl:sameAs <http://rdaregistry.info/Elements/u/donor> ;
	skos:closeMatch "http://id.loc.gov/vocabulary/relators/dnr"@en ;
	skos:definition "Relates a resource to a former owner of a resource who donated that resource to another owner."@en .

<http://rdaregistry.info/Elements/u/P60092> reg:hasSubproperty <http://rdaregistry.info/Elements/i/P40008> ;
	reg:name "seller"@en ;
	reg:status status:1001 ;
	a rdf:Property ;
	rdfs:isDefinedBy <http://rdaregistry.info/Elements/u/> ;
	rdfs:label "has seller"@en ;
	rdfs:subPropertyOf <http://rdaregistry.info/Elements/u/P60401> ;
	owl:inverseOf <http://rdaregistry.info/Elements/u/P60013> ;
	owl:sameAs <http://rdaregistry.info/Elements/u/seller> ;
	skos:closeMatch "http://id.loc.gov/vocabulary/relators/sll"@en ;
	skos:definition "Relates a resource to a former owner of a resource who sold that resource to another owner."@en .

<http://rdaregistry.info/Elements/u/P60093> reg:hasSubproperty <http://rdaregistry.info/Elements/m/P30018> ;
	reg:name "fileType"@en ;
	reg:status status:1001 ;
	a rdf:Property ;
	rdfs:isDefinedBy <http://rdaregistry.info/Elements/u/> ;
	rdfs:label "has file type"@en ;
	rdfs:subPropertyOf <http://rdaregistry.info/Elements/u/P60350> ;
	owl:sameAs <http://rdaregistry.info/Elements/u/fileType> ;
	skos:definition "Relates a resource to a general type of data content encoded in a computer file."@en .

<http://rdaregistry.info/Elements/u/P60095> reg:hasSubproperty <http://rdaregistry.info/Elements/a/P50101> ;
	reg:name "affiliation"@en ;
	reg:status status:1001 ;
	a rdf:Property ;
	rdfs:isDefinedBy <http://rdaregistry.info/Elements/u/> ;
	rdfs:label "has affiliation"@en ;
	owl:sameAs <http://rdaregistry.info/Elements/u/affiliation> ;
	skos:definition "Relates a resource to a group with which an agent is affiliated or has been affiliated through employment, membership, cultural identity, etc."@en .

<http://rdaregistry.info/Elements/u/P60096> reg:hasSubproperty <http://rdaregistry.info/Elements/w/P10017> ;
	reg:name "enactingJurisdiction"@en ;
	reg:status status:1001 ;
	a rdf:Property ;
	rdfs:isDefinedBy <http://rdaregistry.info/Elements/u/> ;
	rdfs:label "has enacting jurisdiction"@en ;
	rdfs:subPropertyOf <http://rdaregistry.info/Elements/u/P60447> ;
	owl:inverseOf <http://rdaregistry.info/Elements/u/P60014> ;
	owl:sameAs <http://rdaregistry.info/Elements/u/enactingJurisdiction> ;
	skos:closeMatch "http://id.loc.gov/vocabulary/relators/enj"@en ;
	skos:definition "Relates a resource to a jurisdiction enacting a law, regulation, constitution, court rule, etc."@en .

<http://rdaregistry.info/Elements/u/P60097> reg:hasSubproperty <http://rdaregistry.info/Elements/w/P10018> ;
	reg:name "jurisdictionGoverned"@en ;
	reg:status status:1001 ;
	a rdf:Property ;
	rdfs:isDefinedBy <http://rdaregistry.info/Elements/u/> ;
	rdfs:label "has jurisdiction governed"@en ;
	rdfs:subPropertyOf <http://rdaregistry.info/Elements/u/P60374> ;
	owl:inverseOf <http://rdaregistry.info/Elements/u/P60015> ;
	owl:sameAs <http://rdaregistry.info/Elements/u/jurisdictionGoverned> ;
	skos:closeMatch "http://id.loc.gov/vocabulary/relators/jug"@en ;
	skos:definition "Relates a resource to a jurisdiction governed by a law, regulation, etc., that was enacted by another jurisdiction."@en .

<http://rdaregistry.info/Elements/u/P60098> reg:hasSubproperty <http://rdaregistry.info/Elements/a/P50102> ;
	reg:name "languageOfTheAgent"@en ;
	reg:status status:1001 ;
	a rdf:Property ;
	rdfs:isDefinedBy <http://rdaregistry.info/Elements/u/> ;
	rdfs:label "has language of the agent"@en ;
	owl:sameAs <http://rdaregistry.info/Elements/u/languageOfTheAgent> ;
	skos:definition "Relates a resource to a language an agent uses in its communications, when writing for publication, broadcasting, etc."@en .

<http://rdaregistry.info/Elements/u/P60099> reg:hasSubproperty <http://rdaregistry.info/Elements/e/P20006> , <http://rdaregistry.info/Elements/e/P20007> ;
	reg:name "languageOfTheContent"@en ;
	reg:status status:1001 ;
	a rdf:Property ;
	rdfs:isDefinedBy <http://rdaregistry.info/Elements/u/> ;
	rdfs:label "has language of the content"@en ;
	owl:sameAs <http://rdaregistry.info/Elements/u/languageOfTheContent> ;
	skos:definition "Relates a resource to a language used to express the content of a resource."@en .

<http://rdaregistry.info/Elements/u/P60100> reg:hasSubproperty <http://rdaregistry.info/Elements/m/P30019> ;
	reg:name "facsimileContainedIn"@en ;
	reg:status status:1001 ;
	a rdf:Property ;
	rdfs:isDefinedBy <http://rdaregistry.info/Elements/u/> ;
	rdfs:label "is facsimile contained in"@en ;
	rdfs:subPropertyOf <http://rdaregistry.info/Elements/u/P60101> ;
	owl:inverseOf <http://rdaregistry.info/Elements/u/P60300> ;
	owl:sameAs <http://rdaregistry.info/Elements/u/facsimileContainedIn> ;
	skos:definition "Relates a resource to a larger resource of which a part is a discrete component that exactly reproduces another resource embodying the resource."@en .

<http://rdaregistry.info/Elements/u/P60101> reg:hasSubproperty <http://rdaregistry.info/Elements/e/P20074> , <http://rdaregistry.info/Elements/i/P40009> , <http://rdaregistry.info/Elements/m/P30020> , <http://rdaregistry.info/Elements/u/P60100> , <http://rdaregistry.info/Elements/u/P60192> , <http://rdaregistry.info/Elements/u/P60193> , <http://rdaregistry.info/Elements/u/P60194> , <http://rdaregistry.info/Elements/u/P60317> , <http://rdaregistry.info/Elements/w/P10019> ;
	reg:name "containedIn"@en ;
	reg:status status:1001 ;
	a rdf:Property ;
	rdfs:isDefinedBy <http://rdaregistry.info/Elements/u/> ;
	rdfs:label "is contained in"@en ;
	rdfs:subPropertyOf <http://rdaregistry.info/Elements/u/P60714> ;
	owl:inverseOf <http://rdaregistry.info/Elements/u/P60249> ;
	owl:sameAs <http://rdaregistry.info/Elements/u/containedIn> ;
	skos:definition "Relates a resource to a larger resource of which the resource is a discrete component."@en .

<http://rdaregistry.info/Elements/u/P60102> reg:hasSubproperty <http://rdaregistry.info/Elements/w/P10020> ;
	reg:name "sequel"@en ;
	reg:status status:1001 ;
	a rdf:Property ;
	rdfs:isDefinedBy <http://rdaregistry.info/Elements/u/> ;
	rdfs:label "is sequel"@en ;
	rdfs:subPropertyOf <http://rdaregistry.info/Elements/u/P60278> ;
	owl:inverseOf <http://rdaregistry.info/Elements/u/P60577> ;
	owl:sameAs <http://rdaregistry.info/Elements/u/sequel> ;
	skos:definition "Relates a resource to a later resource that continues the narrative of an earlier resource."@en .

<http://rdaregistry.info/Elements/u/P60103> reg:hasSubproperty <http://rdaregistry.info/Elements/e/P20075> , <http://rdaregistry.info/Elements/w/P10021> ;
	reg:name "replacedInPartBy"@en ;
	reg:status status:1001 ;
	a rdf:Property ;
	rdfs:isDefinedBy <http://rdaregistry.info/Elements/u/> ;
	rdfs:label "is replaced in part by"@en ;
	rdfs:subPropertyOf <http://rdaregistry.info/Elements/u/P60278> ;
	owl:inverseOf <http://rdaregistry.info/Elements/u/P60479> ;
	owl:sameAs <http://rdaregistry.info/Elements/u/replacedInPartBy> , <http://rdaregistry.info/Elements/u/supersededInPartBy> ;
	skos:definition "Relates a resource to a later resource used in part in place of an earlier resource, usually because the later resource contains updated or new information that makes part of the earlier resource obsolete."@en .

<http://rdaregistry.info/Elements/u/P60104> reg:hasSubproperty <http://rdaregistry.info/Elements/e/P20076> , <http://rdaregistry.info/Elements/w/P10022> ;
	reg:name "replacedBy"@en ;
	reg:status status:1001 ;
	a rdf:Property ;
	rdfs:isDefinedBy <http://rdaregistry.info/Elements/u/> ;
	rdfs:label "is replaced by"@en ;
	rdfs:subPropertyOf <http://rdaregistry.info/Elements/u/P60278> ;
	owl:inverseOf <http://rdaregistry.info/Elements/u/P60480> ;
	owl:sameAs <http://rdaregistry.info/Elements/u/replacedBy> , <http://rdaregistry.info/Elements/u/supersededBy> ;
	skos:definition "Relates a resource to a later resource used in place of an earlier resource, usually because the later resource contains updated or new information that makes the earlier resource obsolete."@en .

<http://rdaregistry.info/Elements/u/P60105> reg:hasSubproperty <http://rdaregistry.info/Elements/e/P20008> ;
	reg:name "artisticAndOrTechnicalCredit"@en ;
	reg:status status:1001 ;
	a rdf:Property ;
	rdfs:isDefinedBy <http://rdaregistry.info/Elements/u/> ;
	rdfs:label "has artistic and/or technical credit"@en ;
	owl:sameAs <http://rdaregistry.info/Elements/u/artisticAndOrTechnicalCredit> ;
	skos:definition "Relates a resource to a listing of agents, families, or corporate bodies making contributions to the artistic and/or technical production of a resource."@en .

<http://rdaregistry.info/Elements/u/P60106> reg:hasSubproperty <http://rdaregistry.info/Elements/e/P20077> , <http://rdaregistry.info/Elements/w/P10023> ;
	reg:name "verseAdaptation"@en ;
	reg:status status:1001 ;
	a rdf:Property ;
	rdfs:isDefinedBy <http://rdaregistry.info/Elements/u/> ;
	rdfs:label "is verse adaptation"@en ;
	rdfs:subPropertyOf <http://rdaregistry.info/Elements/u/P60260> ;
	owl:inverseOf <http://rdaregistry.info/Elements/u/P60226> ;
	owl:sameAs <http://rdaregistry.info/Elements/u/verseAdaptation> ;
	skos:definition "Relates a resource to a literary composition in verse form adapted from the source resource."@en .

<http://rdaregistry.info/Elements/u/P60107> reg:name "locationOfConferenceEtc"@en ;
	reg:status status:1001 ;
	a rdf:Property ;
	rdfs:isDefinedBy <http://rdaregistry.info/Elements/u/> ;
	rdfs:label "has location of conference, etc."@en ;
	rdfs:subPropertyOf <http://rdaregistry.info/Elements/u/P60325> ;
	owl:sameAs <http://rdaregistry.info/Elements/u/locationOfConferenceEtc> ;
	skos:definition "Relates a resource to a local place in which a conference, congress, meeting, exhibition, fair, festival, etc., was held."@en .

<http://rdaregistry.info/Elements/u/P60108> reg:hasSubproperty <http://rdaregistry.info/Elements/m/P30049> ;
	reg:name "parallelManufacturersName"@en ;
	reg:status status:1001 ;
	a rdf:Property ;
	rdfs:isDefinedBy <http://rdaregistry.info/Elements/u/> ;
	rdfs:label "has parallel manufacturer's name"@en ;
	owl:sameAs <http://rdaregistry.info/Elements/u/parallelManufacturersName> ;
	skos:definition "Relates a resource to a manufacturer’s name in a language and/or script that differs from that recorded in the manufacturer’s name element."@en .

<http://rdaregistry.info/Elements/u/P60109> reg:hasSubproperty <http://rdaregistry.info/Elements/u/P60345> , <http://rdaregistry.info/Elements/u/P60346> , <http://rdaregistry.info/Elements/u/P60347> , <http://rdaregistry.info/Elements/w/P10024> ;
	reg:name "coordinatesOfCartographicContent"@en ;
	reg:status status:1001 ;
	a rdf:Property ;
	rdfs:isDefinedBy <http://rdaregistry.info/Elements/u/> ;
	rdfs:label "has coordinates of cartographic content"@en ;
	owl:sameAs <http://rdaregistry.info/Elements/u/coordinatesOfCartographicContent> ;
	skos:definition "Relates a resource to a mathematical system for identifying the area covered by the cartographic content of a resource."@en .

<http://rdaregistry.info/Elements/u/P60110> reg:hasSubproperty <http://rdaregistry.info/Elements/e/P20009> , <http://rdaregistry.info/Elements/w/P10025> ;
	reg:name "adaptedAsAMotionPicture"@en ;
	reg:status status:1001 ;
	a rdf:Property ;
	rdfs:isDefinedBy <http://rdaregistry.info/Elements/u/> ;
	rdfs:label "is adapted as motion picture"@en ;
	rdfs:subPropertyOf <http://rdaregistry.info/Elements/u/P60260> ;
	owl:inverseOf <http://rdaregistry.info/Elements/u/P60227> ;
	owl:sameAs <http://rdaregistry.info/Elements/u/adaptedAsAMotionPicture> ;
	skos:definition "Relates a resource to a motion picture based on the source resource."@en .

<http://rdaregistry.info/Elements/u/P60111> reg:hasSubproperty <http://rdaregistry.info/Elements/e/P20078> ;
	reg:name "dubbedVersionOf"@en ;
	reg:status status:1001 ;
	a rdf:Property ;
	rdfs:isDefinedBy <http://rdaregistry.info/Elements/u/> ;
	rdfs:label "is dubbed version of"@en ;
	rdfs:subPropertyOf <http://rdaregistry.info/Elements/u/P60244> ;
	owl:inverseOf <http://rdaregistry.info/Elements/u/P60112> ;
	owl:sameAs <http://rdaregistry.info/Elements/u/dubbedVersionOf> ;
	skos:definition "Relates a resource to a moving image resource in which the spoken dialogue has been translated into a language different from that of the original resource."@en .

<http://rdaregistry.info/Elements/u/P60112> reg:hasSubproperty <http://rdaregistry.info/Elements/e/P20079> ;
	reg:name "dubbedVersion"@en ;
	reg:status status:1001 ;
	a rdf:Property ;
	rdfs:isDefinedBy <http://rdaregistry.info/Elements/u/> ;
	rdfs:label "is dubbed version"@en ;
	rdfs:subPropertyOf <http://rdaregistry.info/Elements/u/P60280> ;
	owl:inverseOf <http://rdaregistry.info/Elements/u/P60111> ;
	owl:sameAs <http://rdaregistry.info/Elements/u/dubbedVersion> ;
	skos:definition "Relates a resource to a moving image resource that translates the spoken dialogue of the original resource into a different language."@en .

<http://rdaregistry.info/Elements/u/P60113> reg:hasSubproperty <http://rdaregistry.info/Elements/e/P20080> , <http://rdaregistry.info/Elements/w/P10026> ;
	reg:name "cadenza"@en ;
	reg:status status:1001 ;
	a rdf:Property ;
	rdfs:isDefinedBy <http://rdaregistry.info/Elements/u/> ;
	rdfs:label "is cadenza"@en ;
	rdfs:subPropertyOf <http://rdaregistry.info/Elements/u/P60204> ;
	owl:inverseOf <http://rdaregistry.info/Elements/u/P60116> ;
	owl:sameAs <http://rdaregistry.info/Elements/u/cadenza> ;
	skos:definition "Relates a resource to a musical resource consisting of an ornamental passage for a soloist, added to a musical resource such as a concerto, either by the same or a different composer."@en .

<http://rdaregistry.info/Elements/u/P60114> reg:hasSubproperty <http://rdaregistry.info/Elements/e/P20081> , <http://rdaregistry.info/Elements/w/P10027> ;
	reg:name "musicalVariationsBasedOn"@en ;
	reg:status status:1001 ;
	a rdf:Property ;
	rdfs:isDefinedBy <http://rdaregistry.info/Elements/u/> ;
	rdfs:label "is musical variations based on"@en ;
	rdfs:subPropertyOf <http://rdaregistry.info/Elements/u/P60305> ;
	owl:inverseOf <http://rdaregistry.info/Elements/u/P60115> ;
	owl:sameAs <http://rdaregistry.info/Elements/u/musicalVariationsBasedOn> ;
	skos:definition "Relates a resource to a musical resource from which melodic, thematic, or harmonic material is taken to form a discrete theme, which is repeated one or more times with subsequent modifications."@en .

<http://rdaregistry.info/Elements/u/P60115> reg:hasSubproperty <http://rdaregistry.info/Elements/e/P20082> , <http://rdaregistry.info/Elements/w/P10028> ;
	reg:name "musicalVariations"@en ;
	reg:status status:1001 ;
	a rdf:Property ;
	rdfs:isDefinedBy <http://rdaregistry.info/Elements/u/> ;
	rdfs:label "is musical variations"@en ;
	rdfs:subPropertyOf <http://rdaregistry.info/Elements/u/P60250> ;
	owl:inverseOf <http://rdaregistry.info/Elements/u/P60114> ;
	owl:sameAs <http://rdaregistry.info/Elements/u/musicalVariations> ;
	skos:definition "Relates a resource to a musical resource in which melodic, thematic, or harmonic material is taken from the source resource to form a discrete theme, which is repeated one or more times with subsequent modifications."@en .

<http://rdaregistry.info/Elements/u/P60116> reg:hasSubproperty <http://rdaregistry.info/Elements/e/P20083> , <http://rdaregistry.info/Elements/w/P10029> ;
	reg:name "cadenzaComposedFor"@en ;
	reg:status status:1001 ;
	a rdf:Property ;
	rdfs:isDefinedBy <http://rdaregistry.info/Elements/u/> ;
	rdfs:label "is cadenza composed for"@en ;
	rdfs:subPropertyOf <http://rdaregistry.info/Elements/u/P60307> ;
	owl:inverseOf <http://rdaregistry.info/Elements/u/P60113> ;
	owl:sameAs <http://rdaregistry.info/Elements/u/cadenzaComposedFor> ;
	skos:definition "Relates a resource to a musical resource such as a concerto for which an ornamental passage for a soloist has been composed, either by the same or a different composer."@en .

<http://rdaregistry.info/Elements/u/P60117> reg:hasSubproperty <http://rdaregistry.info/Elements/e/P20084> , <http://rdaregistry.info/Elements/w/P10030> ;
	reg:name "librettoFor"@en ;
	reg:status status:1001 ;
	a rdf:Property ;
	rdfs:isDefinedBy <http://rdaregistry.info/Elements/u/> ;
	rdfs:label "is libretto for"@en ;
	rdfs:subPropertyOf <http://rdaregistry.info/Elements/u/P60198> ;
	owl:inverseOf <http://rdaregistry.info/Elements/u/P60270> ;
	owl:sameAs <http://rdaregistry.info/Elements/u/librettoFor> ;
	skos:definition "Relates a resource to a musical resource such as an opera or other resource for the musical stage, or an oratorio, that uses the text of the related resource as a libretto."@en .

<http://rdaregistry.info/Elements/u/P60118> reg:hasSubproperty <http://rdaregistry.info/Elements/e/P20085> , <http://rdaregistry.info/Elements/w/P10031> ;
	reg:name "incidentalMusic"@en ;
	reg:status status:1001 ;
	a rdf:Property ;
	rdfs:isDefinedBy <http://rdaregistry.info/Elements/u/> ;
	rdfs:label "is incidental music"@en ;
	rdfs:subPropertyOf <http://rdaregistry.info/Elements/u/P60723> ;
	owl:inverseOf <http://rdaregistry.info/Elements/u/P60202> ;
	owl:sameAs <http://rdaregistry.info/Elements/u/incidentalMusic> ;
	skos:definition "Relates a resource to a musical resource that provides the incidental music for a play or other spoken work for the stage."@en .

<http://rdaregistry.info/Elements/u/P60119> reg:hasSubproperty <http://rdaregistry.info/Elements/a/P50054> , <http://rdaregistry.info/Elements/a/P50103> ;
	reg:name "variantNameForTheAgent"@en ;
	reg:status status:1001 ;
	a rdf:Property ;
	rdfs:isDefinedBy <http://rdaregistry.info/Elements/u/> ;
	rdfs:label "has variant name for the agent"@en ;
	rdfs:subPropertyOf <http://rdaregistry.info/Elements/u/P60368> ;
	owl:sameAs <http://rdaregistry.info/Elements/u/variantNameForTheAgent> ;
	skos:definition "Relates a resource to a name or form of name by which an agent is known that differs from the name or form of name chosen as the preferred name."@en .

<http://rdaregistry.info/Elements/u/P60120> reg:hasSubproperty <http://rdaregistry.info/Elements/e/P20086> , <http://rdaregistry.info/Elements/w/P10032> ;
	reg:name "remadeAs"@en ;
	reg:status status:1001 ;
	a rdf:Property ;
	rdfs:isDefinedBy <http://rdaregistry.info/Elements/u/> ;
	rdfs:label "is remade as"@en ;
	rdfs:subPropertyOf <http://rdaregistry.info/Elements/u/P60250> ;
	owl:inverseOf <http://rdaregistry.info/Elements/u/P60295> ;
	owl:sameAs <http://rdaregistry.info/Elements/u/remadeAs> ;
	skos:definition "Relates a resource to a new motion picture, radio program, television program, or video based on an earlier resource."@en .

<http://rdaregistry.info/Elements/u/P60121> reg:hasSubproperty <http://rdaregistry.info/Elements/e/P20087> , <http://rdaregistry.info/Elements/w/P10033> ;
	reg:name "musicalSetting"@en ;
	reg:status status:1001 ;
	a rdf:Property ;
	rdfs:isDefinedBy <http://rdaregistry.info/Elements/u/> ;
	rdfs:label "is musical setting"@en ;
	rdfs:subPropertyOf <http://rdaregistry.info/Elements/u/P60250> ;
	owl:inverseOf <http://rdaregistry.info/Elements/u/P60266> ;
	owl:sameAs <http://rdaregistry.info/Elements/u/musicalSetting> ;
	skos:definition "Relates a resource to a non-dramatic musical resource, other than an oratorio, that uses the text of the source resource."@en .

<http://rdaregistry.info/Elements/u/P60122> reg:hasSubproperty <http://rdaregistry.info/Elements/m/P30050> ;
	reg:name "noteOnIssuePartOrIterationUsedAsTheBasisForIdentificationOfTheResource"@en ;
	reg:status status:1001 ;
	a rdf:Property ;
	rdfs:isDefinedBy <http://rdaregistry.info/Elements/u/> ;
	rdfs:label "has note on issue, part, or iteration used as the basis for identification of the resource"@en ;
	rdfs:subPropertyOf <http://rdaregistry.info/Elements/u/P60470> ;
	owl:sameAs <http://rdaregistry.info/Elements/u/noteOnIssuePartOrIterationUsedAsTheBasisForIdentificationOfTheResource> ;
	skos:definition "Relates a resource to a note identifying the issue or part of a multipart monograph or serial, or the iteration of an integrating resource that has been used as the basis for the identification of a resource."@en .

<http://rdaregistry.info/Elements/u/P60123> reg:hasSubproperty <http://rdaregistry.info/Elements/e/P20010> ;
	reg:name "noteOnChangesInContentCharacteristics"@en ;
	reg:status status:1001 ;
	a rdf:Property ;
	rdfs:isDefinedBy <http://rdaregistry.info/Elements/u/> ;
	rdfs:label "has note on changes in content characteristics"@en ;
	rdfs:subPropertyOf <http://rdaregistry.info/Elements/u/P60470> ;
	owl:sameAs <http://rdaregistry.info/Elements/u/noteOnChangesInContentCharacteristics> ;
	skos:definition "Relates a resource to a note on changes in content characteristics that occur in subsequent issues or parts of a resource issued in successive parts or between iterations of an integrating resource."@en .

<http://rdaregistry.info/Elements/u/P60124> reg:hasSubproperty <http://rdaregistry.info/Elements/m/P30051> ;
	reg:name "noteOnChangesInCarrierCharacteristics"@en ;
	reg:status status:1001 ;
	a rdf:Property ;
	rdfs:isDefinedBy <http://rdaregistry.info/Elements/u/> ;
	rdfs:label "has note on changes in carrier characteristics"@en ;
	rdfs:subPropertyOf <http://rdaregistry.info/Elements/u/P60470> ;
	owl:sameAs <http://rdaregistry.info/Elements/u/noteOnChangesInCarrierCharacteristics> ;
	skos:definition "Relates a resource to a note on changes in the characteristics of the carrier that occur in subsequent issues or parts of a resource issued in successive parts or between iterations of an integrating resource."@en .

<http://rdaregistry.info/Elements/u/P60125> reg:hasSubproperty <http://rdaregistry.info/Elements/m/P30052> ;
	reg:name "noteOnDistributionStatement"@en ;
	reg:status status:1001 ;
	a rdf:Property ;
	rdfs:isDefinedBy <http://rdaregistry.info/Elements/u/> ;
	rdfs:label "has note on distribution statement"@en ;
	rdfs:subPropertyOf <http://rdaregistry.info/Elements/u/P60470> ;
	owl:sameAs <http://rdaregistry.info/Elements/u/noteOnDistributionStatement> ;
	skos:definition "Relates a resource to a note providing details on place of distribution, distributor, or date of distribution, or information on changes in the place of distribution, distributor, or distributor’s name."@en .

<http://rdaregistry.info/Elements/u/P60126> reg:hasSubproperty <http://rdaregistry.info/Elements/m/P30053> ;
	reg:name "noteOnManufactureStatement"@en ;
	reg:status status:1001 ;
	a rdf:Property ;
	rdfs:isDefinedBy <http://rdaregistry.info/Elements/u/> ;
	rdfs:label "has note on manufacture statement"@en ;
	rdfs:subPropertyOf <http://rdaregistry.info/Elements/u/P60470> ;
	owl:sameAs <http://rdaregistry.info/Elements/u/noteOnManufactureStatement> ;
	skos:definition "Relates a resource to a note providing details on place of manufacture, manufacturer, or date of manufacture, or information on changes in the place of manufacture, manufacturer, or manufacturer’s name."@en .

<http://rdaregistry.info/Elements/u/P60127> reg:hasSubproperty <http://rdaregistry.info/Elements/m/P30054> ;
	reg:name "noteOnProductionStatement"@en ;
	reg:status status:1001 ;
	a rdf:Property ;
	rdfs:isDefinedBy <http://rdaregistry.info/Elements/u/> ;
	rdfs:label "has note on production statement"@en ;
	rdfs:subPropertyOf <http://rdaregistry.info/Elements/u/P60470> ;
	owl:sameAs <http://rdaregistry.info/Elements/u/noteOnProductionStatement> ;
	skos:definition "Relates a resource to a note providing details on place of production, producer, or date of production, or information on changes in the place of production, producer, or producer’s name."@en .

<http://rdaregistry.info/Elements/u/P60128> reg:hasSubproperty <http://rdaregistry.info/Elements/m/P30055> ;
	reg:name "noteOnPublicationStatement"@en ;
	reg:status status:1001 ;
	a rdf:Property ;
	rdfs:isDefinedBy <http://rdaregistry.info/Elements/u/> ;
	rdfs:label "has note on publication statement"@en ;
	rdfs:subPropertyOf <http://rdaregistry.info/Elements/u/P60470> ;
	owl:sameAs <http://rdaregistry.info/Elements/u/noteOnPublicationStatement> ;
	skos:definition "Relates a resource to a note providing details on place of publication, publisher, or date of publication, information on changes in the place of publication, publisher, or publisher’s name, or on suspension of publication."@en .

<http://rdaregistry.info/Elements/u/P60129> reg:hasSubproperty <http://rdaregistry.info/Elements/m/P30056> ;
	reg:name "noteOnFrequency"@en ;
	reg:status status:1001 ;
	a rdf:Property ;
	rdfs:isDefinedBy <http://rdaregistry.info/Elements/u/> ;
	rdfs:label "has note on frequency"@en ;
	rdfs:subPropertyOf <http://rdaregistry.info/Elements/u/P60470> ;
	owl:sameAs <http://rdaregistry.info/Elements/u/noteOnFrequency> ;
	skos:definition "Relates a resource to a note providing details on the currency of the contents, on the frequency of release of issues or parts of a serial or the frequency of updates to an integrating resource, or on changes in frequency."@en .

<http://rdaregistry.info/Elements/u/P60130> reg:hasSubproperty <http://rdaregistry.info/Elements/m/P30057> ;
	reg:name "noteOnStatementOfResponsibility"@en ;
	reg:status status:1001 ;
	a rdf:Property ;
	rdfs:isDefinedBy <http://rdaregistry.info/Elements/u/> ;
	rdfs:label "has note on statement of responsibility"@en ;
	rdfs:subPropertyOf <http://rdaregistry.info/Elements/u/P60470> ;
	owl:sameAs <http://rdaregistry.info/Elements/u/noteOnStatementOfResponsibility> ;
	skos:definition "Relates a resource to a note providing information on an agent not named in a statement of responsibility to whom responsibility for the intellectual or artistic content of the resource has been attributed, on variant forms of names appearing in the resource, on changes in statements of responsibility, or on other details relating to a statement of responsibility."@en .

<http://rdaregistry.info/Elements/u/P60131> reg:hasSubproperty <http://rdaregistry.info/Elements/m/P30058> ;
	reg:name "noteOnSeriesStatement"@en ;
	reg:status status:1001 ;
	a rdf:Property ;
	rdfs:isDefinedBy <http://rdaregistry.info/Elements/u/> ;
	rdfs:label "has note on series statement"@en ;
	rdfs:subPropertyOf <http://rdaregistry.info/Elements/u/P60470> ;
	owl:sameAs <http://rdaregistry.info/Elements/u/noteOnSeriesStatement> ;
	skos:definition "Relates a resource to a note providing information on complex series statements, incorrect numbering within series, or changes in series statements."@en .

<http://rdaregistry.info/Elements/u/P60132> reg:hasSubproperty <http://rdaregistry.info/Elements/m/P30059> ;
	reg:name "noteOnCopyrightDate"@en ;
	reg:status status:1001 ;
	a rdf:Property ;
	rdfs:isDefinedBy <http://rdaregistry.info/Elements/u/> ;
	rdfs:label "has note on copyright date"@en ;
	rdfs:subPropertyOf <http://rdaregistry.info/Elements/u/P60470> ;
	owl:sameAs <http://rdaregistry.info/Elements/u/noteOnCopyrightDate> ;
	skos:definition "Relates a resource to a note providing information on copyright dates not recorded as part of the copyright date element."@en .

<http://rdaregistry.info/Elements/u/P60133> reg:hasSubproperty <http://rdaregistry.info/Elements/i/P40010> , <http://rdaregistry.info/Elements/m/P30060> ;
	reg:name "noteOnDimensionsOfResource"@en ;
	reg:status status:1001 ;
	a rdf:Property ;
	rdfs:isDefinedBy <http://rdaregistry.info/Elements/u/> ;
	rdfs:label "has note on dimensions of resource"@en ;
	rdfs:subPropertyOf <http://rdaregistry.info/Elements/u/P60470> ;
	owl:sameAs <http://rdaregistry.info/Elements/u/noteOnDimensionsOfResource> ;
	skos:definition "Relates a resource to a note providing information on the dimensions of a resource that is not recorded as part of the dimensions element."@en .

<http://rdaregistry.info/Elements/u/P60134> reg:hasSubproperty <http://rdaregistry.info/Elements/i/P40011> , <http://rdaregistry.info/Elements/m/P30061> ;
	reg:name "noteOnExtentOfResource"@en ;
	reg:status status:1001 ;
	a rdf:Property ;
	rdfs:isDefinedBy <http://rdaregistry.info/Elements/u/> ;
	rdfs:label "has note on extent of resource"@en ;
	rdfs:subPropertyOf <http://rdaregistry.info/Elements/u/P60470> ;
	owl:sameAs <http://rdaregistry.info/Elements/u/noteOnExtentOfResource> ;
	skos:definition "Relates a resource to a note providing information on the extent of a resource that is not recorded as part of the extent element."@en .

<http://rdaregistry.info/Elements/u/P60135> reg:hasSubproperty <http://rdaregistry.info/Elements/m/P30062> ;
	reg:name "noteOnNumberingOfSerials"@en ;
	reg:status status:1001 ;
	a rdf:Property ;
	rdfs:isDefinedBy <http://rdaregistry.info/Elements/u/> ;
	rdfs:label "has note on numbering of serials"@en ;
	rdfs:subPropertyOf <http://rdaregistry.info/Elements/u/P60470> ;
	owl:sameAs <http://rdaregistry.info/Elements/u/noteOnNumberingOfSerials> ;
	skos:definition "Relates a resource to a note providing information on the numbering of the first and/or last issue or part, on complex or irregular numbering (including numbering errors), or on the period covered by a volume, issue, part, etc."@en .

<http://rdaregistry.info/Elements/u/P60136> reg:hasSubproperty <http://rdaregistry.info/Elements/m/P30063> ;
	reg:name "noteOnTitle"@en ;
	reg:status status:1001 ;
	a rdf:Property ;
	rdfs:isDefinedBy <http://rdaregistry.info/Elements/u/> ;
	rdfs:label "has note on title"@en ;
	rdfs:subPropertyOf <http://rdaregistry.info/Elements/u/P60470> ;
	owl:sameAs <http://rdaregistry.info/Elements/u/noteOnTitle> ;
	skos:definition "Relates a resource to a note providing information on the source from which a title was taken, the date the title was viewed, variations in titles, inaccuracies, deletions, etc., or other information relating to a title."@en .

<http://rdaregistry.info/Elements/u/P60137> reg:hasSubproperty <http://rdaregistry.info/Elements/m/P30064> ;
	reg:name "noteOnEditionStatement"@en ;
	reg:status status:1001 ;
	a rdf:Property ;
	rdfs:isDefinedBy <http://rdaregistry.info/Elements/u/> ;
	rdfs:label "has note on edition statement"@en ;
	rdfs:subPropertyOf <http://rdaregistry.info/Elements/u/P60470> ;
	owl:sameAs <http://rdaregistry.info/Elements/u/noteOnEditionStatement> ;
	skos:definition "Relates a resource to a note providing information on the source of an edition statement, on edition statements relating to issues, parts, etc., on changes in edition statements, or other information relating to an edition statement."@en .

<http://rdaregistry.info/Elements/u/P60138> reg:hasSubproperty <http://rdaregistry.info/Elements/e/P20088> , <http://rdaregistry.info/Elements/w/P10034> ;
	reg:name "novelization"@en ;
	reg:status status:1001 ;
	a rdf:Property ;
	rdfs:isDefinedBy <http://rdaregistry.info/Elements/u/> ;
	rdfs:label "is novelization"@en ;
	rdfs:subPropertyOf <http://rdaregistry.info/Elements/u/P60260> ;
	owl:inverseOf <http://rdaregistry.info/Elements/u/P60228> ;
	owl:sameAs <http://rdaregistry.info/Elements/u/novelization> ;
	skos:definition "Relates a resource to a novel adapted from the source resource."@en .

<http://rdaregistry.info/Elements/u/P60139> reg:hasSubproperty <http://rdaregistry.info/Elements/m/P30065> ;
	reg:name "publishersNumberForMusic"@en ;
	reg:status status:1001 ;
	a rdf:Property ;
	rdfs:isDefinedBy <http://rdaregistry.info/Elements/u/> ;
	rdfs:label "has publisher's number for music"@en ;
	rdfs:subPropertyOf <http://rdaregistry.info/Elements/u/P60052> ;
	owl:sameAs <http://rdaregistry.info/Elements/u/publishersNumberForMusic> ;
	skos:definition "Relates a resource to a numbering designation assigned to a resource by a music publisher, appearing normally only on the title page, the cover, and/or the first page of music."@en .

<http://rdaregistry.info/Elements/u/P60140> reg:hasSubproperty <http://rdaregistry.info/Elements/m/P30066> ;
	reg:name "plateNumberForMusic"@en ;
	reg:status status:1001 ;
	a rdf:Property ;
	rdfs:isDefinedBy <http://rdaregistry.info/Elements/u/> ;
	rdfs:label "has plate number for music"@en ;
	rdfs:subPropertyOf <http://rdaregistry.info/Elements/u/P60052> ;
	owl:sameAs <http://rdaregistry.info/Elements/u/plateNumberForMusic> ;
	skos:definition "Relates a resource to a numbering designation assigned to a resource by a music publisher."@en .

<http://rdaregistry.info/Elements/u/P60141> reg:hasSubproperty <http://rdaregistry.info/Elements/e/P20011> ;
	reg:name "conductor"@en ;
	reg:status status:1001 ;
	a rdf:Property ;
	rdfs:isDefinedBy <http://rdaregistry.info/Elements/u/> ;
	rdfs:label "has conductor"@en ;
	rdfs:subPropertyOf <http://rdaregistry.info/Elements/u/P60387> ;
	owl:inverseOf <http://rdaregistry.info/Elements/u/P60016> ;
	owl:sameAs <http://rdaregistry.info/Elements/u/conductor> ;
	skos:closeMatch "http://id.loc.gov/vocabulary/relators/cnd"@en ;
	skos:definition "Relates a resource to a performer contributing to a musical resource by leading a performing group (orchestra, chorus, opera, etc.) in a musical or dramatic presentation, etc."@en .

<http://rdaregistry.info/Elements/u/P60142> reg:hasSubproperty <http://rdaregistry.info/Elements/e/P20012> , <http://rdaregistry.info/Elements/u/P60152> ;
	reg:name "actor"@en ;
	reg:status status:1001 ;
	a rdf:Property ;
	rdfs:isDefinedBy <http://rdaregistry.info/Elements/u/> ;
	rdfs:label "has actor"@en ;
	rdfs:subPropertyOf <http://rdaregistry.info/Elements/u/P60387> ;
	owl:inverseOf <http://rdaregistry.info/Elements/u/P60017> ;
	owl:sameAs <http://rdaregistry.info/Elements/u/actor> ;
	skos:closeMatch "http://id.loc.gov/vocabulary/relators/act"@en ;
	skos:definition "Relates a resource to a performer contributing to a resource by acting as a cast member or player in a musical or dramatic presentation, etc."@en .

<http://rdaregistry.info/Elements/u/P60143> reg:hasSubproperty <http://rdaregistry.info/Elements/e/P20013> ;
	reg:name "onScreenPresenter"@en ;
	reg:status status:1001 ;
	a rdf:Property ;
	rdfs:isDefinedBy <http://rdaregistry.info/Elements/u/> ;
	rdfs:label "has on-screen presenter"@en ;
	rdfs:subPropertyOf <http://rdaregistry.info/Elements/u/P60387> ;
	owl:inverseOf <http://rdaregistry.info/Elements/u/P60018> ;
	owl:sameAs <http://rdaregistry.info/Elements/u/onScreenPresenter> ;
	skos:closeMatch "http://id.loc.gov/vocabulary/relators/osp"@en ;
	skos:definition "Relates a resource to a performer contributing to a resource by appearing on screen to provide contextual or background information. an on-screen presenter may appear in nonfiction moving image materials or in introductions to fiction moving image materials."@en .

<http://rdaregistry.info/Elements/u/P60144> reg:hasSubproperty <http://rdaregistry.info/Elements/e/P20014> ;
	reg:name "dancer"@en ;
	reg:status status:1001 ;
	a rdf:Property ;
	rdfs:isDefinedBy <http://rdaregistry.info/Elements/u/> ;
	rdfs:label "has dancer"@en ;
	rdfs:subPropertyOf <http://rdaregistry.info/Elements/u/P60387> ;
	owl:inverseOf <http://rdaregistry.info/Elements/u/P60019> ;
	owl:sameAs <http://rdaregistry.info/Elements/u/dancer> ;
	skos:closeMatch "http://id.loc.gov/vocabulary/relators/dnc"@en ;
	skos:definition "Relates a resource to a performer contributing to a resource by dancing in a musical, dramatic, etc., presentation."@en .

<http://rdaregistry.info/Elements/u/P60145> reg:hasSubproperty <http://rdaregistry.info/Elements/e/P20015> ;
	reg:name "teacher"@en ;
	reg:status status:1001 ;
	a rdf:Property ;
	rdfs:isDefinedBy <http://rdaregistry.info/Elements/u/> ;
	rdfs:label "has teacher"@en ;
	rdfs:subPropertyOf <http://rdaregistry.info/Elements/u/P60387> ;
	owl:inverseOf <http://rdaregistry.info/Elements/u/P60020> ;
	owl:sameAs <http://rdaregistry.info/Elements/u/teacher> ;
	skos:closeMatch "http://id.loc.gov/vocabulary/relators/tch"@en ;
	skos:definition "Relates a resource to a performer contributing to a resource by giving instruction or providing a demonstration."@en .

<http://rdaregistry.info/Elements/u/P60146> reg:hasSubproperty <http://rdaregistry.info/Elements/e/P20016> ;
	reg:name "host"@en ;
	reg:status status:1001 ;
	a rdf:Property ;
	rdfs:isDefinedBy <http://rdaregistry.info/Elements/u/> ;
	rdfs:label "has host"@en ;
	rdfs:subPropertyOf <http://rdaregistry.info/Elements/u/P60387> ;
	owl:inverseOf <http://rdaregistry.info/Elements/u/P60021> ;
	owl:sameAs <http://rdaregistry.info/Elements/u/host> ;
	skos:closeMatch "http://id.loc.gov/vocabulary/relators/hst"@en ;
	skos:definition "Relates a resource to a performer contributing to a resource by leading a program (often broadcast) that includes other guests, performers, etc. (e.g., talk show host)."@en .

<http://rdaregistry.info/Elements/u/P60147> reg:hasSubproperty <http://rdaregistry.info/Elements/e/P20017> ;
	reg:name "moderator"@en ;
	reg:status status:1001 ;
	a rdf:Property ;
	rdfs:isDefinedBy <http://rdaregistry.info/Elements/u/> ;
	rdfs:label "has moderator"@en ;
	rdfs:subPropertyOf <http://rdaregistry.info/Elements/u/P60387> ;
	owl:inverseOf <http://rdaregistry.info/Elements/u/P60022> ;
	owl:sameAs <http://rdaregistry.info/Elements/u/moderator> ;
	skos:closeMatch "http://id.loc.gov/vocabulary/relators/mod"@en ;
	skos:definition "Relates a resource to a performer contributing to a resource by leading a program (often broadcast) where topics are discussed, usually with participation of experts in fields related to the discussion."@en .

<http://rdaregistry.info/Elements/u/P60148> reg:hasSubproperty <http://rdaregistry.info/Elements/e/P20018> ;
	reg:name "puppeteer"@en ;
	reg:status status:1001 ;
	a rdf:Property ;
	rdfs:isDefinedBy <http://rdaregistry.info/Elements/u/> ;
	rdfs:label "has puppeteer"@en ;
	rdfs:subPropertyOf <http://rdaregistry.info/Elements/u/P60387> ;
	owl:inverseOf <http://rdaregistry.info/Elements/u/P60023> ;
	owl:sameAs <http://rdaregistry.info/Elements/u/puppeteer> ;
	skos:closeMatch "http://id.loc.gov/vocabulary/relators/ppt"@en ;
	skos:definition "Relates a resource to a performer contributing to a resource by manipulating, controlling, or directing puppets or marionettes in a moving image production or a musical or dramatic presentation or entertainment."@en .

<http://rdaregistry.info/Elements/u/P60149> reg:hasSubproperty <http://rdaregistry.info/Elements/e/P20019> ;
	reg:name "panelist"@en ;
	reg:status status:1001 ;
	a rdf:Property ;
	rdfs:isDefinedBy <http://rdaregistry.info/Elements/u/> ;
	rdfs:label "has panelist"@en ;
	rdfs:subPropertyOf <http://rdaregistry.info/Elements/u/P60387> ;
	owl:inverseOf <http://rdaregistry.info/Elements/u/P60024> ;
	owl:sameAs <http://rdaregistry.info/Elements/u/panelist> ;
	skos:closeMatch "http://id.loc.gov/vocabulary/relators/pan"@en ;
	skos:definition "Relates a resource to a performer contributing to a resource by participating in a program (often broadcast) where topics are discussed, usually with participation of experts in fields related to the discussion."@en .

<http://rdaregistry.info/Elements/u/P60150> reg:hasSubproperty <http://rdaregistry.info/Elements/e/P20020> ;
	reg:name "instrumentalist"@en ;
	reg:status status:1001 ;
	a rdf:Property ;
	rdfs:isDefinedBy <http://rdaregistry.info/Elements/u/> ;
	rdfs:label "has instrumentalist"@en ;
	rdfs:subPropertyOf <http://rdaregistry.info/Elements/u/P60387> ;
	owl:inverseOf <http://rdaregistry.info/Elements/u/P60025> ;
	owl:sameAs <http://rdaregistry.info/Elements/u/instrumentalist> ;
	skos:closeMatch "http://id.loc.gov/vocabulary/relators/itr"@en ;
	skos:definition "Relates a resource to a performer contributing to a resource by playing a musical instrument."@en .

<http://rdaregistry.info/Elements/u/P60151> reg:hasSubproperty <http://rdaregistry.info/Elements/e/P20021> ;
	reg:name "commentator"@en ;
	reg:status status:1001 ;
	a rdf:Property ;
	rdfs:isDefinedBy <http://rdaregistry.info/Elements/u/> ;
	rdfs:label "has commentator"@en ;
	rdfs:subPropertyOf <http://rdaregistry.info/Elements/u/P60387> ;
	owl:inverseOf <http://rdaregistry.info/Elements/u/P60026> ;
	owl:sameAs <http://rdaregistry.info/Elements/u/commentator> ;
	skos:closeMatch "http://id.loc.gov/vocabulary/relators/cmm"@en ;
	skos:definition "Relates a resource to a performer contributing to a resource by providing interpretation, analysis, or a discussion of the subject matter on a recording, film, or other audiovisual medium."@en .

<http://rdaregistry.info/Elements/u/P60152> reg:hasSubproperty <http://rdaregistry.info/Elements/e/P20070> ;
	reg:name "voiceActor"@en ;
	reg:status status:1001 ;
	a rdf:Property ;
	rdfs:isDefinedBy <http://rdaregistry.info/Elements/u/> ;
	rdfs:label "has voice actor"@en ;
	rdfs:subPropertyOf <http://rdaregistry.info/Elements/u/P60142> ;
	owl:inverseOf <http://rdaregistry.info/Elements/u/P60027> ;
	owl:sameAs <http://rdaregistry.info/Elements/u/voiceActor> ;
	skos:closeMatch "http://id.loc.gov/vocabulary/relators/vac"@en ;
	skos:definition "Relates a resource to a performer contributing to a resource by providing the voice for characters in radio and audio productions and for animated characters in moving image resources as well as by providing voice-overs in radio and television commercials, dubbed resources, etc."@en .

<http://rdaregistry.info/Elements/u/P60153> reg:hasSubproperty <http://rdaregistry.info/Elements/e/P20022> ;
	reg:name "narrator"@en ;
	reg:status status:1001 ;
	a rdf:Property ;
	rdfs:isDefinedBy <http://rdaregistry.info/Elements/u/> ;
	rdfs:label "has narrator"@en ;
	rdfs:subPropertyOf <http://rdaregistry.info/Elements/u/P60387> ;
	owl:inverseOf <http://rdaregistry.info/Elements/u/P60028> ;
	owl:sameAs <http://rdaregistry.info/Elements/u/narrator> ;
	skos:closeMatch "http://id.loc.gov/vocabulary/relators/nrt"@en ;
	skos:definition "Relates a resource to a performer contributing to a resource by reading or speaking in order to give an account of an act, occurrence, course of events, etc."@en .

<http://rdaregistry.info/Elements/u/P60154> reg:hasSubproperty <http://rdaregistry.info/Elements/e/P20023> ;
	reg:name "storyteller"@en ;
	reg:status status:1001 ;
	a rdf:Property ;
	rdfs:isDefinedBy <http://rdaregistry.info/Elements/u/> ;
	rdfs:label "has storyteller"@en ;
	rdfs:subPropertyOf <http://rdaregistry.info/Elements/u/P60387> ;
	owl:inverseOf <http://rdaregistry.info/Elements/u/P60029> ;
	owl:sameAs <http://rdaregistry.info/Elements/u/storyteller> ;
	skos:closeMatch "http://id.loc.gov/vocabulary/relators/stl"@en ;
	skos:definition "Relates a resource to a performer contributing to a resource by relaying a creator’s original story with dramatic or theatrical interpretation."@en .

<http://rdaregistry.info/Elements/u/P60155> reg:hasSubproperty <http://rdaregistry.info/Elements/e/P20024> ;
	reg:name "speaker"@en ;
	reg:status status:1001 ;
	a rdf:Property ;
	rdfs:isDefinedBy <http://rdaregistry.info/Elements/u/> ;
	rdfs:label "has speaker"@en ;
	rdfs:subPropertyOf <http://rdaregistry.info/Elements/u/P60387> ;
	owl:inverseOf <http://rdaregistry.info/Elements/u/P60030> ;
	owl:sameAs <http://rdaregistry.info/Elements/u/speaker> ;
	skos:closeMatch "http://id.loc.gov/vocabulary/relators/spk"@en ;
	skos:definition "Relates a resource to a performer contributing to a resource by speaking words, such as a lecture, speech, etc."@en .

<http://rdaregistry.info/Elements/u/P60156> reg:hasSubproperty <http://rdaregistry.info/Elements/e/P20025> ;
	reg:name "singer"@en ;
	reg:status status:1001 ;
	a rdf:Property ;
	rdfs:isDefinedBy <http://rdaregistry.info/Elements/u/> ;
	rdfs:label "has singer"@en ;
	rdfs:subPropertyOf <http://rdaregistry.info/Elements/u/P60387> ;
	owl:inverseOf <http://rdaregistry.info/Elements/u/P60031> ;
	owl:sameAs <http://rdaregistry.info/Elements/u/singer> ;
	skos:closeMatch "http://id.loc.gov/vocabulary/relators/sng"@en ;
	skos:definition "Relates a resource to a performer contributing to a resource by using his/her/their voice, with or without instrumental accompaniment, to produce music. a singer’s performance may or may not include actual words."@en .

<http://rdaregistry.info/Elements/u/P60157> reg:hasSubproperty <http://rdaregistry.info/Elements/w/P10036> ;
	reg:name "medium"@en ;
	reg:status status:1001 ;
	a rdf:Property ;
	rdfs:isDefinedBy <http://rdaregistry.info/Elements/u/> ;
	rdfs:label "has medium"@en ;
	rdfs:subPropertyOf <http://rdaregistry.info/Elements/u/P60374> ;
	owl:inverseOf <http://rdaregistry.info/Elements/u/P60032> ;
	owl:sameAs <http://rdaregistry.info/Elements/u/medium> ;
	skos:closeMatch "http://id.loc.gov/vocabulary/relators/med"@en ;
	skos:definition "Relates a resource to a person held to be a channel of communication between the earthly world and a world of spirits."@en .

<http://rdaregistry.info/Elements/u/P60158> reg:status status:1008 ;
	rdfs:isDefinedBy <http://rdaregistry.info/Elements/u/> .

<http://rdaregistry.info/Elements/u/P60159> reg:hasSubproperty <http://rdaregistry.info/Elements/m/P30084> , <http://rdaregistry.info/Elements/u/P60344> ;
	reg:name "appliedMaterial"@en ;
	reg:status status:1001 ;
	a rdf:Property ;
	rdfs:isDefinedBy <http://rdaregistry.info/Elements/u/> ;
	rdfs:label "has applied material"@en ;
	owl:sameAs <http://rdaregistry.info/Elements/u/appliedMaterial> ;
	skos:definition "Relates a resource to a physical or chemical substance applied to a base material of a resource."@en .

<http://rdaregistry.info/Elements/u/P60160> reg:hasSubproperty <http://rdaregistry.info/Elements/m/P30085> ;
	reg:name "placeOfDistribution"@en ;
	reg:status status:1001 ;
	a rdf:Property ;
	rdfs:isDefinedBy <http://rdaregistry.info/Elements/u/> ;
	rdfs:label "has place of distribution"@en ;
	owl:sameAs <http://rdaregistry.info/Elements/u/placeOfDistribution> ;
	skos:definition "Relates a resource to a place associated with the distribution of a resource in a published form."@en .

<http://rdaregistry.info/Elements/u/P60161> reg:hasSubproperty <http://rdaregistry.info/Elements/m/P30086> ;
	reg:name "placeOfProduction"@en ;
	reg:status status:1001 ;
	a rdf:Property ;
	rdfs:isDefinedBy <http://rdaregistry.info/Elements/u/> ;
	rdfs:label "has place of production"@en ;
	owl:sameAs <http://rdaregistry.info/Elements/u/placeOfProduction> ;
	skos:definition "Relates a resource to a place associated with the inscription, fabrication, construction, etc., of a resource in an unpublished form."@en .

<http://rdaregistry.info/Elements/u/P60162> reg:hasSubproperty <http://rdaregistry.info/Elements/m/P30087> ;
	reg:name "placeOfManufacture"@en ;
	reg:status status:1001 ;
	a rdf:Property ;
	rdfs:isDefinedBy <http://rdaregistry.info/Elements/u/> ;
	rdfs:label "has place of manufacture"@en ;
	owl:sameAs <http://rdaregistry.info/Elements/u/placeOfManufacture> ;
	skos:definition "Relates a resource to a place associated with the printing, duplicating, casting, etc., of a resource in a published form."@en .

<http://rdaregistry.info/Elements/u/P60163> reg:hasSubproperty <http://rdaregistry.info/Elements/m/P30088> ;
	reg:name "placeOfPublication"@en ;
	reg:status status:1001 ;
	a rdf:Property ;
	rdfs:isDefinedBy <http://rdaregistry.info/Elements/u/> ;
	rdfs:label "has place of publication"@en ;
	owl:sameAs <http://rdaregistry.info/Elements/u/placeOfPublication> ;
	skos:definition "Relates a resource to a place associated with the publication, release, or issuing of a resource."@en .

<http://rdaregistry.info/Elements/u/P60164> reg:hasSubproperty <http://rdaregistry.info/Elements/m/P30089> ;
	reg:name "parallelPlaceOfDistribution"@en ;
	reg:status status:1001 ;
	a rdf:Property ;
	rdfs:isDefinedBy <http://rdaregistry.info/Elements/u/> ;
	rdfs:label "has parallel place of distribution"@en ;
	owl:sameAs <http://rdaregistry.info/Elements/u/parallelPlaceOfDistribution> ;
	skos:definition "Relates a resource to a place of distribution in a language and/or script that differs from that recorded in the place of distribution element."@en .

<http://rdaregistry.info/Elements/u/P60165> reg:hasSubproperty <http://rdaregistry.info/Elements/m/P30090> ;
	reg:name "parallelPlaceOfManufacture"@en ;
	reg:status status:1001 ;
	a rdf:Property ;
	rdfs:isDefinedBy <http://rdaregistry.info/Elements/u/> ;
	rdfs:label "has parallel place of manufacture"@en ;
	owl:sameAs <http://rdaregistry.info/Elements/u/parallelPlaceOfManufacture> ;
	skos:definition "Relates a resource to a place of manufacture in a language and/or script that differs from that recorded in the place of manufacture element."@en .

<http://rdaregistry.info/Elements/u/P60166> reg:hasSubproperty <http://rdaregistry.info/Elements/m/P30091> ;
	reg:name "parallelPlaceOfProduction"@en ;
	reg:status status:1001 ;
	a rdf:Property ;
	rdfs:isDefinedBy <http://rdaregistry.info/Elements/u/> ;
	rdfs:label "has parallel place of production"@en ;
	owl:sameAs <http://rdaregistry.info/Elements/u/parallelPlaceOfProduction> ;
	skos:definition "Relates a resource to a place of production in a language and/or script that differs from that recorded in the place of production element."@en .

<http://rdaregistry.info/Elements/u/P60167> reg:hasSubproperty <http://rdaregistry.info/Elements/m/P30092> ;
	reg:name "parallelPlaceOfPublication"@en ;
	reg:status status:1001 ;
	a rdf:Property ;
	rdfs:isDefinedBy <http://rdaregistry.info/Elements/u/> ;
	rdfs:label "has parallel place of publication"@en ;
	owl:sameAs <http://rdaregistry.info/Elements/u/parallelPlaceOfPublication> ;
	skos:definition "Relates a resource to a place of publication in a language and/or script that differs from that recorded in the place of publication element."@en .

<http://rdaregistry.info/Elements/u/P60168> reg:hasSubproperty <http://rdaregistry.info/Elements/i/P40038> , <http://rdaregistry.info/Elements/m/P30093> ;
	reg:name "reprintOf"@en ;
	reg:status status:1001 ;
	a rdf:Property ;
	rdfs:isDefinedBy <http://rdaregistry.info/Elements/u/> ;
	rdfs:label "is reprint of"@en ;
	rdfs:subPropertyOf <http://rdaregistry.info/Elements/u/P60297> ;
	owl:inverseOf <http://rdaregistry.info/Elements/u/P60271> ;
	owl:sameAs <http://rdaregistry.info/Elements/u/reprintOf> ;
	skos:definition "Relates a resource to a printed resource that is used as the basis for a reissue with the same content as the resource being described."@en .

<http://rdaregistry.info/Elements/u/P60169> reg:hasSubproperty <http://rdaregistry.info/Elements/w/P10073> ;
	reg:name "filmProducer"@en ;
	reg:status status:1001 ;
	a rdf:Property ;
	rdfs:isDefinedBy <http://rdaregistry.info/Elements/u/> ;
	rdfs:label "has film producer"@en ;
	rdfs:subPropertyOf <http://rdaregistry.info/Elements/u/P60441> ;
	owl:inverseOf <http://rdaregistry.info/Elements/u/P60033> ;
	owl:sameAs <http://rdaregistry.info/Elements/u/filmProducer> ;
	skos:closeMatch "http://id.loc.gov/vocabulary/relators/fmp"@en ;
	skos:definition "Relates a resource to a producer responsible for most of the business aspects of a film."@en .

<http://rdaregistry.info/Elements/u/P60170> reg:hasSubproperty <http://rdaregistry.info/Elements/w/P10074> ;
	reg:name "radioProducer"@en ;
	reg:status status:1001 ;
	a rdf:Property ;
	rdfs:isDefinedBy <http://rdaregistry.info/Elements/u/> ;
	rdfs:label "has radio producer"@en ;
	rdfs:subPropertyOf <http://rdaregistry.info/Elements/u/P60441> ;
	owl:inverseOf <http://rdaregistry.info/Elements/u/P60034> ;
	owl:sameAs <http://rdaregistry.info/Elements/u/radioProducer> ;
	skos:closeMatch "http://id.loc.gov/vocabulary/relators/rpc"@en ;
	skos:definition "Relates a resource to a producer responsible for most of the business aspects of a radio program."@en .

<http://rdaregistry.info/Elements/u/P60171> reg:hasSubproperty <http://rdaregistry.info/Elements/w/P10075> ;
	reg:name "televisionProducer"@en ;
	reg:status status:1001 ;
	a rdf:Property ;
	rdfs:isDefinedBy <http://rdaregistry.info/Elements/u/> ;
	rdfs:label "has television producer"@en ;
	rdfs:subPropertyOf <http://rdaregistry.info/Elements/u/P60441> ;
	owl:inverseOf <http://rdaregistry.info/Elements/u/P60035> ;
	owl:sameAs <http://rdaregistry.info/Elements/u/televisionProducer> ;
	skos:closeMatch "http://id.loc.gov/vocabulary/relators/tlp"@en ;
	skos:definition "Relates a resource to a producer responsible for most of the business aspects of a television program."@en .

<http://rdaregistry.info/Elements/u/P60172> reg:hasSubproperty <http://rdaregistry.info/Elements/m/P30094> ;
	reg:name "parallelProducersName"@en ;
	reg:status status:1001 ;
	a rdf:Property ;
	rdfs:isDefinedBy <http://rdaregistry.info/Elements/u/> ;
	rdfs:label "has parallel producer's name"@en ;
	owl:sameAs <http://rdaregistry.info/Elements/u/parallelProducersName> ;
	skos:definition "Relates a resource to a producer’s name in a language and/or script that differs from that recorded in the producer’s name element."@en .

<http://rdaregistry.info/Elements/u/P60173> reg:hasSubproperty <http://rdaregistry.info/Elements/m/P30095> ;
	reg:name "parallelPublishersName"@en ;
	reg:status status:1001 ;
	a rdf:Property ;
	rdfs:isDefinedBy <http://rdaregistry.info/Elements/u/> ;
	rdfs:label "has parallel publisher's name"@en ;
	owl:sameAs <http://rdaregistry.info/Elements/u/parallelPublishersName> ;
	skos:definition "Relates a resource to a publisher’s name in a language and/or script that differs from that recorded in the publisher’s name element."@en .

<http://rdaregistry.info/Elements/u/P60174> reg:hasSubproperty <http://rdaregistry.info/Elements/e/P20060> , <http://rdaregistry.info/Elements/w/P10076> ;
	reg:name "adaptedAsARadioProgram"@en ;
	reg:status status:1001 ;
	a rdf:Property ;
	rdfs:isDefinedBy <http://rdaregistry.info/Elements/u/> ;
	rdfs:label "is adapted as radio program"@en ;
	rdfs:subPropertyOf <http://rdaregistry.info/Elements/u/P60260> ;
	owl:inverseOf <http://rdaregistry.info/Elements/u/P60229> ;
	owl:sameAs <http://rdaregistry.info/Elements/u/adaptedAsARadioProgram> ;
	skos:definition "Relates a resource to a radio program based on the source resource."@en .

<http://rdaregistry.info/Elements/u/P60175> reg:hasSubproperty <http://rdaregistry.info/Elements/w/P10077> ;
	reg:name "academicDegree"@en ;
	reg:status status:1001 ;
	a rdf:Property ;
	rdfs:isDefinedBy <http://rdaregistry.info/Elements/u/> ;
	rdfs:label "has academic degree"@en ;
	owl:sameAs <http://rdaregistry.info/Elements/u/academicDegree> ;
	skos:definition "Relates a resource to a rank conferred as a guarantee of academic proficiency."@en .

<http://rdaregistry.info/Elements/u/P60176> reg:hasSubproperty <http://rdaregistry.info/Elements/i/P40026> ;
	reg:name "custodialHistoryOfResource"@en ;
	reg:status status:1001 ;
	a rdf:Property ;
	rdfs:isDefinedBy <http://rdaregistry.info/Elements/u/> ;
	rdfs:label "has custodial history of resource"@en ;
	owl:sameAs <http://rdaregistry.info/Elements/u/custodialHistoryOfResource> ;
	skos:definition "Relates a resource to a record of previous ownership or custodianship of a resource."@en .

<http://rdaregistry.info/Elements/u/P60177> reg:hasSubproperty <http://rdaregistry.info/Elements/e/P20090> , <http://rdaregistry.info/Elements/w/P10089> ;
	reg:name "abstractedIn"@en ;
	reg:status status:1001 ;
	a rdf:Property ;
	rdfs:isDefinedBy <http://rdaregistry.info/Elements/u/> ;
	rdfs:label "is abstracted in"@en ;
	rdfs:subPropertyOf <http://rdaregistry.info/Elements/u/P60250> ;
	owl:inverseOf <http://rdaregistry.info/Elements/u/P60308> ;
	owl:sameAs <http://rdaregistry.info/Elements/u/abstractedIn> ;
	skos:definition "Relates a resource to a resource (an abstracting and indexing service) that abstracts the contents of a source resource."@en .

<http://rdaregistry.info/Elements/u/P60178> reg:hasSubproperty <http://rdaregistry.info/Elements/e/P20091> , <http://rdaregistry.info/Elements/w/P10090> ;
	reg:name "indexedIn"@en ;
	reg:status status:1001 ;
	a rdf:Property ;
	rdfs:isDefinedBy <http://rdaregistry.info/Elements/u/> ;
	rdfs:label "is indexed in"@en ;
	rdfs:subPropertyOf <http://rdaregistry.info/Elements/u/P60250> ;
	owl:inverseOf <http://rdaregistry.info/Elements/u/P60309> ;
	owl:sameAs <http://rdaregistry.info/Elements/u/indexedIn> ;
	skos:definition "Relates a resource to a resource (an abstracting and indexing service) that indexes the contents of the source resource."@en .

<http://rdaregistry.info/Elements/u/P60179> reg:hasSubproperty <http://rdaregistry.info/Elements/m/P30021> ;
	reg:name "preservationFacsimile"@en ;
	reg:status status:1001 ;
	a rdf:Property ;
	rdfs:isDefinedBy <http://rdaregistry.info/Elements/u/> ;
	rdfs:label "is preservation facsimile"@en ;
	rdfs:subPropertyOf <http://rdaregistry.info/Elements/u/P60217> ;
	owl:inverseOf <http://rdaregistry.info/Elements/u/P60299> ;
	owl:sameAs <http://rdaregistry.info/Elements/u/preservationFacsimile> ;
	skos:definition "Relates a resource to a resource consisting of an exact reproduction on preservation-quality media, such as acid-free permanent or archival paper."@en .

<http://rdaregistry.info/Elements/u/P60180> reg:hasSubproperty <http://rdaregistry.info/Elements/e/P20092> , <http://rdaregistry.info/Elements/w/P10091> ;
	reg:name "choreography"@en ;
	reg:status status:1001 ;
	a rdf:Property ;
	rdfs:isDefinedBy <http://rdaregistry.info/Elements/u/> ;
	rdfs:label "is choreography"@en ;
	rdfs:subPropertyOf <http://rdaregistry.info/Elements/u/P60250> ;
	owl:inverseOf <http://rdaregistry.info/Elements/u/P60293> ;
	owl:sameAs <http://rdaregistry.info/Elements/u/choreography> ;
	skos:definition "Relates a resource to a resource consisting of dance based on the source resource."@en .

<http://rdaregistry.info/Elements/u/P60181> reg:hasSubproperty <http://rdaregistry.info/Elements/e/P20093> , <http://rdaregistry.info/Elements/w/P10092> ;
	reg:name "errata"@en ;
	reg:status status:1001 ;
	a rdf:Property ;
	rdfs:isDefinedBy <http://rdaregistry.info/Elements/u/> ;
	rdfs:label "is errata"@en ;
	rdfs:subPropertyOf <http://rdaregistry.info/Elements/u/P60204> ;
	owl:inverseOf <http://rdaregistry.info/Elements/u/P60251> ;
	owl:sameAs <http://rdaregistry.info/Elements/u/errata> ;
	skos:definition "Relates a resource to a resource consisting of errors discovered after the publication of the predominant resource, with their corrections."@en .

<http://rdaregistry.info/Elements/u/P60182> reg:hasSubproperty <http://rdaregistry.info/Elements/e/P20094> , <http://rdaregistry.info/Elements/w/P10093> ;
	reg:name "illustrations"@en ;
	reg:status status:1001 ;
	a rdf:Property ;
	rdfs:isDefinedBy <http://rdaregistry.info/Elements/u/> ;
	rdfs:label "is illustrations"@en ;
	rdfs:subPropertyOf <http://rdaregistry.info/Elements/u/P60204> ;
	owl:inverseOf <http://rdaregistry.info/Elements/u/P60254> ;
	owl:sameAs <http://rdaregistry.info/Elements/u/illustrations> ;
	skos:definition "Relates a resource to a resource consisting of pictorial content designed to explain or decorate the augmented resource."@en .

<http://rdaregistry.info/Elements/u/P60183> reg:hasSubproperty <http://rdaregistry.info/Elements/m/P30022> ;
	reg:name "insert"@en ;
	reg:status status:1001 ;
	a rdf:Property ;
	rdfs:isDefinedBy <http://rdaregistry.info/Elements/u/> ;
	rdfs:label "is insert"@en ;
	rdfs:subPropertyOf <http://rdaregistry.info/Elements/u/P60249> ;
	owl:inverseOf <http://rdaregistry.info/Elements/u/P60194> ;
	owl:sameAs <http://rdaregistry.info/Elements/u/insert> ;
	skos:definition "Relates a resource to a resource consisting of separately issued material that is not an integral part of the larger resource into which it has been inserted."@en .

<http://rdaregistry.info/Elements/u/P60184> reg:hasSubproperty <http://rdaregistry.info/Elements/e/P20095> , <http://rdaregistry.info/Elements/w/P10094> ;
	reg:name "adaptedAsAMotionPictureScreenplay"@en ;
	reg:status status:1001 ;
	a rdf:Property ;
	rdfs:isDefinedBy <http://rdaregistry.info/Elements/u/> ;
	rdfs:label "is adapted as motion picture screenplay"@en ;
	rdfs:subPropertyOf <http://rdaregistry.info/Elements/u/P60185> ;
	owl:inverseOf <http://rdaregistry.info/Elements/u/P60232> ;
	owl:sameAs <http://rdaregistry.info/Elements/u/adaptedAsAMotionPictureScreenplay> ;
	skos:definition "Relates a resource to a resource consisting of the screenplay for a motion picture, based on the source resource."@en .

<http://rdaregistry.info/Elements/u/P60185> reg:hasSubproperty <http://rdaregistry.info/Elements/e/P20096> , <http://rdaregistry.info/Elements/u/P60184> , <http://rdaregistry.info/Elements/u/P60186> , <http://rdaregistry.info/Elements/u/P60187> , <http://rdaregistry.info/Elements/w/P10095> ;
	reg:name "adaptedAsAScreenplay"@en ;
	reg:status status:1001 ;
	a rdf:Property ;
	rdfs:isDefinedBy <http://rdaregistry.info/Elements/u/> ;
	rdfs:label "is adapted as screenplay"@en ;
	rdfs:subPropertyOf <http://rdaregistry.info/Elements/u/P60260> ;
	owl:inverseOf <http://rdaregistry.info/Elements/u/P60231> ;
	owl:sameAs <http://rdaregistry.info/Elements/u/adaptedAsAScreenplay> ;
	skos:definition "Relates a resource to a resource consisting of the screenplay for a motion picture, television program, or video, based on the source resource."@en .

<http://rdaregistry.info/Elements/u/P60186> reg:hasSubproperty <http://rdaregistry.info/Elements/e/P20097> , <http://rdaregistry.info/Elements/w/P10096> ;
	reg:name "adaptedAsATelevisionScreenplay"@en ;
	reg:status status:1001 ;
	a rdf:Property ;
	rdfs:isDefinedBy <http://rdaregistry.info/Elements/u/> ;
	rdfs:label "is adapted as television screenplay"@en ;
	rdfs:subPropertyOf <http://rdaregistry.info/Elements/u/P60185> ;
	owl:inverseOf <http://rdaregistry.info/Elements/u/P60233> ;
	owl:sameAs <http://rdaregistry.info/Elements/u/adaptedAsATelevisionScreenplay> ;
	skos:definition "Relates a resource to a resource consisting of the screenplay for a television program, based on the source resource."@en .

<http://rdaregistry.info/Elements/u/P60187> reg:hasSubproperty <http://rdaregistry.info/Elements/e/P20098> , <http://rdaregistry.info/Elements/w/P10097> ;
	reg:name "adaptedAsAVideoScreenplay"@en ;
	reg:status status:1001 ;
	a rdf:Property ;
	rdfs:isDefinedBy <http://rdaregistry.info/Elements/u/> ;
	rdfs:label "is adapted as video screenplay"@en ;
	rdfs:subPropertyOf <http://rdaregistry.info/Elements/u/P60185> ;
	owl:inverseOf <http://rdaregistry.info/Elements/u/P60234> ;
	owl:sameAs <http://rdaregistry.info/Elements/u/adaptedAsAVideoScreenplay> ;
	skos:definition "Relates a resource to a resource consisting of the screenplay for a video, based on the source resource."@en .

<http://rdaregistry.info/Elements/u/P60188> reg:hasSubproperty <http://rdaregistry.info/Elements/e/P20099> , <http://rdaregistry.info/Elements/w/P10098> ;
	reg:name "adaptedAsARadioScript"@en ;
	reg:status status:1001 ;
	a rdf:Property ;
	rdfs:isDefinedBy <http://rdaregistry.info/Elements/u/> ;
	rdfs:label "is adapted as radio script"@en ;
	rdfs:subPropertyOf <http://rdaregistry.info/Elements/u/P60260> ;
	owl:inverseOf <http://rdaregistry.info/Elements/u/P60235> ;
	owl:sameAs <http://rdaregistry.info/Elements/u/adaptedAsARadioScript> ;
	skos:definition "Relates a resource to a resource consisting of the script for a radio program, based on the source resource."@en .

<http://rdaregistry.info/Elements/u/P60189> reg:hasSubproperty <http://rdaregistry.info/Elements/e/P20119> , <http://rdaregistry.info/Elements/w/P10099> ;
	reg:name "freelyTranslatedAs"@en ;
	reg:status status:1001 ;
	a rdf:Property ;
	rdfs:isDefinedBy <http://rdaregistry.info/Elements/u/> ;
	rdfs:label "is freely translated as"@en ;
	rdfs:subPropertyOf <http://rdaregistry.info/Elements/u/P60250> ;
	owl:inverseOf <http://rdaregistry.info/Elements/u/P60243> ;
	owl:sameAs <http://rdaregistry.info/Elements/u/freelyTranslatedAs> ;
	skos:definition "Relates a resource to a resource created by freely translating the source resource into another language, preserving the spirit of the original, but not its linguistic details."@en .

<http://rdaregistry.info/Elements/u/P60190> reg:hasSubproperty <http://rdaregistry.info/Elements/e/P20072> , <http://rdaregistry.info/Elements/i/P40030> , <http://rdaregistry.info/Elements/m/P30023> , <http://rdaregistry.info/Elements/u/P60239> , <http://rdaregistry.info/Elements/u/P60255> , <http://rdaregistry.info/Elements/u/P60288> , <http://rdaregistry.info/Elements/u/P60292> , <http://rdaregistry.info/Elements/u/P60298> , <http://rdaregistry.info/Elements/w/P10100> ;
	reg:name "descriptionOf"@en ;
	reg:status status:1001 ;
	a rdf:Property ;
	rdfs:isDefinedBy <http://rdaregistry.info/Elements/u/> ;
	rdfs:label "is description of"@en ;
	rdfs:subPropertyOf <http://rdaregistry.info/Elements/u/P60711> ;
	owl:inverseOf <http://rdaregistry.info/Elements/u/P60215> ;
	owl:sameAs <http://rdaregistry.info/Elements/u/descriptionOf> ;
	skos:definition "Relates a resource to a resource described by a describing resource."@en .

<http://rdaregistry.info/Elements/u/P60191> reg:hasSubproperty <http://rdaregistry.info/Elements/i/P40031> , <http://rdaregistry.info/Elements/m/P30024> , <http://rdaregistry.info/Elements/u/P60195> , <http://rdaregistry.info/Elements/u/P60197> , <http://rdaregistry.info/Elements/u/P60272> , <http://rdaregistry.info/Elements/u/P60297> ;
	reg:name "equivalent"@en ;
	reg:status status:1001 ;
	a rdf:Property ;
	rdfs:isDefinedBy <http://rdaregistry.info/Elements/u/> ;
	rdfs:label "is equivalent"@en ;
	rdfs:subPropertyOf <http://rdaregistry.info/Elements/u/P60712> ;
	owl:inverseOf <http://rdaregistry.info/Elements/u/P60191> ;
	owl:sameAs <http://rdaregistry.info/Elements/u/equivalent> ;
	skos:definition "Relates a resource to a resource embodying the resource."@en .

<http://rdaregistry.info/Elements/u/P60192> reg:hasSubproperty <http://rdaregistry.info/Elements/w/P10101> ;
	reg:name "subseriesOf"@en ;
	reg:status status:1001 ;
	a rdf:Property ;
	rdfs:isDefinedBy <http://rdaregistry.info/Elements/u/> ;
	rdfs:label "is subseries of"@en ;
	rdfs:subPropertyOf <http://rdaregistry.info/Elements/u/P60101> ;
	owl:inverseOf <http://rdaregistry.info/Elements/u/P60316> ;
	owl:sameAs <http://rdaregistry.info/Elements/u/subseriesOf> ;
	skos:definition "Relates a resource to a resource in which the part consistently appears; the title of the larger resource appears on all issues or parts of the subseries."@en .

<http://rdaregistry.info/Elements/u/P60193> reg:hasSubproperty <http://rdaregistry.info/Elements/w/P10102> ;
	reg:name "inSeries"@en ;
	reg:status status:1001 ;
	a rdf:Property ;
	rdfs:isDefinedBy <http://rdaregistry.info/Elements/u/> ;
	rdfs:label "is in series"@en ;
	rdfs:subPropertyOf <http://rdaregistry.info/Elements/u/P60101> ;
	owl:inverseOf <http://rdaregistry.info/Elements/u/P60240> ;
	owl:sameAs <http://rdaregistry.info/Elements/u/inSeries> ;
	skos:definition "Relates a resource to a resource in which the part has been issued; the title of the larger resource appears on the part."@en .

<http://rdaregistry.info/Elements/u/P60194> reg:hasSubproperty <http://rdaregistry.info/Elements/m/P30025> ;
	reg:name "insertedIn"@en ;
	reg:status status:1001 ;
	a rdf:Property ;
	rdfs:isDefinedBy <http://rdaregistry.info/Elements/u/> ;
	rdfs:label "is inserted in"@en ;
	rdfs:subPropertyOf <http://rdaregistry.info/Elements/u/P60101> ;
	owl:inverseOf <http://rdaregistry.info/Elements/u/P60183> ;
	owl:sameAs <http://rdaregistry.info/Elements/u/insertedIn> ;
	skos:definition "Relates a resource to a resource into which material has been inserted that is not an integral part of the publication."@en .

<http://rdaregistry.info/Elements/u/P60195> reg:hasSubproperty <http://rdaregistry.info/Elements/m/P30026> ;
	reg:name "alsoIssuedAs"@en ;
	reg:status status:1001 ;
	a rdf:Property ;
	rdfs:isDefinedBy <http://rdaregistry.info/Elements/u/> ;
	rdfs:label "is also issued as"@en ;
	rdfs:subPropertyOf <http://rdaregistry.info/Elements/u/P60191> ;
	owl:inverseOf <http://rdaregistry.info/Elements/u/P60195> ;
	owl:sameAs <http://rdaregistry.info/Elements/u/alsoIssuedAs> ;
	skos:definition "Relates a resource to a resource issued in a different format embodying the resource being described."@en .

<http://rdaregistry.info/Elements/u/P60196> reg:hasSubproperty <http://rdaregistry.info/Elements/i/P40029> , <http://rdaregistry.info/Elements/m/P30027> , <http://rdaregistry.info/Elements/u/P60237> , <http://rdaregistry.info/Elements/u/P60256> ;
	reg:name "accompaniedBy"@en ;
	reg:status status:1001 ;
	a rdf:Property ;
	rdfs:isDefinedBy <http://rdaregistry.info/Elements/u/> ;
	rdfs:label "is accompanied by"@en ;
	rdfs:subPropertyOf <http://rdaregistry.info/Elements/u/P60709> ;
	owl:inverseOf <http://rdaregistry.info/Elements/u/P60196> ;
	owl:sameAs <http://rdaregistry.info/Elements/u/accompaniedBy> ;
	skos:definition "Relates a resource to a resource issued with another resource, without any relationship to its content."@en .

<http://rdaregistry.info/Elements/u/P60197> reg:hasSubproperty <http://rdaregistry.info/Elements/m/P30028> ;
	reg:name "mirrorSite"@en ;
	reg:status status:1001 ;
	a rdf:Property ;
	rdfs:isDefinedBy <http://rdaregistry.info/Elements/u/> ;
	rdfs:label "is mirror site"@en ;
	rdfs:subPropertyOf <http://rdaregistry.info/Elements/u/P60191> ;
	owl:inverseOf <http://rdaregistry.info/Elements/u/P60197> ;
	owl:sameAs <http://rdaregistry.info/Elements/u/mirrorSite> ;
	skos:definition "Relates a resource to a resource of a website that is an exact copy, used to reduce network traffic or improve the availability of the original site."@en .

<http://rdaregistry.info/Elements/u/P60198> reg:hasSubproperty <http://rdaregistry.info/Elements/e/P20100> , <http://rdaregistry.info/Elements/u/P60117> , <http://rdaregistry.info/Elements/u/P60201> , <http://rdaregistry.info/Elements/u/P60264> , <http://rdaregistry.info/Elements/u/P60267> , <http://rdaregistry.info/Elements/u/P60270> , <http://rdaregistry.info/Elements/u/P60285> , <http://rdaregistry.info/Elements/w/P10103> ;
	reg:name "complementedBy"@en ;
	reg:status status:1001 ;
	a rdf:Property ;
	rdfs:isDefinedBy <http://rdaregistry.info/Elements/u/> ;
	rdfs:label "is complemented by"@en ;
	rdfs:subPropertyOf <http://rdaregistry.info/Elements/u/P60709> ;
	owl:inverseOf <http://rdaregistry.info/Elements/u/P60198> ;
	owl:sameAs <http://rdaregistry.info/Elements/u/complementedBy> ;
	skos:definition "Relates a resource to a resource paired with another resource without either resource being considered to predominate."@en .

<http://rdaregistry.info/Elements/u/P60199> reg:hasSubproperty <http://rdaregistry.info/Elements/e/P20101> , <http://rdaregistry.info/Elements/w/P10104> ;
	reg:name "continuedInPartBy"@en ;
	reg:status status:1001 ;
	a rdf:Property ;
	rdfs:isDefinedBy <http://rdaregistry.info/Elements/u/> ;
	rdfs:label "is continued in part by"@en ;
	rdfs:subPropertyOf <http://rdaregistry.info/Elements/u/P60278> ;
	owl:inverseOf <http://rdaregistry.info/Elements/u/P60277> ;
	owl:sameAs <http://rdaregistry.info/Elements/u/continuedInPartBy> ;
	skos:definition "Relates a resource to a resource part of whose content separated from an earlier resource to form a new resource."@en .

<http://rdaregistry.info/Elements/u/P60200> reg:hasSubproperty <http://rdaregistry.info/Elements/m/P30029> ;
	reg:name "digitalTransfer"@en ;
	reg:status status:1001 ;
	a rdf:Property ;
	rdfs:isDefinedBy <http://rdaregistry.info/Elements/u/> ;
	rdfs:label "is digital transfer"@en ;
	rdfs:subPropertyOf <http://rdaregistry.info/Elements/u/P60272> ;
	owl:inverseOf <http://rdaregistry.info/Elements/u/P60287> ;
	owl:sameAs <http://rdaregistry.info/Elements/u/digitalTransfer> ;
	skos:definition "Relates a resource to a resource resulting from the transfer of a resource from one digital format to another."@en .

<http://rdaregistry.info/Elements/u/P60201> reg:hasSubproperty <http://rdaregistry.info/Elements/e/P20102> , <http://rdaregistry.info/Elements/u/P60282> , <http://rdaregistry.info/Elements/u/P60283> , <http://rdaregistry.info/Elements/u/P60284> , <http://rdaregistry.info/Elements/w/P10105> ;
	reg:name "screenplayFor"@en ;
	reg:status status:1001 ;
	a rdf:Property ;
	rdfs:isDefinedBy <http://rdaregistry.info/Elements/u/> ;
	rdfs:label "is screenplay for"@en ;
	rdfs:subPropertyOf <http://rdaregistry.info/Elements/u/P60198> ;
	owl:inverseOf <http://rdaregistry.info/Elements/u/P60264> ;
	owl:sameAs <http://rdaregistry.info/Elements/u/screenplayFor> ;
	skos:definition "Relates a resource to a resource such as a motion picture, television program, or video, that uses the text of the resource as a screenplay."@en .

<http://rdaregistry.info/Elements/u/P60202> reg:hasSubproperty <http://rdaregistry.info/Elements/e/P20103> , <http://rdaregistry.info/Elements/w/P10106> ;
	reg:name "incidentalMusicFor"@en ;
	reg:status status:1001 ;
	a rdf:Property ;
	rdfs:isDefinedBy <http://rdaregistry.info/Elements/u/> ;
	rdfs:label "is incidental music for"@en ;
	rdfs:subPropertyOf <http://rdaregistry.info/Elements/u/P60724> ;
	owl:inverseOf <http://rdaregistry.info/Elements/u/P60118> ;
	owl:sameAs <http://rdaregistry.info/Elements/u/incidentalMusicFor> ;
	skos:definition "Relates a resource to a resource such as a play or other spoken work for the stage that uses the musical resource as incidental music."@en .

<http://rdaregistry.info/Elements/u/P60203> reg:hasSubproperty <http://rdaregistry.info/Elements/e/P20104> , <http://rdaregistry.info/Elements/w/P10107> ;
	reg:name "abstract"@en ;
	reg:status status:1001 ;
	a rdf:Property ;
	rdfs:isDefinedBy <http://rdaregistry.info/Elements/u/> ;
	rdfs:label "is abstract"@en ;
	rdfs:subPropertyOf <http://rdaregistry.info/Elements/u/P60250> ;
	owl:inverseOf <http://rdaregistry.info/Elements/u/P60224> ;
	owl:sameAs <http://rdaregistry.info/Elements/u/abstract> ;
	skos:definition "Relates a resource to a resource that abbreviates the source resource in a brief, objective manner."@en .

<http://rdaregistry.info/Elements/u/P60204> reg:hasSubproperty <http://rdaregistry.info/Elements/e/P20105> , <http://rdaregistry.info/Elements/u/P60113> , <http://rdaregistry.info/Elements/u/P60181> , <http://rdaregistry.info/Elements/u/P60182> , <http://rdaregistry.info/Elements/u/P60206> , <http://rdaregistry.info/Elements/u/P60208> , <http://rdaregistry.info/Elements/u/P60209> , <http://rdaregistry.info/Elements/u/P60221> , <http://rdaregistry.info/Elements/u/P60222> , <http://rdaregistry.info/Elements/u/P60262> , <http://rdaregistry.info/Elements/u/P60263> , <http://rdaregistry.info/Elements/u/P60281> , <http://rdaregistry.info/Elements/w/P10108> ;
	reg:name "augmentedBy"@en ;
	reg:status status:1001 ;
	a rdf:Property ;
	rdfs:isDefinedBy <http://rdaregistry.info/Elements/u/> ;
	rdfs:label "is augmented by"@en ;
	rdfs:subPropertyOf <http://rdaregistry.info/Elements/u/P60709> ;
	owl:inverseOf <http://rdaregistry.info/Elements/u/P60307> ;
	owl:sameAs <http://rdaregistry.info/Elements/u/augmentedBy> ;
	skos:definition "Relates a resource to a resource that adds to the content of a predominant resource."@en .

<http://rdaregistry.info/Elements/u/P60205> reg:hasSubproperty <http://rdaregistry.info/Elements/e/P20106> , <http://rdaregistry.info/Elements/w/P10109> ;
	reg:name "summary"@en ;
	reg:status status:1001 ;
	a rdf:Property ;
	rdfs:isDefinedBy <http://rdaregistry.info/Elements/u/> ;
	rdfs:label "is summary"@en ;
	rdfs:subPropertyOf <http://rdaregistry.info/Elements/u/P60250> ;
	owl:inverseOf <http://rdaregistry.info/Elements/u/P60289> ;
	owl:sameAs <http://rdaregistry.info/Elements/u/summary> ;
	skos:definition "Relates a resource to a resource that consists of a brief recapitulation of the content of the source resource."@en .

<http://rdaregistry.info/Elements/u/P60206> reg:hasSubproperty <http://rdaregistry.info/Elements/e/P20107> , <http://rdaregistry.info/Elements/w/P10110> ;
	reg:name "catalogue"@en ;
	reg:status status:1001 ;
	a rdf:Property ;
	rdfs:isDefinedBy <http://rdaregistry.info/Elements/u/> ;
	rdfs:label "is catalogue"@en ;
	rdfs:subPropertyOf <http://rdaregistry.info/Elements/u/P60204> ;
	owl:inverseOf <http://rdaregistry.info/Elements/u/P60290> ;
	owl:sameAs <http://rdaregistry.info/Elements/u/catalogue> ;
	skos:definition "Relates a resource to a resource that consists of a complete enumeration of resources arranged systematically."@en .

<http://rdaregistry.info/Elements/u/P60207> reg:hasSubproperty <http://rdaregistry.info/Elements/m/P30030> ;
	reg:name "specialIssue"@en ;
	reg:status status:1001 ;
	a rdf:Property ;
	rdfs:isDefinedBy <http://rdaregistry.info/Elements/u/> ;
	rdfs:label "is special issue"@en ;
	rdfs:subPropertyOf <http://rdaregistry.info/Elements/u/P60249> ;
	owl:inverseOf <http://rdaregistry.info/Elements/u/P60317> ;
	owl:sameAs <http://rdaregistry.info/Elements/u/specialIssue> ;
	skos:definition "Relates a resource to a resource that consists of a single issue or a supplementary section of a serial or newspaper devoted to a special subject."@en .

<http://rdaregistry.info/Elements/u/P60208> reg:hasSubproperty <http://rdaregistry.info/Elements/e/P20108> , <http://rdaregistry.info/Elements/w/P10111> ;
	reg:name "concordance"@en ;
	reg:status status:1001 ;
	a rdf:Property ;
	rdfs:isDefinedBy <http://rdaregistry.info/Elements/u/> ;
	rdfs:label "is concordance"@en ;
	rdfs:subPropertyOf <http://rdaregistry.info/Elements/u/P60204> ;
	owl:inverseOf <http://rdaregistry.info/Elements/u/P60291> ;
	owl:sameAs <http://rdaregistry.info/Elements/u/concordance> ;
	skos:definition "Relates a resource to a resource that consists of an index of all the words in the predominant resource."@en .

<http://rdaregistry.info/Elements/u/P60209> reg:hasSubproperty <http://rdaregistry.info/Elements/e/P20109> , <http://rdaregistry.info/Elements/w/P10112> ;
	reg:name "addenda"@en ;
	reg:status status:1001 ;
	a rdf:Property ;
	rdfs:isDefinedBy <http://rdaregistry.info/Elements/u/> ;
	rdfs:label "is addenda"@en ;
	rdfs:subPropertyOf <http://rdaregistry.info/Elements/u/P60204> ;
	owl:inverseOf <http://rdaregistry.info/Elements/u/P60286> ;
	owl:sameAs <http://rdaregistry.info/Elements/u/addenda> ;
	skos:definition "Relates a resource to a resource that consists of brief additional material, less extensive than a supplement, but essential to the completeness of the text of the predominant resource; it is usually added at the end of the content, but is sometimes issued separately."@en .

<http://rdaregistry.info/Elements/u/P60210> reg:hasSubproperty <http://rdaregistry.info/Elements/e/P20110> , <http://rdaregistry.info/Elements/w/P10113> ;
	reg:name "basisForLibretto"@en ;
	reg:status status:1001 ;
	a rdf:Property ;
	rdfs:isDefinedBy <http://rdaregistry.info/Elements/u/> ;
	rdfs:label "is basis for libretto"@en ;
	rdfs:subPropertyOf <http://rdaregistry.info/Elements/u/P60250> ;
	owl:inverseOf <http://rdaregistry.info/Elements/u/P60304> ;
	owl:sameAs <http://rdaregistry.info/Elements/u/basisForLibretto> ;
	skos:definition "Relates a resource to a resource that consists of the text of an opera or other resource for the musical stage, or an oratorio, based on the source resource."@en .

<http://rdaregistry.info/Elements/u/P60211> reg:hasSubproperty <http://rdaregistry.info/Elements/e/P20111> , <http://rdaregistry.info/Elements/w/P10114> ;
	reg:name "reviewedIn"@en ;
	reg:status status:1001 ;
	a rdf:Property ;
	rdfs:isDefinedBy <http://rdaregistry.info/Elements/u/> ;
	rdfs:label "is reviewed in"@en ;
	rdfs:subPropertyOf <http://rdaregistry.info/Elements/u/P60215> ;
	owl:inverseOf <http://rdaregistry.info/Elements/u/P60288> ;
	owl:sameAs <http://rdaregistry.info/Elements/u/reviewedIn> ;
	skos:definition "Relates a resource to a resource that contains a brief evaluation of the described resource."@en .

<http://rdaregistry.info/Elements/u/P60212> reg:hasSubproperty <http://rdaregistry.info/Elements/e/P20112> , <http://rdaregistry.info/Elements/w/P10115> ;
	reg:name "critiquedIn"@en ;
	reg:status status:1001 ;
	a rdf:Property ;
	rdfs:isDefinedBy <http://rdaregistry.info/Elements/u/> ;
	rdfs:label "is critiqued in"@en ;
	rdfs:subPropertyOf <http://rdaregistry.info/Elements/u/P60215> ;
	owl:inverseOf <http://rdaregistry.info/Elements/u/P60292> ;
	owl:sameAs <http://rdaregistry.info/Elements/u/critiquedIn> ;
	skos:definition "Relates a resource to a resource that contains a critical evaluation of the described resource."@en .

<http://rdaregistry.info/Elements/u/P60213> reg:hasSubproperty <http://rdaregistry.info/Elements/e/P20113> , <http://rdaregistry.info/Elements/w/P10116> ;
	reg:name "commentaryIn"@en ;
	reg:status status:1001 ;
	a rdf:Property ;
	rdfs:isDefinedBy <http://rdaregistry.info/Elements/u/> ;
	rdfs:label "is commentary in"@en ;
	rdfs:subPropertyOf <http://rdaregistry.info/Elements/u/P60215> ;
	owl:inverseOf <http://rdaregistry.info/Elements/u/P60298> ;
	owl:sameAs <http://rdaregistry.info/Elements/u/commentaryIn> ;
	skos:definition "Relates a resource to a resource that contains a set of explanatory or critical notes on the described resource"@en .

<http://rdaregistry.info/Elements/u/P60214> reg:hasSubproperty <http://rdaregistry.info/Elements/e/P20114> , <http://rdaregistry.info/Elements/u/P60246> , <http://rdaregistry.info/Elements/w/P10117> ;
	reg:name "imitatedAs"@en ;
	reg:status status:1001 ;
	a rdf:Property ;
	rdfs:isDefinedBy <http://rdaregistry.info/Elements/u/> ;
	rdfs:label "is imitated as"@en ;
	rdfs:subPropertyOf <http://rdaregistry.info/Elements/u/P60250> ;
	owl:inverseOf <http://rdaregistry.info/Elements/u/P60311> ;
	owl:sameAs <http://rdaregistry.info/Elements/u/imitatedAs> ;
	skos:definition "Relates a resource to a resource that copies the style or content of the source resource."@en .

<http://rdaregistry.info/Elements/u/P60215> reg:hasSubproperty <http://rdaregistry.info/Elements/e/P20202> , <http://rdaregistry.info/Elements/u/P60211> , <http://rdaregistry.info/Elements/u/P60212> , <http://rdaregistry.info/Elements/u/P60213> , <http://rdaregistry.info/Elements/u/P60218> , <http://rdaregistry.info/Elements/u/P60219> , <http://rdaregistry.info/Elements/w/P10118> ;
	reg:name "describedIn"@en ;
	reg:status status:1001 ;
	a rdf:Property ;
	rdfs:isDefinedBy <http://rdaregistry.info/Elements/u/> ;
	rdfs:label "is described in"@en ;
	rdfs:subPropertyOf <http://rdaregistry.info/Elements/u/P60711> ;
	owl:inverseOf <http://rdaregistry.info/Elements/u/P60190> ;
	owl:sameAs <http://rdaregistry.info/Elements/u/describedIn> ;
	skos:definition "Relates a resource to a resource that describes a described resource."@en .

<http://rdaregistry.info/Elements/u/P60216> reg:hasSubproperty <http://rdaregistry.info/Elements/e/P20115> , <http://rdaregistry.info/Elements/w/P10119> ;
	reg:name "expandedAs"@en ;
	reg:status status:1001 ;
	a rdf:Property ;
	rdfs:isDefinedBy <http://rdaregistry.info/Elements/u/> ;
	rdfs:label "is expanded as"@en ;
	rdfs:subPropertyOf <http://rdaregistry.info/Elements/u/P60250> ;
	owl:inverseOf <http://rdaregistry.info/Elements/u/P60294> ;
	owl:sameAs <http://rdaregistry.info/Elements/u/expandedAs> ;
	skos:definition "Relates a resource to a resource that enlarges upon the content of the source resource."@en .

<http://rdaregistry.info/Elements/u/P60217> reg:hasSubproperty <http://rdaregistry.info/Elements/m/P30031> , <http://rdaregistry.info/Elements/u/P60179> ;
	reg:name "facsimile"@en ;
	reg:status status:1001 ;
	a rdf:Property ;
	rdfs:isDefinedBy <http://rdaregistry.info/Elements/u/> ;
	rdfs:label "is facsimile"@en ;
	rdfs:subPropertyOf <http://rdaregistry.info/Elements/u/P60272> ;
	owl:inverseOf <http://rdaregistry.info/Elements/u/P60301> ;
	owl:sameAs <http://rdaregistry.info/Elements/u/facsimile> ;
	skos:definition "Relates a resource to a resource that exactly reproduces another resource embodying the resource."@en .

<http://rdaregistry.info/Elements/u/P60218> reg:hasSubproperty <http://rdaregistry.info/Elements/e/P20116> , <http://rdaregistry.info/Elements/w/P10120> ;
	reg:name "evaluatedIn"@en ;
	reg:status status:1001 ;
	a rdf:Property ;
	rdfs:isDefinedBy <http://rdaregistry.info/Elements/u/> ;
	rdfs:label "is evaluated in"@en ;
	rdfs:subPropertyOf <http://rdaregistry.info/Elements/u/P60215> ;
	owl:inverseOf <http://rdaregistry.info/Elements/u/P60255> ;
	owl:sameAs <http://rdaregistry.info/Elements/u/evaluatedIn> ;
	skos:definition "Relates a resource to a resource that examines or judges the described resource."@en .

<http://rdaregistry.info/Elements/u/P60219> reg:hasSubproperty <http://rdaregistry.info/Elements/e/P20117> , <http://rdaregistry.info/Elements/w/P10121> ;
	reg:name "analysedIn"@en ;
	reg:status status:1001 ;
	a rdf:Property ;
	rdfs:isDefinedBy <http://rdaregistry.info/Elements/u/> ;
	rdfs:label "is analysed in"@en ;
	rdfs:subPropertyOf <http://rdaregistry.info/Elements/u/P60215> ;
	owl:inverseOf <http://rdaregistry.info/Elements/u/P60239> ;
	owl:sameAs <http://rdaregistry.info/Elements/u/analysedIn> ;
	skos:definition "Relates a resource to a resource that examines the source resource to identify its components and their relations."@en .

<http://rdaregistry.info/Elements/u/P60220> reg:hasSubproperty <http://rdaregistry.info/Elements/w/P10122> ;
	reg:name "prequel"@en ;
	reg:status status:1001 ;
	a rdf:Property ;
	rdfs:isDefinedBy <http://rdaregistry.info/Elements/u/> ;
	rdfs:label "is prequel"@en ;
	rdfs:subPropertyOf <http://rdaregistry.info/Elements/u/P60261> ;
	owl:inverseOf <http://rdaregistry.info/Elements/u/P60310> ;
	owl:sameAs <http://rdaregistry.info/Elements/u/prequel> ;
	skos:definition "Relates a resource to a resource that extends the narrative of an earlier resource backwards in time."@en .

<http://rdaregistry.info/Elements/u/P60221> reg:hasSubproperty <http://rdaregistry.info/Elements/e/P20118> , <http://rdaregistry.info/Elements/w/P10123> ;
	reg:name "appendix"@en ;
	reg:status status:1001 ;
	a rdf:Property ;
	rdfs:isDefinedBy <http://rdaregistry.info/Elements/u/> ;
	rdfs:label "is appendix"@en ;
	rdfs:subPropertyOf <http://rdaregistry.info/Elements/u/P60204> ;
	owl:inverseOf <http://rdaregistry.info/Elements/u/P60253> ;
	owl:sameAs <http://rdaregistry.info/Elements/u/appendix> ;
	skos:definition "Relates a resource to a resource that forms an augmenting part of another resource which is not essential to the completeness of the content, such as a list of references, statistical tables, and explanatory matter; it can either be material which comes at the end of the content of the predominant resource, or be issued separately."@en .

<http://rdaregistry.info/Elements/u/P60222> reg:hasSubproperty <http://rdaregistry.info/Elements/e/P20120> , <http://rdaregistry.info/Elements/w/P10124> ;
	reg:name "guide"@en ;
	reg:status status:1001 ;
	a rdf:Property ;
	rdfs:isDefinedBy <http://rdaregistry.info/Elements/u/> ;
	rdfs:label "is guide"@en ;
	rdfs:subPropertyOf <http://rdaregistry.info/Elements/u/P60204> ;
	owl:inverseOf <http://rdaregistry.info/Elements/u/P60252> ;
	owl:sameAs <http://rdaregistry.info/Elements/u/guide> ;
	skos:definition "Relates a resource to a resource that guides a user through the use of the predominant resource, using notes, learning and study aids, exercises, problems, questions and answers, instructor or student materials, etc."@en .

<http://rdaregistry.info/Elements/u/P60223> reg:hasSubproperty <http://rdaregistry.info/Elements/e/P20121> , <http://rdaregistry.info/Elements/w/P10125> ;
	reg:name "abridgementOf"@en ;
	reg:status status:1001 ;
	a rdf:Property ;
	rdfs:isDefinedBy <http://rdaregistry.info/Elements/u/> ;
	rdfs:label "is abridgement of"@en ;
	rdfs:subPropertyOf <http://rdaregistry.info/Elements/u/P60305> ;
	owl:inverseOf <http://rdaregistry.info/Elements/u/P60275> ;
	owl:sameAs <http://rdaregistry.info/Elements/u/abridgementOf> ;
	skos:definition "Relates a resource to a resource that has been abridged, i.e., shortened without changing the general meaning or manner of presentation of the source resource."@en .

<http://rdaregistry.info/Elements/u/P60224> reg:hasSubproperty <http://rdaregistry.info/Elements/e/P20122> , <http://rdaregistry.info/Elements/w/P10126> ;
	reg:name "abstractOf"@en ;
	reg:status status:1001 ;
	a rdf:Property ;
	rdfs:isDefinedBy <http://rdaregistry.info/Elements/u/> ;
	rdfs:label "is abstract of"@en ;
	rdfs:subPropertyOf <http://rdaregistry.info/Elements/u/P60305> ;
	owl:inverseOf <http://rdaregistry.info/Elements/u/P60203> ;
	owl:sameAs <http://rdaregistry.info/Elements/u/abstractOf> ;
	skos:definition "Relates a resource to a resource that has been abstracted, i.e., abbreviated in a brief, objective manner."@en .

<http://rdaregistry.info/Elements/u/P60225> reg:hasSubproperty <http://rdaregistry.info/Elements/e/P20123> , <http://rdaregistry.info/Elements/w/P10127> ;
	reg:name "dramatizationOf"@en ;
	reg:status status:1001 ;
	a rdf:Property ;
	rdfs:isDefinedBy <http://rdaregistry.info/Elements/u/> ;
	rdfs:label "is dramatization of"@en ;
	rdfs:subPropertyOf <http://rdaregistry.info/Elements/u/P60241> ;
	owl:inverseOf <http://rdaregistry.info/Elements/u/P60088> ;
	owl:sameAs <http://rdaregistry.info/Elements/u/dramatizationOf> ;
	skos:definition "Relates a resource to a resource that has been adapted as a drama."@en .

<http://rdaregistry.info/Elements/u/P60226> reg:hasSubproperty <http://rdaregistry.info/Elements/e/P20124> , <http://rdaregistry.info/Elements/w/P10128> ;
	reg:name "verseAdaptationOf"@en ;
	reg:status status:1001 ;
	a rdf:Property ;
	rdfs:isDefinedBy <http://rdaregistry.info/Elements/u/> ;
	rdfs:label "is verse adaptation of"@en ;
	rdfs:subPropertyOf <http://rdaregistry.info/Elements/u/P60241> ;
	owl:inverseOf <http://rdaregistry.info/Elements/u/P60106> ;
	owl:sameAs <http://rdaregistry.info/Elements/u/verseAdaptationOf> ;
	skos:definition "Relates a resource to a resource that has been adapted as a literary composition in verse form."@en .

<http://rdaregistry.info/Elements/u/P60227> reg:hasSubproperty <http://rdaregistry.info/Elements/e/P20125> , <http://rdaregistry.info/Elements/w/P10129> ;
	reg:name "motionPictureAdaptationOf"@en ;
	reg:status status:1001 ;
	a rdf:Property ;
	rdfs:isDefinedBy <http://rdaregistry.info/Elements/u/> ;
	rdfs:label "is motion picture adaptation of"@en ;
	rdfs:subPropertyOf <http://rdaregistry.info/Elements/u/P60241> ;
	owl:inverseOf <http://rdaregistry.info/Elements/u/P60110> ;
	owl:sameAs <http://rdaregistry.info/Elements/u/motionPictureAdaptationOf> ;
	skos:definition "Relates a resource to a resource that has been adapted as a motion picture."@en .

<http://rdaregistry.info/Elements/u/P60228> reg:hasSubproperty <http://rdaregistry.info/Elements/e/P20126> , <http://rdaregistry.info/Elements/w/P10130> ;
	reg:name "novelizationOf"@en ;
	reg:status status:1001 ;
	a rdf:Property ;
	rdfs:isDefinedBy <http://rdaregistry.info/Elements/u/> ;
	rdfs:label "is novelization of"@en ;
	rdfs:subPropertyOf <http://rdaregistry.info/Elements/u/P60241> ;
	owl:inverseOf <http://rdaregistry.info/Elements/u/P60138> ;
	owl:sameAs <http://rdaregistry.info/Elements/u/novelizationOf> ;
	skos:definition "Relates a resource to a resource that has been adapted as a novel."@en .

<http://rdaregistry.info/Elements/u/P60229> reg:hasSubproperty <http://rdaregistry.info/Elements/e/P20127> , <http://rdaregistry.info/Elements/w/P10131> ;
	reg:name "radioAdaptationOf"@en ;
	reg:status status:1001 ;
	a rdf:Property ;
	rdfs:isDefinedBy <http://rdaregistry.info/Elements/u/> ;
	rdfs:label "is radio adaptation of"@en ;
	rdfs:subPropertyOf <http://rdaregistry.info/Elements/u/P60241> ;
	owl:inverseOf <http://rdaregistry.info/Elements/u/P60174> ;
	owl:sameAs <http://rdaregistry.info/Elements/u/radioAdaptationOf> ;
	skos:definition "Relates a resource to a resource that has been adapted as a radio program."@en .

<http://rdaregistry.info/Elements/u/P60230> reg:hasSubproperty <http://rdaregistry.info/Elements/e/P20128> , <http://rdaregistry.info/Elements/w/P10132> ;
	reg:name "televisionAdaptationOf"@en ;
	reg:status status:1001 ;
	a rdf:Property ;
	rdfs:isDefinedBy <http://rdaregistry.info/Elements/u/> ;
	rdfs:label "is television adaptation of"@en ;
	rdfs:subPropertyOf <http://rdaregistry.info/Elements/u/P60241> ;
	owl:inverseOf <http://rdaregistry.info/Elements/u/P60354> ;
	owl:sameAs <http://rdaregistry.info/Elements/u/televisionAdaptationOf> ;
	skos:definition "Relates a resource to a resource that has been adapted as a television program."@en .

<http://rdaregistry.info/Elements/u/P60231> reg:hasSubproperty <http://rdaregistry.info/Elements/e/P20129> , <http://rdaregistry.info/Elements/u/P60232> , <http://rdaregistry.info/Elements/u/P60233> , <http://rdaregistry.info/Elements/u/P60234> , <http://rdaregistry.info/Elements/w/P10133> ;
	reg:name "screenplayBasedOn"@en ;
	reg:status status:1001 ;
	a rdf:Property ;
	rdfs:isDefinedBy <http://rdaregistry.info/Elements/u/> ;
	rdfs:label "is screenplay based on"@en ;
	rdfs:subPropertyOf <http://rdaregistry.info/Elements/u/P60241> ;
	owl:inverseOf <http://rdaregistry.info/Elements/u/P60185> ;
	owl:sameAs <http://rdaregistry.info/Elements/u/screenplayBasedOn> ;
	skos:definition "Relates a resource to a resource that has been adapted as the screenplay for a motion picture, television program, or video."@en .

<http://rdaregistry.info/Elements/u/P60232> reg:hasSubproperty <http://rdaregistry.info/Elements/e/P20130> , <http://rdaregistry.info/Elements/w/P10134> ;
	reg:name "motionPictureScreenplayBasedOn"@en ;
	reg:status status:1001 ;
	a rdf:Property ;
	rdfs:isDefinedBy <http://rdaregistry.info/Elements/u/> ;
	rdfs:label "is motion picture screenplay based on"@en ;
	rdfs:subPropertyOf <http://rdaregistry.info/Elements/u/P60231> ;
	owl:inverseOf <http://rdaregistry.info/Elements/u/P60184> ;
	owl:sameAs <http://rdaregistry.info/Elements/u/motionPictureScreenplayBasedOn> ;
	skos:definition "Relates a resource to a resource that has been adapted as the screenplay for a motion picture."@en .

<http://rdaregistry.info/Elements/u/P60233> reg:hasSubproperty <http://rdaregistry.info/Elements/e/P20131> , <http://rdaregistry.info/Elements/w/P10135> ;
	reg:name "televisionScreenplayBasedOn"@en ;
	reg:status status:1001 ;
	a rdf:Property ;
	rdfs:isDefinedBy <http://rdaregistry.info/Elements/u/> ;
	rdfs:label "is television screenplay based on"@en ;
	rdfs:subPropertyOf <http://rdaregistry.info/Elements/u/P60231> ;
	owl:inverseOf <http://rdaregistry.info/Elements/u/P60186> ;
	owl:sameAs <http://rdaregistry.info/Elements/u/televisionScreenplayBasedOn> ;
	skos:definition "Relates a resource to a resource that has been adapted as the screenplay for a television program."@en .

<http://rdaregistry.info/Elements/u/P60234> reg:hasSubproperty <http://rdaregistry.info/Elements/e/P20132> , <http://rdaregistry.info/Elements/w/P10136> ;
	reg:name "videoScreenplayBasedOn"@en ;
	reg:status status:1001 ;
	a rdf:Property ;
	rdfs:isDefinedBy <http://rdaregistry.info/Elements/u/> ;
	rdfs:label "is video screenplay based on"@en ;
	rdfs:subPropertyOf <http://rdaregistry.info/Elements/u/P60231> ;
	owl:inverseOf <http://rdaregistry.info/Elements/u/P60187> ;
	owl:sameAs <http://rdaregistry.info/Elements/u/videoScreenplayBasedOn> ;
	skos:definition "Relates a resource to a resource that has been adapted as the screenplay for a video."@en .

<http://rdaregistry.info/Elements/u/P60235> reg:hasSubproperty <http://rdaregistry.info/Elements/e/P20133> , <http://rdaregistry.info/Elements/w/P10137> ;
	reg:name "radioScriptBasedOn"@en ;
	reg:status status:1001 ;
	a rdf:Property ;
	rdfs:isDefinedBy <http://rdaregistry.info/Elements/u/> ;
	rdfs:label "is radio script based on"@en ;
	rdfs:subPropertyOf <http://rdaregistry.info/Elements/u/P60241> ;
	owl:inverseOf <http://rdaregistry.info/Elements/u/P60188> ;
	owl:sameAs <http://rdaregistry.info/Elements/u/radioScriptBasedOn> ;
	skos:definition "Relates a resource to a resource that has been adapted as the script for a radio program."@en .

<http://rdaregistry.info/Elements/u/P60236> reg:hasSubproperty <http://rdaregistry.info/Elements/e/P20134> , <http://rdaregistry.info/Elements/w/P10138> ;
	reg:name "videoAdaptationOf"@en ;
	reg:status status:1001 ;
	a rdf:Property ;
	rdfs:isDefinedBy <http://rdaregistry.info/Elements/u/> ;
	rdfs:label "is video adaptation of"@en ;
	rdfs:subPropertyOf <http://rdaregistry.info/Elements/u/P60241> ;
	owl:inverseOf <http://rdaregistry.info/Elements/u/P60361> ;
	owl:sameAs <http://rdaregistry.info/Elements/u/videoAdaptationOf> ;
	skos:definition "Relates a resource to a resource that has been adapted for video."@en .

<http://rdaregistry.info/Elements/u/P60237> reg:hasSubproperty <http://rdaregistry.info/Elements/i/P40032> ;
	reg:name "boundWith"@en ;
	reg:status status:1001 ;
	a rdf:Property ;
	rdfs:isDefinedBy <http://rdaregistry.info/Elements/u/> ;
	rdfs:label "is bound with"@en ;
	rdfs:subPropertyOf <http://rdaregistry.info/Elements/u/P60196> ;
	owl:inverseOf <http://rdaregistry.info/Elements/u/P60237> ;
	owl:sameAs <http://rdaregistry.info/Elements/u/boundWith> ;
	skos:definition "Relates a resource to a resource that has been bound within the same binding as the resource being described."@en .

<http://rdaregistry.info/Elements/u/P60238> reg:hasSubproperty <http://rdaregistry.info/Elements/e/P20135> , <http://rdaregistry.info/Elements/w/P10139> ;
	reg:name "digestOf"@en ;
	reg:status status:1001 ;
	a rdf:Property ;
	rdfs:isDefinedBy <http://rdaregistry.info/Elements/u/> ;
	rdfs:label "is digest of"@en ;
	rdfs:subPropertyOf <http://rdaregistry.info/Elements/u/P60305> ;
	owl:inverseOf <http://rdaregistry.info/Elements/u/P60279> ;
	owl:sameAs <http://rdaregistry.info/Elements/u/digestOf> ;
	skos:definition "Relates a resource to a resource that has been digested, i.e., systematically and comprehensively condensed."@en .

<http://rdaregistry.info/Elements/u/P60239> reg:hasSubproperty <http://rdaregistry.info/Elements/e/P20136> , <http://rdaregistry.info/Elements/i/P40033> , <http://rdaregistry.info/Elements/m/P30032> , <http://rdaregistry.info/Elements/w/P10140> ;
	reg:name "analysisOf"@en ;
	reg:status status:1001 ;
	a rdf:Property ;
	rdfs:isDefinedBy <http://rdaregistry.info/Elements/u/> ;
	rdfs:label "is analysis of"@en ;
	rdfs:subPropertyOf <http://rdaregistry.info/Elements/u/P60190> ;
	owl:inverseOf <http://rdaregistry.info/Elements/u/P60219> ;
	owl:sameAs <http://rdaregistry.info/Elements/u/analysisOf> ;
	skos:definition "Relates a resource to a resource that has been examined to identify its components and their relations."@en .

<http://rdaregistry.info/Elements/u/P60240> reg:hasSubproperty <http://rdaregistry.info/Elements/w/P10141> ;
	reg:name "seriesContainerOf"@en ;
	reg:status status:1001 ;
	a rdf:Property ;
	rdfs:isDefinedBy <http://rdaregistry.info/Elements/u/> ;
	rdfs:label "is series container of"@en ;
	rdfs:subPropertyOf <http://rdaregistry.info/Elements/u/P60249> ;
	owl:inverseOf <http://rdaregistry.info/Elements/u/P60193> ;
	owl:sameAs <http://rdaregistry.info/Elements/u/seriesContainerOf> , <http://rdaregistry.info/Elements/u/seriesContains> ;
	skos:definition "Relates a resource to a resource that has been issued as part of a series."@en .

<http://rdaregistry.info/Elements/u/P60241> reg:hasSubproperty <http://rdaregistry.info/Elements/e/P20152> , <http://rdaregistry.info/Elements/u/P60225> , <http://rdaregistry.info/Elements/u/P60226> , <http://rdaregistry.info/Elements/u/P60227> , <http://rdaregistry.info/Elements/u/P60228> , <http://rdaregistry.info/Elements/u/P60229> , <http://rdaregistry.info/Elements/u/P60230> , <http://rdaregistry.info/Elements/u/P60231> , <http://rdaregistry.info/Elements/u/P60235> , <http://rdaregistry.info/Elements/u/P60236> , <http://rdaregistry.info/Elements/w/P10142> ;
	reg:name "adaptationOf"@en ;
	reg:status status:1001 ;
	a rdf:Property ;
	rdfs:isDefinedBy <http://rdaregistry.info/Elements/u/> ;
	rdfs:label "is adaptation of"@en ;
	rdfs:subPropertyOf <http://rdaregistry.info/Elements/u/P60305> ;
	owl:inverseOf <http://rdaregistry.info/Elements/u/P60260> ;
	owl:sameAs <http://rdaregistry.info/Elements/u/adaptationOf> ;
	skos:definition "Relates a resource to a resource that has been modified for a purpose, use, or medium other than that for which it was originally intended."@en .

<http://rdaregistry.info/Elements/u/P60242> reg:hasSubproperty <http://rdaregistry.info/Elements/e/P20139> ;
	reg:name "musicalArrangementOf"@en ;
	reg:status status:1001 ;
	a rdf:Property ;
	rdfs:isDefinedBy <http://rdaregistry.info/Elements/u/> ;
	rdfs:label "is musical arrangement of"@en ;
	rdfs:subPropertyOf <http://rdaregistry.info/Elements/u/P60305> ;
	owl:inverseOf <http://rdaregistry.info/Elements/u/P60274> ;
	owl:sameAs <http://rdaregistry.info/Elements/u/musicalArrangementOf> ;
	skos:definition "Relates a resource to a resource that has been rewritten for a medium of performance different from that for which the resource was originally intended."@en .

<http://rdaregistry.info/Elements/u/P60243> reg:hasSubproperty <http://rdaregistry.info/Elements/e/P20140> , <http://rdaregistry.info/Elements/w/P10143> ;
	reg:name "freeTranslationOf"@en ;
	reg:status status:1001 ;
	a rdf:Property ;
	rdfs:isDefinedBy <http://rdaregistry.info/Elements/u/> ;
	rdfs:label "is free translation of"@en ;
	rdfs:subPropertyOf <http://rdaregistry.info/Elements/u/P60305> ;
	owl:inverseOf <http://rdaregistry.info/Elements/u/P60189> ;
	owl:sameAs <http://rdaregistry.info/Elements/u/freeTranslationOf> ;
	skos:definition "Relates a resource to a resource that has been translated freely, preserving the spirit of the original, but not its linguistic details."@en .

<http://rdaregistry.info/Elements/u/P60244> reg:hasSubproperty <http://rdaregistry.info/Elements/e/P20141> , <http://rdaregistry.info/Elements/u/P60111> ;
	reg:name "translationOf"@en ;
	reg:status status:1001 ;
	a rdf:Property ;
	rdfs:isDefinedBy <http://rdaregistry.info/Elements/u/> ;
	rdfs:label "is translation of"@en ;
	rdfs:subPropertyOf <http://rdaregistry.info/Elements/u/P60305> ;
	owl:inverseOf <http://rdaregistry.info/Elements/u/P60280> ;
	owl:sameAs <http://rdaregistry.info/Elements/u/translationOf> ;
	skos:definition "Relates a resource to a resource that has been translated, i.e., the text expressed in a language different from that of the original resource."@en .

<http://rdaregistry.info/Elements/u/P60245> reg:hasSubproperty <http://rdaregistry.info/Elements/e/P20211> ;
	reg:name "revisedAs"@en ;
	reg:status status:1001 ;
	a rdf:Property ;
	rdfs:isDefinedBy <http://rdaregistry.info/Elements/u/> ;
	rdfs:label "is revised as"@en ;
	rdfs:subPropertyOf <http://rdaregistry.info/Elements/u/P60250> ;
	owl:inverseOf <http://rdaregistry.info/Elements/u/P60303> ;
	owl:sameAs <http://rdaregistry.info/Elements/u/revisedAs> ;
	skos:definition "Relates a resource to a resource that has been updated, corrected, or expanded."@en .

<http://rdaregistry.info/Elements/u/P60246> reg:hasSubproperty <http://rdaregistry.info/Elements/e/P20142> , <http://rdaregistry.info/Elements/w/P10144> ;
	reg:name "parodiedAs"@en ;
	reg:status status:1001 ;
	a rdf:Property ;
	rdfs:isDefinedBy <http://rdaregistry.info/Elements/u/> ;
	rdfs:label "is parodied as"@en ;
	rdfs:subPropertyOf <http://rdaregistry.info/Elements/u/P60214> ;
	owl:inverseOf <http://rdaregistry.info/Elements/u/P60312> ;
	owl:sameAs <http://rdaregistry.info/Elements/u/parodiedAs> ;
	skos:definition "Relates a resource to a resource that imitates the style or content of the source resource for comic effect."@en .

<http://rdaregistry.info/Elements/u/P60247> reg:hasSubproperty <http://rdaregistry.info/Elements/e/P20143> , <http://rdaregistry.info/Elements/w/P10145> ;
	reg:name "absorbedBy"@en ;
	reg:status status:1001 ;
	a rdf:Property ;
	rdfs:isDefinedBy <http://rdaregistry.info/Elements/u/> ;
	rdfs:label "is absorbed by"@en ;
	rdfs:subPropertyOf <http://rdaregistry.info/Elements/u/P60278> ;
	owl:inverseOf <http://rdaregistry.info/Elements/u/P60574> ;
	owl:sameAs <http://rdaregistry.info/Elements/u/absorbedBy> ;
	skos:definition "Relates a resource to a resource that incorporates another resource."@en .

<http://rdaregistry.info/Elements/u/P60248> reg:hasSubproperty <http://rdaregistry.info/Elements/e/P20144> , <http://rdaregistry.info/Elements/w/P10146> ;
	reg:name "absorbedInPartBy"@en ;
	reg:status status:1001 ;
	a rdf:Property ;
	rdfs:isDefinedBy <http://rdaregistry.info/Elements/u/> ;
	rdfs:label "is absorbed in part by"@en ;
	rdfs:subPropertyOf <http://rdaregistry.info/Elements/u/P60278> ;
	owl:inverseOf <http://rdaregistry.info/Elements/u/P60575> ;
	owl:sameAs <http://rdaregistry.info/Elements/u/absorbedInPartBy> ;
	skos:definition "Relates a resource to a resource that incorporates part of the content of another resource."@en .

<http://rdaregistry.info/Elements/u/P60249> reg:hasSubproperty <http://rdaregistry.info/Elements/e/P20145> , <http://rdaregistry.info/Elements/i/P40034> , <http://rdaregistry.info/Elements/m/P30033> , <http://rdaregistry.info/Elements/u/P60183> , <http://rdaregistry.info/Elements/u/P60207> , <http://rdaregistry.info/Elements/u/P60240> , <http://rdaregistry.info/Elements/u/P60300> , <http://rdaregistry.info/Elements/u/P60316> , <http://rdaregistry.info/Elements/w/P10147> ;
	reg:name "containerOf"@en ;
	reg:status status:1001 ;
	a rdf:Property ;
	rdfs:isDefinedBy <http://rdaregistry.info/Elements/u/> ;
	rdfs:label "is container of"@en ;
	rdfs:subPropertyOf <http://rdaregistry.info/Elements/u/P60714> ;
	owl:inverseOf <http://rdaregistry.info/Elements/u/P60101> ;
	owl:sameAs <http://rdaregistry.info/Elements/u/containerOf> , <http://rdaregistry.info/Elements/u/contains> ;
	skos:definition "Relates a resource to a resource that is a discrete component of a larger resource."@en .

<http://rdaregistry.info/Elements/u/P60250> reg:hasSubproperty <http://rdaregistry.info/Elements/e/P20203> , <http://rdaregistry.info/Elements/u/P60115> , <http://rdaregistry.info/Elements/u/P60120> , <http://rdaregistry.info/Elements/u/P60121> , <http://rdaregistry.info/Elements/u/P60177> , <http://rdaregistry.info/Elements/u/P60178> , <http://rdaregistry.info/Elements/u/P60180> , <http://rdaregistry.info/Elements/u/P60189> , <http://rdaregistry.info/Elements/u/P60203> , <http://rdaregistry.info/Elements/u/P60205> , <http://rdaregistry.info/Elements/u/P60210> , <http://rdaregistry.info/Elements/u/P60214> , <http://rdaregistry.info/Elements/u/P60216> , <http://rdaregistry.info/Elements/u/P60245> , <http://rdaregistry.info/Elements/u/P60260> , <http://rdaregistry.info/Elements/u/P60273> , <http://rdaregistry.info/Elements/u/P60274> , <http://rdaregistry.info/Elements/u/P60275> , <http://rdaregistry.info/Elements/u/P60279> , <http://rdaregistry.info/Elements/u/P60280> , <http://rdaregistry.info/Elements/w/P10148> ;
	reg:name "derivative"@en ;
	reg:status status:1001 ;
	a rdf:Property ;
	rdfs:isDefinedBy <http://rdaregistry.info/Elements/u/> ;
	rdfs:label "is derivative"@en ;
	rdfs:subPropertyOf <http://rdaregistry.info/Elements/u/P60710> ;
	owl:inverseOf <http://rdaregistry.info/Elements/u/P60305> ;
	owl:sameAs <http://rdaregistry.info/Elements/u/derivative> ;
	skos:definition "Relates a resource to a resource that is a modification of a source resource."@en .

<http://rdaregistry.info/Elements/u/P60251> reg:hasSubproperty <http://rdaregistry.info/Elements/e/P20146> , <http://rdaregistry.info/Elements/w/P10149> ;
	reg:name "errataTo"@en ;
	reg:status status:1001 ;
	a rdf:Property ;
	rdfs:isDefinedBy <http://rdaregistry.info/Elements/u/> ;
	rdfs:label "is errata to"@en ;
	rdfs:subPropertyOf <http://rdaregistry.info/Elements/u/P60307> ;
	owl:inverseOf <http://rdaregistry.info/Elements/u/P60181> ;
	owl:sameAs <http://rdaregistry.info/Elements/u/errataTo> ;
	skos:definition "Relates a resource to a resource that is augmented by a list of errors in the predominant resource, discovered after publication, with their corrections."@en .

<http://rdaregistry.info/Elements/u/P60252> reg:hasSubproperty <http://rdaregistry.info/Elements/e/P20147> , <http://rdaregistry.info/Elements/w/P10150> ;
	reg:name "guideTo"@en ;
	reg:status status:1001 ;
	a rdf:Property ;
	rdfs:isDefinedBy <http://rdaregistry.info/Elements/u/> ;
	rdfs:label "is guide to"@en ;
	rdfs:subPropertyOf <http://rdaregistry.info/Elements/u/P60307> ;
	owl:inverseOf <http://rdaregistry.info/Elements/u/P60222> ;
	owl:sameAs <http://rdaregistry.info/Elements/u/guideTo> ;
	skos:definition "Relates a resource to a resource that is augmented by another resource consisting of material to help the user of the predominant resource, such as notes, learning and study aids, exercises, problems, questions and answers, instructor or student materials, etc."@en .

<http://rdaregistry.info/Elements/u/P60253> reg:hasSubproperty <http://rdaregistry.info/Elements/e/P20089> , <http://rdaregistry.info/Elements/w/P10151> ;
	reg:name "appendixTo"@en ;
	reg:status status:1001 ;
	a rdf:Property ;
	rdfs:isDefinedBy <http://rdaregistry.info/Elements/u/> ;
	rdfs:label "is appendix to"@en ;
	rdfs:subPropertyOf <http://rdaregistry.info/Elements/u/P60307> ;
	owl:inverseOf <http://rdaregistry.info/Elements/u/P60221> ;
	owl:sameAs <http://rdaregistry.info/Elements/u/appendixTo> ;
	skos:definition "Relates a resource to a resource that is augmented by another resource that consists of material that is not essential to the completeness of the content, such as a list of references, statistical tables, and explanatory matter; the augmenting resource can either come at the end of the content, or be issued separately."@en .

<http://rdaregistry.info/Elements/u/P60254> reg:hasSubproperty <http://rdaregistry.info/Elements/e/P20148> , <http://rdaregistry.info/Elements/w/P10152> ;
	reg:name "illustrationsFor"@en ;
	reg:status status:1001 ;
	a rdf:Property ;
	rdfs:isDefinedBy <http://rdaregistry.info/Elements/u/> ;
	rdfs:label "is illustrations for"@en ;
	rdfs:subPropertyOf <http://rdaregistry.info/Elements/u/P60307> ;
	owl:inverseOf <http://rdaregistry.info/Elements/u/P60182> ;
	owl:sameAs <http://rdaregistry.info/Elements/u/illustrationsFor> ;
	skos:definition "Relates a resource to a resource that is augmented by pictorial content designed to explain or decorate it."@en .

<http://rdaregistry.info/Elements/u/P60255> reg:hasSubproperty <http://rdaregistry.info/Elements/e/P20150> , <http://rdaregistry.info/Elements/i/P40037> , <http://rdaregistry.info/Elements/m/P30034> , <http://rdaregistry.info/Elements/w/P10153> ;
	reg:name "evaluationOf"@en ;
	reg:status status:1001 ;
	a rdf:Property ;
	rdfs:isDefinedBy <http://rdaregistry.info/Elements/u/> ;
	rdfs:label "is evaluation of"@en ;
	rdfs:subPropertyOf <http://rdaregistry.info/Elements/u/P60190> ;
	owl:inverseOf <http://rdaregistry.info/Elements/u/P60218> ;
	owl:sameAs <http://rdaregistry.info/Elements/u/evaluationOf> ;
	skos:definition "Relates a resource to a resource that is examined or judged."@en .

<http://rdaregistry.info/Elements/u/P60256> reg:hasSubproperty <http://rdaregistry.info/Elements/m/P30035> , <http://rdaregistry.info/Elements/u/P60257> , <http://rdaregistry.info/Elements/u/P60258> ;
	reg:name "issuedWith"@en ;
	reg:status status:1001 ;
	a rdf:Property ;
	rdfs:isDefinedBy <http://rdaregistry.info/Elements/u/> ;
	rdfs:label "is issued with"@en ;
	rdfs:subPropertyOf <http://rdaregistry.info/Elements/u/P60196> ;
	owl:inverseOf <http://rdaregistry.info/Elements/u/P60256> ;
	owl:sameAs <http://rdaregistry.info/Elements/u/issuedWith> ;
	skos:definition "Relates a resource to a resource that is issued on the same carrier as the resource being described."@en .

<http://rdaregistry.info/Elements/u/P60257> reg:hasSubproperty <http://rdaregistry.info/Elements/i/P40035> , <http://rdaregistry.info/Elements/m/P30036> ;
	reg:name "onDiscWith"@en ;
	reg:status status:1001 ;
	a rdf:Property ;
	rdfs:isDefinedBy <http://rdaregistry.info/Elements/u/> ;
	rdfs:label "is on disc with"@en ;
	rdfs:subPropertyOf <http://rdaregistry.info/Elements/u/P60256> ;
	owl:inverseOf <http://rdaregistry.info/Elements/u/P60257> ;
	owl:sameAs <http://rdaregistry.info/Elements/u/onDiscWith> ;
	skos:definition "Relates a resource to a resource that is issued on the same disc with the resource being described."@en .

<http://rdaregistry.info/Elements/u/P60258> reg:hasSubproperty <http://rdaregistry.info/Elements/i/P40036> , <http://rdaregistry.info/Elements/m/P30037> ;
	reg:name "filmedWith"@en ;
	reg:status status:1001 ;
	a rdf:Property ;
	rdfs:isDefinedBy <http://rdaregistry.info/Elements/u/> ;
	rdfs:label "is filmed with"@en ;
	rdfs:subPropertyOf <http://rdaregistry.info/Elements/u/P60256> ;
	owl:inverseOf <http://rdaregistry.info/Elements/u/P60258> ;
	owl:sameAs <http://rdaregistry.info/Elements/u/filmedWith> ;
	skos:definition "Relates a resource to a resource that is issued on the same microform with the resource being described."@en .

<http://rdaregistry.info/Elements/u/P60259> reg:hasSubproperty <http://rdaregistry.info/Elements/e/P20151> , <http://rdaregistry.info/Elements/w/P10154> ;
	reg:name "supplementTo"@en ;
	reg:status status:1001 ;
	a rdf:Property ;
	rdfs:isDefinedBy <http://rdaregistry.info/Elements/u/> ;
	rdfs:label "is supplement to"@en ;
	rdfs:subPropertyOf <http://rdaregistry.info/Elements/u/P60307> ;
	owl:inverseOf <http://rdaregistry.info/Elements/u/P60281> ;
	owl:sameAs <http://rdaregistry.info/Elements/u/supplementTo> ;
	skos:definition "Relates a resource to a resource that is updated or otherwise complemented by the augmenting resource."@en .

<http://rdaregistry.info/Elements/u/P60260> reg:hasSubproperty <http://rdaregistry.info/Elements/e/P20153> , <http://rdaregistry.info/Elements/u/P60088> , <http://rdaregistry.info/Elements/u/P60106> , <http://rdaregistry.info/Elements/u/P60110> , <http://rdaregistry.info/Elements/u/P60138> , <http://rdaregistry.info/Elements/u/P60174> , <http://rdaregistry.info/Elements/u/P60185> , <http://rdaregistry.info/Elements/u/P60188> , <http://rdaregistry.info/Elements/u/P60354> , <http://rdaregistry.info/Elements/u/P60361> , <http://rdaregistry.info/Elements/w/P10155> ;
	reg:name "adaptedAs"@en ;
	reg:status status:1001 ;
	a rdf:Property ;
	rdfs:isDefinedBy <http://rdaregistry.info/Elements/u/> ;
	rdfs:label "is adapted as"@en ;
	rdfs:subPropertyOf <http://rdaregistry.info/Elements/u/P60250> ;
	owl:inverseOf <http://rdaregistry.info/Elements/u/P60241> ;
	owl:sameAs <http://rdaregistry.info/Elements/u/adaptedAs> ;
	skos:definition "Relates a resource to a resource that modifies the source resource for a purpose, use, or medium other than that for which it was originally intended."@en .

<http://rdaregistry.info/Elements/u/P60261> reg:hasSubproperty <http://rdaregistry.info/Elements/e/P20154> , <http://rdaregistry.info/Elements/u/P60220> , <http://rdaregistry.info/Elements/u/P60276> , <http://rdaregistry.info/Elements/u/P60277> , <http://rdaregistry.info/Elements/u/P60479> , <http://rdaregistry.info/Elements/u/P60480> , <http://rdaregistry.info/Elements/u/P60505> , <http://rdaregistry.info/Elements/u/P60574> , <http://rdaregistry.info/Elements/u/P60575> , <http://rdaregistry.info/Elements/u/P60576> , <http://rdaregistry.info/Elements/u/P60577> , <http://rdaregistry.info/Elements/w/P10156> ;
	reg:name "precededBy"@en ;
	reg:status status:1001 ;
	a rdf:Property ;
	rdfs:isDefinedBy <http://rdaregistry.info/Elements/u/> ;
	rdfs:label "is preceded by"@en ;
	rdfs:subPropertyOf <http://rdaregistry.info/Elements/u/P60713> ;
	owl:inverseOf <http://rdaregistry.info/Elements/u/P60278> ;
	owl:sameAs <http://rdaregistry.info/Elements/u/precededBy> ;
	skos:definition "Relates a resource to a resource that precedes (e.g., is earlier in time or before in a narrative) the succeeding resource."@en .

<http://rdaregistry.info/Elements/u/P60262> reg:hasSubproperty <http://rdaregistry.info/Elements/e/P20155> , <http://rdaregistry.info/Elements/w/P10157> ;
	reg:name "findingAid"@en ;
	reg:status status:1001 ;
	a rdf:Property ;
	rdfs:isDefinedBy <http://rdaregistry.info/Elements/u/> ;
	rdfs:label "is finding aid"@en ;
	rdfs:subPropertyOf <http://rdaregistry.info/Elements/u/P60204> ;
	owl:inverseOf <http://rdaregistry.info/Elements/u/P60474> ;
	owl:sameAs <http://rdaregistry.info/Elements/u/findingAid> ;
	skos:definition "Relates a resource to a resource that provides a guide to the organization, arrangement, and contents of an archival collection."@en .

<http://rdaregistry.info/Elements/u/P60263> reg:hasSubproperty <http://rdaregistry.info/Elements/e/P20156> , <http://rdaregistry.info/Elements/w/P10158> ;
	reg:name "index"@en ;
	reg:status status:1001 ;
	a rdf:Property ;
	rdfs:isDefinedBy <http://rdaregistry.info/Elements/u/> ;
	rdfs:label "is index"@en ;
	rdfs:subPropertyOf <http://rdaregistry.info/Elements/u/P60204> ;
	owl:inverseOf <http://rdaregistry.info/Elements/u/P60302> ;
	owl:sameAs <http://rdaregistry.info/Elements/u/index> ;
	skos:definition "Relates a resource to a resource that provides a systematic, alphabetical guide to the contents of the predominant resource, usually keyed to page numbers or other reference codes."@en .

<http://rdaregistry.info/Elements/u/P60264> reg:hasSubproperty <http://rdaregistry.info/Elements/e/P20157> , <http://rdaregistry.info/Elements/u/P60265> , <http://rdaregistry.info/Elements/u/P60268> , <http://rdaregistry.info/Elements/u/P60269> , <http://rdaregistry.info/Elements/w/P10159> ;
	reg:name "screenplay"@en ;
	reg:status status:1001 ;
	a rdf:Property ;
	rdfs:isDefinedBy <http://rdaregistry.info/Elements/u/> ;
	rdfs:label "is screenplay"@en ;
	rdfs:subPropertyOf <http://rdaregistry.info/Elements/u/P60198> ;
	owl:inverseOf <http://rdaregistry.info/Elements/u/P60201> ;
	owl:sameAs <http://rdaregistry.info/Elements/u/screenplay> ;
	skos:definition "Relates a resource to a resource that provides the text for a motion picture, television program or video."@en .

<http://rdaregistry.info/Elements/u/P60265> reg:hasSubproperty <http://rdaregistry.info/Elements/e/P20158> , <http://rdaregistry.info/Elements/w/P10160> ;
	reg:name "motionPictureScreenplay"@en ;
	reg:status status:1001 ;
	a rdf:Property ;
	rdfs:isDefinedBy <http://rdaregistry.info/Elements/u/> ;
	rdfs:label "is motion picture screenplay"@en ;
	rdfs:subPropertyOf <http://rdaregistry.info/Elements/u/P60264> ;
	owl:inverseOf <http://rdaregistry.info/Elements/u/P60282> ;
	owl:sameAs <http://rdaregistry.info/Elements/u/motionPictureScreenplay> ;
	skos:definition "Relates a resource to a resource that provides the text for a motion picture."@en .

<http://rdaregistry.info/Elements/u/P60266> reg:hasSubproperty <http://rdaregistry.info/Elements/e/P20159> , <http://rdaregistry.info/Elements/w/P10161> ;
	reg:name "musicalSettingOf"@en ;
	reg:status status:1001 ;
	a rdf:Property ;
	rdfs:isDefinedBy <http://rdaregistry.info/Elements/u/> ;
	rdfs:label "is musical setting of"@en ;
	rdfs:subPropertyOf <http://rdaregistry.info/Elements/u/P60305> ;
	owl:inverseOf <http://rdaregistry.info/Elements/u/P60121> ;
	owl:sameAs <http://rdaregistry.info/Elements/u/musicalSettingOf> ;
	skos:definition "Relates a resource to a resource that provides the text for a non-dramatic musical resource, other than an oratorio."@en .

<http://rdaregistry.info/Elements/u/P60267> reg:hasSubproperty <http://rdaregistry.info/Elements/e/P20160> , <http://rdaregistry.info/Elements/w/P10162> ;
	reg:name "radioScript"@en ;
	reg:status status:1001 ;
	a rdf:Property ;
	rdfs:isDefinedBy <http://rdaregistry.info/Elements/u/> ;
	rdfs:label "is radio script"@en ;
	rdfs:subPropertyOf <http://rdaregistry.info/Elements/u/P60198> ;
	owl:inverseOf <http://rdaregistry.info/Elements/u/P60285> ;
	owl:sameAs <http://rdaregistry.info/Elements/u/radioScript> ;
	skos:definition "Relates a resource to a resource that provides the text for a radio program."@en .

<http://rdaregistry.info/Elements/u/P60268> reg:hasSubproperty <http://rdaregistry.info/Elements/e/P20161> , <http://rdaregistry.info/Elements/w/P10163> ;
	reg:name "televisionScreenplay"@en ;
	reg:status status:1001 ;
	a rdf:Property ;
	rdfs:isDefinedBy <http://rdaregistry.info/Elements/u/> ;
	rdfs:label "is television screenplay"@en ;
	rdfs:subPropertyOf <http://rdaregistry.info/Elements/u/P60264> ;
	owl:inverseOf <http://rdaregistry.info/Elements/u/P60283> ;
	owl:sameAs <http://rdaregistry.info/Elements/u/televisionScreenplay> ;
	skos:definition "Relates a resource to a resource that provides the text for a television program."@en .

<http://rdaregistry.info/Elements/u/P60269> reg:hasSubproperty <http://rdaregistry.info/Elements/e/P20162> , <http://rdaregistry.info/Elements/w/P10164> ;
	reg:name "videoScreenplay"@en ;
	reg:status status:1001 ;
	a rdf:Property ;
	rdfs:isDefinedBy <http://rdaregistry.info/Elements/u/> ;
	rdfs:label "is video screenplay"@en ;
	rdfs:subPropertyOf <http://rdaregistry.info/Elements/u/P60264> ;
	owl:inverseOf <http://rdaregistry.info/Elements/u/P60284> ;
	owl:sameAs <http://rdaregistry.info/Elements/u/videoScreenplay> ;
	skos:definition "Relates a resource to a resource that provides the text for a video."@en .

<http://rdaregistry.info/Elements/u/P60270> reg:hasSubproperty <http://rdaregistry.info/Elements/e/P20163> , <http://rdaregistry.info/Elements/w/P10165> ;
	reg:name "libretto"@en ;
	reg:status status:1001 ;
	a rdf:Property ;
	rdfs:isDefinedBy <http://rdaregistry.info/Elements/u/> ;
	rdfs:label "is libretto"@en ;
	rdfs:subPropertyOf <http://rdaregistry.info/Elements/u/P60198> ;
	owl:inverseOf <http://rdaregistry.info/Elements/u/P60117> ;
	owl:sameAs <http://rdaregistry.info/Elements/u/libretto> ;
	skos:definition "Relates a resource to a resource that provides the text of an opera or other resource for the musical stage, or an oratorio."@en .

<http://rdaregistry.info/Elements/u/P60271> reg:hasSubproperty <http://rdaregistry.info/Elements/m/P30038> ;
	reg:name "reprintedAs"@en ;
	reg:status status:1001 ;
	a rdf:Property ;
	rdfs:isDefinedBy <http://rdaregistry.info/Elements/u/> ;
	rdfs:label "is reprinted as"@en ;
	rdfs:subPropertyOf <http://rdaregistry.info/Elements/u/P60272> ;
	owl:inverseOf <http://rdaregistry.info/Elements/u/P60168> ;
	owl:sameAs <http://rdaregistry.info/Elements/u/reprintedAs> ;
	skos:definition "Relates a resource to a resource that reissues the same expression of the resource as the printed resource being described."@en .

<http://rdaregistry.info/Elements/u/P60272> reg:hasSubproperty <http://rdaregistry.info/Elements/m/P30039> , <http://rdaregistry.info/Elements/u/P60083> , <http://rdaregistry.info/Elements/u/P60200> , <http://rdaregistry.info/Elements/u/P60217> , <http://rdaregistry.info/Elements/u/P60271> ;
	reg:name "reproducedAs"@en ;
	reg:status status:1001 ;
	a rdf:Property ;
	rdfs:isDefinedBy <http://rdaregistry.info/Elements/u/> ;
	rdfs:label "is reproduced as"@en ;
	rdfs:subPropertyOf <http://rdaregistry.info/Elements/u/P60191> ;
	owl:inverseOf <http://rdaregistry.info/Elements/u/P60297> ;
	owl:sameAs <http://rdaregistry.info/Elements/u/reproducedAs> ;
	skos:definition "Relates a resource to a resource that reproduces another resource embodying the resource."@en .

<http://rdaregistry.info/Elements/u/P60273> reg:hasSubproperty <http://rdaregistry.info/Elements/e/P20164> , <http://rdaregistry.info/Elements/w/P10166> ;
	reg:name "paraphrasedAs"@en ;
	reg:status status:1001 ;
	a rdf:Property ;
	rdfs:isDefinedBy <http://rdaregistry.info/Elements/u/> ;
	rdfs:label "is paraphrased as"@en ;
	rdfs:subPropertyOf <http://rdaregistry.info/Elements/u/P60250> ;
	owl:inverseOf <http://rdaregistry.info/Elements/u/P60296> ;
	owl:sameAs <http://rdaregistry.info/Elements/u/paraphrasedAs> ;
	skos:definition "Relates a resource to a resource that restates the content of the source resource in a different form."@en .

<http://rdaregistry.info/Elements/u/P60274> reg:hasSubproperty <http://rdaregistry.info/Elements/e/P20165> ;
	reg:name "musicalArrangement"@en ;
	reg:status status:1001 ;
	a rdf:Property ;
	rdfs:isDefinedBy <http://rdaregistry.info/Elements/u/> ;
	rdfs:label "is musical arrangement"@en ;
	rdfs:subPropertyOf <http://rdaregistry.info/Elements/u/P60250> ;
	owl:inverseOf <http://rdaregistry.info/Elements/u/P60242> ;
	owl:sameAs <http://rdaregistry.info/Elements/u/musicalArrangement> ;
	skos:definition "Relates a resource to a resource that rewrites the source entity for a medium of performance different from that for which the resource was originally intended."@en .

<http://rdaregistry.info/Elements/u/P60275> reg:hasSubproperty <http://rdaregistry.info/Elements/e/P20166> , <http://rdaregistry.info/Elements/w/P10167> ;
	reg:name "abridgedAs"@en ;
	reg:status status:1001 ;
	a rdf:Property ;
	rdfs:isDefinedBy <http://rdaregistry.info/Elements/u/> ;
	rdfs:label "is abridged as"@en ;
	rdfs:subPropertyOf <http://rdaregistry.info/Elements/u/P60250> ;
	owl:inverseOf <http://rdaregistry.info/Elements/u/P60223> ;
	owl:sameAs <http://rdaregistry.info/Elements/u/abridgedAs> ;
	skos:definition "Relates a resource to a resource that shortens the source resource without changing the general meaning or manner of presentation."@en .

<http://rdaregistry.info/Elements/u/P60276> reg:hasSubproperty <http://rdaregistry.info/Elements/e/P20167> , <http://rdaregistry.info/Elements/w/P10168> ;
	reg:name "continuationInPartOf"@en ;
	reg:status status:1001 ;
	a rdf:Property ;
	rdfs:isDefinedBy <http://rdaregistry.info/Elements/u/> ;
	rdfs:label "is continuation in part of"@en ;
	rdfs:subPropertyOf <http://rdaregistry.info/Elements/u/P60261> ;
	owl:inverseOf <http://rdaregistry.info/Elements/u/P60503> ;
	owl:sameAs <http://rdaregistry.info/Elements/u/continuationInPartOf> , <http://rdaregistry.info/Elements/u/continuesInPart> ;
	skos:definition "Relates a resource to a resource that split into two or more separate resources with new titles."@en .

<http://rdaregistry.info/Elements/u/P60277> reg:hasSubproperty <http://rdaregistry.info/Elements/e/P20168> , <http://rdaregistry.info/Elements/w/P10169> ;
	reg:name "separatedFrom"@en ;
	reg:status status:1001 ;
	a rdf:Property ;
	rdfs:isDefinedBy <http://rdaregistry.info/Elements/u/> ;
	rdfs:label "is separated from"@en ;
	rdfs:subPropertyOf <http://rdaregistry.info/Elements/u/P60261> ;
	owl:inverseOf <http://rdaregistry.info/Elements/u/P60199> ;
	owl:sameAs <http://rdaregistry.info/Elements/u/separatedFrom> ;
	skos:definition "Relates a resource to a resource that spun off a part of its content to form a new resource."@en .

<http://rdaregistry.info/Elements/u/P60278> reg:hasSubproperty <http://rdaregistry.info/Elements/e/P20169> , <http://rdaregistry.info/Elements/u/P60102> , <http://rdaregistry.info/Elements/u/P60103> , <http://rdaregistry.info/Elements/u/P60104> , <http://rdaregistry.info/Elements/u/P60199> , <http://rdaregistry.info/Elements/u/P60247> , <http://rdaregistry.info/Elements/u/P60248> , <http://rdaregistry.info/Elements/u/P60306> , <http://rdaregistry.info/Elements/u/P60310> , <http://rdaregistry.info/Elements/u/P60503> , <http://rdaregistry.info/Elements/u/P60504> , <http://rdaregistry.info/Elements/w/P10170> ;
	reg:name "succeededBy"@en ;
	reg:status status:1001 ;
	a rdf:Property ;
	rdfs:isDefinedBy <http://rdaregistry.info/Elements/u/> ;
	rdfs:label "is succeeded by"@en ;
	rdfs:subPropertyOf <http://rdaregistry.info/Elements/u/P60713> ;
	owl:inverseOf <http://rdaregistry.info/Elements/u/P60261> ;
	owl:sameAs <http://rdaregistry.info/Elements/u/succeededBy> ;
	skos:definition "Relates a resource to a resource that succeeds (e.g., later in time or after in a narrative) the preceding resource."@en .

<http://rdaregistry.info/Elements/u/P60279> reg:hasSubproperty <http://rdaregistry.info/Elements/e/P20170> , <http://rdaregistry.info/Elements/w/P10171> ;
	reg:name "digest"@en ;
	reg:status status:1001 ;
	a rdf:Property ;
	rdfs:isDefinedBy <http://rdaregistry.info/Elements/u/> ;
	rdfs:label "is digest"@en ;
	rdfs:subPropertyOf <http://rdaregistry.info/Elements/u/P60250> ;
	owl:inverseOf <http://rdaregistry.info/Elements/u/P60238> ;
	owl:sameAs <http://rdaregistry.info/Elements/u/digest> ;
	skos:definition "Relates a resource to a resource that systematically and comprehensively condenses the source resource."@en .

<http://rdaregistry.info/Elements/u/P60280> reg:hasSubproperty <http://rdaregistry.info/Elements/e/P20171> , <http://rdaregistry.info/Elements/u/P60112> ;
	reg:name "translatedAs"@en ;
	reg:status status:1001 ;
	a rdf:Property ;
	rdfs:isDefinedBy <http://rdaregistry.info/Elements/u/> ;
	rdfs:label "is translated as"@en ;
	rdfs:subPropertyOf <http://rdaregistry.info/Elements/u/P60250> ;
	owl:inverseOf <http://rdaregistry.info/Elements/u/P60244> ;
	owl:sameAs <http://rdaregistry.info/Elements/u/translatedAs> ;
	skos:definition "Relates a resource to a resource that translates the text of the source entity into a language different from that of the original resource."@en .

<http://rdaregistry.info/Elements/u/P60281> reg:hasSubproperty <http://rdaregistry.info/Elements/e/P20172> , <http://rdaregistry.info/Elements/w/P10172> ;
	reg:name "supplement"@en ;
	reg:status status:1001 ;
	a rdf:Property ;
	rdfs:isDefinedBy <http://rdaregistry.info/Elements/u/> ;
	rdfs:label "is supplement"@en ;
	rdfs:subPropertyOf <http://rdaregistry.info/Elements/u/P60204> ;
	owl:inverseOf <http://rdaregistry.info/Elements/u/P60259> ;
	owl:sameAs <http://rdaregistry.info/Elements/u/supplement> ;
	skos:definition "Relates a resource to a resource that updates or otherwise complements the predominant resource."@en .

<http://rdaregistry.info/Elements/u/P60282> reg:hasSubproperty <http://rdaregistry.info/Elements/e/P20173> , <http://rdaregistry.info/Elements/w/P10173> ;
	reg:name "screenplayForTheMotionPicture"@en ;
	reg:status status:1001 ;
	a rdf:Property ;
	rdfs:isDefinedBy <http://rdaregistry.info/Elements/u/> ;
	rdfs:label "is screenplay for motion picture"@en ;
	rdfs:subPropertyOf <http://rdaregistry.info/Elements/u/P60201> ;
	owl:inverseOf <http://rdaregistry.info/Elements/u/P60265> ;
	owl:sameAs <http://rdaregistry.info/Elements/u/screenplayForTheMotionPicture> ;
	skos:definition "Relates a resource to a resource that uses the text as a screenplay for a motion picture."@en .

<http://rdaregistry.info/Elements/u/P60283> reg:hasSubproperty <http://rdaregistry.info/Elements/e/P20174> , <http://rdaregistry.info/Elements/w/P10174> ;
	reg:name "screenplayForTheTelevisionProgram"@en ;
	reg:status status:1001 ;
	a rdf:Property ;
	rdfs:isDefinedBy <http://rdaregistry.info/Elements/u/> ;
	rdfs:label "is screenplay for television program"@en ;
	rdfs:subPropertyOf <http://rdaregistry.info/Elements/u/P60201> ;
	owl:inverseOf <http://rdaregistry.info/Elements/u/P60268> ;
	owl:sameAs <http://rdaregistry.info/Elements/u/screenplayForTheTelevisionProgram> ;
	skos:definition "Relates a resource to a resource that uses the text as a screenplay for a television program."@en .

<http://rdaregistry.info/Elements/u/P60284> reg:hasSubproperty <http://rdaregistry.info/Elements/e/P20175> , <http://rdaregistry.info/Elements/w/P10175> ;
	reg:name "screenplayForTheVideo"@en ;
	reg:status status:1001 ;
	a rdf:Property ;
	rdfs:isDefinedBy <http://rdaregistry.info/Elements/u/> ;
	rdfs:label "is screenplay for video"@en ;
	rdfs:subPropertyOf <http://rdaregistry.info/Elements/u/P60201> ;
	owl:inverseOf <http://rdaregistry.info/Elements/u/P60269> ;
	owl:sameAs <http://rdaregistry.info/Elements/u/screenplayForTheVideo> ;
	skos:definition "Relates a resource to a resource that uses the text as a screenplay for a video."@en .

<http://rdaregistry.info/Elements/u/P60285> reg:hasSubproperty <http://rdaregistry.info/Elements/e/P20176> , <http://rdaregistry.info/Elements/w/P10176> ;
	reg:name "scriptForTheRadioProgram"@en ;
	reg:status status:1001 ;
	a rdf:Property ;
	rdfs:isDefinedBy <http://rdaregistry.info/Elements/u/> ;
	rdfs:label "is script for radio program"@en ;
	rdfs:subPropertyOf <http://rdaregistry.info/Elements/u/P60198> ;
	owl:inverseOf <http://rdaregistry.info/Elements/u/P60267> ;
	owl:sameAs <http://rdaregistry.info/Elements/u/scriptForTheRadioProgram> ;
	skos:definition "Relates a resource to a resource that uses the text of the source resource as the script for a radio program."@en .

<http://rdaregistry.info/Elements/u/P60286> reg:hasSubproperty <http://rdaregistry.info/Elements/e/P20177> , <http://rdaregistry.info/Elements/w/P10177> ;
	reg:name "addendaTo"@en ;
	reg:status status:1001 ;
	a rdf:Property ;
	rdfs:isDefinedBy <http://rdaregistry.info/Elements/u/> ;
	rdfs:label "is addenda to"@en ;
	rdfs:subPropertyOf <http://rdaregistry.info/Elements/u/P60307> ;
	owl:inverseOf <http://rdaregistry.info/Elements/u/P60209> ;
	owl:sameAs <http://rdaregistry.info/Elements/u/addendaTo> ;
	skos:definition "Relates a resource to a resource to which is added brief additional material, less extensive than a supplement, but essential to the completeness of the content of the resource; it is usually added at the end of the resource, but is sometimes issued separately."@en .

<http://rdaregistry.info/Elements/u/P60287> reg:hasSubproperty <http://rdaregistry.info/Elements/i/P40039> , <http://rdaregistry.info/Elements/m/P30040> ;
	reg:name "digitalTransferOf"@en ;
	reg:status status:1001 ;
	a rdf:Property ;
	rdfs:isDefinedBy <http://rdaregistry.info/Elements/u/> ;
	rdfs:label "is digital transfer of"@en ;
	rdfs:subPropertyOf <http://rdaregistry.info/Elements/u/P60297> ;
	owl:inverseOf <http://rdaregistry.info/Elements/u/P60200> ;
	owl:sameAs <http://rdaregistry.info/Elements/u/digitalTransferOf> ;
	skos:definition "Relates a resource to a resource transferred from one digital format to another."@en .

<http://rdaregistry.info/Elements/u/P60288> reg:hasSubproperty <http://rdaregistry.info/Elements/e/P20178> , <http://rdaregistry.info/Elements/i/P40040> , <http://rdaregistry.info/Elements/m/P30041> , <http://rdaregistry.info/Elements/w/P10178> ;
	reg:name "reviewOf"@en ;
	reg:status status:1001 ;
	a rdf:Property ;
	rdfs:isDefinedBy <http://rdaregistry.info/Elements/u/> ;
	rdfs:label "is review of"@en ;
	rdfs:subPropertyOf <http://rdaregistry.info/Elements/u/P60190> ;
	owl:inverseOf <http://rdaregistry.info/Elements/u/P60211> ;
	owl:sameAs <http://rdaregistry.info/Elements/u/reviewOf> ;
	skos:definition "Relates a resource to a resource used as the basis for a brief evaluation."@en .

<http://rdaregistry.info/Elements/u/P60289> reg:hasSubproperty <http://rdaregistry.info/Elements/e/P20179> , <http://rdaregistry.info/Elements/w/P10179> ;
	reg:name "summaryOf"@en ;
	reg:status status:1001 ;
	a rdf:Property ;
	rdfs:isDefinedBy <http://rdaregistry.info/Elements/u/> ;
	rdfs:label "is summary of"@en ;
	rdfs:subPropertyOf <http://rdaregistry.info/Elements/u/P60305> ;
	owl:inverseOf <http://rdaregistry.info/Elements/u/P60205> ;
	owl:sameAs <http://rdaregistry.info/Elements/u/summaryOf> ;
	skos:definition "Relates a resource to a resource used as the basis for a brief recapitulation of its content."@en .

<http://rdaregistry.info/Elements/u/P60290> reg:hasSubproperty <http://rdaregistry.info/Elements/e/P20180> , <http://rdaregistry.info/Elements/w/P10180> ;
	reg:name "catalogueOf"@en ;
	reg:status status:1001 ;
	a rdf:Property ;
	rdfs:isDefinedBy <http://rdaregistry.info/Elements/u/> ;
	rdfs:label "is catalogue of"@en ;
	rdfs:subPropertyOf <http://rdaregistry.info/Elements/u/P60307> ;
	owl:inverseOf <http://rdaregistry.info/Elements/u/P60206> ;
	owl:sameAs <http://rdaregistry.info/Elements/u/catalogueOf> ;
	skos:definition "Relates a resource to a resource used as the basis for a catalogue, i.e., a complete enumeration of resources arranged systematically."@en .

<http://rdaregistry.info/Elements/u/P60291> reg:hasSubproperty <http://rdaregistry.info/Elements/e/P20181> , <http://rdaregistry.info/Elements/w/P10181> ;
	reg:name "concordanceTo"@en ;
	reg:status status:1001 ;
	a rdf:Property ;
	rdfs:isDefinedBy <http://rdaregistry.info/Elements/u/> ;
	rdfs:label "is concordance to"@en ;
	rdfs:subPropertyOf <http://rdaregistry.info/Elements/u/P60307> ;
	owl:inverseOf <http://rdaregistry.info/Elements/u/P60208> ;
	owl:sameAs <http://rdaregistry.info/Elements/u/concordanceTo> ;
	skos:definition "Relates a resource to a resource used as the basis for a concordance, i.e. an index of all the words in the predominant resource."@en .

<http://rdaregistry.info/Elements/u/P60292> reg:hasSubproperty <http://rdaregistry.info/Elements/e/P20182> , <http://rdaregistry.info/Elements/i/P40041> , <http://rdaregistry.info/Elements/m/P30042> , <http://rdaregistry.info/Elements/w/P10182> ;
	reg:name "critiqueOf"@en ;
	reg:status status:1001 ;
	a rdf:Property ;
	rdfs:isDefinedBy <http://rdaregistry.info/Elements/u/> ;
	rdfs:label "is critique of"@en ;
	rdfs:subPropertyOf <http://rdaregistry.info/Elements/u/P60190> ;
	owl:inverseOf <http://rdaregistry.info/Elements/u/P60212> ;
	owl:sameAs <http://rdaregistry.info/Elements/u/critiqueOf> ;
	skos:definition "Relates a resource to a resource used as the basis for a critical evaluation."@en .

<http://rdaregistry.info/Elements/u/P60293> reg:hasSubproperty <http://rdaregistry.info/Elements/e/P20183> , <http://rdaregistry.info/Elements/w/P10183> ;
	reg:name "choreographyFor"@en ;
	reg:status status:1001 ;
	a rdf:Property ;
	rdfs:isDefinedBy <http://rdaregistry.info/Elements/u/> ;
	rdfs:label "is choreography for"@en ;
	rdfs:subPropertyOf <http://rdaregistry.info/Elements/u/P60305> ;
	owl:inverseOf <http://rdaregistry.info/Elements/u/P60180> ;
	owl:sameAs <http://rdaregistry.info/Elements/u/choreographyFor> ;
	skos:definition "Relates a resource to a resource used as the basis for a derivative resource consisting of dance."@en .

<http://rdaregistry.info/Elements/u/P60294> reg:hasSubproperty <http://rdaregistry.info/Elements/e/P20184> , <http://rdaregistry.info/Elements/w/P10184> ;
	reg:name "expandedVersionOf"@en ;
	reg:status status:1001 ;
	a rdf:Property ;
	rdfs:isDefinedBy <http://rdaregistry.info/Elements/u/> ;
	rdfs:label "is expanded version of"@en ;
	rdfs:subPropertyOf <http://rdaregistry.info/Elements/u/P60305> ;
	owl:inverseOf <http://rdaregistry.info/Elements/u/P60216> ;
	owl:sameAs <http://rdaregistry.info/Elements/u/expandedVersionOf> ;
	skos:definition "Relates a resource to a resource used as the basis for a derivative resource that enlarges upon the content of the source resource."@en .

<http://rdaregistry.info/Elements/u/P60295> reg:hasSubproperty <http://rdaregistry.info/Elements/e/P20185> , <http://rdaregistry.info/Elements/w/P10185> ;
	reg:name "remakeOf"@en ;
	reg:status status:1001 ;
	a rdf:Property ;
	rdfs:isDefinedBy <http://rdaregistry.info/Elements/u/> ;
	rdfs:label "is remake of"@en ;
	rdfs:subPropertyOf <http://rdaregistry.info/Elements/u/P60305> ;
	owl:inverseOf <http://rdaregistry.info/Elements/u/P60120> ;
	owl:sameAs <http://rdaregistry.info/Elements/u/remakeOf> ;
	skos:definition "Relates a resource to a resource used as the basis for a new motion picture, radio program, television program, or video."@en .

<http://rdaregistry.info/Elements/u/P60296> reg:hasSubproperty <http://rdaregistry.info/Elements/e/P20186> , <http://rdaregistry.info/Elements/w/P10186> ;
	reg:name "paraphraseOf"@en ;
	reg:status status:1001 ;
	a rdf:Property ;
	rdfs:isDefinedBy <http://rdaregistry.info/Elements/u/> ;
	rdfs:label "is paraphrase of"@en ;
	rdfs:subPropertyOf <http://rdaregistry.info/Elements/u/P60305> ;
	owl:inverseOf <http://rdaregistry.info/Elements/u/P60273> ;
	owl:sameAs <http://rdaregistry.info/Elements/u/paraphraseOf> ;
	skos:definition "Relates a resource to a resource used as the basis for a paraphrase, i.e., a restating of the content of the source resource in a different form."@en .

<http://rdaregistry.info/Elements/u/P60297> reg:hasSubproperty <http://rdaregistry.info/Elements/i/P40042> , <http://rdaregistry.info/Elements/m/P30043> , <http://rdaregistry.info/Elements/u/P60168> , <http://rdaregistry.info/Elements/u/P60287> , <http://rdaregistry.info/Elements/u/P60301> , <http://rdaregistry.info/Elements/u/P60469> ;
	reg:name "reproductionOf"@en ;
	reg:status status:1001 ;
	a rdf:Property ;
	rdfs:isDefinedBy <http://rdaregistry.info/Elements/u/> ;
	rdfs:label "is reproduction of"@en ;
	rdfs:subPropertyOf <http://rdaregistry.info/Elements/u/P60191> ;
	owl:inverseOf <http://rdaregistry.info/Elements/u/P60272> ;
	owl:sameAs <http://rdaregistry.info/Elements/u/reproductionOf> ;
	skos:definition "Relates a resource to a resource used as the basis for a reproduction."@en .

<http://rdaregistry.info/Elements/u/P60298> reg:hasSubproperty <http://rdaregistry.info/Elements/e/P20187> , <http://rdaregistry.info/Elements/i/P40043> , <http://rdaregistry.info/Elements/m/P30044> , <http://rdaregistry.info/Elements/w/P10187> ;
	reg:name "commentaryOn"@en ;
	reg:status status:1001 ;
	a rdf:Property ;
	rdfs:isDefinedBy <http://rdaregistry.info/Elements/u/> ;
	rdfs:label "is commentary on"@en ;
	rdfs:subPropertyOf <http://rdaregistry.info/Elements/u/P60190> ;
	owl:inverseOf <http://rdaregistry.info/Elements/u/P60213> ;
	owl:sameAs <http://rdaregistry.info/Elements/u/commentaryOn> ;
	skos:definition "Relates a resource to a resource used as the basis for a set of explanatory or critical notes."@en .

<http://rdaregistry.info/Elements/u/P60299> reg:hasSubproperty <http://rdaregistry.info/Elements/i/P40044> , <http://rdaregistry.info/Elements/m/P30045> ;
	reg:name "preservationFacsimileOf"@en ;
	reg:status status:1001 ;
	a rdf:Property ;
	rdfs:isDefinedBy <http://rdaregistry.info/Elements/u/> ;
	rdfs:label "is preservation facsimile of"@en ;
	rdfs:subPropertyOf <http://rdaregistry.info/Elements/u/P60301> ;
	owl:inverseOf <http://rdaregistry.info/Elements/u/P60179> ;
	owl:sameAs <http://rdaregistry.info/Elements/u/preservationFacsimileOf> ;
	skos:definition "Relates a resource to a resource used as the basis for an exact reproduction on preservation-quality media, such as acid-free permanent or archival paper."@en .

<http://rdaregistry.info/Elements/u/P60300> reg:hasSubproperty <http://rdaregistry.info/Elements/m/P30046> ;
	reg:name "facsimileContainerOf"@en ;
	reg:status status:1001 ;
	a rdf:Property ;
	rdfs:isDefinedBy <http://rdaregistry.info/Elements/u/> ;
	rdfs:label "is facsimile container of"@en ;
	rdfs:subPropertyOf <http://rdaregistry.info/Elements/u/P60249> ;
	owl:inverseOf <http://rdaregistry.info/Elements/u/P60100> ;
	owl:sameAs <http://rdaregistry.info/Elements/u/containsFacsimileOf> , <http://rdaregistry.info/Elements/u/facsimileContainerOf> ;
	skos:definition "Relates a resource to a resource used as the basis for an exact reproduction that is a discrete component of a larger entity."@en .

<http://rdaregistry.info/Elements/u/P60301> reg:hasSubproperty <http://rdaregistry.info/Elements/i/P40045> , <http://rdaregistry.info/Elements/m/P30047> , <http://rdaregistry.info/Elements/u/P60299> ;
	reg:name "facsimileOf"@en ;
	reg:status status:1001 ;
	a rdf:Property ;
	rdfs:isDefinedBy <http://rdaregistry.info/Elements/u/> ;
	rdfs:label "is facsimile of"@en ;
	rdfs:subPropertyOf <http://rdaregistry.info/Elements/u/P60297> ;
	owl:inverseOf <http://rdaregistry.info/Elements/u/P60217> ;
	owl:sameAs <http://rdaregistry.info/Elements/u/facsimileOf> ;
	skos:definition "Relates a resource to a resource used as the basis for an exact reproduction."@en .

<http://rdaregistry.info/Elements/u/P60302> reg:hasSubproperty <http://rdaregistry.info/Elements/e/P20188> , <http://rdaregistry.info/Elements/w/P10188> ;
	reg:name "indexTo"@en ;
	reg:status status:1001 ;
	a rdf:Property ;
	rdfs:isDefinedBy <http://rdaregistry.info/Elements/u/> ;
	rdfs:label "is index to"@en ;
	rdfs:subPropertyOf <http://rdaregistry.info/Elements/u/P60307> ;
	owl:inverseOf <http://rdaregistry.info/Elements/u/P60263> ;
	owl:sameAs <http://rdaregistry.info/Elements/u/indexTo> ;
	skos:definition "Relates a resource to a resource used as the basis for an index, i.e., a systematic, alphabetical guide to the contents of the predominant resource, usually keyed to page numbers or other reference codes."@en .

<http://rdaregistry.info/Elements/u/P60303> reg:hasSubproperty <http://rdaregistry.info/Elements/e/P20189> ;
	reg:name "revisionOf"@en ;
	reg:status status:1001 ;
	a rdf:Property ;
	rdfs:isDefinedBy <http://rdaregistry.info/Elements/u/> ;
	rdfs:label "is revision of"@en ;
	rdfs:subPropertyOf <http://rdaregistry.info/Elements/u/P60305> ;
	owl:inverseOf <http://rdaregistry.info/Elements/u/P60245> ;
	owl:sameAs <http://rdaregistry.info/Elements/u/revisionOf> ;
	skos:definition "Relates a resource to a resource used as the basis for an updated, corrected, or expanded version."@en .

<http://rdaregistry.info/Elements/u/P60304> reg:hasSubproperty <http://rdaregistry.info/Elements/e/P20190> , <http://rdaregistry.info/Elements/w/P10189> ;
	reg:name "librettoBasedOn"@en ;
	reg:status status:1001 ;
	a rdf:Property ;
	rdfs:isDefinedBy <http://rdaregistry.info/Elements/u/> ;
	rdfs:label "is libretto based on"@en ;
	rdfs:subPropertyOf <http://rdaregistry.info/Elements/u/P60305> ;
	owl:inverseOf <http://rdaregistry.info/Elements/u/P60210> ;
	owl:sameAs <http://rdaregistry.info/Elements/u/librettoBasedOn> ;
	skos:definition "Relates a resource to a resource used as the basis for the text of an opera or other resource for the musical stage, or an oratorio."@en .

<http://rdaregistry.info/Elements/u/P60305> reg:hasSubproperty <http://rdaregistry.info/Elements/e/P20204> , <http://rdaregistry.info/Elements/u/P60114> , <http://rdaregistry.info/Elements/u/P60223> , <http://rdaregistry.info/Elements/u/P60224> , <http://rdaregistry.info/Elements/u/P60238> , <http://rdaregistry.info/Elements/u/P60241> , <http://rdaregistry.info/Elements/u/P60242> , <http://rdaregistry.info/Elements/u/P60243> , <http://rdaregistry.info/Elements/u/P60244> , <http://rdaregistry.info/Elements/u/P60266> , <http://rdaregistry.info/Elements/u/P60289> , <http://rdaregistry.info/Elements/u/P60293> , <http://rdaregistry.info/Elements/u/P60294> , <http://rdaregistry.info/Elements/u/P60295> , <http://rdaregistry.info/Elements/u/P60296> , <http://rdaregistry.info/Elements/u/P60303> , <http://rdaregistry.info/Elements/u/P60304> , <http://rdaregistry.info/Elements/u/P60308> , <http://rdaregistry.info/Elements/u/P60309> , <http://rdaregistry.info/Elements/u/P60311> , <http://rdaregistry.info/Elements/w/P10190> ;
	reg:name "basedOn"@en ;
	reg:status status:1001 ;
	a rdf:Property ;
	rdfs:isDefinedBy <http://rdaregistry.info/Elements/u/> ;
	rdfs:label "is based on"@en ;
	rdfs:subPropertyOf <http://rdaregistry.info/Elements/u/P60710> ;
	owl:inverseOf <http://rdaregistry.info/Elements/u/P60250> ;
	owl:sameAs <http://rdaregistry.info/Elements/u/basedOn> ;
	skos:definition "Relates a resource to a resource used as the source for a derivative resource."@en .

<http://rdaregistry.info/Elements/u/P60306> reg:hasSubproperty <http://rdaregistry.info/Elements/e/P20191> , <http://rdaregistry.info/Elements/w/P10191> ;
	reg:name "continuedBy"@en ;
	reg:status status:1001 ;
	a rdf:Property ;
	rdfs:isDefinedBy <http://rdaregistry.info/Elements/u/> ;
	rdfs:label "is continued by"@en ;
	rdfs:subPropertyOf <http://rdaregistry.info/Elements/u/P60278> ;
	owl:inverseOf <http://rdaregistry.info/Elements/u/P60576> ;
	owl:sameAs <http://rdaregistry.info/Elements/u/continuedBy> ;
	skos:definition "Relates a resource to a resource whose content continues an earlier resource."@en .

<http://rdaregistry.info/Elements/u/P60307> reg:hasSubproperty <http://rdaregistry.info/Elements/e/P20192> , <http://rdaregistry.info/Elements/u/P60116> , <http://rdaregistry.info/Elements/u/P60251> , <http://rdaregistry.info/Elements/u/P60252> , <http://rdaregistry.info/Elements/u/P60253> , <http://rdaregistry.info/Elements/u/P60254> , <http://rdaregistry.info/Elements/u/P60259> , <http://rdaregistry.info/Elements/u/P60286> , <http://rdaregistry.info/Elements/u/P60290> , <http://rdaregistry.info/Elements/u/P60291> , <http://rdaregistry.info/Elements/u/P60302> , <http://rdaregistry.info/Elements/u/P60474> , <http://rdaregistry.info/Elements/w/P10192> ;
	reg:name "augmentationOf"@en ;
	reg:status status:1001 ;
	a rdf:Property ;
	rdfs:isDefinedBy <http://rdaregistry.info/Elements/u/> ;
	rdfs:label "is augmentation of"@en ;
	rdfs:subPropertyOf <http://rdaregistry.info/Elements/u/P60709> ;
	owl:inverseOf <http://rdaregistry.info/Elements/u/P60204> ;
	owl:sameAs <http://rdaregistry.info/Elements/u/augmentationOf> ;
	skos:definition "Relates a resource to a resource whose content is added to by another resource."@en .

<http://rdaregistry.info/Elements/u/P60308> reg:hasSubproperty <http://rdaregistry.info/Elements/e/P20193> , <http://rdaregistry.info/Elements/w/P10193> ;
	reg:name "abstractsFor"@en ;
	reg:status status:1001 ;
	a rdf:Property ;
	rdfs:isDefinedBy <http://rdaregistry.info/Elements/u/> ;
	rdfs:label "is abstracts for"@en ;
	rdfs:subPropertyOf <http://rdaregistry.info/Elements/u/P60305> ;
	owl:inverseOf <http://rdaregistry.info/Elements/u/P60177> ;
	owl:sameAs <http://rdaregistry.info/Elements/u/abstractsFor> ;
	skos:definition "Relates a resource to a resource whose contents have been abstracted by an abstracting and indexing service."@en .

<http://rdaregistry.info/Elements/u/P60309> reg:hasSubproperty <http://rdaregistry.info/Elements/e/P20194> , <http://rdaregistry.info/Elements/w/P10194> ;
	reg:name "indexingFor"@en ;
	reg:status status:1001 ;
	a rdf:Property ;
	rdfs:isDefinedBy <http://rdaregistry.info/Elements/u/> ;
	rdfs:label "is indexing for"@en ;
	rdfs:subPropertyOf <http://rdaregistry.info/Elements/u/P60305> ;
	owl:inverseOf <http://rdaregistry.info/Elements/u/P60178> ;
	owl:sameAs <http://rdaregistry.info/Elements/u/indexingFor> ;
	skos:definition "Relates a resource to a resource whose contents have been indexed by an abstracting and indexing service."@en .

<http://rdaregistry.info/Elements/u/P60310> reg:hasSubproperty <http://rdaregistry.info/Elements/w/P10195> ;
	reg:name "prequelTo"@en ;
	reg:status status:1001 ;
	a rdf:Property ;
	rdfs:isDefinedBy <http://rdaregistry.info/Elements/u/> ;
	rdfs:label "is prequel to"@en ;
	rdfs:subPropertyOf <http://rdaregistry.info/Elements/u/P60278> ;
	owl:inverseOf <http://rdaregistry.info/Elements/u/P60220> ;
	owl:sameAs <http://rdaregistry.info/Elements/u/prequelTo> ;
	skos:definition "Relates a resource to a resource whose narrative is extended backwards in time by the later resource."@en .

<http://rdaregistry.info/Elements/u/P60311> reg:hasSubproperty <http://rdaregistry.info/Elements/e/P20195> , <http://rdaregistry.info/Elements/u/P60312> , <http://rdaregistry.info/Elements/w/P10196> ;
	reg:name "imitationOf"@en ;
	reg:status status:1001 ;
	a rdf:Property ;
	rdfs:isDefinedBy <http://rdaregistry.info/Elements/u/> ;
	rdfs:label "is imitation of"@en ;
	rdfs:subPropertyOf <http://rdaregistry.info/Elements/u/P60305> ;
	owl:inverseOf <http://rdaregistry.info/Elements/u/P60214> ;
	owl:sameAs <http://rdaregistry.info/Elements/u/imitationOf> ;
	skos:definition "Relates a resource to a resource whose style or content is copied in a derivative resource."@en .

<http://rdaregistry.info/Elements/u/P60312> reg:hasSubproperty <http://rdaregistry.info/Elements/e/P20196> , <http://rdaregistry.info/Elements/w/P10197> ;
	reg:name "parodyOf"@en ;
	reg:status status:1001 ;
	a rdf:Property ;
	rdfs:isDefinedBy <http://rdaregistry.info/Elements/u/> ;
	rdfs:label "is parody of"@en ;
	rdfs:subPropertyOf <http://rdaregistry.info/Elements/u/P60311> ;
	owl:inverseOf <http://rdaregistry.info/Elements/u/P60246> ;
	owl:sameAs <http://rdaregistry.info/Elements/u/parodyOf> ;
	skos:definition "Relates a resource to a resource whose style or content is imitated for comic effect."@en .

<http://rdaregistry.info/Elements/u/P60313> reg:hasSubproperty <http://rdaregistry.info/Elements/e/P20205> , <http://rdaregistry.info/Elements/m/P30048> , <http://rdaregistry.info/Elements/m/P30140> , <http://rdaregistry.info/Elements/w/P10198> ;
	reg:name "relatedResource"@en ;
	reg:status status:1001 ;
	a rdf:Property ;
	rdfs:isDefinedBy <http://rdaregistry.info/Elements/u/> ;
	rdfs:label "has related resource"@en ;
	owl:sameAs <http://rdaregistry.info/Elements/u/relatedResource> ;
	skos:definition "Relates a resource to a resource, represented by an identifier, an authorized access point, or a description, that is related to the resource being described."@en .

<http://rdaregistry.info/Elements/u/P60314> reg:hasSubproperty <http://rdaregistry.info/Elements/m/P30096> ;
	reg:name "encodingFormat"@en ;
	reg:status status:1001 ;
	a rdf:Property ;
	rdfs:isDefinedBy <http://rdaregistry.info/Elements/u/> ;
	rdfs:label "has encoding format"@en ;
	rdfs:subPropertyOf <http://rdaregistry.info/Elements/u/P60350> ;
	owl:sameAs <http://rdaregistry.info/Elements/u/encodingFormat> ;
	skos:definition "Relates a resource to a schema, standard, etc., used to encode the digital content of a resource."@en .

<http://rdaregistry.info/Elements/u/P60315> reg:hasSubproperty <http://rdaregistry.info/Elements/w/P10079> ;
	reg:name "numericDesignationOfAMusicalResource"@en ;
	reg:status status:1001 ;
	a rdf:Property ;
	rdfs:isDefinedBy <http://rdaregistry.info/Elements/u/> ;
	rdfs:label "has numeric designation of a musical resource"@en ;
	owl:sameAs <http://rdaregistry.info/Elements/u/numericDesignationOfAMusicalResource> ;
	skos:definition "Relates a resource to a serial number, opus number, or thematic index number assigned to a musical resource by a composer, publisher, or a musicologist."@en .

<http://rdaregistry.info/Elements/u/P60316> reg:hasSubproperty <http://rdaregistry.info/Elements/w/P10080> ;
	reg:name "subseries"@en ;
	reg:status status:1001 ;
	a rdf:Property ;
	rdfs:isDefinedBy <http://rdaregistry.info/Elements/u/> ;
	rdfs:label "is subseries"@en ;
	rdfs:subPropertyOf <http://rdaregistry.info/Elements/u/P60249> ;
	owl:inverseOf <http://rdaregistry.info/Elements/u/P60192> ;
	owl:sameAs <http://rdaregistry.info/Elements/u/subseries> ;
	skos:definition "Relates a resource to a serial or multipart resource that consistently appears in a larger resource; the title of the larger resource appears on all issues or parts of the subseries"@en .

<http://rdaregistry.info/Elements/u/P60317> reg:hasSubproperty <http://rdaregistry.info/Elements/m/P30101> ;
	reg:name "specialIssueOf"@en ;
	reg:status status:1001 ;
	a rdf:Property ;
	rdfs:isDefinedBy <http://rdaregistry.info/Elements/u/> ;
	rdfs:label "is special issue of"@en ;
	rdfs:subPropertyOf <http://rdaregistry.info/Elements/u/P60101> ;
	owl:inverseOf <http://rdaregistry.info/Elements/u/P60207> ;
	owl:sameAs <http://rdaregistry.info/Elements/u/specialIssueOf> ;
	skos:definition "Relates a resource to a serial or newspaper containing a single issue or a supplementary section devoted to a special subject, with or without serial numbering, such as an anniversary number of a periodical or newspaper."@en .

<http://rdaregistry.info/Elements/u/P60318> reg:hasSubproperty <http://rdaregistry.info/Elements/e/P20061> ;
	reg:name "formOfTactileNotation"@en ;
	reg:status status:1001 ;
	a rdf:Property ;
	rdfs:isDefinedBy <http://rdaregistry.info/Elements/u/> ;
	rdfs:label "has form of tactile notation"@en ;
	rdfs:subPropertyOf <http://rdaregistry.info/Elements/u/P60319> ;
	owl:sameAs <http://rdaregistry.info/Elements/u/formOfTactileNotation> ;
	skos:definition "Relates a resource to a set of characters and/or symbols used to express the content of a resource in a form that can be perceived through touch."@en .

<http://rdaregistry.info/Elements/u/P60319> reg:hasSubproperty <http://rdaregistry.info/Elements/e/P20062> , <http://rdaregistry.info/Elements/u/P60318> , <http://rdaregistry.info/Elements/u/P60320> , <http://rdaregistry.info/Elements/u/P60321> , <http://rdaregistry.info/Elements/u/P60322> ;
	reg:name "formOfNotation"@en ;
	reg:status status:1001 ;
	a rdf:Property ;
	rdfs:isDefinedBy <http://rdaregistry.info/Elements/u/> ;
	rdfs:label "has form of notation"@en ;
	owl:sameAs <http://rdaregistry.info/Elements/u/formOfNotation> ;
	skos:definition "Relates a resource to a set of characters and/or symbols used to express the content of a resource."@en .

<http://rdaregistry.info/Elements/u/P60320> reg:hasSubproperty <http://rdaregistry.info/Elements/e/P20063> ;
	reg:name "formOfNotatedMovement"@en ;
	reg:status status:1001 ;
	a rdf:Property ;
	rdfs:isDefinedBy <http://rdaregistry.info/Elements/u/> ;
	rdfs:label "has form of notated movement"@en ;
	rdfs:subPropertyOf <http://rdaregistry.info/Elements/u/P60319> ;
	owl:sameAs <http://rdaregistry.info/Elements/u/formOfNotatedMovement> ;
	skos:definition "Relates a resource to a set of characters and/or symbols used to express the movement content of a resource."@en .

<http://rdaregistry.info/Elements/u/P60321> reg:hasSubproperty <http://rdaregistry.info/Elements/e/P20064> ;
	reg:name "formOfMusicalNotation"@en ;
	reg:status status:1001 ;
	a rdf:Property ;
	rdfs:isDefinedBy <http://rdaregistry.info/Elements/u/> ;
	rdfs:label "has form of musical notation"@en ;
	rdfs:subPropertyOf <http://rdaregistry.info/Elements/u/P60319> ;
	owl:sameAs <http://rdaregistry.info/Elements/u/formOfMusicalNotation> ;
	skos:definition "Relates a resource to a set of characters and/or symbols used to express the musical content of a resource."@en .

<http://rdaregistry.info/Elements/u/P60322> reg:hasSubproperty <http://rdaregistry.info/Elements/e/P20065> ;
	reg:name "script"@en ;
	reg:status status:1001 ;
	a rdf:Property ;
	rdfs:isDefinedBy <http://rdaregistry.info/Elements/u/> ;
	rdfs:label "has script"@en ;
	rdfs:subPropertyOf <http://rdaregistry.info/Elements/u/P60319> ;
	owl:sameAs <http://rdaregistry.info/Elements/u/script> ;
	skos:definition "Relates a resource to a set of characters and/or symbols used to express the written language content of a resource."@en .

<http://rdaregistry.info/Elements/u/P60323> reg:hasSubproperty <http://rdaregistry.info/Elements/m/P30102> ;
	reg:name "digitalRepresentationOfCartographicContent"@en ;
	reg:status status:1001 ;
	a rdf:Property ;
	rdfs:isDefinedBy <http://rdaregistry.info/Elements/u/> ;
	rdfs:label "has digital representation of cartographic content"@en ;
	rdfs:subPropertyOf <http://rdaregistry.info/Elements/u/P60350> ;
	owl:sameAs <http://rdaregistry.info/Elements/u/digitalRepresentationOfCartographicContent> ;
	skos:definition "Relates a resource to a set of technical details relating to the encoding of geospatial information in a cartographic resource."@en .

<http://rdaregistry.info/Elements/u/P60324> reg:hasSubproperty <http://rdaregistry.info/Elements/a/P50040> , <http://rdaregistry.info/Elements/a/P50058> , <http://rdaregistry.info/Elements/a/P50107> , <http://rdaregistry.info/Elements/u/P60076> , <http://rdaregistry.info/Elements/u/P60524> , <http://rdaregistry.info/Elements/u/P60525> , <http://rdaregistry.info/Elements/u/P60526> , <http://rdaregistry.info/Elements/u/P60598> , <http://rdaregistry.info/Elements/u/P60599> ;
	reg:name "dateAssociatedWithTheAgent"@en ;
	reg:status status:1001 ;
	a rdf:Property ;
	rdfs:isDefinedBy <http://rdaregistry.info/Elements/u/> ;
	rdfs:label "has date associated with the agent"@en ;
	owl:sameAs <http://rdaregistry.info/Elements/u/dateAssociatedWithTheAgent> ;
	skos:definition "Relates a resource to a significant date associated with an agent (e.g., date of birth, date of death), or the date or range of dates on which a conference, etc., was held, or a date with which an agent is otherwise associated (e.g., date of founding)."@en .

<http://rdaregistry.info/Elements/u/P60325> reg:hasSubproperty <http://rdaregistry.info/Elements/a/P50031> , <http://rdaregistry.info/Elements/a/P50057> , <http://rdaregistry.info/Elements/u/P60064> , <http://rdaregistry.info/Elements/u/P60107> ;
	reg:name "placeAssociatedWithTheAgent"@en ;
	reg:status status:1001 ;
	a rdf:Property ;
	rdfs:isDefinedBy <http://rdaregistry.info/Elements/u/> ;
	rdfs:label "has place associated with the agent"@en ;
	owl:sameAs <http://rdaregistry.info/Elements/u/placeAssociatedWithTheAgent> ;
	skos:definition "Relates a resource to a significant location associated with an agent (e.g., location of a conference, etc., location of the headquarters of an organization, or a place where an agent resides or has resided or has some connection."@en .

<http://rdaregistry.info/Elements/u/P60326> reg:hasSubproperty <http://rdaregistry.info/Elements/m/P30104> ;
	reg:name "videoFormat"@en ;
	reg:status status:1001 ;
	a rdf:Property ;
	rdfs:isDefinedBy <http://rdaregistry.info/Elements/u/> ;
	rdfs:label "has video format"@en ;
	rdfs:subPropertyOf <http://rdaregistry.info/Elements/u/P60352> ;
	owl:sameAs <http://rdaregistry.info/Elements/u/videoFormat> ;
	skos:definition "Relates a resource to a standard, etc., used to encode the analog video content of a resource."@en .

<http://rdaregistry.info/Elements/u/P60327> reg:hasSubproperty <http://rdaregistry.info/Elements/m/P30105> ;
	reg:name "statementOfResponsibilityRelatingToTitleProper"@en ;
	reg:status status:1001 ;
	a rdf:Property ;
	rdfs:isDefinedBy <http://rdaregistry.info/Elements/u/> ;
	rdfs:label "has statement of responsibility relating to title proper"@en ;
	rdfs:subPropertyOf <http://rdaregistry.info/Elements/u/P60339> ;
	owl:sameAs <http://rdaregistry.info/Elements/u/statementOfResponsibilityRelatingToTitleProper> ;
	skos:definition "Relates a resource to a statement associated with the title proper of a resource that relates to the identification and/or function of any agents responsible for the creation of, or contributing to the realization of, the intellectual or artistic content of the resource."@en .

<http://rdaregistry.info/Elements/u/P60328> reg:hasSubproperty <http://rdaregistry.info/Elements/m/P30106> ;
	reg:name "seriesStatement"@en ;
	reg:status status:1001 ;
	a rdf:Property ;
	rdfs:isDefinedBy <http://rdaregistry.info/Elements/u/> ;
	rdfs:label "has series statement"@en ;
	owl:sameAs <http://rdaregistry.info/Elements/u/seriesStatement> ;
	skos:definition "Relates a resource to a statement identifying a series to which a resource belongs and the numbering of the resource within the series."@en .

<http://rdaregistry.info/Elements/u/P60329> reg:hasSubproperty <http://rdaregistry.info/Elements/m/P30107> ;
	reg:name "editionStatement"@en ;
	reg:status status:1001 ;
	a rdf:Property ;
	rdfs:isDefinedBy <http://rdaregistry.info/Elements/u/> ;
	rdfs:label "has edition statement"@en ;
	owl:sameAs <http://rdaregistry.info/Elements/u/editionStatement> ;
	skos:definition "Relates a resource to a statement identifying the edition to which a resource belongs."@en .

<http://rdaregistry.info/Elements/u/P60330> reg:hasSubproperty <http://rdaregistry.info/Elements/m/P30108> ;
	reg:name "distributionStatement"@en ;
	reg:status status:1001 ;
	a rdf:Property ;
	rdfs:isDefinedBy <http://rdaregistry.info/Elements/u/> ;
	rdfs:label "has distribution statement"@en ;
	owl:sameAs <http://rdaregistry.info/Elements/u/distributionStatement> ;
	skos:definition "Relates a resource to a statement identifying the place or places of distribution, distributor or distributors, and date or dates of distribution of a resource in a published form."@en .

<http://rdaregistry.info/Elements/u/P60331> reg:hasSubproperty <http://rdaregistry.info/Elements/m/P30109> ;
	reg:name "manufactureStatement"@en ;
	reg:status status:1001 ;
	a rdf:Property ;
	rdfs:isDefinedBy <http://rdaregistry.info/Elements/u/> ;
	rdfs:label "has manufacture statement"@en ;
	owl:sameAs <http://rdaregistry.info/Elements/u/manufactureStatement> ;
	skos:definition "Relates a resource to a statement identifying the place or places of manufacture, manufacturer or manufacturers, and date or dates of manufacture of a resource in a published form."@en .

<http://rdaregistry.info/Elements/u/P60332> reg:hasSubproperty <http://rdaregistry.info/Elements/m/P30110> ;
	reg:name "productionStatement"@en ;
	reg:status status:1001 ;
	a rdf:Property ;
	rdfs:isDefinedBy <http://rdaregistry.info/Elements/u/> ;
	rdfs:label "has production statement"@en ;
	owl:sameAs <http://rdaregistry.info/Elements/u/productionStatement> ;
	skos:definition "Relates a resource to a statement identifying the place or places of production, producer or producers, and date or dates of production of a resource in an unpublished form."@en .

<http://rdaregistry.info/Elements/u/P60333> reg:hasSubproperty <http://rdaregistry.info/Elements/m/P30111> ;
	reg:name "publicationStatement"@en ;
	reg:status status:1001 ;
	a rdf:Property ;
	rdfs:isDefinedBy <http://rdaregistry.info/Elements/u/> ;
	rdfs:label "has publication statement"@en ;
	owl:sameAs <http://rdaregistry.info/Elements/u/publicationStatement> ;
	skos:definition "Relates a resource to a statement identifying the place or places of publication, publisher or publishers, and date or dates of publication of a resource."@en .

<http://rdaregistry.info/Elements/u/P60334> reg:hasSubproperty <http://rdaregistry.info/Elements/m/P30112> ;
	reg:name "parallelStatementOfResponsibilityRelatingToANamedRevisionOfAnEdition"@en ;
	reg:status status:1001 ;
	a rdf:Property ;
	rdfs:isDefinedBy <http://rdaregistry.info/Elements/u/> ;
	rdfs:label "has parallel statement of responsibility relating to a named revision of an edition"@en ;
	owl:sameAs <http://rdaregistry.info/Elements/u/parallelStatementOfResponsibilityRelatingToANamedRevisionOfAnEdition> ;
	skos:definition "Relates a resource to a statement of responsibility relating to a named revision of an edition in a language and/or script that differs from that recorded in the statement of responsibility relating to a named revision of an edition element."@en .

<http://rdaregistry.info/Elements/u/P60335> reg:hasSubproperty <http://rdaregistry.info/Elements/m/P30113> ;
	reg:name "parallelStatementOfResponsibilityRelatingToSeries"@en ;
	reg:status status:1001 ;
	a rdf:Property ;
	rdfs:isDefinedBy <http://rdaregistry.info/Elements/u/> ;
	rdfs:label "has parallel statement of responsibility relating to series"@en ;
	owl:sameAs <http://rdaregistry.info/Elements/u/parallelStatementOfResponsibilityRelatingToSeries> ;
	skos:definition "Relates a resource to a statement of responsibility relating to series in a language and/or script that differs from that recorded in the statement of responsibility relating to series element."@en .

<http://rdaregistry.info/Elements/u/P60336> reg:hasSubproperty <http://rdaregistry.info/Elements/m/P30114> ;
	reg:name "parallelStatementOfResponsibilityRelatingToSubseries"@en ;
	reg:status status:1001 ;
	a rdf:Property ;
	rdfs:isDefinedBy <http://rdaregistry.info/Elements/u/> ;
	rdfs:label "has parallel statement of responsibility relating to subseries"@en ;
	owl:sameAs <http://rdaregistry.info/Elements/u/parallelStatementOfResponsibilityRelatingToSubseries> ;
	skos:definition "Relates a resource to a statement of responsibility relating to subseries in a language and/or script that differs from that recorded in the statement of responsibility relating to subseries element."@en .

<http://rdaregistry.info/Elements/u/P60337> reg:hasSubproperty <http://rdaregistry.info/Elements/m/P30115> ;
	reg:name "parallelStatementOfResponsibilityRelatingToTheEdition"@en ;
	reg:status status:1001 ;
	a rdf:Property ;
	rdfs:isDefinedBy <http://rdaregistry.info/Elements/u/> ;
	rdfs:label "has parallel statement of responsibility relating to the edition"@en ;
	owl:sameAs <http://rdaregistry.info/Elements/u/parallelStatementOfResponsibilityRelatingToTheEdition> ;
	skos:definition "Relates a resource to a statement of responsibility relating to the edition in a language and/or script that differs from that recorded in the statement of responsibility relating to the edition element."@en .

<http://rdaregistry.info/Elements/u/P60338> reg:hasSubproperty <http://rdaregistry.info/Elements/m/P30116> ;
	reg:name "parallelStatementOfResponsibilityRelatingToTitleProper"@en ;
	reg:status status:1001 ;
	a rdf:Property ;
	rdfs:isDefinedBy <http://rdaregistry.info/Elements/u/> ;
	rdfs:label "has parallel statement of responsibility relating to title proper"@en ;
	rdfs:subPropertyOf <http://rdaregistry.info/Elements/u/P60339> ;
	owl:sameAs <http://rdaregistry.info/Elements/u/parallelStatementOfResponsibilityRelatingToTitleProper> ;
	skos:definition "Relates a resource to a statement of responsibility relating to title proper in a language and/or script that differs from that recorded in the statement of responsibility relating to title proper element."@en .

<http://rdaregistry.info/Elements/u/P60339> reg:hasSubproperty <http://rdaregistry.info/Elements/m/P30117> , <http://rdaregistry.info/Elements/u/P60327> , <http://rdaregistry.info/Elements/u/P60338> ;
	reg:name "statementOfResponsibility"@en ;
	reg:status status:1001 ;
	a rdf:Property ;
	rdfs:isDefinedBy <http://rdaregistry.info/Elements/u/> ;
	rdfs:label "has statement of responsibility"@en ;
	owl:sameAs <http://rdaregistry.info/Elements/u/statementOfResponsibility> ;
	skos:definition "Relates a resource to a statement relating to the identification and/or function of any agents responsible for the creation of, or contributing to the realization of, the intellectual or artistic content of a resource."@en .

<http://rdaregistry.info/Elements/u/P60340> reg:hasSubproperty <http://rdaregistry.info/Elements/m/P30118> ;
	reg:name "statementOfResponsibilityRelatingToANamedRevisionOfAnEdition"@en ;
	reg:status status:1001 ;
	a rdf:Property ;
	rdfs:isDefinedBy <http://rdaregistry.info/Elements/u/> ;
	rdfs:label "has statement of responsibility relating to a named revision of an edition"@en ;
	owl:sameAs <http://rdaregistry.info/Elements/u/statementOfResponsibilityRelatingToANamedRevisionOfAnEdition> ;
	skos:definition "Relates a resource to a statement relating to the identification of any agents responsible for a named revision of an edition."@en .

<http://rdaregistry.info/Elements/u/P60341> reg:hasSubproperty <http://rdaregistry.info/Elements/m/P30119> ;
	reg:name "statementOfResponsibilityRelatingToSeries"@en ;
	reg:status status:1001 ;
	a rdf:Property ;
	rdfs:isDefinedBy <http://rdaregistry.info/Elements/u/> ;
	rdfs:label "has statement of responsibility relating to series"@en ;
	owl:sameAs <http://rdaregistry.info/Elements/u/statementOfResponsibilityRelatingToSeries> ;
	skos:definition "Relates a resource to a statement relating to the identification of any agents responsible for a series."@en .

<http://rdaregistry.info/Elements/u/P60342> reg:hasSubproperty <http://rdaregistry.info/Elements/m/P30120> ;
	reg:name "statementOfResponsibilityRelatingToSubseries"@en ;
	reg:status status:1001 ;
	a rdf:Property ;
	rdfs:isDefinedBy <http://rdaregistry.info/Elements/u/> ;
	rdfs:label "has statement of responsibility relating to subseries"@en ;
	owl:sameAs <http://rdaregistry.info/Elements/u/statementOfResponsibilityRelatingToSubseries> ;
	skos:definition "Relates a resource to a statement relating to the identification of any agents responsible for a subseries."@en .

<http://rdaregistry.info/Elements/u/P60343> reg:hasSubproperty <http://rdaregistry.info/Elements/m/P30121> ;
	reg:name "statementOfResponsibilityRelatingToTheEdition"@en ;
	reg:status status:1001 ;
	a rdf:Property ;
	rdfs:isDefinedBy <http://rdaregistry.info/Elements/u/> ;
	rdfs:label "has statement of responsibility relating to the edition"@en ;
	owl:sameAs <http://rdaregistry.info/Elements/u/statementOfResponsibilityRelatingToTheEdition> ;
	skos:definition "Relates a resource to a statement relating to the identification of any agents responsible for the edition being described but not to all editions."@en .

<http://rdaregistry.info/Elements/u/P60344> reg:hasSubproperty <http://rdaregistry.info/Elements/m/P30122> ;
	reg:name "emulsionOnMicrofilmAndMicrofiche"@en ;
	reg:status status:1001 ;
	a rdf:Property ;
	rdfs:isDefinedBy <http://rdaregistry.info/Elements/u/> ;
	rdfs:label "has emulsion on microfilm and microfiche"@en ;
	rdfs:subPropertyOf <http://rdaregistry.info/Elements/u/P60159> ;
	owl:sameAs <http://rdaregistry.info/Elements/u/emulsionOnMicrofilmAndMicrofiche> ;
	skos:definition "Relates a resource to a suspension of light-sensitive chemicals used as a coating on a microfilm or microfiche (e.g., silver halide)."@en .

<http://rdaregistry.info/Elements/u/P60345> reg:hasSubproperty <http://rdaregistry.info/Elements/w/P10081> ;
	reg:name "longitudeAndLatitude"@en ;
	reg:status status:1001 ;
	a rdf:Property ;
	rdfs:isDefinedBy <http://rdaregistry.info/Elements/u/> ;
	rdfs:label "has longitude and latitude"@en ;
	rdfs:subPropertyOf <http://rdaregistry.info/Elements/u/P60109> ;
	owl:sameAs <http://rdaregistry.info/Elements/u/longitudeAndLatitude> ;
	skos:definition "Relates a resource to a system for identifying the area covered by the cartographic content of a resource using longitude of the westernmost and easternmost boundaries and latitude of the northernmost and southernmost boundaries."@en .

<http://rdaregistry.info/Elements/u/P60346> reg:hasSubproperty <http://rdaregistry.info/Elements/w/P10082> ;
	reg:name "rightAscensionAndDeclination"@en ;
	reg:status status:1001 ;
	a rdf:Property ;
	rdfs:isDefinedBy <http://rdaregistry.info/Elements/u/> ;
	rdfs:label "has right ascension and declination"@en ;
	rdfs:subPropertyOf <http://rdaregistry.info/Elements/u/P60109> ;
	owl:sameAs <http://rdaregistry.info/Elements/u/rightAscensionAndDeclination> ;
	skos:definition "Relates a resource to a system for identifying the location of a celestial object in the sky covered by the cartographic content of a resource using the angles of right ascension and declination."@en .

<http://rdaregistry.info/Elements/u/P60347> reg:hasSubproperty <http://rdaregistry.info/Elements/w/P10083> ;
	reg:name "stringsOfCoordinatePairs"@en ;
	reg:status status:1001 ;
	a rdf:Property ;
	rdfs:isDefinedBy <http://rdaregistry.info/Elements/u/> ;
	rdfs:label "has strings of coordinate pairs"@en ;
	rdfs:subPropertyOf <http://rdaregistry.info/Elements/u/P60109> ;
	owl:sameAs <http://rdaregistry.info/Elements/u/stringsOfCoordinatePairs> ;
	skos:definition "Relates a resource to a system for identifying the precise area covered by the cartographic content of a resource using coordinates for each vertex of a polygon."@en .

<http://rdaregistry.info/Elements/u/P60348> reg:hasSubproperty <http://rdaregistry.info/Elements/w/P10084> ;
	reg:name "systemOfOrganization"@en ;
	reg:status status:1001 ;
	a rdf:Property ;
	rdfs:isDefinedBy <http://rdaregistry.info/Elements/u/> ;
	rdfs:label "has system of organization"@en ;
	owl:sameAs <http://rdaregistry.info/Elements/u/systemOfOrganization> ;
	skos:definition "Relates a resource to a system of arranging materials in an archival resource or a collection."@en .

<http://rdaregistry.info/Elements/u/P60349> reg:hasSubproperty <http://rdaregistry.info/Elements/m/P30123> ;
	reg:name "broadcastStandard"@en ;
	reg:status status:1001 ;
	a rdf:Property ;
	rdfs:isDefinedBy <http://rdaregistry.info/Elements/u/> ;
	rdfs:label "has broadcast standard"@en ;
	rdfs:subPropertyOf <http://rdaregistry.info/Elements/u/P60352> ;
	owl:sameAs <http://rdaregistry.info/Elements/u/broadcastStandard> ;
	skos:definition "Relates a resource to a system used to format a video resource for television broadcast."@en .

<http://rdaregistry.info/Elements/u/P60350> reg:hasSubproperty <http://rdaregistry.info/Elements/m/P30124> , <http://rdaregistry.info/Elements/u/P60059> , <http://rdaregistry.info/Elements/u/P60093> , <http://rdaregistry.info/Elements/u/P60314> , <http://rdaregistry.info/Elements/u/P60323> , <http://rdaregistry.info/Elements/u/P60519> , <http://rdaregistry.info/Elements/u/P60551> , <http://rdaregistry.info/Elements/u/P60587> ;
	reg:name "digitalFileCharacteristic"@en ;
	reg:status status:1001 ;
	a rdf:Property ;
	rdfs:isDefinedBy <http://rdaregistry.info/Elements/u/> ;
	rdfs:label "has digital file characteristic"@en ;
	owl:sameAs <http://rdaregistry.info/Elements/u/digitalFileCharacteristic> ;
	skos:definition "Relates a resource to a technical specification relating to the digital encoding of text, image, audio, video, and other types of data in a resource."@en .

<http://rdaregistry.info/Elements/u/P60351> reg:hasSubproperty <http://rdaregistry.info/Elements/m/P30125> , <http://rdaregistry.info/Elements/u/P60481> , <http://rdaregistry.info/Elements/u/P60522> , <http://rdaregistry.info/Elements/u/P60532> , <http://rdaregistry.info/Elements/u/P60543> , <http://rdaregistry.info/Elements/u/P60552> , <http://rdaregistry.info/Elements/u/P60553> , <http://rdaregistry.info/Elements/u/P60586> , <http://rdaregistry.info/Elements/u/P60594> ;
	reg:name "soundCharacteristic"@en ;
	reg:status status:1001 ;
	a rdf:Property ;
	rdfs:isDefinedBy <http://rdaregistry.info/Elements/u/> ;
	rdfs:label "has sound characteristic"@en ;
	owl:sameAs <http://rdaregistry.info/Elements/u/soundCharacteristic> ;
	skos:definition "Relates a resource to a technical specification relating to the encoding of sound in a resource."@en .

<http://rdaregistry.info/Elements/u/P60352> reg:hasSubproperty <http://rdaregistry.info/Elements/m/P30126> , <http://rdaregistry.info/Elements/u/P60326> , <http://rdaregistry.info/Elements/u/P60349> ;
	reg:name "videoCharacteristic"@en ;
	reg:status status:1001 ;
	a rdf:Property ;
	rdfs:isDefinedBy <http://rdaregistry.info/Elements/u/> ;
	rdfs:label "has video characteristic"@en ;
	owl:sameAs <http://rdaregistry.info/Elements/u/videoCharacteristic> ;
	skos:definition "Relates a resource to a technical specification relating to the encoding of video images in a resource."@en .

<http://rdaregistry.info/Elements/u/P60353> reg:hasSubproperty <http://rdaregistry.info/Elements/m/P30127> , <http://rdaregistry.info/Elements/u/P60529> , <http://rdaregistry.info/Elements/u/P60585> ;
	reg:name "projectionCharacteristicOfMotionPictureFilm"@en ;
	reg:status status:1001 ;
	a rdf:Property ;
	rdfs:isDefinedBy <http://rdaregistry.info/Elements/u/> ;
	rdfs:label "has projection characteristic of motion picture film"@en ;
	owl:sameAs <http://rdaregistry.info/Elements/u/projectionCharacteristicOfMotionPictureFilm> ;
	skos:definition "Relates a resource to a technical specification relating to the projection of a motion picture film."@en .

<http://rdaregistry.info/Elements/u/P60354> reg:hasSubproperty <http://rdaregistry.info/Elements/e/P20066> , <http://rdaregistry.info/Elements/w/P10085> ;
	reg:name "adaptedAsATelevisionProgram"@en ;
	reg:status status:1001 ;
	a rdf:Property ;
	rdfs:isDefinedBy <http://rdaregistry.info/Elements/u/> ;
	rdfs:label "is adapted as television program"@en ;
	rdfs:subPropertyOf <http://rdaregistry.info/Elements/u/P60260> ;
	owl:inverseOf <http://rdaregistry.info/Elements/u/P60230> ;
	owl:sameAs <http://rdaregistry.info/Elements/u/adaptedAsATelevisionProgram> ;
	skos:definition "Relates a resource to a television program based on the source resource."@en .

<http://rdaregistry.info/Elements/u/P60355> reg:hasSubproperty <http://rdaregistry.info/Elements/m/P30128> , <http://rdaregistry.info/Elements/w/P10086> ;
	reg:name "variantTitle"@en ;
	reg:status status:1001 ;
	a rdf:Property ;
	rdfs:isDefinedBy <http://rdaregistry.info/Elements/u/> ;
	rdfs:label "has variant title"@en ;
	rdfs:subPropertyOf <http://rdaregistry.info/Elements/u/P60369> ;
	owl:sameAs <http://rdaregistry.info/Elements/u/variantTitle> ;
	skos:definition "Relates a resource to a title associated with a resource that differs from a title recorded as the preferred title, title proper, a parallel title proper, other title information, parallel other title information, earlier title proper, later title proper, key title, or abbreviated title."@en .

<http://rdaregistry.info/Elements/u/P60356> reg:hasSubproperty <http://rdaregistry.info/Elements/a/P50059> ;
	reg:name "hereditaryTitle"@en ;
	reg:status status:1001 ;
	a rdf:Property ;
	rdfs:isDefinedBy <http://rdaregistry.info/Elements/u/> ;
	rdfs:label "has hereditary title"@en ;
	owl:sameAs <http://rdaregistry.info/Elements/u/hereditaryTitle> ;
	skos:definition "Relates a resource to a title of nobility, etc., associated with an agent."@en .

<http://rdaregistry.info/Elements/u/P60357> reg:hasSubproperty <http://rdaregistry.info/Elements/m/P30129> ;
	reg:name "laterTitleProper"@en ;
	reg:status status:1001 ;
	a rdf:Property ;
	rdfs:isDefinedBy <http://rdaregistry.info/Elements/u/> ;
	rdfs:label "has later title proper"@en ;
	rdfs:subPropertyOf <http://rdaregistry.info/Elements/u/P60369> ;
	owl:sameAs <http://rdaregistry.info/Elements/u/laterTitleProper> ;
	skos:definition "Relates a resource to a title proper appearing on a later issue or part of a multipart monograph or serial that differs from that on the first or earliest issue or part."@en .

<http://rdaregistry.info/Elements/u/P60358> reg:hasSubproperty <http://rdaregistry.info/Elements/m/P30130> ;
	reg:name "earlierTitleProper"@en ;
	reg:status status:1001 ;
	a rdf:Property ;
	rdfs:isDefinedBy <http://rdaregistry.info/Elements/u/> ;
	rdfs:label "has earlier title proper"@en ;
	rdfs:subPropertyOf <http://rdaregistry.info/Elements/u/P60369> ;
	owl:sameAs <http://rdaregistry.info/Elements/u/earlierTitleProper> ;
	skos:definition "Relates a resource to a title proper appearing on an earlier iteration of an integrating resource that differs from that on the current iteration."@en .

<http://rdaregistry.info/Elements/u/P60359> reg:hasSubproperty <http://rdaregistry.info/Elements/m/P30131> ;
	reg:name "abbreviatedTitle"@en ;
	reg:status status:1001 ;
	a rdf:Property ;
	rdfs:isDefinedBy <http://rdaregistry.info/Elements/u/> ;
	rdfs:label "has abbreviated title"@en ;
	rdfs:subPropertyOf <http://rdaregistry.info/Elements/u/P60369> ;
	owl:sameAs <http://rdaregistry.info/Elements/u/abbreviatedTitle> ;
	skos:definition "Relates a resource to a title that has been abbreviated for purposes of indexing or identification."@en .

<http://rdaregistry.info/Elements/u/P60360> reg:hasSubproperty <http://rdaregistry.info/Elements/a/P50109> ;
	reg:name "placeOfResidenceEtc"@en ;
	reg:status status:1001 ;
	a rdf:Property ;
	rdfs:isDefinedBy <http://rdaregistry.info/Elements/u/> ;
	rdfs:label "has place of residence, etc."@en ;
	owl:sameAs <http://rdaregistry.info/Elements/u/placeOfResidenceEtc> ;
	skos:definition "Relates a resource to a town, city, province, state, and/or country in which an agent resides or has resided, or another significant place associated with the agent other than place of birth, place of death, or residence (e.g., a place where an agent has worked or studied)."@en .

<http://rdaregistry.info/Elements/u/P60361> reg:hasSubproperty <http://rdaregistry.info/Elements/e/P20067> , <http://rdaregistry.info/Elements/w/P10087> ;
	reg:name "adaptedAsAVideo"@en ;
	reg:status status:1001 ;
	a rdf:Property ;
	rdfs:isDefinedBy <http://rdaregistry.info/Elements/u/> ;
	rdfs:label "is adapted as video"@en ;
	rdfs:subPropertyOf <http://rdaregistry.info/Elements/u/P60260> ;
	owl:inverseOf <http://rdaregistry.info/Elements/u/P60236> ;
	owl:sameAs <http://rdaregistry.info/Elements/u/adaptedAsAVideo> ;
	skos:definition "Relates a resource to a video based on the source resource."@en .

<http://rdaregistry.info/Elements/u/P60362> reg:hasSubproperty <http://rdaregistry.info/Elements/a/P50060> ;
	reg:name "prominentMemberOfTheFamily"@en ;
	reg:status status:1001 ;
	a rdf:Property ;
	rdfs:isDefinedBy <http://rdaregistry.info/Elements/u/> ;
	rdfs:label "has prominent member of the agent"@en ;
	owl:sameAs <http://rdaregistry.info/Elements/u/prominentMemberOfTheFamily> ;
	skos:definition "Relates a resource to a well-known individual who is a member of an agent."@en .

<http://rdaregistry.info/Elements/u/P60363> reg:hasSubproperty <http://rdaregistry.info/Elements/a/P50110> ;
	reg:name "titleOfTheAgent"@en ;
	reg:status status:1001 ;
	a rdf:Property ;
	rdfs:isDefinedBy <http://rdaregistry.info/Elements/u/> ;
	rdfs:label "has title of the agent"@en ;
	owl:sameAs <http://rdaregistry.info/Elements/u/titleOfTheAgent> ;
	skos:definition "Relates a resource to a word or phrase indicative of royalty, nobility, or ecclesiastical rank or office, a term of address for an agent of religious vocation, or another term indicative of rank, honour, or office."@en .

<http://rdaregistry.info/Elements/u/P60364> reg:hasSubproperty <http://rdaregistry.info/Elements/m/P30132> ;
	reg:name "designationOfANamedRevisionOfAnEdition"@en ;
	reg:status status:1001 ;
	a rdf:Property ;
	rdfs:isDefinedBy <http://rdaregistry.info/Elements/u/> ;
	rdfs:label "has designation of a named revision of an edition"@en ;
	owl:sameAs <http://rdaregistry.info/Elements/u/designationOfANamedRevisionOfAnEdition> ;
	skos:definition "Relates a resource to a word, character or group of words and/or characters, identifying a particular revision of a named edition."@en .

<http://rdaregistry.info/Elements/u/P60365> reg:hasSubproperty <http://rdaregistry.info/Elements/m/P30133> ;
	reg:name "designationOfEdition"@en ;
	reg:status status:1001 ;
	a rdf:Property ;
	rdfs:isDefinedBy <http://rdaregistry.info/Elements/u/> ;
	rdfs:label "has designation of edition"@en ;
	owl:sameAs <http://rdaregistry.info/Elements/u/designationOfEdition> ;
	skos:definition "Relates a resource to a word, character or group of words and/or characters, identifying the edition to which a resource belongs."@en .

<http://rdaregistry.info/Elements/u/P60366> reg:hasSubproperty <http://rdaregistry.info/Elements/u/P60548> ;
	reg:name "nameOfThePlace"@en ;
	reg:status status:1001 ;
	a rdf:Property ;
	rdfs:isDefinedBy <http://rdaregistry.info/Elements/u/> ;
	rdfs:label "has name of the place"@en ;
	owl:sameAs <http://rdaregistry.info/Elements/u/nameOfThePlace> ;
	skos:definition "Relates a resource to a word, character, or group of words and/or characters by which a place is known."@en .

<http://rdaregistry.info/Elements/u/P60367> reg:hasSubproperty <http://rdaregistry.info/Elements/u/P60588> , <http://rdaregistry.info/Elements/w/P10088> ;
	reg:name "titleOfTheResource"@en ;
	reg:status status:1001 ;
	a rdf:Property ;
	rdfs:isDefinedBy <http://rdaregistry.info/Elements/u/> ;
	rdfs:label "has title of the resource"@en ;
	owl:sameAs <http://rdaregistry.info/Elements/u/titleOfTheResource> ;
	skos:definition "Relates a resource to a word, character, or group of words and/or characters by which a resource is known."@en .

<http://rdaregistry.info/Elements/u/P60368> reg:hasSubproperty <http://rdaregistry.info/Elements/a/P50032> , <http://rdaregistry.info/Elements/a/P50061> , <http://rdaregistry.info/Elements/a/P50111> , <http://rdaregistry.info/Elements/u/P60119> , <http://rdaregistry.info/Elements/u/P60549> ;
	reg:name "nameOfTheAgent"@en ;
	reg:status status:1001 ;
	a rdf:Property ;
	rdfs:isDefinedBy <http://rdaregistry.info/Elements/u/> ;
	rdfs:label "has name of the agent"@en ;
	owl:sameAs <http://rdaregistry.info/Elements/u/nameOfTheAgent> ;
	skos:definition "Relates a resource to a word, character, or group of words and/or characters by which an agent is known."@en .

<http://rdaregistry.info/Elements/u/P60369> reg:hasSubproperty <http://rdaregistry.info/Elements/m/P30134> , <http://rdaregistry.info/Elements/u/P60355> , <http://rdaregistry.info/Elements/u/P60357> , <http://rdaregistry.info/Elements/u/P60358> , <http://rdaregistry.info/Elements/u/P60359> , <http://rdaregistry.info/Elements/u/P60493> , <http://rdaregistry.info/Elements/u/P60507> , <http://rdaregistry.info/Elements/u/P60515> , <http://rdaregistry.info/Elements/u/P60589> , <http://rdaregistry.info/Elements/u/P60597> ;
	reg:name "title"@en ;
	reg:status status:1001 ;
	a rdf:Property ;
	rdfs:isDefinedBy <http://rdaregistry.info/Elements/u/> ;
	rdfs:label "has title"@en ;
	owl:sameAs <http://rdaregistry.info/Elements/u/title> ;
	skos:definition "Relates a resource to a word, character, or group of words and/or characters that names a resource or a resource contained in it."@en .

<http://rdaregistry.info/Elements/u/P60370> reg:hasSubproperty <http://rdaregistry.info/Elements/a/P50033> , <http://rdaregistry.info/Elements/a/P50108> ;
	reg:name "otherDesignationAssociatedWithTheAgent"@en ;
	reg:status status:1001 ;
	a rdf:Property ;
	rdfs:isDefinedBy <http://rdaregistry.info/Elements/u/> ;
	rdfs:label "has other designation associated with the agent"@en ;
	owl:sameAs <http://rdaregistry.info/Elements/u/otherDesignationAssociatedWithTheAgent> ;
	skos:definition "Relates a resource to a word, phrase, or abbreviation indicating incorporation or legal status of an agent, or any term serving to differentiate the body from other corporate bodies, persons, etc., or a term other than a title that is associated with an agent’s name."@en .

<http://rdaregistry.info/Elements/u/P60371> reg:hasSubproperty <http://rdaregistry.info/Elements/e/P20068> ;
	reg:name "writerOfAddedLyrics"@en ;
	reg:status status:1001 ;
	a rdf:Property ;
	rdfs:isDefinedBy <http://rdaregistry.info/Elements/u/> ;
	rdfs:label "has writer of added lyrics"@en ;
	rdfs:subPropertyOf <http://rdaregistry.info/Elements/u/P60380> ;
	owl:inverseOf <http://rdaregistry.info/Elements/u/P60600> ;
	owl:sameAs <http://rdaregistry.info/Elements/u/writerOfAddedLyrics> ;
	skos:closeMatch "http://id.loc.gov/vocabulary/relators/wal"@en ;
	skos:definition "Relates a resource to a writer of words added to a musical resource."@en .

<http://rdaregistry.info/Elements/u/P60372> reg:hasSubproperty <http://rdaregistry.info/Elements/e/P20069> ;
	reg:name "summarizationOfTheContent"@en ;
	reg:status status:1001 ;
	a rdf:Property ;
	rdfs:isDefinedBy <http://rdaregistry.info/Elements/u/> ;
	rdfs:label "has summarization of the content"@en ;
	owl:sameAs <http://rdaregistry.info/Elements/u/summarizationOfTheContent> ;
	skos:definition "Relates a resource to an abstract, summary, synopsis, etc., of the content of a resource."@en .

<http://rdaregistry.info/Elements/u/P60373> reg:hasSubproperty <http://rdaregistry.info/Elements/w/P10005> , <http://rdaregistry.info/Elements/w/P10035> , <http://rdaregistry.info/Elements/w/P10037> ;
	reg:name "appellee"@en ;
	reg:status status:1001 ;
	a rdf:Property ;
	rdfs:isDefinedBy <http://rdaregistry.info/Elements/u/> ;
	rdfs:label "has appellee"@en ;
	rdfs:subPropertyOf <http://rdaregistry.info/Elements/u/P60374> ;
	owl:inverseOf <http://rdaregistry.info/Elements/u/P60601> ;
	owl:sameAs <http://rdaregistry.info/Elements/u/appellee> ;
	skos:closeMatch "http://id.loc.gov/vocabulary/relators/ape"@en ;
	skos:definition "Relates a resource to an agent against whom an appeal is taken."@en .

<http://rdaregistry.info/Elements/u/P60374> reg:hasSubproperty <http://rdaregistry.info/Elements/i/P40023> , <http://rdaregistry.info/Elements/m/P30079> , <http://rdaregistry.info/Elements/u/P60060> , <http://rdaregistry.info/Elements/u/P60061> , <http://rdaregistry.info/Elements/u/P60062> , <http://rdaregistry.info/Elements/u/P60065> , <http://rdaregistry.info/Elements/u/P60097> , <http://rdaregistry.info/Elements/u/P60157> , <http://rdaregistry.info/Elements/u/P60373> , <http://rdaregistry.info/Elements/u/P60375> , <http://rdaregistry.info/Elements/u/P60376> , <http://rdaregistry.info/Elements/u/P60406> , <http://rdaregistry.info/Elements/u/P60421> , <http://rdaregistry.info/Elements/u/P60441> , <http://rdaregistry.info/Elements/u/P60449> , <http://rdaregistry.info/Elements/u/P60450> , <http://rdaregistry.info/Elements/u/P60451> , <http://rdaregistry.info/Elements/u/P60455> , <http://rdaregistry.info/Elements/u/P60456> , <http://rdaregistry.info/Elements/u/P60457> , <http://rdaregistry.info/Elements/u/P60458> , <http://rdaregistry.info/Elements/u/P60459> , <http://rdaregistry.info/Elements/u/P60460> , <http://rdaregistry.info/Elements/u/P60461> , <http://rdaregistry.info/Elements/u/P60462> , <http://rdaregistry.info/Elements/u/P60464> , <http://rdaregistry.info/Elements/u/P60466> , <http://rdaregistry.info/Elements/u/P60467> , <http://rdaregistry.info/Elements/w/P10047> ;
	reg:name "otherPFCAssociatedWithAResource"@en ;
	reg:status status:1001 ;
	a rdf:Property ;
	rdfs:isDefinedBy <http://rdaregistry.info/Elements/u/> ;
	rdfs:label "has other agent associated with a resource"@en ;
	owl:inverseOf <http://rdaregistry.info/Elements/u/P60602> ;
	owl:sameAs <http://rdaregistry.info/Elements/u/otherAgentAssociatedWithAResource> , <http://rdaregistry.info/Elements/u/otherPFCResource> ;
	skos:definition "Relates a resource to an agent other than a creator, custodian, owner, producer, publisher, distributor or manufacturer associated with a resource."@en ;
	skos:scopeNote "Includes book designers, platemakers, etc. Includes persons, etc., to whom correspondence is addressed, persons, etc., honoured by a festschrift, directors, cinematographers, sponsoring bodies, production companies, institutions, etc., hosting an exhibition or event, etc. Includes curators, binders, restorationists, etc."@en .

<http://rdaregistry.info/Elements/u/P60375> reg:hasSubproperty <http://rdaregistry.info/Elements/w/P10048> ;
	reg:name "dedicator"@en ;
	reg:status status:1001 ;
	a rdf:Property ;
	rdfs:isDefinedBy <http://rdaregistry.info/Elements/u/> ;
	rdfs:label "has dedicator"@en ;
	rdfs:subPropertyOf <http://rdaregistry.info/Elements/u/P60374> ;
	owl:inverseOf <http://rdaregistry.info/Elements/u/P60603> ;
	owl:sameAs <http://rdaregistry.info/Elements/u/dedicator> ;
	skos:closeMatch "http://id.loc.gov/vocabulary/relators/dto"@en ;
	skos:definition "Relates a resource to an agent by whom a resource is dedicated."@en .

<http://rdaregistry.info/Elements/u/P60376> reg:hasSubproperty <http://rdaregistry.info/Elements/i/P40017> , <http://rdaregistry.info/Elements/u/P60066> , <http://rdaregistry.info/Elements/u/P60067> ;
	reg:name "curator"@en ;
	reg:status status:1001 ;
	a rdf:Property ;
	rdfs:isDefinedBy <http://rdaregistry.info/Elements/u/> ;
	rdfs:label "has curator"@en ;
	rdfs:subPropertyOf <http://rdaregistry.info/Elements/u/P60374> ;
	owl:inverseOf <http://rdaregistry.info/Elements/u/P60604> ;
	owl:sameAs <http://rdaregistry.info/Elements/u/curator> ;
	skos:closeMatch "http://id.loc.gov/vocabulary/relators/cur"@en ;
	skos:definition "Relates a resource to an agent conceiving, aggregating, and/or organizing an exhibition, collection, or other resource."@en .

<http://rdaregistry.info/Elements/u/P60377> reg:hasSubproperty <http://rdaregistry.info/Elements/e/P20027> ;
	reg:name "surveyor"@en ;
	reg:status status:1001 ;
	a rdf:Property ;
	rdfs:isDefinedBy <http://rdaregistry.info/Elements/u/> ;
	rdfs:label "has surveyor"@en ;
	rdfs:subPropertyOf <http://rdaregistry.info/Elements/u/P60398> ;
	owl:inverseOf <http://rdaregistry.info/Elements/u/P60605> ;
	owl:sameAs <http://rdaregistry.info/Elements/u/surveyor> ;
	skos:closeMatch "http://id.loc.gov/vocabulary/relators/srv"@en ;
	skos:definition "Relates a resource to an agent contributing to a cartographic resource by providing measurements or dimensional relationships for the geographic area represented."@en .

<http://rdaregistry.info/Elements/u/P60378> reg:hasSubproperty <http://rdaregistry.info/Elements/e/P20028> ;
	reg:name "animator"@en ;
	reg:status status:1001 ;
	a rdf:Property ;
	rdfs:isDefinedBy <http://rdaregistry.info/Elements/u/> ;
	rdfs:label "has animator"@en ;
	rdfs:subPropertyOf <http://rdaregistry.info/Elements/u/P60398> ;
	owl:inverseOf <http://rdaregistry.info/Elements/u/P60606> ;
	owl:sameAs <http://rdaregistry.info/Elements/u/animator> ;
	skos:closeMatch "http://id.loc.gov/vocabulary/relators/anm"@en ;
	skos:definition "Relates a resource to an agent contributing to a moving image resource or computer program by giving apparent movement to inanimate objects or drawings."@en .

<http://rdaregistry.info/Elements/u/P60379> reg:hasSubproperty <http://rdaregistry.info/Elements/e/P20029> ;
	reg:name "arrangerOfMusic"@en ;
	reg:status status:1001 ;
	a rdf:Property ;
	rdfs:isDefinedBy <http://rdaregistry.info/Elements/u/> ;
	rdfs:label "has arranger of music"@en ;
	rdfs:subPropertyOf <http://rdaregistry.info/Elements/u/P60398> ;
	owl:inverseOf <http://rdaregistry.info/Elements/u/P60607> ;
	owl:sameAs <http://rdaregistry.info/Elements/u/arrangerOfMusic> ;
	skos:closeMatch "http://id.loc.gov/vocabulary/relators/arr"@en ;
	skos:definition "Relates a resource to an agent contributing to a musical resource by rewriting the composition for a medium of performance different from that for which the resource was originally intended."@en .

<http://rdaregistry.info/Elements/u/P60380> reg:hasSubproperty <http://rdaregistry.info/Elements/e/P20030> , <http://rdaregistry.info/Elements/u/P60371> ;
	reg:name "writerOfAddedText"@en ;
	reg:status status:1001 ;
	a rdf:Property ;
	rdfs:isDefinedBy <http://rdaregistry.info/Elements/u/> ;
	rdfs:label "has writer of added text"@en ;
	rdfs:subPropertyOf <http://rdaregistry.info/Elements/u/P60392> ;
	owl:inverseOf <http://rdaregistry.info/Elements/u/P60608> ;
	owl:sameAs <http://rdaregistry.info/Elements/u/writerOfAddedText> ;
	skos:closeMatch "http://id.loc.gov/vocabulary/relators/wat"@en ;
	skos:definition "Relates a resource to an agent contributing to a primarily non-textual resource by providing text for the non-textual resource (e.g., writing captions for photographs, descriptions of maps)."@en .

<http://rdaregistry.info/Elements/u/P60381> reg:hasSubproperty <http://rdaregistry.info/Elements/e/P20033> ;
	reg:name "draftsman"@en ;
	reg:status status:1001 ;
	a rdf:Property ;
	rdfs:isDefinedBy <http://rdaregistry.info/Elements/u/> ;
	rdfs:label "has draftsman"@en ;
	rdfs:subPropertyOf <http://rdaregistry.info/Elements/u/P60398> ;
	owl:inverseOf <http://rdaregistry.info/Elements/u/P60609> ;
	owl:sameAs <http://rdaregistry.info/Elements/u/draftsman> ;
	skos:closeMatch "http://id.loc.gov/vocabulary/relators/drm"@en ;
	skos:definition "Relates a resource to an agent contributing to a resource by an architect, inventor, etc., by making detailed plans or drawings for buildings, ships, aircraft, machines, objects, etc."@en .

<http://rdaregistry.info/Elements/u/P60382> reg:hasSubproperty <http://rdaregistry.info/Elements/e/P20034> ;
	reg:name "transcriber"@en ;
	reg:status status:1001 ;
	a rdf:Property ;
	rdfs:isDefinedBy <http://rdaregistry.info/Elements/u/> ;
	rdfs:label "has transcriber"@en ;
	rdfs:subPropertyOf <http://rdaregistry.info/Elements/u/P60398> ;
	owl:inverseOf <http://rdaregistry.info/Elements/u/P60610> ;
	owl:sameAs <http://rdaregistry.info/Elements/u/transcriber> ;
	skos:closeMatch "http://id.loc.gov/vocabulary/relators/trc"@en ;
	skos:definition "Relates a resource to an agent contributing to a resource by changing it from one system of notation to another."@en .

<http://rdaregistry.info/Elements/u/P60383> reg:hasSubproperty <http://rdaregistry.info/Elements/e/P20035> ;
	reg:name "musicalDirector"@en ;
	reg:status status:1001 ;
	a rdf:Property ;
	rdfs:isDefinedBy <http://rdaregistry.info/Elements/u/> ;
	rdfs:label "has musical director"@en ;
	rdfs:subPropertyOf <http://rdaregistry.info/Elements/u/P60398> ;
	owl:inverseOf <http://rdaregistry.info/Elements/u/P60611> ;
	owl:sameAs <http://rdaregistry.info/Elements/u/musicalDirector> ;
	skos:closeMatch "http://id.loc.gov/vocabulary/relators/msd"@en ;
	skos:definition "Relates a resource to an agent contributing to a resource by coordinating the activities of the composer, the sound editor, and sound mixers for a moving image production or for a musical or dramatic presentation or entertainment."@en .

<http://rdaregistry.info/Elements/u/P60384> reg:hasSubproperty <http://rdaregistry.info/Elements/e/P20036> ;
	reg:name "costumeDesigner"@en ;
	reg:status status:1001 ;
	a rdf:Property ;
	rdfs:isDefinedBy <http://rdaregistry.info/Elements/u/> ;
	rdfs:label "has costume designer"@en ;
	rdfs:subPropertyOf <http://rdaregistry.info/Elements/u/P60398> ;
	owl:inverseOf <http://rdaregistry.info/Elements/u/P60612> ;
	owl:sameAs <http://rdaregistry.info/Elements/u/costumeDesigner> ;
	skos:closeMatch "http://id.loc.gov/vocabulary/relators/cst"@en ;
	skos:definition "Relates a resource to an agent contributing to a resource by designing the costumes for a moving image production or for a musical or dramatic presentation or entertainment."@en .

<http://rdaregistry.info/Elements/u/P60385> reg:hasSubproperty <http://rdaregistry.info/Elements/e/P20037> ;
	reg:name "translator"@en ;
	reg:status status:1001 ;
	a rdf:Property ;
	rdfs:isDefinedBy <http://rdaregistry.info/Elements/u/> ;
	rdfs:label "has translator"@en ;
	rdfs:subPropertyOf <http://rdaregistry.info/Elements/u/P60398> ;
	owl:inverseOf <http://rdaregistry.info/Elements/u/P60613> ;
	owl:sameAs <http://rdaregistry.info/Elements/u/translator> ;
	skos:closeMatch "http://id.loc.gov/vocabulary/relators/trl"@en ;
	skos:definition """Relates a resource to an agent contributing to a resource by expressing the original text of the resource in a language different from that of the original resource.
"""@en .

<http://rdaregistry.info/Elements/u/P60386> reg:hasSubproperty <http://rdaregistry.info/Elements/e/P20038> ;
	reg:name "artDirector"@en ;
	reg:status status:1001 ;
	a rdf:Property ;
	rdfs:isDefinedBy <http://rdaregistry.info/Elements/u/> ;
	rdfs:label "has art director"@en ;
	rdfs:subPropertyOf <http://rdaregistry.info/Elements/u/P60398> ;
	owl:inverseOf <http://rdaregistry.info/Elements/u/P60614> ;
	owl:sameAs <http://rdaregistry.info/Elements/u/artDirector> ;
	skos:closeMatch "http://id.loc.gov/vocabulary/relators/adi"@en ;
	skos:definition "Relates a resource to an agent contributing to a resource by overseeing the artists and craftspeople who build the sets for moving image productions."@en .

<http://rdaregistry.info/Elements/u/P60387> reg:hasSubproperty <http://rdaregistry.info/Elements/e/P20039> , <http://rdaregistry.info/Elements/u/P60141> , <http://rdaregistry.info/Elements/u/P60142> , <http://rdaregistry.info/Elements/u/P60143> , <http://rdaregistry.info/Elements/u/P60144> , <http://rdaregistry.info/Elements/u/P60145> , <http://rdaregistry.info/Elements/u/P60146> , <http://rdaregistry.info/Elements/u/P60147> , <http://rdaregistry.info/Elements/u/P60148> , <http://rdaregistry.info/Elements/u/P60149> , <http://rdaregistry.info/Elements/u/P60150> , <http://rdaregistry.info/Elements/u/P60151> , <http://rdaregistry.info/Elements/u/P60153> , <http://rdaregistry.info/Elements/u/P60154> , <http://rdaregistry.info/Elements/u/P60155> , <http://rdaregistry.info/Elements/u/P60156> ;
	reg:name "performer"@en ;
	reg:status status:1001 ;
	a rdf:Property ;
	rdfs:isDefinedBy <http://rdaregistry.info/Elements/u/> ;
	rdfs:label "has performer"@en ;
	rdfs:subPropertyOf <http://rdaregistry.info/Elements/u/P60398> ;
	owl:inverseOf <http://rdaregistry.info/Elements/u/P60615> ;
	owl:sameAs <http://rdaregistry.info/Elements/u/performer> ;
	skos:closeMatch "http://id.loc.gov/vocabulary/relators/prf"@en ;
	skos:definition "Relates a resource to an agent contributing to a resource by performing music, acting, dancing, speaking, etc., often in a musical or dramatic presentation, etc."@en .

<http://rdaregistry.info/Elements/u/P60388> reg:hasSubproperty <http://rdaregistry.info/Elements/e/P20040> ;
	reg:name "courtReporter"@en ;
	reg:status status:1001 ;
	a rdf:Property ;
	rdfs:isDefinedBy <http://rdaregistry.info/Elements/u/> ;
	rdfs:label "has court reporter"@en ;
	rdfs:subPropertyOf <http://rdaregistry.info/Elements/u/P60398> ;
	owl:inverseOf <http://rdaregistry.info/Elements/u/P60616> ;
	owl:sameAs <http://rdaregistry.info/Elements/u/courtReporter> ;
	skos:closeMatch "http://id.loc.gov/vocabulary/relators/crt"@en ;
	skos:definition "Relates a resource to an agent contributing to a resource by preparing a court’s opinions for publication."@en .

<http://rdaregistry.info/Elements/u/P60389> reg:hasSubproperty <http://rdaregistry.info/Elements/e/P20041> ;
	reg:name "writerOfPreface"@en ;
	reg:status status:1001 ;
	a rdf:Property ;
	rdfs:isDefinedBy <http://rdaregistry.info/Elements/u/> ;
	rdfs:label "has writer of preface"@en ;
	rdfs:subPropertyOf <http://rdaregistry.info/Elements/u/P60392> ;
	owl:inverseOf <http://rdaregistry.info/Elements/u/P60617> ;
	owl:sameAs <http://rdaregistry.info/Elements/u/writerOfPreface> ;
	skos:closeMatch "http://id.loc.gov/vocabulary/relators/wpr"@en ;
	skos:definition "Relates a resource to an agent contributing to a resource by providing a preface to the original resource."@en .

<http://rdaregistry.info/Elements/u/P60390> reg:hasSubproperty <http://rdaregistry.info/Elements/e/P20044> ;
	reg:name "writerOfAddedCommentary"@en ;
	reg:status status:1001 ;
	a rdf:Property ;
	rdfs:isDefinedBy <http://rdaregistry.info/Elements/u/> ;
	rdfs:label "has writer of added commentary"@en ;
	rdfs:subPropertyOf <http://rdaregistry.info/Elements/u/P60392> ;
	owl:inverseOf <http://rdaregistry.info/Elements/u/P60618> ;
	owl:sameAs <http://rdaregistry.info/Elements/u/writerOfAddedCommentary> ;
	skos:closeMatch "http://id.loc.gov/vocabulary/relators/wac"@en ;
	skos:definition "Relates a resource to an agent contributing to a resource by providing an interpretation or critical explanation of the original resource."@en .

<http://rdaregistry.info/Elements/u/P60391> reg:hasSubproperty <http://rdaregistry.info/Elements/e/P20045> ;
	reg:name "writerOfIntroduction"@en ;
	reg:status status:1001 ;
	a rdf:Property ;
	rdfs:isDefinedBy <http://rdaregistry.info/Elements/u/> ;
	rdfs:label "has writer of introduction"@en ;
	rdfs:subPropertyOf <http://rdaregistry.info/Elements/u/P60392> ;
	owl:inverseOf <http://rdaregistry.info/Elements/u/P60619> ;
	owl:sameAs <http://rdaregistry.info/Elements/u/writerOfIntroduction> ;
	skos:closeMatch "http://id.loc.gov/vocabulary/relators/win"@en ;
	skos:definition "Relates a resource to an agent contributing to a resource by providing an introduction to the original resource."@en .

<http://rdaregistry.info/Elements/u/P60392> reg:hasSubproperty <http://rdaregistry.info/Elements/e/P20046> , <http://rdaregistry.info/Elements/u/P60380> , <http://rdaregistry.info/Elements/u/P60389> , <http://rdaregistry.info/Elements/u/P60390> , <http://rdaregistry.info/Elements/u/P60391> ;
	reg:name "writerOfSupplementaryTextualContent"@en ;
	reg:status status:1001 ;
	a rdf:Property ;
	rdfs:isDefinedBy <http://rdaregistry.info/Elements/u/> ;
	rdfs:label "has writer of supplementary textual content"@en ;
	rdfs:subPropertyOf <http://rdaregistry.info/Elements/u/P60398> ;
	owl:inverseOf <http://rdaregistry.info/Elements/u/P60620> ;
	owl:sameAs <http://rdaregistry.info/Elements/u/writerOfSupplementaryTextualContent> ;
	skos:closeMatch "http://id.loc.gov/vocabulary/relators/wst"@en ;
	skos:definition "Relates a resource to an agent contributing to a resource by providing supplementary textual content (e.g., an appendix, an introduction, a preface) to the original resource."@en .

<http://rdaregistry.info/Elements/u/P60393> reg:hasSubproperty <http://rdaregistry.info/Elements/e/P20048> ;
	reg:name "editor"@en ;
	reg:status status:1001 ;
	a rdf:Property ;
	rdfs:isDefinedBy <http://rdaregistry.info/Elements/u/> ;
	rdfs:label "has editor"@en ;
	rdfs:subPropertyOf <http://rdaregistry.info/Elements/u/P60398> ;
	owl:inverseOf <http://rdaregistry.info/Elements/u/P60621> ;
	owl:sameAs <http://rdaregistry.info/Elements/u/editor> ;
	skos:closeMatch "http://id.loc.gov/vocabulary/relators/edt"@en ;
	skos:definition "Relates a resource to an agent contributing to a resource by revising or clarifying the content, e.g., adding an introduction, notes, or other critical matter."@en .

<http://rdaregistry.info/Elements/u/P60394> reg:hasSubproperty <http://rdaregistry.info/Elements/e/P20049> ;
	reg:name "abridger"@en ;
	reg:status status:1001 ;
	a rdf:Property ;
	rdfs:isDefinedBy <http://rdaregistry.info/Elements/u/> ;
	rdfs:label "has abridger"@en ;
	rdfs:subPropertyOf <http://rdaregistry.info/Elements/u/P60398> ;
	owl:inverseOf <http://rdaregistry.info/Elements/u/P60622> ;
	owl:sameAs <http://rdaregistry.info/Elements/u/abridger> ;
	skos:closeMatch "http://id.loc.gov/vocabulary/relators/abr"@en ;
	skos:definition "Relates a resource to an agent contributing to a resource by shortening or condensing the original resource but leaving the nature and content of the original resource substantially unchanged."@en .

<http://rdaregistry.info/Elements/u/P60395> reg:hasSubproperty <http://rdaregistry.info/Elements/e/P20050> ;
	reg:name "recordingEngineer"@en ;
	reg:status status:1001 ;
	a rdf:Property ;
	rdfs:isDefinedBy <http://rdaregistry.info/Elements/u/> ;
	rdfs:label "has recording engineer"@en ;
	rdfs:subPropertyOf <http://rdaregistry.info/Elements/u/P60398> ;
	owl:inverseOf <http://rdaregistry.info/Elements/u/P60623> ;
	owl:sameAs <http://rdaregistry.info/Elements/u/recordingEngineer> ;
	skos:closeMatch "http://id.loc.gov/vocabulary/relators/rce"@en ;
	skos:definition "Relates a resource to an agent contributing to a resource by supervising the technical aspects of a sound or video recording session."@en .

<http://rdaregistry.info/Elements/u/P60396> reg:hasSubproperty <http://rdaregistry.info/Elements/e/P20051> ;
	reg:name "illustrator"@en ;
	reg:status status:1001 ;
	a rdf:Property ;
	rdfs:isDefinedBy <http://rdaregistry.info/Elements/u/> ;
	rdfs:label "has illustrator"@en ;
	rdfs:subPropertyOf <http://rdaregistry.info/Elements/u/P60398> ;
	owl:inverseOf <http://rdaregistry.info/Elements/u/P60624> ;
	owl:sameAs <http://rdaregistry.info/Elements/u/illustrator> ;
	skos:closeMatch "http://id.loc.gov/vocabulary/relators/ill"@en ;
	skos:definition "Relates a resource to an agent contributing to a resource by supplementing the primary content with drawings, diagrams, photographs, etc."@en .

<http://rdaregistry.info/Elements/u/P60397> reg:hasSubproperty <http://rdaregistry.info/Elements/e/P20052> ;
	reg:name "recordist"@en ;
	reg:status status:1001 ;
	a rdf:Property ;
	rdfs:isDefinedBy <http://rdaregistry.info/Elements/u/> ;
	rdfs:label "has recordist"@en ;
	rdfs:subPropertyOf <http://rdaregistry.info/Elements/u/P60398> ;
	owl:inverseOf <http://rdaregistry.info/Elements/u/P60625> ;
	owl:sameAs <http://rdaregistry.info/Elements/u/recordist> ;
	skos:closeMatch "http://id.loc.gov/vocabulary/relators/rcd"@en ;
	skos:definition "Relates a resource to an agent contributing to a resource by using a recording device to capture sound and/or video during a recording session, including field recordings of natural sounds, folkloric events, music, etc."@en .

<http://rdaregistry.info/Elements/u/P60398> reg:hasSubproperty <http://rdaregistry.info/Elements/e/P20053> , <http://rdaregistry.info/Elements/u/P60377> , <http://rdaregistry.info/Elements/u/P60378> , <http://rdaregistry.info/Elements/u/P60379> , <http://rdaregistry.info/Elements/u/P60381> , <http://rdaregistry.info/Elements/u/P60382> , <http://rdaregistry.info/Elements/u/P60383> , <http://rdaregistry.info/Elements/u/P60384> , <http://rdaregistry.info/Elements/u/P60385> , <http://rdaregistry.info/Elements/u/P60386> , <http://rdaregistry.info/Elements/u/P60387> , <http://rdaregistry.info/Elements/u/P60388> , <http://rdaregistry.info/Elements/u/P60392> , <http://rdaregistry.info/Elements/u/P60393> , <http://rdaregistry.info/Elements/u/P60394> , <http://rdaregistry.info/Elements/u/P60395> , <http://rdaregistry.info/Elements/u/P60396> , <http://rdaregistry.info/Elements/u/P60397> , <http://rdaregistry.info/Elements/u/P60399> , <http://rdaregistry.info/Elements/u/P60419> , <http://rdaregistry.info/Elements/u/P60422> , <http://rdaregistry.info/Elements/u/P60437> , <http://rdaregistry.info/Elements/u/P60446> ;
	reg:name "contributor"@en ;
	reg:status status:1001 ;
	a rdf:Property ;
	rdfs:isDefinedBy <http://rdaregistry.info/Elements/u/> ;
	rdfs:label "has contributor"@en ;
	owl:inverseOf <http://rdaregistry.info/Elements/u/P60626> ;
	owl:sameAs <http://rdaregistry.info/Elements/u/contributor> ;
	skos:closeMatch "http://id.loc.gov/vocabulary/relators/ctb"@en ;
	skos:definition "Relates a resource to an agent contributing to a resource."@en ;
	skos:scopeNote "Contributors include editors, translators, arrangers of music, performers, etc."@en .

<http://rdaregistry.info/Elements/u/P60399> reg:hasSubproperty <http://rdaregistry.info/Elements/e/P20031> ;
	reg:name "stageDirector"@en ;
	reg:status status:1001 ;
	a rdf:Property ;
	rdfs:isDefinedBy <http://rdaregistry.info/Elements/u/> ;
	rdfs:label "has stage director"@en ;
	rdfs:subPropertyOf <http://rdaregistry.info/Elements/u/P60398> ;
	owl:inverseOf <http://rdaregistry.info/Elements/u/P60627> ;
	owl:sameAs <http://rdaregistry.info/Elements/u/stageDirector> ;
	skos:closeMatch "http://id.loc.gov/vocabulary/relators/sgd"@en ;
	skos:definition "Relates a resource to an agent contributing to a stage resource through the general management and supervision of a performance."@en .

<http://rdaregistry.info/Elements/u/P60400> reg:hasSubproperty <http://rdaregistry.info/Elements/i/P40018> , <http://rdaregistry.info/Elements/u/P60068> ;
	reg:name "currentOwner"@en ;
	reg:status status:1001 ;
	a rdf:Property ;
	rdfs:isDefinedBy <http://rdaregistry.info/Elements/u/> ;
	rdfs:label "has current owner"@en ;
	rdfs:subPropertyOf <http://rdaregistry.info/Elements/u/P60404> ;
	owl:inverseOf <http://rdaregistry.info/Elements/u/P60628> ;
	owl:sameAs <http://rdaregistry.info/Elements/u/currentOwner> ;
	skos:closeMatch "http://id.loc.gov/vocabulary/relators/own"@en ;
	skos:definition "Relates a resource to an agent currently having legal possession of a resource."@en .

<http://rdaregistry.info/Elements/u/P60401> reg:hasSubproperty <http://rdaregistry.info/Elements/i/P40019> , <http://rdaregistry.info/Elements/u/P60091> , <http://rdaregistry.info/Elements/u/P60092> ;
	reg:name "formerOwner"@en ;
	reg:status status:1001 ;
	a rdf:Property ;
	rdfs:isDefinedBy <http://rdaregistry.info/Elements/u/> ;
	rdfs:label "has former owner"@en ;
	rdfs:subPropertyOf <http://rdaregistry.info/Elements/u/P60404> ;
	owl:inverseOf <http://rdaregistry.info/Elements/u/P60630> ;
	owl:sameAs <http://rdaregistry.info/Elements/u/formerOwner> ;
	skos:closeMatch "http://id.loc.gov/vocabulary/relators/fmo"@en ;
	skos:definition "Relates a resource to an agent formerly having legal possession of a resource."@en .

<http://rdaregistry.info/Elements/u/P60402> reg:hasSubproperty <http://rdaregistry.info/Elements/i/P40020> ;
	reg:name "custodian"@en ;
	reg:status status:1001 ;
	a rdf:Property ;
	rdfs:isDefinedBy <http://rdaregistry.info/Elements/u/> ;
	rdfs:label "has custodian"@en ;
	owl:inverseOf <http://rdaregistry.info/Elements/u/P60631> ;
	owl:sameAs <http://rdaregistry.info/Elements/u/custodian> ;
	skos:definition "Relates a resource to an agent having legal custody of a resource."@en .

<http://rdaregistry.info/Elements/u/P60404> reg:hasSubproperty <http://rdaregistry.info/Elements/i/P40021> , <http://rdaregistry.info/Elements/u/P60400> , <http://rdaregistry.info/Elements/u/P60401> ;
	reg:name "owner"@en ;
	reg:status status:1001 ;
	a rdf:Property ;
	rdfs:isDefinedBy <http://rdaregistry.info/Elements/u/> ;
	rdfs:label "has owner"@en ;
	owl:inverseOf <http://rdaregistry.info/Elements/u/P60632> ;
	owl:sameAs <http://rdaregistry.info/Elements/u/owner> ;
	skos:broadMatch "http://id.loc.gov/vocabulary/relators/own"@en ;
	skos:definition "Relates a resource to an agent having legal possession of a resource."@en .

<http://rdaregistry.info/Elements/u/P60406> reg:hasSubproperty <http://rdaregistry.info/Elements/i/P40022> , <http://rdaregistry.info/Elements/w/P10049> ;
	reg:name "honouree"@en ;
	reg:status status:1001 ;
	a rdf:Property ;
	rdfs:isDefinedBy <http://rdaregistry.info/Elements/u/> ;
	rdfs:label "has honouree"@en ;
	rdfs:subPropertyOf <http://rdaregistry.info/Elements/u/P60374> ;
	owl:inverseOf <http://rdaregistry.info/Elements/u/P60634> ;
	owl:sameAs <http://rdaregistry.info/Elements/u/honouree> ;
	skos:closeMatch "http://id.loc.gov/vocabulary/relators/hnr"@en ;
	skos:definition "Relates a resource to an agent honoured by a resource (e.g., the honouree of a festschrift)."@en .

<http://rdaregistry.info/Elements/u/P60407> reg:hasSubproperty <http://rdaregistry.info/Elements/m/P30067> ;
	reg:name "broadcaster"@en ;
	reg:status status:1001 ;
	a rdf:Property ;
	rdfs:isDefinedBy <http://rdaregistry.info/Elements/u/> ;
	rdfs:label "has broadcaster"@en ;
	rdfs:subPropertyOf <http://rdaregistry.info/Elements/u/P60444> ;
	owl:inverseOf <http://rdaregistry.info/Elements/u/P60635> ;
	owl:sameAs <http://rdaregistry.info/Elements/u/broadcaster> ;
	skos:closeMatch "http://id.loc.gov/vocabulary/relators/brd"@en ;
	skos:definition "Relates a resource to an agent involved in broadcasting a resource to an audience via radio, television, webcast, etc."@en .

<http://rdaregistry.info/Elements/u/P60408> reg:hasSubproperty <http://rdaregistry.info/Elements/m/P30068> ;
	reg:name "filmDistributor"@en ;
	reg:status status:1001 ;
	a rdf:Property ;
	rdfs:isDefinedBy <http://rdaregistry.info/Elements/u/> ;
	rdfs:label "has film distributor"@en ;
	rdfs:subPropertyOf <http://rdaregistry.info/Elements/u/P60438> ;
	owl:inverseOf <http://rdaregistry.info/Elements/u/P60636> ;
	owl:sameAs <http://rdaregistry.info/Elements/u/filmDistributor> ;
	skos:closeMatch "http://id.loc.gov/vocabulary/relators/fds"@en ;
	skos:definition "Relates a resource to an agent involved in distributing a moving image resource to theatres or other distribution channels."@en .

<http://rdaregistry.info/Elements/u/P60409> reg:hasSubproperty <http://rdaregistry.info/Elements/m/P30069> ;
	reg:name "bookDesigner"@en ;
	reg:status status:1001 ;
	a rdf:Property ;
	rdfs:isDefinedBy <http://rdaregistry.info/Elements/u/> ;
	rdfs:label "has book designer"@en ;
	rdfs:subPropertyOf <http://rdaregistry.info/Elements/u/P60443> ;
	owl:inverseOf <http://rdaregistry.info/Elements/u/P60637> ;
	owl:sameAs <http://rdaregistry.info/Elements/u/bookDesigner> ;
	skos:closeMatch "http://id.loc.gov/vocabulary/relators/bkd"@en ;
	skos:definition "Relates a resource to an agent involved in manufacturing a resource by being responsible for the entire graphic design of a book, including arrangement of type and illustration, choice of materials, and process used."@en .

<http://rdaregistry.info/Elements/u/P60410> reg:hasSubproperty <http://rdaregistry.info/Elements/m/P30070> ;
	reg:name "engraver"@en ;
	reg:status status:1001 ;
	a rdf:Property ;
	rdfs:isDefinedBy <http://rdaregistry.info/Elements/u/> ;
	rdfs:label "has engraver"@en ;
	rdfs:subPropertyOf <http://rdaregistry.info/Elements/u/P60443> ;
	owl:inverseOf <http://rdaregistry.info/Elements/u/P60638> ;
	owl:sameAs <http://rdaregistry.info/Elements/u/engraver> ;
	skos:closeMatch "http://id.loc.gov/vocabulary/relators/egr"@en ;
	skos:definition "Relates a resource to an agent involved in manufacturing a resource by cutting letters, figures, etc., on a surface such as a wooden or metal plate used for printing."@en .

<http://rdaregistry.info/Elements/u/P60411> reg:hasSubproperty <http://rdaregistry.info/Elements/m/P30071> ;
	reg:name "brailleEmbosser"@en ;
	reg:status status:1001 ;
	a rdf:Property ;
	rdfs:isDefinedBy <http://rdaregistry.info/Elements/u/> ;
	rdfs:label "has braille embosser"@en ;
	rdfs:subPropertyOf <http://rdaregistry.info/Elements/u/P60443> ;
	owl:inverseOf <http://rdaregistry.info/Elements/u/P60639> ;
	owl:sameAs <http://rdaregistry.info/Elements/u/brailleEmbosser> ;
	skos:closeMatch "http://id.loc.gov/vocabulary/relators/brl"@en ;
	skos:definition "Relates a resource to an agent involved in manufacturing a resource by embossing braille cells using a stylus, special embossing printer, or other device."@en .

<http://rdaregistry.info/Elements/u/P60412> reg:hasSubproperty <http://rdaregistry.info/Elements/m/P30072> ;
	reg:name "printmaker"@en ;
	reg:status status:1001 ;
	a rdf:Property ;
	rdfs:isDefinedBy <http://rdaregistry.info/Elements/u/> ;
	rdfs:label "has printmaker"@en ;
	rdfs:subPropertyOf <http://rdaregistry.info/Elements/u/P60443> ;
	owl:inverseOf <http://rdaregistry.info/Elements/u/P60640> ;
	owl:sameAs <http://rdaregistry.info/Elements/u/printmaker> ;
	skos:closeMatch "http://id.loc.gov/vocabulary/relators/prm"@en ;
	skos:definition "Relates a resource to an agent involved in manufacturing a resource by making a relief, intaglio, or planographic printing surface."@en .

<http://rdaregistry.info/Elements/u/P60413> reg:hasSubproperty <http://rdaregistry.info/Elements/m/P30073> ;
	reg:name "caster"@en ;
	reg:status status:1001 ;
	a rdf:Property ;
	rdfs:isDefinedBy <http://rdaregistry.info/Elements/u/> ;
	rdfs:label "has caster"@en ;
	rdfs:subPropertyOf <http://rdaregistry.info/Elements/u/P60443> ;
	owl:inverseOf <http://rdaregistry.info/Elements/u/P60641> ;
	owl:sameAs <http://rdaregistry.info/Elements/u/caster> ;
	skos:closeMatch "http://id.loc.gov/vocabulary/relators/cas"@en ;
	skos:definition "Relates a resource to an agent involved in manufacturing a resource by pouring a liquid or molten substance into a mold and leaving it to solidify to take the shape of the mold."@en .

<http://rdaregistry.info/Elements/u/P60414> reg:hasSubproperty <http://rdaregistry.info/Elements/m/P30074> ;
	reg:name "lithographer"@en ;
	reg:status status:1001 ;
	a rdf:Property ;
	rdfs:isDefinedBy <http://rdaregistry.info/Elements/u/> ;
	rdfs:label "has lithographer"@en ;
	rdfs:subPropertyOf <http://rdaregistry.info/Elements/u/P60443> ;
	owl:inverseOf <http://rdaregistry.info/Elements/u/P60642> ;
	owl:sameAs <http://rdaregistry.info/Elements/u/lithographer> ;
	skos:closeMatch "http://id.loc.gov/vocabulary/relators/ltg"@en ;
	skos:definition "Relates a resource to an agent involved in manufacturing a resource by preparing a stone or plate for lithographic printing, including a graphic artist creating a design directly on the surface from which printing will be done."@en .

<http://rdaregistry.info/Elements/u/P60415> reg:hasSubproperty <http://rdaregistry.info/Elements/m/P30075> ;
	reg:name "platemaker"@en ;
	reg:status status:1001 ;
	a rdf:Property ;
	rdfs:isDefinedBy <http://rdaregistry.info/Elements/u/> ;
	rdfs:label "has platemaker"@en ;
	rdfs:subPropertyOf <http://rdaregistry.info/Elements/u/P60443> ;
	owl:inverseOf <http://rdaregistry.info/Elements/u/P60643> ;
	owl:sameAs <http://rdaregistry.info/Elements/u/platemaker> ;
	skos:closeMatch "http://id.loc.gov/vocabulary/relators/plt"@en ;
	skos:definition "Relates a resource to an agent involved in manufacturing a resource by preparing plates used in the production of printed images and/or text."@en .

<http://rdaregistry.info/Elements/u/P60416> reg:hasSubproperty <http://rdaregistry.info/Elements/m/P30076> ;
	reg:name "etcher"@en ;
	reg:status status:1001 ;
	a rdf:Property ;
	rdfs:isDefinedBy <http://rdaregistry.info/Elements/u/> ;
	rdfs:label "has etcher"@en ;
	rdfs:subPropertyOf <http://rdaregistry.info/Elements/u/P60443> ;
	owl:inverseOf <http://rdaregistry.info/Elements/u/P60644> ;
	owl:sameAs <http://rdaregistry.info/Elements/u/etcher> ;
	skos:closeMatch "http://id.loc.gov/vocabulary/relators/etr"@en ;
	skos:definition "Relates a resource to an agent involved in manufacturing a resource by subjecting metal, glass, or some other surface used for printing, to acid or another corrosive substance."@en .

<http://rdaregistry.info/Elements/u/P60417> reg:hasSubproperty <http://rdaregistry.info/Elements/m/P30077> ;
	reg:name "collotyper"@en ;
	reg:status status:1001 ;
	a rdf:Property ;
	rdfs:isDefinedBy <http://rdaregistry.info/Elements/u/> ;
	rdfs:label "has collotyper"@en ;
	rdfs:subPropertyOf <http://rdaregistry.info/Elements/u/P60443> ;
	owl:inverseOf <http://rdaregistry.info/Elements/u/P60645> ;
	owl:sameAs <http://rdaregistry.info/Elements/u/collotyper> ;
	skos:closeMatch "http://id.loc.gov/vocabulary/relators/clt"@en ;
	skos:definition "Relates a resource to an agent involved in manufacturing a resource of photographic prints from film or other colloid that has ink-receptive and ink-repellent surfaces."@en .

<http://rdaregistry.info/Elements/u/P60418> reg:hasSubproperty <http://rdaregistry.info/Elements/m/P30078> ;
	reg:name "printer"@en ;
	reg:status status:1001 ;
	a rdf:Property ;
	rdfs:isDefinedBy <http://rdaregistry.info/Elements/u/> ;
	rdfs:label "has printer"@en ;
	rdfs:subPropertyOf <http://rdaregistry.info/Elements/u/P60443> ;
	owl:inverseOf <http://rdaregistry.info/Elements/u/P60646> ;
	owl:sameAs <http://rdaregistry.info/Elements/u/printer> ;
	skos:closeMatch "http://id.loc.gov/vocabulary/relators/prt"@en ;
	skos:definition "Relates a resource to an agent involved in manufacturing a resource of printed text, notated music, etc., from type or plates, such as a book, newspaper, magazine, broadside, score, etc."@en .

<http://rdaregistry.info/Elements/u/P60419> reg:hasSubproperty <http://rdaregistry.info/Elements/e/P20054> ;
	reg:name "presenter"@en ;
	reg:status status:1001 ;
	a rdf:Property ;
	rdfs:isDefinedBy <http://rdaregistry.info/Elements/u/> ;
	rdfs:label "has presenter"@en ;
	rdfs:subPropertyOf <http://rdaregistry.info/Elements/u/P60398> ;
	owl:inverseOf <http://rdaregistry.info/Elements/u/P60647> ;
	owl:sameAs <http://rdaregistry.info/Elements/u/presenter> ;
	skos:closeMatch "http://id.loc.gov/vocabulary/relators/pre"@en ;
	skos:definition "Relates a resource to an agent mentioned in an “x presents” credit for moving image materials and who is probably associated with production, finance, or distribution in some way."@en .

<http://rdaregistry.info/Elements/u/P60420> reg:hasSubproperty <http://rdaregistry.info/Elements/w/P10041> ;
	reg:name "degreeSupervisor"@en ;
	reg:status status:1001 ;
	a rdf:Property ;
	rdfs:isDefinedBy <http://rdaregistry.info/Elements/u/> ;
	rdfs:label "has degree supervisor"@en ;
	rdfs:subPropertyOf <http://rdaregistry.info/Elements/u/P60447> ;
	owl:inverseOf <http://rdaregistry.info/Elements/u/P60649> ;
	owl:sameAs <http://rdaregistry.info/Elements/u/degreeSupervisor> ;
	skos:closeMatch "http://id.loc.gov/vocabulary/relators/dgs"@en ;
	skos:definition "Relates a resource to an agent overseeing a higher-level academic degree."@en .

<http://rdaregistry.info/Elements/u/P60421> reg:hasSubproperty <http://rdaregistry.info/Elements/i/P40012> ;
	reg:name "illuminator"@en ;
	reg:status status:1001 ;
	a rdf:Property ;
	rdfs:isDefinedBy <http://rdaregistry.info/Elements/u/> ;
	rdfs:label "has illuminator"@en ;
	rdfs:subPropertyOf <http://rdaregistry.info/Elements/u/P60374> ;
	owl:inverseOf <http://rdaregistry.info/Elements/u/P60650> ;
	owl:sameAs <http://rdaregistry.info/Elements/u/illuminator> ;
	skos:closeMatch "http://id.loc.gov/vocabulary/relators/ilu"@en ;
	skos:definition "Relates a resource to an agent providing decoration to a specific resource using precious metals or color, often with elaborate designs and motifs."@en .

<http://rdaregistry.info/Elements/u/P60422> reg:hasSubproperty <http://rdaregistry.info/Elements/e/P20055> ;
	reg:name "editorOfMovingImageWork"@en ;
	reg:status status:1001 ;
	a rdf:Property ;
	rdfs:isDefinedBy <http://rdaregistry.info/Elements/u/> ;
	rdfs:label "has editor of moving image work"@en ;
	rdfs:subPropertyOf <http://rdaregistry.info/Elements/u/P60398> ;
	owl:inverseOf <http://rdaregistry.info/Elements/u/P60651> ;
	owl:sameAs <http://rdaregistry.info/Elements/u/editorOfMovingImageWork> ;
	skos:closeMatch "http://id.loc.gov/vocabulary/relators/edm"@en ;
	skos:definition "Relates a resource to an agent responsible for assembling, arranging, and trimming film, video, or other moving image formats, including both visual and audio aspects."@en .

<http://rdaregistry.info/Elements/u/P60423> reg:hasSubproperty <http://rdaregistry.info/Elements/w/P10050> ;
	reg:name "programmer"@en ;
	reg:status status:1001 ;
	a rdf:Property ;
	rdfs:isDefinedBy <http://rdaregistry.info/Elements/u/> ;
	rdfs:label "has programmer"@en ;
	rdfs:subPropertyOf <http://rdaregistry.info/Elements/u/P60447> ;
	owl:inverseOf <http://rdaregistry.info/Elements/u/P60652> ;
	owl:sameAs <http://rdaregistry.info/Elements/u/programmer> ;
	skos:closeMatch "http://id.loc.gov/vocabulary/relators/prg"@en ;
	skos:definition "Relates a resource to an agent responsible for creating a computer program."@en .

<http://rdaregistry.info/Elements/u/P60424> reg:hasSubproperty <http://rdaregistry.info/Elements/w/P10051> ;
	reg:name "designer"@en ;
	reg:status status:1001 ;
	a rdf:Property ;
	rdfs:isDefinedBy <http://rdaregistry.info/Elements/u/> ;
	rdfs:label "has designer"@en ;
	rdfs:subPropertyOf <http://rdaregistry.info/Elements/u/P60447> ;
	owl:inverseOf <http://rdaregistry.info/Elements/u/P60653> ;
	owl:sameAs <http://rdaregistry.info/Elements/u/designer> ;
	skos:closeMatch "http://id.loc.gov/vocabulary/relators/dsr"@en ;
	skos:definition "Relates a resource to an agent responsible for creating a design for an object."@en .

<http://rdaregistry.info/Elements/u/P60425> reg:hasSubproperty <http://rdaregistry.info/Elements/e/P20042> , <http://rdaregistry.info/Elements/w/P10052> ;
	reg:name "cartographer"@en ;
	reg:status status:1001 ;
	a rdf:Property ;
	rdfs:isDefinedBy <http://rdaregistry.info/Elements/u/> ;
	rdfs:label "has cartographer"@en ;
	rdfs:subPropertyOf <http://rdaregistry.info/Elements/u/P60447> ;
	owl:inverseOf <http://rdaregistry.info/Elements/u/P60654> ;
	owl:sameAs <http://rdaregistry.info/Elements/u/cartographer> ;
	skos:closeMatch "http://id.loc.gov/vocabulary/relators/ctg"@en ;
	skos:definition "Relates a resource to an agent responsible for creating a map, atlas, globe, or other cartographic resource."@en .

<http://rdaregistry.info/Elements/u/P60426> reg:hasSubproperty <http://rdaregistry.info/Elements/e/P20026> , <http://rdaregistry.info/Elements/w/P10053> ;
	reg:name "composer"@en ;
	reg:status status:1001 ;
	a rdf:Property ;
	rdfs:isDefinedBy <http://rdaregistry.info/Elements/u/> ;
	rdfs:label "has composer"@en ;
	rdfs:subPropertyOf <http://rdaregistry.info/Elements/u/P60447> ;
	owl:inverseOf <http://rdaregistry.info/Elements/u/P60655> ;
	owl:sameAs <http://rdaregistry.info/Elements/u/composer> ;
	skos:closeMatch "http://id.loc.gov/vocabulary/relators/cmp"@en ;
	skos:definition "Relates a resource to an agent responsible for creating a musical resource."@en .

<http://rdaregistry.info/Elements/u/P60427> reg:hasSubproperty <http://rdaregistry.info/Elements/w/P10054> ;
	reg:name "inventor"@en ;
	reg:status status:1001 ;
	a rdf:Property ;
	rdfs:isDefinedBy <http://rdaregistry.info/Elements/u/> ;
	rdfs:label "has inventor"@en ;
	rdfs:subPropertyOf <http://rdaregistry.info/Elements/u/P60447> ;
	owl:inverseOf <http://rdaregistry.info/Elements/u/P60656> ;
	owl:sameAs <http://rdaregistry.info/Elements/u/inventor> ;
	skos:closeMatch "http://id.loc.gov/vocabulary/relators/inv"@en ;
	skos:definition "Relates a resource to an agent responsible for creating a new device or process."@en .

<http://rdaregistry.info/Elements/u/P60428> reg:hasSubproperty <http://rdaregistry.info/Elements/w/P10055> ;
	reg:name "compiler"@en ;
	reg:status status:1001 ;
	a rdf:Property ;
	rdfs:isDefinedBy <http://rdaregistry.info/Elements/u/> ;
	rdfs:label "has compiler"@en ;
	rdfs:subPropertyOf <http://rdaregistry.info/Elements/u/P60447> ;
	owl:inverseOf <http://rdaregistry.info/Elements/u/P60657> ;
	owl:sameAs <http://rdaregistry.info/Elements/u/compiler> ;
	skos:closeMatch "http://id.loc.gov/vocabulary/relators/com"@en ;
	skos:definition "Relates a resource to an agent responsible for creating a new resource (e.g., a bibliography, a directory) by selecting, arranging, aggregating, and editing data, information, etc."@en .

<http://rdaregistry.info/Elements/u/P60429> reg:hasSubproperty <http://rdaregistry.info/Elements/w/P10056> ;
	reg:name "photographer"@en ;
	reg:status status:1001 ;
	a rdf:Property ;
	rdfs:isDefinedBy <http://rdaregistry.info/Elements/u/> ;
	rdfs:label "has photographer"@en ;
	rdfs:subPropertyOf <http://rdaregistry.info/Elements/u/P60447> ;
	owl:inverseOf <http://rdaregistry.info/Elements/u/P60658> ;
	owl:sameAs <http://rdaregistry.info/Elements/u/photographer> ;
	skos:closeMatch "http://id.loc.gov/vocabulary/relators/pht"@en ;
	skos:definition "Relates a resource to an agent responsible for creating a photographic resource."@en .

<http://rdaregistry.info/Elements/u/P60430> reg:hasSubproperty <http://rdaregistry.info/Elements/e/P20032> , <http://rdaregistry.info/Elements/w/P10057> ;
	reg:name "interviewer"@en ;
	reg:status status:1001 ;
	a rdf:Property ;
	rdfs:isDefinedBy <http://rdaregistry.info/Elements/u/> ;
	rdfs:label "has interviewer"@en ;
	rdfs:subPropertyOf <http://rdaregistry.info/Elements/u/P60447> ;
	owl:inverseOf <http://rdaregistry.info/Elements/u/P60659> ;
	owl:sameAs <http://rdaregistry.info/Elements/u/interviewer> ;
	skos:closeMatch "http://id.loc.gov/vocabulary/relators/ivr"@en ;
	skos:definition "Relates a resource to an agent responsible for creating a resource by acting as an interviewer, reporter, pollster, or some other information gathering agent."@en .

<http://rdaregistry.info/Elements/u/P60431> reg:hasSubproperty <http://rdaregistry.info/Elements/u/P60475> , <http://rdaregistry.info/Elements/w/P10058> ;
	reg:name "artist"@en ;
	reg:status status:1001 ;
	a rdf:Property ;
	rdfs:isDefinedBy <http://rdaregistry.info/Elements/u/> ;
	rdfs:label "has artist"@en ;
	rdfs:subPropertyOf <http://rdaregistry.info/Elements/u/P60447> ;
	owl:inverseOf <http://rdaregistry.info/Elements/u/P60660> ;
	owl:sameAs <http://rdaregistry.info/Elements/u/artist> ;
	skos:closeMatch "http://id.loc.gov/vocabulary/relators/art"@en ;
	skos:definition "Relates a resource to an agent responsible for creating a resource by conceiving, and often implementing, an original graphic design, drawing, painting, etc."@en .

<http://rdaregistry.info/Elements/u/P60432> reg:hasSubproperty <http://rdaregistry.info/Elements/e/P20047> , <http://rdaregistry.info/Elements/w/P10059> ;
	reg:name "interviewee"@en ;
	reg:status status:1001 ;
	a rdf:Property ;
	rdfs:isDefinedBy <http://rdaregistry.info/Elements/u/> ;
	rdfs:label "has interviewee"@en ;
	rdfs:subPropertyOf <http://rdaregistry.info/Elements/u/P60447> ;
	owl:inverseOf <http://rdaregistry.info/Elements/u/P60661> ;
	owl:sameAs <http://rdaregistry.info/Elements/u/interviewee> ;
	skos:closeMatch "http://id.loc.gov/vocabulary/relators/ive"@en ;
	skos:definition "Relates a resource to an agent responsible for creating a resource by responding to an interviewer, usually a reporter, pollster, or some other information gathering agent."@en .

<http://rdaregistry.info/Elements/u/P60433> reg:hasSubproperty <http://rdaregistry.info/Elements/e/P20043> , <http://rdaregistry.info/Elements/w/P10060> ;
	reg:name "choreographer"@en ;
	reg:status status:1001 ;
	a rdf:Property ;
	rdfs:isDefinedBy <http://rdaregistry.info/Elements/u/> ;
	rdfs:label "has choreographer"@en ;
	rdfs:subPropertyOf <http://rdaregistry.info/Elements/u/P60447> ;
	owl:inverseOf <http://rdaregistry.info/Elements/u/P60662> ;
	owl:sameAs <http://rdaregistry.info/Elements/u/choreographer> ;
	skos:closeMatch "http://id.loc.gov/vocabulary/relators/chr"@en ;
	skos:definition "Relates a resource to an agent responsible for creating a resource of movement."@en .

<http://rdaregistry.info/Elements/u/P60434> reg:hasSubproperty <http://rdaregistry.info/Elements/u/P60476> , <http://rdaregistry.info/Elements/u/P60477> , <http://rdaregistry.info/Elements/u/P60478> , <http://rdaregistry.info/Elements/w/P10061> ;
	reg:name "author"@en ;
	reg:status status:1001 ;
	a rdf:Property ;
	rdfs:isDefinedBy <http://rdaregistry.info/Elements/u/> ;
	rdfs:label "has author"@en ;
	rdfs:subPropertyOf <http://rdaregistry.info/Elements/u/P60447> ;
	owl:inverseOf <http://rdaregistry.info/Elements/u/P60663> ;
	owl:sameAs <http://rdaregistry.info/Elements/u/author> ;
	skos:closeMatch "http://id.loc.gov/vocabulary/relators/aut"@en ;
	skos:definition "Relates a resource to an agent responsible for creating a resource that is primarily textual in content, regardless of media type (e.g., printed text, spoken word, electronic text, tactile text) or genre (e.g., poems, novels, screenplays, blogs)."@en .

<http://rdaregistry.info/Elements/u/P60435> reg:hasSubproperty <http://rdaregistry.info/Elements/u/P60473> , <http://rdaregistry.info/Elements/w/P10062> ;
	reg:name "architect"@en ;
	reg:status status:1001 ;
	a rdf:Property ;
	rdfs:isDefinedBy <http://rdaregistry.info/Elements/u/> ;
	rdfs:label "has architect"@en ;
	rdfs:subPropertyOf <http://rdaregistry.info/Elements/u/P60447> ;
	owl:inverseOf <http://rdaregistry.info/Elements/u/P60664> ;
	owl:sameAs <http://rdaregistry.info/Elements/u/architect> ;
	skos:closeMatch "http://id.loc.gov/vocabulary/relators/arc"@en ;
	skos:definition "Relates a resource to an agent responsible for creating an architectural design, including a pictorial representation intended to show how a building, etc., will look when completed."@en .

<http://rdaregistry.info/Elements/u/P60436> reg:hasSubproperty <http://rdaregistry.info/Elements/w/P10063> ;
	reg:name "filmmaker"@en ;
	reg:status status:1001 ;
	a rdf:Property ;
	rdfs:isDefinedBy <http://rdaregistry.info/Elements/u/> ;
	rdfs:label "has filmmaker"@en ;
	rdfs:subPropertyOf <http://rdaregistry.info/Elements/u/P60447> ;
	owl:inverseOf <http://rdaregistry.info/Elements/u/P60665> ;
	owl:sameAs <http://rdaregistry.info/Elements/u/filmmaker> ;
	skos:closeMatch "http://id.loc.gov/vocabulary/relators/fmk"@en ;
	skos:definition "Relates a resource to an agent responsible for creating an independent or personal film."@en .

<http://rdaregistry.info/Elements/u/P60437> reg:hasSubproperty <http://rdaregistry.info/Elements/e/P20056> ;
	reg:name "productionDesigner"@en ;
	reg:status status:1001 ;
	a rdf:Property ;
	rdfs:isDefinedBy <http://rdaregistry.info/Elements/u/> ;
	rdfs:label "has production designer"@en ;
	rdfs:subPropertyOf <http://rdaregistry.info/Elements/u/P60398> ;
	owl:inverseOf <http://rdaregistry.info/Elements/u/P60666> ;
	owl:sameAs <http://rdaregistry.info/Elements/u/productionDesigner> ;
	skos:closeMatch "http://id.loc.gov/vocabulary/relators/prs"@en ;
	skos:definition "Relates a resource to an agent responsible for designing the overall visual appearance of a moving image production."@en .

<http://rdaregistry.info/Elements/u/P60438> reg:hasSubproperty <http://rdaregistry.info/Elements/m/P30080> , <http://rdaregistry.info/Elements/u/P60408> ;
	reg:name "distributor"@en ;
	reg:status status:1001 ;
	a rdf:Property ;
	rdfs:isDefinedBy <http://rdaregistry.info/Elements/u/> ;
	rdfs:label "has distributor"@en ;
	owl:inverseOf <http://rdaregistry.info/Elements/u/P60667> ;
	owl:sameAs <http://rdaregistry.info/Elements/u/distributor> ;
	skos:closeMatch "http://id.loc.gov/vocabulary/relators/dst"@en ;
	skos:definition "Relates a resource to an agent responsible for distributing a resource."@en .

<http://rdaregistry.info/Elements/u/P60440> reg:hasSubproperty <http://rdaregistry.info/Elements/m/P30081> ;
	reg:name "producerOfAnUnpublishedResource"@en ;
	reg:status status:1001 ;
	a rdf:Property ;
	rdfs:isDefinedBy <http://rdaregistry.info/Elements/u/> ;
	rdfs:label "has producer of an unpublished resource"@en ;
	owl:sameAs <http://rdaregistry.info/Elements/u/producerOfAnUnpublishedResource> ;
	skos:definition "Relates a resource to an agent responsible for inscribing, fabricating, constructing, etc., a resource in an unpublished form."@en .

<http://rdaregistry.info/Elements/u/P60441> reg:hasSubproperty <http://rdaregistry.info/Elements/u/P60169> , <http://rdaregistry.info/Elements/u/P60170> , <http://rdaregistry.info/Elements/u/P60171> , <http://rdaregistry.info/Elements/w/P10064> ;
	reg:name "producer"@en ;
	reg:status status:1001 ;
	a rdf:Property ;
	rdfs:isDefinedBy <http://rdaregistry.info/Elements/u/> ;
	rdfs:label "has producer"@en ;
	rdfs:subPropertyOf <http://rdaregistry.info/Elements/u/P60374> ;
	owl:inverseOf <http://rdaregistry.info/Elements/u/P60668> ;
	owl:sameAs <http://rdaregistry.info/Elements/u/producer> ;
	skos:closeMatch "http://id.loc.gov/vocabulary/relators/pro"@en ;
	skos:definition "Relates a resource to an agent responsible for most of the business aspects of a production for screen, sound recording, television, webcast, etc. the producer is generally responsible for fund raising, managing the production, hiring key personnel, arranging for distributors, etc."@en .

<http://rdaregistry.info/Elements/u/P60442> reg:hasSubproperty <http://rdaregistry.info/Elements/e/P20057> ;
	reg:name "performerNarratorAndOrPresenter"@en ;
	reg:status status:1001 ;
	a rdf:Property ;
	rdfs:isDefinedBy <http://rdaregistry.info/Elements/u/> ;
	rdfs:label "has performer, narrator, and/or presenter"@en ;
	owl:sameAs <http://rdaregistry.info/Elements/u/performerNarratorAndOrPresenter> ;
	skos:definition "Relates a resource to an agent responsible for performing, narrating, and/or presenting a resource."@en .

<http://rdaregistry.info/Elements/u/P60443> reg:hasSubproperty <http://rdaregistry.info/Elements/m/P30082> , <http://rdaregistry.info/Elements/u/P60409> , <http://rdaregistry.info/Elements/u/P60410> , <http://rdaregistry.info/Elements/u/P60411> , <http://rdaregistry.info/Elements/u/P60412> , <http://rdaregistry.info/Elements/u/P60413> , <http://rdaregistry.info/Elements/u/P60414> , <http://rdaregistry.info/Elements/u/P60415> , <http://rdaregistry.info/Elements/u/P60416> , <http://rdaregistry.info/Elements/u/P60417> , <http://rdaregistry.info/Elements/u/P60418> ;
	reg:name "manufacturer"@en ;
	reg:status status:1001 ;
	a rdf:Property ;
	rdfs:isDefinedBy <http://rdaregistry.info/Elements/u/> ;
	rdfs:label "has manufacturer"@en ;
	owl:inverseOf <http://rdaregistry.info/Elements/u/P60669> ;
	owl:sameAs <http://rdaregistry.info/Elements/u/manufacturer> ;
	skos:closeMatch "http://id.loc.gov/vocabulary/relators/mfr"@en ;
	skos:definition "Relates a resource to an agent responsible for printing, duplicating, casting, etc., a resource in a published form."@en .

<http://rdaregistry.info/Elements/u/P60444> reg:hasSubproperty <http://rdaregistry.info/Elements/m/P30083> , <http://rdaregistry.info/Elements/u/P60407> ;
	reg:name "publisher"@en ;
	reg:status status:1001 ;
	a rdf:Property ;
	rdfs:isDefinedBy <http://rdaregistry.info/Elements/u/> ;
	rdfs:label "has publisher"@en ;
	owl:inverseOf <http://rdaregistry.info/Elements/u/P60670> ;
	owl:sameAs <http://rdaregistry.info/Elements/u/publisher> ;
	skos:closeMatch "http://id.loc.gov/vocabulary/relators/pbl"@en ;
	skos:definition "Relates a resource to an agent responsible for publishing, releasing, or issuing a resource."@en .

<http://rdaregistry.info/Elements/u/P60446> reg:hasSubproperty <http://rdaregistry.info/Elements/e/P20058> ;
	reg:name "minuteTaker"@en ;
	reg:status status:1001 ;
	a rdf:Property ;
	rdfs:isDefinedBy <http://rdaregistry.info/Elements/u/> ;
	rdfs:label "has minute taker"@en ;
	rdfs:subPropertyOf <http://rdaregistry.info/Elements/u/P60398> ;
	owl:inverseOf <http://rdaregistry.info/Elements/u/P60671> ;
	owl:sameAs <http://rdaregistry.info/Elements/u/minuteTaker> ;
	skos:closeMatch "http://id.loc.gov/vocabulary/relators/mtk"@en ;
	skos:definition "Relates a resource to an agent responsible for recording the minutes of a meeting."@en .

<http://rdaregistry.info/Elements/u/P60447> reg:hasSubproperty <http://rdaregistry.info/Elements/u/P60045> , <http://rdaregistry.info/Elements/u/P60096> , <http://rdaregistry.info/Elements/u/P60420> , <http://rdaregistry.info/Elements/u/P60423> , <http://rdaregistry.info/Elements/u/P60424> , <http://rdaregistry.info/Elements/u/P60425> , <http://rdaregistry.info/Elements/u/P60426> , <http://rdaregistry.info/Elements/u/P60427> , <http://rdaregistry.info/Elements/u/P60428> , <http://rdaregistry.info/Elements/u/P60429> , <http://rdaregistry.info/Elements/u/P60430> , <http://rdaregistry.info/Elements/u/P60431> , <http://rdaregistry.info/Elements/u/P60432> , <http://rdaregistry.info/Elements/u/P60433> , <http://rdaregistry.info/Elements/u/P60434> , <http://rdaregistry.info/Elements/u/P60435> , <http://rdaregistry.info/Elements/u/P60436> , <http://rdaregistry.info/Elements/u/P60463> , <http://rdaregistry.info/Elements/u/P60465> , <http://rdaregistry.info/Elements/w/P10065> ;
	reg:name "creator"@en ;
	reg:status status:1001 ;
	a rdf:Property ;
	rdfs:isDefinedBy <http://rdaregistry.info/Elements/u/> ;
	rdfs:label "has creator"@en ;
	owl:inverseOf <http://rdaregistry.info/Elements/u/P60672> ;
	owl:sameAs <http://rdaregistry.info/Elements/u/creator> ;
	skos:closeMatch "http://id.loc.gov/vocabulary/relators/cre"@en ;
	skos:definition "Relates a resource to an agent responsible for the creation of a resource"@en .

<http://rdaregistry.info/Elements/u/P60449> reg:hasSubproperty <http://rdaregistry.info/Elements/u/P60084> , <http://rdaregistry.info/Elements/u/P60085> , <http://rdaregistry.info/Elements/u/P60086> , <http://rdaregistry.info/Elements/w/P10066> ;
	reg:name "director"@en ;
	reg:status status:1001 ;
	a rdf:Property ;
	rdfs:isDefinedBy <http://rdaregistry.info/Elements/u/> ;
	rdfs:label "has director"@en ;
	rdfs:subPropertyOf <http://rdaregistry.info/Elements/u/P60374> ;
	owl:inverseOf <http://rdaregistry.info/Elements/u/P60673> ;
	owl:sameAs <http://rdaregistry.info/Elements/u/director> ;
	skos:closeMatch "http://id.loc.gov/vocabulary/relators/drt"@en ;
	skos:definition "Relates a resource to an agent responsible for the general management and supervision of a filmed performance, a radio or television program, etc."@en .

<http://rdaregistry.info/Elements/u/P60450> reg:hasSubproperty <http://rdaregistry.info/Elements/i/P40024> ;
	reg:name "restorationist"@en ;
	reg:status status:1001 ;
	a rdf:Property ;
	rdfs:isDefinedBy <http://rdaregistry.info/Elements/u/> ;
	rdfs:label "has restorationist"@en ;
	rdfs:subPropertyOf <http://rdaregistry.info/Elements/u/P60374> ;
	owl:inverseOf <http://rdaregistry.info/Elements/u/P60674> ;
	owl:sameAs <http://rdaregistry.info/Elements/u/restorationist> ;
	skos:closeMatch "http://id.loc.gov/vocabulary/relators/rsr"@en ;
	skos:definition "Relates a resource to an agent responsible for the set of technical, editorial, and intellectual procedures aimed at compensating for the degradation of a resource by bringing it back to a state as close as possible to its original condition."@en .

<http://rdaregistry.info/Elements/u/P60451> reg:hasSubproperty <http://rdaregistry.info/Elements/w/P10067> ;
	reg:name "sponsoringBody"@en ;
	reg:status status:1001 ;
	a rdf:Property ;
	rdfs:isDefinedBy <http://rdaregistry.info/Elements/u/> ;
	rdfs:label "has sponsoring body"@en ;
	rdfs:subPropertyOf <http://rdaregistry.info/Elements/u/P60374> ;
	owl:inverseOf <http://rdaregistry.info/Elements/u/P60675> ;
	owl:sameAs <http://rdaregistry.info/Elements/u/sponsoringBody> ;
	skos:closeMatch "http://id.loc.gov/vocabulary/relators/spn"@en ;
	skos:definition "Relates a resource to an agent sponsoring some aspect of a resource, e.g., funding research, sponsoring an event."@en .

<http://rdaregistry.info/Elements/u/P60452> reg:name "directorOfPhotography"@en ;
	reg:status status:1001 ;
	a rdf:Property ;
	rdfs:isDefinedBy <http://rdaregistry.info/Elements/u/> ;
	rdfs:label "has director of photography"@en ;
	rdfs:subPropertyOf <http://rdaregistry.info/Elements/u/P60374> ;
	owl:inverseOf <http://rdaregistry.info/Elements/u/P60678> ;
	skos:definition "Relates a resource to an agent that captures images, either electronically or on film or video stock, and often selects and arranges the lighting. the director of photography for a movie is also called the chief cinematographer."@en ;
	skos:narrowMatch "http://id.loc.gov/vocabulary/relators/cng"@en , "http://id.loc.gov/vocabulary/relators/vdg"@en .

<http://rdaregistry.info/Elements/u/P60454> reg:hasSubproperty <http://rdaregistry.info/Elements/a/P50218> , <http://rdaregistry.info/Elements/a/P50219> , <http://rdaregistry.info/Elements/a/P50220> ;
	reg:name "relatedAgent"@en ;
	reg:status status:1001 ;
	a rdf:Property ;
	rdfs:isDefinedBy <http://rdaregistry.info/Elements/u/> ;
	rdfs:label "has related agent"@en ;
	owl:sameAs <http://rdaregistry.info/Elements/u/relatedAgent> ;
	skos:definition "Relates a resource to an agent that is associated with the agent being identified."@en ;
	skos:scopeNote "Related corporate bodies include corporate bodies that precede or succeed the corporate body being identified as the result of a change of name."@en .

<http://rdaregistry.info/Elements/u/P60455> reg:hasSubproperty <http://rdaregistry.info/Elements/i/P40025> , <http://rdaregistry.info/Elements/w/P10069> ;
	reg:name "dedicatee"@en ;
	reg:status status:1001 ;
	a rdf:Property ;
	rdfs:isDefinedBy <http://rdaregistry.info/Elements/u/> ;
	rdfs:label "has dedicatee"@en ;
	rdfs:subPropertyOf <http://rdaregistry.info/Elements/u/P60374> ;
	owl:inverseOf <http://rdaregistry.info/Elements/u/P60689> ;
	owl:sameAs <http://rdaregistry.info/Elements/u/dedicatee> ;
	skos:closeMatch "http://id.loc.gov/vocabulary/relators/dte"@en ;
	skos:definition "Relates a resource to an agent to whom a resource is dedicated."@en .

<http://rdaregistry.info/Elements/u/P60456> reg:hasSubproperty <http://rdaregistry.info/Elements/w/P10070> ;
	reg:name "addressee"@en ;
	reg:status status:1001 ;
	a rdf:Property ;
	rdfs:isDefinedBy <http://rdaregistry.info/Elements/u/> ;
	rdfs:label "has addressee"@en ;
	rdfs:subPropertyOf <http://rdaregistry.info/Elements/u/P60374> ;
	owl:inverseOf <http://rdaregistry.info/Elements/u/P60690> ;
	owl:sameAs <http://rdaregistry.info/Elements/u/addressee> ;
	skos:closeMatch "http://id.loc.gov/vocabulary/relators/rcp"@en ;
	skos:definition "Relates a resource to an agent to whom a resource or part of a resource is addressed."@en .

<http://rdaregistry.info/Elements/u/P60457> reg:hasSubproperty <http://rdaregistry.info/Elements/w/P10009> , <http://rdaregistry.info/Elements/w/P10038> , <http://rdaregistry.info/Elements/w/P10042> ;
	reg:name "appellant"@en ;
	reg:status status:1001 ;
	a rdf:Property ;
	rdfs:isDefinedBy <http://rdaregistry.info/Elements/u/> ;
	rdfs:label "has appellant"@en ;
	rdfs:subPropertyOf <http://rdaregistry.info/Elements/u/P60374> ;
	owl:inverseOf <http://rdaregistry.info/Elements/u/P60691> ;
	owl:sameAs <http://rdaregistry.info/Elements/u/appellant> ;
	skos:closeMatch "http://id.loc.gov/vocabulary/relators/apl"@en ;
	skos:definition "Relates a resource to an agent who appeals a lower court’s decision."@en .

<http://rdaregistry.info/Elements/u/P60458> reg:hasSubproperty <http://rdaregistry.info/Elements/i/P40013> ;
	reg:name "binder"@en ;
	reg:status status:1001 ;
	a rdf:Property ;
	rdfs:isDefinedBy <http://rdaregistry.info/Elements/u/> ;
	rdfs:label "has binder"@en ;
	rdfs:subPropertyOf <http://rdaregistry.info/Elements/u/P60374> ;
	owl:inverseOf <http://rdaregistry.info/Elements/u/P60692> ;
	owl:sameAs <http://rdaregistry.info/Elements/u/binder> ;
	skos:closeMatch "http://id.loc.gov/vocabulary/relators/bnd"@en ;
	skos:definition "Relates a resource to an agent who binds a resource."@en .

<http://rdaregistry.info/Elements/u/P60459> reg:hasSubproperty <http://rdaregistry.info/Elements/w/P10010> , <http://rdaregistry.info/Elements/w/P10039> , <http://rdaregistry.info/Elements/w/P10043> ;
	reg:name "plaintiff"@en ;
	reg:status status:1001 ;
	a rdf:Property ;
	rdfs:isDefinedBy <http://rdaregistry.info/Elements/u/> ;
	rdfs:label "has plaintiff"@en ;
	rdfs:subPropertyOf <http://rdaregistry.info/Elements/u/P60374> ;
	owl:inverseOf <http://rdaregistry.info/Elements/u/P60693> ;
	owl:sameAs <http://rdaregistry.info/Elements/u/plaintiff> ;
	skos:closeMatch "http://id.loc.gov/vocabulary/relators/ptf"@en ;
	skos:definition "Relates a resource to an agent who brings a suit in a civil proceeding."@en .

<http://rdaregistry.info/Elements/u/P60460> reg:hasSubproperty <http://rdaregistry.info/Elements/i/P40014> ;
	reg:name "inscriber"@en ;
	reg:status status:1001 ;
	a rdf:Property ;
	rdfs:isDefinedBy <http://rdaregistry.info/Elements/u/> ;
	rdfs:label "has inscriber"@en ;
	rdfs:subPropertyOf <http://rdaregistry.info/Elements/u/P60374> ;
	owl:inverseOf <http://rdaregistry.info/Elements/u/P60695> ;
	owl:sameAs <http://rdaregistry.info/Elements/u/inscriber> ;
	skos:closeMatch "http://id.loc.gov/vocabulary/relators/ins"@en ;
	skos:definition "Relates a resource to an agent who has written a statement of dedication or gift on a resource."@en .

<http://rdaregistry.info/Elements/u/P60461> reg:hasSubproperty <http://rdaregistry.info/Elements/w/P10044> ;
	reg:name "judge"@en ;
	reg:status status:1001 ;
	a rdf:Property ;
	rdfs:isDefinedBy <http://rdaregistry.info/Elements/u/> ;
	rdfs:label "has judge"@en ;
	rdfs:subPropertyOf <http://rdaregistry.info/Elements/u/P60374> ;
	owl:inverseOf <http://rdaregistry.info/Elements/u/P60696> ;
	owl:sameAs <http://rdaregistry.info/Elements/u/judge> ;
	skos:closeMatch "http://id.loc.gov/vocabulary/relators/jud"@en ;
	skos:definition "Relates a resource to an agent who hears and decides on legal matters in court."@en .

<http://rdaregistry.info/Elements/u/P60462> reg:hasSubproperty <http://rdaregistry.info/Elements/w/P10040> ;
	reg:name "defendant"@en ;
	reg:status status:1001 ;
	a rdf:Property ;
	rdfs:isDefinedBy <http://rdaregistry.info/Elements/u/> ;
	rdfs:label "has defendant"@en ;
	rdfs:subPropertyOf <http://rdaregistry.info/Elements/u/P60374> ;
	owl:inverseOf <http://rdaregistry.info/Elements/u/P60698> ;
	owl:sameAs <http://rdaregistry.info/Elements/u/defendant> ;
	skos:closeMatch "http://id.loc.gov/vocabulary/relators/dfd"@en ;
	skos:definition "Relates a resource to an agent who is accused in a criminal proceeding or sued in a civil proceeding."@en .

<http://rdaregistry.info/Elements/u/P60463> reg:hasSubproperty <http://rdaregistry.info/Elements/w/P10045> ;
	reg:name "praeses"@en ;
	reg:status status:1001 ;
	a rdf:Property ;
	rdfs:isDefinedBy <http://rdaregistry.info/Elements/u/> ;
	rdfs:label "has praeses"@en ;
	rdfs:subPropertyOf <http://rdaregistry.info/Elements/u/P60447> ;
	owl:inverseOf <http://rdaregistry.info/Elements/u/P60699> ;
	owl:sameAs <http://rdaregistry.info/Elements/u/praeses> ;
	skos:closeMatch "http://id.loc.gov/vocabulary/relators/pra"@en ;
	skos:definition "Relates a resource to an agent who is the faculty moderator of an academic disputation, normally proposing a thesis and participating in the ensuing disputation."@en .

<http://rdaregistry.info/Elements/u/P60464> reg:hasSubproperty <http://rdaregistry.info/Elements/i/P40015> ;
	reg:name "annotator"@en ;
	reg:status status:1001 ;
	a rdf:Property ;
	rdfs:isDefinedBy <http://rdaregistry.info/Elements/u/> ;
	rdfs:label "has annotator"@en ;
	rdfs:subPropertyOf <http://rdaregistry.info/Elements/u/P60374> ;
	owl:inverseOf <http://rdaregistry.info/Elements/u/P60700> ;
	owl:sameAs <http://rdaregistry.info/Elements/u/annotator> ;
	skos:closeMatch "http://id.loc.gov/vocabulary/relators/ann"@en ;
	skos:definition "Relates a resource to an agent who makes manuscript annotations on a resource."@en .

<http://rdaregistry.info/Elements/u/P60465> reg:hasSubproperty <http://rdaregistry.info/Elements/w/P10071> ;
	reg:name "consultant"@en ;
	reg:status status:1001 ;
	a rdf:Property ;
	rdfs:isDefinedBy <http://rdaregistry.info/Elements/u/> ;
	rdfs:label "has consultant"@en ;
	rdfs:subPropertyOf <http://rdaregistry.info/Elements/u/P60447> ;
	owl:inverseOf <http://rdaregistry.info/Elements/u/P60701> ;
	owl:sameAs <http://rdaregistry.info/Elements/u/consultant> ;
	skos:closeMatch "http://id.loc.gov/vocabulary/relators/csl"@en ;
	skos:definition "Relates a resource to an agent who provides consultation services, and often makes recommendations, for another person, family or corporate body that is represented as the creator of a resource."@en .

<http://rdaregistry.info/Elements/u/P60466> reg:hasSubproperty <http://rdaregistry.info/Elements/i/P40016> ;
	reg:name "autographer"@en ;
	reg:status status:1001 ;
	a rdf:Property ;
	rdfs:isDefinedBy <http://rdaregistry.info/Elements/u/> ;
	rdfs:label "has autographer"@en ;
	rdfs:subPropertyOf <http://rdaregistry.info/Elements/u/P60374> ;
	owl:inverseOf <http://rdaregistry.info/Elements/u/P60702> ;
	owl:sameAs <http://rdaregistry.info/Elements/u/autographer> ;
	skos:closeMatch "http://id.loc.gov/vocabulary/relators/ato"@en ;
	skos:definition "Relates a resource to an agent whose manuscript signature appears on a resource."@en .

<http://rdaregistry.info/Elements/u/P60467> reg:hasSubproperty <http://rdaregistry.info/Elements/w/P10046> ;
	reg:name "issuingBody"@en ;
	reg:status status:1001 ;
	a rdf:Property ;
	rdfs:isDefinedBy <http://rdaregistry.info/Elements/u/> ;
	rdfs:label "has issuing body"@en ;
	rdfs:subPropertyOf <http://rdaregistry.info/Elements/u/P60374> ;
	owl:inverseOf <http://rdaregistry.info/Elements/u/P60703> ;
	owl:sameAs <http://rdaregistry.info/Elements/u/issuingBody> ;
	skos:closeMatch "http://id.loc.gov/vocabulary/relators/isb"@en ;
	skos:definition "Relates a resource to an agent, family or corporate body issuing a resource, such as an official organ of the body."@en .

<http://rdaregistry.info/Elements/u/P60468> reg:hasSubproperty <http://rdaregistry.info/Elements/a/P50104> ;
	reg:name "professionOrOccupation"@en ;
	reg:status status:1001 ;
	a rdf:Property ;
	rdfs:isDefinedBy <http://rdaregistry.info/Elements/u/> ;
	rdfs:label "has profession or occupation"@en ;
	owl:sameAs <http://rdaregistry.info/Elements/u/professionOrOccupation> ;
	skos:definition "Relates a resource to an agent’s vocation or avocation."@en .

<http://rdaregistry.info/Elements/u/P60469> reg:hasSubproperty <http://rdaregistry.info/Elements/i/P40027> , <http://rdaregistry.info/Elements/m/P30136> ;
	reg:name "electronicReproductionOf"@en ;
	reg:status status:1001 ;
	a rdf:Property ;
	rdfs:isDefinedBy <http://rdaregistry.info/Elements/u/> ;
	rdfs:label "is electronic reproduction of"@en ;
	rdfs:subPropertyOf <http://rdaregistry.info/Elements/u/P60297> ;
	owl:inverseOf <http://rdaregistry.info/Elements/u/P60083> ;
	owl:sameAs <http://rdaregistry.info/Elements/u/electronicReproductionOf> ;
	skos:definition "Relates a resource to an analog resource used as the basis for an electronic reproduction."@en .

<http://rdaregistry.info/Elements/u/P60470> reg:hasSubproperty <http://rdaregistry.info/Elements/e/P20071> , <http://rdaregistry.info/Elements/u/P60123> ;
	reg:name "noteOnResource"@en ;
	reg:status status:1001 ;
	a rdf:Property ;
	rdfs:isDefinedBy <http://rdaregistry.info/Elements/u/> ;
	rdfs:label "has note on resource"@en ;
	owl:sameAs <http://rdaregistry.info/Elements/u/noteOnResource> ;
	skos:definition "Relates a resource to an annotation providing additional information about content recorded as a resource attribute."@en .

<http://rdaregistry.info/Elements/u/P60471> reg:status status:1008 ;
	rdfs:isDefinedBy <http://rdaregistry.info/Elements/u/> .

<http://rdaregistry.info/Elements/u/P60472> reg:hasSubproperty <http://rdaregistry.info/Elements/w/P10199> ;
	reg:name "epoch"@en ;
	reg:status status:1001 ;
	a rdf:Property ;
	rdfs:isDefinedBy <http://rdaregistry.info/Elements/u/> ;
	rdfs:label "has epoch"@en ;
	owl:sameAs <http://rdaregistry.info/Elements/u/epoch> ;
	skos:definition "Relates a resource to an arbitrary moment in time to which measurements of position for a body or orientation for an orbit are referred."@en .

<http://rdaregistry.info/Elements/u/P60473> reg:hasSubproperty <http://rdaregistry.info/Elements/w/P10200> ;
	reg:name "landscapeArchitect"@en ;
	reg:status status:1001 ;
	a rdf:Property ;
	rdfs:isDefinedBy <http://rdaregistry.info/Elements/u/> ;
	rdfs:label "has landscape architect"@en ;
	rdfs:subPropertyOf <http://rdaregistry.info/Elements/u/P60435> ;
	owl:inverseOf <http://rdaregistry.info/Elements/u/P60704> ;
	owl:sameAs <http://rdaregistry.info/Elements/u/landscapeArchitect> ;
	skos:closeMatch "http://id.loc.gov/vocabulary/relators/lsa"@en ;
	skos:definition "Relates a resource to an architect responsible for creating landscape resources."@en .

<http://rdaregistry.info/Elements/u/P60474> reg:hasSubproperty <http://rdaregistry.info/Elements/e/P20197> , <http://rdaregistry.info/Elements/w/P10201> ;
	reg:name "findingAidFor"@en ;
	reg:status status:1001 ;
	a rdf:Property ;
	rdfs:isDefinedBy <http://rdaregistry.info/Elements/u/> ;
	rdfs:label "is finding aid for"@en ;
	rdfs:subPropertyOf <http://rdaregistry.info/Elements/u/P60307> ;
	owl:inverseOf <http://rdaregistry.info/Elements/u/P60262> ;
	owl:sameAs <http://rdaregistry.info/Elements/u/findingAidFor> ;
	skos:definition "Relates a resource to an archival collection that is described in a finding aid, i.e., a guide to the organization, arrangement, and contents of the collection."@en .

<http://rdaregistry.info/Elements/u/P60475> reg:hasSubproperty <http://rdaregistry.info/Elements/w/P10202> ;
	reg:name "sculptor"@en ;
	reg:status status:1001 ;
	a rdf:Property ;
	rdfs:isDefinedBy <http://rdaregistry.info/Elements/u/> ;
	rdfs:label "has sculptor"@en ;
	rdfs:subPropertyOf <http://rdaregistry.info/Elements/u/P60431> ;
	owl:inverseOf <http://rdaregistry.info/Elements/u/P60705> ;
	owl:sameAs <http://rdaregistry.info/Elements/u/sculptor> ;
	skos:closeMatch "http://id.loc.gov/vocabulary/relators/scl"@en ;
	skos:definition "Relates a resource to an artist responsible for creating a three-dimensional resource by modeling, carving, or similar technique."@en .

<http://rdaregistry.info/Elements/u/P60476> reg:hasSubproperty <http://rdaregistry.info/Elements/w/P10203> ;
	reg:name "screenwriter"@en ;
	reg:status status:1001 ;
	a rdf:Property ;
	rdfs:isDefinedBy <http://rdaregistry.info/Elements/u/> ;
	rdfs:label "has screenwriter"@en ;
	rdfs:subPropertyOf <http://rdaregistry.info/Elements/u/P60434> ;
	owl:inverseOf <http://rdaregistry.info/Elements/u/P60706> ;
	owl:sameAs <http://rdaregistry.info/Elements/u/screenwriter> ;
	skos:closeMatch "http://id.loc.gov/vocabulary/relators/aus"@en ;
	skos:definition "Relates a resource to an author of a screenplay, script, or scene."@en .

<http://rdaregistry.info/Elements/u/P60477> reg:hasSubproperty <http://rdaregistry.info/Elements/w/P10204> ;
	reg:name "lyricist"@en ;
	reg:status status:1001 ;
	a rdf:Property ;
	rdfs:isDefinedBy <http://rdaregistry.info/Elements/u/> ;
	rdfs:label "has lyricist"@en ;
	rdfs:subPropertyOf <http://rdaregistry.info/Elements/u/P60434> ;
	owl:inverseOf <http://rdaregistry.info/Elements/u/P60707> ;
	owl:sameAs <http://rdaregistry.info/Elements/u/lyricist> ;
	skos:closeMatch "http://id.loc.gov/vocabulary/relators/lyr"@en ;
	skos:definition "Relates a resource to an author of the words of a popular song, including a song or songs from a musical."@en .

<http://rdaregistry.info/Elements/u/P60478> reg:hasSubproperty <http://rdaregistry.info/Elements/w/P10205> ;
	reg:name "librettist"@en ;
	reg:status status:1001 ;
	a rdf:Property ;
	rdfs:isDefinedBy <http://rdaregistry.info/Elements/u/> ;
	rdfs:label "has librettist"@en ;
	rdfs:subPropertyOf <http://rdaregistry.info/Elements/u/P60434> ;
	owl:inverseOf <http://rdaregistry.info/Elements/u/P60708> ;
	owl:sameAs <http://rdaregistry.info/Elements/u/librettist> ;
	skos:closeMatch "http://id.loc.gov/vocabulary/relators/lbt"@en ;
	skos:definition "Relates a resource to an author of the words of an opera or other musical stage resource or an oratorio."@en .

<http://rdaregistry.info/Elements/u/P60479> reg:hasSubproperty <http://rdaregistry.info/Elements/e/P20198> , <http://rdaregistry.info/Elements/w/P10206> ;
	reg:name "replacementInPartOf"@en ;
	reg:status status:1001 ;
	a rdf:Property ;
	rdfs:isDefinedBy <http://rdaregistry.info/Elements/u/> ;
	rdfs:label "is replacement in part of"@en ;
	rdfs:subPropertyOf <http://rdaregistry.info/Elements/u/P60261> ;
	owl:inverseOf <http://rdaregistry.info/Elements/u/P60103> ;
	owl:sameAs <http://rdaregistry.info/Elements/u/replacementInPartOf> , <http://rdaregistry.info/Elements/u/supersedesInPart> ;
	skos:definition "Relates a resource to an earlier resource whose content has been partially replaced by a later resource, usually because the later resource contains updated or new information that makes the earlier resource obsolete."@en .

<http://rdaregistry.info/Elements/u/P60480> reg:hasSubproperty <http://rdaregistry.info/Elements/e/P20199> , <http://rdaregistry.info/Elements/w/P10207> ;
	reg:name "replacementOf"@en ;
	reg:status status:1001 ;
	a rdf:Property ;
	rdfs:isDefinedBy <http://rdaregistry.info/Elements/u/> ;
	rdfs:label "is replacement of"@en ;
	rdfs:subPropertyOf <http://rdaregistry.info/Elements/u/P60261> ;
	owl:inverseOf <http://rdaregistry.info/Elements/u/P60104> ;
	owl:sameAs <http://rdaregistry.info/Elements/u/replacementOf> , <http://rdaregistry.info/Elements/u/supersedes> ;
	skos:definition "Relates a resource to an earlier resource whose content has been replaced by a later resource, usually because the later resource contains updated or new information that makes the earlier resource obsolete."@en .

<http://rdaregistry.info/Elements/u/P60481> reg:hasSubproperty <http://rdaregistry.info/Elements/m/P30138> ;
	reg:name "specialPlaybackCharacteristic"@en ;
	reg:status status:1001 ;
	a rdf:Property ;
	rdfs:isDefinedBy <http://rdaregistry.info/Elements/u/> ;
	rdfs:label "has special playback characteristic"@en ;
	rdfs:subPropertyOf <http://rdaregistry.info/Elements/u/P60351> ;
	owl:sameAs <http://rdaregistry.info/Elements/u/specialPlaybackCharacteristic> ;
	skos:definition "Relates a resource to an equalization system, noise reduction system, etc., used in making an audio recording."@en .

<http://rdaregistry.info/Elements/u/P60482> reg:hasSubproperty <http://rdaregistry.info/Elements/a/P50034> ;
	reg:name "associatedInstitution"@en ;
	reg:status status:1001 ;
	a rdf:Property ;
	rdfs:isDefinedBy <http://rdaregistry.info/Elements/u/> ;
	rdfs:label "has associated institution"@en ;
	owl:sameAs <http://rdaregistry.info/Elements/u/associatedInstitution> ;
	skos:definition "Relates a resource to an institution commonly associated with an agent."@en .

<http://rdaregistry.info/Elements/u/P60483> reg:hasSubproperty <http://rdaregistry.info/Elements/w/P10208> ;
	reg:name "grantingInstitutionOrFaculty"@en ;
	reg:status status:1001 ;
	a rdf:Property ;
	rdfs:isDefinedBy <http://rdaregistry.info/Elements/u/> ;
	rdfs:label "has granting institution or faculty"@en ;
	owl:sameAs <http://rdaregistry.info/Elements/u/grantingInstitutionOrFaculty> ;
	skos:definition "Relates a resource to an institution or faculty conferring an academic degree on a candidate."@en .

<http://rdaregistry.info/Elements/u/P60484> reg:hasSubproperty <http://rdaregistry.info/Elements/a/P50035> , <http://rdaregistry.info/Elements/a/P50064> ;
	reg:name "agentHistory"@en ;
	reg:status status:1001 ;
	a rdf:Property ;
	rdfs:isDefinedBy <http://rdaregistry.info/Elements/u/> ;
	rdfs:label "has agent history"@en ;
	owl:sameAs <http://rdaregistry.info/Elements/u/agentHistory> ;
	skos:definition "Relates a resource to biographical or historical information about the agent."@en .

<http://rdaregistry.info/Elements/u/P60485> reg:hasSubproperty <http://rdaregistry.info/Elements/e/P20206> ;
	reg:name "supplementaryContent"@en ;
	reg:status status:1001 ;
	a rdf:Property ;
	rdfs:isDefinedBy <http://rdaregistry.info/Elements/u/> ;
	rdfs:label "has supplementary content"@en ;
	owl:sameAs <http://rdaregistry.info/Elements/u/supplementaryContent> ;
	skos:definition "Relates a resource to content (e.g., an index, a bibliography, an appendix) designed to supplement the primary content of a resource."@en .

<http://rdaregistry.info/Elements/u/P60486> reg:hasSubproperty <http://rdaregistry.info/Elements/e/P20207> ;
	reg:name "illustrativeContent"@en ;
	reg:status status:1001 ;
	a rdf:Property ;
	rdfs:isDefinedBy <http://rdaregistry.info/Elements/u/> ;
	rdfs:label "has illustrative content"@en ;
	owl:sameAs <http://rdaregistry.info/Elements/u/illustrativeContent> ;
	skos:definition "Relates a resource to content designed to illustrate the primary content of a resource."@en .

<http://rdaregistry.info/Elements/u/P60487> reg:hasSubproperty <http://rdaregistry.info/Elements/e/P20208> ;
	reg:name "accessibilityContent"@en ;
	reg:status status:1001 ;
	a rdf:Property ;
	rdfs:isDefinedBy <http://rdaregistry.info/Elements/u/> ;
	rdfs:label "has accessibility content"@en ;
	owl:sameAs <http://rdaregistry.info/Elements/u/accessibilityContent> ;
	skos:definition "Relates a resource to content that assists those with a sensory impairment in the greater understanding of content which their impairment prevents them fully seeing or hearing."@en .

<http://rdaregistry.info/Elements/u/P60488> reg:hasSubproperty <http://rdaregistry.info/Elements/e/P20209> ;
	reg:name "formatOfNotatedMusic"@en ;
	reg:status status:1001 ;
	a rdf:Property ;
	rdfs:isDefinedBy <http://rdaregistry.info/Elements/u/> ;
	rdfs:label "has format of notated music"@en ;
	owl:sameAs <http://rdaregistry.info/Elements/u/formatOfNotatedMusic> ;
	skos:definition "Relates a resource to the musical or physical layout of the content of a resource that is presented in the form of musical notation."@en .

<http://rdaregistry.info/Elements/u/P60489> reg:hasSubproperty <http://rdaregistry.info/Elements/w/P10209> ;
	reg:name "dissertationOrThesisInformation"@en ;
	reg:status status:1001 ;
	a rdf:Property ;
	rdfs:isDefinedBy <http://rdaregistry.info/Elements/u/> ;
	rdfs:label "has dissertation or thesis information"@en ;
	owl:sameAs <http://rdaregistry.info/Elements/u/dissertationOrThesisInformation> ;
	skos:definition "Relates a resource to information about a resource presented as part of the formal requirements for an academic degree."@en .

<http://rdaregistry.info/Elements/u/P60490> reg:hasSubproperty <http://rdaregistry.info/Elements/m/P30141> ;
	reg:name "contactInformation"@en ;
	reg:status status:1001 ;
	a rdf:Property ;
	rdfs:isDefinedBy <http://rdaregistry.info/Elements/u/> ;
	rdfs:label "has contact information"@en ;
	owl:sameAs <http://rdaregistry.info/Elements/u/contactInformation> ;
	skos:definition "Relates a resource to information about an organization, etc., from which a resource may be obtained."@en .

<http://rdaregistry.info/Elements/u/P60491> reg:hasSubproperty <http://rdaregistry.info/Elements/w/P10210> ;
	reg:name "historyOfTheResource"@en ;
	reg:status status:1001 ;
	a rdf:Property ;
	rdfs:isDefinedBy <http://rdaregistry.info/Elements/u/> ;
	rdfs:label "has history of the resource"@en ;
	owl:sameAs <http://rdaregistry.info/Elements/u/historyOfTheResource> ;
	skos:definition "Relates a resource to information about the history of a resource."@en .

<http://rdaregistry.info/Elements/u/P60492> reg:hasSubproperty <http://rdaregistry.info/Elements/a/P50113> ;
	reg:name "biographicalInformation"@en ;
	reg:status status:1001 ;
	a rdf:Property ;
	rdfs:isDefinedBy <http://rdaregistry.info/Elements/u/> ;
	rdfs:label "has biographical information"@en ;
	owl:sameAs <http://rdaregistry.info/Elements/u/biographicalInformation> ;
	skos:definition "Relates a resource to information about the life or history of an agent."@en .

<http://rdaregistry.info/Elements/u/P60493> reg:hasSubproperty <http://rdaregistry.info/Elements/m/P30142> ;
	reg:name "otherTitleInformation"@en ;
	reg:status status:1001 ;
	a rdf:Property ;
	rdfs:isDefinedBy <http://rdaregistry.info/Elements/u/> ;
	rdfs:label "has other title information"@en ;
	rdfs:subPropertyOf <http://rdaregistry.info/Elements/u/P60369> ;
	owl:sameAs <http://rdaregistry.info/Elements/u/otherTitleInformation> ;
	skos:definition "Relates a resource to information that appears in conjunction with, and is subordinate to, the title proper of a resource."@en .

<http://rdaregistry.info/Elements/u/P60494> reg:hasSubproperty <http://rdaregistry.info/Elements/m/P30143> ;
	reg:name "otherTitleInformationOfSeries"@en ;
	reg:status status:1001 ;
	a rdf:Property ;
	rdfs:isDefinedBy <http://rdaregistry.info/Elements/u/> ;
	rdfs:label "has other title information of series"@en ;
	owl:sameAs <http://rdaregistry.info/Elements/u/otherTitleInformationOfSeries> ;
	skos:definition "Relates a resource to information that appears in conjunction with, and is subordinate to, the title proper of a series."@en .

<http://rdaregistry.info/Elements/u/P60495> reg:hasSubproperty <http://rdaregistry.info/Elements/m/P30144> ;
	reg:name "otherTitleInformationOfSubseries"@en ;
	reg:status status:1001 ;
	a rdf:Property ;
	rdfs:isDefinedBy <http://rdaregistry.info/Elements/u/> ;
	rdfs:label "has other title information of subseries"@en ;
	owl:sameAs <http://rdaregistry.info/Elements/u/otherTitleInformationOfSubseries> ;
	skos:definition "Relates a resource to information that appears in conjunction with, and is subordinate to, the title proper of a subseries."@en .

<http://rdaregistry.info/Elements/u/P60496> reg:hasSubproperty <http://rdaregistry.info/Elements/i/P40047> , <http://rdaregistry.info/Elements/m/P30145> ;
	reg:name "restrictionsOnAccess"@en ;
	reg:status status:1001 ;
	a rdf:Property ;
	rdfs:isDefinedBy <http://rdaregistry.info/Elements/u/> ;
	rdfs:label "has restrictions on access"@en ;
	owl:sameAs <http://rdaregistry.info/Elements/u/restrictionsOnAccess> ;
	skos:definition "Relates a resource to limitations placed on access to a resource."@en .

<http://rdaregistry.info/Elements/u/P60497> reg:hasSubproperty <http://rdaregistry.info/Elements/i/P40048> , <http://rdaregistry.info/Elements/m/P30146> ;
	reg:name "restrictionsOnUse"@en ;
	reg:status status:1001 ;
	a rdf:Property ;
	rdfs:isDefinedBy <http://rdaregistry.info/Elements/u/> ;
	rdfs:label "has restrictions on use"@en ;
	owl:sameAs <http://rdaregistry.info/Elements/u/restrictionsOnUse> ;
	skos:definition "Relates a resource to limitations placed on uses such as reproduction, publication, exhibition, etc."@en .

<http://rdaregistry.info/Elements/u/P60498> reg:hasSubproperty <http://rdaregistry.info/Elements/e/P20210> ;
	reg:name "otherDetailsOfCartographicContent"@en ;
	reg:status status:1001 ;
	a rdf:Property ;
	rdfs:isDefinedBy <http://rdaregistry.info/Elements/u/> ;
	rdfs:label "has other details of cartographic content"@en ;
	owl:sameAs <http://rdaregistry.info/Elements/u/otherDetailsOfCartographicContent> ;
	skos:definition "Relates a resource to mathematical data and other features of the cartographic content of a resource not recorded in statements of scale, projection, and coordinates."@en .

<http://rdaregistry.info/Elements/u/P60499> reg:hasSubproperty <http://rdaregistry.info/Elements/m/P30097> , <http://rdaregistry.info/Elements/m/P30147> ;
	reg:name "numericAndOrAlphabeticDesignationOfFirstIssueOrPartOfSequence"@en ;
	reg:status status:1001 ;
	a rdf:Property ;
	rdfs:isDefinedBy <http://rdaregistry.info/Elements/u/> ;
	rdfs:label "has numeric and/or alphabetic designation of first issue or part of sequence"@en ;
	rdfs:subPropertyOf <http://rdaregistry.info/Elements/u/P60533> ;
	owl:sameAs <http://rdaregistry.info/Elements/u/numericAndOrAlphabeticDesignationOfFirstIssueOrPartOfSequence> ;
	skos:definition "Relates a resource to numbering presented in numeric and/or alphabetic form on the first issue or part of a sequence of numbering for a serial."@en .

<http://rdaregistry.info/Elements/u/P60500> reg:hasSubproperty <http://rdaregistry.info/Elements/m/P30098> , <http://rdaregistry.info/Elements/m/P30148> ;
	reg:name "numericAndOrAlphabeticDesignationOfLastIssueOrPartOfSequence"@en ;
	reg:status status:1001 ;
	a rdf:Property ;
	rdfs:isDefinedBy <http://rdaregistry.info/Elements/u/> ;
	rdfs:label "has numeric and/or alphabetic designation of last issue or part of sequence"@en ;
	rdfs:subPropertyOf <http://rdaregistry.info/Elements/u/P60533> ;
	owl:sameAs <http://rdaregistry.info/Elements/u/numericAndOrAlphabeticDesignationOfLastIssueOrPartOfSequence> ;
	skos:definition "Relates a resource to numbering presented in numeric and/or alphabetic form on the last issue or part of a sequence of numbering for a serial."@en .

<http://rdaregistry.info/Elements/u/P60501> reg:hasSubproperty <http://rdaregistry.info/Elements/m/P30099> , <http://rdaregistry.info/Elements/m/P30149> ;
	reg:name "chronologicalDesignationOfFirstIssueOrPartOfSequence"@en ;
	reg:status status:1001 ;
	a rdf:Property ;
	rdfs:isDefinedBy <http://rdaregistry.info/Elements/u/> ;
	rdfs:label "has chronological designation of first issue or part of sequence"@en ;
	rdfs:subPropertyOf <http://rdaregistry.info/Elements/u/P60533> ;
	owl:sameAs <http://rdaregistry.info/Elements/u/chronologicalDesignationOfFirstIssueOrPartOfSequence> ;
	skos:definition "Relates a resource to numbering presented in the form of a date (e.g., a year; year and month; month, day, and year) on the first issue or part of a sequence of numbering for a serial."@en .

<http://rdaregistry.info/Elements/u/P60502> reg:hasSubproperty <http://rdaregistry.info/Elements/m/P30100> , <http://rdaregistry.info/Elements/m/P30150> ;
	reg:name "chronologicalDesignationOfLastIssueOrPartOfSequence"@en ;
	reg:status status:1001 ;
	a rdf:Property ;
	rdfs:isDefinedBy <http://rdaregistry.info/Elements/u/> ;
	rdfs:label "has chronological designation of last issue or part of sequence"@en ;
	rdfs:subPropertyOf <http://rdaregistry.info/Elements/u/P60533> ;
	owl:sameAs <http://rdaregistry.info/Elements/u/chronologicalDesignationOfLastIssueOrPartOfSequence> ;
	skos:definition "Relates a resource to numbering presented in the form of a date (e.g., a year; year and month; month, day, and year) on the last issue or part of a sequence of numbering for a serial."@en .

<http://rdaregistry.info/Elements/u/P60503> reg:hasSubproperty <http://rdaregistry.info/Elements/e/P20200> , <http://rdaregistry.info/Elements/w/P10211> ;
	reg:name "splitInto"@en ;
	reg:status status:1001 ;
	a rdf:Property ;
	rdfs:isDefinedBy <http://rdaregistry.info/Elements/u/> ;
	rdfs:label "is split into"@en ;
	rdfs:subPropertyOf <http://rdaregistry.info/Elements/u/P60278> ;
	owl:inverseOf <http://rdaregistry.info/Elements/u/P60276> ;
	owl:sameAs <http://rdaregistry.info/Elements/u/splitInto> ;
	skos:definition "Relates a resource to one of two or more resources resulting from the division of an earlier resource into separate resources."@en .

<http://rdaregistry.info/Elements/u/P60504> reg:hasSubproperty <http://rdaregistry.info/Elements/e/P20212> , <http://rdaregistry.info/Elements/w/P10212> ;
	reg:name "mergedToForm"@en ;
	reg:status status:1001 ;
	a rdf:Property ;
	rdfs:isDefinedBy <http://rdaregistry.info/Elements/u/> ;
	rdfs:label "is merged to form"@en ;
	rdfs:subPropertyOf <http://rdaregistry.info/Elements/u/P60278> ;
	owl:inverseOf <http://rdaregistry.info/Elements/u/P60505> ;
	owl:sameAs <http://rdaregistry.info/Elements/u/mergedToForm> ;
	skos:definition "Relates a resource to a resource which brings the resource together with another resource"@en .

<http://rdaregistry.info/Elements/u/P60505> reg:hasSubproperty <http://rdaregistry.info/Elements/e/P20201> , <http://rdaregistry.info/Elements/w/P10213> ;
	reg:name "mergerOf"@en ;
	reg:status status:1001 ;
	a rdf:Property ;
	rdfs:isDefinedBy <http://rdaregistry.info/Elements/u/> ;
	rdfs:label "is merger of"@en ;
	rdfs:subPropertyOf <http://rdaregistry.info/Elements/u/P60261> ;
	owl:inverseOf <http://rdaregistry.info/Elements/u/P60504> ;
	owl:sameAs <http://rdaregistry.info/Elements/u/mergerOf> ;
	skos:definition "Relates a resource to one of the resources which come together to form the resource"@en .

<http://rdaregistry.info/Elements/u/P60506> reg:hasSubproperty <http://rdaregistry.info/Elements/w/P10214> ;
	reg:name "equinox"@en ;
	reg:status status:1001 ;
	a rdf:Property ;
	rdfs:isDefinedBy <http://rdaregistry.info/Elements/u/> ;
	rdfs:label "has equinox"@en ;
	owl:sameAs <http://rdaregistry.info/Elements/u/equinox> ;
	skos:definition "Relates a resource to one of two points of intersection of the ecliptic and the celestial equator, occupied by the sun when its declination is 0°."@en .

<http://rdaregistry.info/Elements/u/P60507> reg:hasSubproperty <http://rdaregistry.info/Elements/m/P30151> ;
	reg:name "parallelOtherTitleInformation"@en ;
	reg:status status:1001 ;
	a rdf:Property ;
	rdfs:isDefinedBy <http://rdaregistry.info/Elements/u/> ;
	rdfs:label "has parallel other title information"@en ;
	rdfs:subPropertyOf <http://rdaregistry.info/Elements/u/P60369> ;
	owl:sameAs <http://rdaregistry.info/Elements/u/parallelOtherTitleInformation> ;
	skos:definition "Relates a resource to other title information in a language and/or script that differs from that recorded in the other title information element."@en .

<http://rdaregistry.info/Elements/u/P60508> reg:hasSubproperty <http://rdaregistry.info/Elements/m/P30152> ;
	reg:name "parallelOtherTitleInformationOfSeries"@en ;
	reg:status status:1001 ;
	a rdf:Property ;
	rdfs:isDefinedBy <http://rdaregistry.info/Elements/u/> ;
	rdfs:label "has parallel other title information of series"@en ;
	owl:sameAs <http://rdaregistry.info/Elements/u/parallelOtherTitleInformationOfSeries> ;
	skos:definition "Relates a resource to other title information of a series in a language and/or script that differs from that recorded in the other title information of series element."@en .

<http://rdaregistry.info/Elements/u/P60509> reg:hasSubproperty <http://rdaregistry.info/Elements/m/P30153> ;
	reg:name "parallelOtherTitleInformationOfSubseries"@en ;
	reg:status status:1001 ;
	a rdf:Property ;
	rdfs:isDefinedBy <http://rdaregistry.info/Elements/u/> ;
	rdfs:label "has parallel other title information of subseries"@en ;
	owl:sameAs <http://rdaregistry.info/Elements/u/parallelOtherTitleInformationOfSubseries> ;
	skos:definition "Relates a resource to other title information of a subseries in a language and/or script that differs from that recorded in the other title information of subseries element."@en .

<http://rdaregistry.info/Elements/u/P60510> reg:hasSubproperty <http://rdaregistry.info/Elements/e/P20213> ;
	reg:name "additionalScaleInformation"@en ;
	reg:status status:1001 ;
	a rdf:Property ;
	rdfs:isDefinedBy <http://rdaregistry.info/Elements/u/> ;
	rdfs:label "has additional scale information"@en ;
	rdfs:subPropertyOf <http://rdaregistry.info/Elements/u/P60565> ;
	owl:sameAs <http://rdaregistry.info/Elements/u/additionalScaleInformation> ;
	skos:definition "Relates a resource to supplemental information about scale such as a statement of comparative measurements or limitation of the scale to particular parts of the content of a resource."@en .

<http://rdaregistry.info/Elements/u/P60511> reg:hasSubproperty <http://rdaregistry.info/Elements/m/P30154> ;
	reg:name "uniformResourceLocator"@en ;
	reg:status status:1001 ;
	a rdf:Property ;
	rdfs:isDefinedBy <http://rdaregistry.info/Elements/u/> ;
	rdfs:label "has uniform resource locator"@en ;
	owl:sameAs <http://rdaregistry.info/Elements/u/uniformResourceLocator> ;
	skos:definition "Relates a resource to the address of a remote access resource."@en .

<http://rdaregistry.info/Elements/u/P60512> reg:hasSubproperty <http://rdaregistry.info/Elements/a/P50036> , <http://rdaregistry.info/Elements/a/P50114> ;
	reg:name "addressOfTheAgent"@en ;
	reg:status status:1001 ;
	a rdf:Property ;
	rdfs:isDefinedBy <http://rdaregistry.info/Elements/u/> ;
	rdfs:label "has address of the agent"@en ;
	owl:sameAs <http://rdaregistry.info/Elements/u/addressOfTheAgent> ;
	skos:definition "Relates a resource to the address of an agent’s place of residence, business, or employer, headquarters or offices, or an e-mail or internet address."@en .

<http://rdaregistry.info/Elements/u/P60513> reg:hasSubproperty <http://rdaregistry.info/Elements/m/P30155> ;
	reg:name "layout"@en ;
	reg:status status:1001 ;
	a rdf:Property ;
	rdfs:isDefinedBy <http://rdaregistry.info/Elements/u/> ;
	rdfs:label "has layout"@en ;
	owl:sameAs <http://rdaregistry.info/Elements/u/layout> ;
	skos:definition "Relates a resource to the arrangement of text, images, tactile notation, etc., in a resource."@en .

<http://rdaregistry.info/Elements/u/P60514> reg:hasSubproperty <http://rdaregistry.info/Elements/w/P10215> ;
	reg:name "yearDegreeGranted"@en ;
	reg:status status:1001 ;
	a rdf:Property ;
	rdfs:isDefinedBy <http://rdaregistry.info/Elements/u/> ;
	rdfs:label "has year degree granted"@en ;
	owl:sameAs <http://rdaregistry.info/Elements/u/yearDegreeGranted> ;
	skos:definition "Relates a resource to the calendar year in which a granting institution or faculty conferred an academic degree on a candidate."@en .

<http://rdaregistry.info/Elements/u/P60515> reg:hasSubproperty <http://rdaregistry.info/Elements/m/P30156> ;
	reg:name "titleProper"@en ;
	reg:status status:1001 ;
	a rdf:Property ;
	rdfs:isDefinedBy <http://rdaregistry.info/Elements/u/> ;
	rdfs:label "has title proper"@en ;
	rdfs:subPropertyOf <http://rdaregistry.info/Elements/u/P60369> ;
	owl:sameAs <http://rdaregistry.info/Elements/u/titleProper> ;
	skos:definition "Relates a resource to the chief name of a resource (i.e., the title normally used when citing the resource)."@en .

<http://rdaregistry.info/Elements/u/P60516> reg:hasSubproperty <http://rdaregistry.info/Elements/m/P30157> ;
	reg:name "titleProperOfSeries"@en ;
	reg:status status:1001 ;
	a rdf:Property ;
	rdfs:isDefinedBy <http://rdaregistry.info/Elements/u/> ;
	rdfs:label "has title proper of series"@en ;
	owl:sameAs <http://rdaregistry.info/Elements/u/titleProperOfSeries> ;
	skos:definition "Relates a resource to the chief name of a series (i.e., the title normally used when citing the series)."@en .

<http://rdaregistry.info/Elements/u/P60517> reg:hasSubproperty <http://rdaregistry.info/Elements/m/P30158> ;
	reg:name "titleProperOfSubseries"@en ;
	reg:status status:1001 ;
	a rdf:Property ;
	rdfs:isDefinedBy <http://rdaregistry.info/Elements/u/> ;
	rdfs:label "has title proper of subseries"@en ;
	owl:sameAs <http://rdaregistry.info/Elements/u/titleProperOfSubseries> ;
	skos:definition "Relates a resource to the chief name of a subseries (i.e., the title normally used when citing the subseries)."@en .

<http://rdaregistry.info/Elements/u/P60518> reg:hasSubproperty <http://rdaregistry.info/Elements/w/P10216> ;
	reg:name "coverageOfTheContent"@en ;
	reg:status status:1001 ;
	a rdf:Property ;
	rdfs:isDefinedBy <http://rdaregistry.info/Elements/u/> ;
	rdfs:label "has coverage of the content"@en ;
	owl:sameAs <http://rdaregistry.info/Elements/u/coverageOfTheContent> ;
	skos:definition "Relates a resource to the chronological or geographic coverage of the content of a resource."@en .

<http://rdaregistry.info/Elements/u/P60519> reg:hasSubproperty <http://rdaregistry.info/Elements/m/P30159> ;
	reg:name "resolution"@en ;
	reg:status status:1001 ;
	a rdf:Property ;
	rdfs:isDefinedBy <http://rdaregistry.info/Elements/u/> ;
	rdfs:label "has resolution"@en ;
	rdfs:subPropertyOf <http://rdaregistry.info/Elements/u/P60350> ;
	owl:sameAs <http://rdaregistry.info/Elements/u/resolution> ;
	skos:definition "Relates a resource to the clarity or fineness of detail in a digital image, expressed by the measurement of the image in pixels, etc."@en .

<http://rdaregistry.info/Elements/u/P60520> reg:hasSubproperty <http://rdaregistry.info/Elements/w/P10217> ;
	reg:name "intendedAudience"@en ;
	reg:status status:1001 ;
	a rdf:Property ;
	rdfs:isDefinedBy <http://rdaregistry.info/Elements/u/> ;
	rdfs:label "has intended audience"@en ;
	owl:sameAs <http://rdaregistry.info/Elements/u/intendedAudience> ;
	skos:definition "Relates a resource to the class of user for which the content of a resource is intended, or for whom the content is considered suitable."@en .

<http://rdaregistry.info/Elements/u/P60521> reg:hasSubproperty <http://rdaregistry.info/Elements/m/P30160> ;
	reg:name "termsOfAvailability"@en ;
	reg:status status:1001 ;
	a rdf:Property ;
	rdfs:isDefinedBy <http://rdaregistry.info/Elements/u/> ;
	rdfs:label "has terms of availability"@en ;
	owl:sameAs <http://rdaregistry.info/Elements/u/termsOfAvailability> ;
	skos:definition "Relates a resource to the conditions under which the publisher, distributor, etc., will normally supply a resource or the price of a resource."@en .

<http://rdaregistry.info/Elements/u/P60522> reg:hasSubproperty <http://rdaregistry.info/Elements/m/P30161> ;
	reg:name "trackConfiguration"@en ;
	reg:status status:1001 ;
	a rdf:Property ;
	rdfs:isDefinedBy <http://rdaregistry.info/Elements/u/> ;
	rdfs:label "has track configuration"@en ;
	rdfs:subPropertyOf <http://rdaregistry.info/Elements/u/P60351> ;
	owl:sameAs <http://rdaregistry.info/Elements/u/trackConfiguration> ;
	skos:definition "Relates a resource to the configuration of the audio track on a sound-track film (e.g., centre track)."@en .

<http://rdaregistry.info/Elements/u/P60523> reg:hasSubproperty <http://rdaregistry.info/Elements/w/P10218> ;
	reg:name "placeOfOriginOfTheResource"@en ;
	reg:status status:1001 ;
	a rdf:Property ;
	rdfs:isDefinedBy <http://rdaregistry.info/Elements/u/> ;
	rdfs:label "has place of origin of the resource"@en ;
	owl:sameAs <http://rdaregistry.info/Elements/u/placeOfOriginOfTheResource> ;
	skos:definition "Relates a resource to the country or other territorial jurisdiction from which a resource originated."@en .

<http://rdaregistry.info/Elements/u/P60524> reg:hasSubproperty <http://rdaregistry.info/Elements/a/P50037> ;
	reg:name "dateOfEstablishment"@en ;
	reg:status status:1001 ;
	a rdf:Property ;
	rdfs:isDefinedBy <http://rdaregistry.info/Elements/u/> ;
	rdfs:label "has date of establishment"@en ;
	rdfs:subPropertyOf <http://rdaregistry.info/Elements/u/P60324> ;
	owl:sameAs <http://rdaregistry.info/Elements/u/dateOfEstablishment> ;
	skos:definition "Relates a resource to the date on which an agent was established or founded."@en .

<http://rdaregistry.info/Elements/u/P60525> reg:hasSubproperty <http://rdaregistry.info/Elements/a/P50038> ;
	reg:name "dateOfTermination"@en ;
	reg:status status:1001 ;
	a rdf:Property ;
	rdfs:isDefinedBy <http://rdaregistry.info/Elements/u/> ;
	rdfs:label "has date of termination"@en ;
	rdfs:subPropertyOf <http://rdaregistry.info/Elements/u/P60324> ;
	owl:sameAs <http://rdaregistry.info/Elements/u/dateOfTermination> ;
	skos:definition "Relates a resource to the date on which an agent was terminated or dissolved."@en .

<http://rdaregistry.info/Elements/u/P60526> reg:hasSubproperty <http://rdaregistry.info/Elements/a/P50039> ;
	reg:name "dateOfConferenceEtc"@en ;
	reg:status status:1001 ;
	a rdf:Property ;
	rdfs:isDefinedBy <http://rdaregistry.info/Elements/u/> ;
	rdfs:label "has date of conference, etc."@en ;
	rdfs:subPropertyOf <http://rdaregistry.info/Elements/u/P60324> ;
	owl:sameAs <http://rdaregistry.info/Elements/u/dateOfConferenceEtc> ;
	skos:definition "Relates a resource to the date or range of dates on which a conference, congress, meeting, exhibition, fair, festival, etc., was held."@en .

<http://rdaregistry.info/Elements/u/P60527> reg:hasSubproperty <http://rdaregistry.info/Elements/e/P20214> , <http://rdaregistry.info/Elements/w/P10219> ;
	reg:name "dateOfResource"@en ;
	reg:status status:1001 ;
	a rdf:Property ;
	rdfs:isDefinedBy <http://rdaregistry.info/Elements/u/> ;
	rdfs:label "has date of resource"@en ;
	owl:sameAs <http://rdaregistry.info/Elements/u/dateOfResource> ;
	skos:definition "Relates a resource to the earliest date associated with a resource."@en .

<http://rdaregistry.info/Elements/u/P60528> reg:hasSubproperty <http://rdaregistry.info/Elements/m/P30162> ;
	reg:name "equipmentOrSystemRequirement"@en ;
	reg:status status:1001 ;
	a rdf:Property ;
	rdfs:isDefinedBy <http://rdaregistry.info/Elements/u/> ;
	rdfs:label "has equipment or system requirement"@en ;
	owl:sameAs <http://rdaregistry.info/Elements/u/equipmentOrSystemRequirement> ;
	skos:definition "Relates a resource to the equipment or system required for use, playback, etc., of an analog, digital, etc., resource."@en .

<http://rdaregistry.info/Elements/u/P60529> reg:hasSubproperty <http://rdaregistry.info/Elements/m/P30163> ;
	reg:name "presentationFormat"@en ;
	reg:status status:1001 ;
	a rdf:Property ;
	rdfs:isDefinedBy <http://rdaregistry.info/Elements/u/> ;
	rdfs:label "has presentation format"@en ;
	rdfs:subPropertyOf <http://rdaregistry.info/Elements/u/P60353> ;
	owl:sameAs <http://rdaregistry.info/Elements/u/presentationFormat> ;
	skos:definition "Relates a resource to the format used in the production of a projected image (e.g., cinerama, imax)."@en .

<http://rdaregistry.info/Elements/u/P60530> reg:hasSubproperty <http://rdaregistry.info/Elements/a/P50115> ;
	reg:name "fullerFormOfName"@en ;
	reg:status status:1001 ;
	a rdf:Property ;
	rdfs:isDefinedBy <http://rdaregistry.info/Elements/u/> ;
	rdfs:label "has fuller form of name"@en ;
	owl:sameAs <http://rdaregistry.info/Elements/u/fullerFormOfName> ;
	skos:definition "Relates a resource to the full form of a part of a name represented only by an initial or abbreviation in the form chosen as the preferred name, or a part of the name not included in the form chosen as the preferred name."@en .

<http://rdaregistry.info/Elements/u/P60531> reg:hasSubproperty <http://rdaregistry.info/Elements/a/P50116> ;
	reg:name "gender"@en ;
	reg:status status:1001 ;
	a rdf:Property ;
	rdfs:isDefinedBy <http://rdaregistry.info/Elements/u/> ;
	rdfs:label "has gender"@en ;
	owl:sameAs <http://rdaregistry.info/Elements/u/gender> ;
	skos:definition "Relates a resource to the gender with which an agent identifies."@en .

<http://rdaregistry.info/Elements/u/P60532> reg:hasSubproperty <http://rdaregistry.info/Elements/m/P30164> ;
	reg:name "grooveCharacteristic"@en ;
	reg:status status:1001 ;
	a rdf:Property ;
	rdfs:isDefinedBy <http://rdaregistry.info/Elements/u/> ;
	rdfs:label "has groove characteristic"@en ;
	rdfs:subPropertyOf <http://rdaregistry.info/Elements/u/P60351> ;
	owl:sameAs <http://rdaregistry.info/Elements/u/grooveCharacteristic> ;
	skos:definition "Relates a resource to the groove width of an analog disc or the groove pitch of an analog cylinder."@en .

<http://rdaregistry.info/Elements/u/P60533> reg:hasSubproperty <http://rdaregistry.info/Elements/m/P30165> , <http://rdaregistry.info/Elements/u/P60499> , <http://rdaregistry.info/Elements/u/P60500> , <http://rdaregistry.info/Elements/u/P60501> , <http://rdaregistry.info/Elements/u/P60502> ;
	reg:name "numberingOfSerials"@en ;
	reg:status status:1001 ;
	a rdf:Property ;
	rdfs:isDefinedBy <http://rdaregistry.info/Elements/u/> ;
	rdfs:label "has numbering of serials"@en ;
	owl:sameAs <http://rdaregistry.info/Elements/u/numberingOfSerials> ;
	skos:definition "Relates a resource to the identification of each of the issues or parts of a serial. numbering of serials may include a numeral, a letter, any other character, or the combination of these with or without an accompanying caption (volume, number, etc.) and/or a chronological designation."@en .

<http://rdaregistry.info/Elements/u/P60534> reg:hasSubproperty <http://rdaregistry.info/Elements/m/P30166> ;
	reg:name "issnOfSeries"@en ;
	reg:status status:1001 ;
	a rdf:Property ;
	rdfs:isDefinedBy <http://rdaregistry.info/Elements/u/> ;
	rdfs:label "has issn of series"@en ;
	owl:sameAs <http://rdaregistry.info/Elements/u/issnOfSeries> ;
	skos:definition "Relates a resource to the identifier assigned to a series by an issn registration agency."@en .

<http://rdaregistry.info/Elements/u/P60535> reg:hasSubproperty <http://rdaregistry.info/Elements/m/P30167> ;
	reg:name "issnOfSubseries"@en ;
	reg:status status:1001 ;
	a rdf:Property ;
	rdfs:isDefinedBy <http://rdaregistry.info/Elements/u/> ;
	rdfs:label "has issn of subseries"@en ;
	owl:sameAs <http://rdaregistry.info/Elements/u/issnOfSubseries> ;
	skos:definition "Relates a resource to the identifier assigned to a subseries by an issn registration agency."@en .

<http://rdaregistry.info/Elements/u/P60536> reg:hasSubproperty <http://rdaregistry.info/Elements/w/P10220> ;
	reg:name "mediumOfPerformance"@en ;
	reg:status status:1001 ;
	a rdf:Property ;
	rdfs:isDefinedBy <http://rdaregistry.info/Elements/u/> ;
	rdfs:label "has medium of performance"@en ;
	owl:sameAs <http://rdaregistry.info/Elements/u/mediumOfPerformance> ;
	skos:definition "Relates a resource to the instrument, instruments, voice, voices, etc., for which a musical resource was originally conceived."@en .

<http://rdaregistry.info/Elements/u/P60537> reg:hasSubproperty <http://rdaregistry.info/Elements/e/P20215> ;
	reg:name "mediumOfPerformanceOfMusicalContent"@en ;
	reg:status status:1001 ;
	a rdf:Property ;
	rdfs:isDefinedBy <http://rdaregistry.info/Elements/u/> ;
	rdfs:label "has medium of performance of musical content"@en ;
	owl:sameAs <http://rdaregistry.info/Elements/u/mediumOfPerformanceOfMusicalContent> ;
	skos:definition "Relates a resource to the instrument, instruments, voice, voices, etc., used (or intended to be used) for performance of musical content."@en .

<http://rdaregistry.info/Elements/u/P60538> reg:hasSubproperty <http://rdaregistry.info/Elements/m/P30168> ;
	reg:name "frequency"@en ;
	reg:status status:1001 ;
	a rdf:Property ;
	rdfs:isDefinedBy <http://rdaregistry.info/Elements/u/> ;
	rdfs:label "has frequency"@en ;
	owl:sameAs <http://rdaregistry.info/Elements/u/frequency> ;
	skos:definition "Relates a resource to the intervals at which the issues or parts of a serial or the updates to an integrating resource are issued."@en .

<http://rdaregistry.info/Elements/u/P60539> reg:hasSubproperty <http://rdaregistry.info/Elements/m/P30169> , <http://rdaregistry.info/Elements/u/P60540> , <http://rdaregistry.info/Elements/u/P60541> ;
	reg:name "dimensions"@en ;
	reg:status status:1001 ;
	a rdf:Property ;
	rdfs:isDefinedBy <http://rdaregistry.info/Elements/u/> ;
	rdfs:label "has dimensions"@en ;
	owl:sameAs <http://rdaregistry.info/Elements/u/dimensions> ;
	skos:definition "Relates a resource to the measurements of the carrier or carriers and/or the container of a resource."@en .

<http://rdaregistry.info/Elements/u/P60540> reg:hasSubproperty <http://rdaregistry.info/Elements/m/P30170> ;
	reg:name "dimensionsOfMapEtc"@en ;
	reg:status status:1001 ;
	a rdf:Property ;
	rdfs:isDefinedBy <http://rdaregistry.info/Elements/u/> ;
	rdfs:label "has dimensions of map, etc."@en ;
	rdfs:subPropertyOf <http://rdaregistry.info/Elements/u/P60539> ;
	owl:sameAs <http://rdaregistry.info/Elements/u/dimensionsOfMapEtc> ;
	skos:definition "Relates a resource to the measurements of the face of a map, etc."@en .

<http://rdaregistry.info/Elements/u/P60541> reg:hasSubproperty <http://rdaregistry.info/Elements/m/P30171> ;
	reg:name "dimensionsOfStillImage"@en ;
	reg:status status:1001 ;
	a rdf:Property ;
	rdfs:isDefinedBy <http://rdaregistry.info/Elements/u/> ;
	rdfs:label "has dimensions of still image"@en ;
	rdfs:subPropertyOf <http://rdaregistry.info/Elements/u/P60539> ;
	owl:sameAs <http://rdaregistry.info/Elements/u/dimensionsOfStillImage> ;
	skos:definition "Relates a resource to the measurements of the pictorial area of a still image."@en .

<http://rdaregistry.info/Elements/u/P60542> reg:hasSubproperty <http://rdaregistry.info/Elements/e/P20216> ;
	reg:name "projectionOfCartographicContent"@en ;
	reg:status status:1001 ;
	a rdf:Property ;
	rdfs:isDefinedBy <http://rdaregistry.info/Elements/u/> ;
	rdfs:label "has projection of cartographic content"@en ;
	owl:sameAs <http://rdaregistry.info/Elements/u/projectionOfCartographicContent> ;
	skos:definition "Relates a resource to the method or system used to represent the surface of the earth or of a celestial sphere on a plane."@en .

<http://rdaregistry.info/Elements/u/P60543> reg:hasSubproperty <http://rdaregistry.info/Elements/m/P30172> ;
	reg:name "typeOfRecording"@en ;
	reg:status status:1001 ;
	a rdf:Property ;
	rdfs:isDefinedBy <http://rdaregistry.info/Elements/u/> ;
	rdfs:label "has type of recording"@en ;
	rdfs:subPropertyOf <http://rdaregistry.info/Elements/u/P60351> ;
	owl:sameAs <http://rdaregistry.info/Elements/u/typeOfRecording> ;
	skos:definition "Relates a resource to the method used to encode audio content for playback (e.g., analog or digital)."@en .

<http://rdaregistry.info/Elements/u/P60544> reg:hasSubproperty <http://rdaregistry.info/Elements/m/P30173> ;
	reg:name "distributorsName"@en ;
	reg:status status:1001 ;
	a rdf:Property ;
	rdfs:isDefinedBy <http://rdaregistry.info/Elements/u/> ;
	rdfs:label "has distributor's name"@en ;
	owl:sameAs <http://rdaregistry.info/Elements/u/distributorsName> ;
	skos:definition "Relates a resource to the name of an agent responsible for distributing a resource in a published form."@en .

<http://rdaregistry.info/Elements/u/P60545> reg:hasSubproperty <http://rdaregistry.info/Elements/m/P30174> ;
	reg:name "producersName"@en ;
	reg:status status:1001 ;
	a rdf:Property ;
	rdfs:isDefinedBy <http://rdaregistry.info/Elements/u/> ;
	rdfs:label "has producer's name"@en ;
	owl:sameAs <http://rdaregistry.info/Elements/u/producersName> ;
	skos:definition "Relates a resource to the name of an agent responsible for inscribing, fabricating, constructing, etc., a resource in an unpublished form."@en .

<http://rdaregistry.info/Elements/u/P60546> reg:hasSubproperty <http://rdaregistry.info/Elements/m/P30175> ;
	reg:name "manufacturersName"@en ;
	reg:status status:1001 ;
	a rdf:Property ;
	rdfs:isDefinedBy <http://rdaregistry.info/Elements/u/> ;
	rdfs:label "has manufacturer's name"@en ;
	owl:sameAs <http://rdaregistry.info/Elements/u/manufacturersName> ;
	skos:definition "Relates a resource to the name of an agent responsible for printing, duplicating, casting, etc., a resource in a published form."@en .

<http://rdaregistry.info/Elements/u/P60547> reg:hasSubproperty <http://rdaregistry.info/Elements/m/P30176> ;
	reg:name "publishersName"@en ;
	reg:status status:1001 ;
	a rdf:Property ;
	rdfs:isDefinedBy <http://rdaregistry.info/Elements/u/> ;
	rdfs:label "has publisher's name"@en ;
	owl:sameAs <http://rdaregistry.info/Elements/u/publishersName> ;
	skos:definition "Relates a resource to the name of an agent responsible for publishing, releasing, or issuing a resource."@en .

<http://rdaregistry.info/Elements/u/P60548> reg:name "preferredNameForThePlace"@en ;
	reg:status status:1001 ;
	a rdf:Property ;
	rdfs:isDefinedBy <http://rdaregistry.info/Elements/u/> ;
	rdfs:label "has preferred name for the place"@en ;
	rdfs:subPropertyOf <http://rdaregistry.info/Elements/u/P60366> ;
	owl:sameAs <http://rdaregistry.info/Elements/u/preferredNameForThePlace> ;
	skos:definition "Relates a resource to the name or form of name chosen to identify a place."@en .

<http://rdaregistry.info/Elements/u/P60549> reg:hasSubproperty <http://rdaregistry.info/Elements/a/P50041> , <http://rdaregistry.info/Elements/a/P50065> , <http://rdaregistry.info/Elements/a/P50117> ;
	reg:name "preferredNameForTheAgent"@en ;
	reg:status status:1001 ;
	a rdf:Property ;
	rdfs:isDefinedBy <http://rdaregistry.info/Elements/u/> ;
	rdfs:label "has preferred name for the agent"@en ;
	rdfs:subPropertyOf <http://rdaregistry.info/Elements/u/P60368> ;
	owl:sameAs <http://rdaregistry.info/Elements/u/preferredNameForTheAgent> ;
	skos:definition "Relates a resource to the name or form of name chosen to identify the agent. it is also the basis for the authorized access point representing that body."@en .

<http://rdaregistry.info/Elements/u/P60550> reg:hasSubproperty <http://rdaregistry.info/Elements/m/P30177> , <http://rdaregistry.info/Elements/m/P30178> , <http://rdaregistry.info/Elements/m/P30179> , <http://rdaregistry.info/Elements/m/P30180> , <http://rdaregistry.info/Elements/m/P30181> , <http://rdaregistry.info/Elements/m/P30182> ;
	reg:name "extent"@en ;
	reg:status status:1001 ;
	a rdf:Property ;
	rdfs:isDefinedBy <http://rdaregistry.info/Elements/u/> ;
	rdfs:label "has extent"@en ;
	owl:sameAs <http://rdaregistry.info/Elements/u/extent> ;
	skos:definition "Relates a resource to the number and type of units and/or subunits making up a resource."@en .

<http://rdaregistry.info/Elements/u/P60551> reg:hasSubproperty <http://rdaregistry.info/Elements/m/P30183> ;
	reg:name "fileSize"@en ;
	reg:status status:1001 ;
	a rdf:Property ;
	rdfs:isDefinedBy <http://rdaregistry.info/Elements/u/> ;
	rdfs:label "has file size"@en ;
	rdfs:subPropertyOf <http://rdaregistry.info/Elements/u/P60350> ;
	owl:sameAs <http://rdaregistry.info/Elements/u/fileSize> ;
	skos:definition "Relates a resource to the number of bytes in a digital file."@en .

<http://rdaregistry.info/Elements/u/P60552> reg:hasSubproperty <http://rdaregistry.info/Elements/m/P30184> ;
	reg:name "configurationOfPlaybackChannels"@en ;
	reg:status status:1001 ;
	a rdf:Property ;
	rdfs:isDefinedBy <http://rdaregistry.info/Elements/u/> ;
	rdfs:label "has configuration of playback channels"@en ;
	rdfs:subPropertyOf <http://rdaregistry.info/Elements/u/P60351> ;
	owl:sameAs <http://rdaregistry.info/Elements/u/configurationOfPlaybackChannels> ;
	skos:definition "Relates a resource to the number of sound channels used to make a recording (e.g., one channel for a monophonic recording, two channels for a stereophonic recording)."@en .

<http://rdaregistry.info/Elements/u/P60553> reg:hasSubproperty <http://rdaregistry.info/Elements/m/P30185> ;
	reg:name "tapeConfiguration"@en ;
	reg:status status:1001 ;
	a rdf:Property ;
	rdfs:isDefinedBy <http://rdaregistry.info/Elements/u/> ;
	rdfs:label "has tape configuration"@en ;
	rdfs:subPropertyOf <http://rdaregistry.info/Elements/u/P60351> ;
	owl:sameAs <http://rdaregistry.info/Elements/u/tapeConfiguration> ;
	skos:definition "Relates a resource to the number of tracks on an audiotape."@en .

<http://rdaregistry.info/Elements/u/P60554> reg:hasSubproperty <http://rdaregistry.info/Elements/m/P30186> ;
	reg:name "mount"@en ;
	reg:status status:1001 ;
	a rdf:Property ;
	rdfs:isDefinedBy <http://rdaregistry.info/Elements/u/> ;
	rdfs:label "has mount"@en ;
	owl:sameAs <http://rdaregistry.info/Elements/u/mount> ;
	skos:definition "Relates a resource to the physical material used for the support or backing to which the base material of a resource has been attached."@en .

<http://rdaregistry.info/Elements/u/P60555> reg:hasSubproperty <http://rdaregistry.info/Elements/e/P20217> ;
	reg:name "placeAndDateOfCapture"@en ;
	reg:status status:1001 ;
	a rdf:Property ;
	rdfs:isDefinedBy <http://rdaregistry.info/Elements/u/> ;
	rdfs:label "has place and date of capture"@en ;
	owl:sameAs <http://rdaregistry.info/Elements/u/placeAndDateOfCapture> ;
	skos:definition "Relates a resource to the place and date associated with the capture (i.e., recording, filming, etc.) of the content of a resource."@en .

<http://rdaregistry.info/Elements/u/P60556> reg:hasSubproperty <http://rdaregistry.info/Elements/e/P20218> ;
	reg:name "placeOfCapture"@en ;
	reg:status status:1001 ;
	a rdf:Property ;
	rdfs:isDefinedBy <http://rdaregistry.info/Elements/u/> ;
	rdfs:label "has place of capture"@en ;
	owl:sameAs <http://rdaregistry.info/Elements/u/placeOfCapture> ;
	skos:definition "Relates a resource to the place associated with the capture (i.e., recording, filming, etc.) of the content of a resource."@en .

<http://rdaregistry.info/Elements/u/P60557> reg:hasSubproperty <http://rdaregistry.info/Elements/e/P20219> ;
	reg:name "duration"@en ;
	reg:status status:1001 ;
	a rdf:Property ;
	rdfs:isDefinedBy <http://rdaregistry.info/Elements/u/> ;
	rdfs:label "has duration"@en ;
	owl:sameAs <http://rdaregistry.info/Elements/u/duration> ;
	skos:definition "Relates a resource to the playing time, running time, etc., of the content of a resource."@en .

<http://rdaregistry.info/Elements/u/P60558> reg:hasSubproperty <http://rdaregistry.info/Elements/e/P20220> , <http://rdaregistry.info/Elements/e/P20221> , <http://rdaregistry.info/Elements/e/P20222> , <http://rdaregistry.info/Elements/e/P20223> , <http://rdaregistry.info/Elements/e/P20224> ;
	reg:name "colourContent"@en ;
	reg:status status:1001 ;
	a rdf:Property ;
	rdfs:isDefinedBy <http://rdaregistry.info/Elements/u/> ;
	rdfs:label "has colour content"@en ;
	owl:sameAs <http://rdaregistry.info/Elements/u/colourContent> ;
	skos:definition "Relates a resource to the presence of colour, tone, etc., in the content of a resource. colour content is also the specific colours, tones, etc., (including black and white) present in the content of a resource."@en .

<http://rdaregistry.info/Elements/u/P60559> reg:hasSubproperty <http://rdaregistry.info/Elements/e/P20225> ;
	reg:name "soundContent"@en ;
	reg:status status:1001 ;
	a rdf:Property ;
	rdfs:isDefinedBy <http://rdaregistry.info/Elements/u/> ;
	rdfs:label "has sound content"@en ;
	owl:sameAs <http://rdaregistry.info/Elements/u/soundContent> ;
	skos:definition "Relates a resource to the presence of sound in a resource other than one that consists primarily of recorded sound."@en .

<http://rdaregistry.info/Elements/u/P60560> reg:hasSubproperty <http://rdaregistry.info/Elements/m/P30187> , <http://rdaregistry.info/Elements/u/P60561> , <http://rdaregistry.info/Elements/u/P60562> ;
	reg:name "productionMethod"@en ;
	reg:status status:1001 ;
	a rdf:Property ;
	rdfs:isDefinedBy <http://rdaregistry.info/Elements/u/> ;
	rdfs:label "has production method"@en ;
	owl:sameAs <http://rdaregistry.info/Elements/u/productionMethod> ;
	skos:definition "Relates a resource to the process used to produce a resource."@en .

<http://rdaregistry.info/Elements/u/P60561> reg:hasSubproperty <http://rdaregistry.info/Elements/m/P30188> ;
	reg:name "productionMethodForTactileResource"@en ;
	reg:status status:1001 ;
	a rdf:Property ;
	rdfs:isDefinedBy <http://rdaregistry.info/Elements/u/> ;
	rdfs:label "has production method for tactile resource"@en ;
	rdfs:subPropertyOf <http://rdaregistry.info/Elements/u/P60560> ;
	owl:sameAs <http://rdaregistry.info/Elements/u/productionMethodForTactileResource> ;
	skos:definition "Relates a resource to the process used to produce a tactile resource (e.g., embossing, thermoform)."@en .

<http://rdaregistry.info/Elements/u/P60562> reg:name "productionMethodForManuscript"@en ;
	reg:status status:1001 ;
	a rdf:Property ;
	rdfs:isDefinedBy <http://rdaregistry.info/Elements/u/> ;
	rdfs:label "has production method for manuscript"@en ;
	rdfs:subPropertyOf <http://rdaregistry.info/Elements/u/P60560> ;
	owl:sameAs <http://rdaregistry.info/Elements/u/productionMethodForManuscript> ;
	skos:definition "Relates a resource to the process used to produce an original manuscript or a copy."@en .

<http://rdaregistry.info/Elements/u/P60563> reg:hasSubproperty <http://rdaregistry.info/Elements/e/P20226> ;
	reg:name "horizontalScaleOfCartographicContent"@en ;
	reg:status status:1001 ;
	a rdf:Property ;
	rdfs:isDefinedBy <http://rdaregistry.info/Elements/u/> ;
	rdfs:label "has horizontal scale of cartographic content"@en ;
	rdfs:subPropertyOf <http://rdaregistry.info/Elements/u/P60565> ;
	owl:sameAs <http://rdaregistry.info/Elements/u/horizontalScaleOfCartographicContent> ;
	skos:definition "Relates a resource to the ratio of horizontal distances in the cartographic content of a resource to the actual distances they represent."@en .

<http://rdaregistry.info/Elements/u/P60564> reg:hasSubproperty <http://rdaregistry.info/Elements/e/P20227> ;
	reg:name "scaleOfStillImageOrThreeDimensionalForm"@en ;
	reg:status status:1001 ;
	a rdf:Property ;
	rdfs:isDefinedBy <http://rdaregistry.info/Elements/u/> ;
	rdfs:label "has scale of still image or three-dimensional form"@en ;
	rdfs:subPropertyOf <http://rdaregistry.info/Elements/u/P60565> ;
	owl:sameAs <http://rdaregistry.info/Elements/u/scaleOfStillImageOrThreeDimensionalForm> ;
	skos:definition "Relates a resource to the ratio of the dimensions of a still image or three-dimensional form contained or embodied in a resource to the dimensions of the entity it represents."@en .

<http://rdaregistry.info/Elements/u/P60565> reg:hasSubproperty <http://rdaregistry.info/Elements/e/P20228> , <http://rdaregistry.info/Elements/u/P60510> , <http://rdaregistry.info/Elements/u/P60563> , <http://rdaregistry.info/Elements/u/P60564> , <http://rdaregistry.info/Elements/u/P60579> ;
	reg:name "scale"@en ;
	reg:status status:1001 ;
	a rdf:Property ;
	rdfs:isDefinedBy <http://rdaregistry.info/Elements/u/> ;
	rdfs:label "has scale"@en ;
	owl:sameAs <http://rdaregistry.info/Elements/u/scale> ;
	skos:definition "Relates a resource to the ratio of the dimensions of an image or three-dimensional form contained or embodied in a resource to the dimensions of the entity it represents."@en .

<http://rdaregistry.info/Elements/u/P60566> reg:hasSubproperty <http://rdaregistry.info/Elements/e/P20229> ;
	reg:name "aspectRatio"@en ;
	reg:status status:1001 ;
	a rdf:Property ;
	rdfs:isDefinedBy <http://rdaregistry.info/Elements/u/> ;
	rdfs:label "has aspect ratio"@en ;
	owl:sameAs <http://rdaregistry.info/Elements/u/aspectRatio> ;
	skos:definition "Relates a resource to the ratio of the width to the height of a moving image."@en .

<http://rdaregistry.info/Elements/u/P60567> reg:hasSubproperty <http://rdaregistry.info/Elements/m/P30190> ;
	reg:name "generationOfAudioRecording"@en ;
	reg:status status:1001 ;
	a rdf:Property ;
	rdfs:isDefinedBy <http://rdaregistry.info/Elements/u/> ;
	rdfs:label "has generation of audio recording"@en ;
	rdfs:subPropertyOf <http://rdaregistry.info/Elements/u/P60568> ;
	owl:sameAs <http://rdaregistry.info/Elements/u/generationOfAudioRecording> ;
	skos:definition "Relates a resource to the relationship between an original audio carrier and the carrier of a reproduction made from the original (e.g., a tape duplication master, a test pressing)."@en .

<http://rdaregistry.info/Elements/u/P60568> reg:hasSubproperty <http://rdaregistry.info/Elements/m/P30191> , <http://rdaregistry.info/Elements/u/P60567> , <http://rdaregistry.info/Elements/u/P60569> , <http://rdaregistry.info/Elements/u/P60570> , <http://rdaregistry.info/Elements/u/P60571> , <http://rdaregistry.info/Elements/u/P60572> ;
	reg:name "generation"@en ;
	reg:status status:1001 ;
	a rdf:Property ;
	rdfs:isDefinedBy <http://rdaregistry.info/Elements/u/> ;
	rdfs:label "has generation"@en ;
	owl:sameAs <http://rdaregistry.info/Elements/u/generation> ;
	skos:definition "Relates a resource to the relationship between an original carrier and the carrier of a reproduction made from the original (e.g., a first generation camera master, a second generation printing master)."@en .

<http://rdaregistry.info/Elements/u/P60569> reg:hasSubproperty <http://rdaregistry.info/Elements/m/P30192> ;
	reg:name "generationOfDigitalResource"@en ;
	reg:status status:1001 ;
	a rdf:Property ;
	rdfs:isDefinedBy <http://rdaregistry.info/Elements/u/> ;
	rdfs:label "has generation of digital resource"@en ;
	rdfs:subPropertyOf <http://rdaregistry.info/Elements/u/P60568> ;
	owl:sameAs <http://rdaregistry.info/Elements/u/generationOfDigitalResource> ;
	skos:definition "Relates a resource to the relationship between an original carrier of a digital resource and the carrier of a reproduction made from the original (e.g., a derivative master)."@en .

<http://rdaregistry.info/Elements/u/P60570> reg:hasSubproperty <http://rdaregistry.info/Elements/m/P30193> ;
	reg:name "generationOfMotionPictureFilm"@en ;
	reg:status status:1001 ;
	a rdf:Property ;
	rdfs:isDefinedBy <http://rdaregistry.info/Elements/u/> ;
	rdfs:label "has generation of motion picture film"@en ;
	rdfs:subPropertyOf <http://rdaregistry.info/Elements/u/P60568> ;
	owl:sameAs <http://rdaregistry.info/Elements/u/generationOfMotionPictureFilm> ;
	skos:definition "Relates a resource to the relationship between an original carrier of a motion picture film resource and the carrier of a reproduction made from the original (e.g., a reference print)."@en .

<http://rdaregistry.info/Elements/u/P60571> reg:hasSubproperty <http://rdaregistry.info/Elements/m/P30194> ;
	reg:name "generationOfVideotape"@en ;
	reg:status status:1001 ;
	a rdf:Property ;
	rdfs:isDefinedBy <http://rdaregistry.info/Elements/u/> ;
	rdfs:label "has generation of videotape"@en ;
	rdfs:subPropertyOf <http://rdaregistry.info/Elements/u/P60568> ;
	owl:sameAs <http://rdaregistry.info/Elements/u/generationOfVideotape> ;
	skos:definition "Relates a resource to the relationship between an original carrier of a videotape resource and the carrier of a reproduction made from the original (e.g., a show copy)."@en .

<http://rdaregistry.info/Elements/u/P60572> reg:hasSubproperty <http://rdaregistry.info/Elements/m/P30195> ;
	reg:name "generationOfMicroform"@en ;
	reg:status status:1001 ;
	a rdf:Property ;
	rdfs:isDefinedBy <http://rdaregistry.info/Elements/u/> ;
	rdfs:label "has generation of microform"@en ;
	rdfs:subPropertyOf <http://rdaregistry.info/Elements/u/P60568> ;
	owl:sameAs <http://rdaregistry.info/Elements/u/generationOfMicroform> ;
	skos:definition "Relates a resource to the relationship between an original microform carrier and the carrier of a reproduction made from the original (e.g., a printing master)."@en .

<http://rdaregistry.info/Elements/u/P60573> reg:hasSubproperty <http://rdaregistry.info/Elements/m/P30196> ;
	reg:name "polarity"@en ;
	reg:status status:1001 ;
	a rdf:Property ;
	rdfs:isDefinedBy <http://rdaregistry.info/Elements/u/> ;
	rdfs:label "has polarity"@en ;
	owl:sameAs <http://rdaregistry.info/Elements/u/polarity> ;
	skos:definition "Relates a resource to the relationship of the colours and tones in an image to the colours and tones of the object reproduced (e.g., positive, negative)."@en .

<http://rdaregistry.info/Elements/u/P60574> reg:hasSubproperty <http://rdaregistry.info/Elements/e/P20137> , <http://rdaregistry.info/Elements/w/P10224> ;
	reg:name "absorptionOf"@en ;
	reg:status status:1001 ;
	a rdf:Property ;
	rdfs:isDefinedBy <http://rdaregistry.info/Elements/u/> ;
	rdfs:label "is absorption of"@en ;
	rdfs:subPropertyOf <http://rdaregistry.info/Elements/u/P60261> ;
	owl:inverseOf <http://rdaregistry.info/Elements/u/P60247> ;
	owl:sameAs <http://rdaregistry.info/Elements/u/absorbed> , <http://rdaregistry.info/Elements/u/absorptionOf> ;
	skos:definition "Relates a resource to the resource that has been incorporated into another resource."@en .

<http://rdaregistry.info/Elements/u/P60575> reg:hasSubproperty <http://rdaregistry.info/Elements/e/P20138> , <http://rdaregistry.info/Elements/w/P10225> ;
	reg:name "absorptionInPartOf"@en ;
	reg:status status:1001 ;
	a rdf:Property ;
	rdfs:isDefinedBy <http://rdaregistry.info/Elements/u/> ;
	rdfs:label "is absorption in part of"@en ;
	rdfs:subPropertyOf <http://rdaregistry.info/Elements/u/P60261> ;
	owl:inverseOf <http://rdaregistry.info/Elements/u/P60248> ;
	owl:sameAs <http://rdaregistry.info/Elements/u/absorbedInPart> , <http://rdaregistry.info/Elements/u/absorptionInPartOf> ;
	skos:definition "Relates a resource to the resource that has been partially incorporated into another resource."@en .

<http://rdaregistry.info/Elements/u/P60576> reg:hasSubproperty <http://rdaregistry.info/Elements/e/P20149> , <http://rdaregistry.info/Elements/w/P10226> ;
	reg:name "continuationOf"@en ;
	reg:status status:1001 ;
	a rdf:Property ;
	rdfs:isDefinedBy <http://rdaregistry.info/Elements/u/> ;
	rdfs:label "is continuation of"@en ;
	rdfs:subPropertyOf <http://rdaregistry.info/Elements/u/P60261> ;
	owl:inverseOf <http://rdaregistry.info/Elements/u/P60306> ;
	owl:sameAs <http://rdaregistry.info/Elements/u/continuationOf> , <http://rdaregistry.info/Elements/u/continues> ;
	skos:definition "Relates a resource to the resource that is continued by the content of a later resource."@en .

<http://rdaregistry.info/Elements/u/P60577> reg:hasSubproperty <http://rdaregistry.info/Elements/w/P10227> ;
	reg:name "sequelTo"@en ;
	reg:status status:1001 ;
	a rdf:Property ;
	rdfs:isDefinedBy <http://rdaregistry.info/Elements/u/> ;
	rdfs:label "is sequel to"@en ;
	rdfs:subPropertyOf <http://rdaregistry.info/Elements/u/P60261> ;
	owl:inverseOf <http://rdaregistry.info/Elements/u/P60102> ;
	owl:sameAs <http://rdaregistry.info/Elements/u/sequelTo> ;
	skos:definition "Relates a resource to the resource whose narrative is continued by the later resource."@en .

<http://rdaregistry.info/Elements/u/P60578> reg:hasSubproperty <http://rdaregistry.info/Elements/m/P30197> ;
	reg:name "bookFormat"@en ;
	reg:status status:1001 ;
	a rdf:Property ;
	rdfs:isDefinedBy <http://rdaregistry.info/Elements/u/> ;
	rdfs:label "has book format"@en ;
	owl:sameAs <http://rdaregistry.info/Elements/u/bookFormat> ;
	skos:definition "Relates a resource to the result of folding a printed sheet to form a gathering of leaves (e.g., a sheet folded once to form a folio, twice to form a quarto, three times to form an octavo, etc.)."@en .

<http://rdaregistry.info/Elements/u/P60579> reg:hasSubproperty <http://rdaregistry.info/Elements/e/P20230> ;
	reg:name "verticalScaleOfCartographicContent"@en ;
	reg:status status:1001 ;
	a rdf:Property ;
	rdfs:isDefinedBy <http://rdaregistry.info/Elements/u/> ;
	rdfs:label "has vertical scale of cartographic content"@en ;
	rdfs:subPropertyOf <http://rdaregistry.info/Elements/u/P60565> ;
	owl:sameAs <http://rdaregistry.info/Elements/u/verticalScaleOfCartographicContent> ;
	skos:definition "Relates a resource to the scale of elevation or vertical dimension of the cartographic content of a resource."@en .

<http://rdaregistry.info/Elements/u/P60580> reg:hasSubproperty <http://rdaregistry.info/Elements/w/P10221> ;
	reg:name "key"@en ;
	reg:status status:1001 ;
	a rdf:Property ;
	rdfs:isDefinedBy <http://rdaregistry.info/Elements/u/> ;
	rdfs:label "has key"@en ;
	owl:sameAs <http://rdaregistry.info/Elements/u/key> ;
	skos:definition "Relates a resource to the set of pitch relationships that establishes the tonal centre, or principal tonal centre, of a musical resource."@en .

<http://rdaregistry.info/Elements/u/P60581> reg:hasSubproperty <http://rdaregistry.info/Elements/m/P30198> ;
	reg:name "reductionRatio"@en ;
	reg:status status:1001 ;
	a rdf:Property ;
	rdfs:isDefinedBy <http://rdaregistry.info/Elements/u/> ;
	rdfs:label "has reduction ratio"@en ;
	owl:sameAs <http://rdaregistry.info/Elements/u/reductionRatio> ;
	skos:definition "Relates a resource to the size of a micro-image in relation to the original from which it was produced."@en .

<http://rdaregistry.info/Elements/u/P60582> reg:hasSubproperty <http://rdaregistry.info/Elements/m/P30199> ;
	reg:name "fontSize"@en ;
	reg:status status:1001 ;
	a rdf:Property ;
	rdfs:isDefinedBy <http://rdaregistry.info/Elements/u/> ;
	rdfs:label "has font size"@en ;
	owl:sameAs <http://rdaregistry.info/Elements/u/fontSize> ;
	skos:definition "Relates a resource to the size of the type used to represent the characters and symbols in a resource."@en .

<http://rdaregistry.info/Elements/u/P60583> reg:hasSubproperty <http://rdaregistry.info/Elements/i/P40050> ;
	reg:name "immediateSourceOfAcquisitionOfItem"@en ;
	reg:status status:1001 ;
	a rdf:Property ;
	rdfs:isDefinedBy <http://rdaregistry.info/Elements/u/> ;
	rdfs:label "has immediate source of acquisition of resource"@en ;
	owl:sameAs <http://rdaregistry.info/Elements/u/immediateSourceOfAcquisitionOfItem> ;
	skos:definition "Relates a resource to the source from which the agency directly acquired a resource and the circumstances under which it was received."@en .

<http://rdaregistry.info/Elements/u/P60584> reg:hasSubproperty <http://rdaregistry.info/Elements/w/P10222> ;
	reg:name "natureOfTheContent"@en ;
	reg:status status:1001 ;
	a rdf:Property ;
	rdfs:isDefinedBy <http://rdaregistry.info/Elements/u/> ;
	rdfs:label "has nature of the content"@en ;
	owl:sameAs <http://rdaregistry.info/Elements/u/natureOfTheContent> ;
	skos:definition "Relates a resource to the specific character of the primary content of a resource (e.g., legal articles, interim report)."@en .

<http://rdaregistry.info/Elements/u/P60585> reg:hasSubproperty <http://rdaregistry.info/Elements/m/P30200> ;
	reg:name "projectionSpeed"@en ;
	reg:status status:1001 ;
	a rdf:Property ;
	rdfs:isDefinedBy <http://rdaregistry.info/Elements/u/> ;
	rdfs:label "has projection speed"@en ;
	rdfs:subPropertyOf <http://rdaregistry.info/Elements/u/P60353> ;
	owl:sameAs <http://rdaregistry.info/Elements/u/projectionSpeed> ;
	skos:definition "Relates a resource to the speed at which a projected carrier must be operated to produce the moving image intended."@en .

<http://rdaregistry.info/Elements/u/P60586> reg:hasSubproperty <http://rdaregistry.info/Elements/m/P30201> ;
	reg:name "playingSpeed"@en ;
	reg:status status:1001 ;
	a rdf:Property ;
	rdfs:isDefinedBy <http://rdaregistry.info/Elements/u/> ;
	rdfs:label "has playing speed"@en ;
	rdfs:subPropertyOf <http://rdaregistry.info/Elements/u/P60351> ;
	owl:sameAs <http://rdaregistry.info/Elements/u/playingSpeed> ;
	skos:definition "Relates a resource to the speed at which an audio carrier must be operated to produce the sound intended."@en .

<http://rdaregistry.info/Elements/u/P60587> reg:hasSubproperty <http://rdaregistry.info/Elements/m/P30202> ;
	reg:name "encodedBitrate"@en ;
	reg:status status:1001 ;
	a rdf:Property ;
	rdfs:isDefinedBy <http://rdaregistry.info/Elements/u/> ;
	rdfs:label "has encoded bitrate"@en ;
	rdfs:subPropertyOf <http://rdaregistry.info/Elements/u/P60350> ;
	owl:sameAs <http://rdaregistry.info/Elements/u/encodedBitrate> ;
	skos:definition "Relates a resource to the speed at which streaming audio, video, etc., is designed to play."@en .

<http://rdaregistry.info/Elements/u/P60588> reg:hasSubproperty <http://rdaregistry.info/Elements/w/P10223> ;
	reg:name "preferredTitleForTheResource"@en ;
	reg:status status:1001 ;
	a rdf:Property ;
	rdfs:isDefinedBy <http://rdaregistry.info/Elements/u/> ;
	rdfs:label "has preferred title for the resource"@en ;
	rdfs:subPropertyOf <http://rdaregistry.info/Elements/u/P60367> ;
	owl:sameAs <http://rdaregistry.info/Elements/u/preferredTitleForTheResource> ;
	skos:definition "Relates a resource to the title or form of title chosen to identify the resource."@en .

<http://rdaregistry.info/Elements/u/P60589> reg:hasSubproperty <http://rdaregistry.info/Elements/m/P30203> ;
	reg:name "parallelTitleProper"@en ;
	reg:status status:1001 ;
	a rdf:Property ;
	rdfs:isDefinedBy <http://rdaregistry.info/Elements/u/> ;
	rdfs:label "has parallel title proper"@en ;
	rdfs:subPropertyOf <http://rdaregistry.info/Elements/u/P60369> ;
	owl:sameAs <http://rdaregistry.info/Elements/u/parallelTitleProper> ;
	skos:definition "Relates a resource to the title proper in another language and/or script."@en .

<http://rdaregistry.info/Elements/u/P60590> reg:hasSubproperty <http://rdaregistry.info/Elements/m/P30204> ;
	reg:name "parallelTitleProperOfSeries"@en ;
	reg:status status:1001 ;
	a rdf:Property ;
	rdfs:isDefinedBy <http://rdaregistry.info/Elements/u/> ;
	rdfs:label "has parallel title proper of series"@en ;
	owl:sameAs <http://rdaregistry.info/Elements/u/parallelTitleProperOfSeries> ;
	skos:definition "Relates a resource to the title proper of a series in another language and/or script."@en .

<http://rdaregistry.info/Elements/u/P60591> reg:hasSubproperty <http://rdaregistry.info/Elements/m/P30205> ;
	reg:name "parallelTitleProperOfSubseries"@en ;
	reg:status status:1001 ;
	a rdf:Property ;
	rdfs:isDefinedBy <http://rdaregistry.info/Elements/u/> ;
	rdfs:label "has parallel title proper of subseries"@en ;
	owl:sameAs <http://rdaregistry.info/Elements/u/parallelTitleProperOfSubseries> ;
	skos:definition "Relates a resource to the title proper of a subseries in another language and/or script."@en .

<http://rdaregistry.info/Elements/u/P60592> reg:hasSubproperty <http://rdaregistry.info/Elements/a/P50118> ;
	reg:name "placeOfDeath"@en ;
	reg:status status:1001 ;
	a rdf:Property ;
	rdfs:isDefinedBy <http://rdaregistry.info/Elements/u/> ;
	rdfs:label "has place of death"@en ;
	owl:sameAs <http://rdaregistry.info/Elements/u/placeOfDeath> ;
	skos:definition "Relates a resource to the town, city, province, state, and/or country in which an agent died."@en .

<http://rdaregistry.info/Elements/u/P60593> reg:hasSubproperty <http://rdaregistry.info/Elements/a/P50119> ;
	reg:name "placeOfBirth"@en ;
	reg:status status:1001 ;
	a rdf:Property ;
	rdfs:isDefinedBy <http://rdaregistry.info/Elements/u/> ;
	rdfs:label "has place of birth"@en ;
	owl:sameAs <http://rdaregistry.info/Elements/u/placeOfBirth> ;
	skos:definition "Relates a resource to the town, city, province, state, and/or country in which an agent was born."@en .

<http://rdaregistry.info/Elements/u/P60594> reg:hasSubproperty <http://rdaregistry.info/Elements/m/P30206> ;
	reg:name "recordingMedium"@en ;
	reg:status status:1001 ;
	a rdf:Property ;
	rdfs:isDefinedBy <http://rdaregistry.info/Elements/u/> ;
	rdfs:label "has recording medium"@en ;
	rdfs:subPropertyOf <http://rdaregistry.info/Elements/u/P60351> ;
	owl:sameAs <http://rdaregistry.info/Elements/u/recordingMedium> ;
	skos:definition "Relates a resource to the type of medium used to record sound on an audio carrier (e.g., magnetic, optical)."@en .

<http://rdaregistry.info/Elements/u/P60595> reg:hasSubproperty <http://rdaregistry.info/Elements/m/P30207> ;
	reg:name "baseMaterialForMicrofilmMicrofichePhotographicFilmAndMotionPictureFilm"@en ;
	reg:status status:1001 ;
	a rdf:Property ;
	rdfs:isDefinedBy <http://rdaregistry.info/Elements/u/> ;
	rdfs:label "has base material for microfilm, microfiche, photographic film, and motion picture film"@en ;
	rdfs:subPropertyOf <http://rdaregistry.info/Elements/u/P60596> ;
	owl:sameAs <http://rdaregistry.info/Elements/u/baseMaterialForMicrofilmMicrofichePhotographicFilmAndMotionPictureFilm> ;
	skos:definition "Relates a resource to the underlying physical material of a microfilm, microfiche, photographic film, or motion picture film resource."@en .

<http://rdaregistry.info/Elements/u/P60596> reg:hasSubproperty <http://rdaregistry.info/Elements/m/P30208> , <http://rdaregistry.info/Elements/u/P60595> ;
	reg:name "baseMaterial"@en ;
	reg:status status:1001 ;
	a rdf:Property ;
	rdfs:isDefinedBy <http://rdaregistry.info/Elements/u/> ;
	rdfs:label "has base material"@en ;
	owl:sameAs <http://rdaregistry.info/Elements/u/baseMaterial> ;
	skos:definition "Relates a resource to the underlying physical material of a resource."@en .

<http://rdaregistry.info/Elements/u/P60597> reg:hasSubproperty <http://rdaregistry.info/Elements/m/P30209> ;
	reg:name "keyTitle"@en ;
	reg:status status:1001 ;
	a rdf:Property ;
	rdfs:isDefinedBy <http://rdaregistry.info/Elements/u/> ;
	rdfs:label "has key title"@en ;
	rdfs:subPropertyOf <http://rdaregistry.info/Elements/u/P60369> ;
	owl:sameAs <http://rdaregistry.info/Elements/u/keyTitle> ;
	skos:definition "Relates a resource to the unique name assigned to a resource by an issn registration agency."@en .

<http://rdaregistry.info/Elements/u/P60598> reg:hasSubproperty <http://rdaregistry.info/Elements/a/P50120> ;
	reg:name "dateOfDeath"@en ;
	reg:status status:1001 ;
	a rdf:Property ;
	rdfs:isDefinedBy <http://rdaregistry.info/Elements/u/> ;
	rdfs:label "has date of death"@en ;
	rdfs:subPropertyOf <http://rdaregistry.info/Elements/u/P60324> ;
	owl:sameAs <http://rdaregistry.info/Elements/u/dateOfDeath> ;
	skos:definition "Relates a resource to the year an agent died."@en .

<http://rdaregistry.info/Elements/u/P60599> reg:hasSubproperty <http://rdaregistry.info/Elements/a/P50121> ;
	reg:name "dateOfBirth"@en ;
	reg:status status:1001 ;
	a rdf:Property ;
	rdfs:isDefinedBy <http://rdaregistry.info/Elements/u/> ;
	rdfs:label "has date of birth"@en ;
	rdfs:subPropertyOf <http://rdaregistry.info/Elements/u/P60324> ;
	owl:sameAs <http://rdaregistry.info/Elements/u/dateOfBirth> ;
	skos:definition "Relates a resource to the year an agent was born."@en .

<http://rdaregistry.info/Elements/u/P60600> reg:hasSubproperty <http://rdaregistry.info/Elements/a/P50216> ;
	reg:name "writerOfAddedLyricsOf"@en ;
	reg:status status:1001 ;
	a rdf:Property ;
	rdfs:isDefinedBy <http://rdaregistry.info/Elements/u/> ;
	rdfs:label "is writer of added lyrics of"@en ;
	rdfs:subPropertyOf <http://rdaregistry.info/Elements/u/P60608> ;
	owl:inverseOf <http://rdaregistry.info/Elements/u/P60371> ;
	owl:sameAs <http://rdaregistry.info/Elements/u/writerOfAddedLyricsOf> ;
	skos:definition "Relates a writer of words added to a musical resource to the resource."@en .

<http://rdaregistry.info/Elements/u/P60601> reg:hasSubproperty <http://rdaregistry.info/Elements/a/P50085> , <http://rdaregistry.info/Elements/a/P50087> ;
	reg:name "appelleeOf"@en ;
	reg:status status:1001 ;
	a rdf:Property ;
	rdfs:isDefinedBy <http://rdaregistry.info/Elements/u/> ;
	rdfs:label "is appellee of"@en ;
	rdfs:subPropertyOf <http://rdaregistry.info/Elements/u/P60602> ;
	owl:inverseOf <http://rdaregistry.info/Elements/u/P60373> ;
	owl:sameAs <http://rdaregistry.info/Elements/u/appelleeOf> ;
	skos:definition "Relates an agent against whom an appeal is taken to the resource."@en .

<http://rdaregistry.info/Elements/u/P60602> reg:hasSubproperty <http://rdaregistry.info/Elements/u/P60002> , <http://rdaregistry.info/Elements/u/P60003> , <http://rdaregistry.info/Elements/u/P60004> , <http://rdaregistry.info/Elements/u/P60005> , <http://rdaregistry.info/Elements/u/P60015> , <http://rdaregistry.info/Elements/u/P60032> , <http://rdaregistry.info/Elements/u/P60601> , <http://rdaregistry.info/Elements/u/P60603> , <http://rdaregistry.info/Elements/u/P60604> , <http://rdaregistry.info/Elements/u/P60634> , <http://rdaregistry.info/Elements/u/P60650> , <http://rdaregistry.info/Elements/u/P60668> , <http://rdaregistry.info/Elements/u/P60673> , <http://rdaregistry.info/Elements/u/P60674> , <http://rdaregistry.info/Elements/u/P60675> , <http://rdaregistry.info/Elements/u/P60678> , <http://rdaregistry.info/Elements/u/P60689> , <http://rdaregistry.info/Elements/u/P60690> , <http://rdaregistry.info/Elements/u/P60691> , <http://rdaregistry.info/Elements/u/P60692> , <http://rdaregistry.info/Elements/u/P60693> , <http://rdaregistry.info/Elements/u/P60695> , <http://rdaregistry.info/Elements/u/P60696> , <http://rdaregistry.info/Elements/u/P60698> , <http://rdaregistry.info/Elements/u/P60700> , <http://rdaregistry.info/Elements/u/P60702> , <http://rdaregistry.info/Elements/u/P60703> ;
	reg:name "otherAgentAssociatedWithAResourceOf"@en ;
	reg:status status:1001 ;
	a rdf:Property ;
	rdfs:isDefinedBy <http://rdaregistry.info/Elements/u/> ;
	rdfs:label "is other agent associated with a resource of"@en ;
	owl:inverseOf <http://rdaregistry.info/Elements/u/P60374> ;
	owl:sameAs <http://rdaregistry.info/Elements/u/otherAgentAssociatedWithAResourceOf> , <http://rdaregistry.info/Elements/u/otherPFCResourceOf> ;
	skos:definition "Relates an agent associated with a resource other than as a creator to the resource."@en .

<http://rdaregistry.info/Elements/u/P60603> reg:hasSubproperty <http://rdaregistry.info/Elements/a/P50132> ;
	reg:name "dedicatorOf"@en ;
	reg:status status:1001 ;
	a rdf:Property ;
	rdfs:isDefinedBy <http://rdaregistry.info/Elements/u/> ;
	rdfs:label "is dedicator of"@en ;
	rdfs:subPropertyOf <http://rdaregistry.info/Elements/u/P60602> ;
	owl:inverseOf <http://rdaregistry.info/Elements/u/P60375> ;
	owl:sameAs <http://rdaregistry.info/Elements/u/dedicatorOf> ;
	skos:definition "Relates an agent by whom a resource is dedicated to the resource."@en .

<http://rdaregistry.info/Elements/u/P60604> reg:hasSubproperty <http://rdaregistry.info/Elements/a/P50133> , <http://rdaregistry.info/Elements/u/P60006> , <http://rdaregistry.info/Elements/u/P60007> ;
	reg:name "curatorOf"@en ;
	reg:status status:1001 ;
	a rdf:Property ;
	rdfs:isDefinedBy <http://rdaregistry.info/Elements/u/> ;
	rdfs:label "is curator of"@en ;
	rdfs:subPropertyOf <http://rdaregistry.info/Elements/u/P60602> ;
	owl:inverseOf <http://rdaregistry.info/Elements/u/P60376> ;
	owl:sameAs <http://rdaregistry.info/Elements/u/curatorOf> ;
	skos:definition "Relates an agent conceiving, aggregating, and/or organizing an exhibition, collection, or other resource to the resource."@en .

<http://rdaregistry.info/Elements/u/P60605> reg:hasSubproperty <http://rdaregistry.info/Elements/a/P50135> ;
	reg:name "surveyorOf"@en ;
	reg:status status:1001 ;
	a rdf:Property ;
	rdfs:isDefinedBy <http://rdaregistry.info/Elements/u/> ;
	rdfs:label "is surveyor of"@en ;
	rdfs:subPropertyOf <http://rdaregistry.info/Elements/u/P60626> ;
	owl:inverseOf <http://rdaregistry.info/Elements/u/P60377> ;
	owl:sameAs <http://rdaregistry.info/Elements/u/surveyorOf> ;
	skos:definition "Relates an agent contributing to a cartographic resource by providing measurements or dimensional relationships for the geographic area represented to the resource."@en .

<http://rdaregistry.info/Elements/u/P60606> reg:hasSubproperty <http://rdaregistry.info/Elements/a/P50136> ;
	reg:name "animatorOf"@en ;
	reg:status status:1001 ;
	a rdf:Property ;
	rdfs:isDefinedBy <http://rdaregistry.info/Elements/u/> ;
	rdfs:label "is animator of"@en ;
	rdfs:subPropertyOf <http://rdaregistry.info/Elements/u/P60626> ;
	owl:inverseOf <http://rdaregistry.info/Elements/u/P60378> ;
	owl:sameAs <http://rdaregistry.info/Elements/u/animatorOf> ;
	skos:definition "Relates an agent contributing to a moving image resource or computer program by giving apparent movement to inanimate objects or drawings to the resource."@en .

<http://rdaregistry.info/Elements/u/P60607> reg:hasSubproperty <http://rdaregistry.info/Elements/a/P50137> ;
	reg:name "arrangerOfMusicOf"@en ;
	reg:status status:1001 ;
	a rdf:Property ;
	rdfs:isDefinedBy <http://rdaregistry.info/Elements/u/> ;
	rdfs:label "is arranger of music of"@en ;
	rdfs:subPropertyOf <http://rdaregistry.info/Elements/u/P60626> ;
	owl:inverseOf <http://rdaregistry.info/Elements/u/P60379> ;
	owl:sameAs <http://rdaregistry.info/Elements/u/arrangerOfMusicOf> ;
	skos:definition "Relates an agent contributing to a musical resource by rewriting the composition for a medium of performance different from that for which the resource was originally intended to the resource."@en .

<http://rdaregistry.info/Elements/u/P60608> reg:hasSubproperty <http://rdaregistry.info/Elements/a/P50138> , <http://rdaregistry.info/Elements/u/P60600> ;
	reg:name "writerOfAddedTextOf"@en ;
	reg:status status:1001 ;
	a rdf:Property ;
	rdfs:isDefinedBy <http://rdaregistry.info/Elements/u/> ;
	rdfs:label "is writer of added text of"@en ;
	rdfs:subPropertyOf <http://rdaregistry.info/Elements/u/P60620> ;
	owl:inverseOf <http://rdaregistry.info/Elements/u/P60380> ;
	owl:sameAs <http://rdaregistry.info/Elements/u/writerOfAddedTextOf> ;
	skos:definition "Relates an agent contributing to a primarily non-textual resource by providing text for the non-textual resource (e.g., writing captions for photographs, descriptions of maps) to the resource."@en .

<http://rdaregistry.info/Elements/u/P60609> reg:hasSubproperty <http://rdaregistry.info/Elements/a/P50141> ;
	reg:name "draftsmanOf"@en ;
	reg:status status:1001 ;
	a rdf:Property ;
	rdfs:isDefinedBy <http://rdaregistry.info/Elements/u/> ;
	rdfs:label "is draftsman of"@en ;
	rdfs:subPropertyOf <http://rdaregistry.info/Elements/u/P60626> ;
	owl:inverseOf <http://rdaregistry.info/Elements/u/P60381> ;
	owl:sameAs <http://rdaregistry.info/Elements/u/draftsmanOf> ;
	skos:definition "Relates an agent contributing to a resource by an architect, inventor, etc., by making detailed plans or drawings for buildings, ships, aircraft, machines, objects, etc. to the resource."@en .

<http://rdaregistry.info/Elements/u/P60610> reg:hasSubproperty <http://rdaregistry.info/Elements/a/P50142> ;
	reg:name "transcriberOf"@en ;
	reg:status status:1001 ;
	a rdf:Property ;
	rdfs:isDefinedBy <http://rdaregistry.info/Elements/u/> ;
	rdfs:label "is transcriber of"@en ;
	rdfs:subPropertyOf <http://rdaregistry.info/Elements/u/P60626> ;
	owl:inverseOf <http://rdaregistry.info/Elements/u/P60382> ;
	owl:sameAs <http://rdaregistry.info/Elements/u/transcriberOf> ;
	skos:definition "Relates an agent contributing to a resource by changing it from one system of notation to another to the resource."@en .

<http://rdaregistry.info/Elements/u/P60611> reg:hasSubproperty <http://rdaregistry.info/Elements/a/P50143> ;
	reg:name "musicalDirectorOf"@en ;
	reg:status status:1001 ;
	a rdf:Property ;
	rdfs:isDefinedBy <http://rdaregistry.info/Elements/u/> ;
	rdfs:label "is musical director of"@en ;
	rdfs:subPropertyOf <http://rdaregistry.info/Elements/u/P60626> ;
	owl:inverseOf <http://rdaregistry.info/Elements/u/P60383> ;
	owl:sameAs <http://rdaregistry.info/Elements/u/musicalDirectorOf> ;
	skos:definition "Relates an agent contributing to a resource by coordinating the activities of the composer, the sound editor, and sound mixers for a moving image production or for a musical or dramatic presentation or entertainment to the resource."@en .

<http://rdaregistry.info/Elements/u/P60612> reg:hasSubproperty <http://rdaregistry.info/Elements/a/P50144> ;
	reg:name "costumeDesignerOf"@en ;
	reg:status status:1001 ;
	a rdf:Property ;
	rdfs:isDefinedBy <http://rdaregistry.info/Elements/u/> ;
	rdfs:label "is costume designer of"@en ;
	rdfs:subPropertyOf <http://rdaregistry.info/Elements/u/P60626> ;
	owl:inverseOf <http://rdaregistry.info/Elements/u/P60384> ;
	owl:sameAs <http://rdaregistry.info/Elements/u/costumeDesignerOf> ;
	skos:definition "Relates an agent contributing to a resource by designing the costumes for a moving image production or for a musical or dramatic presentation or entertainment to the resource."@en .

<http://rdaregistry.info/Elements/u/P60613> reg:hasSubproperty <http://rdaregistry.info/Elements/a/P50145> ;
	reg:name "translatorOf"@en ;
	reg:status status:1001 ;
	a rdf:Property ;
	rdfs:isDefinedBy <http://rdaregistry.info/Elements/u/> ;
	rdfs:label "is translator of"@en ;
	rdfs:subPropertyOf <http://rdaregistry.info/Elements/u/P60626> ;
	owl:inverseOf <http://rdaregistry.info/Elements/u/P60385> ;
	owl:sameAs <http://rdaregistry.info/Elements/u/translatorOf> ;
	skos:definition "Relates an agent contributing to a resource by expressing the original text of the resource in a language different from that of the original resource to the resource."@en .

<http://rdaregistry.info/Elements/u/P60614> reg:hasSubproperty <http://rdaregistry.info/Elements/a/P50146> ;
	reg:name "artDirectorOf"@en ;
	reg:status status:1001 ;
	a rdf:Property ;
	rdfs:isDefinedBy <http://rdaregistry.info/Elements/u/> ;
	rdfs:label "is art director of"@en ;
	rdfs:subPropertyOf <http://rdaregistry.info/Elements/u/P60626> ;
	owl:inverseOf <http://rdaregistry.info/Elements/u/P60386> ;
	owl:sameAs <http://rdaregistry.info/Elements/u/artDirectorOf> ;
	skos:definition "Relates an agent contributing to a resource by overseeing the artists and craftspeople who build the sets for moving image productions to the resource."@en .

<http://rdaregistry.info/Elements/u/P60615> reg:hasSubproperty <http://rdaregistry.info/Elements/a/P50147> , <http://rdaregistry.info/Elements/u/P60016> , <http://rdaregistry.info/Elements/u/P60017> , <http://rdaregistry.info/Elements/u/P60018> , <http://rdaregistry.info/Elements/u/P60019> , <http://rdaregistry.info/Elements/u/P60020> , <http://rdaregistry.info/Elements/u/P60021> , <http://rdaregistry.info/Elements/u/P60022> , <http://rdaregistry.info/Elements/u/P60023> , <http://rdaregistry.info/Elements/u/P60024> , <http://rdaregistry.info/Elements/u/P60025> , <http://rdaregistry.info/Elements/u/P60026> , <http://rdaregistry.info/Elements/u/P60028> , <http://rdaregistry.info/Elements/u/P60029> , <http://rdaregistry.info/Elements/u/P60030> , <http://rdaregistry.info/Elements/u/P60031> ;
	reg:name "performerOf"@en ;
	reg:status status:1001 ;
	a rdf:Property ;
	rdfs:isDefinedBy <http://rdaregistry.info/Elements/u/> ;
	rdfs:label "is performer of"@en ;
	rdfs:subPropertyOf <http://rdaregistry.info/Elements/u/P60626> ;
	owl:inverseOf <http://rdaregistry.info/Elements/u/P60387> ;
	owl:sameAs <http://rdaregistry.info/Elements/u/performerOf> ;
	skos:definition "Relates an agent contributing to a resource by performing music, acting, dancing, speaking, etc., often in a musical or dramatic presentation, etc. to the resource."@en .

<http://rdaregistry.info/Elements/u/P60616> reg:hasSubproperty <http://rdaregistry.info/Elements/a/P50148> ;
	reg:name "courtReporterOf"@en ;
	reg:status status:1001 ;
	a rdf:Property ;
	rdfs:isDefinedBy <http://rdaregistry.info/Elements/u/> ;
	rdfs:label "is court reporter of"@en ;
	rdfs:subPropertyOf <http://rdaregistry.info/Elements/u/P60626> ;
	owl:inverseOf <http://rdaregistry.info/Elements/u/P60388> ;
	owl:sameAs <http://rdaregistry.info/Elements/u/courtReporterOf> ;
	skos:definition "Relates an agent contributing to a resource by preparing a court’s opinions for publication to the resource."@en .

<http://rdaregistry.info/Elements/u/P60617> reg:hasSubproperty <http://rdaregistry.info/Elements/a/P50149> ;
	reg:name "writerOfPrefaceOf"@en ;
	reg:status status:1001 ;
	a rdf:Property ;
	rdfs:isDefinedBy <http://rdaregistry.info/Elements/u/> ;
	rdfs:label "is writer of preface of"@en ;
	rdfs:subPropertyOf <http://rdaregistry.info/Elements/u/P60620> ;
	owl:inverseOf <http://rdaregistry.info/Elements/u/P60389> ;
	owl:sameAs <http://rdaregistry.info/Elements/u/writerOfPrefaceOf> ;
	skos:definition "Relates an agent contributing to a resource by providing a preface to the original resource to the resource."@en .

<http://rdaregistry.info/Elements/u/P60618> reg:hasSubproperty <http://rdaregistry.info/Elements/a/P50152> ;
	reg:name "writerOfAddedCommentaryOf"@en ;
	reg:status status:1001 ;
	a rdf:Property ;
	rdfs:isDefinedBy <http://rdaregistry.info/Elements/u/> ;
	rdfs:label "is writer of added commentary of"@en ;
	rdfs:subPropertyOf <http://rdaregistry.info/Elements/u/P60620> ;
	owl:inverseOf <http://rdaregistry.info/Elements/u/P60390> ;
	owl:sameAs <http://rdaregistry.info/Elements/u/writerOfAddedCommentaryOf> ;
	skos:definition "Relates an agent contributing to a resource by providing an interpretation or critical explanation of the original resource to the resource."@en .

<http://rdaregistry.info/Elements/u/P60619> reg:hasSubproperty <http://rdaregistry.info/Elements/a/P50153> ;
	reg:name "writerOfIntroductionOf"@en ;
	reg:status status:1001 ;
	a rdf:Property ;
	rdfs:isDefinedBy <http://rdaregistry.info/Elements/u/> ;
	rdfs:label "is writer of introduction of"@en ;
	rdfs:subPropertyOf <http://rdaregistry.info/Elements/u/P60620> ;
	owl:inverseOf <http://rdaregistry.info/Elements/u/P60391> ;
	owl:sameAs <http://rdaregistry.info/Elements/u/writerOfIntroductionOf> ;
	skos:definition "Relates an agent contributing to a resource by providing an introduction to the original resource to the resource."@en .

<http://rdaregistry.info/Elements/u/P60620> reg:hasSubproperty <http://rdaregistry.info/Elements/a/P50154> , <http://rdaregistry.info/Elements/u/P60608> , <http://rdaregistry.info/Elements/u/P60617> , <http://rdaregistry.info/Elements/u/P60618> , <http://rdaregistry.info/Elements/u/P60619> ;
	reg:name "writerOfSupplementaryTextualContentOf"@en ;
	reg:status status:1001 ;
	a rdf:Property ;
	rdfs:isDefinedBy <http://rdaregistry.info/Elements/u/> ;
	rdfs:label "is writer of supplementary textual content of"@en ;
	rdfs:subPropertyOf <http://rdaregistry.info/Elements/u/P60626> ;
	owl:inverseOf <http://rdaregistry.info/Elements/u/P60392> ;
	owl:sameAs <http://rdaregistry.info/Elements/u/writerOfSupplementaryTextualContentOf> ;
	skos:definition "Relates an agent contributing to a resource by providing supplementary textual content (e.g., an appendix, an introduction, a preface) to the original resource to the resource."@en .

<http://rdaregistry.info/Elements/u/P60621> reg:hasSubproperty <http://rdaregistry.info/Elements/a/P50156> ;
	reg:name "editorOf"@en ;
	reg:status status:1001 ;
	a rdf:Property ;
	rdfs:isDefinedBy <http://rdaregistry.info/Elements/u/> ;
	rdfs:label "is editor of"@en ;
	rdfs:subPropertyOf <http://rdaregistry.info/Elements/u/P60626> ;
	owl:inverseOf <http://rdaregistry.info/Elements/u/P60393> ;
	owl:sameAs <http://rdaregistry.info/Elements/u/editorOf> ;
	skos:definition "Relates an agent contributing to a resource by revising or clarifying the content, e.g., adding an introduction, notes, or other critical matter to the resource."@en .

<http://rdaregistry.info/Elements/u/P60622> reg:hasSubproperty <http://rdaregistry.info/Elements/a/P50157> ;
	reg:name "abridgerOf"@en ;
	reg:status status:1001 ;
	a rdf:Property ;
	rdfs:isDefinedBy <http://rdaregistry.info/Elements/u/> ;
	rdfs:label "is abridger of"@en ;
	rdfs:subPropertyOf <http://rdaregistry.info/Elements/u/P60626> ;
	owl:inverseOf <http://rdaregistry.info/Elements/u/P60394> ;
	owl:sameAs <http://rdaregistry.info/Elements/u/abridgerOf> ;
	skos:definition "Relates an agent contributing to a resource by shortening or condensing the original resource but leaving the nature and content of the original resource substantially unchanged to the resource."@en .

<http://rdaregistry.info/Elements/u/P60623> reg:hasSubproperty <http://rdaregistry.info/Elements/a/P50158> ;
	reg:name "recordingEngineerOf"@en ;
	reg:status status:1001 ;
	a rdf:Property ;
	rdfs:isDefinedBy <http://rdaregistry.info/Elements/u/> ;
	rdfs:label "is recording engineer of"@en ;
	rdfs:subPropertyOf <http://rdaregistry.info/Elements/u/P60626> ;
	owl:inverseOf <http://rdaregistry.info/Elements/u/P60395> ;
	owl:sameAs <http://rdaregistry.info/Elements/u/recordingEngineerOf> ;
	skos:definition "Relates an agent contributing to a resource by supervising the technical aspects of a sound or video recording session to the resource."@en .

<http://rdaregistry.info/Elements/u/P60624> reg:hasSubproperty <http://rdaregistry.info/Elements/a/P50159> ;
	reg:name "illustratorOf"@en ;
	reg:status status:1001 ;
	a rdf:Property ;
	rdfs:isDefinedBy <http://rdaregistry.info/Elements/u/> ;
	rdfs:label "is illustrator of"@en ;
	rdfs:subPropertyOf <http://rdaregistry.info/Elements/u/P60626> ;
	owl:inverseOf <http://rdaregistry.info/Elements/u/P60396> ;
	owl:sameAs <http://rdaregistry.info/Elements/u/illustratorOf> ;
	skos:definition "Relates an agent contributing to a resource by supplementing the primary content with drawings, diagrams, photographs, etc. to the resource."@en .

<http://rdaregistry.info/Elements/u/P60625> reg:hasSubproperty <http://rdaregistry.info/Elements/a/P50160> ;
	reg:name "recordistOf"@en ;
	reg:status status:1001 ;
	a rdf:Property ;
	rdfs:isDefinedBy <http://rdaregistry.info/Elements/u/> ;
	rdfs:label "is recordist of"@en ;
	rdfs:subPropertyOf <http://rdaregistry.info/Elements/u/P60626> ;
	owl:inverseOf <http://rdaregistry.info/Elements/u/P60397> ;
	owl:sameAs <http://rdaregistry.info/Elements/u/recordistOf> ;
	skos:definition "Relates an agent contributing to a resource by using a recording device to capture sound and/or video during a recording session, including field recordings of natural sounds, folkloric events, music, etc. to the resource."@en .

<http://rdaregistry.info/Elements/u/P60626> reg:hasSubproperty <http://rdaregistry.info/Elements/a/P50161> , <http://rdaregistry.info/Elements/u/P60605> , <http://rdaregistry.info/Elements/u/P60606> , <http://rdaregistry.info/Elements/u/P60607> , <http://rdaregistry.info/Elements/u/P60609> , <http://rdaregistry.info/Elements/u/P60610> , <http://rdaregistry.info/Elements/u/P60611> , <http://rdaregistry.info/Elements/u/P60612> , <http://rdaregistry.info/Elements/u/P60613> , <http://rdaregistry.info/Elements/u/P60614> , <http://rdaregistry.info/Elements/u/P60615> , <http://rdaregistry.info/Elements/u/P60616> , <http://rdaregistry.info/Elements/u/P60620> , <http://rdaregistry.info/Elements/u/P60621> , <http://rdaregistry.info/Elements/u/P60622> , <http://rdaregistry.info/Elements/u/P60623> , <http://rdaregistry.info/Elements/u/P60624> , <http://rdaregistry.info/Elements/u/P60625> , <http://rdaregistry.info/Elements/u/P60627> , <http://rdaregistry.info/Elements/u/P60647> , <http://rdaregistry.info/Elements/u/P60651> , <http://rdaregistry.info/Elements/u/P60666> , <http://rdaregistry.info/Elements/u/P60671> ;
	reg:name "contributorOf"@en ;
	reg:status status:1001 ;
	a rdf:Property ;
	rdfs:isDefinedBy <http://rdaregistry.info/Elements/u/> ;
	rdfs:label "is contributor of"@en ;
	owl:inverseOf <http://rdaregistry.info/Elements/u/P60398> ;
	owl:sameAs <http://rdaregistry.info/Elements/u/contributorOf> ;
	skos:definition "Relates an agent contributing to a resource to the resource."@en .

<http://rdaregistry.info/Elements/u/P60627> reg:hasSubproperty <http://rdaregistry.info/Elements/a/P50139> ;
	reg:name "stageDirectorOf"@en ;
	reg:status status:1001 ;
	a rdf:Property ;
	rdfs:isDefinedBy <http://rdaregistry.info/Elements/u/> ;
	rdfs:label "is stage director of"@en ;
	rdfs:subPropertyOf <http://rdaregistry.info/Elements/u/P60626> ;
	owl:inverseOf <http://rdaregistry.info/Elements/u/P60399> ;
	owl:sameAs <http://rdaregistry.info/Elements/u/stageDirectorOf> ;
	skos:definition "Relates an agent contributing to a stage resource through the general management and supervision of a performance to the resource."@en .

<http://rdaregistry.info/Elements/u/P60628> reg:hasSubproperty <http://rdaregistry.info/Elements/a/P50162> , <http://rdaregistry.info/Elements/u/P60008> ;
	reg:name "currentOwnerOf"@en ;
	reg:status status:1001 ;
	a rdf:Property ;
	rdfs:isDefinedBy <http://rdaregistry.info/Elements/u/> ;
	rdfs:label "is current owner of"@en ;
	rdfs:subPropertyOf <http://rdaregistry.info/Elements/u/P60632> ;
	owl:inverseOf <http://rdaregistry.info/Elements/u/P60400> ;
	owl:sameAs <http://rdaregistry.info/Elements/u/currentOwnerOf> ;
	skos:definition "Relates an agent currently having legal possession of a resource to the resource."@en .

<http://rdaregistry.info/Elements/u/P60629> reg:hasSubproperty <http://rdaregistry.info/Elements/a/P50026> ;
	reg:name "employee"@en ;
	reg:status status:1001 ;
	a rdf:Property ;
	rdfs:isDefinedBy <http://rdaregistry.info/Elements/u/> ;
	rdfs:label "has employee"@en ;
	owl:inverseOf <http://rdaregistry.info/Elements/u/P60679> ;
	owl:sameAs <http://rdaregistry.info/Elements/u/employee> ;
	skos:definition "Relates an agent employed by the agent to the agent."@en .

<http://rdaregistry.info/Elements/u/P60630> reg:hasSubproperty <http://rdaregistry.info/Elements/a/P50163> , <http://rdaregistry.info/Elements/u/P60012> , <http://rdaregistry.info/Elements/u/P60013> ;
	reg:name "formerOwnerOf"@en ;
	reg:status status:1001 ;
	a rdf:Property ;
	rdfs:isDefinedBy <http://rdaregistry.info/Elements/u/> ;
	rdfs:label "is former owner of"@en ;
	rdfs:subPropertyOf <http://rdaregistry.info/Elements/u/P60632> ;
	owl:inverseOf <http://rdaregistry.info/Elements/u/P60401> ;
	owl:sameAs <http://rdaregistry.info/Elements/u/formerOwnerOf> ;
	skos:definition "Relates an agent formerly having legal possession of a resource to the resource."@en .

<http://rdaregistry.info/Elements/u/P60631> reg:name "custodianOf"@en ;
	reg:status status:1001 ;
	a rdf:Property ;
	rdfs:isDefinedBy <http://rdaregistry.info/Elements/u/> ;
	rdfs:label "is custodian of"@en ;
	owl:inverseOf <http://rdaregistry.info/Elements/u/P60402> ;
	owl:sameAs <http://rdaregistry.info/Elements/u/custodianOf> ;
	skos:definition "Relates an agent having legal custody of a resource to the resource."@en .

<http://rdaregistry.info/Elements/u/P60632> reg:hasSubproperty <http://rdaregistry.info/Elements/u/P60628> , <http://rdaregistry.info/Elements/u/P60630> ;
	reg:name "ownerOf"@en ;
	reg:status status:1001 ;
	a rdf:Property ;
	rdfs:isDefinedBy <http://rdaregistry.info/Elements/u/> ;
	rdfs:label "is owner of"@en ;
	owl:inverseOf <http://rdaregistry.info/Elements/u/P60404> ;
	owl:sameAs <http://rdaregistry.info/Elements/u/ownerOf> ;
	skos:definition "Relates an agent having legal possession of a resource to the resource."@en .

<http://rdaregistry.info/Elements/u/P60633> reg:hasSubproperty <http://rdaregistry.info/Elements/a/P50027> ;
	reg:name "incumbent"@en ;
	reg:status status:1001 ;
	a rdf:Property ;
	rdfs:isDefinedBy <http://rdaregistry.info/Elements/u/> ;
	rdfs:label "has incumbent"@en ;
	owl:inverseOf <http://rdaregistry.info/Elements/u/P60633> ;
	owl:sameAs <http://rdaregistry.info/Elements/u/incumbent> ;
	skos:definition "Relates an agent holding an office in the agent to the agent."@en .

<http://rdaregistry.info/Elements/u/P60634> reg:hasSubproperty <http://rdaregistry.info/Elements/a/P50166> , <http://rdaregistry.info/Elements/a/P50167> ;
	reg:name "honoureeOf"@en ;
	reg:status status:1001 ;
	a rdf:Property ;
	rdfs:isDefinedBy <http://rdaregistry.info/Elements/u/> ;
	rdfs:label "is honouree of"@en ;
	rdfs:subPropertyOf <http://rdaregistry.info/Elements/u/P60602> ;
	owl:inverseOf <http://rdaregistry.info/Elements/u/P60406> ;
	owl:sameAs <http://rdaregistry.info/Elements/u/honoureeOf> ;
	skos:definition "Relates an agent honoured by a resource (e.g., the honouree of a festschrift) to the resource."@en .

<http://rdaregistry.info/Elements/u/P60635> reg:hasSubproperty <http://rdaregistry.info/Elements/a/P50168> ;
	reg:name "broadcasterOf"@en ;
	reg:status status:1001 ;
	a rdf:Property ;
	rdfs:isDefinedBy <http://rdaregistry.info/Elements/u/> ;
	rdfs:label "is broadcaster of"@en ;
	rdfs:subPropertyOf <http://rdaregistry.info/Elements/u/P60670> ;
	owl:inverseOf <http://rdaregistry.info/Elements/u/P60407> ;
	owl:sameAs <http://rdaregistry.info/Elements/u/broadcasterOf> ;
	skos:definition "Relates an agent involved in broadcasting a resource to an audience via radio, television, webcast, etc. to the resource."@en .

<http://rdaregistry.info/Elements/u/P60636> reg:hasSubproperty <http://rdaregistry.info/Elements/a/P50169> ;
	reg:name "filmDistributorOf"@en ;
	reg:status status:1001 ;
	a rdf:Property ;
	rdfs:isDefinedBy <http://rdaregistry.info/Elements/u/> ;
	rdfs:label "is film distributor of"@en ;
	rdfs:subPropertyOf <http://rdaregistry.info/Elements/u/P60667> ;
	owl:inverseOf <http://rdaregistry.info/Elements/u/P60408> ;
	owl:sameAs <http://rdaregistry.info/Elements/u/filmDistributorOf> ;
	skos:definition "Relates an agent involved in distributing a moving image resource to theatres or other distribution channels to the resource."@en .

<http://rdaregistry.info/Elements/u/P60637> reg:hasSubproperty <http://rdaregistry.info/Elements/a/P50170> ;
	reg:name "bookDesignerOf"@en ;
	reg:status status:1001 ;
	a rdf:Property ;
	rdfs:isDefinedBy <http://rdaregistry.info/Elements/u/> ;
	rdfs:label "is book designer of"@en ;
	rdfs:subPropertyOf <http://rdaregistry.info/Elements/u/P60669> ;
	owl:inverseOf <http://rdaregistry.info/Elements/u/P60409> ;
	owl:sameAs <http://rdaregistry.info/Elements/u/bookDesignerOf> ;
	skos:definition "Relates an agent involved in manufacturing a resource by being responsible for the entire graphic design of a book, including arrangement of type and illustration, choice of materials, and process used to the resource."@en .

<http://rdaregistry.info/Elements/u/P60638> reg:hasSubproperty <http://rdaregistry.info/Elements/a/P50171> ;
	reg:name "engraverOf"@en ;
	reg:status status:1001 ;
	a rdf:Property ;
	rdfs:isDefinedBy <http://rdaregistry.info/Elements/u/> ;
	rdfs:label "is engraver of"@en ;
	rdfs:subPropertyOf <http://rdaregistry.info/Elements/u/P60669> ;
	owl:inverseOf <http://rdaregistry.info/Elements/u/P60410> ;
	owl:sameAs <http://rdaregistry.info/Elements/u/engraverOf> ;
	skos:definition "Relates an agent involved in manufacturing a resource by cutting letters, figures, etc., on a surface such as a wooden or metal plate used for printing to the resource."@en .

<http://rdaregistry.info/Elements/u/P60639> reg:hasSubproperty <http://rdaregistry.info/Elements/a/P50172> ;
	reg:name "brailleEmbosserOf"@en ;
	reg:status status:1001 ;
	a rdf:Property ;
	rdfs:isDefinedBy <http://rdaregistry.info/Elements/u/> ;
	rdfs:label "is braille embosser of"@en ;
	rdfs:subPropertyOf <http://rdaregistry.info/Elements/u/P60669> ;
	owl:inverseOf <http://rdaregistry.info/Elements/u/P60411> ;
	owl:sameAs <http://rdaregistry.info/Elements/u/brailleEmbosserOf> ;
	skos:definition "Relates an agent involved in manufacturing a resource by embossing braille cells using a stylus, special embossing printer, or other device to the resource."@en .

<http://rdaregistry.info/Elements/u/P60640> reg:hasSubproperty <http://rdaregistry.info/Elements/a/P50173> ;
	reg:name "printmakerOf"@en ;
	reg:status status:1001 ;
	a rdf:Property ;
	rdfs:isDefinedBy <http://rdaregistry.info/Elements/u/> ;
	rdfs:label "is printmaker of"@en ;
	rdfs:subPropertyOf <http://rdaregistry.info/Elements/u/P60669> ;
	owl:inverseOf <http://rdaregistry.info/Elements/u/P60412> ;
	owl:sameAs <http://rdaregistry.info/Elements/u/printmakerOf> ;
	skos:definition "Relates an agent involved in manufacturing a resource by making a relief, intaglio, or planographic printing surface to the resource."@en .

<http://rdaregistry.info/Elements/u/P60641> reg:hasSubproperty <http://rdaregistry.info/Elements/a/P50174> ;
	reg:name "casterOf"@en ;
	reg:status status:1001 ;
	a rdf:Property ;
	rdfs:isDefinedBy <http://rdaregistry.info/Elements/u/> ;
	rdfs:label "is caster of"@en ;
	rdfs:subPropertyOf <http://rdaregistry.info/Elements/u/P60669> ;
	owl:inverseOf <http://rdaregistry.info/Elements/u/P60413> ;
	owl:sameAs <http://rdaregistry.info/Elements/u/casterOf> ;
	skos:definition "Relates an agent involved in manufacturing a resource by pouring a liquid or molten substance into a mold and leaving it to solidify to take the shape of the mold to the resource."@en .

<http://rdaregistry.info/Elements/u/P60642> reg:hasSubproperty <http://rdaregistry.info/Elements/a/P50175> ;
	reg:name "lithographerOf"@en ;
	reg:status status:1001 ;
	a rdf:Property ;
	rdfs:isDefinedBy <http://rdaregistry.info/Elements/u/> ;
	rdfs:label "is lithographer of"@en ;
	rdfs:subPropertyOf <http://rdaregistry.info/Elements/u/P60669> ;
	owl:inverseOf <http://rdaregistry.info/Elements/u/P60414> ;
	owl:sameAs <http://rdaregistry.info/Elements/u/lithographerOf> ;
	skos:definition "Relates an agent involved in manufacturing a resource by preparing a stone or plate for lithographic printing, including a graphic artist creating a design directly on the surface from which printing will be done to the resource."@en .

<http://rdaregistry.info/Elements/u/P60643> reg:hasSubproperty <http://rdaregistry.info/Elements/a/P50176> ;
	reg:name "platemakerOf"@en ;
	reg:status status:1001 ;
	a rdf:Property ;
	rdfs:isDefinedBy <http://rdaregistry.info/Elements/u/> ;
	rdfs:label "is platemaker of"@en ;
	rdfs:subPropertyOf <http://rdaregistry.info/Elements/u/P60669> ;
	owl:inverseOf <http://rdaregistry.info/Elements/u/P60415> ;
	owl:sameAs <http://rdaregistry.info/Elements/u/platemakerOf> ;
	skos:definition "Relates an agent involved in manufacturing a resource by preparing plates used in the production of printed images and/or text to the resource."@en .

<http://rdaregistry.info/Elements/u/P60644> reg:hasSubproperty <http://rdaregistry.info/Elements/a/P50177> ;
	reg:name "etcherOf"@en ;
	reg:status status:1001 ;
	a rdf:Property ;
	rdfs:isDefinedBy <http://rdaregistry.info/Elements/u/> ;
	rdfs:label "is etcher of"@en ;
	rdfs:subPropertyOf <http://rdaregistry.info/Elements/u/P60669> ;
	owl:inverseOf <http://rdaregistry.info/Elements/u/P60416> ;
	owl:sameAs <http://rdaregistry.info/Elements/u/etcherOf> ;
	skos:definition "Relates an agent involved in manufacturing a resource by subjecting metal, glass, or some other surface used for printing, to acid or another corrosive substance to the resource."@en .

<http://rdaregistry.info/Elements/u/P60645> reg:hasSubproperty <http://rdaregistry.info/Elements/a/P50178> ;
	reg:name "collotyperOf"@en ;
	reg:status status:1001 ;
	a rdf:Property ;
	rdfs:isDefinedBy <http://rdaregistry.info/Elements/u/> ;
	rdfs:label "is collotyper of"@en ;
	rdfs:subPropertyOf <http://rdaregistry.info/Elements/u/P60669> ;
	owl:inverseOf <http://rdaregistry.info/Elements/u/P60417> ;
	owl:sameAs <http://rdaregistry.info/Elements/u/collotyperOf> ;
	skos:definition "Relates an agent involved in manufacturing a resource of photographic prints from film or other colloid that has ink-receptive and ink-repellent surfaces to the resource."@en .

<http://rdaregistry.info/Elements/u/P60646> reg:hasSubproperty <http://rdaregistry.info/Elements/a/P50179> ;
	reg:name "printerOf"@en ;
	reg:status status:1001 ;
	a rdf:Property ;
	rdfs:isDefinedBy <http://rdaregistry.info/Elements/u/> ;
	rdfs:label "is printer of"@en ;
	rdfs:subPropertyOf <http://rdaregistry.info/Elements/u/P60669> ;
	owl:inverseOf <http://rdaregistry.info/Elements/u/P60418> ;
	owl:sameAs <http://rdaregistry.info/Elements/u/printerOf> ;
	skos:definition "Relates an agent involved in manufacturing a resource of printed text, notated music, etc., from type or plates, such as a book, newspaper, magazine, broadside, score, etc. to the resource."@en .

<http://rdaregistry.info/Elements/u/P60647> reg:hasSubproperty <http://rdaregistry.info/Elements/a/P50180> ;
	reg:name "presenterOf"@en ;
	reg:status status:1001 ;
	a rdf:Property ;
	rdfs:isDefinedBy <http://rdaregistry.info/Elements/u/> ;
	rdfs:label "is presenter of"@en ;
	rdfs:subPropertyOf <http://rdaregistry.info/Elements/u/P60626> ;
	owl:inverseOf <http://rdaregistry.info/Elements/u/P60419> ;
	owl:sameAs <http://rdaregistry.info/Elements/u/presenterOf> ;
	skos:definition "Relates an agent mentioned in an “x presents” credit for moving image materials and who is probably associated with production, finance, or distribution in some way to the resource."@en .

<http://rdaregistry.info/Elements/u/P60648> reg:hasSubproperty <http://rdaregistry.info/Elements/a/P50095> ;
	reg:name "memberOf"@en ;
	reg:status status:1001 ;
	a rdf:Property ;
	rdfs:isDefinedBy <http://rdaregistry.info/Elements/u/> ;
	rdfs:label "has member of"@en ;
	owl:inverseOf <http://rdaregistry.info/Elements/u/P60697> ;
	owl:sameAs <http://rdaregistry.info/Elements/u/memberOf> ;
	skos:definition "Relates an agent of which the agent is a member to the agent."@en .

<http://rdaregistry.info/Elements/u/P60649> reg:hasSubproperty <http://rdaregistry.info/Elements/a/P50091> ;
	reg:name "degreeSupervisorOf"@en ;
	reg:status status:1001 ;
	a rdf:Property ;
	rdfs:isDefinedBy <http://rdaregistry.info/Elements/u/> ;
	rdfs:label "is degree supervisor of"@en ;
	rdfs:subPropertyOf <http://rdaregistry.info/Elements/u/P60672> ;
	owl:inverseOf <http://rdaregistry.info/Elements/u/P60420> ;
	owl:sameAs <http://rdaregistry.info/Elements/u/degreeSupervisorOf> ;
	skos:definition "Relates an agent overseeing a higher-level academic degree to the resource."@en .

<http://rdaregistry.info/Elements/u/P60650> reg:hasSubproperty <http://rdaregistry.info/Elements/a/P50092> ;
	reg:name "illuminatorOf"@en ;
	reg:status status:1001 ;
	a rdf:Property ;
	rdfs:isDefinedBy <http://rdaregistry.info/Elements/u/> ;
	rdfs:label "is illuminator of"@en ;
	rdfs:subPropertyOf <http://rdaregistry.info/Elements/u/P60602> ;
	owl:inverseOf <http://rdaregistry.info/Elements/u/P60421> ;
	owl:sameAs <http://rdaregistry.info/Elements/u/illuminatorOf> ;
	skos:definition "Relates an agent providing decoration to a specific resource using precious metals or color, often with elaborate designs and motifs to the resource."@en .

<http://rdaregistry.info/Elements/u/P60651> reg:hasSubproperty <http://rdaregistry.info/Elements/a/P50183> ;
	reg:name "editorOfMovingImageWorkOf"@en ;
	reg:status status:1001 ;
	a rdf:Property ;
	rdfs:isDefinedBy <http://rdaregistry.info/Elements/u/> ;
	rdfs:label "is editor of moving image work of"@en ;
	rdfs:subPropertyOf <http://rdaregistry.info/Elements/u/P60626> ;
	owl:inverseOf <http://rdaregistry.info/Elements/u/P60422> ;
	owl:sameAs <http://rdaregistry.info/Elements/u/editorOfMovingImageWorkOf> ;
	skos:definition "Relates an agent responsible for assembling, arranging, and trimming film, video, or other moving image formats, including both visual and audio aspects to the resource."@en .

<http://rdaregistry.info/Elements/u/P60652> reg:hasSubproperty <http://rdaregistry.info/Elements/a/P50184> ;
	reg:name "programmerOf"@en ;
	reg:status status:1001 ;
	a rdf:Property ;
	rdfs:isDefinedBy <http://rdaregistry.info/Elements/u/> ;
	rdfs:label "is programmer of"@en ;
	rdfs:subPropertyOf <http://rdaregistry.info/Elements/u/P60672> ;
	owl:inverseOf <http://rdaregistry.info/Elements/u/P60423> ;
	owl:sameAs <http://rdaregistry.info/Elements/u/programmerOf> ;
	skos:definition "Relates an agent responsible for creating a computer program to the resource."@en .

<http://rdaregistry.info/Elements/u/P60653> reg:hasSubproperty <http://rdaregistry.info/Elements/a/P50185> ;
	reg:name "designerOf"@en ;
	reg:status status:1001 ;
	a rdf:Property ;
	rdfs:isDefinedBy <http://rdaregistry.info/Elements/u/> ;
	rdfs:label "is designer of"@en ;
	rdfs:subPropertyOf <http://rdaregistry.info/Elements/u/P60672> ;
	owl:inverseOf <http://rdaregistry.info/Elements/u/P60424> ;
	owl:sameAs <http://rdaregistry.info/Elements/u/designerOf> ;
	skos:definition "Relates an agent responsible for creating a design for an object to the resource."@en .

<http://rdaregistry.info/Elements/u/P60654> reg:hasSubproperty <http://rdaregistry.info/Elements/a/P50150> , <http://rdaregistry.info/Elements/a/P50186> ;
	reg:name "cartographerOf"@en ;
	reg:status status:1001 ;
	a rdf:Property ;
	rdfs:isDefinedBy <http://rdaregistry.info/Elements/u/> ;
	rdfs:label "is cartographer of"@en ;
	rdfs:subPropertyOf <http://rdaregistry.info/Elements/u/P60672> ;
	owl:inverseOf <http://rdaregistry.info/Elements/u/P60425> ;
	owl:sameAs <http://rdaregistry.info/Elements/u/cartographerOf> ;
	skos:definition "Relates an agent responsible for creating a map, atlas, globe, or other cartographic resource to the resource."@en .

<http://rdaregistry.info/Elements/u/P60655> reg:hasSubproperty <http://rdaregistry.info/Elements/a/P50134> , <http://rdaregistry.info/Elements/a/P50187> ;
	reg:name "composerOf"@en ;
	reg:status status:1001 ;
	a rdf:Property ;
	rdfs:isDefinedBy <http://rdaregistry.info/Elements/u/> ;
	rdfs:label "is composer of"@en ;
	rdfs:subPropertyOf <http://rdaregistry.info/Elements/u/P60672> ;
	owl:inverseOf <http://rdaregistry.info/Elements/u/P60426> ;
	owl:sameAs <http://rdaregistry.info/Elements/u/composerOf> ;
	skos:definition "Relates an agent responsible for creating a musical resource to the resource."@en .

<http://rdaregistry.info/Elements/u/P60656> reg:hasSubproperty <http://rdaregistry.info/Elements/a/P50188> ;
	reg:name "inventorOf"@en ;
	reg:status status:1001 ;
	a rdf:Property ;
	rdfs:isDefinedBy <http://rdaregistry.info/Elements/u/> ;
	rdfs:label "is inventor of"@en ;
	rdfs:subPropertyOf <http://rdaregistry.info/Elements/u/P60672> ;
	owl:inverseOf <http://rdaregistry.info/Elements/u/P60427> ;
	owl:sameAs <http://rdaregistry.info/Elements/u/inventorOf> ;
	skos:definition "Relates an agent responsible for creating a new device or process to the resource."@en .

<http://rdaregistry.info/Elements/u/P60657> reg:hasSubproperty <http://rdaregistry.info/Elements/a/P50189> ;
	reg:name "compilerOf"@en ;
	reg:status status:1001 ;
	a rdf:Property ;
	rdfs:isDefinedBy <http://rdaregistry.info/Elements/u/> ;
	rdfs:label "is compiler of"@en ;
	rdfs:subPropertyOf <http://rdaregistry.info/Elements/u/P60672> ;
	owl:inverseOf <http://rdaregistry.info/Elements/u/P60428> ;
	owl:sameAs <http://rdaregistry.info/Elements/u/compilerOf> ;
	skos:definition "Relates an agent responsible for creating a new resource (e.g., a bibliography, a directory) by selecting, arranging, aggregating, and editing data, information, etc. to the resource."@en .

<http://rdaregistry.info/Elements/u/P60658> reg:hasSubproperty <http://rdaregistry.info/Elements/a/P50190> ;
	reg:name "photographerOf"@en ;
	reg:status status:1001 ;
	a rdf:Property ;
	rdfs:isDefinedBy <http://rdaregistry.info/Elements/u/> ;
	rdfs:label "is photographer of"@en ;
	rdfs:subPropertyOf <http://rdaregistry.info/Elements/u/P60672> ;
	owl:inverseOf <http://rdaregistry.info/Elements/u/P60429> ;
	owl:sameAs <http://rdaregistry.info/Elements/u/photographerOf> ;
	skos:definition "Relates an agent responsible for creating a photographic resource to the resource."@en .

<http://rdaregistry.info/Elements/u/P60659> reg:hasSubproperty <http://rdaregistry.info/Elements/a/P50140> , <http://rdaregistry.info/Elements/a/P50191> ;
	reg:name "interviewerOf"@en ;
	reg:status status:1001 ;
	a rdf:Property ;
	rdfs:isDefinedBy <http://rdaregistry.info/Elements/u/> ;
	rdfs:label "is interviewer of"@en ;
	rdfs:subPropertyOf <http://rdaregistry.info/Elements/u/P60672> ;
	owl:inverseOf <http://rdaregistry.info/Elements/u/P60430> ;
	owl:sameAs <http://rdaregistry.info/Elements/u/interviewerOf> ;
	skos:definition "Relates an agent responsible for creating a resource by acting as an interviewer, reporter, pollster, or some other information gathering agent to the resource."@en .

<http://rdaregistry.info/Elements/u/P60660> reg:hasSubproperty <http://rdaregistry.info/Elements/a/P50192> , <http://rdaregistry.info/Elements/u/P60705> ;
	reg:name "artistOf"@en ;
	reg:status status:1001 ;
	a rdf:Property ;
	rdfs:isDefinedBy <http://rdaregistry.info/Elements/u/> ;
	rdfs:label "is artist of"@en ;
	rdfs:subPropertyOf <http://rdaregistry.info/Elements/u/P60672> ;
	owl:inverseOf <http://rdaregistry.info/Elements/u/P60431> ;
	owl:sameAs <http://rdaregistry.info/Elements/u/artistOf> ;
	skos:definition "Relates an agent responsible for creating a resource by conceiving, and often implementing, an original graphic design, drawing, painting, etc. to the resource."@en .

<http://rdaregistry.info/Elements/u/P60661> reg:hasSubproperty <http://rdaregistry.info/Elements/a/P50155> , <http://rdaregistry.info/Elements/a/P50193> ;
	reg:name "intervieweeOf"@en ;
	reg:status status:1001 ;
	a rdf:Property ;
	rdfs:isDefinedBy <http://rdaregistry.info/Elements/u/> ;
	rdfs:label "is interviewee of"@en ;
	rdfs:subPropertyOf <http://rdaregistry.info/Elements/u/P60672> ;
	owl:inverseOf <http://rdaregistry.info/Elements/u/P60432> ;
	owl:sameAs <http://rdaregistry.info/Elements/u/intervieweeOf> ;
	skos:definition "Relates an agent responsible for creating a resource by responding to an interviewer, usually a reporter, pollster, or some other information gathering agent to the resource."@en .

<http://rdaregistry.info/Elements/u/P60662> reg:hasSubproperty <http://rdaregistry.info/Elements/a/P50151> , <http://rdaregistry.info/Elements/a/P50194> ;
	reg:name "choreographerOf"@en ;
	reg:status status:1001 ;
	a rdf:Property ;
	rdfs:isDefinedBy <http://rdaregistry.info/Elements/u/> ;
	rdfs:label "is choreographer of"@en ;
	rdfs:subPropertyOf <http://rdaregistry.info/Elements/u/P60672> ;
	owl:inverseOf <http://rdaregistry.info/Elements/u/P60433> ;
	owl:sameAs <http://rdaregistry.info/Elements/u/choreographerOf> ;
	skos:definition "Relates an agent responsible for creating a resource of movement to the resource."@en .

<http://rdaregistry.info/Elements/u/P60663> reg:hasSubproperty <http://rdaregistry.info/Elements/a/P50195> , <http://rdaregistry.info/Elements/u/P60706> , <http://rdaregistry.info/Elements/u/P60707> , <http://rdaregistry.info/Elements/u/P60708> ;
	reg:name "authorOf"@en ;
	reg:status status:1001 ;
	a rdf:Property ;
	rdfs:isDefinedBy <http://rdaregistry.info/Elements/u/> ;
	rdfs:label "is author of"@en ;
	rdfs:subPropertyOf <http://rdaregistry.info/Elements/u/P60672> ;
	owl:inverseOf <http://rdaregistry.info/Elements/u/P60434> ;
	owl:sameAs <http://rdaregistry.info/Elements/u/authorOf> ;
	skos:definition "Relates an agent responsible for creating a resource that is primarily textual in content, regardless of media type (e.g., printed text, spoken word, electronic text, tactile text) or genre (e.g., poems, novels, screenplays, blogs) to the resource."@en .

<http://rdaregistry.info/Elements/u/P60664> reg:hasSubproperty <http://rdaregistry.info/Elements/a/P50196> , <http://rdaregistry.info/Elements/u/P60704> ;
	reg:name "architectOf"@en ;
	reg:status status:1001 ;
	a rdf:Property ;
	rdfs:isDefinedBy <http://rdaregistry.info/Elements/u/> ;
	rdfs:label "is architect of"@en ;
	rdfs:subPropertyOf <http://rdaregistry.info/Elements/u/P60672> ;
	owl:inverseOf <http://rdaregistry.info/Elements/u/P60435> ;
	owl:sameAs <http://rdaregistry.info/Elements/u/architectOf> ;
	skos:definition "Relates an agent responsible for creating an architectural design, including a pictorial representation intended to show how a building, etc., will look when completed to the resource."@en .

<http://rdaregistry.info/Elements/u/P60665> reg:hasSubproperty <http://rdaregistry.info/Elements/a/P50197> ;
	reg:name "filmmakerOf"@en ;
	reg:status status:1001 ;
	a rdf:Property ;
	rdfs:isDefinedBy <http://rdaregistry.info/Elements/u/> ;
	rdfs:label "is filmmaker of"@en ;
	rdfs:subPropertyOf <http://rdaregistry.info/Elements/u/P60672> ;
	owl:inverseOf <http://rdaregistry.info/Elements/u/P60436> ;
	owl:sameAs <http://rdaregistry.info/Elements/u/filmmakerOf> ;
	skos:definition "Relates an agent responsible for creating an independent or personal film to the resource."@en .

<http://rdaregistry.info/Elements/u/P60666> reg:hasSubproperty <http://rdaregistry.info/Elements/a/P50198> ;
	reg:name "productionDesignerOf"@en ;
	reg:status status:1001 ;
	a rdf:Property ;
	rdfs:isDefinedBy <http://rdaregistry.info/Elements/u/> ;
	rdfs:label "is production designer of"@en ;
	rdfs:subPropertyOf <http://rdaregistry.info/Elements/u/P60626> ;
	owl:inverseOf <http://rdaregistry.info/Elements/u/P60437> ;
	owl:sameAs <http://rdaregistry.info/Elements/u/productionDesignerOf> ;
	skos:definition "Relates an agent responsible for designing the overall visual appearance of a moving image production to the resource."@en .

<http://rdaregistry.info/Elements/u/P60667> reg:hasSubproperty <http://rdaregistry.info/Elements/u/P60636> ;
	reg:name "distributorOf"@en ;
	reg:status status:1001 ;
	a rdf:Property ;
	rdfs:isDefinedBy <http://rdaregistry.info/Elements/u/> ;
	rdfs:label "is distributor of"@en ;
	owl:inverseOf <http://rdaregistry.info/Elements/u/P60438> ;
	owl:sameAs <http://rdaregistry.info/Elements/u/distributorOf> ;
	skos:definition "Relates an agent responsible for distributing a resource to the resource."@en .

<http://rdaregistry.info/Elements/u/P60668> reg:hasSubproperty <http://rdaregistry.info/Elements/a/P50201> , <http://rdaregistry.info/Elements/u/P60033> , <http://rdaregistry.info/Elements/u/P60034> , <http://rdaregistry.info/Elements/u/P60035> ;
	reg:name "producerOf"@en ;
	reg:status status:1001 ;
	a rdf:Property ;
	rdfs:isDefinedBy <http://rdaregistry.info/Elements/u/> ;
	rdfs:label "is producer of"@en ;
	rdfs:subPropertyOf <http://rdaregistry.info/Elements/u/P60602> ;
	owl:inverseOf <http://rdaregistry.info/Elements/u/P60441> ;
	owl:sameAs <http://rdaregistry.info/Elements/u/producerOf> ;
	skos:definition "Relates an agent responsible for most of the business aspects of a production for screen, sound recording, television, webcast, etc. the producer is generally responsible for fund raising, managing the production, hiring key personnel, arranging for distributors, etc. to the resource."@en .

<http://rdaregistry.info/Elements/u/P60669> reg:hasSubproperty <http://rdaregistry.info/Elements/u/P60637> , <http://rdaregistry.info/Elements/u/P60638> , <http://rdaregistry.info/Elements/u/P60639> , <http://rdaregistry.info/Elements/u/P60640> , <http://rdaregistry.info/Elements/u/P60641> , <http://rdaregistry.info/Elements/u/P60642> , <http://rdaregistry.info/Elements/u/P60643> , <http://rdaregistry.info/Elements/u/P60644> , <http://rdaregistry.info/Elements/u/P60645> , <http://rdaregistry.info/Elements/u/P60646> ;
	reg:name "manufacturerOf"@en ;
	reg:status status:1001 ;
	a rdf:Property ;
	rdfs:isDefinedBy <http://rdaregistry.info/Elements/u/> ;
	rdfs:label "is manufacturer of"@en ;
	owl:inverseOf <http://rdaregistry.info/Elements/u/P60443> ;
	owl:sameAs <http://rdaregistry.info/Elements/u/manufacturerOf> ;
	skos:definition "Relates an agent responsible for printing, duplicating, casting, etc., a resource in a published form to the resource."@en .

<http://rdaregistry.info/Elements/u/P60670> reg:hasSubproperty <http://rdaregistry.info/Elements/u/P60635> ;
	reg:name "publisherOf"@en ;
	reg:status status:1001 ;
	a rdf:Property ;
	rdfs:isDefinedBy <http://rdaregistry.info/Elements/u/> ;
	rdfs:label "is publisher of"@en ;
	owl:inverseOf <http://rdaregistry.info/Elements/u/P60444> ;
	owl:sameAs <http://rdaregistry.info/Elements/u/publisherOf> ;
	skos:definition "Relates an agent responsible for publishing, releasing, or issuing a resource to the resource."@en .

<http://rdaregistry.info/Elements/u/P60671> reg:hasSubproperty <http://rdaregistry.info/Elements/a/P50212> ;
	reg:name "minuteTakerOf"@en ;
	reg:status status:1001 ;
	a rdf:Property ;
	rdfs:isDefinedBy <http://rdaregistry.info/Elements/u/> ;
	rdfs:label "is minute taker of"@en ;
	rdfs:subPropertyOf <http://rdaregistry.info/Elements/u/P60626> ;
	owl:inverseOf <http://rdaregistry.info/Elements/u/P60446> ;
	owl:sameAs <http://rdaregistry.info/Elements/u/minuteTakerOf> ;
	skos:definition "Relates an agent responsible for recording the minutes of a meeting to the resource."@en .

<http://rdaregistry.info/Elements/u/P60672> reg:hasSubproperty <http://rdaregistry.info/Elements/u/P60001> , <http://rdaregistry.info/Elements/u/P60014> , <http://rdaregistry.info/Elements/u/P60649> , <http://rdaregistry.info/Elements/u/P60652> , <http://rdaregistry.info/Elements/u/P60653> , <http://rdaregistry.info/Elements/u/P60654> , <http://rdaregistry.info/Elements/u/P60655> , <http://rdaregistry.info/Elements/u/P60656> , <http://rdaregistry.info/Elements/u/P60657> , <http://rdaregistry.info/Elements/u/P60658> , <http://rdaregistry.info/Elements/u/P60659> , <http://rdaregistry.info/Elements/u/P60660> , <http://rdaregistry.info/Elements/u/P60661> , <http://rdaregistry.info/Elements/u/P60662> , <http://rdaregistry.info/Elements/u/P60663> , <http://rdaregistry.info/Elements/u/P60664> , <http://rdaregistry.info/Elements/u/P60665> , <http://rdaregistry.info/Elements/u/P60699> , <http://rdaregistry.info/Elements/u/P60701> ;
	reg:name "creatorOf"@en ;
	reg:status status:1001 ;
	a rdf:Property ;
	rdfs:isDefinedBy <http://rdaregistry.info/Elements/u/> ;
	rdfs:label "is creator of"@en ;
	owl:inverseOf <http://rdaregistry.info/Elements/u/P60447> ;
	owl:sameAs <http://rdaregistry.info/Elements/u/creatorOf> ;
	skos:definition "Relates an agent responsible for the creation of a resourc to the resource."@en .

<http://rdaregistry.info/Elements/u/P60673> reg:name "directorOf"@en ;
	reg:status status:1001 ;
	a rdf:Property ;
	rdfs:isDefinedBy <http://rdaregistry.info/Elements/u/> ;
	rdfs:label "is director of"@en ;
	rdfs:subPropertyOf <http://rdaregistry.info/Elements/u/P60602> ;
	owl:inverseOf <http://rdaregistry.info/Elements/u/P60449> ;
	owl:sameAs <http://rdaregistry.info/Elements/u/directorOf> ;
	skos:definition "Relates an agent responsible for the general management and supervision of a filmed performance, a radio or television program, etc. to the resource."@en .

<http://rdaregistry.info/Elements/u/P60674> reg:hasSubproperty <http://rdaregistry.info/Elements/a/P50206> ;
	reg:name "restorationistOf"@en ;
	reg:status status:1001 ;
	a rdf:Property ;
	rdfs:isDefinedBy <http://rdaregistry.info/Elements/u/> ;
	rdfs:label "is restorationist of"@en ;
	rdfs:subPropertyOf <http://rdaregistry.info/Elements/u/P60602> ;
	owl:inverseOf <http://rdaregistry.info/Elements/u/P60450> ;
	owl:sameAs <http://rdaregistry.info/Elements/u/restorationistOf> ;
	skos:definition "Relates an agent responsible for the set of technical, editorial, and intellectual procedures aimed at compensating for the degradation of a resource by bringing it back to a state as close as possible to its original condition to the resource."@en .

<http://rdaregistry.info/Elements/u/P60675> reg:hasSubproperty <http://rdaregistry.info/Elements/a/P50226> ;
	reg:name "sponsoringBodyOf"@en ;
	reg:status status:1001 ;
	a rdf:Property ;
	rdfs:isDefinedBy <http://rdaregistry.info/Elements/u/> ;
	rdfs:label "is sponsoring body of"@en ;
	rdfs:subPropertyOf <http://rdaregistry.info/Elements/u/P60602> ;
	owl:inverseOf <http://rdaregistry.info/Elements/u/P60451> ;
	owl:sameAs <http://rdaregistry.info/Elements/u/sponsoringBodyOf> ;
	skos:definition "Relates an agent sponsoring some aspect of a resource, e.g., funding research, sponsoring an event to the resource."@en .

<http://rdaregistry.info/Elements/u/P60676> reg:hasSubproperty <http://rdaregistry.info/Elements/a/P50028> ;
	reg:name "sponsor"@en ;
	reg:status status:1001 ;
	a rdf:Property ;
	rdfs:isDefinedBy <http://rdaregistry.info/Elements/u/> ;
	rdfs:label "has sponsor"@en ;
	owl:inverseOf <http://rdaregistry.info/Elements/u/P60688> ;
	owl:sameAs <http://rdaregistry.info/Elements/u/sponsor> ;
	skos:closeMatch "http://id.loc.gov/vocabulary/relators/spn"@en ;
	skos:definition "Relates an agent sponsoring the agent to the agent."@en .

<http://rdaregistry.info/Elements/u/P60678> reg:hasSubproperty <http://rdaregistry.info/Elements/a/P50207> ;
	reg:name "directorOfPhotographyOf"@en ;
	reg:status status:1001 ;
	a rdf:Property ;
	rdfs:isDefinedBy <http://rdaregistry.info/Elements/u/> ;
	rdfs:label "is director of photography of"@en ;
	rdfs:subPropertyOf <http://rdaregistry.info/Elements/u/P60602> ;
	owl:inverseOf <http://rdaregistry.info/Elements/u/P60452> ;
	owl:sameAs <http://rdaregistry.info/Elements/u/directorOfPhotographyOf> ;
	skos:definition "Relates an agent that captures images, either electronically or on film or video stock, and often selects and arranges the lighting. the director of photography for a movie is also called the chief cinematographer to the resource."@en .

<http://rdaregistry.info/Elements/u/P60679> reg:hasSubproperty <http://rdaregistry.info/Elements/a/P50096> ;
	reg:name "employer"@en ;
	reg:status status:1001 ;
	a rdf:Property ;
	rdfs:isDefinedBy <http://rdaregistry.info/Elements/u/> ;
	rdfs:label "has employer"@en ;
	owl:inverseOf <http://rdaregistry.info/Elements/u/P60629> ;
	owl:sameAs <http://rdaregistry.info/Elements/u/employer> ;
	skos:definition "Relates an agent that employs the agent to the agent."@en .

<http://rdaregistry.info/Elements/u/P60680> reg:name "hierarchicalSuperior"@en ;
	reg:status status:1001 ;
	a rdf:Property ;
	rdfs:isDefinedBy <http://rdaregistry.info/Elements/u/> ;
	rdfs:label "has hierarchical superior"@en ;
	owl:inverseOf <http://rdaregistry.info/Elements/u/P60681> ;
	owl:sameAs <http://rdaregistry.info/Elements/u/hierarchicalSuperior> ;
	skos:definition "Relates an agent that is hierarchically superior to the other agent to the agent."@en .

<http://rdaregistry.info/Elements/u/P60681> reg:name "hierarchicalSubordinate"@en ;
	reg:status status:1001 ;
	a rdf:Property ;
	rdfs:isDefinedBy <http://rdaregistry.info/Elements/u/> ;
	rdfs:label "has hierarchical subordinate"@en ;
	owl:inverseOf <http://rdaregistry.info/Elements/u/P60680> ;
	owl:sameAs <http://rdaregistry.info/Elements/u/hierarchicalSubordinate> ;
	skos:definition "Relates an agent that is subordinate to the other agent to the agent."@en .

<http://rdaregistry.info/Elements/u/P60682> reg:name "mergee"@en ;
	reg:status status:1001 ;
	a rdf:Property ;
	rdfs:isDefinedBy <http://rdaregistry.info/Elements/u/> ;
	rdfs:label "has mergee"@en ;
	owl:inverseOf <http://rdaregistry.info/Elements/u/P60682> ;
	owl:sameAs <http://rdaregistry.info/Elements/u/mergee> ;
	skos:definition "Relates an agent that merged with the other agent to form a third to the agent."@en .

<http://rdaregistry.info/Elements/u/P60683> reg:hasSubproperty <http://rdaregistry.info/Elements/a/P50055> ;
	reg:name "predecessor"@en ;
	reg:status status:1001 ;
	a rdf:Property ;
	rdfs:isDefinedBy <http://rdaregistry.info/Elements/u/> ;
	rdfs:label "has predecessor"@en ;
	owl:inverseOf <http://rdaregistry.info/Elements/u/P60686> ;
	owl:sameAs <http://rdaregistry.info/Elements/u/predecessor> ;
	skos:definition "Relates an agent that precedes the other agent to the agent."@en .

<http://rdaregistry.info/Elements/u/P60684> reg:name "productOfAMerger"@en ;
	reg:status status:1001 ;
	a rdf:Property ;
	rdfs:isDefinedBy <http://rdaregistry.info/Elements/u/> ;
	rdfs:label "has product of merger"@en ;
	owl:inverseOf <http://rdaregistry.info/Elements/u/P60736> ;
	owl:sameAs <http://rdaregistry.info/Elements/u/productOfAMerger> ;
	skos:definition "Relates an agent that resulted from a merger of two or more other agents to the agent."@en .

<http://rdaregistry.info/Elements/u/P60685> reg:name "productOfASplit"@en ;
	reg:status status:1001 ;
	a rdf:Property ;
	rdfs:isDefinedBy <http://rdaregistry.info/Elements/u/> ;
	rdfs:label "has product of split"@en ;
	owl:inverseOf <http://rdaregistry.info/Elements/u/P60733> ;
	owl:sameAs <http://rdaregistry.info/Elements/u/productOfASplit> ;
	skos:definition "Relates an agent that resulted from a split or division of the other agent to the agent."@en .

<http://rdaregistry.info/Elements/u/P60686> reg:hasSubproperty <http://rdaregistry.info/Elements/a/P50053> , <http://rdaregistry.info/Elements/a/P50099> ;
	reg:name "successor"@en ;
	reg:status status:1001 ;
	a rdf:Property ;
	rdfs:isDefinedBy <http://rdaregistry.info/Elements/u/> ;
	rdfs:label "has successor"@en ;
	owl:inverseOf <http://rdaregistry.info/Elements/u/P60683> ;
	owl:sameAs <http://rdaregistry.info/Elements/u/successor> ;
	skos:definition "Relates an agent that succeeds or follows the other agent to the agent."@en .

<http://rdaregistry.info/Elements/u/P60687> reg:hasSubproperty <http://rdaregistry.info/Elements/a/P50062> , <http://rdaregistry.info/Elements/a/P50112> ;
	reg:name "foundedEntity"@en ;
	reg:status status:1001 ;
	a rdf:Property ;
	rdfs:isDefinedBy <http://rdaregistry.info/Elements/u/> ;
	rdfs:label "has founded entity"@en ;
	owl:inverseOf <http://rdaregistry.info/Elements/u/P60694> ;
	owl:sameAs <http://rdaregistry.info/Elements/u/foundedEntity> ;
	skos:definition "Relates an agent that the agent founded to the agent."@en .

<http://rdaregistry.info/Elements/u/P60688> reg:hasSubproperty <http://rdaregistry.info/Elements/a/P50063> ;
	reg:name "sponsoredEntity"@en ;
	reg:status status:1001 ;
	a rdf:Property ;
	rdfs:isDefinedBy <http://rdaregistry.info/Elements/u/> ;
	rdfs:label "has sponsored entity"@en ;
	owl:inverseOf <http://rdaregistry.info/Elements/u/P60676> ;
	owl:sameAs <http://rdaregistry.info/Elements/u/sponsoredEntity> ;
	skos:definition "Relates an agent that the agent sponsors to the agent."@en .

<http://rdaregistry.info/Elements/u/P60689> reg:hasSubproperty <http://rdaregistry.info/Elements/a/P50208> , <http://rdaregistry.info/Elements/a/P50210> ;
	reg:name "dedicateeOf"@en ;
	reg:status status:1001 ;
	a rdf:Property ;
	rdfs:isDefinedBy <http://rdaregistry.info/Elements/u/> ;
	rdfs:label "is dedicatee of"@en ;
	rdfs:subPropertyOf <http://rdaregistry.info/Elements/u/P60602> ;
	owl:inverseOf <http://rdaregistry.info/Elements/u/P60455> ;
	owl:sameAs <http://rdaregistry.info/Elements/u/dedicateeOf> ;
	skos:definition "Relates an agent to whom a resource is dedicated to the resource."@en .

<http://rdaregistry.info/Elements/u/P60690> reg:hasSubproperty <http://rdaregistry.info/Elements/a/P50209> ;
	reg:name "addresseeOf"@en ;
	reg:status status:1001 ;
	a rdf:Property ;
	rdfs:isDefinedBy <http://rdaregistry.info/Elements/u/> ;
	rdfs:label "is addressee of"@en ;
	rdfs:subPropertyOf <http://rdaregistry.info/Elements/u/P60602> ;
	owl:inverseOf <http://rdaregistry.info/Elements/u/P60456> ;
	owl:sameAs <http://rdaregistry.info/Elements/u/addresseeOf> ;
	skos:definition "Relates an agent to whom a resource or part of a resource is addressed to the resource."@en .

<http://rdaregistry.info/Elements/u/P60691> reg:hasSubproperty <http://rdaregistry.info/Elements/a/P50042> , <http://rdaregistry.info/Elements/a/P50088> , <http://rdaregistry.info/Elements/a/P50122> ;
	reg:name "appellantOf"@en ;
	reg:status status:1001 ;
	a rdf:Property ;
	rdfs:isDefinedBy <http://rdaregistry.info/Elements/u/> ;
	rdfs:label "is appellant of"@en ;
	rdfs:subPropertyOf <http://rdaregistry.info/Elements/u/P60602> ;
	owl:inverseOf <http://rdaregistry.info/Elements/u/P60457> ;
	owl:sameAs <http://rdaregistry.info/Elements/u/appellantOf> ;
	skos:definition "Relates an agent who appeals a lower court’s decision to the resource."@en .

<http://rdaregistry.info/Elements/u/P60692> reg:hasSubproperty <http://rdaregistry.info/Elements/a/P50123> ;
	reg:name "binderOf"@en ;
	reg:status status:1001 ;
	a rdf:Property ;
	rdfs:isDefinedBy <http://rdaregistry.info/Elements/u/> ;
	rdfs:label "is binder of"@en ;
	rdfs:subPropertyOf <http://rdaregistry.info/Elements/u/P60602> ;
	owl:inverseOf <http://rdaregistry.info/Elements/u/P60458> ;
	owl:sameAs <http://rdaregistry.info/Elements/u/binderOf> ;
	skos:definition "Relates an agent who binds a resource to the resource."@en .

<http://rdaregistry.info/Elements/u/P60693> reg:hasSubproperty <http://rdaregistry.info/Elements/a/P50043> , <http://rdaregistry.info/Elements/a/P50089> , <http://rdaregistry.info/Elements/a/P50124> ;
	reg:name "plaintiffOf"@en ;
	reg:status status:1001 ;
	a rdf:Property ;
	rdfs:isDefinedBy <http://rdaregistry.info/Elements/u/> ;
	rdfs:label "is plaintiff of"@en ;
	rdfs:subPropertyOf <http://rdaregistry.info/Elements/u/P60602> ;
	owl:inverseOf <http://rdaregistry.info/Elements/u/P60459> ;
	owl:sameAs <http://rdaregistry.info/Elements/u/plaintiffOf> ;
	skos:definition "Relates an agent who brings a suit in a civil proceeding to the resource."@en .

<http://rdaregistry.info/Elements/u/P60694> reg:hasSubproperty <http://rdaregistry.info/Elements/a/P50029> ;
	reg:name "founder"@en ;
	reg:status status:1001 ;
	a rdf:Property ;
	rdfs:isDefinedBy <http://rdaregistry.info/Elements/u/> ;
	rdfs:label "has founder"@en ;
	owl:inverseOf <http://rdaregistry.info/Elements/u/P60687> ;
	owl:sameAs <http://rdaregistry.info/Elements/u/founder> ;
	skos:definition "Relates an agent who founded the agent to the agent."@en .

<http://rdaregistry.info/Elements/u/P60695> reg:hasSubproperty <http://rdaregistry.info/Elements/a/P50125> ;
	reg:name "inscriberOf"@en ;
	reg:status status:1001 ;
	a rdf:Property ;
	rdfs:isDefinedBy <http://rdaregistry.info/Elements/u/> ;
	rdfs:label "is inscriber of"@en ;
	rdfs:subPropertyOf <http://rdaregistry.info/Elements/u/P60602> ;
	owl:inverseOf <http://rdaregistry.info/Elements/u/P60460> ;
	owl:sameAs <http://rdaregistry.info/Elements/u/inscriberOf> ;
	skos:definition "Relates an agent who has written a statement of dedication or gift on a resource to the resource."@en .

<http://rdaregistry.info/Elements/u/P60696> reg:hasSubproperty <http://rdaregistry.info/Elements/a/P50126> ;
	reg:name "judgeOf"@en ;
	reg:status status:1001 ;
	a rdf:Property ;
	rdfs:isDefinedBy <http://rdaregistry.info/Elements/u/> ;
	rdfs:label "is judge of"@en ;
	rdfs:subPropertyOf <http://rdaregistry.info/Elements/u/P60602> ;
	owl:inverseOf <http://rdaregistry.info/Elements/u/P60461> ;
	owl:sameAs <http://rdaregistry.info/Elements/u/judgeOf> ;
	skos:definition "Relates an agent who hears and decides on legal matters in court to the resource."@en .

<http://rdaregistry.info/Elements/u/P60697> reg:hasSubproperty <http://rdaregistry.info/Elements/a/P50030> ;
	reg:name "member"@en ;
	reg:status status:1001 ;
	a rdf:Property ;
	rdfs:isDefinedBy <http://rdaregistry.info/Elements/u/> ;
	rdfs:label "has member"@en ;
	owl:inverseOf <http://rdaregistry.info/Elements/u/P60648> ;
	owl:sameAs <http://rdaregistry.info/Elements/u/member> ;
	skos:definition "Relates an agent who is a member of the agent to the agent."@en .

<http://rdaregistry.info/Elements/u/P60698> reg:hasSubproperty <http://rdaregistry.info/Elements/a/P50090> ;
	reg:name "defendantOf"@en ;
	reg:status status:1001 ;
	a rdf:Property ;
	rdfs:isDefinedBy <http://rdaregistry.info/Elements/u/> ;
	rdfs:label "is defendant of"@en ;
	rdfs:subPropertyOf <http://rdaregistry.info/Elements/u/P60602> ;
	owl:inverseOf <http://rdaregistry.info/Elements/u/P60462> ;
	owl:sameAs <http://rdaregistry.info/Elements/u/defendantOf> ;
	skos:definition "Relates an agent who is accused in a criminal proceeding or sued in a civil proceeding to the resource."@en .

<http://rdaregistry.info/Elements/u/P60699> reg:hasSubproperty <http://rdaregistry.info/Elements/a/P50127> ;
	reg:name "praesesOf"@en ;
	reg:status status:1001 ;
	a rdf:Property ;
	rdfs:isDefinedBy <http://rdaregistry.info/Elements/u/> ;
	rdfs:label "is praeses of"@en ;
	rdfs:subPropertyOf <http://rdaregistry.info/Elements/u/P60672> ;
	owl:inverseOf <http://rdaregistry.info/Elements/u/P60463> ;
	owl:sameAs <http://rdaregistry.info/Elements/u/praesesOf> ;
	skos:definition "Relates an agent who is the faculty moderator of an academic disputation, normally proposing a thesis and participating in the ensuing disputation to the resource."@en .

<http://rdaregistry.info/Elements/u/P60700> reg:hasSubproperty <http://rdaregistry.info/Elements/a/P50128> ;
	reg:name "annotatorOf"@en ;
	reg:status status:1001 ;
	a rdf:Property ;
	rdfs:isDefinedBy <http://rdaregistry.info/Elements/u/> ;
	rdfs:label "is annotator of"@en ;
	rdfs:subPropertyOf <http://rdaregistry.info/Elements/u/P60602> ;
	owl:inverseOf <http://rdaregistry.info/Elements/u/P60464> ;
	owl:sameAs <http://rdaregistry.info/Elements/u/annotatorOf> ;
	skos:definition "Relates an agent who makes manuscript annotations on a resource to the resource."@en .

<http://rdaregistry.info/Elements/u/P60701> reg:hasSubproperty <http://rdaregistry.info/Elements/a/P50211> ;
	reg:name "consultantOf"@en ;
	reg:status status:1001 ;
	a rdf:Property ;
	rdfs:isDefinedBy <http://rdaregistry.info/Elements/u/> ;
	rdfs:label "is consultant of"@en ;
	rdfs:subPropertyOf <http://rdaregistry.info/Elements/u/P60672> ;
	owl:inverseOf <http://rdaregistry.info/Elements/u/P60465> ;
	owl:sameAs <http://rdaregistry.info/Elements/u/consultantOf> ;
	skos:definition "Relates an agent who provides consultation services, and often makes recommendations, for another person, family or corporate body that is represented as the creator of a resource to the resource."@en .

<http://rdaregistry.info/Elements/u/P60702> reg:hasSubproperty <http://rdaregistry.info/Elements/a/P50129> ;
	reg:name "autographerOf"@en ;
	reg:status status:1001 ;
	a rdf:Property ;
	rdfs:isDefinedBy <http://rdaregistry.info/Elements/u/> ;
	rdfs:label "is autographer of"@en ;
	rdfs:subPropertyOf <http://rdaregistry.info/Elements/u/P60602> ;
	owl:inverseOf <http://rdaregistry.info/Elements/u/P60466> ;
	owl:sameAs <http://rdaregistry.info/Elements/u/autographerOf> ;
	skos:definition "Relates an agent whose manuscript signature appears on a resource to the resource."@en .

<http://rdaregistry.info/Elements/u/P60703> reg:hasSubproperty <http://rdaregistry.info/Elements/a/P50130> ;
	reg:name "issuingBodyOf"@en ;
	reg:status status:1001 ;
	a rdf:Property ;
	rdfs:isDefinedBy <http://rdaregistry.info/Elements/u/> ;
	rdfs:label "is issuing body of"@en ;
	rdfs:subPropertyOf <http://rdaregistry.info/Elements/u/P60602> ;
	owl:inverseOf <http://rdaregistry.info/Elements/u/P60467> ;
	owl:sameAs <http://rdaregistry.info/Elements/u/issuingBodyOf> ;
	skos:definition "Relates an agent, family or corporate body issuing a resource, such as an official organ of the body to the resource."@en .

<http://rdaregistry.info/Elements/u/P60704> reg:hasSubproperty <http://rdaregistry.info/Elements/a/P50221> ;
	reg:name "landscapeArchitectOf"@en ;
	reg:status status:1001 ;
	a rdf:Property ;
	rdfs:isDefinedBy <http://rdaregistry.info/Elements/u/> ;
	rdfs:label "is landscape architect of"@en ;
	rdfs:subPropertyOf <http://rdaregistry.info/Elements/u/P60664> ;
	owl:inverseOf <http://rdaregistry.info/Elements/u/P60473> ;
	owl:sameAs <http://rdaregistry.info/Elements/u/landscapeArchitectOf> ;
	skos:definition "Relates an architect responsible for creating landscape resources to the resource."@en .

<http://rdaregistry.info/Elements/u/P60705> reg:hasSubproperty <http://rdaregistry.info/Elements/a/P50222> ;
	reg:name "sculptorOf"@en ;
	reg:status status:1001 ;
	a rdf:Property ;
	rdfs:isDefinedBy <http://rdaregistry.info/Elements/u/> ;
	rdfs:label "is sculptor of"@en ;
	rdfs:subPropertyOf <http://rdaregistry.info/Elements/u/P60660> ;
	owl:inverseOf <http://rdaregistry.info/Elements/u/P60475> ;
	owl:sameAs <http://rdaregistry.info/Elements/u/sculptorOf> ;
	skos:definition "Relates an artist responsible for creating a three-dimensional resource by modeling, carving, or similar technique to the resource."@en .

<http://rdaregistry.info/Elements/u/P60706> reg:hasSubproperty <http://rdaregistry.info/Elements/a/P50223> ;
	reg:name "screenwriterOf"@en ;
	reg:status status:1001 ;
	a rdf:Property ;
	rdfs:isDefinedBy <http://rdaregistry.info/Elements/u/> ;
	rdfs:label "is screenwriter of"@en ;
	rdfs:subPropertyOf <http://rdaregistry.info/Elements/u/P60663> ;
	owl:inverseOf <http://rdaregistry.info/Elements/u/P60476> ;
	owl:sameAs <http://rdaregistry.info/Elements/u/screenwriterOf> ;
	skos:definition "Relates an author of a screenplay, script, or scene to the resource."@en .

<http://rdaregistry.info/Elements/u/P60707> reg:hasSubproperty <http://rdaregistry.info/Elements/a/P50224> ;
	reg:name "lyricistOf"@en ;
	reg:status status:1001 ;
	a rdf:Property ;
	rdfs:isDefinedBy <http://rdaregistry.info/Elements/u/> ;
	rdfs:label "is lyricist of"@en ;
	rdfs:subPropertyOf <http://rdaregistry.info/Elements/u/P60663> ;
	owl:inverseOf <http://rdaregistry.info/Elements/u/P60477> ;
	owl:sameAs <http://rdaregistry.info/Elements/u/lyricistOf> ;
	skos:definition "Relates an author of the words of a popular song, including a song or songs from a musical to the resource."@en .

<http://rdaregistry.info/Elements/u/P60708> reg:hasSubproperty <http://rdaregistry.info/Elements/a/P50225> ;
	reg:name "librettistOf"@en ;
	reg:status status:1001 ;
	a rdf:Property ;
	rdfs:isDefinedBy <http://rdaregistry.info/Elements/u/> ;
	rdfs:label "is librettist of"@en ;
	rdfs:subPropertyOf <http://rdaregistry.info/Elements/u/P60663> ;
	owl:inverseOf <http://rdaregistry.info/Elements/u/P60478> ;
	owl:sameAs <http://rdaregistry.info/Elements/u/librettistOf> ;
	skos:definition "Relates an author of the words of an opera or other musical stage resource or an oratorio to the resource."@en .

<http://rdaregistry.info/Elements/u/P60709> reg:hasSubproperty <http://rdaregistry.info/Elements/e/P20232> , <http://rdaregistry.info/Elements/i/P40051> , <http://rdaregistry.info/Elements/m/P30210> , <http://rdaregistry.info/Elements/u/P60196> , <http://rdaregistry.info/Elements/u/P60198> , <http://rdaregistry.info/Elements/u/P60204> , <http://rdaregistry.info/Elements/u/P60307> , <http://rdaregistry.info/Elements/w/P10228> ;
	reg:name "accompanyingResourceRelationshipWith"@en ;
	reg:status status:1001 ;
	a rdf:Property ;
	rdfs:isDefinedBy <http://rdaregistry.info/Elements/u/> ;
	rdfs:label "has accompanying resource relationship with"@en ;
	owl:inverseOf <http://rdaregistry.info/Elements/u/P60709> ;
	owl:sameAs <http://rdaregistry.info/Elements/u/accompanyingRelationship> , <http://rdaregistry.info/Elements/u/accompanyingResourceRelationshipWith> ;
	skos:definition "Relates a resource to a resource that is an augmentation of, or is augmented by, or is complemented by, or accompanies, or is accompanied by the resource."@en .

<http://rdaregistry.info/Elements/u/P60710> reg:hasSubproperty <http://rdaregistry.info/Elements/e/P20233> , <http://rdaregistry.info/Elements/u/P60250> , <http://rdaregistry.info/Elements/u/P60305> , <http://rdaregistry.info/Elements/w/P10229> ;
	reg:name "derivativeResourceRelationshipWith"@en ;
	reg:status status:1001 ;
	a rdf:Property ;
	rdfs:isDefinedBy <http://rdaregistry.info/Elements/u/> ;
	rdfs:label "has derivative resource relationship with"@en ;
	owl:inverseOf <http://rdaregistry.info/Elements/u/P60710> ;
	owl:sameAs <http://rdaregistry.info/Elements/u/derivativeRelationship> , <http://rdaregistry.info/Elements/u/derivativeResourceRelationshipWith> ;
	skos:definition "Relates a resource to a resource that is based on or is a derivative of the resource."@en .

<http://rdaregistry.info/Elements/u/P60711> reg:hasSubproperty <http://rdaregistry.info/Elements/e/P20234> , <http://rdaregistry.info/Elements/i/P40052> , <http://rdaregistry.info/Elements/m/P30211> , <http://rdaregistry.info/Elements/u/P60190> , <http://rdaregistry.info/Elements/u/P60215> , <http://rdaregistry.info/Elements/w/P10230> ;
	reg:name "descriptiveResourceRelationshipWith"@en ;
	reg:status status:1001 ;
	a rdf:Property ;
	rdfs:isDefinedBy <http://rdaregistry.info/Elements/u/> ;
	rdfs:label "has descriptive resource relationship with"@en ;
	owl:inverseOf <http://rdaregistry.info/Elements/u/P60711> ;
	owl:sameAs <http://rdaregistry.info/Elements/u/descriptiveRelationship> , <http://rdaregistry.info/Elements/u/descriptiveResourceRelationshipWith> ;
	skos:definition "Relates a resource to a resource that is described in or is a description of the resource."@en .

<http://rdaregistry.info/Elements/u/P60712> reg:hasSubproperty <http://rdaregistry.info/Elements/i/P40053> , <http://rdaregistry.info/Elements/u/P60191> ;
	reg:name "equivalentResourceRelationshipWith"@en ;
	reg:status status:1001 ;
	a rdf:Property ;
	rdfs:isDefinedBy <http://rdaregistry.info/Elements/u/> ;
	rdfs:label "has equivalent resource relationship with"@en ;
	owl:inverseOf <http://rdaregistry.info/Elements/u/P60712> ;
	owl:sameAs <http://rdaregistry.info/Elements/u/equivalentRelationship> , <http://rdaregistry.info/Elements/u/equivalentResourceRelationshipWith> ;
	skos:definition "Relates a resource to a resource that is equivalent to the resource."@en .

<http://rdaregistry.info/Elements/u/P60713> reg:hasSubproperty <http://rdaregistry.info/Elements/u/P60261> , <http://rdaregistry.info/Elements/u/P60278> ;
	reg:name "sequentialResourceRelationshipWith"@en ;
	reg:status status:1001 ;
	a rdf:Property ;
	rdfs:isDefinedBy <http://rdaregistry.info/Elements/u/> ;
	rdfs:label "has sequential resource relationship with"@en ;
	owl:inverseOf <http://rdaregistry.info/Elements/u/P60713> ;
	owl:sameAs <http://rdaregistry.info/Elements/u/sequentialRelationship> , <http://rdaregistry.info/Elements/u/sequentialResourceRelationshipWith> ;
	skos:definition "Relates a resource to a resource that is preceded by or succeeded by the resource."@en .

<http://rdaregistry.info/Elements/u/P60714> reg:hasSubproperty <http://rdaregistry.info/Elements/u/P60101> , <http://rdaregistry.info/Elements/u/P60249> , <http://rdaregistry.info/Elements/w/P10232> ;
	reg:name "wholePartResourceRelationshipWith"@en ;
	reg:status status:1001 ;
	a rdf:Property ;
	rdfs:isDefinedBy <http://rdaregistry.info/Elements/u/> ;
	rdfs:label "has whole-part resource relationship with"@en ;
	owl:inverseOf <http://rdaregistry.info/Elements/u/P60714> ;
	owl:sameAs <http://rdaregistry.info/Elements/u/wholePartRelationship> , <http://rdaregistry.info/Elements/u/wholePartResourceRelationshipWith> ;
	skos:definition "Relates a resource to a resource that is contained in or contains the resource."@en .

<http://rdaregistry.info/Elements/u/P60715> reg:name "writerOfAfterword"@en ;
	reg:status status:1001 ;
	a rdf:Property ;
	rdfs:isDefinedBy <http://rdaregistry.info/Elements/u/> ;
	rdfs:label "has writer of afterword"@en ;
	rdfs:subPropertyOf <http://rdaregistry.info/Elements/u/P60392> ;
	owl:inverseOf <http://rdaregistry.info/Elements/u/P60717> ;
	owl:sameAs <http://rdaregistry.info/Elements/u/writerOfAfterword> ;
	skos:definition "Relates a resource to an agent contributing to a resource by providing an afterword to the original resource."@en .

<http://rdaregistry.info/Elements/u/P60716> reg:name "writerOfPostface"@en ;
	reg:status status:1001 ;
	a rdf:Property ;
	rdfs:isDefinedBy <http://rdaregistry.info/Elements/u/> ;
	rdfs:label "has writer of postface"@en ;
	rdfs:subPropertyOf <http://rdaregistry.info/Elements/u/P60392> ;
	owl:inverseOf <http://rdaregistry.info/Elements/u/P60718> ;
	owl:sameAs <http://rdaregistry.info/Elements/u/writerOfPostface> ;
	skos:definition "Relates a resource to an agent contributing to a resource by providing a postface to the original resource."@en .

<http://rdaregistry.info/Elements/u/P60717> reg:name "writerOfAfterwordOf"@en ;
	reg:status status:1001 ;
	a rdf:Property ;
	rdfs:isDefinedBy <http://rdaregistry.info/Elements/u/> ;
	rdfs:label "is writer of afterword of"@en ;
	rdfs:subPropertyOf <http://rdaregistry.info/Elements/u/P60620> ;
	owl:inverseOf <http://rdaregistry.info/Elements/u/P60715> ;
	owl:sameAs <http://rdaregistry.info/Elements/u/writerOfAfterwordOf> ;
	skos:definition "Relates an agent contributing to a resource by providing an afterword to the original resource to the resource."@en .

<http://rdaregistry.info/Elements/u/P60718> reg:name "writerOfPostfaceOf"@en ;
	reg:status status:1001 ;
	a rdf:Property ;
	rdfs:isDefinedBy <http://rdaregistry.info/Elements/u/> ;
	rdfs:label "is writer of postface of"@en ;
	rdfs:subPropertyOf <http://rdaregistry.info/Elements/u/P60620> ;
	owl:inverseOf <http://rdaregistry.info/Elements/u/P60716> ;
	owl:sameAs <http://rdaregistry.info/Elements/u/writerOfPostfaceOf> ;
	skos:definition "Relates an agent contributing to a resource by providing a postface to the original resource to the resource."@en .

<http://rdaregistry.info/Elements/u/P60719> reg:name "musicalTheatreAdaptationOf"@en ;
	reg:status status:1001 ;
	a rdf:Property ;
	rdfs:isDefinedBy <http://rdaregistry.info/Elements/u/> ;
	rdfs:label "is musical theatre adaptation of"@en ;
	rdfs:subPropertyOf <http://rdaregistry.info/Elements/u/P60241> ;
	owl:inverseOf <http://rdaregistry.info/Elements/u/P60721> ;
	owl:sameAs <http://rdaregistry.info/Elements/u/musicalTheatreAdaptationOf> ;
	skos:definition "Relates a resource to a resource that has been adapted as a musical theatre resource."@en .

<http://rdaregistry.info/Elements/u/P60720> reg:name "operaAdaptationOf"@en ;
	reg:status status:1001 ;
	a rdf:Property ;
	rdfs:isDefinedBy <http://rdaregistry.info/Elements/u/> ;
	rdfs:label "is opera adaptation of"@en ;
	rdfs:subPropertyOf <http://rdaregistry.info/Elements/u/P60241> ;
	owl:inverseOf <http://rdaregistry.info/Elements/u/P60722> ;
	owl:sameAs <http://rdaregistry.info/Elements/u/operaAdaptationOf> ;
	skos:definition "Relates a resource to a resource that has been adapted as opera."@en .

<http://rdaregistry.info/Elements/u/P60721> reg:name "adaptedAsMusicalTheatre"@en ;
	reg:status status:1001 ;
	a rdf:Property ;
	rdfs:isDefinedBy <http://rdaregistry.info/Elements/u/> ;
	rdfs:label "is adapted as musical theatre"@en ;
	rdfs:subPropertyOf <http://rdaregistry.info/Elements/u/P60260> ;
	owl:inverseOf <http://rdaregistry.info/Elements/u/P60719> ;
	owl:sameAs <http://rdaregistry.info/Elements/u/adaptedAsMusicalTheatre> ;
	skos:definition "Relates a resource to a musical theatre resource based on the source resource."@en .

<http://rdaregistry.info/Elements/u/P60722> reg:name "adaptedAsOpera"@en ;
	reg:status status:1001 ;
	a rdf:Property ;
	rdfs:isDefinedBy <http://rdaregistry.info/Elements/u/> ;
	rdfs:label "is adapted as opera"@en ;
	rdfs:subPropertyOf <http://rdaregistry.info/Elements/u/P60260> ;
	owl:inverseOf <http://rdaregistry.info/Elements/u/P60720> ;
	owl:sameAs <http://rdaregistry.info/Elements/u/adaptedAsOpera> ;
	skos:definition "Relates a resource to an opera based on the source resource."@en .

<http://rdaregistry.info/Elements/u/P60723> reg:name "music"@en ;
	reg:status status:1001 ;
	a rdf:Property ;
	rdfs:isDefinedBy <http://rdaregistry.info/Elements/u/> ;
	rdfs:label "is music"@en ;
	rdfs:subPropertyOf <http://rdaregistry.info/Elements/u/P60198> ;
	owl:inverseOf <http://rdaregistry.info/Elements/u/P60724> ;
	owl:sameAs <http://rdaregistry.info/Elements/u/music> ;
	skos:definition "Relates a resource to a musical resource that is used in a motion picture, play, television program, etc."@en .

<http://rdaregistry.info/Elements/u/P60724> reg:name "musicFor"@en ;
	reg:status status:1001 ;
	a rdf:Property ;
	rdfs:isDefinedBy <http://rdaregistry.info/Elements/u/> ;
	rdfs:label "is music for"@en ;
	rdfs:subPropertyOf <http://rdaregistry.info/Elements/u/P60198> ;
	owl:inverseOf <http://rdaregistry.info/Elements/u/P60723> ;
	owl:sameAs <http://rdaregistry.info/Elements/u/musicFor> ;
	skos:definition "Relates a resource to a resource such as a motion picture, play, television program, etc. that uses the musical resource."@en .

<http://rdaregistry.info/Elements/u/P60725> reg:name "videoMusic"@en ;
	reg:status status:1001 ;
	a rdf:Property ;
	rdfs:isDefinedBy <http://rdaregistry.info/Elements/u/> ;
	rdfs:label "is video music"@en ;
	rdfs:subPropertyOf <http://rdaregistry.info/Elements/u/P60723> ;
	owl:inverseOf <http://rdaregistry.info/Elements/u/P60726> ;
	owl:sameAs <http://rdaregistry.info/Elements/u/videoMusic> ;
	skos:definition "Relates a resource to a musical resource that is used in a video."@en .

<http://rdaregistry.info/Elements/u/P60726> reg:name "musicForVideo"@en ;
	reg:status status:1001 ;
	a rdf:Property ;
	rdfs:isDefinedBy <http://rdaregistry.info/Elements/u/> ;
	rdfs:label "is music for video"@en ;
	rdfs:subPropertyOf <http://rdaregistry.info/Elements/u/P60724> ;
	owl:inverseOf <http://rdaregistry.info/Elements/u/P60725> ;
	owl:sameAs <http://rdaregistry.info/Elements/u/musicForVideo> ;
	skos:definition "Relates a resource to a resource that uses the musical resource in a video."@en .

<http://rdaregistry.info/Elements/u/P60727> reg:name "televisionProgramMusic"@en ;
	reg:status status:1001 ;
	a rdf:Property ;
	rdfs:isDefinedBy <http://rdaregistry.info/Elements/u/> ;
	rdfs:label "is television program music"@en ;
	rdfs:subPropertyOf <http://rdaregistry.info/Elements/u/P60723> ;
	owl:inverseOf <http://rdaregistry.info/Elements/u/P60728> ;
	owl:sameAs <http://rdaregistry.info/Elements/u/televisionProgramMusic> ;
	skos:definition "Relates a resource to a musical resource that is used in a television program."@en .

<http://rdaregistry.info/Elements/u/P60728> reg:name "musicForTelevisionProgram"@en ;
	reg:status status:1001 ;
	a rdf:Property ;
	rdfs:isDefinedBy <http://rdaregistry.info/Elements/u/> ;
	rdfs:label "is music for television program"@en ;
	rdfs:subPropertyOf <http://rdaregistry.info/Elements/u/P60724> ;
	owl:inverseOf <http://rdaregistry.info/Elements/u/P60727> ;
	owl:sameAs <http://rdaregistry.info/Elements/u/musicForTelevisionProgram> ;
	skos:definition "Relates a resource to a resource that uses the musical resource in a television program."@en .

<http://rdaregistry.info/Elements/u/P60729> reg:name "radioProgramMusic"@en ;
	reg:status status:1001 ;
	a rdf:Property ;
	rdfs:isDefinedBy <http://rdaregistry.info/Elements/u/> ;
	rdfs:label "is radio program music"@en ;
	rdfs:subPropertyOf <http://rdaregistry.info/Elements/u/P60723> ;
	owl:inverseOf <http://rdaregistry.info/Elements/u/P60730> ;
	owl:sameAs <http://rdaregistry.info/Elements/u/radioProgramMusic> ;
	skos:definition "Relates a resource to a musical resource that is used in a radio program."@en .

<http://rdaregistry.info/Elements/u/P60730> reg:name "musicForRadioProgram"@en ;
	reg:status status:1001 ;
	a rdf:Property ;
	rdfs:isDefinedBy <http://rdaregistry.info/Elements/u/> ;
	rdfs:label "is music for radio program"@en ;
	rdfs:subPropertyOf <http://rdaregistry.info/Elements/u/P60724> ;
	owl:inverseOf <http://rdaregistry.info/Elements/u/P60729> ;
	owl:sameAs <http://rdaregistry.info/Elements/u/musicForRadioProgram> ;
	skos:definition "Relates a resource to a resource that uses the musical resource in a radio program."@en .

<http://rdaregistry.info/Elements/u/P60731> reg:name "musicForMotionPicture"@en ;
	reg:status status:1001 ;
	a rdf:Property ;
	rdfs:isDefinedBy <http://rdaregistry.info/Elements/u/> ;
	rdfs:label "is music for motion picture"@en ;
	rdfs:subPropertyOf <http://rdaregistry.info/Elements/u/P60723> ;
	owl:inverseOf <http://rdaregistry.info/Elements/u/P60732> ;
	owl:sameAs <http://rdaregistry.info/Elements/u/musicForMotionPicture> ;
	skos:definition "Relates a resource to a resource that uses the musical resource in a motion picture."@en .

<http://rdaregistry.info/Elements/u/P60732> reg:name "motionPictureMusic"@en ;
	reg:status status:1001 ;
	a rdf:Property ;
	rdfs:isDefinedBy <http://rdaregistry.info/Elements/u/> ;
	rdfs:label "is motion picture music"@en ;
	rdfs:subPropertyOf <http://rdaregistry.info/Elements/u/P60724> ;
	owl:inverseOf <http://rdaregistry.info/Elements/u/P60731> ;
	owl:sameAs <http://rdaregistry.info/Elements/u/motionPictureMusic> ;
	skos:definition "Relates a resource to a musical resource that is used in a motion picture."@en .

<http://rdaregistry.info/Elements/u/P60733> reg:name "predecessorOfSplit"@en ;
	reg:status status:1001 ;
	a rdf:Property ;
	rdfs:isDefinedBy <http://rdaregistry.info/Elements/u/> ;
	rdfs:label "has predecessor of split"@en ;
	owl:inverseOf <http://rdaregistry.info/Elements/u/P60685> ;
	owl:sameAs <http://rdaregistry.info/Elements/u/predecessorOfSplit> ;
	skos:definition "Relates an agent that split or divided into the other agent to the agent."@en .

<http://rdaregistry.info/Elements/u/P60736> reg:name "componentOfAMerger"@en ;
	reg:status status:1001 ;
	a rdf:Property ;
	rdfs:isDefinedBy <http://rdaregistry.info/Elements/u/> ;
	rdfs:label "has component of a merger"@en ;
	owl:inverseOf <http://rdaregistry.info/Elements/u/P60684> ;
	owl:sameAs <http://rdaregistry.info/Elements/u/componentOfAMerger> ;
	skos:definition "Relates an agent that formed the other agent by merging with one or more other agents to the agent."@en .

<http://rdaregistry.info/Elements/u/P60737> reg:name "officiatedAgent"@en ;
	reg:status status:1001 ;
	a rdf:Property ;
	rdfs:isDefinedBy <http://rdaregistry.info/Elements/u/> ;
	rdfs:label "has officiated agent"@en ;
	owl:inverseOf <http://rdaregistry.info/Elements/u/P60633> ;
	owl:sameAs <http://rdaregistry.info/Elements/u/officiatedAgent> ;
	skos:definition "Relates an agent in which the agent holds an office to the agent."@en .
