@prefix : <http://data.opendiscoveryspace.eu/lom_ontology_ods.owl#> .
@prefix cc: <http://creativecommons.org/ns#> .
@prefix dc: <http://purl.org/dc/elements/1.1/> .
@prefix ns: <http://www.w3.org/2006/vcard/ns#> .
@prefix owl: <http://www.w3.org/2002/07/owl#> .
@prefix rdf: <http://www.w3.org/1999/02/22-rdf-syntax-ns#> .
@prefix xml: <http://www.w3.org/XML/1998/namespace> .
@prefix xsd: <http://www.w3.org/2001/XMLSchema#> .
@prefix rdfs: <http://www.w3.org/2000/01/rdf-schema#> .
@prefix terms: <http://purl.org/dc/terms/> .
@prefix lom2owl: <http://data.opendiscoveryspace.eu/lom_ontology_ods.owl#> .
@prefix owl2xml: <http://www.w3.org/2006/12/owl2-xml#> .
@base <http://data.opendiscoveryspace.eu/lom_ontology_ods.owl#> .

<http://data.opendiscoveryspace.eu/lom_ontology_ods.owl#> rdf:type owl:Ontology ;
                                                          
                                                          owl:versionInfo 1.0 ;
                                                          
                                                          dc:issued "2014-05-20"^^xsd:date ;
                                                          
                                                          dc:modified "2015-03-30"^^xsd:date ;
                                                          
                                                          dc:rights "Copyright Â© 2015 University of Alcala, Information Engineering (IE) research unit (http://www.ieru.org/) " ;
                                                          
                                                          dc:creator """
			Enayat Rajabi (enayat.rajabi@uah.es)
		""" ;
                                                          
                                                          dc:publisher """
University of Alcala (www.uah.es) """ ;
                                                          
                                                          rdfs:comment "-Version 1.0: covers a complete mapping of IEEE LOM to Linked Open Data"@en ;
                                                          
                                                          dc:title "A vocabulary for exposing IEEE LOM metadata as Linked Open Data"@en ;
                                                          
                                                          dc:description """An ontology and vocabulary used for exposing IEEE LOM, a metadata standard for educational contents, as Linked Data. 
		It is intended as a bridge for linkage of educational metadata into Linked Open Data (LOD). 
		In this ontology, we designed a mapping of IEEE LOM elements to RDF based on Linked Data principles. """@en ;
                                                          
                                                          cc:license <http://creativecommons.org/licenses/by/3.0/> .


#################################################################
#
#    Annotation properties
#
#################################################################


###  http://purl.org/dc/elements/1.1/publisher

dc:publisher rdf:type owl:AnnotationProperty .



###  http://purl.org/dc/terms/coverage

terms:coverage rdf:type owl:AnnotationProperty .



###  http://purl.org/dc/terms/description

terms:description rdf:type owl:AnnotationProperty .



###  http://purl.org/dc/terms/format

terms:format rdf:type owl:AnnotationProperty .



###  http://purl.org/dc/terms/identifier

terms:identifier rdf:type owl:AnnotationProperty .



###  http://purl.org/dc/terms/language

terms:language rdf:type owl:AnnotationProperty .



###  http://purl.org/dc/terms/publisher

terms:publisher rdf:type owl:AnnotationProperty .



###  http://purl.org/dc/terms/rights

terms:rights rdf:type owl:AnnotationProperty .



###  http://purl.org/dc/terms/title

terms:title rdf:type owl:AnnotationProperty .



###  http://purl.org/dc/terms/type

terms:type rdf:type owl:AnnotationProperty .



###  http://www.w3.org/1999/02/22-rdf-syntax-ns#value

rdf:value rdf:type owl:AnnotationProperty .



###  http://www.w3.org/2006/vcard/ns#FN

ns:FN rdf:type owl:AnnotationProperty .



###  http://www.w3.org/2006/vcard/ns#N

ns:N rdf:type owl:AnnotationProperty .



###  http://www.w3.org/2006/vcard/ns#ORG

ns:ORG rdf:type owl:AnnotationProperty .



###  http://www.w3.org/2006/vcard/ns#email

ns:email rdf:type owl:AnnotationProperty .





#################################################################
#
#    Object Properties
#
#################################################################


###  http://data.opendiscoveryspace.eu/lom_ontology_ods.owl#annotation

:annotation rdf:type owl:ObjectProperty ;
            
            rdfs:comment "Comments on the educational use of a learning object, containing information on when and by whom the comments were created. This category enables educators to share their assessments of learning objects, suggestions for use, etc. IEEE LOM element 8."@en ;
            
            rdfs:range :Annotation .



###  http://data.opendiscoveryspace.eu/lom_ontology_ods.owl#annotationDate

:annotationDate rdf:type owl:ObjectProperty ;
                
                rdfs:comment "Date that this annotation was created. IEEE LOM element 8.2."@en ;
                
                rdfs:domain :Annotation ;
                
                rdfs:range :DateTime .



###  http://data.opendiscoveryspace.eu/lom_ontology_ods.owl#annotationEntity

:annotationEntity rdf:type owl:ObjectProperty ;
                  
                  rdfs:comment "Entity (i.e., people, organization) that created this annotation. IEEE LOM element 8.1."@en ;
                  
                  rdfs:domain :Annotation .



###  http://data.opendiscoveryspace.eu/lom_ontology_ods.owl#classification

:classification rdf:type owl:ObjectProperty ;
                
                rdfs:comment "Description of where a learning object falls within a particular classification system. IEEE LOM element 9."@en ;
                
                rdfs:range :Classification .



###  http://data.opendiscoveryspace.eu/lom_ontology_ods.owl#classificationKeyword

:classificationKeyword rdf:type owl:ObjectProperty ;
                       
                       rdfs:comment "Keywords and phrases descriptive of the learning object relative to the stated 9.1:Classification.Purpose of this specific classification, such as accessibility, security level, etc., most relevant first. IEEE LOM element 9.4"^^xsd:string ;
                       
                       rdfs:domain :Classification .



###  http://data.opendiscoveryspace.eu/lom_ontology_ods.owl#classificationTaxon

:classificationTaxon rdf:type owl:ObjectProperty ;
                     
                     rdfs:comment "A particular term within a taxonomy which serves to classify a learning object. IEEE LOM element 9.2.2."@en ;
                     
                     rdfs:range :Taxon ;
                     
                     rdfs:domain :TaxonPath .



###  http://data.opendiscoveryspace.eu/lom_ontology_ods.owl#contributionDateTime

:contributionDateTime rdf:type owl:ObjectProperty ;
                      
                      rdfs:comment "The date of the contribution. IEEE LOM element 3.2.3."@en ;
                      
                      rdfs:domain :Contribution ;
                      
                      rdfs:range :DateTime .



###  http://data.opendiscoveryspace.eu/lom_ontology_ods.owl#contributionEntity

:contributionEntity rdf:type owl:ObjectProperty ;
                    
                    rdfs:comment "The identification of and information about entities (i.e., people, organizations) contributing to this learning object. The entities shall be ordered as most relevant first. IEEE LOM element 3.2.2."^^xsd:string ;
                    
                    rdfs:domain :Contribution ;
                    
                    rdfs:range :VCard .



###  http://data.opendiscoveryspace.eu/lom_ontology_ods.owl#coverage

:coverage rdf:type owl:ObjectProperty ;
          
          terms:coverage ""^^rdfs:Literal ;
          
          rdfs:comment """The time, culture, geography or region to which this learning object applies.
The extent or scope of the content of the learning object. Coverage will typically include spatial location (a place name or geographic coordinates), temporal period (a period label, date, or date range) or jurisdiction (such as a named administrative entity). Recommended best practice is to select a value from a controlled vocabulary (for example, the Thesaurus of Geographic Names [TGN]) and that, where appropriate, named places or time periods be used in preference to numeric identifiers such as sets of coordinates or date ranges. IEEE LOM element 1.6."""@en ;
          
          rdfs:domain :LearningObject .



###  http://data.opendiscoveryspace.eu/lom_ontology_ods.owl#description

:description rdf:type owl:ObjectProperty ;
             
             terms:description ""^^rdfs:Literal ;
             
             rdfs:comment "Comments on how this learning object is to be used. IEEE LOM element 5.10"^^xsd:string ,
                          "A textual description of the content of this learning object. IEEE LOM element 1.4."@en ;
             
             rdfs:domain :LearningObject .



###  http://data.opendiscoveryspace.eu/lom_ontology_ods.owl#duration

:duration rdf:type owl:ObjectProperty ;
          
          rdfs:domain :Duration .



###  http://data.opendiscoveryspace.eu/lom_ontology_ods.owl#educational

:educational rdf:type owl:ObjectProperty ;
             
             rdfs:comment "This category describes the key educational or pedagogic characteristics of this learning object. IEEE LOM element 5."^^xsd:string ;
             
             rdfs:range :Educational ;
             
             rdfs:domain :LearningObject .



###  http://data.opendiscoveryspace.eu/lom_ontology_ods.owl#educationalTypicalAgeRange

:educationalTypicalAgeRange rdf:type owl:ObjectProperty ;
                            
                            rdf:value ""^^rdfs:Literal ;
                            
                            rdfs:comment "Age of the typical intended user. IEEE LOM element 5.7."^^xsd:string ;
                            
                            rdfs:domain :Educational .



###  http://data.opendiscoveryspace.eu/lom_ontology_ods.owl#educationalTypicalLearningTime

:educationalTypicalLearningTime rdf:type owl:ObjectProperty ;
                                
                                rdfs:range :Duration ;
                                
                                rdfs:domain :Educational .



###  http://data.opendiscoveryspace.eu/lom_ontology_ods.owl#hasRelatedResource

:hasRelatedResource rdf:type owl:ObjectProperty ;
                    
                    rdfs:comment "The target learning object that a relationship references. IEEE LOM element 7.2."@en ;
                    
                    rdfs:range :Identifier ;
                    
                    rdfs:domain :Relation .



###  http://data.opendiscoveryspace.eu/lom_ontology_ods.owl#hasResourceIdentifier

:hasResourceIdentifier rdf:type owl:ObjectProperty ;
                       
                       rdfs:comment "A globally unique label that identifies the target  learning object. IEEE LOM element 7.2.1."@en ;
                       
                       rdfs:range :Identifier .



###  http://data.opendiscoveryspace.eu/lom_ontology_ods.owl#identifier

:identifier rdf:type owl:InverseFunctionalProperty ,
                     owl:ObjectProperty ;
            
            rdfs:comment "This predicate represents the fact that a learning object has a label that identifies it. IEEE LOM element 1.1."@en ;
            
            rdfs:range :Identifier ;
            
            rdfs:domain :LearningObject .



###  http://data.opendiscoveryspace.eu/lom_ontology_ods.owl#includesSingleLangString

:includesSingleLangString rdf:type owl:ObjectProperty ;
                          
                          rdfs:comment "LangString values may include multiple semantically equivalent character strings, such as translations or alternative descriptions. Each of these is represented by a singleLangString."@en ;
                          
                          rdfs:range :LangString .



###  http://data.opendiscoveryspace.eu/lom_ontology_ods.owl#isCompositeOf

:isCompositeOf rdf:type owl:ObjectProperty ;
               
               rdfs:comment "When grouping multiple requirements, the composite requirement is satisfied when one of the component requirements is satisfied, i.e., the logical connector is OR. IEEE LOM element 4.4.1."@en ;
               
               rdfs:range :SingleTechnicalRequirement ;
               
               rdfs:domain :TechnicalRequirement .



###  http://data.opendiscoveryspace.eu/lom_ontology_ods.owl#keyword

:keyword rdf:type owl:ObjectProperty ;
         
         rdf:value ""^^rdfs:Literal ;
         
         rdfs:comment "A keyword or phrase describing the topic of this learning object. This data element should not be used for characteristics that can be described by other data elements. IEEE LOM element 1.5."@en ;
         
         rdfs:domain :LearningObject .



###  http://data.opendiscoveryspace.eu/lom_ontology_ods.owl#lifeCycleContribution

:lifeCycleContribution rdf:type owl:ObjectProperty .



###  http://data.opendiscoveryspace.eu/lom_ontology_ods.owl#metaMetadataContribution

:metaMetadataContribution rdf:type owl:ObjectProperty ;
                          
                          rdfs:comment "Those entities (i.e., people, organizations) that have contributed to the state of this learning object during its life cycle (e.g.,creation, edits, publication)."@en ;
                          
                          rdfs:domain :LearningObject ;
                          
                          rdfs:range :LifeCycleContribution .



###  http://data.opendiscoveryspace.eu/lom_ontology_ods.owl#metaMetadataIdentifier

:metaMetadataIdentifier rdf:type owl:ObjectProperty ;
                        
                        rdfs:comment "A globally unique label that identifies this metadata record. IEEE LOM element 3.1."^^xsd:string ;
                        
                        rdfs:range :Identifier ;
                        
                        rdfs:domain :LearningObject .



###  http://data.opendiscoveryspace.eu/lom_ontology_ods.owl#relatedResourceDescription

:relatedResourceDescription rdf:type owl:ObjectProperty ;
                            
                            terms:description ""^^rdfs:Literal ;
                            
                            rdfs:range :LangString ;
                            
                            rdfs:domain :Relation .



###  http://data.opendiscoveryspace.eu/lom_ontology_ods.owl#relation

:relation rdf:type owl:ObjectProperty ;
          
          rdfs:comment "Relationship between a learning object and other learning objects, if any."@en ;
          
          rdfs:range :Relation .



###  http://data.opendiscoveryspace.eu/lom_ontology_ods.owl#taxonPath

:taxonPath rdf:type owl:ObjectProperty ;
           
           rdfs:comment "A taxonomic path in a specific classification system according to which a learning object is classified. IEEE LOM element 9.2."@en ;
           
           rdfs:domain :Classification ;
           
           rdfs:range :TaxonPath .



###  http://data.opendiscoveryspace.eu/lom_ontology_ods.owl#technicalDuration

:technicalDuration rdf:type owl:ObjectProperty ;
                   
                   rdfs:domain :Duration ;
                   
                   rdfs:range :LearningObject .



###  http://data.opendiscoveryspace.eu/lom_ontology_ods.owl#technicalRequirements

:technicalRequirements rdf:type owl:ObjectProperty ;
                       
                       rdfs:comment "A technical capability necessary for using a learning object. IEEE LOM Element \"4.4. Requirement\"."@en ;
                       
                       rdfs:range :TechnicalRequirement .





#################################################################
#
#    Data properties
#
#################################################################


###  http://data.opendiscoveryspace.eu/lom_ontology_ods.owl#aggregationLevel

:aggregationLevel rdf:type owl:DatatypeProperty ;
                  
                  rdfs:comment "The functional granularity of this learning object. IEEE LOM element 1.8."@en ;
                  
                  rdfs:domain :LearningObject ;
                  
                  rdfs:range [ rdf:type rdfs:Datatype ;
                               owl:oneOf [ rdf:type rdf:List ;
                                           rdf:first "1"^^xsd:string ;
                                           rdf:rest [ rdf:type rdf:List ;
                                                      rdf:first "2"^^xsd:string ;
                                                      rdf:rest [ rdf:type rdf:List ;
                                                                 rdf:first "3"^^xsd:string ;
                                                                 rdf:rest [ rdf:type rdf:List ;
                                                                            rdf:first "4"^^xsd:string ;
                                                                            rdf:rest rdf:nil
                                                                          ]
                                                               ]
                                                    ]
                                         ]
                             ] .



###  http://data.opendiscoveryspace.eu/lom_ontology_ods.owl#annotationDescription

:annotationDescription rdf:type owl:DatatypeProperty ;
                       
                       rdfs:domain :Annotation ;
                       
                       rdfs:range rdfs:Literal .



###  http://data.opendiscoveryspace.eu/lom_ontology_ods.owl#annotationEntity

:annotationEntity rdf:type owl:DatatypeProperty ;
                  
                  rdfs:comment "Entity (i.e., people, organization) that created this annotation. IEEE LOM element 8.1."@en ;
                  
                  rdfs:range xsd:string .



###  http://data.opendiscoveryspace.eu/lom_ontology_ods.owl#classificationDescription

:classificationDescription rdf:type owl:DatatypeProperty ;
                           
                           rdfs:domain :Classification ;
                           
                           rdfs:range rdfs:Literal .



###  http://data.opendiscoveryspace.eu/lom_ontology_ods.owl#classificationPurpose

:classificationPurpose rdf:type owl:DatatypeProperty ;
                       
                       rdfs:comment "The purpose of classifying a learning object. IEEE LOM element 9.1."@en ;
                       
                       rdfs:domain :Classification ;
                       
                       rdfs:range [ rdf:type rdfs:Datatype ;
                                    owl:oneOf [ rdf:type rdf:List ;
                                                rdf:first "accessibility"^^xsd:string ;
                                                rdf:rest [ rdf:type rdf:List ;
                                                           rdf:first "competency"^^xsd:string ;
                                                           rdf:rest [ rdf:type rdf:List ;
                                                                      rdf:first "discipline"^^xsd:string ;
                                                                      rdf:rest [ rdf:type rdf:List ;
                                                                                 rdf:first "educational level"^^xsd:string ;
                                                                                 rdf:rest [ rdf:type rdf:List ;
                                                                                            rdf:first "educational objective"^^xsd:string ;
                                                                                            rdf:rest [ rdf:type rdf:List ;
                                                                                                       rdf:first "idea"^^xsd:string ;
                                                                                                       rdf:rest [ rdf:type rdf:List ;
                                                                                                                  rdf:first "prerequisite"^^xsd:string ;
                                                                                                                  rdf:rest [ rdf:type rdf:List ;
                                                                                                                             rdf:first "restrictions"^^xsd:string ;
                                                                                                                             rdf:rest [ rdf:type rdf:List ;
                                                                                                                                        rdf:first "security level"^^xsd:string ;
                                                                                                                                        rdf:rest [ rdf:type rdf:List ;
                                                                                                                                                   rdf:first "skill level"^^xsd:string ;
                                                                                                                                                   rdf:rest rdf:nil
                                                                                                                                                 ]
                                                                                                                                      ]
                                                                                                                           ]
                                                                                                                ]
                                                                                                     ]
                                                                                          ]
                                                                               ]
                                                                    ]
                                                         ]
                                              ]
                                  ] .



###  http://data.opendiscoveryspace.eu/lom_ontology_ods.owl#copyrightAndOtherRestrictions

:copyrightAndOtherRestrictions rdf:type owl:DatatypeProperty ;
                               
                               rdfs:comment "Whether copyright or other restrictions apply to the use of this learning object. IEEE LOM element 6.2."@en ;
                               
                               rdfs:range xsd:boolean .



###  http://data.opendiscoveryspace.eu/lom_ontology_ods.owl#copyrightDescription

:copyrightDescription rdf:type owl:DatatypeProperty ;
                      
                      rdfs:domain :LearningObject ;
                      
                      rdfs:range rdfs:Literal .



###  http://data.opendiscoveryspace.eu/lom_ontology_ods.owl#cost

:cost rdf:type owl:DatatypeProperty ;
      
      rdfs:comment "Whether use of the learning object requires payment. IEEE LOM element 6.1."@en ;
      
      rdfs:range xsd:boolean .



###  http://data.opendiscoveryspace.eu/lom_ontology_ods.owl#dateTimeDescription

:dateTimeDescription rdf:type owl:DatatypeProperty ;
                     
                     rdfs:domain :Contribution ;
                     
                     rdfs:range rdfs:Literal .



###  http://data.opendiscoveryspace.eu/lom_ontology_ods.owl#dateTimeValue

:dateTimeValue rdf:type owl:DatatypeProperty ;
               
               rdfs:comment "Date time value in format: YYYY[-MM[-DD[Thh[:mm[:ss[.s[TZD]]]]]]]"@en ;
               
               rdfs:domain :DateTime ;
               
               rdfs:range xsd:dateTime .



###  http://data.opendiscoveryspace.eu/lom_ontology_ods.owl#durationDescription

:durationDescription rdf:type owl:DatatypeProperty ;
                     
                     rdfs:domain :Duration ;
                     
                     rdfs:range rdfs:Literal .



###  http://data.opendiscoveryspace.eu/lom_ontology_ods.owl#durationValue

:durationValue rdf:type owl:DatatypeProperty ;
               
               rdfs:domain :Duration ;
               
               rdfs:range rdfs:Literal .



###  http://data.opendiscoveryspace.eu/lom_ontology_ods.owl#educationalContext

:educationalContext rdf:type owl:DatatypeProperty ;
                    
                    rdfs:comment "The principal environment within which the learning and use of this learning object is intended to take place. IEEE LOM element 5.6."@en ;
                    
                    rdfs:domain :Educational ;
                    
                    rdfs:range rdfs:Literal ,
                               xsd:short ,
                               [ rdf:type rdfs:Datatype ;
                                 owl:oneOf [ rdf:type rdf:List ;
                                             rdf:first "higher education"^^xsd:string ;
                                             rdf:rest [ rdf:type rdf:List ;
                                                        rdf:first "other"^^xsd:string ;
                                                        rdf:rest [ rdf:type rdf:List ;
                                                                   rdf:first "school"^^xsd:string ;
                                                                   rdf:rest [ rdf:type rdf:List ;
                                                                              rdf:first "training"^^xsd:string ;
                                                                              rdf:rest rdf:nil
                                                                            ]
                                                                 ]
                                                      ]
                                           ]
                               ] .



###  http://data.opendiscoveryspace.eu/lom_ontology_ods.owl#educationalDifficulty

:educationalDifficulty rdf:type owl:DatatypeProperty ;
                       
                       rdfs:comment "How hard it is to work with or through this learning object for the typical intended target audience. IEEE LOM element 5.8"@en ;
                       
                       rdfs:domain :Educational ;
                       
                       rdfs:range [ rdf:type rdfs:Datatype ;
                                    owl:oneOf [ rdf:type rdf:List ;
                                                rdf:first "difficult"^^xsd:string ;
                                                rdf:rest [ rdf:type rdf:List ;
                                                           rdf:first "easy"^^xsd:string ;
                                                           rdf:rest [ rdf:type rdf:List ;
                                                                      rdf:first "medium"^^xsd:string ;
                                                                      rdf:rest [ rdf:type rdf:List ;
                                                                                 rdf:first "very difficult"^^xsd:string ;
                                                                                 rdf:rest [ rdf:type rdf:List ;
                                                                                            rdf:first "very easy"^^xsd:string ;
                                                                                            rdf:rest rdf:nil
                                                                                          ]
                                                                               ]
                                                                    ]
                                                         ]
                                              ]
                                  ] .



###  http://data.opendiscoveryspace.eu/lom_ontology_ods.owl#educationalIntendedUserRole

:educationalIntendedUserRole rdf:type owl:DatatypeProperty ;
                             
                             rdfs:comment "Principal user(s) for which this learning object was designed, most dominant first. IEEE LOM element 5.5."@en ;
                             
                             rdfs:domain :Educational ;
                             
                             rdfs:range [ rdf:type rdfs:Datatype ;
                                          owl:oneOf [ rdf:type rdf:List ;
                                                      rdf:first "author"^^xsd:string ;
                                                      rdf:rest [ rdf:type rdf:List ;
                                                                 rdf:first "learner"^^xsd:string ;
                                                                 rdf:rest [ rdf:type rdf:List ;
                                                                            rdf:first "manager"^^xsd:string ;
                                                                            rdf:rest [ rdf:type rdf:List ;
                                                                                       rdf:first "teacher"^^xsd:string ;
                                                                                       rdf:rest rdf:nil
                                                                                     ]
                                                                          ]
                                                               ]
                                                    ]
                                        ] .



###  http://data.opendiscoveryspace.eu/lom_ontology_ods.owl#educationalInteractivityLevel

:educationalInteractivityLevel rdf:type owl:DatatypeProperty ;
                               
                               rdfs:comment "The degree of interactivity characterizing this learning object. Interactivity in this context refers to the degree to which the learner can influence the aspect or behavior of the learning object. IEEE LOM element 5.3."^^xsd:string ;
                               
                               rdfs:domain :Educational ;
                               
                               rdfs:range [ rdf:type rdfs:Datatype ;
                                            owl:oneOf [ rdf:type rdf:List ;
                                                        rdf:first "high"^^xsd:string ;
                                                        rdf:rest [ rdf:type rdf:List ;
                                                                   rdf:first "low"^^xsd:string ;
                                                                   rdf:rest [ rdf:type rdf:List ;
                                                                              rdf:first "medium"^^xsd:string ;
                                                                              rdf:rest [ rdf:type rdf:List ;
                                                                                         rdf:first "very high"^^xsd:string ;
                                                                                         rdf:rest [ rdf:type rdf:List ;
                                                                                                    rdf:first "very low"^^xsd:string ;
                                                                                                    rdf:rest rdf:nil
                                                                                                  ]
                                                                                       ]
                                                                            ]
                                                                 ]
                                                      ]
                                          ] .



###  http://data.opendiscoveryspace.eu/lom_ontology_ods.owl#educationalInteractivityType

:educationalInteractivityType rdf:type owl:DatatypeProperty ;
                              
                              rdfs:comment "Predominant mode of learning supported by this learning object. IEEE LOM element 5.1."@en ;
                              
                              rdfs:domain :Educational ;
                              
                              rdfs:range [ rdf:type rdfs:Datatype ;
                                           owl:oneOf [ rdf:type rdf:List ;
                                                       rdf:first "active"^^xsd:string ;
                                                       rdf:rest [ rdf:type rdf:List ;
                                                                  rdf:first "expositive"^^xsd:string ;
                                                                  rdf:rest [ rdf:type rdf:List ;
                                                                             rdf:first "mised"^^xsd:string ;
                                                                             rdf:rest rdf:nil
                                                                           ]
                                                                ]
                                                     ]
                                         ] .



###  http://data.opendiscoveryspace.eu/lom_ontology_ods.owl#educationalLanguage

:educationalLanguage rdf:type owl:DatatypeProperty ;
                     
                     rdfs:comment "The primary human language or languages used within this learning object to communicate to the intended user. If the learning object had no lingual content (as in the case of a picture of the Mona Lisa, for example), then the appropriate value for this data element would be \"none\". IEEE LOM element 1.3."@en ;
                     
                     rdfs:domain :LearningObject ;
                     
                     rdfs:range [ rdf:type rdfs:Datatype ;
                                  owl:oneOf [ rdf:type rdf:List ;
                                              rdf:first "ba"^^xsd:string ;
                                              rdf:rest [ rdf:type rdf:List ;
                                                         rdf:first "ca"^^xsd:string ;
                                                         rdf:rest [ rdf:type rdf:List ;
                                                                    rdf:first "es"^^xsd:string ;
                                                                    rdf:rest [ rdf:type rdf:List ;
                                                                               rdf:first "ga"^^xsd:string ;
                                                                               rdf:rest [ rdf:type rdf:List ;
                                                                                          rdf:first "none"^^xsd:string ;
                                                                                          rdf:rest rdf:nil
                                                                                        ]
                                                                             ]
                                                                  ]
                                                       ]
                                            ]
                                ] .



###  http://data.opendiscoveryspace.eu/lom_ontology_ods.owl#educationalSemanticDensity

:educationalSemanticDensity rdf:type owl:DatatypeProperty ;
                            
                            rdfs:comment "The degree of conciseness of a learning object. The semantic density of a learning object may be estimated in terms of its size, span, or --in the case of self-timed resources such as audio or video-- duration. IEEE LOM element 5.4."^^xsd:string ;
                            
                            rdfs:domain :Educational ;
                            
                            rdfs:range xsd:string ,
                                       [ rdf:type rdfs:Datatype ;
                                         owl:oneOf [ rdf:type rdf:List ;
                                                     rdf:first "higherEducation"^^xsd:string ;
                                                     rdf:rest [ rdf:type rdf:List ;
                                                                rdf:first "other"^^xsd:string ;
                                                                rdf:rest [ rdf:type rdf:List ;
                                                                           rdf:first "school"^^xsd:string ;
                                                                           rdf:rest [ rdf:type rdf:List ;
                                                                                      rdf:first "training"^^xsd:string ;
                                                                                      rdf:rest rdf:nil
                                                                                    ]
                                                                         ]
                                                              ]
                                                   ]
                                       ] ,
                                       [ rdf:type rdfs:Datatype ;
                                         owl:oneOf [ rdf:type rdf:List ;
                                                     rdf:first "high"^^xsd:string ;
                                                     rdf:rest [ rdf:type rdf:List ;
                                                                rdf:first "low"^^xsd:string ;
                                                                rdf:rest [ rdf:type rdf:List ;
                                                                           rdf:first "medium"^^xsd:string ;
                                                                           rdf:rest [ rdf:type rdf:List ;
                                                                                      rdf:first "very high"^^xsd:string ;
                                                                                      rdf:rest [ rdf:type rdf:List ;
                                                                                                 rdf:first "very low"^^xsd:string ;
                                                                                                 rdf:rest rdf:nil
                                                                                               ]
                                                                                    ]
                                                                         ]
                                                              ]
                                                   ]
                                       ] .



###  http://data.opendiscoveryspace.eu/lom_ontology_ods.owl#email

:email rdf:type owl:DatatypeProperty ;
       
       rdfs:comment "Email as it appears in the vCard"^^xsd:string ;
       
       rdfs:domain :VCard ;
       
       rdfs:range xsd:string .



###  http://data.opendiscoveryspace.eu/lom_ontology_ods.owl#hasTechnicalFormat

:hasTechnicalFormat rdf:type owl:DatatypeProperty ;
                    
                    rdfs:comment "Technical datatype(s) of (all the components of) this learning object. This information is used to identify the software needed to access the learning object. IEEE LOM element 4.1."@en ;
                    
                    rdfs:domain :LearningObject ;
                    
                    rdfs:range xsd:string .



###  http://data.opendiscoveryspace.eu/lom_ontology_ods.owl#hasValue

:hasValue rdf:type owl:DatatypeProperty ;
          
          rdfs:comment "This predicate relates a singleLangString to the character string containing its textual description."@en ;
          
          rdfs:range xsd:string .



###  http://data.opendiscoveryspace.eu/lom_ontology_ods.owl#identifierCatalog

:identifierCatalog rdf:type owl:DatatypeProperty ,
                            owl:FunctionalProperty ;
                   
                   rdfs:comment "This predicate relates a lomIdentifier to the name or designator of the identification or cataloging scheme used for its identification. It is usually a namespace scheme. IEEE LOM element 1.1, 3.1, 7.2.1."@en ;
                   
                   rdfs:domain :Identifier ;
                   
                   rdfs:range xsd:string .



###  http://data.opendiscoveryspace.eu/lom_ontology_ods.owl#identifierEntry

:identifierEntry rdf:type owl:DatatypeProperty ,
                          owl:FunctionalProperty ;
                 
                 rdfs:comment "This predicate relates a lomIdentifier to the value of the identifier within the identification or cataloging scheme that designates or identifies a learning object or a learning object metadata record (a namespace specific string).  IEEE LOM element 1.1, 3.1, 7.2.1."@en ;
                 
                 rdfs:domain :Identifier ;
                 
                 rdfs:range xsd:string .



###  http://data.opendiscoveryspace.eu/lom_ontology_ods.owl#lifeCycleContributionRole

:lifeCycleContributionRole rdf:type owl:DatatypeProperty ;
                           
                           rdfs:comment "Kind of contribution. IEEE LOM element 2.3.1."@en ;
                           
                           rdfs:domain :LifeCycleContribution ;
                           
                           rdfs:range [ rdf:type rdfs:Datatype ;
                                        owl:oneOf [ rdf:type rdf:List ;
                                                    rdf:first "author"^^xsd:string ;
                                                    rdf:rest [ rdf:type rdf:List ;
                                                               rdf:first "content provider"^^xsd:string ;
                                                               rdf:rest [ rdf:type rdf:List ;
                                                                          rdf:first "editor"^^xsd:string ;
                                                                          rdf:rest [ rdf:type rdf:List ;
                                                                                     rdf:first "educational validator"^^xsd:string ;
                                                                                     rdf:rest [ rdf:type rdf:List ;
                                                                                                rdf:first "graphical designer"^^xsd:string ;
                                                                                                rdf:rest [ rdf:type rdf:List ;
                                                                                                           rdf:first "initiator"^^xsd:string ;
                                                                                                           rdf:rest [ rdf:type rdf:List ;
                                                                                                                      rdf:first "instructional designer"^^xsd:string ;
                                                                                                                      rdf:rest [ rdf:type rdf:List ;
                                                                                                                                 rdf:first "publisher"^^xsd:string ;
                                                                                                                                 rdf:rest [ rdf:type rdf:List ;
                                                                                                                                            rdf:first "script writer"^^xsd:string ;
                                                                                                                                            rdf:rest [ rdf:type rdf:List ;
                                                                                                                                                       rdf:first "subject matter expert"^^xsd:string ;
                                                                                                                                                       rdf:rest [ rdf:type rdf:List ;
                                                                                                                                                                  rdf:first "technical implementer"^^xsd:string ;
                                                                                                                                                                  rdf:rest [ rdf:type rdf:List ;
                                                                                                                                                                             rdf:first "technical validator"^^xsd:string ;
                                                                                                                                                                             rdf:rest [ rdf:type rdf:List ;
                                                                                                                                                                                        rdf:first "terminator"^^xsd:string ;
                                                                                                                                                                                        rdf:rest [ rdf:type rdf:List ;
                                                                                                                                                                                                   rdf:first "unknown"^^xsd:string ;
                                                                                                                                                                                                   rdf:rest [ rdf:type rdf:List ;
                                                                                                                                                                                                              rdf:first "validator"^^xsd:string ;
                                                                                                                                                                                                              rdf:rest rdf:nil
                                                                                                                                                                                                            ]
                                                                                                                                                                                                 ]
                                                                                                                                                                                      ]
                                                                                                                                                                           ]
                                                                                                                                                                ]
                                                                                                                                                     ]
                                                                                                                                          ]
                                                                                                                               ]
                                                                                                                    ]
                                                                                                         ]
                                                                                              ]
                                                                                   ]
                                                                        ]
                                                             ]
                                                  ]
                                      ] .



###  http://data.opendiscoveryspace.eu/lom_ontology_ods.owl#lifeCycleStatus

:lifeCycleStatus rdf:type owl:DatatypeProperty ;
                 
                 rdfs:comment "The completion status or condition of this learning object. IEEE LOM element 2.2"^^xsd:string ;
                 
                 rdfs:domain :LearningObject ;
                 
                 rdfs:range [ rdf:type rdfs:Datatype ;
                              owl:oneOf [ rdf:type rdf:List ;
                                          rdf:first "draft"^^xsd:string ;
                                          rdf:rest [ rdf:type rdf:List ;
                                                     rdf:first "final"^^xsd:string ;
                                                     rdf:rest [ rdf:type rdf:List ;
                                                                rdf:first "revised"^^xsd:string ;
                                                                rdf:rest [ rdf:type rdf:List ;
                                                                           rdf:first "unavalaible"^^xsd:string ;
                                                                           rdf:rest rdf:nil
                                                                         ]
                                                              ]
                                                   ]
                                        ]
                            ] .



###  http://data.opendiscoveryspace.eu/lom_ontology_ods.owl#lifeCycleVersion

:lifeCycleVersion rdf:type owl:DatatypeProperty ;
                  
                  rdfs:domain :LearningObject ;
                  
                  rdfs:range rdfs:Literal .



###  http://data.opendiscoveryspace.eu/lom_ontology_ods.owl#metaMetadataContributionRole

:metaMetadataContributionRole rdf:type owl:DatatypeProperty ;
                              
                              rdfs:comment "Kind of contribution. IEEE LOM element 3.2.1."^^xsd:string ;
                              
                              rdfs:domain :MetaMetadataContribution ;
                              
                              rdfs:range xsd:string .



###  http://data.opendiscoveryspace.eu/lom_ontology_ods.owl#metaMetadataLanguage

:metaMetadataLanguage rdf:type owl:DatatypeProperty ;
                      
                      rdfs:comment "Language of this metadata instance. This is the default language for all LangString values in this metadata instance. If a value for this data element is not present in a metadata instance, then there is no default language for LangString values. IEEE LOM element 3.4."@en ;
                      
                      rdfs:domain :LearningObject ;
                      
                      rdfs:range [ rdf:type rdfs:Datatype ;
                                   owl:oneOf [ rdf:type rdf:List ;
                                               rdf:first "ba"^^xsd:string ;
                                               rdf:rest [ rdf:type rdf:List ;
                                                          rdf:first "ca"^^xsd:string ;
                                                          rdf:rest [ rdf:type rdf:List ;
                                                                     rdf:first "es"^^xsd:string ;
                                                                     rdf:rest [ rdf:type rdf:List ;
                                                                                rdf:first "ga"^^xsd:string ;
                                                                                rdf:rest rdf:nil
                                                                              ]
                                                                   ]
                                                        ]
                                             ]
                                 ] .



###  http://data.opendiscoveryspace.eu/lom_ontology_ods.owl#metadataSchema

:metadataSchema rdf:type owl:DatatypeProperty ;
                
                rdfs:comment "The name and version of the authoritative specification used to create this metadata instance. IEEE LOM element 3.3."@en ;
                
                rdfs:domain :LearningObject ;
                
                rdfs:range xsd:string .



###  http://data.opendiscoveryspace.eu/lom_ontology_ods.owl#orCompositeMaximumVersion

:orCompositeMaximumVersion rdf:type owl:DatatypeProperty ;
                           
                           rdfs:comment "Highest possible version of the required technology to use the learning object. IEEE LOM element 4.4.1.4."@en ;
                           
                           rdfs:domain :SingleTechnicalRequirement ;
                           
                           rdfs:range xsd:string .



###  http://data.opendiscoveryspace.eu/lom_ontology_ods.owl#orCompositeMinimumVersion

:orCompositeMinimumVersion rdf:type owl:DatatypeProperty ;
                           
                           rdfs:comment "Lowest possible version of the required technology to use the learning object. IEEE LOM element 4.4.1.3."@en ;
                           
                           rdfs:domain :SingleTechnicalRequirement ;
                           
                           rdfs:range xsd:string .



###  http://data.opendiscoveryspace.eu/lom_ontology_ods.owl#orCompositeName

:orCompositeName rdf:type owl:DatatypeProperty ;
                 
                 rdfs:comment "Name of the required technology to use a learning object. IEEE LOM element 4.4.1.2."@en ;
                 
                 rdfs:domain :SingleTechnicalRequirement ;
                 
                 rdfs:range xsd:string .



###  http://data.opendiscoveryspace.eu/lom_ontology_ods.owl#orCompositeType

:orCompositeType rdf:type owl:DatatypeProperty ;
                 
                 rdfs:comment "The technology required to use this learning object, e.g., hardware, software, network, etc. IEEE LOM element 4.4.1.1."@en ;
                 
                 rdfs:domain :SingleTechnicalRequirement ;
                 
                 rdfs:range [ rdf:type rdfs:Datatype ;
                              owl:oneOf [ rdf:type rdf:List ;
                                          rdf:first "browser"^^xsd:string ;
                                          rdf:rest [ rdf:type rdf:List ;
                                                     rdf:first "operating system"^^xsd:string ;
                                                     rdf:rest rdf:nil
                                                   ]
                                        ]
                            ] .



###  http://data.opendiscoveryspace.eu/lom_ontology_ods.owl#otherPlatformRequirements

:otherPlatformRequirements rdf:type owl:DatatypeProperty ;
                           
                           rdfs:domain :LearningObject ;
                           
                           rdfs:range rdfs:Literal .



###  http://data.opendiscoveryspace.eu/lom_ontology_ods.owl#relationKind

:relationKind rdf:type owl:DatatypeProperty ;
              
              rdfs:comment "Nature of the relationship between a learning object and the target learning object, identified by 7.2:Relation.Resource. IEEE LOM element 7.1."@en ;
              
              rdfs:domain :Relation ;
              
              rdfs:range [ rdf:type rdfs:Datatype ;
                           owl:oneOf [ rdf:type rdf:List ;
                                       rdf:first "hasFormat"^^xsd:string ;
                                       rdf:rest [ rdf:type rdf:List ;
                                                  rdf:first "hasPart"^^xsd:string ;
                                                  rdf:rest [ rdf:type rdf:List ;
                                                             rdf:first "hasVersion"^^xsd:string ;
                                                             rdf:rest [ rdf:type rdf:List ;
                                                                        rdf:first "isBasedOn"^^xsd:string ;
                                                                        rdf:rest [ rdf:type rdf:List ;
                                                                                   rdf:first "isBasisFor"^^xsd:string ;
                                                                                   rdf:rest [ rdf:type rdf:List ;
                                                                                              rdf:first "isFormatOf"^^xsd:string ;
                                                                                              rdf:rest [ rdf:type rdf:List ;
                                                                                                         rdf:first "isPartOf"^^xsd:string ;
                                                                                                         rdf:rest [ rdf:type rdf:List ;
                                                                                                                    rdf:first "isReferencedBy"^^xsd:string ;
                                                                                                                    rdf:rest [ rdf:type rdf:List ;
                                                                                                                               rdf:first "isRequiredBy"^^xsd:string ;
                                                                                                                               rdf:rest [ rdf:type rdf:List ;
                                                                                                                                          rdf:first "isVersionOf"^^xsd:string ;
                                                                                                                                          rdf:rest [ rdf:type rdf:List ;
                                                                                                                                                     rdf:first "references"^^xsd:string ;
                                                                                                                                                     rdf:rest [ rdf:type rdf:List ;
                                                                                                                                                                rdf:first "requires"^^xsd:string ;
                                                                                                                                                                rdf:rest rdf:nil
                                                                                                                                                              ]
                                                                                                                                                   ]
                                                                                                                                        ]
                                                                                                                             ]
                                                                                                                  ]
                                                                                                       ]
                                                                                            ]
                                                                                 ]
                                                                      ]
                                                           ]
                                                ]
                                     ]
                         ] .



###  http://data.opendiscoveryspace.eu/lom_ontology_ods.owl#structure

:structure rdf:type owl:DatatypeProperty ;
           
           rdfs:comment "Underlying organizational structure of this learning object. IEEE LOM element 1.7."@en ;
           
           rdfs:domain :LearningObject ;
           
           rdfs:range [ rdf:type rdfs:Datatype ;
                        owl:oneOf [ rdf:type rdf:List ;
                                    rdf:first "atomic"^^xsd:string ;
                                    rdf:rest [ rdf:type rdf:List ;
                                               rdf:first "collection"^^xsd:string ;
                                               rdf:rest [ rdf:type rdf:List ;
                                                          rdf:first "hierarchical"^^xsd:string ;
                                                          rdf:rest [ rdf:type rdf:List ;
                                                                     rdf:first "linear"^^xsd:string ;
                                                                     rdf:rest [ rdf:type rdf:List ;
                                                                                rdf:first "networked"^^xsd:string ;
                                                                                rdf:rest rdf:nil
                                                                              ]
                                                                   ]
                                                        ]
                                             ]
                                  ]
                      ] .



###  http://data.opendiscoveryspace.eu/lom_ontology_ods.owl#taxonEntry

:taxonEntry rdf:type owl:DatatypeProperty ;
            
            rdfs:range rdfs:Literal .



###  http://data.opendiscoveryspace.eu/lom_ontology_ods.owl#taxonId

:taxonId rdf:type owl:DatatypeProperty ;
         
         rdfs:comment "The identifier of the taxon, such as a number or letter combination provided by the source of the taxonomy. IEEE LOM element 9.2.2.1."@en ;
         
         rdfs:domain :Taxon ;
         
         rdfs:range xsd:string .



###  http://data.opendiscoveryspace.eu/lom_ontology_ods.owl#taxonpathSource

:taxonpathSource rdf:type owl:DatatypeProperty ;
                 
                 rdfs:domain :TaxonPath ;
                 
                 rdfs:range rdfs:Literal .



###  http://data.opendiscoveryspace.eu/lom_ontology_ods.owl#technicalInstallationRemarks

:technicalInstallationRemarks rdf:type owl:DatatypeProperty ;
                              
                              rdfs:domain :LearningObject ;
                              
                              rdfs:range rdfs:Literal .



###  http://data.opendiscoveryspace.eu/lom_ontology_ods.owl#technicalLocation

:technicalLocation rdf:type owl:DatatypeProperty ;
                   
                   rdfs:comment "A string that is used to access this learning object. It may be a location  (e.g., Universal Resource Locator), or a method that resolves to a location (e.g., Universal Resource Identifier). The first element of this list shall be the preferable location. IEEE LOM element 4.3."@en ;
                   
                   rdfs:domain :LearningObject ;
                   
                   rdfs:range xsd:string .



###  http://data.opendiscoveryspace.eu/lom_ontology_ods.owl#technicalSize

:technicalSize rdf:type owl:DatatypeProperty ;
               
               rdfs:comment "The size of the digital learning object in bytes (not Mbytes, GB, etc.). The size is represented as a decimal value. This data element shall refer to the actual size of this learning object. If the learning object is compressed, then this data element shall refer to the uncompressed size. IEEE LOM element 4.2."@en ;
               
               rdfs:domain :LearningObject ;
               
               rdfs:range xsd:string .





#################################################################
#
#    Classes
#
#################################################################


###  http://data.opendiscoveryspace.eu/lom_ontology_ods.owl#Annotation

:Annotation rdf:type owl:Class ;
            
            rdfs:subClassOf owl:Thing ,
                            [ rdf:type owl:Restriction ;
                              owl:onProperty :dateTimeDescription ;
                              owl:cardinality "1"^^xsd:nonNegativeInteger
                            ] ,
                            [ rdf:type owl:Restriction ;
                              owl:onProperty :annotationEntity ;
                              owl:onClass :VCard ;
                              owl:qualifiedCardinality "1"^^xsd:nonNegativeInteger
                            ] ,
                            [ rdf:type owl:Restriction ;
                              owl:onProperty :annotationDescription ;
                              owl:someValuesFrom rdfs:Literal
                            ] ,
                            [ rdf:type owl:Restriction ;
                              owl:onProperty :dateTimeValue ;
                              owl:cardinality "1"^^xsd:nonNegativeInteger
                            ] ;
            
            rdfs:comment "Comments on the educational use of a learning object, including information on when and by whom the comments were created."@en .



###  http://data.opendiscoveryspace.eu/lom_ontology_ods.owl#Classification

:Classification rdf:type owl:Class ;
                
                rdfs:subClassOf owl:Thing ,
                                [ rdf:type owl:Restriction ;
                                  owl:onProperty :taxonPath ;
                                  owl:onClass :TaxonPath ;
                                  owl:maxQualifiedCardinality "15"^^xsd:nonNegativeInteger
                                ] ,
                                [ rdf:type owl:Restriction ;
                                  owl:onProperty :classificationKeyword ;
                                  owl:onClass :LangString ;
                                  owl:maxQualifiedCardinality "40"^^xsd:nonNegativeInteger
                                ] ,
                                [ rdf:type owl:Restriction ;
                                  owl:onProperty :classificationPurpose ;
                                  owl:cardinality "1"^^xsd:nonNegativeInteger
                                ] ,
                                [ rdf:type owl:Restriction ;
                                  owl:onProperty :classificationDescription ;
                                  owl:someValuesFrom rdfs:Literal
                                ] ;
                
                rdfs:comment "Description of where a learning object falls within a particular classification system. To define multiple classifications, there may be multiple instances of this category for a learning object."@en .



###  http://data.opendiscoveryspace.eu/lom_ontology_ods.owl#Contribution

:Contribution rdf:type owl:Class ;
              
              rdfs:subClassOf owl:Thing ;
              
              rdfs:comment "Those entities (i.e., people, organizations) that have contributed to the state of this learning object during its life cycle (e.g., creation, edits, publication)."^^xsd:string .



###  http://data.opendiscoveryspace.eu/lom_ontology_ods.owl#DateTime

:DateTime rdf:type owl:Class ;
          
          rdfs:subClassOf owl:Thing ,
                          [ rdf:type owl:Restriction ;
                            owl:onProperty :dateTimeValue ;
                            owl:qualifiedCardinality "1"^^xsd:nonNegativeInteger ;
                            owl:onDataRange xsd:dateTime
                          ] ;
          
          rdfs:comment "A point in time with accuracy at least as small as one second, as described by IEEE LOM in clause 8 (IEEE 1484.12.1-2002)."@en .



###  http://data.opendiscoveryspace.eu/lom_ontology_ods.owl#Duration

:Duration rdf:type owl:Class ;
          
          rdfs:subClassOf owl:Thing ,
                          [ rdf:type owl:Restriction ;
                            owl:onProperty :durationValue ;
                            owl:qualifiedCardinality "1"^^xsd:nonNegativeInteger ;
                            owl:onDataRange rdf:XMLLiteral
                          ] ,
                          [ rdf:type owl:Restriction ;
                            owl:onProperty :durationDescription ;
                            owl:qualifiedCardinality "1"^^xsd:nonNegativeInteger ;
                            owl:onDataRange rdf:XMLLiteral
                          ] ;
          
          rdfs:comment "An interval in time with accuracy at least as small as one second."@en .



###  http://data.opendiscoveryspace.eu/lom_ontology_ods.owl#Educational

:Educational rdf:type owl:Class ;
             
             rdfs:subClassOf owl:Thing ,
                             [ rdf:type owl:Restriction ;
                               owl:onProperty :educationalContext ;
                               owl:maxCardinality "10"^^xsd:nonNegativeInteger
                             ] ,
                             [ rdf:type owl:Restriction ;
                               owl:onProperty :educationalSemanticDensity ;
                               owl:cardinality "1"^^xsd:nonNegativeInteger
                             ] ,
                             [ rdf:type owl:Restriction ;
                               owl:onProperty :educationalInteractivityType ;
                               owl:cardinality "1"^^xsd:nonNegativeInteger
                             ] ,
                             [ rdf:type owl:Restriction ;
                               owl:onProperty :educationalTypicalLearningTime ;
                               owl:onClass :Duration ;
                               owl:qualifiedCardinality "1"^^xsd:nonNegativeInteger
                             ] ,
                             [ rdf:type owl:Restriction ;
                               owl:onProperty :educationalIntendedUserRole ;
                               owl:maxCardinality "10"^^xsd:nonNegativeInteger
                             ] ,
                             [ rdf:type owl:Restriction ;
                               owl:onProperty :educationalInteractivityLevel ;
                               owl:cardinality "1"^^xsd:nonNegativeInteger
                             ] ,
                             [ rdf:type owl:Restriction ;
                               owl:onProperty :educationalLanguage ;
                               owl:maxCardinality "10"^^xsd:nonNegativeInteger
                             ] ,
                             [ rdf:type owl:Restriction ;
                               owl:onProperty :educationalTypicalAgeRange ;
                               owl:onClass :LangString ;
                               owl:maxQualifiedCardinality "5"^^xsd:nonNegativeInteger
                             ] ,
                             [ rdf:type owl:Restriction ;
                               owl:onProperty :educationalDifficulty ;
                               owl:cardinality "1"^^xsd:nonNegativeInteger
                             ] ,
                             [ rdf:type owl:Restriction ;
                               owl:onProperty :description ;
                               owl:onClass :LangString ;
                               owl:maxQualifiedCardinality "10"^^xsd:nonNegativeInteger
                             ] ;
             
             terms:type ""^^rdfs:Literal .



###  http://data.opendiscoveryspace.eu/lom_ontology_ods.owl#Identifier

:Identifier rdf:type owl:Class ;
            
            rdfs:subClassOf owl:Thing ,
                            [ rdf:type owl:Restriction ;
                              owl:onProperty :identifierCatalog ;
                              owl:cardinality "1"^^xsd:nonNegativeInteger
                            ] ;
            
            terms:identifier ""^^rdfs:Literal ;
            
            rdfs:comment "A globally unique label that identifies either a learning object or a learning object metadata record."@en .



###  http://data.opendiscoveryspace.eu/lom_ontology_ods.owl#LangString

:LangString rdf:type owl:Class ;
            
            rdfs:subClassOf owl:Thing ,
                            [ rdf:type owl:Restriction ;
                              owl:onProperty :hasValue ;
                              owl:someValuesFrom rdfs:Literal
                            ] ;
            
            rdfs:comment "Each of the possible semantically equivalent character strings of a langString."@en .



###  http://data.opendiscoveryspace.eu/lom_ontology_ods.owl#LearningObject

:LearningObject rdf:type owl:Class ;
                
                rdfs:subClassOf owl:Thing ,
                                [ rdf:type owl:Restriction ;
                                  owl:onProperty :technicalLocation ;
                                  owl:maxCardinality "10"^^xsd:nonNegativeInteger
                                ] ,
                                [ rdf:type owl:Restriction ;
                                  owl:onProperty :annotation ;
                                  owl:onClass :Annotation ;
                                  owl:maxQualifiedCardinality "30"^^xsd:nonNegativeInteger
                                ] ,
                                [ rdf:type owl:Restriction ;
                                  owl:onProperty :description ;
                                  owl:onClass :LangString ;
                                  owl:maxQualifiedCardinality "10"^^xsd:nonNegativeInteger
                                ] ,
                                [ rdf:type owl:Restriction ;
                                  owl:onProperty :lifeCycleStatus ;
                                  owl:cardinality "1"^^xsd:nonNegativeInteger
                                ] ,
                                [ rdf:type owl:Restriction ;
                                  owl:onProperty :metadataSchema ;
                                  owl:maxCardinality "10"^^xsd:nonNegativeInteger
                                ] ,
                                [ rdf:type owl:Restriction ;
                                  owl:onProperty :technicalSize ;
                                  owl:cardinality "1"^^xsd:nonNegativeInteger
                                ] ,
                                [ rdf:type owl:Restriction ;
                                  owl:onProperty :classification ;
                                  owl:onClass :Classification ;
                                  owl:maxQualifiedCardinality "40"^^xsd:nonNegativeInteger
                                ] ,
                                [ rdf:type owl:Restriction ;
                                  owl:onProperty :metaMetadataLanguage ;
                                  owl:cardinality "1"^^xsd:nonNegativeInteger
                                ] ,
                                [ rdf:type owl:Restriction ;
                                  owl:onProperty :structure ;
                                  owl:cardinality "1"^^xsd:nonNegativeInteger
                                ] ,
                                [ rdf:type owl:Restriction ;
                                  owl:onProperty :keyword ;
                                  owl:onClass :LangString ;
                                  owl:maxQualifiedCardinality "10"^^xsd:nonNegativeInteger
                                ] ,
                                [ rdf:type owl:Restriction ;
                                  owl:onProperty :technicalRequirements ;
                                  owl:onClass :TechnicalRequirement ;
                                  owl:maxQualifiedCardinality "40"^^xsd:nonNegativeInteger
                                ] ,
                                [ rdf:type owl:Restriction ;
                                  owl:onProperty :lifeCycleVersion ;
                                  owl:someValuesFrom rdfs:Literal
                                ] ,
                                [ rdf:type owl:Restriction ;
                                  owl:onProperty :metaMetadataContribution ;
                                  owl:onClass :MetaMetadataContribution ;
                                  owl:maxQualifiedCardinality "10"^^xsd:nonNegativeInteger
                                ] ,
                                [ rdf:type owl:Restriction ;
                                  owl:onProperty :lifeCycleContribution ;
                                  owl:onClass :LifeCycleContribution ;
                                  owl:maxQualifiedCardinality "30"^^xsd:nonNegativeInteger
                                ] ,
                                [ rdf:type owl:Restriction ;
                                  owl:onProperty :educational ;
                                  owl:onClass :Educational ;
                                  owl:maxQualifiedCardinality "100"^^xsd:nonNegativeInteger
                                ] ,
                                [ rdf:type owl:Restriction ;
                                  owl:onProperty :copyrightAndOtherRestrictions ;
                                  owl:qualifiedCardinality "1"^^xsd:nonNegativeInteger ;
                                  owl:onDataRange xsd:boolean
                                ] ,
                                [ rdf:type owl:Restriction ;
                                  owl:onProperty :cost ;
                                  owl:qualifiedCardinality "1"^^xsd:nonNegativeInteger ;
                                  owl:onDataRange xsd:boolean
                                ] ,
                                [ rdf:type owl:Restriction ;
                                  owl:onProperty :technicalInstallationRemarks ;
                                  owl:someValuesFrom rdfs:Literal
                                ] ,
                                [ rdf:type owl:Restriction ;
                                  owl:onProperty :aggregationLevel ;
                                  owl:cardinality "1"^^xsd:nonNegativeInteger
                                ] ,
                                [ rdf:type owl:Restriction ;
                                  owl:onProperty :relation ;
                                  owl:onClass :Relation ;
                                  owl:maxQualifiedCardinality "100"^^xsd:nonNegativeInteger
                                ] ,
                                [ rdf:type owl:Restriction ;
                                  owl:onProperty :identifier ;
                                  owl:onClass :Identifier ;
                                  owl:maxQualifiedCardinality "10"^^xsd:nonNegativeInteger
                                ] ,
                                [ rdf:type owl:Restriction ;
                                  owl:onProperty :technicalDuration ;
                                  owl:onClass :Duration ;
                                  owl:qualifiedCardinality "1"^^xsd:nonNegativeInteger
                                ] ,
                                [ rdf:type owl:Restriction ;
                                  owl:onProperty :metaMetadataIdentifier ;
                                  owl:onClass :Identifier ;
                                  owl:maxQualifiedCardinality "10"^^xsd:nonNegativeInteger
                                ] ,
                                [ rdf:type owl:Restriction ;
                                  owl:onProperty :otherPlatformRequirements ;
                                  owl:someValuesFrom rdfs:Literal
                                ] ,
                                [ rdf:type owl:Restriction ;
                                  owl:onProperty :coverage ;
                                  owl:onClass :LangString ;
                                  owl:maxQualifiedCardinality "10"^^xsd:nonNegativeInteger
                                ] ;
                
                terms:rights ""^^rdfs:Literal ;
                
                terms:publisher ""^^rdfs:Literal ;
                
                terms:language ""^^rdfs:Literal ;
                
                terms:format ""^^rdfs:Literal ;
                
                rdfs:comment "Learning Object" .



###  http://data.opendiscoveryspace.eu/lom_ontology_ods.owl#LifeCycleContribution

:LifeCycleContribution rdf:type owl:Class ;
                       
                       rdfs:subClassOf :Contribution ,
                                       [ rdf:type owl:Restriction ;
                                         owl:onProperty :lifeCycleContributionRole ;
                                         owl:maxCardinality "1"^^xsd:nonNegativeInteger
                                       ] ,
                                       [ rdf:type owl:Restriction ;
                                         owl:onProperty :dateTimeDescription ;
                                         owl:cardinality "1"^^xsd:nonNegativeInteger
                                       ] ,
                                       [ rdf:type owl:Restriction ;
                                         owl:onProperty :dateTimeValue ;
                                         owl:cardinality "1"^^xsd:nonNegativeInteger
                                       ] .



###  http://data.opendiscoveryspace.eu/lom_ontology_ods.owl#MetaMetadataContribution

:MetaMetadataContribution rdf:type owl:Class ;
                          
                          rdfs:subClassOf :Contribution ,
                                          [ rdf:type owl:Restriction ;
                                            owl:onProperty :dateTimeDescription ;
                                            owl:cardinality "1"^^xsd:nonNegativeInteger
                                          ] ,
                                          [ rdf:type owl:Restriction ;
                                            owl:onProperty :metaMetadataContributionRole ;
                                            owl:maxCardinality "1"^^xsd:nonNegativeInteger
                                          ] ,
                                          [ rdf:type owl:Restriction ;
                                            owl:onProperty :dateTimeValue ;
                                            owl:cardinality "1"^^xsd:nonNegativeInteger
                                          ] .



###  http://data.opendiscoveryspace.eu/lom_ontology_ods.owl#Relation

:Relation rdf:type owl:Class ;
          
          rdfs:subClassOf owl:Thing ,
                          [ rdf:type owl:Restriction ;
                            owl:onProperty :relatedResourceDescription ;
                            owl:onClass :LangString ;
                            owl:maxQualifiedCardinality "10"^^xsd:nonNegativeInteger
                          ] ,
                          [ rdf:type owl:Restriction ;
                            owl:onProperty :relationKind ;
                            owl:cardinality "1"^^xsd:nonNegativeInteger
                          ] ,
                          [ rdf:type owl:Restriction ;
                            owl:onProperty :identifier ;
                            owl:onClass :Identifier ;
                            owl:maxQualifiedCardinality "10"^^xsd:nonNegativeInteger
                          ] ;
          
          rdfs:comment "A concept which defines the relationship between a learning object and other learning objects, if any."@en .



###  http://data.opendiscoveryspace.eu/lom_ontology_ods.owl#SingleTechnicalRequirement

:SingleTechnicalRequirement rdf:type owl:Class ;
                            
                            rdfs:subClassOf owl:Thing ,
                                            [ rdf:type owl:Restriction ;
                                              owl:onProperty :orCompositeMaximumVersion ;
                                              owl:maxCardinality "1"^^xsd:nonNegativeInteger
                                            ] ,
                                            [ rdf:type owl:Restriction ;
                                              owl:onProperty :orCompositeType ;
                                              owl:cardinality "1"^^xsd:nonNegativeInteger
                                            ] ,
                                            [ rdf:type owl:Restriction ;
                                              owl:onProperty :orCompositeName ;
                                              owl:cardinality "1"^^xsd:nonNegativeInteger
                                            ] ,
                                            [ rdf:type owl:Restriction ;
                                              owl:onProperty :orCompositeMinimumVersion ;
                                              owl:maxCardinality "1"^^xsd:nonNegativeInteger
                                            ] ;
                            
                            rdfs:comment "A technical capability necessary for using a learning object."@en .



###  http://data.opendiscoveryspace.eu/lom_ontology_ods.owl#Taxon

:Taxon rdf:type owl:Class ;
       
       rdfs:subClassOf owl:Thing ,
                       [ rdf:type owl:Restriction ;
                         owl:onProperty :taxonEntry ;
                         owl:someValuesFrom rdfs:Literal
                       ] ,
                       [ rdf:type owl:Restriction ;
                         owl:onProperty :taxonId ;
                         owl:cardinality "1"^^xsd:nonNegativeInteger
                       ] ;
       
       rdfs:comment """A particular term within a taxonomy. A taxon is a node that has a defined label or
term. A taxon may also have an alphanumeric designation or identifier for standardized reference. Either or both the label and the entry may be used to designate a particular taxon. An ordered list of taxons creates a taxonomic path, i.e., \"taxonomic stairway\": this is a path from a more general to more specific entry in a classification."""@en .



###  http://data.opendiscoveryspace.eu/lom_ontology_ods.owl#TaxonPath

:TaxonPath rdf:type owl:Class ;
           
           rdfs:subClassOf owl:Thing ,
                           [ rdf:type owl:Restriction ;
                             owl:onProperty :taxonpathSource ;
                             owl:someValuesFrom rdfs:Literal
                           ] ,
                           [ rdf:type owl:Restriction ;
                             owl:onProperty :classificationTaxon ;
                             owl:onClass :Taxon ;
                             owl:maxQualifiedCardinality "15"^^xsd:nonNegativeInteger
                           ] ;
           
           rdfs:comment "A taxonomic path in a specific classification system. Each succeeding level is a refinement in the definition of the preceding level. There may be different paths, in the same or different classifications, which describe the same characteristic."@en .



###  http://data.opendiscoveryspace.eu/lom_ontology_ods.owl#TechnicalRequirement

:TechnicalRequirement rdf:type owl:Class ;
                      
                      rdfs:subClassOf owl:Thing ,
                                      [ rdf:type owl:Restriction ;
                                        owl:onProperty :isCompositeOf ;
                                        owl:onClass :SingleTechnicalRequirement ;
                                        owl:maxQualifiedCardinality "40"^^xsd:nonNegativeInteger
                                      ] ;
                      
                      rdfs:comment "The technical capabilities necessary for using a learning object. There can be multiple requirements, in which case all are required, i.e., the logical connector is AND."@en .



###  http://data.opendiscoveryspace.eu/lom_ontology_ods.owl#VCard

:VCard rdf:type owl:Class ;
       
       rdfs:subClassOf owl:Thing ;
       
       ns:email ""^^rdfs:Literal ;
       
       ns:FN ""^^rdfs:Literal ;
       
       ns:N ""^^rdfs:Literal ;
       
       ns:ORG ""^^rdfs:Literal ;
       
       rdfs:comment "A vCard is a collection of one or more properties. A property is a uniquely named value. A set of properties can be grouped within a vCard. For example, the properties for a telephone number and comment can be grouped in order to preserve the coupling of the annotation with the telephone number. In addition to property groupings, a vC. versit  is developing a comprehensive family of PDI technologies based on open specifications and interoperability agreements to help meet this technology need."^^xsd:string .



###  http://www.w3.org/2002/07/owl#Thing

owl:Thing rdf:type owl:Class .





#################################################################
#
#    Individuals
#
#################################################################


###  http://data.opendiscoveryspace.eu/lom_ontology_ods.owl#annotationEntity

:annotationEntity rdf:type owl:NamedIndividual ,
                           owl:Thing ;
                  
                  rdfs:comment "Entity (i.e., people, organization) that created this annotation. IEEE LOM element 8.1."@en .




###  Generated by the OWL API (version 3.5.0) http://owlapi.sourceforge.net

