@prefix dc:    <http://purl.org/dc/elements/1.1/> .
@prefix rdfs:  <http://www.w3.org/2000/01/rdf-schema#> .
@prefix ex:    <http://purl.org/net/ns/ex#> .
@prefix foaf:  <http://xmlns.com/foaf/0.1/> .
@prefix ont:   <http://purl.org/net/ns/ontology-annot#> .
@prefix wn:    <http://xmlns.com/wordnet/1.6/> .
@prefix owl:   <http://www.w3.org/2002/07/owl#> .
@prefix rdf:   <http://www.w3.org/1999/02/22-rdf-syntax-ns#> .
@prefix m:     <http://www.kanzaki.com/ns/music#> .
@prefix dcterms: <http://purl.org/dc/terms/> .

<http://www.kanzaki.com/works/2007/misc/music-vocab-sample2.png>
        a           foaf:Image ;
        rdfs:label  "'circles and arrows' graphical representation of this example" .

m:A-dur  a                   m:Key ;
        rdfs:comment         "Major key based on A, whose key signature has 3 sharps." ;
        rdfs:isDefinedBy     <http://www.kanzaki.com/ns/music> ;
        rdfs:label           "A dur" ;
        dcterms:alternative  "A major" ;
        dcterms:description  <http://en.wikipedia.org/wiki/A_major> .

m:es-moll  a                 m:Key ;
        rdfs:comment         "Minor key based on E flat, whose key signature has 6 flats." ;
        rdfs:isDefinedBy     <http://www.kanzaki.com/ns/music> ;
        rdfs:label           "es moll" ;
        dcterms:alternative  "E-Flat minor" ;
        dcterms:description  <http://en.wikipedia.org/wiki/E_flat_minor> .

m:e-moll  a                  m:Key ;
        rdfs:comment         "Minor key based on E, whose key signature has 1 sharp." ;
        rdfs:isDefinedBy     <http://www.kanzaki.com/ns/music> ;
        rdfs:label           "e moll" ;
        dcterms:alternative  "E minor" ;
        dcterms:description  <http://en.wikipedia.org/wiki/E_minor> .

m:b-moll  a                  m:Key ;
        rdfs:comment         "Minor key based on B flat, whose key signature has 5 flats." ;
        rdfs:isDefinedBy     <http://www.kanzaki.com/ns/music> ;
        rdfs:label           "b moll" ;
        dcterms:alternative  "B-Flat minor" ;
        dcterms:description  <http://en.wikipedia.org/wiki/B_flat_minor> .

m:Woodwind_Instrument
        a                 owl:Class ;
        rdfs:comment      "A wind musical instrument, in which sound is produced by the vibration of reeds in the mouthpiece, or by the passing of air across the mouthpiece." ;
        rdfs:isDefinedBy  <http://www.kanzaki.com/ns/music> ;
        rdfs:label        "Woodwind Instrument" ;
        rdfs:subClassOf   m:Musical_Instrument .

m:artist_description  a   owl:ObjectProperty ;
        rdfs:comment      "A description of the subject artist or agent. Super-property of #plays, #performs." ;
        rdfs:domain       foaf:Agent ;
        rdfs:isDefinedBy  <http://www.kanzaki.com/ns/music> ;
        rdfs:label        "Artist Description" ;
        rdfs:range        owl:Thing .

m:conductorName  a          owl:DatatypeProperty ;
        rdfs:comment        "The subject musical event has a conductor. Literal version of #conductor." ;
        rdfs:isDefinedBy    <http://www.kanzaki.com/ns/music> ;
        rdfs:label          "Conductor Name" ;
        rdfs:subPropertyOf  m:performerName .

m:f-moll  a                  m:Key ;
        rdfs:comment         "Minor key based on F, whose key signature has 4 flats." ;
        rdfs:isDefinedBy     <http://www.kanzaki.com/ns/music> ;
        rdfs:label           "f moll" ;
        dcterms:alternative  "F minor" ;
        dcterms:description  <http://en.wikipedia.org/wiki/F_minor> .

m:Overture  a             owl:Class ;
        rdfs:comment      "An orchestral music composed for the opening of an opera or oratorio, often played as an independend work in concerts" ;
        rdfs:isDefinedBy  <http://www.kanzaki.com/ns/music> ;
        rdfs:label        "Overture" ;
        rdfs:subClassOf   m:Orchestral_Work .

m:as-moll  a                 m:Key ;
        rdfs:comment         "Minor key based on A flat, whose key signature has 7 flats." ;
        rdfs:isDefinedBy     <http://www.kanzaki.com/ns/music> ;
        rdfs:label           "as moll" ;
        dcterms:alternative  "A-Flat minor" ;
        dcterms:description  <http://en.wikipedia.org/wiki/A_flat_minor> .

m:form  a                   owl:DatatypeProperty ;
        rdfs:comment        "The subject musical work or its movement has a form, such as sonata, minuet, etc. Would be better defined as ObjectProperty." ;
        rdfs:domain         m:Musical_Work ;
        rdfs:isDefinedBy    <http://www.kanzaki.com/ns/music> ;
        rdfs:label          "Form" ;
        rdfs:range          rdfs:Literal ;
        rdfs:subPropertyOf  dc:description .

<http://en.wikipedia.org/wiki/F_major>
        a       foaf:Document .

m:Player  a               owl:Class ;
        rdfs:comment      "An artist who performs a musical instrument" ;
        rdfs:isDefinedBy  <http://www.kanzaki.com/ns/music> ;
        rdfs:label        "Player" ;
        rdfs:subClassOf   m:Musician .

m:SopranoClarinet  a      owl:Class ;
        rdfs:comment      "A smaller member of the clarinet family, commonly in key E-flat." ;
        rdfs:isDefinedBy  <http://www.kanzaki.com/ns/music> ;
        rdfs:label        "Soprano Clarinet" ;
        rdfs:subClassOf   m:Clarinet .

m:ais-moll  a                m:Key ;
        rdfs:comment         "Minor key based on A sharp, whose key signature has 7 sharps." ;
        rdfs:isDefinedBy     <http://www.kanzaki.com/ns/music> ;
        rdfs:label           "ais moll" ;
        dcterms:alternative  "A-Sharp minor" ;
        dcterms:description  <http://en.wikipedia.org/wiki/A_sharp_minor> .

<http://en.wikipedia.org/wiki/E_minor>
        a       foaf:Document .

m:Piano  a                owl:Class ;
        rdfs:comment      "A musical instrument with a manual keyboard actuating hammers that strike wire strings. A pianoforte." ;
        rdfs:isDefinedBy  <http://www.kanzaki.com/ns/music> ;
        rdfs:label        "Pian" ;
        rdfs:subClassOf   m:Keyboard_Instrument .

m:Pianist  a              owl:Class ;
        rdfs:comment      "A Piano player" ;
        rdfs:isDefinedBy  <http://www.kanzaki.com/ns/music> ;
        rdfs:label        "Pianist" ;
        rdfs:subClassOf   m:Player ;
        rdfs:subClassOf   [ a                   owl:Restriction ;
                            owl:onProperty      m:plays ;
                            owl:someValuesFrom  m:Piano
                          ] .

m:Chorus  a               owl:Class ;
        rdfs:comment      "A musical group of singers." ;
        rdfs:isDefinedBy  <http://www.kanzaki.com/ns/music> ;
        rdfs:label        "Chorus" ;
        rdfs:subClassOf   m:MusicalGroup .

<http://en.wikipedia.org/wiki/B_major>
        a       foaf:Document .

m:programLine  a            owl:DatatypeProperty ;
        rdfs:comment        "The subject musical event presents a musical work as its program. Literal version of #program." ;
        rdfs:domain         m:Musical_Event ;
        rdfs:isDefinedBy    <http://www.kanzaki.com/ns/music> ;
        rdfs:label          "Program Line" ;
        rdfs:range          rdfs:Literal ;
        rdfs:subPropertyOf  dc:description .

m:opus  a                   owl:DatatypeProperty ;
        rdfs:comment        "The subject musical composition has an identifier assigned by a composer (e.g. 'op.131') or other editor (e.g. 'KV.551')" ;
        rdfs:domain         m:Oeuvre ;
        rdfs:isDefinedBy    <http://www.kanzaki.com/ns/music> ;
        rdfs:label          "Opus" ;
        rdfs:range          rdfs:Literal ;
        rdfs:subPropertyOf  dc:identifier .

m:Oratorio  a             owl:Class ;
        rdfs:comment      "A large musical composition for orchestra, vocal soloists and chorus" ;
        rdfs:isDefinedBy  <http://www.kanzaki.com/ns/music> ;
        rdfs:label        "Oratorio" ;
        rdfs:subClassOf   m:Choral_Music .

m:H-dur  a                   m:Key ;
        rdfs:comment         "Major key based on B, whose key signature has 5 sharps." ;
        rdfs:isDefinedBy     <http://www.kanzaki.com/ns/music> ;
        rdfs:label           "H dur" ;
        dcterms:alternative  "B major" ;
        dcterms:description  <http://en.wikipedia.org/wiki/B_major> .

m:published  a              owl:ObjectProperty ;
        rdfs:comment        "The subject musical work is published as a score or sheet music (still not sure what kind of class is appropriate as the range)" ;
        rdfs:isDefinedBy    <http://www.kanzaki.com/ns/music> ;
        rdfs:label          "published" ;
        rdfs:range          m:Written_Representation ;
        rdfs:subPropertyOf  m:description ;
        ex:example          [ a        ex:Example ;
                              ex:code  "\n<m:Symphony>\n <m:composer foaf:name=\"Beethoven\"/>\n <dc:title>Symphony No.9</dc:title>\n <m:opus>Op.125</m:opus>\n <m:published>\n  <m:Score>\n   <dc:date>1826-08</dc:date>\n   <dc:description>The first published edition</dc:description>\n   <dc:publisher>Schott</dc:publisher>\n  </m:Score>\n </m:published>\n</m:Symphony>\n"
                            ] .

m:Fis-dur  a                 m:Key ;
        rdfs:comment         "Major key based on F sharp, whose key signature has 6 sharps." ;
        rdfs:isDefinedBy     <http://www.kanzaki.com/ns/music> ;
        rdfs:label           "Fis dur" ;
        dcterms:alternative  "F-Sharp major" ;
        dcterms:description  <http://en.wikipedia.org/wiki/F_sharp_major> .

<http://en.wikipedia.org/wiki/A_flat_minor>
        a       foaf:Document .

m:E-dur  a                   m:Key ;
        rdfs:comment         "Major key based on E, whose key signature has 4 sharps." ;
        rdfs:isDefinedBy     <http://www.kanzaki.com/ns/music> ;
        rdfs:label           "E dur" ;
        dcterms:alternative  "E major" ;
        dcterms:description  <http://en.wikipedia.org/wiki/E_major> .

m:cis-moll  a                m:Key ;
        rdfs:comment         "Minor key based on C sharp, whose key signature has 4 sharps." ;
        rdfs:isDefinedBy     <http://www.kanzaki.com/ns/music> ;
        rdfs:label           "cis moll" ;
        dcterms:alternative  "C-Sharp minor" ;
        dcterms:description  <http://en.wikipedia.org/wiki/C_sharp_minor> .

m:Text  a                 owl:Class ;
        rdfs:comment      "Text of a musical work (e.g. lyric or verse)" ;
        rdfs:isDefinedBy  <http://www.kanzaki.com/ns/music> ;
        rdfs:label        "Text" ;
        rdfs:subClassOf   m:Oeuvre .

m:Trumpeter  a            owl:Class ;
        rdfs:comment      "A Trumpet player" ;
        rdfs:isDefinedBy  <http://www.kanzaki.com/ns/music> ;
        rdfs:label        "Trumpeter" ;
        rdfs:subClassOf   m:Player ;
        rdfs:subClassOf   [ a                   owl:Restriction ;
                            owl:onProperty      m:plays ;
                            owl:someValuesFrom  m:Trumpet
                          ] .

m:B-dur  a                   m:Key ;
        rdfs:comment         "Major key based on B flat, whose key signature has 2 flats." ;
        rdfs:isDefinedBy     <http://www.kanzaki.com/ns/music> ;
        rdfs:label           "B dur" ;
        dcterms:alternative  "B-Flat major" ;
        dcterms:description  <http://en.wikipedia.org/wiki/B_flat_major> .

m:Concert  a              owl:Class ;
        rdfs:comment      "An event of musical performance by players or singers not involving theatrical staging" ;
        rdfs:isDefinedBy  <http://www.kanzaki.com/ns/music> ;
        rdfs:label        "Concert" ;
        rdfs:subClassOf   m:Musical_Event .

m:String_Quartet  a       owl:Class ;
        rdfs:comment      "A music composed for instrumental quartet with 2 violins and a viola and a cello. Note 'StringQuartetEnsemble' is SQ ensemble in this vocabulary." ;
        rdfs:isDefinedBy  <http://www.kanzaki.com/ns/music> ;
        rdfs:label        "String Quartet" ;
        rdfs:subClassOf   m:Chamber_Music .

m:Singer  a               owl:Class ;
        rdfs:comment      "An artist who sings a song" ;
        rdfs:isDefinedBy  <http://www.kanzaki.com/ns/music> ;
        rdfs:label        "Singer" ;
        rdfs:subClassOf   m:Musician .

<http://en.wikipedia.org/wiki/A_sharp_minor>
        a       foaf:Document .

m:Composer  a             owl:Class ;
        rdfs:comment      "A person (or any agent) who composed art works" ;
        rdfs:isDefinedBy  <http://www.kanzaki.com/ns/music> ;
        rdfs:label        "Composer" ;
        rdfs:subClassOf   m:Artist .

m:Violin  a               owl:Class ;
        rdfs:comment      "A musical instrument played with a bow, having four strings. Usually plays the highest part of the string section." ;
        rdfs:isDefinedBy  <http://www.kanzaki.com/ns/music> ;
        rdfs:label        "Violin" ;
        rdfs:subClassOf   m:String_Instrument .

m:performs  a               owl:ObjectProperty ;
        rdfs:comment        "The subject artist (or group, machine, etc) performs a musical work." ;
        rdfs:domain         foaf:Agent ;
        rdfs:isDefinedBy    <http://www.kanzaki.com/ns/music> ;
        rdfs:label          "Performs" ;
        rdfs:subPropertyOf  m:artist_description ;
        owl:inverseOf       m:performer .

dc:identifier  a  owl:DatatypeProperty .

m:Harpist  a              owl:Class ;
        rdfs:comment      "A Harp player" ;
        rdfs:isDefinedBy  <http://www.kanzaki.com/ns/music> ;
        rdfs:label        "Harpist" ;
        rdfs:subClassOf   m:Player ;
        rdfs:subClassOf   [ a                   owl:Restriction ;
                            owl:onProperty      m:plays ;
                            owl:someValuesFrom  m:Harp
                          ] .

m:performer  a            owl:ObjectProperty ;
        rdfs:comment      "The subject has a performer (an artist, a group, a machine etc.). The preferred domain of this property is #Performance, so as to model that \"a concert presents a performance (of a musical work) that is realized by this performer\". However, in natural language, we often say that \"a concert has performers who play these musical works\", i.e. the domain of 'performer' is #Musical_Event in this case, and it would be more intuitive model. Hence, the domain is leave unrestricted here for a moment. " ;
        rdfs:isDefinedBy  <http://www.kanzaki.com/ns/music> ;
        rdfs:label        "Performer" ;
        rdfs:range        foaf:Agent ;
        ex:example        [ a        ex:Example ;
                            ex:code  "\n<!--Possibly more intuitive description.-->\n<m:Concert>\n <m:conductor foaf:name=\"Sir Roger Norrington\"/>\n <m:performer foaf:name=\"R.S.O. Stuttgart\"/>\n <m:program>\n  <m:Symphony>\n   <m:composer foaf:name=\"Brahms\"/>\n   <dc:title>Symphony No.2 D major</dc:title>\n  </m:Symphony>\n </m:program>\n</m:Concert>\n\n<!-- An application may infer that:\n{X a m:Concert; m:performer Y; m:program Z.} =>\n{X m:presents [a m:Performance; m:performer Y; m:represents Z] .}\n-->\n"
                          ] ;
        ex:example        [ a        ex:Example ;
                            ex:code  "\n<!--Preferred description.-->\n<m:Concert>\n <m:presents>\n  <m:Performance>\n   <m:conductor foaf:name=\"Sir Roger Norrington\"/>\n   <m:performer foaf:name=\"R.S.O. Stuttgart\"/>\n   <m:represents>\n    <m:Symphony>\n     <m:composer foaf:name=\"Brahms\"/>\n     <dc:title>Symphony No.2 D major</dc:title>\n    </m:Symphony>\n   </m:represents>\n  </m:Performance>\n </m:presents>\n</m:Concert>\n"
                          ] .

m:As-dur  a                  m:Key ;
        rdfs:comment         "Major key based on A flat, whose key signature has 4 flats." ;
        rdfs:isDefinedBy     <http://www.kanzaki.com/ns/music> ;
        rdfs:label           "As dur" ;
        dcterms:alternative  "A-Flat major" ;
        dcterms:description  <http://en.wikipedia.org/wiki/A_flat_major> .

m:Symphonic_Poem  a       owl:Class ;
        rdfs:comment      "An orchestral composition based on a thematic subject" ;
        rdfs:isDefinedBy  <http://www.kanzaki.com/ns/music> ;
        rdfs:label        "Symphonic Poem" ;
        rdfs:subClassOf   m:Orchestral_Work .

<http://en.wikipedia.org/wiki/E_flat_minor>
        a       foaf:Document .

m:F-dur  a                   m:Key ;
        rdfs:comment         "Major key based on F, whose key signature has 1 flat." ;
        rdfs:isDefinedBy     <http://www.kanzaki.com/ns/music> ;
        rdfs:label           "F dur" ;
        dcterms:alternative  "F major" ;
        dcterms:description  <http://en.wikipedia.org/wiki/F_major> .

<http://en.wikipedia.org/wiki/B_flat_minor>
        a       foaf:Document .

m:Es-dur  a                  m:Key ;
        rdfs:comment         "Major key based on E flat, whose key signature has 3 flats." ;
        rdfs:isDefinedBy     <http://www.kanzaki.com/ns/music> ;
        rdfs:label           "Es dur" ;
        dcterms:alternative  "E-Flat major" ;
        dcterms:description  <http://en.wikipedia.org/wiki/E_flat_major> .

m:MezzoSoprano  a         owl:Class ;
        rdfs:comment      "A Mezzo Soprano singer" ;
        rdfs:isDefinedBy  <http://www.kanzaki.com/ns/music> ;
        rdfs:label        "Mezzo Soprano" ;
        rdfs:subClassOf   m:Singer .

m:Musical_Event  a        owl:Class ;
        rdfs:comment      "An event of musical performance by players or singers, including theatrical staging. Typically the event has date and location. Note this is different from Performance, which is a 'representation' of a musical work realized at a musical event or recording, etc." ;
        rdfs:isDefinedBy  <http://www.kanzaki.com/ns/music> ;
        rdfs:label        "Musical Event" .

m:Musical_Work  a         owl:Class ;
        rdfs:comment      "A musical work in any form, e.g. a composition, its movement, phrase, theme etc." ;
        rdfs:isDefinedBy  <http://www.kanzaki.com/ns/music> ;
        rdfs:label        "Musical Work" .

m:C-dur  a                   m:Key ;
        rdfs:comment         "Major key based on C, whose key signature has no sharp or flat." ;
        rdfs:isDefinedBy     <http://www.kanzaki.com/ns/music> ;
        rdfs:label           "C dur" ;
        dcterms:alternative  "C major" ;
        dcterms:description  <http://en.wikipedia.org/wiki/C_major> .

m:Alto  a                 owl:Class ;
        rdfs:comment      "An Alto singer" ;
        rdfs:isDefinedBy  <http://www.kanzaki.com/ns/music> ;
        rdfs:label        "Alto" ;
        rdfs:subClassOf   m:Singer .

m:soloist  a                owl:ObjectProperty ;
        rdfs:comment        "The subject performance is performed by this soloist (or the subject musical event has a soloist. See comment of #performer." ;
        rdfs:isDefinedBy    <http://www.kanzaki.com/ns/music> ;
        rdfs:label          "Soloist" ;
        rdfs:subPropertyOf  m:performer .

<http://en.wikipedia.org/wiki/E_major>
        a       foaf:Document .

m:premiere  a               owl:ObjectProperty ;
        rdfs:comment        "The subject musical work was first performed at an concert" ;
        rdfs:isDefinedBy    <http://www.kanzaki.com/ns/music> ;
        rdfs:label          "Premiere" ;
        rdfs:range          m:Musical_Event ;
        rdfs:subPropertyOf  m:description ;
        ex:example          [ a        ex:Example ;
                              ex:code  "\n<m:Symphony>\n <m:composer foaf:name=\"Shubert\"/>\n <dc:title>Symohony No.7 'Unfinished'</dc:title>\n <m:opus>D.759</m:opus>\n <dcterms:created>1822-01</dcterms:created>\n <m:premiere rdf:parseType=\"Resource\">\n  <dc:date>1865-12-17</dc:date>\n  <cal:location>Wien Musikfereinsall</cal:location>\n </m:premiere>\n</m:Symphony>\n"
                            ] .

m:Ballet  a               owl:Class ;
        rdfs:comment      "A musical work for a dance form featuring a staged presentation of group or solo dancing. Note 'Ballet_Event' in this vocabulary describes the performance of a ballet." ;
        rdfs:isDefinedBy  <http://www.kanzaki.com/ns/music> ;
        rdfs:label        "Ballet (Work)" ;
        rdfs:subClassOf   m:Oeuvre .

m:CelestaPlayer  a        owl:Class ;
        rdfs:comment      "A Celesta player" ;
        rdfs:isDefinedBy  <http://www.kanzaki.com/ns/music> ;
        rdfs:label        "CelestaPlayer" ;
        rdfs:subClassOf   m:Player ;
        rdfs:subClassOf   [ a                   owl:Restriction ;
                            owl:onProperty      m:plays ;
                            owl:someValuesFrom  m:Celesta
                          ] .

m:Piccolo  a              owl:Class ;
        rdfs:comment      "A piccolo flute, smaller member of the flute family." ;
        rdfs:isDefinedBy  <http://www.kanzaki.com/ns/music> ;
        rdfs:label        "Piccolo" ;
        rdfs:subClassOf   m:Flute .

m:composition  a            owl:ObjectProperty ;
        rdfs:comment        "Describes the composition process of the subject. Composition period or completion date, place, revision etc. can be described as properties of the object composition process." ;
        rdfs:isDefinedBy    <http://www.kanzaki.com/ns/music> ;
        rdfs:label          "Composition" ;
        rdfs:subPropertyOf  m:description .

m:EnglishHorn  a          owl:Class ;
        rdfs:comment      "A double-reed woodwind instrument, larger member of the oboe family." ;
        rdfs:isDefinedBy  <http://www.kanzaki.com/ns/music> ;
        rdfs:label        "English Horn" ;
        rdfs:subClassOf   m:Oboe .

<http://en.wikipedia.org/wiki/D_minor>
        a       foaf:Document .

m:Contrafagotto  a        owl:Class ;
        rdfs:comment      "A larger mebmer of the basoon family, producing the lowest tone in the woodwind section." ;
        rdfs:isDefinedBy  <http://www.kanzaki.com/ns/music> ;
        rdfs:label        "Contrafagotto" ;
        rdfs:subClassOf   m:Bassoon .

dcterms:alternative  a  owl:DatatypeProperty .

m:Opera_Performance  a       owl:Class , owl:DeprecatedClass ;
        owl:equivalentClass  m:Opera_Event .

m:key   a                   owl:ObjectProperty ;
        rdfs:comment        "The subject musical work or its movement has a key, such as C major, d minor, etc." ;
        rdfs:domain         m:Musical_Work ;
        rdfs:isDefinedBy    <http://www.kanzaki.com/ns/music> ;
        rdfs:label          "Key" ;
        rdfs:range          m:Key ;
        rdfs:subPropertyOf  m:description .

<http://en.wikipedia.org/wiki/A_major>
        a       foaf:Document .

m:Percussionist  a        owl:Class ;
        rdfs:comment      "A Percussion player" ;
        rdfs:isDefinedBy  <http://www.kanzaki.com/ns/music> ;
        rdfs:label        "Percussionist" ;
        rdfs:subClassOf   m:Player ;
        rdfs:subClassOf   [ a                   owl:Restriction ;
                            owl:onProperty      m:plays ;
                            owl:someValuesFrom  m:Percussion
                          ] .

m:Timpani  a              owl:Class ;
        rdfs:comment      "A set of large copper or brass hemispherical drums with a parchment head that can be tuned by adjusting the tension." ;
        rdfs:isDefinedBy  <http://www.kanzaki.com/ns/music> ;
        rdfs:label        "Timpani" ;
        rdfs:subClassOf   m:Percussion .

<http://en.wikipedia.org/wiki/D_sharp_minor>
        a       foaf:Document .

m:Ensemble  a             owl:Class ;
        rdfs:comment      "A musical group which perfroms in relatively small size, particularly chamber music" ;
        rdfs:isDefinedBy  <http://www.kanzaki.com/ns/music> ;
        rdfs:label        "Ensemble" ;
        rdfs:subClassOf   m:MusicalGroup .

m:gis-moll  a                m:Key ;
        rdfs:comment         "Minor key based on G sharp, whose key signature has 5 sharps." ;
        rdfs:isDefinedBy     <http://www.kanzaki.com/ns/music> ;
        rdfs:label           "gis moll" ;
        dcterms:alternative  "G-Sharp minor" ;
        dcterms:description  <http://en.wikipedia.org/wiki/G_sharp_minor> .

dc:creator  a   owl:ObjectProperty .

m:Flute  a                owl:Class ;
        rdfs:comment      "A high-pitched woodwind instrument; a slender tube closed at one end with finger holes on one end and an opening near the closed end across which the breath is blown" ;
        rdfs:isDefinedBy  <http://www.kanzaki.com/ns/music> ;
        rdfs:label        "Flute" ;
        rdfs:subClassOf   m:Woodwind_Instrument .

m:Chamber_Music  a        owl:Class ;
        rdfs:comment      "A genre of music composed for performance by small ensemble" ;
        rdfs:isDefinedBy  <http://www.kanzaki.com/ns/music> ;
        rdfs:label        "Chamber Music" ;
        rdfs:subClassOf   m:Oeuvre .

m:Flutist  a              owl:Class ;
        rdfs:comment      "A Flute player" ;
        rdfs:isDefinedBy  <http://www.kanzaki.com/ns/music> ;
        rdfs:label        "Flutist" ;
        rdfs:subClassOf   m:Player ;
        rdfs:subClassOf   [ a                   owl:Restriction ;
                            owl:onProperty      m:plays ;
                            owl:someValuesFrom  m:Flute
                          ] .

m:Orchestral_Work  a      owl:Class ;
        rdfs:comment      "A composition for orchestra (and a soloist or soloists, optionally with chorus)" ;
        rdfs:isDefinedBy  <http://www.kanzaki.com/ns/music> ;
        rdfs:label        "Orchestral Work" ;
        rdfs:subClassOf   m:Oeuvre .

m:program  a                owl:ObjectProperty ;
        rdfs:comment        "The subject musical event presents a musical work as its program" ;
        rdfs:isDefinedBy    <http://www.kanzaki.com/ns/music> ;
        rdfs:label          "Program" ;
        rdfs:range          m:Oeuvre ;
        rdfs:subPropertyOf  m:event_description .

m:Viola  a                owl:Class ;
        rdfs:comment      "A stringed instrument of the violin family, slightly larger than a violin, tuned a fifth lower, and having a deeper, more sonorous tone." ;
        rdfs:isDefinedBy  <http://www.kanzaki.com/ns/music> ;
        rdfs:label        "Viola" ;
        rdfs:subClassOf   m:String_Instrument .

m:Cantata  a              owl:Class ;
        rdfs:comment      "A vocal composition accompanied by instruments and generally containing more than one movement." ;
        rdfs:isDefinedBy  <http://www.kanzaki.com/ns/music> ;
        rdfs:label        "Cantata" ;
        rdfs:subClassOf   m:Choral_Music .

m:Harp  a                 owl:Class ;
        rdfs:comment      "An instrument with usually 46 or 47 strings that are played by plucking with the fingers." ;
        rdfs:isDefinedBy  <http://www.kanzaki.com/ns/music> ;
        rdfs:label        "Harp" ;
        rdfs:subClassOf   m:String_Instrument .

m:StringQuartetEnsemble
        a                 owl:Class ;
        rdfs:comment      "A musical group of four string players. Note 'String_Quartette' is SQ as musical work in this vocabulary." ;
        rdfs:isDefinedBy  <http://www.kanzaki.com/ns/music> ;
        rdfs:label        "Qtring Quartet" ;
        rdfs:subClassOf   m:MusicalGroup .

m:Movement  a             owl:Class ;
        rdfs:comment      "A subsection of a musical work. Typically a movement of a symphony, but also a piece of suit, etc." ;
        rdfs:isDefinedBy  <http://www.kanzaki.com/ns/music> ;
        rdfs:label        "Movement" ;
        rdfs:subClassOf   m:Musical_Work .

m:Guitarist  a            owl:Class ;
        rdfs:comment      "A Guitar player" ;
        rdfs:isDefinedBy  <http://www.kanzaki.com/ns/music> ;
        rdfs:label        "Guitarist" ;
        rdfs:subClassOf   m:Player ;
        rdfs:subClassOf   [ a                   owl:Restriction ;
                            owl:onProperty      m:plays ;
                            owl:someValuesFrom  m:Guitar
                          ] .

m:G-dur  a                   m:Key ;
        rdfs:comment         "Major key based on G, whose key signature has 1 sharp." ;
        rdfs:isDefinedBy     <http://www.kanzaki.com/ns/music> ;
        rdfs:label           "G dur" ;
        dcterms:alternative  "G major" ;
        dcterms:description  <http://en.wikipedia.org/wiki/G_major> .

m:Ballet_Event  a         owl:Class ;
        rdfs:comment      "An event of ballet performance\n  " ;
        rdfs:isDefinedBy  <http://www.kanzaki.com/ns/music> ;
        rdfs:label        "Ballet Event" ;
        rdfs:subClassOf   m:Musical_Event .

m:Opera_Event  a          owl:Class ;
        rdfs:comment      "An event of opera performance (not an opera as a musical work, which is defined here as 'Opera')" ;
        rdfs:isDefinedBy  <http://www.kanzaki.com/ns/music> ;
        rdfs:label        "Opera Event" ;
        rdfs:subClassOf   m:Musical_Event .

m:Bass  a                 owl:Class ;
        rdfs:comment      "A Bass singer" ;
        rdfs:isDefinedBy  <http://www.kanzaki.com/ns/music> ;
        rdfs:label        "Bass" ;
        rdfs:subClassOf   m:Singer .

m:Written_Representation
        a                 owl:Class ;
        rdfs:comment      "Representation of a musical work in the form of a written expression, e.g. score, parts, autograph, printed music, sketch, etc." ;
        rdfs:isDefinedBy  <http://www.kanzaki.com/ns/music> ;
        rdfs:label        "Written Representation" ;
        rdfs:subClassOf   m:Musical_Representation .

m:D-dur  a                   m:Key ;
        rdfs:comment         "Major key based on D, whose key signature has 2 sharps." ;
        rdfs:isDefinedBy     <http://www.kanzaki.com/ns/music> ;
        rdfs:label           "D dur" ;
        dcterms:alternative  "D major" ;
        dcterms:description  <http://en.wikipedia.org/wiki/D_major> .

m:Oeuvre  a               owl:Class ;
        rdfs:comment      "A (complete) musical work by a composer." ;
        rdfs:isDefinedBy  <http://www.kanzaki.com/ns/music> ;
        rdfs:label        "Oeuvre" ;
        rdfs:subClassOf   m:Musical_Work .

m:Baritone  a             owl:Class ;
        rdfs:comment      "A Baritone singer" ;
        rdfs:isDefinedBy  <http://www.kanzaki.com/ns/music> ;
        rdfs:label        "Baritone" ;
        rdfs:subClassOf   m:Singer .

m:Clarinet  a             owl:Class ;
        rdfs:comment      "A woodwind instrument having a straight cylindrical tube with a flaring bell and a single-reed mouthpiece." ;
        rdfs:isDefinedBy  <http://www.kanzaki.com/ns/music> ;
        rdfs:label        "Clarinet" ;
        rdfs:subClassOf   m:Woodwind_Instrument .

[ a             ex:Example ;
  rdfs:comment  "交響曲の楽曲情報と楽章データの記述例。調性の記述をURIに変更。"@ja , "A description of a symphony with its composition data and descriptions of movements. Note now key values are expressed as URIs." ;
  ex:code       "\n<m:Symphony>\n <m:composer rdf:parseType=\"Resource\">\n  <foaf:name>シューベルト</foaf:name>\n  <foaf:homepage rdf:resource=\"http://www.kanzaki.com/music/mw/sym/schubert\"/>\n </m:composer>\n <dc:title>Symohony No.7 'Unfinished'</dc:title>\n <m:opus>D.759</m:opus>\n <m:key rdf:resource=\"http://www.kanzaki.com/ns/music#h-moll\"/>\n <dcterms:created>1822-01</dcterms:created>\n <m:premiere rdf:parseType=\"Resource\">\n  <dc:date>1865-12-17</dc:date>\n  <cal:location>Wien Musikfereinsall</cal:location>\n </m:premiere>\n <m:sections rdf:parseType=\"Collection\">\n  <m:Movement>\n   <m:marks>Allegro moderato</m:marks>\n   <m:key rdf:resource=\"http://www.kanzaki.com/ns/music#h-moll\"/>\n   <m:meter>3/4</m:meter>\n  </m:Movement>\n  <m:Movement>\n   <m:marks>Andante con moto</m:marks>\n   <m:key rdf:resource=\"http://www.kanzaki.com/ns/music#Es-dur\"/>\n   <m:meter>3/8</m:meter>\n  </m:Movement>\n </m:sections>\n</m:Symphony>\n " ;
  ex:exampleOf  <http://www.kanzaki.com/ns/music> ;
  ex:image      <http://www.kanzaki.com/works/2007/misc/music-vocab-sample3.png> ;
  ex:pfx        "m:" ;
  ex:trial      <http://purl.org/net/masterwork/schubert/D.759>
] .

m:Violist  a              owl:Class ;
        rdfs:comment      "A Viola player" ;
        rdfs:isDefinedBy  <http://www.kanzaki.com/ns/music> ;
        rdfs:label        "Violist" ;
        rdfs:subClassOf   m:Player ;
        rdfs:subClassOf   [ a                   owl:Restriction ;
                            owl:onProperty      m:plays ;
                            owl:someValuesFrom  m:Viola
                          ] .

m:Musical_Representation
        a                 owl:Class ;
        rdfs:comment      "Representation of a musical work, such as a score, sheet music, perfornamce, recoding, etc." ;
        rdfs:isDefinedBy  <http://www.kanzaki.com/ns/music> ;
        rdfs:label        "Musical Representation" .

dc:source  a    owl:ObjectProperty .

dc:description  a  owl:DatatypeProperty .

m:derivedFrom  a            owl:ObjectProperty ;
        rdfs:comment        "The subject is (was) derived from the object, e.g a copy score is derived from the composer manuscript (or, possibly, a CD recording is derived from a performance at a concert)." ;
        rdfs:domain         m:Musical_Representation ;
        rdfs:isDefinedBy    <http://www.kanzaki.com/ns/music> ;
        rdfs:label          "Derived From" ;
        rdfs:range          m:Musical_Representation ;
        rdfs:subPropertyOf  dc:source ;
        ex:example          [ a        ex:Example ;
                              ex:code  "\n<m:Symphony rdf:about=\"http://purl.org/net/masterwork/beethoven/op.125\">\n <m:source>\n  <m:Score rdf:about=\"urn:musicalsource:lvb/125/autograph\">\n   <dc:title>Autograph score</dc:title>\n  </m:Score>\n </m:source>\n <m:source>\n  <m:Score rdf:about=\"urn:musicalsource:lvb/125/copystscore1\">\n   <dc:title>A copyist's socore used as engraver's copy</dc:title>\n   <m:derivedFrom rdf:resource=\"urn:musicalsource:lvb/125/autograph\"/>\n  </m:Score>\n </m:source>\n</m:Symphony>\n"
                            ] .

m:Countertenor  a         owl:Class ;
        rdfs:comment      "A Countertenor singer" ;
        rdfs:isDefinedBy  <http://www.kanzaki.com/ns/music> ;
        rdfs:label        "Countertenor" ;
        rdfs:subClassOf   m:Singer .

m:Tuba  a                 owl:Class ;
        rdfs:comment      "A large, valved, brass instrument with a bass pitch." ;
        rdfs:isDefinedBy  <http://www.kanzaki.com/ns/music> ;
        rdfs:label        "Tuba" ;
        rdfs:subClassOf   m:Brass_Instrument .

m:c-moll  a                  m:Key ;
        rdfs:comment         "Minor key based on C, whose key signature has 3 flats." ;
        rdfs:isDefinedBy     <http://www.kanzaki.com/ns/music> ;
        rdfs:label           "c moll" ;
        dcterms:alternative  "C minor" ;
        dcterms:description  <http://en.wikipedia.org/wiki/C_minor> .

m:marks  a                  owl:DatatypeProperty ;
        rdfs:comment        "The subject musical work or its movement has instruction mark(s) of tempo and/or expression" ;
        rdfs:domain         m:Musical_Work ;
        rdfs:isDefinedBy    <http://www.kanzaki.com/ns/music> ;
        rdfs:label          "Marks" ;
        rdfs:range          rdfs:Literal ;
        rdfs:subPropertyOf  dc:description .

m:Bassoon  a              owl:Class ;
        rdfs:comment      "A low-pitched woodwind instrument with a double reed, having a long wooden body attached to a U-shaped lateral tube that leads to the mouthpiece. A Fagotto." ;
        rdfs:isDefinedBy  <http://www.kanzaki.com/ns/music> ;
        rdfs:label        "Bassoon" ;
        rdfs:subClassOf   m:Woodwind_Instrument .

m:Hornist  a              owl:Class ;
        rdfs:comment      "A Horn player" ;
        rdfs:isDefinedBy  <http://www.kanzaki.com/ns/music> ;
        rdfs:label        "Hornist" ;
        rdfs:subClassOf   m:Player ;
        rdfs:subClassOf   [ a                   owl:Restriction ;
                            owl:onProperty      m:plays ;
                            owl:someValuesFrom  m:Horn
                          ] .

m:g-moll  a                  m:Key ;
        rdfs:comment         "Minor key based on G, whose key signature has 2 flats." ;
        rdfs:isDefinedBy     <http://www.kanzaki.com/ns/music> ;
        rdfs:label           "g moll" ;
        dcterms:alternative  "G minor" ;
        dcterms:description  <http://en.wikipedia.org/wiki/G_minor> .

m:Harpsichord  a          owl:Class ;
        rdfs:comment      "A keyboard instrument whose strings are plucked by means of quills or plectrums. Cembalo." ;
        rdfs:isDefinedBy  <http://www.kanzaki.com/ns/music> ;
        rdfs:label        "Harpsichord" ;
        rdfs:subClassOf   m:Keyboard_Instrument .

m:Concerto  a             owl:Class ;
        rdfs:comment      "A composition for orchestra and a soloist" ;
        rdfs:isDefinedBy  <http://www.kanzaki.com/ns/music> ;
        rdfs:label        "Concerto" ;
        rdfs:subClassOf   m:Orchestral_Work .

m:PiccoloPlayer  a        owl:Class ;
        rdfs:comment      "A Piccolo flute player" ;
        rdfs:isDefinedBy  <http://www.kanzaki.com/ns/music> ;
        rdfs:label        "Piccolo player" ;
        rdfs:subClassOf   m:Flutist ;
        rdfs:subClassOf   [ a                   owl:Restriction ;
                            owl:onProperty      m:plays ;
                            owl:someValuesFrom  m:Piccolo
                          ] .

m:d-moll  a                  m:Key ;
        rdfs:comment         "Minor key based on D, whose key signature has 1 flat." ;
        rdfs:isDefinedBy     <http://www.kanzaki.com/ns/music> ;
        rdfs:label           "d moll" ;
        dcterms:alternative  "D minor" ;
        dcterms:description  <http://en.wikipedia.org/wiki/D_minor> .

<http://en.wikipedia.org/wiki/F_sharp_major>
        a       foaf:Document .

m:Artist  a               owl:Class ;
        rdfs:comment      "A person or group (or any agent) who creates or performs art works" ;
        rdfs:isDefinedBy  <http://www.kanzaki.com/ns/music> ;
        rdfs:label        "Artist" ;
        rdfs:subClassOf   foaf:Agent .

<http://en.wikipedia.org/wiki/G_minor>
        a       foaf:Document .

m:h-moll  a                  m:Key ;
        rdfs:comment         "Minor key based on B, whose key signature has 2 sharps." ;
        rdfs:isDefinedBy     <http://www.kanzaki.com/ns/music> ;
        rdfs:label           "h moll" ;
        dcterms:alternative  "B minor" ;
        dcterms:description  <http://en.wikipedia.org/wiki/B_minor> .

m:Mandolin  a             owl:Class ;
        rdfs:comment      "A pear-shaped small stringed instrument descended from the lute, played with a pick." ;
        rdfs:isDefinedBy  <http://www.kanzaki.com/ns/music> ;
        rdfs:label        "Mandolin" ;
        rdfs:subClassOf   m:String_Instrument .

m:Trumpet  a              owl:Class ;
        rdfs:comment      "A A soprano brass instrument consisting of a long metal tube looped once and ending in a flared bell, usually being equipped with valves or pistons." ;
        rdfs:isDefinedBy  <http://www.kanzaki.com/ns/music> ;
        rdfs:label        "Trumpet" ;
        rdfs:subClassOf   m:Brass_Instrument .

m:Suite  a                owl:Class ;
        rdfs:comment      "A musical composition of several movements only loosely connected" ;
        rdfs:isDefinedBy  <http://www.kanzaki.com/ns/music> ;
        rdfs:label        "Suite" ;
        rdfs:subClassOf   m:Oeuvre .

m:Venue  a                owl:Class ;
        rdfs:comment      "A venue for musical performance, e.g. concert hall, opera house, recital hall, etc." ;
        rdfs:isDefinedBy  <http://www.kanzaki.com/ns/music> ;
        rdfs:label        "Venue" .

m:fis-moll  a                m:Key ;
        rdfs:comment         "Minor key based on F sharp, whose key signature has 3 sharps." ;
        rdfs:isDefinedBy     <http://www.kanzaki.com/ns/music> ;
        rdfs:label           "fis moll" ;
        dcterms:alternative  "F-Sharp minor" ;
        dcterms:description  <http://en.wikipedia.org/wiki/F_sharp_minor> .

m:conductor  a              owl:ObjectProperty ;
        rdfs:comment        "The subject performance is coducted by the object (or the subject musical event has a conductor). See comment of #performer." ;
        rdfs:isDefinedBy    <http://www.kanzaki.com/ns/music> ;
        rdfs:label          "Conductor" ;
        rdfs:subPropertyOf  m:performer .

m:BassClarinettist  a     owl:Class ;
        rdfs:comment      "A Bass Clarinet player" ;
        rdfs:isDefinedBy  <http://www.kanzaki.com/ns/music> ;
        rdfs:label        "Bass_Clarinettist" ;
        rdfs:subClassOf   m:Clarinettist ;
        rdfs:subClassOf   [ a                   owl:Restriction ;
                            owl:onProperty      m:plays ;
                            owl:someValuesFrom  m:BassClarinet
                          ] .

<http://en.wikipedia.org/wiki/D_major>
        a       foaf:Document .

<http://en.wikipedia.org/wiki/G_sharp_minor>
        a       foaf:Document .

m:Bassoonist  a           owl:Class ;
        rdfs:comment      "A Fagotto player" ;
        rdfs:isDefinedBy  <http://www.kanzaki.com/ns/music> ;
        rdfs:label        "Bassoonist" ;
        rdfs:subClassOf   m:Player ;
        rdfs:subClassOf   [ a                   owl:Restriction ;
                            owl:onProperty      m:plays ;
                            owl:someValuesFrom  m:Bassoon
                          ] .

<http://en.wikipedia.org/wiki/C_minor>
        a       foaf:Document .

m:performerName  a          owl:DatatypeProperty ;
        rdfs:comment        "The subject musical event has a performer. Literal version of #performer." ;
        rdfs:domain         m:Musical_Event ;
        rdfs:isDefinedBy    <http://www.kanzaki.com/ns/music> ;
        rdfs:label          "PerformerName" ;
        rdfs:range          rdfs:Literal ;
        rdfs:subPropertyOf  dc:description .

<http://www.kanzaki.com/ns/music-rdfs.rdf>
        a       owl:Ontology .

m:Percussion  a           owl:Class ;
        rdfs:comment      "A musical instrument that produces sound by striking the body." ;
        rdfs:isDefinedBy  <http://www.kanzaki.com/ns/music> ;
        rdfs:label        "Percussion" ;
        rdfs:subClassOf   m:Musical_Instrument .

m:source  a                 owl:ObjectProperty ;
        rdfs:comment        "The subject musical work has a historical source, such as sketch, autograph score or published score." ;
        rdfs:isDefinedBy    <http://www.kanzaki.com/ns/music> ;
        rdfs:label          "Source" ;
        rdfs:range          m:Written_Representation ;
        rdfs:subPropertyOf  m:description .

m:Performance  a          owl:Class ;
        rdfs:comment      "Representation of a musical work in the form of performace, e.g. playing instruments, singing etc. Note a concert is a Musical_Event where a Performance is presented." ;
        rdfs:isDefinedBy  <http://www.kanzaki.com/ns/music> ;
        rdfs:label        "Peroformance" ;
        rdfs:subClassOf   m:Musical_Representation .

m:Musical_Instrument  a   owl:Class ;
        rdfs:comment      "An instrument to play music" ;
        rdfs:isDefinedBy  <http://www.kanzaki.com/ns/music> ;
        rdfs:label        "Musical Instrument" .

m:Part  a                 owl:Class ;
        rdfs:comment      "A music for a particular instrument or voice taken from a full score (Note: in this ontology, Part is not a division of an orchestra)." ;
        rdfs:isDefinedBy  <http://www.kanzaki.com/ns/music> ;
        rdfs:label        "Part" ;
        rdfs:subClassOf   m:Written_Representation .

m:MusicDirector  a        owl:Class ;
        rdfs:comment      "The person who leads a musical group" ;
        rdfs:isDefinedBy  <http://www.kanzaki.com/ns/music> ;
        rdfs:label        "Music Director" ;
        rdfs:subClassOf   m:Musician , m:Director .

m:Director  a             owl:Class ;
        rdfs:comment      "An artist who directs a musical group" ;
        rdfs:isDefinedBy  <http://www.kanzaki.com/ns/music> ;
        rdfs:label        "Director" ;
        rdfs:subClassOf   m:Artist .

m:sections  a               owl:ObjectProperty ;
        rdfs:comment        "The subject musical work has subsections such as movements. Current model recommends RDF Collection as the object." ;
        rdfs:domain         m:Oeuvre ;
        rdfs:isDefinedBy    <http://www.kanzaki.com/ns/music> ;
        rdfs:label          "Sections" ;
        rdfs:range          owl:Thing ;
        rdfs:subPropertyOf  m:description .

m:BassetHorn  a           owl:Class ;
        rdfs:comment      "A larger member of the clarinet family, typically in lower F, and has darker and less brilliant timbre." ;
        rdfs:isDefinedBy  <http://www.kanzaki.com/ns/music> ;
        rdfs:label        "Basset Horn" ;
        rdfs:subClassOf   m:Clarinet .

m:plays  a                  owl:ObjectProperty ;
        rdfs:comment        "The subject artist (or group, machine, etc) plays an musical instrument. If :me :plays :Violin, then :me a :Violininst." ;
        rdfs:isDefinedBy    <http://www.kanzaki.com/ns/music> ;
        rdfs:label          "Plays" ;
        rdfs:range          m:Musical_Instrument ;
        rdfs:subPropertyOf  m:artist_description .

m:Choreographer  a        owl:Class ;
        rdfs:comment      "someone who creates new dances, or directs an opera" ;
        rdfs:isDefinedBy  <http://www.kanzaki.com/ns/music> ;
        rdfs:label        "Choreographer" ;
        rdfs:subClassOf   m:Director .

m:Des-dur  a                 m:Key ;
        rdfs:comment         "Major key based on D flat, whose key signature has 5 flats." ;
        rdfs:isDefinedBy     <http://www.kanzaki.com/ns/music> ;
        rdfs:label           "Des dur" ;
        dcterms:alternative  "D-Flat major" ;
        dcterms:description  <http://en.wikipedia.org/wiki/D_flat_major> .

m:Contrabass  a           owl:Class ;
        rdfs:comment      "The largest member of string insrtument, usually with four or five strings." ;
        rdfs:isDefinedBy  <http://www.kanzaki.com/ns/music> ;
        rdfs:label        "Contrabass" ;
        rdfs:subClassOf   m:String_Instrument .

<http://en.wikipedia.org/wiki/C_sharp_minor>
        a       foaf:Document .

m:description  a          owl:ObjectProperty ;
        rdfs:comment      "A description of the subject musical work. Super-property of some properties in this vocabulary, as well as description of a general descriptive resource such as time-line of composing process." ;
        rdfs:domain       m:Musical_Work ;
        rdfs:isDefinedBy  <http://www.kanzaki.com/ns/music> ;
        rdfs:label        "Description" ;
        rdfs:range        owl:Thing .

m:Brass_Instrument  a     owl:Class ;
        rdfs:comment      "A wind musical instrument, that consists of a brass tube  blown by means of a cup-shaped or funnel-shaped mouthpiece." ;
        rdfs:isDefinedBy  <http://www.kanzaki.com/ns/music> ;
        rdfs:label        "Brass Instrument" ;
        rdfs:subClassOf   m:Musical_Instrument .

[ a             ex:Example ;
  rdfs:comment  "演奏会の簡単な記述例。"@ja , "A simple description of a concert." ;
  ex:code       "\n<m:Concert>\n <dc:date>2008-02-11</dc:date>\n <m:conductor>\n  <m:Conductor rdf:about=\"http://www.kanzaki.com/bass/conductor#長田雅人\">\n   <foaf:name>Masato Osada</foaf:name>\n  </m:Conductor>\n </m:conductor>\n <m:performer>\n  <m:Orchestra rdf:about=\"http://www.kanzaki.com/bass/orch#オーケストラ・ダスビダーニャ\">\n   <foaf:name>orchestra 'do svidanya'</foaf:name>\n  </m:Orchestra>\n </m:performer>\n <m:program>\n  <m:Symphony rdf:about=\"http://www.kanzaki.com/music/mcat/shostakovich/op.103#s\">\n   <dc:title>Symphony No.11 g-minor</dc:title>\n   <m:opus>op.103</m:opus>\n   <m:composer>\n    <m:Composer rdf:about=\"http://www.kanzaki.com/ns/psi/en/Dmitri_Shostakovich#s\"/>\n   </m:composer>\n  </m:Symphony>\n </m:program>\n</m:Concert>\n " ;
  ex:exampleOf  <http://www.kanzaki.com/ns/music> ;
  ex:image      <http://www.kanzaki.com/works/2007/misc/music-vocab-sample1.png> ;
  ex:pfx        "m:"
] .

m:Trombonist  a           owl:Class ;
        rdfs:comment      "A Trombone player" ;
        rdfs:isDefinedBy  <http://www.kanzaki.com/ns/music> ;
        rdfs:label        "Trombonist" ;
        rdfs:subClassOf   m:Player ;
        rdfs:subClassOf   [ a                   owl:Restriction ;
                            owl:onProperty      m:plays ;
                            owl:someValuesFrom  m:Trombone
                          ] .

<http://en.wikipedia.org/wiki/A_minor>
        a       foaf:Document .

<http://en.wikipedia.org/wiki/C_flat_major>
        a       foaf:Document .

m:Symphony  a             owl:Class ;
        rdfs:comment      "A large and complex work for symphony orchestra" ;
        rdfs:isDefinedBy  <http://www.kanzaki.com/ns/music> ;
        rdfs:label        "Symphony" ;
        rdfs:subClassOf   m:Orchestral_Work .

m:Key   a                 owl:Class ;
        rdfs:comment      "A key of a musical work (e.g. C-dur, b-moll)" ;
        rdfs:isDefinedBy  <http://www.kanzaki.com/ns/music> ;
        rdfs:label        "Key" .

<http://www.kanzaki.com/ns/music>
        a                owl:Ontology ;
        rdfs:comment     "音楽作品、楽器、演奏情報を記述するためのボキャブラリ。Opera_Event（演奏）とOpera（作品）や、String_Quartette（作品）とStringQuartetEnsemble（団体）のように、日常語では両方の意味に使われるクラスの区別に注意。このバージョンでは、音楽作品、その表現（演奏、楽譜など）とイベント（演奏会）をより精密にモデリングするべく実験中。"@ja , "A vocabulary, or music ontology, to describe classical music and performances. Classes (categories) for musical works, events, instruments and performers, as well as related properties are defined. Make sure to distinguish musical works (e.g. Opera) from performance events (Opera_Event), or works (String_Quartette) from performer (StringQuartetEnsemble in this vocab), whose natural language terms are used interchangeblly. The present version experiments more precise model to describe a musical work, its representations (performances, scores, etc) and a musical event to present a representation (a concert). Includes 30 keys as individuals." ;
        rdfs:label       "Music Vocabulary" ;
        ont:created      "2003-07-04" ;
        ont:creator      [ a              foaf:Person ;
                           rdfs:seeAlso   <http://www.kanzaki.com/info/webwho.rdf> ;
                           foaf:homepage  <http://www.kanzaki.com/> ;
                           foaf:name      "神崎正英"@ja
                         ] ;
        ont:modified     "2007-10-31" ;
        owl:imports      <http://www.kanzaki.com/ns/dliser.rdf> ;
        owl:versionInfo  "Version 0.9.6 - OWL DL version. Some stable, some experimental. Changed terms: Opera_Performance to Opera_Event, Ballet_Performance to Ballet_Event." .

m:Orchestra  a            owl:Class ;
        rdfs:comment      "A musical group which perfroms large scale symphonic works" ;
        rdfs:isDefinedBy  <http://www.kanzaki.com/ns/music> ;
        rdfs:label        "Orchestra" ;
        rdfs:subClassOf   m:MusicalGroup .

foaf:Agent  a   owl:Class .

m:Ballet_Performance  a      owl:Class , owl:DeprecatedClass ;
        owl:equivalentClass  m:Ballet_Event .

<http://www.kanzaki.com/works/2007/misc/music-vocab-sample3.png>
        a           foaf:Image ;
        rdfs:label  "'circles and arrows' graphical representation of this example" .

m:Celesta  a              owl:Class ;
        rdfs:comment      "A musical instrument with a keyboard and metal plates struck by hammers that produce bell-like tones." ;
        rdfs:isDefinedBy  <http://www.kanzaki.com/ns/music> ;
        rdfs:label        "Celesta" ;
        rdfs:subClassOf   m:Keyboard_Instrument .

m:event_description  a    owl:ObjectProperty ;
        rdfs:comment      "A description of the subject musical event. Super-property of #program, #presents, #venue." ;
        rdfs:domain       m:Musical_Event ;
        rdfs:isDefinedBy  <http://www.kanzaki.com/ns/music> ;
        rdfs:label        "Event Description" ;
        rdfs:range        owl:Thing .

m:represents  a           owl:ObjectProperty ;
        rdfs:comment      "The subject (performance, score, etc) is a representation of the object musical work. An experiment to have better model." ;
        rdfs:domain       m:Musical_Representation ;
        rdfs:isDefinedBy  <http://www.kanzaki.com/ns/music> ;
        rdfs:label        "Represents" ;
        rdfs:range        m:Musical_Work .

m:venue  a                  owl:ObjectProperty ;
        rdfs:comment        "The subject musical event is presented at the object venue." ;
        rdfs:isDefinedBy    <http://www.kanzaki.com/ns/music> ;
        rdfs:label          "Venue" ;
        rdfs:range          m:Venue ;
        rdfs:subPropertyOf  m:event_description .

[ a             ex:Example ;
  rdfs:comment  "ある演奏会の名称、日時、プログラム、会場を、文字列だけで記述する例。"@ja , "A simplified description of a concert with its title, date, program and venue. All property values are literal string here." ;
  ex:code       "\n<m:Concert>\n <dc:title>Tokyo Green Symphony Orchestra 12th Concert</dc:title>\n <dc:date>2003-11-02T14:00+09:00</dc:date>\n <m:conductorName>Yuri Nitta</m:conductorName>\n <m:performerName>Violin: Tomoko Kawada</m:performerName>\n <m:performerName>Orchestra: Tokyo Green Symphony Orchestra</m:performerName>\n <m:programLine>Bruch: Violin Concerto No.1 g minor</m:programLine>\n <m:programLine>Brahms: Symphony No.2 D major</m:programLine>\n <cal:location>Sumida Triphony</cal:location>\n</m:Concert>\n " ;
  ex:exampleOf  <http://www.kanzaki.com/ns/music> ;
  ex:pfx        "m:"
] .

m:Soprano  a              owl:Class ;
        rdfs:comment      "A Soprano singer" ;
        rdfs:isDefinedBy  <http://www.kanzaki.com/ns/music> ;
        rdfs:label        "Soprano" ;
        rdfs:subClassOf   m:Singer .

dcterms:description  a  owl:ObjectProperty .

m:keyName  a                owl:DatatypeProperty ;
        rdfs:comment        "The subject musical work or its movement has a key. Textual version of #key." ;
        rdfs:domain         m:Musical_Work ;
        rdfs:isDefinedBy    <http://www.kanzaki.com/ns/music> ;
        rdfs:label          "Key Name" ;
        rdfs:range          rdfs:Literal ;
        rdfs:subPropertyOf  dc:description .

m:Musician  a             owl:Class ;
        rdfs:comment      "An artist who performs, composes or conducts music" ;
        rdfs:isDefinedBy  <http://www.kanzaki.com/ns/music> ;
        rdfs:label        "Musician" ;
        rdfs:subClassOf   m:Artist .

m:Recital  a              owl:Class ;
        rdfs:comment      "An event of musical performance especially by soloists" ;
        rdfs:isDefinedBy  <http://www.kanzaki.com/ns/music> ;
        rdfs:label        "Recital" ;
        rdfs:subClassOf   m:Musical_Event .

m:Oboist  a               owl:Class ;
        rdfs:comment      "An Oboe player" ;
        rdfs:isDefinedBy  <http://www.kanzaki.com/ns/music> ;
        rdfs:label        "Oboist" ;
        rdfs:subClassOf   m:Player ;
        rdfs:subClassOf   [ a                   owl:Restriction ;
                            owl:onProperty      m:plays ;
                            owl:someValuesFrom  m:Oboe
                          ] .

m:MusicalGroup  a         owl:Class ;
        rdfs:comment      "A group that performs art works" ;
        rdfs:isDefinedBy  <http://www.kanzaki.com/ns/music> ;
        rdfs:label        "Musical Group" ;
        rdfs:subClassOf   m:Artist .

<http://en.wikipedia.org/wiki/G_major>
        a       foaf:Document .

m:Conductor  a            owl:Class ;
        rdfs:comment      "A Conductor" ;
        rdfs:isDefinedBy  <http://www.kanzaki.com/ns/music> ;
        rdfs:label        "Conductor" ;
        rdfs:subClassOf   m:Musician , m:Director .

m:TubaPlayer  a           owl:Class ;
        rdfs:comment      "A Tuba player" ;
        rdfs:isDefinedBy  <http://www.kanzaki.com/ns/music> ;
        rdfs:label        "TubaPlayer" ;
        rdfs:subClassOf   m:Player ;
        rdfs:subClassOf   [ a                   owl:Restriction ;
                            owl:onProperty      m:plays ;
                            owl:someValuesFrom  m:Tuba
                          ] .

<http://en.wikipedia.org/wiki/F_minor>
        a       foaf:Document .

m:Timpanist  a            owl:Class ;
        rdfs:comment      "A Timpani player" ;
        rdfs:isDefinedBy  <http://www.kanzaki.com/ns/music> ;
        rdfs:label        "Timpanist" ;
        rdfs:subClassOf   m:Player ;
        rdfs:subClassOf   [ a                   owl:Restriction ;
                            owl:onProperty      m:plays ;
                            owl:someValuesFrom  m:Timpani
                          ] .

m:Contrabassist  a        owl:Class ;
        rdfs:comment      "A Contrabass player" ;
        rdfs:isDefinedBy  <http://www.kanzaki.com/ns/music> ;
        rdfs:label        "Contrabassist" ;
        rdfs:subClassOf   m:Player ;
        rdfs:subClassOf   [ a                   owl:Restriction ;
                            owl:onProperty      m:plays ;
                            owl:someValuesFrom  m:Contrabass
                          ] .

m:presents  a               owl:ObjectProperty ;
        rdfs:comment        "The subject musical event presents a performance of a musical work. An experiment to have better model to describe musical work, its representation and an event to present the representation." ;
        rdfs:isDefinedBy    <http://www.kanzaki.com/ns/music> ;
        rdfs:label          "Presents" ;
        rdfs:range          m:Performance ;
        rdfs:subPropertyOf  m:event_description .

m:Violinist  a            owl:Class ;
        rdfs:comment      "A Violn player" ;
        rdfs:isDefinedBy  <http://www.kanzaki.com/ns/music> ;
        rdfs:label        "Violinist" ;
        rdfs:subClassOf   m:Player ;
        rdfs:subClassOf   [ a                   owl:Restriction ;
                            owl:onProperty      m:plays ;
                            owl:someValuesFrom  m:Violin
                          ] .

m:Tenor  a                owl:Class ;
        rdfs:comment      "A Tenor singer" ;
        rdfs:isDefinedBy  <http://www.kanzaki.com/ns/music> ;
        rdfs:label        "Tenor" ;
        rdfs:subClassOf   m:Singer .

<http://en.wikipedia.org/wiki/A_flat_major>
        a       foaf:Document .

m:Guitar  a               owl:Class ;
        rdfs:comment      "A musical instrument having a large flat-backed sound box, a long fretted neck, and usually six strings, played by strumming or plucking." ;
        rdfs:isDefinedBy  <http://www.kanzaki.com/ns/music> ;
        rdfs:label        "Guitar" ;
        rdfs:subClassOf   m:String_Instrument .

<http://en.wikipedia.org/wiki/D_flat_major>
        a       foaf:Document .

<http://en.wikipedia.org/wiki/G_flat_major>
        a       foaf:Document .

m:BassClarinet  a         owl:Class ;
        rdfs:comment      "A larger member of the clarinet family, usually in key B-flat." ;
        rdfs:isDefinedBy  <http://www.kanzaki.com/ns/music> ;
        rdfs:label        "Bass Clarinet" ;
        rdfs:subClassOf   m:Clarinet .

m:Oboe  a                 owl:Class ;
        rdfs:comment      "A woodwind instrument with a conical bore and a double-reed mouthpiece." ;
        rdfs:isDefinedBy  <http://www.kanzaki.com/ns/music> ;
        rdfs:label        "Oboe" ;
        rdfs:subClassOf   m:Woodwind_Instrument .

m:Clarinettist  a         owl:Class ;
        rdfs:comment      "A Clarinet player" ;
        rdfs:isDefinedBy  <http://www.kanzaki.com/ns/music> ;
        rdfs:label        "Clarinettist" ;
        rdfs:subClassOf   m:Player ;
        rdfs:subClassOf   [ a                   owl:Restriction ;
                            owl:onProperty      m:plays ;
                            owl:someValuesFrom  m:Clarinet
                          ] .

<http://en.wikipedia.org/wiki/C_major>
        a       foaf:Document .

m:Ges-dur  a                 m:Key ;
        rdfs:comment         "Major key based on G flat, whose key signature has 6 flats." ;
        rdfs:isDefinedBy     <http://www.kanzaki.com/ns/music> ;
        rdfs:label           "Ges dur" ;
        dcterms:alternative  "G-Flat major" ;
        dcterms:description  <http://en.wikipedia.org/wiki/G_flat_major> .

<http://en.wikipedia.org/wiki/F_sharp_minor>
        a       foaf:Document .

m:composer  a               owl:ObjectProperty ;
        rdfs:comment        "The subject musical work is composed by a person, a group, a software program etc." ;
        rdfs:domain         m:Oeuvre ;
        rdfs:isDefinedBy    <http://www.kanzaki.com/ns/music> ;
        rdfs:label          "Composer" ;
        rdfs:range          foaf:Agent ;
        rdfs:subPropertyOf  dc:creator , m:description .

m:Trombone  a             owl:Class ;
        rdfs:comment      "A brass instrument consisting of a long cylindrical tube, and having a movable U-shaped slide for producing different pitches." ;
        rdfs:isDefinedBy  <http://www.kanzaki.com/ns/music> ;
        rdfs:label        "Trombone" ;
        rdfs:subClassOf   m:Brass_Instrument .

<http://en.wikipedia.org/wiki/B_minor>
        a       foaf:Document .

m:Score  a                owl:Class ;
        rdfs:comment      "A full score or piano-vocal score of a work, either published or manuscript." ;
        rdfs:isDefinedBy  <http://www.kanzaki.com/ns/music> ;
        rdfs:label        "Score" ;
        rdfs:subClassOf   m:Written_Representation .

m:String_Instrument  a    owl:Class ;
        rdfs:comment      "A stringed musical instrument, in which sound is produced by plucking, striking, or bowing taut strings." ;
        rdfs:isDefinedBy  <http://www.kanzaki.com/ns/music> ;
        rdfs:label        "String Instrument" ;
        rdfs:subClassOf   m:Musical_Instrument .

m:Choral_Music  a         owl:Class ;
        rdfs:comment      "A genre of music composed for performance by a chorus or choir" ;
        rdfs:isDefinedBy  <http://www.kanzaki.com/ns/music> ;
        rdfs:label        "Choral Music" ;
        rdfs:subClassOf   m:Oeuvre .

m:Religious_Music  a      owl:Class ;
        rdfs:comment      "A genre of music composed for performance as part of religious ceremonies" ;
        rdfs:isDefinedBy  <http://www.kanzaki.com/ns/music> ;
        rdfs:label        "Religious Music" ;
        rdfs:subClassOf   m:Oeuvre .

m:Ces-dur  a                 m:Key ;
        rdfs:comment         "Major key based on C flat, whose key signature has 7 flats." ;
        rdfs:isDefinedBy     <http://www.kanzaki.com/ns/music> ;
        rdfs:label           "Ces dur" ;
        dcterms:alternative  "C-Flat major" ;
        dcterms:description  <http://en.wikipedia.org/wiki/C_flat_major> .

m:OperaCompany  a         owl:Class ;
        rdfs:comment      "A musical group that performs opera works." ;
        rdfs:isDefinedBy  <http://www.kanzaki.com/ns/music> ;
        rdfs:label        "Opera Company" ;
        rdfs:subClassOf   m:MusicalGroup .

<http://en.wikipedia.org/wiki/C_sharp_major>
        a       foaf:Document .

[ a             ex:Example ;
  rdfs:comment  "ある演奏会の名称、日時、プログラム、会場の記述例。より精密なモデルの案として、'performer'の定義セクションにある例も参照。"@ja , "Another description of a concert with its title, date, program and venue. See also examples in the definition of 'performer' for more erabolate model (the preferred domain of this property is m:Performance, not m:Concert)." ;
  ex:code       "\n<m:Concert>\n <dc:title>Tokyo Green Symphony Orchestra 12th Concert</dc:title>\n <dc:date>2003-11-02T14:00+09:00</dc:date>\n <m:conductor foaf:name=\"Yuri Nitta\"/>\n <m:performer>\n  <m:Violinist>\n   <foaf:name>Tomoko Kawada</foaf:name>\n   <m:performs rdf:nodeID=\"p1\"/>\n  </m:Violinist>\n </m:performer>\n <m:performer>\n  <m:Orchestra foaf:name=\"Tokyo Green Symphony Orchestra\"/>\n </m:performer>\n <m:program>\n  <m:Concerto rdf:nodeID=\"p1\">\n   <m:composer foaf:name=\"Bruch\"/>\n   <dc:title>Violin Concerto No.1 g minor</dc:title>\n   <m:opus>op.26</m:opus>\n  </m:Concerto>\n </m:program>\n <m:program>\n  <m:Symphony>\n   <m:composer foaf:name=\"Brahms\"/>\n   <dc:title>Symphony No.2 D major</dc:title>\n   <m:opus>op.73</m:opus>\n  </m:Symphony>\n </m:program>\n <m:venue>\n  <m:Venue geo:lat=\"35.69\" geo:long=\"139.81\">\n   <dc:title>Sumida Triphony</dc:title>\n  </m:Venue>\n </m:venue>\n</m:Concert>\n " ;
  ex:exampleOf  <http://www.kanzaki.com/ns/music> ;
  ex:image      <http://www.kanzaki.com/works/2007/misc/music-vocab-sample2.png> ;
  ex:pfx        "m:"
] .

m:ContrafagottoPlayer
        a                 owl:Class ;
        rdfs:comment      "A Contrafagotto player" ;
        rdfs:isDefinedBy  <http://www.kanzaki.com/ns/music> ;
        rdfs:label        "ContrafagottoPlayer" ;
        rdfs:subClassOf   m:Bassoonist ;
        rdfs:subClassOf   [ a                   owl:Restriction ;
                            owl:onProperty      m:plays ;
                            owl:someValuesFrom  m:Contrafagotto
                          ] .

m:Cis-dur  a                 m:Key ;
        rdfs:comment         "Major key based on C sharp, whose key signature has 7 sharps." ;
        rdfs:isDefinedBy     <http://www.kanzaki.com/ns/music> ;
        rdfs:label           "Cis dur" ;
        dcterms:alternative  "C-Sharp major" ;
        dcterms:description  <http://en.wikipedia.org/wiki/C_sharp_major> .

m:String_Quartette  a        owl:Class , owl:DeprecatedClass ;
        owl:equivalentClass  m:String_Quartet .

m:Keyboard_Instrument
        a                 owl:Class ;
        rdfs:comment      "A musical instrument that has a set of keys that consist of scale." ;
        rdfs:isDefinedBy  <http://www.kanzaki.com/ns/music> ;
        rdfs:label        "Keyboard Instrument" ;
        rdfs:subClassOf   m:Musical_Instrument .

m:BalletCompany  a        owl:Class ;
        rdfs:comment      "A musical group that performs ballet works." ;
        rdfs:isDefinedBy  <http://www.kanzaki.com/ns/music> ;
        rdfs:label        "Ballet Company" ;
        rdfs:subClassOf   m:MusicalGroup .

m:Opera  a                owl:Class ;
        rdfs:comment      "A musical work with drama, song, chorus and orchestral music. Note 'Opera_Event' in this vocabulary describes the performance of an opera." ;
        rdfs:isDefinedBy  <http://www.kanzaki.com/ns/music> ;
        rdfs:label        "Opera (Work)" ;
        rdfs:subClassOf   m:Oeuvre .

m:meter  a                  owl:DatatypeProperty ;
        rdfs:comment        "The subject musical work or its movement has a time measure such as 3/4, 4/4, 6/8 etc" ;
        rdfs:domain         m:Musical_Work ;
        rdfs:isDefinedBy    <http://www.kanzaki.com/ns/music> ;
        rdfs:label          "Meter" ;
        rdfs:range          rdfs:Literal ;
        rdfs:subPropertyOf  dc:description .

m:Horn  a                 owl:Class ;
        rdfs:comment      "A brass instrument with a long narrow tube that is coiled in a circle before ending in a flaring bell, usually being equipped with valves. A French Horn." ;
        rdfs:isDefinedBy  <http://www.kanzaki.com/ns/music> ;
        rdfs:label        "Horn" ;
        rdfs:subClassOf   m:Brass_Instrument .

m:dis-moll  a                m:Key ;
        rdfs:comment         "Minor key based on D sharp, whose key signature has 6 sharps." ;
        rdfs:isDefinedBy     <http://www.kanzaki.com/ns/music> ;
        rdfs:label           "dis moll" ;
        dcterms:alternative  "D-Sharp minor" ;
        dcterms:description  <http://en.wikipedia.org/wiki/D_sharp_minor> .

m:Cellist  a              owl:Class ;
        rdfs:comment      "A Cello player" ;
        rdfs:isDefinedBy  <http://www.kanzaki.com/ns/music> ;
        rdfs:label        "Cellist" ;
        rdfs:subClassOf   m:Player ;
        rdfs:subClassOf   [ a                   owl:Restriction ;
                            owl:onProperty      m:plays ;
                            owl:someValuesFrom  m:Cello
                          ] .

m:EnglishHornPlayer  a    owl:Class ;
        rdfs:comment      "An English Horn player" ;
        rdfs:isDefinedBy  <http://www.kanzaki.com/ns/music> ;
        rdfs:label        "English Horn player" ;
        rdfs:subClassOf   m:Oboist ;
        rdfs:subClassOf   [ a                   owl:Restriction ;
                            owl:onProperty      m:plays ;
                            owl:someValuesFrom  m:EnglishHorn
                          ] .

m:a-moll  a                  m:Key ;
        rdfs:comment         "" ;
        rdfs:isDefinedBy     <http://www.kanzaki.com/ns/music> ;
        rdfs:label           "a moll" ;
        dcterms:alternative  "A minor" ;
        dcterms:description  <http://en.wikipedia.org/wiki/A_minor> .

<http://en.wikipedia.org/wiki/B_flat_major>
        a       foaf:Document .

m:Saxophone  a            owl:Class ;
        rdfs:comment      "A woodwind instrument with a single-reed mouthpiece and a (usually curved) conical metal tube, including soprano, alto, tenor, and baritone sizes." ;
        rdfs:isDefinedBy  <http://www.kanzaki.com/ns/music> ;
        rdfs:label        "Saxophone" ;
        rdfs:subClassOf   m:Woodwind_Instrument .

<http://en.wikipedia.org/wiki/E_flat_major>
        a       foaf:Document .

m:Cello  a                owl:Class ;
        rdfs:comment      "A stringed instrument of the violin family, with bass to tenor tone. Usually played in sitting position." ;
        rdfs:isDefinedBy  <http://www.kanzaki.com/ns/music> ;
        rdfs:label        "Cello" ;
        rdfs:subClassOf   m:String_Instrument .

m:Sketch  a               owl:Class ;
        rdfs:comment      "A sketch, or a brief prelimary composition of a work." ;
        rdfs:isDefinedBy  <http://www.kanzaki.com/ns/music> ;
        rdfs:label        "Sketch" ;
        rdfs:subClassOf   m:Written_Representation .
