@prefix :      <http://purl.org/onto-ocds/ocds#> .
@prefix rdfs:  <http://www.w3.org/2000/01/rdf-schema#> .
@prefix foaf:  <http://xmlns.com/foaf/0.1/> .
@prefix pc:    <http://purl.org/procurement/public-contracts#> .
@prefix owl:   <http://www.w3.org/2002/07/owl#> .
@prefix seq:   <http://www.ontologydesignpatterns.org/cp/owl/sequence.owl#> .
@prefix xsd:   <http://www.w3.org/2001/XMLSchema#> .
@prefix rdf:   <http://www.w3.org/1999/02/22-rdf-syntax-ns#> .
@prefix xml:   <http://www.w3.org/XML/1998/namespace> .
@prefix sch:   <http://schema.org#> .
@prefix gr:    <http://purl.org/goodrelations/v1#> .
@prefix dcterms: <http://purl.org/dc/terms/> .

:contractValue  a     owl:FunctionalProperty , owl:ObjectProperty ;
        rdfs:comment  "The total value of this contract."@en ;
        rdfs:domain   :Contract ;
        rdfs:label    "Contract value"@en ;
        rdfs:range    :Value .

:dncpContractCode  a  owl:FunctionalProperty , owl:DatatypeProperty ;
        rdfs:comment  "Código de contrato de la DNCP"@es ;
        rdfs:domain   :Contract ;
        rdfs:label    "Código de contrato"@es ;
        rdfs:range    xsd:string .

:Item   a                owl:Class ;
        rdfs:comment     "A good, service, or work to be contracted."@en ;
        rdfs:label       "Item"@en ;
        rdfs:subClassOf  gr:Offering .

:streetAddress  a     owl:FunctionalProperty , owl:DatatypeProperty ;
        rdfs:comment  "The street address. For example, 1600 Amphitheatre Pkwy"@en ;
        rdfs:domain   :Address ;
        rdfs:label    "Street address"@en ;
        rdfs:range    xsd:string .

:classificationId  a  owl:FunctionalProperty , owl:DatatypeProperty ;
        rdfs:comment  "The classification code drawn from the selected scheme."@en ;
        rdfs:domain   :Classification ;
        rdfs:label    "Classification ID"@en ;
        rdfs:range    xsd:string , xsd:integer .

:awardStatusActive  a  :AwardStatus , owl:NamedIndividual ;
        rdfs:comment   "This award has been made, and is currently in force."@en ;
        rdfs:label     "active"@en ;
        dcterms:title  "Active"@en .

:milestoneStatus  a   owl:FunctionalProperty , owl:DatatypeProperty ;
        rdfs:comment  "The status that was realized on the date provided in dateModified, drawn from the [milestoneStatus codelist](http://standard.open-contracting.org/latest/en/schema/codelists/#milestone-status)."@en ;
        rdfs:domain   :Milestone ;
        rdfs:label    "Milestone status"@en ;
        rdfs:range    xsd:string .

:budgetDescription  a  owl:DatatypeProperty ;
        rdfs:domain  :Budget ;
        rdfs:range   xsd:string .

:transactionSource  a  owl:FunctionalProperty , owl:ObjectProperty ;
        rdfs:comment  "Used to point either to a corresponding Budget Data Package, IATI file, or machine or human-readable source where users can find further information on the budget line item identifiers, or project identifiers, provided here."@en ;
        rdfs:domain   :Transaction ;
        rdfs:label    "Transaction Data Source"@en ;
        rdfs:range    rdfs:Resource .

:former_value  a      owl:FunctionalProperty , owl:ObjectProperty ;
        rdfs:comment  "The previous value of the changed property, in whatever type the property is."@en ;
        rdfs:domain   :Change ;
        rdfs:label    "Former value"@en ;
        rdfs:range    rdfs:Resource .

:project  a           owl:FunctionalProperty , owl:DatatypeProperty ;
        rdfs:comment  "The name of the project that through which this contracting process is funded (if applicable). Some organizations maintain a registry of projects, and the data should use the name by which the project is known in that registry. No translation option is offered for this string, as translated values can be provided in third-party data, linked from the data source above."@en ;
        rdfs:domain   :Budget ;
        rdfs:label    "Project Title"@en ;
        rdfs:range    xsd:string .

:email  a             owl:FunctionalProperty , owl:DatatypeProperty ;
        rdfs:comment  "The e-mail address of the contact point/person."@en ;
        rdfs:domain   :ContactPoint ;
        rdfs:label    "Email"@en ;
        rdfs:range    xsd:string .

:Classification  a  owl:Class ;
        rdfs:label  "Classification"@en .

:lotItems  a         owl:ObjectProperty ;
        rdfs:domain  :Lot ;
        rdfs:range   :Item .

:releaseTagTenderUpdate
        a              :ReleaseTag , owl:NamedIndividual ;
        rdfs:comment   "An updated to an existing tender release. There should be at least one tender release with the same ocid, but an earlier releaseDate, before a tenderUpdate is published. An update may add new information or make corrections to prior published information. It should not be used for formal legal amendments to a tender, for which the tenderAmendment tag should be used."@en ;
        rdfs:label     "tenderUpdate"@en ;
        dcterms:title  "Tender Update"@en .

:Document  a             owl:Class ;
        rdfs:comment     "Links to, or descriptions of, external documents can be attached at various locations within the standard. Documents may be supporting information, formal notices, downloadable forms, or any other kind of resource that should be made public as part of full open contracting."@en ;
        rdfs:label       "Document"@en ;
        rdfs:subClassOf  foaf:Document .

:Value  a                    owl:Class ;
        rdfs:label           "Value"@en ;
        owl:equivalentClass  gr:PriceSpecification .

:eligibilityCriteria  a  owl:FunctionalProperty , owl:DatatypeProperty ;
        rdfs:comment  "A description of any eligibility criteria for potential suppliers."@en ;
        rdfs:domain   :Tender ;
        rdfs:label    "Eligibility criteria"@en ;
        rdfs:range    xsd:string .

:ics_GSIN  a           :ItemClassificationScheme , owl:NamedIndividual ;
        rdfs:comment   "The Canadia federal government uses Goods and Services Identification Number (GSIN) codes to identify generic product descriptions for its procurement activities. The full list is published and maintained at buyandsell.gc.ca"@en ;
        rdfs:label     "GSIN"@en ;
        dcterms:title  "Goods and Services Identification Number"@en .

:submissionMethodWritten
        a              :SubmissionMethod , owl:NamedIndividual ;
        rdfs:label     "written"@en ;
        dcterms:title  "Written"@en .

:releaseTagTenderAmendment
        a              :ReleaseTag , owl:NamedIndividual ;
        rdfs:comment   "An amendment to an existing tender release. There should be at least one tender release with the same ocid, but an earlier releaseDate, before a tenderAmendment is published. The term amendment has legal meaning in many jurisdictions."@en ;
        rdfs:label     "tenderAmendment"@en ;
        dcterms:title  "Tender Amendment"@en .

:awardTitle  a       owl:FunctionalProperty , owl:DatatypeProperty ;
        rdfs:domain  :Award ;
        rdfs:label   "Award title"@en ;
        rdfs:range   xsd:string .

:contractStatus  a    owl:FunctionalProperty , owl:ObjectProperty ;
        rdfs:comment  "The current status of the contract. Drawn from the [contractStatus codelist](http://standard.open-contracting.org/latest/en/schema/codelists/#contract-status)"@en ;
        rdfs:domain   :Contract ;
        rdfs:label    "Contract status"@en ;
        rdfs:range    :ContractStatus .

:ois_AF-MOE  a         :OrganizationIdentifierScheme , owl:NamedIndividual ;
        rdfs:comment   ""@en ;
        rdfs:label     "AF-MOE"@en ;
        dcterms:title  "Ministry of Economy"@en .

:awardStatus  a       owl:FunctionalProperty , owl:ObjectProperty ;
        rdfs:comment  "The current status of the award drawn from the [awardStatus codelist](http://standard.open-contracting.org/latest/en/schema/codelists/#award-status)" ;
        rdfs:domain   :Award ;
        rdfs:label    "Award status" ;
        rdfs:range    :AwardStatus .

:identifierScheme  a  owl:FunctionalProperty , owl:ObjectProperty ;
        rdfs:comment  "Organization identifiers be drawn from an existing identification scheme. This field is used to indicate the scheme or codelist in which the identifier will be found. This value should be drawn from the [Organization Identifier Scheme](http://standard.open-contracting.org/latest/en/schema/codelists/#organization-identifier-scheme)."@en ;
        rdfs:domain   :Identifier ;
        rdfs:label    "Identifier scheme"@en ;
        rdfs:range    :OrganizationIdentifierScheme .

:documents  a         owl:ObjectProperty ;
        rdfs:comment  "A list of documents related to the planning process."@en ;
        rdfs:domain   :Planning ;
        rdfs:label    "Documents"@en ;
        rdfs:range    :Document .

:documentDateModified
        a             owl:FunctionalProperty , owl:DatatypeProperty ;
        rdfs:comment  "Date that the document was last modified"@en ;
        rdfs:domain   :Document ;
        rdfs:label    "Document modification date"@en ;
        rdfs:range    xsd:dateTime .

:unitValue  a        owl:ObjectProperty ;
        rdfs:domain  :Unit ;
        rdfs:label   "Unit value"@en ;
        rdfs:range   :Value .

:amendmentRationale  a  owl:FunctionalProperty , owl:DatatypeProperty ;
        rdfs:comment  "An explanation for the amendment."@en ;
        rdfs:domain   :Amendment ;
        rdfs:label    "Amendment rationale"@en ;
        rdfs:range    xsd:string .

:implementation  a    owl:FunctionalProperty , owl:ObjectProperty ;
        rdfs:comment  "Information related to the implementation of the contract in accordance with the obligations laid out therein."@en ;
        rdfs:domain   :Contract ;
        rdfs:label    "Implementation"@en ;
        rdfs:range    :Implementation .

:documentTitle  a     owl:FunctionalProperty , owl:DatatypeProperty ;
        rdfs:comment  "The document title."@en ;
        rdfs:domain   :Document ;
        rdfs:label    "Document title"@en ;
        rdfs:range    xsd:string .

:documentLanguage  a  owl:FunctionalProperty , owl:DatatypeProperty ;
        rdfs:comment  "Specifies the language of the linked document using either two-digit [ISO 639-1](https://en.wikipedia.org/wiki/List_of_ISO_639-1_codes), or extended [BCP47 language tags](http://www.w3.org/International/articles/language-tags/). The use of two-letter codes from [ISO 639-1](https://en.wikipedia.org/wiki/List_of_ISO_639-1_codes) is strongly recommended unless there is a clear user need for distinguishing the language subtype."@en ;
        rdfs:domain   :Document ;
        rdfs:label    "Document language"@en ;
        rdfs:range    xsd:string .

:tenderStatusComplete
        a              :TenderStatus , owl:NamedIndividual ;
        rdfs:comment   "The tender process as unsucessful."@en ;
        rdfs:label     "complete"@en ;
        dcterms:title  "Complete"@en .

:AwardStatus  a              owl:Class ;
        rdfs:comment         "An award move through multiple states. Releases over time may update the status of an award."@en ;
        rdfs:label           "Codelist Award Status"@en ;
        owl:equivalentClass  [ a          owl:Class ;
                               owl:oneOf  ( :awardStatusActive :awardStatusCancelled :awardStatusPending :awardStatusUnsuccessful )
                             ] .

:contractAmendment  a  owl:ObjectProperty ;
        rdfs:domain  :Contract ;
        rdfs:label   "Contract amendment"@en ;
        rdfs:range   :Amendment .

:tenderStatusActive  a  :TenderStatus , owl:NamedIndividual ;
        rdfs:comment   "A tender process is currently taking place."@en ;
        rdfs:label     "active"@en ;
        dcterms:title  "Active"@en .

:Planning  a          owl:Class ;
        rdfs:comment  "nformation from the planning phase of the contracting process. Note that many other fields may be filled in a planning release, in the appropriate fields in other schema sections, these would likely be estimates at this stage e.g. totalValue in tender"@en ;
        rdfs:label    "Planning"@en .

:awardID  a           owl:FunctionalProperty , owl:ObjectProperty ;
        rdfs:comment  "The award against which this contract is being issued."@en ;
        rdfs:domain   :Contract ;
        rdfs:label    "Award ID"@en ;
        rdfs:range    :Award .

:Identifier  a      owl:Class ;
        rdfs:label  "Identifier"@en .

:startDate  a         owl:FunctionalProperty , owl:DatatypeProperty ;
        rdfs:comment  "The start date for the period."@en ;
        rdfs:domain   :Period ;
        rdfs:label    "Start date"@en ;
        rdfs:range    xsd:dateTime .

:contractStatusActive
        a              :ContractStatus , owl:NamedIndividual ;
        rdfs:comment   "This contract has been signed by all the parties, and is now legally in force."@en ;
        rdfs:label     "active"@en ;
        dcterms:title  "Active"@en .

:releaseTagContractTermination
        a              :ReleaseTag , owl:NamedIndividual ;
        rdfs:label     "contractTermination"@en ;
        dcterms:title  "Contract Termination"@en .

:itemDescription  a   owl:FunctionalProperty , owl:DatatypeProperty ;
        rdfs:comment  "A description of the goods, services to be provided."@en ;
        rdfs:domain   :Item ;
        rdfs:label    "Item description"@en ;
        rdfs:range    xsd:string .

:ocid   a             owl:FunctionalProperty , owl:DatatypeProperty ;
        rdfs:comment  "A globally unique identifier for this Open Contracting Process. Composed of a publisher prefix and an identifier for the contracting process. For more information see the [Open Contracting Identifier guidance](http://standard.open-contracting.org/latest/en/schema/identifiers/)"@en ;
        rdfs:domain   :Release ;
        rdfs:label    "Open Contracting ID"@en ;
        rdfs:range    xsd:string .

:Transaction  a       owl:Class ;
        rdfs:comment  "A spending transaction related to the contracting process. Draws upon the data models of the [Budget Data Package](https://github.com/openspending/budget-data-package/blob/master/specification.md) and the [International Aid Transpareny Initiative](http://iatistandard.org/activity-standard/iati-activities/iati-activity/transaction/) and should be used to cross-reference to more detailed information held using a Budget Data Package, IATI file, or to provide enough information to allow a user to manually or automatically cross-reference with some other published source of transactional spending data."@en ;
        rdfs:label    "Transaction Information"@en .

:awardCriteria  a     owl:FunctionalProperty , owl:DatatypeProperty ;
        rdfs:comment  "Specify the award criteria for the procurement, using the [award criteria codelist](http://standard.open-contracting.org/latest/en/schema/codelists/#award-criteria)"@en ;
        rdfs:domain   :Tender ;
        rdfs:label    "Award criteria"@en ;
        rdfs:range    xsd:string .

:tenderId  a          owl:FunctionalProperty , owl:DatatypeProperty ;
        rdfs:comment  "An identifier for this tender process. This may be the same as the ocid, or may be drawn from an internally held identifier for this tender."@en ;
        rdfs:domain   :Tender ;
        rdfs:label    "Tender ID"@en ;
        rdfs:range    xsd:string , xsd:integer .

:Budget  a            owl:Class ;
        rdfs:comment  "This section contain information about the budget line, and associated projects, through which this contracting process is funded. It draws upon data model of the [Budget Data Package](https://github.com/openspending/budget-data-package/blob/master/specification.md), and should be used to cross-reference to more detailed information held using a Budget Data Package, or, where no linked Budget Data Package is available, to provide enough information to allow a user to manually or automatically cross-reference with another published source of budget and project information."@en ;
        rdfs:label    "Budget"@en .

:       a                owl:Ontology ;
        dcterms:author   <https://twitter.com/CMaudry> ;
        dcterms:license  <https://creativecommons.org/licenses/by/2.0/> ;
        dcterms:title    "Schema for an Open Contracting Release"@en ;
        owl:imports      <http://www.ontologydesignpatterns.org/cp/owl/sequence.owl> ;
        foaf:homepage    <https://github.com/ColinMaudry/open-contracting-ld> .

:documentTypeAwardNotice
        a              :DocumentType , owl:NamedIndividual ;
        rdfs:comment   "The formal notice that gives details of the contract award. This may be a link to a downloadable document, to a web page, or to an official gazette in which the notice is contained."@en ;
        rdfs:label     "awardNotice"@en ;
        dcterms:title  "Award Notice"@en .

:milestoneId  a       owl:FunctionalProperty , owl:DatatypeProperty ;
        rdfs:comment  "A local identifier for this milestone, unique within this block. This field is used to keep track of multiple revisions of a milestone through the compilation from release to record mechanism."@en ;
        rdfs:domain   :Milestone ;
        rdfs:label    "Milestone ID"@en ;
        rdfs:range    xsd:string , xsd:integer .

:datePublished  a     owl:FunctionalProperty , owl:DatatypeProperty ;
        rdfs:comment  "The date on which the document was first published. This is particularly important for legally important documents such as notices of a tender."@en ;
        rdfs:domain   :Document ;
        rdfs:label    "Publication date"@en ;
        rdfs:range    xsd:dateTime .

:SubmissionMethod  a  owl:Class ;
        rdfs:comment  "The submission method codelist is used to identify the mechanism through which a submission may be made."@en ;
        rdfs:label    "Codelist Submission Method"@en .

:awardDocuments  a    owl:ObjectProperty ;
        rdfs:comment  "All documents and attachments related to the award, including any notices."@en ;
        rdfs:domain   :Award ;
        rdfs:label    "Award documents"@en ;
        rdfs:range    :Document .

:awardURL  a         owl:DatatypeProperty ;
        rdfs:domain  :Award ;
        rdfs:range   xsd:anyURI .

:Change  a          owl:Class ;
        rdfs:label  "Change"@en .

:awardCriteriaSingleBidOnly
        a              :AwardCriteria , owl:NamedIndividual ;
        rdfs:label     "singleBidOnly"@en ;
        dcterms:title  "Single Bid Only"@en .

:documentId  a        owl:FunctionalProperty , owl:DatatypeProperty ;
        rdfs:comment  "A local, unique identifier for this document. This field is used to keep track of multiple revisions of a document through the compilation from release to record mechanism."@en ;
        rdfs:domain   :Document ;
        rdfs:label    "Document ID"@en ;
        rdfs:range    xsd:string , xsd:integer .

:ics_UNSPSC  a         :ItemClassificationScheme , owl:NamedIndividual ;
        rdfs:comment   "The United Nations Standard Products and Services Code (UNSPSC) is a hierarchical convention that is used to classify all products and services. Machine readable meta-data for UNSPSC is not provided as open data: and so publishers should consider alternative classification shemes that do provide open data lookup tables wherever possible."@en ;
        rdfs:label     "UNSPSC"@en ;
        dcterms:title  "United Nations Standard Products and Services Code®"@en .

:releaseTagImplementation
        a              :ReleaseTag , owl:NamedIndividual ;
        rdfs:label     "implementation"@en ;
        dcterms:title  "Implementation"@en .

:tenderUrl  a         owl:FunctionalProperty , owl:DatatypeProperty ;
        rdfs:comment  "Url para poder identificar el servicio que es utilizado para generar la convocatoria"@es ;
        rdfs:domain   :Tender ;
        rdfs:label    "Tender URL"@es ;
        rdfs:range    xsd:anyURI .

:ics_CPV  a            :ItemClassificationScheme , owl:NamedIndividual ;
        rdfs:comment   "The Common Procurement Vocabulary is a standard adopted by the Commission of the European Community, and consisting of a main vocabulary for defining the subject of a contract, and a supplementary vocabulary for adding further qualitative information. The main vocabulary, identified in OCDS by the code CPV, is based on a tree structure comprising codes of up to 9 digits (an 8 digit code plus a check digit) associated with a wording that describes the type of supplies, works or services forming the subject of the contract."@en ;
        rdfs:label     "CPV"@en ;
        dcterms:title  "EC Common Procurement Vocabulary"@en .

:tenderers  a         owl:ObjectProperty ;
        rdfs:comment  "All entities who submit a tender."@en ;
        rdfs:domain   :Tender ;
        rdfs:label    "Tenderers"@en ;
        rdfs:range    :Organization .

:methodSelective  a    :Method , owl:NamedIndividual ;
        rdfs:comment   "Selective tendering means a procurement method whereby only qualified suppliers are invited by the procuring entity to submit a tender."@en ;
        rdfs:label     "selective"@en ;
        dcterms:title  "Selective"@en .

:ItemClassificationScheme
        a       owl:Class .

rdfs:Resource  a  owl:Class .

:ics_CDNCP  a          :ItemClassificationScheme , owl:NamedIndividual ;
        rdfs:comment   "Catálogo de productos, bienes y servicios de la Dirección Nacional de Contrataciones Públicas del Paraguay Nivel 5, basado en UNSPSC."@es ;
        rdfs:label     "CDNCP"@en ;
        dcterms:title  "Catálogo de productos, bienes y servicios de la Dirección Nacional de Contrataciones Públicas del Paraguay"@es .

:identifierUri  a     owl:FunctionalProperty , owl:ObjectProperty ;
        rdfs:comment  "A URI to identify the organization, such as those provided by [Open Corporates](http://www.opencorporates.com) or some other relevant URI provider. This is not for listing the website of the organization: that can be done through the url field of the Organization contact point."@en ;
        rdfs:domain   :Identifier ;
        rdfs:label    "Identifier URI"@en ;
        rdfs:range    dcterms:URI .

:releaseTagAwardCancellation
        a              :ReleaseTag , owl:NamedIndividual ;
        rdfs:label     "awardCancellation"@en ;
        dcterms:title  "Award Cancellation"@en .

:unitName  a          owl:FunctionalProperty , owl:DatatypeProperty ;
        rdfs:comment  "Name of the unit"@en ;
        rdfs:domain   :Unit ;
        rdfs:label    "Unit name"@en ;
        rdfs:range    xsd:string .

:contractTitle  a    owl:FunctionalProperty , owl:DatatypeProperty ;
        rdfs:domain  :Contract ;
        rdfs:label   "Contract title" ;
        rdfs:range   xsd:string .

:OrganizationIdentifierScheme
        a             owl:Class ;
        rdfs:comment  "The Organization Identifier Scheme currently uses the codes from the International Aid Transparency Initiative ‘Organisation Registration Agency’ codelist. See the identifiers section for more information on organization identifiers."@en ;
        rdfs:label    "Codelist Organization Identifier Scheme"@en .

:budgetUri  a         owl:FunctionalProperty , owl:ObjectProperty ;
        rdfs:comment  "A URI pointing directly to a machine-readable record about the related budget or projects for this contracting process."@en ;
        rdfs:domain   :Budget ;
        rdfs:label    "Linked budget information"@en ;
        rdfs:range    dcterms:URI .

:submissionMethodDetails
        a             owl:FunctionalProperty , owl:DatatypeProperty ;
        rdfs:comment  "Any detailed or further information on the submission method. This may include the address, e-mail address or online service to which bids should be submitted, and any special requirements to be followed for submissions."@en ;
        rdfs:domain   :Tender ;
        rdfs:label    "Submission method details"@en ;
        rdfs:range    xsd:string .

:transactionAmount  a  owl:ObjectProperty ;
        rdfs:comment  "The value of the transaction."@en ;
        rdfs:domain   :Transaction ;
        rdfs:label    "Transaction amount"@en ;
        rdfs:range    :Value .

:ContactPoint  a         owl:Class ;
        rdfs:comment     "An person, contact point or department to contact in relation to this contracting process."@en ;
        rdfs:label       "Contact point"@en ;
        rdfs:subClassOf  sch:ContactPoint .

:transactions  a      owl:ObjectProperty ;
        rdfs:comment  "A list of the spending transactions made against this contract"@en ;
        rdfs:domain   :Implementation ;
        rdfs:label    "Transactions"@en ;
        rdfs:range    :Transaction .

:Address  a              owl:Class ;
        rdfs:comment     "An address. This may be the legally registered address of the organization, or may be a correspondence address for this particular contracting process."@en ;
        rdfs:label       "Address"@en ;
        rdfs:subClassOf  sch:PostalAddress .

:identifier  a        owl:ObjectProperty ;
        rdfs:comment  "The primary identifier for this organization. Identifiers that uniquely pick out a legal entity should be preferred. Consult the [organization identifier guidance](http://standard.open-contracting.org/latest/en/schema/identifiers/) for the preferred scheme and identifier to use."@en ;
        rdfs:domain   :Organization ;
        rdfs:label    "Organization identifier"@en ;
        rdfs:range    :Identifier .

:identifierId  a      owl:FunctionalProperty , owl:DatatypeProperty ;
        rdfs:comment  "The identifier of the organization in the selected scheme."@en ;
        rdfs:domain   :Identifier ;
        rdfs:label    "Identifier ID"@en ;
        rdfs:range    xsd:string , xsd:integer .

:Period  a          owl:Class ;
        rdfs:label  "Period"@en .

:ReleaseTag  a               owl:Class ;
        rdfs:comment         "A contracting process may result in a number of releases of information over time. These should be tagged to indicate the stage of the contracting process they relate to."@en ;
        rdfs:label           "Codelist ReleaseTag"@en ;
        owl:equivalentClass  [ a          owl:Class ;
                               owl:oneOf  ( :releaseTagAward :releaseTagAwardCancellation :releaseTagAwardUpdate :releaseTagCompiled :releaseTagContract :releaseTagContractAmendment :releaseTagContractTermination :releaseTagContractUpdate :releaseTagImplementation :releaseTagImplementationUpdate :releaseTagPlanning :releaseTagTender :releaseTagTenderAmendment :releaseTagTenderCancellation :releaseTagTenderUpdate )
                             ] .

:tenderStatusUnsuccessful
        a              :TenderStatus , owl:NamedIndividual ;
        rdfs:comment   "The tender process as unsucessful."@en ;
        rdfs:label     "unsuccessful"@en ;
        dcterms:title  "Unsuccessful"@en .

:submissionMethodElectronicSubmission
        a              :SubmissionMethod , owl:NamedIndividual ;
        rdfs:label     "electronicSubmission"@en ;
        dcterms:title  "Electronic Submission"@en .

:ois_AF-CBR  a         :OrganizationIdentifierScheme , owl:NamedIndividual ;
        rdfs:comment   "Website not yet searchable."@en ;
        rdfs:label     "AF-CBR"@en ;
        dcterms:title  "Afghanistan Central Business Registry"@en .

:initiationTypeTender
        a              :InitiationType , owl:NamedIndividual ;
        rdfs:comment   "An open competitive bidding or tendering to form contracts. The process generally involves publicly inviting prospective contractors to submit bids for evaluation and selecting a winner or winners."@en ;
        rdfs:label     "tender"@en ;
        dcterms:title  "Tender"@en .

:awardId  a           owl:FunctionalProperty , owl:DatatypeProperty ;
        rdfs:comment  "The identifier for this award. It must be unique and cannot change within the Open Contracting Process it is part of (defined by a single ocid). See the [identifier guidance](http://standard.open-contracting.org/latest/en/schema/identifiers/) for further details."@en ;
        rdfs:domain   :Award ;
        rdfs:label    "Award ID"@en ;
        rdfs:range    xsd:string .

:ics_CPVS  a           :ItemClassificationScheme , owl:NamedIndividual ;
        rdfs:comment   "The Common Procurement Vocabulary is a standard adopted by the Commission of the European Community, and consisting of a main vocabulary for defining the subject of a contract, and a supplementary vocabulary for adding further qualitative information. The supplementary vocabulary, identified in OCDS by the code CPVS, is made up of an alphanumeric code with a corresponding wording allowing further details to be added regarding the specific nature or destination of the goods to be purchased."@en ;
        rdfs:label     "CPVS"@en ;
        dcterms:title  "EC Common Procurement Vocabulary - Supplementary Codelists"@en .

:milestoneDocuments  a  owl:ObjectProperty ;
        rdfs:comment  "List of documents associated with this milestone."@en ;
        rdfs:domain   :Milestone ;
        rdfs:label    "Milestone documents"@en ;
        rdfs:range    :Document .

:AwardCriteria  a     owl:Class ;
        rdfs:comment  "The award criteria code list describes the basis on which contract awards will be made."@en ;
        rdfs:label    "Codelist Award Criteria"@en .

:planningPrecedes  a        owl:ObjectProperty ;
        rdfs:domain         :Planning ;
        rdfs:range          :Tender ;
        rdfs:subPropertyOf  seq:directlyPrecedes .

:quantity  a          owl:FunctionalProperty , owl:DatatypeProperty ;
        rdfs:comment  "The number of units required"@en ;
        rdfs:domain   :Item ;
        rdfs:label    "quantity"@en ;
        rdfs:range    xsd:integer .

:awardStatusPending  a  :AwardStatus , owl:NamedIndividual ;
        rdfs:comment   "This award has been proposed, but is not yet in force. This may be due to a cooling off period, or some other process."@en ;
        rdfs:label     "pending"@en ;
        dcterms:title  "Pending"@en .

:documentType  a      owl:FunctionalProperty , owl:ObjectProperty ;
        rdfs:comment  "A classification of the document described taken from the [documentType codelist](http://standard.open-contracting.org/latest/en/schema/codelists/#document-type). Values from the provided codelist should be used wherever possible, though extended values can be provided if the codelist does not have a relevant code."@en ;
        rdfs:domain   :Document ;
        rdfs:label    "Document type"@en ;
        rdfs:range    :DocumentType .

:Lot    a             owl:Class ;
        rdfs:comment  "Es una conexión de uno o más ítems"@es ;
        rdfs:label    "Lote"@es .

:milestoneDateModified
        a             owl:FunctionalProperty , owl:DatatypeProperty ;
        rdfs:comment  "The date the milestone was last reviewed or modified and the status was altered or confirmed to still be correct."@en ;
        rdfs:domain   :Milestone ;
        rdfs:label    "Milestone modification date"@en ;
        rdfs:range    xsd:dateTime .

:contractDocuments  a  owl:ObjectProperty ;
        rdfs:comment  "All documents and attachments related to the contract, including any notices."@en ;
        rdfs:domain   :Contract ;
        rdfs:label    "Contract documents"@en ;
        rdfs:range    :Document .

:transactionUri  a    owl:FunctionalProperty , owl:ObjectProperty ;
        rdfs:comment  "A URI pointing directly to a machine-readable record about this spending transaction."@en ;
        rdfs:domain   :Transaction ;
        rdfs:label    "Linked spending information"@en ;
        rdfs:range    dcterms:URI .

:tenderValue  a       owl:FunctionalProperty , owl:ObjectProperty ;
        rdfs:comment  "The total upper estimated value of the procurement."@en ;
        rdfs:domain   :Tender ;
        rdfs:label    "Tender value"@en ;
        rdfs:range    :Value .

:tenderDescription  a  owl:FunctionalProperty , owl:DatatypeProperty ;
        rdfs:domain  :Tender ;
        rdfs:label   "Tender description" ;
        rdfs:range   xsd:string .

:unit   a             owl:FunctionalProperty , owl:ObjectProperty ;
        rdfs:comment  "Description of the unit which the good comes in e.g. hours, kilograms. Made up of a unit name, and the value of a single unit."@en ;
        rdfs:domain   :Item ;
        rdfs:label    "Unit"@en ;
        rdfs:range    :Unit .

:dateSigned  a        owl:FunctionalProperty , owl:DatatypeProperty ;
        rdfs:comment  "The date the contract was signed. In the case of multiple signatures, the date of the last signature."@en ;
        rdfs:domain   :Contract ;
        rdfs:label    "Date of signature"@en ;
        rdfs:range    xsd:dateTime .

:initiationType  a    owl:FunctionalProperty , owl:ObjectProperty ;
        rdfs:comment  "String specifying the type of initiation process used for this contract, taken from the [initiationType](http://standard.open-contracting.org/latest/en/schema/codelists/#initiation-type) codelist. Currently only tender is supported."@en ;
        rdfs:domain   :Release ;
        rdfs:label    "Initiation Type"@en ;
        rdfs:range    :InitiationType .

:ContractStatus  a           owl:Class ;
        rdfs:comment         "Contracts can move through multiple states. Releases over time may update the status of a contract."@en ;
        rdfs:label           "Codelist Contract Status"@en ;
        owl:equivalentClass  [ a          owl:Class ;
                               owl:oneOf  ( :contractStatusActive :contractStatusCancelled :contractStatusPending :contractStatusTerminated )
                             ] .

:budget  a           owl:FunctionalProperty , owl:ObjectProperty ;
        rdfs:domain  :Planning ;
        rdfs:label   "Budget"@en ;
        rdfs:range   :Budget .

:tenderPeriod  a      owl:FunctionalProperty , owl:ObjectProperty ;
        rdfs:comment  "The period when the tender is open for submissions. The end date is the closing date for tender submissions."@en ;
        rdfs:domain   :Tender ;
        rdfs:label    "Tender period"@en ;
        rdfs:range    :Period .

:documentDescription  a  owl:FunctionalProperty , owl:DatatypeProperty ;
        rdfs:comment  "A short description of the document. We recommend descriptions do not exceed 250 words. In the event the document is not accessible online, the description field can be used to describe arrangements for obtaining a copy of the document."@en ;
        rdfs:domain   :Document ;
        rdfs:label    "Document description"@en ;
        rdfs:range    xsd:string .

:methodLimited  a      :Method , owl:NamedIndividual ;
        rdfs:comment   "Limited tendering means a procurement method whereby the procuring entity contacts a supplier or suppliers of its choice."@en ;
        rdfs:label     "limited"@en ;
        dcterms:title  "Limited"@en .

:Tender  a               owl:Class ;
        rdfs:comment     "Data regarding tender process - publicly inviting prospective contractors to submit bids for evaluation and selecting a winner or winners"@en ;
        rdfs:label       "Tender"@en ;
        rdfs:subClassOf  pc:Tender .

:releaseDate  a       owl:FunctionalProperty , owl:DatatypeProperty ;
        rdfs:comment  "The date this information is released, it may well be the same as the parent publishedDate, it must not be later than the publishedDate from the parent package. It is used to determine merge order."@en ;
        rdfs:domain   :Release ;
        rdfs:label    "Release Date" ;
        rdfs:range    xsd:dateTime .

:organizationName  a  owl:FunctionalProperty , owl:DatatypeProperty ;
        rdfs:comment  "The common name of the organization. The ID property provides an space for the formal legal name, and so this may either repeat that value, or could provide the common name by which this organization is known. This field could also include details of the department or sub-unit involved in this contracting process."@en ;
        rdfs:domain   :Organization ;
        rdfs:label    "Organization name"@en ;
        rdfs:range    xsd:string .

:Implementation  a    owl:Class ;
        rdfs:comment  "Information during the performance / implementation stage of the contract."@en ;
        rdfs:label    "Implementation" .

:releaseTagAward  a    :ReleaseTag , owl:NamedIndividual ;
        rdfs:label     "award"@en ;
        dcterms:title  "Award"@en .

:contractStatusCancelled
        a              :ContractStatus , owl:NamedIndividual ;
        rdfs:comment   "This contract has been cancelled prior to being signed."@en ;
        rdfs:label     "cancelled"@en ;
        dcterms:title  "Cancelled"@en .

:projectID  a         owl:FunctionalProperty , owl:DatatypeProperty ;
        rdfs:comment  "An external identifier for the project that this contracting process forms part of, or is funded via (if applicable). Some organizations maintain a registry of projects, and the data should use the identifier from the relevant registry of projects."@en ;
        rdfs:domain   :Budget ;
        rdfs:label    "Project Identifier"@en ;
        rdfs:range    xsd:string , xsd:integer .

:Contract  a             owl:Class ;
        rdfs:comment     "Information regarding the signed contract between the buyer and supplier(s)."@en ;
        rdfs:label       "Contract"@en ;
        rdfs:subClassOf  pc:Contract .

:releaseTagImplementationUpdate
        a              :ReleaseTag , owl:NamedIndividual ;
        rdfs:label     "implementationUpdate"@en ;
        dcterms:title  "Implementation Update"@en .

:releaseTagContractUpdate
        a              :ReleaseTag , owl:NamedIndividual ;
        rdfs:label     "contractUpdate"@en ;
        dcterms:title  "Contract Update"@en .

:budgetId  a          owl:FunctionalProperty , owl:DatatypeProperty ;
        rdfs:comment  "An identifier for the budget line item which provides funds for this contracting process. This identifier should be possible to cross-reference against the provided data source."@en ;
        rdfs:domain   :Budget ;
        rdfs:label    "Budget ID"@en ;
        rdfs:range    xsd:string , xsd:integer .

:Award  a             owl:Class ;
        rdfs:comment  "An award for the given procurement. There may be more than one award per contracting process e.g. because the contract is split amongst different providers, or because it is a standing offer."@en ;
        rdfs:label    "Award"@en .

:amendmentDate  a     owl:FunctionalProperty , owl:DatatypeProperty ;
        rdfs:comment  "The data of this amendment."@en ;
        rdfs:domain   :Amendment ;
        rdfs:label    "Amendment Date"@en ;
        rdfs:range    xsd:dateTime .

:awardCriteriaBestProposal
        a              :AwardCriteria , owl:NamedIndividual ;
        rdfs:label     "bestProposal"@en ;
        dcterms:title  "Best Proposal Cost"@en .

:additionalIdentifiers
        a             owl:ObjectProperty ;
        rdfs:comment  "A list of additional / supplemental identifiers for the organization, using the [organization identifier guidance](http://standard.open-contracting.org/latest/en/schema/identifiers/). This could be used to provide an internally used identifier for this organization in addition to the primary legal entity identifier."@en ;
        rdfs:domain   :Organization ;
        rdfs:label    "Additional identifiers"@en ;
        rdfs:range    :Identifier .

:awardStatusCancelled
        a              :AwardStatus , owl:NamedIndividual ;
        rdfs:comment   "This award has been cancelled."@en ;
        rdfs:label     "cancelled"@en ;
        dcterms:title  "Cancelled"@en .

:contractItems  a     owl:ObjectProperty ;
        rdfs:comment  "The goods, services, and any intangible outcomes in this contract. Note: If the items are the same as the award do not repeat."@en ;
        rdfs:domain   :Contract ;
        rdfs:label    "Items Contracted"@en ;
        rdfs:range    :Item .

:awardCriteriaDetails
        a             owl:FunctionalProperty , owl:DatatypeProperty ;
        rdfs:comment  "Any detailed or further information on the award or selection criteria."@en ;
        rdfs:domain   :Tender ;
        rdfs:label    "Award criteria details"@en ;
        rdfs:range    xsd:string .

:changes  a           owl:ObjectProperty ;
        rdfs:comment  "Comma-separated list of affected fields."@en ;
        rdfs:domain   :Amendment ;
        rdfs:label    "Amended fields"@en ;
        rdfs:range    :Change .

:classificationDescription
        a             owl:FunctionalProperty , owl:DatatypeProperty ;
        rdfs:comment  "A textual description or title for the code."@en ;
        rdfs:domain   :Classification ;
        rdfs:label    "Classification description"@en ;
        rdfs:range    xsd:string .

:format  a            owl:FunctionalProperty , owl:DatatypeProperty ;
        rdfs:comment  "The format of the document taken from the [IANA Media Types code list](http://www.iana.org/assignments/media-types/), with the addition of one extra value for 'offline/print', used when this document entry is being used to describe the offline publication of a document. Use values from the template column. Links to web pages should be tagged 'text/html'."@en ;
        rdfs:domain   :Document ;
        rdfs:label    "Format"@en ;
        rdfs:range    xsd:string .

:contractFollows  a         owl:ObjectProperty ;
        rdfs:domain         :Contract ;
        rdfs:range          :Award ;
        rdfs:subPropertyOf  seq:directlyFollows .

:classificationUri  a  owl:FunctionalProperty , owl:ObjectProperty ;
        rdfs:comment  "A URI to identify the code. In the event individual URIs are not available for items in the identifier scheme this value should be left blank."@en ;
        rdfs:domain   :Classification ;
        rdfs:label    "Classification URI"@en ;
        rdfs:range    dcterms:URI .

:planningRationale  a  owl:FunctionalProperty , owl:DatatypeProperty ;
        rdfs:comment  "The rationale for the procurement provided in free text. More detail can be provided in an attached document."@en ;
        rdfs:domain   :Planning ;
        rdfs:label    "Planning rationale"@en ;
        rdfs:range    xsd:string .

:Amendment  a       owl:Class ;
        rdfs:label  "Amendment"@en .

dcterms:title  a  owl:AnnotationProperty .

:faxNumber  a         owl:FunctionalProperty , owl:DatatypeProperty ;
        rdfs:comment  "The fax number of the contact point/person. This should include the international dialling code."@en ;
        rdfs:domain   :ContactPoint ;
        rdfs:label    "Fax number"@en ;
        rdfs:range    xsd:string .

:awardStatusUnsuccessful
        a              :AwardStatus , owl:NamedIndividual ;
        rdfs:comment   "This award could not be successfully made. If items or supplier details are included within the award section, then these narrow the scope of the unsuccessful award (i.e. the award of noted items, or an award to the noted supplier, was unsuccessful, but there may be other successful awards for different items listed in the tender, or to different suppliers)."@en ;
        rdfs:label     "unsuccessful"@en ;
        dcterms:title  "Unsuccessful"@en .

:milestoneDescription
        a             owl:FunctionalProperty , owl:DatatypeProperty ;
        rdfs:comment  "A description of the milestone."@en ;
        rdfs:domain   :Milestone ;
        rdfs:label    "Milestone description"@en ;
        rdfs:range    xsd:string .

:valueAmount  a       owl:FunctionalProperty , owl:DatatypeProperty ;
        rdfs:comment  "Amount as a number."@en ;
        rdfs:domain   :Value ;
        rdfs:label    "Amount"@en ;
        rdfs:range    xsd:integer .

:id     a             owl:FunctionalProperty , owl:DatatypeProperty ;
        rdfs:comment  "A unique identifier that identifies this release. A release ID must be unique within a release-package and must not contain the # character."@en ;
        rdfs:domain   :Release ;
        rdfs:label    "Release ID" ;
        rdfs:range    xsd:string .

:awardDescription  a  owl:FunctionalProperty , owl:DatatypeProperty ;
        rdfs:domain  :Award ;
        rdfs:label   "Award description" ;
        rdfs:range   xsd:string .

:suppliers  a         owl:ObjectProperty ;
        rdfs:comment  "The suppliers awarded this award. If different suppliers have been awarded different items of values, these should be split into separate award blocks."@en ;
        rdfs:domain   :Award ;
        rdfs:label    "Suppliers"@en ;
        rdfs:range    :Organization .

:tenderPrecedes  a          owl:ObjectProperty ;
        rdfs:domain         :Tender ;
        rdfs:range          :Award ;
        rdfs:subPropertyOf  seq:directlyPrecedes .

:contactPointName  a  owl:FunctionalProperty , owl:DatatypeProperty ;
        rdfs:comment  "The name of the contact person, department, or contact point, for correspondence relating to this contracting process."@en ;
        rdfs:domain   :ContactPoint ;
        rdfs:label    "Contact point name"@en ;
        rdfs:range    xsd:string .

:tenderStatus  a      owl:FunctionalProperty , owl:ObjectProperty ;
        rdfs:comment  "The current status of the tender based on the [tenderStatus codelist](http://standard.open-contracting.org/latest/en/schema/codelists/#tender-status)"@en ;
        rdfs:domain   :Tender ;
        rdfs:label    "Tender Status"@en ;
        rdfs:range    :TenderStatus .

:locality  a          owl:FunctionalProperty , owl:DatatypeProperty ;
        rdfs:comment  "The locality. For example, Mountain View."@en ;
        rdfs:domain   :Address ;
        rdfs:label    "Locality"@en ;
        rdfs:range    xsd:string .

:Unit   a           owl:Class ;
        rdfs:label  "Unit"@en .

:Method  a                   owl:Class ;
        rdfs:comment         "The method codelist is based upon the GPA Definitions provided here."@en ;
        rdfs:label           "Codelist Method"@en ;
        owl:equivalentClass  [ a          owl:Class ;
                               owl:oneOf  ( :methodLimited :methodOpen :methodSelective )
                             ] .

:implementationMilestones
        a             owl:ObjectProperty ;
        rdfs:comment  "As milestones are completed, milestone completions should be documented."@en ;
        rdfs:domain   :Implementation ;
        rdfs:label    "Implementation milestones"@en ;
        rdfs:range    :Milestone .

dcterms:URI  a  owl:Class .

:contractStatusTerminated
        a              :ContractStatus , owl:NamedIndividual ;
        rdfs:comment   "This contract was signed and in force, and has now come to a close. This may be due to successful completion of the contract, or may be early termination due to some non-completion."@en ;
        rdfs:label     "terminated"@en ;
        dcterms:title  "Terminated"@en .

:contractStatusPending
        a              :ContractStatus , owl:NamedIndividual ;
        rdfs:comment   "This contract has been proposed, but is not yet in force. It may be awaiting signature."@en ;
        rdfs:label     "pending"@en ;
        dcterms:title  "Pending"@en .

:methodOpen  a         :Method , owl:NamedIndividual ;
        rdfs:comment   "Open tendering means a procurement method whereby all interested suppliers may submit a tender."@en ;
        rdfs:label     "open"@en ;
        dcterms:title  "Open"@en .

:procurementMethod  a  owl:FunctionalProperty , owl:ObjectProperty ;
        rdfs:comment  "Specify tendering method against the [method codelist](http://standard.open-contracting.org/latest/en/schema/codelists/#method) as per [GPA definitions](http://www.wto.org/english/docs_e/legal_e/rev-gpr-94_01_e.htm) of Open, Selective, Limited"@en ;
        rdfs:domain   :Tender ;
        rdfs:label    "Procurement method"@en ;
        rdfs:range    :Method .

:tenderLots  a        owl:ObjectProperty ;
        rdfs:comment  "List of lots associated with the tender"@en ;
        rdfs:domain   :Tender ;
        rdfs:label    "Tender lots"@en ;
        rdfs:range    :Lot .

:classificationScheme
        a             owl:FunctionalProperty , owl:ObjectProperty ;
        rdfs:comment  "An classification should be drawn from an existing scheme or list of codes. This field is used to indicate the scheme/codelist from which the classification is drawn. For line item classifications, this value should represent an known [Item Classification Scheme](http://standard.open-contracting.org/latest/en/schema/codelists/#item-classification-scheme) wherever possible."@en ;
        rdfs:domain   :Classification ;
        rdfs:label    "Classification scheme"@en ;
        rdfs:range    :ItemClassificationScheme .

:documentUrl  a       owl:FunctionalProperty , owl:ObjectProperty ;
        rdfs:comment  "Direct link to the document or attachment. The server providing access to this document should be configured to correctly report the document mime type."@en ;
        rdfs:domain   :Document ;
        rdfs:label    "Document URL"@en ;
        rdfs:range    dcterms:URI .

:Milestone  a       owl:Class ;
        rdfs:label  "Milestone"@en .

:award  a             owl:InverseFunctionalProperty , owl:ObjectProperty ;
        rdfs:comment  "Information from the award phase of the contracting process. There may be more than one award per contracting process e.g. because the contract is split amongst different providers, or because it is a standing offer."@en ;
        rdfs:domain   :Release ;
        rdfs:label    "Awards"@en ;
        rdfs:range    :Award .

:legalName  a         owl:FunctionalProperty , owl:DatatypeProperty ;
        rdfs:comment  "The legally registered name of the organization."@en ;
        rdfs:domain   :Identifier ;
        rdfs:label    "Legal name"@en ;
        rdfs:range    xsd:string .

:enquiryPeriod  a     owl:FunctionalProperty , owl:ObjectProperty ;
        rdfs:comment  "The period during which enquiries may be made and answered."@en ;
        rdfs:domain   :Tender ;
        rdfs:label    "Enquiry period"@en ;
        rdfs:range    :Period .

:tender  a            owl:InverseFunctionalProperty , owl:ObjectProperty ;
        rdfs:comment  "The activities undertaken in order to enter into a contract."@en ;
        rdfs:domain   :Release ;
        rdfs:label    "Tender"@en ;
        rdfs:range    :Tender .

:awardPrecedes  a           owl:ObjectProperty ;
        rdfs:domain         :Award ;
        rdfs:range          :Contract ;
        rdfs:subPropertyOf  seq:directlyPrecedes .

:releaseTagContractAmendment
        a              :ReleaseTag , owl:NamedIndividual ;
        rdfs:label     "contractAmendment"@en ;
        dcterms:title  "Contract Amendment"@en .

:documentTypeTenderNotice
        a              :DocumentType , owl:NamedIndividual ;
        rdfs:comment   "The formal notice that gives details of a tender. This may be a link to a downloadable document, to a web page, or to an official gazette in which the notice is contained."@en ;
        rdfs:label     "tenderNotice"@en ;
        dcterms:title  "Tender Notice"@en .

:tenderStatusCancelled
        a              :TenderStatus , owl:NamedIndividual ;
        rdfs:comment   "The tender process has been cancelled."@en ;
        rdfs:label     "cancelled"@en ;
        dcterms:title  "Cancelled"@en .

:contractId  a        owl:FunctionalProperty , owl:DatatypeProperty ;
        rdfs:comment  "The identifier for this contract. It must be unique and cannot change within its Open Contracting Process (defined by a single ocid). See the [identifier guidance](http://standard.open-contracting.org/latest/en/schema/identifiers/) for further details."@en ;
        rdfs:domain   :Contract ;
        rdfs:label    "Contract ID"@en ;
        rdfs:range    xsd:string , xsd:integer .

:budgetAmount  a      owl:ObjectProperty ;
        rdfs:comment  "The value of the budget line item."@en ;
        rdfs:domain   :Budget ;
        rdfs:label    "Budget amount"@en ;
        rdfs:range    :Value .

:tenderTitle  a      owl:FunctionalProperty , owl:DatatypeProperty ;
        rdfs:domain  :Tender ;
        rdfs:label   "Tender title"@en ;
        rdfs:range   xsd:string .

:tenderFollows  a           owl:ObjectProperty ;
        rdfs:domain         :Tender ;
        rdfs:range          :Planning ;
        rdfs:subPropertyOf  seq:directlyFollows .

:property  a          owl:FunctionalProperty , owl:DatatypeProperty ;
        rdfs:comment  "The property name that has been changed relative to the place the amendment is. For example if the contract value has changed, then the property under changes within the contract.amendment would be value.amount."@en ;
        rdfs:domain   :Change ;
        rdfs:label    "Property"@en ;
        rdfs:range    xsd:string .

:submissionMethodElectronicAuction
        a              :SubmissionMethod , owl:NamedIndividual ;
        rdfs:label     "electronicAuction"@en ;
        dcterms:title  "Electronic Auction"@en .

:classification  a    owl:FunctionalProperty , owl:ObjectProperty ;
        rdfs:comment  "The primary classification for the item. See the [itemClassificationScheme](http://standard.open-contracting.org/latest/en/schema/codelists/#item-classification-scheme) to identify preferred classification lists, including CPV and GSIN."@en ;
        rdfs:domain   :Item ;
        rdfs:label    "Classification"@en ;
        rdfs:range    :Classification .

:TenderStatus  a             owl:Class ;
        rdfs:comment         "The tender.status field is used to indicate the current status of a tender process."@en ;
        rdfs:label           "Codelist Tender Status"@en ;
        owl:equivalentClass  [ a          owl:Class ;
                               owl:oneOf  ( :tenderStatusActive :tenderStatusCancelled :tenderStatusComplete :tenderStatusPlanned :tenderStatusUnsuccessful )
                             ] .

:Release  a         owl:Class ;
        rdfs:label  "Open Contracting Release"@en .

:providerOrganization
        a             owl:ObjectProperty ;
        rdfs:comment  "The Organization Identifier for the organization from which the funds in this transaction originate. Expressed following the Organizational Identifier standard - consult the documentation and the codelist."@en ;
        rdfs:domain   :Transaction ;
        rdfs:label    "Provider organization"@en ;
        rdfs:range    :Identifier .

:awardFollows  a            owl:ObjectProperty ;
        rdfs:domain         :Award ;
        rdfs:range          :Tender ;
        rdfs:subPropertyOf  seq:directlyFollows .

:releaseTagTender  a   :ReleaseTag , owl:NamedIndividual ;
        rdfs:comment   "Announcing a new tender (call for proposals) process. Tender release should contain details of the goods or services being sought."@en ;
        rdfs:label     "tender"@en ;
        dcterms:title  "Tender"@en .

:releaseTagContract  a  :ReleaseTag , owl:NamedIndividual ;
        rdfs:label     "contract"@en ;
        dcterms:title  "Contract"@en .

:telephone  a         owl:DatatypeProperty ;
        rdfs:comment  "The telephone number of the contact point/person. This should include the international dialling code."@en ;
        rdfs:domain   :ContactPoint ;
        rdfs:label    "Telephone"@en ;
        rdfs:range    xsd:string .

:tenderDocuments  a   owl:ObjectProperty ;
        rdfs:comment  "All documents and attachments related to the tender, including any notices. See the [documentType codelist](http://standard.open-contracting.org/latest/en/schema/codelists/#document-type) for details of potential documents to include."@en ;
        rdfs:domain   :Tender ;
        rdfs:label    "Tender documents"@en ;
        rdfs:range    :Document .

:contactPoint  a     owl:ObjectProperty ;
        rdfs:domain  :Organization ;
        rdfs:label   "Contact point"@en ;
        rdfs:range   :ContactPoint .

:contactPointUrl  a   owl:FunctionalProperty , owl:ObjectProperty ;
        rdfs:comment  "A web address for the contact point/person."@en ;
        rdfs:domain   :ContactPoint ;
        rdfs:label    "Contact point URL"@en ;
        rdfs:range    dcterms:URI .

:InitiationType  a           owl:Class ;
        rdfs:comment         "Contracting processes may be formed under a number of different processes. Currently, only ‘tender’ is supported in this codelist. Future versions of the standard may support other Initiation Types. The initiation type may be provide information to consuming applications on the different blocks of data and releases they should expect from a contracting process."@en ;
        rdfs:label           "Codelist Initiation Type"@en ;
        owl:equivalentClass  [ a          owl:Class ;
                               owl:oneOf  ( :initiationTypeTender )
                             ] .

:submissionMethod  a  owl:FunctionalProperty , owl:DatatypeProperty ;
        rdfs:comment  "pecify the method by which bids must be submitted, in person, written, or electronic auction. Using the [submission method codelist](http://standard.open-contracting.org/latest/en/schema/codelists/#submission-method)"@en ;
        rdfs:domain   :Tender ;
        rdfs:label    "Submission method"@en ;
        rdfs:range    xsd:string .

:contracts  a         owl:InverseFunctionalProperty , owl:ObjectProperty ;
        rdfs:comment  "Information from the contract creation phase of the procurement process."@en ;
        rdfs:domain   :Release ;
        rdfs:label    "Contracts"@en ;
        rdfs:range    :Contract .

:countryName  a       owl:FunctionalProperty , owl:DatatypeProperty ;
        rdfs:comment  "The country name. For example, United States."@en ;
        rdfs:domain   :Address ;
        rdfs:label    "Country name"@en ;
        rdfs:range    xsd:string .

:region  a            owl:FunctionalProperty , owl:DatatypeProperty ;
        rdfs:comment  "The region. For example, CA."@en ;
        rdfs:domain   :Address ;
        rdfs:label    "Region"@en ;
        rdfs:range    xsd:string .

:procurementMethodRationale
        a             owl:FunctionalProperty , owl:DatatypeProperty ;
        rdfs:comment  "Rationale of procurement method, especially in the case of Limited tendering."@en ;
        rdfs:domain   :Tender ;
        rdfs:label    "Procurement method rationale"@en ;
        rdfs:range    xsd:string .

:releaseTagTenderCancellation
        a              :ReleaseTag , owl:NamedIndividual ;
        rdfs:label     "tenderCancellation"@en ;
        dcterms:title  "Tender Cancellation"@en .

:awardValue  a        owl:FunctionalProperty , owl:ObjectProperty ;
        rdfs:comment  "The total value of this award. In the case of a framework contract this may be the total estimated lifetime value, or maximum value, of the agreement. There may be more than one award per procurement."@en ;
        rdfs:domain   :Award ;
        rdfs:label    "Award value"@en ;
        rdfs:range    :Value .

:dueDate  a           owl:FunctionalProperty , owl:DatatypeProperty ;
        rdfs:comment  "The date the milestone is due."@en ;
        rdfs:domain   :Milestone ;
        rdfs:label    "Due date"@en ;
        rdfs:range    xsd:dateTime .

:hasEnquiries  a      owl:FunctionalProperty , owl:DatatypeProperty ;
        rdfs:comment  " Yes/No field to indicate whether enquiries were part of tender process."@en ;
        rdfs:domain   :Tender ;
        rdfs:label    "Has enquiries"@en ;
        rdfs:range    xsd:boolean .

:planningUrl  a       owl:FunctionalProperty , owl:DatatypeProperty ;
        rdfs:comment  "Url para poder identificar el servicio que es utilizado para generar la planificación"@es ;
        rdfs:domain   :Planning ;
        rdfs:label    "Planning URL"@es ;
        rdfs:range    xsd:anyURI .

:transactionDate  a   owl:FunctionalProperty , owl:DatatypeProperty ;
        rdfs:comment  "The date of the transaction"@en ;
        rdfs:domain   :Transaction ;
        rdfs:label    "Transaction date"@en ;
        rdfs:range    xsd:dateTime .

:planning  a          owl:FunctionalProperty , owl:ObjectProperty ;
        rdfs:comment  "Information from the planning phase of the contracting process. This includes information related to the process of deciding what to contract for, when and how."@en ;
        rdfs:domain   :Release ;
        rdfs:label    "Planning"@en ;
        rdfs:range    :Planning .

:transactionId  a     owl:FunctionalProperty , owl:DatatypeProperty ;
        rdfs:comment  "A unique identifier for this transaction. This identifier should be possible to cross-reference against the provided data source. For the budget data package this is the id, for IATI, the transaction reference."@en ;
        rdfs:domain   :Transaction ;
        rdfs:label    "Transaction ID"@en ;
        rdfs:range    xsd:string , xsd:integer .

:awardDate  a         owl:FunctionalProperty , owl:DatatypeProperty ;
        rdfs:comment  "The date of the contract award. This is usually the date on which a decision to award was made." ;
        rdfs:domain   :Award ;
        rdfs:label    "Award date"@en ;
        rdfs:range    xsd:dateTime .

:endDate  a           owl:FunctionalProperty , owl:DatatypeProperty ;
        rdfs:comment  "The end date for the period."@en ;
        rdfs:domain   :Period ;
        rdfs:label    "End date"@en ;
        rdfs:range    xsd:dateTime .

:additionalClassifications
        a             owl:ObjectProperty ;
        rdfs:comment  "An array of additional classifications for the item. See the [itemClassificationScheme](http://standard.open-contracting.org/latest/en/schema/codelists/#item-classification-scheme) codelist for common options to use in OCDS. This may also be used to present codes from an internal classification scheme."@en ;
        rdfs:domain   :Item ;
        rdfs:label    "Additional classifications"@en ;
        rdfs:range    :Classification .

:buyer  a             owl:FunctionalProperty , owl:ObjectProperty ;
        rdfs:comment  "The buyer is the entity whose budget will be used to purchase the goods. This may be different from the procuring agency who may be specified in the tender data."@en ;
        rdfs:domain   :Release ;
        rdfs:label    "Buyer"@en ;
        rdfs:range    :Organization .

:lotTitle  a         owl:FunctionalProperty , owl:DatatypeProperty ;
        rdfs:domain  :Lot ;
        rdfs:range   xsd:string .

:receiverOrganization
        a             owl:ObjectProperty ;
        rdfs:comment  "The Organization Identifier for the organization which receives the funds in this transaction. Expressed following the Organizational Identifier standard - consult the documentation and the codelist."@en ;
        rdfs:domain   :Transaction ;
        rdfs:label    "Receiver organization"@en ;
        rdfs:range    :Identifier .

:address  a          owl:ObjectProperty ;
        rdfs:domain  :Organization ;
        rdfs:label   "Address"@en ;
        rdfs:range   :Address .

:milestones  a        owl:ObjectProperty ;
        rdfs:comment  "A list of milestones associated with the tender."@en ;
        rdfs:domain   :Tender ;
        rdfs:label    "Milestones"@en ;
        rdfs:range    :Milestone .

:postalCode  a        owl:FunctionalProperty , owl:DatatypeProperty ;
        rdfs:comment  "The postal code. For example, 94043."@en ;
        rdfs:domain   :Address ;
        rdfs:label    "Postal code"@en ;
        rdfs:range    xsd:string .

:budgetSource  a      owl:FunctionalProperty , owl:ObjectProperty ;
        rdfs:comment  "Used to point either to a corresponding Budget Data Package, or to a machine or human-readable source where users can find further information on the budget line item identifiers, or project identifiers, provided here." ;
        rdfs:domain   :Budget ;
        rdfs:label    "Budget Data Source"@en ;
        rdfs:range    rdfs:Resource .

:contractSuppliers  a  owl:ObjectProperty ;
        rdfs:comment  "The suppliers awarded this contract. Is an implementacion of DNCP"@en ;
        rdfs:domain   :Contract ;
        rdfs:label    "Contract Suppliers"@en ;
        rdfs:range    :Organization .

:releaseTagPlanning  a  :ReleaseTag , owl:NamedIndividual ;
        rdfs:label     "planning"@en ;
        dcterms:title  "Planning"@en .

:submissionMethodInPerson
        a              :SubmissionMethod , owl:NamedIndividual ;
        rdfs:label     "inPerson"@en ;
        dcterms:title  "In Person"@en .

:implementationDocuments
        a             owl:ObjectProperty ;
        rdfs:comment  "Documents and reports that are part of the implementation phase e.g. audit and evaluation reports."@en ;
        rdfs:domain   :Implementation ;
        rdfs:label    "Implementation documents"@en ;
        rdfs:range    :Document .

:tenderItems  a       owl:ObjectProperty ;
        rdfs:comment  "The goods and services to be purchased, broken into line items wherever possible. Items should not be duplicated, but a quantity of 2 specified instead."@en ;
        rdfs:domain   :Tender ;
        rdfs:label    "Items to be procured"@en ;
        rdfs:range    :Item .

:procuringEntity  a   owl:FunctionalProperty , owl:ObjectProperty ;
        rdfs:comment  "The entity managing the procurement, which may be different from the buyer who is paying / using the items being procured."@en ;
        rdfs:domain   :Tender ;
        rdfs:label    "Procuring entity"@en ;
        rdfs:range    :Organization .

:milestoneTitle  a   owl:FunctionalProperty , owl:DatatypeProperty ;
        rdfs:domain  :Milestone ;
        rdfs:label   "Milestone title"@en ;
        rdfs:range   xsd:string .

:contractLots  a      owl:ObjectProperty ;
        rdfs:comment  "List of lots associated with the contract"@en ;
        rdfs:domain   :Contract ;
        rdfs:label    "Contract lots"@en ;
        rdfs:range    :Lot .

:releaseLanguage  a   owl:FunctionalProperty , owl:DatatypeProperty ;
        rdfs:comment  "pecifies the default language of the data using either two-digit ISO 639-1, or extended BCP47 language tags. The use of two-letter codes from ISO 639-1 is strongly recommended."@en ;
        rdfs:domain   :Release ;
        rdfs:label    "Release language"@en ;
        rdfs:range    xsd:string .

:contractPeriod  a    owl:FunctionalProperty , owl:ObjectProperty ;
        rdfs:comment  "The start and end date for the contract."@en , "The period for which the contract has been awarded."@en ;
        rdfs:domain   :Contract , :Award ;
        rdfs:label    "Contract period"@en ;
        rdfs:range    :Period .

:awardPeriod  a       owl:FunctionalProperty , owl:ObjectProperty ;
        rdfs:comment  "The date or period on which an award is anticipated to be made."@en ;
        rdfs:domain   :Tender ;
        rdfs:label    "Award period"@en ;
        rdfs:range    :Period .

:numberOfTenderers  a  owl:FunctionalProperty , owl:DatatypeProperty ;
        rdfs:comment  "The number of entities who submit a tender."@en ;
        rdfs:domain   :Tender ;
        rdfs:label    "Number of tenders"@en ;
        rdfs:range    xsd:integer .

:awardCriteriaBestValueToGovernment
        a              :AwardCriteria , owl:NamedIndividual ;
        rdfs:label     "bestValueToGovernment"@en ;
        dcterms:title  "Best Value to Government"@en .

:DocumentType  a      owl:Class ;
        rdfs:comment  "This list provides details of the documents that publishers may wish to provide at various points their contracting process."@en ;
        rdfs:label    "Codelist Document Type"@en .

:tenderAmendment  a   owl:ObjectProperty ;
        rdfs:comment  ""@en ;
        rdfs:domain   :Tender ;
        rdfs:label    "Tender amendment"@en ;
        rdfs:range    :Amendment .

:awardCriteriaLowestCost
        a              :AwardCriteria , owl:NamedIndividual ;
        rdfs:label     "lowestCost"@en ;
        dcterms:title  "Lowest Cost"@en .

:releaseTagAwardUpdate
        a              :ReleaseTag , owl:NamedIndividual ;
        rdfs:label     "awardUpdate"@en ;
        dcterms:title  "Award Update"@en .

:itemId  a            owl:FunctionalProperty , owl:DatatypeProperty ;
        rdfs:comment  "A local identifier to reference and merge the items by. Must be unique within a given array of items."@en ;
        rdfs:domain   :Item ;
        rdfs:label    "Item ID"@en ;
        rdfs:range    xsd:string , xsd:integer .

:tenderStatusPlanned  a  :TenderStatus , owl:NamedIndividual ;
        rdfs:comment   "This tender has been proposed, but is not yet taking place."@en ;
        rdfs:label     "planned"@en ;
        dcterms:title  "Planned"@en .

:minValue  a          owl:FunctionalProperty , owl:ObjectProperty ;
        rdfs:comment  "The minimum estimated value of the procurement."@en ;
        rdfs:domain   :Tender ;
        rdfs:label    "Minimum value"@en ;
        rdfs:range    :Value .

:tag    a             owl:FunctionalProperty , owl:ObjectProperty ;
        rdfs:comment  "A value from the [releaseTag codelist](http://standard.open-contracting.org/latest/en/schema/codelists/#release-tag) that identifies the nature of the release being made. Tags may be used to filter release, or, in future, for for advanced validation when certain kinds of releases should contain certain fields."@en ;
        rdfs:domain   :Release ;
        rdfs:label    "Release Tag"@en ;
        rdfs:range    :ReleaseTag .

:awardAmendment  a   owl:ObjectProperty ;
        rdfs:domain  :Award ;
        rdfs:label   "Award amendment"@en ;
        rdfs:range   :Amendment .

:Organization  a             owl:Class ;
        rdfs:comment         "An organization."@en ;
        rdfs:label           "Organization"@en ;
        owl:equivalentClass  gr:BusinessEntity .

:contractDescription  a  owl:FunctionalProperty , owl:DatatypeProperty ;
        rdfs:domain  :Contract ;
        rdfs:label   "Contract description"@en ;
        rdfs:range   xsd:string .

:currency  a          owl:FunctionalProperty , owl:DatatypeProperty ;
        rdfs:comment  "The currency in 3-letter ISO 4217 format."@en ;
        rdfs:domain   :Value ;
        rdfs:label    "Currency"@en ;
        rdfs:range    xsd:string .

:releaseTagCompiled  a  :ReleaseTag , owl:NamedIndividual ;
        rdfs:comment   "This tag is used only in compiled records, which have merged together multiple releases to provide a snapshot view of the contract, and a version history."@en ;
        rdfs:label     "compiled"@en ;
        dcterms:title  "Compiled Record"@en .

:lotId  a            owl:FunctionalProperty , owl:DatatypeProperty ;
        rdfs:domain  :Lot ;
        rdfs:range   xsd:string .
