@prefix foaf:  <http://xmlns.com/foaf/0.1/> .
@prefix ssn:   <https://www.w3.org/ns/ssn/> .
@prefix vann:  <http://purl.org/vocab/vann/> .
@prefix cdt:   <http://w3id.org/lindt/custom_datatypes#> .
@prefix vs:    <http://www.w3.org/2003/06/sw-vocab-status/ns#> .
@prefix qb:    <http://purl.org/linked-data/cube#> .
@prefix dcterms: <http://purl.org/dc/terms/> .
@prefix voaf:  <http://purl.org/vocommons/voaf#> .
@prefix rdfs:  <http://www.w3.org/2000/01/rdf-schema#> .
@prefix seas:  <https://w3id.org/seas/> .
@prefix dul:   <http://www.ontologydesignpatterns.org/ont/dul/DUL.owl#> .
@prefix xsd:   <http://www.w3.org/2001/XMLSchema#> .
@prefix owl:   <http://www.w3.org/2002/07/owl#> .
@prefix rdf:   <http://www.w3.org/1999/02/22-rdf-syntax-ns#> .
@prefix liner: <https://w3id.org/liner/> .
@prefix sdmx:  <http://purl.org/linked-data/sdmx#> .
@prefix skos:  <http://www.w3.org/2004/02/skos/core#> .
@prefix cc:    <http://creativecommons.org/ns#> .

seas:DistributionMeanEvaluation
        a                 owl:Class ;
        rdfs:comment      "The evaluated value is the mean of the property value distribution."@en ;
        rdfs:isDefinedBy  seas:StatisticsOntology ;
        rdfs:label        "Distribution Mean Evaluation"@en ;
        rdfs:subClassOf   seas:Evaluation ;
        vs:term_status    "testing" .

dcterms:description  a  owl:AnnotationProperty .

dcterms:creator  a  owl:AnnotationProperty .

seas:DistributionMinimumEvaluation
        a                 owl:Class ;
        rdfs:comment      "The evaluated value is the minimum of the property value distribution."@en ;
        rdfs:isDefinedBy  seas:StatisticsOntology ;
        rdfs:label        "Distribution Minimum Evaluation"@en ;
        rdfs:subClassOf   seas:Evaluation ;
        vs:term_status    "testing" .

voaf:Vocabulary  a  owl:Class .

dcterms:modified  a  owl:AnnotationProperty .

dcterms:contributor  a  owl:AnnotationProperty .

seas:RankedDistributionEvaluation
        a                 owl:Class ;
        rdfs:comment      "The evaluated value is to be interpreted with respect to a rank, which is given as the object of property `seas:rank`."@en ;
        rdfs:isDefinedBy  seas:StatisticsOntology ;
        rdfs:label        "Ranked Distribution Evaluation"@en ;
        rdfs:subClassOf   seas:Evaluation ;
        rdfs:subClassOf   [ owl:cardinality  1 ;
                            owl:onProperty   seas:rank
                          ] ;
        vs:term_status    "testing" .

seas:rank  a              owl:FunctionalProperty , owl:DatatypeProperty ;
        rdfs:comment      "Rank number of a ranked distribution evaluation, such as for quartiles, deciles or percentiles."@en ;
        rdfs:domain       seas:RankedDistributionEvaluation ;
        rdfs:isDefinedBy  seas:StatisticsOntology ;
        rdfs:label        "rank"@en ;
        rdfs:range        xsd:integer ;
        vs:term_status    "testing" .

cc:license  a   owl:AnnotationProperty .

dcterms:issued  a  owl:AnnotationProperty .

seas:DistributionMaximumEvaluation
        a                 owl:Class ;
        rdfs:comment      "The evaluated value is the maximum of the property value distribution."@en ;
        rdfs:isDefinedBy  seas:StatisticsOntology ;
        rdfs:label        "Distribution Maximum Evaluation"@en ;
        rdfs:subClassOf   seas:Evaluation ;
        vs:term_status    "testing" .

foaf:name  a    owl:DatatypeProperty .

vs:term_status  a  owl:AnnotationProperty .

seas:PercentileEvaluation
        a                 owl:Class ;
        rdfs:comment      "The evaluated value is one of the percentiles of the property value distribution. The rank of the percentile is the object of property `seas:rank`."@en ;
        rdfs:isDefinedBy  seas:StatisticsOntology ;
        rdfs:label        "Percentile Evaluation"@en ;
        rdfs:subClassOf   seas:RankedDistributionEvaluation ;
        vs:term_status    "testing" .

seas:QuartileEvaluation
        a                 owl:Class ;
        rdfs:comment      "The evaluated value is one of the quartiles of the property value distribution. The rank of the quartile is the object of property `seas:rank`."@en ;
        rdfs:isDefinedBy  seas:StatisticsOntology ;
        rdfs:label        "Quartile Evaluation"@en ;
        rdfs:subClassOf   seas:RankedDistributionEvaluation ;
        vs:term_status    "testing" .

seas:StatisticsOntology
        a                              owl:Ontology , voaf:Vocabulary ;
        cc:license                     <https://www.apache.org/licenses/LICENSE-2.0> ;
        dcterms:creator                <http://www.maxime-lefrancois.info/me#> ;
        dcterms:description            "This ontology defines common evaluation interpretation concepts for statistics."@en ;
        dcterms:issued                 "2016-07-21"^^xsd:date ;
        dcterms:modified               "2016-07-21"^^xsd:date ;
        dcterms:title                  "The SEAS Statistics ontology."@en ;
        vann:preferredNamespacePrefix  "seas" ;
        vann:preferredNamespaceUri     seas: ;
        owl:imports                    seas:EvaluationOntology ;
        owl:versionIRI                 seas:StatisticsOntology-1.0 ;
        owl:versionInfo                "v1.0" .

foaf:Person  a  owl:Class .

seas:DecileEvaluation
        a                 owl:Class ;
        rdfs:comment      "The evaluated value is one of the deciles of the property value distribution. The rank of the decile is the object of property `seas:rank`."@en ;
        rdfs:isDefinedBy  seas:StatisticsOntology ;
        rdfs:label        "Decile Evaluation"@en ;
        rdfs:subClassOf   seas:RankedDistributionEvaluation ;
        vs:term_status    "testing" .

seas:DistributionMedianEvaluation
        a                 owl:Class ;
        rdfs:comment      "The evaluated value is the median of the property value distribution."@en ;
        rdfs:isDefinedBy  seas:StatisticsOntology ;
        rdfs:label        "Distribution Median Evaluation"@en ;
        rdfs:subClassOf   seas:Evaluation ;
        vs:term_status    "testing" .

dcterms:title  a  owl:AnnotationProperty .

vann:preferredNamespaceUri
        a       owl:AnnotationProperty .

seas:StandardDeviationEvaluation
        a                 owl:Class ;
        rdfs:comment      "The evaluated value is the standard deviation of the property value distribution."@en ;
        rdfs:isDefinedBy  seas:StatisticsOntology ;
        rdfs:label        "Standard Deviation Evaluation"@en ;
        rdfs:subClassOf   seas:Evaluation ;
        vs:term_status    "testing" .

vann:preferredNamespacePrefix
        a       owl:AnnotationProperty .
