@prefix dc:    <http://purl.org/dc/elements/1.1/> .
@prefix rdfs:  <http://www.w3.org/2000/01/rdf-schema#> .
@prefix foaf:  <http://xmlns.com/foaf/0.1/> .
@prefix bibo:  <http://purl.org/ontology/bibo/> .
@prefix owl:   <http://www.w3.org/2002/07/owl#> .
@prefix xsd:   <http://www.w3.org/2001/XMLSchema#> .
@prefix rdf:   <http://www.w3.org/1999/02/22-rdf-syntax-ns#> .
@prefix vann:  <http://purl.org/vocab/vann/> .
@prefix cerif: <http://www.eurocris.org/ontologies/cerif/1.3#> .

cerif:CurriculumVitae
        a                 owl:Class , rdfs:Class ;
        rdfs:comment      "Curriculum Vitae" ;
        rdfs:isDefinedBy  <http://www.eurocris.org/ontologies/cerif/1.3> ;
        rdfs:label        "Curriculum Vitae" ;
        rdfs:subClassOf   cerif:SecondLevelEntity .

cerif:acronym  a          rdf:Property ;
        rdfs:comment      "Acronym of a given Project or an Organisation Unit" ;
        rdfs:domain       cerif:OrganizationalUnit , cerif:Project ;
        rdfs:isDefinedBy  <http://www.eurocris.org/ontologies/cerif/1.3> ;
        rdfs:label        "Acronym" .

cerif:ruizrube  a  foaf:Person ;
        foaf:name  "Iv√°n Ruiz Rube" .

cerif:money  a            owl:DatatypeProperty , rdf:Property ;
        rdfs:comment      "This property embraces all Currency-dependent properties " ;
        rdfs:isDefinedBy  <http://www.eurocris.org/ontologies/cerif/1.3> ;
        rdfs:label        "Money" ;
        rdfs:range        xsd:float .

cerif:headcount  a        rdf:Property ;
        rdfs:comment      "Number of persons enrolled in a Organisation Unit" ;
        rdfs:domain       cerif:OrganizationalUnit ;
        rdfs:isDefinedBy  <http://www.eurocris.org/ontologies/cerif/1.3> ;
        rdfs:label        "Headcount" .

cerif:link  a             rdf:Property ;
        rdfs:comment      "It is a generalisation for relationship and classification properties" ;
        rdfs:isDefinedBy  <http://www.eurocris.org/ontologies/cerif/1.3> ;
        rdfs:label        "Link" .

cerif:registrationDate
        a                   rdf:Property ;
        rdfs:comment        "Registration Date of a patent" ;
        rdfs:domain         cerif:Patent ;
        rdfs:isDefinedBy    <http://www.eurocris.org/ontologies/cerif/1.3> ;
        rdfs:label          "Registration Date" ;
        rdfs:subPropertyOf  dc:date .

cerif:Person  a           owl:Class , rdfs:Class ;
        rdfs:comment      "A given person" ;
        rdfs:isDefinedBy  <http://www.eurocris.org/ontologies/cerif/1.3> ;
        rdfs:label        "Person (cfPers)" ;
        rdfs:subClassOf   foaf:Person , cerif:BaseEntity .

cerif:linksToOrganisationUnit
        a                   rdf:Property ;
        rdfs:comment        "It relates a entity with a given Organisation Unit through a time-stamped link." ;
        rdfs:isDefinedBy    <http://www.eurocris.org/ontologies/cerif/1.3> ;
        rdfs:label          "Links To a Organisation Unit" ;
        rdfs:subPropertyOf  cerif:linksToEntity .

cerif:productNumber  a      rdf:Property ;
        rdfs:comment        "Number of a Product" ;
        rdfs:isDefinedBy    <http://www.eurocris.org/ontologies/cerif/1.3> ;
        rdfs:label          "Product Number" ;
        rdfs:subPropertyOf  dc:identifier .

cerif:priceCurrencyCode
        a                   rdf:Property ;
        rdfs:isDefinedBy    <http://www.eurocris.org/ontologies/cerif/1.3> ;
        rdfs:label          "Price Currency Code" ;
        rdfs:subPropertyOf  cerif:currencyCode .

cerif:role  a               rdf:Property ;
        rdfs:comment        "Indicates a role for the association or composition between two CERIF entities indicated by a term from a suitable external vocabulary" ;
        rdfs:domain         cerif:Relationship ;
        rdfs:isDefinedBy    <http://www.eurocris.org/ontologies/cerif/1.3> ;
        rdfs:label          "Role" ;
        rdfs:range          rdfs:Resource ;
        rdfs:subPropertyOf  cerif:link .

cerif:fraction  a         owl:DatatypeProperty , rdf:Property ;
        rdfs:comment      "Fractional value to indicate a classification reference or a % allocation in the relationship between entities." ;
        rdfs:isDefinedBy  <http://www.eurocris.org/ontologies/cerif/1.3> ;
        rdfs:label        "Fraction" ;
        rdfs:range        xsd:float .

cerif:ElectronicAddress
        a                 owl:Class , rdfs:Class ;
        rdfs:comment      "ElectronicAddress" ;
        rdfs:isDefinedBy  <http://www.eurocris.org/ontologies/cerif/1.3> ;
        rdfs:label        "Electronic Address" ;
        rdfs:subClassOf   cerif:SecondLevelEntity .

cerif:code  a             rdf:Property ;
        rdfs:comment      "Generic property for represent international and shared codes" ;
        rdfs:isDefinedBy  <http://www.eurocris.org/ontologies/cerif/1.3> ;
        rdfs:label        "Code" .

cerif:PostalAddress  a    owl:Class , rdfs:Class ;
        rdfs:comment      "Postal Address" ;
        rdfs:isDefinedBy  <http://www.eurocris.org/ontologies/cerif/1.3> ;
        rdfs:label        "Postal Address" ;
        rdfs:subClassOf   cerif:SecondLevelEntity .

cerif:abstract  a         rdf:Property ;
        rdfs:comment      "Abstract of a given Project" ;
        rdfs:domain       cerif:Project ;
        rdfs:isDefinedBy  <http://www.eurocris.org/ontologies/cerif/1.3> ;
        rdfs:label        "Abstract" .

cerif:Qualification  a    owl:Class , rdfs:Class ;
        rdfs:comment      "Qualification" ;
        rdfs:isDefinedBy  <http://www.eurocris.org/ontologies/cerif/1.3> ;
        rdfs:label        "Qualification" ;
        rdfs:subClassOf   cerif:SecondLevelEntity .

cerif:OrganizationalUnit
        a                 owl:Class , rdfs:Class ;
        rdfs:comment      "A given organizational unit" ;
        rdfs:isDefinedBy  <http://www.eurocris.org/ontologies/cerif/1.3> ;
        rdfs:label        "Organizational Unit (cfOrgUnit)" ;
        rdfs:subClassOf   cerif:BaseEntity , foaf:Organization .

cerif:ResultEntity  a     owl:Class , rdfs:Class ;
        rdfs:comment      "Represents a research result" ;
        rdfs:isDefinedBy  <http://www.eurocris.org/ontologies/cerif/1.3> ;
        rdfs:label        "Result Entity" .

cerif:geert  a     foaf:Person ;
        foaf:name  "Geert van Grootel" .

cerif:Entity  a           owl:Class , rdfs:Class ;
        rdfs:comment      "Common superclass of all non-link entities, as an aid in querying." ;
        rdfs:isDefinedBy  <http://www.eurocris.org/ontologies/cerif/1.3> ;
        rdfs:label        "Entity" .

cerif:Classification  a   owl:Class , rdfs:Class ;
        rdfs:comment      "Represents the classification of a given entity" ;
        rdfs:isDefinedBy  <http://www.eurocris.org/ontologies/cerif/1.3> ;
        rdfs:label        "Classification" .

cerif:isLinkedByPerson
        a                   rdf:Property ;
        rdfs:comment        "A given Person is related with a entity through a time-stamped link. " ;
        rdfs:isDefinedBy    <http://www.eurocris.org/ontologies/cerif/1.3> ;
        rdfs:label          "Is Linked By a Person" ;
        rdfs:subPropertyOf  cerif:isLinkedByEntity .

cerif:isLinkedByOrganisationUnit
        a                   rdf:Property ;
        rdfs:comment        "A given Organisation Unit is related with a entity through a time-stamped link." ;
        rdfs:isDefinedBy    <http://www.eurocris.org/ontologies/cerif/1.3> ;
        rdfs:label          "Is Linked By a Organisation Unit" ;
        rdfs:subPropertyOf  cerif:isLinkedByEntity .

cerif:Equipment  a        owl:Class , rdfs:Class ;
        rdfs:comment      "Equipment" ;
        rdfs:isDefinedBy  <http://www.eurocris.org/ontologies/cerif/1.3> ;
        rdfs:label        "Equipment" ;
        rdfs:subClassOf   cerif:InfrastructureEntity .

cerif:linksToFunding  a     rdf:Property ;
        rdfs:comment        "It relates a entity with a given Funding entity through a time-stamped link." ;
        rdfs:isDefinedBy    <http://www.eurocris.org/ontologies/cerif/1.3> ;
        rdfs:label          "Links to Funding" ;
        rdfs:subPropertyOf  cerif:linksToEntity .

cerif:price  a              rdf:Property ;
        rdfs:comment        "Quantity of payment or compensation given by one party to another in return for goods or service (measured in a specific currency)" ;
        rdfs:isDefinedBy    <http://www.eurocris.org/ontologies/cerif/1.3> ;
        rdfs:label          "Price" ;
        rdfs:subPropertyOf  cerif:money .

cerif:funding  a            rdf:Property ;
        rdfs:comment        "Amount of a given Funding (measured in a specific currency)" ;
        rdfs:domain         cerif:Funding ;
        rdfs:isDefinedBy    <http://www.eurocris.org/ontologies/cerif/1.3> ;
        rdfs:label          "Funding" ;
        rdfs:subPropertyOf  cerif:money .

cerif:feeOrFree  a        rdf:Property ;
        rdfs:comment      "Flag indicating if the event is fee or free" ;
        rdfs:domain       cerif:Event ;
        rdfs:isDefinedBy  <http://www.eurocris.org/ontologies/cerif/1.3> ;
        rdfs:label        "Fee Or Free" .

cerif:Project  a          owl:Class , rdfs:Class ;
        rdfs:comment      "A research project" ;
        rdfs:isDefinedBy  <http://www.eurocris.org/ontologies/cerif/1.3> ;
        rdfs:label        "Project" ;
        rdfs:subClassOf   cerif:BaseEntity , foaf:Project .

cerif:birthdate  a          rdf:Property ;
        rdfs:comment        "BirthDate of a Person" ;
        rdfs:domain         cerif:Person ;
        rdfs:isDefinedBy    <http://www.eurocris.org/ontologies/cerif/1.3> ;
        rdfs:label          "Birthdate" ;
        rdfs:subPropertyOf  foaf:birthday .

cerif:manufacturerIdentifier
        a                   rdf:Property ;
        rdfs:comment        "The equipment manufacturer's ID." ;
        rdfs:domain         cerif:Equipment ;
        rdfs:isDefinedBy    <http://www.eurocris.org/ontologies/cerif/1.3> ;
        rdfs:label          "Manufacturer Identifier" ;
        rdfs:subPropertyOf  dc:identifier .

cerif:agrovoc  a            rdf:Property ;
        rdfs:comment        "External Classification Scheme according to Agrovoc Vocabulary" ;
        rdfs:isDefinedBy    <http://www.eurocris.org/ontologies/cerif/1.3> ;
        rdfs:label          "Agrovoc Classification" ;
        rdfs:subPropertyOf  dc:subject .

cerif:keith  a     foaf:Person ;
        foaf:name  "Keith G Jeffery" .

cerif:turnoverCurrencyCode
        a                   rdf:Property ;
        rdfs:comment        "Currency Code used to denote turnovers" ;
        rdfs:isDefinedBy    <http://www.eurocris.org/ontologies/cerif/1.3> ;
        rdfs:label          "Turnover Currency Code" ;
        rdfs:subPropertyOf  cerif:currencyCode .

cerif:isLinkedByEntity
        a                 rdf:Property ;
        rdfs:comment      "This is an abstract property to group all properties that inversely relate a entity with other through a time-stamped link." ;
        rdfs:domain       cerif:InfrastructureEntity , cerif:SecondLevelEntity , cerif:BaseEntity , cerif:ResultEntity ;
        rdfs:isDefinedBy  <http://www.eurocris.org/ontologies/cerif/1.3> ;
        rdfs:label        "Is Linked by Entity" ;
        rdfs:range        cerif:Relationship .

cerif:SecondLevelEntity
        a                 owl:Class , rdfs:Class ;
        rdfs:comment      "The 2nd level entities allow for the representation of the research context by linking to them from the base and result entities." ;
        rdfs:isDefinedBy  <http://www.eurocris.org/ontologies/cerif/1.3> ;
        rdfs:label        "Second-level Entity" ;
        rdfs:subClassOf   cerif:Entity .

cerif:currency  a         rdf:Property ;
        rdfs:comment      "Specific currency used for denote amounts, prices and turnovers. Linking with http://dbpedia.org/ontology/Language" ;
        rdfs:isDefinedBy  <http://www.eurocris.org/ontologies/cerif/1.3> ;
        rdfs:label        "Currency" .

cerif:Product  a          owl:Class , rdfs:Class ;
        rdfs:comment      "A research result that is classified neither as a patent nor as a publication." ;
        rdfs:isDefinedBy  <http://www.eurocris.org/ontologies/cerif/1.3> ;
        rdfs:label        "Product" ;
        rdfs:subClassOf   cerif:ResultEntity .

cerif:endDate  a            rdf:Property ;
        rdfs:comment        "End of a period of time" ;
        rdfs:domain         cerif:Project , cerif:ResultEntity , cerif:Relationship , cerif:Funding , cerif:Event ;
        rdfs:isDefinedBy    <http://www.eurocris.org/ontologies/cerif/1.3> ;
        rdfs:label          "End Date" ;
        rdfs:subPropertyOf  dc:date .

cerif:Cite  a             owl:Class , rdfs:Class ;
        rdfs:comment      "Cite" ;
        rdfs:isDefinedBy  <http://www.eurocris.org/ontologies/cerif/1.3> ;
        rdfs:label        "Cite" ;
        rdfs:subClassOf   cerif:SecondLevelEntity .

cerif:isLinkedByProject
        a                   rdf:Property ;
        rdfs:comment        "A given Project is related with a entity through a time-stamped link." ;
        rdfs:isDefinedBy    <http://www.eurocris.org/ontologies/cerif/1.3> ;
        rdfs:label          "is Linked By Project" ;
        rdfs:subPropertyOf  cerif:isLinkedByEntity .

cerif:Publication  a      owl:Class , rdfs:Class ;
        rdfs:comment      "Represents a scientific or academic publication " ;
        rdfs:isDefinedBy  <http://www.eurocris.org/ontologies/cerif/1.3> ;
        rdfs:label        "Publication" ;
        rdfs:subClassOf   bibo:Document , cerif:ResultEntity .

cerif:uri  a                rdf:Property ;
        rdfs:comment        "Uniform Resource Identifier related with a given CERIF entity" ;
        rdfs:domain         cerif:ResultEntity , cerif:SecondLevelEntity , cerif:BaseEntity ;
        rdfs:isDefinedBy    <http://www.eurocris.org/ontologies/cerif/1.3> ;
        rdfs:label          "URI" ;
        rdfs:subPropertyOf  foaf:homepage .

cerif:currencyCode  a       rdf:Property ;
        rdfs:comment        "Code of a specific currency used for denote amounts, prices and turnovers." ;
        rdfs:isDefinedBy    <http://www.eurocris.org/ontologies/cerif/1.3> ;
        rdfs:label          "Currency Code" ;
        rdfs:subPropertyOf  cerif:code .

cerif:Event  a            owl:Class , rdfs:Class ;
        rdfs:comment      "Event" ;
        rdfs:isDefinedBy  <http://www.eurocris.org/ontologies/cerif/1.3> ;
        rdfs:label        "Event" ;
        rdfs:subClassOf   cerif:SecondLevelEntity .

cerif:patentNumber  a       rdf:Property ;
        rdfs:comment        "Number of a Registered Patent" ;
        rdfs:isDefinedBy    <http://www.eurocris.org/ontologies/cerif/1.3> ;
        rdfs:label          "Patent Number" ;
        rdfs:subPropertyOf  dc:identifier .

cerif:countryCode  a        rdf:Property ;
        rdfs:comment        "International code of a given country " ;
        rdfs:domain         cerif:PostalAddress , cerif:Event , cerif:Patent ;
        rdfs:isDefinedBy    <http://www.eurocris.org/ontologies/cerif/1.3> ;
        rdfs:label          "Country Code" ;
        rdfs:subPropertyOf  cerif:code .

cerif:BaseEntity  a       owl:Class , rdfs:Class ;
        rdfs:comment      "This abstract class brings together the main entities of the CERIF model." ;
        rdfs:isDefinedBy  <http://www.eurocris.org/ontologies/cerif/1.3> ;
        rdfs:label        "Base Entity" ;
        rdfs:subClassOf   cerif:Entity .

cerif:digitalCV  a        rdf:Property ;
        rdfs:comment      "Digital CV" ;
        rdfs:domain       cerif:CurriculumVitae ;
        rdfs:isDefinedBy  <http://www.eurocris.org/ontologies/cerif/1.3> ;
        rdfs:label        "Digital CV" .

cerif:gender  a             rdf:Property ;
        rdfs:comment        "Gender of a CERIF person" ;
        rdfs:domain         cerif:Person ;
        rdfs:isDefinedBy    <http://www.eurocris.org/ontologies/cerif/1.3> ;
        rdfs:label          "Gender" ;
        rdfs:subPropertyOf  foaf:gender .

cerif:linksToPublication
        a                   rdf:Property ;
        rdfs:comment        "It relates a entity with a given Publication through a time-stamped link." ;
        rdfs:isDefinedBy    <http://www.eurocris.org/ontologies/cerif/1.3> ;
        rdfs:label          "Links To a Publication" ;
        rdfs:subPropertyOf  cerif:linksToEntity .

cerif:country  a          rdf:Property ;
        rdfs:comment      "A given country - http://dbpedia.org/ontology/Country" ;
        rdfs:isDefinedBy  <http://www.eurocris.org/ontologies/cerif/1.3> ;
        rdfs:label        "Country " .

cerif:brigitte  a  foaf:Person ;
        foaf:name  "Brigitte Joerg" .

cerif:linksToPerson  a      rdf:Property ;
        rdfs:comment        "It relates a entity with a given Person through a time-stamped link." ;
        rdfs:isDefinedBy    <http://www.eurocris.org/ontologies/cerif/1.3> ;
        rdfs:label          "Is Linked By a Person" ;
        rdfs:subPropertyOf  cerif:linksToEntity .

cerif:startDate  a          rdf:Property ;
        rdfs:comment        "Beginning of a period of time" ;
        rdfs:domain         cerif:Event , cerif:Funding , cerif:Project , cerif:Relationship , cerif:Classification ;
        rdfs:isDefinedBy    <http://www.eurocris.org/ontologies/cerif/1.3> ;
        rdfs:label          "Start Date" ;
        rdfs:subPropertyOf  dc:date .

cerif:PriceAward  a       owl:Class , rdfs:Class ;
        rdfs:comment      "Price Award" ;
        rdfs:isDefinedBy  <http://www.eurocris.org/ontologies/cerif/1.3> ;
        rdfs:label        "Price Award" ;
        rdfs:subClassOf   cerif:SecondLevelEntity .

cerif:name  a               rdf:Property ;
        rdfs:comment        "Name of a CERIF entity, e.g.: Person, or Organization Unit" ;
        rdfs:domain         cerif:Project , cerif:Person ;
        rdfs:isDefinedBy    <http://www.eurocris.org/ontologies/cerif/1.3> ;
        rdfs:label          "Name" ;
        rdfs:subPropertyOf  foaf:name .

<http://www.eurocris.org/ontologies/cerif/1.3>
        a                              owl:Ontology ;
        dc:creator                     cerif:msicilia , cerif:keith , cerif:jan , cerif:brigitte , cerif:ruizrube , cerif:geert ;
        dc:description                 "The <em>Common European Research Information Format (CERIF) Ontology Specification</em> provides basic concepts and properties for describing research information as semantic data. This document contains a friendly description of the <em>Common European Research Information Format (CERIF) Ontology</em> developed by EuroCRIS." ;
        dc:modified                    "2015-03-26"^^xsd:date ;
        dc:title                       "CERIF Ontology 1.3" ;
        vann:preferredNamespacePrefix  "cerif" ;
        vann:preferredNamespaceUri     "http://www.eurocris.org/ontologies/cerif/1.3#" ;
        foaf:page                      <http://www.eurocris.org/ontologies/cerif/1.3.html> .

cerif:jan  a       foaf:Person ;
        foaf:name  "Jan Dvorak" .

cerif:approvalDate  a       rdf:Property ;
        rdfs:comment        "Approval Date of a patent" ;
        rdfs:domain         cerif:Patent ;
        rdfs:isDefinedBy    <http://www.eurocris.org/ontologies/cerif/1.3> ;
        rdfs:label          "Approval Date" ;
        rdfs:subPropertyOf  dc:date .

cerif:Relationship  a     owl:Class , rdfs:Class ;
        rdfs:comment      "intermediate entity between two entities." ;
        rdfs:isDefinedBy  <http://www.eurocris.org/ontologies/cerif/1.3> ;
        rdfs:label        "Relationship" .

cerif:Metrics  a          owl:Class , rdfs:Class ;
        rdfs:comment      "Metrics" ;
        rdfs:isDefinedBy  <http://www.eurocris.org/ontologies/cerif/1.3> ;
        rdfs:label        "Metrics" ;
        rdfs:subClassOf   cerif:SecondLevelEntity .

cerif:addressLine  a      rdf:Property ;
        rdfs:comment      "Numbered line of a given postal address" ;
        rdfs:domain       cerif:PostalAddress ;
        rdfs:isDefinedBy  <http://www.eurocris.org/ontologies/cerif/1.3> ;
        rdfs:label        "Address Line" .

cerif:language  a         rdf:Property ;
        rdfs:comment      "A given language. Linking to http://dbpedia.org/ontology/Language" ;
        rdfs:isDefinedBy  <http://www.eurocris.org/ontologies/cerif/1.3> ;
        rdfs:label        "Language" .

cerif:Patent  a           owl:Class , rdfs:Class ;
        rdfs:comment      "A registered patent as a research result" ;
        rdfs:isDefinedBy  <http://www.eurocris.org/ontologies/cerif/1.3> ;
        rdfs:label        "Patent" ;
        rdfs:subClassOf   bibo:Patent , cerif:ResultEntity .

cerif:cityTown  a         rdf:Property ;
        rdfs:comment      "City Town of an physical localisation" ;
        rdfs:domain       cerif:PostalAddress , cerif:Event ;
        rdfs:isDefinedBy  <http://www.eurocris.org/ontologies/cerif/1.3> ;
        rdfs:label        "City Town" .

cerif:researchInterests
        a                 rdf:Property ;
        rdfs:comment      "Research Interests" ;
        rdfs:domain       cerif:Person ;
        rdfs:isDefinedBy  <http://www.eurocris.org/ontologies/cerif/1.3> ;
        rdfs:label        "Research Interests" .

cerif:Funding  a          owl:Class , rdfs:Class ;
        rdfs:comment      "Funding" ;
        rdfs:isDefinedBy  <http://www.eurocris.org/ontologies/cerif/1.3> ;
        rdfs:label        "Funding" ;
        rdfs:subClassOf   cerif:SecondLevelEntity .

cerif:linksToPostalAddress
        a                   rdf:Property ;
        rdfs:comment        "It relates a entity with a given Postal Address through a time-stamped link. Used, for example, in Persons and Organisation Units" ;
        rdfs:isDefinedBy    <http://www.eurocris.org/ontologies/cerif/1.3> ;
        rdfs:label          "Links to a Postal Address" ;
        rdfs:subPropertyOf  cerif:linksToEntity .

cerif:inventoryIdentifier
        a                   rdf:Property ;
        rdfs:comment        "The equipment owner's inventory identifier." ;
        rdfs:domain         cerif:Equipment ;
        rdfs:isDefinedBy    <http://www.eurocris.org/ontologies/cerif/1.3> ;
        rdfs:label          "Inventory Identifier" ;
        rdfs:subPropertyOf  dc:identifier .

cerif:isClassifiedBy  a   rdf:Property ;
        rdfs:comment      "A entity is classified within a time interval according to CERIF Semantic Vocabulary." ;
        rdfs:domain       cerif:InfrastructureEntity , cerif:ResultEntity , cerif:SecondLevelEntity , cerif:BaseEntity ;
        rdfs:isDefinedBy  <http://www.eurocris.org/ontologies/cerif/1.3> ;
        rdfs:label        "Is Classified By" ;
        rdfs:range        cerif:Classification .

cerif:ExpSkill  a         owl:Class , rdfs:Class ;
        rdfs:comment      "Expertise and skills" ;
        rdfs:isDefinedBy  <http://www.eurocris.org/ontologies/cerif/1.3> ;
        rdfs:label        "Expertise and skills" ;
        rdfs:subClassOf   cerif:SecondLevelEntity .

cerif:turnover  a           rdf:Property ;
        rdfs:comment        "Turnover of a Organisation Unit (measured in a specific currency)" ;
        rdfs:domain         cerif:OrganizationalUnit ;
        rdfs:isDefinedBy    <http://www.eurocris.org/ontologies/cerif/1.3> ;
        rdfs:label          "Turnover" ;
        rdfs:subPropertyOf  cerif:money .

cerif:InfrastructureEntity
        a                 owl:Class , rdfs:Class ;
        rdfs:comment      "Abstract entity for representing infrastructures" ;
        rdfs:isDefinedBy  <http://www.eurocris.org/ontologies/cerif/1.3> ;
        rdfs:label        "Infrastructure Entity" ;
        rdfs:subClassOf   cerif:Entity .

cerif:linksToEntity  a    rdf:Property ;
        rdfs:comment      "This is an abstract property to group all properties that directly relate a entity with other through a time-stamped link." ;
        rdfs:domain       cerif:InfrastructureEntity , cerif:SecondLevelEntity , cerif:ResultEntity , cerif:BaseEntity ;
        rdfs:isDefinedBy  <http://www.eurocris.org/ontologies/cerif/1.3> ;
        rdfs:label        "Links to Entity" ;
        rdfs:range        cerif:Relationship .

cerif:msicilia  a  foaf:Person ;
        foaf:name  "Miguel √Ångel Sicilia" .

cerif:keyword  a            rdf:Property ;
        rdfs:comment        "Keywords of a given entity" ;
        rdfs:domain         cerif:SecondLevelEntity , cerif:BaseEntity , cerif:ResultEntity ;
        rdfs:isDefinedBy    <http://www.eurocris.org/ontologies/cerif/1.3> ;
        rdfs:label          "Keyword" ;
        rdfs:subPropertyOf  dc:subject .

cerif:internalIdentifier
        a                   rdf:Property ;
        rdfs:comment        "Internal Identifier for a research entity. It fits with the primary key in the corresponding table from the internal database" ;
        rdfs:domain         cerif:SecondLevelEntity , cerif:BaseEntity , cerif:ResultEntity ;
        rdfs:isDefinedBy    <http://www.eurocris.org/ontologies/cerif/1.3> ;
        rdfs:label          "Internal Identifier" ;
        rdfs:subPropertyOf  dc:identifier .

cerif:Facility  a         owl:Class , rdfs:Class ;
        rdfs:comment      "Facility" ;
        rdfs:isDefinedBy  <http://www.eurocris.org/ontologies/cerif/1.3> ;
        rdfs:label        "Facility" ;
        rdfs:subClassOf   cerif:InfrastructureEntity .

cerif:postCode  a           rdf:Property ;
        rdfs:comment        "Postal Code of a given Address" ;
        rdfs:domain         cerif:PostalAddress ;
        rdfs:isDefinedBy    <http://www.eurocris.org/ontologies/cerif/1.3> ;
        rdfs:label          "Post Code" ;
        rdfs:subPropertyOf  cerif:code .

cerif:isLinkedByFunding
        a                   rdf:Property ;
        rdfs:comment        "A given Funding is related with a entity through a time-stamped link." ;
        rdfs:isDefinedBy    <http://www.eurocris.org/ontologies/cerif/1.3> ;
        rdfs:label          "Is Linked By Funding" ;
        rdfs:subPropertyOf  cerif:isLinkedByEntity .

cerif:languageCode  a       rdf:Property ;
        rdfs:comment        "International code of a given language" ;
        rdfs:isDefinedBy    <http://www.eurocris.org/ontologies/cerif/1.3> ;
        rdfs:label          "Language Code" ;
        rdfs:subPropertyOf  cerif:code .

cerif:classification  a     rdf:Property ;
        rdfs:comment        "Indicates a classification for a entity according to a suitable external vocabulary" ;
        rdfs:domain         cerif:Classification ;
        rdfs:isDefinedBy    <http://www.eurocris.org/ontologies/cerif/1.3> ;
        rdfs:label          "Classification" ;
        rdfs:range          rdfs:Resource ;
        rdfs:subPropertyOf  cerif:link .

cerif:Service  a          owl:Class , rdfs:Class ;
        rdfs:comment      "Service" ;
        rdfs:isDefinedBy  <http://www.eurocris.org/ontologies/cerif/1.3> ;
        rdfs:label        "Service" ;
        rdfs:subClassOf   cerif:InfrastructureEntity .

cerif:linksToProject  a     rdf:Property ;
        rdfs:comment        "It relates a  entity with a given Project through a time-stamped link." ;
        rdfs:isDefinedBy    <http://www.eurocris.org/ontologies/cerif/1.3> ;
        rdfs:label          "Links To a Project" ;
        rdfs:subPropertyOf  cerif:linksToEntity .

cerif:researchActivities
        a                 rdf:Property ;
        rdfs:comment      "Research Activities" ;
        rdfs:domain       cerif:OrganizationalUnit ;
        rdfs:isDefinedBy  <http://www.eurocris.org/ontologies/cerif/1.3> ;
        rdfs:label        "Research Activities" .

cerif:title  a              rdf:Property ;
        rdfs:comment        "Title of a given CERIF entity" ;
        rdfs:isDefinedBy    <http://www.eurocris.org/ontologies/cerif/1.3> ;
        rdfs:label          "Title" ;
        rdfs:subPropertyOf  dc:title .

cerif:fundingCurrencyCode
        a                   rdf:Property ;
        rdfs:comment        "Currency code used to denote the funding amount" ;
        rdfs:isDefinedBy    <http://www.eurocris.org/ontologies/cerif/1.3> ;
        rdfs:label          "Funding Currency Code" ;
        rdfs:subPropertyOf  cerif:currencyCode .

cerif:isLinkedByPublication
        a                   rdf:Property ;
        rdfs:comment        "A given Publication is related with a entity through a time-stamped link." ;
        rdfs:isDefinedBy    <http://www.eurocris.org/ontologies/cerif/1.3> ;
        rdfs:label          "is Linked By Publication" ;
        rdfs:subPropertyOf  cerif:isLinkedByEntity .
