@prefix wine:  <http://www.w3.org/TR/2003/PR-owl-guide-20031209/wine#> .
@prefix fowl:  <http://www.w3.org/TR/2003/PR-owl-guide-20031209/food#> .
@prefix foaf:  <http://xmlns.com/foaf/0.1/> .
@prefix status: <http://www.w3.org/2003/06/sw-vocab-status/ns#> .
@prefix yago:  <http://dbpedia.org/class/yago/> .
@prefix vann:  <http://purl.org/vocab/vann/> .
@prefix dcterms: <http://purl.org/dc/terms/> .
@prefix adms:  <http://www.w3.org/ns/adms#> .
@prefix rdfs:  <http://www.w3.org/2000/01/rdf-schema#> .
@prefix time:  <http://www.w3.org/2006/time#> .
@prefix beverage: <http://rdfs.co/bevon/beverage/> .
@prefix food:  <http://data.lirmm.fr/ontologies/food#> .
@prefix container: <http://rdfs.co/bevon/container/> .
@prefix owl:   <http://www.w3.org/2002/07/owl#> .
@prefix dbpedia: <http://dbpedia.org/ontology/> .
@prefix xsd:   <http://www.w3.org/2001/XMLSchema#> .
@prefix rdf:   <http://www.w3.org/1999/02/22-rdf-syntax-ns#> .
@prefix whisky: <http://purl.org/vocab/whisky/terms/> .
@prefix pto:   <http://www.productontology.org/id/> .
@prefix bevon: <http://rdfs.co/bevon/> .
@prefix gr:    <http://purl.org/goodrelations/v1#> .
@prefix skos:  <http://www.w3.org/2004/02/skos/core#> .
@prefix cc:    <http://creativecommons.org/ns#> .

bevon:GlassBottle  a        owl:Class ;
        rdfs:comment        "\n    Glass bottles can vary in size considerably, but are most commonly found in\n    sizes ranging between about 10ml and 5 litres.\n    "@en ;
        rdfs:isDefinedBy    bevon: ;
        rdfs:seeAlso        <http://en.wikipedia.org/wiki/Glass_bottle> ;
        rdfs:subClassOf     bevon:Container ;
        dcterms:issued      "2013-07-04+09:00"^^xsd:date ;
        dcterms:modified    "2014-03-01+09:00"^^xsd:date ;
        status:term_status  "unstable"@en ;
        skos:definition     "\n    A glass bottle is a bottle created from glass.\n    "@en ;
        skos:prefLabel      "Glass Bottle"@en , "유리병"@ko .

container:30lBeerKeg  a  bevon:BeerKeg , owl:NamedIndividual ;
        bevon:volume    [ a                        gr:QuantitativeValueInteger ;
                          gr:hasUnitOfMeasurement  "LTR" ;
                          gr:hasValue              "30"^^xsd:int
                        ] ;
        skos:prefLabel  "30l 맥주 케그"@ko , "30l Beer Keg"@en .

bevon:SingleMaltScotch
        a                   owl:Class ;
        rdfs:comment        "\n    As with any Scotch whisky, a single malt Scotch must be distilled in\n    Scotland and matured in oak casks in Scotland for at least three years\n    (most single malts are matured longer).\n    "@en ;
        rdfs:isDefinedBy    bevon: ;
        rdfs:seeAlso        <http://en.wikipedia.org/wiki/Single_malt_Scotch> ;
        rdfs:subClassOf     bevon:ScotchWhisky , pto:Single_malt_Scotch , bevon:SingleMaltWhisky ;
        dcterms:issued      "2013-07-04+09:00"^^xsd:date ;
        dcterms:modified    "2014-03-01+09:00"^^xsd:date ;
        status:term_status  "unstable"@en ;
        skos:definition     "\n    Single Malt Scotch is single malt whisky made in Scotland using a pot still\n    distillation process at a single distillery, with malted barley as the only\n    grain ingredient.\n    "@en ;
        skos:prefLabel      "Single Malt Scotch"@en , "싱글 몰트 스카치"@ko .

bevon:DryStout  a           owl:Class ;
        rdfs:isDefinedBy    bevon: ;
        rdfs:subClassOf     bevon:Stout ;
        dcterms:issued      "2013-07-04+09:00"^^xsd:date ;
        dcterms:modified    "2014-03-01+09:00"^^xsd:date ;
        status:term_status  "unstable"@en ;
        skos:altLabel       "Irish Stout"@en ;
        skos:definition     "\n    Irish stout or dry stout is very dark or rich in color and it often has a\n    \"roasted\" or coffee-like taste.\n    "@en ;
        skos:prefLabel      "Dry Stout"@en , "드라이 스타우트"@ko .

bevon:Rum  a                owl:Class ;
        rdfs:comment        "\n    The distillate, a clear liquid, is then usually aged in\n    oak barrels.\n    "@en ;
        rdfs:isDefinedBy    bevon: ;
        rdfs:seeAlso        <http://en.wikipedia.org/wiki/Rum> ;
        rdfs:subClassOf     bevon:DistilledBeverage , pto:Rum ;
        dcterms:issued      "2013-07-04+09:00"^^xsd:date ;
        dcterms:modified    "2014-03-01+09:00"^^xsd:date ;
        status:term_status  "testing"@en ;
        skos:definition     "\n    Rum is a distilled alcoholic beverage made from sugarcane byproducts, such\n    as molasses, or directly from sugarcane juice, by a process of fermentation\n    and distillation.\n    "@en ;
        skos:prefLabel      "Ron"@es , "Rum"@en , "럼"@ko .

bevon:quantity  a           owl:ObjectProperty ;
        rdfs:domain         food:Ingredient ;
        rdfs:isDefinedBy    bevon: ;
        rdfs:range          gr:QuantitativeValue ;
        dcterms:issued      "2013-07-04+09:00"^^xsd:date ;
        dcterms:modified    "2014-03-01+09:00"^^xsd:date ;
        status:term_status  "unstable"@en ;
        skos:definition     "\n    This property specifies the quantity of the ingredient with a type\n    in the UN/CEFACT Common Code.\n    "@en ;
        skos:prefLabel      "quantity"@en , "양"@ko .

bevon:Water  a              owl:Class ;
        rdfs:isDefinedBy    bevon: ;
        rdfs:seeAlso        <http://en.wikipedia.org/wiki/Water> ;
        rdfs:subClassOf     bevon:NonAlcoholicBeverage , pto:Water ;
        dcterms:issued      "2013-07-04+09:00"^^xsd:date ;
        dcterms:modified    "2014-03-01+09:00"^^xsd:date ;
        status:term_status  "testing"@en ;
        skos:definition     "\n    In the Beverage Ontology, Water means a drinking water.\n    "@en ;
        skos:prefLabel      "물"@ko , "Water"@en .

bevon:variantOf  a          owl:ObjectProperty ;
        rdfs:domain         bevon:Beverage ;
        rdfs:isDefinedBy    bevon: ;
        rdfs:range          bevon:Beverage ;
        rdfs:subPropertyOf  dbpedia:variantOf , bevon:related , gr:isVariantOf ;
        dcterms:issued      "2013-07-04+09:00"^^xsd:date ;
        dcterms:modified    "2014-03-01+09:00"^^xsd:date ;
        owl:inverseOf       bevon:variant ;
        status:term_status  "unstable"@en ;
        skos:definition     "\n    This property states that a beverage is a variant of another beverage.\n    "@en ;
        skos:prefLabel      "variant of"@en , "바탕"@ko .

bevon:proof  a              owl:DatatypeProperty ;
        rdfs:comment        "\n    The term was originally used in the United Kingdom and was defined as 7/4\n    times the alcohol by volume (ABV). The UK now uses the ABV standard instead\n    of alcohol proof. In the United States, alcoholic proof is defined as twice\n    the percentage of ABV.\n    "@en ;
        rdfs:domain         bevon:Beverage ;
        rdfs:isDefinedBy    bevon: ;
        rdfs:range          xsd:decimal ;
        rdfs:seeAlso        <http://en.wikipedia.org/wiki/Alcohol_proof> ;
        dcterms:issued      "2013-07-04+09:00"^^xsd:date ;
        dcterms:modified    "2014-03-01+09:00"^^xsd:date ;
        status:term_status  "unstable"@en ;
        skos:altLabel       "alcohol proof"@en ;
        skos:definition     "\n    Alcohol proof is a measure of how much alcohol (ethanol) is contained in an\n    alcoholic beverage.\n    "@en ;
        skos:prefLabel      "프루프"@ko , "proof"@en .

<http://jayg.me/>  a       foaf:Person ;
        foaf:homepage      <http://jayg.org/> ;
        foaf:mbox_sha1sum  "a637717b7e34b83694018e8fdd3ff334fffcd4f3" ;
        foaf:name          "김보람"@ko , "James G. Kim"@en .

container:330mlLongneck
        a               bevon:Longneck , owl:NamedIndividual ;
        bevon:volume    [ a                        gr:QuantitativeValueInteger ;
                          gr:hasUnitOfMeasurement  "MLT" ;
                          gr:hasValue              "330"^^xsd:int
                        ] ;
        skos:prefLabel  "330ml 긴목 맥주병"@ko , "330ml Longneck Bottle"@en .

bevon:AlcoholicBeverage
        a                   owl:Class ;
        rdfs:isDefinedBy    bevon: ;
        rdfs:seeAlso        <http://en.wikipedia.org/wiki/Alcoholic_beverage> ;
        rdfs:subClassOf     bevon:Beverage , pto:Alcoholic_beverage ;
        dcterms:issued      "2013-07-04+09:00"^^xsd:date ;
        dcterms:modified    "2014-03-01+09:00"^^xsd:date ;
        owl:disjointWith    bevon:NonAlcoholicBeverage ;
        status:term_status  "testing"@en ;
        skos:definition     "\n     An alcoholic beverage is a drink and psychoactive drug containing\n     ethyl alcohol which is commonly referred to as ethanol.\n     "@en ;
        skos:prefLabel      "알코올 음료"@ko , "Alcoholic Beverage"@en .

bevon:Dunkel  a             owl:Class ;
        rdfs:comment        "\n    Dunkel is the German word meaning dark, and dunkel beers typically range in\n    color from amber to dark reddish brown. They are characterized by their\n    smooth malty flavor.\n    "@en ;
        rdfs:isDefinedBy    bevon: ;
        rdfs:seeAlso        <https://en.wikipedia.org/wiki/Dunkel> ;
        rdfs:subClassOf     pto:Dunkel , bevon:Lager ;
        dcterms:issued      "2013-07-04+09:00"^^xsd:date ;
        dcterms:modified    "2014-03-01+09:00"^^xsd:date ;
        status:term_status  "unstable"@en ;
        skos:altLabel       "Dunkles"@en ;
        skos:definition     "\n    Dunkel, or Dunkles, is a word used for several types of dark German lager.\n    "@en ;
        skos:prefLabel      "둔켈"@ko , "Dunkel"@en .

bevon:previous_content
        a                   owl:ObjectProperty ;
        rdfs:domain         bevon:Aging ;
        rdfs:isDefinedBy    bevon: ;
        rdfs:range          fowl:PotableLiquid ;
        dcterms:issued      "2013-07-04+09:00"^^xsd:date ;
        dcterms:modified    "2014-03-01+09:00"^^xsd:date ;
        status:term_status  "unstable"@en ;
        skos:definition     "\n    This property specifies what as in the cask before the aging.\n    "@en ;
        skos:prefLabel      "이전 내용물"@ko , "previous content"@en .

bevon:Sake  a               owl:Class ;
        rdfs:isDefinedBy    bevon: ;
        rdfs:seeAlso        <http://en.wikipedia.org/wiki/Sake> ;
        rdfs:subClassOf     bevon:FermentedBeverage , pto:Sake ;
        dcterms:issued      "2013-07-04+09:00"^^xsd:date ;
        dcterms:modified    "2014-03-01+09:00"^^xsd:date ;
        status:term_status  "testing"@en ;
        skos:altLabel       "Rice Wine"@en ;
        skos:definition     "\n    Sake or saké is an alcoholic beverage of Japanese origin that is made from\n    fermented rice.\n    "@en ;
        skos:prefLabel      "사케"@ko , "Saké"@fr , "Sake"@en .

bevon:food  a               owl:ObjectProperty ;
        rdfs:domain         food:Ingredient ;
        rdfs:isDefinedBy    bevon: ;
        rdfs:range          food:Food ;
        rdfs:subPropertyOf  food:food ;
        dcterms:issued      "2013-07-04+09:00"^^xsd:date ;
        dcterms:modified    "2014-03-01+09:00"^^xsd:date ;
        status:term_status  "unstable"@en ;
        skos:definition     "\n    This property describes food that is an ingredient of a mixed drink.\n    "@en ;
        skos:prefLabel      "음식"@ko , "food"@en .

bevon:Beverage  a           owl:Class ;
        rdfs:isDefinedBy    bevon: ;
        rdfs:seeAlso        <http://en.wikipedia.org/wiki/Beverage> ;
        rdfs:subClassOf     fowl:PotableLiquid , pto:Drink , food:Food ;
        dcterms:issued      "2013-07-04+09:00"^^xsd:date ;
        dcterms:modified    "2014-03-01+09:00"^^xsd:date ;
        status:term_status  "testing"@en ;
        skos:altLabel       "Drink"@en ;
        skos:definition     "\n    A beverage, or drink, is a kind of liquid which is specifically prepared\n    for human consumption.\n    "@en ;
        skos:prefLabel      "음료"@ko , "Beverage"@en .

bevon:origin  a             owl:ObjectProperty ;
        rdfs:domain         bevon:Beverage ;
        rdfs:isDefinedBy    bevon: ;
        rdfs:range          dbpedia:Place ;
        dcterms:issued      "2013-07-04+09:00"^^xsd:date ;
        dcterms:modified    "2014-03-01+09:00"^^xsd:date ;
        status:term_status  "unstable"@en ;
        skos:definition     "\n    This property indicates the place where the beverage was first invented.\n    "@en ;
        skos:prefLabel      "origin"@en , "원산지"@ko .

wine:Wine  rdfs:subClassOf  bevon:Wine .

bevon:PaleLager  a          owl:Class ;
        rdfs:isDefinedBy    bevon: ;
        rdfs:seeAlso        <http://en.wikipedia.org/wiki/Pale_lager> ;
        rdfs:subClassOf     bevon:Lager , pto:Pale_lager ;
        dcterms:issued      "2013-07-04+09:00"^^xsd:date ;
        dcterms:modified    "2014-03-01+09:00"^^xsd:date ;
        status:term_status  "unstable"@en ;
        skos:definition     "\n    Pale lager is a very pale to golden-colored beer with a well attenuated\n    body and a varying degree of noble hop bitterness.\n    "@en ;
        skos:prefLabel      "페일 라거"@ko , "Pale Lager"@en .

beverage:Chamisul  a        gr:ProductOrServiceModel , bevon:DilutedSoju , owl:NamedIndividual ;
        rdfs:seeAlso        <http://ko.wikipedia.org/wiki/참이슬> ;
        bevon:abv           "19"^^xsd:decimal ;
        bevon:color         [ a              dbpedia:Colour ;
                              dcterms:title  "Clear"@en ;
                              owl:sameAs     <http://dbpedia.org/resource/Clear_(color)>
                            ] ;
        bevon:container     container:1_8lPlasticBottle , container:640mlPlasticBottle , container:200mlPlasticBottle , container:360mlGlassBottle ;
        bevon:description   "\n    Chamisul is the diluted soju produced by HITEJiro.\n    "@en ;
        bevon:launch        "1998"^^xsd:gYear ;
        bevon:manufacturer  <http://dbpedia.org/resource/Jinro> ;
        bevon:name          "Chamisul"@en , "참이슬"@ko ;
        bevon:origin        <http://dbpedia.org/resource/South_Korea> .

beverage:Kilkenny  a             bevon:IrishRedAle , gr:ProductOrServiceModel , owl:NamedIndividual ;
        rdfs:seeAlso             <http://en.wikipedia.org/wiki/Kilkenny_(beer)> ;
        bevon:abv                4.3 ;
        bevon:container          container:440mlBeverageCan , container:30lBeerKeg ;
        bevon:description        "\n    Kilkenny is a nitrogenated Irish cream ale from the makers of Guinness,\n    which originated in Kilkenny, Ireland. The brand is managed and produced\n    by Diageo. It is available in draught and cans. It is brewed in Ireland\n    and its heritage dates back to the 14th century.\n    "@en ;
        bevon:fermentation_base  <http://dbpedia.org/resource/Barley> ;
        bevon:ibu                "23"^^xsd:nonNegativeInteger ;
        bevon:launch             "1710"^^xsd:gYear ;
        bevon:manufacturer       <http://dbpedia.org/resource/Diageo> ;
        bevon:name               "킬케니 아이리쉬 크림 에일"@ko , "Kilkenny Irish Cream Ale"@en ;
        bevon:origin             <http://dbpedia.org/resource/Kilkenny> ;
        bevon:similar            beverage:Smithwicks ;
        bevon:srm                "14"^^xsd:nonNegativeInteger ;
        owl:sameAs               <http://dbpedia.org/resource/Kilkenny_(beer)> .

bevon:MaltWhisky  a         owl:Class ;
        rdfs:isDefinedBy    bevon: ;
        rdfs:seeAlso        <http://en.wikipedia.org/wiki/Malt_whisky> ;
        rdfs:subClassOf     bevon:Whisky , pto:Malt_whisky ;
        dcterms:issued      "2013-07-04+09:00"^^xsd:date ;
        dcterms:modified    "2014-03-01+09:00"^^xsd:date ;
        status:term_status  "unstable"@en ;
        skos:altLabel       "Malt Whiskey"@en ;
        skos:definition     "\n    Malt whisky is whisky that is made from a fermented mash produced primarily\n    from a malted grain.\n    "@en ;
        skos:prefLabel      "Malt Whisky"@en , "몰트 위스키"@ko .

beverage:DonJulioBlanco
        a                        owl:NamedIndividual , gr:ProductOrServiceModel , bevon:TequilaBlanco ;
        rdfs:seeAlso             <http://www.donjulio.com/blanco.aspx> ;
        bevon:abv                "40"^^xsd:decimal ;
        bevon:color              [ a              dbpedia:Colour ;
                                   dcterms:title  "Clear"@en ;
                                   owl:sameAs     <http://dbpedia.org/resource/Clear_(color)>
                                 ] ;
        bevon:container          container:750mlGlassBottle ;
        bevon:description        "\n    Tequila Don Julio Blanco is the base from which all of our other variants\n    are derived. Commonly referred to as \"silver\" tequila, its crisp agave\n    flavor and hints of citrus make it an essential component to a variety of\n    innovative drinks including margaritas. It can also be enjoyed neat or on\n    the rocks.\n    "@en ;
        bevon:fermentation_base  <http://dbpedia.org/resource/Agave> ;
        bevon:launch             "1942"^^xsd:gYear ;
        bevon:manufacturer       <http://dbpedia.org/resource/Diageo> ;
        bevon:name               "Don Julio Blanco"@en , "돈 훌리오 블랑코"@ko ;
        bevon:origin             <http://dbpedia.org/resource/Mexico> ;
        bevon:proof              "80"^^xsd:decimal .

bevon:PlasticBottle  a      owl:Class ;
        rdfs:comment        "\n    Plastic bottles are typically used to store liquids such as water, soft\n    drinks, motor oil, cooking oil, medicine, shampoo, milk, and ink.\n    "@en ;
        rdfs:isDefinedBy    bevon: ;
        rdfs:seeAlso        <http://en.wikipedia.org/wiki/Plastic_bottle> ;
        rdfs:subClassOf     bevon:Container ;
        dcterms:issued      "2013-07-04+09:00"^^xsd:date ;
        dcterms:modified    "2014-03-01+09:00"^^xsd:date ;
        status:term_status  "unstable"@en ;
        skos:definition     "\n    A plastic bottle is a bottle constructed of plastic.\n    "@en ;
        skos:prefLabel      "Plastic Bottle"@en , "플라스틱 병"@ko .

bevon:BeverageCan  a        owl:Class ;
        rdfs:comment        "\n    Beverage cans are made of aluminium (75% of worldwide production) or\n    tin-plated steel (25% worldwide production).\n    "@en ;
        rdfs:isDefinedBy    bevon: ;
        rdfs:seeAlso        <http://en.wikipedia.org/wiki/Beverage_can> ;
        rdfs:subClassOf     bevon:Container ;
        dcterms:issued      "2013-07-04+09:00"^^xsd:date ;
        dcterms:modified    "2014-03-01+09:00"^^xsd:date ;
        status:term_status  "unstable"@en ;
        skos:definition     "\n    A beverage can is a metal container designed to hold a fixed portion of\n    liquid such as a carbonated soft drinks, alcoholic beverages, fruit juices,\n    teas, tisanes, energy drinks, etc.\n    "@en ;
        skos:prefLabel      "Beverage Can"@en , "음료 캔"@ko .

bevon:volume  a             owl:ObjectProperty ;
        rdfs:domain         bevon:Container ;
        rdfs:isDefinedBy    bevon: ;
        rdfs:range          gr:QuantitativeValue ;
        dcterms:issued      "2013-07-04+09:00"^^xsd:date ;
        dcterms:modified    "2014-03-01+09:00"^^xsd:date ;
        status:term_status  "unstable"@en ;
        skos:definition     "\n    This property specifies the volume of the container.\n    "@en ;
        skos:prefLabel      "용량"@ko , "volume"@en .

bevon:material  a           owl:ObjectProperty ;
        rdfs:domain         bevon:Aging ;
        rdfs:isDefinedBy    bevon: ;
        dcterms:issued      "2013-07-04+09:00"^^xsd:date ;
        dcterms:modified    "2014-03-01+09:00"^^xsd:date ;
        status:term_status  "unstable"@en ;
        skos:definition     "\n    This property specifies what the aging cask was made of.\n    "@en ;
        skos:prefLabel      "소재"@ko , "material"@en .

bevon:Mocktail  a           owl:Class ;
        rdfs:isDefinedBy    bevon: ;
        rdfs:subClassOf     bevon:MixedDrink , bevon:NonAlcoholicBeverage ;
        dcterms:issued      "2013-07-04+09:00"^^xsd:date ;
        dcterms:modified    "2014-03-01+09:00"^^xsd:date ;
        owl:disjointWith    bevon:Cocktail ;
        status:term_status  "unstable"@en ;
        skos:definition     "\n    Mocktails are mock cocktails, or those that do not contain any alcohol.\n    "@en ;
        skos:prefLabel      "목테일"@ko , "Mocktail"@en .

bevon:ingredient  a         owl:ObjectProperty ;
        rdfs:domain         bevon:MixedDrink ;
        rdfs:isDefinedBy    bevon: ;
        rdfs:range          food:Ingredient ;
        rdfs:subPropertyOf  food:containsIngredient ;
        dcterms:issued      "2013-07-04+09:00"^^xsd:date ;
        dcterms:modified    "2014-03-01+09:00"^^xsd:date ;
        status:term_status  "unstable"@en ;
        skos:definition     "\n    This property specifies an ingredient of the mixed drink.\n    "@en ;
        skos:prefLabel      "재료"@ko , "ingredient"@en .

bevon:FermentedBeverage
        a                   owl:Class ;
        rdfs:isDefinedBy    bevon: ;
        rdfs:subClassOf     bevon:AlcoholicBeverage ;
        dcterms:issued      "2013-07-04+09:00"^^xsd:date ;
        dcterms:modified    "2014-03-01+09:00"^^xsd:date ;
        status:term_status  "testing"@en ;
        skos:altLabel       "발효주"@ko ;
        skos:definition     "\n    A fermented beverage is a drink produced by fermenting grain, fruit, or\n    vegetables.\n    "@en ;
        skos:prefLabel      "양조주"@ko , "Fermented Beverage"@en .

bevon:ibu  a                owl:DatatypeProperty ;
        rdfs:domain         bevon:Beer ;
        rdfs:isDefinedBy    bevon: ;
        rdfs:range          xsd:nonNegativeInteger ;
        rdfs:seeAlso        <http://en.wikipedia.org/wiki/International_Bitterness_Units_scale> ;
        dcterms:issued      "2013-07-04+09:00"^^xsd:date ;
        dcterms:modified    "2014-03-01+09:00"^^xsd:date ;
        status:term_status  "unstable"@en ;
        skos:altLabel       "International Bitterness Unit scale"@en ;
        skos:definition     "\n    The International Bittering Units scale, or simply IBU scale, provides a\n    measure of the bitterness of beer, which is provided by the hops used\n    during brewing.\n    "@en ;
        skos:prefLabel      "IBU scale"@en , "IBU 척도"@ko .

<http://rdfs.co/bevon/0.7/rdf>
        dcterms:format  [ a           dcterms:IMT ;
                          rdf:value   "application/rdf+xml" ;
                          rdfs:label  "RDF/XML"@en
                        ] .

bevon:BeerKeg  a            owl:Class ;
        rdfs:isDefinedBy    bevon: ;
        rdfs:subClassOf     bevon:Keg ;
        dcterms:issued      "2013-07-04+09:00"^^xsd:date ;
        dcterms:modified    "2014-03-01+09:00"^^xsd:date ;
        status:term_status  "unstable"@en ;
        skos:definition     "\n    Beer kegs are made of stainless steel, or less commonly, of aluminium.\n    "@en ;
        skos:prefLabel      "맥주 케그"@ko , "Beer Keg"@en .

bevon:name  a               owl:DatatypeProperty ;
        rdfs:domain         bevon:Beverage ;
        rdfs:isDefinedBy    bevon: ;
        rdfs:range          xsd:string ;
        rdfs:subPropertyOf  gr:name , foaf:name , dcterms:title ;
        dcterms:issued      "2013-07-04+09:00"^^xsd:date ;
        dcterms:modified    "2014-03-01+09:00"^^xsd:date ;
        status:term_status  "testing"@en ;
        skos:definition     "\n    This property indicates the name of the beverage.\n    "@en ;
        skos:prefLabel      "이름"@ko , "name"@en .

container:50lBeerKeg  a  bevon:BeerKeg , owl:NamedIndividual ;
        bevon:volume    [ a                        gr:QuantitativeValueInteger ;
                          gr:hasUnitOfMeasurement  "LTR" ;
                          gr:hasValue              "50"^^xsd:int
                        ] ;
        skos:prefLabel  "50l 맥주 케그"@ko , "50l Beer Keg"@en .

bevon:Porter  a             owl:Class ;
        rdfs:comment        "\n    The name came about as a result of its popularity with street and river\n    porters.\n    "@en ;
        rdfs:isDefinedBy    bevon: ;
        rdfs:seeAlso        <http://en.wikipedia.org/wiki/English_porter> ;
        rdfs:subClassOf     pto:English_porter , bevon:Ale ;
        dcterms:issued      "2013-07-04+09:00"^^xsd:date ;
        dcterms:modified    "2014-03-01+09:00"^^xsd:date ;
        status:term_status  "unstable"@en ;
        skos:altLabel       "English Porter"@en ;
        skos:definition     "\n    Porter is a dark style of beer originating in London in the 18th century,\n    descended from brown beer, a well hopped beer made from brown malt.\n    "@en ;
        skos:prefLabel      "Porter"@en , "포터"@ko .

bevon:container  a          owl:ObjectProperty ;
        rdfs:domain         bevon:Beverage ;
        rdfs:isDefinedBy    bevon: ;
        rdfs:range          bevon:Container ;
        dcterms:issued      "2013-07-04+09:00"^^xsd:date ;
        dcterms:modified    "2014-03-01+09:00"^^xsd:date ;
        status:term_status  "unstable"@en ;
        skos:definition     "\n    This property can be used to indicate that the beverage is available in a\n    type of container.\n    "@en ;
        skos:prefLabel      "용기"@ko , "container"@en .

bevon:CarbonatedWater
        a                   owl:Class ;
        rdfs:isDefinedBy    bevon: ;
        rdfs:seeAlso        <http://en.wikipedia.org/wiki/Carbonated_water> ;
        rdfs:subClassOf     bevon:Water , pto:Carbonated_water ;
        dcterms:issued      "2013-07-04+09:00"^^xsd:date ;
        dcterms:modified    "2014-03-01+09:00"^^xsd:date ;
        status:term_status  "unstable"@en ;
        skos:altLabel       "클럽소다"@ko , "소다수"@ko , "Seltzer Water"@en , "Soda Water"@en , "Sparkling Water"@en , "Fizzy Water"@en , "Club Soda"@en ;
        skos:definition     "\n    Carbonated water is water into which carbon dioxide gas under pressure has\n    been dissolved.\n    "@en ;
        skos:prefLabel      "Carbonated Water"@en , "탄산수"@ko .

container:15lBeerKeg  a  bevon:BeerKeg , owl:NamedIndividual ;
        bevon:volume    [ a                        gr:QuantitativeValueInteger ;
                          gr:hasUnitOfMeasurement  "LTR" ;
                          gr:hasValue              "15"^^xsd:int
                        ] ;
        skos:prefLabel  "15l 맥주 케그"@ko , "15l Beer Keg"@en .

bevon:Wine  a               owl:Class ;
        rdfs:isDefinedBy    bevon: ;
        rdfs:seeAlso        <http://en.wikipedia.org/wiki/Wine> ;
        rdfs:subClassOf     bevon:FermentedBeverage , pto:Wine ;
        dcterms:issued      "2013-07-04+09:00"^^xsd:date ;
        dcterms:modified    "2014-03-07+09:00"^^xsd:date ;
        status:term_status  "testing"@en ;
        skos:definition     "\n    Wine is an alcoholic beverage made from fermented grapes or other fruits.\n    "@en ;
        skos:historyNote    [ rdf:value        "\n      Changed the semantics of bevon:Wine not to be the same as wine:Wine\n      "@en ;
                              dcterms:creator  <http://jayg.me/> ;
                              dcterms:date     "2014-03-07+09:00"^^xsd:date
                            ] ;
        skos:prefLabel      "Wine"@en , "Vin"@fr , "와인"@ko .

bevon:FruitWine  a          owl:Class ;
        rdfs:comment        "\n    This definition is sometimes broadened to include any fermented alcoholic\n    beverage except beer. For historical reasons, mead, cider, and perry are\n    also excluded from the definition of fruit wine.\n    "@en ;
        rdfs:isDefinedBy    bevon: ;
        rdfs:seeAlso        <http://en.wikipedia.org/wiki/Fruit_wine> ;
        rdfs:subClassOf     pto:Fruit_wine , bevon:Wine ;
        dcterms:issued      "2014-03-07+09:00"^^xsd:date ;
        dcterms:modified    "2014-03-07+09:00"^^xsd:date ;
        status:term_status  "testing"@en ;
        skos:definition     "\n    Fruit wines are fermented alcoholic beverages made from a variety of base\n    ingredients (other than grapes); they may also have additional flavors\n    taken from fruits, flowers, and herbs.\n    "@en ;
        skos:prefLabel      "Fruit Wine"@en , "과실주"@ko , "Vin de Sureau"@fr .

bevon:IrishWhiskey  a       owl:Class ;
        rdfs:comment        "\n    Key regulations defining Irish whiskey and its production are established\n    by the Irish Whiskey Act of 1980.\n    "@en ;
        rdfs:isDefinedBy    bevon: ;
        rdfs:seeAlso        <http://en.wikipedia.org/wiki/Irish_whiskey> ;
        rdfs:subClassOf     pto:Irish_whiskey , bevon:Whisky ;
        dcterms:issued      "2013-07-04+09:00"^^xsd:date ;
        dcterms:modified    "2014-03-01+09:00"^^xsd:date ;
        status:term_status  "unstable"@en ;
        skos:altLabel       "Irish Whisky"@en ;
        skos:definition     "\n    Irish whiskey is whisky made in Ireland.\n    "@en ;
        skos:prefLabel      "Irish Whiskey"@en , "아이리쉬 위스키"@ko , "Fuisce"@ga .

bevon:Stout  a              owl:Class ;
        rdfs:comment        "\n    Stouts were traditionally the generic term for the strongest or stoutest\n    porters, typically 7% or 8%, produced by a brewery.\n    "@en ;
        rdfs:isDefinedBy    bevon: ;
        rdfs:seeAlso        <http://en.wikipedia.org/wiki/Stout> ;
        rdfs:subClassOf     pto:Stout , bevon:Porter ;
        dcterms:issued      "2013-07-04+09:00"^^xsd:date ;
        dcterms:modified    "2014-03-01+09:00"^^xsd:date ;
        status:term_status  "unstable"@en ;
        skos:altLabel       "Strong Porter"@en ;
        skos:definition     "\n    Stout is a dark beer made using roasted malt or roasted barley, hops, water\n    and yeast.\n    "@en ;
        skos:prefLabel      "Stout"@en , "스타우트"@ko .

bevon:ContainerGroup  a  rdf:Bag ;
        rdf:_1        bevon:Container ;
        rdf:_2        bevon:BeverageCan ;
        rdf:_3        bevon:GlassBottle ;
        rdf:_4        bevon:PlasticBottle ;
        rdf:_5        bevon:Keg ;
        rdf:_6        bevon:volume ;
        rdfs:comment  "\n    These classes and properties are used to describe beverage containers.\n    "@en ;
        rdfs:label    "Container Terms"@en .

bevon:Whisky  a             owl:Class ;
        rdfs:comment        "\n    Different grains are used for different varieties, including barley, malted\n    barley, rye, malted rye, wheat, and corn. Whisky is typically aged in\n    wooden casks, made generally of charred white oak.\n    "@en ;
        rdfs:isDefinedBy    bevon: ;
        rdfs:seeAlso        <http://en.wikipedia.org/wiki/Whisky> ;
        rdfs:subClassOf     pto:Whisky , bevon:DistilledBeverage ;
        dcterms:issued      "2013-07-04+09:00"^^xsd:date ;
        dcterms:modified    "2014-03-01+09:00"^^xsd:date ;
        owl:sameAs          whisky:Whiskey ;
        status:term_status  "testing"@en ;
        skos:altLabel       "Whiskey"@en ;
        skos:definition     "\n    Whisky or whiskey is a type of distilled alcoholic beverage made from\n    fermented grain mash.\n    "@en ;
        skos:prefLabel      "Whisky"@en , "위스키"@en .

whisky:abv  rdfs:subPropertyOf  bevon:abv .

bevon:related  a            owl:ObjectProperty ;
        rdfs:domain         bevon:Beverage ;
        rdfs:isDefinedBy    bevon: ;
        rdfs:range          bevon:Beverage ;
        dcterms:issued      "2013-07-04+09:00"^^xsd:date ;
        dcterms:modified    "2014-03-01+09:00"^^xsd:date ;
        status:term_status  "unstable"@en ;
        skos:definition     "\n    This property states that a beverage is related to another beverage.\n    "@en ;
        skos:prefLabel      "연관"@ko , "related"@en .

bevon:Tequila  a            owl:Class ;
        rdfs:isDefinedBy    bevon: ;
        rdfs:seeAlso        <http://en.wikipedia.org/wiki/Tequila> ;
        rdfs:subClassOf     bevon:DistilledBeverage , pto:Tequila ;
        dcterms:issued      "2013-07-04+09:00"^^xsd:date ;
        dcterms:modified    "2014-03-01+09:00"^^xsd:date ;
        status:term_status  "testing"@en ;
        skos:definition     "\n    Tequila is a distilled beverage made from the blue agave plant, primarily\n    in the area surrounding the city of Tequila, 65 kilometres (40 mi)\n    northwest of Guadalajara, and in the highlands (Los Altos) of the western\n    Mexican state of Jalisco.\n    "@en ;
        skos:prefLabel      "Tequila"@en , "테킬라"@ko .

bevon:Ale  a                owl:Class ;
        rdfs:comment        "\n    The yeast will ferment the beer quickly, giving it a sweet, full bodied and\n    fruity taste.\n    "@en ;
        rdfs:isDefinedBy    bevon: ;
        rdfs:seeAlso        <http://en.wikipedia.org/wiki/Ale> ;
        rdfs:subClassOf     bevon:Beer , pto:Ale ;
        dcterms:issued      "2013-07-04+09:00"^^xsd:date ;
        dcterms:modified    "2014-03-01+09:00"^^xsd:date ;
        status:term_status  "unstable"@en ;
        skos:definition     "\n    Ale is a type of beer brewed from malted barley using a warm-fermentation\n    with a strain of brewers' yeast.\n    "@en ;
        skos:prefLabel      "에일"@ko , "Ale"@en .

bevon:WhiteWine  a          owl:Class ;
        rdfs:comment        "\n    It is produced by the alcoholic fermentation of the non-coloured pulp of\n    grapes which may have a white or black skin. It is treated so as to\n    maintain a yellow transparent colour in the final product.\n    "@en ;
        rdfs:isDefinedBy    bevon: ;
        rdfs:seeAlso        <http://en.wikipedia.org/wiki/White_wine> ;
        rdfs:subClassOf     bevon:Wine , pto:White_wine ;
        dcterms:issued      "2014-03-07+09:00"^^xsd:date ;
        dcterms:modified    "2014-03-07+09:00"^^xsd:date ;
        owl:sameAs          wine:WhiteWine ;
        status:term_status  "testing"@en ;
        skos:definition     "\n    White wine is a wine whose colour can be straw-yellow, yellow-green, or\n    yellow-gold coloured.\n    "@en ;
        skos:prefLabel      "Vin Blanc"@fr , "White Wine"@en , "화이트 와인"@ko .

whisky:distillery  rdfs:subPropertyOf  bevon:distillery .

bevon:WhiskyGroup  a  rdf:Bag ;
        rdf:_1        bevon:Whisky ;
        rdf:_10       bevon:SingleMaltScotch ;
        rdf:_11       bevon:SpeysideSingleMalt ;
        rdf:_2        bevon:AmericanWhiskey ;
        rdf:_3        bevon:BourbonWhiskey ;
        rdf:_4        bevon:CanadianWhisky ;
        rdf:_5        bevon:IrishWhiskey ;
        rdf:_6        bevon:JapaneseWhisky ;
        rdf:_7        bevon:ScotchWhisky ;
        rdf:_8        bevon:MaltWhisky ;
        rdf:_9        bevon:SingleMaltWhisky ;
        rdfs:comment  "\n    These classes describe types of whiskies.\n    "@en ;
        rdfs:label    "Whisky Terms"@en .

bevon:DistilledBeverage
        a                   owl:Class ;
        rdfs:comment        "\n     This excludes undistilled fermented beverages such as beer, wine, and\n     cider.\n     "@en ;
        rdfs:isDefinedBy    bevon: ;
        rdfs:seeAlso        <http://en.wikipedia.org/wiki/Distilled_beverage> ;
        rdfs:subClassOf     pto:Distilled_beverage , bevon:AlcoholicBeverage ;
        dcterms:issued      "2013-07-04+09:00"^^xsd:date ;
        dcterms:modified    "2014-03-01+09:00"^^xsd:date ;
        status:term_status  "testing"@en ;
        skos:altLabel       "Spirit"@en , "Liquor"@en ;
        skos:definition     "\n     A distilled beverage, spirit, or liquor is an alcoholic beverage\n     containing ethanol that is produced by distilling (i.e., concentrating\n     by distillation) ethanol produced by means of fermenting grain, fruit,\n     or vegetables.\n     "@en ;
        skos:prefLabel      "증류주"@ko , "Distilled Beverage"@en .

<http://rdfs.co/bevon/0.7/html>
        dcterms:format  [ a           dcterms:IMT ;
                          rdf:value   "text/html" ;
                          rdfs:label  "HTML"@en
                        ] .

bevon:WineGroup  a    rdf:Bag ;
        rdf:_1        bevon:Wine ;
        rdf:_2        bevon:RedWine ;
        rdf:_3        bevon:WhiteWine ;
        rdf:_4        bevon:FruitWine ;
        rdfs:comment  "\n    These classes describe types of wines.\n    "@en ;
        rdfs:label    "Wine Terms"@en .

container:640mlLongneck
        a               bevon:Longneck , owl:NamedIndividual ;
        bevon:volume    [ a                        gr:QuantitativeValueInteger ;
                          gr:hasUnitOfMeasurement  "MLT" ;
                          gr:hasValue              "640"^^xsd:int
                        ] ;
        skos:prefLabel  "640ml 긴목 맥주병"@ko , "640ml Longneck Bottle"@en .

bevon:IrishRedAle  a        owl:Class ;
        rdfs:isDefinedBy    bevon: ;
        rdfs:seeAlso        <http://en.wikipedia.org/wiki/Irish_red_ale> ;
        rdfs:subClassOf     bevon:PaleAle ;
        dcterms:issued      "2013-07-04+09:00"^^xsd:date ;
        dcterms:modified    "2014-03-01+09:00"^^xsd:date ;
        status:term_status  "unstable"@en ;
        skos:definition     "\n    Irish red ale, red ale, or Irish ale is a name used by brewers in Ireland.\n    "@en ;
        skos:prefLabel      "Irish Red Ale"@en , "아이리쉬 레드 에일"@ko .

bevon:RedWine  a            owl:Class ;
        rdfs:comment        "\n    The actual colour of the wine can range from intense violet, typical of\n    young wines, through to brick red for mature wines and brown for older red\n    wines.\n    "@en ;
        rdfs:isDefinedBy    bevon: ;
        rdfs:seeAlso        <http://en.wikipedia.org/wiki/Red_wine> ;
        rdfs:subClassOf     bevon:Wine , pto:Red_wine ;
        dcterms:issued      "2014-03-07+09:00"^^xsd:date ;
        dcterms:modified    "2014-03-07+09:00"^^xsd:date ;
        owl:sameAs          wine:RedWine ;
        status:term_status  "testing"@en ;
        skos:definition     "\n    Red wine is a type of wine made from dark-coloured (black) grape varieties.\n    "@en ;
        skos:prefLabel      "Vin Rouge"@fr , "Red Wine"@en , "레드 와인"@ko .

container:700mlGlassBottle
        a               bevon:GlassBottle , owl:NamedIndividual ;
        bevon:volume    [ a                        gr:QuantitativeValueInteger ;
                          gr:hasUnitOfMeasurement  "MLT" ;
                          gr:hasValue              "700"^^xsd:int
                        ] ;
        skos:altLabel   "70cl Glass Bottle"@en ;
        skos:prefLabel  "700ml 유리병"@ko , "700ml Glass Bottle"@en .

bevon:similar  a            owl:SymmetricProperty ;
        rdfs:domain         bevon:Beverage ;
        rdfs:isDefinedBy    bevon: ;
        rdfs:range          bevon:Beverage ;
        rdfs:subPropertyOf  bevon:related , gr:isSimilarTo ;
        dcterms:issued      "2013-07-04+09:00"^^xsd:date ;
        dcterms:modified    "2014-03-01+09:00"^^xsd:date ;
        status:term_status  "unstable"@en ;
        skos:definition     "\n    This property states that a beverage is similar to another beverage.\n    "@en ;
        skos:prefLabel      "similar"@en , "유사"@ko .

bevon:abv  a                owl:DatatypeProperty ;
        rdfs:domain         bevon:Beverage ;
        rdfs:isDefinedBy    bevon: ;
        rdfs:range          xsd:decimal ;
        rdfs:seeAlso        <http://en.wikipedia.org/wiki/Alcohol_by_volume> ;
        dcterms:issued      "2013-07-04+09:00"^^xsd:date ;
        dcterms:modified    "2014-03-01+09:00"^^xsd:date ;
        status:term_status  "testing"@en ;
        skos:altLabel       "alcohol by volume"@en ;
        skos:definition     "\n    ABV (Alcohol by Volume) is a standard measure of how much alcohol is\n    contained in the drink.\n    "@en ;
        skos:prefLabel      "알코올 도수"@ko , "ABV"@en .

bevon:0.7  a                           adms:SemanticAsset , owl:Ontology , cc:Work ;
        rdfs:comment                   "\n    <div>\n      The master version of this vocabulary is maintained in <a\n      href=\"https://github.com/jgkim/bevon\">the GitHub repository</a> so others\n      can contribute edits and improvements.\n    </div>\n    "^^rdf:XMLLiteral , "\n    Most of the descriptions given here are from Wikipedia or from the websites\n    of the related products.\n    "@en ;
        rdfs:seeAlso                   <https://github.com/jgkim/bevon> ;
        cc:license                     <http://creativecommons.org/licenses/by/4.0/> ;
        dcterms:creator                <http://jayg.me/> ;
        dcterms:description            "\n    Beverage Ontology is a Web vocabulary for describing beverages, mainly\n    alcoholic.\n    "@en ;
        dcterms:hasFormat              <http://rdfs.co/bevon/0.7/rdf> , <http://rdfs.co/bevon/0.7/html> , <http://rdfs.co/bevon/0.7/ttl> ;
        dcterms:identifier             "http://rdfs.co/bevon/0.7" ;
        dcterms:isVersionOf            bevon: ;
        dcterms:issued                 "2013-07-04+09:00"^^xsd:date ;
        dcterms:modified               "2014-03-06+09:00"^^xsd:date ;
        dcterms:replaces               bevon:0.6 ;
        dcterms:rights                 "Copyright © 2013-2014 James G. Kim Some Rights Reserved." ;
        dcterms:title                  "BEVON: Beverage Ontology"@en ;
        dcterms:type                   <http://purl.org/adms/assettype/Ontology> ;
        vann:example                   [ rdfs:comment  "\n    <pre><code>beverage:WhiskyAndSoda\n  a owl:NamedIndividual, bevon:Highball , gr:ProductOrServiceModel ;\n  bevon:name \"Whisky &amp; Soda\"@en , \"위스키 소다\"@ko ;\n  bevon:description \"\"\"\n    Whisky &amp; Soda is a kind of mixed drinks that are composed of whisky and\n    carbonated water.\n    \"\"\"@en ;\n  bevon:ingredient [\n    a food:Ingredient ;\n    bevon:food [\n      a bevon:Whisky ;\n      owl:sameAs &lt;http://dbpedia.org/resource/Whisky&gt; ;\n      dcterms:title \"Whisky\"@en\n    ] ;\n    bevon:quantity [\n      a gr:QuantitativeValueInteger ;\n      gr:hasUnitOfMeasurement \"OZA\" ;\n      gr:hasValue \"2\"^^xsd:int\n    ]\n  ] , [\n    a food:Ingredient ;\n    bevon:food [\n      a bevon:CarbonatedWater ;\n      owl:sameAs &lt;http://dbpedia.org/resource/Carbonated_water&gt; ;\n      dcterms:title \"Carbonated Water\"@en\n    ]\n  ] .</code></pre>\n    "^^rdf:XMLLiteral ;
                                         rdfs:label    "Whisky & Soda"@en
                                       ] ;
        vann:example                   [ rdfs:comment  "\n    <pre><code>beverage:Glenfiddich12YearOld\n  a owl:NamedIndividual, bevon:SpeysideSingleMalt , gr:ProductOrServiceModel ;\n  bevon:name \"Glenfiddich 12 Year Old\"@en , \"글렌피딕 12년\"@ko ;\n  bevon:description \"\"\"\n    Carefully matured in the finest American bourbon and Spanish sherry oak\n    casks for at least 12 years. Married and mellowed in oak marrying tuns for\n    complete harmony of aroma and flavor.\n\n    A single malt Scotch whisky with distinctive fresh pear, creamy with subtle\n    oak flavors and a long smooth and mellow finish.\n    \"\"\"@en ;\n  bevon:origin &lt;http://dbpedia.org/resource/Strathspey,_Scotland&gt; ;\n  bevon:launch \"1887\"^^xsd:gYear ;\n  bevon:distillery [\n    a bevon:Distillery ;\n    owl:sameAs &lt;http://dbpedia.org/resource/Glenfiddich_distillery&gt; ;\n    whisky:region &lt;http://dbpedia.org/resource/Strathspey,_Scotland&gt; ;\n    whisky:owner &lt;http://dbpedia.org/resource/William_Grant_%26_Sons&gt; ;\n    whisky:waterSource [\n      a whisky:WaterSource ;\n      dcterms:title \"Robbie Dhu Springs\"@en , \"로비 듀 수원지\"@ko\n    ]\n  ] ;\n  bevon:manufacturer &lt;http://dbpedia.org/resource/William_Grant_%26_Sons&gt; ;\n  bevon:fermentation_base &lt;http://dbpedia.org/resource/Barley&gt; ;\n  bevon:aging [\n    a bevon:Aging ;\n    bevon:material &lt;http://dbpedia.org/resource/Oak&gt; ;\n    bevon:previous_content\n      &lt;http://dbpedia.org/resource/Bourbon_whiskey&gt; ,\n      &lt;http://dbpedia.org/resource/Sherry&gt; ;\n    bevon:duration [\n      a time:DurationDescription ;\n      time:years \"12\"^^xsd:decimal\n    ]\n  ] ;\n  bevon:color [\n    a dbpedia:Colour ;\n    owl:sameAs &lt;http://dbpedia.org/resource/Gold_(color)&gt; ;\n    owl:sameAs &lt;http://purl.org/colors/rgb/FFD700&gt; ;\n    dcterms:title \"Gold\"@en\n  ] ;\n  bevon:abv \"40\"^^xsd:decimal ;\n  bevon:container container:700mlGlassBottle .\n\ncontainer:700mlGlassBottle a owl:NamedIndividual, bevon:GlassBottle ;\n  skos:prefLabel \"700ml Glass Bottle\"@en , \"700ml 유리병\"@ko ;\n  skos:altLabel \"70cl Glass Bottle\"@en ;\n  bevon:volume [\n    a gr:QuantitativeValueInteger ;\n    gr:hasUnitOfMeasurement \"MLT\" ;\n    gr:hasValue \"700\"^^xsd:int\n  ] .</code></pre>\n    "^^rdf:XMLLiteral ;
                                         rdfs:label    "Glenfiddich 12 Year Old"@en
                                       ] ;
        vann:preferredNamespacePrefix  "bevon" ;
        vann:preferredNamespaceUri     "http://rdfs.co/bevon/" ;
        vann:termGroup                 bevon:RelationGroup , bevon:WineGroup , bevon:BeerGroup , bevon:ContainerGroup , bevon:CocktailGroup , bevon:CoreGroup , bevon:WhiskyGroup ;
        owl:versionInfo                "0.7" ;
        skos:changeNote                [ rdf:value        "\n      Added term groups for core, relation, container, beer, whisky and cocktail\n      terms\n      "@en ;
                                         dcterms:creator  <http://jayg.me/> ;
                                         dcterms:date     "2014-03-06+09:00"^^xsd:date
                                       ] ;
        skos:changeNote                [ rdf:value        "\n      Added a link to the GitHub repository\n      "@en ;
                                         dcterms:creator  <http://jayg.me/> ;
                                         dcterms:date     "2014-03-03+09:00"^^xsd:date
                                       ] ;
        skos:changeNote                [ rdf:value        "\n      Minor revisions for documentation\n      "@en ;
                                         dcterms:creator  <http://jayg.me/> ;
                                         dcterms:date     "2014-03-01+09:00"^^xsd:date
                                       ] ;
        skos:historyNote               [ rdf:value        "\n      Changed bevon:FermentedBeverages to bevon:FermentedBeverage for the\n      consistency\n      "@en ;
                                         dcterms:creator  <http://jayg.me/> ;
                                         dcterms:date     "2014-03-06+09:00"^^xsd:date
                                       ] ;
        skos:historyNote               [ rdf:value        "\n      Changed the semantics of bevon:Wine to be a superclass of wine:Wine\n      "@en ;
                                         dcterms:creator  <http://jayg.me/> ;
                                         dcterms:date     "2014-03-07+09:00"^^xsd:date
                                       ] ;
        skos:historyNote               [ rdf:value        "\n      Added bevon:RedWine, bevon:WhiteWine and bevon:FruitWine\n      "@en ;
                                         dcterms:creator  <http://jayg.me/> ;
                                         dcterms:date     "2014-03-07+09:00"^^xsd:date
                                       ] ;
        adms:status                    <http://purl.org/adms/status/UnderDevelopment> .

bevon:Cognac  a             owl:Class ;
        rdfs:comment        "\n    It is produced in the wine-growing region surrounding the town from which\n    it takes its name, in the French Departements of Charente and\n    Charente-Maritime.\n    "@en ;
        rdfs:isDefinedBy    bevon: ;
        rdfs:seeAlso        <http://en.wikipedia.org/wiki/Cognac> ;
        rdfs:subClassOf     bevon:Brandy , pto:Cognac ;
        dcterms:issued      "2013-07-04+09:00"^^xsd:date ;
        dcterms:modified    "2014-03-01+09:00"^^xsd:date ;
        status:term_status  "testing"@en ;
        skos:definition     "\n    Cognac, named after the town of Cognac in France, is a variety of brandy.\n    "@en ;
        skos:prefLabel      "코냑"@ko , "Cognac"@en .

bevon:MixedDrink  a         owl:Class ;
        rdfs:comment        "\n    Some mixed drinks are alcoholic beverages that contain liquor; others are\n    non-alcoholic.\n    "@en ;
        rdfs:isDefinedBy    bevon: ;
        rdfs:seeAlso        <http://en.wikipedia.org/wiki/Mixed_drink> ;
        rdfs:subClassOf     pto:Mixed_drink , bevon:Beverage ;
        dcterms:issued      "2013-07-04+09:00"^^xsd:date ;
        dcterms:modified    "2014-03-01+09:00"^^xsd:date ;
        status:term_status  "testing"@en ;
        skos:definition     "\n    A mixed drink is a beverage in which two or more ingredients are mixed.\n    "@en ;
        skos:prefLabel      "혼합 음료"@ko , "Mixed Drink"@en .

bevon:color  a              owl:DatatypeProperty ;
        rdfs:domain         bevon:Beverage ;
        rdfs:isDefinedBy    bevon: ;
        rdfs:range          dbpedia:Colour ;
        dcterms:issued      "2013-07-04+09:00"^^xsd:date ;
        dcterms:modified    "2014-03-01+09:00"^^xsd:date ;
        status:term_status  "unstable"@en ;
        skos:definition     "\n    This property specifies the color of the beverage.\n    "@en ;
        skos:prefLabel      "color"@en , "색상"@ko .

bevon:SpeysideSingleMalt
        a                   owl:Class ;
        rdfs:isDefinedBy    bevon: ;
        rdfs:seeAlso        <http://en.wikipedia.org/wiki/Speyside_single_malts> ;
        rdfs:subClassOf     bevon:SingleMaltScotch , pto:Speyside_single_malts ;
        dcterms:issued      "2013-07-04+09:00"^^xsd:date ;
        dcterms:modified    "2014-03-01+09:00"^^xsd:date ;
        status:term_status  "unstable"@en ;
        skos:definition     "\n    Speyside single malts are single malt Scotch whiskies, distilled in\n    Strathspey, the area around the River Spey in Moray and Badenoch and\n    Strathspey, in northeastern Scotland.\n    "@en ;
        skos:prefLabel      "스페이사이드 싱글 몰트"@ko , "Speyside Single Malt"@en .

beverage:WhiskyAndSoda
        a                  bevon:Highball , gr:ProductOrServiceModel , owl:NamedIndividual ;
        bevon:description  "\n    Whisky & Soda is a kind of mixed drinks that are composed of whisky and\n    carbonated water.\n    "@en ;
        bevon:ingredient   [ a           food:Ingredient ;
                             bevon:food  [ a              bevon:CarbonatedWater ;
                                           dcterms:title  "Carbonated Water"@en ;
                                           owl:sameAs     <http://dbpedia.org/resource/Carbonated_water>
                                         ]
                           ] ;
        bevon:ingredient   [ a               food:Ingredient ;
                             bevon:food      [ a              bevon:Whisky ;
                                               dcterms:title  "Whisky"@en ;
                                               owl:sameAs     <http://dbpedia.org/resource/Whisky>
                                             ] ;
                             bevon:quantity  [ a                        gr:QuantitativeValueInteger ;
                                               gr:hasUnitOfMeasurement  "OZA" ;
                                               gr:hasValue              "2"^^xsd:int
                                             ]
                           ] ;
        bevon:name         "위스키 소다"@ko , "Whisky & Soda"@en .

<http://rdfs.co/bevon/0.7/ttl>
        dcterms:format  [ a           dcterms:IMT ;
                          rdf:value   "text/turtle" ;
                          rdfs:label  "Turtle"@en
                        ] .

bevon:Gin  a                owl:Class ;
        rdfs:isDefinedBy    bevon: ;
        rdfs:seeAlso        <http://en.wikipedia.org/wiki/Gin> ;
        rdfs:subClassOf     bevon:DistilledBeverage , pto:Gin ;
        dcterms:issued      "2013-07-04+09:00"^^xsd:date ;
        dcterms:modified    "2014-03-01+09:00"^^xsd:date ;
        status:term_status  "testing"@en ;
        skos:definition     "\n    Gin is a spirit which derives its predominant flavor from juniper berries\n    (Juniperus communis).\n    "@en ;
        skos:prefLabel      "진"@ko , "Gin"@en .

beverage:KozelDark  a            bevon:Dunkel , owl:NamedIndividual , gr:ProductOrServiceModel ;
        bevon:abv                3.8 ;
        bevon:container          container:500mlLongneck ;
        bevon:description        "\n    Velkopopovický Kozel Dark beer is brewed to the original recipe using a\n    special mix of dark malts, clean water from our own well close to the\n    brewery, and a selection of the best hops. The caramelized malt gives this\n    beer a unique ruby color and sweet flavor, thanks to which it is\n    appreciated and respected all over the world.\n    "@en ;
        bevon:fermentation_base  <http://dbpedia.org/resource/Barley> ;
        bevon:launch             "1874"^^xsd:gYear ;
        bevon:manufacturer       <http://dbpedia.org/resource/SABMiller> ;
        bevon:name               "Velkopopovický Kozel Dark"@en , "코젤 다크"@ko , "Velkopopovický Kozel Černý"@cs ;
        bevon:origin             <http://dbpedia.org/resource/Velké_Popovice> .

bevon:Lager  a              owl:Class ;
        rdfs:isDefinedBy    bevon: ;
        rdfs:seeAlso        <http://en.wikipedia.org/wiki/Lager> ;
        rdfs:subClassOf     bevon:Beer , pto:Lager ;
        dcterms:issued      "2013-07-04+09:00"^^xsd:date ;
        dcterms:modified    "2014-03-01+09:00"^^xsd:date ;
        status:term_status  "unstable"@en ;
        skos:definition     "\n    Lager is a type of beer that is fermented and conditioned at low\n    temperatures.\n    "@en ;
        skos:prefLabel      "Lager"@en , "라거"@ko .

bevon:manufacturer  a       owl:ObjectProperty ;
        rdfs:domain         bevon:Beverage ;
        rdfs:isDefinedBy    bevon: ;
        rdfs:range          foaf:Agent ;
        rdfs:subPropertyOf  gr:hasManufacturer ;
        dcterms:issued      "2013-07-04+09:00"^^xsd:date ;
        dcterms:modified    "2014-03-01+09:00"^^xsd:date ;
        status:term_status  "unstable"@en ;
        skos:definition     "\n    This property specifies the manufacturer of the beverage.\n    "@en ;
        skos:prefLabel      "manufacturer"@en , "제조사"@ko .

bevon:Vodka  a              owl:Class ;
        rdfs:comment        "\n    Vodka is made by the distillation of fermented substances such as grains,\n    potatoes, or sometimes fruits or sugar.\n    "@en ;
        rdfs:isDefinedBy    bevon: ;
        rdfs:seeAlso        <http://en.wikipedia.org/wiki/Vodka> ;
        rdfs:subClassOf     pto:Vodka , bevon:DistilledBeverage ;
        dcterms:issued      "2013-07-04+09:00"^^xsd:date ;
        dcterms:modified    "2014-03-01+09:00"^^xsd:date ;
        status:term_status  "testing"@en ;
        skos:definition     "\n    Vodka is a distilled beverage composed primarily of water and ethanol,\n    sometimes with traces of impurities and flavorings.\n    "@en ;
        skos:prefLabel      "보드카"@ko , "Vodka"@en , "водка"@ru , "Wódka"@pl .

bevon:FermentationBase
        a                   owl:Class ;
        rdfs:isDefinedBy    bevon: ;
        dcterms:issued      "2013-07-04+09:00"^^xsd:date ;
        dcterms:modified    "2014-03-01+09:00"^^xsd:date ;
        status:term_status  "unstable"@en ;
        skos:definition     "\n    A fruit or grain which provides the sugar for fermentation from which a\n    alcoholic beverage is made.\n    "@en ;
        skos:prefLabel      "발효 주재료"@ko , "Fermentation Base"@en .

bevon:brewery  a            owl:ObjectProperty ;
        rdfs:domain         bevon:Beer ;
        rdfs:isDefinedBy    bevon: ;
        rdfs:range          bevon:Brewery ;
        rdfs:seeAlso        <http://en.wikipedia.org/wiki/Brewery> ;
        dcterms:issued      "2013-07-04+09:00"^^xsd:date ;
        dcterms:modified    "2014-03-01+09:00"^^xsd:date ;
        status:term_status  "unstable"@en ;
        skos:definition     "\n    This property relates a beer to its brewery.\n    "@en ;
        skos:prefLabel      "양조장"@ko , "Brewery"@en .

container:500mlLongneck
        a               bevon:Longneck , owl:NamedIndividual ;
        bevon:volume    [ a                        gr:QuantitativeValueInteger ;
                          gr:hasUnitOfMeasurement  "MLT" ;
                          gr:hasValue              "500"^^xsd:int
                        ] ;
        skos:prefLabel  "500ml 긴목 맥주병"@ko , "500ml Longneck Bottle"@en .

bevon:Container  a          owl:Class ;
        rdfs:isDefinedBy    bevon: ;
        rdfs:seeAlso        <http://en.wikipedia.org/wiki/Container> ;
        rdfs:subClassOf     yago:Containers ;
        dcterms:issued      "2013-07-04+09:00"^^xsd:date ;
        dcterms:modified    "2014-03-01+09:00"^^xsd:date ;
        status:term_status  "unstable"@en ;
        skos:definition     "\n    A container is an item used to contain, store, and transport a beverage.\n    "@en ;
        skos:prefLabel      "Container"@en , "용기"@ko .

beverage:Smithwicks  a           owl:NamedIndividual , gr:ProductOrServiceModel , bevon:IrishRedAle ;
        rdfs:seeAlso             <http://en.wikipedia.org/wiki/Smithwick%27s> ;
        bevon:abv                3.8 ;
        bevon:color              [ a              dbpedia:Colour ;
                                   dcterms:title  "Ruby Red"@en ;
                                   owl:sameAs     <http://purl.org/colors/rgb/9B111E> , <http://dbpedia.org/resource/Ruby_(color)__Ruby_Red__1>
                                 ] ;
        bevon:container          container:330mlLongneck , container:30lBeerKeg , container:440mlBeverageCan ;
        bevon:description        "\n    Smithwick's is an Irish red ale style beer from Kilkenny, Ireland. It is a\n    clear beer with a rich ruby color and creamy head.\n    "@en ;
        bevon:fermentation_base  <http://dbpedia.org/resource/Barley> ;
        bevon:ibu                "20"^^xsd:nonNegativeInteger ;
        bevon:launch             "1710"^^xsd:gYear ;
        bevon:manufacturer       <http://dbpedia.org/resource/Diageo> ;
        bevon:name               "Smithwick's Superior Irish Ale"@en , "스미딕스 슈페리어 아이리쉬 에일"@ko ;
        bevon:origin             <http://dbpedia.org/resource/Kilkenny> ;
        bevon:similar            beverage:Kilkenny ;
        bevon:srm                "14"^^xsd:nonNegativeInteger ;
        owl:sameAs               <http://dbpedia.org/resource/Smithwick%27s> .

bevon:Highball  a           owl:Class ;
        rdfs:isDefinedBy    bevon: ;
        rdfs:seeAlso        <http://en.wikipedia.org/wiki/Highball> ;
        rdfs:subClassOf     bevon:Cocktail , pto:Highball ;
        dcterms:issued      "2013-07-04+09:00"^^xsd:date ;
        dcterms:modified    "2014-03-01+09:00"^^xsd:date ;
        status:term_status  "unstable"@en ;
        skos:definition     "\n    Highball is the name for a family of mixed drinks that are composed of an\n    alcoholic base spirit and a larger proportion of a non-alcoholic mixer.\n    "@en ;
        skos:prefLabel      "하이볼"@ko , "Highball"@en .

bevon:non_alcoholic_version
        a                   owl:ObjectProperty ;
        rdfs:domain         bevon:AlcoholicBeverage ;
        rdfs:isDefinedBy    bevon: ;
        rdfs:range          bevon:NonAlcoholicBeverage ;
        rdfs:subPropertyOf  bevon:related ;
        dcterms:issued      "2013-07-04+09:00"^^xsd:date ;
        dcterms:modified    "2014-03-01+09:00"^^xsd:date ;
        status:term_status  "unstable"@en ;
        skos:definition     "\n    Some alcoholic beverages have non-alcoholic versions, such as non-alcoholic\n    beer (\"near beer\") and cocktails (\"mocktails\").\n    "@en ;
        skos:prefLabel      "non-alcoholic version"@en , "비알코올 버전"@ko .

container:330mlBeverageCan
        a               bevon:BeverageCan , owl:NamedIndividual ;
        bevon:volume    [ a                        gr:QuantitativeValueInteger ;
                          gr:hasUnitOfMeasurement  "MLT" ;
                          gr:hasValue              "330"^^xsd:int
                        ] ;
        skos:prefLabel  "330ml 음료 캔"@ko , "330ml Beverage Can"@en .

bevon:MineralWater  a       owl:Class ;
        rdfs:comment        "\n    Mineral water may be sparkling due to contained gases.\n    "@en ;
        rdfs:isDefinedBy    bevon: ;
        rdfs:seeAlso        <http://en.wikipedia.org/wiki/Mineral_water> ;
        rdfs:subClassOf     bevon:Water , pto:Mineral_water ;
        dcterms:issued      "2013-07-04+09:00"^^xsd:date ;
        dcterms:modified    "2014-03-01+09:00"^^xsd:date ;
        status:term_status  "unstable"@en ;
        skos:definition     "\n    Mineral water is water from a mineral spring containing various minerals\n    such as salts and sulfur compounds.\n    "@en ;
        skos:prefLabel      "광천수"@ko , "Mineral Water"@en .

container:360mlGlassBottle
        a               bevon:GlassBottle , owl:NamedIndividual ;
        bevon:volume    [ a                        gr:QuantitativeValueInteger ;
                          gr:hasUnitOfMeasurement  "MLT" ;
                          gr:hasValue              "360"^^xsd:int
                        ] ;
        skos:prefLabel  "360ml 유리병"@ko , "360ml Glass Bottle"@en .

bevon:ScotchWhisky  a       owl:Class ;
        rdfs:comment        "\n    All Scotch whisky was originally made from malt barley. Commercial\n    distilleries began introducing whisky made from wheat and rye in the late\n    eighteenth century.\n    "@en ;
        rdfs:isDefinedBy    bevon: ;
        rdfs:seeAlso        <http://en.wikipedia.org/wiki/Scotch_whisky> ;
        rdfs:subClassOf     bevon:Whisky , pto:Scotch_whisky ;
        dcterms:issued      "2013-07-04+09:00"^^xsd:date ;
        dcterms:modified    "2014-03-01+09:00"^^xsd:date ;
        status:term_status  "unstable"@en ;
        skos:altLabel       "Scotch Whiskey"@en ;
        skos:definition     "\n    Scotch whisky (often referred to simply as \"Scotch\") is malt whisky or grain\n    whisky made in Scotland.\n    "@en ;
        skos:prefLabel      "Scotch Whisky"@en , "스카치 위스키"@ko .

bevon:BeerCocktail  a       owl:Class ;
        rdfs:isDefinedBy    bevon: ;
        rdfs:seeAlso        <http://en.wikipedia.org/wiki/Beer_cocktail> ;
        rdfs:subClassOf     bevon:Cocktail , pto:Beer_cocktail ;
        dcterms:issued      "2013-07-04+09:00"^^xsd:date ;
        dcterms:modified    "2014-03-01+09:00"^^xsd:date ;
        status:term_status  "unstable"@en ;
        skos:definition     "\n    A beer cocktail is a cocktail that is made by mixing beer with a distilled\n    beverage. In this type of cocktail, the primary ingredient is beer.\n    "@en ;
        skos:prefLabel      "Beer Cocktail"@en , "맥주 칵테일"@ko .

beverage:Budweiser  a            gr:ProductOrServiceModel , bevon:PaleLager , owl:NamedIndividual ;
        rdfs:seeAlso             <https://en.wikipedia.org/wiki/Budweiser_(Anheuser-Busch)> ;
        bevon:abv                "5"^^xsd:decimal ;
        bevon:container          container:330mlLongneck , container:500mlBeverageCan , container:355mlBeverageCan ;
        bevon:description        "\n    Budweiser is a pale lager produced by Anheuser–Busch InBev. Introduced in\n    1876 by Adolphus Busch it has grown to become one of the highest selling\n    beers in the United States, and is available in over 80 markets worldwide.\n    "@en ;
        bevon:fermentation_base  <http://dbpedia.org/resource/Barley> ;
        bevon:ibu                "12"^^xsd:nonNegativeInteger ;
        bevon:launch             "1876"^^xsd:gYear ;
        bevon:manufacturer       <http://dbpedia.org/resource/Anheuser–Busch_InBev> ;
        bevon:name               "버드와이저"@ko , "Budweiser"@en ;
        bevon:origin             <http://dbpedia.org/resource/United_States> ;
        bevon:srm                "3"^^xsd:nonNegativeInteger .

bevon:launch  a             owl:DatatypeProperty ;
        rdfs:domain         bevon:Beverage ;
        rdfs:isDefinedBy    bevon: ;
        rdfs:range          xsd:gYear ;
        dcterms:issued      "2013-07-04+09:00"^^xsd:date ;
        dcterms:modified    "2014-03-01+09:00"^^xsd:date ;
        status:term_status  "unstable"@en ;
        skos:definition     "\n    This property specifies the year when the beverage was first introduced to\n    the market.\n    "@en ;
        skos:prefLabel      "launch"@en , "출시년도"@ko .

container:355mlBeverageCan
        a               bevon:BeverageCan , owl:NamedIndividual ;
        bevon:volume    [ a                        gr:QuantitativeValueInteger ;
                          gr:hasUnitOfMeasurement  "MLT" ;
                          gr:hasValue              "355"^^xsd:int
                        ] ;
        skos:prefLabel  "355ml 음료 캔"@ko , "355ml Beverage Can"@en .

container:25lBeerKeg  a  bevon:BeerKeg , owl:NamedIndividual ;
        bevon:volume    [ a                        gr:QuantitativeValueInteger ;
                          gr:hasUnitOfMeasurement  "LTR" ;
                          gr:hasValue              "25"^^xsd:int
                        ] ;
        skos:prefLabel  "25l 맥주 케그"@ko , "25l Beer Keg"@en .

container:1_8lPlasticBottle
        a               bevon:PlasticBottle , owl:NamedIndividual ;
        bevon:volume    [ a                        gr:QuantitativeValueFloat ;
                          gr:hasUnitOfMeasurement  "LTR" ;
                          gr:hasValue              "1.8"^^xsd:float
                        ] ;
        skos:prefLabel  "1.8l 플라스틱 병"@ko , "1.8l Plastic Bottle"@en .

beverage:Guinness  a             owl:NamedIndividual , gr:ProductOrServiceModel , bevon:DryStout ;
        rdfs:seeAlso             <http://en.wikipedia.org/wiki/Guinness> ;
        bevon:abv                4.2 ;
        bevon:container          container:15lBeerKeg , container:330mlLongneck , container:30lBeerKeg , container:330mlBeverageCan ;
        bevon:description        "\n    Guinness is a popular Irish dry stout that originated in the brewery of\n    Arthur Guinness (1725–1803) at St. James's Gate, Dublin. Guinness is one\n    of the most successful beer brands worldwide.\n    "@en ;
        bevon:fermentation_base  <http://dbpedia.org/resource/Barley> ;
        bevon:ibu                "37"^^xsd:nonNegativeInteger ;
        bevon:launch             "1759"^^xsd:gYear ;
        bevon:manufacturer       <http://dbpedia.org/resource/Diageo> ;
        bevon:name               "기네스 드래프트"@ko , "Guinness Draught"@en ;
        bevon:origin             <http://dbpedia.org/resource/Dublin> ;
        bevon:srm                "32"^^xsd:nonNegativeInteger ;
        owl:sameAs               <http://dbpedia.org/resource/Guinness> .

bevon:Cocktail  a           owl:Class ;
        rdfs:comment        "\n    Cocktails were originally a mixture of spirits, sugar, water, and bitters.\n    It is now often used for almost any mixed drink that contains alcohol,\n    including mixers, mixed shots, etc. A cocktail today usually contains one\n    or more kinds of spirit and one or more mixers, such as soda or fruit juice.\n    Additional ingredients may be sugar, honey, milk, cream, and various herbs.\n    "@en ;
        rdfs:isDefinedBy    bevon: ;
        rdfs:seeAlso        <http://en.wikipedia.org/wiki/Cocktail> ;
        rdfs:subClassOf     bevon:MixedDrink , pto:Cocktail , bevon:AlcoholicBeverage ;
        dcterms:issued      "2013-07-04+09:00"^^xsd:date ;
        dcterms:modified    "2014-03-01+09:00"^^xsd:date ;
        owl:disjointWith    bevon:Mocktail ;
        status:term_status  "unstable"@en ;
        skos:definition     "\n    A cocktail is a mixed drink that contains alcohol, including mixers, mixed\n    shots, etc.\n    "@en ;
        skos:prefLabel      "칵테일"@ko , "Cocktail"@en .

bevon:Keg  a                owl:Class ;
        rdfs:isDefinedBy    bevon: ;
        rdfs:seeAlso        <http://en.wikipedia.org/wiki/Keg> ;
        rdfs:subClassOf     bevon:Container ;
        dcterms:issued      "2013-07-04+09:00"^^xsd:date ;
        dcterms:modified    "2014-03-01+09:00"^^xsd:date ;
        status:term_status  "unstable"@en ;
        skos:definition     "\n    A keg is a small barrel.\n    "@en ;
        skos:prefLabel      "Keg"@en , "케그"@ko .

bevon:Liqueur  a            owl:Class ;
        rdfs:comment        "\n    Liqueurs are typically quite sweet; they are usually not aged for long\n    after the ingredients are mixed, but may have resting periods during their\n    production to allow flavors to marry.\n    "@en ;
        rdfs:isDefinedBy    bevon: ;
        rdfs:seeAlso        <http://en.wikipedia.org/wiki/Liqueur> ;
        rdfs:subClassOf     pto:Liqueur , bevon:DistilledBeverage ;
        dcterms:issued      "2013-07-04+09:00"^^xsd:date ;
        dcterms:modified    "2014-03-01+09:00"^^xsd:date ;
        status:term_status  "testing"@en ;
        skos:altLabel       "Cordials"@en , "Schnapps"@en ;
        skos:definition     "\n    A liqueur is an alcoholic beverage made from a distilled spirit that has\n    been flavored with fruit, cream, herbs, spices, flowers or nuts and bottled\n    with added sugar or other sweetener (such as high-fructose corn syrup).\n    "@en ;
        skos:prefLabel      "리큐어"@ko , "Liqueur"@en .

bevon:Soju  a               owl:Class ;
        rdfs:comment        "\n    Its taste is comparable to vodka, though often slightly sweeter due to\n    sugars added in the manufacturing process.\n    "@en ;
        rdfs:isDefinedBy    bevon: ;
        rdfs:seeAlso        <http://en.wikipedia.org/wiki/Soju> ;
        rdfs:subClassOf     pto:Soju , bevon:DistilledBeverage ;
        dcterms:issued      "2013-07-04+09:00"^^xsd:date ;
        dcterms:modified    "2014-03-01+09:00"^^xsd:date ;
        status:term_status  "testing"@en ;
        skos:definition     "\n    Soju is a distilled beverage native to Korea.\n    "@en ;
        skos:prefLabel      "Soju"@en , "소주"@ko .

container:500mlBeverageCan
        a               bevon:BeverageCan , owl:NamedIndividual ;
        bevon:volume    [ a                        gr:QuantitativeValueInteger ;
                          gr:hasUnitOfMeasurement  "MLT" ;
                          gr:hasValue              "500"^^xsd:int
                        ] ;
        skos:prefLabel  "500ml 음료 캔"@ko , "500ml Beverage Can"@en .

bevon:JapaneseWhisky  a     owl:Class ;
        rdfs:comment        "\n    Whisky production in Japan began around 1870, but the first commercial\n    production was in 1924 upon the opening of the country's first distillery,\n    Yamazaki. Broadly speaking the style of Japanese whisky is more similar to\n    that of Scotch whisky than Irish, American, or Canadian styles of whisky,\n    and thus the spelling typically follows the Scottish convention (omitting\n    the letter \"e\").\n    "@en ;
        rdfs:isDefinedBy    bevon: ;
        rdfs:seeAlso        <http://en.wikipedia.org/wiki/Japanese_whisky> ;
        rdfs:subClassOf     pto:Japanese_whisky , bevon:Whisky ;
        dcterms:issued      "2013-07-04+09:00"^^xsd:date ;
        dcterms:modified    "2014-03-01+09:00"^^xsd:date ;
        status:term_status  "unstable"@en ;
        skos:altLabel       "Japanese Whiskey"@en ;
        skos:definition     "\n    Japanese whisky is whisky made in Japan.\n    "@en ;
        skos:prefLabel      "재패니즈 위스키"@ko , "Japanese Whisky"@en .

beverage:Chum-Churum  a     bevon:DilutedSoju , gr:ProductOrServiceModel , owl:NamedIndividual ;
        rdfs:seeAlso        <http://ko.wikipedia.org/wiki/처음처럼_(주류)> ;
        bevon:abv           19.5 ;
        bevon:color         [ a              dbpedia:Colour ;
                              dcterms:title  "Clear"@en ;
                              owl:sameAs     <http://dbpedia.org/resource/Clear_(color)>
                            ] ;
        bevon:container     container:640mlPlasticBottle , container:200mlPlasticBottle , container:360mlGlassBottle , container:1_8lPlasticBottle , container:360mlPlasticBottle ;
        bevon:description   "\n    Chum-Churum is the diluted soju produced by Lotte Liquor.\n    "@en ;
        bevon:launch        "2006"^^xsd:gYear ;
        bevon:manufacturer  [ a              foaf:Organization ;
                              rdfs:seeAlso   <http://ko.wikipedia.org/wiki/롯데칠성음료> ;
                              foaf:homepage  <http://www.lotteliquor.com> ;
                              foaf:name      "롯데주류"@ko , "Lotte Liquor"@en
                            ] ;
        bevon:name          "Chum-Churum"@en , "처음처럼"@ko ;
        bevon:origin        <http://dbpedia.org/resource/South_Korea> ;
        owl:sameAs          <http://dbpedia.org/resource/Chum-Churum> .

bevon:DilutedSoju  a        owl:Class ;
        rdfs:isDefinedBy    bevon: ;
        rdfs:subClassOf     bevon:Soju ;
        dcterms:issued      "2013-07-04+09:00"^^xsd:date ;
        dcterms:modified    "2014-03-01+09:00"^^xsd:date ;
        owl:disjointWith    bevon:DistilledSoju ;
        status:term_status  "unstable"@en ;
        skos:definition     "\n    Diluted Soju is made by mixing pure ethanol distilled from various grains,\n    such as potatoes, wheat, barley, sweet potatoes, or tapioca, with water and\n    flavoring.\n    "@en ;
        skos:prefLabel      "Diluted Soju"@en , "희석식 소주"@ko .

bevon:CoreGroup  a    rdf:Bag ;
        rdf:_1        bevon:Beverage ;
        rdf:_10       bevon:Distillery ;
        rdf:_11       bevon:name ;
        rdf:_12       bevon:description ;
        rdf:_13       bevon:origin ;
        rdf:_14       bevon:manufacturer ;
        rdf:_15       bevon:color ;
        rdf:_16       bevon:launch ;
        rdf:_17       bevon:abv ;
        rdf:_18       bevon:proof ;
        rdf:_19       bevon:container ;
        rdf:_2        bevon:AlcoholicBeverage ;
        rdf:_20       bevon:aging ;
        rdf:_21       bevon:fermentation_base ;
        rdf:_22       bevon:distillery ;
        rdf:_23       bevon:ingredient ;
        rdf:_3        bevon:FermentedBeverage ;
        rdf:_4        bevon:DistilledBeverage ;
        rdf:_5        bevon:NonAlcoholicBeverage ;
        rdf:_6        bevon:MixedDrink ;
        rdf:_7        bevon:Container ;
        rdf:_8        bevon:Aging ;
        rdf:_9        bevon:FermentationBase ;
        rdfs:comment  "\n    These classes and properties form the core of BEVON. They describe\n    characteristics of beverages in relatively broad terms.\n    "@en ;
        rdfs:label    "Core Terms"@en .

bevon:CocktailGroup  a  rdf:Bag ;
        rdf:_1        bevon:Cocktail ;
        rdf:_2        bevon:Highball ;
        rdf:_3        bevon:BeerCocktail ;
        rdf:_4        bevon:Shandy ;
        rdf:_5        bevon:Mocktail ;
        rdfs:comment  "\n    These classes and properties are for describing beverages categorized under\n    Mixed Drink.\n    "@en ;
        rdfs:label    "Cocktail Terms"@en .

bevon:TequilaBlanco  a      owl:Class ;
        rdfs:isDefinedBy    bevon: ;
        rdfs:subClassOf     bevon:Tequila ;
        dcterms:issued      "2013-07-04+09:00"^^xsd:date ;
        dcterms:modified    "2014-03-01+09:00"^^xsd:date ;
        status:term_status  "unstable"@en ;
        skos:altLabel       "Tequila Plata"@en ;
        skos:definition     "\n    Tequila Blanco (\"white\") or Plata (\"silver\") is a white spirit, un-aged and\n    bottled or stored immediately after distillation, or aged less than two\n    months in stainless steel or neutral oak barrels.\n    "@en ;
        skos:prefLabel      "테킬라 블랑코"@ko , "Tequila Blanco"@en .

bevon:Aging  a              owl:Class ;
        rdfs:isDefinedBy    bevon: ;
        dcterms:issued      "2013-07-04+09:00"^^xsd:date ;
        dcterms:modified    "2014-03-01+09:00"^^xsd:date ;
        status:term_status  "unstable"@en ;
        skos:definition     "\n    Aging is the process of storing beverages in casks for a specific period of\n    time to remove harsh flavors and add distinct characteristics found in the\n    cask's wood.\n    "@en ;
        skos:prefLabel      "숙성"@ko , "Aging"@en .

bevon:description  a        owl:DatatypeProperty ;
        rdfs:domain         bevon:Beverage ;
        rdfs:isDefinedBy    bevon: ;
        rdfs:range          xsd:string ;
        rdfs:subPropertyOf  gr:description , dcterms:description ;
        dcterms:issued      "2013-07-04+09:00"^^xsd:date ;
        dcterms:modified    "2014-03-01+09:00"^^xsd:date ;
        status:term_status  "testing"@en ;
        skos:definition     "\n    This property specifies the short text description of the beverage.\n    "@en ;
        skos:prefLabel      "설명"@ko , "description"@en .

bevon:RelationGroup  a  rdf:Bag ;
        rdf:_1        bevon:related ;
        rdf:_2        bevon:similar ;
        rdf:_3        bevon:variant ;
        rdf:_4        bevon:variantOf ;
        rdf:_5        bevon:non_alcoholic_version ;
        rdfs:comment  "\n    These properties are used for describing relations between beverages.\n    "@en ;
        rdfs:label    "Relation Terms"@en .

bevon:Beer  a               owl:Class ;
        rdfs:comment        "\n    The starch and saccharification enzymes are often derived from malted cereal\n    grains, most commonly malted barley and malted wheat.\n    "@en ;
        rdfs:isDefinedBy    bevon: ;
        rdfs:seeAlso        <http://en.wikipedia.org/wiki/Beer> ;
        rdfs:subClassOf     bevon:FermentedBeverage , pto:Beer ;
        dcterms:issued      "2013-07-04+09:00"^^xsd:date ;
        dcterms:modified    "2014-03-01+09:00"^^xsd:date ;
        owl:disjointWith    bevon:NonAlcoholicBeer ;
        status:term_status  "testing"@en ;
        skos:definition     "\n    Beer is an alcoholic beverage produced by the saccharification of starch and\n    fermentation of the resulting sugar.\n    "@en ;
        skos:prefLabel      "맥주"@ko , "Beer"@en .

bevon:srm  a                owl:DatatypeProperty ;
        rdfs:domain         bevon:Beer ;
        rdfs:isDefinedBy    bevon: ;
        rdfs:range          xsd:nonNegativeInteger ;
        rdfs:seeAlso        <http://en.wikipedia.org/wiki/Standard_Reference_Method> ;
        dcterms:issued      "2013-07-04+09:00"^^xsd:date ;
        dcterms:modified    "2014-03-01+09:00"^^xsd:date ;
        status:term_status  "unstable"@en ;
        skos:altLabel       "Standard Reference Method"@en ;
        skos:definition     "\n    The Standard Reference Method or SRM is one of several systems modern\n    brewers use to specify beer color.\n    "@en ;
        skos:prefLabel      "SRM"@en .

whisky:Distillery  rdfs:subClassOf  bevon:Distillery .

bevon:fermentation_base
        a                   owl:ObjectProperty ;
        rdfs:domain         bevon:AlcoholicBeverage ;
        rdfs:isDefinedBy    bevon: ;
        rdfs:range          bevon:FermentationBase ;
        dcterms:issued      "2013-07-04+09:00"^^xsd:date ;
        dcterms:modified    "2014-03-01+09:00"^^xsd:date ;
        status:term_status  "unstable"@en ;
        skos:definition     "\n    This property indicates which fermentation base is used to make the\n    alcoholic beverage.\n    "@en ;
        skos:prefLabel      "발효 주재료"@ko , "fermentation base"@en .

bevon:Pilsner  a            owl:Class ;
        rdfs:comment        "\n    It took its name from the city of Pilsen (Plzeň, Bohemia, Czech Republic,\n    where it was first produced in 1842).\n    "@en ;
        rdfs:isDefinedBy    bevon: ;
        rdfs:seeAlso        <http://en.wikipedia.org/wiki/Pilsner> ;
        rdfs:subClassOf     pto:Pilsner , bevon:PaleLager ;
        dcterms:issued      "2013-07-04+09:00"^^xsd:date ;
        dcterms:modified    "2014-03-01+09:00"^^xsd:date ;
        status:term_status  "unstable"@en ;
        skos:altLabel       "Pilsener"@en , "Pils"@en ;
        skos:definition     "\n    Pilsner (also pilsener or simply pils) is a type of pale lager.\n    "@en ;
        skos:prefLabel      "필스너"@ko , "Pilsner"@en .

bevon:Distillery  a         owl:Class ;
        rdfs:isDefinedBy    bevon: ;
        rdfs:seeAlso        <http://en.wikipedia.org/wiki/Distillation> ;
        dcterms:issued      "2013-07-04+09:00"^^xsd:date ;
        dcterms:modified    "2014-03-01+09:00"^^xsd:date ;
        status:term_status  "unstable"@en ;
        skos:definition     "\n    A distillery is a premise where distillation takes place, especially\n    distillation of alcohol.\n    "@en ;
        skos:prefLabel      "증류소"@ko , "Distillery"@en .

container:750mlGlassBottle
        a               bevon:GlassBottle , owl:NamedIndividual ;
        bevon:volume    [ a                        gr:QuantitativeValueInteger ;
                          gr:hasUnitOfMeasurement  "MLT" ;
                          gr:hasValue              "750"^^xsd:int
                        ] ;
        skos:altLabel   "75cl Glass Bottle"@en ;
        skos:prefLabel  "750ml 유리병"@ko , "750ml Glass Bottle"@en .

container:440mlBeverageCan
        a               bevon:BeverageCan , owl:NamedIndividual ;
        bevon:volume    [ a                        gr:QuantitativeValueInteger ;
                          gr:hasUnitOfMeasurement  "MLT" ;
                          gr:hasValue              "440"^^xsd:int
                        ] ;
        skos:prefLabel  "440ml 음료 캔"@ko , "440ml Beverage Can"@en .

container:640mlPlasticBottle
        a               bevon:PlasticBottle , owl:NamedIndividual ;
        bevon:volume    [ a                        gr:QuantitativeValueInteger ;
                          gr:hasUnitOfMeasurement  "MLT" ;
                          gr:hasValue              "640"^^xsd:int
                        ] ;
        skos:prefLabel  "640ml 플라스틱 병"@ko , "640ml Plastic Bottle"@en .

bevon:Pisco  a              owl:Class ;
        rdfs:isDefinedBy    bevon: ;
        rdfs:seeAlso        <http://en.wikipedia.org/wiki/Pisco> ;
        rdfs:subClassOf     pto:Pisco , bevon:Brandy ;
        dcterms:issued      "2013-07-04+09:00"^^xsd:date ;
        dcterms:modified    "2014-03-01+09:00"^^xsd:date ;
        status:term_status  "testing"@en ;
        skos:definition     "\n    Pisco is a colorless or yellowish-to-amber colored grape brandy produced\n    in winemaking regions of Peru and Chile.\n    "@en ;
        skos:prefLabel      "Pisco"@en , "피스코"@ko .

bevon:CanadianWhisky  a     owl:Class ;
        rdfs:comment        "\n    Most Canadian whiskies are blended multi-grain liquors containing a large\n    percentage of corn spirits, and are typically lighter and smoother than\n    other whisky styles.\n    "@en ;
        rdfs:isDefinedBy    bevon: ;
        rdfs:seeAlso        <http://en.wikipedia.org/wiki/Canadian_whisky> ;
        rdfs:subClassOf     pto:Canadian_whisky , bevon:Whisky ;
        dcterms:issued      "2013-07-04+09:00"^^xsd:date ;
        dcterms:modified    "2014-03-01+09:00"^^xsd:date ;
        status:term_status  "unstable"@en ;
        skos:altLabel       "Canadian Whiskey"@en ;
        skos:definition     "\n    Canadian whisky is a type of whisky produced in Canada.\n    "@en ;
        skos:prefLabel      "캐내디언 위스키"@ko , "Canadian Whisky"@en .

bevon:BourbonWhiskey  a     owl:Class ;
        rdfs:comment        "\n    The name of the spirit derives from its historical association with an area\n    known as Old Bourbon, around what is now Bourbon County, Kentucky (which,\n    in turn, was named after the French House of Bourbon royal family). It has\n    been produced since the 18th century. While it may be made anywhere in the\n    United States, it is strongly associated with the American South in\n    general, and Kentucky in particular.\n    "@en ;
        rdfs:isDefinedBy    bevon: ;
        rdfs:seeAlso        <http://en.wikipedia.org/wiki/Bourbon_whiskey> ;
        rdfs:subClassOf     bevon:AmericanWhisky , pto:Bourbon_whiskey ;
        dcterms:issued      "2013-07-04+09:00"^^xsd:date ;
        dcterms:modified    "2014-03-01+09:00"^^xsd:date ;
        status:term_status  "unstable"@en ;
        skos:altLabel       "Bourbon Whisky"@en ;
        skos:definition     "\n    Bourbon whiskey is a type of American whiskey – a barrel-aged distilled\n    spirit made primarily from corn.\n    "@en ;
        skos:prefLabel      "버번 위스키"@ko , "Bourbon Whiskey"@en .

bevon:Longneck  a           owl:Class ;
        rdfs:comment        "\n    It is known as the standard longneck bottle or industry standard bottle\n    (ISB). The ISB longnecks have a uniform capacity, height, weight and\n    diameter and can be reused on average 16 times. The long neck offers a long\n    cushion of air to absorb the pressure of carbonation to reduce the risk of\n    exploding. The longneck also provides a handle for drinking directly from\n    the bottle without transferring body heat to the beer from one's hand.\n    "@en ;
        rdfs:isDefinedBy    bevon: ;
        rdfs:subClassOf     bevon:BeerBottle ;
        dcterms:issued      "2013-07-04+09:00"^^xsd:date ;
        dcterms:modified    "2014-03-01+09:00"^^xsd:date ;
        status:term_status  "unstable"@en ;
        skos:altLabel       "North American Longneck"@en , "Industry Standard Bottle"@en ;
        skos:definition     "\n    A longneck is a type of beer bottle with a long neck.\n    "@en ;
        skos:prefLabel      "긴목 맥주병"@ko , "Longneck"@en .

bevon:BeerGroup  a    rdf:Bag ;
        rdf:_1        bevon:Beer ;
        rdf:_10       bevon:PaleLager ;
        rdf:_11       bevon:Pilsner ;
        rdf:_12       bevon:NonAlcoholicBeer ;
        rdf:_13       bevon:Brewery ;
        rdf:_14       bevon:BeerBottle ;
        rdf:_15       bevon:Longneck ;
        rdf:_16       bevon:BeerKeg ;
        rdf:_17       bevon:ibu ;
        rdf:_18       bevon:srm ;
        rdf:_19       bevon:brewery ;
        rdf:_2        bevon:Ale ;
        rdf:_3        bevon:PaleAle ;
        rdf:_4        bevon:IrishRedAle ;
        rdf:_5        bevon:Porter ;
        rdf:_6        bevon:Stout ;
        rdf:_7        bevon:DryStout ;
        rdf:_8        bevon:Lager ;
        rdf:_9        bevon:Dunkel ;
        rdfs:comment  "\n    In addition to the BEVON core terms, there are a number of terms for use\n    when describing beverages categorized under Beer.\n    "@en ;
        rdfs:label    "Beer Terms"@en .

bevon:DistilledSoju  a      owl:Class ;
        rdfs:isDefinedBy    bevon: ;
        rdfs:subClassOf     bevon:Soju ;
        dcterms:issued      "2013-07-04+09:00"^^xsd:date ;
        dcterms:modified    "2014-03-01+09:00"^^xsd:date ;
        owl:disjointWith    bevon:DilutedSoju ;
        status:term_status  "unstable"@en ;
        skos:definition     "\n    Distilled Soju is manufactured traditionally by distillation from grains,\n    mainly rice.\n    "@en ;
        skos:prefLabel      "증류식 소주"@ko , "Distilled Soju"@en .

beverage:Glenfiddich12YearOld
        a                        bevon:SpeysideSingleMalt , gr:ProductOrServiceModel , owl:NamedIndividual ;
        bevon:abv                "40"^^xsd:decimal ;
        bevon:aging              [ a                       bevon:Aging ;
                                   bevon:duration          [ a           time:DurationDescription ;
                                                             time:years  "12"^^xsd:decimal
                                                           ] ;
                                   bevon:material          <http://dbpedia.org/resource/Oak> ;
                                   bevon:previous_content  <http://dbpedia.org/resource/Sherry> , <http://dbpedia.org/resource/Bourbon_whiskey>
                                 ] ;
        bevon:color              [ a              dbpedia:Colour ;
                                   dcterms:title  "Gold"@en ;
                                   owl:sameAs     <http://purl.org/colors/rgb/FFD700> , <http://dbpedia.org/resource/Gold_(color)>
                                 ] ;
        bevon:container          container:700mlGlassBottle ;
        bevon:description        "\n    Carefully matured in the finest American bourbon and Spanish sherry oak\n    casks for at least 12 years. Married and mellowed in oak marrying tuns for\n    complete harmony of aroma and flavor.\n\n    A single malt Scotch whisky with distinctive fresh pear, creamy with subtle\n    oak flavors and a long smooth and mellow finish.\n    "@en ;
        bevon:distillery         [ a                   bevon:Distillery ;
                                   whisky:owner        <http://dbpedia.org/resource/William_Grant_%26_Sons> ;
                                   whisky:region       <http://dbpedia.org/resource/Strathspey,_Scotland> ;
                                   whisky:waterSource  [ a              whisky:WaterSource ;
                                                         dcterms:title  "로비 듀 수원지"@ko , "Robbie Dhu Springs"@en
                                                       ] ;
                                   owl:sameAs          <http://dbpedia.org/resource/Glenfiddich_distillery>
                                 ] ;
        bevon:fermentation_base  <http://dbpedia.org/resource/Barley> ;
        bevon:launch             "1887"^^xsd:gYear ;
        bevon:manufacturer       <http://dbpedia.org/resource/William_Grant_%26_Sons> ;
        bevon:name               "Glenfiddich 12 Year Old"@en , "글렌피딕 12년"@ko ;
        bevon:origin             <http://dbpedia.org/resource/Strathspey,_Scotland> .

beverage:Tsingtao  a             owl:NamedIndividual , gr:ProductOrServiceModel , bevon:Pilsner ;
        bevon:abv                4.7 ;
        bevon:brewery            <http://dbpedia.org/resource/Tsingtao_Brewery> ;
        bevon:container          container:330mlLongneck , container:500mlBeverageCan , container:355mlBeverageCan , container:640mlLongneck ;
        bevon:description        "\n    Tsingtao Lager, a well-hopped standard pilsner of 4.7% alcohol, is the\n    flagship brew, accounting for most of the brewery's production.\n    "@en ;
        bevon:fermentation_base  <http://dbpedia.org/resource/Barley> ;
        bevon:ibu                "20"^^xsd:nonNegativeInteger ;
        bevon:launch             "1904"^^xsd:gYear ;
        bevon:manufacturer       <http://dbpedia.org/resource/Tsingtao_Brewery> ;
        bevon:name               "칭타오 라거"@ko , "Tsingtao Lager"@en ;
        bevon:origin             <http://dbpedia.org/resource/Qingdao> ;
        bevon:srm                "4"^^xsd:nonNegativeInteger .

bevon:Brandy  a             owl:Class ;
        rdfs:comment        "\n    Brandy generally contains 35–60% alcohol by volume (70–120 US proof) and is\n    typically taken as an after-dinner drink. Some brandies are aged in wooden\n    casks, some are colored with caramel coloring to imitate the effect of\n    aging, and some brandies are produced using a combination of both aging and\n    coloring.\n    "@en ;
        rdfs:isDefinedBy    bevon: ;
        rdfs:seeAlso        <http://en.wikipedia.org/wiki/Brandy> ;
        rdfs:subClassOf     pto:Brandy , bevon:DistilledBeverage ;
        dcterms:issued      "2013-07-04+09:00"^^xsd:date ;
        dcterms:modified    "2014-03-01+09:00"^^xsd:date ;
        status:term_status  "testing"@en ;
        skos:definition     "\n    Brandy (from brandywine, derived from Dutch brandewijn—\"burnt wine\") is a\n    spirit produced by distilling wine.\n    "@en ;
        skos:prefLabel      "Brandy"@en , "브랜디"@ko .

bevon:SingleMaltWhisky
        a                   owl:Class ;
        rdfs:isDefinedBy    bevon: ;
        rdfs:seeAlso        <http://en.wikipedia.org/wiki/Single_malt_whisky> ;
        rdfs:subClassOf     pto:Single_malt_whisky , bevon:MaltWhisky ;
        dcterms:issued      "2013-07-04+09:00"^^xsd:date ;
        dcterms:modified    "2014-03-01+09:00"^^xsd:date ;
        status:term_status  "unstable"@en ;
        skos:altLabel       "Single Malt Whiskey"@en ;
        skos:definition     "\n    Single malt whisky is a whisky made at one particular distillery from a\n    mash that uses only malted grain, ordinarily barley.\n    "@en ;
        skos:prefLabel      "싱글 몰트 위스키"@ko , "Single Malt Whisky"@en .

bevon:PaleAle  a            owl:Class ;
        rdfs:comment        "\n    It is one of the world's major beer styles.\n    "@en ;
        rdfs:isDefinedBy    bevon: ;
        rdfs:seeAlso        <http://en.wikipedia.org/wiki/Pale_ale> ;
        rdfs:subClassOf     bevon:Ale , pto:Pale_ale ;
        dcterms:issued      "2013-07-04+09:00"^^xsd:date ;
        dcterms:modified    "2014-03-01+09:00"^^xsd:date ;
        status:term_status  "unstable"@en ;
        skos:definition     "\n    Pale ale is a beer made by warm fermentation using predominantly pale malt.\n    "@en ;
        skos:prefLabel      "페일 에일"@ko , "Pale Ale"@en .

container:360mlPlasticBottle
        a               bevon:PlasticBottle , owl:NamedIndividual ;
        bevon:volume    [ a                        gr:QuantitativeValueInteger ;
                          gr:hasUnitOfMeasurement  "MLT" ;
                          gr:hasValue              "360"^^xsd:int
                        ] ;
        skos:prefLabel  "360ml 플라스틱 병"@ko , "360ml Plastic Bottle"@en .

bevon:duration  a           owl:ObjectProperty ;
        rdfs:domain         bevon:Aging ;
        rdfs:isDefinedBy    bevon: ;
        rdfs:range          time:DurationDescription ;
        rdfs:subPropertyOf  time:hasDurationDescription ;
        dcterms:issued      "2013-07-04+09:00"^^xsd:date ;
        dcterms:modified    "2014-03-01+09:00"^^xsd:date ;
        status:term_status  "unstable"@en ;
        skos:definition     "\n    This property describes how long the beverage was aged in the cask.\n    "@en ;
        skos:prefLabel      "duration"@en , "기간"@ko .

container:200mlPlasticBottle
        a               bevon:PlasticBottle , owl:NamedIndividual ;
        bevon:volume    [ a                        gr:QuantitativeValueInteger ;
                          gr:hasUnitOfMeasurement  "MLT" ;
                          gr:hasValue              "200"^^xsd:int
                        ] ;
        skos:prefLabel  "200ml 플라스틱 병"@ko , "200ml Plastic Bottle"@en .

bevon:Shandy  a             owl:Class ;
        rdfs:comment        "\n    The proportions of the two ingredients are adjusted to taste, usually\n    half-and-half.\n    "@en ;
        rdfs:isDefinedBy    bevon: ;
        rdfs:seeAlso        <http://en.wikipedia.org/wiki/Shandy> ;
        rdfs:subClassOf     pto:Shandy , bevon:Cocktail ;
        dcterms:issued      "2013-07-04+09:00"^^xsd:date ;
        dcterms:modified    "2014-03-01+09:00"^^xsd:date ;
        status:term_status  "unstable"@en ;
        skos:definition     "\n    A shandy, or shandygaff, is beer mixed with a soft drink, carbonated\n    lemonade, ginger beer, ginger ale, or apple juice.\n    "@en ;
        skos:prefLabel      "Shandy"@en , "섄디"@ko .

bevon:variant  a            owl:ObjectProperty ;
        rdfs:domain         bevon:Beverage ;
        rdfs:isDefinedBy    bevon: ;
        rdfs:range          bevon:Beverage ;
        rdfs:subPropertyOf  bevon:related ;
        dcterms:issued      "2013-07-04+09:00"^^xsd:date ;
        dcterms:modified    "2014-03-01+09:00"^^xsd:date ;
        owl:inverseOf       bevon:variantOf ;
        status:term_status  "unstable"@en ;
        skos:definition     "\n    This property states that a beverage has a variant.\n    "@en ;
        skos:prefLabel      "variant"@en , "변형"@ko .

bevon:aging  a              owl:ObjectProperty ;
        rdfs:domain         bevon:AlcoholicBeverage ;
        rdfs:isDefinedBy    bevon: ;
        rdfs:range          bevon:Aging ;
        dcterms:issued      "2013-07-04+09:00"^^xsd:date ;
        dcterms:modified    "2014-03-01+09:00"^^xsd:date ;
        status:term_status  "unstable"@en ;
        skos:definition     "\n    This property specifies how the beverage has been aged.\n    "@en ;
        skos:prefLabel      "숙성"@ko , "aging"@en .

bevon:AmericanWhiskey
        a                   owl:Class ;
        rdfs:comment        "\n    The production and labeling of American whiskey are governed by Title 27 of\n    the U.S. Code of Federal Regulations.\n    "@en ;
        rdfs:isDefinedBy    bevon: ;
        rdfs:seeAlso        <http://en.wikipedia.org/wiki/American_whiskey> ;
        rdfs:subClassOf     pto:American_whiskey , bevon:Whisky ;
        dcterms:issued      "2013-07-04+09:00"^^xsd:date ;
        dcterms:modified    "2014-03-01+09:00"^^xsd:date ;
        status:term_status  "unstable"@en ;
        skos:altLabel       "American Whisky"@en ;
        skos:definition     "\n    American whiskey is a distilled beverage produced in the United States from\n    a fermented mash of cereal grain.\n    "@en ;
        skos:prefLabel      "American Whiskey"@en , "아메리칸 위스키"@ko .

bevon:NonAlcoholicBeer
        a                   owl:Class ;
        rdfs:isDefinedBy    bevon: ;
        rdfs:seeAlso        <http://en.wikipedia.org/wiki/Low-alcohol_beer> ;
        rdfs:subClassOf     pto:Low-alcohol_beer , bevon:NonAlcoholicBeverage ;
        dcterms:issued      "2013-07-04+09:00"^^xsd:date ;
        dcterms:modified    "2014-03-01+09:00"^^xsd:date ;
        owl:disjointWith    bevon:Beer ;
        status:term_status  "unstable"@en ;
        skos:altLabel       "Low-alcoholic Beer"@en ;
        skos:definition     "\n    Non-alcohol beer (also called light beer, low-alcoholic beer, small beer,\n    small ale, or near-beer) is beer with low alcohol content or no alcohol,\n    which aim to reproduce the taste of beer without the inebriating effects of\n    standard alcoholic brews.\n    "@en ;
        skos:prefLabel      "Non-alcoholic Beer"@en , "비알코올 맥주"@ko .

bevon:distillery  a         owl:ObjectProperty ;
        rdfs:domain         bevon:DistilledBeverage ;
        rdfs:isDefinedBy    bevon: ;
        rdfs:range          bevon:Distillery ;
        rdfs:seeAlso        <http://en.wikipedia.org/wiki/Distillation> ;
        dcterms:issued      "2013-07-04+09:00"^^xsd:date ;
        dcterms:modified    "2014-03-01+09:00"^^xsd:date ;
        status:term_status  "unstable"@en ;
        skos:definition     "\n    This property relates a distilled beverage to its distillery.\n    "@en ;
        skos:prefLabel      "증류소"@ko , "Distillery"@en .

bevon:Brewery  a            owl:Class ;
        rdfs:comment        "\n    A company that makes beer is called either a brewery or a brewing company.\n    "@en ;
        rdfs:isDefinedBy    bevon: ;
        rdfs:seeAlso        <http://en.wikipedia.org/wiki/Brewery> ;
        dcterms:issued      "2013-07-04+09:00"^^xsd:date ;
        dcterms:modified    "2014-03-01+09:00"^^xsd:date ;
        status:term_status  "unstable"@en ;
        skos:definition     "\n    A brewery is a dedicated building for the making of beer, though beer can\n    be made at home, and has been for much of beer's history.\n    "@en ;
        skos:prefLabel      "양조장"@ko , "Brewery"@en .

bevon:NonAlcoholicBeverage
        a                   owl:Class ;
        rdfs:isDefinedBy    bevon: ;
        rdfs:seeAlso        <http://en.wikipedia.org/wiki/Non-alcoholic_beverage> ;
        rdfs:subClassOf     bevon:Beverage , pto:Non-alcoholic_beverage ;
        dcterms:issued      "2013-07-04+09:00"^^xsd:date ;
        dcterms:modified    "2014-03-01+09:00"^^xsd:date ;
        owl:disjointWith    bevon:AlcoholicBeverage ;
        status:term_status  "testing"@en ;
        skos:definition     "\n     A non-alcoholic beverage (also known as a virgin drink) is defined\n     in the U.S. as a beverage that contains less than 0.5% alcohol by volume.\n     "@en ;
        skos:prefLabel      "Non-alcoholic Beverage"@en , "비알코올 음료"@ko .

bevon:BeerBottle  a         owl:Class ;
        rdfs:comment        "\n    Dark amber or brown glass greatly reduces UV light from spoiling the beer.\n    However, lighter colored bottles are often used for marketing reasons.\n    "@en ;
        rdfs:isDefinedBy    bevon: ;
        rdfs:seeAlso        <http://en.wikipedia.org/wiki/Beer_bottle> ;
        rdfs:subClassOf     bevon:GlassBottle ;
        dcterms:issued      "2013-07-04+09:00"^^xsd:date ;
        dcterms:modified    "2014-03-01+09:00"^^xsd:date ;
        status:term_status  "unstable"@en ;
        skos:definition     "\n    A beer bottle is a bottle made to contain beer, usually made of glass and\n    come in various sizes, shapes and colors.\n    "@en ;
        skos:prefLabel      "맥주병"@ko , "Beer Bottle"@en .
