@prefix voaf: <http://purl.org/vocommons/voaf#> .
@prefix rdfs: <http://www.w3.org/2000/01/rdf-schema#> .
@prefix foaf: <http://xmlns.com/foaf/0.1/> .
@prefix dct: <http://purl.org/dc/terms/> .
@prefix xsd: <http://www.w3.org/2001/XMLSchema#> .
@prefix owl: <http://www.w3.org/2002/07/owl#> .
@prefix vann: <http://purl.org/vocab/vann/> .
@prefix rdf: <http://www.w3.org/1999/02/22-rdf-syntax-ns#> .
@prefix oh: <http://semweb.mmlab.be/ns/oh#> .

<http://semweb.mmlab.be/ns/oh> a owl:Ontology , voaf:Vocabulary ;
	vann:preferredNamespacePrefix "oh" ;
	vann:preferredNamespaceUri <http://semweb.mmlab.be/ns/oh#> ;
	dct:description "A vocabulary to describe opening hours using calendars (recommended: iCal, RDFCal or schema.org) published on the Web." ;
	dct:title "The Opening Hours vocabulary"@en ;
	dct:issued "2013-12-05"^^xsd:date ;
	dct:modified "2014-06-16"^^xsd:date .

_:node18qove8qvx5 foaf:mbox "Pieter.Colpaert@UGent.be" ;
	foaf:name "Pieter Colpaert" .

<http://semweb.mmlab.be/ns/oh> dct:creator _:node18qove8qvx5 .

_:node18qove8qvx6 foaf:mbox "Laurens.DeVocht@UGent.be" ;
	foaf:name "Laurens De Vocht" .

<http://semweb.mmlab.be/ns/oh> dct:creator _:node18qove8qvx6 .

_:node18qove8qvx7 foaf:mbox "Anastasia.Dimou@UGent.be" ;
	foaf:name "Anastasia Dimou" .

<http://semweb.mmlab.be/ns/oh> dct:creator _:node18qove8qvx7 .

_:node18qove8qvx8 foaf:mbox "Steven.Verstockt@UGent.be" ;
	foaf:name "Steven Verstockt" .

<http://semweb.mmlab.be/ns/oh> dct:creator _:node18qove8qvx8 .

oh:OpeningHours a owl:Class ;
	rdfs:subClassOf owl:Thing ;
	rdfs:label "Opening Hours" ;
	rdfs:comment "A class to identify opening hours" ;
	rdfs:isDefinedBy <http://semweb.mmlab.be/ns/oh> .

oh:OpeningHoursType a owl:Class ;
	rdfs:subClassOf owl:Thing ;
	rdfs:label "Opening Hours Type" ;
	rdfs:comment "A class to identify the type of opening hours" ;
	rdfs:isDefinedBy <http://semweb.mmlab.be/ns/oh> .

oh:Calendar a owl:Class ;
	rdfs:subClassOf owl:Thing ;
	rdfs:label "A calendar" ;
	rdfs:comment "A calendar which can be used for opening hours" ;
	rdfs:isDefinedBy <http://semweb.mmlab.be/ns/oh> .

oh:calendar a owl:ObjectProperty ;
	rdfs:comment "A property to tell oh:OpeningHours to keep this calendar into account"@en ;
	rdfs:domain oh:Calendar ;
	rdfs:range rdf:List .

oh:type a owl:ObjectProperty ;
	rdfs:label "has Opening Hours Type" ;
	rdfs:comment "Give a type to an oh:OpeningHours instance"@en ;
	rdfs:domain oh:Calendar ;
	rdfs:range oh:OpeningHoursType .

oh:closinghours a owl:DatatypeProperty ;
	rdfs:label "Are Closing Hours" ;
	rdfs:comment "Tell whether or not this oh:Calendar specifies closing hours." ;
	rdfs:domain xsd:boolean ;
	rdfs:range oh:Calendar .
