@prefix dc:    <http://purl.org/dc/elements/1.1/> .
@prefix rdfs:  <http://www.w3.org/2000/01/rdf-schema#> .
@prefix foaf:  <http://xmlns.com/foaf/0.1/> .
@prefix dm2e:  <http://onto.dm2e.eu/schemas/dm2e/> .
@prefix owl:   <http://www.w3.org/2002/07/owl#> .
@prefix xsd:   <http://www.w3.org/2001/XMLSchema#> .
@prefix rdf:   <http://www.w3.org/1999/02/22-rdf-syntax-ns#> .
@prefix vann:  <http://purl.org/vocab/vann/> .
@prefix dcterms: <http://purl.org/dc/terms/> .

dm2e:Page  a          owl:Class , rdfs:Class ;
        rdfs:comment  "One side of a sheet of paper. Can be part of another CHO, e.g. dm2e:Manuscript." ;
        rdfs:label    "Page" .

dm2e:support  a             rdf:Property ;
        rdfs:label          "support" ;
        rdfs:subPropertyOf  dc:description .

dm2e:callNumber  a          owl:DatatypeProperty , rdf:Property ;
        rdfs:label          "callNumber" ;
        rdfs:range          rdfs:Literal ;
        rdfs:subPropertyOf  dc:identifier .

dm2e:holdingInstitution
        a           rdf:Property ;
        rdfs:label  "holdingInstitution" ;
        rdfs:range  foaf:Organization .

<http://onto.dm2e.eu/schemas/dm2e#ttl>
        dcterms:FileFormat  <http://onto.dm2e.eu/schemas/dm2e> .

dm2e:DataResource  a     owl:Class , rdfs:Class ;
        rdfs:comment     "The dataset that contains the RDF statements provided in via this data resource." ;
        rdfs:label       "DataResource" ;
        rdfs:subClassOf  foaf:Document .

dm2e:scopeNote  a     rdf:Property ;
        rdfs:comment  "This property describes the dm2e-specific usage of the resource." ;
        rdfs:label    "scopeNote" .

dm2e:cover  a               rdf:Property ;
        rdfs:label          "cover" ;
        rdfs:subPropertyOf  dc:description .

dm2e:Poster  a        owl:Class , rdfs:Class ;
        rdfs:comment  "ProvidedCHO of type poster. Basically any piece of printed paper (often on a large sheet) that can be attached to a wall. dm2e:Poster does also include, but is not restricted to, conference posters." ;
        rdfs:label    "Poster" .

dm2e:Collection  a    owl:Class , rdfs:Class ;
        rdfs:comment  "The collection of CHOs as provided by a data provider." ;
        rdfs:label    "Collection" .

dm2e:Document  a      owl:Class , rdfs:Class ;
        rdfs:comment  "ProvidedCHO of type document. Unlike foaf:Document, dm2e:Document refers to a physical document." ;
        rdfs:label    "Document" .

dm2e:artist  a              rdf:Property ;
        rdfs:label          "artist" ;
        rdfs:range          foaf:Person ;
        rdfs:subPropertyOf  dc:creator .

dm2e:writer  a              rdf:Property ;
        rdfs:label          "writer" ;
        rdfs:range          foaf:Person ;
        rdfs:subPropertyOf  dc:creator .

dm2e:subtitle  a            owl:DatatypeProperty , rdf:Property ;
        rdfs:label          "subtitle" ;
        rdfs:range          rdfs:Literal ;
        rdfs:subPropertyOf  dc:title .

dm2e:sponsor  a     rdf:Property ;
        rdfs:label  "sponsor" .

dm2e:principal  a   rdf:Property ;
        rdfs:label  "principal" .

dm2e:explicit  a            owl:DatatypeProperty , rdf:Property ;
        rdfs:comment        "Final words of a manuscript. A language tag in ISO 639-2 should be added to the Literal." ;
        rdfs:label          "explicit" ;
        rdfs:range          rdfs:Literal ;
        rdfs:subPropertyOf  dc:description .

<http://onto.dm2e.eu/schemas/dm2e>
        a                              owl:Ontology ;
        dc:creator                     <http://onto.dm2e.eu/schemas/dm2e#s.hennicke> , <http://onto.dm2e.eu/schemas/dm2e#JIwanowa> , <http://onto.dm2e.eu/schemas/dm2e#Evelyn> , <http://onto.dm2e.eu/schemas/dm2e#konstantin> ;
        dcterms:created                "2015-01-20"^^xsd:date ;
        dcterms:description            "The DM2E model is a specialisation of the Europeana Data Model (EDM) and can be used for the description of manuscripts in the cultural heritage domain." ;
        dcterms:modified               "2015-01-20"^^xsd:date ;
        dcterms:partOf                 <http://onto.dm2e.eu> ;
        dcterms:publisher              "http://onto.dm2e.eu/schemas/dm2e#School%20for%20Library%20and%20Information%20Science" ;
        dcterms:status                 <http://purl.org/adms/status/UnderDevelopment> ;
        dcterms:title                  "DM2E model" ;
        dcterms:type                   <http://purl.org/adms/assettype/Ontology> ;
        vann:preferredNamespacePrefix  "dm2e" ;
        vann:preferredNamespaceUri     "http://onto.dm2e.eu/schemas/dm2e/" ;
        foaf:homepage                  <http://onto.dm2e.eu/schemas/dm2e.html> .

dm2e:levelOfHierarchy
        a           rdf:Property ;
        rdfs:label  "levelOfHierarchy" .

<http://onto.dm2e.eu/schemas/dm2e#Evelyn>
        a              foaf:Person ;
        foaf:homepage  <http://onto.dm2e.eu/schemas/dm2e> ;
        foaf:name      "Evelyn Dr√∂ge" .

dm2e:printedAt  a           rdf:Property ;
        rdfs:label          "printed at" ;
        rdfs:subPropertyOf  dcterms:spatial .

dm2e:shelfmarkLocation
        a                   owl:DatatypeProperty , rdf:Property ;
        rdfs:label          "shelfmarkLocation" ;
        rdfs:range          rdfs:Literal ;
        rdfs:subPropertyOf  dc:description .

dm2e:hasAnnotatableVersionAt
        a           rdf:Property ;
        rdfs:label  "hasAnnotatableVersionAt" .

dm2e:File  a          owl:Class , rdfs:Class ;
        rdfs:comment  "Archival Item." ;
        rdfs:label    "File" .

dm2e:composer  a            rdf:Property ;
        rdfs:label          "composer" ;
        rdfs:range          foaf:Person ;
        rdfs:subPropertyOf  dc:creator .

dm2e:previousOwner  a  rdf:Property ;
        rdfs:label  "previous owner" .

dm2e:displayLevel  a  owl:DatatypeProperty , rdf:Property ;
        rdfs:label  "displayLevel" ;
        rdfs:range  xsd:boolean .

<http://onto.dm2e.eu/schemas/dm2e#IBI>
        a              dcterms:Agent ;
        foaf:homepage  <http://onto.dm2e.eu/schemas/dm2e> ;
        foaf:member    <http://onto.dm2e.eu/schemas/dm2e#s.hennicke> ;
        foaf:name      "IBI" .

<http://onto.dm2e.eu/schemas/dm2e#JIwanowa>
        a              foaf:Person ;
        foaf:homepage  <http://onto.dm2e.eu/schemas/dm2e> ;
        foaf:name      "Julia Iwanowa" .

dm2e:modeOfAcquisition
        a                   rdf:Property ;
        rdfs:label          "modeOfAcquisition" ;
        rdfs:subPropertyOf  dcterms:provenance .

dm2e:incipit  a             owl:DatatypeProperty , rdf:Property ;
        rdfs:comment        "Opening words of a manuscript. A language tag in ISO 639-2 should be added to the Literal." ;
        rdfs:label          "incipit" ;
        rdfs:range          rdfs:Literal ;
        rdfs:subPropertyOf  dc:description .

dm2e:illustration  a        rdf:Property ;
        rdfs:comment        "Generic description of illustrations in the CHO." ;
        rdfs:label          "illustration" ;
        rdfs:subPropertyOf  dc:description .

<http://onto.dm2e.eu/schemas/dm2e#rdf>
        dcterms:FileFormat  <http://onto.dm2e.eu/schemas/dm2e> .

dm2e:owner  a       rdf:Property ;
        rdfs:label  "owner" .

<http://onto.dm2e.eu/schemas/dm2e#School%20for%20Library%20and%20Information%20Science>
        a              dcterms:Agent ;
        foaf:homepage  <http://www.ibi.hu-berlin.de> ;
        foaf:member    <http://onto.dm2e.eu/schemas/dm2e#JIwanowa> ;
        foaf:name      "School for Library and Information Science" .

dm2e:watermark  a           owl:DatatypeProperty , rdf:Property ;
        rdfs:label          "watermark" ;
        rdfs:range          rdfs:Literal ;
        rdfs:subPropertyOf  dc:description .

dm2e:portrayed  a           rdf:Property ;
        rdfs:label          "portrayed" ;
        rdfs:range          foaf:Person ;
        rdfs:subPropertyOf  dm2e:mentioned .

dm2e:writtenAreaDimension
        a                   owl:DatatypeProperty , rdf:Property ;
        rdfs:label          "written area dimension" ;
        rdfs:range          rdfs:Literal ;
        rdfs:subPropertyOf  dcterms:extent .

dm2e:copyist  a     rdf:Property ;
        rdfs:label  "copyist" ;
        rdfs:range  foaf:Person .

<http://onto.dm2e.eu/schemas/dm2e#konstantin>
        a              foaf:Person ;
        foaf:homepage  <http://onto.dm2e.eu/schemas/dm2e> ;
        foaf:name      "Konstantin Baierer" .

dm2e:publishedAt  a         rdf:Property ;
        rdfs:label          "published at" ;
        rdfs:subPropertyOf  dcterms:spatial .

dm2e:Photo  a            owl:Class , rdfs:Class ;
        rdfs:comment     "ProvidedCHO of type photo." ;
        rdfs:label       "Photo" ;
        rdfs:subClassOf  foaf:Image .

dm2e:Fragment  a      owl:Class , rdfs:Class ;
        rdfs:comment  "A physical fragment of a document, e.g. a collection of pages of a manuscript." ;
        rdfs:label    "Fragment" .

dm2e:painter  a             rdf:Property ;
        rdfs:label          "painter" ;
        rdfs:range          foaf:Person ;
        rdfs:subPropertyOf  dc:contributor .

<http://onto.dm2e.eu/schemas/dm2e#s.hennicke>
        a              foaf:Person ;
        foaf:homepage  <http://onto.dm2e.eu/schemas/dm2e> ;
        foaf:name      "Steffen Hennicke" .

dm2e:Manuscript  a    owl:Class , rdfs:Class ;
        rdfs:comment  "ProvidedCHO of type manuscript, e.g. Wittgensteins brown book. Not equivalent to bibo:Manuscript. Not equivalent to bibo:Manuscript." ;
        rdfs:label    "Manuscript" .

dm2e:Paragraph  a     owl:Class , rdfs:Class ;
        rdfs:comment  "ProvidedCHO of type paragraph. Can be part of another (textual) CHO, e.g. dm2e:Manuscript." ;
        rdfs:label    "Paragraph" .

dm2e:mentioned  a   rdf:Property ;
        rdfs:label  "mentioned" .

dm2e:Work  a          owl:Class , rdfs:Class ;
        rdfs:comment  "A non-physical piece of work of an agent, e.g. the theoretical concept of a manuscript." ;
        rdfs:label    "Work" .

dm2e:genre  a               rdf:Property ;
        rdfs:label          "genre" ;
        rdfs:subPropertyOf  dc:type .

dm2e:refersTo  a            rdf:Property ;
        rdfs:label          "refers to" ;
        rdfs:subPropertyOf  dcterms:references .

dm2e:honoree  a     rdf:Property ;
        rdfs:label  "honoree" ;
        rdfs:range  foaf:Person .

dm2e:pageDimension  a       owl:DatatypeProperty , rdf:Property ;
        rdfs:label          "page dimension" ;
        rdfs:range          rdfs:Literal ;
        rdfs:subPropertyOf  dcterms:extent .

dm2e:writtenAt  a           rdf:Property ;
        rdfs:label          "written at" ;
        rdfs:subPropertyOf  dcterms:spatial .
