@prefix : <http://ns.cerise-project.nl/energy/def/cim-smartgrid#> .
@prefix dc: <http://purl.org/dc/elements/1.1/> .
@prefix rdfs: <http://www.w3.org/2000/01/rdf-schema#> .
@prefix xsd: <http://www.w3.org/2001/XMLSchema#> .
@prefix owl: <http://www.w3.org/2002/07/owl#> .
@prefix rdf: <http://www.w3.org/1999/02/22-rdf-syntax-ns#> .
@prefix uml: <http://langdale.com.au/2005/UML#> .
@prefix msg: <http://langdale.com.au/2005/Message#> .

<http://ns.cerise-project.nl/energy/def/cim-smartgrid> a owl:Ontology ;
	dc:publisher <http://www.cerise-project.nl/> ;
	dc:creator "Maarten Steen (TNO)" ;
	rdfs:seeAlso <http://www.iec.ch/smartgrid/standards/> ;
	owl:versionInfo "22/5/2014"^^xsd:string ;
	rdfs:comment "A Profile of the IEC Common Information Model for Smart Grids, developed by the Cerise-SG project."^^xsd:string ;
	rdfs:label "A CIM Profile for Smart Grids"^^xsd:string .

:Status a owl:Class ;
	rdfs:subClassOf _:node1912nb34nx1 .

_:node1912nb34nx1 a owl:Restriction ;
	owl:allValuesFrom xsd:string ;
	owl:onProperty <http://ns.cerise-project.nl/energy/def/cim-smartgrid#Status.remark> .

<http://ns.cerise-project.nl/energy/def/cim-smartgrid#Status.remark> a owl:DatatypeProperty .

:Status rdfs:subClassOf _:node1912nb34nx2 .

_:node1912nb34nx2 a owl:Restriction ;
	owl:cardinality "1"^^xsd:int ;
	owl:onProperty <http://ns.cerise-project.nl/energy/def/cim-smartgrid#Status.remark> .

:Status rdfs:subClassOf _:node1912nb34nx3 .

_:node1912nb34nx3 a owl:Restriction ;
	owl:allValuesFrom xsd:string ;
	owl:onProperty <http://ns.cerise-project.nl/energy/def/cim-smartgrid#Status.reason> .

<http://ns.cerise-project.nl/energy/def/cim-smartgrid#Status.reason> a owl:DatatypeProperty .

:Status rdfs:subClassOf _:node1912nb34nx4 .

_:node1912nb34nx4 a owl:Restriction ;
	owl:cardinality "1"^^xsd:int ;
	owl:onProperty <http://ns.cerise-project.nl/energy/def/cim-smartgrid#Status.reason> .

:Status rdfs:label "Status" ;
	rdfs:subClassOf _:node1912nb34nx5 .

_:node1912nb34nx5 a owl:Restriction ;
	owl:cardinality "1"^^xsd:int ;
	owl:onProperty <http://ns.cerise-project.nl/energy/def/cim-smartgrid#Status.dateTime> .

<http://ns.cerise-project.nl/energy/def/cim-smartgrid#Status.dateTime> a owl:DatatypeProperty .

:Status rdfs:comment "Current status information relevant to an entity." ;
	rdfs:subClassOf _:node1912nb34nx6 .

_:node1912nb34nx6 a owl:Restriction ;
	owl:allValuesFrom xsd:dateTime ;
	owl:onProperty <http://ns.cerise-project.nl/energy/def/cim-smartgrid#Status.dateTime> .

:Status rdfs:subClassOf _:node1912nb34nx7 .

_:node1912nb34nx7 a owl:Restriction ;
	owl:cardinality "1"^^xsd:int ;
	owl:onProperty <http://ns.cerise-project.nl/energy/def/cim-smartgrid#Status.value> .

<http://ns.cerise-project.nl/energy/def/cim-smartgrid#Status.value> a owl:DatatypeProperty .

:Status rdfs:subClassOf _:node1912nb34nx8 .

_:node1912nb34nx8 a owl:Restriction ;
	owl:allValuesFrom xsd:string ;
	owl:onProperty <http://ns.cerise-project.nl/energy/def/cim-smartgrid#Status.value> .

:Status uml:hasStereotype uml:compound ;
	rdfs:isDefinedBy :Package_Common .

:Package_Common a uml:Package ;
	rdfs:label "Common" ;
	rdfs:comment "This package contains the information classes that support distribution management in general." ;
	rdfs:isDefinedBy :Package_IEC61968 .

:Package_IEC61968 a uml:Package ;
	rdfs:comment """The IEC 61968 subpackages of the CIM are developed, standardized and maintained by IEC TC57 Working Group 14: interfaces for distribution management (WG14).
Currently, normative parts of the model support the needs of information exchange defined in IEC 61968-3, IEC 61968-4, IEC 61968-9 and in IEC 61968-13.""" ;
	rdfs:label "IEC61968" ;
	rdfs:isDefinedBy :Package_TC57CIM .

:Package_TC57CIM a uml:Package ;
	rdfs:label "TC57CIM" ;
	rdfs:comment "Top package for IEC TC57 CIM." ;
	rdfs:isDefinedBy :global_package .

:global_package a uml:Package ;
	rdfs:label "Global" .

:ElectronicAddress a owl:Class ;
	rdfs:subClassOf _:node1912nb34nx9 .

_:node1912nb34nx9 a owl:Restriction ;
	owl:cardinality "1"^^xsd:int ;
	owl:onProperty <http://ns.cerise-project.nl/energy/def/cim-smartgrid#ElectronicAddress.web> .

<http://ns.cerise-project.nl/energy/def/cim-smartgrid#ElectronicAddress.web> a owl:DatatypeProperty .

:ElectronicAddress rdfs:subClassOf _:node1912nb34nx10 .

_:node1912nb34nx10 a owl:Restriction ;
	owl:allValuesFrom xsd:string ;
	owl:onProperty <http://ns.cerise-project.nl/energy/def/cim-smartgrid#ElectronicAddress.password> .

<http://ns.cerise-project.nl/energy/def/cim-smartgrid#ElectronicAddress.password> a owl:DatatypeProperty .

:ElectronicAddress rdfs:subClassOf _:node1912nb34nx11 .

_:node1912nb34nx11 a owl:Restriction ;
	owl:cardinality "1"^^xsd:int ;
	owl:onProperty <http://ns.cerise-project.nl/energy/def/cim-smartgrid#ElectronicAddress.email1> .

<http://ns.cerise-project.nl/energy/def/cim-smartgrid#ElectronicAddress.email1> a owl:DatatypeProperty .

:ElectronicAddress rdfs:label "ElectronicAddress" ;
	rdfs:subClassOf _:node1912nb34nx12 .

_:node1912nb34nx12 a owl:Restriction ;
	owl:cardinality "1"^^xsd:int ;
	owl:onProperty <http://ns.cerise-project.nl/energy/def/cim-smartgrid#ElectronicAddress.password> .

:ElectronicAddress rdfs:subClassOf _:node1912nb34nx13 .

_:node1912nb34nx13 a owl:Restriction ;
	owl:cardinality "1"^^xsd:int ;
	owl:onProperty <http://ns.cerise-project.nl/energy/def/cim-smartgrid#ElectronicAddress.email2> .

<http://ns.cerise-project.nl/energy/def/cim-smartgrid#ElectronicAddress.email2> a owl:DatatypeProperty .

:ElectronicAddress rdfs:subClassOf _:node1912nb34nx14 .

_:node1912nb34nx14 a owl:Restriction ;
	owl:cardinality "1"^^xsd:int ;
	owl:onProperty <http://ns.cerise-project.nl/energy/def/cim-smartgrid#ElectronicAddress.userID> .

<http://ns.cerise-project.nl/energy/def/cim-smartgrid#ElectronicAddress.userID> a owl:DatatypeProperty .

:ElectronicAddress rdfs:subClassOf _:node1912nb34nx15 .

_:node1912nb34nx15 a owl:Restriction ;
	owl:cardinality "1"^^xsd:int ;
	owl:onProperty <http://ns.cerise-project.nl/energy/def/cim-smartgrid#ElectronicAddress.radio> .

<http://ns.cerise-project.nl/energy/def/cim-smartgrid#ElectronicAddress.radio> a owl:DatatypeProperty .

:ElectronicAddress rdfs:subClassOf _:node1912nb34nx16 .

_:node1912nb34nx16 a owl:Restriction ;
	owl:allValuesFrom xsd:string ;
	owl:onProperty <http://ns.cerise-project.nl/energy/def/cim-smartgrid#ElectronicAddress.lan> .

<http://ns.cerise-project.nl/energy/def/cim-smartgrid#ElectronicAddress.lan> a owl:DatatypeProperty .

:ElectronicAddress uml:hasStereotype uml:compound ;
	rdfs:subClassOf _:node1912nb34nx17 .

_:node1912nb34nx17 a owl:Restriction ;
	owl:allValuesFrom xsd:string ;
	owl:onProperty <http://ns.cerise-project.nl/energy/def/cim-smartgrid#ElectronicAddress.email2> .

:ElectronicAddress rdfs:comment "Electronic address information." ;
	rdfs:subClassOf _:node1912nb34nx18 .

_:node1912nb34nx18 a owl:Restriction ;
	owl:allValuesFrom xsd:string ;
	owl:onProperty <http://ns.cerise-project.nl/energy/def/cim-smartgrid#ElectronicAddress.mac> .

<http://ns.cerise-project.nl/energy/def/cim-smartgrid#ElectronicAddress.mac> a owl:DatatypeProperty .

:ElectronicAddress rdfs:subClassOf _:node1912nb34nx19 .

_:node1912nb34nx19 a owl:Restriction ;
	owl:allValuesFrom xsd:string ;
	owl:onProperty <http://ns.cerise-project.nl/energy/def/cim-smartgrid#ElectronicAddress.email1> .

:ElectronicAddress rdfs:subClassOf _:node1912nb34nx20 .

_:node1912nb34nx20 a owl:Restriction ;
	owl:allValuesFrom xsd:string ;
	owl:onProperty <http://ns.cerise-project.nl/energy/def/cim-smartgrid#ElectronicAddress.userID> .

:ElectronicAddress rdfs:subClassOf _:node1912nb34nx21 .

_:node1912nb34nx21 a owl:Restriction ;
	owl:cardinality "1"^^xsd:int ;
	owl:onProperty <http://ns.cerise-project.nl/energy/def/cim-smartgrid#ElectronicAddress.lan> .

:ElectronicAddress rdfs:subClassOf _:node1912nb34nx22 .

_:node1912nb34nx22 a owl:Restriction ;
	owl:allValuesFrom xsd:string ;
	owl:onProperty <http://ns.cerise-project.nl/energy/def/cim-smartgrid#ElectronicAddress.radio> .

:ElectronicAddress rdfs:isDefinedBy :Package_Common ;
	rdfs:subClassOf _:node1912nb34nx23 .

_:node1912nb34nx23 a owl:Restriction ;
	owl:cardinality "1"^^xsd:int ;
	owl:onProperty <http://ns.cerise-project.nl/energy/def/cim-smartgrid#ElectronicAddress.mac> .

:ElectronicAddress rdfs:subClassOf _:node1912nb34nx24 .

_:node1912nb34nx24 a owl:Restriction ;
	owl:allValuesFrom xsd:string ;
	owl:onProperty <http://ns.cerise-project.nl/energy/def/cim-smartgrid#ElectronicAddress.web> .

:EndDeviceFunction a owl:Class ;
	rdfs:subClassOf _:node1912nb34nx25 .

_:node1912nb34nx25 a owl:Restriction ;
	owl:cardinality "1"^^xsd:int ;
	owl:onProperty <http://ns.cerise-project.nl/energy/def/cim-smartgrid#EndDeviceFunction.EndDevice> .

<http://ns.cerise-project.nl/energy/def/cim-smartgrid#EndDeviceFunction.EndDevice> a owl:ObjectProperty .

:EndDeviceFunction rdfs:subClassOf _:node1912nb34nx26 .

_:node1912nb34nx26 a owl:Restriction ;
	owl:allValuesFrom :EndDevice .

:EndDevice a owl:Class .

_:node1912nb34nx26 owl:onProperty <http://ns.cerise-project.nl/energy/def/cim-smartgrid#EndDeviceFunction.EndDevice> .

:EndDeviceFunction rdfs:subClassOf :IdentifiedObject .

:IdentifiedObject a owl:Class .

:EndDeviceFunction rdfs:comment "Function performed by an end device such as a meter, communication equipment, controllers, etc." ;
	rdfs:label "EndDeviceFunction" ;
	rdfs:isDefinedBy :Package_Metering .

:Package_Metering a uml:Package ;
	rdfs:label "Metering" ;
	rdfs:comment "This package contains the core information classes that support end device applications with specialized classes for metering and premise are network devices, and remote reading functions. These classes are generally associated with the point where a service is delivered to the customer." ;
	rdfs:isDefinedBy :Package_IEC61968 .

:IntervalReading a owl:Class ;
	rdfs:label "IntervalReading" ;
	rdfs:subClassOf _:node1912nb34nx27 .

_:node1912nb34nx27 a owl:Restriction ;
	owl:minCardinality "1"^^xsd:int ;
	owl:onProperty <http://ns.cerise-project.nl/energy/def/cim-smartgrid#IntervalReading.IntervalBlocks> .

<http://ns.cerise-project.nl/energy/def/cim-smartgrid#IntervalReading.IntervalBlocks> a owl:ObjectProperty .

:IntervalReading rdfs:subClassOf _:node1912nb34nx28 .

_:node1912nb34nx28 a owl:Restriction ;
	owl:onProperty <http://ns.cerise-project.nl/energy/def/cim-smartgrid#IntervalReading.IntervalBlocks> ;
	owl:allValuesFrom :IntervalBlock .

:IntervalBlock a owl:Class .

:IntervalReading rdfs:comment """Data captured at regular intervals of time. Interval data could be captured as incremental data, absolute data, or relative data. The source for the data is usually a tariff quantity or an engineering quantity. Data is typically captured in time-tagged, uniform, fixed-length intervals of 5 min, 10 min, 15 min, 30 min, or 60 min.
Note: Interval Data is sometimes also called \"Interval Data Readings\" (IDR).""" ;
	rdfs:subClassOf :BaseReading .

:BaseReading a owl:Class .

:IntervalReading rdfs:isDefinedBy :Package_Metering .

:MeterMultiplierKind a owl:Class ;
	uml:hasStereotype uml:enumeration ;
	rdfs:comment "Kind of meter multiplier." ;
	rdfs:label "MeterMultiplierKind" ;
	rdfs:isDefinedBy :Package_Metering .

:CoordinateSystem a owl:Class ;
	rdfs:label "CoordinateSystem" ;
	rdfs:subClassOf _:node1912nb34nx29 .

_:node1912nb34nx29 a owl:Restriction ;
	owl:minCardinality "1"^^xsd:int ;
	owl:onProperty <http://ns.cerise-project.nl/energy/def/cim-smartgrid#CoordinateSystem.Location> .

<http://ns.cerise-project.nl/energy/def/cim-smartgrid#CoordinateSystem.Location> a owl:ObjectProperty .

:CoordinateSystem rdfs:subClassOf _:node1912nb34nx30 .

_:node1912nb34nx30 a owl:Restriction ;
	owl:allValuesFrom :Location .

:Location a owl:Class .

_:node1912nb34nx30 owl:onProperty <http://ns.cerise-project.nl/energy/def/cim-smartgrid#CoordinateSystem.Location> .

:CoordinateSystem rdfs:subClassOf _:node1912nb34nx31 .

_:node1912nb34nx31 a owl:Restriction ;
	owl:cardinality "1"^^xsd:int ;
	owl:onProperty <http://ns.cerise-project.nl/energy/def/cim-smartgrid#CoordinateSystem.crsUrn> .

<http://ns.cerise-project.nl/energy/def/cim-smartgrid#CoordinateSystem.crsUrn> a owl:DatatypeProperty .

:CoordinateSystem rdfs:subClassOf _:node1912nb34nx32 .

_:node1912nb34nx32 a owl:Restriction ;
	owl:allValuesFrom xsd:string ;
	owl:onProperty <http://ns.cerise-project.nl/energy/def/cim-smartgrid#CoordinateSystem.crsUrn> .

:CoordinateSystem rdfs:subClassOf :IdentifiedObject ;
	rdfs:comment "Coordinate reference system." ;
	rdfs:isDefinedBy :Package_Common .

:StreetDetail a owl:Class ;
	rdfs:isDefinedBy :Package_Common ;
	rdfs:subClassOf _:node1912nb34nx33 .

_:node1912nb34nx33 a owl:Restriction ;
	owl:cardinality "1"^^xsd:int ;
	owl:onProperty <http://ns.cerise-project.nl/energy/def/cim-smartgrid#StreetDetail.code> .

<http://ns.cerise-project.nl/energy/def/cim-smartgrid#StreetDetail.code> a owl:DatatypeProperty .

:StreetDetail rdfs:label "StreetDetail" ;
	uml:hasStereotype uml:compound ;
	rdfs:subClassOf _:node1912nb34nx34 .

_:node1912nb34nx34 a owl:Restriction ;
	owl:cardinality "1"^^xsd:int ;
	owl:onProperty <http://ns.cerise-project.nl/energy/def/cim-smartgrid#StreetDetail.prefix> .

<http://ns.cerise-project.nl/energy/def/cim-smartgrid#StreetDetail.prefix> a owl:DatatypeProperty .

:StreetDetail rdfs:subClassOf _:node1912nb34nx35 .

_:node1912nb34nx35 a owl:Restriction ;
	owl:cardinality "1"^^xsd:int ;
	owl:onProperty <http://ns.cerise-project.nl/energy/def/cim-smartgrid#StreetDetail.suiteNumber> .

<http://ns.cerise-project.nl/energy/def/cim-smartgrid#StreetDetail.suiteNumber> a owl:DatatypeProperty .

:StreetDetail rdfs:subClassOf _:node1912nb34nx36 .

_:node1912nb34nx36 a owl:Restriction ;
	owl:allValuesFrom xsd:boolean ;
	owl:onProperty <http://ns.cerise-project.nl/energy/def/cim-smartgrid#StreetDetail.withinTownLimits> .

<http://ns.cerise-project.nl/energy/def/cim-smartgrid#StreetDetail.withinTownLimits> a owl:DatatypeProperty .

:StreetDetail rdfs:subClassOf _:node1912nb34nx37 .

_:node1912nb34nx37 a owl:Restriction ;
	owl:cardinality "1"^^xsd:int ;
	owl:onProperty <http://ns.cerise-project.nl/energy/def/cim-smartgrid#StreetDetail.type> .

<http://ns.cerise-project.nl/energy/def/cim-smartgrid#StreetDetail.type> a owl:DatatypeProperty .

:StreetDetail rdfs:subClassOf _:node1912nb34nx38 .

_:node1912nb34nx38 a owl:Restriction ;
	owl:allValuesFrom xsd:string ;
	owl:onProperty <http://ns.cerise-project.nl/energy/def/cim-smartgrid#StreetDetail.suffix> .

<http://ns.cerise-project.nl/energy/def/cim-smartgrid#StreetDetail.suffix> a owl:DatatypeProperty .

:StreetDetail rdfs:subClassOf _:node1912nb34nx39 .

_:node1912nb34nx39 a owl:Restriction ;
	owl:allValuesFrom xsd:string ;
	owl:onProperty <http://ns.cerise-project.nl/energy/def/cim-smartgrid#StreetDetail.suiteNumber> .

:StreetDetail rdfs:subClassOf _:node1912nb34nx40 .

_:node1912nb34nx40 a owl:Restriction ;
	owl:cardinality "1"^^xsd:int ;
	owl:onProperty <http://ns.cerise-project.nl/energy/def/cim-smartgrid#StreetDetail.buildingName> .

<http://ns.cerise-project.nl/energy/def/cim-smartgrid#StreetDetail.buildingName> a owl:DatatypeProperty .

:StreetDetail rdfs:subClassOf _:node1912nb34nx41 .

_:node1912nb34nx41 a owl:Restriction ;
	owl:cardinality "1"^^xsd:int ;
	owl:onProperty <http://ns.cerise-project.nl/energy/def/cim-smartgrid#StreetDetail.addressGeneral> .

<http://ns.cerise-project.nl/energy/def/cim-smartgrid#StreetDetail.addressGeneral> a owl:DatatypeProperty .

:StreetDetail rdfs:subClassOf _:node1912nb34nx42 .

_:node1912nb34nx42 a owl:Restriction ;
	owl:cardinality "1"^^xsd:int ;
	owl:onProperty <http://ns.cerise-project.nl/energy/def/cim-smartgrid#StreetDetail.withinTownLimits> .

:StreetDetail rdfs:subClassOf _:node1912nb34nx43 .

_:node1912nb34nx43 a owl:Restriction ;
	owl:cardinality "1"^^xsd:int ;
	owl:onProperty <http://ns.cerise-project.nl/energy/def/cim-smartgrid#StreetDetail.name> .

<http://ns.cerise-project.nl/energy/def/cim-smartgrid#StreetDetail.name> a owl:DatatypeProperty .

:StreetDetail rdfs:comment "Street details, in the context of address." ;
	rdfs:subClassOf _:node1912nb34nx44 .

_:node1912nb34nx44 a owl:Restriction ;
	owl:allValuesFrom xsd:string ;
	owl:onProperty <http://ns.cerise-project.nl/energy/def/cim-smartgrid#StreetDetail.type> .

:StreetDetail rdfs:subClassOf _:node1912nb34nx45 .

_:node1912nb34nx45 a owl:Restriction ;
	owl:allValuesFrom xsd:string ;
	owl:onProperty <http://ns.cerise-project.nl/energy/def/cim-smartgrid#StreetDetail.addressGeneral> .

:StreetDetail rdfs:subClassOf _:node1912nb34nx46 .

_:node1912nb34nx46 a owl:Restriction ;
	owl:allValuesFrom xsd:string ;
	owl:onProperty <http://ns.cerise-project.nl/energy/def/cim-smartgrid#StreetDetail.buildingName> .

:StreetDetail rdfs:subClassOf _:node1912nb34nx47 .

_:node1912nb34nx47 a owl:Restriction ;
	owl:cardinality "1"^^xsd:int ;
	owl:onProperty <http://ns.cerise-project.nl/energy/def/cim-smartgrid#StreetDetail.suffix> .

:StreetDetail rdfs:subClassOf _:node1912nb34nx48 .

_:node1912nb34nx48 a owl:Restriction ;
	owl:cardinality "1"^^xsd:int ;
	owl:onProperty <http://ns.cerise-project.nl/energy/def/cim-smartgrid#StreetDetail.number> .

<http://ns.cerise-project.nl/energy/def/cim-smartgrid#StreetDetail.number> a owl:DatatypeProperty .

:StreetDetail rdfs:subClassOf _:node1912nb34nx49 .

_:node1912nb34nx49 a owl:Restriction ;
	owl:allValuesFrom xsd:string ;
	owl:onProperty <http://ns.cerise-project.nl/energy/def/cim-smartgrid#StreetDetail.code> .

:StreetDetail rdfs:subClassOf _:node1912nb34nx50 .

_:node1912nb34nx50 a owl:Restriction ;
	owl:allValuesFrom xsd:string ;
	owl:onProperty <http://ns.cerise-project.nl/energy/def/cim-smartgrid#StreetDetail.prefix> .

:StreetDetail rdfs:subClassOf _:node1912nb34nx51 .

_:node1912nb34nx51 a owl:Restriction ;
	owl:allValuesFrom xsd:string ;
	owl:onProperty <http://ns.cerise-project.nl/energy/def/cim-smartgrid#StreetDetail.number> .

:StreetDetail rdfs:subClassOf _:node1912nb34nx52 .

_:node1912nb34nx52 a owl:Restriction ;
	owl:allValuesFrom xsd:string ;
	owl:onProperty <http://ns.cerise-project.nl/energy/def/cim-smartgrid#StreetDetail.name> .

:MeterMultiplier a owl:Class ;
	rdfs:comment "Multiplier applied at the meter." ;
	rdfs:subClassOf _:node1912nb34nx53 .

_:node1912nb34nx53 a owl:Restriction ;
	owl:cardinality "1"^^xsd:int ;
	owl:onProperty <http://ns.cerise-project.nl/energy/def/cim-smartgrid#MeterMultiplier.Meter> .

<http://ns.cerise-project.nl/energy/def/cim-smartgrid#MeterMultiplier.Meter> a owl:ObjectProperty .

:MeterMultiplier rdfs:subClassOf _:node1912nb34nx54 .

_:node1912nb34nx54 a owl:Restriction ;
	owl:allValuesFrom :MeterMultiplierKind ;
	owl:onProperty <http://ns.cerise-project.nl/energy/def/cim-smartgrid#MeterMultiplier.kind> .

<http://ns.cerise-project.nl/energy/def/cim-smartgrid#MeterMultiplier.kind> a owl:ObjectProperty .

:MeterMultiplier rdfs:subClassOf :IdentifiedObject , _:node1912nb34nx55 .

_:node1912nb34nx55 a owl:Restriction ;
	owl:onProperty <http://ns.cerise-project.nl/energy/def/cim-smartgrid#MeterMultiplier.Meter> ;
	owl:allValuesFrom :Meter .

:Meter a owl:Class .

:MeterMultiplier rdfs:subClassOf _:node1912nb34nx56 .

_:node1912nb34nx56 a owl:Restriction ;
	owl:cardinality "1"^^xsd:int ;
	owl:onProperty <http://ns.cerise-project.nl/energy/def/cim-smartgrid#MeterMultiplier.kind> .

:MeterMultiplier rdfs:subClassOf _:node1912nb34nx57 .

_:node1912nb34nx57 a owl:Restriction ;
	owl:cardinality "1"^^xsd:int ;
	owl:onProperty <http://ns.cerise-project.nl/energy/def/cim-smartgrid#MeterMultiplier.value> .

<http://ns.cerise-project.nl/energy/def/cim-smartgrid#MeterMultiplier.value> a owl:DatatypeProperty .

:MeterMultiplier rdfs:label "MeterMultiplier" ;
	rdfs:isDefinedBy :Package_Metering ;
	rdfs:subClassOf _:node1912nb34nx58 .

_:node1912nb34nx58 a owl:Restriction ;
	owl:allValuesFrom xsd:float ;
	owl:onProperty <http://ns.cerise-project.nl/energy/def/cim-smartgrid#MeterMultiplier.value> .

:EndDevice rdfs:subClassOf _:node1912nb34nx59 .

_:node1912nb34nx59 a owl:Restriction ;
	owl:cardinality "1"^^xsd:int ;
	owl:onProperty <http://ns.cerise-project.nl/energy/def/cim-smartgrid#EndDevice.isVirtual> .

<http://ns.cerise-project.nl/energy/def/cim-smartgrid#EndDevice.isVirtual> a owl:DatatypeProperty .

:EndDevice rdfs:subClassOf _:node1912nb34nx60 .

_:node1912nb34nx60 a owl:Restriction ;
	owl:onProperty <http://ns.cerise-project.nl/energy/def/cim-smartgrid#EndDevice.UsagePoint> .

<http://ns.cerise-project.nl/energy/def/cim-smartgrid#EndDevice.UsagePoint> a owl:ObjectProperty .

_:node1912nb34nx60 owl:allValuesFrom :UsagePoint .

:UsagePoint a owl:Class .

:EndDevice rdfs:subClassOf _:node1912nb34nx61 .

_:node1912nb34nx61 a owl:Restriction ;
	owl:minCardinality "1"^^xsd:int ;
	owl:onProperty <http://ns.cerise-project.nl/energy/def/cim-smartgrid#EndDevice.EndDeviceFunctions> .

<http://ns.cerise-project.nl/energy/def/cim-smartgrid#EndDevice.EndDeviceFunctions> a owl:ObjectProperty .

:EndDevice rdfs:subClassOf _:node1912nb34nx62 .

_:node1912nb34nx62 a owl:Restriction ;
	owl:onProperty <http://ns.cerise-project.nl/energy/def/cim-smartgrid#EndDevice.EndDeviceFunctions> ;
	owl:allValuesFrom :EndDeviceFunction .

:EndDevice rdfs:label "EndDevice" ;
	rdfs:subClassOf _:node1912nb34nx63 .

_:node1912nb34nx63 a owl:Restriction ;
	owl:cardinality "1"^^xsd:int ;
	owl:onProperty <http://ns.cerise-project.nl/energy/def/cim-smartgrid#EndDevice.UsagePoint> .

:EndDevice rdfs:subClassOf _:node1912nb34nx64 .

_:node1912nb34nx64 a owl:Restriction ;
	owl:allValuesFrom xsd:boolean ;
	owl:onProperty <http://ns.cerise-project.nl/energy/def/cim-smartgrid#EndDevice.isVirtual> .

:EndDevice rdfs:subClassOf :IdentifiedObject ;
	rdfs:isDefinedBy :Package_Metering ;
	rdfs:subClassOf _:node1912nb34nx65 .

_:node1912nb34nx65 a owl:Restriction ;
	owl:cardinality "1"^^xsd:int ;
	owl:onProperty <http://ns.cerise-project.nl/energy/def/cim-smartgrid#EndDevice.installCode> .

<http://ns.cerise-project.nl/energy/def/cim-smartgrid#EndDevice.installCode> a owl:DatatypeProperty .

:EndDevice rdfs:comment """Asset container that performs one or more end device functions. One type of end device is a meter which can perform metering, load management, connect/disconnect, accounting functions, etc. Some end devices, such as ones monitoring and controlling air conditioner, refrigerator, pool pumps may be connected to a meter. All end devices may have communication capability defined by the associated communication function(s). An end device may be owned by a consumer, a service provider, utility or otherwise.
There may be a related end device function that identifies a sensor or control point within a metering application or communications systems (e.g., water, gas, electricity).
Some devices may use an optical port that conforms to the ANSI C12.18 standard for communications.""" ;
	rdfs:subClassOf _:node1912nb34nx66 .

_:node1912nb34nx66 a owl:Restriction ;
	owl:allValuesFrom xsd:string ;
	owl:onProperty <http://ns.cerise-project.nl/energy/def/cim-smartgrid#EndDevice.installCode> .

:UsagePointLocation a owl:Class ;
	rdfs:label "UsagePointLocation" ;
	rdfs:comment "Location of an individual usage point." ;
	rdfs:subClassOf :Location ;
	rdfs:isDefinedBy :Package_Metering .

:AmiBillingReadyKind a owl:Class ;
	uml:hasStereotype uml:enumeration ;
	rdfs:comment "Lifecycle states of the metering installation at a usage point with respect to readiness for billing via advanced metering infrastructure reads." ;
	rdfs:label "AmiBillingReadyKind" ;
	rdfs:isDefinedBy :Package_Metering .

:ReadingType a owl:Class ;
	rdfs:subClassOf _:node1912nb34nx67 .

_:node1912nb34nx67 a owl:Restriction ;
	owl:allValuesFrom xsd:string ;
	owl:onProperty <http://ns.cerise-project.nl/energy/def/cim-smartgrid#ReadingType.unit> .

<http://ns.cerise-project.nl/energy/def/cim-smartgrid#ReadingType.unit> a owl:DatatypeProperty .

:ReadingType rdfs:subClassOf _:node1912nb34nx68 .

_:node1912nb34nx68 a owl:Restriction ;
	owl:cardinality "1"^^xsd:int ;
	owl:onProperty <http://ns.cerise-project.nl/energy/def/cim-smartgrid#ReadingType.unit> .

:ReadingType rdfs:subClassOf _:node1912nb34nx69 .

_:node1912nb34nx69 a owl:Restriction ;
	owl:allValuesFrom xsd:string ;
	owl:onProperty <http://ns.cerise-project.nl/energy/def/cim-smartgrid#ReadingType.measuringPeriod> .

<http://ns.cerise-project.nl/energy/def/cim-smartgrid#ReadingType.measuringPeriod> a owl:DatatypeProperty .

:ReadingType rdfs:subClassOf _:node1912nb34nx70 .

_:node1912nb34nx70 a owl:Restriction ;
	owl:cardinality "1"^^xsd:int ;
	owl:onProperty <http://ns.cerise-project.nl/energy/def/cim-smartgrid#ReadingType.accumulation> .

<http://ns.cerise-project.nl/energy/def/cim-smartgrid#ReadingType.accumulation> a owl:DatatypeProperty .

:ReadingType rdfs:subClassOf _:node1912nb34nx71 .

_:node1912nb34nx71 a owl:Restriction ;
	owl:cardinality "1"^^xsd:int ;
	owl:onProperty <http://ns.cerise-project.nl/energy/def/cim-smartgrid#ReadingType.commodity> .

<http://ns.cerise-project.nl/energy/def/cim-smartgrid#ReadingType.commodity> a owl:DatatypeProperty .

:ReadingType rdfs:subClassOf _:node1912nb34nx72 .

_:node1912nb34nx72 a owl:Restriction ;
	owl:allValuesFrom xsd:string ;
	owl:onProperty <http://ns.cerise-project.nl/energy/def/cim-smartgrid#ReadingType.commodity> .

:ReadingType rdfs:subClassOf _:node1912nb34nx73 .

_:node1912nb34nx73 a owl:Restriction ;
	owl:allValuesFrom xsd:string ;
	owl:onProperty <http://ns.cerise-project.nl/energy/def/cim-smartgrid#ReadingType.aggregate> .

<http://ns.cerise-project.nl/energy/def/cim-smartgrid#ReadingType.aggregate> a owl:DatatypeProperty .

:ReadingType rdfs:isDefinedBy :Package_Metering ;
	rdfs:subClassOf _:node1912nb34nx74 .

_:node1912nb34nx74 a owl:Restriction ;
	owl:allValuesFrom xsd:string ;
	owl:onProperty <http://ns.cerise-project.nl/energy/def/cim-smartgrid#ReadingType.accumulation> .

:ReadingType rdfs:subClassOf _:node1912nb34nx75 .

_:node1912nb34nx75 a owl:Restriction ;
	owl:allValuesFrom xsd:string ;
	owl:onProperty <http://ns.cerise-project.nl/energy/def/cim-smartgrid#ReadingType.measurementKind> .

<http://ns.cerise-project.nl/energy/def/cim-smartgrid#ReadingType.measurementKind> a owl:DatatypeProperty .

:ReadingType rdfs:label "ReadingType" ;
	rdfs:subClassOf _:node1912nb34nx76 .

_:node1912nb34nx76 a owl:Restriction ;
	owl:cardinality "1"^^xsd:int ;
	owl:onProperty <http://ns.cerise-project.nl/energy/def/cim-smartgrid#ReadingType.measuringPeriod> .

:ReadingType rdfs:subClassOf _:node1912nb34nx77 .

_:node1912nb34nx77 a owl:Restriction ;
	owl:cardinality "1"^^xsd:int ;
	owl:onProperty <http://ns.cerise-project.nl/energy/def/cim-smartgrid#ReadingType.measurementKind> .

:ReadingType rdfs:subClassOf _:node1912nb34nx78 .

_:node1912nb34nx78 a owl:Restriction ;
	owl:allValuesFrom xsd:string ;
	owl:onProperty <http://ns.cerise-project.nl/energy/def/cim-smartgrid#ReadingType.flowDirection> .

<http://ns.cerise-project.nl/energy/def/cim-smartgrid#ReadingType.flowDirection> a owl:DatatypeProperty .

:ReadingType rdfs:subClassOf _:node1912nb34nx79 .

_:node1912nb34nx79 a owl:Restriction ;
	owl:cardinality "1"^^xsd:int ;
	owl:onProperty <http://ns.cerise-project.nl/energy/def/cim-smartgrid#ReadingType.aggregate> .

:ReadingType rdfs:subClassOf _:node1912nb34nx80 .

_:node1912nb34nx80 a owl:Restriction ;
	owl:cardinality "1"^^xsd:int ;
	owl:onProperty <http://ns.cerise-project.nl/energy/def/cim-smartgrid#ReadingType.flowDirection> .

:ReadingType rdfs:comment "Detailed description for a type of a reading value. Values in attributes allow for creation of recommended codes to be used for identifying reading value types as follows: &lt;macroPeriod&gt;.&lt;aggregate&gt;.&lt;measuringPeriod&gt;.&lt;accumulation&gt;.&lt;flowDirection&gt;.&lt;commodity&gt;.&lt;measurementKind&gt;.&lt;interharmonic.numerator&gt;.&lt;interharmonic.denominator&gt;.&lt;argument.numerator&gt;.&lt;argument.denominator&gt;.&lt;tou&gt;.&lt;cpp&gt;.&lt;consumptionTier&gt;.&lt;phases&gt;.&lt;multiplier&gt;.&lt;unit&gt;.&lt;currency&gt;." ;
	rdfs:subClassOf :IdentifiedObject .

:BaseReading rdfs:subClassOf _:node1912nb34nx81 .

_:node1912nb34nx81 a owl:Restriction ;
	owl:onProperty <http://ns.cerise-project.nl/energy/def/cim-smartgrid#BaseReading.timePeriod> .

<http://ns.cerise-project.nl/energy/def/cim-smartgrid#BaseReading.timePeriod> a owl:ObjectProperty .

_:node1912nb34nx81 owl:allValuesFrom :DateTimeInterval .

:DateTimeInterval a owl:Class .

:BaseReading rdfs:subClassOf _:node1912nb34nx82 .

_:node1912nb34nx82 a owl:Restriction ;
	owl:cardinality "1"^^xsd:int ;
	owl:onProperty <http://ns.cerise-project.nl/energy/def/cim-smartgrid#BaseReading.source> .

<http://ns.cerise-project.nl/energy/def/cim-smartgrid#BaseReading.source> a owl:DatatypeProperty .

:BaseReading rdfs:subClassOf _:node1912nb34nx83 .

_:node1912nb34nx83 a owl:Restriction ;
	owl:cardinality "1"^^xsd:int ;
	owl:onProperty <http://ns.cerise-project.nl/energy/def/cim-smartgrid#BaseReading.value> .

<http://ns.cerise-project.nl/energy/def/cim-smartgrid#BaseReading.value> a owl:DatatypeProperty .

:BaseReading rdfs:subClassOf _:node1912nb34nx84 .

_:node1912nb34nx84 a owl:Restriction ;
	owl:cardinality "1"^^xsd:int ;
	owl:onProperty <http://ns.cerise-project.nl/energy/def/cim-smartgrid#BaseReading.timePeriod> .

:BaseReading rdfs:isDefinedBy :Package_Metering ;
	rdfs:comment "Common representation for reading values. Note that a reading value may have multiple qualities, as produced by various systems ('ReadingQuality.source')." ;
	rdfs:label "BaseReading" ;
	rdfs:subClassOf _:node1912nb34nx85 .

_:node1912nb34nx85 a owl:Restriction ;
	owl:allValuesFrom xsd:string ;
	owl:onProperty <http://ns.cerise-project.nl/energy/def/cim-smartgrid#BaseReading.value> .

:BaseReading rdfs:subClassOf _:node1912nb34nx86 .

_:node1912nb34nx86 a owl:Restriction ;
	owl:allValuesFrom xsd:string ;
	owl:onProperty <http://ns.cerise-project.nl/energy/def/cim-smartgrid#BaseReading.source> .

:BaseReading rdfs:subClassOf :IdentifiedObject .

:IdentifiedObject rdfs:subClassOf _:node1912nb34nx87 .

_:node1912nb34nx87 a owl:Restriction ;
	owl:cardinality "1"^^xsd:int ;
	owl:onProperty <http://ns.cerise-project.nl/energy/def/cim-smartgrid#IdentifiedObject.aliasName> .

<http://ns.cerise-project.nl/energy/def/cim-smartgrid#IdentifiedObject.aliasName> a owl:DatatypeProperty .

:IdentifiedObject rdfs:subClassOf _:node1912nb34nx88 .

_:node1912nb34nx88 a owl:Restriction ;
	owl:allValuesFrom xsd:string ;
	owl:onProperty <http://ns.cerise-project.nl/energy/def/cim-smartgrid#IdentifiedObject.mRID> .

<http://ns.cerise-project.nl/energy/def/cim-smartgrid#IdentifiedObject.mRID> a owl:DatatypeProperty .

:IdentifiedObject rdfs:comment "This is a root class to provide common identification for all classes needing identification and naming attributes." ;
	rdfs:subClassOf _:node1912nb34nx89 .

_:node1912nb34nx89 a owl:Restriction ;
	owl:cardinality "1"^^xsd:int ;
	owl:onProperty <http://ns.cerise-project.nl/energy/def/cim-smartgrid#IdentifiedObject.name> .

<http://ns.cerise-project.nl/energy/def/cim-smartgrid#IdentifiedObject.name> a owl:DatatypeProperty .

:IdentifiedObject rdfs:label "IdentifiedObject" ;
	rdfs:subClassOf _:node1912nb34nx90 .

_:node1912nb34nx90 a owl:Restriction ;
	owl:allValuesFrom xsd:string ;
	owl:onProperty <http://ns.cerise-project.nl/energy/def/cim-smartgrid#IdentifiedObject.name> .

:IdentifiedObject rdfs:subClassOf _:node1912nb34nx91 .

_:node1912nb34nx91 a owl:Restriction ;
	owl:allValuesFrom xsd:string ;
	owl:onProperty <http://ns.cerise-project.nl/energy/def/cim-smartgrid#IdentifiedObject.description> .

<http://ns.cerise-project.nl/energy/def/cim-smartgrid#IdentifiedObject.description> a owl:DatatypeProperty .

:IdentifiedObject rdfs:isDefinedBy :Package_Core .

:Package_Core a uml:Package ;
	rdfs:comment "Contains the core PowerSystemResource and ConductingEquipment entities shared by all applications plus common collections of those entities. Not all applications require all the Core entities.  This package does not depend on any other package except the Domain package, but most of the other packages have associations and generalizations that depend on it." ;
	rdfs:label "Core" ;
	rdfs:isDefinedBy :Package_Base .

:Package_Base a uml:Package ;
	rdfs:label "Base" ;
	rdfs:isDefinedBy :Package_IEC61970 .

:Package_IEC61970 a uml:Package ;
	rdfs:comment "Top package for IEC 61970." ;
	rdfs:label "IEC61970" ;
	rdfs:isDefinedBy :Package_TC57CIM .

:IdentifiedObject rdfs:subClassOf _:node1912nb34nx92 .

_:node1912nb34nx92 a owl:Restriction ;
	owl:cardinality "1"^^xsd:int ;
	owl:onProperty <http://ns.cerise-project.nl/energy/def/cim-smartgrid#IdentifiedObject.mRID> .

:IdentifiedObject rdfs:subClassOf _:node1912nb34nx93 .

_:node1912nb34nx93 a owl:Restriction ;
	owl:cardinality "1"^^xsd:int ;
	owl:onProperty <http://ns.cerise-project.nl/energy/def/cim-smartgrid#IdentifiedObject.description> .

:IdentifiedObject rdfs:subClassOf _:node1912nb34nx94 .

_:node1912nb34nx94 a owl:Restriction ;
	owl:allValuesFrom xsd:string ;
	owl:onProperty <http://ns.cerise-project.nl/energy/def/cim-smartgrid#IdentifiedObject.aliasName> .

:ServiceKind a owl:Class ;
	uml:hasStereotype uml:enumeration ;
	rdfs:comment "Kind of service." ;
	rdfs:label "ServiceKind" ;
	rdfs:isDefinedBy :Package_Customers .

:Package_Customers a uml:Package ;
	rdfs:comment "This package contains the core information classes that support customer billing applications." ;
	rdfs:label "Customers" ;
	rdfs:isDefinedBy :Package_IEC61968 .

:ServiceCategory a owl:Class ;
	rdfs:isDefinedBy :Package_Customers ;
	rdfs:subClassOf _:node1912nb34nx95 .

_:node1912nb34nx95 a owl:Restriction ;
	owl:cardinality "1"^^xsd:int ;
	owl:onProperty <http://ns.cerise-project.nl/energy/def/cim-smartgrid#ServiceCategory.kind> .

<http://ns.cerise-project.nl/energy/def/cim-smartgrid#ServiceCategory.kind> a owl:ObjectProperty .

:ServiceCategory rdfs:subClassOf _:node1912nb34nx96 .

_:node1912nb34nx96 a owl:Restriction ;
	owl:onProperty <http://ns.cerise-project.nl/energy/def/cim-smartgrid#ServiceCategory.kind> ;
	owl:allValuesFrom :ServiceKind .

:ServiceCategory rdfs:comment "Category of service provided to the customer." ;
	rdfs:label "ServiceCategory" ;
	rdfs:subClassOf :IdentifiedObject .

:EndDeviceFunctionKind a owl:Class ;
	uml:hasStereotype uml:enumeration ;
	rdfs:comment "Kind of end device function." ;
	rdfs:label "EndDeviceFunctionKind" ;
	rdfs:isDefinedBy :Package_Metering .

:StreetAddress a owl:Class ;
	rdfs:subClassOf _:node1912nb34nx97 .

_:node1912nb34nx97 a owl:Restriction ;
	owl:cardinality "1"^^xsd:int ;
	owl:onProperty <http://ns.cerise-project.nl/energy/def/cim-smartgrid#StreetAddress.townDetail> .

<http://ns.cerise-project.nl/energy/def/cim-smartgrid#StreetAddress.townDetail> a owl:ObjectProperty .

:StreetAddress rdfs:subClassOf _:node1912nb34nx98 .

_:node1912nb34nx98 a owl:Restriction ;
	owl:allValuesFrom :TownDetail .

:TownDetail a owl:Class .

_:node1912nb34nx98 owl:onProperty <http://ns.cerise-project.nl/energy/def/cim-smartgrid#StreetAddress.townDetail> .

:StreetAddress rdfs:subClassOf _:node1912nb34nx99 .

_:node1912nb34nx99 a owl:Restriction ;
	owl:cardinality "1"^^xsd:int ;
	owl:onProperty <http://ns.cerise-project.nl/energy/def/cim-smartgrid#StreetAddress.streetDetail> .

<http://ns.cerise-project.nl/energy/def/cim-smartgrid#StreetAddress.streetDetail> a owl:ObjectProperty .

:StreetAddress rdfs:subClassOf _:node1912nb34nx100 .

_:node1912nb34nx100 a owl:Restriction ;
	owl:allValuesFrom :StreetDetail ;
	owl:onProperty <http://ns.cerise-project.nl/energy/def/cim-smartgrid#StreetAddress.streetDetail> .

:StreetAddress uml:hasStereotype uml:compound ;
	rdfs:comment "General purpose street address information." ;
	rdfs:label "StreetAddress" ;
	rdfs:isDefinedBy :Package_Common .

:PositionPoint a owl:Class ;
	rdfs:subClassOf _:node1912nb34nx101 .

_:node1912nb34nx101 a owl:Restriction ;
	owl:cardinality "1"^^xsd:int ;
	owl:onProperty <http://ns.cerise-project.nl/energy/def/cim-smartgrid#PositionPoint.sequenceNumber> .

<http://ns.cerise-project.nl/energy/def/cim-smartgrid#PositionPoint.sequenceNumber> a owl:DatatypeProperty .

:PositionPoint rdfs:subClassOf _:node1912nb34nx102 .

_:node1912nb34nx102 a owl:Restriction ;
	owl:cardinality "1"^^xsd:int ;
	owl:onProperty <http://ns.cerise-project.nl/energy/def/cim-smartgrid#PositionPoint.xPosition> .

<http://ns.cerise-project.nl/energy/def/cim-smartgrid#PositionPoint.xPosition> a owl:DatatypeProperty .

:PositionPoint rdfs:label "PositionPoint" ;
	rdfs:subClassOf _:node1912nb34nx103 .

_:node1912nb34nx103 a owl:Restriction ;
	owl:allValuesFrom :Location ;
	owl:onProperty <http://ns.cerise-project.nl/energy/def/cim-smartgrid#PositionPoint.Location> .

<http://ns.cerise-project.nl/energy/def/cim-smartgrid#PositionPoint.Location> a owl:ObjectProperty .

:PositionPoint rdfs:subClassOf _:node1912nb34nx104 .

_:node1912nb34nx104 a owl:Restriction ;
	owl:allValuesFrom xsd:string ;
	owl:onProperty <http://ns.cerise-project.nl/energy/def/cim-smartgrid#PositionPoint.xPosition> .

:PositionPoint rdfs:subClassOf _:node1912nb34nx105 .

_:node1912nb34nx105 a owl:Restriction ;
	owl:allValuesFrom xsd:string ;
	owl:onProperty <http://ns.cerise-project.nl/energy/def/cim-smartgrid#PositionPoint.zPosition> .

<http://ns.cerise-project.nl/energy/def/cim-smartgrid#PositionPoint.zPosition> a owl:DatatypeProperty .

:PositionPoint rdfs:subClassOf _:node1912nb34nx106 .

_:node1912nb34nx106 a owl:Restriction ;
	owl:allValuesFrom xsd:integer ;
	owl:onProperty <http://ns.cerise-project.nl/energy/def/cim-smartgrid#PositionPoint.sequenceNumber> .

:PositionPoint rdfs:comment "Set of spatial coordinates that determine a point, defined in coordinate system specified in 'Location.CoordinateSystem'. Use a single position point instance to desribe a point-oriented location. Use a sequence of position points to describe a line-oriented object (physical location of non-point oriented objects like cables or lines), or area of an object (like a substation or a geographical zone - in this case, have first and last position point with the same values)." ;
	rdfs:isDefinedBy :Package_Common ;
	rdfs:subClassOf _:node1912nb34nx107 .

_:node1912nb34nx107 a owl:Restriction ;
	owl:cardinality "1"^^xsd:int ;
	owl:onProperty <http://ns.cerise-project.nl/energy/def/cim-smartgrid#PositionPoint.yPosition> .

<http://ns.cerise-project.nl/energy/def/cim-smartgrid#PositionPoint.yPosition> a owl:DatatypeProperty .

:PositionPoint rdfs:subClassOf _:node1912nb34nx108 .

_:node1912nb34nx108 a owl:Restriction ;
	owl:cardinality "1"^^xsd:int ;
	owl:onProperty <http://ns.cerise-project.nl/energy/def/cim-smartgrid#PositionPoint.Location> .

:PositionPoint rdfs:subClassOf _:node1912nb34nx109 .

_:node1912nb34nx109 a owl:Restriction ;
	owl:cardinality "1"^^xsd:int ;
	owl:onProperty <http://ns.cerise-project.nl/energy/def/cim-smartgrid#PositionPoint.zPosition> .

:PositionPoint rdfs:subClassOf _:node1912nb34nx110 .

_:node1912nb34nx110 a owl:Restriction ;
	owl:allValuesFrom xsd:string ;
	owl:onProperty <http://ns.cerise-project.nl/energy/def/cim-smartgrid#PositionPoint.yPosition> .

:SupplierKind a owl:Class ;
	rdfs:label "SupplierKind" ;
	uml:hasStereotype uml:enumeration ;
	rdfs:comment "Kind of supplier." ;
	rdfs:isDefinedBy :Package_PaymentMetering .

:Package_PaymentMetering a uml:Package ;
	rdfs:label "PaymentMetering" ;
	rdfs:comment "This package is an extension of the Metering package and contains the information classes that support specialised applications such as prepayment metering. These classes are generally associated with the collection and control of revenue from the customer for a delivered service." ;
	rdfs:isDefinedBy :Package_IEC61968 .

:MeterReading a owl:Class ;
	rdfs:subClassOf :IdentifiedObject , _:node1912nb34nx111 .

_:node1912nb34nx111 a owl:Restriction ;
	owl:allValuesFrom :Reading .

:Reading a owl:Class .

_:node1912nb34nx111 owl:onProperty <http://ns.cerise-project.nl/energy/def/cim-smartgrid#MeterReading.Readings> .

<http://ns.cerise-project.nl/energy/def/cim-smartgrid#MeterReading.Readings> a owl:ObjectProperty .

:MeterReading rdfs:subClassOf _:node1912nb34nx112 .

_:node1912nb34nx112 a owl:Restriction ;
	owl:minCardinality "1"^^xsd:int ;
	owl:onProperty <http://ns.cerise-project.nl/energy/def/cim-smartgrid#MeterReading.Readings> .

:MeterReading rdfs:subClassOf _:node1912nb34nx113 .

_:node1912nb34nx113 a owl:Restriction ;
	owl:cardinality "1"^^xsd:int ;
	owl:onProperty <http://ns.cerise-project.nl/energy/def/cim-smartgrid#MeterReading.UsagePoint> .

<http://ns.cerise-project.nl/energy/def/cim-smartgrid#MeterReading.UsagePoint> a owl:ObjectProperty .

:MeterReading rdfs:subClassOf _:node1912nb34nx114 .

_:node1912nb34nx114 a owl:Restriction ;
	owl:cardinality "1"^^xsd:int ;
	owl:onProperty <http://ns.cerise-project.nl/energy/def/cim-smartgrid#MeterReading.CustomerAgreement> .

<http://ns.cerise-project.nl/energy/def/cim-smartgrid#MeterReading.CustomerAgreement> a owl:ObjectProperty .

:MeterReading rdfs:subClassOf _:node1912nb34nx115 .

_:node1912nb34nx115 a owl:Restriction ;
	owl:allValuesFrom :UsagePoint ;
	owl:onProperty <http://ns.cerise-project.nl/energy/def/cim-smartgrid#MeterReading.UsagePoint> .

:MeterReading rdfs:comment "Set of values obtained from the meter." ;
	rdfs:subClassOf _:node1912nb34nx116 .

_:node1912nb34nx116 a owl:Restriction ;
	owl:allValuesFrom :CustomerAgreement .

:CustomerAgreement a owl:Class .

_:node1912nb34nx116 owl:onProperty <http://ns.cerise-project.nl/energy/def/cim-smartgrid#MeterReading.CustomerAgreement> .

:MeterReading rdfs:subClassOf _:node1912nb34nx117 .

_:node1912nb34nx117 a owl:Restriction ;
	owl:cardinality "1"^^xsd:int ;
	owl:onProperty <http://ns.cerise-project.nl/energy/def/cim-smartgrid#MeterReading.Meter> .

<http://ns.cerise-project.nl/energy/def/cim-smartgrid#MeterReading.Meter> a owl:ObjectProperty .

:MeterReading rdfs:subClassOf _:node1912nb34nx118 .

_:node1912nb34nx118 a owl:Restriction ;
	owl:cardinality "1"^^xsd:int ;
	owl:onProperty <http://ns.cerise-project.nl/energy/def/cim-smartgrid#MeterReading.valuesInterval> .

<http://ns.cerise-project.nl/energy/def/cim-smartgrid#MeterReading.valuesInterval> a owl:ObjectProperty .

:MeterReading rdfs:isDefinedBy :Package_Metering ;
	rdfs:subClassOf _:node1912nb34nx119 .

_:node1912nb34nx119 a owl:Restriction ;
	owl:onProperty <http://ns.cerise-project.nl/energy/def/cim-smartgrid#MeterReading.valuesInterval> ;
	owl:allValuesFrom :DateTimeInterval .

:MeterReading rdfs:subClassOf _:node1912nb34nx120 .

_:node1912nb34nx120 a owl:Restriction ;
	owl:allValuesFrom :Meter ;
	owl:onProperty <http://ns.cerise-project.nl/energy/def/cim-smartgrid#MeterReading.Meter> .

:MeterReading rdfs:label "MeterReading" .

:Location rdfs:subClassOf _:node1912nb34nx121 .

_:node1912nb34nx121 a owl:Restriction ;
	owl:cardinality "1"^^xsd:int ;
	owl:onProperty <http://ns.cerise-project.nl/energy/def/cim-smartgrid#Location.mainAddress> .

<http://ns.cerise-project.nl/energy/def/cim-smartgrid#Location.mainAddress> a owl:ObjectProperty .

:Location rdfs:subClassOf _:node1912nb34nx122 .

_:node1912nb34nx122 a owl:Restriction ;
	owl:allValuesFrom :StreetAddress ;
	owl:onProperty <http://ns.cerise-project.nl/energy/def/cim-smartgrid#Location.mainAddress> .

:Location rdfs:subClassOf _:node1912nb34nx123 .

_:node1912nb34nx123 a owl:Restriction ;
	owl:onProperty <http://ns.cerise-project.nl/energy/def/cim-smartgrid#Location.electronicAddress> .

<http://ns.cerise-project.nl/energy/def/cim-smartgrid#Location.electronicAddress> a owl:ObjectProperty .

_:node1912nb34nx123 owl:allValuesFrom :ElectronicAddress .

:Location rdfs:subClassOf _:node1912nb34nx124 .

_:node1912nb34nx124 a owl:Restriction ;
	owl:cardinality "1"^^xsd:int ;
	owl:onProperty <http://ns.cerise-project.nl/energy/def/cim-smartgrid#Location.type> .

<http://ns.cerise-project.nl/energy/def/cim-smartgrid#Location.type> a owl:DatatypeProperty .

:Location rdfs:subClassOf _:node1912nb34nx125 .

_:node1912nb34nx125 a owl:Restriction ;
	owl:cardinality "1"^^xsd:int ;
	owl:onProperty <http://ns.cerise-project.nl/energy/def/cim-smartgrid#Location.phone2> .

<http://ns.cerise-project.nl/energy/def/cim-smartgrid#Location.phone2> a owl:ObjectProperty .

:Location rdfs:subClassOf _:node1912nb34nx126 .

_:node1912nb34nx126 a owl:Restriction ;
	owl:cardinality "1"^^xsd:int ;
	owl:onProperty <http://ns.cerise-project.nl/energy/def/cim-smartgrid#Location.electronicAddress> .

:Location rdfs:subClassOf :IdentifiedObject , _:node1912nb34nx127 .

_:node1912nb34nx127 a owl:Restriction ;
	owl:cardinality "1"^^xsd:int ;
	owl:onProperty <http://ns.cerise-project.nl/energy/def/cim-smartgrid#Location.geoInfoReference> .

<http://ns.cerise-project.nl/energy/def/cim-smartgrid#Location.geoInfoReference> a owl:DatatypeProperty .

:Location rdfs:subClassOf _:node1912nb34nx128 .

_:node1912nb34nx128 a owl:Restriction ;
	owl:onProperty <http://ns.cerise-project.nl/energy/def/cim-smartgrid#Location.status> .

<http://ns.cerise-project.nl/energy/def/cim-smartgrid#Location.status> a owl:ObjectProperty .

_:node1912nb34nx128 owl:allValuesFrom :Status .

:Location rdfs:subClassOf _:node1912nb34nx129 .

_:node1912nb34nx129 a owl:Restriction ;
	owl:minCardinality "1"^^xsd:int ;
	owl:onProperty <http://ns.cerise-project.nl/energy/def/cim-smartgrid#Location.PositionPoints> .

<http://ns.cerise-project.nl/energy/def/cim-smartgrid#Location.PositionPoints> a owl:ObjectProperty .

:Location rdfs:subClassOf _:node1912nb34nx130 .

_:node1912nb34nx130 a owl:Restriction ;
	owl:onProperty <http://ns.cerise-project.nl/energy/def/cim-smartgrid#Location.CoordinateSystem> .

<http://ns.cerise-project.nl/energy/def/cim-smartgrid#Location.CoordinateSystem> a owl:ObjectProperty .

_:node1912nb34nx130 owl:allValuesFrom :CoordinateSystem .

:Location rdfs:subClassOf _:node1912nb34nx131 .

_:node1912nb34nx131 a owl:Restriction ;
	owl:allValuesFrom :StreetAddress ;
	owl:onProperty <http://ns.cerise-project.nl/energy/def/cim-smartgrid#Location.secondaryAddress> .

<http://ns.cerise-project.nl/energy/def/cim-smartgrid#Location.secondaryAddress> a owl:ObjectProperty .

:Location rdfs:subClassOf _:node1912nb34nx132 .

_:node1912nb34nx132 a owl:Restriction ;
	owl:cardinality "1"^^xsd:int ;
	owl:onProperty <http://ns.cerise-project.nl/energy/def/cim-smartgrid#Location.secondaryAddress> .

:Location rdfs:label "Location" ;
	rdfs:subClassOf _:node1912nb34nx133 .

_:node1912nb34nx133 a owl:Restriction ;
	owl:cardinality "1"^^xsd:int ;
	owl:onProperty <http://ns.cerise-project.nl/energy/def/cim-smartgrid#Location.phone1> .

<http://ns.cerise-project.nl/energy/def/cim-smartgrid#Location.phone1> a owl:ObjectProperty .

:Location rdfs:isDefinedBy :Package_Common ;
	rdfs:subClassOf _:node1912nb34nx134 .

_:node1912nb34nx134 a owl:Restriction ;
	owl:cardinality "1"^^xsd:int ;
	owl:onProperty <http://ns.cerise-project.nl/energy/def/cim-smartgrid#Location.CoordinateSystem> .

:Location rdfs:subClassOf _:node1912nb34nx135 .

_:node1912nb34nx135 a owl:Restriction ;
	owl:onProperty <http://ns.cerise-project.nl/energy/def/cim-smartgrid#Location.phone1> ;
	owl:allValuesFrom :TelephoneNumber .

:TelephoneNumber a owl:Class .

:Location rdfs:subClassOf _:node1912nb34nx136 .

_:node1912nb34nx136 a owl:Restriction ;
	owl:allValuesFrom xsd:string ;
	owl:onProperty <http://ns.cerise-project.nl/energy/def/cim-smartgrid#Location.geoInfoReference> .

:Location rdfs:subClassOf _:node1912nb34nx137 .

_:node1912nb34nx137 a owl:Restriction ;
	owl:allValuesFrom xsd:string ;
	owl:onProperty <http://ns.cerise-project.nl/energy/def/cim-smartgrid#Location.type> .

:Location rdfs:subClassOf _:node1912nb34nx138 .

_:node1912nb34nx138 a owl:Restriction ;
	owl:allValuesFrom :TelephoneNumber ;
	owl:onProperty <http://ns.cerise-project.nl/energy/def/cim-smartgrid#Location.phone2> .

:Location rdfs:comment "The place, scene, or point of something where someone or something has been, is, and/or will be at a given moment in time. It can be defined with one or more postition points (coordinates) in a given coordinate system." ;
	rdfs:subClassOf _:node1912nb34nx139 .

_:node1912nb34nx139 a owl:Restriction ;
	owl:cardinality "1"^^xsd:int ;
	owl:onProperty <http://ns.cerise-project.nl/energy/def/cim-smartgrid#Location.status> .

:Location rdfs:subClassOf _:node1912nb34nx140 .

_:node1912nb34nx140 a owl:Restriction ;
	owl:allValuesFrom :PositionPoint ;
	owl:onProperty <http://ns.cerise-project.nl/energy/def/cim-smartgrid#Location.PositionPoints> .

:IntervalBlock rdfs:subClassOf _:node1912nb34nx141 .

_:node1912nb34nx141 a owl:Restriction ;
	owl:minCardinality "1"^^xsd:int ;
	owl:onProperty <http://ns.cerise-project.nl/energy/def/cim-smartgrid#IntervalBlock.IntervalReadings> .

<http://ns.cerise-project.nl/energy/def/cim-smartgrid#IntervalBlock.IntervalReadings> a owl:ObjectProperty .

:IntervalBlock rdfs:label "IntervalBlock" ;
	rdfs:subClassOf _:node1912nb34nx142 .

_:node1912nb34nx142 a owl:Restriction ;
	owl:cardinality "1"^^xsd:int ;
	owl:onProperty <http://ns.cerise-project.nl/energy/def/cim-smartgrid#IntervalBlock.MeterReading> .

<http://ns.cerise-project.nl/energy/def/cim-smartgrid#IntervalBlock.MeterReading> a owl:ObjectProperty .

:IntervalBlock rdfs:subClassOf _:node1912nb34nx143 .

_:node1912nb34nx143 a owl:Restriction ;
	owl:allValuesFrom :ReadingType ;
	owl:onProperty <http://ns.cerise-project.nl/energy/def/cim-smartgrid#IntervalBlock.ReadingType> .

<http://ns.cerise-project.nl/energy/def/cim-smartgrid#IntervalBlock.ReadingType> a owl:ObjectProperty .

:IntervalBlock rdfs:comment "Time sequence of readings of the same reading type. Contained interval readings may need conversion through the application of an offset and a scalar defined in associated pending." ;
	rdfs:subClassOf _:node1912nb34nx144 .

_:node1912nb34nx144 a owl:Restriction ;
	owl:onProperty <http://ns.cerise-project.nl/energy/def/cim-smartgrid#IntervalBlock.IntervalReadings> ;
	owl:allValuesFrom :IntervalReading .

:IntervalBlock rdfs:subClassOf _:node1912nb34nx145 .

_:node1912nb34nx145 a owl:Restriction ;
	owl:cardinality "1"^^xsd:int ;
	owl:onProperty <http://ns.cerise-project.nl/energy/def/cim-smartgrid#IntervalBlock.ReadingType> .

:IntervalBlock rdfs:isDefinedBy :Package_Metering ;
	rdfs:subClassOf _:node1912nb34nx146 .

_:node1912nb34nx146 a owl:Restriction ;
	owl:allValuesFrom :MeterReading ;
	owl:onProperty <http://ns.cerise-project.nl/energy/def/cim-smartgrid#IntervalBlock.MeterReading> .

:SimpleEndDeviceFunction a owl:Class ;
	rdfs:subClassOf _:node1912nb34nx147 .

_:node1912nb34nx147 a owl:Restriction ;
	owl:cardinality "1"^^xsd:int ;
	owl:onProperty <http://ns.cerise-project.nl/energy/def/cim-smartgrid#SimpleEndDeviceFunction.kind> .

<http://ns.cerise-project.nl/energy/def/cim-smartgrid#SimpleEndDeviceFunction.kind> a owl:ObjectProperty .

:SimpleEndDeviceFunction rdfs:subClassOf _:node1912nb34nx148 .

_:node1912nb34nx148 a owl:Restriction ;
	owl:allValuesFrom :EndDeviceFunctionKind ;
	owl:onProperty <http://ns.cerise-project.nl/energy/def/cim-smartgrid#SimpleEndDeviceFunction.kind> .

:SimpleEndDeviceFunction rdfs:subClassOf :EndDeviceFunction ;
	rdfs:comment "Simple end device function distinguished by 'kind'. Use this class for instances that cannot be represented by another end device function specialisations." ;
	rdfs:label "SimpleEndDeviceFunction" ;
	rdfs:isDefinedBy :Package_Metering .

:Meter rdfs:subClassOf _:node1912nb34nx149 .

_:node1912nb34nx149 a owl:Restriction ;
	owl:allValuesFrom :MeterMultiplier ;
	owl:onProperty <http://ns.cerise-project.nl/energy/def/cim-smartgrid#Meter.MeterMultipliers> .

<http://ns.cerise-project.nl/energy/def/cim-smartgrid#Meter.MeterMultipliers> a owl:ObjectProperty .

:Meter rdfs:isDefinedBy :Package_Metering ;
	rdfs:label "Meter" ;
	rdfs:subClassOf _:node1912nb34nx150 .

_:node1912nb34nx150 a owl:Restriction ;
	owl:minCardinality "1"^^xsd:int ;
	owl:onProperty <http://ns.cerise-project.nl/energy/def/cim-smartgrid#Meter.MeterReadings> .

<http://ns.cerise-project.nl/energy/def/cim-smartgrid#Meter.MeterReadings> a owl:ObjectProperty .

:Meter rdfs:subClassOf _:node1912nb34nx151 .

_:node1912nb34nx151 a owl:Restriction ;
	owl:cardinality "1"^^xsd:int ;
	owl:onProperty <http://ns.cerise-project.nl/energy/def/cim-smartgrid#Meter.formNumber> .

<http://ns.cerise-project.nl/energy/def/cim-smartgrid#Meter.formNumber> a owl:DatatypeProperty .

:Meter rdfs:comment "Physical asset that performs the metering role of the usage point. Used for measuring consumption and detection of events." ;
	rdfs:subClassOf _:node1912nb34nx152 .

_:node1912nb34nx152 a owl:Restriction ;
	owl:onProperty <http://ns.cerise-project.nl/energy/def/cim-smartgrid#Meter.MeterReadings> ;
	owl:allValuesFrom :MeterReading .

:Meter rdfs:subClassOf _:node1912nb34nx153 .

_:node1912nb34nx153 a owl:Restriction ;
	owl:allValuesFrom xsd:string ;
	owl:onProperty <http://ns.cerise-project.nl/energy/def/cim-smartgrid#Meter.formNumber> .

:Meter rdfs:subClassOf :EndDevice , _:node1912nb34nx154 .

_:node1912nb34nx154 a owl:Restriction ;
	owl:minCardinality "1"^^xsd:int ;
	owl:onProperty <http://ns.cerise-project.nl/energy/def/cim-smartgrid#Meter.MeterMultipliers> .

:CustomerAgreement rdfs:subClassOf _:node1912nb34nx155 .

_:node1912nb34nx155 a owl:Restriction ;
	owl:allValuesFrom :ServiceCategory ;
	owl:onProperty <http://ns.cerise-project.nl/energy/def/cim-smartgrid#CustomerAgreement.ServiceCategory> .

<http://ns.cerise-project.nl/energy/def/cim-smartgrid#CustomerAgreement.ServiceCategory> a owl:ObjectProperty .

:CustomerAgreement rdfs:label "CustomerAgreement" ;
	rdfs:subClassOf :IdentifiedObject , _:node1912nb34nx156 .

_:node1912nb34nx156 a owl:Restriction ;
	owl:cardinality "1"^^xsd:int ;
	owl:onProperty <http://ns.cerise-project.nl/energy/def/cim-smartgrid#CustomerAgreement.Customer> .

<http://ns.cerise-project.nl/energy/def/cim-smartgrid#CustomerAgreement.Customer> a owl:ObjectProperty .

:CustomerAgreement rdfs:isDefinedBy :Package_Customers ;
	rdfs:subClassOf _:node1912nb34nx157 .

_:node1912nb34nx157 a owl:Restriction ;
	owl:allValuesFrom :Customer .

:Customer a owl:Class .

_:node1912nb34nx157 owl:onProperty <http://ns.cerise-project.nl/energy/def/cim-smartgrid#CustomerAgreement.Customer> .

:CustomerAgreement rdfs:subClassOf _:node1912nb34nx158 .

_:node1912nb34nx158 a owl:Restriction ;
	owl:cardinality "1"^^xsd:int ;
	owl:onProperty <http://ns.cerise-project.nl/energy/def/cim-smartgrid#CustomerAgreement.ServiceCategory> .

:CustomerAgreement rdfs:subClassOf _:node1912nb34nx159 .

_:node1912nb34nx159 a owl:Restriction ;
	owl:cardinality "1"^^xsd:int ;
	owl:onProperty <http://ns.cerise-project.nl/energy/def/cim-smartgrid#CustomerAgreement.ServiceSupplier> .

<http://ns.cerise-project.nl/energy/def/cim-smartgrid#CustomerAgreement.ServiceSupplier> a owl:ObjectProperty .

:CustomerAgreement rdfs:comment "Agreement between the customer and the service supplier to pay for service at a specific service location. It records certain billing information about the type of service provided at the service location and is used during charge creation to determine the type of service." ;
	rdfs:subClassOf _:node1912nb34nx160 .

_:node1912nb34nx160 a owl:Restriction ;
	owl:allValuesFrom :ServiceSupplier .

:ServiceSupplier a owl:Class .

_:node1912nb34nx160 owl:onProperty <http://ns.cerise-project.nl/energy/def/cim-smartgrid#CustomerAgreement.ServiceSupplier> .

:Reading rdfs:subClassOf _:node1912nb34nx161 .

_:node1912nb34nx161 a owl:Restriction ;
	owl:minCardinality "1"^^xsd:int ;
	owl:onProperty <http://ns.cerise-project.nl/energy/def/cim-smartgrid#Reading.MeterReadings> .

<http://ns.cerise-project.nl/energy/def/cim-smartgrid#Reading.MeterReadings> a owl:ObjectProperty .

:Reading rdfs:subClassOf _:node1912nb34nx162 .

_:node1912nb34nx162 a owl:Restriction ;
	owl:onProperty <http://ns.cerise-project.nl/energy/def/cim-smartgrid#Reading.MeterReadings> ;
	owl:allValuesFrom :MeterReading .

:Reading rdfs:subClassOf _:node1912nb34nx163 .

_:node1912nb34nx163 a owl:Restriction ;
	owl:cardinality "1"^^xsd:int ;
	owl:onProperty <http://ns.cerise-project.nl/energy/def/cim-smartgrid#Reading.ReadingType> .

<http://ns.cerise-project.nl/energy/def/cim-smartgrid#Reading.ReadingType> a owl:ObjectProperty .

:Reading rdfs:subClassOf _:node1912nb34nx164 .

_:node1912nb34nx164 a owl:Restriction ;
	owl:allValuesFrom :ReadingType ;
	owl:onProperty <http://ns.cerise-project.nl/energy/def/cim-smartgrid#Reading.ReadingType> .

:Reading rdfs:subClassOf :BaseReading ;
	rdfs:comment "Specific value measured by a meter or other asset, or calculated by a system. Each Reading is associated with a specific ReadingType." ;
	rdfs:label "Reading" ;
	rdfs:isDefinedBy :Package_Metering .

:CustomerKind a owl:Class ;
	uml:hasStereotype uml:enumeration ;
	rdfs:comment "Kind of customer." ;
	rdfs:label "CustomerKind" ;
	rdfs:isDefinedBy :Package_Customers .

:UsagePoint rdfs:subClassOf _:node1912nb34nx165 .

_:node1912nb34nx165 a owl:Restriction ;
	owl:cardinality "1"^^xsd:int ;
	owl:onProperty <http://ns.cerise-project.nl/energy/def/cim-smartgrid#UsagePoint.ServiceSupplier> .

<http://ns.cerise-project.nl/energy/def/cim-smartgrid#UsagePoint.ServiceSupplier> a owl:ObjectProperty .

:UsagePoint rdfs:subClassOf :IdentifiedObject , _:node1912nb34nx166 .

_:node1912nb34nx166 a owl:Restriction ;
	owl:allValuesFrom xsd:boolean ;
	owl:onProperty <http://ns.cerise-project.nl/energy/def/cim-smartgrid#UsagePoint.isVirtual> .

<http://ns.cerise-project.nl/energy/def/cim-smartgrid#UsagePoint.isVirtual> a owl:DatatypeProperty .

:UsagePoint rdfs:subClassOf _:node1912nb34nx167 .

_:node1912nb34nx167 a owl:Restriction ;
	owl:cardinality "1"^^xsd:int ;
	owl:onProperty <http://ns.cerise-project.nl/energy/def/cim-smartgrid#UsagePoint.ServiceCategory> .

<http://ns.cerise-project.nl/energy/def/cim-smartgrid#UsagePoint.ServiceCategory> a owl:ObjectProperty .

:UsagePoint rdfs:subClassOf _:node1912nb34nx168 .

_:node1912nb34nx168 a owl:Restriction ;
	owl:allValuesFrom :ServiceSupplier ;
	owl:onProperty <http://ns.cerise-project.nl/energy/def/cim-smartgrid#UsagePoint.ServiceSupplier> .

:UsagePoint rdfs:subClassOf _:node1912nb34nx169 .

_:node1912nb34nx169 a owl:Restriction ;
	owl:allValuesFrom :CustomerAgreement ;
	owl:onProperty <http://ns.cerise-project.nl/energy/def/cim-smartgrid#UsagePoint.CustomerAgreement> .

<http://ns.cerise-project.nl/energy/def/cim-smartgrid#UsagePoint.CustomerAgreement> a owl:ObjectProperty .

:UsagePoint rdfs:subClassOf _:node1912nb34nx170 .

_:node1912nb34nx170 a owl:Restriction ;
	owl:onProperty <http://ns.cerise-project.nl/energy/def/cim-smartgrid#UsagePoint.ServiceCategory> ;
	owl:allValuesFrom :ServiceCategory .

:UsagePoint rdfs:label "UsagePoint" ;
	rdfs:subClassOf _:node1912nb34nx171 .

_:node1912nb34nx171 a owl:Restriction ;
	owl:minCardinality "1"^^xsd:int ;
	owl:onProperty <http://ns.cerise-project.nl/energy/def/cim-smartgrid#UsagePoint.MeterReadings> .

<http://ns.cerise-project.nl/energy/def/cim-smartgrid#UsagePoint.MeterReadings> a owl:ObjectProperty .

:UsagePoint rdfs:comment "Logical or physical point in the network to which readings or events may be attributed. Used at the place where a physical or virtual meter may be located; however, it is not required that a meter be present." ;
	rdfs:subClassOf _:node1912nb34nx172 .

_:node1912nb34nx172 a owl:Restriction ;
	owl:cardinality "1"^^xsd:int ;
	owl:onProperty <http://ns.cerise-project.nl/energy/def/cim-smartgrid#UsagePoint.amiBillingReady> .

<http://ns.cerise-project.nl/energy/def/cim-smartgrid#UsagePoint.amiBillingReady> a owl:ObjectProperty .

:UsagePoint rdfs:subClassOf _:node1912nb34nx173 .

_:node1912nb34nx173 a owl:Restriction ;
	owl:onProperty <http://ns.cerise-project.nl/energy/def/cim-smartgrid#UsagePoint.UsagePointLocation> .

<http://ns.cerise-project.nl/energy/def/cim-smartgrid#UsagePoint.UsagePointLocation> a owl:ObjectProperty .

_:node1912nb34nx173 owl:allValuesFrom :UsagePointLocation .

:UsagePoint rdfs:subClassOf _:node1912nb34nx174 .

_:node1912nb34nx174 a owl:Restriction ;
	owl:cardinality "1"^^xsd:int ;
	owl:onProperty <http://ns.cerise-project.nl/energy/def/cim-smartgrid#UsagePoint.CustomerAgreement> .

:UsagePoint rdfs:isDefinedBy :Package_Metering ;
	rdfs:subClassOf _:node1912nb34nx175 .

_:node1912nb34nx175 a owl:Restriction ;
	owl:onProperty <http://ns.cerise-project.nl/energy/def/cim-smartgrid#UsagePoint.amiBillingReady> ;
	owl:allValuesFrom :AmiBillingReadyKind .

:UsagePoint rdfs:subClassOf _:node1912nb34nx176 .

_:node1912nb34nx176 a owl:Restriction ;
	owl:allValuesFrom xsd:boolean ;
	owl:onProperty <http://ns.cerise-project.nl/energy/def/cim-smartgrid#UsagePoint.isSdp> .

<http://ns.cerise-project.nl/energy/def/cim-smartgrid#UsagePoint.isSdp> a owl:DatatypeProperty .

:UsagePoint rdfs:subClassOf _:node1912nb34nx177 .

_:node1912nb34nx177 a owl:Restriction ;
	owl:cardinality "1"^^xsd:int ;
	owl:onProperty <http://ns.cerise-project.nl/energy/def/cim-smartgrid#UsagePoint.UsagePointLocation> .

:UsagePoint rdfs:subClassOf _:node1912nb34nx178 .

_:node1912nb34nx178 a owl:Restriction ;
	owl:cardinality "1"^^xsd:int ;
	owl:onProperty <http://ns.cerise-project.nl/energy/def/cim-smartgrid#UsagePoint.isVirtual> .

:UsagePoint rdfs:subClassOf _:node1912nb34nx179 .

_:node1912nb34nx179 a owl:Restriction ;
	owl:cardinality "1"^^xsd:int ;
	owl:onProperty <http://ns.cerise-project.nl/energy/def/cim-smartgrid#UsagePoint.isSdp> .

:UsagePoint rdfs:subClassOf _:node1912nb34nx180 .

_:node1912nb34nx180 a owl:Restriction ;
	owl:allValuesFrom :MeterReading ;
	owl:onProperty <http://ns.cerise-project.nl/energy/def/cim-smartgrid#UsagePoint.MeterReadings> .

:ServiceSupplier rdfs:subClassOf _:node1912nb34nx181 .

_:node1912nb34nx181 a owl:Restriction ;
	owl:cardinality "1"^^xsd:int ;
	owl:onProperty <http://ns.cerise-project.nl/energy/def/cim-smartgrid#ServiceSupplier.issuerIdentificationNumber> .

<http://ns.cerise-project.nl/energy/def/cim-smartgrid#ServiceSupplier.issuerIdentificationNumber> a owl:DatatypeProperty .

:ServiceSupplier rdfs:subClassOf _:node1912nb34nx182 .

_:node1912nb34nx182 a owl:Restriction ;
	owl:allValuesFrom xsd:string ;
	owl:onProperty <http://ns.cerise-project.nl/energy/def/cim-smartgrid#ServiceSupplier.issuerIdentificationNumber> .

:ServiceSupplier rdfs:subClassOf _:node1912nb34nx183 .

_:node1912nb34nx183 a owl:Restriction ;
	owl:cardinality "1"^^xsd:int ;
	owl:onProperty <http://ns.cerise-project.nl/energy/def/cim-smartgrid#ServiceSupplier.kind> .

<http://ns.cerise-project.nl/energy/def/cim-smartgrid#ServiceSupplier.kind> a owl:ObjectProperty .

:ServiceSupplier rdfs:subClassOf _:node1912nb34nx184 .

_:node1912nb34nx184 a owl:Restriction ;
	owl:onProperty <http://ns.cerise-project.nl/energy/def/cim-smartgrid#ServiceSupplier.kind> ;
	owl:allValuesFrom :SupplierKind .

:ServiceSupplier rdfs:subClassOf :OrganisationRole .

:OrganisationRole a owl:Class .

:ServiceSupplier rdfs:comment "Organisation that provides services to customers." ;
	rdfs:label "ServiceSupplier" ;
	rdfs:isDefinedBy :Package_PaymentMetering .

:OrganisationRole rdfs:subClassOf :IdentifiedObject ;
	rdfs:comment "Identifies a way in which an organisation may participate in the utility enterprise (e.g., customer, manufacturer, etc)." ;
	rdfs:label "OrganisationRole" ;
	rdfs:isDefinedBy :Package_Common .

:Customer rdfs:isDefinedBy :Package_Customers ;
	rdfs:subClassOf _:node1912nb34nx185 .

_:node1912nb34nx185 a owl:Restriction ;
	owl:cardinality "1"^^xsd:int ;
	owl:onProperty <http://ns.cerise-project.nl/energy/def/cim-smartgrid#Customer.kind> .

<http://ns.cerise-project.nl/energy/def/cim-smartgrid#Customer.kind> a owl:ObjectProperty .

:Customer rdfs:subClassOf _:node1912nb34nx186 .

_:node1912nb34nx186 a owl:Restriction ;
	owl:allValuesFrom :CustomerKind ;
	owl:onProperty <http://ns.cerise-project.nl/energy/def/cim-smartgrid#Customer.kind> .

:Customer rdfs:comment "Organisation receiving services from service supplier." ;
	rdfs:label "Customer" ;
	rdfs:subClassOf :OrganisationRole .

:TownDetail rdfs:subClassOf _:node1912nb34nx187 .

_:node1912nb34nx187 a owl:Restriction ;
	owl:allValuesFrom xsd:string ;
	owl:onProperty <http://ns.cerise-project.nl/energy/def/cim-smartgrid#TownDetail.section> .

<http://ns.cerise-project.nl/energy/def/cim-smartgrid#TownDetail.section> a owl:DatatypeProperty .

:TownDetail uml:hasStereotype uml:compound ;
	rdfs:subClassOf _:node1912nb34nx188 .

_:node1912nb34nx188 a owl:Restriction ;
	owl:cardinality "1"^^xsd:int ;
	owl:onProperty <http://ns.cerise-project.nl/energy/def/cim-smartgrid#TownDetail.section> .

:TownDetail rdfs:comment "Town details, in the context of address." ;
	rdfs:subClassOf _:node1912nb34nx189 .

_:node1912nb34nx189 a owl:Restriction ;
	owl:cardinality "1"^^xsd:int ;
	owl:onProperty <http://ns.cerise-project.nl/energy/def/cim-smartgrid#TownDetail.stateOrProvince> .

<http://ns.cerise-project.nl/energy/def/cim-smartgrid#TownDetail.stateOrProvince> a owl:DatatypeProperty .

:TownDetail rdfs:subClassOf _:node1912nb34nx190 .

_:node1912nb34nx190 a owl:Restriction ;
	owl:allValuesFrom xsd:string ;
	owl:onProperty <http://ns.cerise-project.nl/energy/def/cim-smartgrid#TownDetail.name> .

<http://ns.cerise-project.nl/energy/def/cim-smartgrid#TownDetail.name> a owl:DatatypeProperty .

:TownDetail rdfs:subClassOf _:node1912nb34nx191 .

_:node1912nb34nx191 a owl:Restriction ;
	owl:allValuesFrom xsd:string ;
	owl:onProperty <http://ns.cerise-project.nl/energy/def/cim-smartgrid#TownDetail.country> .

<http://ns.cerise-project.nl/energy/def/cim-smartgrid#TownDetail.country> a owl:DatatypeProperty .

:TownDetail rdfs:subClassOf _:node1912nb34nx192 .

_:node1912nb34nx192 a owl:Restriction ;
	owl:cardinality "1"^^xsd:int ;
	owl:onProperty <http://ns.cerise-project.nl/energy/def/cim-smartgrid#TownDetail.name> .

:TownDetail rdfs:subClassOf _:node1912nb34nx193 .

_:node1912nb34nx193 a owl:Restriction ;
	owl:cardinality "1"^^xsd:int ;
	owl:onProperty <http://ns.cerise-project.nl/energy/def/cim-smartgrid#TownDetail.code> .

<http://ns.cerise-project.nl/energy/def/cim-smartgrid#TownDetail.code> a owl:DatatypeProperty .

:TownDetail rdfs:subClassOf _:node1912nb34nx194 .

_:node1912nb34nx194 a owl:Restriction ;
	owl:allValuesFrom xsd:string ;
	owl:onProperty <http://ns.cerise-project.nl/energy/def/cim-smartgrid#TownDetail.code> .

:TownDetail rdfs:label "TownDetail" ;
	rdfs:subClassOf _:node1912nb34nx195 .

_:node1912nb34nx195 a owl:Restriction ;
	owl:allValuesFrom xsd:string ;
	owl:onProperty <http://ns.cerise-project.nl/energy/def/cim-smartgrid#TownDetail.stateOrProvince> .

:TownDetail rdfs:subClassOf _:node1912nb34nx196 .

_:node1912nb34nx196 a owl:Restriction ;
	owl:cardinality "1"^^xsd:int ;
	owl:onProperty <http://ns.cerise-project.nl/energy/def/cim-smartgrid#TownDetail.country> .

:TownDetail rdfs:isDefinedBy :Package_Common .

:TelephoneNumber uml:hasStereotype uml:compound ;
	rdfs:isDefinedBy :Package_Common ;
	rdfs:subClassOf _:node1912nb34nx197 .

_:node1912nb34nx197 a owl:Restriction ;
	owl:allValuesFrom xsd:string ;
	owl:onProperty <http://ns.cerise-project.nl/energy/def/cim-smartgrid#TelephoneNumber.localNumber> .

<http://ns.cerise-project.nl/energy/def/cim-smartgrid#TelephoneNumber.localNumber> a owl:DatatypeProperty .

:TelephoneNumber rdfs:subClassOf _:node1912nb34nx198 .

_:node1912nb34nx198 a owl:Restriction ;
	owl:allValuesFrom xsd:string ;
	owl:onProperty <http://ns.cerise-project.nl/energy/def/cim-smartgrid#TelephoneNumber.extension> .

<http://ns.cerise-project.nl/energy/def/cim-smartgrid#TelephoneNumber.extension> a owl:DatatypeProperty .

:TelephoneNumber rdfs:comment "Telephone number." ;
	rdfs:subClassOf _:node1912nb34nx199 .

_:node1912nb34nx199 a owl:Restriction ;
	owl:cardinality "1"^^xsd:int ;
	owl:onProperty <http://ns.cerise-project.nl/energy/def/cim-smartgrid#TelephoneNumber.countryCode> .

<http://ns.cerise-project.nl/energy/def/cim-smartgrid#TelephoneNumber.countryCode> a owl:DatatypeProperty .

:TelephoneNumber rdfs:subClassOf _:node1912nb34nx200 .

_:node1912nb34nx200 a owl:Restriction ;
	owl:allValuesFrom xsd:string ;
	owl:onProperty <http://ns.cerise-project.nl/energy/def/cim-smartgrid#TelephoneNumber.countryCode> .

:TelephoneNumber rdfs:label "TelephoneNumber" ;
	rdfs:subClassOf _:node1912nb34nx201 .

_:node1912nb34nx201 a owl:Restriction ;
	owl:cardinality "1"^^xsd:int ;
	owl:onProperty <http://ns.cerise-project.nl/energy/def/cim-smartgrid#TelephoneNumber.areaCode> .

<http://ns.cerise-project.nl/energy/def/cim-smartgrid#TelephoneNumber.areaCode> a owl:DatatypeProperty .

:TelephoneNumber rdfs:subClassOf _:node1912nb34nx202 .

_:node1912nb34nx202 a owl:Restriction ;
	owl:cardinality "1"^^xsd:int ;
	owl:onProperty <http://ns.cerise-project.nl/energy/def/cim-smartgrid#TelephoneNumber.cityCode> .

<http://ns.cerise-project.nl/energy/def/cim-smartgrid#TelephoneNumber.cityCode> a owl:DatatypeProperty .

:TelephoneNumber rdfs:subClassOf _:node1912nb34nx203 .

_:node1912nb34nx203 a owl:Restriction ;
	owl:allValuesFrom xsd:string ;
	owl:onProperty <http://ns.cerise-project.nl/energy/def/cim-smartgrid#TelephoneNumber.areaCode> .

:TelephoneNumber rdfs:subClassOf _:node1912nb34nx204 .

_:node1912nb34nx204 a owl:Restriction ;
	owl:cardinality "1"^^xsd:int ;
	owl:onProperty <http://ns.cerise-project.nl/energy/def/cim-smartgrid#TelephoneNumber.extension> .

:TelephoneNumber rdfs:subClassOf _:node1912nb34nx205 .

_:node1912nb34nx205 a owl:Restriction ;
	owl:cardinality "1"^^xsd:int ;
	owl:onProperty <http://ns.cerise-project.nl/energy/def/cim-smartgrid#TelephoneNumber.localNumber> .

:TelephoneNumber rdfs:subClassOf _:node1912nb34nx206 .

_:node1912nb34nx206 a owl:Restriction ;
	owl:allValuesFrom xsd:string ;
	owl:onProperty <http://ns.cerise-project.nl/energy/def/cim-smartgrid#TelephoneNumber.cityCode> .

:DateTimeInterval rdfs:subClassOf _:node1912nb34nx207 .

_:node1912nb34nx207 a owl:Restriction ;
	owl:cardinality "1"^^xsd:int ;
	owl:onProperty <http://ns.cerise-project.nl/energy/def/cim-smartgrid#DateTimeInterval.start> .

<http://ns.cerise-project.nl/energy/def/cim-smartgrid#DateTimeInterval.start> a owl:DatatypeProperty .

:DateTimeInterval rdfs:subClassOf _:node1912nb34nx208 .

_:node1912nb34nx208 a owl:Restriction ;
	owl:allValuesFrom xsd:dateTime ;
	owl:onProperty <http://ns.cerise-project.nl/energy/def/cim-smartgrid#DateTimeInterval.start> .

:DateTimeInterval rdfs:subClassOf _:node1912nb34nx209 .

_:node1912nb34nx209 a owl:Restriction ;
	owl:cardinality "1"^^xsd:int ;
	owl:onProperty <http://ns.cerise-project.nl/energy/def/cim-smartgrid#DateTimeInterval.end> .

<http://ns.cerise-project.nl/energy/def/cim-smartgrid#DateTimeInterval.end> a owl:DatatypeProperty .

:DateTimeInterval rdfs:subClassOf _:node1912nb34nx210 .

_:node1912nb34nx210 a owl:Restriction ;
	owl:allValuesFrom xsd:dateTime ;
	owl:onProperty <http://ns.cerise-project.nl/energy/def/cim-smartgrid#DateTimeInterval.end> .

:DateTimeInterval rdfs:label "DateTimeInterval" ;
	uml:hasStereotype uml:compound ;
	rdfs:comment "Interval between two date and time points." ;
	rdfs:isDefinedBy :Package_Domain .

:Package_Domain a uml:Package ;
	rdfs:comment """The domain package define primitive datatypes that are used by classes in other packages. Stereotypes are used to describe the datatypes. The following stereotypes are defined:
&lt;&lt;enumeration&gt;&gt; A list of permissible constant values.
&lt;&lt;Primitive&gt;&gt; The most basic data types used to compose all other data types.
&lt;&lt;CIMDatatype&gt;&gt; A datatype that contains a value attribute, an optional unit of measure and a unit multiplier. The unit and multiplier may be specified as a static variable initialized to the allowed value.
&lt;&lt;Compound&gt;&gt; A composite of Primitive, enumeration, CIMDatatype or othe Compound classes, as long as the Compound classes do not recurse.""" ;
	rdfs:label "Domain" ;
	rdfs:isDefinedBy :Package_Base .

<http://ns.cerise-project.nl/energy/def/cim-smartgrid#UsagePoint.UsagePointLocation> rdfs:comment "Location of this usage point." ;
	rdfs:label "UsagePointLocation" .

<http://ns.cerise-project.nl/energy/def/cim-smartgrid#Location.CoordinateSystem> rdfs:comment "Coordinate system used to describe position points of this location." ;
	rdfs:label "CoordinateSystem" ;
	owl:inverseOf <http://ns.cerise-project.nl/energy/def/cim-smartgrid#CoordinateSystem.Location> .

<http://ns.cerise-project.nl/energy/def/cim-smartgrid#CustomerAgreement.Customer> rdfs:comment "Customer for this agreement." ;
	rdfs:label "Customer" .

<http://ns.cerise-project.nl/energy/def/cim-smartgrid#MeterMultiplier.Meter> rdfs:comment "Meter applying this multiplier." ;
	rdfs:label "Meter" ;
	owl:inverseOf <http://ns.cerise-project.nl/energy/def/cim-smartgrid#Meter.MeterMultipliers> .

<http://ns.cerise-project.nl/energy/def/cim-smartgrid#IntervalBlock.MeterReading> rdfs:comment "Meter reading containing this interval block." ;
	rdfs:label "MeterReading" .

<http://ns.cerise-project.nl/energy/def/cim-smartgrid#StreetAddress.streetDetail> uml:hasStereotype uml:attribute ;
	rdfs:comment "Street detail." ;
	rdfs:label "streetDetail" .

<http://ns.cerise-project.nl/energy/def/cim-smartgrid#MeterMultiplier.kind> uml:hasStereotype uml:attribute ;
	rdfs:comment "Kind of multiplier." ;
	rdfs:label "kind" .

<http://ns.cerise-project.nl/energy/def/cim-smartgrid#Meter.MeterReadings> rdfs:comment "All meter readings provided by this meter." ;
	rdfs:label "MeterReadings" ;
	owl:inverseOf <http://ns.cerise-project.nl/energy/def/cim-smartgrid#MeterReading.Meter> .

<http://ns.cerise-project.nl/energy/def/cim-smartgrid#IntervalBlock.IntervalReadings> rdfs:comment "Interval reading contained in this block." ;
	rdfs:label "IntervalReadings" ;
	owl:inverseOf <http://ns.cerise-project.nl/energy/def/cim-smartgrid#IntervalReading.IntervalBlocks> .

<http://ns.cerise-project.nl/energy/def/cim-smartgrid#EndDeviceFunction.EndDevice> rdfs:comment "End device that performs this function." ;
	rdfs:label "EndDevice" ;
	owl:inverseOf <http://ns.cerise-project.nl/energy/def/cim-smartgrid#EndDevice.EndDeviceFunctions> .

<http://ns.cerise-project.nl/energy/def/cim-smartgrid#MeterReading.UsagePoint> rdfs:comment "Usage point from which this meter reading (set of values) has been obtained." ;
	rdfs:label "UsagePoint" ;
	owl:inverseOf <http://ns.cerise-project.nl/energy/def/cim-smartgrid#UsagePoint.MeterReadings> .

<http://ns.cerise-project.nl/energy/def/cim-smartgrid#MeterReading.Readings> rdfs:comment "All reading values contained within this meter reading." ;
	rdfs:label "Readings" ;
	owl:inverseOf <http://ns.cerise-project.nl/energy/def/cim-smartgrid#Reading.MeterReadings> .

<http://ns.cerise-project.nl/energy/def/cim-smartgrid#UsagePoint.ServiceSupplier> rdfs:comment "ServiceSupplier (Utility) utilising this usage point to deliver a service." ;
	rdfs:label "ServiceSupplier" .

<http://ns.cerise-project.nl/energy/def/cim-smartgrid#SimpleEndDeviceFunction.kind> uml:hasStereotype uml:attribute ;
	rdfs:comment "Kind of this function." ;
	rdfs:label "kind" .

<http://ns.cerise-project.nl/energy/def/cim-smartgrid#StreetAddress.townDetail> uml:hasStereotype uml:attribute ;
	rdfs:comment "Town detail." ;
	rdfs:label "townDetail" .

<http://ns.cerise-project.nl/energy/def/cim-smartgrid#Location.phone2> uml:hasStereotype uml:attribute ;
	rdfs:comment "Additional phone number." ;
	rdfs:label "phone2" .

<http://ns.cerise-project.nl/energy/def/cim-smartgrid#Meter.MeterMultipliers> rdfs:comment "All multipliers applied at this meter." ;
	rdfs:label "MeterMultipliers" ;
	owl:inverseOf <http://ns.cerise-project.nl/energy/def/cim-smartgrid#MeterMultiplier.Meter> .

<http://ns.cerise-project.nl/energy/def/cim-smartgrid#Reading.ReadingType> rdfs:comment "Type information for this reading value." ;
	rdfs:label "ReadingType" .

<http://ns.cerise-project.nl/energy/def/cim-smartgrid#EndDevice.EndDeviceFunctions> rdfs:comment "All end device functions this end device performs." ;
	rdfs:label "EndDeviceFunctions" ;
	owl:inverseOf <http://ns.cerise-project.nl/energy/def/cim-smartgrid#EndDeviceFunction.EndDevice> .

<http://ns.cerise-project.nl/energy/def/cim-smartgrid#Reading.MeterReadings> rdfs:comment "All meter readings (sets of values) containing this reading value." ;
	rdfs:label "MeterReadings" ;
	owl:inverseOf <http://ns.cerise-project.nl/energy/def/cim-smartgrid#MeterReading.Readings> .

<http://ns.cerise-project.nl/energy/def/cim-smartgrid#UsagePoint.MeterReadings> rdfs:comment "All meter readings obtained from this usage point." ;
	rdfs:label "MeterReadings" ;
	owl:inverseOf <http://ns.cerise-project.nl/energy/def/cim-smartgrid#MeterReading.UsagePoint> .

<http://ns.cerise-project.nl/energy/def/cim-smartgrid#CustomerAgreement.ServiceSupplier> rdfs:comment "Service supplier for this customer agreement." ;
	rdfs:label "ServiceSupplier" .

<http://ns.cerise-project.nl/energy/def/cim-smartgrid#UsagePoint.amiBillingReady> uml:hasStereotype uml:attribute ;
	rdfs:comment "Tracks the lifecycle of the metering installation at a usage point with respect to readiness for billing via advanced metering infrastructure reads." ;
	rdfs:label "amiBillingReady" .

<http://ns.cerise-project.nl/energy/def/cim-smartgrid#CustomerAgreement.ServiceCategory> rdfs:comment "Service category for this agreement." ;
	rdfs:label "ServiceCategory" .

<http://ns.cerise-project.nl/energy/def/cim-smartgrid#IntervalReading.IntervalBlocks> rdfs:comment "All blocks containing this interval reading." ;
	rdfs:label "IntervalBlocks" ;
	owl:inverseOf <http://ns.cerise-project.nl/energy/def/cim-smartgrid#IntervalBlock.IntervalReadings> .

<http://ns.cerise-project.nl/energy/def/cim-smartgrid#Location.status> uml:hasStereotype uml:attribute ;
	rdfs:comment "Status of this location." ;
	rdfs:label "status" .

<http://ns.cerise-project.nl/energy/def/cim-smartgrid#CoordinateSystem.Location> rdfs:comment "All locations described with position points in this coordinate system." ;
	rdfs:label "Location" ;
	owl:inverseOf <http://ns.cerise-project.nl/energy/def/cim-smartgrid#Location.CoordinateSystem> .

<http://ns.cerise-project.nl/energy/def/cim-smartgrid#Location.electronicAddress> uml:hasStereotype uml:attribute ;
	rdfs:comment "Electronic address." ;
	rdfs:label "electronicAddress" .

<http://ns.cerise-project.nl/energy/def/cim-smartgrid#ServiceCategory.kind> uml:hasStereotype uml:attribute ;
	rdfs:comment "Kind of service." ;
	rdfs:label "kind" .

<http://ns.cerise-project.nl/energy/def/cim-smartgrid#PositionPoint.Location> rdfs:comment "Location described by this position point." ;
	rdfs:label "Location" ;
	owl:inverseOf <http://ns.cerise-project.nl/energy/def/cim-smartgrid#Location.PositionPoints> .

<http://ns.cerise-project.nl/energy/def/cim-smartgrid#ServiceSupplier.kind> uml:hasStereotype uml:attribute ;
	rdfs:comment "Kind of supplier." ;
	rdfs:label "kind" .

<http://ns.cerise-project.nl/energy/def/cim-smartgrid#UsagePoint.CustomerAgreement> rdfs:comment "Customer agreement regulating this service delivery point." ;
	rdfs:label "CustomerAgreement" .

<http://ns.cerise-project.nl/energy/def/cim-smartgrid#Location.PositionPoints> rdfs:comment "Sequence of position points describing this location, expressed in coordinate system 'Location.CoordinateSystem'." ;
	rdfs:label "PositionPoints" ;
	owl:inverseOf <http://ns.cerise-project.nl/energy/def/cim-smartgrid#PositionPoint.Location> .

<http://ns.cerise-project.nl/energy/def/cim-smartgrid#Location.secondaryAddress> uml:hasStereotype uml:attribute ;
	rdfs:comment "Secondary address of the location. For example, PO Box address may have different ZIP code than that in the 'mainAddress'." ;
	rdfs:label "secondaryAddress" .

<http://ns.cerise-project.nl/energy/def/cim-smartgrid#Location.phone1> uml:hasStereotype uml:attribute ;
	rdfs:comment "Phone number." ;
	rdfs:label "phone1" .

<http://ns.cerise-project.nl/energy/def/cim-smartgrid#Location.mainAddress> uml:hasStereotype uml:attribute ;
	rdfs:comment "Main address of the location." ;
	rdfs:label "mainAddress" .

<http://ns.cerise-project.nl/energy/def/cim-smartgrid#UsagePoint.ServiceCategory> rdfs:comment "Service category delivered by this usage point." ;
	rdfs:label "ServiceCategory" .

<http://ns.cerise-project.nl/energy/def/cim-smartgrid#MeterReading.valuesInterval> uml:hasStereotype uml:attribute ;
	rdfs:comment "Date and time interval of the data items contained within this meter reading." ;
	rdfs:label "valuesInterval" .

<http://ns.cerise-project.nl/energy/def/cim-smartgrid#EndDevice.UsagePoint> rdfs:comment "Usage point to which this end device belongs." ;
	rdfs:label "UsagePoint" .

<http://ns.cerise-project.nl/energy/def/cim-smartgrid#MeterReading.Meter> rdfs:comment "Meter providing this reading." ;
	rdfs:label "Meter" ;
	owl:inverseOf <http://ns.cerise-project.nl/energy/def/cim-smartgrid#Meter.MeterReadings> .

<http://ns.cerise-project.nl/energy/def/cim-smartgrid#Customer.kind> uml:hasStereotype uml:attribute ;
	rdfs:comment "Kind of customer." ;
	rdfs:label "kind" .

<http://ns.cerise-project.nl/energy/def/cim-smartgrid#MeterReading.CustomerAgreement> rdfs:comment "(could be deprecated in the future) Customer agreement for this meter reading." ;
	rdfs:label "CustomerAgreement" .

<http://ns.cerise-project.nl/energy/def/cim-smartgrid#BaseReading.timePeriod> uml:hasStereotype uml:attribute ;
	rdfs:comment "Start and end of the period for those readings whose type has a time attribute such as 'billing', seasonal' or 'forTheSpecifiedPeriod'." ;
	rdfs:label "timePeriod" .

<http://ns.cerise-project.nl/energy/def/cim-smartgrid#IntervalBlock.ReadingType> rdfs:comment "Type information for interval reading values contained in this block." ;
	rdfs:label "ReadingType" .

<http://ns.cerise-project.nl/energy/def/cim-smartgrid#DateTimeInterval.end> uml:hasStereotype uml:attribute ;
	rdfs:comment "End date and time of this interval." ;
	rdfs:label "end" .

<http://ns.cerise-project.nl/energy/def/cim-smartgrid#ReadingType.measurementKind> uml:hasStereotype uml:attribute ;
	rdfs:comment "Identifies \"what\" is being measured, as refinement of 'commodity'. When combined with 'unit', it provides detail to the unit of measure. For example, 'energy' with a unit of measure of 'kWh' indicates to the user that active energy is being measured, while with 'kVAh' or 'kVArh', it indicates apparent energy and reactive energy, respectively. 'power' can be combined in a similar way with various power units of measure: Distortion power ('distortionVoltAmperes') with 'kVA' is different from 'power' with 'kVA'." ;
	rdfs:label "measurementKind" .

<http://ns.cerise-project.nl/energy/def/cim-smartgrid#UsagePoint.isVirtual> uml:hasStereotype uml:attribute ;
	rdfs:comment "If true, this usage point is virtual, i.e., no physical location exists in the network where a meter could be located to collect the meter readings. For example, one may define a virtual usage point to serve as an aggregation of usage for all of a companies premises distributed widely across the distribution territory. Otherwise, the usage point is physical, i.e., there is a logical point in the network where a meter could be located to collect meter readings." ;
	rdfs:label "isVirtual" .

<http://ns.cerise-project.nl/energy/def/cim-smartgrid#DateTimeInterval.start> uml:hasStereotype uml:attribute ;
	rdfs:comment "Start date and time of this interval." ;
	rdfs:label "start" .

<http://ns.cerise-project.nl/energy/def/cim-smartgrid#IdentifiedObject.name> uml:hasStereotype uml:attribute ;
	rdfs:comment "The name is any free human readable and possibly non unique text naming the object." ;
	rdfs:label "name" .

<http://ns.cerise-project.nl/energy/def/cim-smartgrid#TelephoneNumber.localNumber> uml:hasStereotype uml:attribute ;
	rdfs:comment "Main (local) part of this telephone number." ;
	rdfs:label "localNumber" .

<http://ns.cerise-project.nl/energy/def/cim-smartgrid#TelephoneNumber.areaCode> uml:hasStereotype uml:attribute ;
	rdfs:comment "Area or region code." ;
	rdfs:label "areaCode" .

<http://ns.cerise-project.nl/energy/def/cim-smartgrid#ElectronicAddress.lan> uml:hasStereotype uml:attribute ;
	rdfs:comment "Address on local area network." ;
	rdfs:label "lan" .

<http://ns.cerise-project.nl/energy/def/cim-smartgrid#StreetDetail.number> uml:hasStereotype uml:attribute ;
	rdfs:comment "Designator of the specific location on the street." ;
	rdfs:label "number" .

<http://ns.cerise-project.nl/energy/def/cim-smartgrid#ServiceSupplier.issuerIdentificationNumber> uml:hasStereotype uml:attribute ;
	rdfs:comment "Unique transaction reference prefix number issued to an entity by the International Standards Organisation for the purpose of tagging onto electronic financial transactions, as defined in ISO/IEC 7812-1 and ISO/IEC 7812-2." ;
	rdfs:label "issuerIdentificationNumber" .

<http://ns.cerise-project.nl/energy/def/cim-smartgrid#StreetDetail.code> uml:hasStereotype uml:attribute ;
	rdfs:comment "(if applicable) Utilities often make use of external reference systems, such as those of the town-planner's department or surveyor general's mapping system, that allocate global reference codes to streets." ;
	rdfs:label "code" .

<http://ns.cerise-project.nl/energy/def/cim-smartgrid#IdentifiedObject.description> uml:hasStereotype uml:attribute ;
	rdfs:comment "The description is a free human readable text describing or naming the object. It may be non unique and may not correlate to a naming hierarchy." ;
	rdfs:label "description" .

<http://ns.cerise-project.nl/energy/def/cim-smartgrid#PositionPoint.xPosition> uml:hasStereotype uml:attribute ;
	rdfs:comment "X axis position." ;
	rdfs:label "xPosition" .

<http://ns.cerise-project.nl/energy/def/cim-smartgrid#ReadingType.flowDirection> uml:hasStereotype uml:attribute ;
	rdfs:comment "Flow direction for a reading where the direction of flow of the commodity is important (for electricity measurements this includes current, energy, power, and demand)." ;
	rdfs:label "flowDirection" .

<http://ns.cerise-project.nl/energy/def/cim-smartgrid#EndDevice.isVirtual> uml:hasStereotype uml:attribute ;
	rdfs:comment "If true, there is no physical device. As an example, a virtual meter can be defined to aggregate the consumption for two or more physical meters. Otherwise, this is a physical hardware device." ;
	rdfs:label "isVirtual" .

<http://ns.cerise-project.nl/energy/def/cim-smartgrid#BaseReading.source> uml:hasStereotype uml:attribute ;
	rdfs:comment "System that originally supplied the reading (e.g., customer, AMI system, handheld reading system, another enterprise system, etc.)." ;
	rdfs:label "source" .

<http://ns.cerise-project.nl/energy/def/cim-smartgrid#StreetDetail.suffix> uml:hasStereotype uml:attribute ;
	rdfs:comment "Suffix to the street name. For example: North, South, East, West." ;
	rdfs:label "suffix" .

<http://ns.cerise-project.nl/energy/def/cim-smartgrid#IdentifiedObject.mRID> uml:hasStereotype uml:attribute ;
	rdfs:comment """Master resource identifier issued by a model authority. The mRID must semantically be a UUID as specified in RFC 4122. The mRID is globally unique.
For CIMXML data files in RDF syntax, the mRID is mapped to rdf:ID or rdf:about attributes that identify CIM object elements.""" ;
	rdfs:label "mRID" .

<http://ns.cerise-project.nl/energy/def/cim-smartgrid#ElectronicAddress.mac> uml:hasStereotype uml:attribute ;
	rdfs:comment "MAC (Media Access Control) address." ;
	rdfs:label "mac" .

<http://ns.cerise-project.nl/energy/def/cim-smartgrid#StreetDetail.addressGeneral> uml:hasStereotype uml:attribute ;
	rdfs:comment "Additional address information, for example a mailstop." ;
	rdfs:label "addressGeneral" .

<http://ns.cerise-project.nl/energy/def/cim-smartgrid#Status.value> uml:hasStereotype uml:attribute ;
	rdfs:comment "Status value at 'dateTime'; prior status changes may have been kept in instances of activity records associated with the object to which this status applies." ;
	rdfs:label "value" .

<http://ns.cerise-project.nl/energy/def/cim-smartgrid#StreetDetail.withinTownLimits> uml:hasStereotype uml:attribute ;
	rdfs:comment "True if this street is within the legal geographical boundaries of the specified town (default)." ;
	rdfs:label "withinTownLimits" .

<http://ns.cerise-project.nl/energy/def/cim-smartgrid#ReadingType.measuringPeriod> uml:hasStereotype uml:attribute ;
	rdfs:comment """Time attribute inherent or fundamental to the reading value (as opposed to 'macroPeriod' that supplies an \"adjective\" to describe aspects of a time period with regard to the measurement). It refers to the way the value was originally measured and not to the frequency at which it is reported or presented. For example, an hourly interval of consumption data would have value 'hourly' as an attribute. However in the case of an hourly sampled voltage value, the meterReadings schema would carry the 'hourly' interval size information.
It is common for meters to report demand in a form that is measured over the course of a portion of an hour, while enterprise applications however commonly assume the demand (in kW or kVAr) normalised to 1 hour. The sytem that receives readings directly from the meter therefore must perform this transformation before publishing readings for use by the other enterprise systems. The scalar used is chosen based on the block size (not any sub-interval size).""" ;
	rdfs:label "measuringPeriod" .

<http://ns.cerise-project.nl/energy/def/cim-smartgrid#Status.remark> uml:hasStereotype uml:attribute ;
	rdfs:comment "Pertinent information regarding the current 'value', as free form text." ;
	rdfs:label "remark" .

<http://ns.cerise-project.nl/energy/def/cim-smartgrid#TownDetail.code> uml:hasStereotype uml:attribute ;
	rdfs:comment "Town code." ;
	rdfs:label "code" .

<http://ns.cerise-project.nl/energy/def/cim-smartgrid#ReadingType.unit> uml:hasStereotype uml:attribute ;
	rdfs:comment "Metering-specific unit." ;
	rdfs:label "unit" .

<http://ns.cerise-project.nl/energy/def/cim-smartgrid#Location.type> uml:hasStereotype uml:attribute ;
	rdfs:comment "Classification by utility's corporate standards and practices, relative to the location itself (e.g., geographical, functional accounting, etc., not a given property that happens to exist at that location)." ;
	rdfs:label "type" .

<http://ns.cerise-project.nl/energy/def/cim-smartgrid#StreetDetail.suiteNumber> uml:hasStereotype uml:attribute ;
	rdfs:comment "Number of the apartment or suite." ;
	rdfs:label "suiteNumber" .

<http://ns.cerise-project.nl/energy/def/cim-smartgrid#ElectronicAddress.email2> uml:hasStereotype uml:attribute ;
	rdfs:comment "Alternate email address." ;
	rdfs:label "email2" .

<http://ns.cerise-project.nl/energy/def/cim-smartgrid#TelephoneNumber.extension> uml:hasStereotype uml:attribute ;
	rdfs:comment "(if applicable) Extension for this telephone number." ;
	rdfs:label "extension" .

<http://ns.cerise-project.nl/energy/def/cim-smartgrid#ReadingType.accumulation> uml:hasStereotype uml:attribute ;
	rdfs:comment "Accumulation behaviour of a reading over time, usually 'measuringPeriod', to be used with individual endpoints (as opposed to 'macroPeriod' and 'aggregate' that are used to describe aggregations of data from individual endpoints)." ;
	rdfs:label "accumulation" .

<http://ns.cerise-project.nl/energy/def/cim-smartgrid#StreetDetail.name> uml:hasStereotype uml:attribute ;
	rdfs:comment "Name of the street." ;
	rdfs:label "name" .

<http://ns.cerise-project.nl/energy/def/cim-smartgrid#ElectronicAddress.radio> uml:hasStereotype uml:attribute ;
	rdfs:comment "Radio address." ;
	rdfs:label "radio" .

<http://ns.cerise-project.nl/energy/def/cim-smartgrid#ReadingType.aggregate> uml:hasStereotype uml:attribute ;
	rdfs:comment "Salient attribute of the reading data aggregated from individual endpoints. This is mainly used to define a mathematical operation carried out over 'macroPeriod', but may also be used to describe an attribute of the data when the 'macroPeriod' is not defined." ;
	rdfs:label "aggregate" .

<http://ns.cerise-project.nl/energy/def/cim-smartgrid#TownDetail.section> uml:hasStereotype uml:attribute ;
	rdfs:comment "Town section. For example, it is common for there to be 36 sections per township." ;
	rdfs:label "section" .

<http://ns.cerise-project.nl/energy/def/cim-smartgrid#Status.dateTime> uml:hasStereotype uml:attribute ;
	rdfs:comment "Date and time for which status 'value' applies." ;
	rdfs:label "dateTime" .

<http://ns.cerise-project.nl/energy/def/cim-smartgrid#TelephoneNumber.countryCode> uml:hasStereotype uml:attribute ;
	rdfs:comment "Country code." ;
	rdfs:label "countryCode" .

<http://ns.cerise-project.nl/energy/def/cim-smartgrid#EndDevice.installCode> uml:hasStereotype uml:attribute ;
	rdfs:comment "Installation code." ;
	rdfs:label "installCode" .

<http://ns.cerise-project.nl/energy/def/cim-smartgrid#UsagePoint.isSdp> uml:hasStereotype uml:attribute ;
	rdfs:comment "If true, this usage point is a service delivery point, i.e., a usage point where the ownership of the service changes hands." ;
	rdfs:label "isSdp" .

<http://ns.cerise-project.nl/energy/def/cim-smartgrid#TelephoneNumber.cityCode> uml:hasStereotype uml:attribute ;
	rdfs:comment "(if applicable) City code." ;
	rdfs:label "cityCode" .

<http://ns.cerise-project.nl/energy/def/cim-smartgrid#CoordinateSystem.crsUrn> uml:hasStereotype uml:attribute ;
	rdfs:comment """A Uniform Resource Name (URN) for the coordinate reference system (crs) used to define 'Location.PositionPoints'.
An example would be the European Petroleum Survey Group (EPSG) code for a coordinate reference system, defined in URN under the Open Geospatial Consortium (OGC) namespace as: urn:ogc :def:uom:EPSG::XXXX, where XXXX is an EPSG code (a full list of codes can be found at the EPSG Registry website http://www.epsg-registry.org/). To define the coordinate system as being WGS84 (latitude, longitude) using an EPSG OGC, this attribute would be urn:ogc:def:uom:EPSG::4236.
A profile should limit this code to a set of allowed URNs agreed to by all sending and receiving parties.""" ;
	rdfs:label "crsUrn" .

<http://ns.cerise-project.nl/energy/def/cim-smartgrid#Meter.formNumber> uml:hasStereotype uml:attribute ;
	rdfs:comment "Meter form designation per ANSI C12.10 or other applicable standard. An alphanumeric designation denoting the circuit arrangement for which the meter is applicable and its specific terminal arrangement." ;
	rdfs:label "formNumber" .

<http://ns.cerise-project.nl/energy/def/cim-smartgrid#TownDetail.country> uml:hasStereotype uml:attribute ;
	rdfs:comment "Name of the country." ;
	rdfs:label "country" .

<http://ns.cerise-project.nl/energy/def/cim-smartgrid#TownDetail.stateOrProvince> uml:hasStereotype uml:attribute ;
	rdfs:comment "Name of the state or province." ;
	rdfs:label "stateOrProvince" .

<http://ns.cerise-project.nl/energy/def/cim-smartgrid#StreetDetail.prefix> uml:hasStereotype uml:attribute ;
	rdfs:comment "Prefix to the street name. For example: North, South, East, West." ;
	rdfs:label "prefix" .

<http://ns.cerise-project.nl/energy/def/cim-smartgrid#ElectronicAddress.email1> uml:hasStereotype uml:attribute ;
	rdfs:comment "Primary email address." ;
	rdfs:label "email1" .

<http://ns.cerise-project.nl/energy/def/cim-smartgrid#IdentifiedObject.aliasName> uml:hasStereotype uml:attribute ;
	rdfs:comment """The aliasName is free text human readable name of the object alternative to IdentifiedObject.name. It may be non unique and may not correlate to a naming hierarchy.
The attribute aliasName is retained because of backwards compatibility between CIM relases. It is however recommended to replace aliasName with the Name class as aliasName is planned for retirement at a future time.""" ;
	rdfs:label "aliasName" .

<http://ns.cerise-project.nl/energy/def/cim-smartgrid#BaseReading.value> uml:hasStereotype uml:attribute ;
	rdfs:comment "Value of this reading." ;
	rdfs:label "value" .

<http://ns.cerise-project.nl/energy/def/cim-smartgrid#StreetDetail.buildingName> uml:hasStereotype uml:attribute ;
	rdfs:comment "(if applicable) In certain cases the physical location of the place of interest does not have a direct point of entry from the street, but may be located inside a larger structure such as a building, complex, office block, apartment, etc." ;
	rdfs:label "buildingName" .

<http://ns.cerise-project.nl/energy/def/cim-smartgrid#ElectronicAddress.userID> uml:hasStereotype uml:attribute ;
	rdfs:comment "User ID needed to log in, which can be for an individual person, an organisation, a location, etc." ;
	rdfs:label "userID" .

<http://ns.cerise-project.nl/energy/def/cim-smartgrid#MeterMultiplier.value> uml:hasStereotype uml:attribute ;
	rdfs:comment "Multiplier value." ;
	rdfs:label "value" .

<http://ns.cerise-project.nl/energy/def/cim-smartgrid#ElectronicAddress.web> uml:hasStereotype uml:attribute ;
	rdfs:comment "World wide web address." ;
	rdfs:label "web" .

<http://ns.cerise-project.nl/energy/def/cim-smartgrid#PositionPoint.sequenceNumber> uml:hasStereotype uml:attribute ;
	rdfs:comment "Zero-relative sequence number of this point within a series of points." ;
	rdfs:label "sequenceNumber" .

<http://ns.cerise-project.nl/energy/def/cim-smartgrid#PositionPoint.zPosition> uml:hasStereotype uml:attribute ;
	rdfs:comment "(if applicable) Z axis position." ;
	rdfs:label "zPosition" .

<http://ns.cerise-project.nl/energy/def/cim-smartgrid#Status.reason> uml:hasStereotype uml:attribute ;
	rdfs:comment "Reason code or explanation for why an object went to the current status 'value'." ;
	rdfs:label "reason" .

<http://ns.cerise-project.nl/energy/def/cim-smartgrid#PositionPoint.yPosition> uml:hasStereotype uml:attribute ;
	rdfs:comment "Y axis position." ;
	rdfs:label "yPosition" .

<http://ns.cerise-project.nl/energy/def/cim-smartgrid#ElectronicAddress.password> uml:hasStereotype uml:attribute ;
	rdfs:comment "Password needed to log in." ;
	rdfs:label "password" .

<http://ns.cerise-project.nl/energy/def/cim-smartgrid#Location.geoInfoReference> uml:hasStereotype uml:attribute ;
	rdfs:comment "(if applicable) Reference to geographical information source, often external to the utility." ;
	rdfs:label "geoInfoReference" .

<http://ns.cerise-project.nl/energy/def/cim-smartgrid#StreetDetail.type> uml:hasStereotype uml:attribute ;
	rdfs:comment "Type of street. Examples include: street, circle, boulevard, avenue, road, drive, etc." ;
	rdfs:label "type" .

<http://ns.cerise-project.nl/energy/def/cim-smartgrid#TownDetail.name> uml:hasStereotype uml:attribute ;
	rdfs:comment "Town name." ;
	rdfs:label "name" .

<http://ns.cerise-project.nl/energy/def/cim-smartgrid#ReadingType.commodity> uml:hasStereotype uml:attribute ;
	rdfs:comment "Commodity being measured." ;
	rdfs:label "commodity" .

<http://ns.cerise-project.nl/energy/def/cim-smartgrid#CustomerKind.residentialFarmService> a :CustomerKind ;
	rdfs:comment "Residential farm service customer." ;
	rdfs:label "residentialFarmService" .

<http://ns.cerise-project.nl/energy/def/cim-smartgrid#CustomerKind.pumpingLoad> a :CustomerKind ;
	rdfs:comment "Pumping load customer." ;
	rdfs:label "pumpingLoad" .

<http://ns.cerise-project.nl/energy/def/cim-smartgrid#CustomerKind.residentialStreetlightOthers> a :CustomerKind ;
	rdfs:comment "Residential streetlight or other related customer." ;
	rdfs:label "residentialStreetlightOthers" .

<http://ns.cerise-project.nl/energy/def/cim-smartgrid#CustomerKind.other> a :CustomerKind ;
	rdfs:comment "Other kind of customer." ;
	rdfs:label "other" .

<http://ns.cerise-project.nl/energy/def/cim-smartgrid#MeterMultiplierKind.transformerRatio> a :MeterMultiplierKind ;
	rdfs:comment "Product of the CT ratio and PT ratio." ;
	rdfs:label "transformerRatio" .

<http://ns.cerise-project.nl/energy/def/cim-smartgrid#EndDeviceFunctionKind.reverseFlow> a :EndDeviceFunctionKind ;
	rdfs:comment "Detection and monitoring of reverse flow." ;
	rdfs:label "reverseFlow" .

<http://ns.cerise-project.nl/energy/def/cim-smartgrid#CustomerKind.internalUse> a :CustomerKind ;
	rdfs:comment "Internal use customer." ;
	rdfs:label "internalUse" .

<http://ns.cerise-project.nl/energy/def/cim-smartgrid#AmiBillingReadyKind.nonAmi> a :AmiBillingReadyKind ;
	rdfs:comment "Usage point is equipped with a non AMI capable meter." ;
	rdfs:label "nonAmi" .

<http://ns.cerise-project.nl/energy/def/cim-smartgrid#CustomerKind.residential> a :CustomerKind ;
	rdfs:comment "Residential customer." ;
	rdfs:label "residential" .

<http://ns.cerise-project.nl/energy/def/cim-smartgrid#AmiBillingReadyKind.enabled> a :AmiBillingReadyKind ;
	rdfs:comment "Usage point is equipped with an AMI capable meter having communications capability." ;
	rdfs:label "enabled" .

<http://ns.cerise-project.nl/energy/def/cim-smartgrid#ServiceKind.electricity> a :ServiceKind ;
	rdfs:comment "Electricity service." ;
	rdfs:label "electricity" .

<http://ns.cerise-project.nl/energy/def/cim-smartgrid#AmiBillingReadyKind.amiDisabled> a :AmiBillingReadyKind ;
	rdfs:comment "Usage point is equipped with an AMI capable meter; however, the AMI functionality has been disabled or is not being used." ;
	rdfs:label "amiDisabled" .

<http://ns.cerise-project.nl/energy/def/cim-smartgrid#AmiBillingReadyKind.operable> a :AmiBillingReadyKind ;
	rdfs:comment "Usage point is equipped with an AMI capable meter that is functioning and communicating with the AMI network." ;
	rdfs:label "operable" .

<http://ns.cerise-project.nl/energy/def/cim-smartgrid#EndDeviceFunctionKind.metrology> a :EndDeviceFunctionKind ;
	rdfs:comment "Presentation of metered values to a user or another system (always a function of a meter, but might not be supported by a load control unit)." ;
	rdfs:label "metrology" .

<http://ns.cerise-project.nl/energy/def/cim-smartgrid#CustomerKind.energyServiceSupplier> a :CustomerKind ;
	rdfs:comment "Customer as energy service supplier." ;
	rdfs:label "energyServiceSupplier" .

<http://ns.cerise-project.nl/energy/def/cim-smartgrid#EndDeviceFunctionKind.waterMetering> a :EndDeviceFunctionKind ;
	rdfs:comment "Water metering." ;
	rdfs:label "waterMetering" .

<http://ns.cerise-project.nl/energy/def/cim-smartgrid#MeterMultiplierKind.kH> a :MeterMultiplierKind ;
	rdfs:comment "Meter kh (watthour) constant. The number of watthours that must be applied to the meter to cause one disk revolution for an electromechanical meter or the number of watthours represented by one increment pulse for an electronic meter." ;
	rdfs:label "kH" .

<http://ns.cerise-project.nl/energy/def/cim-smartgrid#ServiceKind.other> a :ServiceKind ;
	rdfs:comment "Other kind of service." ;
	rdfs:label "other" .

<http://ns.cerise-project.nl/energy/def/cim-smartgrid#ServiceKind.refuse> a :ServiceKind ;
	rdfs:comment "Refuse (waster) service." ;
	rdfs:label "refuse" .

<http://ns.cerise-project.nl/energy/def/cim-smartgrid#MeterMultiplierKind.ptRatio> a :MeterMultiplierKind ;
	rdfs:comment "Potential transformer ratio used to convert associated quantities to real measurements." ;
	rdfs:label "ptRatio" .

<http://ns.cerise-project.nl/energy/def/cim-smartgrid#CustomerKind.commercialIndustrial> a :CustomerKind ;
	rdfs:comment "Commercial industrial customer." ;
	rdfs:label "commercialIndustrial" .

<http://ns.cerise-project.nl/energy/def/cim-smartgrid#ServiceKind.internet> a :ServiceKind ;
	rdfs:comment "Internet service." ;
	rdfs:label "internet" .

<http://ns.cerise-project.nl/energy/def/cim-smartgrid#EndDeviceFunctionKind.outageHistory> a :EndDeviceFunctionKind ;
	rdfs:comment "Reporting historical power interruption data." ;
	rdfs:label "outageHistory" .

<http://ns.cerise-project.nl/energy/def/cim-smartgrid#MeterMultiplierKind.kE> a :MeterMultiplierKind ;
	rdfs:comment "Test constant." ;
	rdfs:label "kE" .

<http://ns.cerise-project.nl/energy/def/cim-smartgrid#AmiBillingReadyKind.amiCapable> a :AmiBillingReadyKind ;
	rdfs:comment "Usage point is equipped with an AMI capable meter that is not yet currently equipped with a communications module." ;
	rdfs:label "amiCapable" .

<http://ns.cerise-project.nl/energy/def/cim-smartgrid#EndDeviceFunctionKind.gasMetering> a :EndDeviceFunctionKind ;
	rdfs:comment "Gas metering." ;
	rdfs:label "gasMetering" .

<http://ns.cerise-project.nl/energy/def/cim-smartgrid#EndDeviceFunctionKind.relaysProgramming> a :EndDeviceFunctionKind ;
	rdfs:comment "Support for one or more relays that may be programmable in the meter (and tied to TOU, time pulse, load control or other functions)." ;
	rdfs:label "relaysProgramming" .

<http://ns.cerise-project.nl/energy/def/cim-smartgrid#AmiBillingReadyKind.billingApproved> a :AmiBillingReadyKind ;
	rdfs:comment "Usage point is equipped with an operating AMI capable meter and accuracy has been certified for billing purposes." ;
	rdfs:label "billingApproved" .

<http://ns.cerise-project.nl/energy/def/cim-smartgrid#MeterMultiplierKind.ctRatio> a :MeterMultiplierKind ;
	rdfs:comment "Current transformer ratio used to convert associated quantities to real measurements." ;
	rdfs:label "ctRatio" .

<http://ns.cerise-project.nl/energy/def/cim-smartgrid#SupplierKind.utility> a :SupplierKind ;
	rdfs:comment "Entity that delivers the service to the customer." ;
	rdfs:label "utility" .

<http://ns.cerise-project.nl/energy/def/cim-smartgrid#MeterMultiplierKind.kR> a :MeterMultiplierKind ;
	rdfs:comment "Register multiplier. The number to multiply the register reading by in order to get kWh." ;
	rdfs:label "kR" .

<http://ns.cerise-project.nl/energy/def/cim-smartgrid#CustomerKind.windMachine> a :CustomerKind ;
	rdfs:comment "Wind machine customer." ;
	rdfs:label "windMachine" .

<http://ns.cerise-project.nl/energy/def/cim-smartgrid#EndDeviceFunctionKind.electricMetering> a :EndDeviceFunctionKind ;
	rdfs:comment "Electricity metering." ;
	rdfs:label "electricMetering" .

<http://ns.cerise-project.nl/energy/def/cim-smartgrid#AmiBillingReadyKind.nonMetered> a :AmiBillingReadyKind ;
	rdfs:comment "Usage point is not currently equipped with a meter." ;
	rdfs:label "nonMetered" .

<http://ns.cerise-project.nl/energy/def/cim-smartgrid#EndDeviceFunctionKind.onRequestRead> a :EndDeviceFunctionKind ;
	rdfs:comment "On-request reads." ;
	rdfs:label "onRequestRead" .

<http://ns.cerise-project.nl/energy/def/cim-smartgrid#ServiceKind.water> a :ServiceKind ;
	rdfs:comment "Water service." ;
	rdfs:label "water" .

<http://ns.cerise-project.nl/energy/def/cim-smartgrid#EndDeviceFunctionKind.autonomousDst> a :EndDeviceFunctionKind ;
	rdfs:comment "Autonomous application of daylight savings time (DST)." ;
	rdfs:label "autonomousDst" .

<http://ns.cerise-project.nl/energy/def/cim-smartgrid#ServiceKind.gas> a :ServiceKind ;
	rdfs:comment "Gas service." ;
	rdfs:label "gas" .

<http://ns.cerise-project.nl/energy/def/cim-smartgrid#CustomerKind.energyServiceScheduler> a :CustomerKind ;
	rdfs:comment "Customer as energy service scheduler." ;
	rdfs:label "energyServiceScheduler" .

<http://ns.cerise-project.nl/energy/def/cim-smartgrid#ServiceKind.time> a :ServiceKind ;
	rdfs:comment "Time service." ;
	rdfs:label "time" .

<http://ns.cerise-project.nl/energy/def/cim-smartgrid#CustomerKind.residentialAndCommercial> a :CustomerKind ;
	rdfs:comment "Residential and commercial customer." ;
	rdfs:label "residentialAndCommercial" .

<http://ns.cerise-project.nl/energy/def/cim-smartgrid#SupplierKind.other> a :SupplierKind ;
	rdfs:comment "Other kind of supplier." ;
	rdfs:label "other" .

<http://ns.cerise-project.nl/energy/def/cim-smartgrid#ServiceKind.tvLicence> a :ServiceKind ;
	rdfs:comment "TV license service." ;
	rdfs:label "tvLicence" .

<http://ns.cerise-project.nl/energy/def/cim-smartgrid#ServiceKind.rates> a :ServiceKind ;
	rdfs:comment "Rates (e.g. tax, charge, toll, duty, tariff, etc.) service." ;
	rdfs:label "rates" .

<http://ns.cerise-project.nl/energy/def/cim-smartgrid#EndDeviceFunctionKind.demandResponse> a :EndDeviceFunctionKind ;
	rdfs:comment "Demand response functions." ;
	rdfs:label "demandResponse" .

<http://ns.cerise-project.nl/energy/def/cim-smartgrid#ServiceKind.heat> a :ServiceKind ;
	rdfs:comment "Heat service." ;
	rdfs:label "heat" .

<http://ns.cerise-project.nl/energy/def/cim-smartgrid#CustomerKind.residentialAndStreetlight> a :CustomerKind ;
	rdfs:comment "Residential and streetlight customer." ;
	rdfs:label "residentialAndStreetlight" .

<http://ns.cerise-project.nl/energy/def/cim-smartgrid#ServiceKind.sewerage> a :ServiceKind ;
	rdfs:comment "Sewerage service." ;
	rdfs:label "sewerage" .

<http://ns.cerise-project.nl/energy/def/cim-smartgrid#SupplierKind.retailer> a :SupplierKind ;
	rdfs:comment "Entity that sells the service, but does not deliver to the customer; applies to the deregulated markets." ;
	rdfs:label "retailer" .

:Status rdfs:subClassOf _:node1912nb34nx211 .

_:node1912nb34nx211 a owl:Restriction ;
	owl:allValuesFrom xsd:string ;
	owl:onProperty <http://ns.cerise-project.nl/energy/def/cim-smartgrid#Status.remark> .

:Status rdfs:subClassOf _:node1912nb34nx212 .

_:node1912nb34nx212 a owl:Restriction ;
	owl:cardinality "1"^^xsd:int ;
	owl:onProperty <http://ns.cerise-project.nl/energy/def/cim-smartgrid#Status.remark> .

:Status rdfs:subClassOf _:node1912nb34nx213 .

_:node1912nb34nx213 a owl:Restriction ;
	owl:allValuesFrom xsd:string ;
	owl:onProperty <http://ns.cerise-project.nl/energy/def/cim-smartgrid#Status.reason> .

:Status rdfs:subClassOf _:node1912nb34nx214 .

_:node1912nb34nx214 a owl:Restriction ;
	owl:cardinality "1"^^xsd:int ;
	owl:onProperty <http://ns.cerise-project.nl/energy/def/cim-smartgrid#Status.reason> .

:Status rdfs:subClassOf _:node1912nb34nx215 .

_:node1912nb34nx215 a owl:Restriction ;
	owl:cardinality "1"^^xsd:int ;
	owl:onProperty <http://ns.cerise-project.nl/energy/def/cim-smartgrid#Status.dateTime> .

:Status rdfs:subClassOf _:node1912nb34nx216 .

_:node1912nb34nx216 a owl:Restriction ;
	owl:allValuesFrom xsd:dateTime ;
	owl:onProperty <http://ns.cerise-project.nl/energy/def/cim-smartgrid#Status.dateTime> .

:Status rdfs:subClassOf _:node1912nb34nx217 .

_:node1912nb34nx217 a owl:Restriction ;
	owl:cardinality "1"^^xsd:int ;
	owl:onProperty <http://ns.cerise-project.nl/energy/def/cim-smartgrid#Status.value> .

:Status rdfs:subClassOf _:node1912nb34nx218 .

_:node1912nb34nx218 a owl:Restriction ;
	owl:allValuesFrom xsd:string ;
	owl:onProperty <http://ns.cerise-project.nl/energy/def/cim-smartgrid#Status.value> .

:ElectronicAddress rdfs:subClassOf _:node1912nb34nx219 .

_:node1912nb34nx219 a owl:Restriction ;
	owl:cardinality "1"^^xsd:int ;
	owl:onProperty <http://ns.cerise-project.nl/energy/def/cim-smartgrid#ElectronicAddress.web> .

:ElectronicAddress rdfs:subClassOf _:node1912nb34nx220 .

_:node1912nb34nx220 a owl:Restriction ;
	owl:allValuesFrom xsd:string ;
	owl:onProperty <http://ns.cerise-project.nl/energy/def/cim-smartgrid#ElectronicAddress.password> .

:ElectronicAddress rdfs:subClassOf _:node1912nb34nx221 .

_:node1912nb34nx221 a owl:Restriction ;
	owl:cardinality "1"^^xsd:int ;
	owl:onProperty <http://ns.cerise-project.nl/energy/def/cim-smartgrid#ElectronicAddress.email1> .

:ElectronicAddress rdfs:subClassOf _:node1912nb34nx222 .

_:node1912nb34nx222 a owl:Restriction ;
	owl:cardinality "1"^^xsd:int ;
	owl:onProperty <http://ns.cerise-project.nl/energy/def/cim-smartgrid#ElectronicAddress.password> .

:ElectronicAddress rdfs:subClassOf _:node1912nb34nx223 .

_:node1912nb34nx223 a owl:Restriction ;
	owl:cardinality "1"^^xsd:int ;
	owl:onProperty <http://ns.cerise-project.nl/energy/def/cim-smartgrid#ElectronicAddress.email2> .

:ElectronicAddress rdfs:subClassOf _:node1912nb34nx224 .

_:node1912nb34nx224 a owl:Restriction ;
	owl:cardinality "1"^^xsd:int ;
	owl:onProperty <http://ns.cerise-project.nl/energy/def/cim-smartgrid#ElectronicAddress.userID> .

:ElectronicAddress rdfs:subClassOf _:node1912nb34nx225 .

_:node1912nb34nx225 a owl:Restriction ;
	owl:cardinality "1"^^xsd:int ;
	owl:onProperty <http://ns.cerise-project.nl/energy/def/cim-smartgrid#ElectronicAddress.radio> .

:ElectronicAddress rdfs:subClassOf _:node1912nb34nx226 .

_:node1912nb34nx226 a owl:Restriction ;
	owl:allValuesFrom xsd:string ;
	owl:onProperty <http://ns.cerise-project.nl/energy/def/cim-smartgrid#ElectronicAddress.lan> .

:ElectronicAddress rdfs:subClassOf _:node1912nb34nx227 .

_:node1912nb34nx227 a owl:Restriction ;
	owl:allValuesFrom xsd:string ;
	owl:onProperty <http://ns.cerise-project.nl/energy/def/cim-smartgrid#ElectronicAddress.email2> .

:ElectronicAddress rdfs:subClassOf _:node1912nb34nx228 .

_:node1912nb34nx228 a owl:Restriction ;
	owl:allValuesFrom xsd:string ;
	owl:onProperty <http://ns.cerise-project.nl/energy/def/cim-smartgrid#ElectronicAddress.mac> .

:ElectronicAddress rdfs:subClassOf _:node1912nb34nx229 .

_:node1912nb34nx229 a owl:Restriction ;
	owl:allValuesFrom xsd:string ;
	owl:onProperty <http://ns.cerise-project.nl/energy/def/cim-smartgrid#ElectronicAddress.email1> .

:ElectronicAddress rdfs:subClassOf _:node1912nb34nx230 .

_:node1912nb34nx230 a owl:Restriction ;
	owl:allValuesFrom xsd:string ;
	owl:onProperty <http://ns.cerise-project.nl/energy/def/cim-smartgrid#ElectronicAddress.userID> .

:ElectronicAddress rdfs:subClassOf _:node1912nb34nx231 .

_:node1912nb34nx231 a owl:Restriction ;
	owl:cardinality "1"^^xsd:int ;
	owl:onProperty <http://ns.cerise-project.nl/energy/def/cim-smartgrid#ElectronicAddress.lan> .

:ElectronicAddress rdfs:subClassOf _:node1912nb34nx232 .

_:node1912nb34nx232 a owl:Restriction ;
	owl:allValuesFrom xsd:string ;
	owl:onProperty <http://ns.cerise-project.nl/energy/def/cim-smartgrid#ElectronicAddress.radio> .

:ElectronicAddress rdfs:subClassOf _:node1912nb34nx233 .

_:node1912nb34nx233 a owl:Restriction ;
	owl:cardinality "1"^^xsd:int ;
	owl:onProperty <http://ns.cerise-project.nl/energy/def/cim-smartgrid#ElectronicAddress.mac> .

:ElectronicAddress rdfs:subClassOf _:node1912nb34nx234 .

_:node1912nb34nx234 a owl:Restriction ;
	owl:allValuesFrom xsd:string ;
	owl:onProperty <http://ns.cerise-project.nl/energy/def/cim-smartgrid#ElectronicAddress.web> .

:EndDeviceFunction rdfs:subClassOf _:node1912nb34nx235 .

_:node1912nb34nx235 a owl:Restriction ;
	owl:cardinality "1"^^xsd:int ;
	owl:onProperty <http://ns.cerise-project.nl/energy/def/cim-smartgrid#EndDeviceFunction.EndDevice> .

:EndDeviceFunction rdfs:subClassOf _:node1912nb34nx236 .

_:node1912nb34nx236 a owl:Restriction ;
	owl:allValuesFrom :EndDevice ;
	owl:onProperty <http://ns.cerise-project.nl/energy/def/cim-smartgrid#EndDeviceFunction.EndDevice> .

:IntervalReading rdfs:subClassOf _:node1912nb34nx237 .

_:node1912nb34nx237 a owl:Restriction ;
	owl:minCardinality "1"^^xsd:int ;
	owl:onProperty <http://ns.cerise-project.nl/energy/def/cim-smartgrid#IntervalReading.IntervalBlocks> .

:IntervalReading rdfs:subClassOf _:node1912nb34nx238 .

_:node1912nb34nx238 a owl:Restriction ;
	owl:onProperty <http://ns.cerise-project.nl/energy/def/cim-smartgrid#IntervalReading.IntervalBlocks> ;
	owl:allValuesFrom :IntervalBlock .

:CoordinateSystem rdfs:subClassOf _:node1912nb34nx239 .

_:node1912nb34nx239 a owl:Restriction ;
	owl:minCardinality "1"^^xsd:int ;
	owl:onProperty <http://ns.cerise-project.nl/energy/def/cim-smartgrid#CoordinateSystem.Location> .

:CoordinateSystem rdfs:subClassOf _:node1912nb34nx240 .

_:node1912nb34nx240 a owl:Restriction ;
	owl:allValuesFrom :Location ;
	owl:onProperty <http://ns.cerise-project.nl/energy/def/cim-smartgrid#CoordinateSystem.Location> .

:CoordinateSystem rdfs:subClassOf _:node1912nb34nx241 .

_:node1912nb34nx241 a owl:Restriction ;
	owl:cardinality "1"^^xsd:int ;
	owl:onProperty <http://ns.cerise-project.nl/energy/def/cim-smartgrid#CoordinateSystem.crsUrn> .

:CoordinateSystem rdfs:subClassOf _:node1912nb34nx242 .

_:node1912nb34nx242 a owl:Restriction ;
	owl:allValuesFrom xsd:string ;
	owl:onProperty <http://ns.cerise-project.nl/energy/def/cim-smartgrid#CoordinateSystem.crsUrn> .

:StreetDetail rdfs:subClassOf _:node1912nb34nx243 .

_:node1912nb34nx243 a owl:Restriction ;
	owl:cardinality "1"^^xsd:int ;
	owl:onProperty <http://ns.cerise-project.nl/energy/def/cim-smartgrid#StreetDetail.code> .

:StreetDetail rdfs:subClassOf _:node1912nb34nx244 .

_:node1912nb34nx244 a owl:Restriction ;
	owl:cardinality "1"^^xsd:int ;
	owl:onProperty <http://ns.cerise-project.nl/energy/def/cim-smartgrid#StreetDetail.prefix> .

:StreetDetail rdfs:subClassOf _:node1912nb34nx245 .

_:node1912nb34nx245 a owl:Restriction ;
	owl:cardinality "1"^^xsd:int ;
	owl:onProperty <http://ns.cerise-project.nl/energy/def/cim-smartgrid#StreetDetail.suiteNumber> .

:StreetDetail rdfs:subClassOf _:node1912nb34nx246 .

_:node1912nb34nx246 a owl:Restriction ;
	owl:allValuesFrom xsd:boolean ;
	owl:onProperty <http://ns.cerise-project.nl/energy/def/cim-smartgrid#StreetDetail.withinTownLimits> .

:StreetDetail rdfs:subClassOf _:node1912nb34nx247 .

_:node1912nb34nx247 a owl:Restriction ;
	owl:cardinality "1"^^xsd:int ;
	owl:onProperty <http://ns.cerise-project.nl/energy/def/cim-smartgrid#StreetDetail.type> .

:StreetDetail rdfs:subClassOf _:node1912nb34nx248 .

_:node1912nb34nx248 a owl:Restriction ;
	owl:allValuesFrom xsd:string ;
	owl:onProperty <http://ns.cerise-project.nl/energy/def/cim-smartgrid#StreetDetail.suffix> .

:StreetDetail rdfs:subClassOf _:node1912nb34nx249 .

_:node1912nb34nx249 a owl:Restriction ;
	owl:allValuesFrom xsd:string ;
	owl:onProperty <http://ns.cerise-project.nl/energy/def/cim-smartgrid#StreetDetail.suiteNumber> .

:StreetDetail rdfs:subClassOf _:node1912nb34nx250 .

_:node1912nb34nx250 a owl:Restriction ;
	owl:cardinality "1"^^xsd:int ;
	owl:onProperty <http://ns.cerise-project.nl/energy/def/cim-smartgrid#StreetDetail.buildingName> .

:StreetDetail rdfs:subClassOf _:node1912nb34nx251 .

_:node1912nb34nx251 a owl:Restriction ;
	owl:cardinality "1"^^xsd:int ;
	owl:onProperty <http://ns.cerise-project.nl/energy/def/cim-smartgrid#StreetDetail.addressGeneral> .

:StreetDetail rdfs:subClassOf _:node1912nb34nx252 .

_:node1912nb34nx252 a owl:Restriction ;
	owl:cardinality "1"^^xsd:int ;
	owl:onProperty <http://ns.cerise-project.nl/energy/def/cim-smartgrid#StreetDetail.withinTownLimits> .

:StreetDetail rdfs:subClassOf _:node1912nb34nx253 .

_:node1912nb34nx253 a owl:Restriction ;
	owl:cardinality "1"^^xsd:int ;
	owl:onProperty <http://ns.cerise-project.nl/energy/def/cim-smartgrid#StreetDetail.name> .

:StreetDetail rdfs:subClassOf _:node1912nb34nx254 .

_:node1912nb34nx254 a owl:Restriction ;
	owl:allValuesFrom xsd:string ;
	owl:onProperty <http://ns.cerise-project.nl/energy/def/cim-smartgrid#StreetDetail.type> .

:StreetDetail rdfs:subClassOf _:node1912nb34nx255 .

_:node1912nb34nx255 a owl:Restriction ;
	owl:allValuesFrom xsd:string ;
	owl:onProperty <http://ns.cerise-project.nl/energy/def/cim-smartgrid#StreetDetail.addressGeneral> .

:StreetDetail rdfs:subClassOf _:node1912nb34nx256 .

_:node1912nb34nx256 a owl:Restriction ;
	owl:allValuesFrom xsd:string ;
	owl:onProperty <http://ns.cerise-project.nl/energy/def/cim-smartgrid#StreetDetail.buildingName> .

:StreetDetail rdfs:subClassOf _:node1912nb34nx257 .

_:node1912nb34nx257 a owl:Restriction ;
	owl:cardinality "1"^^xsd:int ;
	owl:onProperty <http://ns.cerise-project.nl/energy/def/cim-smartgrid#StreetDetail.suffix> .

:StreetDetail rdfs:subClassOf _:node1912nb34nx258 .

_:node1912nb34nx258 a owl:Restriction ;
	owl:cardinality "1"^^xsd:int ;
	owl:onProperty <http://ns.cerise-project.nl/energy/def/cim-smartgrid#StreetDetail.number> .

:StreetDetail rdfs:subClassOf _:node1912nb34nx259 .

_:node1912nb34nx259 a owl:Restriction ;
	owl:allValuesFrom xsd:string ;
	owl:onProperty <http://ns.cerise-project.nl/energy/def/cim-smartgrid#StreetDetail.code> .

:StreetDetail rdfs:subClassOf _:node1912nb34nx260 .

_:node1912nb34nx260 a owl:Restriction ;
	owl:allValuesFrom xsd:string ;
	owl:onProperty <http://ns.cerise-project.nl/energy/def/cim-smartgrid#StreetDetail.prefix> .

:StreetDetail rdfs:subClassOf _:node1912nb34nx261 .

_:node1912nb34nx261 a owl:Restriction ;
	owl:allValuesFrom xsd:string ;
	owl:onProperty <http://ns.cerise-project.nl/energy/def/cim-smartgrid#StreetDetail.number> .

:StreetDetail rdfs:subClassOf _:node1912nb34nx262 .

_:node1912nb34nx262 a owl:Restriction ;
	owl:allValuesFrom xsd:string ;
	owl:onProperty <http://ns.cerise-project.nl/energy/def/cim-smartgrid#StreetDetail.name> .

:MeterMultiplier rdfs:subClassOf _:node1912nb34nx263 .

_:node1912nb34nx263 a owl:Restriction ;
	owl:cardinality "1"^^xsd:int ;
	owl:onProperty <http://ns.cerise-project.nl/energy/def/cim-smartgrid#MeterMultiplier.Meter> .

:MeterMultiplier rdfs:subClassOf _:node1912nb34nx264 .

_:node1912nb34nx264 a owl:Restriction ;
	owl:allValuesFrom :MeterMultiplierKind ;
	owl:onProperty <http://ns.cerise-project.nl/energy/def/cim-smartgrid#MeterMultiplier.kind> .

:MeterMultiplier rdfs:subClassOf _:node1912nb34nx265 .

_:node1912nb34nx265 a owl:Restriction ;
	owl:onProperty <http://ns.cerise-project.nl/energy/def/cim-smartgrid#MeterMultiplier.Meter> ;
	owl:allValuesFrom :Meter .

:MeterMultiplier rdfs:subClassOf _:node1912nb34nx266 .

_:node1912nb34nx266 a owl:Restriction ;
	owl:cardinality "1"^^xsd:int ;
	owl:onProperty <http://ns.cerise-project.nl/energy/def/cim-smartgrid#MeterMultiplier.kind> .

:MeterMultiplier rdfs:subClassOf _:node1912nb34nx267 .

_:node1912nb34nx267 a owl:Restriction ;
	owl:cardinality "1"^^xsd:int ;
	owl:onProperty <http://ns.cerise-project.nl/energy/def/cim-smartgrid#MeterMultiplier.value> .

:MeterMultiplier rdfs:subClassOf _:node1912nb34nx268 .

_:node1912nb34nx268 a owl:Restriction ;
	owl:allValuesFrom xsd:float ;
	owl:onProperty <http://ns.cerise-project.nl/energy/def/cim-smartgrid#MeterMultiplier.value> .

:EndDevice rdfs:subClassOf _:node1912nb34nx269 .

_:node1912nb34nx269 a owl:Restriction ;
	owl:cardinality "1"^^xsd:int ;
	owl:onProperty <http://ns.cerise-project.nl/energy/def/cim-smartgrid#EndDevice.isVirtual> .

:EndDevice rdfs:subClassOf _:node1912nb34nx270 .

_:node1912nb34nx270 a owl:Restriction ;
	owl:onProperty <http://ns.cerise-project.nl/energy/def/cim-smartgrid#EndDevice.UsagePoint> ;
	owl:allValuesFrom :UsagePoint .

:EndDevice rdfs:subClassOf _:node1912nb34nx271 .

_:node1912nb34nx271 a owl:Restriction ;
	owl:minCardinality "1"^^xsd:int ;
	owl:onProperty <http://ns.cerise-project.nl/energy/def/cim-smartgrid#EndDevice.EndDeviceFunctions> .

:EndDevice rdfs:subClassOf _:node1912nb34nx272 .

_:node1912nb34nx272 a owl:Restriction ;
	owl:onProperty <http://ns.cerise-project.nl/energy/def/cim-smartgrid#EndDevice.EndDeviceFunctions> ;
	owl:allValuesFrom :EndDeviceFunction .

:EndDevice rdfs:subClassOf _:node1912nb34nx273 .

_:node1912nb34nx273 a owl:Restriction ;
	owl:cardinality "1"^^xsd:int ;
	owl:onProperty <http://ns.cerise-project.nl/energy/def/cim-smartgrid#EndDevice.UsagePoint> .

:EndDevice rdfs:subClassOf _:node1912nb34nx274 .

_:node1912nb34nx274 a owl:Restriction ;
	owl:allValuesFrom xsd:boolean ;
	owl:onProperty <http://ns.cerise-project.nl/energy/def/cim-smartgrid#EndDevice.isVirtual> .

:EndDevice rdfs:subClassOf _:node1912nb34nx275 .

_:node1912nb34nx275 a owl:Restriction ;
	owl:cardinality "1"^^xsd:int ;
	owl:onProperty <http://ns.cerise-project.nl/energy/def/cim-smartgrid#EndDevice.installCode> .

:EndDevice rdfs:subClassOf _:node1912nb34nx276 .

_:node1912nb34nx276 a owl:Restriction ;
	owl:allValuesFrom xsd:string ;
	owl:onProperty <http://ns.cerise-project.nl/energy/def/cim-smartgrid#EndDevice.installCode> .

:ReadingType rdfs:subClassOf _:node1912nb34nx277 .

_:node1912nb34nx277 a owl:Restriction ;
	owl:allValuesFrom xsd:string ;
	owl:onProperty <http://ns.cerise-project.nl/energy/def/cim-smartgrid#ReadingType.unit> .

:ReadingType rdfs:subClassOf _:node1912nb34nx278 .

_:node1912nb34nx278 a owl:Restriction ;
	owl:cardinality "1"^^xsd:int ;
	owl:onProperty <http://ns.cerise-project.nl/energy/def/cim-smartgrid#ReadingType.unit> .

:ReadingType rdfs:subClassOf _:node1912nb34nx279 .

_:node1912nb34nx279 a owl:Restriction ;
	owl:allValuesFrom xsd:string ;
	owl:onProperty <http://ns.cerise-project.nl/energy/def/cim-smartgrid#ReadingType.measuringPeriod> .

:ReadingType rdfs:subClassOf _:node1912nb34nx280 .

_:node1912nb34nx280 a owl:Restriction ;
	owl:cardinality "1"^^xsd:int ;
	owl:onProperty <http://ns.cerise-project.nl/energy/def/cim-smartgrid#ReadingType.accumulation> .

:ReadingType rdfs:subClassOf _:node1912nb34nx281 .

_:node1912nb34nx281 a owl:Restriction ;
	owl:cardinality "1"^^xsd:int ;
	owl:onProperty <http://ns.cerise-project.nl/energy/def/cim-smartgrid#ReadingType.commodity> .

:ReadingType rdfs:subClassOf _:node1912nb34nx282 .

_:node1912nb34nx282 a owl:Restriction ;
	owl:allValuesFrom xsd:string ;
	owl:onProperty <http://ns.cerise-project.nl/energy/def/cim-smartgrid#ReadingType.commodity> .

:ReadingType rdfs:subClassOf _:node1912nb34nx283 .

_:node1912nb34nx283 a owl:Restriction ;
	owl:allValuesFrom xsd:string ;
	owl:onProperty <http://ns.cerise-project.nl/energy/def/cim-smartgrid#ReadingType.aggregate> .

:ReadingType rdfs:subClassOf _:node1912nb34nx284 .

_:node1912nb34nx284 a owl:Restriction ;
	owl:allValuesFrom xsd:string ;
	owl:onProperty <http://ns.cerise-project.nl/energy/def/cim-smartgrid#ReadingType.accumulation> .

:ReadingType rdfs:subClassOf _:node1912nb34nx285 .

_:node1912nb34nx285 a owl:Restriction ;
	owl:allValuesFrom xsd:string ;
	owl:onProperty <http://ns.cerise-project.nl/energy/def/cim-smartgrid#ReadingType.measurementKind> .

:ReadingType rdfs:subClassOf _:node1912nb34nx286 .

_:node1912nb34nx286 a owl:Restriction ;
	owl:cardinality "1"^^xsd:int ;
	owl:onProperty <http://ns.cerise-project.nl/energy/def/cim-smartgrid#ReadingType.measuringPeriod> .

:ReadingType rdfs:subClassOf _:node1912nb34nx287 .

_:node1912nb34nx287 a owl:Restriction ;
	owl:cardinality "1"^^xsd:int ;
	owl:onProperty <http://ns.cerise-project.nl/energy/def/cim-smartgrid#ReadingType.measurementKind> .

:ReadingType rdfs:subClassOf _:node1912nb34nx288 .

_:node1912nb34nx288 a owl:Restriction ;
	owl:allValuesFrom xsd:string ;
	owl:onProperty <http://ns.cerise-project.nl/energy/def/cim-smartgrid#ReadingType.flowDirection> .

:ReadingType rdfs:subClassOf _:node1912nb34nx289 .

_:node1912nb34nx289 a owl:Restriction ;
	owl:cardinality "1"^^xsd:int ;
	owl:onProperty <http://ns.cerise-project.nl/energy/def/cim-smartgrid#ReadingType.aggregate> .

:ReadingType rdfs:subClassOf _:node1912nb34nx290 .

_:node1912nb34nx290 a owl:Restriction ;
	owl:cardinality "1"^^xsd:int ;
	owl:onProperty <http://ns.cerise-project.nl/energy/def/cim-smartgrid#ReadingType.flowDirection> .

:BaseReading rdfs:subClassOf _:node1912nb34nx291 .

_:node1912nb34nx291 a owl:Restriction ;
	owl:onProperty <http://ns.cerise-project.nl/energy/def/cim-smartgrid#BaseReading.timePeriod> ;
	owl:allValuesFrom :DateTimeInterval .

:BaseReading rdfs:subClassOf _:node1912nb34nx292 .

_:node1912nb34nx292 a owl:Restriction ;
	owl:cardinality "1"^^xsd:int ;
	owl:onProperty <http://ns.cerise-project.nl/energy/def/cim-smartgrid#BaseReading.source> .

:BaseReading rdfs:subClassOf _:node1912nb34nx293 .

_:node1912nb34nx293 a owl:Restriction ;
	owl:cardinality "1"^^xsd:int ;
	owl:onProperty <http://ns.cerise-project.nl/energy/def/cim-smartgrid#BaseReading.value> .

:BaseReading rdfs:subClassOf _:node1912nb34nx294 .

_:node1912nb34nx294 a owl:Restriction ;
	owl:cardinality "1"^^xsd:int ;
	owl:onProperty <http://ns.cerise-project.nl/energy/def/cim-smartgrid#BaseReading.timePeriod> .

:BaseReading rdfs:subClassOf _:node1912nb34nx295 .

_:node1912nb34nx295 a owl:Restriction ;
	owl:allValuesFrom xsd:string ;
	owl:onProperty <http://ns.cerise-project.nl/energy/def/cim-smartgrid#BaseReading.value> .

:BaseReading rdfs:subClassOf _:node1912nb34nx296 .

_:node1912nb34nx296 a owl:Restriction ;
	owl:allValuesFrom xsd:string ;
	owl:onProperty <http://ns.cerise-project.nl/energy/def/cim-smartgrid#BaseReading.source> .

:IdentifiedObject rdfs:subClassOf _:node1912nb34nx297 .

_:node1912nb34nx297 a owl:Restriction ;
	owl:cardinality "1"^^xsd:int ;
	owl:onProperty <http://ns.cerise-project.nl/energy/def/cim-smartgrid#IdentifiedObject.aliasName> .

:IdentifiedObject rdfs:subClassOf _:node1912nb34nx298 .

_:node1912nb34nx298 a owl:Restriction ;
	owl:allValuesFrom xsd:string ;
	owl:onProperty <http://ns.cerise-project.nl/energy/def/cim-smartgrid#IdentifiedObject.mRID> .

:IdentifiedObject rdfs:subClassOf _:node1912nb34nx299 .

_:node1912nb34nx299 a owl:Restriction ;
	owl:cardinality "1"^^xsd:int ;
	owl:onProperty <http://ns.cerise-project.nl/energy/def/cim-smartgrid#IdentifiedObject.name> .

:IdentifiedObject rdfs:subClassOf _:node1912nb34nx300 .

_:node1912nb34nx300 a owl:Restriction ;
	owl:allValuesFrom xsd:string ;
	owl:onProperty <http://ns.cerise-project.nl/energy/def/cim-smartgrid#IdentifiedObject.name> .

:IdentifiedObject rdfs:subClassOf _:node1912nb34nx301 .

_:node1912nb34nx301 a owl:Restriction ;
	owl:allValuesFrom xsd:string ;
	owl:onProperty <http://ns.cerise-project.nl/energy/def/cim-smartgrid#IdentifiedObject.description> .

:IdentifiedObject rdfs:subClassOf _:node1912nb34nx302 .

_:node1912nb34nx302 a owl:Restriction ;
	owl:cardinality "1"^^xsd:int ;
	owl:onProperty <http://ns.cerise-project.nl/energy/def/cim-smartgrid#IdentifiedObject.mRID> .

:IdentifiedObject rdfs:subClassOf _:node1912nb34nx303 .

_:node1912nb34nx303 a owl:Restriction ;
	owl:cardinality "1"^^xsd:int ;
	owl:onProperty <http://ns.cerise-project.nl/energy/def/cim-smartgrid#IdentifiedObject.description> .

:IdentifiedObject rdfs:subClassOf _:node1912nb34nx304 .

_:node1912nb34nx304 a owl:Restriction ;
	owl:allValuesFrom xsd:string ;
	owl:onProperty <http://ns.cerise-project.nl/energy/def/cim-smartgrid#IdentifiedObject.aliasName> .

:ServiceCategory rdfs:subClassOf _:node1912nb34nx305 .

_:node1912nb34nx305 a owl:Restriction ;
	owl:cardinality "1"^^xsd:int ;
	owl:onProperty <http://ns.cerise-project.nl/energy/def/cim-smartgrid#ServiceCategory.kind> .

:ServiceCategory rdfs:subClassOf _:node1912nb34nx306 .

_:node1912nb34nx306 a owl:Restriction ;
	owl:onProperty <http://ns.cerise-project.nl/energy/def/cim-smartgrid#ServiceCategory.kind> ;
	owl:allValuesFrom :ServiceKind .

:StreetAddress rdfs:subClassOf _:node1912nb34nx307 .

_:node1912nb34nx307 a owl:Restriction ;
	owl:cardinality "1"^^xsd:int ;
	owl:onProperty <http://ns.cerise-project.nl/energy/def/cim-smartgrid#StreetAddress.townDetail> .

:StreetAddress rdfs:subClassOf _:node1912nb34nx308 .

_:node1912nb34nx308 a owl:Restriction ;
	owl:allValuesFrom :TownDetail ;
	owl:onProperty <http://ns.cerise-project.nl/energy/def/cim-smartgrid#StreetAddress.townDetail> .

:StreetAddress rdfs:subClassOf _:node1912nb34nx309 .

_:node1912nb34nx309 a owl:Restriction ;
	owl:cardinality "1"^^xsd:int ;
	owl:onProperty <http://ns.cerise-project.nl/energy/def/cim-smartgrid#StreetAddress.streetDetail> .

:StreetAddress rdfs:subClassOf _:node1912nb34nx310 .

_:node1912nb34nx310 a owl:Restriction ;
	owl:allValuesFrom :StreetDetail ;
	owl:onProperty <http://ns.cerise-project.nl/energy/def/cim-smartgrid#StreetAddress.streetDetail> .

:PositionPoint rdfs:subClassOf _:node1912nb34nx311 .

_:node1912nb34nx311 a owl:Restriction ;
	owl:cardinality "1"^^xsd:int ;
	owl:onProperty <http://ns.cerise-project.nl/energy/def/cim-smartgrid#PositionPoint.sequenceNumber> .

:PositionPoint rdfs:subClassOf _:node1912nb34nx312 .

_:node1912nb34nx312 a owl:Restriction ;
	owl:cardinality "1"^^xsd:int ;
	owl:onProperty <http://ns.cerise-project.nl/energy/def/cim-smartgrid#PositionPoint.xPosition> .

:PositionPoint rdfs:subClassOf _:node1912nb34nx313 .

_:node1912nb34nx313 a owl:Restriction ;
	owl:allValuesFrom :Location ;
	owl:onProperty <http://ns.cerise-project.nl/energy/def/cim-smartgrid#PositionPoint.Location> .

:PositionPoint rdfs:subClassOf _:node1912nb34nx314 .

_:node1912nb34nx314 a owl:Restriction ;
	owl:allValuesFrom xsd:string ;
	owl:onProperty <http://ns.cerise-project.nl/energy/def/cim-smartgrid#PositionPoint.xPosition> .

:PositionPoint rdfs:subClassOf _:node1912nb34nx315 .

_:node1912nb34nx315 a owl:Restriction ;
	owl:allValuesFrom xsd:string ;
	owl:onProperty <http://ns.cerise-project.nl/energy/def/cim-smartgrid#PositionPoint.zPosition> .

:PositionPoint rdfs:subClassOf _:node1912nb34nx316 .

_:node1912nb34nx316 a owl:Restriction ;
	owl:allValuesFrom xsd:integer ;
	owl:onProperty <http://ns.cerise-project.nl/energy/def/cim-smartgrid#PositionPoint.sequenceNumber> .

:PositionPoint rdfs:subClassOf _:node1912nb34nx317 .

_:node1912nb34nx317 a owl:Restriction ;
	owl:cardinality "1"^^xsd:int ;
	owl:onProperty <http://ns.cerise-project.nl/energy/def/cim-smartgrid#PositionPoint.yPosition> .

:PositionPoint rdfs:subClassOf _:node1912nb34nx318 .

_:node1912nb34nx318 a owl:Restriction ;
	owl:cardinality "1"^^xsd:int ;
	owl:onProperty <http://ns.cerise-project.nl/energy/def/cim-smartgrid#PositionPoint.Location> .

:PositionPoint rdfs:subClassOf _:node1912nb34nx319 .

_:node1912nb34nx319 a owl:Restriction ;
	owl:cardinality "1"^^xsd:int ;
	owl:onProperty <http://ns.cerise-project.nl/energy/def/cim-smartgrid#PositionPoint.zPosition> .

:PositionPoint rdfs:subClassOf _:node1912nb34nx320 .

_:node1912nb34nx320 a owl:Restriction ;
	owl:allValuesFrom xsd:string ;
	owl:onProperty <http://ns.cerise-project.nl/energy/def/cim-smartgrid#PositionPoint.yPosition> .

:MeterReading rdfs:subClassOf _:node1912nb34nx321 .

_:node1912nb34nx321 a owl:Restriction ;
	owl:allValuesFrom :Reading ;
	owl:onProperty <http://ns.cerise-project.nl/energy/def/cim-smartgrid#MeterReading.Readings> .

:MeterReading rdfs:subClassOf _:node1912nb34nx322 .

_:node1912nb34nx322 a owl:Restriction ;
	owl:minCardinality "1"^^xsd:int ;
	owl:onProperty <http://ns.cerise-project.nl/energy/def/cim-smartgrid#MeterReading.Readings> .

:MeterReading rdfs:subClassOf _:node1912nb34nx323 .

_:node1912nb34nx323 a owl:Restriction ;
	owl:cardinality "1"^^xsd:int ;
	owl:onProperty <http://ns.cerise-project.nl/energy/def/cim-smartgrid#MeterReading.UsagePoint> .

:MeterReading rdfs:subClassOf _:node1912nb34nx324 .

_:node1912nb34nx324 a owl:Restriction ;
	owl:cardinality "1"^^xsd:int ;
	owl:onProperty <http://ns.cerise-project.nl/energy/def/cim-smartgrid#MeterReading.CustomerAgreement> .

:MeterReading rdfs:subClassOf _:node1912nb34nx325 .

_:node1912nb34nx325 a owl:Restriction ;
	owl:allValuesFrom :UsagePoint ;
	owl:onProperty <http://ns.cerise-project.nl/energy/def/cim-smartgrid#MeterReading.UsagePoint> .

:MeterReading rdfs:subClassOf _:node1912nb34nx326 .

_:node1912nb34nx326 a owl:Restriction ;
	owl:allValuesFrom :CustomerAgreement ;
	owl:onProperty <http://ns.cerise-project.nl/energy/def/cim-smartgrid#MeterReading.CustomerAgreement> .

:MeterReading rdfs:subClassOf _:node1912nb34nx327 .

_:node1912nb34nx327 a owl:Restriction ;
	owl:cardinality "1"^^xsd:int ;
	owl:onProperty <http://ns.cerise-project.nl/energy/def/cim-smartgrid#MeterReading.Meter> .

:MeterReading rdfs:subClassOf _:node1912nb34nx328 .

_:node1912nb34nx328 a owl:Restriction ;
	owl:cardinality "1"^^xsd:int ;
	owl:onProperty <http://ns.cerise-project.nl/energy/def/cim-smartgrid#MeterReading.valuesInterval> .

:MeterReading rdfs:subClassOf _:node1912nb34nx329 .

_:node1912nb34nx329 a owl:Restriction ;
	owl:onProperty <http://ns.cerise-project.nl/energy/def/cim-smartgrid#MeterReading.valuesInterval> ;
	owl:allValuesFrom :DateTimeInterval .

:MeterReading rdfs:subClassOf _:node1912nb34nx330 .

_:node1912nb34nx330 a owl:Restriction ;
	owl:allValuesFrom :Meter ;
	owl:onProperty <http://ns.cerise-project.nl/energy/def/cim-smartgrid#MeterReading.Meter> .

:Location rdfs:subClassOf _:node1912nb34nx331 .

_:node1912nb34nx331 a owl:Restriction ;
	owl:cardinality "1"^^xsd:int ;
	owl:onProperty <http://ns.cerise-project.nl/energy/def/cim-smartgrid#Location.mainAddress> .

:Location rdfs:subClassOf _:node1912nb34nx332 .

_:node1912nb34nx332 a owl:Restriction ;
	owl:allValuesFrom :StreetAddress ;
	owl:onProperty <http://ns.cerise-project.nl/energy/def/cim-smartgrid#Location.mainAddress> .

:Location rdfs:subClassOf _:node1912nb34nx333 .

_:node1912nb34nx333 a owl:Restriction ;
	owl:onProperty <http://ns.cerise-project.nl/energy/def/cim-smartgrid#Location.electronicAddress> ;
	owl:allValuesFrom :ElectronicAddress .

:Location rdfs:subClassOf _:node1912nb34nx334 .

_:node1912nb34nx334 a owl:Restriction ;
	owl:cardinality "1"^^xsd:int ;
	owl:onProperty <http://ns.cerise-project.nl/energy/def/cim-smartgrid#Location.type> .

:Location rdfs:subClassOf _:node1912nb34nx335 .

_:node1912nb34nx335 a owl:Restriction ;
	owl:cardinality "1"^^xsd:int ;
	owl:onProperty <http://ns.cerise-project.nl/energy/def/cim-smartgrid#Location.phone2> .

:Location rdfs:subClassOf _:node1912nb34nx336 .

_:node1912nb34nx336 a owl:Restriction ;
	owl:cardinality "1"^^xsd:int ;
	owl:onProperty <http://ns.cerise-project.nl/energy/def/cim-smartgrid#Location.electronicAddress> .

:Location rdfs:subClassOf _:node1912nb34nx337 .

_:node1912nb34nx337 a owl:Restriction ;
	owl:cardinality "1"^^xsd:int ;
	owl:onProperty <http://ns.cerise-project.nl/energy/def/cim-smartgrid#Location.geoInfoReference> .

:Location rdfs:subClassOf _:node1912nb34nx338 .

_:node1912nb34nx338 a owl:Restriction ;
	owl:onProperty <http://ns.cerise-project.nl/energy/def/cim-smartgrid#Location.status> ;
	owl:allValuesFrom :Status .

:Location rdfs:subClassOf _:node1912nb34nx339 .

_:node1912nb34nx339 a owl:Restriction ;
	owl:minCardinality "1"^^xsd:int ;
	owl:onProperty <http://ns.cerise-project.nl/energy/def/cim-smartgrid#Location.PositionPoints> .

:Location rdfs:subClassOf _:node1912nb34nx340 .

_:node1912nb34nx340 a owl:Restriction ;
	owl:onProperty <http://ns.cerise-project.nl/energy/def/cim-smartgrid#Location.CoordinateSystem> ;
	owl:allValuesFrom :CoordinateSystem .

:Location rdfs:subClassOf _:node1912nb34nx341 .

_:node1912nb34nx341 a owl:Restriction ;
	owl:allValuesFrom :StreetAddress ;
	owl:onProperty <http://ns.cerise-project.nl/energy/def/cim-smartgrid#Location.secondaryAddress> .

:Location rdfs:subClassOf _:node1912nb34nx342 .

_:node1912nb34nx342 a owl:Restriction ;
	owl:cardinality "1"^^xsd:int ;
	owl:onProperty <http://ns.cerise-project.nl/energy/def/cim-smartgrid#Location.secondaryAddress> .

:Location rdfs:subClassOf _:node1912nb34nx343 .

_:node1912nb34nx343 a owl:Restriction ;
	owl:cardinality "1"^^xsd:int ;
	owl:onProperty <http://ns.cerise-project.nl/energy/def/cim-smartgrid#Location.phone1> .

:Location rdfs:subClassOf _:node1912nb34nx344 .

_:node1912nb34nx344 a owl:Restriction ;
	owl:cardinality "1"^^xsd:int ;
	owl:onProperty <http://ns.cerise-project.nl/energy/def/cim-smartgrid#Location.CoordinateSystem> .

:Location rdfs:subClassOf _:node1912nb34nx345 .

_:node1912nb34nx345 a owl:Restriction ;
	owl:onProperty <http://ns.cerise-project.nl/energy/def/cim-smartgrid#Location.phone1> ;
	owl:allValuesFrom :TelephoneNumber .

:Location rdfs:subClassOf _:node1912nb34nx346 .

_:node1912nb34nx346 a owl:Restriction ;
	owl:allValuesFrom xsd:string ;
	owl:onProperty <http://ns.cerise-project.nl/energy/def/cim-smartgrid#Location.geoInfoReference> .

:Location rdfs:subClassOf _:node1912nb34nx347 .

_:node1912nb34nx347 a owl:Restriction ;
	owl:allValuesFrom xsd:string ;
	owl:onProperty <http://ns.cerise-project.nl/energy/def/cim-smartgrid#Location.type> .

:Location rdfs:subClassOf _:node1912nb34nx348 .

_:node1912nb34nx348 a owl:Restriction ;
	owl:allValuesFrom :TelephoneNumber ;
	owl:onProperty <http://ns.cerise-project.nl/energy/def/cim-smartgrid#Location.phone2> .

:Location rdfs:subClassOf _:node1912nb34nx349 .

_:node1912nb34nx349 a owl:Restriction ;
	owl:cardinality "1"^^xsd:int ;
	owl:onProperty <http://ns.cerise-project.nl/energy/def/cim-smartgrid#Location.status> .

:Location rdfs:subClassOf _:node1912nb34nx350 .

_:node1912nb34nx350 a owl:Restriction ;
	owl:allValuesFrom :PositionPoint ;
	owl:onProperty <http://ns.cerise-project.nl/energy/def/cim-smartgrid#Location.PositionPoints> .

:IntervalBlock rdfs:subClassOf _:node1912nb34nx351 .

_:node1912nb34nx351 a owl:Restriction ;
	owl:minCardinality "1"^^xsd:int ;
	owl:onProperty <http://ns.cerise-project.nl/energy/def/cim-smartgrid#IntervalBlock.IntervalReadings> .

:IntervalBlock rdfs:subClassOf _:node1912nb34nx352 .

_:node1912nb34nx352 a owl:Restriction ;
	owl:cardinality "1"^^xsd:int ;
	owl:onProperty <http://ns.cerise-project.nl/energy/def/cim-smartgrid#IntervalBlock.MeterReading> .

:IntervalBlock rdfs:subClassOf _:node1912nb34nx353 .

_:node1912nb34nx353 a owl:Restriction ;
	owl:allValuesFrom :ReadingType ;
	owl:onProperty <http://ns.cerise-project.nl/energy/def/cim-smartgrid#IntervalBlock.ReadingType> .

:IntervalBlock rdfs:subClassOf _:node1912nb34nx354 .

_:node1912nb34nx354 a owl:Restriction ;
	owl:onProperty <http://ns.cerise-project.nl/energy/def/cim-smartgrid#IntervalBlock.IntervalReadings> ;
	owl:allValuesFrom :IntervalReading .

:IntervalBlock rdfs:subClassOf _:node1912nb34nx355 .

_:node1912nb34nx355 a owl:Restriction ;
	owl:cardinality "1"^^xsd:int ;
	owl:onProperty <http://ns.cerise-project.nl/energy/def/cim-smartgrid#IntervalBlock.ReadingType> .

:IntervalBlock rdfs:subClassOf _:node1912nb34nx356 .

_:node1912nb34nx356 a owl:Restriction ;
	owl:allValuesFrom :MeterReading ;
	owl:onProperty <http://ns.cerise-project.nl/energy/def/cim-smartgrid#IntervalBlock.MeterReading> .

:SimpleEndDeviceFunction rdfs:subClassOf _:node1912nb34nx357 .

_:node1912nb34nx357 a owl:Restriction ;
	owl:cardinality "1"^^xsd:int ;
	owl:onProperty <http://ns.cerise-project.nl/energy/def/cim-smartgrid#SimpleEndDeviceFunction.kind> .

:SimpleEndDeviceFunction rdfs:subClassOf _:node1912nb34nx358 .

_:node1912nb34nx358 a owl:Restriction ;
	owl:allValuesFrom :EndDeviceFunctionKind ;
	owl:onProperty <http://ns.cerise-project.nl/energy/def/cim-smartgrid#SimpleEndDeviceFunction.kind> .

:Meter rdfs:subClassOf _:node1912nb34nx359 .

_:node1912nb34nx359 a owl:Restriction ;
	owl:allValuesFrom :MeterMultiplier ;
	owl:onProperty <http://ns.cerise-project.nl/energy/def/cim-smartgrid#Meter.MeterMultipliers> .

:Meter rdfs:subClassOf _:node1912nb34nx360 .

_:node1912nb34nx360 a owl:Restriction ;
	owl:minCardinality "1"^^xsd:int ;
	owl:onProperty <http://ns.cerise-project.nl/energy/def/cim-smartgrid#Meter.MeterReadings> .

:Meter rdfs:subClassOf _:node1912nb34nx361 .

_:node1912nb34nx361 a owl:Restriction ;
	owl:cardinality "1"^^xsd:int ;
	owl:onProperty <http://ns.cerise-project.nl/energy/def/cim-smartgrid#Meter.formNumber> .

:Meter rdfs:subClassOf _:node1912nb34nx362 .

_:node1912nb34nx362 a owl:Restriction ;
	owl:onProperty <http://ns.cerise-project.nl/energy/def/cim-smartgrid#Meter.MeterReadings> ;
	owl:allValuesFrom :MeterReading .

:Meter rdfs:subClassOf _:node1912nb34nx363 .

_:node1912nb34nx363 a owl:Restriction ;
	owl:allValuesFrom xsd:string ;
	owl:onProperty <http://ns.cerise-project.nl/energy/def/cim-smartgrid#Meter.formNumber> .

:Meter rdfs:subClassOf _:node1912nb34nx364 .

_:node1912nb34nx364 a owl:Restriction ;
	owl:minCardinality "1"^^xsd:int ;
	owl:onProperty <http://ns.cerise-project.nl/energy/def/cim-smartgrid#Meter.MeterMultipliers> .

:CustomerAgreement rdfs:subClassOf _:node1912nb34nx365 .

_:node1912nb34nx365 a owl:Restriction ;
	owl:allValuesFrom :ServiceCategory ;
	owl:onProperty <http://ns.cerise-project.nl/energy/def/cim-smartgrid#CustomerAgreement.ServiceCategory> .

:CustomerAgreement rdfs:subClassOf _:node1912nb34nx366 .

_:node1912nb34nx366 a owl:Restriction ;
	owl:cardinality "1"^^xsd:int ;
	owl:onProperty <http://ns.cerise-project.nl/energy/def/cim-smartgrid#CustomerAgreement.Customer> .

:CustomerAgreement rdfs:subClassOf _:node1912nb34nx367 .

_:node1912nb34nx367 a owl:Restriction ;
	owl:allValuesFrom :Customer ;
	owl:onProperty <http://ns.cerise-project.nl/energy/def/cim-smartgrid#CustomerAgreement.Customer> .

:CustomerAgreement rdfs:subClassOf _:node1912nb34nx368 .

_:node1912nb34nx368 a owl:Restriction ;
	owl:cardinality "1"^^xsd:int ;
	owl:onProperty <http://ns.cerise-project.nl/energy/def/cim-smartgrid#CustomerAgreement.ServiceCategory> .

:CustomerAgreement rdfs:subClassOf _:node1912nb34nx369 .

_:node1912nb34nx369 a owl:Restriction ;
	owl:cardinality "1"^^xsd:int ;
	owl:onProperty <http://ns.cerise-project.nl/energy/def/cim-smartgrid#CustomerAgreement.ServiceSupplier> .

:CustomerAgreement rdfs:subClassOf _:node1912nb34nx370 .

_:node1912nb34nx370 a owl:Restriction ;
	owl:allValuesFrom :ServiceSupplier ;
	owl:onProperty <http://ns.cerise-project.nl/energy/def/cim-smartgrid#CustomerAgreement.ServiceSupplier> .

:Reading rdfs:subClassOf _:node1912nb34nx371 .

_:node1912nb34nx371 a owl:Restriction ;
	owl:minCardinality "1"^^xsd:int ;
	owl:onProperty <http://ns.cerise-project.nl/energy/def/cim-smartgrid#Reading.MeterReadings> .

:Reading rdfs:subClassOf _:node1912nb34nx372 .

_:node1912nb34nx372 a owl:Restriction ;
	owl:onProperty <http://ns.cerise-project.nl/energy/def/cim-smartgrid#Reading.MeterReadings> ;
	owl:allValuesFrom :MeterReading .

:Reading rdfs:subClassOf _:node1912nb34nx373 .

_:node1912nb34nx373 a owl:Restriction ;
	owl:cardinality "1"^^xsd:int ;
	owl:onProperty <http://ns.cerise-project.nl/energy/def/cim-smartgrid#Reading.ReadingType> .

:Reading rdfs:subClassOf _:node1912nb34nx374 .

_:node1912nb34nx374 a owl:Restriction ;
	owl:allValuesFrom :ReadingType ;
	owl:onProperty <http://ns.cerise-project.nl/energy/def/cim-smartgrid#Reading.ReadingType> .

:UsagePoint rdfs:subClassOf _:node1912nb34nx375 .

_:node1912nb34nx375 a owl:Restriction ;
	owl:cardinality "1"^^xsd:int ;
	owl:onProperty <http://ns.cerise-project.nl/energy/def/cim-smartgrid#UsagePoint.ServiceSupplier> .

:UsagePoint rdfs:subClassOf _:node1912nb34nx376 .

_:node1912nb34nx376 a owl:Restriction ;
	owl:allValuesFrom xsd:boolean ;
	owl:onProperty <http://ns.cerise-project.nl/energy/def/cim-smartgrid#UsagePoint.isVirtual> .

:UsagePoint rdfs:subClassOf _:node1912nb34nx377 .

_:node1912nb34nx377 a owl:Restriction ;
	owl:cardinality "1"^^xsd:int ;
	owl:onProperty <http://ns.cerise-project.nl/energy/def/cim-smartgrid#UsagePoint.ServiceCategory> .

:UsagePoint rdfs:subClassOf _:node1912nb34nx378 .

_:node1912nb34nx378 a owl:Restriction ;
	owl:allValuesFrom :ServiceSupplier ;
	owl:onProperty <http://ns.cerise-project.nl/energy/def/cim-smartgrid#UsagePoint.ServiceSupplier> .

:UsagePoint rdfs:subClassOf _:node1912nb34nx379 .

_:node1912nb34nx379 a owl:Restriction ;
	owl:allValuesFrom :CustomerAgreement ;
	owl:onProperty <http://ns.cerise-project.nl/energy/def/cim-smartgrid#UsagePoint.CustomerAgreement> .

:UsagePoint rdfs:subClassOf _:node1912nb34nx380 .

_:node1912nb34nx380 a owl:Restriction ;
	owl:onProperty <http://ns.cerise-project.nl/energy/def/cim-smartgrid#UsagePoint.ServiceCategory> ;
	owl:allValuesFrom :ServiceCategory .

:UsagePoint rdfs:subClassOf _:node1912nb34nx381 .

_:node1912nb34nx381 a owl:Restriction ;
	owl:minCardinality "1"^^xsd:int ;
	owl:onProperty <http://ns.cerise-project.nl/energy/def/cim-smartgrid#UsagePoint.MeterReadings> .

:UsagePoint rdfs:subClassOf _:node1912nb34nx382 .

_:node1912nb34nx382 a owl:Restriction ;
	owl:cardinality "1"^^xsd:int ;
	owl:onProperty <http://ns.cerise-project.nl/energy/def/cim-smartgrid#UsagePoint.amiBillingReady> .

:UsagePoint rdfs:subClassOf _:node1912nb34nx383 .

_:node1912nb34nx383 a owl:Restriction ;
	owl:onProperty <http://ns.cerise-project.nl/energy/def/cim-smartgrid#UsagePoint.UsagePointLocation> ;
	owl:allValuesFrom :UsagePointLocation .

:UsagePoint rdfs:subClassOf _:node1912nb34nx384 .

_:node1912nb34nx384 a owl:Restriction ;
	owl:cardinality "1"^^xsd:int ;
	owl:onProperty <http://ns.cerise-project.nl/energy/def/cim-smartgrid#UsagePoint.CustomerAgreement> .

:UsagePoint rdfs:subClassOf _:node1912nb34nx385 .

_:node1912nb34nx385 a owl:Restriction ;
	owl:onProperty <http://ns.cerise-project.nl/energy/def/cim-smartgrid#UsagePoint.amiBillingReady> ;
	owl:allValuesFrom :AmiBillingReadyKind .

:UsagePoint rdfs:subClassOf _:node1912nb34nx386 .

_:node1912nb34nx386 a owl:Restriction ;
	owl:allValuesFrom xsd:boolean ;
	owl:onProperty <http://ns.cerise-project.nl/energy/def/cim-smartgrid#UsagePoint.isSdp> .

:UsagePoint rdfs:subClassOf _:node1912nb34nx387 .

_:node1912nb34nx387 a owl:Restriction ;
	owl:cardinality "1"^^xsd:int ;
	owl:onProperty <http://ns.cerise-project.nl/energy/def/cim-smartgrid#UsagePoint.UsagePointLocation> .

:UsagePoint rdfs:subClassOf _:node1912nb34nx388 .

_:node1912nb34nx388 a owl:Restriction ;
	owl:cardinality "1"^^xsd:int ;
	owl:onProperty <http://ns.cerise-project.nl/energy/def/cim-smartgrid#UsagePoint.isVirtual> .

:UsagePoint rdfs:subClassOf _:node1912nb34nx389 .

_:node1912nb34nx389 a owl:Restriction ;
	owl:cardinality "1"^^xsd:int ;
	owl:onProperty <http://ns.cerise-project.nl/energy/def/cim-smartgrid#UsagePoint.isSdp> .

:UsagePoint rdfs:subClassOf _:node1912nb34nx390 .

_:node1912nb34nx390 a owl:Restriction ;
	owl:allValuesFrom :MeterReading ;
	owl:onProperty <http://ns.cerise-project.nl/energy/def/cim-smartgrid#UsagePoint.MeterReadings> .

:ServiceSupplier rdfs:subClassOf _:node1912nb34nx391 .

_:node1912nb34nx391 a owl:Restriction ;
	owl:cardinality "1"^^xsd:int ;
	owl:onProperty <http://ns.cerise-project.nl/energy/def/cim-smartgrid#ServiceSupplier.issuerIdentificationNumber> .

:ServiceSupplier rdfs:subClassOf _:node1912nb34nx392 .

_:node1912nb34nx392 a owl:Restriction ;
	owl:allValuesFrom xsd:string ;
	owl:onProperty <http://ns.cerise-project.nl/energy/def/cim-smartgrid#ServiceSupplier.issuerIdentificationNumber> .

:ServiceSupplier rdfs:subClassOf _:node1912nb34nx393 .

_:node1912nb34nx393 a owl:Restriction ;
	owl:cardinality "1"^^xsd:int ;
	owl:onProperty <http://ns.cerise-project.nl/energy/def/cim-smartgrid#ServiceSupplier.kind> .

:ServiceSupplier rdfs:subClassOf _:node1912nb34nx394 .

_:node1912nb34nx394 a owl:Restriction ;
	owl:onProperty <http://ns.cerise-project.nl/energy/def/cim-smartgrid#ServiceSupplier.kind> ;
	owl:allValuesFrom :SupplierKind .

:Customer rdfs:subClassOf _:node1912nb34nx395 .

_:node1912nb34nx395 a owl:Restriction ;
	owl:cardinality "1"^^xsd:int ;
	owl:onProperty <http://ns.cerise-project.nl/energy/def/cim-smartgrid#Customer.kind> .

:Customer rdfs:subClassOf _:node1912nb34nx396 .

_:node1912nb34nx396 a owl:Restriction ;
	owl:allValuesFrom :CustomerKind ;
	owl:onProperty <http://ns.cerise-project.nl/energy/def/cim-smartgrid#Customer.kind> .

:TownDetail rdfs:subClassOf _:node1912nb34nx397 .

_:node1912nb34nx397 a owl:Restriction ;
	owl:allValuesFrom xsd:string ;
	owl:onProperty <http://ns.cerise-project.nl/energy/def/cim-smartgrid#TownDetail.section> .

:TownDetail rdfs:subClassOf _:node1912nb34nx398 .

_:node1912nb34nx398 a owl:Restriction ;
	owl:cardinality "1"^^xsd:int ;
	owl:onProperty <http://ns.cerise-project.nl/energy/def/cim-smartgrid#TownDetail.section> .

:TownDetail rdfs:subClassOf _:node1912nb34nx399 .

_:node1912nb34nx399 a owl:Restriction ;
	owl:cardinality "1"^^xsd:int ;
	owl:onProperty <http://ns.cerise-project.nl/energy/def/cim-smartgrid#TownDetail.stateOrProvince> .

:TownDetail rdfs:subClassOf _:node1912nb34nx400 .

_:node1912nb34nx400 a owl:Restriction ;
	owl:allValuesFrom xsd:string ;
	owl:onProperty <http://ns.cerise-project.nl/energy/def/cim-smartgrid#TownDetail.name> .

:TownDetail rdfs:subClassOf _:node1912nb34nx401 .

_:node1912nb34nx401 a owl:Restriction ;
	owl:allValuesFrom xsd:string ;
	owl:onProperty <http://ns.cerise-project.nl/energy/def/cim-smartgrid#TownDetail.country> .

:TownDetail rdfs:subClassOf _:node1912nb34nx402 .

_:node1912nb34nx402 a owl:Restriction ;
	owl:cardinality "1"^^xsd:int ;
	owl:onProperty <http://ns.cerise-project.nl/energy/def/cim-smartgrid#TownDetail.name> .

:TownDetail rdfs:subClassOf _:node1912nb34nx403 .

_:node1912nb34nx403 a owl:Restriction ;
	owl:cardinality "1"^^xsd:int ;
	owl:onProperty <http://ns.cerise-project.nl/energy/def/cim-smartgrid#TownDetail.code> .

:TownDetail rdfs:subClassOf _:node1912nb34nx404 .

_:node1912nb34nx404 a owl:Restriction ;
	owl:allValuesFrom xsd:string ;
	owl:onProperty <http://ns.cerise-project.nl/energy/def/cim-smartgrid#TownDetail.code> .

:TownDetail rdfs:subClassOf _:node1912nb34nx405 .

_:node1912nb34nx405 a owl:Restriction ;
	owl:allValuesFrom xsd:string ;
	owl:onProperty <http://ns.cerise-project.nl/energy/def/cim-smartgrid#TownDetail.stateOrProvince> .

:TownDetail rdfs:subClassOf _:node1912nb34nx406 .

_:node1912nb34nx406 a owl:Restriction ;
	owl:cardinality "1"^^xsd:int ;
	owl:onProperty <http://ns.cerise-project.nl/energy/def/cim-smartgrid#TownDetail.country> .

:TelephoneNumber rdfs:subClassOf _:node1912nb34nx407 .

_:node1912nb34nx407 a owl:Restriction ;
	owl:allValuesFrom xsd:string ;
	owl:onProperty <http://ns.cerise-project.nl/energy/def/cim-smartgrid#TelephoneNumber.localNumber> .

:TelephoneNumber rdfs:subClassOf _:node1912nb34nx408 .

_:node1912nb34nx408 a owl:Restriction ;
	owl:allValuesFrom xsd:string ;
	owl:onProperty <http://ns.cerise-project.nl/energy/def/cim-smartgrid#TelephoneNumber.extension> .

:TelephoneNumber rdfs:subClassOf _:node1912nb34nx409 .

_:node1912nb34nx409 a owl:Restriction ;
	owl:cardinality "1"^^xsd:int ;
	owl:onProperty <http://ns.cerise-project.nl/energy/def/cim-smartgrid#TelephoneNumber.countryCode> .

:TelephoneNumber rdfs:subClassOf _:node1912nb34nx410 .

_:node1912nb34nx410 a owl:Restriction ;
	owl:allValuesFrom xsd:string ;
	owl:onProperty <http://ns.cerise-project.nl/energy/def/cim-smartgrid#TelephoneNumber.countryCode> .

:TelephoneNumber rdfs:subClassOf _:node1912nb34nx411 .

_:node1912nb34nx411 a owl:Restriction ;
	owl:cardinality "1"^^xsd:int ;
	owl:onProperty <http://ns.cerise-project.nl/energy/def/cim-smartgrid#TelephoneNumber.areaCode> .

:TelephoneNumber rdfs:subClassOf _:node1912nb34nx412 .

_:node1912nb34nx412 a owl:Restriction ;
	owl:cardinality "1"^^xsd:int ;
	owl:onProperty <http://ns.cerise-project.nl/energy/def/cim-smartgrid#TelephoneNumber.cityCode> .

:TelephoneNumber rdfs:subClassOf _:node1912nb34nx413 .

_:node1912nb34nx413 a owl:Restriction ;
	owl:allValuesFrom xsd:string ;
	owl:onProperty <http://ns.cerise-project.nl/energy/def/cim-smartgrid#TelephoneNumber.areaCode> .

:TelephoneNumber rdfs:subClassOf _:node1912nb34nx414 .

_:node1912nb34nx414 a owl:Restriction ;
	owl:cardinality "1"^^xsd:int ;
	owl:onProperty <http://ns.cerise-project.nl/energy/def/cim-smartgrid#TelephoneNumber.extension> .

:TelephoneNumber rdfs:subClassOf _:node1912nb34nx415 .

_:node1912nb34nx415 a owl:Restriction ;
	owl:cardinality "1"^^xsd:int ;
	owl:onProperty <http://ns.cerise-project.nl/energy/def/cim-smartgrid#TelephoneNumber.localNumber> .

:TelephoneNumber rdfs:subClassOf _:node1912nb34nx416 .

_:node1912nb34nx416 a owl:Restriction ;
	owl:allValuesFrom xsd:string ;
	owl:onProperty <http://ns.cerise-project.nl/energy/def/cim-smartgrid#TelephoneNumber.cityCode> .

:DateTimeInterval rdfs:subClassOf _:node1912nb34nx417 .

_:node1912nb34nx417 a owl:Restriction ;
	owl:cardinality "1"^^xsd:int ;
	owl:onProperty <http://ns.cerise-project.nl/energy/def/cim-smartgrid#DateTimeInterval.start> .

:DateTimeInterval rdfs:subClassOf _:node1912nb34nx418 .

_:node1912nb34nx418 a owl:Restriction ;
	owl:allValuesFrom xsd:dateTime ;
	owl:onProperty <http://ns.cerise-project.nl/energy/def/cim-smartgrid#DateTimeInterval.start> .

:DateTimeInterval rdfs:subClassOf _:node1912nb34nx419 .

_:node1912nb34nx419 a owl:Restriction ;
	owl:cardinality "1"^^xsd:int ;
	owl:onProperty <http://ns.cerise-project.nl/energy/def/cim-smartgrid#DateTimeInterval.end> .

:DateTimeInterval rdfs:subClassOf _:node1912nb34nx420 .

_:node1912nb34nx420 a owl:Restriction ;
	owl:allValuesFrom xsd:dateTime ;
	owl:onProperty <http://ns.cerise-project.nl/energy/def/cim-smartgrid#DateTimeInterval.end> .
