@prefix dc: <http://purl.org/dc/elements/1.1/> .
@prefix nao: <http://www.semanticdesktop.org/ontologies/2007/08/15/nao#> .
@prefix nrl: <http://www.semanticdesktop.org/ontologies/2007/08/15/nrl#> .
@prefix owl: <http://www.w3.org/2002/07/owl#> .
@prefix rdf: <http://www.w3.org/1999/02/22-rdf-syntax-ns#> .
@prefix xml: <http://www.w3.org/XML/1998/namespace> .
@prefix xsd: <http://www.w3.org/2001/XMLSchema#> .
@prefix pimo: <http://www.semanticdesktop.org/ontologies/2007/11/01/pimo#> .
@prefix rdfs: <http://www.w3.org/2000/01/rdf-schema#> .
@prefix dcterms: <http://purl.org/dc/terms/> .
@base <http://www.w3.org/2002/07/owl#> .



#################################################################
#
#    Annotation properties
#
#################################################################


###  http://purl.org/dc/elements/1.1/contributor

dc:contributor rdf:type owl:AnnotationProperty .



###  http://purl.org/dc/elements/1.1/creator

dc:creator rdf:type owl:AnnotationProperty .



###  http://purl.org/dc/terms/modified

dcterms:modified rdf:type owl:AnnotationProperty .



###  http://www.semanticdesktop.org/ontologies/2007/08/15/nao#altLabel

nao:altLabel rdf:type owl:AnnotationProperty ;
             
             rdfs:label "alternative label" ;
             
             rdfs:comment "An alternative label alongside the preferred label for a resource" ;
             
             rdfs:range rdfs:Literal ;
             
             rdfs:subPropertyOf rdfs:label .



###  http://www.semanticdesktop.org/ontologies/2007/08/15/nao#annotation

nao:annotation rdf:type owl:AnnotationProperty ;
               
               rdfs:label "annotation" ;
               
               rdfs:comment "Generic annotation for a resource" ;
               
               rdfs:domain rdfs:Resource .



###  http://www.semanticdesktop.org/ontologies/2007/08/15/nao#contributor

nao:contributor rdf:type owl:AnnotationProperty ;
                
                rdfs:label "contributor" ;
                
                rdfs:comment "Refers to a single or a group of individuals that contributed to a resource" ;
                
                rdfs:subPropertyOf dc:contributor ,
                                   nao:annotation .



###  http://www.semanticdesktop.org/ontologies/2007/08/15/nao#creator

nao:creator rdf:type owl:AnnotationProperty ;
            
            rdfs:label "creator" ;
            
            nrl:maxCardinality "1"^^xsd:nonNegativeInteger ;
            
            rdfs:comment "Refers to the single or group of individuals that created the resource" ;
            
            rdfs:subPropertyOf dc:creator ,
                               nao:annotation .



###  http://www.semanticdesktop.org/ontologies/2007/08/15/nao#description

nao:description rdf:type owl:AnnotationProperty ;
                
                rdfs:label "description" ;
                
                rdfs:comment "A non-technical textual annotation for a resource" ;
                
                rdfs:subPropertyOf nao:annotation ;
                
                rdfs:range rdfs:Literal ;
                
                rdfs:subPropertyOf rdfs:comment .



###  http://www.semanticdesktop.org/ontologies/2007/08/15/nao#directTrust

nao:directTrust rdf:type owl:AnnotationProperty ;
                
                rdfs:label "direct trust" ;
                
                rdfs:comment "A direct trust value assigned to an agent, either manually by a user or semi-/automatically by a system. Allowed values range from 0 (no trust) to 1 (very high trust)." ;
                
                rdfs:subPropertyOf nao:trustLevel ;
                
                rdfs:domain pimo:Agent ;
                
                rdfs:range xsd:double .



###  http://www.semanticdesktop.org/ontologies/2007/08/15/nao#engineeringTool

nao:engineeringTool rdf:type owl:AnnotationProperty ;
                    
                    rdfs:label "engineering tool" ;
                    
                    rdfs:comment "Specifies the engineering tool used to generate the graph" ;
                    
                    rdfs:subPropertyOf nao:annotation ;
                    
                    rdfs:domain nrl:Data ;
                    
                    rdfs:range rdfs:Literal .



###  http://www.semanticdesktop.org/ontologies/2007/08/15/nao#externalIdentifier

nao:externalIdentifier rdf:type owl:AnnotationProperty ;
                       
                       rdfs:label "external identifier" ;
                       
                       rdfs:comment "An external identifier for a resource that has been retreived from an external source." ;
                       
                       rdfs:subPropertyOf nao:identifier .



###  http://www.semanticdesktop.org/ontologies/2007/08/15/nao#hasDefaultNamespace

nao:hasDefaultNamespace rdf:type owl:AnnotationProperty ;
                        
                        rdfs:label "has default namespace" ;
                        
                        nrl:maxCardinality "1"^^xsd:nonNegativeInteger ;
                        
                        rdfs:comment "Defines the default static namespace for a graph" ;
                        
                        rdfs:subPropertyOf nao:annotation ;
                        
                        rdfs:domain nrl:Data .



###  http://www.semanticdesktop.org/ontologies/2007/08/15/nao#hasDefaultNamespaceAbbreviation

nao:hasDefaultNamespaceAbbreviation rdf:type owl:AnnotationProperty ;
                                    
                                    rdfs:label "has default namespace abbreviation" ;
                                    
                                    nrl:maxCardinality "1"^^xsd:nonNegativeInteger ;
                                    
                                    rdfs:comment "Defines the default static namespace abbreviation for a graph" ;
                                    
                                    rdfs:subPropertyOf nao:annotation ;
                                    
                                    rdfs:domain nrl:Data .



###  http://www.semanticdesktop.org/ontologies/2007/08/15/nao#hasTag

nao:hasTag rdf:type owl:AnnotationProperty ;
           
           rdfs:label "has tag" ;
           
           rdfs:comment "Defines an existing tag for a resource" ;
           
           rdfs:subPropertyOf nao:annotation ;
           
           nrl:inverseProperty nao:isTagFor .



###  http://www.semanticdesktop.org/ontologies/2007/08/15/nao#iconName

nao:iconName rdf:type owl:AnnotationProperty ;
             
             rdfs:label "iconname" ;
             
             nrl:minCardinality "1"^^xsd:nonNegativeInteger ;
             
             rdfs:comment "Defines a name for a FreeDesktop Icon as defined in the FreeDesktop Icon Naming Standard" ;
             
             rdfs:subPropertyOf nao:identifier .



###  http://www.semanticdesktop.org/ontologies/2007/08/15/nao#identifier

nao:identifier rdf:type owl:AnnotationProperty ;
               
               rdfs:label "identifier" ;
               
               rdfs:comment "Defines a generic identifier for a resource" ;
               
               rdfs:domain rdfs:Resource .



###  http://www.semanticdesktop.org/ontologies/2007/08/15/nao#isRelated

nao:isRelated rdf:type owl:AnnotationProperty ;
              
              rdfs:label "is related to" ;
              
              rdfs:comment "Defines an annotation for a resource in the form of a relationship between the subject resource and another resource" ;
              
              rdfs:subPropertyOf nao:annotation .



###  http://www.semanticdesktop.org/ontologies/2007/08/15/nao#isTagFor

nao:isTagFor rdf:type owl:AnnotationProperty ;
             
             rdfs:label "is tag for" ;
             
             rdfs:comment "States which resources a tag is associated with" ;
             
             rdfs:subPropertyOf nao:annotation ;
             
             nrl:inverseProperty nao:hasTag .



###  http://www.semanticdesktop.org/ontologies/2007/08/15/nao#maintainedBy

nao:maintainedBy rdf:type owl:AnnotationProperty ;
                 
                 rdfs:label "maintained by" ;
                 
                 rdfs:comment "The agent that maintains this resource, ie. created it and knows what to do with it." ;
                 
                 rdfs:range nao:Agent ;
                 
                 rdfs:subPropertyOf nao:annotation ;
                 
                 rdfs:domain rdfs:Resource .



###  http://www.semanticdesktop.org/ontologies/2007/08/15/nao#modified

nao:modified rdf:type owl:AnnotationProperty ;
             
             rdfs:label "modified at" ;
             
             rdfs:comment "States the modification time for a resource" ;
             
             rdfs:subPropertyOf dcterms:modified ,
                                nao:annotation .



###  http://www.semanticdesktop.org/ontologies/2007/08/15/nao#networkTrust

nao:networkTrust rdf:type owl:AnnotationProperty ;
                 
                 rdfs:label "network trust" ;
                 
                 rdfs:comment "A network-derived trust value assigned to an agent, based on the shared direct trust values for the same agent, as set by participating agents in a network. Allowed values range from 0 (no trust) to 1 (very high trust)." ;
                 
                 rdfs:subPropertyOf nao:trustLevel ;
                 
                 rdfs:domain pimo:Agent ;
                 
                 rdfs:range xsd:double .



###  http://www.semanticdesktop.org/ontologies/2007/08/15/nao#numericRating

nao:numericRating rdf:type owl:AnnotationProperty ;
                  
                  rdfs:label "numeric rating" ;
                  
                  nrl:maxCardinality "1"^^xsd:nonNegativeInteger ;
                  
                  rdfs:comment " Annotation for a resource in the form of a numeric rating (float value), allowed values are between 1 and 10 whereas 0 is interpreted as not set" ;
                  
                  rdfs:subPropertyOf nao:rating .



###  http://www.semanticdesktop.org/ontologies/2007/08/15/nao#personalIdentifier

nao:personalIdentifier rdf:type owl:AnnotationProperty ;
                       
                       rdfs:label "personal identifier" ;
                       
                       rdfs:comment "Defines a personal string identifier for a resource" ;
                       
                       rdfs:subPropertyOf nao:identifier .



###  http://www.semanticdesktop.org/ontologies/2007/08/15/nao#pluralPrefLabel

nao:pluralPrefLabel rdf:type owl:AnnotationProperty ;
                    
                    rdfs:label "preferred label plural form" ;
                    
                    nrl:maxCardinality "1"^^xsd:nonNegativeInteger ;
                    
                    rdfs:comment "The plural form of the preferred label for a resource" ;
                    
                    rdfs:range rdfs:Literal ;
                    
                    rdfs:subPropertyOf rdfs:label .



###  http://www.semanticdesktop.org/ontologies/2007/08/15/nao#prefLabel

nao:prefLabel rdf:type owl:AnnotationProperty ;
              
              rdfs:label "preferred label" ;
              
              nrl:maxCardinality "1"^^xsd:nonNegativeInteger ;
              
              rdfs:comment "A preferred label for a resource" ;
              
              rdfs:range rdfs:Literal ;
              
              rdfs:subPropertyOf rdfs:label .



###  http://www.semanticdesktop.org/ontologies/2007/08/15/nao#privacyLevel

nao:privacyLevel rdf:type owl:AnnotationProperty ;
                 
                 rdfs:label "privacy level" ;
                 
                 rdfs:comment "A privacy level as defined for a resource. Allowed values range from 0 (private) to 1 (public)." ;
                 
                 rdfs:subPropertyOf nao:annotation ;
                 
                 rdfs:domain rdfs:Resource ;
                 
                 rdfs:range xsd:double .



###  http://www.semanticdesktop.org/ontologies/2007/08/15/nao#rating

nao:rating rdf:type owl:AnnotationProperty ;
           
           rdfs:label "rating" ;
           
           rdfs:comment "Annotation for a resource in the form of an unrestricted rating" ;
           
           rdfs:subPropertyOf nao:annotation ;
           
           rdfs:domain rdfs:Resource .



###  http://www.semanticdesktop.org/ontologies/2007/08/15/nao#score

nao:score rdf:type owl:AnnotationProperty ;
          
          rdfs:label "score" ;
          
          nrl:maxCardinality "1"^^xsd:nonNegativeInteger ;
          
          rdfs:comment "An authoritative score for an item valued between 0 and 1" ;
          
          rdfs:subPropertyOf nao:annotation .



###  http://www.semanticdesktop.org/ontologies/2007/08/15/nao#scoreParameter

nao:scoreParameter rdf:type owl:AnnotationProperty ;
                   
                   rdfs:label "scoreparameter" ;
                   
                   rdfs:comment "A marker property to mark selected properties which are input to a mathematical algorithm to generate scores for resources. Properties are marked by being defined as subproperties of this property" ;
                   
                   rdfs:subPropertyOf nao:annotation .



###  http://www.semanticdesktop.org/ontologies/2007/08/15/nao#serializationLanguage

nao:serializationLanguage rdf:type owl:AnnotationProperty ;
                          
                          rdfs:label "serialization language" ;
                          
                          nrl:maxCardinality "1"^^xsd:nonNegativeInteger ;
                          
                          rdfs:comment "States the serialization language for a named graph that is represented within a document" ;
                          
                          rdfs:domain nrl:DocumentGraph .



###  http://www.semanticdesktop.org/ontologies/2007/08/15/nao#status

nao:status rdf:type owl:AnnotationProperty ;
           
           rdfs:label "status" ;
           
           nrl:maxCardinality "1"^^xsd:nonNegativeInteger ;
           
           rdfs:comment "Specifies the status of a graph, stable, unstable or testing" ;
           
           rdfs:subPropertyOf nao:annotation ;
           
           rdfs:domain nrl:Data .



###  http://www.semanticdesktop.org/ontologies/2007/08/15/nao#trustLevel

nao:trustLevel rdf:type owl:AnnotationProperty ;
               
               rdfs:label "trust level" ;
               
               rdfs:comment "A generalised trust level assigned to an agent, based on a combination of direct and network trust values it possesses. Allowed values range from 0 (no trust) to 1 (very high trust)." ;
               
               rdfs:subPropertyOf nao:annotation ;
               
               rdfs:domain pimo:Agent ;
               
               rdfs:range xsd:double .



###  http://www.semanticdesktop.org/ontologies/2007/08/15/nao#version

nao:version rdf:type owl:AnnotationProperty ;
            
            rdfs:label "version" ;
            
            nrl:maxCardinality "1"^^xsd:nonNegativeInteger ;
            
            rdfs:comment "Specifies the version of a graph, in numeric format" ;
            
            rdfs:subPropertyOf nao:annotation ;
            
            rdfs:domain nrl:Data .



###  http://www.semanticdesktop.org/ontologies/2007/08/15/nrl#inverseProperty

nrl:inverseProperty rdf:type owl:AnnotationProperty .



###  http://www.semanticdesktop.org/ontologies/2007/08/15/nrl#maxCardinality

nrl:maxCardinality rdf:type owl:AnnotationProperty .



###  http://www.semanticdesktop.org/ontologies/2007/08/15/nrl#minCardinality

nrl:minCardinality rdf:type owl:AnnotationProperty .





#################################################################
#
#    Object Properties
#
#################################################################


###  http://www.semanticdesktop.org/ontologies/2007/08/15/nao#altSymbol

nao:altSymbol rdf:type owl:ObjectProperty ;
              
              rdfs:label "alternative symbol" ;
              
              rdfs:comment "An alternative symbol representation for a resource" ;
              
              rdfs:range nao:Symbol ;
              
              rdfs:subPropertyOf nao:hasSymbol ;
              
              rdfs:domain rdfs:Resource .



###  http://www.semanticdesktop.org/ontologies/2007/08/15/nao#contributor

nao:contributor rdf:type owl:ObjectProperty ;
                
                rdfs:label "contributor" ;
                
                rdfs:comment "Refers to a single or a group of individuals that contributed to a resource" ;
                
                rdfs:range nao:Party ;
                
                rdfs:domain rdfs:Resource .



###  http://www.semanticdesktop.org/ontologies/2007/08/15/nao#creator

nao:creator rdf:type owl:ObjectProperty ;
            
            rdfs:label "creator" ;
            
            nrl:maxCardinality "1"^^xsd:nonNegativeInteger ;
            
            rdfs:comment "Refers to the single or group of individuals that created the resource" ;
            
            rdfs:range nao:Party ;
            
            rdfs:domain rdfs:Resource .



###  http://www.semanticdesktop.org/ontologies/2007/08/15/nao#deprecated

nao:deprecated rdf:type owl:ObjectProperty ;
               
               rdfs:label "deprecated" ;
               
               nrl:maxCardinality "1"^^xsd:nonNegativeInteger ;
               
               rdfs:comment "If this property is assigned, the subject class, property, or resource, is deprecated and should not be used in production systems any longer. It may be removed without further notice." ;
               
               rdfs:domain rdfs:Resource ;
               
               rdfs:range rdfs:Resource .



###  http://www.semanticdesktop.org/ontologies/2007/08/15/nao#endorsedBy

nao:endorsedBy rdf:type owl:ObjectProperty ;
               
               rdfs:label "endorsed by" ;
               
               rdfs:comment "Signifies social endorsment of a resource by a specific agent. Endorsement includes social actions like favouriting, liking, voting for, starring a resource." ;
               
               rdfs:range nao:Party ;
               
               rdfs:domain rdfs:Resource .



###  http://www.semanticdesktop.org/ontologies/2007/08/15/nao#favouritedBy

nao:favouritedBy rdf:type owl:ObjectProperty ;
                 
                 rdfs:label "favourited by" ;
                 
                 rdfs:comment "Signifies social endorsment by an agent, by way of marking the resource as a favourite." ;
                 
                 rdfs:range nao:Party ;
                 
                 rdfs:subPropertyOf nao:endorsedBy ;
                 
                 rdfs:domain rdfs:Resource .



###  http://www.semanticdesktop.org/ontologies/2007/08/15/nao#hasDataGraph

nao:hasDataGraph rdf:type owl:ObjectProperty ;
                 
                 rdfs:label "has data graph" ;
                 
                 rdfs:comment "Links a resource to the graph which contains its metadata. Its typical usage would be to link the file resource to the graph containing its extracted file metadata. This allows for easy maintenance later on. Inverse property of nao:isDataGraphFor." ;
                 
                 nrl:inverseProperty nao:isDataGraphFor ;
                 
                 rdfs:range nrl:InstanceBase ;
                 
                 rdfs:domain rdfs:Resource .



###  http://www.semanticdesktop.org/ontologies/2007/08/15/nao#hasSubResource

nao:hasSubResource rdf:type owl:ObjectProperty ;
                   
                   rdfs:label "has Subresource" ;
                   
                   rdfs:comment "Defines a relationship between a resource and one or more sub resources. Descriptions of sub-resources are only interpretable when the super-resource exists. Deleting a super-resource should then also delete all sub-resources, and transferring a super-resource (for example, sending it to another user) must also include the sub-resource." ;
                   
                   nrl:inverseProperty nao:hasSuperResource ;
                   
                   rdfs:subPropertyOf nao:isRelated ;
                   
                   rdfs:range rdfs:Resource .



###  http://www.semanticdesktop.org/ontologies/2007/08/15/nao#hasSuperResource

nao:hasSuperResource rdf:type owl:ObjectProperty ;
                     
                     rdfs:label "has Superresource" ;
                     
                     rdfs:comment "Defines a relationship between a resource and one or more super resources" ;
                     
                     nrl:inverseProperty nao:hasSubResource ;
                     
                     rdfs:subPropertyOf nao:isRelated ;
                     
                     rdfs:range rdfs:Resource .



###  http://www.semanticdesktop.org/ontologies/2007/08/15/nao#hasSymbol

nao:hasSymbol rdf:type owl:ObjectProperty ;
              
              rdfs:label "has symbol" ;
              
              rdfs:comment "Annotation for a resource in the form of a visual representation. Typically the symbol is a double-typed image file or a nao:FreeDesktopIcon." ;
              
              rdfs:range nao:Symbol ;
              
              rdfs:domain rdfs:Resource .



###  http://www.semanticdesktop.org/ontologies/2007/08/15/nao#hasTag

nao:hasTag rdf:type owl:ObjectProperty ;
           
           rdfs:label "has tag" ;
           
           rdfs:comment "Defines an existing tag for a resource" ;
           
           rdfs:range nao:Tag ;
           
           nrl:inverseProperty nao:isTagFor ;
           
           rdfs:domain rdfs:Resource .



###  http://www.semanticdesktop.org/ontologies/2007/08/15/nao#hasTopic

nao:hasTopic rdf:type owl:ObjectProperty ;
             
             rdfs:label "has topic" ;
             
             rdfs:comment "Defines a relationship between two resources, where the object is a topic of the subject" ;
             
             rdfs:subPropertyOf nao:isRelated ;
             
             nrl:inverseProperty nao:isTopicOf ;
             
             rdfs:range rdfs:Resource .



###  http://www.semanticdesktop.org/ontologies/2007/08/15/nao#isDataGraphFor

nao:isDataGraphFor rdf:type owl:ObjectProperty ;
                   
                   rdfs:label "is data graph for" ;
                   
                   rdfs:comment "Links a named graph to the resource for which it contains metadata. Its typical usage would be to link the graph containing extracted file metadata to the file resource. This allows for easy maintenance later on. Inverse property of nao:hasDataGraph." ;
                   
                   nrl:inverseProperty nao:hasDataGraph ;
                   
                   rdfs:domain nrl:InstanceBase ;
                   
                   rdfs:range rdfs:Resource .



###  http://www.semanticdesktop.org/ontologies/2007/08/15/nao#isRelated

nao:isRelated rdf:type owl:ObjectProperty ;
              
              rdfs:label "is related to" ;
              
              rdfs:comment "Defines an annotation for a resource in the form of a relationship between the subject resource and another resource" ;
              
              rdfs:range rdfs:Resource .



###  http://www.semanticdesktop.org/ontologies/2007/08/15/nao#isTagFor

nao:isTagFor rdf:type owl:ObjectProperty ;
             
             rdfs:label "is tag for" ;
             
             rdfs:comment "States which resources a tag is associated with" ;
             
             rdfs:domain nao:Tag ;
             
             nrl:inverseProperty nao:hasTag ;
             
             rdfs:range rdfs:Resource .



###  http://www.semanticdesktop.org/ontologies/2007/08/15/nao#isTopicOf

nao:isTopicOf rdf:type owl:ObjectProperty ;
              
              rdfs:label "is topic of" ;
              
              rdfs:comment "Defines a relationship between two resources, where the subject is a topic of the object" ;
              
              nrl:inverseProperty nao:hasTopic ;
              
              rdfs:subPropertyOf nao:isRelated ;
              
              rdfs:range rdfs:Resource .



###  http://www.semanticdesktop.org/ontologies/2007/08/15/nao#prefSymbol

nao:prefSymbol rdf:type owl:ObjectProperty ;
               
               rdfs:label "preferred symbol" ;
               
               nrl:maxCardinality "1"^^xsd:nonNegativeInteger ;
               
               rdfs:comment "A unique preferred symbol representation for a resource" ;
               
               rdfs:range nao:Symbol ;
               
               rdfs:subPropertyOf nao:hasSymbol ;
               
               rdfs:domain rdfs:Resource .





#################################################################
#
#    Data properties
#
#################################################################


###  http://www.semanticdesktop.org/ontologies/2007/08/15/nao#created

nao:created rdf:type owl:DatatypeProperty ;
            
            rdfs:label "created at" ;
            
            nrl:maxCardinality "1"^^xsd:nonNegativeInteger ;
            
            rdfs:comment "States the creation, or first modification time for a resource" ;
            
            rdfs:subPropertyOf nao:modified ;
            
            rdfs:domain rdfs:Resource ;
            
            rdfs:range xsd:dateTime .



###  http://www.semanticdesktop.org/ontologies/2007/08/15/nao#externalIdentifier

nao:externalIdentifier rdf:type owl:DatatypeProperty ;
                       
                       rdfs:label "external identifier" ;
                       
                       rdfs:comment "An external identifier for a resource that has been retreived from an external source." ;
                       
                       rdfs:range rdfs:Literal ;
                       
                       rdfs:domain rdfs:Resource .



###  http://www.semanticdesktop.org/ontologies/2007/08/15/nao#hasDefaultNamespace

nao:hasDefaultNamespace rdf:type owl:DatatypeProperty ;
                        
                        rdfs:label "has default namespace" ;
                        
                        nrl:maxCardinality "1"^^xsd:nonNegativeInteger ;
                        
                        rdfs:comment "Defines the default static namespace for a graph" ;
                        
                        rdfs:range rdfs:Literal .



###  http://www.semanticdesktop.org/ontologies/2007/08/15/nao#hasDefaultNamespaceAbbreviation

nao:hasDefaultNamespaceAbbreviation rdf:type owl:DatatypeProperty ;
                                    
                                    rdfs:label "has default namespace abbreviation" ;
                                    
                                    nrl:maxCardinality "1"^^xsd:nonNegativeInteger ;
                                    
                                    rdfs:comment "Defines the default static namespace abbreviation for a graph" ;
                                    
                                    rdfs:range rdfs:Literal .



###  http://www.semanticdesktop.org/ontologies/2007/08/15/nao#iconName

nao:iconName rdf:type owl:DatatypeProperty ;
             
             rdfs:label "iconname" ;
             
             nrl:minCardinality "1"^^xsd:nonNegativeInteger ;
             
             rdfs:comment "Defines a name for a FreeDesktop Icon as defined in the FreeDesktop Icon Naming Standard" ;
             
             rdfs:domain nao:FreeDesktopIcon ;
             
             rdfs:range rdfs:Literal .



###  http://www.semanticdesktop.org/ontologies/2007/08/15/nao#lastModified

nao:lastModified rdf:type owl:DatatypeProperty ;
                 
                 rdfs:label "last modified at" ;
                 
                 nrl:maxCardinality "1"^^xsd:nonNegativeInteger ;
                 
                 rdfs:comment "States the last modification time for a resource" ;
                 
                 rdfs:subPropertyOf nao:modified ;
                 
                 rdfs:domain rdfs:Resource ;
                 
                 rdfs:range xsd:dateTime .



###  http://www.semanticdesktop.org/ontologies/2007/08/15/nao#modified

nao:modified rdf:type owl:DatatypeProperty ;
             
             rdfs:label "modified at" ;
             
             rdfs:comment "States the modification time for a resource" ;
             
             rdfs:domain rdfs:Resource ;
             
             rdfs:range xsd:dateTime .



###  http://www.semanticdesktop.org/ontologies/2007/08/15/nao#numericRating

nao:numericRating rdf:type owl:DatatypeProperty ;
                  
                  rdfs:label "numeric rating" ;
                  
                  nrl:maxCardinality "1"^^xsd:nonNegativeInteger ;
                  
                  rdfs:comment " Annotation for a resource in the form of a numeric rating (float value), allowed values are between 1 and 10 whereas 0 is interpreted as not set" ;
                  
                  rdfs:subPropertyOf nao:scoreParameter ;
                  
                  rdfs:domain rdfs:Resource ;
                  
                  rdfs:range xsd:integer .



###  http://www.semanticdesktop.org/ontologies/2007/08/15/nao#personalIdentifier

nao:personalIdentifier rdf:type owl:DatatypeProperty ;
                       
                       rdfs:label "personal identifier" ;
                       
                       rdfs:comment "Defines a personal string identifier for a resource" ;
                       
                       rdfs:range rdfs:Literal .



###  http://www.semanticdesktop.org/ontologies/2007/08/15/nao#score

nao:score rdf:type owl:DatatypeProperty ;
          
          rdfs:label "score" ;
          
          nrl:maxCardinality "1"^^xsd:nonNegativeInteger ;
          
          rdfs:comment "An authoritative score for an item valued between 0 and 1" ;
          
          rdfs:domain rdfs:Resource ;
          
          rdfs:range xsd:float .



###  http://www.semanticdesktop.org/ontologies/2007/08/15/nao#scoreParameter

nao:scoreParameter rdf:type owl:DatatypeProperty ;
                   
                   rdfs:label "scoreparameter" ;
                   
                   rdfs:comment "A marker property to mark selected properties which are input to a mathematical algorithm to generate scores for resources. Properties are marked by being defined as subproperties of this property" ;
                   
                   rdfs:domain rdfs:Resource ;
                   
                   rdfs:range xsd:float .



###  http://www.semanticdesktop.org/ontologies/2007/08/15/nao#serializationLanguage

nao:serializationLanguage rdf:type owl:DatatypeProperty ;
                          
                          rdfs:label "serialization language" ;
                          
                          nrl:maxCardinality "1"^^xsd:nonNegativeInteger ;
                          
                          rdfs:comment "States the serialization language for a named graph that is represented within a document" ;
                          
                          rdfs:range rdfs:Literal .



###  http://www.semanticdesktop.org/ontologies/2007/08/15/nao#status

nao:status rdf:type owl:DatatypeProperty ;
           
           rdfs:label "status" ;
           
           nrl:maxCardinality "1"^^xsd:nonNegativeInteger ;
           
           rdfs:comment "Specifies the status of a graph, stable, unstable or testing" ;
           
           rdfs:range rdfs:Literal .



###  http://www.semanticdesktop.org/ontologies/2007/08/15/nao#userVisible

nao:userVisible rdf:type owl:DatatypeProperty ;
                
                rdfs:label "user visible" ;
                
                nrl:maxCardinality 1 ;
                
                rdfs:comment "Mark a property, class, or even resource as user visible or not. Non-user-visible entities should never be presented to the user. By default everything is user-visible." ;
                
                rdfs:domain rdfs:Resource ;
                
                rdfs:range xsd:boolean .



###  http://www.semanticdesktop.org/ontologies/2007/08/15/nao#version

nao:version rdf:type owl:DatatypeProperty ;
            
            rdfs:label "version" ;
            
            nrl:maxCardinality "1"^^xsd:nonNegativeInteger ;
            
            rdfs:comment "Specifies the version of a graph, in numeric format" ;
            
            rdfs:range xsd:float .





#################################################################
#
#    Classes
#
#################################################################


###  http://www.semanticdesktop.org/ontologies/2007/08/15/nao#Agent

nao:Agent rdf:type owl:Class ;
          
          rdfs:label "agent" ;
          
          rdfs:subClassOf rdfs:Resource ;
          
          rdfs:comment "An agent is the artificial counterpart to nao:Party. It can be a software component or some service." .



###  http://www.semanticdesktop.org/ontologies/2007/08/15/nao#FreeDesktopIcon

nao:FreeDesktopIcon rdf:type owl:Class ;
                    
                    rdfs:label "freedesktopicon" ;
                    
                    rdfs:subClassOf nao:Symbol ;
                    
                    rdfs:comment "Represents a desktop icon as defined in the FreeDesktop Icon Naming Standard (http://standards.freedesktop.org/icon-naming-spec/icon-naming-spec-latest.html)." .



###  http://www.semanticdesktop.org/ontologies/2007/08/15/nao#Party

nao:Party rdf:type owl:Class ;
          
          rdfs:label "party" ;
          
          rdfs:subClassOf rdfs:Resource ;
          
          rdfs:comment "Represents a single or a group of individuals" .



###  http://www.semanticdesktop.org/ontologies/2007/08/15/nao#Symbol

nao:Symbol rdf:type owl:Class ;
           
           rdfs:label "symbol" ;
           
           rdfs:subClassOf rdfs:Resource ;
           
           rdfs:comment "Represents a symbol, a visual representation of a resource. Typically a local or remote file would be double-typed to be used as a symbol. An alternative is nao:FreeDesktopIcon." .



###  http://www.semanticdesktop.org/ontologies/2007/08/15/nao#Tag

nao:Tag rdf:type owl:Class ;
        
        rdfs:label "tag" ;
        
        rdfs:subClassOf rdfs:Resource ;
        
        rdfs:comment "Represents a generic tag" .



###  http://www.semanticdesktop.org/ontologies/2007/08/15/nrl#InstanceBase

nrl:InstanceBase rdf:type owl:Class .



###  http://www.semanticdesktop.org/ontologies/2007/08/15/nrl#InverseFunctionalProperty

nrl:InverseFunctionalProperty rdf:type owl:Class .



###  http://www.semanticdesktop.org/ontologies/2007/08/15/nrl#SymmetricProperty

nrl:SymmetricProperty rdf:type owl:Class .



###  http://www.w3.org/2000/01/rdf-schema#Resource

rdfs:Resource rdf:type owl:Class .





#################################################################
#
#    Individuals
#
#################################################################


###  http://www.semanticdesktop.org/ontologies/2007/08/15/nao#isRelated

nao:isRelated rdf:type nrl:SymmetricProperty ,
                       owl:NamedIndividual ;
              
              rdfs:label "is related to" ;
              
              rdfs:comment "Defines an annotation for a resource in the form of a relationship between the subject resource and another resource" .



###  http://www.semanticdesktop.org/ontologies/2007/08/15/nao#personalIdentifier

nao:personalIdentifier rdf:type nrl:InverseFunctionalProperty ,
                                owl:NamedIndividual ;
                       
                       rdfs:label "personal identifier" ;
                       
                       rdfs:comment "Defines a personal string identifier for a resource" .



###  http://www.semanticdesktop.org/ontologies/2007/08/15/nao#userVisible

nao:userVisible rdf:type owl:DatatypeProperty ,
                         owl:NamedIndividual ;
                
                rdfs:label "user visible" ;
                
                nrl:maxCardinality 1 ;
                
                nao:userVisible "false"^^xsd:boolean ;
                
                rdfs:comment "Mark a property, class, or even resource as user visible or not. Non-user-visible entities should never be presented to the user. By default everything is user-visible." .




###  Generated by the OWL API (version 3.5.0) http://owlapi.sourceforge.net

