@prefix foaf:  <http://xmlns.com/foaf/0.1/> .
@prefix qudt-unit: <http://data.qudt.org/qudt/owl/1.0.0/unit.owl#> .
@prefix ssn:   <http://www.w3.org/ns/ssn/> .
@prefix vann:  <http://purl.org/vocab/vann/> .
@prefix vs:    <http://www.w3.org/2003/06/sw-vocab-status/ns#> .
@prefix qudt:  <http://data.qudt.org/qudt/owl/1.0.0/qudt.owl#> .
@prefix dcterms: <http://purl.org/dc/terms/> .
@prefix voaf:  <http://purl.org/vocommons/voaf#> .
@prefix rdfs:  <http://www.w3.org/2000/01/rdf-schema#> .
@prefix seas:  <https://w3id.org/seas/> .
@prefix xsd:   <http://www.w3.org/2001/XMLSchema#> .
@prefix owl:   <http://www.w3.org/2002/07/owl#> .
@prefix rdf:   <http://www.w3.org/1999/02/22-rdf-syntax-ns#> .
@prefix saref: <http://ontology.tno.nl/saref#> .
@prefix sdmx:  <http://purl.org/linked-data/sdmx#> .
@prefix skos:  <http://www.w3.org/2004/02/skos/core#> .
@prefix cc:    <http://creativecommons.org/ns#> .

dcterms:description  a  owl:AnnotationProperty .

dcterms:creator  a  owl:AnnotationProperty .

voaf:Vocabulary  a  owl:Class .

dcterms:modified  a  owl:AnnotationProperty .

dcterms:contributor  a  owl:AnnotationProperty .

seas:MinimumOperatingEvaluation
        a                 owl:Class ;
        rdfs:comment      "The evaluated value is the minimum operating value of the property."@en ;
        rdfs:isDefinedBy  seas:OperatingOntology ;
        rdfs:label        "Minimum Operating Evaluation"@en ;
        rdfs:subClassOf   seas:Evaluation ;
        vs:term_status    "test" .

cc:license  a   owl:AnnotationProperty .

seas:MaximumPeakRatingEvaluation
        a                 owl:Class ;
        rdfs:comment      "The evaluated value is the maximum peak rating value of the property."@en ;
        rdfs:isDefinedBy  seas:OperatingOntology ;
        rdfs:label        "Maximum Peak Rating Evaluation"@en ;
        rdfs:subClassOf   seas:Evaluation ;
        vs:term_status    "test" .

dcterms:issued  a  owl:AnnotationProperty .

foaf:name  a    owl:DatatypeProperty .

vs:term_status  a  owl:AnnotationProperty .

foaf:Person  a  owl:Class .

dcterms:title  a  owl:AnnotationProperty .

seas:MaximumContinuousOperatingEvaluation
        a                 owl:Class ;
        rdfs:comment      "The evaluated value is the maximum continuous operating value of the property."@en ;
        rdfs:isDefinedBy  seas:OperatingOntology ;
        rdfs:label        "Maximum Continuous Operating Evaluation"@en ;
        rdfs:subClassOf   seas:Evaluation ;
        vs:term_status    "test" .

seas:OperatingOntology
        a                              voaf:Vocabulary , owl:Ontology ;
        cc:license                     <https://www.apache.org/licenses/LICENSE-2.0> ;
        dcterms:creator                <http://www.maxime-lefrancois.info/me#> ;
        dcterms:description            "The SEAS Operating Ontology defines evaluations of operating features of interest."@en ;
        dcterms:issued                 "2016-07-24"^^xsd:date ;
        dcterms:modified               "2016-07-24"^^xsd:date ;
        dcterms:title                  "The SEAS Failable System ontology"@en ;
        vann:preferredNamespacePrefix  "seas" ;
        vann:preferredNamespaceUri     seas: ;
        owl:imports                    seas:EvaluationOntology ;
        owl:versionIRI                 seas:OperatingOntology-1.0 ;
        owl:versionInfo                "v1.0" .

vann:preferredNamespaceUri
        a       owl:AnnotationProperty .

seas:NominalOperatingEvaluation
        a                 owl:Class ;
        rdfs:comment      "The evaluated value is the nominal operating value of the property."@en ;
        rdfs:isDefinedBy  seas:OperatingOntology ;
        rdfs:label        "Nominal"@en ;
        rdfs:subClassOf   seas:Evaluation ;
        vs:term_status    "test" .

vann:preferredNamespacePrefix
        a       owl:AnnotationProperty .
