@prefix : <http://www.w3.org/1999/xhtml> .
@prefix rdfs: <http://www.w3.org/2000/01/rdf-schema#> .
@prefix biol: <http://purl.org/NET/biol/ns#> .
@prefix sections: <http://buzzword.org.uk/rdf/sections#> .
@prefix foaf: <http://xmlns.com/foaf/0.1/> .
@prefix dcmitype: <http://purl.org/dc/dcmitype/> .
@prefix link: <http://www.w3.org/2006/link#> .
@prefix owl: <http://www.w3.org/2002/07/owl#> .
@prefix rdf: <http://www.w3.org/1999/02/22-rdf-syntax-ns#> .
@prefix xhv: <http://www.w3.org/1999/xhtml/vocab#> .
@prefix cc: <http://creativecommons.org/ns#> .
@prefix dcterms: <http://purl.org/dc/terms/> .

<http://purl.org/NET/biol/ns#> a owl:Ontology ;
	dcterms:title "Biological Taxonomy Vocabulary 0.2 (Core)"@en ;
	dcterms:modified "2008-10-06"@en ;
	dcterms:creator _:node17a83moltx1 .

_:node17a83moltx1 a foaf:Person ;
	foaf:name "Toby Inkster"@en ;
	foaf:page <http://tobyinkster.co.uk/> ;
	biol:hasTaxonomy _:node17a83moltx2 .

_:node17a83moltx2 dcterms:date "2008-05-08"@en ;
	biol:name "Homo sapiens"@en ;
	biol:seeAlso <http://species.wikimedia.org/wiki/Homo_sapiens> ;
	biol:species "Sapiens"@en ;
	biol:phylum "Chordata"@en ;
	biol:order "Primates"@en ;
	biol:class "Mammalia"@en ;
	biol:authority "Linnaeus, 1758"@en ;
	biol:family "Hominidae"@en ;
	biol:genus "Homo"@en ;
	biol:kingdom "Animalia"@en .

<http://purl.org/NET/biol/ns#> xhv:license <http://creativecommons.org/licenses/by-sa/2.0/uk/> .

<http://creativecommons.org/licenses/by-sa/2.0/uk/> a cc:License ;
	dcterms:title "Creative Commons Attribution-Share Alike 2.0 (UK: England & Wales) Licence" .

<http://purl.org/NET/biol/ns#> dcterms:bibliographicCitation <http://en.wikipedia.org/wiki/Taxonomic_rank> .

<http://en.wikipedia.org/wiki/Taxonomic_rank> dcterms:title "Taxonomic rank"@en ;
	dcterms:publisher "Wikipedia"@en .

<http://purl.org/NET/biol/ns#> dcterms:bibliographicCitation <http://microformats.org/wiki/species> .

<http://microformats.org/wiki/species> dcterms:title "species"@en ;
	dcterms:publisher "microformats.org"@en .

<http://purl.org/NET/biol/ns#> dcterms:conformsTo <http://www.w3.org/TR/rdfa-syntax> ;
	dcterms:license <http://creativecommons.org/licenses/by-sa/2.0/uk/> ;
	xhv:alternate <http://purl.org/NET/biol/ns-20081006.rdf> ;
	xhv:appendix <http://purl.org/NET/biol/ns.html#section_Acknowledgments> , <http://purl.org/NET/biol/ns.html#section_Changes> , <http://purl.org/NET/biol/ns.html#section_References> ;
	xhv:bookmark <http://purl.org/NET/biol/ns.html#example_basic> , <http://purl.org/NET/biol/ns.html#example_class> , <http://purl.org/NET/biol/ns.html#example_full> , <http://purl.org/NET/biol/ns.html#example_hierarchy> , <http://purl.org/NET/biol/ns.html#example_lifedoc> , <http://purl.org/NET/biol/ns.html#example_simple_rdfa> , <http://purl.org/NET/biol/ns.html#example_taxodoc> , <http://purl.org/NET/biol/ns.html#example_uri> , <http://purl.org/NET/biol/ns.html#section_Acknowledgments> , <http://purl.org/NET/biol/ns.html#section_Changes> , <http://purl.org/NET/biol/ns.html#section_Classes> , <http://purl.org/NET/biol/ns.html#section_Examples> , <http://purl.org/NET/biol/ns.html#section_Properties> , <http://purl.org/NET/biol/ns.html#section_References> , <http://purl.org/NET/biol/ns.html#section_References-I> , <http://purl.org/NET/biol/ns.html#term_BotTaxonomy> , <http://purl.org/NET/biol/ns.html#term_Taxonomy> , <http://purl.org/NET/biol/ns.html#term_ZooTaxonomy> , <http://purl.org/NET/biol/ns.html#term_authority> , <http://purl.org/NET/biol/ns.html#term_class> , <http://purl.org/NET/biol/ns.html#term_commonName> , <http://purl.org/NET/biol/ns.html#term_division> , <http://purl.org/NET/biol/ns.html#term_family> , <http://purl.org/NET/biol/ns.html#term_genus> , <http://purl.org/NET/biol/ns.html#term_hasTaxonomy> , <http://purl.org/NET/biol/ns.html#term_kingdom> , <http://purl.org/NET/biol/ns.html#term_morePrecise> , <http://purl.org/NET/biol/ns.html#term_name> , <http://purl.org/NET/biol/ns.html#term_order> , <http://purl.org/NET/biol/ns.html#term_phylum> , <http://purl.org/NET/biol/ns.html#term_rank> , <http://purl.org/NET/biol/ns.html#term_secondLevelClassification> , <http://purl.org/NET/biol/ns.html#term_seeAlso> , <http://purl.org/NET/biol/ns.html#term_species> , <http://purl.org/NET/biol/ns.html#toc> ;
	xhv:chapter <http://purl.org/NET/biol/ns.html#section_Classes> , <http://purl.org/NET/biol/ns.html#section_Examples> , <http://purl.org/NET/biol/ns.html#section_Properties> ;
	xhv:contents <http://purl.org/NET/biol/ns.html#toc> ;
	xhv:help <http://purl.org/NET/biol/ns.html#section_Examples> ;
	xhv:section <http://purl.org/NET/biol/ns.html#section_Acknowledgments> , <http://purl.org/NET/biol/ns.html#section_Changes> , <http://purl.org/NET/biol/ns.html#section_Classes> , <http://purl.org/NET/biol/ns.html#section_Examples> , <http://purl.org/NET/biol/ns.html#section_Properties> , <http://purl.org/NET/biol/ns.html#section_References> ;
	xhv:subsection <http://purl.org/NET/biol/ns.html#example_basic> , <http://purl.org/NET/biol/ns.html#example_class> , <http://purl.org/NET/biol/ns.html#example_full> , <http://purl.org/NET/biol/ns.html#example_hierarchy> , <http://purl.org/NET/biol/ns.html#example_lifedoc> , <http://purl.org/NET/biol/ns.html#example_simple_rdfa> , <http://purl.org/NET/biol/ns.html#example_taxodoc> , <http://purl.org/NET/biol/ns.html#example_uri> , <http://purl.org/NET/biol/ns.html#section_References-I> , <http://purl.org/NET/biol/ns.html#term_BotTaxonomy> , <http://purl.org/NET/biol/ns.html#term_Taxonomy> , <http://purl.org/NET/biol/ns.html#term_ZooTaxonomy> , <http://purl.org/NET/biol/ns.html#term_authority> , <http://purl.org/NET/biol/ns.html#term_class> , <http://purl.org/NET/biol/ns.html#term_commonName> , <http://purl.org/NET/biol/ns.html#term_division> , <http://purl.org/NET/biol/ns.html#term_family> , <http://purl.org/NET/biol/ns.html#term_genus> , <http://purl.org/NET/biol/ns.html#term_hasTaxonomy> , <http://purl.org/NET/biol/ns.html#term_kingdom> , <http://purl.org/NET/biol/ns.html#term_morePrecise> , <http://purl.org/NET/biol/ns.html#term_name> , <http://purl.org/NET/biol/ns.html#term_order> , <http://purl.org/NET/biol/ns.html#term_phylum> , <http://purl.org/NET/biol/ns.html#term_rank> , <http://purl.org/NET/biol/ns.html#term_secondLevelClassification> , <http://purl.org/NET/biol/ns.html#term_seeAlso> , <http://purl.org/NET/biol/ns.html#term_species> .

biol:BotTaxonomy a rdfs:Class ;
	rdfs:subClassOf biol:Taxonomy ;
	rdfs:isDefinedBy <http://purl.org/NET/biol/ns.html#term_BotTaxonomy> ;
	dcterms:description """A BotTaxonomy is a subclass of Taxonomy. It is not necessarily used to
describe a plant. Most of the time, it is more appropriate to use Taxonomy
instead."""@en ;
	xhv:bookmark <http://purl.org/NET/biol/ns.html#term_BotTaxonomy> ;
	rdfs:label "Botanical Taxonomy"@en .

biol:Taxonomy a rdfs:Class ;
	rdfs:subClassOf rdfs:Class ;
	rdfs:isDefinedBy <http://purl.org/NET/biol/ns.html#term_Taxonomy> ;
	dcterms:description "A taxonomy is a classification for something. An animal or plant <em xmlns=\"http://www.w3.org/1999/xhtml\">has</em> a taxonomy; an animal or plant <em xmlns=\"http://www.w3.org/1999/xhtml\">is not</em> a taxonomy. For those familiar with object-oriented programming, think of a taxonomy as being analogous to a class, not an object."^^rdf:XMLLiteral ;
	xhv:bookmark <http://purl.org/NET/biol/ns.html#term_Taxonomy> ;
	rdfs:label "Taxonomy"@en .

biol:ZooTaxonomy a rdfs:Class ;
	rdfs:subClassOf biol:Taxonomy ;
	rdfs:isDefinedBy <http://purl.org/NET/biol/ns.html#term_ZooTaxonomy> ;
	dcterms:description """A ZooTaxonomy is a subclass of Taxonomy. It is not necessarily used to
describe an animal, but it indicates that certain ambiguous terms, such as
\"division\" should be interpreted the way zoologists use them. Most of the
time, it is more appropriate to use Taxonomy instead."""@en ;
	xhv:bookmark <http://purl.org/NET/biol/ns.html#term_ZooTaxonomy> ;
	rdfs:label "Zoological Taxonomy"@en .

biol:authority a rdf:Property ;
	dcterms:description "The authority who classified this form of life. For example \"Linnaeus, 1758\"."@en ;
	xhv:bookmark <http://purl.org/NET/biol/ns.html#term_authority> ;
	rdfs:range rdfs:Literal ;
	rdfs:label "authority"@en ;
	rdfs:isDefinedBy <http://purl.org/NET/biol/ns.html#term_authority> ;
	rdfs:domain biol:Taxonomy .

biol:class a rdf:Property ;
	dcterms:description "The third highest level of classification. For example <i xmlns=\"http://www.w3.org/1999/xhtml\" class=\"taxon\">Mammalia</i>."^^rdf:XMLLiteral ;
	xhv:bookmark <http://purl.org/NET/biol/ns.html#term_class> ;
	rdfs:range rdfs:Literal ;
	rdfs:label "class"@en ;
	rdfs:isDefinedBy <http://purl.org/NET/biol/ns.html#term_class> ;
	rdfs:domain biol:Taxonomy ;
	rdfs:subPropertyOf biol:rank .

biol:commonName a rdf:Property ;
	dcterms:description "A non-scientific name. For example, \"Human\"."@en ;
	xhv:bookmark <http://purl.org/NET/biol/ns.html#term_commonName> ;
	rdfs:range rdfs:Literal ;
	rdfs:label "common name"@en ;
	rdfs:isDefinedBy <http://purl.org/NET/biol/ns.html#term_commonName> ;
	rdfs:domain biol:Taxonomy ;
	rdfs:subPropertyOf rdfs:label .

biol:division a rdf:Property ;
	dcterms:description """The second highest level of classification, as used by botanists. Note that
division may be used to describe any form of life — the use of division is
not meant to imply that the entity being described is a plant, merely that
botanical names of ranks are being used. Zoologists use the term \"division\"
to describe a rank between an \"infraclass\" and a \"cohort\". biol:division
should not be used for this purpose — use biol:rank instead."""@en ;
	xhv:bookmark <http://purl.org/NET/biol/ns.html#term_division> ;
	rdfs:range rdfs:Literal ;
	rdfs:label "division"@en ;
	rdfs:isDefinedBy <http://purl.org/NET/biol/ns.html#term_division> ;
	rdfs:domain biol:Taxonomy ;
	rdfs:subPropertyOf biol:secondLevelClassification .

biol:family a rdf:Property ;
	dcterms:description "The fifth highest level of classification. For example <i xmlns=\"http://www.w3.org/1999/xhtml\" class=\"taxon\">Hominidae</i>."^^rdf:XMLLiteral ;
	xhv:bookmark <http://purl.org/NET/biol/ns.html#term_family> ;
	rdfs:range rdfs:Literal ;
	rdfs:label "family"@en ;
	rdfs:isDefinedBy <http://purl.org/NET/biol/ns.html#term_family> ;
	rdfs:domain biol:Taxonomy ;
	rdfs:subPropertyOf biol:rank .

biol:genus a rdf:Property ;
	dcterms:description "The sixth highest level of classification. For example <i xmlns=\"http://www.w3.org/1999/xhtml\" class=\"taxon\">Homo</i>."^^rdf:XMLLiteral ;
	xhv:bookmark <http://purl.org/NET/biol/ns.html#term_genus> ;
	rdfs:range rdfs:Literal ;
	rdfs:label "genus"@en ;
	rdfs:isDefinedBy <http://purl.org/NET/biol/ns.html#term_genus> ;
	rdfs:domain biol:Taxonomy ;
	rdfs:subPropertyOf biol:rank .

biol:hasTaxonomy a rdf:Property ;
	rdfs:isDefinedBy <http://purl.org/NET/biol/ns.html#term_hasTaxonomy> ;
	dcterms:description "This property provides a relationship between an entity (such as a <a xmlns=\"http://www.w3.org/1999/xhtml\" href=\"http://xmlns.com/foaf/spec/#term_Person\">foaf:Person</a>) and a taxonomy. Because biologists don't always agree on how to classify life, a single entity may have multiple taxonomies, each of which may be differentiated between using <a xmlns=\"http://www.w3.org/1999/xhtml\" href=\"#term_authority\">biol:authority</a> or dc:date."^^rdf:XMLLiteral ;
	rdfs:subPropertyOf rdf:type ;
	xhv:bookmark <http://purl.org/NET/biol/ns.html#term_hasTaxonomy> ;
	rdfs:range biol:Taxonomy ;
	rdfs:label "taxonomy"@en .

biol:kingdom a rdf:Property ;
	dcterms:description "The highest-level and least specific level of classification. Example kingdoms are <i xmlns=\"http://www.w3.org/1999/xhtml\" class=\"taxon\">Animalia</i> and <i xmlns=\"http://www.w3.org/1999/xhtml\" class=\"taxon\">Plantae</i>."^^rdf:XMLLiteral ;
	xhv:bookmark <http://purl.org/NET/biol/ns.html#term_kingdom> ;
	rdfs:range rdfs:Literal ;
	rdfs:label "kingdom"@en ;
	rdfs:isDefinedBy <http://purl.org/NET/biol/ns.html#term_kingdom> ;
	rdfs:domain biol:Taxonomy ;
	rdfs:subPropertyOf biol:rank .

biol:morePrecise a rdf:Property ;
	dcterms:description """Connects a taxonomy to a more precise taxonomy. For example, the taxonomy
\"Mammal\" might have a \"more precise\" property linking to \"Primate\"."""@en ;
	xhv:bookmark <http://purl.org/NET/biol/ns.html#term_morePrecise> ;
	rdfs:range biol:Taxonomy ;
	rdfs:label "more precise"@en ;
	rdfs:isDefinedBy <http://purl.org/NET/biol/ns.html#term_morePrecise> ;
	rdfs:domain biol:Taxonomy ;
	rdfs:subPropertyOf _:node17a83moltx3 .

_:node17a83moltx3 owl:inverseOf rdfs:subClassOf .

biol:name a rdf:Property ;
	dcterms:description "A scientific name; a binomial or trinomial. For example, <i xmlns=\"http://www.w3.org/1999/xhtml\" class=\"taxon\">Homo sapiens</i>."^^rdf:XMLLiteral ;
	xhv:bookmark <http://purl.org/NET/biol/ns.html#term_name> ;
	rdfs:range rdfs:Literal ;
	rdfs:label "name"@en ;
	rdfs:isDefinedBy <http://purl.org/NET/biol/ns.html#term_name> ;
	rdfs:domain biol:Taxonomy .

biol:order a rdf:Property ;
	dcterms:description "The fourth highest level of classification. For example \"Primates\"."@en ;
	xhv:bookmark <http://purl.org/NET/biol/ns.html#term_order> ;
	rdfs:range rdfs:Literal ;
	rdfs:label "order"@en ;
	rdfs:isDefinedBy <http://purl.org/NET/biol/ns.html#term_order> ;
	rdfs:domain biol:Taxonomy ;
	rdfs:subPropertyOf biol:rank .

biol:phylum a rdf:Property ;
	dcterms:description """The second highest level of classification, as used by zoologists. Note that
phylum may be used to describe any form of life — the use of phylum is not
meant to imply that the entity being described is an animal, merely that
zoological names of ranks are being used."""@en ;
	xhv:bookmark <http://purl.org/NET/biol/ns.html#term_phylum> ;
	rdfs:range rdfs:Literal ;
	rdfs:label "phylum"@en ;
	rdfs:isDefinedBy <http://purl.org/NET/biol/ns.html#term_phylum> ;
	rdfs:domain biol:Taxonomy ;
	rdfs:subPropertyOf biol:secondLevelClassification .

biol:rank a rdf:Property ;
	dcterms:description "An unspecified classification. This should not normally be used."@en ;
	xhv:bookmark <http://purl.org/NET/biol/ns.html#term_rank> ;
	rdfs:range rdfs:Literal ;
	rdfs:label "rank"@en ;
	rdfs:isDefinedBy <http://purl.org/NET/biol/ns.html#term_rank> ;
	rdfs:domain biol:Taxonomy ;
	rdfs:subPropertyOf <urn:lsid:ubio.org:predicates:taxonomicGroup> .

biol:secondLevelClassification a rdf:Property ;
	dcterms:description "The second highest level of classification. Zoologists call these <i xmlns=\"http://www.w3.org/1999/xhtml\">phyla</i> and botanists call them \"divisions\". In general, you should pick one of those terms and use it instead."^^rdf:XMLLiteral ;
	xhv:bookmark <http://purl.org/NET/biol/ns.html#term_secondLevelClassification> ;
	rdfs:range rdfs:Literal ;
	rdfs:label "second level classification"@en ;
	rdfs:isDefinedBy <http://purl.org/NET/biol/ns.html#term_secondLevelClassification> ;
	rdfs:domain biol:Taxonomy ;
	rdfs:subPropertyOf biol:rank .

biol:seeAlso a rdf:Property ;
	dcterms:description "A link to another resource further describing this form of life."@en ;
	xhv:bookmark <http://purl.org/NET/biol/ns.html#term_seeAlso> ;
	rdfs:range rdfs:Resource ;
	rdfs:label "see also"@en ;
	rdfs:isDefinedBy <http://purl.org/NET/biol/ns.html#term_seeAlso> ;
	rdfs:domain biol:Taxonomy ;
	rdfs:subPropertyOf rdfs:seeAlso .

biol:species a rdf:Property ;
	dcterms:description "The lowest level of classification supported by this vocabulary. For example <i xmlns=\"http://www.w3.org/1999/xhtml\" class=\"taxon\">Sapiens</i>. To include information more specific than species, use <a xmlns=\"http://www.w3.org/1999/xhtml\" href=\"#term_rank\">biol:rank</a> or <a xmlns=\"http://www.w3.org/1999/xhtml\" href=\"#section_Abstract\">a more specialist vocabulary</a>."^^rdf:XMLLiteral ;
	xhv:bookmark <http://purl.org/NET/biol/ns.html#term_species> ;
	rdfs:range rdfs:Literal ;
	rdfs:label "species"@en ;
	rdfs:isDefinedBy <http://purl.org/NET/biol/ns.html#term_species> ;
	rdfs:domain biol:Taxonomy ;
	rdfs:subPropertyOf biol:rank .

rdf:type rdfs:isDefinedBy <http://www.w3.org/TR/rdf-schema/#ch_type> .

rdfs:Class rdfs:isDefinedBy <http://www.w3.org/TR/rdf-schema/#ch_class> .

rdfs:Literal rdfs:isDefinedBy <http://www.w3.org/TR/rdf-schema/#ch_literal> .

rdfs:Resource rdfs:isDefinedBy <http://www.w3.org/TR/rdf-schema/#ch_resource> .

rdfs:label rdfs:isDefinedBy <http://www.w3.org/TR/rdf-schema/#ch_label> .

rdfs:seeAlso rdfs:isDefinedBy <http://www.w3.org/TR/rdf-schema/#ch_seealso> .

rdfs:subClassOf rdfs:isDefinedBy <http://www.w3.org/TR/rdf-schema/#ch_subclassof> .

<http://purl.org/NET/biol/ns#> dcterms:creator _:node17a83moltx4 .

_:node17a83moltx4 a foaf:Person ;
	foaf:name "Toby Inkster"@en ;
	foaf:page <http://tobyinkster.co.uk/> ;
	biol:hasTaxonomy _:node17a83moltx5 .

_:node17a83moltx5 dcterms:date "2008-05-08"@en ;
	biol:name "Homo sapiens"@en ;
	biol:seeAlso <http://species.wikimedia.org/wiki/Homo_sapiens> ;
	biol:species "Sapiens"@en ;
	biol:phylum "Chordata"@en ;
	biol:order "Primates"@en ;
	biol:class "Mammalia"@en ;
	biol:authority "Linnaeus, 1758"@en ;
	biol:family "Hominidae"@en ;
	biol:genus "Homo"@en ;
	biol:kingdom "Animalia"@en .

biol:morePrecise rdfs:subPropertyOf _:node17a83moltx6 .

_:node17a83moltx6 owl:inverseOf rdfs:subClassOf .
