@prefix dc: <http://purl.org/dc/elements/1.1/> .
@prefix : <http://www.w3.org/2001/03/earl/0.95#> .
@prefix rdfs: <http://www.w3.org/2000/01/rdf-schema#> .
@prefix doc: <http://www.w3.org/2000/10/swap/pim/doc#> .
@prefix earldata: <http://www.w3.org/2001/03/earl/0.95datatypes#> .
@prefix rdf: <http://www.w3.org/1999/02/22-rdf-syntax-ns#> .
@prefix earl9: <http://www.w3.org/2001/03/earl/0.9#> .
@prefix daml: <http://www.daml.org/2001/03/daml+oil#> .
@prefix rcs: <http://www.w3.org/2001/03swell/rcs#> .

<http://www.w3.org/1999/02/22-rdf-syntax-ns> dc:title "EARL (Evaluation And Report Language) 0.95 RDF Schema" ;
	rdfs:seeAlso <http://www.w3.org/2001/03/earl/0.95.n3> , <http://www.w3.org/2001/03/earl/0.95inferences> ;
	doc:derivedFrom <http://www.w3.org/2001/03/earl/0.9> ;
	doc:obsoletes <http://www.w3.org/2001/03/earl/0.9> ;
	rcs:id "$Id$" .

:Assertion daml:intersectionOf _:node174ns8legx1 .

_:node174ns8legx1 daml:first _:node174ns8legx2 .

_:node174ns8legx2 daml:onProperty rdf:subject ;
	daml:toClass :TestSubject .

_:node174ns8legx1 daml:rest _:node174ns8legx3 .

_:node174ns8legx3 daml:first _:node174ns8legx4 .

_:node174ns8legx4 daml:onProperty rdf:predicate ;
	daml:toClass :ResultProperty .

_:node174ns8legx3 daml:rest _:node174ns8legx5 .

_:node174ns8legx5 daml:first _:node174ns8legx6 .

_:node174ns8legx6 daml:onProperty rdf:object ;
	daml:toClass :TestCase .

_:node174ns8legx5 daml:rest daml:nil .

:Assertion rdfs:comment """These could be free standing units - used outside of 
                   earl:Evaluation(s) if required""" ;
	rdfs:subClassOf rdf:Statement .

:Assertor rdfs:comment """The entity making the assertion (e.g. running the test). This 
                   could be anonymous if for example you want to declare other 
                   context information.""" ;
	rdfs:subClassOf _:node174ns8legx7 .

_:node174ns8legx7 daml:onProperty :platform ;
	daml:toClass :TestPlatform .

:Assertor rdfs:subClassOf _:node174ns8legx8 .

_:node174ns8legx8 daml:onProperty :asserts ;
	daml:toClass :Assertion .

:Auto a :TestMode .

:CannotTell a :ValidityState .

:Date daml:disjointUnionOf _:node174ns8legx9 .

_:node174ns8legx9 daml:first :DateRange ;
	daml:rest _:node174ns8legx10 .

_:node174ns8legx10 daml:first earldata:Date ;
	daml:rest daml:nil .

:DateRange daml:intersectionOf _:node174ns8legx11 .

_:node174ns8legx11 daml:first _:node174ns8legx12 .

_:node174ns8legx12 daml:onProperty :fromDate ;
	daml:hasClass earldata:Date .

_:node174ns8legx11 daml:rest _:node174ns8legx13 .

_:node174ns8legx13 daml:first _:node174ns8legx14 .

_:node174ns8legx14 daml:onProperty :toDate ;
	daml:hasClass earldata:Date .

_:node174ns8legx13 daml:rest daml:nil .

:EARL rdfs:label "EARL (Evaluation And Report Language)" ;
	:version "0.95" .

:Evaluation daml:intersectionOf _:node174ns8legx15 .

_:node174ns8legx15 daml:first _:node174ns8legx16 .

_:node174ns8legx16 daml:onProperty rdf:subject ;
	daml:toClass :Assertor .

_:node174ns8legx15 daml:rest _:node174ns8legx17 .

_:node174ns8legx17 daml:first _:node174ns8legx18 .

_:node174ns8legx18 daml:onProperty rdf:predicate ;
	daml:hasValue :asserts .

_:node174ns8legx17 daml:rest _:node174ns8legx19 .

_:node174ns8legx19 daml:first _:node174ns8legx20 .

_:node174ns8legx20 daml:onProperty rdf:object ;
	daml:toClass :Assertion .

_:node174ns8legx19 daml:rest daml:nil .

:Evaluation rdfs:comment "An Evaluation is the most basic unit of EARL as it stands" ;
	rdfs:subClassOf rdf:Statement .

:Fail a :ValidityState .

:Heuristic a :TestMode .

:High a :ConfidenceLevel .

:Low a :ConfidenceLevel .

:Manual a :TestMode .

:Medium a :ConfidenceLevel .

:NotApplicable a :ValidityState .

:NotTested a :ValidityState .

:Operator rdfs:seeAlso :Person .

:Pass a :ValidityState .

:Person a rdfs:Class ;
	rdfs:subClassOf :Assertor .

:Platform rdfs:comment "The general platform on which something runs" .

:RepairInfo rdfs:subClassOf _:node174ns8legx21 .

_:node174ns8legx21 daml:onProperty :expectedResult ;
	daml:toClass :ExpectedResult .

:ResultProperty rdfs:subClassOf _:node174ns8legx22 .

_:node174ns8legx22 daml:onProperty :note ;
	daml:toClass rdfs:Resource .

:ResultProperty rdfs:subClassOf rdf:Property .

:Suite daml:disjointWith :Id .

:TestCase a rdfs:Class .

:TestCriteria daml:unionOf _:node174ns8legx23 .

_:node174ns8legx23 daml:first _:node174ns8legx24 .

_:node174ns8legx24 daml:onProperty :level ;
	daml:minCardinality "1" .

_:node174ns8legx23 daml:rest _:node174ns8legx25 .

_:node174ns8legx25 daml:first _:node174ns8legx26 .

_:node174ns8legx26 daml:onProperty :excludes ;
	daml:minCardinality "1" .

_:node174ns8legx25 daml:rest daml:nil .

:TestPlatform rdfs:comment "The platform on which the test(s) were run" .

:TestSubject a rdfs:Class ;
	rdfs:subClassOf _:node174ns8legx27 .

_:node174ns8legx27 daml:onProperty :date ;
	daml:minCardinality "1" .

:TestSubject rdfs:subClassOf _:node174ns8legx28 .

_:node174ns8legx28 daml:onProperty :platform ;
	daml:toClass :Platform .

:Tool daml:disjointWith :UserAgent ;
	rdfs:subClassOf :TestSubject .

:UserAgent rdfs:subClassOf :TestSubject .

:WebContent daml:disjointWith :Tool , :UserAgent ;
	rdfs:subClassOf :TestSubject .

:asserts rdfs:comment """For earl:asserts(x,y), in general, the assertor (x) 
                             asserts the assertion (y). EARL has specific 
                             classes for these""" .

:ccppSetting rdfs:subPropertyOf :platform .

:confidence rdfs:domain :ResultProperty ;
	rdfs:range :ConfidenceLevel .

:contactInfo a rdf:Property ;
	rdfs:domain :Assertor ;
	rdfs:range :ContactInfo .

:date a daml:DatatypeProperty ;
	rdfs:range :Date .

:email a rdf:Property ;
	rdfs:comment """Generally, for earl:email(x, y) x has an email address of y. This is not 
        a daml:UnambiguousProperty - use foaf:mbox for that purpose""" ;
	rdfs:range :Email ;
	rdfs:subPropertyOf :contactInfo .

:excludes rdfs:domain :TestCriteria ;
	rdfs:range :Exclusion .

:fails a :ResultProperty ;
	:confidence :High ;
	:validity :Fail .

:fromDate a daml:UniqueProperty .

:id rdfs:comment "A single guideline, checkpoint, etc." ;
	rdfs:domain _:node174ns8legx29 .

_:node174ns8legx29 daml:disjointUnionOf _:node174ns8legx30 .

_:node174ns8legx30 daml:first :TestCase ;
	daml:rest _:node174ns8legx31 .

_:node174ns8legx31 daml:first :TestCriteria ;
	daml:rest _:node174ns8legx32 .

_:node174ns8legx32 daml:first :Exclusion ;
	daml:rest daml:nil .

:id rdfs:range :Id .

:lastModified rdfs:domain :TestSubject ;
	rdfs:range :Date ;
	rdfs:subPropertyOf :date .

:level rdfs:comment """This is a generic level of test criteria, for example, 
                   the priorities/levels in WCAG. These shouldn't be a 
                   string literal""" ;
	rdfs:domain _:node174ns8legx33 .

_:node174ns8legx33 daml:disjointUnionOf _:node174ns8legx34 .

_:node174ns8legx34 daml:first :TestCriteria ;
	daml:rest _:node174ns8legx35 .

_:node174ns8legx35 daml:first :Exclusion ;
	daml:rest daml:nil .

:name a rdf:Property ;
	rdfs:comment "The common proper name for some earl:Assertor" ;
	rdfs:domain :Assertor ;
	rdfs:range rdfs:Literal .

:operator rdfs:range :Operator .

:operatorInstructions rdfs:domain :TestCase ;
	rdfs:range rdfs:Literal .

:os rdfs:label "Operating System" ;
	rdfs:subPropertyOf :platform .

:passes a :ResultProperty ;
	:confidence :High ;
	:validity :Pass .

:platform a rdf:Property ;
	rdfs:comment """e.g. the platform on which the test(s) were run, or the 
                   general platform on which something runs""" .

:purpose rdfs:domain :TestCase ;
	rdfs:range rdfs:Literal .

:released rdfs:domain :TestSubject ;
	rdfs:range :Date ;
	rdfs:subPropertyOf :date .

:repairInfo rdfs:range :RepairInfo .

:reproducableStep rdfs:domain :TestCase ;
	rdfs:range rdfs:Literal .

:sameSubjectAs daml:inverseOf :sameSubjectAs ;
	rdf:range :TestSubject ;
	rdfs:comment """For earl:sameSubjectAs(x, y), x is defined as being the same 
                   subject being evaluated (in an assertion) as y. In other 
                   words, there is some property of sameness between the two - 
                   the exact semantics of which are not defined here, but may 
                   be useful to individual processors.""" ;
	rdfs:domain :TestSubject ;
	rdfs:seeAlso daml:equivalentTo .

:snapshot rdfs:domain :TestSubject .

:suite rdfs:comment """A suite of checkpoints, guidelines, or any other form of 
                   rules that an earl:TestSubject can be evaluated against. 
                   e.g. WCAG 1.0""" ;
	rdfs:domain _:node174ns8legx36 .

_:node174ns8legx36 daml:disjointUnionOf _:node174ns8legx37 .

_:node174ns8legx37 daml:first :TestCase ;
	daml:rest _:node174ns8legx38 .

_:node174ns8legx38 daml:first :TestCriteria ;
	daml:rest _:node174ns8legx39 .

_:node174ns8legx39 daml:first :Exclusion ;
	daml:rest daml:nil .

:suite rdfs:range :Suite .

:testCriteria rdfs:domain :TestCase ;
	rdfs:range :TestCriteria .

:testId rdfs:comment """Points to a particular example of a technology against which 
                   one checked the particular subject (which in EARL would be 
                   an earl:TestSubject)""" ;
	rdfs:range :TestId .

:testMode a rdf:Property ;
	rdfs:domain :TestCase ;
	rdfs:range :TestMode .

:testSubject a daml:UniqueProperty ;
	rdfs:domain :TestSubject ;
	rdfs:range rdfs:Resource .

:testSuite rdfs:comment """Points to a suite of technologies against which one checked 
                   the particular subject (which in EARL would be an 
                   earl:TestSubject), e.g., the W3C's SVG Test Suite""" ;
	rdfs:range :TestSuite .

:toDate a daml:UniqueProperty .

:validity rdfs:domain :ResultProperty ;
	rdfs:range :ValidityState .

:version a rdf:Property ;
	rdfs:comment "For earl:version(x, y), read: x is of version y" .

:Assertion daml:intersectionOf _:node174ns8legx40 .

_:node174ns8legx40 daml:first _:node174ns8legx41 .

_:node174ns8legx41 daml:onProperty rdf:subject ;
	daml:toClass :TestSubject .

_:node174ns8legx40 daml:rest _:node174ns8legx42 .

_:node174ns8legx42 daml:first _:node174ns8legx43 .

_:node174ns8legx43 daml:onProperty rdf:predicate ;
	daml:toClass :ResultProperty .

_:node174ns8legx42 daml:rest _:node174ns8legx44 .

_:node174ns8legx44 daml:first _:node174ns8legx45 .

_:node174ns8legx45 daml:onProperty rdf:object ;
	daml:toClass :TestCase .

_:node174ns8legx44 daml:rest daml:nil .

:Assertor rdfs:subClassOf _:node174ns8legx46 .

_:node174ns8legx46 daml:onProperty :platform ;
	daml:toClass :TestPlatform .

:Assertor rdfs:subClassOf _:node174ns8legx47 .

_:node174ns8legx47 daml:onProperty :asserts ;
	daml:toClass :Assertion .

:Date daml:disjointUnionOf _:node174ns8legx48 .

_:node174ns8legx48 daml:first :DateRange ;
	daml:rest _:node174ns8legx49 .

_:node174ns8legx49 daml:first earldata:Date ;
	daml:rest daml:nil .

:DateRange daml:intersectionOf _:node174ns8legx50 .

_:node174ns8legx50 daml:first _:node174ns8legx51 .

_:node174ns8legx51 daml:onProperty :fromDate ;
	daml:hasClass earldata:Date .

_:node174ns8legx50 daml:rest _:node174ns8legx52 .

_:node174ns8legx52 daml:first _:node174ns8legx53 .

_:node174ns8legx53 daml:onProperty :toDate ;
	daml:hasClass earldata:Date .

_:node174ns8legx52 daml:rest daml:nil .

:Evaluation daml:intersectionOf _:node174ns8legx54 .

_:node174ns8legx54 daml:first _:node174ns8legx55 .

_:node174ns8legx55 daml:onProperty rdf:subject ;
	daml:toClass :Assertor .

_:node174ns8legx54 daml:rest _:node174ns8legx56 .

_:node174ns8legx56 daml:first _:node174ns8legx57 .

_:node174ns8legx57 daml:onProperty rdf:predicate ;
	daml:hasValue :asserts .

_:node174ns8legx56 daml:rest _:node174ns8legx58 .

_:node174ns8legx58 daml:first _:node174ns8legx59 .

_:node174ns8legx59 daml:onProperty rdf:object ;
	daml:toClass :Assertion .

_:node174ns8legx58 daml:rest daml:nil .

:RepairInfo rdfs:subClassOf _:node174ns8legx60 .

_:node174ns8legx60 daml:onProperty :expectedResult ;
	daml:toClass :ExpectedResult .

:ResultProperty rdfs:subClassOf _:node174ns8legx61 .

_:node174ns8legx61 daml:onProperty :note ;
	daml:toClass rdfs:Resource .

:TestCriteria daml:unionOf _:node174ns8legx62 .

_:node174ns8legx62 daml:first _:node174ns8legx63 .

_:node174ns8legx63 daml:onProperty :level ;
	daml:minCardinality "1" .

_:node174ns8legx62 daml:rest _:node174ns8legx64 .

_:node174ns8legx64 daml:first _:node174ns8legx65 .

_:node174ns8legx65 daml:onProperty :excludes ;
	daml:minCardinality "1" .

_:node174ns8legx64 daml:rest daml:nil .

:TestSubject rdfs:subClassOf _:node174ns8legx66 .

_:node174ns8legx66 daml:onProperty :date ;
	daml:minCardinality "1" .

:TestSubject rdfs:subClassOf _:node174ns8legx67 .

_:node174ns8legx67 daml:onProperty :platform ;
	daml:toClass :Platform .

:id rdfs:domain _:node174ns8legx68 .

_:node174ns8legx68 daml:disjointUnionOf _:node174ns8legx69 .

_:node174ns8legx69 daml:first :TestCase ;
	daml:rest _:node174ns8legx70 .

_:node174ns8legx70 daml:first :TestCriteria ;
	daml:rest _:node174ns8legx71 .

_:node174ns8legx71 daml:first :Exclusion ;
	daml:rest daml:nil .

:level rdfs:domain _:node174ns8legx72 .

_:node174ns8legx72 daml:disjointUnionOf _:node174ns8legx73 .

_:node174ns8legx73 daml:first :TestCriteria ;
	daml:rest _:node174ns8legx74 .

_:node174ns8legx74 daml:first :Exclusion ;
	daml:rest daml:nil .

:suite rdfs:domain _:node174ns8legx75 .

_:node174ns8legx75 daml:disjointUnionOf _:node174ns8legx76 .

_:node174ns8legx76 daml:first :TestCase ;
	daml:rest _:node174ns8legx77 .

_:node174ns8legx77 daml:first :TestCriteria ;
	daml:rest _:node174ns8legx78 .

_:node174ns8legx78 daml:first :Exclusion ;
	daml:rest daml:nil .
