@prefix rdfs:  <http://www.w3.org/2000/01/rdf-schema#> .
@prefix ns3:   <http://purl.org/net/dbm/ontology#> .
@prefix foaf:  <http://xmlns.com/foaf/0.1/> .
@prefix owl:   <http://www.w3.org/2002/07/owl#> .
@prefix xsd:   <http://www.w3.org/2001/XMLSchema#> .
@prefix ns9:   <http://purl.org/vocab/vann/> .
@prefix rdf:   <http://www.w3.org/1999/02/22-rdf-syntax-ns#> .
@prefix ns5:   <http://wifo5-04.informatik.uni-mannheim.de/drugbank/resource/drugbank/> .
@prefix ns7:   <http://purl.org/dc/terms/> .
@prefix ns10:  <http://creativecommons.org/ns#> .
@prefix ns8:   <http://purl.org/net/dbm/> .

ns3:Drug  a           owl:Class ;
        rdfs:comment  "This class represents a Drug entity from the Macedonian Drug Bureau." .

ns3:manufacturer  a   owl:DatatypeProperty ;
        rdfs:comment  "This property represents a manufacturer of a drug." ;
        rdfs:domain   ns3:Drug ;
        rdfs:range    xsd:string .

ns3:approvedOn  a     owl:DatatypeProperty ;
        rdfs:comment  "This property represents the date the company was given the approval by the Macedonian Drug Bureau for the drug." ;
        rdfs:domain   ns3:Drug ;
        rdfs:range    xsd:dateTime .

ns3:referencePrice  a  owl:DatatypeProperty ;
        rdfs:comment  "This property represents the reference price for the drug, as assigned by the Ministry of Health of the Republic of Macedonia." ;
        rdfs:domain   ns3:Drug ;
        rdfs:range    xsd:float .

ns5:brandName  a      owl:DatatypeProperty ;
        rdfs:comment  "This property represents the brand name of the drug." ;
        rdfs:domain   ns3:Drug ;
        rdfs:range    xsd:string .

ns5:atcCode  a        owl:DatatypeProperty ;
        rdfs:comment  "This property represents the ATC code of the drug." ;
        rdfs:domain   ns3:Drug ;
        rdfs:range    xsd:string .

ns3:packaging  a      owl:DatatypeProperty ;
        rdfs:comment  "This property represents the packaging information of the drug." ;
        rdfs:domain   ns3:Drug ;
        rdfs:range    xsd:string .

ns5:drugs  a    owl:Class .

rdfs:label  a         owl:DatatypeProperty ;
        rdfs:comment  "This property holds the brand name of the drug, as a label." ;
        rdfs:domain   ns3:Drug ;
        rdfs:range    xsd:string .

ns3:updateDate  a     owl:DatatypeProperty ;
        rdfs:comment  "This property represents the date the drug data has been updated." ;
        rdfs:domain   ns3:Drug ;
        rdfs:range    xsd:dateTime .

ns3:eanCode  a        owl:DatatypeProperty , owl:FunctionalProperty ;
        rdfs:comment  "This property represents the EAN code of the drug." ;
        rdfs:domain   ns3:Drug ;
        rdfs:range    xsd:string .

ns3:strength  a       owl:DatatypeProperty ;
        rdfs:comment  "This property represents the strength of the drug." ;
        rdfs:domain   ns3:Drug ;
        rdfs:range    xsd:string .

ns3:priceWithVAT  a   owl:DatatypeProperty ;
        rdfs:comment  "This property represents the price of the drug in Macedonian Denars (MKD), with VAT calculated." ;
        rdfs:domain   ns3:Drug ;
        rdfs:range    xsd:float .

ns3:brailleSupport  a  owl:DatatypeProperty ;
        rdfs:comment  "This property indicates wether the drug packaging has Braille support or not." ;
        rdfs:domain   ns3:Drug ;
        rdfs:range    xsd:string .

ns3:brandNameCyrillic
        a             owl:DatatypeProperty ;
        rdfs:comment  "This property represents the brand name of the drug, in cyrillic alphabet." ;
        rdfs:domain   ns3:Drug ;
        rdfs:range    xsd:string .

ns3:summaryReport  a  owl:DatatypeProperty , owl:FunctionalProperty ;
        rdfs:comment  "This property holds the URL to the summary report for the drug, published by the Macedonian Drug Bureau." ;
        rdfs:domain   ns3:Drug ;
        rdfs:range    xsd:string .

ns3:usageGuidelines  a  owl:DatatypeProperty , owl:FunctionalProperty ;
        rdfs:comment  "This property holds the URL to the usage guidelines for the drug, published by the Macedonian Drug Bureau." ;
        rdfs:domain   ns3:Drug ;
        rdfs:range    xsd:string .

foaf:page  a          owl:FunctionalProperty , owl:DatatypeProperty ;
        rdfs:comment  "This property holds the URL of the drug information page on the Macedonian Drug Bureau website." ;
        rdfs:domain   ns3:Drug ;
        rdfs:range    xsd:string .

ns3:positiveList  a   owl:DatatypeProperty ;
        rdfs:comment  "This property tells if the drug is featured on the positive list of drugs, or not." ;
        rdfs:domain   ns3:Drug ;
        rdfs:range    xsd:string .

rdfs:seeAlso  a       owl:ObjectProperty ;
        rdfs:comment  "This property links a drug from the Macedonian Drug Bureau with a drug from DrugBank, based on the ATC code." ;
        rdfs:domain   ns3:Drug ;
        rdfs:range    ns5:drugs .

ns5:genericName  a    owl:DatatypeProperty ;
        rdfs:comment  "This property represents the generic name of the drug." ;
        rdfs:domain   ns3:Drug ;
        rdfs:range    xsd:string .

ns3:atcCodeExtended  a  owl:DatatypeProperty ;
        rdfs:comment  "This property represents the extended ATC code for the drug, assigned by the Ministry of Health, of the Republic of Macedonia." ;
        rdfs:domain   ns3:Drug ;
        rdfs:range    xsd:string .

ns3:dosage  a         owl:DatatypeProperty ;
        rdfs:comment  "This property represents the dosage information for the drug." ;
        rdfs:domain   ns3:Drug ;
        rdfs:range    xsd:string .

ns3:    a                             owl:Ontology ;
        rdfs:comment                  "An ontology for the Drug Bureau of Macedonia (DBM)." ;
        rdfs:isDefinedBy              ns8:ontology ;
        rdfs:label                    "DBM Ontology" ;
        ns10:license                  <https://creativecommons.org/licenses/by/3.0/> ;
        ns7:creator                   <https://plus.google.com/+MilosJovanovik> ;
        ns7:description               "An ontology for describing brand-name drugs." ;
        ns7:issued                    "2014-09-01" ;
        ns7:modified                  "2016-08-28" ;
        ns7:publisher                 <http://finki.ukim.mk/> ;
        ns7:rights                    "Copyright 2014, Milos Jovanovik" ;
        ns7:title                     "DBM Ontology" ;
        ns9:preferredNamespacePrefix  "dbm" ;
        ns9:preferredNamespaceUri     "http://purl.org/net/dbm/ontology#" ;
        owl:versionInfo               "1.1" .

ns3:approvalNumber  a  owl:DatatypeProperty ;
        rdfs:comment  "This property represents the approval number assigned by the Macedonian Drug Bureau, for the company." ;
        rdfs:domain   ns3:Drug ;
        rdfs:range    xsd:string .

ns3:approvedFor  a    owl:DatatypeProperty ;
        rdfs:comment  "This property represents the company which holds the approval by the Macedonian Drug Bureau for the drug." ;
        rdfs:domain   ns3:Drug ;
        rdfs:range    xsd:string .

ns3:approvedUntil  a  owl:DatatypeProperty ;
        rdfs:comment  "This property represents the expiry date of the approval which the company was given by the Macedonian Drug Bureau for the drug." ;
        rdfs:domain   ns3:Drug ;
        rdfs:range    xsd:dateTime .

ns3:hifmCode  a       owl:FunctionalProperty , owl:DatatypeProperty ;
        rdfs:comment  "This is the code that the drug instance has in the local system of the Health Insurance Fund of Macedonia." ;
        rdfs:domain   ns3:Drug ;
        rdfs:range    xsd:string .

ns3:priceWithoutVAT  a  owl:DatatypeProperty ;
        rdfs:comment  "This property represents the price of the drug in Macedonian Denars (MKD), with no VAT calculated." ;
        rdfs:domain   ns3:Drug ;
        rdfs:range    xsd:float .

ns3:similarTo  a      owl:SymmetricProperty , owl:TransitiveProperty , owl:ObjectProperty ;
        rdfs:comment  "This property is used to represent that the drugs in question are similar in their purpose, i.e. contain the same active substance." ;
        rdfs:domain   ns3:Drug ;
        rdfs:range    ns3:Drug .
