@prefix dc: <http://purl.org/dc/elements/1.1/> .
@prefix : <http://data.fundacionctic.org/vocab/catalog/datasets#> .
@prefix rdfs: <http://www.w3.org/2000/01/rdf-schema#> .
@prefix dctype: <http://purl.org/dc/dcmitype/> .
@prefix foaf: <http://xmlns.com/foaf/0.1/> .
@prefix xsd: <http://www.w3.org/2001/XMLSchema#> .
@prefix owl: <http://www.w3.org/2002/07/owl#> .
@prefix vann: <http://purl.org/vocab/vann/> .
@prefix rdf: <http://www.w3.org/1999/02/22-rdf-syntax-ns#> .
@prefix skos: <http://www.w3.org/2004/02/skos/core#> .
@prefix cc: <http://web.resource.org/cc/> .
@prefix dcterms: <http://purl.org/dc/terms/> .

<http://data.fundacionctic.org/vocab/catalog> a owl:Ontology ;
	dc:identifier "http://data.fundacionctic.org/vocab/catalog/datasets_20090928" ;
	dc:date "2009-09-28" ;
	dcterms:issued "2009-09-28" ;
	dc:title "Vocabulario de Catálogos de Datasets"@es , "Dataset Catalog Vocabulary"@en ;
	rdfs:comment "Este vocabulario se utiliza para modelar los catálogos de conjuntos de datos y las relaciones con los datasets"@es , "This vocabulary is used for modelling catalogs of datasets and its relationships with the datasets"@en ;
	dcterms:isVersionOf <http://data.fundacionctic.org/vocab/catalog/datasets#> ;
	dc:creator "CTIC CT" ;
	cc:license <http://creativecommons.org/licenses/by-nc-sa/3.0> ;
	dc:rights "CTIC CT - Creative Commons 3.0 (BY-NC-SA)"@es , "CTIC CT - Creative Commons 3.0 (BY-NC-SA)"@en ;
	vann:preferredNamespaceUri "http://data.fundacionctic.org/vocab/catalog/datasets#" ;
	vann:preferredNamespacePrefix "ds" ;
	dcterms:hasFormat <http://data.fundacionctic.org/vocab/catalog/datasets_20090928.html> .

<http://data.fundacionctic.org/vocab/catalog/datasets_20090928.html> a dctype:Text ;
	dc:format _:node179lhib2px1 .

_:node179lhib2px1 a dcterms:IMT ;
	rdf:value "text/html" ;
	rdfs:label "HTML" .

<http://data.fundacionctic.org/vocab/catalog> dcterms:hasFormat <http://data.fundacionctic.org/vocab/catalog/datasets_20090928.rdf> .

<http://data.fundacionctic.org/vocab/catalog/datasets_20090928.rdf> a dctype:Text ;
	dc:format _:node179lhib2px2 .

_:node179lhib2px2 a dcterms:IMT ;
	rdf:value "application/rdf+xml" ;
	rdfs:label "RDF" .

:Catalog a rdfs:Class ;
	rdfs:isDefinedBy <http://data.fundacionctic.org/vocab/catalog/datasets#> ;
	rdfs:label "Catálogo de datasets"@es ;
	rdfs:comment "Catálogo donde se expresan conjuntos de datos"@es ;
	skos:definition "Catálogo donde se expresan conjuntos de datos"@es ;
	rdfs:label "Catalog of Datasets"@en ;
	rdfs:comment "Catalog which have defined datasets in"@en ;
	skos:definition "Catalog which have defined datasets in"@en ;
	dcterms:issued "2009-09-28" .

:Dataset a rdfs:Class ;
	rdfs:isDefinedBy <http://data.fundacionctic.org/vocab/catalog/datasets#> ;
	rdfs:label "Dataset"@es ;
	rdfs:comment "Un conjunto de datos"@es ;
	skos:definition "Un conjunto de datos"@es ;
	rdfs:label "Dataset"@en ;
	rdfs:comment "A dataset"@en ;
	skos:definition "A dataset"@en ;
	rdfs:subClassOf <http://rdfs.org/ns/void#Dataset> ;
	dcterms:issued "2009-09-28" .

:memberOf a rdf:Property ;
	rdfs:isDefinedBy <http://data.fundacionctic.org/vocab/catalog/datasets#> ;
	rdfs:label "Un Dataset es miembro de un Catálogo"@es ;
	rdfs:comment "Propiedad que define que un Dataset forma parte de un Catálogo"@es ;
	skos:definition "Propiedad que define que un Dataset forma parte de un Catálogo"@es ;
	rdfs:label "A Dataset is a member of a Catalog"@en ;
	rdfs:comment "Property which defines a Dataset which is a member of a Catalog"@en ;
	skos:definition "Property which defines a Dataset which is a member of a Catalog"@en ;
	rdfs:range :Catalog ;
	rdfs:domain :Dataset ;
	dcterms:issued "2009-09-28" .

<http://data.fundacionctic.org/vocab/catalog/datasets_20090928.html> dc:format _:node179lhib2px3 .

_:node179lhib2px3 a dcterms:IMT ;
	rdf:value "text/html" ;
	rdfs:label "HTML" .

<http://data.fundacionctic.org/vocab/catalog/datasets_20090928.rdf> dc:format _:node179lhib2px4 .

_:node179lhib2px4 a dcterms:IMT ;
	rdf:value "application/rdf+xml" ;
	rdfs:label "RDF" .
