@prefix :      <http://linked.earth/ontology#> .
@prefix rdfs:  <http://www.w3.org/2000/01/rdf-schema#> .
@prefix owl:   <http://www.w3.org/2002/07/owl#> .
@prefix xsd:   <http://www.w3.org/2001/XMLSchema#> .
@prefix rdf:   <http://www.w3.org/1999/02/22-rdf-syntax-ns#> .
@prefix vann:  <http://purl.org/vocab/vann/> .
@prefix dcterms: <http://purl.org/dc/terms/> .

:MeasurementTable  a     owl:Class ;
        rdfs:comment     "Table that contains the measuredVariables made on the Archive"@en ;
        rdfs:label       "MeasurementTable"@en ;
        rdfs:subClassOf  :DataTable .

:Person  a                   owl:Class ;
        rdfs:comment         "A person that has participated directly or indirectly in the authoring or contribution of any resources in  Linked Earth."@en ;
        rdfs:label           "Person"@en ;
        owl:equivalentClass  <http://xmlns.com/foaf/0.1/Person> .

:PaleoDataTable  a       owl:Class ;
        rdfs:comment     "DataTable containig PaleoData Variables"@en ;
        rdfs:label       "PaleoDataTable"@en ;
        rdfs:subClassOf  :DataTable .

:calibrationReferences
        a                   owl:ObjectProperty ;
        rdfs:comment        "The publication that describes the calibration. The string should follow the model set in the publication class"@en ;
        rdfs:domain         :CalibrationModel ;
        rdfs:label          "calibrationReferences"@en ;
        rdfs:range          :Publication ;
        rdfs:subPropertyOf  dcterms:references .

:IsotopeInterpretation
        a                owl:Class ;
        rdfs:comment     "A suite of metadata that describe how a MeasuredVariable with instance Isotope is interpreted to reflect past variability, including environmental variability" ;
        rdfs:label       "IsotopeInterpretation"@en ;
        rdfs:subClassOf  :Interpretation .

:Interpretation  a    owl:Class ;
        rdfs:comment  "A suite of metadata that describe how a variable is interpreted to reflect past variability, including environmental variability"@en ;
        rdfs:label    "Interpretation"@en .

:Resolution  a        owl:Class ;
        rdfs:comment  "Refers to the distance (physical or temporal) between each point on the archive. May or May not be related to sampling. Value with units"@en ;
        rdfs:label    "Resolution"@en .

dcterms:bibliographicCitation
        a                 owl:DatatypeProperty ;
        rdfs:isDefinedBy  dcterms: .

:warnings  a                owl:DatatypeProperty ;
        rdfs:comment        "Warnings of the variable or dataset being annotated"@en ;
        rdfs:domain         :Variable , :Dataset ;
        rdfs:label          "warnings"@en ;
        rdfs:range          rdfs:Literal ;
        rdfs:subPropertyOf  :notes .

:hasLink  a           owl:DatatypeProperty ;
        rdfs:comment  "A downloadable link of a resource"@en ;
        rdfs:label    "hasLink"@en ;
        rdfs:range    rdfs:Literal .

:ArchiveModel  a          owl:Class ;
        rdfs:comment      "A simplified description of how the sensor either creates or emplaces the signal into the archive. sensu Evans et al. 2013."@en ;
        rdfs:isDefinedBy  <http://www.sciencedirect.com/science/article/pii/S0277379113002011> ;
        rdfs:label        "ArchiveModel"@en ;
        rdfs:subClassOf   :Model .

:hasISBN  a                 owl:DatatypeProperty ;
        rdfs:comment        "Identifier used commonly to refer to publications."@en ;
        rdfs:domain         :Publication ;
        rdfs:label          "hasISBN"@en ;
        rdfs:range          xsd:string ;
        rdfs:subPropertyOf  dcterms:identifier .

:principalInvestigator
        a             owl:ObjectProperty ;
        rdfs:comment  "Who is the PrincipalInvestigator of the Funding grant?"@en ;
        rdfs:domain   :Funding ;
        rdfs:label    "principalInvestigator"@en ;
        rdfs:range    :Person .

<http://www.w3.org/2003/01/geo/wgs84_pos#SpatialThing>
        a                 owl:Class ;
        rdfs:isDefinedBy  <http://www.w3.org/2003/01/geo/wgs84_pos#> .

:datasetVersion  a    owl:FunctionalProperty , owl:DatatypeProperty ;
        rdfs:comment  "The version of the dataset. It should follow the x.y.z notation where x refers to changes in metadata and data following a publication (for instance, the creation of a new age model using a different code), y refers to changes to the data following a publication (for instance, adding data further back in time without changing the model underlying the interpretation), and z refers to changes not associated with a publication (for instance, typos)."@en ;
        rdfs:domain   :Dataset ;
        rdfs:label    "datasetVersion"@en .

<http://orcid.org/0000-0001-5920-4751>
        a       owl:NamedIndividual .

:hasUncertainty  a    owl:ObjectProperty ;
        rdfs:comment  "What is the Uncertainty associated with the Observations, Model, and Calibration?"@en ;
        rdfs:domain   [ a            owl:Class ;
                        owl:unionOf  ( :CalibrationModel :Instrument :Model :Variable )
                      ] ;
        rdfs:label    "hasUncertainty"@en ;
        rdfs:range    :Uncertainty .

:fundedBy  a          owl:ObjectProperty ;
        rdfs:comment  "Property that indicated the funding which made the dataset possible"@en ;
        rdfs:domain   :Dataset ;
        rdfs:label    "fundedBy"@en ;
        rdfs:range    :Funding .

:ProxySystemModel  a      owl:Class ;
        rdfs:comment      "In the Evans et al. (2013) framework, this is the combination of sensor, archive and observation models . \"A generalized proxy system model encapuslates a simplified representation of prior physical, chemical, biological, and/or geological understanding of the ways in which environmental variation ultimately results in the observations used to retrieve paleoclimatic information.\""@en ;
        rdfs:isDefinedBy  <http://www.sciencedirect.com/science/article/pii/S0277379113002011> ;
        rdfs:label        "ProxySystemModel"@en ;
        rdfs:subClassOf   :Model .

:hasUnits  a          owl:FunctionalProperty , owl:DatatypeProperty ;
        rdfs:comment  "units in which a resource is measured The resource can be a Variable, an Observation, a Resolution, or an Uncertainty"@en ;
        rdfs:domain   [ a            owl:Class ;
                        owl:unionOf  ( :Observation :Resolution :Uncertainty :Variable )
                      ] ;
        rdfs:label    "hasUnits"@en ;
        rdfs:range    xsd:string .

:Model  a             owl:Class ;
        rdfs:comment  "Any system that is at least partially isomorphic to some target system and used to derive information about the structure and/or dynamics of the target system."@en ;
        rdfs:label    "Model"@en .

<http://w3id.org/people/dgarijo>
        a       owl:NamedIndividual .

:uncertaintyLevel  a  owl:DatatypeProperty ;
        rdfs:comment  "Quantile or number of standard deviations along a probability distribution of a Variable." ;
        rdfs:domain   :Uncertainty ;
        rdfs:label    "uncertaintyLevel"@en ;
        rdfs:range    xsd:string .

:observedAs  a        owl:ObjectProperty ;
        rdfs:comment  "What Observations were made?"@en ;
        rdfs:domain   :Proxy ;
        rdfs:label    "observedAs"@en ;
        rdfs:range    :Observation .

:hasPart  a           owl:ObjectProperty ;
        rdfs:comment  "What are the components of the ProxySystemModel?" ;
        rdfs:domain   :ProxySystemModel ;
        rdfs:label    "hasPart"@en ;
        rdfs:range    [ a            owl:Class ;
                        owl:unionOf  ( :ArchiveModel :ObservationModel :SensorModel )
                      ] .

:inferredFrom  a      owl:ObjectProperty ;
        rdfs:comment  "From which measured variable is the current inferred variable obtained?"@en ;
        rdfs:domain   :InferredVariable ;
        rdfs:label    "inferredFrom"@en ;
        rdfs:range    :MeasuredVariable .

<http://www.w3.org/2003/01/geo/wgs84_pos#alt>
        a                   owl:DatatypeProperty ;
        rdfs:domain         <http://www.w3.org/2003/01/geo/wgs84_pos#SpatialThing> ;
        rdfs:isDefinedBy    <http://www.w3.org/2003/01/geo/wgs84_pos#> ;
        rdfs:range          xsd:string ;
        rdfs:subPropertyOf  owl:topDataProperty .

:grantNumber  a       owl:DatatypeProperty ;
        rdfs:comment  "The grant number associated with the development of the Dataset?"@en ;
        rdfs:domain   :Funding ;
        rdfs:label    "grantNumber"@en ;
        rdfs:range    xsd:string .

:hasFileName  a       owl:FunctionalProperty , owl:DatatypeProperty ;
        rdfs:comment  "Name of the CSV file containing the data table"@en ;
        rdfs:domain   :DataTable ;
        rdfs:label    "hasFileName"@en ;
        rdfs:range    xsd:string .

:MeasuredVariable  a     owl:Class ;
        rdfs:comment     "Is the variable measured with an instrument?"@en ;
        rdfs:label       "MeasuredVariable"@en ;
        rdfs:subClassOf  :Variable .

:measuredOn  a              owl:ObjectProperty ;
        rdfs:comment        "On what Archive were the Observations measured on?"@en ;
        rdfs:domain         :MeasuredVariable ;
        rdfs:label          "measuredOn"@en ;
        rdfs:range          :Archive ;
        rdfs:subPropertyOf  owl:topObjectProperty .

:includesData  a      owl:ObjectProperty ;
        rdfs:comment  "What are the paleoenvironmental and chronological Data included in the Dataset?"@en ;
        rdfs:domain   :Dataset ;
        rdfs:label    "includesData"@en ;
        rdfs:range    :Data .

dcterms:identifier  a     owl:DatatypeProperty ;
        rdfs:isDefinedBy  dcterms: .

dcterms:created  a        owl:DatatypeProperty ;
        rdfs:isDefinedBy  dcterms: .

:SensorModel  a           owl:Class ;
        rdfs:comment      "A formalization of the behavior of the sensor in response to environmental forcing. Sensu Evans et al. 2013."@en ;
        rdfs:isDefinedBy  <http://www.sciencedirect.com/science/article/pii/S0277379113002011> ;
        rdfs:label        "SensorModel"@en ;
        rdfs:subClassOf   :Model .

:ChronProxy  a           owl:Class ;
        rdfs:comment     "The data and metadata associated with how the chronology information was obtained."@en ;
        rdfs:label       "ChronProxy"@en ;
        rdfs:subClassOf  :Proxy .

:Data   a             owl:Class ;
        rdfs:comment  "An aggregation of DataTables and supporting information regarging the paleoenvironmental and/or chronological interpretation "@en ;
        rdfs:label    "Data"@en .

:chronModeledBy  a          owl:ObjectProperty ;
        rdfs:comment        "How was the chron data modeled?"@en ;
        rdfs:domain         [ a            owl:Class ;
                              owl:unionOf  ( :ChronData )
                            ] ;
        rdfs:label          "chronModeledBy"@en ;
        rdfs:range          :ChronModel ;
        rdfs:subPropertyOf  :modeledBy .

:Uncertainty  a           owl:Class ;
        rdfs:comment      "A state of incomplete knowledge that can result from a lack of information or from disagreement about what is known or  even knowable. Uncertainty may come from many sources, from imprecision in the data to ambigously defined concepts or terminology, or uncertain projections of human bahavior. Uncertainty can be represented by quantitative measures (e.g., probability density function) or by qualitative statement (e.g., reflecting the judgement of a team of experts. Sensu IPCC AR5"@en ;
        rdfs:isDefinedBy  <https://www.ipcc.ch/pdf/assessment-report/ar5/wg1/WG1AR5_AnnexIII_FINAL.pdf> ;
        rdfs:label        "Uncertainty"@en .

:modelReferences  a         owl:ObjectProperty ;
        rdfs:comment        "The publication that describes the model. "@en ;
        rdfs:domain         :Model ;
        rdfs:label          "modelReferences"@en ;
        rdfs:range          :Publication ;
        rdfs:subPropertyOf  dcterms:references .

:archivedIn  a        owl:ObjectProperty ;
        rdfs:comment  "How was the climate or chronological information encoded into the Archive?"@en ;
        rdfs:domain   :Proxy ;
        rdfs:label    "archivedIn"@en ;
        rdfs:range    :Archive .

:DataTable  a         owl:Class ;
        rdfs:comment  "A set of Variables organized in columns"@en ;
        rdfs:label    "DataTable"@en .

<http://xmlns.com/foaf/0.1/Person>
        a                 owl:Class ;
        rdfs:isDefinedBy  <http://xmlns.com/foaf/0.1/> .

:SummaryTable  a         owl:Class ;
        rdfs:label       "Table containing relevant statistics from the ensemble table"@en , "SummaryTable"@en ;
        rdfs:subClassOf  :DataTable .

:foundInTable  a      owl:ObjectProperty ;
        rdfs:comment  "Property that indicated the table where the described data can be found"@en ;
        rdfs:domain   [ a            owl:Class ;
                        owl:unionOf  ( :Data :Model :Variable )
                      ] ;
        rdfs:label    "foundInTable"@en ;
        rdfs:range    :DataTable .

:Archive  a               owl:Class ;
        rdfs:comment      "The medium in which the response of a sensor to environmental forcing is recorded (e.g., marine sediments, ice core, lake sediments, speleothems). Sensu Evans et al. (2013)"@en ;
        rdfs:isDefinedBy  <http://www.sciencedirect.com/science/article/pii/S0277379113002011> ;
        rdfs:label        "Archive"@en .

:ChronModel  a           owl:Class ;
        rdfs:comment     "Model used to obtain the chronology"@en ;
        rdfs:label       "ChronModel"@en ;
        rdfs:subClassOf  :Model .

:UncertaintyModel  a     owl:Class ;
        rdfs:comment     "A formalization of the way the uncertainty is accounted for"@en ;
        rdfs:label       "UndertaintyModel"@en ;
        rdfs:subClassOf  :Model .

:includesPaleoData  a       owl:ObjectProperty ;
        rdfs:comment        "The paleo data included as part of a dataset"@en ;
        rdfs:domain         :Dataset ;
        rdfs:label          "includesPaleoData"@en ;
        rdfs:range          :PaleoData ;
        rdfs:subPropertyOf  :includesData .

:issue  a             owl:FunctionalProperty , owl:DatatypeProperty ;
        rdfs:comment  "The issue number for the publication"@en ;
        rdfs:domain   :Publication ;
        rdfs:label    "issue"@en ;
        rdfs:range    xsd:int .

:hasID  a             owl:DatatypeProperty ;
        rdfs:comment  "ID for a variable in a table"@en ;
        rdfs:domain   :Variable ;
        rdfs:label    "hasID"@en ;
        rdfs:range    xsd:string .

:standard  a          owl:DatatypeProperty ;
        rdfs:comment  "The standard against which the observations are reported (for instance, VSMOW or VPDB)"@en ;
        rdfs:domain   :MeasuredVariable ;
        rdfs:label    "standard"@en .

:hasResolution  a     owl:ObjectProperty ;
        rdfs:comment  "What is the Resolution of the Archive?" ;
        rdfs:domain   :Archive ;
        rdfs:label    "hasResolution"@en ;
        rdfs:range    :Resolution .

<http://earth.usc.edu/~khider/>
        a       owl:NamedIndividual .

:title  a                   owl:DatatypeProperty ;
        rdfs:comment        "Title of a publication"@en ;
        rdfs:domain         :Publication ;
        rdfs:label          "title"@en ;
        rdfs:range          xsd:string ;
        rdfs:subPropertyOf  dcterms:title .

:Instrument  a        owl:Class ;
        rdfs:comment  "A tool or implement used to produce MeasuredVariables"@en ;
        rdfs:label    "Instrument"@en .

:citation  a                owl:DatatypeProperty ;
        rdfs:comment        "Sentence indicating how a paper should be published"@en ;
        rdfs:domain         :Publication ;
        rdfs:label          "citation"@en ;
        rdfs:range          rdfs:Literal ;
        rdfs:subPropertyOf  dcterms:bibliographicCitation .

:fundingCountry  a    owl:FunctionalProperty , owl:DatatypeProperty ;
        rdfs:comment  "Country which awarded the funding for the dataset"@en ;
        rdfs:domain   :Funding ;
        rdfs:label    "fundingCountry"@en .

:equation  a          owl:DatatypeProperty ;
        rdfs:comment  "The mathematical statement used to describe the model."@en ;
        rdfs:domain   :Model ;
        rdfs:label    "equation"@en ;
        rdfs:range    xsd:string .

:pages  a             owl:FunctionalProperty , owl:DatatypeProperty ;
        rdfs:comment  "The page range for the article."@en ;
        rdfs:domain   :Publication ;
        rdfs:label    "pages"@en ;
        rdfs:range    xsd:string .

:basedOn  a           owl:ObjectProperty ;
        rdfs:comment  "How are the data obtained?"@en ;
        rdfs:domain   :Data ;
        rdfs:label    "basedOn"@en ;
        rdfs:range    :Proxy .

:hasExecutionEnvironment
        a             owl:DatatypeProperty ;
        rdfs:comment  "Execution environment of the code"@en ;
        rdfs:domain   :SoftwareCode ;
        rdfs:label    "hasExecutionEnvironment"@en ;
        rdfs:range    xsd:string .

:orcidNumber  a       owl:FunctionalProperty , owl:DatatypeProperty ;
        rdfs:comment  "The ORCID number of the Person" ;
        rdfs:domain   :Person ;
        rdfs:label    "orcidNumber"@en ;
        rdfs:range    xsd:string .

:Sensor  a                owl:Class ;
        rdfs:comment      "The sensor comprises physical, chemical and/or biological components that react to environmental conditions (e.g, foraminifera, coral polyps, cave, catchment basin). sensu Evans et al. (2013)"@en ;
        rdfs:isDefinedBy  <http://www.sciencedirect.com/science/article/pii/S0277379113002011> ;
        rdfs:label        "Sensor"@en .

:detail  a            owl:DatatypeProperty ;
        rdfs:comment  "Answers the \"of what\" question for a Variable."@en ;
        rdfs:domain   :Interpretation ;
        rdfs:label    "detail"@en ;
        rdfs:range    xsd:string .

:notes  a             owl:DatatypeProperty ;
        rdfs:comment  "Notes regarding the cells in the DataTable"@en ;
        rdfs:domain   :Variable , :Model , :Dataset ;
        rdfs:label    "notes"@en ;
        rdfs:range    xsd:string .

<http://www.opengis.net/ont/geosparql#hasGeometry>
        a                 owl:ObjectProperty ;
        rdfs:domain       <http://www.opengis.net/ont/geosparql#Feature> ;
        rdfs:isDefinedBy  <http://www.opengis.net/spec/geosparql/1.0> ;
        rdfs:range        <http://www.opengis.net/ont/geosparql#Geometry> .

:calibratedFrom  a    owl:ObjectProperty ;
        rdfs:comment  "Property that indicates how the measured variable was calibrated"@en ;
        rdfs:domain   :MeasuredVariable ;
        rdfs:label    "calibratedFrom"@en ;
        rdfs:range    :CalibrationModel .

:method  a            owl:DatatypeProperty ;
        rdfs:comment  "Method used to obtain the information from the resource"@en ;
        rdfs:domain   [ a            owl:Class ;
                        owl:unionOf  ( :Archive :Model :Observation )
                      ] ;
        rdfs:label    "method"@en ;
        rdfs:range    xsd:string .

:foundInDistributionTable
        a                   owl:FunctionalProperty , owl:ObjectProperty ;
        rdfs:comment        "Property that indicates that a variable or data is found in a distribution table"@en ;
        rdfs:domain         [ a            owl:Class ;
                              owl:unionOf  ( :ChronModel :PaleoModel )
                            ] ;
        rdfs:label          "foundInDistributionTable"@en ;
        rdfs:range          :DistributionTable ;
        rdfs:subPropertyOf  :foundInTable .

:paleoModeledBy  a          owl:ObjectProperty ;
        rdfs:comment        "How was the paleoData modeled?"@en ;
        rdfs:domain         [ a            owl:Class ;
                              owl:unionOf  ( :PaleoData )
                            ] ;
        rdfs:label          "paleoModeledBy"@en ;
        rdfs:range          :PaleoModel ;
        rdfs:subPropertyOf  :modeledBy .

:sensorGenus  a       owl:DatatypeProperty ;
        rdfs:comment  "The Genus of the sensor" ;
        rdfs:domain   :OrganicSensor ;
        rdfs:label    "sensorGenus"@en ;
        rdfs:range    xsd:string .

:volume  a            owl:FunctionalProperty , owl:DatatypeProperty ;
        rdfs:comment  "The volume number in which the publication appeared."@en ;
        rdfs:domain   :Publication ;
        rdfs:label    "volume"@en ;
        rdfs:range    xsd:string .

:interpretationReferences
        a                   owl:ObjectProperty ;
        rdfs:comment        "Describes the basis by which the proxy variable is interpreted in terms of climate. "@en ;
        rdfs:domain         :Interpretation ;
        rdfs:label          "interpretationReferences"@en ;
        rdfs:range          :Publication ;
        rdfs:subPropertyOf  dcterms:references .

:hasMissingValue  a               owl:FunctionalProperty , owl:DatatypeProperty ;
        rdfs:comment              "Indicates how the missing values are flagged in a dataset"@en ;
        rdfs:domain               [ a            owl:Class ;
                                    owl:unionOf  ( :Uncertainty :Variable )
                                  ] ;
        rdfs:label                "hasMissingValue"@en ;
        rdfs:range                xsd:string ;
        owl:propertyDisjointWith  :hasValue .

:collectedFrom  a     owl:ObjectProperty ;
        rdfs:comment  "Where was the data in the dataset collected from? Generally, this is the site where the archive was collected. "@en ;
        rdfs:domain   :Dataset ;
        rdfs:label    "collectedFrom"@en ;
        rdfs:range    :Location .

:Funding  a           owl:Class ;
        rdfs:comment  "A source of funding for the creation of the Dataset"@en ;
        rdfs:label    "Funding"@en .

:sensingWith  a       owl:ObjectProperty ;
        rdfs:comment  "How does the proxy system senses the environment?"@en ;
        rdfs:domain   :Proxy ;
        rdfs:label    "sensingWith"@en ;
        rdfs:range    :Sensor .

:EnsembleTable  a        owl:Class ;
        rdfs:comment     "Table containing possible series of age models or proxy variability"@en ;
        rdfs:label       "EnsembleTable"@en ;
        rdfs:subClassOf  :DataTable .

:hasCode  a           owl:FunctionalProperty , owl:ObjectProperty ;
        rdfs:comment  "What is the mathematical formulation that describes the Model?"@en ;
        rdfs:domain   :Model ;
        rdfs:label    "hasCode"@en ;
        rdfs:range    :SoftwareCode .

dcterms:title  a          owl:DatatypeProperty ;
        rdfs:isDefinedBy  dcterms: .

:datasetDate  a             owl:FunctionalProperty , owl:DatatypeProperty ;
        rdfs:comment        "Date when the dataset was published. "@en ;
        rdfs:domain         :Dataset ;
        rdfs:label          "datasetDate"@en ;
        rdfs:range          xsd:dateTime ;
        rdfs:subPropertyOf  dcterms:created .

:Variable  a          owl:Class ;
        rdfs:comment  "Quantities which can be measured or inferred independently in an experiment"@en ;
        rdfs:label    "Variable"@en .

<http://www.w3.org/2003/01/geo/wgs84_pos#lat>
        a                 owl:DatatypeProperty ;
        rdfs:domain       <http://www.w3.org/2003/01/geo/wgs84_pos#SpatialThing> ;
        rdfs:isDefinedBy  <http://www.w3.org/2003/01/geo/wgs84_pos#> ;
        rdfs:range        xsd:string .

:DistributionTable  a    owl:Class ;
        rdfs:comment     "Table that contains the probability on the inferred variables"@en ;
        rdfs:label       "DistributionTable"@en ;
        rdfs:subClassOf  :DataTable .

:hasExecutionCommand  a  owl:DatatypeProperty ;
        rdfs:comment  "The execution command needed to run the script or software"@en ;
        rdfs:domain   :SoftwareCode ;
        rdfs:label    "hasExecutionCommand"@en ;
        rdfs:range    xsd:string .

:SoftwareCode  a      owl:Class ;
        rdfs:comment  "A script that describes the model, in any programming language (e.g., Excel, Matlab, Python, R)"@en ;
        rdfs:label    "SoftwareCode"@en .

:Proxy  a             owl:Class ;
        rdfs:comment  "a measured variable used to infer the value of a variable of interest"@en ;
        rdfs:label    "Proxy"@en .

:PaleoModel  a           owl:Class ;
        rdfs:comment     "Model describing how the measuredVariables are transformed into inferredVariables"@en ;
        rdfs:label       "PaleoModel"@en ;
        rdfs:subClassOf  :Model .

:includesChronData  a       owl:ObjectProperty ;
        rdfs:comment        "Pointer to the chron data included in the dataset"@en ;
        rdfs:domain         :Dataset ;
        rdfs:label          "includesChronData"@en ;
        rdfs:range          :ChronData ;
        rdfs:subPropertyOf  :includesData .

<http://schema.org/name>
        a                 owl:DatatypeProperty ;
        rdfs:domain       owl:Thing ;
        rdfs:isDefinedBy  <http://schema.org/> ;
        rdfs:range        xsd:string .

:description  a       owl:DatatypeProperty ;
        rdfs:comment  "The description of a resource. This property may be used to provide further details on instrument descriptions, uncertainty description,etc."@en ;
        rdfs:label    "description"@en ;
        rdfs:range    xsd:string .

:PaleoData  a            owl:Class ;
        rdfs:comment     "The Data pertaining to past environmental variability"@en ;
        rdfs:label       "PaleoData"@en ;
        rdfs:subClassOf  :Data .

dcterms:creator  a        owl:ObjectProperty ;
        rdfs:isDefinedBy  dcterms: .

<http://www.isi.edu/~gil/>
        a       owl:NamedIndividual .

:ObservationModel  a      owl:Class ;
        rdfs:comment      "The simplified representation of the way in which observations are made on the archive. sensu Evans et al. 2013."@en ;
        rdfs:isDefinedBy  <http://www.sciencedirect.com/science/article/pii/S0277379113002011> ;
        rdfs:label        "ObservationModel"@en ;
        rdfs:subClassOf   :Model .

<http://www.cefns.nau.edu/~npm4/>
        a       owl:NamedIndividual .

:isLocal  a           owl:FunctionalProperty , owl:DatatypeProperty ;
        rdfs:comment  "Whether the influence on the MeasuredVariable (and therefore the Interpretation) is local or far-field. The literal is a string." ;
        rdfs:domain   :Interpretation ;
        rdfs:label    "isLocal"@en ;
        rdfs:range    xsd:string .

:interpretedAs  a     owl:ObjectProperty ;
        rdfs:comment  "how is the variable interpreted?"@en ;
        rdfs:domain   :Variable ;
        rdfs:label    "interpretedAs"@en ;
        rdfs:range    :Interpretation .

:foundInEnsembleTable
        a                   owl:FunctionalProperty , owl:ObjectProperty ;
        rdfs:comment        "Property that indicates that the data or variable described was found in an ensemble table"@en ;
        rdfs:domain         [ a            owl:Class ;
                              owl:unionOf  ( :ChronModel :PaleoModel )
                            ] ;
        rdfs:label          "foundInEnsembleTable"@en ;
        rdfs:range          :EnsembleTable ;
        rdfs:subPropertyOf  :foundInTable .

:CalibrationModel  a     owl:Class ;
        rdfs:comment     "Metadata about how the variable was calibrated to reflect an environmental variable"@en ;
        rdfs:label       "CalibrationModel"@en ;
        rdfs:subClassOf  :Model .

<http://www.opengis.net/ont/geosparql#asWKT>
        a                 owl:DatatypeProperty ;
        rdfs:domain       <http://www.opengis.net/ont/geosparql#Geometry> ;
        rdfs:isDefinedBy  <http://www.opengis.net/ont/geosparql#> ;
        rdfs:range        rdfs:Literal .

:journal  a           owl:DatatypeProperty ;
        rdfs:comment  "Property that indicated the journal in which the publication has been published"@en ;
        rdfs:domain   :Publication ;
        rdfs:label    "journal"@en ;
        rdfs:range    xsd:string .

:Publication  a       owl:Class ;
        rdfs:comment  "A document that serves as reference for a Dataset or its components"@en ;
        rdfs:label    "Publication"@en .

:foundInMeasurementTable
        a                   owl:ObjectProperty ;
        rdfs:comment        "Property that indicates that a variable was found in a measurement table"@en ;
        rdfs:domain         [ a            owl:Class ;
                              owl:unionOf  ( :Data )
                            ] ;
        rdfs:label          "foundInMeasurementTable"@en ;
        rdfs:range          :MeasurementTable ;
        rdfs:subPropertyOf  :foundInTable .

:Location  a             owl:Class ;
        rdfs:comment     "The geographic data and metadata for the dataset"@en ;
        rdfs:label       "Location"@en ;
        rdfs:subClassOf  <http://www.w3.org/2003/01/geo/wgs84_pos#SpatialThing> , <http://www.opengis.net/ont/geosparql#Feature> .

:InorganicSensor  a       owl:Class ;
        rdfs:comment      "An inorganic senso like.karst system, catchment basin, etc."@en ;
        rdfs:label        "InorganicSensor"@en ;
        rdfs:subClassOf   :Sensor ;
        owl:disjointWith  :OrganicSensor .

:includesVariable  a  owl:ObjectProperty ;
        rdfs:comment  "What are the Variables included in the DataTable?"@en ;
        rdfs:domain   :DataTable ;
        rdfs:label    "includesVariable"@en ;
        rdfs:range    :Variable .

:hasDOI  a                  owl:FunctionalProperty , owl:DatatypeProperty ;
        rdfs:comment        "As Digital Object Identifier for a given resource. For example: \"oi:10.1191/095968301673881493\""@en ;
        rdfs:domain         [ a            owl:Class ;
                              owl:unionOf  ( :Dataset :Publication :SoftwareCode )
                            ] ;
        rdfs:label          "hasDOI"@en ;
        rdfs:range          xsd:string ;
        rdfs:subPropertyOf  dcterms:identifier .

:interpretationDirection
        a             owl:FunctionalProperty , owl:DatatypeProperty ;
        rdfs:comment  "Describes whether the interpreted environmental variable increases (positive) or decreases (negative) as the paleoDataVariableValue increases. The literal is a string , either \"positive\" or \"negative\""@en ;
        rdfs:domain   :Interpretation ;
        rdfs:label    "interpretationDirection"@en ;
        rdfs:range    xsd:string .

:foundInSummaryTable  a     owl:FunctionalProperty , owl:ObjectProperty ;
        rdfs:comment        "Property that indicates that the describer data or variable was found in a summary table"@en ;
        rdfs:domain         [ a            owl:Class ;
                              owl:unionOf  ( :ChronModel :PaleoModel )
                            ] ;
        rdfs:label          "foundInSummaryTable"@en ;
        rdfs:range          :SummaryTable ;
        rdfs:subPropertyOf  :foundInTable .

:ChronDataTable  a        owl:Class ;
        rdfs:comment      "DataTable containing the Chronology Variables"@en ;
        rdfs:label        "ChronDataTable"@en ;
        rdfs:subClassOf   :DataTable ;
        owl:disjointWith  :PaleoDataTable .

:contributor  a             owl:ObjectProperty ;
        rdfs:comment        "Contributor of the resource (dataset, publication, etc.)"@en ;
        rdfs:domain         :Dataset ;
        rdfs:label          "contributor"@en ;
        rdfs:range          :Person ;
        rdfs:subPropertyOf  dcterms:contributor .

:Dataset  a           owl:Class ;
        rdfs:comment  "A structured collection of related information, including - but not limited to - geographical, chronological, and measured or modeled paleoenvironmental data"@en ;
        rdfs:label    "Dataset"@en .

:book   a             owl:DatatypeProperty ;
        rdfs:comment  "Book in which the publication was published"@en ;
        rdfs:domain   :Publication ;
        rdfs:label    "book"@en ;
        rdfs:range    xsd:string .

:hasISSN  a                 owl:DatatypeProperty ;
        rdfs:comment        "8-digit code used to udentify publications"@en ;
        rdfs:domain         :Publication ;
        rdfs:label          "hasISSN"@en ;
        rdfs:range          xsd:string ;
        rdfs:subPropertyOf  dcterms:identifier .

:author  a                  owl:ObjectProperty ;
        rdfs:comment        "Author of the resource"@en ;
        rdfs:domain         [ a            owl:Class ;
                              owl:unionOf  ( :Dataset :Publication )
                            ] ;
        rdfs:label          "author"@en ;
        rdfs:range          :Person ;
        rdfs:subPropertyOf  dcterms:creator .

:hasRank  a           owl:FunctionalProperty , owl:DatatypeProperty ;
        rdfs:comment  "Describes the importance of the ClimateInterpretation. For instance, d18Ocalcite is influenced by both temperature and d18Osw. If temperature is the dominant influence, then its rank is 1." ;
        rdfs:domain   :Interpretation ;
        rdfs:label    "hasRank"@en ;
        rdfs:range    xsd:int .

<http://www.w3.org/2003/01/geo/wgs84_pos#long>
        a                 owl:DatatypeProperty ;
        rdfs:domain       <http://www.w3.org/2003/01/geo/wgs84_pos#SpatialThing> ;
        rdfs:isDefinedBy  <http://www.w3.org/2003/01/geo/wgs84_pos#> ;
        rdfs:range        xsd:string .

:InferredVariable  a      owl:Class ;
        rdfs:comment      "Is the variable inferred from a measured variable?"@en ;
        rdfs:label        "InferredVariable"@en ;
        rdfs:subClassOf   :Variable ;
        owl:disjointWith  :MeasuredVariable .

:ClimateInterpretation
        a                owl:Class ;
        rdfs:comment     "A suite of metadata that describe how a variable is interpreted to reflect past environmental variability" ;
        rdfs:label       "ClimateInterpretation"@en ;
        rdfs:subClassOf  :Interpretation .

:hasValue  a          owl:DatatypeProperty ;
        rdfs:comment  "A column of values for the variable. The literal can be in the form of a vector of values (for instance d18O PaleoObservations),  a vector of strings (for instance different paleoArchiveNames),  a matrix or both"@en ;
        rdfs:domain   [ a            owl:Class ;
                        owl:unionOf  ( :Uncertainty :Variable )
                      ] ;
        rdfs:label    "hasValue"@en ;
        rdfs:range    xsd:string .

:NonPeerReviewedPublication
        a                 owl:Class ;
        rdfs:comment      "A publication that has not undergone a formal review process; for instance, a Dataset attached to a dissertation."@en ;
        rdfs:label        "NonPeerReviewedPublication"@en ;
        rdfs:subClassOf   :Publication ;
        owl:disjointWith  :PeerReviewedPublication .

:modeledBy  a         owl:ObjectProperty ;
        rdfs:comment  "How was the process modeled?"@en ;
        rdfs:domain   [ a            owl:Class ;
                        owl:unionOf  ( :Data :Proxy )
                      ] ;
        rdfs:label    "modeledBy"@en ;
        rdfs:range    :Model .

:fundingAgency  a     owl:FunctionalProperty , owl:DatatypeProperty ;
        rdfs:comment  "The agency that funded the development of the Dataset"@en ;
        rdfs:domain   :Funding ;
        rdfs:label    "fundingAgency"@en ;
        rdfs:range    xsd:string .

:publishedIn  a       owl:ObjectProperty ;
        rdfs:comment  "Where was the Dataset published? Property that relates a dataset to the publication where it was published."@en ;
        rdfs:domain   :Dataset ;
        rdfs:label    "publishedIn"@en ;
        rdfs:range    :Publication .

:OrganicSensor  a        owl:Class ;
        rdfs:comment     "An organic sensor (e.g., foraminifera, tree, corals...)"@en ;
        rdfs:label       "OrganicSensor"@en ;
        rdfs:subClassOf  :Sensor .

dcterms:references  a     owl:ObjectProperty ;
        rdfs:isDefinedBy  dcterms: .

:email  a             owl:DatatypeProperty ;
        rdfs:comment  "email of an author or contributor"@en ;
        rdfs:domain   :Person ;
        rdfs:label    "email"@en ;
        rdfs:range    xsd:string .

<http://www.opengis.net/ont/geosparql#Feature>
        a                 owl:Class ;
        rdfs:isDefinedBy  <http://www.opengis.net/ont/geosparql> .

dcterms:contributor  a    owl:ObjectProperty ;
        rdfs:isDefinedBy  dcterms: .

:name   a                   owl:DatatypeProperty ;
        rdfs:comment        "Name of the described resource"@en ;
        rdfs:label          "name"@en ;
        rdfs:range          xsd:string ;
        rdfs:subPropertyOf  <http://schema.org/name> .

:measuredBy  a        owl:ObjectProperty ;
        rdfs:comment  "What Instrument was used to obtain the MeasuredVariables and Observations?"@en ;
        rdfs:domain   :MeasuredVariable ;
        rdfs:label    "measuredBy"@en ;
        rdfs:range    :Instrument .

:PeerReviewedPublication
        a                owl:Class ;
        rdfs:comment     "A publication that has undergone a formal peer-reviewed process."@en ;
        rdfs:label       "PeerReviewedPublication"@en ;
        rdfs:subClassOf  :Publication .

:IntegrationTime  a      owl:Class ;
        rdfs:comment     "The integration time of the Archive or the Sensor" ;
        rdfs:label       "IntegrationTime"@en ;
        rdfs:subClassOf  :SensorModel , :ArchiveModel .

:seasonality  a       owl:DatatypeProperty ;
        rdfs:comment  "fluctuating or restricted according to the season or time of year"@en ;
        rdfs:domain   :Sensor , :Interpretation ;
        rdfs:label    "seasonality"@en ;
        rdfs:range    xsd:string .

:ChronData  a            owl:Class ;
        rdfs:comment     "The Data pertaining to chronological information"@en ;
        rdfs:label       "CrhonData"@en ;
        rdfs:subClassOf  :Data .

:       a                              owl:NamedIndividual , owl:Ontology ;
        rdfs:comment                   "The Linked Earth Ontology aims to provide a common vocabulary for annotating paleoclimatology data"@en ;
        dcterms:contributor            <http://www.isi.edu/~gil/> , <http://w3id.org/people/dgarijo> ;
        dcterms:creator                <http://www.cefns.nau.edu/~npm4/> , <http://orcid.org/0000-0001-5920-4751> , <http://earth.usc.edu/~khider/> ;
        dcterms:license                "http://creativecommons.org/licenses/by-nc-sa/2.0/" ;
        dcterms:title                  "The Linked Earth Ontology"@en , "The Linked Earth Ontology" ;
        vann:preferredNamespacePrefix  "le" ;
        vann:preferredNamespaceUri     "http://linked.earth/ontology#" ;
        owl:versionInfo                "1.0.0"@en .

:Observation  a           owl:Class ;
        rdfs:comment      "The measurements made on the archives, whether chemical (e.g., Mg/Ca, d18O, TEX86, Sr/Ca....), physical (e.g. density, layer thickness) or biological (e.g. species abundance). Evans et al. (2013). Observations are MeasuredVariables"@en ;
        rdfs:isDefinedBy  <http://www.sciencedirect.com/science/article/pii/S0277379113002011> ;
        rdfs:label        "Observation"@en ;
        rdfs:subClassOf   :MeasuredVariable .

rdfs:Literal  owl:equivalentClass  xsd:string .

:sensorSpecies  a     owl:DatatypeProperty ;
        rdfs:comment  "The species of the sensor" ;
        rdfs:domain   :OrganicSensor ;
        rdfs:label    "sensorSpecies"@en ;
        rdfs:range    xsd:string .

:publicationYear  a         owl:FunctionalProperty , owl:DatatypeProperty ;
        rdfs:comment        "Year when the publication was published. The literal is a numeric value in the format yyyy"@en ;
        rdfs:domain         :Publication ;
        rdfs:label          "publicationYear"@en ;
        rdfs:range          xsd:int ;
        rdfs:subPropertyOf  dcterms:created .

<http://www.opengis.net/ont/geosparql#Geometry>
        a                 owl:Class ;
        rdfs:isDefinedBy  <http://www.opengis.net/spec/geosparql/1.0> .

:ClimateProxy  a         owl:Class ;
        rdfs:comment     "Climate observations prior to the instrumental era are necessarily indirect. These observations are made on climate proxies in various geological (e.g. lake or marine sediments, living or fossil coral reefs, cave deposits), glaciological (ice cores or snow pits) or biological (trees) archives. Many types of measurements can be made on each archives, each sensing a different aspect of the environment (sometimes, several aspects at once). A paleoclimate dataset is a set of observations made on an archive."@en ;
        rdfs:label       "ClimateProxy"@en ;
        rdfs:subClassOf  :Proxy .

:calibratedWith  a    owl:ObjectProperty ;
        rdfs:comment  "How was the variable calibrated to represent climate or chronology?"@en ;
        rdfs:domain   :InferredVariable ;
        rdfs:label    "calibratedWith"@en ;
        rdfs:range    :CalibrationModel .

:relevantQuote  a           owl:DatatypeProperty ;
        rdfs:comment        "Relevant summary or preferably quotation from the referenced Publication" ;
        rdfs:label          "relevantQuote"@en ;
        rdfs:range          xsd:string ;
        rdfs:subPropertyOf  :description .
