@prefix dc: <http://purl.org/dc/elements/1.1/> .
@prefix op: <http://environment.data.gov.au/def/op#> .
@prefix foaf: <http://xmlns.com/foaf/0.1/> .
@prefix void: <http://rdfs.org/ns/void#> .
@prefix vann: <http://purl.org/vocab/vann/> .
@prefix prov-dc: <http://www.w3.org/ns/prov-dc#> .
@prefix qudt: <http://qudt.org/schema/qudt#> .
@prefix rdfs: <http://www.w3.org/2000/01/rdf-schema#> .
@prefix voaf: <http://purl.org/vocommons/voaf#> .
@prefix dct: <http://purl.org/dc/terms/> .
@prefix owl: <http://www.w3.org/2002/07/owl#> .
@prefix xsd: <http://www.w3.org/2001/XMLSchema#> .
@prefix rdf: <http://www.w3.org/1999/02/22-rdf-syntax-ns#> .
@prefix skos: <http://www.w3.org/2004/02/skos/core#> .
@prefix cc: <http://creativecommons.org/ns#> .

<http://environment.data.gov.au/def/op> a voaf:Vocabulary ;
	rdfs:comment """A general purpose ontology for observable properties. The ontology supports description of both qualitative and quantitative properties. The allowed scale or units of measure may be specified. A property may be linked to substances-or-taxa and to features or realms, if they play a role in the definition. 

This ontology was developed to enable publication of a vocabulary of water quality properties for the Bioregional Assessments and eReefs projects.

This ontology extends the QUDT schema. 

Some key classes and properties are linked to SKOS, so that instances of an observable-property vocabulary are implicitly also SKOS concepts, and may be accessed through general purpose vocabulary APIs based on SKOS."""^^xsd:string ;
	dc:publisher "AGIMO"^^xsd:string ;
	dct:hasPart op:PropertyKind .

op:PropertyKind a owl:Class .

<http://environment.data.gov.au/def/op> dct:hasPart op:SubstanceOrTaxon .

op:SubstanceOrTaxon a owl:Class .

<http://environment.data.gov.au/def/op> owl:imports <http://www.w3.org/2004/02/skos/core> ;
	dct:hasPart op:objectOfInterest .

op:objectOfInterest a owl:ObjectProperty .

<http://environment.data.gov.au/def/op> voaf:extends <http://qudt.org/schema/qudt> ;
	void:vocabulary <http://qudt.org/schema/qudt> ;
	vann:preferredNamespaceUri "http://environment.data.gov.au/def/op#"^^xsd:string ;
	dct:hasPart op:matrix .

op:matrix a owl:ObjectProperty .

<http://environment.data.gov.au/def/op> dc:creator "Bruce A Simons"^^xsd:string , "Simon J D Cox"^^xsd:string ;
	dct:license <http://creativecommons.org/licenses/by/3.0/> ;
	dct:modified "2013-12-03"^^xsd:string ;
	owl:imports <http://purl.org/vocommons/voaf> ;
	rdfs:label "Observable-Properties ontology"^^xsd:string ;
	dct:hasPart op:procedure .

op:procedure a owl:ObjectProperty .

<http://environment.data.gov.au/def/op> owl:imports <http://purl.org/vocab/vann/> , <http://www.w3.org/ns/prov> ;
	a owl:Ontology ;
	owl:imports <http://purl.org/dc/elements/1.1/> ;
	dc:rights "Copyright Â© 2012-2013 CSIRO"^^xsd:string ;
	dc:title "Observable properties"^^xsd:string ;
	dc:creator "Jonathan Yu"^^xsd:string ;
	owl:imports <http://qudt.org/1.1/vocab/quantity> ;
	dct:hasPart op:QualityKind .

op:QualityKind a owl:Class .

<http://environment.data.gov.au/def/op> dct:hasPart op:constraint .

op:constraint a owl:ObjectProperty .

<http://environment.data.gov.au/def/op> dct:hasPart op:featureOfInterest .

op:featureOfInterest a owl:ObjectProperty .

<http://environment.data.gov.au/def/op> owl:imports <http://www.w3.org/2003/06/sw-vocab-status/ns> ;
	dc:description "A general purpose ontology for observable properties. The ontology supports description of both qualitative and quantitative properties. The allowed scale or units of measure may be specified. A property may be linked to substances-or-taxa and to features or realms, if they play a role in the definition."^^xsd:string ;
	dct:hasPart op:qualityKind .

op:qualityKind a owl:ObjectProperty .

<http://environment.data.gov.au/def/op> dct:hasPart op:propertyKind .

op:propertyKind a owl:ObjectProperty .

<http://environment.data.gov.au/def/op> owl:imports <http://rdfs.org/ns/void> ;
	dct:created "2013"^^xsd:gYear ;
	void:uriSpace "http://environment.data.gov.au/def/op#"^^xsd:string ;
	dct:hasPart op:applicableVocabulary .

op:applicableVocabulary a owl:ObjectProperty .

<http://environment.data.gov.au/def/op> owl:imports <http://xmlns.com/foaf/0.1/> ;
	dct:hasPart op:ScaledQuantityKind .

op:ScaledQuantityKind a owl:Class .

<http://environment.data.gov.au/def/op> dc:publisher "CSIRO"^^xsd:string ;
	vann:preferredNamespacePrefix "op"^^xsd:string .

op:PropertyKind rdfs:isDefinedBy <http://environment.data.gov.au/def/op> ;
	rdfs:subClassOf _:node18fvu5s29x12 .

_:node18fvu5s29x12 a owl:Restriction ;
	owl:onProperty op:objectOfInterest ;
	owl:allValuesFrom op:SubstanceOrTaxon .

op:PropertyKind rdfs:label "Property kind"@en ;
	rdfs:subClassOf qudt:EnumeratedValue .

qudt:EnumeratedValue rdfs:subClassOf skos:Concept .

op:PropertyKind rdfs:subClassOf _:node18fvu5s29x13 .

_:node18fvu5s29x13 a owl:Restriction ;
	owl:onProperty op:constraint ;
	owl:minCardinality "0"^^xsd:nonNegativeInteger .

op:PropertyKind rdfs:subClassOf _:node18fvu5s29x14 .

_:node18fvu5s29x14 a owl:Restriction ;
	owl:onProperty op:procedure ;
	owl:minCardinality "0"^^xsd:nonNegativeInteger .

op:PropertyKind rdfs:comment """Superclass of qudt:QuantityKind
This class accommodates all kinds of properties, including those (qualities) that are not described by quantities (numeric values). 
May carry an objectOfInterest property, to point to the substance or taxon with which the property is associated - e.g. tree-height, organism-count, nitrogen-concentration"""^^xsd:string ;
	rdfs:subClassOf _:node18fvu5s29x15 .

_:node18fvu5s29x15 a owl:Restriction ;
	owl:onProperty qudt:generalization .

qudt:generalization rdfs:subPropertyOf skos:broader .

_:node18fvu5s29x15 owl:allValuesFrom op:PropertyKind .

op:PropertyKind rdfs:subClassOf _:node18fvu5s29x16 .

_:node18fvu5s29x16 a owl:Restriction ;
	owl:onProperty op:featureOfInterest ;
	owl:minCardinality "0"^^xsd:nonNegativeInteger .

op:QualityKind rdfs:isDefinedBy <http://environment.data.gov.au/def/op> ;
	owl:disjointWith op:ScaledQuantityKind ;
	rdfs:subClassOf _:node18fvu5s29x17 .

_:node18fvu5s29x17 a owl:Restriction ;
	owl:onProperty op:applicableVocabulary ;
	owl:minCardinality "0"^^xsd:nonNegativeInteger .

op:QualityKind rdfs:subClassOf op:PropertyKind ;
	rdfs:label "Quality Kind"@en ;
	rdfs:comment "non-numeric PropertyKind"^^xsd:string .

op:ScaledQuantityKind rdfs:comment """Scaled quantity kind has one or more unit properties, which indicate valid units of measure for this quantity kind. 

It is likely that this class is equivalent to qudt:QuantityKind, but has been declared independently for governance of the qudt:unit property"""^^xsd:string ;
	rdfs:subClassOf _:node18fvu5s29x18 .

_:node18fvu5s29x18 a owl:Restriction ;
	owl:onProperty qudt:unit ;
	owl:allValuesFrom qudt:Unit .

qudt:Unit rdfs:subClassOf skos:Concept .

op:ScaledQuantityKind rdfs:label "Scaled Quantity Kind"@en ;
	rdfs:subClassOf _:node18fvu5s29x19 .

_:node18fvu5s29x19 a owl:Restriction ;
	owl:onProperty qudt:unit ;
	owl:minCardinality "1"^^xsd:nonNegativeInteger .

op:ScaledQuantityKind rdfs:isDefinedBy <http://environment.data.gov.au/def/op> ;
	rdfs:subClassOf op:PropertyKind ;
	owl:equivalentClass qudt:QuantityKind .

qudt:QuantityKind rdfs:subClassOf op:PropertyKind .

op:ScaledQuantityKind owl:disjointWith op:QualityKind .

op:SubstanceOrTaxon rdfs:isDefinedBy <http://environment.data.gov.au/def/op> ;
	rdfs:subClassOf qudt:EnumeratedValue ;
	rdfs:label "Substance or Taxon"@en ;
	rdfs:comment "Class of stuff and things, individuals of which identify a class of stuff and things that make observed properties concrete."^^xsd:string .

op:applicableVocabulary rdfs:isDefinedBy <http://environment.data.gov.au/def/op> ;
	rdfs:range _:node18fvu5s29x20 .

_:node18fvu5s29x20 a owl:Class ;
	owl:unionOf _:node18fvu5s29x21 .

_:node18fvu5s29x21 rdf:first skos:ConceptScheme ;
	rdf:rest _:node18fvu5s29x22 .

_:node18fvu5s29x22 rdf:first skos:Collection ;
	rdf:rest rdf:nil .

op:applicableVocabulary rdfs:label "applicable vocabulary"@en ;
	rdfs:domain op:QualityKind ;
	rdfs:comment """Set of terms or concepts from which the value must be drawn

Compare with QUDT2 'applicable unit'"""^^xsd:string .

op:featureOfInterest rdfs:isDefinedBy <http://environment.data.gov.au/def/op> ;
	rdfs:subPropertyOf <http://def.seegrid.csiro.au/isotc211/iso19156/2011/observation#featureOfInterest> , op:constraint ;
	rdfs:comment "In an observable property definition, the feature-of-interest constrains the feature realm that the property is associated with."^^xsd:string ;
	rdfs:domain op:PropertyKind ;
	rdfs:label "feature of interest"@en .

op:matrix rdfs:isDefinedBy <http://environment.data.gov.au/def/op> ;
	rdfs:subPropertyOf op:featureOfInterest ;
	rdfs:comment "In an observable property definition, the matrix is a special case of a feature-of-interest that provides the context (container feeaure or medium) for an observable property."^^xsd:string ;
	rdfs:label "matrix"@en .

op:qualityKind rdfs:isDefinedBy <http://environment.data.gov.au/def/op> ;
	owl:propertyDisjointWith qudt:quantityKind .

qudt:quantityKind rdfs:subPropertyOf op:propertyKind .

op:qualityKind rdfs:subPropertyOf op:propertyKind ;
	rdfs:range op:QualityKind ;
	rdfs:label "quality kind"@en .

op:procedure rdfs:isDefinedBy <http://environment.data.gov.au/def/op> ;
	rdfs:comment "link to procedure or sensor system used in making observation or estimate of property value"^^xsd:string ;
	rdfs:subPropertyOf <http://def.seegrid.csiro.au/isotc211/iso19156/2011/observation#procedure> , op:constraint ;
	rdfs:domain op:PropertyKind ;
	rdfs:label "procedure"@en .

op:propertyKind rdfs:isDefinedBy <http://environment.data.gov.au/def/op> ;
	rdfs:subPropertyOf <http://def.seegrid.csiro.au/isotc211/iso19156/2011/observation#observedProperty> , skos:related ;
	rdfs:range op:PropertyKind ;
	rdfs:label "property kind"@en .

op:objectOfInterest rdfs:isDefinedBy <http://environment.data.gov.au/def/op> ;
	rdfs:subPropertyOf op:constraint ;
	rdfs:range op:SubstanceOrTaxon ;
	rdfs:comment "In an observable property definition, the object-of-interest constrains the substance or taxon involved in a count, concentration, presence, or other simialr property."^^xsd:string ;
	rdfs:domain op:PropertyKind ;
	rdfs:label "object of interest"@en .

op:constraint rdfs:isDefinedBy <http://environment.data.gov.au/def/op> ;
	rdfs:subPropertyOf skos:related ;
	rdfs:comment "Constraint that refines the definition of an abservable property definition. This may include concerns such as realm of application, substance or taxon involved, applicable units or vocabulary."^^xsd:string ;
	rdfs:domain op:PropertyKind ;
	rdfs:label "constraint"@en .

qudt:specialization rdfs:subPropertyOf skos:narrower .
