@prefix :      <http://softeng.polito.it/rs-context-ontology#> .
@prefix dc:    <http://purl.org/dc/elements/1.1/> .
@prefix rdfs:  <http://www.w3.org/2000/01/rdf-schema#> .
@prefix ns:    <http://creativecommons.org/ns#> .
@prefix foaf:  <http://xmlns.com/foaf/0.1/> .
@prefix terms: <http://purl.org/dc/terms/> .
@prefix owl:   <http://www.w3.org/2002/07/owl#> .
@prefix xsd:   <http://www.w3.org/2001/XMLSchema#> .
@prefix rdf:   <http://www.w3.org/1999/02/22-rdf-syntax-ns#> .
@prefix vann:  <http://purl.org/vocab/vann/> .
@prefix skos:  <http://www.w3.org/2004/02/skos/core#> .

[ a            owl:AllDisjointClasses ;
  owl:members  ( <http://softeng.polito.it/rsctx#AnchorPoint> <http://softeng.polito.it/rsctx#CompanionHome> <http://softeng.polito.it/rsctx#PublicPlace> )
] .

<http://softeng.polito.it/rsctx#Season>
        a                owl:Class ;
        rdfs:comment     "A season is a division of the year marked by changes in weather."@en ;
        rdfs:seeAlso     "https://en.wikipedia.org/wiki/Season" ;
        rdfs:subClassOf  <http://softeng.polito.it/rsctx#TimeInterval> .

<http://softeng.polito.it/rsctx#12>
        a       <http://softeng.polito.it/rsctx#Hour> , owl:NamedIndividual .

<http://softeng.polito.it/rsctx#symbolicLocation>
        a             owl:FunctionalProperty , owl:ObjectProperty ;
        rdfs:comment  "It indicates to which symbolic location that POI corresponds to (if any), such as the home or the workplace of the user or a public place (e.g. a cinema)."@en ;
        rdfs:domain   <http://ns.inria.fr/prissma/v2#POI> ;
        rdfs:label    "symbolic location"@en ;
        rdfs:range    <http://softeng.polito.it/rsctx#SymbolicLocation> .

<http://softeng.polito.it/rsctx#country>
        a             owl:FunctionalProperty , owl:ObjectProperty ;
        rdfs:comment  "It indicates the country of a Location."@en ;
        rdfs:domain   <http://ns.inria.fr/prissma/v2#POI> ;
        rdfs:label    "country"@en ;
        rdfs:range    <http://rdfs.co/juso/Country> .

<http://softeng.polito.it/rsctx#VeryWarm>
        a           <http://softeng.polito.it/rsctx#Temperature> , owl:NamedIndividual ;
        rdfs:label  "Very Warm"@en .

<http://softeng.polito.it/rsctx#respiration>
        a             owl:FunctionalProperty , owl:DatatypeProperty ;
        rdfs:comment  "This property indicates the respiration of a PhysiologicalState (in breaths per minute)."@en ;
        rdfs:domain   <http://softeng.polito.it/rsctx#PhysiologicalState> ;
        rdfs:label    "respiration"@en ;
        rdfs:range    [ a                     rdfs:Datatype ;
                        owl:onDatatype        xsd:int ;
                        owl:withRestrictions  ( [ xsd:minExclusive
                                          0 ] )
                      ] .

<http://softeng.polito.it/rsctx>
        a                              owl:Ontology ;
        rdfs:comment                   "This ontology represent context which may be interesting in providing recommendations to users."@en ;
        ns:license                     "http://creativecommons.org/licenses/by/3.0/" ;
        dc:contributor                 "Aleksandra Karpus" , "Krzysztof Goczyla" ;
        dc:creator                     "Iacopo Vagliano" ;
        dc:issued                      "2016-05-04"^^xsd:date ;
        dc:modified                    "2017-01-17"^^xsd:date ;
        dc:publisher                   <http://dbpedia.org/resource/Polytechnic_University_of_Turin> ;
        dc:title                       "Recommender System Context"@en ;
        vann:preferredNamespacePrefix  "rsctx" ;
        vann:preferredNamespaceUri     "http://softeng.polito.it/rsctx#" ;
        owl:imports                    <https://www.auto.tuwien.ac.at/downloads/thinkhome/ontology/WeatherOntology.owl> , <http://www.w3.org/2006/time> , <http://www.ontologydesignpatterns.org/ont/dul/DUL.owl> , <http://www.w3.org/2007/uwa/context/deliverycontext.owl> , <http://ns.inria.fr/prissma/v2#> , <http://rdfs.co/juso/0.1.2> , <http://gumo.org/2.0/> , foaf: , <http://ns.inria.fr/emoca> , <http://vocab.deri.ie/rooms> ;
        owl:versionInfo                1.2 ;
        foaf:page                      <http://softeng.polito.it/rsctx/> .

<http://softeng.polito.it/rsctx#good>
        a           <http://softeng.polito.it/rsctx#Fitness> , owl:NamedIndividual ;
        rdfs:label  "good"@en .

<http://softeng.polito.it/rsctx#Home>
        a           <http://softeng.polito.it/rsctx#AnchorPoint> , owl:NamedIndividual ;
        rdfs:label  "Home"@en .

<http://dbpedia.org/resource/Polytechnic_University_of_Turin>
        a       foaf:Organization .

<http://softeng.polito.it/rsctx#TropicalSeason>
        a                    owl:Class ;
        rdfs:comment         "Season which occur in hot regions. It includes the rainy (or wet, or monsoon) season and the dry season, In some tropical areas, a cool or mild season is also present.\n\nWARNING This class has just the purpose to organize the seasons. It SHOULD NOT have instances."@en ;
        rdfs:label           "Tropical season"@en ;
        rdfs:subClassOf      <http://softeng.polito.it/rsctx#Season> ;
        owl:equivalentClass  [ a          owl:Class ;
                               owl:oneOf  ( <http://softeng.polito.it/rsctx#MildSeason> <http://softeng.polito.it/rsctx#WetSeason> <http://softeng.polito.it/rsctx#DrySeason> )
                             ] .

<http://softeng.polito.it/rsctx#cognitiveLoad>
        a           <http://softeng.polito.it/rsctx#MentalState> , owl:NamedIndividual ;
        rdfs:label  "cognitive load"@en .

<http://softeng.polito.it/rsctx#transportationMean>
        a             owl:ObjectProperty ;
        rdfs:comment  "It indicates which TransportationMean the user is using or is going to use."@en ;
        rdfs:domain   <http://ns.inria.fr/prissma/v2#Environment> ;
        rdfs:label    "transportation mean"@en ;
        rdfs:range    <http://softeng.polito.it/rsctx#TransportationMean> .

<http://softeng.polito.it/rsctx#worry>
        a           <http://softeng.polito.it/rsctx#EmotionalState> , owl:NamedIndividual ;
        rdfs:label  "worry"@en .

<http://softeng.polito.it/rsctx#season>
        a             owl:FunctionalProperty , owl:ObjectProperty ;
        rdfs:comment  "It indicates the season in which a Time is included in."@en ;
        rdfs:domain   <http://softeng.polito.it/rsctx#Time> ;
        rdfs:label    "season"@en ;
        rdfs:range    <http://softeng.polito.it/rsctx#Season> .

<http://softeng.polito.it/rsctx#inFit>
        a           <http://softeng.polito.it/rsctx#Fitness> , owl:NamedIndividual ;
        rdfs:label  "in fit"@en .

<http://softeng.polito.it/rsctx#injured>
        a           <http://softeng.polito.it/rsctx#Fitness> , owl:NamedIndividual ;
        rdfs:label  "injured"@en .

<http://softeng.polito.it/rsctx#06>
        a       <http://softeng.polito.it/rsctx#Hour> , owl:NamedIndividual .

<http://softeng.polito.it/rsctx#dayOfWeek>
        a             owl:FunctionalProperty , owl:ObjectProperty ;
        rdfs:comment  "This property indicates the day of week of a Time."@en ;
        rdfs:domain   <http://softeng.polito.it/rsctx#Time> ;
        rdfs:label    "day of week"@en ;
        rdfs:range    <http://softeng.polito.it/rsctx#DayOfWeek> .

<http://softeng.polito.it/rsctx#Taxi>
        a           <http://softeng.polito.it/rsctx#TransportationMean> , owl:NamedIndividual ;
        rdfs:label  "Taxi"@en .

<http://softeng.polito.it/rsctx#Cold>
        a           <http://softeng.polito.it/rsctx#Temperature> , owl:NamedIndividual ;
        rdfs:label  "Cold"@en .

<http://softeng.polito.it/rsctx#18>
        a       <http://softeng.polito.it/rsctx#Hour> , owl:NamedIndividual .

<http://softeng.polito.it/rsctx#Region>
        a             owl:Class ;
        rdfs:comment  "A political or geographical region.\n\nWARNING dbpedia-owl represents regions too but it refer to broader sense of region which include any area which is possible to distinguish in geography. In this sense any other geographical unit defined in this ontology (such as country, province, etc.) is a region, while we intend only to represent geographical regions or specific administrative area named regions in some countries (e.g. Italy, France, Belgium)."@en ;
        rdfs:label    "Region"@en .

<http://softeng.polito.it/rsctx#hasPhysiologicalState>
        a             owl:FunctionalProperty , owl:ObjectProperty ;
        rdfs:comment  "This property indicates the phsysiological state of a user."@en ;
        rdfs:domain   <http://ns.inria.fr/prissma/v2#User> ;
        rdfs:label    "has physiological state"@en ;
        rdfs:range    <http://softeng.polito.it/rsctx#PhysiologicalState> .

<http://softeng.polito.it/rsctx#tired>
        a           <http://softeng.polito.it/rsctx#Fitness> , owl:NamedIndividual ;
        rdfs:label  "tired"@en .

<http://softeng.polito.it/rsctx#NoiseLevel>
        a             owl:Class ;
        rdfs:comment  "This class represents the current level of noise. It is intended a symbolic level such as very noisy, silent, etc."@en ;
        rdfs:label    "Noise Level"@en .

<http://softeng.polito.it/rsctx#Pleasant>
        a           <http://softeng.polito.it/rsctx#Temperature> , owl:NamedIndividual ;
        rdfs:label  "Pleasant"@en .

<http://softeng.polito.it/rsctx#Temperature>
        a                    owl:Class ;
        rdfs:comment         "It represents the exterior temperature by means of a symbolic value, such as warm or cool.\n\nTODO Map the individuals with temperature ranges?"@en ;
        rdfs:label           "Temperature"@en ;
        rdfs:subClassOf      <https://www.auto.tuwien.ac.at/downloads/thinkhome/ontology/WeatherOntology.owl#WeatherPhenomenon> ;
        owl:equivalentClass  [ a          owl:Class ;
                               owl:oneOf  ( <http://softeng.polito.it/rsctx#Hot> <http://softeng.polito.it/rsctx#Warm> <http://softeng.polito.it/rsctx#Freezing> <http://softeng.polito.it/rsctx#VeryCold> <http://softeng.polito.it/rsctx#Mild> <http://softeng.polito.it/rsctx#Cool> <http://softeng.polito.it/rsctx#Cold> <http://softeng.polito.it/rsctx#Pleasant> <http://softeng.polito.it/rsctx#VeryWarm> )
                             ] .

<http://softeng.polito.it/rsctx#Night>
        a             <http://softeng.polito.it/rsctx#PartOfDay> , owl:NamedIndividual ;
        rdfs:comment  "The period of time between the sunset and the sunrise when the Sun is below the horizon.The mapping with respect the hours is possible but not defined becaus it may vary with the location and the habits."@en ;
        rdfs:label    "Night"@en .

<http://softeng.polito.it/rsctx#Spring>
        a           <http://softeng.polito.it/rsctx#Season> , owl:NamedIndividual ;
        rdfs:label  "Spring"@en .

<http://softeng.polito.it/rsctx#relief>
        a           <http://softeng.polito.it/rsctx#EmotionalState> , owl:NamedIndividual ;
        rdfs:label  "relief"@en .

<http://softeng.polito.it/rsctx#anxiety>
        a           <http://softeng.polito.it/rsctx#EmotionalState> , owl:NamedIndividual ;
        rdfs:label  "anxiety"@en .

<http://softeng.polito.it/rsctx#region>
        a             owl:FunctionalProperty , owl:ObjectProperty ;
        rdfs:comment  "It indicates the Region of a Location."@en ;
        rdfs:domain   <http://ns.inria.fr/prissma/v2#POI> ;
        rdfs:label    "region"@en ;
        rdfs:range    <http://softeng.polito.it/rsctx#Region> .

<http://softeng.polito.it/rsctx#01>
        a       <http://softeng.polito.it/rsctx#Hour> , owl:NamedIndividual .

<http://softeng.polito.it/rsctx#shame>
        a           <http://softeng.polito.it/rsctx#EmotionalState> , owl:NamedIndividual ;
        rdfs:label  "shame"@en .

<http://softeng.polito.it/rsctx#exteriorTemperature>
        a             owl:FunctionalProperty , owl:DatatypeProperty ;
        rdfs:comment  "It indicates the exterior temperature in degree Celsius."@en ;
        rdfs:domain   <https://www.auto.tuwien.ac.at/downloads/thinkhome/ontology/WeatherOntology.owl#WeatherState> ;
        rdfs:label    "exterior temperature"@en ;
        rdfs:range    xsd:decimal .

<http://softeng.polito.it/rsctx#lighting>
        a             owl:FunctionalProperty , owl:DatatypeProperty ;
        rdfs:comment  "It indicates the light level in lux."@en ;
        rdfs:domain   <http://ns.inria.fr/prissma/v2#Environment> ;
        rdfs:label    "lighting"@en ;
        rdfs:range    [ a                     rdfs:Datatype ;
                        owl:onDatatype        xsd:decimal ;
                        owl:withRestrictions  ( [ xsd:minExclusive
                                          0 ] )
                      ] .

<http://softeng.polito.it/rsctx#MentalState>
        a                    owl:Class ;
        rdfs:comment         "A mental condition in which the qualities of a state are relatively constant even though the state itself may be dynamic, such as depression, cognitive load, nervousness.\n\nWARNING The possible values are represented as individuals while in the GUMO ontology are classes."@en ;
        rdfs:label           "Mental State"@en ;
        owl:equivalentClass  <http://gumo.org/2.0/#MentalState.700017> ;
        owl:equivalentClass  [ a          owl:Class ;
                               owl:oneOf  ( <http://softeng.polito.it/rsctx#trauma> <http://softeng.polito.it/rsctx#timePressure> <http://softeng.polito.it/rsctx#hypnosis> <http://softeng.polito.it/rsctx#cognitiveLoad> <http://softeng.polito.it/rsctx#irritation> <http://softeng.polito.it/rsctx#nervousness> <http://softeng.polito.it/rsctx#trance> <http://softeng.polito.it/rsctx#psychopathy> <http://softeng.polito.it/rsctx#depression> )
                             ] .

<http://softeng.polito.it/rsctx#Summer>
        a           <http://softeng.polito.it/rsctx#Season> , owl:NamedIndividual ;
        rdfs:label  "Summer"@en .

<http://softeng.polito.it/rsctx#SymbolicLocation>
        a             owl:Class ;
        rdfs:comment  "In general, it represents an abstract ideas of where an object is (e.g. next to a mailbox). In the context of the ontology, it can be an anchor point (i.e. a frequently visited location) or a public place or the anchor point of another user.\n\nWARNING Other kind of symbolic location such as bankomat, mailbox, or a train approaching Dublin are not considered."@en ;
        rdfs:label    "Symbolic Location"@en .

<http://softeng.polito.it/rsctx#holiday>
        a             owl:FunctionalProperty , owl:DatatypeProperty ;
        rdfs:comment  "This property indicates if a Time is holiday or a working day."@en ;
        rdfs:domain   <http://softeng.polito.it/rsctx#Time> ;
        rdfs:label    "is holiday"@en ;
        rdfs:range    xsd:boolean .

<http://softeng.polito.it/rsctx#13>
        a       <http://softeng.polito.it/rsctx#Hour> , owl:NamedIndividual .

<http://softeng.polito.it/rsctx#Freezing>
        a           <http://softeng.polito.it/rsctx#Temperature> , owl:NamedIndividual ;
        rdfs:label  "Freezing"@en .

<http://softeng.polito.it/rsctx#firstLevelAdministrativeDivision>
        a             owl:FunctionalProperty , owl:ObjectProperty ;
        rdfs:comment  "It indicates the first level administrative division of a Location."@en ;
        rdfs:domain   <http://ns.inria.fr/prissma/v2#POI> ;
        rdfs:label    "first level administrative division"@en ;
        rdfs:range    <http://rdfs.co/juso/FirstLevelAdministrativeDivision> .

<http://softeng.polito.it/rsctx#thirdLevelAdministrativeDivision>
        a             owl:FunctionalProperty , owl:ObjectProperty ;
        rdfs:comment  "It indicates the third level administrative division of a Location."@en ;
        rdfs:domain   <http://ns.inria.fr/prissma/v2#POI> ;
        rdfs:label    "third level administrative division"@en ;
        rdfs:range    <http://rdfs.co/juso/ThirdLevelAdministrativeDivision> .

<http://softeng.polito.it/rsctx#perspiration>
        a             owl:FunctionalProperty , owl:DatatypeProperty ;
        rdfs:comment  "This property indicates the perspiration (in liters per hours) of a PhysiologicalState."@en ;
        rdfs:domain   <http://softeng.polito.it/rsctx#PhysiologicalState> ;
        rdfs:label    "perspiration"@en ;
        rdfs:range    [ a                     rdfs:Datatype ;
                        owl:onDatatype        xsd:decimal ;
                        owl:withRestrictions  ( [ xsd:minExclusive
                                          0 ] )
                      ] .

<http://softeng.polito.it/rsctx#hypnosis>
        a           <http://softeng.polito.it/rsctx#MentalState> , owl:NamedIndividual ;
        rdfs:label  "hypnosis"@en .

<http://softeng.polito.it/rsctx#Nobody>
        a                owl:Class ;
        rdfs:comment     "The user is alone."@en ;
        rdfs:label       "Nobody"@en ;
        rdfs:subClassOf  <http://softeng.polito.it/rsctx#Companion> .

<http://softeng.polito.it/rsctx#street>
        a             owl:FunctionalProperty , owl:ObjectProperty ;
        rdfs:comment  "It indicates the Street of a Location."@en ;
        rdfs:domain   <http://ns.inria.fr/prissma/v2#POI> ;
        rdfs:label    "street"@en ;
        rdfs:range    <http://vocab.deri.ie/rooms#Site> .

<http://softeng.polito.it/rsctx#07>
        a       <http://softeng.polito.it/rsctx#Hour> , owl:NamedIndividual .

<http://softeng.polito.it/rsctx#CalendarSeason>
        a                    owl:Class ;
        rdfs:comment         "Season which is generally recognized in temperate and subpolar regions, include summer, spring, winter and fall (or autumn).\n\nWARNING This class has just the purpose to organize the seasons. It SHOULD NOT have instances."@en ;
        rdfs:label           "Calendar Season"@en ;
        rdfs:subClassOf      <http://softeng.polito.it/rsctx#Season> ;
        owl:disjointWith     <http://softeng.polito.it/rsctx#TropicalSeason> ;
        owl:equivalentClass  [ a          owl:Class ;
                               owl:oneOf  ( <http://softeng.polito.it/rsctx#Spring> <http://softeng.polito.it/rsctx#Fall> <http://softeng.polito.it/rsctx#Summer> <http://softeng.polito.it/rsctx#Winter> )
                             ] .

<http://softeng.polito.it/rsctx#depression>
        a           <http://softeng.polito.it/rsctx#MentalState> , owl:NamedIndividual ;
        rdfs:label  "depression"@en .

<http://softeng.polito.it/rsctx#Colleague>
        a                owl:Class ;
        rdfs:comment     "The user is with one or more colleagues."@en ;
        rdfs:label       "Colleague"@en ;
        rdfs:subClassOf  <http://softeng.polito.it/rsctx#Companion> .

<http://softeng.polito.it/rsctx#PartOfDay>
        a                    owl:Class ;
        rdfs:comment         "This class represents the time intervals in which a day can be divided in."@en ;
        rdfs:label           "Part of Day"@en ;
        rdfs:subClassOf      <http://softeng.polito.it/rsctx#TimeInterval> ;
        owl:equivalentClass  [ a          owl:Class ;
                               owl:oneOf  ( <http://softeng.polito.it/rsctx#Night> <http://softeng.polito.it/rsctx#Evening> <http://softeng.polito.it/rsctx#Afternoon> <http://softeng.polito.it/rsctx#Morning> )
                             ] .

[ a            owl:AllDisjointClasses ;
  owl:members  ( <http://softeng.polito.it/rsctx#Boss> <http://softeng.polito.it/rsctx#BusinessPartner> <http://softeng.polito.it/rsctx#Child> <http://softeng.polito.it/rsctx#Colleague> <http://softeng.polito.it/rsctx#Family> <http://softeng.polito.it/rsctx#Friend> <http://softeng.polito.it/rsctx#Nobody> <http://softeng.polito.it/rsctx#Partner> )
] .

<http://softeng.polito.it/rsctx#Companion>
        a             owl:Class ;
        rdfs:comment  "Companion class indicates which kind of company the user as at the moment. For example, it may be with family, friends or colleagues.\n\nWARNING Its subclasses not as individual, because the individual could be a person (e.g. Bob or Alice), and it is an istance also of one of companion sublasses to indicate which in kind of companion the individual is for the user in the current context (e.g. is family or colleagues or friend)."@en ;
        rdfs:label    "Companion"@en .

<http://softeng.polito.it/rsctx#Warm>
        a           <http://softeng.polito.it/rsctx#Temperature> , owl:NamedIndividual ;
        rdfs:label  "Warm"@en .

<http://softeng.polito.it/rsctx#Partner>
        a                owl:Class ;
        rdfs:comment     "The user is with her/his boyfriend/girlfriend or husband/wife."@en ;
        rdfs:label       "Partner"@en ;
        rdfs:subClassOf  <http://softeng.polito.it/rsctx#Companion> .

<http://softeng.polito.it/rsctx#Purpose>
        a                    owl:Class ;
        rdfs:comment         "The description of a situation that is desired by an Agent, and usually associated to a plan that describes how to actually achieve it. In the context of this ontology, it indicates the purpose of the item to be recommended. E.g. the user may be interested in receiving recommendation of movies for educating about a specific topic (for instance in the case of a teacher, which wants to show a movie in class) or for having fun (see a movie with some friends in the night)."@en , "Purpose"@en ;
        owl:equivalentClass  <http://www.ontologydesignpatterns.org/ont/dul/DUL.owl#Goal> .

<http://softeng.polito.it/rsctx#Moderate>
        a           <http://softeng.polito.it/rsctx#TrafficLevel> , owl:NamedIndividual ;
        rdfs:label  "Moderate"@en .

<http://softeng.polito.it/rsctx#19>
        a       <http://softeng.polito.it/rsctx#Hour> , owl:NamedIndividual .

<http://softeng.polito.it/rsctx#floor>
        a             owl:FunctionalProperty , owl:ObjectProperty ;
        rdfs:comment  "It indicates the Floor of a Location."@en ;
        rdfs:domain   <http://ns.inria.fr/prissma/v2#POI> ;
        rdfs:label    "floor"@en ;
        rdfs:range    <http://vocab.deri.ie/rooms#Floor> .

<http://softeng.polito.it/rsctx#AdministrativeRegion>
        a                owl:Class ;
        rdfs:comment     "A  specific type of subnational entity in a number of countries, e.g. Belgium, Italy, France."@en ;
        rdfs:label       "Administrative Region"@en ;
        rdfs:subClassOf  <http://softeng.polito.it/rsctx#Region> .

<http://softeng.polito.it/rsctx#nervousness>
        a           <http://softeng.polito.it/rsctx#MentalState> , owl:NamedIndividual ;
        rdfs:label  "nervousness"@en .

<http://softeng.polito.it/rsctx#hate>
        a           <http://softeng.polito.it/rsctx#EmotionalState> , owl:NamedIndividual ;
        rdfs:label  "hate"@en .

<http://softeng.polito.it/rsctx#20>
        a       <http://softeng.polito.it/rsctx#Hour> , owl:NamedIndividual .

[ a            owl:AllDisjointClasses ;
  owl:members  ( <http://softeng.polito.it/rsctx#DayOfWeek> <http://softeng.polito.it/rsctx#PartOfDay> <http://softeng.polito.it/rsctx#Season> )
] .

<http://softeng.polito.it/rsctx#time>
        a                   owl:FunctionalProperty , owl:ObjectProperty ;
        rdfs:comment        "It indicates the time associated to the Environment."@en ;
        rdfs:domain         <http://ns.inria.fr/prissma/v2#Environment> ;
        rdfs:label          "time"@en ;
        rdfs:range          <http://softeng.polito.it/rsctx#Time> ;
        rdfs:subPropertyOf  <http://purl.org/ontology/ao/core#time> .

<http://softeng.polito.it/rsctx#district>
        a             owl:FunctionalProperty , owl:ObjectProperty ;
        rdfs:comment  "It indicates the District of a Location."@en ;
        rdfs:domain   <http://ns.inria.fr/prissma/v2#POI> ;
        rdfs:label    "district"@en ;
        rdfs:range    <http://rdfs.co/juso/District> .

<http://softeng.polito.it/rsctx#hasFitness>
        a             owl:FunctionalProperty , owl:ObjectProperty ;
        rdfs:comment  "This property indicates the fitness of a user."@en ;
        rdfs:domain   <http://ns.inria.fr/prissma/v2#User> ;
        rdfs:label    "has fitness"@en ;
        rdfs:range    <http://softeng.polito.it/rsctx#Fitness> .

<http://softeng.polito.it/rsctx#PublicPlace>
        a                owl:Class ;
        rdfs:comment     "A public place such as a cinema or a theatre.\n\nWARNING It is a class and not an individual because the individual can be a specific cinema or theatre (e.g. La Scala theatre in Milan)."@en ;
        rdfs:label       "Public Place"@en ;
        rdfs:subClassOf  <http://softeng.polito.it/rsctx#SymbolicLocation> .

<http://softeng.polito.it/rsctx#sadness>
        a           <http://softeng.polito.it/rsctx#EmotionalState> , owl:NamedIndividual ;
        rdfs:label  "sadness"@en .

<http://softeng.polito.it/rsctx#Bike>
        a           <http://softeng.polito.it/rsctx#TransportationMean> , owl:NamedIndividual ;
        rdfs:label  "Bike"@en , "Bicycle"@en .

<http://softeng.polito.it/rsctx#02>
        a       <http://softeng.polito.it/rsctx#Hour> , owl:NamedIndividual .

<http://softeng.polito.it/rsctx#hasPurpose>
        a                   owl:ObjectProperty ;
        rdfs:comment        "This property indicates the purpose of a user.\n\nWARNING schema:purpose has different domain (three possible classes) and different ranges (2 possible classes). Although one range is Thing, which would enable to consider this porperty as subproperty of schema.org we should add a class in domain, while for the scopes of this ontology only Environment as domain is proper. "@en ;
        rdfs:domain         <http://ns.inria.fr/prissma/v2#Environment> ;
        rdfs:label          "has purpose"@en ;
        rdfs:range          <http://softeng.polito.it/rsctx#Purpose> ;
        rdfs:seeAlso        "https://schema.org/purpose" , "http://dbpedia.org/ontology/purpose" ;
        rdfs:subPropertyOf  owl:topObjectProperty .

<http://softeng.polito.it/rsctx#province>
        a             owl:FunctionalProperty , owl:ObjectProperty ;
        rdfs:comment  "province"@en , "It indicates the Proince of a Location."@en ;
        rdfs:domain   <http://ns.inria.fr/prissma/v2#POI> ;
        rdfs:range    <http://rdfs.co/juso/Province> .

<http://softeng.polito.it/rsctx#TimeInterval>
        a                owl:Class ;
        rdfs:comment     "A period of time between two instants."@en ;
        rdfs:label       "Time Interval"@en ;
        rdfs:subClassOf  <http://www.w3.org/2006/time#ProperInterval> .

<http://softeng.polito.it/rsctx#14>
        a       <http://softeng.polito.it/rsctx#Hour> , owl:NamedIndividual .

<http://softeng.polito.it/rsctx#GeographicalRegion>
        a                owl:Class ;
        rdfs:comment     "A physical or historical region. Such as the Iberian peninsula or the Northwest European Atlantic Protestant Region (i.e. the European \"source regions\" in early American colonization efforts)."@en ;
        rdfs:label       "Geographical Region"@en ;
        rdfs:subClassOf  <http://softeng.polito.it/rsctx#Region> .

<http://softeng.polito.it/rsctx#great>
        a           <http://softeng.polito.it/rsctx#Fitness> , owl:NamedIndividual ;
        rdfs:label  "great"@en .

<http://softeng.polito.it/rsctx#hour>
        a             owl:FunctionalProperty , owl:ObjectProperty ;
        rdfs:comment  "This property indicates the hour which a Time is included."@en ;
        rdfs:domain   <http://softeng.polito.it/rsctx#Time> ;
        rdfs:label    "hour"@en ;
        rdfs:range    <http://softeng.polito.it/rsctx#Hour> .

<http://softeng.polito.it/rsctx#WetSeason>
        a           <http://softeng.polito.it/rsctx#Season> , owl:NamedIndividual ;
        rdfs:label  "Wet Season"@en , "Rainy Season"@en , "Monsoon Season"@en .

<http://softeng.polito.it/rsctx#NoTrasportationMean>
        a           <http://softeng.polito.it/rsctx#TransportationMean> , owl:NamedIndividual ;
        rdfs:label  "No transportation mean"@en .

<http://softeng.polito.it/rsctx#DrySeason>
        a           <http://softeng.polito.it/rsctx#Season> , owl:NamedIndividual ;
        rdfs:label  "Dry Season"@en .

<http://softeng.polito.it/rsctx#parish>
        a             owl:FunctionalProperty , owl:ObjectProperty ;
        rdfs:comment  "parish"@en , "It indicates the Parish of a Location."@en ;
        rdfs:domain   <http://ns.inria.fr/prissma/v2#POI> ;
        rdfs:range    <http://rdfs.co/juso/Parish> .

<http://softeng.polito.it/rsctx#noiseLevel>
        a             owl:FunctionalProperty , owl:ObjectProperty ;
        rdfs:comment  "It indicates a NoiseLevel"@en ;
        rdfs:domain   <http://ns.inria.fr/prissma/v2#Environment> ;
        rdfs:label    "noise level"@en ;
        rdfs:range    <http://softeng.polito.it/rsctx#NoiseLevel> .

<http://softeng.polito.it/rsctx#device>
        a                   owl:FunctionalProperty , owl:ObjectProperty ;
        rdfs:comment        "The property associates a Device to a Context.\n\nWARNING It is useful only if we need the property being functional, otherwise prissma:device should be used."@en ;
        rdfs:domain         <http://ns.inria.fr/prissma/v2#Context> ;
        rdfs:label          "device"@en ;
        rdfs:range          <http://ns.inria.fr/prissma/v2#Device> ;
        rdfs:subPropertyOf  <http://ns.inria.fr/prissma/v2#device> .

<http://softeng.polito.it/rsctx#bloodPressure>
        a             owl:FunctionalProperty , owl:DatatypeProperty ;
        rdfs:comment  "This property indicates the blood pressure (in mmHg) of a PhysiologicalState"@en ;
        rdfs:domain   <http://softeng.polito.it/rsctx#PhysiologicalState> ;
        rdfs:label    "blood preassure"@en ;
        rdfs:range    [ a                     rdfs:Datatype ;
                        owl:onDatatype        xsd:int ;
                        owl:withRestrictions  ( [ xsd:minExclusive
                                          0 ] )
                      ] .

<http://softeng.polito.it/rsctx#satisfaction>
        a           <http://softeng.polito.it/rsctx#EmotionalState> , owl:NamedIndividual ;
        rdfs:label  "satisfaction"@en .

<http://softeng.polito.it/rsctx#bodyTemperature>
        a             owl:FunctionalProperty , owl:DatatypeProperty ;
        rdfs:comment  "This property indicates the temperature (in degree Celsius) of a PhysiologicalState."@en ;
        rdfs:domain   <http://softeng.polito.it/rsctx#PhysiologicalState> ;
        rdfs:label    "body temperature"@en ;
        rdfs:range    [ a                     rdfs:Datatype ;
                        owl:onDatatype        xsd:decimal ;
                        owl:withRestrictions  ( [ xsd:minExclusive
                                          0 ] )
                      ] .

<http://softeng.polito.it/rsctx#irritation>
        a           <http://softeng.polito.it/rsctx#MentalState> , owl:NamedIndividual ;
        rdfs:label  "irritation"@en .

<http://softeng.polito.it/rsctx#08>
        a       <http://softeng.polito.it/rsctx#Hour> , owl:NamedIndividual .

<http://softeng.polito.it/rsctx#budget>
        a             owl:FunctionalProperty , owl:DatatypeProperty ;
        rdfs:comment  "It indicates how much the user want or can spend (for example for a travel or a purchase or to go for a dinner in a restaurant)."@en ;
        rdfs:domain   <http://ns.inria.fr/prissma/v2#Environment> ;
        rdfs:label    "budget"@en ;
        rdfs:range    [ a                     rdfs:Datatype ;
                        owl:onDatatype        xsd:decimal ;
                        owl:withRestrictions  ( [ xsd:minExclusive
                                          0 ] )
                      ] .

<http://softeng.polito.it/rsctx#TrafficLevel>
        a                    owl:Class ;
        rdfs:comment         "This class represents the current traffic situation."@en ;
        rdfs:label           "Traffic Level"@en ;
        owl:equivalentClass  [ a          owl:Class ;
                               owl:oneOf  ( <http://softeng.polito.it/rsctx#Moderate> <http://softeng.polito.it/rsctx#Chaotic> <http://softeng.polito.it/rsctx#Calm> )
                             ] .

<http://softeng.polito.it/rsctx#joy>
        a           <http://softeng.polito.it/rsctx#EmotionalState> , owl:NamedIndividual ;
        rdfs:label  "joy"@en .

<http://softeng.polito.it/rsctx#sleepy>
        a           <http://softeng.polito.it/rsctx#Fitness> , owl:NamedIndividual ;
        rdfs:label  "sleepy"@en .

<http://softeng.polito.it/rsctx#city>
        a             owl:FunctionalProperty , owl:ObjectProperty ;
        rdfs:comment  "It indicates the city of a Location."@en ;
        rdfs:domain   <http://ns.inria.fr/prissma/v2#POI> ;
        rdfs:label    "city"@en ;
        rdfs:range    <http://rdfs.co/juso/City> .

<http://softeng.polito.it/rsctx#Car>
        a           <http://softeng.polito.it/rsctx#TransportationMean> , owl:NamedIndividual ;
        rdfs:label  "Car"@en .

<http://softeng.polito.it/rsctx#address>
        a             owl:FunctionalProperty , owl:DatatypeProperty ;
        rdfs:comment  "It indicates the address of a location"@en ;
        rdfs:domain   <http://ns.inria.fr/prissma/v2#POI> ;
        rdfs:label    "address"@en ;
        rdfs:range    xsd:string .

<http://softeng.polito.it/rsctx#21>
        a       <http://softeng.polito.it/rsctx#Hour> , owl:NamedIndividual .

<http://softeng.polito.it/rsctx#Winter>
        a           <http://softeng.polito.it/rsctx#Season> , owl:NamedIndividual ;
        rdfs:label  "Winter"@en .

<http://softeng.polito.it/rsctx#psychopathy>
        a           <http://softeng.polito.it/rsctx#MentalState> , owl:NamedIndividual ;
        rdfs:label  "psychopathy"@en .

<http://softeng.polito.it/rsctx#confusion>
        a           <http://softeng.polito.it/rsctx#EmotionalState> , owl:NamedIndividual ;
        rdfs:label  "confusion"@en .

<http://softeng.polito.it/rsctx#disgust>
        a           <http://softeng.polito.it/rsctx#EmotionalState> , owl:NamedIndividual ;
        rdfs:label  "disgust"@en .

<http://softeng.polito.it/rsctx#fatigue>
        a             owl:FunctionalProperty , owl:DatatypeProperty ;
        rdfs:comment  "This property indicates the fatigue of a PhysiologicalState. It is represented as string because there are scales such as Samm-Perelli seven point scale and karolinska sleepiness scale with some numbers associated to a string. "@en ;
        rdfs:domain   <http://softeng.polito.it/rsctx#PhysiologicalState> ;
        rdfs:label    "fatigue"@en ;
        rdfs:range    xsd:string .

<http://softeng.polito.it/rsctx#ill>
        a           <http://softeng.polito.it/rsctx#Fitness> , owl:NamedIndividual ;
        rdfs:label  "ill"@en .

<http://softeng.polito.it/rsctx#03>
        a       <http://softeng.polito.it/rsctx#Hour> , owl:NamedIndividual .

<http://softeng.polito.it/rsctx#Child>
        a                owl:Class ;
        rdfs:comment     "The user is with children, not necessarily his family: for example may be a teacher or a baby sitter."@en ;
        rdfs:label       "Kid"@en , "Child"@en ;
        rdfs:subClassOf  <http://softeng.polito.it/rsctx#Companion> .

<http://softeng.polito.it/rsctx#Pleasure>
        a                owl:Class ;
        rdfs:subClassOf  <http://ns.inria.fr/emoca#Component> .

<http://softeng.polito.it/rsctx#Cool>
        a           <http://softeng.polito.it/rsctx#Temperature> , owl:NamedIndividual ;
        rdfs:label  "Cool"@en .

<http://softeng.polito.it/rsctx#Dominance>
        a                owl:Class ;
        rdfs:subClassOf  <http://ns.inria.fr/emoca#Component> .

<http://softeng.polito.it/rsctx#federatedState>
        a             owl:FunctionalProperty , owl:ObjectProperty ;
        rdfs:comment  "It indicates the FederatedState of a Location."@en ;
        rdfs:domain   <http://ns.inria.fr/prissma/v2#POI> ;
        rdfs:label    "federated state"@en ;
        rdfs:range    <http://rdfs.co/juso/FederatedState> .

<http://softeng.polito.it/rsctx#15>
        a       <http://softeng.polito.it/rsctx#Hour> , owl:NamedIndividual .

<http://softeng.polito.it/rsctx#Afternoon>
        a             <http://softeng.polito.it/rsctx#PartOfDay> , owl:NamedIndividual ;
        rdfs:comment  "The time of the day between noon and evening. The mapping with respect the hours is possible but not defined because it may vary with the location and the habits."@en ;
        rdfs:label    "Afternoon"@en .

<http://softeng.polito.it/rsctx#WeekEnd>
        a                    owl:Class ;
        rdfs:comment         "This class indicates the days which made up the weekend (typically not working)."@en ;
        rdfs:label           "Weekend"@en ;
        rdfs:subClassOf      <http://softeng.polito.it/rsctx#DayOfWeek> ;
        owl:disjointWith     <http://softeng.polito.it/rsctx#Weekday> ;
        owl:equivalentClass  [ a          owl:Class ;
                               owl:oneOf  ( <http://www.w3.org/2006/time#Sunday> <http://www.w3.org/2006/time#Saturday> )
                             ] .

<http://softeng.polito.it/rsctx#Weekday>
        a                    owl:Class ;
        rdfs:comment         "This class includes the day of the week which are typically working (if is not holiday). Days from Monday to Friday are weekdays."@en ;
        rdfs:label           "Weekday"@en ;
        rdfs:subClassOf      <http://softeng.polito.it/rsctx#DayOfWeek> ;
        owl:equivalentClass  [ a          owl:Class ;
                               owl:oneOf  ( <http://www.w3.org/2006/time#Monday> <http://www.w3.org/2006/time#Wednesday> <http://www.w3.org/2006/time#Thursday> <http://www.w3.org/2006/time#Friday> <http://www.w3.org/2006/time#Tuesday> )
                             ] .

<http://softeng.polito.it/rsctx#weak>
        a           <http://softeng.polito.it/rsctx#Fitness> , owl:NamedIndividual ;
        rdfs:label  "weak"@en .

<http://softeng.polito.it/rsctx#nourishment>
        a             owl:FunctionalProperty , owl:DatatypeProperty ;
        rdfs:comment  "This property indicates the nourishment (in BMI) of a PhysiologicalState."@en ;
        rdfs:domain   <http://softeng.polito.it/rsctx#PhysiologicalState> ;
        rdfs:label    "nourishment"@en ;
        rdfs:range    [ a                     rdfs:Datatype ;
                        owl:onDatatype        xsd:decimal ;
                        owl:withRestrictions  ( [ xsd:minExclusive
                                          0 ] )
                      ] .

<http://softeng.polito.it/rsctx#09>
        a       <http://softeng.polito.it/rsctx#Hour> , owl:NamedIndividual .

<http://softeng.polito.it/rsctx#activity>
        a                   owl:ObjectProperty ;
        rdfs:comment        "This property indicates the activity of a user.\n\nWARNING Useful only if need domain and ranges, otherwise it is enough to use ao:activity."@en ;
        rdfs:domain         <http://ns.inria.fr/prissma/v2#Environment> ;
        rdfs:label          "activity"@en ;
        rdfs:range          <http://ns.inria.fr/prissma/v2#Activity> ;
        rdfs:subPropertyOf  <http://purl.org/ontology/ao/core#activity> .

<http://softeng.polito.it/rsctx#pupilsDilation>
        a             owl:FunctionalProperty , owl:DatatypeProperty ;
        rdfs:comment  "This property indicates the pupil dilation (in mm) of a PhysiologicalState."@en ;
        rdfs:domain   <http://softeng.polito.it/rsctx#PhysiologicalState> ;
        rdfs:label    "pupil dilation"@en ;
        rdfs:range    [ a                     rdfs:Datatype ;
                        owl:onDatatype        xsd:int ;
                        owl:withRestrictions  ( [ xsd:minExclusive
                                          0 ] )
                      ] .

<http://softeng.polito.it/rsctx#heartbeat>
        a                   owl:FunctionalProperty , owl:DatatypeProperty ;
        rdfs:comment        "This property indicates the heartbeat of a PhysiologicalState"@en ;
        rdfs:domain         <http://softeng.polito.it/rsctx#PhysiologicalState> ;
        rdfs:label          "heartbeat"@en ;
        rdfs:range          [ a                     rdfs:Datatype ;
                              owl:onDatatype        xsd:int ;
                              owl:withRestrictions  ( [ xsd:minExclusive
                                                0 ] )
                            ] ;
        rdfs:subPropertyOf  owl:topDataProperty .

<http://softeng.polito.it/rsctx#Morning>
        a             <http://softeng.polito.it/rsctx#PartOfDay> , owl:NamedIndividual ;
        rdfs:comment  "The period of time between midnight and noon or, more commonly, the interval between sunrise and noon."@en ;
        rdfs:label    "Morning"@en .

<http://softeng.polito.it/rsctx#10>
        a       <http://softeng.polito.it/rsctx#Hour> , owl:NamedIndividual .

<http://softeng.polito.it/rsctx#Time>
        a                owl:Class ;
        rdfs:comment     "Time is an instant, i.e. a timestamp. Then it can be characterized by some TimeIntervals which it belongs to, such as winter, Monday and morning."@en ;
        rdfs:label       "Time"@en ;
        rdfs:subClassOf  <http://www.w3.org/2006/time#Instant> .

<http://softeng.polito.it/rsctx#timePressure>
        a           <http://softeng.polito.it/rsctx#MentalState> , owl:NamedIndividual ;
        rdfs:label  "time pressure"@en .

<http://softeng.polito.it/rsctx#PhysiologicalState>
        a                    owl:Class ;
        rdfs:comment         "The state of the body or bodily functions.\n\nWARNING The subclasses of PhysiologicalState in GUMO ontology  are represented as datatype properties."@en ;
        rdfs:label           "Physiological State"@en ;
        owl:equivalentClass  <http://gumo.org/2.0/#PhysiologicalState.700016> .

<http://softeng.polito.it/rsctx#Boss>
        a                owl:Class ;
        rdfs:comment     "The user is with his boss. This may be a more formal situation that being with just the colleagues."@en ;
        rdfs:label       "Supervisor"@en , "Superior"@en , "Manager"@en , "Chief"@en , "Boss"@en ;
        rdfs:subClassOf  <http://softeng.polito.it/rsctx#Companion> .

<http://softeng.polito.it/rsctx#anger>
        a           <http://softeng.polito.it/rsctx#EmotionalState> , owl:NamedIndividual ;
        rdfs:label  "anger"@en .

<http://softeng.polito.it/rsctx#partOfDay>
        a             owl:FunctionalProperty , owl:ObjectProperty ;
        rdfs:comment  "This property indicates part of the day in which a Time is included in."@en ;
        rdfs:domain   <http://softeng.polito.it/rsctx#Time> ;
        rdfs:label    "part of day"@en ;
        rdfs:range    <http://softeng.polito.it/rsctx#PartOfDay> .

<http://softeng.polito.it/rsctx#room>
        a             owl:FunctionalProperty , owl:ObjectProperty ;
        rdfs:comment  "It indicates the Room of a Location."@en ;
        rdfs:domain   <http://ns.inria.fr/prissma/v2#POI> ;
        rdfs:label    "room"@en ;
        rdfs:range    <http://vocab.deri.ie/rooms#Room> .

<http://softeng.polito.it/rsctx#22>
        a       <http://softeng.polito.it/rsctx#Hour> , owl:NamedIndividual .

<http://softeng.polito.it/rsctx#DayOfWeek>
        a                owl:Class ;
        rdfs:comment     "This class indicates the day of the week (such as Monday, Tuesday, etc.)."@en ;
        rdfs:label       "Day Of Week"@en ;
        rdfs:subClassOf  <http://www.w3.org/2006/time#DayOfWeek> , <http://softeng.polito.it/rsctx#TimeInterval> .

<http://softeng.polito.it/rsctx#noise>
        a             owl:FunctionalProperty , owl:DatatypeProperty ;
        rdfs:comment  "It indicates the noise in decibel."@en ;
        rdfs:domain   <http://ns.inria.fr/prissma/v2#Environment> ;
        rdfs:label    "noise"@en ;
        rdfs:range    [ a                     rdfs:Datatype ;
                        owl:onDatatype        xsd:decimal ;
                        owl:withRestrictions  ( [ xsd:minExclusive
                                          0 ] )
                      ] .

<http://softeng.polito.it/rsctx#Calm>
        a           <http://softeng.polito.it/rsctx#TrafficLevel> , owl:NamedIndividual ;
        rdfs:label  "Calm"@en .

<http://softeng.polito.it/rsctx#hope>
        a           <http://softeng.polito.it/rsctx#EmotionalState> , owl:NamedIndividual ;
        rdfs:label  "hope"@en .

<http://softeng.polito.it/rsctx#LightLevel>
        a             owl:Class ;
        rdfs:comment  "This class represent the current level of light. It is intended some symbolic level such as dark, sunlight, etc."@en ;
        rdfs:label    "Light Level"@en .

<http://softeng.polito.it/rsctx#04>
        a       <http://softeng.polito.it/rsctx#Hour> , owl:NamedIndividual .

<http://softeng.polito.it/rsctx#Hour>
        a                    owl:Class ;
        rdfs:comment         "The hours of a day."@en ;
        rdfs:label           "Hour"@en ;
        rdfs:subClassOf      <http://softeng.polito.it/rsctx#TimeInterval> ;
        owl:equivalentClass  [ a          owl:Class ;
                               owl:oneOf  ( <http://softeng.polito.it/rsctx#18> <http://softeng.polito.it/rsctx#19> <http://softeng.polito.it/rsctx#14> <http://softeng.polito.it/rsctx#15> <http://softeng.polito.it/rsctx#16> <http://softeng.polito.it/rsctx#17> <http://softeng.polito.it/rsctx#10> <http://softeng.polito.it/rsctx#11> <http://softeng.polito.it/rsctx#12> <http://softeng.polito.it/rsctx#13> <http://softeng.polito.it/rsctx#07> <http://softeng.polito.it/rsctx#08> <http://softeng.polito.it/rsctx#09> <http://softeng.polito.it/rsctx#20> <http://softeng.polito.it/rsctx#03> <http://softeng.polito.it/rsctx#04> <http://softeng.polito.it/rsctx#05> <http://softeng.polito.it/rsctx#06> <http://softeng.polito.it/rsctx#21> <http://softeng.polito.it/rsctx#00> <http://softeng.polito.it/rsctx#22> <http://softeng.polito.it/rsctx#01> <http://softeng.polito.it/rsctx#23> <http://softeng.polito.it/rsctx#02> )
                             ] .

<http://softeng.polito.it/rsctx#ZIPCode>
        a             owl:FunctionalProperty , owl:DatatypeProperty ;
        rdfs:comment  "It indicates the ZIP code of a Location."@en ;
        rdfs:domain   <http://ns.inria.fr/prissma/v2#POI> ;
        rdfs:label    "postal code"@en , "ZIP code"@en ;
        rdfs:range    xsd:string .

<http://softeng.polito.it/rsctx#trauma>
        a           <http://softeng.polito.it/rsctx#MentalState> , owl:NamedIndividual ;
        rdfs:label  "trauma"@en .

<http://softeng.polito.it/rsctx#environment>
        a                   owl:FunctionalProperty , owl:ObjectProperty ;
        rdfs:comment        "The property associates an Environment to a Context.\n\nWARNING It is useful only if we need the property being functional, otherwise prissma:device should be used."@en ;
        rdfs:domain         <http://ns.inria.fr/prissma/v2#Context> ;
        rdfs:label          "environment"@en ;
        rdfs:range          <http://ns.inria.fr/prissma/v2#Environment> ;
        rdfs:subPropertyOf  <http://ns.inria.fr/prissma/v2#environment> .

<http://softeng.polito.it/rsctx/arousal>
        a             owl:FunctionalProperty , owl:DatatypeProperty ;
        rdfs:comment  "This property indicates the arousal of a PhysiologicalState."@en ;
        rdfs:domain   <http://softeng.polito.it/rsctx#PhysiologicalState> ;
        rdfs:label    "arousal"@en ;
        rdfs:range    xsd:string .

<http://softeng.polito.it/rsctx#fear>
        a           <http://softeng.polito.it/rsctx#EmotionalState> , owl:NamedIndividual ;
        rdfs:label  "fear"@en .

<http://softeng.polito.it/rsctx#Motion>
        a                    owl:Class ;
        rdfs:comment         "This class indicates if the user is moving and how, e.g. if he is walking or running."@en ;
        rdfs:label           "Motion" ;
        owl:equivalentClass  <http://gumo.org/2.0/#Motion.700018> .

<http://softeng.polito.it/rsctx#16>
        a       <http://softeng.polito.it/rsctx#Hour> , owl:NamedIndividual .

<http://softeng.polito.it/rsctx#hasEmotionalState>
        a             owl:ObjectProperty ;
        rdfs:comment  "This property indicates the emotional state of a user."@en ;
        rdfs:domain   <http://ns.inria.fr/prissma/v2#User> ;
        rdfs:label    "has emotional state"@en ;
        rdfs:range    <http://softeng.polito.it/rsctx#EmotionalState> .

<http://softeng.polito.it/rsctx#lightLevel>
        a             owl:FunctionalProperty , owl:ObjectProperty ;
        rdfs:comment  "It indicates a LightLevel."@en ;
        rdfs:domain   <http://ns.inria.fr/prissma/v2#Environment> ;
        rdfs:label    "light level"@en ;
        rdfs:range    <http://softeng.polito.it/rsctx#LightLevel> .

<http://softeng.polito.it/rsctx#BusinessPartner>
        a                owl:Class ;
        rdfs:comment     "The user is with a business partner, e.g. a business partner can be a customer or a member of another organizations with which the user is collaborating or a supplier."@en ;
        rdfs:label       "Business Partner"@en ;
        rdfs:subClassOf  <http://softeng.polito.it/rsctx#Companion> .

<http://softeng.polito.it/rsctx#bulding>
        a             owl:FunctionalProperty , owl:ObjectProperty ;
        rdfs:comment  "It indicates the building associated to a location."@en ;
        rdfs:domain   <http://ns.inria.fr/prissma/v2#POI> ;
        rdfs:label    "building"@en ;
        rdfs:range    <http://vocab.deri.ie/rooms#Building> .

<http://softeng.polito.it/rsctx#desk>
        a             owl:FunctionalProperty , owl:ObjectProperty ;
        rdfs:comment  "It indicates the Desk of a Location."@en ;
        rdfs:domain   <http://ns.inria.fr/prissma/v2#POI> ;
        rdfs:label    "desk"@en ;
        rdfs:range    <http://vocab.deri.ie/rooms#Desk> .

<http://softeng.polito.it/rsctx#CompanionHome>
        a                owl:Class ;
        rdfs:comment     "The home of a companion of the user, such as a freind's home or a colleague's home.\n\nWARNING This piece of information can be hard to obtained (unless explicitly asked to the user). It is a class and not an individual because the individual is the specific house (e.g. my friend Bob's house)."@en ;
        rdfs:label       "Comapanion's Home"@en ;
        rdfs:subClassOf  <http://softeng.polito.it/rsctx#SymbolicLocation> .

<http://softeng.polito.it/rsctx#Evening>
        a             <http://softeng.polito.it/rsctx#PartOfDay> , owl:NamedIndividual ;
        rdfs:comment  "The period of time near the end of the day, from the end of afternoon (usually from 6 PM) to nighttime. The mapping with respect the hours is possible but not defined becaus it may vary with the location and the habits."@en ;
        rdfs:label    "Evening"@en .

<http://softeng.polito.it/rsctx#trance>
        a           <http://softeng.polito.it/rsctx#MentalState> , owl:NamedIndividual ;
        rdfs:label  "trance"@en .

<http://softeng.polito.it/rsctx#neighborhood>
        a             owl:FunctionalProperty , owl:ObjectProperty ;
        rdfs:comment  "It indicates the Neighborhood of a Location."@en ;
        rdfs:domain   <http://ns.inria.fr/prissma/v2#POI> ;
        rdfs:label    "neighborhood"@en ;
        rdfs:range    <http://rdfs.co/juso/Neighborhood> .

<http://softeng.polito.it/rsctx#TransportationMean>
        a                    owl:Class ;
        rdfs:comment         "It represents the transportation mean the user is using or is going to use (e.g. to reach a restaurant or to visit a city), such as car, bike, public transport or none (he is going on foot)."@en ;
        rdfs:label           "Transportation Mean"@en ;
        owl:equivalentClass  [ a          owl:Class ;
                               owl:oneOf  ( <http://softeng.polito.it/rsctx#Car> <http://softeng.polito.it/rsctx#Bike> <http://softeng.polito.it/rsctx#PublicTransport> <http://softeng.polito.it/rsctx#Taxi> <http://softeng.polito.it/rsctx#NoTrasportationMean> )
                             ] .

<http://softeng.polito.it/rsctx#Chaotic>
        a           <http://softeng.polito.it/rsctx#TrafficLevel> , owl:NamedIndividual ;
        rdfs:label  "Chaotic"@en .

<http://softeng.polito.it/rsctx#availableTime>
        a             owl:FunctionalProperty , owl:ObjectProperty ;
        rdfs:comment  "It indicates how much time the user can spend (e.g. to visit a city or to go for lunch in lunch brek at work)."@en ;
        rdfs:domain   <http://ns.inria.fr/prissma/v2#Environment> ;
        rdfs:label    "available time"@en ;
        rdfs:range    <http://softeng.polito.it/rsctx#TimeInterval> .

<http://softeng.polito.it/rsctx#Friend>
        a                owl:Class ;
        rdfs:comment     "The user is with one or more friends."@en ;
        rdfs:label       "Friend"@en ;
        rdfs:subClassOf  <http://softeng.polito.it/rsctx#Companion> .

<http://softeng.polito.it/rsctx#Mild>
        a           <http://softeng.polito.it/rsctx#Temperature> , owl:NamedIndividual ;
        rdfs:label  "Mild"@en .

<http://softeng.polito.it/rsctx#11>
        a       <http://softeng.polito.it/rsctx#Hour> , owl:NamedIndividual .

<http://softeng.polito.it/rsctx#VeryCold>
        a           <http://softeng.polito.it/rsctx#Temperature> , owl:NamedIndividual ;
        rdfs:label  "Very Cold"@en .

<http://softeng.polito.it/rsctx#Family>
        a                owl:Class ;
        rdfs:comment     "The user is with his family, not necessarely with children. For instance, this may includes being just with the sister or brother or the parents."@en ;
        rdfs:label       "Family"@en ;
        rdfs:subClassOf  <http://softeng.polito.it/rsctx#Companion> .

<http://softeng.polito.it/rsctx#municipality>
        a             owl:FunctionalProperty , owl:ObjectProperty ;
        rdfs:comment  "It indicates the Municipality of a Location."@en ;
        rdfs:domain   <http://ns.inria.fr/prissma/v2#POI> ;
        rdfs:label    "municipality"@en ;
        rdfs:range    <http://rdfs.co/juso/Municipality> .

<http://softeng.polito.it/rsctx#trafficLevel>
        a             owl:FunctionalProperty , owl:ObjectProperty ;
        rdfs:comment  "It indicates a TrafficLevel"@en ;
        rdfs:domain   <http://ns.inria.fr/prissma/v2#Environment> ;
        rdfs:label    "traffic level"@en ;
        rdfs:range    <http://softeng.polito.it/rsctx#TrafficLevel> .

<http://softeng.polito.it/rsctx#EmotionalState>
        a                    owl:Class ;
        rdfs:comment         "The state of a person's emotions (especially with regard to pleasure or dejection).\n\nWARNING The possible values are represented as individuals while in the GUMO ontology are classes."@en ;
        rdfs:label           "Emotional State"@en ;
        rdfs:subClassOf      <http://ns.inria.fr/emoca#Emotion> ;
        owl:equivalentClass  <http://gumo.org/2.0/#EmotionalState.700014> ;
        owl:equivalentClass  [ a          owl:Class ;
                               owl:oneOf  ( <http://softeng.polito.it/rsctx#hope> <http://softeng.polito.it/rsctx#confusion> <http://softeng.polito.it/rsctx#satisfaction> <http://softeng.polito.it/rsctx#pride> <http://softeng.polito.it/rsctx#anxiety> <http://softeng.polito.it/rsctx#relief> <http://softeng.polito.it/rsctx#joy> <http://softeng.polito.it/rsctx#excitement> <http://softeng.polito.it/rsctx#dread> <http://softeng.polito.it/rsctx#sadness> <http://softeng.polito.it/rsctx#anger> <http://softeng.polito.it/rsctx#disgust> <http://softeng.polito.it/rsctx#shame> <http://softeng.polito.it/rsctx#hate> <http://softeng.polito.it/rsctx#happiness> <http://softeng.polito.it/rsctx#fear> <http://softeng.polito.it/rsctx#boredom> <http://softeng.polito.it/rsctx#love> <http://softeng.polito.it/rsctx#worry> )
                             ] .

<http://softeng.polito.it/rsctx#exahust>
        a           <http://softeng.polito.it/rsctx#Fitness> , owl:NamedIndividual ;
        rdfs:label  "exhaust"@en .

<http://softeng.polito.it/rsctx#AnchorPoint>
        a                    owl:Class ;
        rdfs:comment         "It is a key  location,  such  as  our  home  and  work  place,  that  we\nconsider as \"anchor\" in our understanding of the geographic environment\nwhere we live. In general, an anchor-point is a frequently visited location or a location where one spends a lot of time."@en ;
        rdfs:label           "Anchor Point"@en ;
        rdfs:subClassOf      <http://softeng.polito.it/rsctx#SymbolicLocation> ;
        owl:equivalentClass  [ a          owl:Class ;
                               owl:oneOf  ( <http://softeng.polito.it/rsctx#WorkPlace> <http://softeng.polito.it/rsctx#Home> )
                             ] .

<http://softeng.polito.it/rsctx#23>
        a       <http://softeng.polito.it/rsctx#Hour> , owl:NamedIndividual .

<http://softeng.polito.it/rsctx#hasTemperature>
        a                   owl:FunctionalProperty , owl:ObjectProperty ;
        rdfs:comment        "This property indicates a symbolic value for the temperature (such as warm, cold, etc.).\n\nWARNING Although there was already a temperature class and a temperature property (hw:hasExteriorTemperature) in the WeatherOntology, temperature class has been redefined with values more general and not referred to the house (such as below room temperature). Thus this property has the redefined temperature class as a range."@en ;
        rdfs:domain         <https://www.auto.tuwien.ac.at/downloads/thinkhome/ontology/WeatherOntology.owl#WeatherState> ;
        rdfs:label          "has temperature"@en ;
        rdfs:range          <http://softeng.polito.it/rsctx#Temperature> ;
        rdfs:subPropertyOf  <https://www.auto.tuwien.ac.at/downloads/thinkhome/ontology/WeatherOntology.owl#hasWeatherPhenomenon> .

<http://softeng.polito.it/rsctx#05>
        a       <http://softeng.polito.it/rsctx#Hour> , owl:NamedIndividual .

<http://softeng.polito.it/rsctx#weather>
        a             owl:FunctionalProperty , owl:ObjectProperty ;
        rdfs:comment  "It indicates the weather associated to the current context."@en ;
        rdfs:domain   <http://ns.inria.fr/prissma/v2#Environment> ;
        rdfs:label    "weather"@en ;
        rdfs:range    <https://www.auto.tuwien.ac.at/downloads/thinkhome/ontology/WeatherOntology.owl#WeatherState> .

<http://softeng.polito.it/rsctx#injury>
        a             owl:DatatypeProperty ;
        rdfs:comment  "This property indicates the injury of a PhysiologicalState"@en ;
        rdfs:domain   <http://softeng.polito.it/rsctx#PhysiologicalState> ;
        rdfs:label    "injury"@en ;
        rdfs:range    xsd:string .

<http://softeng.polito.it/rsctx#dread>
        a           <http://softeng.polito.it/rsctx#EmotionalState> , owl:NamedIndividual ;
        rdfs:label  "dread"@en .

<http://softeng.polito.it/rsctx#pride>
        a           <http://softeng.polito.it/rsctx#EmotionalState> , owl:NamedIndividual ;
        rdfs:label  "pride"@en .

<http://softeng.polito.it/rsctx#site>
        a             owl:FunctionalProperty , owl:ObjectProperty ;
        rdfs:comment  "It indicates the Site of a Location."@en ;
        rdfs:domain   <http://ns.inria.fr/prissma/v2#POI> ;
        rdfs:label    "site"@en .

<http://softeng.polito.it/rsctx#county>
        a             owl:FunctionalProperty , owl:ObjectProperty ;
        rdfs:comment  "It indicates the county of a Location."@en ;
        rdfs:domain   <http://ns.inria.fr/prissma/v2#POI> ;
        rdfs:label    "county"@en ;
        rdfs:range    <http://rdfs.co/juso/County> .

<http://softeng.polito.it/rsctx#companion>
        a             owl:ObjectProperty ;
        rdfs:comment  "This property indicates who is the current companion of the user, e.g. a friend a family member or a colleague."@en ;
        rdfs:domain   <http://ns.inria.fr/prissma/v2#Environment> ;
        rdfs:label    "companion"@en ;
        rdfs:range    <http://softeng.polito.it/rsctx#Companion> .

<http://softeng.polito.it/rsctx#17>
        a       <http://softeng.polito.it/rsctx#Hour> , owl:NamedIndividual .

[ a            owl:AllDisjointClasses ;
  owl:members  ( <http://softeng.polito.it/rsctx#EmotionalState> <http://softeng.polito.it/rsctx#Fitness> <http://softeng.polito.it/rsctx#MentalState> <http://softeng.polito.it/rsctx#PhysiologicalState> )
] .

<http://softeng.polito.it/rsctx#hasMentalState>
        a             owl:ObjectProperty ;
        rdfs:comment  "This property indicates the mental state of a user."@en ;
        rdfs:domain   <http://ns.inria.fr/prissma/v2#User> ;
        rdfs:label    "has mental state"@en ;
        rdfs:range    <http://softeng.polito.it/rsctx#MentalState> .

<http://softeng.polito.it/rsctx#secondLevelAdministrativeDivision>
        a             owl:FunctionalProperty , owl:ObjectProperty ;
        rdfs:comment  "It indicates the second level administrative division of a Location."@en ;
        rdfs:domain   <http://ns.inria.fr/prissma/v2#POI> ;
        rdfs:label    "second level administrative division"@en ;
        rdfs:range    <http://rdfs.co/juso/SecondLevelAdministrativeDivision> .

<http://softeng.polito.it/rsctx#fifthLevelAdministrativeDivision>
        a             owl:FunctionalProperty , owl:ObjectProperty ;
        rdfs:comment  "It indicates the Fifth Level Administrative DIvision of a Location."@en ;
        rdfs:domain   <http://ns.inria.fr/prissma/v2#POI> ;
        rdfs:label    "fifth level administrative division"@en ;
        rdfs:range    <http://rdfs.co/juso/FifthLevelAdministrativeDivision> .

<http://softeng.polito.it/rsctx#excitement>
        a           <http://softeng.polito.it/rsctx#EmotionalState> , owl:NamedIndividual ;
        rdfs:label  "excitement"@en .

<http://softeng.polito.it/rsctx#love>
        a           <http://softeng.polito.it/rsctx#EmotionalState> , owl:NamedIndividual ;
        rdfs:label  "love"@en .

<http://softeng.polito.it/rsctx#user>
        a                   owl:FunctionalProperty , owl:ObjectProperty ;
        rdfs:comment        "The property associates a User to a Context.\n\nWARNING It is useful only if we need the property being functional, otherwise prissma:user should be used."@en ;
        rdfs:domain         <http://ns.inria.fr/prissma/v2#Context> ;
        rdfs:label          "user"@en ;
        rdfs:range          <http://ns.inria.fr/prissma/v2#User> ;
        rdfs:subPropertyOf  <http://ns.inria.fr/prissma/v2#user> .

<http://softeng.polito.it/rsctx#Fall>
        a           <http://softeng.polito.it/rsctx#Season> , owl:NamedIndividual ;
        rdfs:label  "Fall"@en , "Autumn"@en .

[ a            owl:AllDisjointClasses ;
  owl:members  ( <http://ns.inria.fr/emoca#Arousal> <http://ns.inria.fr/emoca#Valence> <http://softeng.polito.it/rsctx#Dominance> <http://softeng.polito.it/rsctx#Pleasure> )
] .

<http://softeng.polito.it/rsctx#boredom>
        a           <http://softeng.polito.it/rsctx#EmotionalState> , owl:NamedIndividual ;
        rdfs:label  "boredom"@en .

<http://softeng.polito.it/rsctx#happiness>
        a           <http://softeng.polito.it/rsctx#EmotionalState> , owl:NamedIndividual ;
        rdfs:label  "happiness"@en .

<http://softeng.polito.it/rsctx#hasMotion>
        a                   owl:FunctionalProperty , owl:ObjectProperty ;
        rdfs:comment        "This property indicates the motion of a user.\n\nWARNING Useful only if need domain and ranges, otherwise it is enough to use ao:activity."@en ;
        rdfs:domain         <http://ns.inria.fr/prissma/v2#Environment> ;
        rdfs:label          "has motion"@en ;
        rdfs:range          <http://softeng.polito.it/rsctx#Motion> ;
        rdfs:subPropertyOf  <http://ns.inria.fr/prissma/v2#string> .

<http://softeng.polito.it/rsctx#poi>
        a                   owl:FunctionalProperty , owl:ObjectProperty ;
        rdfs:comment        "The property associates a POI to a prissma:Environment\n\nWARNING It is useful only if we need the property being functional, otherwise prissma:poi should be used."@en ;
        rdfs:domain         <http://ns.inria.fr/prissma/v2#Environment> ;
        rdfs:label          "poi" ;
        rdfs:range          <http://ns.inria.fr/prissma/v2#POI> ;
        rdfs:subPropertyOf  <http://ns.inria.fr/prissma/v2#poi> .

<http://softeng.polito.it/rsctx#00>
        a       <http://softeng.polito.it/rsctx#Hour> , owl:NamedIndividual .

<http://softeng.polito.it/rsctx#fourthLevelAdministrativeDivision>
        a             owl:FunctionalProperty , owl:ObjectProperty ;
        rdfs:comment  "It indicates the fourth level administrative division of a Location."@en ;
        rdfs:domain   <http://ns.inria.fr/prissma/v2#POI> ;
        rdfs:label    "fourth level administrative division"@en ;
        rdfs:range    <http://rdfs.co/juso/FourthLevelAdministrativeDivision> .

<http://softeng.polito.it/rsctx#MildSeason>
        a           <http://softeng.polito.it/rsctx#Season> , owl:NamedIndividual ;
        rdfs:label  "Mild Season"@en , "Cool season"@en .

<http://softeng.polito.it/rsctx#WorkPlace>
        a           <http://softeng.polito.it/rsctx#AnchorPoint> , owl:NamedIndividual ;
        rdfs:label  "Work Place"@en .

<http://softeng.polito.it/rsctx#Hot>
        a           <http://softeng.polito.it/rsctx#Temperature> , owl:NamedIndividual ;
        rdfs:label  "Hot"@en .

<http://softeng.polito.it/rsctx#Fitness>
        a                    owl:Class ;
        rdfs:comment         "It is a value partition which represents the health of the body, it can be seen as a summary of physiological state, since it is possible to map fitness values with physiological indicators ranges (e.g. ill if temperature greater than a certain threshold), although this is up to the designer which is using the ontology."@en ;
        rdfs:label           "Fitness"@en ;
        owl:equivalentClass  [ a          owl:Class ;
                               owl:oneOf  ( <http://softeng.polito.it/rsctx#good> <http://softeng.polito.it/rsctx#great> <http://softeng.polito.it/rsctx#exahust> <http://softeng.polito.it/rsctx#ill> <http://softeng.polito.it/rsctx#sleepy> <http://softeng.polito.it/rsctx#weak> <http://softeng.polito.it/rsctx#inFit> <http://softeng.polito.it/rsctx#tired> <http://softeng.polito.it/rsctx#injured> )
                             ] .

<http://softeng.polito.it/rsctx#PublicTransport>
        a           <http://softeng.polito.it/rsctx#TransportationMean> , owl:NamedIndividual ;
        rdfs:label  "Public Transport"@en .

<http://softeng.polito.it/rsctx#floorSection>
        a             owl:FunctionalProperty , owl:ObjectProperty ;
        rdfs:comment  "It indicates the FloorSection of a Location."@en ;
        rdfs:domain   <http://ns.inria.fr/prissma/v2#POI> ;
        rdfs:label    "floor section"@en ;
        rdfs:range    <http://vocab.deri.ie/rooms#FloorSection> .
