@prefix :      <http://purl.org/olia/ubyCat.owl#> .
@prefix rdfs:  <http://www.w3.org/2000/01/rdf-schema#> .
@prefix system: <http://purl.org/olia/system.owl#> .
@prefix owl:   <http://www.w3.org/2002/07/owl#> .
@prefix xsd:   <http://www.w3.org/2001/XMLSchema#> .
@prefix rdf:   <http://www.w3.org/1999/02/22-rdf-syntax-ns#> .
@prefix skos:  <http://www.w3.org/2004/02/skos/core#> .
@prefix lemon: <http://www.monnet-project.eu/lemon#> .

:hasDefinitionType  a       owl:ObjectProperty ;
        rdfs:label          "definitionType" ;
        rdfs:range          :DefinitionType ;
        rdfs:subPropertyOf  :hasUbyObjectProperty .

:Tense  a                 owl:Class ;
        rdfs:isDefinedBy  "http://www.isocat.org/datcat/DC-3519" ;
        rdfs:label        "tense" ;
        rdfs:subClassOf   :WordFormAttribute .

:pronounDemonstrative
        a                 :PartOfSpeech , owl:NamedIndividual ;
        rdfs:isDefinedBy  "http://www.isocat.org/datcat/DC-1270" ;
        rdfs:label        "pronounDemonstrative" .

:compound  a              :DerivationType , owl:NamedIndividual ;
        rdfs:isDefinedBy  "http://www.isocat.org/datcat/DC-3127" ;
        rdfs:label        "compound" .

:isBreakBefore  a           owl:DatatypeProperty ;
        rdfs:isDefinedBy    "http://www.isocat.org/datcat/DC-4626" ;
        rdfs:label          "isBreakBefore" ;
        rdfs:range          xsd:boolean ;
        rdfs:subPropertyOf  :multiwordFeature .

:objectComplement  a      :GrammaticalFunction , owl:NamedIndividual ;
        rdfs:isDefinedBy  "http://www.isocat.org/datcat/DC-4625" ;
        rdfs:label        "objectComplement" .

:noun   a                 :PartOfSpeech , owl:NamedIndividual ;
        rdfs:isDefinedBy  "http://www.isocat.org/datcat/DC-3347" ;
        rdfs:label        "noun" .

:interjection  a          :PartOfSpeech , owl:NamedIndividual ;
        rdfs:isDefinedBy  "http://www.isocat.org/datcat/DC-1318" ;
        rdfs:label        "interjection" .

:subjectComplement  a     :GrammaticalFunction , owl:NamedIndividual ;
        rdfs:isDefinedBy  "http://www.isocat.org/datcat/DC-4624" ;
        rdfs:label        "subjectComplement" .

:declarativeClause  a     :SyntacticCategory , owl:NamedIndividual ;
        rdfs:isDefinedBy  "http://www.isocat.org/datcat/DC-2300" ;
        rdfs:label        "declarativeClause" .

:nonPredicativeAdjective
        a                 :SyntacticProperty , owl:NamedIndividual ;
        rdfs:isDefinedBy  "http://www.isocat.org/datcat/DC-4618" ;
        rdfs:label        "nonPredicativeAdjective" .

:pronounInterrogative
        a                 :PartOfSpeech , owl:NamedIndividual ;
        rdfs:isDefinedBy  "http://www.isocat.org/datcat/DC-1321" ;
        rdfs:label        "pronounInterrogative" .

:sense  a                       owl:ObjectProperty ;
        rdfs:isDefinedBy        "http://uby.googlecode.com/files/UBY_LMF_0_2_0.dtd" , "http://www.monnet-project.eu/lemon#sense" ;
        rdfs:range              :Sense ;
        owl:equivalentProperty  lemon:sense .

:singular  a              :GrammaticalNumber , owl:NamedIndividual ;
        rdfs:isDefinedBy  "http://www.isocat.org/datcat/DC-252" ;
        rdfs:label        "singular" .

:pronounPossessive  a     :PartOfSpeech , owl:NamedIndividual ;
        rdfs:isDefinedBy  "http://www.isocat.org/datcat/DC-1359" ;
        rdfs:label        "pronounPossessive" .

:Person  a                owl:Class ;
        rdfs:isDefinedBy  "http://www.isocat.org/datcat/DC-3385" ;
        rdfs:label        "person" ;
        rdfs:subClassOf   :WordFormAttribute .

:directObject  a          :GrammaticalFunction , owl:NamedIndividual ;
        rdfs:isDefinedBy  "http://www.isocat.org/datcat/DC-1274" ;
        rdfs:label        "directObject" .

:DerivationalMorphology
        a                owl:Class ;
        rdfs:subClassOf  :LexicalFeature .

:hasSyntacticProperty
        a                   owl:ObjectProperty ;
        rdfs:label          "syntacticProperty" ;
        rdfs:range          :SyntacticProperty ;
        rdfs:subPropertyOf  :hasUbyObjectProperty .

:generator  a               owl:DatatypeProperty ;
        rdfs:isDefinedBy    "http://www.isocat.org/datcat/DC-2511" ;
        rdfs:label          "generator" ;
        rdfs:subPropertyOf  :hasUbyDatatypeProperty .

:genitive  a              :Case , owl:NamedIndividual ;
        rdfs:isDefinedBy  "http://www.isocat.org/datcat/DC-2722" ;
        rdfs:label        "genitive" .

:has_partOfSpeech  a        owl:ObjectProperty ;
        rdfs:isDefinedBy    "http://www.isocat.org/datcat/DC-396" ;
        rdfs:label          "partOfSpeech" ;
        rdfs:subPropertyOf  system:hasFeature .

:coreUnexpressed  a       :CoreType , owl:NamedIndividual ;
        rdfs:isDefinedBy  "http://www.isocat.org/datcat/DC-4464" ;
        rdfs:label        "coreUnexpressed" .

:thatType  a              :Complementizer , owl:NamedIndividual ;
        rdfs:isDefinedBy  "http://www.isocat.org/datcat/DC-4623" ;
        rdfs:label        "thatType" .

:determiner  a            :PartOfSpeech , owl:NamedIndividual ;
        rdfs:isDefinedBy  "http://www.isocat.org/datcat/DC-1272" ;
        rdfs:label        "determiner" .

:hasCoreType  a             owl:ObjectProperty ;
        rdfs:label          "coreType" ;
        rdfs:range          :CoreType ;
        rdfs:subPropertyOf  :hasUbyObjectProperty .

:optionalArgument  a        owl:DatatypeProperty ;
        rdfs:isDefinedBy    "http://www.isocat.org/datcat/DC-4622" ;
        rdfs:label          "optional" ;
        rdfs:range          xsd:boolean ;
        rdfs:subPropertyOf  :hasUbyDatatypeProperty .

lemon:SemanticLabel  a  owl:Class .

:incorporatedSemArg  a      owl:DatatypeProperty , owl:ObjectProperty ;
        rdfs:isDefinedBy    "http://www.isocat.org/datcat/DC-4151" ;
        rdfs:label          "incorporatedSemArg" ;
        rdfs:subPropertyOf  :hasUbyObjectProperty .

:SenseAxisType  a        owl:Class ;
        rdfs:comment     "In Uby-LMF, the attribute senseAxisType of the SenseAxis class indicates, whether the type of linking between to senses or between two synsets. Example values are monolingualSenseAlignment and crosslingualSenseAlignment" ;
        rdfs:label       "senseAxisType" ;
        rdfs:subClassOf  :LinkingFeature .

:DerivationType  a       owl:Class ;
        rdfs:comment     "In UBY-LMF, relType is an attribute of the RelatedForm class which encodes links to derivationally related lexical entries or senses." ;
        rdfs:label       "relType" ;
        rdfs:subClassOf  :DerivationalMorphology ;
        owl:deprecated   true ;
        owl:versionInfo  "It decides the property to use in the mapping, hence deprecated.\nrelType=\"xxx\" is normally uby:xxx\n(with some exceptions, .e.g, relType=\"seeAlso\" is rdfs:seeAlso)" .

:adverbPronominal  a      :PartOfSpeech , owl:NamedIndividual ;
        rdfs:isDefinedBy  "http://www.isocat.org/datcat/DC-2998" ;
        rdfs:label        "adverbPronominal" .

:hasExampleType  a          owl:ObjectProperty ;
        rdfs:label          "exampleType" ;
        rdfs:range          :ExampleType ;
        rdfs:subPropertyOf  :hasUbyObjectProperty .

:bareInfinitive  a        :VerbForm , owl:NamedIndividual ;
        rdfs:isDefinedBy  "http://www.isocat.org/datcat/DC-4163" ;
        rdfs:label        "bareInfinitive" .

:has_WordFormAttribute
        a                   owl:ObjectProperty ;
        rdfs:isDefinedBy    "http://purl.org/olia/ubyCat.owl" ;
        rdfs:label          "WordFormAttribute" ;
        rdfs:subPropertyOf  system:hasFeature .

:hasGrammaticalFunction
        a                   owl:ObjectProperty ;
        rdfs:label          "grammaticalFunction" ;
        rdfs:range          :GrammaticalFunction ;
        rdfs:subPropertyOf  :hasUbyObjectProperty .

:type   a                   owl:DatatypeProperty ;
        rdfs:comment        "Type is an attribute of the UBY-LMF class SemanticLabel. It encodes the name of a SemanticLabel type, e.g.\ntype=semanticField (from WordNet or GermaNet).\nThe label attribute of SemanticLabel holds the corresponding value of the SemanticLabel, e.g. \nlabel=animate (for type=semanticField)." ;
        rdfs:isDefinedBy    "http://www.isocat.org/datcat/DC-1971" ;
        rdfs:label          "type" ;
        rdfs:subPropertyOf  :hasUbyDatatypeProperty ;
        owl:versionInfo     "Should be replaced by the ObjectProperty hasType and the Class Type" .

:LinkingFeature  a       owl:Class ;
        rdfs:subClassOf  :LexicalFeature .

:DictionaryFeature  a    owl:Class ;
        rdfs:subClassOf  :LexicalFeature .

:LexicalEntry  a             owl:Class ;
        rdfs:isDefinedBy     "http://uby.googlecode.com/files/UBY_LMF_0_2_0.dtd" ;
        rdfs:subClassOf      system:UnitOfAnnotation ;
        owl:deprecated       true ;
        owl:equivalentClass  lemon:LexicalEntry ;
        owl:versionInfo      "superseded by lemon:LexicalEntry" .

:subcatFrame  a           :ExampleType , owl:NamedIndividual ;
        rdfs:isDefinedBy  "http://www.isocat.org/datcat/DC-4630" ;
        rdfs:label        "subcatFrame" .

:SyntacticArgument  a     owl:Class ;
        rdfs:isDefinedBy  "http://uby.googlecode.com/files/UBY_LMF_0_2_0.dtd" ;
        rdfs:subClassOf   lemon:Argument , system:UnitOfAnnotation ;
        owl:versionInfo   "see lemon:synArg" .

:affixSuffix  a           :PartOfSpeech , owl:NamedIndividual ;
        rdfs:isDefinedBy  "http://www.isocat.org/datcat/DC-1395" ;
        rdfs:label        "affixSuffix" .

:languageIdentifier  a      owl:DatatypeProperty ;
        rdfs:isDefinedBy    "http://www.isocat.org/datcat/DC-279" ;
        rdfs:label          "languageIdentifier" ;
        rdfs:subPropertyOf  :hasUbyDatatypeProperty ;
        owl:deprecated      true ;
        owl:versionInfo     "replaced by a lang-tag" .

:pronounPersonal  a       :PartOfSpeech , owl:NamedIndividual ;
        rdfs:isDefinedBy  "http://www.isocat.org/datcat/DC-3013" ;
        rdfs:label        "pronounPersonal" .

:prepositionType  a         owl:DatatypeProperty ;
        rdfs:comment        "PrepositionType is an attribute of the UBY-LMF class SyntacticArgument and specifies the particular preposition type (e.g. locative, directional) to be used in prepositional complements.\nThe preposition type is specified in VerbNet." ;
        rdfs:isDefinedBy    "http://www.isocat.org/datcat/DC-4621" ;
        rdfs:label          "prepositionType" ;
        rdfs:subPropertyOf  :hasUbyDatatypeProperty .

:has_degree  a              owl:ObjectProperty ;
        rdfs:label          "degree" ;
        rdfs:range          :Degree ;
        rdfs:subPropertyOf  :has_WordFormAttribute .

:neuter  a                :GrammaticalGender , owl:NamedIndividual ;
        rdfs:isDefinedBy  "http://www.isocat.org/datcat/DC-3336" ;
        rdfs:label        "neuter" .

:adposition  a            :PartOfSpeech , owl:NamedIndividual ;
        rdfs:isDefinedBy  "http://www.isocat.org/datcat/DC-1231" ;
        rdfs:label        "adposition" .

:verbModal  a             :PartOfSpeech , owl:NamedIndividual ;
        rdfs:isDefinedBy  "http://www.isocat.org/datcat/DC-1329" ;
        rdfs:label        "verbModal" .

:accusative  a            :Case , owl:NamedIndividual ;
        rdfs:isDefinedBy  "http://www.isocat.org/datcat/DC-2724" ;
        rdfs:label        "accusative" .

:indefinite  a            :Determiner , owl:NamedIndividual ;
        rdfs:isDefinedBy  "http://www.isocat.org/datcat/DC-1307" ;
        rdfs:label        "indefinite" .

:SyntacticCategory  a     owl:Class ;
        rdfs:isDefinedBy  "http://www.isocat.org/datcat/DC-1506" ;
        rdfs:label        "syntacticCategory" ;
        rdfs:subClassOf   :SyntacticFeature .

:writtenForm  a             owl:DatatypeProperty ;
        rdfs:isDefinedBy    "http://www.isocat.org/datcat/DC-1836" ;
        rdfs:label          "writtenForm" ;
        rdfs:subPropertyOf  :hasUbyDatatypeProperty .

:verbAuxiliary  a         :PartOfSpeech , owl:NamedIndividual ;
        rdfs:isDefinedBy  "http://www.isocat.org/datcat/DC-1244" ;
        rdfs:label        "verbAuxiliary" .

:objectControl  a         :SyntacticProperty , owl:NamedIndividual ;
        rdfs:isDefinedBy  "http://www.isocat.org/datcat/DC-4189" ;
        rdfs:label        "objectControl" .

:taxonomic  a             :RelType , owl:NamedIndividual ;
        rdfs:isDefinedBy  "http://www.isocat.org/datcat/DC-4039" ;
        rdfs:label        "taxonomic" .

:adverbPhrase  a          :SyntacticCategory , owl:NamedIndividual ;
        rdfs:isDefinedBy  "http://www.isocat.org/datcat/DC-2259" ;
        rdfs:label        "adverbPhrase" .

:hasDerivationType  a       owl:ObjectProperty ;
        rdfs:comment        "In UBY-LMF, relType is an attribute of the RelatedForm class which encodes links to derivationally related lexical entries or senses." ;
        rdfs:range          :DerivationType ;
        rdfs:subPropertyOf  :hasUbyObjectProperty ;
        owl:deprecated      true ;
        owl:versionInfo     "It decides the property to use in the mapping, hence deprecated.\nrelType=\"xxx\" is normally uby:xxx\n(with some exceptions, .e.g, relType=\"seeAlso\" is rdfs:seeAlso)" .

:subjectRaising  a        :SyntacticProperty , owl:NamedIndividual ;
        rdfs:isDefinedBy  "http://www.isocat.org/datcat/DC-4188" ;
        rdfs:label        "subjectRaising" .

:extensionalDefinition
        a                 :DefinitionType , owl:NamedIndividual ;
        rdfs:isDefinedBy  "http://www.isocat.org/datcat/DC-171" ;
        rdfs:label        "extensionalDefinition" .

:determinerInterrogative
        a                 :PartOfSpeech , owl:NamedIndividual ;
        rdfs:isDefinedBy  "http://www.isocat.org/datcat/DC-1320" ;
        rdfs:label        "determinerInterrogative" .

:determinerPossessive
        a                 :PartOfSpeech , owl:NamedIndividual ;
        rdfs:isDefinedBy  "http://www.isocat.org/datcat/DC-1357" ;
        rdfs:label        "determinerPossessive" .

:nounCommon  a            :PartOfSpeech , owl:NamedIndividual ;
        rdfs:isDefinedBy  "http://www.isocat.org/datcat/DC-385" ;
        rdfs:label        "nounCommon" .

system:UnitOfAnnotation
        a       owl:Class .

:LexicalAnnotation  a  owl:Class .

:perspectivalized  a        owl:DatatypeProperty ;
        rdfs:isDefinedBy    "http://www.isocat.org/datcat/DC-4391" ;
        rdfs:label          "perspectivalized" ;
        rdfs:range          xsd:boolean ;
        rdfs:subPropertyOf  :hasUbyDatatypeProperty .

:Degree  a                owl:Class ;
        rdfs:isDefinedBy  "http://www.isocat.org/datcat/DC-2779" ;
        rdfs:label        "degree" ;
        rdfs:subClassOf   :WordFormAttribute .

:MonolingualExternalRef
        a                 owl:Class ;
        rdfs:isDefinedBy  "http://www.isocat.org/datcat/DC-1975" ;
        rdfs:label        "monolingualExternalRef" ;
        rdfs:subClassOf   :LexicalFeatureStructure .

:separableParticle  a       owl:DatatypeProperty ;
        rdfs:isDefinedBy    "http://www.isocat.org/datcat/DC-3546" ;
        rdfs:label          "separableParticle" ;
        rdfs:subPropertyOf  :hasUbyDatatypeProperty .

:complement  a            :GrammaticalFunction , owl:NamedIndividual ;
        rdfs:isDefinedBy  "http://www.isocat.org/datcat/DC-1257" ;
        rdfs:label        "complement" .

:plural  a                :GrammaticalNumber , owl:NamedIndividual ;
        rdfs:isDefinedBy  "http://www.isocat.org/datcat/DC-253" ;
        rdfs:label        "plural" .

:Frequency  a            owl:Class ;
        rdfs:comment     "This owl:Class corresponds to the LMF-class Frequency which has been introduced in UBY-LMF as an extension of ISO-LMF." ;
        rdfs:subClassOf  :LexicalFeatureStructure .

lemon:LexicalContext  a  owl:Class ;
        rdfs:subClassOf  :LexicalFeatureStructure .

:imperative  a            :VerbFormMood , owl:NamedIndividual ;
        rdfs:isDefinedBy  "http://www.isocat.org/datcat/DC-1844" ;
        rdfs:label        "imperative" .

:derivationBaseVerb  a    :DerivationType , owl:NamedIndividual ;
        rdfs:isDefinedBy  "http://www.isocat.org/datcat/DC-4614" ;
        rdfs:label        "derivationBaseVerb" .

:prepositionalPhrase  a   :SyntacticCategory , owl:NamedIndividual ;
        rdfs:isDefinedBy  "http://www.isocat.org/datcat/DC-2257" ;
        rdfs:label        "prepositionalPhrase" .

:lexicalized  a             owl:DatatypeProperty ;
        rdfs:isDefinedBy    "http://www.isocat.org/datcat/DC-3295" ;
        rdfs:label          "lexicalized" ;
        rdfs:range          xsd:boolean ;
        rdfs:subPropertyOf  :hasUbyDatatypeProperty .

:whType  a                :Complementizer , owl:NamedIndividual ;
        rdfs:isDefinedBy  "http://www.isocat.org/datcat/DC-2296" ;
        rdfs:label        "whType" .

:pronounIndefinite  a     :PartOfSpeech , owl:NamedIndividual ;
        rdfs:isDefinedBy  "http://www.isocat.org/datcat/DC-1309" ;
        rdfs:label        "pronounIndefinite" .

:hasPosition  a             owl:DatatypeProperty ;
        rdfs:label          "position" ;
        rdfs:subPropertyOf  :hasUbyDatatypeProperty .

:SyntacticProperty  a    owl:Class ;
        rdfs:comment     "Attribute of the UBY-LMF class SubcategorizationFrame." ;
        rdfs:label       "syntacticProperty" ;
        rdfs:subClassOf  :SyntacticFeature .

:has_grammaticalNumber
        a                   owl:ObjectProperty ;
        rdfs:label          "grammaticalNumber" ;
        rdfs:range          :GrammaticalNumber ;
        rdfs:subPropertyOf  :has_WordFormAttribute .

:expletive  a             :SyntacticCategory , owl:NamedIndividual ;
        rdfs:isDefinedBy  "http://www.isocat.org/datcat/DC-3187" ;
        rdfs:label        "expletive" .

:hasUbyObjectProperty
        a                   owl:ObjectProperty ;
        rdfs:comment        "This ObjectProperty could also be named \"hasTypedLexicalFeature\".\nThe current name \"hasUbyObjectProperty\" indicates that it groups Object Properties used in UBY-LMF." ;
        rdfs:subPropertyOf  lemon:property .

:preposition  a             owl:DatatypeProperty ;
        rdfs:comment        "Preposition is an attribute of the UBY-LMF class SyntacticArgument and specifies the particular preposition to be used in prepositional complements that can either be realized as PP or as preposition and subordinate clause.\nExample: That depends on who did it." ;
        rdfs:isDefinedBy    "http://www.isocat.org/datcat/DC-1366" ;
        rdfs:label          "preposition" ;
        rdfs:subPropertyOf  :hasUbyDatatypeProperty .

:Type   a                 owl:Class ;
        rdfs:comment      "Type is an attribute of the UBY-LMF class SemanticLabel. It encodes the name of a SemanticLabel type, e.g.\ntype=semanticField (from WordNet or GermaNet).\nThe label attribute of SemanticLabel holds the corresponding value of the SemanticLabel, e.g. \nlabel=animate (for type=semanticField)." ;
        rdfs:isDefinedBy  "http://www.isocat.org/datcat/DC-1971" ;
        rdfs:label        "type" ;
        rdfs:subClassOf   :MetaFeature ;
        owl:versionInfo   "Should replace the DatatypeProperty type" .

:hasType  a                 owl:ObjectProperty , owl:AnnotationProperty ;
        rdfs:comment        "Type is an attribute of the UBY-LMF class SemanticLabel. It encodes the name of a SemanticLabel type, e.g.\ntype=semanticField (from WordNet or GermaNet).\nThe label attribute of SemanticLabel holds the corresponding value of the SemanticLabel, e.g. \nlabel=animate (for type=semanticField)." ;
        rdfs:isDefinedBy    "http://www.isocat.org/datcat/DC-1971" ;
        rdfs:label          "type" ;
        rdfs:subPropertyOf  :hasUbyDatatypeProperty ;
        owl:versionInfo     "Should replace the DatatypeProperty type" .

:DefinitionType  a       owl:Class ;
        rdfs:label       "definitionType" ;
        rdfs:subClassOf  :DictionaryFeature .

:loanWord  a              :DerivationType , owl:NamedIndividual ;
        rdfs:isDefinedBy  "http://www.isocat.org/datcat/DC-511" ;
        rdfs:label        "loanWord" .

:transparentMeaning  a      owl:DatatypeProperty ;
        rdfs:isDefinedBy    "http://www.isocat.org/datcat/DC-4390" ;
        rdfs:label          "transparentMeaning" ;
        rdfs:range          xsd:boolean ;
        rdfs:subPropertyOf  :hasUbyDatatypeProperty .

:derivative  a            :DerivationType , owl:NamedIndividual ;
        rdfs:isDefinedBy  "http://www.isocat.org/datcat/DC-4611" ;
        rdfs:label        "derivative" .

:first  a                 :Person , owl:NamedIndividual ;
        rdfs:isDefinedBy  "http://www.isocat.org/datcat/DC-3198" ;
        rdfs:label        "first" .

:transliteration  a         owl:DatatypeProperty ;
        rdfs:isDefinedBy    "http://www.isocat.org/datcat/DC-1848" ;
        rdfs:label          "transliteration" ;
        rdfs:subPropertyOf  :hasUbyDatatypeProperty .

:Lemma  a                 owl:Class ;
        rdfs:isDefinedBy  "http://uby.googlecode.com/files/UBY_LMF_0_2_0.dtd" ;
        rdfs:subClassOf   lemon:Form , system:UnitOfAnnotation ;
        owl:deprecated    true ;
        owl:versionInfo   "superseded by lemon:canonicalForm" .

:particleComparative  a   :PartOfSpeech , owl:NamedIndividual ;
        rdfs:isDefinedBy  "http://www.isocat.org/datcat/DC-1922" ;
        rdfs:label        "particleComparative" .

:idiomaticExpression  a   :ExampleType , owl:NamedIndividual ;
        rdfs:isDefinedBy  "http://www.isocat.org/datcat/DC-351" ;
        rdfs:label        "idiomaticExpression" .

:compoundRoot  a          :DerivationType , owl:NamedIndividual ;
        rdfs:isDefinedBy  "http://www.isocat.org/datcat/DC-357" ;
        rdfs:label        "compoundRoot" .

:infinitive  a            :VerbFormMood , owl:NamedIndividual ;
        rdfs:isDefinedBy  "http://www.isocat.org/datcat/DC-1312" ;
        rdfs:label        "infinitive" .

:hasQuantification  a       owl:ObjectProperty , owl:AnnotationProperty ;
        rdfs:comment        "In UBY-LMF, quantification is an attribute of the class SemanticLabel. It can be used, if the value of the semantic label is annotated with a score, e.g. type=sentiment, label=positive, quantification=strong.\n" ;
        rdfs:isDefinedBy    "http://www.isocat.org/datcat/DC-2211" ;
        rdfs:label          "quantification" ;
        rdfs:subPropertyOf  :hasUbyDatatypeProperty ;
        owl:versionInfo     "Should be used to replace the DatatypeProperty quantification" .

:quantification  a          owl:DatatypeProperty ;
        rdfs:comment        "In UBY-LMF, quantification is an attribute of the class SemanticLabel. It can be used, if the value of the semantic label is annotated with a score, e.g. type=sentiment, label=positive, quantification=strong.\n" ;
        rdfs:isDefinedBy    "http://www.isocat.org/datcat/DC-2211" ;
        rdfs:label          "quantification" ;
        rdfs:subPropertyOf  :hasUbyDatatypeProperty ;
        owl:versionInfo     "Should be remodelled as an ObjectProperty in future versions" .

:dative  a                :Case , owl:NamedIndividual ;
        rdfs:isDefinedBy  "http://www.isocat.org/datcat/DC-2723" ;
        rdfs:label        "dative" .

:Lexicon  a                  owl:Class ;
        rdfs:isDefinedBy     "http://uby.googlecode.com/files/UBY_LMF_0_2_0.dtd" ;
        rdfs:subClassOf      :LexicalFeatureStructure ;
        owl:deprecated       true ;
        owl:equivalentClass  lemon:Lexicon ;
        owl:versionInfo      "superseded by lemon:Lexicon" .

:nominative  a            :Case , owl:NamedIndividual ;
        rdfs:isDefinedBy  "http://www.isocat.org/datcat/DC-2721" ;
        rdfs:label        "nominative" .

skos:Concept  a  owl:Class .

:VerbFormMood  a          owl:Class ;
        rdfs:isDefinedBy  "http://www.isocat.org/datcat/DC-1427" ;
        rdfs:label        "verbFormMood" ;
        rdfs:subClassOf   :WordFormAttribute .

:hasVerbForm  a             owl:ObjectProperty ;
        rdfs:label          "verbForm" ;
        rdfs:range          :VerbForm ;
        rdfs:subPropertyOf  :hasUbyObjectProperty .

:SemanticArgument  a      owl:Class ;
        rdfs:isDefinedBy  "http://uby.googlecode.com/files/UBY_LMF_0_2_0.dtd" ;
        rdfs:subClassOf   lemon:Argument , system:UnitOfAnnotation ;
        owl:versionInfo   "subclass of lemon:semArg" .

:feminine  a              :GrammaticalGender , owl:NamedIndividual ;
        rdfs:isDefinedBy  "http://www.isocat.org/datcat/DC-3197" ;
        rdfs:label        "feminine" .

:externalSystem  a          owl:DatatypeProperty ;
        rdfs:isDefinedBy    "http://www.isocat.org/datcat/DC-1974" ;
        rdfs:label          "externalSystem" ;
        rdfs:subPropertyOf  :hasUbyDatatypeProperty .

:semanticRole  a            owl:DatatypeProperty ;
        rdfs:isDefinedBy    "http://www.isocat.org/datcat/DC-3466" ;
        rdfs:label          "semanticRole" ;
        rdfs:subPropertyOf  :hasUbyDatatypeProperty .

:isIncorporated  a          owl:DatatypeProperty ;
        rdfs:isDefinedBy    "http://www.isocat.org/datcat/DC-4151" ;
        rdfs:label          "isIncorporated" ;
        rdfs:range          xsd:boolean ;
        rdfs:subPropertyOf  :hasUbyDatatypeProperty .

:label  a                   owl:DatatypeProperty ;
        rdfs:comment        "Label encodes a name (short - like a tag) and is an attribute of the UBY-LMF class SemanticLabel, SemanticPredicate, " ;
        rdfs:isDefinedBy    "http://www.isocat.org/datcat/DC-1857" ;
        rdfs:label          "label" ;
        rdfs:subPropertyOf  :hasUbyDatatypeProperty .

:present  a               :Tense , owl:NamedIndividual ;
        rdfs:isDefinedBy  "http://www.isocat.org/datcat/DC-3421" ;
        rdfs:label        "present" .

:has_person  a              owl:ObjectProperty ;
        rdfs:label          "person" ;
        rdfs:range          :Person ;
        rdfs:subPropertyOf  :has_WordFormAttribute .

:Synset  a               owl:Class ;
        rdfs:comment     "This owl:Class corresponds to the ISO LMF-class Synset." ;
        rdfs:subClassOf  skos:Concept , :LexicalFeatureStructure ;
        owl:versionInfo  "mapped onto skos:Concept" .

:postpositiveAdjective
        a                 :SyntacticProperty , owl:NamedIndividual ;
        rdfs:isDefinedBy  "http://www.isocat.org/datcat/DC-4619" ;
        rdfs:label        "postpositiveAdjective" .

:abbreviationInitialism
        a                 :PartOfSpeech , owl:NamedIndividual ;
        rdfs:isDefinedBy  "http://www.isocat.org/datcat/DC-333" ;
        rdfs:label        "abbreviationInitialism" .

:subject  a               :GrammaticalFunction , owl:NamedIndividual ;
        rdfs:isDefinedBy  "http://www.isocat.org/datcat/DC-1391" ;
        rdfs:label        "subject" .

:peripheral  a            :CoreType , owl:NamedIndividual ;
        rdfs:isDefinedBy  "http://www.isocat.org/datcat/DC-4463" ;
        rdfs:label        "peripheral" .

:ExampleType  a          owl:Class ;
        rdfs:label       "exampleType" ;
        rdfs:subClassOf  :DictionaryFeature .

:adpositionCircumposition
        a                 :PartOfSpeech , owl:NamedIndividual ;
        rdfs:isDefinedBy  "http://www.isocat.org/datcat/DC-1906" ;
        rdfs:label        "adpositionCircumposition" .

:has_tense  a               owl:ObjectProperty ;
        rdfs:label          "tense" ;
        rdfs:range          :Tense ;
        rdfs:subPropertyOf  :has_WordFormAttribute .

:externalReference  a       owl:DatatypeProperty ;
        rdfs:isDefinedBy    "http://www.isocat.org/datcat/DC-1975" ;
        rdfs:label          "externalReference" ;
        rdfs:subPropertyOf  :hasUbyDatatypeProperty .

:Determiner  a            owl:Class ;
        rdfs:comment      "In UBY-LMF, determiner is an attribute of the LMF class SyntacticArgument. For noun phrase arguments, this attribute encodes specific constraints on the determiner to be used (possessive or indefinite).\n\nExample given in VerbNet (possessive): They allow our smoking.\nExample from VerbNet (indefinite): an indefinite determiner is required for the noun phrase complement of \"echo\" as in \nThere echoed voices through the hall. (verb class sound_existence-47.4)" ;
        rdfs:isDefinedBy  "http://www.isocat.org/datcat/DC-1272" , "http://www.isocat.org/datcat/DC-3159" ;
        rdfs:label        "determiner" ;
        rdfs:subClassOf   :SyntacticFeature .

:verb   a                 :PartOfSpeech , owl:NamedIndividual ;
        rdfs:isDefinedBy  "http://www.isocat.org/datcat/DC-1424" ;
        rdfs:label        "verb" .

:determinerIndefinite
        a                 :PartOfSpeech , owl:NamedIndividual ;
        rdfs:isDefinedBy  "http://www.isocat.org/datcat/DC-1307" ;
        rdfs:label        "determinerIndefinite" .

:derivationBase  a        :DerivationType , owl:NamedIndividual ;
        rdfs:isDefinedBy  "http://www.isocat.org/datcat/DC-4612" ;
        rdfs:label        "derivationBase" .

<http://purl.org/olia/ubyCat.owl>
        a                owl:Ontology ;
        rdfs:comment     "OLiA Annotation Model for Uby Parts of Speech (Gurevych et al, 2012)\nextracted from the Uby DTD (http://purl.org/olia/ubyCat.owl, version of Nov 21th, 2012).\n\nReferences\nIryna Gurevych, Judith Eckle-Kohler, Silvana Hartmann, Michael Matuschek, Christian M. Meyer and Christian Wirth, 2012, Uby - A Large-Scale Unified Lexical-Semantic Resource, Proceedings of the 13th Conference of the European Chapter of the Association for Computational Linguistics (EACL 2012), Avignon, France.\n\nThe DTD is made available under a Creative Commons Attribution-ShareAlike 3.0 Unported (CC BY-SA 3.0) license which is available at http://creativecommons.org/licenses/by-sa/3.0/\nYou are free to share (copy, distribute and transmit) the work, to develop your own extensions (adapt, remix) of the work, and to make commercial use of the work."@en ;
        rdfs:label       "ubyCat.owl" ;
        owl:imports      <http://www.monnet-project.eu/lemon> , <http://purl.org/olia/system.owl> ;
        owl:versionInfo  "2012, Nov 14 created (CC)\n2013, Mar 20 extended by Data Categories from UBY-LMF not related to Parts-of-Speech, reorganized (JEK)\n2013, Jun 21 reorganized: converted terminal classes (encoding attribute values) to individuals, eliminated inferred Part-of-Speech hierarchy (JEK)\n2013, Jun 24-25 Class MultiWordFeature to DatatypeProperty multiWordFeature;\n\t\t\t Class Index to DatatypeProperty hasIndex;\n\t\t\t Class IsIncorporated to DatatypeProperty isIncorporated; eliminate hasIsIncorporated, hasIsHead, hasIsBreakBefore;\n\t\t\t Class Lexicalized to DatatypeProperty lexicalized; eliminate hasLexicalized;\n\t\t\t Class OptionalArgument to DatatypeProperty optionalArgument;\n\t\t\t Class Perspectivalized to DatatypeProperty perspectivalized; eliminate hasPerspectivalized;\n\t\t\t Class TransparentMeaning to DatatypeProperty transparentMeaning; eliminate yes, no;\n\t\t\t (CC)\n2013, Jun 25 hasIndex to index (JMC)\n2013, Jun 26 IsHead to isHead, IsBreakBefore to isBreakBefore\n\tintroduced LexicalDataStructure, reintroduced sense, LexicalEntry, Lexicon, Sense, SemanticPredicate, Definition, Lemma, Context, SubcategorizationFrame, SyntacticArgument, senseRelation, SenseExample, SemanticArgument (these are not actually used in the RDF data, but in the original DTD, hence marked as deprecated here, however, having them in the ontology would allow Uby users to easily rediscover the equivalent lemon concepts)\n\thasSeparableParticle, SeparableParticle to separableParticle, (has)GeographicalVariant to Dataprop geographicalVariant, (has)Hyphenation to Datprop hyphenation, (has)PhoneticForm to Dp phoneticForm, (has)Transliteration to Dp transliteration, (has)Usage to Dp usage, writtenForm to Dp, (has)IncorporatedSemArg to Dp incorporatedSemArg, (has)SemanticRole to Dp semanticRole, (has)Lexeme to Dp lexeme, (has)Preposition to Dp preposition, (has)PrepositionType to Dp prepositionType\n\t(has)ExternalReference to externalReference, (has)ExternalSystem, (has)Generator, (has)Corpus, (has)Label, (has)OrthographyName, (has)Quantification, (has)Sound, (has)Type\n\t(has)LanguageIdentifier to dp languageIdentifier (deprecated)\n\tdp hasMonolingualExternalRef to OP monolingualExternalRef\n\tFrequency subClassOf LexicalFeatureStructure (deprecated)\n\t(has)DerivationType deprecated, JMC: relType ... decides the property to use in the mapping, hence deprecated.\n\tmerged ComplexLexicalFeature and LexicalDataStructure to LexicalFeatureStructure\n\t(CC)\n\nTODO: ObjectProperties and Classes for quantification, semanticRole, incorporatedSemArg, Type\n\t  consistent naming conventions for properties: hasXY for ObjectProperties, isXY for boolean DataProperties, xY for other DataProperties\n\t  domain and range restrictions on properties\n\t  check properties generated from DerivationType (relType)\n\nChristian Chiarcos, chiarcos@cs.uni-frankfurt.de\nJudith Eckle-Kohler, eckle-kohler@ukp.informatik.tu-darmstadt.de\nJohn McCrae, jmccrae@cit-ec.uni-bielefeld.de\n"@en .

:corpus  a                  owl:DatatypeProperty ;
        rdfs:isDefinedBy    "http://www.isocat.org/datcat/DC-4361" ;
        rdfs:label          "corpus" ;
        rdfs:subPropertyOf  :hasUbyDatatypeProperty .

:nounPhrase  a            :SyntacticCategory , owl:NamedIndividual ;
        rdfs:isDefinedBy  "http://www.isocat.org/datcat/DC-2256" ;
        rdfs:label        "nounPhrase" .

:crosslingualSenseAlignment
        a                 :SenseAxisType , owl:NamedIndividual ;
        rdfs:isDefinedBy  "http://www.isocat.org/datcat/DC-4628" ;
        rdfs:label        "crosslingualSenseAlignment" .

:usage  a                   owl:DatatypeProperty ;
        rdfs:isDefinedBy    "http://www.isocat.org/datcat/DC-3764" ;
        rdfs:label          "usage" ;
        rdfs:subPropertyOf  :hasUbyDatatypeProperty ;
        owl:versionInfo     "Never used" .

:affixPrefix  a           :PartOfSpeech , owl:NamedIndividual ;
        rdfs:isDefinedBy  "http://www.isocat.org/datcat/DC-1365" ;
        rdfs:label        "affixPrefix" .

:adverbialComplement  a   :GrammaticalFunction , owl:NamedIndividual ;
        rdfs:isDefinedBy  "http://www.isocat.org/datcat/DC-4639" ;
        rdfs:label        "adverbialComplement" .

:Complementizer  a        owl:Class ;
        rdfs:isDefinedBy  "http://www.isocat.org/datcat/DC-3124" ;
        rdfs:label        "complementizer" ;
        rdfs:subClassOf   :SyntacticFeature .

:hasUbyDatatypeProperty
        a             owl:DatatypeProperty ;
        rdfs:comment  "This DatatypeProperty could also be named \"hasSimpleLexicalFeature\".\nThe current name \"hasUbyDatatypeProperty\" indicates that it groups Data Properties used in UBY-LMF." .

:PartOfSpeech  a          owl:Class ;
        rdfs:comment      "As a convention, the relation is called has_partOfSpeech, partOfSpeech is the top-level *class* of parts of speech" ;
        rdfs:isDefinedBy  "http://purl.org/olia/ubyCat.owl" ;
        rdfs:label        "partOfSpeech" ;
        rdfs:subClassOf   :LexicalFeature , system:Feature .

:RelType  a               owl:Class ;
        rdfs:isDefinedBy  "http://www.isocat.org/datcat/DC-1971" ;
        rdfs:label        "relType" ;
        rdfs:subClassOf   :SemanticFeature .

:abbreviation  a          :PartOfSpeech , owl:NamedIndividual ;
        rdfs:isDefinedBy  "http://www.isocat.org/datcat/DC-329" ;
        rdfs:label        "abbreviation" .

:ingForm  a               :VerbFormMood , :VerbForm , owl:NamedIndividual ;
        rdfs:isDefinedBy  "http://www.isocat.org/datcat/DC-4108" ;
        rdfs:label        "ingForm" .

:extraThematic  a         :CoreType , owl:NamedIndividual ;
        rdfs:isDefinedBy  "http://www.isocat.org/datcat/DC-4465" ;
        rdfs:label        "extraThematic" .

:adpositionPreposition
        a                 :PartOfSpeech , owl:NamedIndividual ;
        rdfs:isDefinedBy  "http://www.isocat.org/datcat/DC-1366" ;
        rdfs:label        "adpositionPreposition" .

:Definition  a               owl:Class ;
        rdfs:isDefinedBy     "http://uby.googlecode.com/files/UBY_LMF_0_2_0.dtd" ;
        rdfs:subClassOf      :LexicalFeatureStructure ;
        owl:deprecated       true ;
        owl:equivalentClass  lemon:SenseDefinition ;
        owl:versionInfo      "superseded by lemon:SenseDefinition" .

system:hasFeature  a  owl:ObjectProperty .

:CoreType  a              owl:Class ;
        rdfs:isDefinedBy  "http://www.isocat.org/datcat/DC-4461" ;
        rdfs:label        "coreType" ;
        rdfs:subClassOf   :SemanticFeature .

:association  a           :RelType , owl:NamedIndividual ;
        rdfs:isDefinedBy  "http://www.isocat.org/datcat/DC-438" ;
        rdfs:label        "association" .

:masculine  a             :GrammaticalGender , owl:NamedIndividual ;
        rdfs:isDefinedBy  "http://www.isocat.org/datcat/DC-3312" ;
        rdfs:label        "masculine" .

:pronounPersonalReflexive
        a                 :PartOfSpeech , owl:NamedIndividual ;
        rdfs:isDefinedBy  "http://www.isocat.org/datcat/DC-3014" ;
        rdfs:label        "pronounPersonalReflexive" .

:infinitiveZu  a          :VerbFormMood , owl:NamedIndividual ;
        rdfs:isDefinedBy  "http://www.isocat.org/datcat/DC-2897" ;
        rdfs:label        "infinitiveZu" .

:pronounPersonalIrreflexive
        a                 :PartOfSpeech , owl:NamedIndividual ;
        rdfs:isDefinedBy  "http://www.isocat.org/datcat/DC-3013" ;
        rdfs:label        "pronounPersonalIrreflexive" .

:hasDeterminer  a           owl:ObjectProperty ;
        rdfs:label          "determiner" ;
        rdfs:range          :Determiner ;
        rdfs:subPropertyOf  :hasUbyObjectProperty .

:SenseExample  a             owl:Class ;
        rdfs:isDefinedBy     "http://uby.googlecode.com/files/UBY_LMF_0_2_0.dtd" ;
        rdfs:subClassOf      :LexicalFeatureStructure ;
        owl:deprecated       true ;
        owl:equivalentClass  lemon:UsageExample ;
        owl:versionInfo      "superseded by lemon:UsageExample" .

:nounProper  a            :PartOfSpeech , owl:NamedIndividual ;
        rdfs:isDefinedBy  "http://www.isocat.org/datcat/DC-1371" ;
        rdfs:label        "nounProper" .

:conjunctionCoordinating
        a                 :PartOfSpeech , owl:NamedIndividual ;
        rdfs:isDefinedBy  "http://www.isocat.org/datcat/DC-1262" ;
        rdfs:label        "conjunctionCoordinating" .

:geographicalVariant  a     owl:DatatypeProperty ;
        rdfs:isDefinedBy    "http://www.isocat.org/datcat/DC-1851" ;
        rdfs:label          "geographicalVariant" ;
        rdfs:subPropertyOf  :hasUbyDatatypeProperty ;
        owl:deprecated      true ;
        owl:versionInfo     "moved into language tags (JMC)" .

:hasComplementizer  a       owl:ObjectProperty ;
        rdfs:label          "complementizer" ;
        rdfs:range          :Complementizer ;
        rdfs:subPropertyOf  :hasUbyObjectProperty .

:syntacticUsage  a        :ExampleType , owl:NamedIndividual ;
        rdfs:isDefinedBy  "http://www.isocat.org/datcat/DC-455" ;
        rdfs:label        "syntacticUsage" .

:symbol  a                :PartOfSpeech , owl:NamedIndividual ;
        rdfs:isDefinedBy  "http://www.isocat.org/datcat/DC-1398" ;
        rdfs:label        "symbol" .

:particleAnswer  a        :PartOfSpeech , owl:NamedIndividual ;
        rdfs:isDefinedBy  "http://www.isocat.org/datcat/DC-2891" ;
        rdfs:label        "particleAnswer" .

:adverb  a                :PartOfSpeech , owl:NamedIndividual ;
        rdfs:isDefinedBy  "http://www.isocat.org/datcat/DC-1232" ;
        rdfs:label        "adverb" .

:orthographyName  a         owl:DatatypeProperty ;
        rdfs:isDefinedBy    "http://www.isocat.org/datcat/DC-2176" ;
        rdfs:label          "orthographyName" ;
        rdfs:subPropertyOf  :hasUbyDatatypeProperty .

:other  a           :ExampleType , owl:NamedIndividual ;
        rdfs:label  "other" .

:subjectControl  a        :SyntacticProperty , owl:NamedIndividual ;
        rdfs:isDefinedBy  "http://www.isocat.org/datcat/DC-4187" ;
        rdfs:label        "subjectControl" .

:positive  a              :Degree , owl:NamedIndividual ;
        rdfs:isDefinedBy  "http://www.isocat.org/datcat/DC-2780" ;
        rdfs:label        "positive" .

:verbPhrase  a            :SyntacticCategory , owl:NamedIndividual ;
        rdfs:isDefinedBy  "http://www.isocat.org/datcat/DC-2255" ;
        rdfs:label        "verbPhrase" .

:Case   a                 owl:Class ;
        rdfs:isDefinedBy  "http://www.isocat.org/datcat/DC-2720" ;
        rdfs:label        "case" ;
        rdfs:subClassOf   :WordFormAttribute .

:past   a                 :Tense , owl:NamedIndividual ;
        rdfs:isDefinedBy  "http://www.isocat.org/datcat/DC-3378" ;
        rdfs:label        "past" .

:LexicalFeatureStructure
        a                owl:Class ;
        rdfs:comment     "LexicalFeatureStructure is a complex lexical Feature Structure (with features and feature values) and corresponds to a class in LMF."@en ;
        rdfs:label       "lexical data structure" , "lexical feature structure" , "complex lexical feature" ;
        rdfs:subClassOf  :LexicalAnnotation ;
        owl:deprecated   true ;
        owl:versionInfo  "superseded by lemon data structures, left here only as a reference"@en , "TODO: check whether these may be LexicalFeatureStructures" .

:Quantification  a        owl:Class ;
        rdfs:comment      "In UBY-LMF, quantification is an attribute of the class SemanticLabel. It can be used, if the value of the semantic label is annotated with a score, e.g. type=sentiment, label=positive, quantification=strong.\n" ;
        rdfs:isDefinedBy  "http://www.isocat.org/datcat/DC-2211" ;
        rdfs:label        "quantification" ;
        rdfs:subClassOf   :MetaFeature ;
        owl:versionInfo   "should be used together with hasQuantification to replace the DatatypeProperty quantification" .

:SemanticLabel  a            owl:Class ;
        rdfs:comment         "This owl:Class corresponds to the LMF-class SemanticLabel which has been introduced in UBY-LMF as an extension of ISO-LMF." ;
        rdfs:subClassOf      :LexicalFeatureStructure ;
        owl:deprecated       true ;
        owl:equivalentClass  lemon:SemanticLabel ;
        owl:versionInfo      "superseded by lemon:SemanticLabel" .

:partWhole  a             :RelType , owl:NamedIndividual ;
        rdfs:isDefinedBy  "http://www.isocat.org/datcat/DC-397" ;
        rdfs:label        "partWhole" .

:nounProperFamilyName
        a                 :PartOfSpeech , owl:NamedIndividual ;
        rdfs:isDefinedBy  "http://www.isocat.org/datcat/DC-4195" ;
        rdfs:label        "nounProperLastName" .

:particleNegative  a      :PartOfSpeech , owl:NamedIndividual ;
        rdfs:isDefinedBy  "http://www.isocat.org/datcat/DC-1894" ;
        rdfs:label        "particleNegative" .

:has_case  a                owl:ObjectProperty ;
        rdfs:label          "case" ;
        rdfs:range          :Case ;
        rdfs:subPropertyOf  :has_WordFormAttribute .

system:Feature  a  owl:Class .

:multiwordFeature  a        owl:DatatypeProperty ;
        rdfs:subPropertyOf  :hasUbyDatatypeProperty .

:nounProperGivenName  a   :PartOfSpeech , owl:NamedIndividual ;
        rdfs:isDefinedBy  "http://www.isocat.org/datcat/DC-4194" ;
        rdfs:label        "nounProperFirstName" .

:etymology  a             :DerivationType , owl:NamedIndividual ;
        rdfs:isDefinedBy  "http://www.isocat.org/datcat/DC-221" ;
        rdfs:label        "etymology" .

:sound  a                   owl:DatatypeProperty ;
        rdfs:isDefinedBy    "http://www.isocat.org/datcat/DC-2250" ;
        rdfs:label          "sound" ;
        rdfs:subPropertyOf  :hasUbyDatatypeProperty .

:affix  a                 :PartOfSpeech , owl:NamedIndividual ;
        rdfs:isDefinedBy  "http://www.isocat.org/datcat/DC-1234" ;
        rdfs:label        "affix" .

:isHead  a                  owl:DatatypeProperty ;
        rdfs:isDefinedBy    "http://www.isocat.org/datcat/DC-4617" ;
        rdfs:label          "isHead" ;
        rdfs:range          xsd:boolean ;
        rdfs:subPropertyOf  :multiwordFeature .

:pronounRelative  a       :PartOfSpeech , owl:NamedIndividual ;
        rdfs:isDefinedBy  "http://www.isocat.org/datcat/DC-1380" ;
        rdfs:label        "pronounRelative" .

:phraseme  a              :PartOfSpeech , owl:NamedIndividual ;
        rdfs:isDefinedBy  "http://www.isocat.org/datcat/DC-339" ;
        rdfs:label        "phraseme" .

:supports  a              :DerivationType , owl:NamedIndividual ;
        rdfs:isDefinedBy  "http://www.isocat.org/datcat/DC-3003" ;
        rdfs:label        "supports" .

:objectRaising  a         :SyntacticProperty , owl:NamedIndividual ;
        rdfs:isDefinedBy  "http://www.isocat.org/datcat/DC-4190" ;
        rdfs:label        "objectRaising" .

:determinerDemonstrative
        a                 :PartOfSpeech , owl:NamedIndividual ;
        rdfs:isDefinedBy  "http://www.isocat.org/datcat/DC-1269" ;
        rdfs:label        "determinerDemonstrative" .

:yesNoType  a             :Complementizer , owl:NamedIndividual ;
        rdfs:isDefinedBy  "http://www.isocat.org/datcat/DC-2297" ;
        rdfs:label        "yesNoType" .

:determinerDefinite  a    :PartOfSpeech , owl:NamedIndividual ;
        rdfs:isDefinedBy  "http://www.isocat.org/datcat/DC-1430" ;
        rdfs:label        "determinerDefinite" .

:SyntacticFeature  a     owl:Class ;
        rdfs:comment     "SyntacticFeature groups attributes of UBY-LMF classes from the ISO LMF Syntax extension package." ;
        rdfs:subClassOf  :LexicalFeature .

:abbreviationAcronym  a   :PartOfSpeech , owl:NamedIndividual ;
        rdfs:isDefinedBy  "http://www.isocat.org/datcat/DC-334" ;
        rdfs:label        "abbreviationAcronym" .

:conjunction  a           :PartOfSpeech , owl:NamedIndividual ;
        rdfs:isDefinedBy  "http://www.isocat.org/datcat/DC-3132" ;
        rdfs:label        "conjunction" .

:Position  a                owl:DatatypeProperty ;
        rdfs:isDefinedBy    "http://www.isocat.org/datcat/DC-2237" ;
        rdfs:label          "position" ;
        rdfs:range          xsd:int ;
        rdfs:subPropertyOf  :multiwordFeature .

:senseRelation  a               owl:ObjectProperty ;
        rdfs:isDefinedBy        "http://uby.googlecode.com/files/UBY_LMF_0_2_0.dtd" ;
        rdfs:label              "SenseRelation" ;
        owl:deprecated          true ;
        owl:equivalentProperty  lemon:senseRelation ;
        owl:versionInfo         "superseded by lemon:senseRelation" .

:partitiveDefinition  a   :DefinitionType , owl:NamedIndividual ;
        rdfs:isDefinedBy  "http://www.isocat.org/datcat/DC-172" ;
        rdfs:label        "partitiveDefinition" .

:WordForm  a              owl:Class ;
        rdfs:isDefinedBy  "http://purl.org/olia/ubyCat.owl" ;
        rdfs:label        "WordForm" ;
        rdfs:subClassOf   system:UnitOfAnnotation .

:subordinateClause  a     :SyntacticCategory , owl:NamedIndividual ;
        rdfs:isDefinedBy  "http://www.isocat.org/datcat/DC-3496" ;
        rdfs:label        "subordinateClause" .

:derivationBaseNoun  a    :DerivationType , owl:NamedIndividual ;
        rdfs:isDefinedBy  "http://www.isocat.org/datcat/DC-4615" ;
        rdfs:label        "derivationBaseNoun" .

:adjective  a             :PartOfSpeech , owl:NamedIndividual ;
        rdfs:isDefinedBy  "http://www.isocat.org/datcat/DC-1230" ;
        rdfs:label        "adjective" .

:participle  a            :VerbFormMood , :VerbForm , owl:NamedIndividual ;
        rdfs:isDefinedBy  "http://www.isocat.org/datcat/DC-3371" ;
        rdfs:label        "participle" .

:lexeme  a                  owl:DatatypeProperty ;
        rdfs:comment        "Lexeme is an attribute of the UBY-LMF class SyntacticArgument and specifies a particular lexeme to be used in realizations of particular complements.\nExample (lexeme = es, ObjectComplement realized as zu-infinitive): Er schafft es, den Termin einzuhalten.\n* Er schafft, den Termin einzuhalten." ;
        rdfs:isDefinedBy    "http://www.isocat.org/datcat/DC-1325" ;
        rdfs:label          "lexeme" ;
        rdfs:subPropertyOf  :hasUbyDatatypeProperty .

:SemanticPredicate  a     owl:Class ;
        rdfs:isDefinedBy  "http://uby.googlecode.com/files/UBY_LMF_0_2_0.dtd" ;
        rdfs:subClassOf   lemon:LexicalSense , system:UnitOfAnnotation ;
        owl:versionInfo   "subClass of lemon:LexicalSense" .

:pronoun  a               :PartOfSpeech , owl:NamedIndividual ;
        rdfs:isDefinedBy  "http://www.isocat.org/datcat/DC-1370" ;
        rdfs:label        "pronoun" .

:particle  a              :PartOfSpeech , owl:NamedIndividual ;
        rdfs:isDefinedBy  "http://www.isocat.org/datcat/DC-3372" ;
        rdfs:label        "particle" .

:third  a                 :Person , owl:NamedIndividual ;
        rdfs:isDefinedBy  "http://www.isocat.org/datcat/DC-3526" ;
        rdfs:label        "third" .

:Sense  a                    owl:Class ;
        rdfs:isDefinedBy     "http://www.monnet-project.eu/lemon#LexicalSense" , "http://uby.googlecode.com/files/UBY_LMF_0_2_0.dtd" ;
        rdfs:subClassOf      :LexicalFeatureStructure , system:UnitOfAnnotation ;
        owl:deprecated       true ;
        owl:equivalentClass  lemon:LexicalSense ;
        owl:versionInfo      "superseded by lemon:LexicalSense" .

:translatedDefinition
        a                 :DefinitionType , owl:NamedIndividual ;
        rdfs:isDefinedBy  "http://www.isocat.org/datcat/DC-173" ;
        rdfs:label        "translatedDefinition" .

:second  a                :Person , owl:NamedIndividual ;
        rdfs:isDefinedBy  "http://www.isocat.org/datcat/DC-3464" ;
        rdfs:label        "second" .

:prepositionalComplement
        a                 :GrammaticalFunction , owl:NamedIndividual ;
        rdfs:isDefinedBy  "http://www.isocat.org/datcat/DC-4638" ;
        rdfs:label        "prepositionalComplement" .

:hasSenseAxisType  a        owl:ObjectProperty ;
        rdfs:range          :SenseAxisType ;
        rdfs:subPropertyOf  :hasUbyObjectProperty .

:complementary  a         :RelType , owl:NamedIndividual ;
        rdfs:isDefinedBy  "http://www.isocat.org/datcat/DC-83" ;
        rdfs:label        "complementary" .

:VerbForm  a             owl:Class ;
        rdfs:comment     "Specifies the verb form to be used in a verb phrase complement." ;
        rdfs:label       "verbForm" ;
        rdfs:subClassOf  :SyntacticFeature .

:subjunctive  a           :VerbFormMood , owl:NamedIndividual ;
        rdfs:isDefinedBy  "http://www.isocat.org/datcat/DC-1843" ;
        rdfs:label        "subjunctive" .

:particleInfinitive  a    :PartOfSpeech , owl:NamedIndividual ;
        rdfs:isDefinedBy  "http://www.isocat.org/datcat/DC-1896" ;
        rdfs:label        "particleInfinitive" .

:indicative  a            :VerbFormMood , owl:NamedIndividual ;
        rdfs:isDefinedBy  "http://www.isocat.org/datcat/DC-1885" ;
        rdfs:label        "indicative" .

:has_grammaticalGender
        a                   owl:ObjectProperty ;
        rdfs:label          "grammaticalGender" ;
        rdfs:range          :GrammaticalGender ;
        rdfs:subPropertyOf  :has_WordFormAttribute .

:adjectivePhrase_nounPhrase
        a           :SyntacticCategory , owl:NamedIndividual ;
        rdfs:label  "adjectivePhrase_nounPhrase" .

:hyphenation  a             owl:DatatypeProperty ;
        rdfs:isDefinedBy    "http://www.isocat.org/datcat/DC-264" ;
        rdfs:label          "hyphenation" ;
        rdfs:subPropertyOf  :hasUbyDatatypeProperty .

:adjectivePhrase  a       :SyntacticCategory , owl:NamedIndividual ;
        rdfs:isDefinedBy  "http://www.isocat.org/datcat/DC-2258" ;
        rdfs:label        "adjectivePhrase" .

:numeral  a               :PartOfSpeech , owl:NamedIndividual ;
        rdfs:isDefinedBy  "http://www.isocat.org/datcat/DC-1334" ;
        rdfs:label        "numeral" .

:hasRelType  a              owl:ObjectProperty ;
        rdfs:label          "relType" ;
        rdfs:range          :RelType ;
        rdfs:subPropertyOf  :hasUbyObjectProperty .

:superlative  a           :Degree , owl:NamedIndividual ;
        rdfs:isDefinedBy  "http://www.isocat.org/datcat/DC-2782" ;
        rdfs:label        "superlative" .

:SubcategorizationFrame
        a                    owl:Class ;
        rdfs:isDefinedBy     "http://uby.googlecode.com/files/UBY_LMF_0_2_0.dtd" ;
        rdfs:subClassOf      system:UnitOfAnnotation ;
        owl:deprecated       true ;
        owl:equivalentClass  lemon:Frame ;
        owl:versionInfo      "superseded by lemon:Frame" .

:has_verbFormMood  a        owl:ObjectProperty ;
        rdfs:label          "verbFormMood" ;
        rdfs:range          :VerbFormMood ;
        rdfs:subPropertyOf  :has_WordFormAttribute .

:GrammaticalFunction  a   owl:Class ;
        rdfs:isDefinedBy  "http://www.isocat.org/datcat/DC-1296" ;
        rdfs:label        "grammaticalFunction" ;
        rdfs:subClassOf   :SyntacticFeature .

:adpositionPostposition
        a                 :PartOfSpeech , owl:NamedIndividual ;
        rdfs:isDefinedBy  "http://www.isocat.org/datcat/DC-1360" ;
        rdfs:label        "adpositionPostposition" .

:conjunctionSubordinating
        a                 :PartOfSpeech , owl:NamedIndividual ;
        rdfs:isDefinedBy  "http://www.isocat.org/datcat/DC-1393" ;
        rdfs:label        "conjunctionSubordinating" .

:verbMain  a              :PartOfSpeech , owl:NamedIndividual ;
        rdfs:isDefinedBy  "http://www.isocat.org/datcat/DC-1400" ;
        rdfs:label        "verbMain" .

:MetaFeature  a          owl:Class ;
        rdfs:subClassOf  :LexicalFeature .

:comparative  a           :Degree , owl:NamedIndividual ;
        rdfs:isDefinedBy  "http://www.isocat.org/datcat/DC-2781" ;
        rdfs:label        "comparative" .

:senseInstance  a         :ExampleType , owl:NamedIndividual ;
        rdfs:isDefinedBy  "http://www.isocat.org/datcat/DC-3778" ;
        rdfs:label        "senseInstance" .

:reflexive  a             :SyntacticCategory , owl:NamedIndividual ;
        rdfs:isDefinedBy  "http://www.isocat.org/datcat/DC-3014" ;
        rdfs:label        "reflexive" .

:possessive  a            :Determiner , owl:NamedIndividual ;
        rdfs:isDefinedBy  "http://www.isocat.org/datcat/DC-1357" ;
        rdfs:label        "possessive" .

:derivationBaseAdj  a     :DerivationType , owl:NamedIndividual ;
        rdfs:isDefinedBy  "http://www.isocat.org/datcat/DC-4616" ;
        rdfs:label        "derivationBaseAdj" .

:intensionalDefinition
        a                 :DefinitionType , owl:NamedIndividual ;
        rdfs:isDefinedBy  "http://www.isocat.org/datcat/DC-170" ;
        rdfs:label        "intensionalDefinition" .

:Context  a                  owl:Class ;
        rdfs:isDefinedBy     "http://uby.googlecode.com/files/UBY_LMF_0_2_0.dtd" ;
        rdfs:subClassOf      :LexicalFeatureStructure ;
        owl:deprecated       true ;
        owl:equivalentClass  lemon:LexicalContext ;
        owl:versionInfo      "superseded by lemon:LexicalContext" .

:monolingualExternalRef
        a                   owl:ObjectProperty , owl:AnnotationProperty ;
        rdfs:domain         :Synset ;
        rdfs:label          "monolingualExternalRef" ;
        rdfs:range          :MonolingualExternalRef ;
        rdfs:subPropertyOf  :hasUbyDatatypeProperty .

:WordFormAttribute  a     owl:Class ;
        rdfs:isDefinedBy  "http://purl.org/olia/ubyCat.owl" ;
        rdfs:label        "WordFormAttribute" ;
        rdfs:subClassOf   :LexicalFeature , system:Feature .

:hasSyntacticCategory
        a                   owl:ObjectProperty ;
        rdfs:label          "syntacticCategory" ;
        rdfs:range          :SyntacticCategory ;
        rdfs:subPropertyOf  :hasUbyObjectProperty .

:GrammaticalNumber  a     owl:Class ;
        rdfs:comment      "In UBY-LMF, number is also an attribute of the UBY-LMF class SyntacticArgument and specifies the grammatical number of an argument.\nExample: These types of fish mix well together." ;
        rdfs:isDefinedBy  "http://www.isocat.org/datcat/DC-251" ;
        rdfs:label        "grammaticalNumber" ;
        rdfs:subClassOf   :WordFormAttribute , :SyntacticFeature .

:SemanticFeature  a      owl:Class ;
        rdfs:subClassOf  :LexicalFeature .

:monolingualSenseAlignment
        a                 :SenseAxisType , owl:NamedIndividual ;
        rdfs:isDefinedBy  "http://www.isocat.org/datcat/DC-4627" ;
        rdfs:label        "monolingualSenseAlignment" .

:toInfinitive  a          :VerbForm , owl:NamedIndividual ;
        rdfs:isDefinedBy  "http://www.isocat.org/datcat/DC-4162" ;
        rdfs:label        "toInfinitive" .

:core   a                 :CoreType , owl:NamedIndividual ;
        rdfs:isDefinedBy  "http://www.isocat.org/datcat/DC-4462" ;
        rdfs:label        "core" .

:index  a                   owl:DatatypeProperty ;
        rdfs:comment        "Index is an attribute of the UBY-LMF class Sense.\nIt encodes a ranking of the senses according to their frequency which is provided, e.g., by WordNet." ;
        rdfs:isDefinedBy    "http://www.isocat.org/datcat/DC-233" ;
        rdfs:label          "index" ;
        rdfs:range          xsd:int ;
        rdfs:subPropertyOf  :hasUbyDatatypeProperty .

:contraction  a           :PartOfSpeech , owl:NamedIndividual ;
        rdfs:isDefinedBy  "http://www.isocat.org/datcat/DC-354" ;
        rdfs:label        "contraction" .

:predicativeAdjective
        a                 :SyntacticProperty , owl:NamedIndividual ;
        rdfs:isDefinedBy  "http://www.isocat.org/datcat/DC-2710" ;
        rdfs:label        "predicativeAdjective" .

:LexicalFeature  a       owl:Class ;
        rdfs:comment     "LexicalFeature groups different kinds of lexical feaures, which correspond to attributes of UBY-LMF classes." ;
        rdfs:subClassOf  :LexicalAnnotation .

:GrammaticalGender  a     owl:Class ;
        rdfs:isDefinedBy  "http://www.isocat.org/datcat/DC-3217" ;
        rdfs:label        "grammaticalGender" ;
        rdfs:subClassOf   :WordFormAttribute .

:phoneticForm  a            owl:DatatypeProperty ;
        rdfs:isDefinedBy    "http://www.isocat.org/datcat/DC-1837" ;
        rdfs:label          "phoneticForm" ;
        rdfs:subPropertyOf  :hasUbyDatatypeProperty .
