@prefix dc:    <http://purl.org/dc/elements/1.1/> .
@prefix rdfs:  <http://www.w3.org/2000/01/rdf-schema#> .
@prefix foaf:  <http://xmlns.com/foaf/0.1/> .
@prefix owl:   <http://www.w3.org/2002/07/owl#> .
@prefix rdf:   <http://www.w3.org/1999/02/22-rdf-syntax-ns#> .
@prefix vann:  <http://purl.org/vocab/vann/> .
@prefix vs:    <http://www.w3.org/2003/06/sw-vocab-status/ns#> .
@prefix fresnel: <http://www.w3.org/2004/09/fresnel#> .
@prefix cc:    <http://creativecommons.org/ns#> .

<http://ns.inria.fr/prissma/v2#poiLabel>
        a                rdf:Property ;
        rdfs:comment     "Associates an identifying resource to a POI (e.g. a given monument, a specific restaurant, etc.)" ;
        rdfs:domain      <http://ns.inria.fr/prissma/v2#POI> ;
        rdfs:label       "poiLabel" ;
        rdfs:subClassOf  rdfs:label ;
        vs:term_status   "stable"@en .

<http://ns.inria.fr/prissma/v2#user>
        a               rdf:Property ;
        rdfs:comment    "The property associates a User to a Purpose" ;
        rdfs:domain     <http://ns.inria.fr/prissma/v2#Context> ;
        rdfs:label      "user" ;
        rdfs:range      <http://ns.inria.fr/prissma/v2#User> ;
        vs:term_status  "stable"@en .

<http://ns.inria.fr/prissma/v2#Prism>
        a                owl:Class , rdfs:Class ;
        rdfs:comment     "Wrapper class for describing the contextual conditions under which a given RDF presentation must be activated." ;
        rdfs:label       "Prism" ;
        rdfs:subClassOf  fresnel:Group ;
        vs:term_status   "stable"@en .

<http://dbpedia.org/resource/National_Institute_for_Research_in_Computer_Science_and_Control>
        a       foaf:Organization .

<http://ns.inria.fr/prissma/v2#Environment>
        a               owl:Class , rdfs:Class ;
        rdfs:comment    "The class Environment models the user context in which the resource consumption takes place, therefore enabling customized resource presentation according to specific situations. " ;
        rdfs:label      "Environment" ;
        vs:term_status  "stable"@en .

<http://ns.inria.fr/prissma/v2#Context>
        a                owl:Class , rdfs:Class ;
        rdfs:comment     "The Context class is represents the mobile context and is equivalent to a fresnel:Purpose" ;
        rdfs:label       "Context" ;
        rdfs:subClassOf  fresnel:Purpose ;
        vs:term_status   "stable"@en .

<http://ns.inria.fr/prissma/v2#>
        a                              owl:Ontology ;
        cc:license                     <http://creativecommons.org/licenses/by/3.0/> ;
        dc:creator                     <http://www-sop.inria.fr/members/Luca.Costabello/foaf.rdf#me> ;
        dc:description                 "A vocabulary to model context-aware presentation knowledge for RDF User Interfaces."@en ;
        dc:issued                      "2012-03-20"^^<http://www.w3.org/2001/XMLSchema#date> ;
        dc:modified                    "2012-03-20"^^<http://www.w3.org/2001/XMLSchema#date> ;
        dc:publisher                   <http://dbpedia.org/resource/National_Institute_for_Research_in_Computer_Science_and_Control> ;
        dc:title                       "PRISSMA: Presentation of Resources for Interoperable Semantic and Shareable Mobile Adaptability" ;
        vann:preferredNamespacePrefix  "prissma" ;
        vann:preferredNamespaceUri     "http://ns.inria.fr/prissma/v2#" ;
        owl:versionInfo                2.0 ;
        foaf:page                      <http://ns.inria.fr/prissma/v2/prissma.html> .

<http://ns.inria.fr/prissma/v2#environment>
        a               rdf:Property ;
        rdfs:comment    "The property associates an Environment to a Purpose" ;
        rdfs:domain     <http://ns.inria.fr/prissma/v2#Context> ;
        rdfs:label      "environment" ;
        rdfs:range      <http://ns.inria.fr/prissma/v2#Environment> ;
        vs:term_status  "stable"@en .

<http://ns.inria.fr/prissma/v2#Device>
        a                owl:Class , rdfs:Class ;
        rdfs:comment     "The Device represents the mobile device on which Web of Data resource consumption takes place. It enables device-specific data representation. It is equivalent to the Device class of the delivery context ontology" ;
        rdfs:label       "Device" ;
        rdfs:subClassOf  <http://www.w3.org/2007/uwa/context/deliveryContext.owl#Device> ;
        vs:term_status   "stable"@en .

<http://ns.inria.fr/prissma/v2#device>
        a               rdf:Property ;
        rdfs:comment    "The property associates a Device to a Purpose" ;
        rdfs:domain     <http://ns.inria.fr/prissma/v2#Context> ;
        rdfs:label      "device" ;
        rdfs:range      <http://ns.inria.fr/prissma/v2#Device> ;
        vs:term_status  "stable"@en .

<http://ns.inria.fr/prissma/v2#POI>
        a                owl:Class , rdfs:Class ;
        rdfs:comment     "The class models a Point of Interest (POI) and consists in a simplified version of W3C Point of Interest Core specifications. POIs are defined as entities that \"describe information about locations such as name, category, unique identifier, or civic address\"." ;
        rdfs:label       "POI" ;
        rdfs:subClassOf  <http://www.w3.org/2003/01/geo/wgs84_pos#SpatialThing> ;
        vs:term_status   "stable"@en .

<http://ns.inria.fr/prissma/v2#motion>
        a               rdf:Property ;
        rdfs:comment    "Associates any given high-level representation of motion to a prissma:Environment" ;
        rdfs:domain     <http://ns.inria.fr/prissma/v2#Environment> ;
        rdfs:label      "motion" ;
        vs:term_status  "testing"@en .

<http://ns.inria.fr/prissma/v2#radius>
        a               owl:DatatypeProperty , rdf:Property ;
        rdfs:comment    "Specifies the geographic extension of a POI. Value is expressed in metres." ;
        rdfs:domain     <http://ns.inria.fr/prissma/v2#POI> ;
        rdfs:label      "radius" ;
        rdfs:range      <http://www.w3.org/2001/XMLSchema#nonNegativeInteger> ;
        vs:term_status  "stable"@en .

<http://ns.inria.fr/prissma/v2#nearbyEntity>
        a               rdf:Property ;
        rdfs:comment    "The environmental proximity of a generic real-world entity can trigger different resource representations. The property is therefore used to associate nearby objects to the Environment model." ;
        rdfs:domain     <http://ns.inria.fr/prissma/v2#Environment> ;
        rdfs:label      "nearbyObject" ;
        rdfs:range      owl:Thing ;
        vs:term_status  "testing"@en .

<http://ns.inria.fr/prissma/v2#poiCategory>
        a               rdf:Property ;
        rdfs:comment    "Associates a category to a POI (e.g. monument, restaurant, etc.)" ;
        rdfs:domain     <http://ns.inria.fr/prissma/v2#POI> ;
        rdfs:label      "poiCategory" ;
        vs:term_status  "stable"@en .

<http://ns.inria.fr/prissma/v2#currentPOI>
        a               rdf:Property ;
        rdfs:comment    "The property associates a POI to a prissma:Environment" ;
        rdfs:domain     <http://ns.inria.fr/prissma/v2#Environment> ;
        rdfs:label      "currentPOI" ;
        rdfs:range      <http://ns.inria.fr/prissma/v2#POI> ;
        vs:term_status  "stable"@en .

<http://ns.inria.fr/prissma/v2#User>
        a                owl:Class , rdfs:Class ;
        rdfs:comment     "Represents the target mobile user associated to a prissma:Context. To provide more flexibility, the class can be used to model both user stereotypes and specific users, according to the designer needs. The class is equivalent to foaf:Person" ;
        rdfs:label       "User" ;
        rdfs:subClassOf  <http://xmlns.com/foaf/v1/Person> ;
        vs:term_status   "stable"@en .

<http://ns.inria.fr/prissma/v2#Activity>
        a               owl:Class , rdfs:Class ;
        rdfs:comment    "The Activity class consists in a placemark aimed at modeling a high-level representation of an user action, such as 'running', 'driving', 'working', 'shopping', etc." ;
        rdfs:label      "Activity" ;
        vs:term_status  "testing"@en .
