@prefix dc:    <http://purl.org/dc/terms/> .
@prefix rdfs:  <http://www.w3.org/2000/01/rdf-schema#> .
@prefix owl:   <http://www.w3.org/2002/07/owl#> .
@prefix rdf:   <http://www.w3.org/1999/02/22-rdf-syntax-ns#> .
@prefix vann:  <http://purl.org/vocab/vann/> .
@prefix cc:    <http://creativecommons.org/ns#> .

<http://swa.cefriel.it/ontologies/botdcat-ap#Intent>
        a                 owl:Class ;
        rdfs:comment      "Mandatory class. An Intent exposed by the Dataset."@en ;
        rdfs:isDefinedBy  <http://swa.cefriel.it/ontologies/botdcat-ap> ;
        rdfs:label        "Intent"@en ;
        rdfs:subClassOf   owl:Thing ;
        vann:usageNote    "Mandatory class. An Intent exposed by the Dataset."@en .

<http://swa.cefriel.it/ontologies/botdcat-ap#hasAssetURL>
        a                 owl:ObjectProperty ;
        rdfs:comment      "Optional property. Cardinality [0..1]. This property contains the access URL provided by a SPARQL endpoint handling the Intent."@en ;
        rdfs:domain       <http://swa.cefriel.it/ontologies/botdcat-ap#Intent> ;
        rdfs:isDefinedBy  <http://swa.cefriel.it/ontologies/botdcat-ap> ;
        rdfs:label        "has Asset URL"@en ;
        rdfs:range        rdfs:Resource ;
        vann:usageNote    "Optional property. Cardinality [0..1]. This property contains the access URL provided by a SPARQL endpoint handling the Intent."@en .

<http://swa.cefriel.it/ontologies/botdcat-ap#hasIntent>
        a                 owl:ObjectProperty ;
        rdfs:comment      "Mandatory property. Cardinality [1..n]. This property refers to an Intent handled by the Dataset."@en ;
        rdfs:domain       <http://www.w3.org/ns/dcat#Dataset> ;
        rdfs:isDefinedBy  <http://swa.cefriel.it/ontologies/botdcat-ap> ;
        rdfs:label        "has Intent"@en ;
        rdfs:range        <http://swa.cefriel.it/ontologies/botdcat-ap#Intent> ;
        vann:usageNote    "Mandatory property. Cardinality [1..n]. This property refers to an Intent handled by the Dataset."@en .

<http://swa.cefriel.it/ontologies/botdcat-ap>
        a                              owl:Ontology , <http://purl.org/vocommons/voaf#Vocabulary> ;
        rdfs:comment                   "A vocabulary to describe data sources in a way they can be easily reused and accessed by chatbots."@en ;
        cc:license                     <http://creativecommons.org/licenses/by/4.0/> ;
        dc:contributor                 "Paolo Cappello" , "Irene Celino" , "Marco Comerio" ;
        dc:creator                     "Irene Celino" , "Paolo Cappello" , "Marco Comerio" ;
        dc:date                        "2017-04-01"^^<http://www.w3.org/2001/XMLSchema#date> ;
        dc:description                 "A vocabulary to describe data sources in a way they can be easily reused and accessed by chatbots."@en ;
        dc:issued                      "2017-04-01"^^<http://www.w3.org/2001/XMLSchema#date> ;
        dc:modified                    "2017-04-01"^^<http://www.w3.org/2001/XMLSchema#date> ;
        dc:publisher                   <http://www.cefriel.com> ;
        dc:rights                      "Copyright Â© 2017 Cefriel" ;
        dc:title                       "BotDCAT-AP - Data Catalogue vocabulary Application Profile for chatbots"@en ;
        vann:preferredNamespacePrefix  "bot" ;
        vann:preferredNamespaceUri     "http://swa.cefriel.it/ontologies/botdcat-ap#" ;
        owl:imports                    <https://www.w3.org/ns/dcat> , <https://joinup.ec.europa.eu/site/core_vocabularies/registry/dcat-ap/DCAT-AP_v1.1.rdf> ;
        owl:versionInfo                1.0 .

<http://swa.cefriel.it/ontologies/botdcat-ap#hasEntitiesList>
        a                 owl:ObjectProperty ;
        rdfs:comment      "Optional property. Cardinality [0..n]. This property refers to an Entities Catalog connected to an Intent."@en ;
        rdfs:domain       <http://swa.cefriel.it/ontologies/botdcat-ap#Intent> ;
        rdfs:isDefinedBy  <http://swa.cefriel.it/ontologies/botdcat-ap> ;
        rdfs:label        "has Entities List"@en ;
        rdfs:range        <http://swa.cefriel.it/ontologies/botdcat-ap#EntitiesCatalog> ;
        vann:usageNote    "Optional property. Cardinality [0..n]. This property refers to an Entities Catalog describing the entities connected to an Intent."@en .

<http://swa.cefriel.it/ontologies/botdcat-ap#EntitiesCatalog>
        a                 owl:Class ;
        rdfs:comment      "Optional class. Represents a list of all the entities that can be associated to an Intent."@en ;
        rdfs:isDefinedBy  <http://swa.cefriel.it/ontologies/botdcat-ap> ;
        rdfs:label        "Entities Catalog"@en ;
        rdfs:subClassOf   owl:Thing ;
        vann:usageNote    "Optional class. Represents a list of all the entities that can be associated to an Intent."@en .

<http://swa.cefriel.it/ontologies/botdcat-ap#hasEntity>
        a                 owl:ObjectProperty ;
        rdfs:comment      "Optional property. Cardinality [0..n]. This property refers to an entity. Note that only one of bot:hasEntity, bot:hasEntityConcept and bot:hasEntityCatalog property for each entity must be used."@en ;
        rdfs:domain       <http://swa.cefriel.it/ontologies/botdcat-ap#EntitiesCatalog> ;
        rdfs:isDefinedBy  <http://swa.cefriel.it/ontologies/botdcat-ap> ;
        rdfs:label        "has Entity"@en ;
        rdfs:range        owl:Class ;
        vann:usageNote    "Optional property. Cardinality [0..n]. This property refers to an entity. Note that only one of bot:hasEntity, bot:hasEntityConcept and bot:hasEntityCatalog property for each entity must be used."@en .

<http://swa.cefriel.it/ontologies/botdcat-ap#hasDocumentation>
        a                 owl:ObjectProperty ;
        rdfs:comment      "Recommended property. Cardinality [0..1]. This property refers to a Resource containg information about an Intent."@en ;
        rdfs:domain       <http://swa.cefriel.it/ontologies/botdcat-ap#Intent> ;
        rdfs:isDefinedBy  <http://swa.cefriel.it/ontologies/botdcat-ap> ;
        rdfs:label        "has Documentation"@en ;
        rdfs:range        rdfs:Resource ;
        vann:usageNote    "Recommended property. Cardinality [0..1]. This property refers to a Resource containg information about an Intent."@en .

<http://swa.cefriel.it/ontologies/botdcat-ap#hasEntityDataset>
        a                 owl:ObjectProperty ;
        rdfs:comment      "Optional property. Cardinality [0..n]. This property refers to a Dataset containing all the istances of an entity. Note that only one of bot:hasEntity, bot:hasEntityConcept and bot:hasEntityCatalog property for each entity must be used."@en ;
        rdfs:domain       <http://swa.cefriel.it/ontologies/botdcat-ap#EntitiesCatalog> ;
        rdfs:isDefinedBy  <http://swa.cefriel.it/ontologies/botdcat-ap> ;
        rdfs:label        "has Entity Dataset"@en ;
        rdfs:range        <http://www.w3.org/ns/dcat#Dataset> ;
        vann:usageNote    "Optional property. Cardinality [0..n]. This property refers to a Dataset containing all the istances of an entity. Note that only one of bot:hasEntity, bot:hasEntityConcept and bot:hasEntityCatalog property for each entity must be used."@en .

<http://swa.cefriel.it/ontologies/botdcat-ap#hasEntityConcept>
        a                 owl:ObjectProperty ;
        rdfs:comment      "Optional property. Cardinality [0..n]. This property refers to an entity specified as a Concept. Note that only one of bot:hasEntity, bot:hasEntityConcept and bot:hasEntityCatalog property for each entity must be used."@en ;
        rdfs:domain       <http://swa.cefriel.it/ontologies/botdcat-ap#EntitiesCatalog> ;
        rdfs:isDefinedBy  <http://swa.cefriel.it/ontologies/botdcat-ap> ;
        rdfs:label        "has Entity Concept"@en ;
        rdfs:range        <http://www.w3.org/2004/02/skos/core#Concept> ;
        vann:usageNote    "Optional property. Cardinality [0..n]. This property refers to an entity specified as a Concept. Note that only one of bot:hasEntity, bot:hasEntityConcept and bot:hasEntityCatalog property for each entity must be used."@en .

<http://swa.cefriel.it/ontologies/botdcat-ap#hasMethodURL>
        a                 owl:ObjectProperty ;
        rdfs:comment      "Optional property. Cardinality [0..1]. This property contains the access URL provided by an API service handling the Intent."@en ;
        rdfs:domain       <http://swa.cefriel.it/ontologies/botdcat-ap#Intent> ;
        rdfs:isDefinedBy  <http://swa.cefriel.it/ontologies/botdcat-ap> ;
        rdfs:label        "has Method URL"@en ;
        rdfs:range        rdfs:Resource ;
        vann:usageNote    "Optional property. Cardinality [0..1]. This property contains the access URL provided by an API service handling the Intent."@en .
