@prefix :      <http://purl.org/net/soron#> .
@prefix dc:    <http://purl.org/dc/elements/1.1/> .
@prefix rdfs:  <http://www.w3.org/2000/01/rdf-schema#> .
@prefix foaf:  <http://xmlns.com/foaf/0.1/> .
@prefix terms: <http://purl.org/dc/terms/> .
@prefix owl:   <http://www.w3.org/2002/07/owl#> .
@prefix xsd:   <http://www.w3.org/2001/XMLSchema#> .
@prefix rdf:   <http://www.w3.org/1999/02/22-rdf-syntax-ns#> .
@prefix vann:  <http://purl.org/vocab/vann/> .

<http://purl.org/net/soron/feltNeutrallyBy>
        a                   owl:ObjectProperty ;
        rdfs:comment        "Describes that a person is being perceived neutrally (mixed feelings) by  another." ;
        rdfs:domain         foaf:Person ;
        rdfs:isDefinedBy    "http://purl.org/net/soron" ;
        rdfs:label          "Felt neutrally by" ;
        rdfs:range          foaf:Person ;
        rdfs:subPropertyOf  owl:differentFrom , <http://purl.org/net/soron/hasSocialRelationship> .

<http://purl.org/net/soron/admiredBy>
        a                   owl:ObjectProperty ;
        rdfs:comment        "Describes that a person is admired by another." ;
        rdfs:domain         foaf:Person ;
        rdfs:isDefinedBy    "http://purl.org/net/soron" ;
        rdfs:label          "Admired by" ;
        rdfs:range          foaf:Person ;
        rdfs:subPropertyOf  owl:differentFrom , <http://purl.org/net/soron/feltPositivelyBy> .

<http://purl.org/net/soron/employs>
        a                   owl:AsymmetricProperty , owl:ObjectProperty ;
        rdfs:comment        "Describes the relationship between the person that hires and the hired person." ;
        rdfs:domain         foaf:Person ;
        rdfs:isDefinedBy    "http://purl.org/net/soron" ;
        rdfs:label          "Employs" ;
        rdfs:range          foaf:Person ;
        rdfs:subPropertyOf  owl:differentFrom , <http://purl.org/net/soron/hasSocialRelationship> .

<http://purl.org/net/soron/loves>
        a                   owl:ObjectProperty ;
        rdfs:comment        "Describes that an individual loves another." ;
        rdfs:domain         foaf:Person ;
        rdfs:isDefinedBy    "http://purl.org/net/soron" ;
        rdfs:label          "Loves" ;
        rdfs:range          foaf:Person ;
        rdfs:subPropertyOf  foaf:knows , owl:differentFrom , <http://purl.org/net/soron/hasPositiveFeelingsFor> .

<http://purl.org/net/soron/hasPersonalRelationshipWith>
        a                   owl:ObjectProperty ;
        rdfs:comment        "Describes that a person has a personal, close relationship (not family related) with another." ;
        rdfs:domain         foaf:Person ;
        rdfs:isDefinedBy    "http://purl.org/net/soron" ;
        rdfs:label          "Has personal relationship with" ;
        rdfs:range          foaf:Person ;
        rdfs:subPropertyOf  foaf:knows , owl:differentFrom , <http://purl.org/net/soron/hasSocialRelationship> .

<http://purl.org/net/soron/ambivalentOf>
        a                   owl:ObjectProperty ;
        rdfs:comment        "Describes that a person is ambivalent of another." ;
        rdfs:domain         foaf:Person ;
        rdfs:isDefinedBy    "http://purl.org/net/soron" ;
        rdfs:label          "Is ambivalent of" ;
        rdfs:range          foaf:Person ;
        rdfs:subPropertyOf  owl:differentFrom , <http://purl.org/net/soron/hasNeutralFeelingsFor> .

<http://purl.org/net/soron/influences>
        a                   owl:ObjectProperty ;
        rdfs:comment        "Describes that a particular person has had some kind of influence on another individual. It does not imply that the person that has that influence on the other is aware of that influence at all." ;
        rdfs:domain         foaf:Person ;
        rdfs:isDefinedBy    "http://purl.org/net/soron" ;
        rdfs:label          "Influences" ;
        rdfs:range          foaf:Person ;
        rdfs:subPropertyOf  owl:differentFrom , <http://purl.org/net/soron/knownBy> .

<http://purl.org/net/soron/performsWith>
        a                   owl:ObjectProperty , owl:SymmetricProperty ;
        rdfs:comment        "Describes that an artist (musicians, artists, etc.) performs with another." ;
        rdfs:domain         foaf:Person ;
        rdfs:isDefinedBy    "http://purl.org/net/soron" ;
        rdfs:label          "Performs with" ;
        rdfs:range          foaf:Person ;
        rdfs:subPropertyOf  owl:differentFrom , <http://purl.org/net/soron/worksWith> , foaf:knows .

<http://purl.org/net/soron/admires>
        a                   owl:ObjectProperty ;
        rdfs:comment        "Describes that an individual feels admiration for another." ;
        rdfs:domain         foaf:Person ;
        rdfs:isDefinedBy    "http://purl.org/net/soron" ;
        rdfs:label          "Admires" ;
        rdfs:range          foaf:Person ;
        rdfs:subPropertyOf  owl:differentFrom , <http://purl.org/net/soron/hasPositiveFeelingsFor> .

<http://purl.org/net/soron/acquaintanceOf>
        a                   owl:ObjectProperty , owl:SymmetricProperty ;
        rdfs:comment        "Describes a person that knows another but there is no strong personal relationship between them." ;
        rdfs:domain         foaf:Person ;
        rdfs:isDefinedBy    "http://purl.org/net/soron" ;
        rdfs:label          "Is acquaintance of" ;
        rdfs:range          foaf:Person ;
        rdfs:subPropertyOf  foaf:knows , owl:differentFrom , <http://purl.org/net/soron/hasPersonalRelationshipWith> .

<http://purl.org/net/soron/associateOf>
        a                   owl:ObjectProperty , owl:SymmetricProperty ;
        rdfs:comment        "Describes that a person is associate of another." ;
        rdfs:domain         foaf:Person ;
        rdfs:isDefinedBy    "http://purl.org/net/soron" ;
        rdfs:label          "Is associate of" ;
        rdfs:range          foaf:Person ;
        rdfs:subPropertyOf  <http://purl.org/net/soron/worksWith> , owl:differentFrom , foaf:knows .

<http://purl.org/net/soron/likes>
        a                   owl:ObjectProperty ;
        rdfs:comment        "Describes that an individual likes another." ;
        rdfs:domain         foaf:Person ;
        rdfs:isDefinedBy    "http://purl.org/net/soron" ;
        rdfs:label          "Likes" ;
        rdfs:range          foaf:Person ;
        rdfs:subPropertyOf  owl:differentFrom , <http://purl.org/net/soron/hasPositiveFeelingsFor> .

terms:license  a  owl:AnnotationProperty .

<http://purl.org/net/soron/knownBy>
        a                   owl:AsymmetricProperty , owl:ObjectProperty ;
        rdfs:comment        "Describes that a person is known by another." ;
        rdfs:domain         foaf:Person ;
        rdfs:isDefinedBy    "http://purl.org/net/soron" ;
        rdfs:label          "Known by" ;
        rdfs:range          foaf:Person ;
        rdfs:subPropertyOf  owl:differentFrom , <http://purl.org/net/soron/hasSocialRelationship> .

<http://purl.org/net/soron/feltPositivelyBy>
        a                   owl:ObjectProperty ;
        rdfs:comment        "Describes that a person is being perceived positively by another." ;
        rdfs:domain         foaf:Person ;
        rdfs:isDefinedBy    "http://purl.org/net/soron" ;
        rdfs:label          "Felt positively by" ;
        rdfs:range          foaf:Person ;
        rdfs:subPropertyOf  owl:differentFrom , <http://purl.org/net/soron/hasSocialRelationship> .

<http://purl.org/net/soron/workPartnerOf>
        a                   owl:SymmetricProperty , owl:ObjectProperty ;
        rdfs:comment        "Describes that someone is work partner of someone else." ;
        rdfs:domain         foaf:Person ;
        rdfs:isDefinedBy    "http://purl.org/net/soron" ;
        rdfs:label          "Is work partner of" ;
        rdfs:range          foaf:Person ;
        rdfs:subPropertyOf  owl:differentFrom , <http://purl.org/net/soron/worksWith> , foaf:knows .

<http://purl.org/net/soron/knows>
        a                   owl:ObjectProperty ;
        rdfs:comment        "Describes the relationship between two individuals that know each other." ;
        rdfs:domain         foaf:Person ;
        rdfs:isDefinedBy    "http://purl.org/net/soron" ;
        rdfs:label          "Knows" ;
        rdfs:range          foaf:Person ;
        rdfs:subPropertyOf  owl:differentFrom , <http://purl.org/net/soron/hasSocialRelationship> .

<http://purl.org/net/soron/hatedBy>
        a                   owl:ObjectProperty ;
        rdfs:comment        "Describes that a person is hated by another." ;
        rdfs:domain         foaf:Person ;
        rdfs:isDefinedBy    "http://purl.org/net/soron" ;
        rdfs:label          "Hated by" ;
        rdfs:range          foaf:Person ;
        rdfs:subPropertyOf  owl:differentFrom , <http://purl.org/net/soron/FeltNegativelyBy> .

<http://purl.org/net/soron/FeltNegativelyBy>
        a                   owl:ObjectProperty ;
        rdfs:comment        "Describes that a person is perceived negatively by another." ;
        rdfs:domain         foaf:Person ;
        rdfs:isDefinedBy    "http://purl.org/net/soron" ;
        rdfs:label          "Felt negatively by" ;
        rdfs:range          foaf:Person ;
        rdfs:subPropertyOf  owl:differentFrom , <http://purl.org/net/soron/hasSocialRelationship> .

<http://purl.org/net/soron/feltAntagonistBy>
        a                   owl:ObjectProperty ;
        rdfs:comment        "Describes that a person is perceived as antagonist by another." ;
        rdfs:domain         foaf:Person ;
        rdfs:isDefinedBy    "http://purl.org/net/soron" ;
        rdfs:label          "Felt as antagonist by" ;
        rdfs:range          foaf:Person ;
        rdfs:subPropertyOf  owl:differentFrom , <http://purl.org/net/soron/FeltNegativelyBy> .

<http://purl.org/net/soron/worksWith>
        a                   owl:SymmetricProperty , owl:ObjectProperty ;
        rdfs:comment        "Describes the relationship between two individuals working together in paid or unpaid tasks in any kind of context/organization." ;
        rdfs:domain         foaf:Person ;
        rdfs:isDefinedBy    "http://purl.org/net/soron" ;
        rdfs:label          "Works with" ;
        rdfs:range          foaf:Person ;
        rdfs:subPropertyOf  owl:differentFrom , <http://purl.org/net/soron/hasSocialRelationship> .

<http://purl.org/net/soron/appreciatedBy>
        a                   owl:ObjectProperty ;
        rdfs:comment        "Describes that a person is appreciated by another." ;
        rdfs:domain         foaf:Person ;
        rdfs:isDefinedBy    "http://purl.org/net/soron" ;
        rdfs:label          "Appreciated by" ;
        rdfs:range          foaf:Person ;
        rdfs:subPropertyOf  owl:differentFrom , <http://purl.org/net/soron/feltPositivelyBy> .

<http://purl.org/net/soron/appreciates>
        a                   owl:ObjectProperty ;
        rdfs:comment        "Describes that an individual appreciates another person." ;
        rdfs:domain         foaf:Person ;
        rdfs:isDefinedBy    "http://purl.org/net/soron" ;
        rdfs:label          "Appreciates" ;
        rdfs:range          foaf:Person ;
        rdfs:subPropertyOf  owl:differentFrom , <http://purl.org/net/soron/hasPositiveFeelingsFor> .

<http://purl.org/net/soron/mentionedBy>
        a                   owl:ObjectProperty ;
        rdfs:comment        "Describes that an individual has been mentioned/referred to by another. It does not imply that the person that is being mentioned knows the person that mentions him/her." ;
        rdfs:domain         foaf:Person ;
        rdfs:isDefinedBy    "http://purl.org/net/soron" ;
        rdfs:label          "Is mentioned by" ;
        rdfs:range          foaf:Person ;
        rdfs:subPropertyOf  owl:differentFrom , <http://purl.org/net/soron/knownBy> .

<http://purl.org/net/soron/disagreedBy>
        a                   owl:ObjectProperty ;
        rdfs:comment        "Describes that a person is disagreed by another." ;
        rdfs:domain         foaf:Person ;
        rdfs:isDefinedBy    "http://purl.org/net/soron" ;
        rdfs:label          "Disagreed by" ;
        rdfs:range          foaf:Person ;
        rdfs:subPropertyOf  owl:differentFrom , <http://purl.org/net/soron/FeltNegativelyBy> .

<http://purl.org/net/soron/antagonistOf>
        a                   owl:ObjectProperty ;
        rdfs:comment        "Describes that a person perceives another as antagonist." ;
        rdfs:domain         foaf:Person ;
        rdfs:isDefinedBy    "http://purl.org/net/soron" ;
        rdfs:label          "Is antagonist of" ;
        rdfs:range          foaf:Person ;
        rdfs:subPropertyOf  owl:differentFrom , <http://purl.org/net/soron/hasNegativeFeelingsFor> .

<http://purl.org/net/soron/critizisedBy>
        a                   owl:ObjectProperty ;
        rdfs:comment        "Describes that a person is critizised by another." ;
        rdfs:domain         foaf:Person ;
        rdfs:isDefinedBy    "http://purl.org/net/soron" ;
        rdfs:label          "Critizised by" ;
        rdfs:range          foaf:Person ;
        rdfs:subPropertyOf  owl:differentFrom , <http://purl.org/net/soron/FeltNegativelyBy> .

<http://purl.org/net/soron/hates>
        a                   owl:ObjectProperty ;
        rdfs:comment        "Describes that a person hates another." ;
        rdfs:domain         foaf:Person ;
        rdfs:isDefinedBy    "http://purl.org/net/soron" ;
        rdfs:label          "Hates" ;
        rdfs:range          foaf:Person ;
        rdfs:subPropertyOf  owl:differentFrom , <http://purl.org/net/soron/hasNegativeFeelingsFor> .

<http://purl.org/net/soron/critizises>
        a                   owl:ObjectProperty ;
        rdfs:comment        "Describes that a person critizises another." ;
        rdfs:domain         foaf:Person ;
        rdfs:isDefinedBy    "http://purl.org/net/soron" ;
        rdfs:label          "Critizises" ;
        rdfs:range          foaf:Person ;
        rdfs:subPropertyOf  owl:differentFrom , <http://purl.org/net/soron/hasNegativeFeelingsFor> .

<http://purl.org/net/soron/rejects>
        a                   owl:ObjectProperty ;
        rdfs:comment        "Describes that a person rejects another." ;
        rdfs:domain         foaf:Person ;
        rdfs:isDefinedBy    "http://purl.org/net/soron" ;
        rdfs:label          "Rejects" ;
        rdfs:range          foaf:Person ;
        rdfs:subPropertyOf  owl:differentFrom , <http://purl.org/net/soron/hasNegativeFeelingsFor> .

<http://purl.org/net/soron/rejectedBy>
        a                   owl:ObjectProperty ;
        rdfs:comment        "Describes that a person is rejected by another." ;
        rdfs:domain         foaf:Person ;
        rdfs:isDefinedBy    "http://purl.org/net/soron" ;
        rdfs:label          "Rejected by" ;
        rdfs:range          foaf:Person ;
        rdfs:subPropertyOf  owl:differentFrom , <http://purl.org/net/soron/FeltNegativelyBy> .

<http://purl.org/net/soron/hasMet>
        a                   owl:SymmetricProperty , owl:ObjectProperty ;
        rdfs:comment        "Describes that a person has met another. It usually implies some kind of physical interaction, but it may also happen virtually." ;
        rdfs:domain         foaf:Person ;
        rdfs:isDefinedBy    "http://purl.org/net/soron" ;
        rdfs:label          "Has met" ;
        rdfs:range          foaf:Person ;
        rdfs:subPropertyOf  <http://purl.org/net/soron/knows> , owl:differentFrom , foaf:knows .

<http://purl.org/net/soron/colleagueOf>
        a                   owl:ObjectProperty , owl:SymmetricProperty ;
        rdfs:comment        "Describes that a person is colleague of someone else (work related)." ;
        rdfs:domain         foaf:Person ;
        rdfs:isDefinedBy    "http://purl.org/net/soron" ;
        rdfs:label          "Is colleague of" ;
        rdfs:range          foaf:Person ;
        rdfs:subPropertyOf  <http://purl.org/net/soron/worksWith> , foaf:knows , owl:differentFrom .

<http://purl.org/net/soron/hasNeutralFeelingsFor>
        a                   owl:ObjectProperty ;
        rdfs:comment        "Describes that a person has neutral (mixed) feelings for another." ;
        rdfs:domain         foaf:Person ;
        rdfs:isDefinedBy    "http://purl.org/net/soron" ;
        rdfs:label          "Has neutral feelings for" ;
        rdfs:range          foaf:Person ;
        rdfs:subPropertyOf  owl:differentFrom , <http://purl.org/net/soron/hasSocialRelationship> .

<http://purl.org/net/soron>
        a                              owl:Ontology ;
        rdfs:comment                   "Originally developed for a research project funded by the Spanish Ministry of Education, Culture and Sport." ;
        dc:creator                     "F. Javier Calzada-Prado (UC3M Carlos III University of Madrid, Spain)." ;
        dc:date                        "May 12, 2015" ;
        dc:description                 "The Social Relationships ONtology (SORON) attempts to describe the different types of social relationships in society (both objective and subjective). Current version focuses on inter-personal 1:1 relationships (except family relationships). Other types of relationships may be covered in later versions. It complements FOAF and RELATIONSHIP ontologies." ;
        dc:title                       "SORON: Social Relationships ONtology" ;
        terms:issued                   "2015-05-12" ;
        terms:license                  "http://creativecommons.org/licenses/by-nc-sa/4.0/" ;
        vann:preferredNamespacePrefix  "sor" ;
        vann:preferredNamespaceUri     "http://purl.org/net/soron" ;
        owl:imports                    foaf: , <http://purl.org/vocab/relationship/> ;
        owl:versionIRI                 <http://purl.org/net/soron/0.1> ;
        owl:versionInfo                0.1 .

<http://purl.org/net/soron/patronOf>
        a                   owl:AsymmetricProperty , owl:ObjectProperty ;
        rdfs:comment        "Describes that a person sponsors the work of another (usually an artist or intellectual)." ;
        rdfs:domain         foaf:Person ;
        rdfs:isDefinedBy    "http://purl.org/net/soron" ;
        rdfs:label          "Is patron of" ;
        rdfs:range          foaf:Person ;
        rdfs:subPropertyOf  <http://purl.org/net/soron/employs> , owl:differentFrom , foaf:knows .

<http://purl.org/net/soron/masterOf>
        a                   owl:AsymmetricProperty , owl:ObjectProperty ;
        rdfs:comment        "Describes the relationship between an expert/master and their apprentice (particularly used in art, craftmanship, etc.). Example: Rubens masterOf Anthony Van Dick   (it implies that Rubens hired Van Dick as apprentice in his studio)." ;
        rdfs:domain         foaf:Person ;
        rdfs:isDefinedBy    "http://purl.org/net/soron" ;
        rdfs:label          "Is master of" ;
        rdfs:range          foaf:Person ;
        rdfs:subPropertyOf  owl:differentFrom , foaf:knows , <http://purl.org/net/soron/employs> .

<http://purl.org/net/soron/mentorOf>
        a                   owl:AsymmetricProperty , owl:ObjectProperty ;
        rdfs:comment        "Describes the relationship between a mentor and a mentee (for instance a supervisor in an academic setting). It implies that it is an unpaid relationship." ;
        rdfs:domain         foaf:Person ;
        rdfs:isDefinedBy    "http://purl.org/net/soron" ;
        rdfs:label          "Is mentor of" ;
        rdfs:range          foaf:Person ;
        rdfs:subPropertyOf  <http://purl.org/net/soron/worksWith> , foaf:knows , owl:differentFrom .

<http://purl.org/net/soron/hasSocialRelationship>
        a                   owl:ObjectProperty ;
        rdfs:comment        "Describes any kind of social relationship that may appear in society." ;
        rdfs:domain         foaf:Person ;
        rdfs:isDefinedBy    "http://purl.org/net/soron" ;
        rdfs:label          "Has social relationship" ;
        rdfs:range          foaf:Person ;
        rdfs:subPropertyOf  owl:differentFrom .

<http://purl.org/net/soron/dislikedBy>
        a                   owl:ObjectProperty ;
        rdfs:comment        "Describes that a person is disliked by another." ;
        rdfs:domain         foaf:Person ;
        rdfs:isDefinedBy    "http://purl.org/net/soron" ;
        rdfs:label          "Disliked by" ;
        rdfs:range          foaf:Person ;
        rdfs:subPropertyOf  owl:differentFrom , <http://purl.org/net/soron/FeltNegativelyBy> .

<http://purl.org/net/soron/apprenticeTo>
        a                   owl:AsymmetricProperty , owl:ObjectProperty ;
        rdfs:comment        "Describes the relationship between an individual and their apprentice (in any kind of profession)." ;
        rdfs:domain         foaf:Person ;
        rdfs:isDefinedBy    "http://purl.org/net/soron" ;
        rdfs:label          "Is apprentice to" ;
        rdfs:range          foaf:Person ;
        rdfs:subPropertyOf  <http://purl.org/net/soron/worksFor> , foaf:knows , owl:differentFrom ;
        owl:inverseOf       <http://purl.org/net/soron/apprenticeIs> .

<http://purl.org/net/soron/worksFor>
        a                   owl:AsymmetricProperty , owl:ObjectProperty ;
        rdfs:comment        "Describes the relationship between a particular individual and the person that hires them." ;
        rdfs:domain         foaf:Person ;
        rdfs:isDefinedBy    "http://purl.org/net/soron" ;
        rdfs:label          "Works for" ;
        rdfs:range          foaf:Person ;
        rdfs:subPropertyOf  owl:differentFrom , <http://purl.org/net/soron/hasSocialRelationship> .

<http://purl.org/net/soron/loverOf>
        a                   owl:ObjectProperty , owl:SymmetricProperty ;
        rdfs:comment        "Describes that a peson is the lover of someone else." ;
        rdfs:domain         foaf:Person ;
        rdfs:isDefinedBy    "http://purl.org/net/soron" ;
        rdfs:label          "Is lover of" ;
        rdfs:range          foaf:Person ;
        rdfs:subPropertyOf  owl:differentFrom , <http://purl.org/net/soron/hasPersonalRelationshipWith> , foaf:knows .

<http://purl.org/net/soron/cites>
        a                   owl:ObjectProperty ;
        rdfs:comment        "Describes an individual's knowledge of someone else and their work by citing their words/ideas/works. It does not imply physical/real knowledge of the cited individual." ;
        rdfs:domain         foaf:Person ;
        rdfs:isDefinedBy    "http://purl.org/net/soron" ;
        rdfs:label          "Cites" ;
        rdfs:range          foaf:Person ;
        rdfs:subPropertyOf  owl:differentFrom , <http://purl.org/net/soron/knows> ;
        owl:inverseOf       <http://purl.org/net/soron/citedBy> .

<http://purl.org/net/soron/lovedBy>
        a                   owl:ObjectProperty ;
        rdfs:comment        "Describes that a person is loved by another." ;
        rdfs:domain         foaf:Person ;
        rdfs:isDefinedBy    "http://purl.org/net/soron" ;
        rdfs:label          "Loved by" ;
        rdfs:range          foaf:Person ;
        rdfs:subPropertyOf  foaf:knows , owl:differentFrom , <http://purl.org/net/soron/feltPositivelyBy> .

<http://purl.org/net/soron/friendOf>
        a                   owl:ObjectProperty , owl:SymmetricProperty ;
        rdfs:comment        "Describes that a person has a strong personal relationship with another." ;
        rdfs:domain         foaf:Person ;
        rdfs:isDefinedBy    "http://purl.org/net/soron" ;
        rdfs:label          "Is friend of" ;
        rdfs:range          foaf:Person ;
        rdfs:subPropertyOf  <http://purl.org/net/soron/hasPersonalRelationshipWith> , foaf:knows , owl:differentFrom .

<http://purl.org/net/soron/assistedBy>
        a                   owl:AsymmetricProperty , owl:ObjectProperty ;
        rdfs:comment        "Describes that a person has someone working for them as assistant." ;
        rdfs:domain         foaf:Person ;
        rdfs:isDefinedBy    "http://purl.org/net/soron" ;
        rdfs:label          "Assisted by" ;
        rdfs:range          foaf:Person ;
        rdfs:subPropertyOf  <http://purl.org/net/soron/employs> , foaf:knows , owl:differentFrom .

<http://purl.org/net/soron/hiredBy>
        a                   owl:AsymmetricProperty , owl:ObjectProperty ;
        rdfs:comment        "Describes that an individual is paid by another to do some kind of work." ;
        rdfs:domain         foaf:Person ;
        rdfs:isDefinedBy    "http://purl.org/net/soron" ;
        rdfs:label          "Hired by" ;
        rdfs:range          foaf:Person ;
        rdfs:subPropertyOf  <http://purl.org/net/soron/worksFor> ;
        owl:inverseOf       <http://purl.org/net/soron/hires> .

<http://purl.org/net/soron/inCahootsWith>
        a                   owl:ObjectProperty , owl:SymmetricProperty ;
        rdfs:comment        "Describes that a person is in cahoots with someone else." ;
        rdfs:domain         foaf:Person ;
        rdfs:isDefinedBy    "http://purl.org/net/soron" ;
        rdfs:label          "In cahoots with" ;
        rdfs:range          foaf:Person ;
        rdfs:subPropertyOf  <http://purl.org/net/soron/worksWith> , foaf:knows , owl:differentFrom .

<http://purl.org/net/soron/feltAmbivalentBy>
        a                   owl:ObjectProperty ;
        rdfs:comment        "Describes that a person is felt ambivalently by another." ;
        rdfs:domain         foaf:Person ;
        rdfs:isDefinedBy    "http://purl.org/net/soron" ;
        rdfs:label          "Felt ambivalent by" ;
        rdfs:range          foaf:Person ;
        rdfs:subPropertyOf  owl:differentFrom , <http://purl.org/net/soron/feltNeutrallyBy> .

<http://purl.org/net/soron/dislikes>
        a                   owl:ObjectProperty ;
        rdfs:comment        "Describes that a person dislikes another." ;
        rdfs:domain         foaf:Person ;
        rdfs:isDefinedBy    "http://purl.org/net/soron" ;
        rdfs:label          "Dislikes" ;
        rdfs:range          foaf:Person ;
        rdfs:subPropertyOf  owl:differentFrom , <http://purl.org/net/soron/hasNegativeFeelingsFor> .

<http://purl.org/net/soron/coauthorsWith>
        a                   owl:SymmetricProperty , owl:ObjectProperty ;
        rdfs:comment        "Describes that a person coauthors a work with someone else." ;
        rdfs:domain         foaf:Person ;
        rdfs:isDefinedBy    "http://purl.org/net/soron" ;
        rdfs:label          "Coauthors with" ;
        rdfs:range          foaf:Person ;
        rdfs:subPropertyOf  owl:differentFrom , <http://purl.org/net/soron/worksWith> , foaf:knows .

<http://purl.org/net/soron/hasPositiveFeelingsFor>
        a                   owl:ObjectProperty ;
        rdfs:comment        "Describes that a person has positive feelings about another." ;
        rdfs:domain         foaf:Person ;
        rdfs:isDefinedBy    "http://purl.org/net/soron" ;
        rdfs:label          "Has positive feelings for" ;
        rdfs:range          foaf:Person ;
        rdfs:subPropertyOf  owl:differentFrom , <http://purl.org/net/soron/hasSocialRelationship> .

<http://purl.org/net/soron/assistantFor>
        a                   owl:AsymmetricProperty , owl:ObjectProperty ;
        rdfs:comment        "Describes that a person works as assistant for someone else." ;
        rdfs:domain         foaf:Person ;
        rdfs:isDefinedBy    "http://purl.org/net/soron" ;
        rdfs:label          "Is assistant for" ;
        rdfs:range          foaf:Person ;
        rdfs:subPropertyOf  owl:differentFrom , foaf:knows , <http://purl.org/net/soron/worksFor> ;
        owl:inverseOf       <http://purl.org/net/soron/assistedBy> .

<http://purl.org/net/soron/hires>
        a                   owl:AsymmetricProperty , owl:ObjectProperty ;
        rdfs:comment        "Describes that an individual pays someone else to do some kind of work." ;
        rdfs:domain         foaf:Person ;
        rdfs:isDefinedBy    "http://purl.org/net/soron" ;
        rdfs:label          "Hires" ;
        rdfs:range          foaf:Person ;
        rdfs:subPropertyOf  owl:differentFrom , <http://purl.org/net/soron/employs> .

<http://purl.org/net/soron/apprenticeIs>
        a                   owl:ObjectProperty , owl:AsymmetricProperty ;
        rdfs:comment        "Describes the relationship between an apprentice and their master (in any kind of profession)." ;
        rdfs:domain         foaf:Person ;
        rdfs:isDefinedBy    "http://purl.org/net/soron" ;
        rdfs:label          "Apprentice is" ;
        rdfs:range          foaf:Person ;
        rdfs:subPropertyOf  <http://purl.org/net/soron/employs> , owl:differentFrom , foaf:knows .

<http://purl.org/net/soron/menteeOf>
        a                   owl:AsymmetricProperty , owl:ObjectProperty ;
        rdfs:comment        "Describes the relationship between a mentee (in an academic setting, the student) and a mentor. It implies that it is an unpaid relationship." ;
        rdfs:domain         foaf:Person ;
        rdfs:isDefinedBy    "http://purl.org/net/soron" ;
        rdfs:label          "Is mentee of" ;
        rdfs:range          foaf:Person ;
        rdfs:subPropertyOf  foaf:knows , owl:differentFrom , <http://purl.org/net/soron/worksWith> ;
        owl:inverseOf       <http://purl.org/net/soron/mentorOf> .

<http://purl.org/net/soron/feltEnemyBy>
        a                   owl:ObjectProperty ;
        rdfs:comment        "Describes that a person is perceived as enemy by another." ;
        rdfs:domain         foaf:Person ;
        rdfs:isDefinedBy    "http://purl.org/net/soron" ;
        rdfs:label          "Felt as enemy by" ;
        rdfs:range          foaf:Person ;
        rdfs:subPropertyOf  owl:differentFrom , <http://purl.org/net/soron/FeltNegativelyBy> .

<http://purl.org/net/soron/citedBy>
        a                   owl:ObjectProperty ;
        rdfs:comment        "Describes that an individual's words/ideas/works have been cited by someone  else. It does not imply that the cited individual has any knowledge of the citing individual or the fact that they had been cited." ;
        rdfs:domain         foaf:Person ;
        rdfs:isDefinedBy    "http://purl.org/net/soron" ;
        rdfs:label          "Cited by" ;
        rdfs:range          foaf:Person ;
        rdfs:subPropertyOf  owl:differentFrom , <http://purl.org/net/soron/knownBy> .

<http://purl.org/net/soron/hasNegativeFeelingsFor>
        a                   owl:ObjectProperty ;
        rdfs:comment        "Describes that a person has negative feelings for another." ;
        rdfs:domain         foaf:Person ;
        rdfs:isDefinedBy    "http://purl.org/net/soron" ;
        rdfs:label          "Has negative feelings for" ;
        rdfs:range          foaf:Person ;
        rdfs:subPropertyOf  owl:differentFrom , <http://purl.org/net/soron/hasSocialRelationship> .

<http://purl.org/net/soron/hasHeardOf>
        a                   owl:ObjectProperty ;
        rdfs:comment        "Describes that a person has heard of another." ;
        rdfs:domain         foaf:Person ;
        rdfs:isDefinedBy    "http://purl.org/net/soron" ;
        rdfs:label          "Has heard of" ;
        rdfs:range          foaf:Person ;
        rdfs:subPropertyOf  owl:differentFrom , <http://purl.org/net/soron/knows> .

<http://purl.org/net/soron/influencedBy>
        a                   owl:ObjectProperty ;
        rdfs:comment        "Describes that a particular person has been influenced by another individual (writer, artist, etc.)." ;
        rdfs:domain         foaf:Person ;
        rdfs:isDefinedBy    "http://purl.org/net/soron" ;
        rdfs:label          "Is influenced by" ;
        rdfs:range          foaf:Person ;
        rdfs:subPropertyOf  owl:differentFrom , <http://purl.org/net/soron/knows> ;
        owl:inverseOf       <http://purl.org/net/soron/influences> .

<http://purl.org/net/soron/patronIs>
        a                   owl:AsymmetricProperty , owl:ObjectProperty ;
        rdfs:comment        "Describes that a person (usually an artist or intellectual) is sponsored by another." ;
        rdfs:domain         foaf:Person ;
        rdfs:isDefinedBy    "http://purl.org/net/soron" ;
        rdfs:label          "Patron is" ;
        rdfs:range          foaf:Person ;
        rdfs:subPropertyOf  <http://purl.org/net/soron/worksFor> , owl:differentFrom , foaf:knows ;
        owl:inverseOf       <http://purl.org/net/soron/patronOf> .

<http://purl.org/net/soron/masterIs>
        a                   owl:ObjectProperty , owl:AsymmetricProperty ;
        rdfs:comment        "Describes the relationship between an individual and their master (particularly used in art, craftmanship, etc.). Example: Anthony Van Dick masterIs Rubens (it implies that Van Dick worked for Rubens' studio)." ;
        rdfs:domain         foaf:Person ;
        rdfs:isDefinedBy    "http://purl.org/net/soron" ;
        rdfs:label          "Master is" ;
        rdfs:range          foaf:Person ;
        rdfs:subPropertyOf  foaf:knows , owl:differentFrom , <http://purl.org/net/soron/worksFor> ;
        owl:inverseOf       <http://purl.org/net/soron/masterOf> .

<http://purl.org/net/soron/enemyOf>
        a                   owl:ObjectProperty ;
        rdfs:comment        "Describes that a person is the enemy of another." ;
        rdfs:domain         foaf:Person ;
        rdfs:isDefinedBy    "http://purl.org/net/soron" ;
        rdfs:label          "Is enemy of" ;
        rdfs:range          foaf:Person ;
        rdfs:subPropertyOf  owl:differentFrom , <http://purl.org/net/soron/hasNegativeFeelingsFor> .

<http://purl.org/net/soron/mentions>
        a                   owl:ObjectProperty ;
        rdfs:comment        "Describes that the name of an individual has been mentioned by another." ;
        rdfs:domain         foaf:Person ;
        rdfs:isDefinedBy    "http://purl.org/net/soron" ;
        rdfs:label          "Mentions" ;
        rdfs:range          foaf:Person ;
        rdfs:subPropertyOf  owl:differentFrom , <http://purl.org/net/soron/knows> ;
        owl:inverseOf       <http://purl.org/net/soron/mentionedBy> .

<http://purl.org/net/soron/fellowStudentOf>
        a                   owl:SymmetricProperty , owl:ObjectProperty ;
        rdfs:comment        "Describes that a person studies with someone else." ;
        rdfs:domain         foaf:Person ;
        rdfs:isDefinedBy    "http://purl.org/net/soron" ;
        rdfs:label          "Is fellow student of" ;
        rdfs:range          foaf:Person ;
        rdfs:subPropertyOf  owl:differentFrom , <http://purl.org/net/soron/worksWith> .

<http://purl.org/net/soron/disagreesWith>
        a                   owl:ObjectProperty ;
        rdfs:comment        "Describes that a person disagrees with another." ;
        rdfs:domain         foaf:Person ;
        rdfs:isDefinedBy    "http://purl.org/net/soron" ;
        rdfs:label          "Disagrees with" ;
        rdfs:range          foaf:Person ;
        rdfs:subPropertyOf  owl:differentFrom , <http://purl.org/net/soron/hasNegativeFeelingsFor> .

<http://purl.org/net/soron/collaboratesWith>
        a                   owl:SymmetricProperty , owl:ObjectProperty ;
        rdfs:comment        "Describes that a person collaborates with another in a particular task/project/work." ;
        rdfs:domain         foaf:Person ;
        rdfs:isDefinedBy    "http://purl.org/net/soron" ;
        rdfs:label          "Collaborates with" ;
        rdfs:range          foaf:Person ;
        rdfs:subPropertyOf  <http://purl.org/net/soron/worksWith> , foaf:knows , owl:differentFrom .

<http://purl.org/net/soron/likedBy>
        a                   owl:ObjectProperty ;
        rdfs:comment        "Describes that a person is liked by another." ;
        rdfs:domain         foaf:Person ;
        rdfs:isDefinedBy    "http://purl.org/net/soron" ;
        rdfs:label          "Liked by" ;
        rdfs:range          foaf:Person ;
        rdfs:subPropertyOf  owl:differentFrom , <http://purl.org/net/soron/feltPositivelyBy> .
