@prefix dc:    <http://purl.org/dc/elements/1.1/> .
@prefix :      <http://d-nb.info/standards/elementset/agrelon.owl#> .
@prefix rdfs:  <http://www.w3.org/2000/01/rdf-schema#> .
@prefix owl:   <http://www.w3.org/2002/07/owl#> .
@prefix xsd:   <http://www.w3.org/2001/XMLSchema#> .
@prefix rdf:   <http://www.w3.org/1999/02/22-rdf-syntax-ns#> .
@prefix dcterms: <http://purl.org/dc/terms/> .

:HasAdoptiveChildParent
        a                owl:Class ;
        rdfs:comment     "This is the n-ary concept for the properties hasAdoptiveChild and hasAdoptiveParent"^^xsd:string ;
        rdfs:label       "ha figlio(a) / genitore adottivo(a)"@it , "tiene hijo(a) / padre / madre adoptivo(a)"@es , "has adoptive child / adoptive parent"@en , "hat Adoptivkind / Adoptivelter"@de ;
        rdfs:seeAlso     :hasAdoptiveParent , :hasAdoptiveChild ;
        rdfs:subClassOf  :HasChildParent .

:hasFosterChild  a          owl:ObjectProperty ;
        rdfs:comment        "A person (subject) fostered a person (object), without being a biological parent."^^xsd:string ;
        rdfs:label          "ha pupillo(a)"@it , "tiene hijo(a) de crianza"@es , "has foster child"@en , "hat Pflegekind"@de ;
        rdfs:subPropertyOf  :hasChild ;
        :correspondsTo      :HasFosterChildParent ;
        owl:inverseOf       :hasFosterParent .

:hasSpiritualContact  a     owl:SymmetricProperty ;
        rdfs:comment        "A person or spiritual entity (subject) has some kind of spiritual relation with a person or spiritual entity (object). The relationship may e.g. be channelling, guru-devotee, or a psychoanalyst-patient."^^xsd:string ;
        rdfs:label          "ha contatto spirituale"@it , "tiene guía espiritual"@es , "has spiritual contact"@en , "hat spirituellen Kontakt"@de ;
        rdfs:subPropertyOf  :relatedAgent ;
        :correspondsTo      :HasSpiritualContact .

rdfs:comment  a  owl:AnnotationProperty .

:hasSubjectObject  a   owl:ObjectProperty ;
        rdfs:comment   "At an n-ary concept's instance (subject), something (object) takes the subject or object role of the symmetric relationship meant by the n-ary concept. \nFor inverse relationsships, the subject and object role follow the naming of the n-ary concept when reading quasi just the first part of the n-ary concept name."^^xsd:string ;
        rdfs:label     "ha soggetto o oggetto"@it , "tiene sujeto u objeto"@es , "has subject or object"@en , "hat Subjekt oder Objekt"@de ;
        owl:inverseOf  :isSubjectObject .

:hasIllegitimateChild
        a                   owl:ObjectProperty ;
        rdfs:comment        "A person (subject) begot/conceived a person (object), without the two biological parents being married at the child's day of birth."^^xsd:string ;
        rdfs:label          "ha figlio(a) illegittimo(a)"@it , "tiene hijo(a) illegítimo(a)"@es , "has illegitimate child"@en , "hat illegitimes Kind"@de ;
        rdfs:subPropertyOf  :hasBiologicalChild ;
        :correspondsTo      :HasIllegitimateChildParent .

:hasColleague  a            owl:SymmetricProperty ;
        rdfs:comment        "A person (subject) works together with a person (object) at the same corporation."^^xsd:string ;
        rdfs:label          "ha collega"@it , "tiene colega"@es , "has colleague"@en , "hat Kollege"@de ;
        rdfs:subPropertyOf  :hasProfessionalContact ;
        :correspondsTo      :HasColleague .

:HasAdoptiveSibling  a   owl:Class ;
        rdfs:comment     "This is the n-ary concept for the property hasAdoptiveSibling"^^xsd:string ;
        rdfs:label       "ha fratello adottato o sorella adottata"@it , "tiene hermano(a) adoptivo(a)"@es , "has adoptive sibling"@en , "hat Adoptivgeschwister"@de ;
        rdfs:seeAlso     :hasAdoptiveSibling ;
        rdfs:subClassOf  :HasSibling .

:       a                owl:Ontology ;
        rdfs:comment     "∼∼∼ Modelling Guidelines ∼∼∼ \nVocabulary elements (properties and concepts) are conceived gender neutral.\nThe identifiers of properties are preferably hasProperty and invers isPropertyOf or hasInverseProperty. \nDomains and ranges of properties are mostly not fixed.\nInstance relations (object properties) are mostly specified bidirectionally.\nImplicit, deducable instance relations are explicitly formulated.\nProperties partly allow imperfect information (e.g. fragmentary dates, names instead of object URIs).\nCorrelations between instance relations, like inversity, transitivity, symmetry, hierarchie, are marked.\nMeta statements are exhibited by modelling person relations as n-ary concepts as well as as properties, corresponding n-ary concepts and properties are correlated."^^xsd:string , "∼∼∼ Introduction ∼∼∼ \nThe ontology of agent relationships, AgRelOn, defines relations of persons to other persons and to organisations, since agents (persons, organisations) and their interconnections are important in the cultural heritage domain. AgRelOn is developed to foster uniform cataloging as well as semantic searchability of and via relations between agents. Therefore, a general set of nearly 70 relationhip types is provided. AgRelOn discerns private acquaintanceship, group affiliation, correspondence, occupational contact,  kinship, spiritual contact, and vital/lethal contact. For these kinds of relations more specific sub-relations are formulated.\nMeta statements are supported to obtain transparency of reliability and provenance as well as validity period of facts.\nThe modelled relations are determined on the one hand by exemplary knowledge base searches, on the other hand by available data sources. Hence, the model consciously is incomplete and pertinent to a cultural area and period."^^xsd:string ;
        rdfs:label       "AgRelOn, an Agent Relationship Ontology"^^xsd:string ;
        dc:publisher     "DNB"^^xsd:string ;
        dcterms:license  <http://creativecommons.org/publicdomain/zero/1.0/> ;
        owl:versionInfo  "V0.9 2011/06/30; URIs are yet instable"^^xsd:string .

:HasMultipleBirthSibling
        a                owl:Class ;
        rdfs:comment     "This is the n-ary concept for the property hasMultipleBirthSibling"^^xsd:string ;
        rdfs:label       "ha fratello o sorella plurigemellare"@it , "tiene hermano(a) gemelo(a)"@es , "has multiple birth sibling"@en , "hat Mehrlingsgeschwister"@de ;
        rdfs:seeAlso     :hasMultipleBirthSibling ;
        rdfs:subClassOf  :HasSibling .

:hasPatron  a                  owl:ObjectProperty ;
        rdfs:comment           "A person or corporation (subject; e.g. an artist or group of artists) who is sponsored/favoured by a person or corporation (object)."^^xsd:string ;
        rdfs:label             "ha mecenate"@it , "tiene mecenas"@es , "has patron"@en , "hat Mäzen"@de ;
        rdfs:subPropertyOf     :hasProfessionalContact ;
        :correspondsToInverse  :IsHasPatron ;
        owl:inverseOf          :isPatronOf .

:HasInfluenceDoneeDonor
        a                owl:Class ;
        rdfs:comment     "This is the n-ary concept for the properties hasInfluenceDonee / hasInfluenceDonor"^^xsd:string ;
        rdfs:label       "ha influenza su / è influenzato(a) da"@it , "tiene influencia sobre / es influenciado(a) por"@es , "has influence on / is influenced by"@en , "hat Einfluss auf / ist beeinflusst durch"@de ;
        rdfs:seeAlso     :hasInfluenceDonor , :hasInfluenceDonee ;
        rdfs:subClassOf  :HasProfessionalContact .

dcterms:license  a  owl:AnnotationProperty .

:hasAcquaintance  a         owl:SymmetricProperty ;
        rdfs:comment        "A person (subject) privately knows a person (object)."^^xsd:string ;
        rdfs:label          "ha conoscente"@it , "tiene conocido(a)"@es , "has acquaintance"@en , "hat Bekannte(n)"@de ;
        rdfs:subPropertyOf  :relatedAgent ;
        :correspondsTo      :HasAcquaintance ;
        :hasGndCode         "beza" .

:HasAssociate  a         owl:Class ;
        rdfs:comment     "This is the n-ary concept for the property hasAssociate"^^xsd:string ;
        rdfs:label       "ha gruppo di appartenenza"@it , "tiene grupo de afiliación"@es , "has group affiliation"@en , "hat Gruppenzugehörigkeit"@de ;
        rdfs:seeAlso     :hasAssociate ;
        rdfs:subClassOf  :RelatedAgent .

:hasVitalLethalContact
        a                   owl:SymmetricProperty ;
        rdfs:comment        "A person or corporate body (subject) has som kind of vital or lethal relation with a person or corporate body (object). The relationship may e.g. include healing, mutilating, life saving, killing."^^xsd:string ;
        rdfs:label          "ha contatto vitale o letale"@it , "tiene contacto vital o letal"@es , "has vital or lethal contact"@en , "hat vitalen oder letalen Kontakt"@de ;
        rdfs:subPropertyOf  :relatedAgent ;
        :correspondsTo      :HasVitalLethalContact .

:hasParent  a                  owl:ObjectProperty ;
        rdfs:comment           "A person has as some kind of parent a person (object)."^^xsd:string ;
        rdfs:label             "ha genitore"@it , "tiene padre o madre"@es , "has parent"@en , "hat Elter"@de ;
        rdfs:subPropertyOf     :hasAncestor ;
        :correspondsToInverse  :HasChildParent ;
        owl:inverseOf          :hasChild .

:hasEmployer  a                owl:ObjectProperty ;
        rdfs:comment           "A person (subject) works for a person or corporation (object)."^^xsd:string ;
        rdfs:label             "ha datore di lavoro"@it , "tiene empleador(a)"@es , "has employer"@en , "hat Arbeitgeber"@de ;
        rdfs:subPropertyOf     :hasProfessionalContact ;
        :correspondsToInverse  :HasEmployeeEmployer ;
        owl:inverseOf          :hasEmployee .

dc:language  a  owl:AnnotationProperty .

:hasGndCode  a        owl:DatatypeProperty ;
        rdfs:comment  "A relationship type (subject) has a correlating GND code (literal). In the context of the project GND (Gemeinsame Normdatei), codes for agent relations correlating to AgRelOn are successively determined in cooperation with the Library of Congress or rather NDMSO (Network Development and MARC Standards Office) to supplement MARC. The codes will be indicated in AgRelOn when they are available."^^xsd:string ;
        rdfs:label    "ha chiave di accesso GND"@it , "tiene código de GND"@es , "has GND code"@en , "hat GND Code"@de ;
        rdfs:range    xsd:string .

:hasFosterSibling  a        owl:SymmetricProperty ;
        rdfs:comment        "A person (subject) has as sibling a person (object), where at least one of the two siblings is foster child of a joint parent."^^xsd:string ;
        rdfs:label          "ha fratello o sorella di latte"@it , "tiene hermano(a) de crianza"@es , "has foster sibling"@en , "has Pflegegeschwister"@de ;
        rdfs:subPropertyOf  :hasSibling ;
        :correspondsTo      :HasFosterSibling .

:HasHalfSibling  a       owl:Class ;
        rdfs:comment     "This is the n-ary concept for the property hasHalfSibling"^^xsd:string ;
        rdfs:label       "ha fratellastro a sorellastra"@it , "tiene medio hermano(a)"@es , "has half sibling"@en , "hat Halbgeschwister"@de ;
        rdfs:seeAlso     :hasHalfSibling ;
        rdfs:subClassOf  :HasSibling .

:HasStudentTeacher  a    owl:Class ;
        rdfs:comment     "This is the n-ary concept for the properties hasStudent / hasTeacher"^^xsd:string ;
        rdfs:label       "ha scolaro(a) / insegnante"@it , "tiene estudiante / maestro(a)"@es , "has Student / teacher"@en , "hat Schüler / Lehrer"@de ;
        rdfs:seeAlso     :hasTeacher , :hasStudent ;
        rdfs:subClassOf  :HasProfessionalContact .

:hasProfessionalContact
        a                   owl:SymmetricProperty ;
        rdfs:comment        "A person or corporation (subject) has some business/profession/occupation related relation with a person or corporation (object)."^^xsd:string ;
        rdfs:label          "ha contatto professionale"@it , "tiene relación profesional"@es , "has professional contact"@en , "hat Berufskontakt"@de ;
        rdfs:subPropertyOf  :relatedAgent ;
        :correspondsTo      :HasProfessionalContact ;
        :hasGndCode         "bezb" .

:hasBiologicalParent  a        owl:ObjectProperty ;
        rdfs:comment           "A person (subject) was begotten/conceived by a person (object)."^^xsd:string ;
        rdfs:label             "ha genitore biologico"@it , "tiene padre o madre biológico(a)"@es , "has biological parent"@en , "hat biologischen Elter"@de ;
        rdfs:subPropertyOf     :hasParent ;
        :correspondsToInverse  :HasBiologicalChildParent .

:hasGrandChild  a           owl:ObjectProperty ;
        rdfs:comment        "A person's (subject) child has a child (object)."^^xsd:string ;
        rdfs:label          "ha nipote (di nonni)"@it , "tiene nieto(a)"@es , "has grandchild"@en , "hat Enkel"@de ;
        rdfs:subPropertyOf  :hasOffspring ;
        :correspondsTo      :HasGrandChildParent .

:hasParentInlaw  a             owl:ObjectProperty ;
        rdfs:comment           "A person's (subject) spouse has a parent (object)."^^xsd:string ;
        rdfs:label             "ha suocero(a)"@it , "tiene suegro(a)"@es , "has parent-in-law"@en , "hat Schwiegerelter"@de ;
        rdfs:subPropertyOf     :hasInlaw ;
        :correspondsToInverse  :HasChildParentInlaw .

:hasChildInlaw  a           owl:ObjectProperty ;
        rdfs:comment        "A person's (subject) child is married with a person (object)."^^xsd:string ;
        rdfs:label          "ha genero o nuora"@it , "tiene yerno o nuera"@es , "has child-in-law"@en , "hat Schwiegerkind"@de ;
        rdfs:subPropertyOf  :hasInlaw ;
        :correspondsTo      :HasChildParentInlaw ;
        owl:inverseOf       :hasParentInlaw .

:hasCorrespondent  a        owl:SymmetricProperty ;
        rdfs:comment        "A person or corporation (subject) exchanges letters with a person or corporation (object)."^^xsd:string ;
        rdfs:label          "ha corrispondente"@it , "tiene correspondente"@es , "has correspondent"@en , "hat Korrespondent"@de ;
        rdfs:subPropertyOf  :relatedAgent ;
        :correspondsTo      :HasCorrespondent .

:hasAdoptiveSibling  a      owl:SymmetricProperty ;
        rdfs:comment        "A person (subject) has as sibling a person (object), where at least one of the two siblings is adoptive child of a joint parent."^^xsd:string ;
        rdfs:label          "ha fratello adottato o sorella adottata"@it , "tiene hermano(a) adoptivo(a)"@es , "has adoptive sibling"@en , "hat Adoptivgeschwister"@de ;
        rdfs:subPropertyOf  :hasSibling ;
        :correspondsTo      :HasAdoptiveSibling .

:HasChildParentInlaw  a  owl:Class ;
        rdfs:comment     "This is the n-ary concept for the properties hasChildInlaw and hasParentInlaw"^^xsd:string ;
        rdfs:label       "ha genero o nuora / suocero(a)"@it , "tiene yerno o nuera / suegro(a)"@es , "has child/parent-in-law"@en , "hat Schwiegerkind / -elter"@de ;
        rdfs:seeAlso     :hasParentInlaw , :hasChildInlaw ;
        rdfs:subClassOf  :HasInlaw .

:isObject  a          owl:ObjectProperty ;
        rdfs:comment  "Something (subject) takes the object role at an n-ary concept's instance (object) of the asymmetric relationship meant by the n-ary concept. \nFor inverse relationsships, the subject and object role follow the naming of the n-ary concept when reading quasi just the first part of the n-ary concept name."^^xsd:string ;
        rdfs:label    "è oggetto"@it , "es objeto"@es , "is object"@en , "ist Objekt"@de .

:HasOffspringAncestor
        a                owl:Class ;
        rdfs:comment     "This is the n-ary concept for the properties hasAncestor / hasOffspring"^^xsd:string ;
        rdfs:label       "ha antenato / discendente"@it , "tiene ancestro / heredero(a)"@es , "has ancestor / offspring"@en , "hat Vorfahr / Nachkomme"@de ;
        rdfs:seeAlso     :hasOffspring , :hasAncestor ;
        rdfs:subClassOf  :HasRelative .

:hasFriend  a               owl:SymmetricProperty ;
        rdfs:comment        "A person (subject) is friends with a person (object)."^^xsd:string ;
        rdfs:label          "ha amico(a)"@it , "tiene amigo(a)"@es , "has friend"@en , "hat Freund"@de ;
        rdfs:subPropertyOf  :hasAcquaintance ;
        :correspondsTo      :HasFriend .

:hasFounder  a              owl:ObjectProperty ;
        rdfs:comment        "A group (subject) has as a founder a person (object)."^^xsd:string ;
        rdfs:label          "ha fondatore o fondatrice"@it , "tiene fundador(a)"@es , "has founder"@en , "hat Gründer"@de ;
        rdfs:subPropertyOf  :hasAssociate ;
        :correspondsTo      :HasIsFounder .

:HasStepChildParent  a   owl:Class ;
        rdfs:comment     "This is the n-ary concept for the properties hasStepChild / hasStepParent"^^xsd:string ;
        rdfs:label       "ha figliastro(a) / padrigno o madrigna"@it , "tiene hijo(a) / padre o madre adoptivo(a)"@es , "has stepchild / stepparent"@en , "hat Stiefkind / Stiefelter"@de ;
        rdfs:seeAlso     :hasStepParent , :hasStepChild ;
        rdfs:subClassOf  :HasChildParent .

:HasAcquaintance  a      owl:Class ;
        rdfs:comment     "This is the n-ary concept for the property hasAcquaintance"^^xsd:string ;
        rdfs:label       "ha conoscente"@it , "tiene conocido(a)"@es , "has acquaintance"@en , "hat Bekannte(n)"@de ;
        rdfs:seeAlso     :hasAcquaintance ;
        rdfs:subClassOf  :RelatedAgent .

:metadataProvenance  a  owl:DatatypeProperty ;
        rdfs:comment  "A statement or fact (subject) originates from a source."^^xsd:string ;
        rdfs:label    "ha provenienza"@it , "tiene origen"@es , "has provenance"@en , "hat Herkunft"@de ;
        rdfs:range    xsd:string .

:hasMurderer  a                owl:ObjectProperty ;
        rdfs:comment           "A person (subject) is murdered by a person or corporate body (object)."^^xsd:string ;
        rdfs:label             "ha assassino(a)"@it , "tiene asesino(a)"@es , "has murderer"@en , "hat Mörder"@de ;
        rdfs:subPropertyOf     :hasVitalLethalContact ;
        :correspondsToInverse  :HasMurdereeMurderer ;
        owl:inverseOf          :hasMurderee .

:HasSpouse  a            owl:Class ;
        rdfs:comment     "This is the n-ary concept for the property hasSpouse"^^xsd:string ;
        rdfs:label       "ha coniuge"@it , "tiene esposo(a)"@es , "has spouse"@en , "hat Ehepartner"@de ;
        rdfs:seeAlso     :hasSpouse ;
        rdfs:subClassOf  :HasInlaw .

:isFounderOf  a                owl:ObjectProperty ;
        rdfs:comment           "A person (subject) ist founder of a group (object)."^^xsd:string ;
        rdfs:label             "è fondatore o fondatrice di"@it , "es fundador(a) de"@es , "is founder of"@en , "ist Gründer von"@de ;
        rdfs:subPropertyOf     :hasAssociate ;
        :correspondsToInverse  :HasIsFounder .

:hasInfluenceDonee  a       owl:ObjectProperty ;
        rdfs:comment        "A person or corporation (subject) who influences a person or corporation (object)."^^xsd:string ;
        rdfs:label          "ha influenza su"@it , "tiene influencia sobre"@es , "has influence on"@en , "hat Einfluss auf"@de ;
        rdfs:subPropertyOf  :hasProfessionalContact ;
        :correspondsTo      :HasInfluenceDoneeDonor .

:hasCooperator  a           owl:SymmetricProperty ;
        rdfs:comment        "A person (subject) works together with a person or corporation (object)."^^xsd:string ;
        rdfs:label          "ha collaboratore o collaboratrice"@it , "tiene colaborador(a)"@es , "has collaborator"@en , "hat Kollaborator"@de ;
        rdfs:subPropertyOf  :hasProfessionalContact ;
        :correspondsTo      :HasCooperator .

:isSubject  a          owl:ObjectProperty ;
        rdfs:comment   "Something (subject) takes the subject role at an n-ary concept's instance (object) of the asymmetric relationship meant by the n-ary concept. \nFor inverse relationsships, the subject and object role follow the naming of the n-ary concept when reading quasi just the first part of the n-ary concept name."^^xsd:string ;
        rdfs:label     "è soggetto di"@it , "es sujeto"@es , "is subject"@en , "ist Subjekt"@de ;
        owl:inverseOf  :hasSubject .

:HasIsChief  a           owl:Class ;
        rdfs:comment     "This is the n-ary concept for the properties hasChief / isChiefOf"^^xsd:string ;
        rdfs:label       "ha capo / è capo di"@it , "tiene jefe / es jefe de"@es , "has chief / is chief of"@en , "hat Chef / ist Chef von"@de ;
        rdfs:seeAlso     :isChiefOf , :hasChief ;
        rdfs:subClassOf  :HasAssociate .

:metadataPeriod  a    owl:ObjectProperty ;
        rdfs:comment  "An n−ary instance (subject) is valid/true in a period (object). The period should be manifested in a blank node, with data properties hasBeginDate or/and hasEndDate set."^^xsd:string ;
        rdfs:label    "ha tempo di validità"@it , "tiene periodo de validez"@es , "has validity period"@en , "hat Gültigkeitszeitraum"@de .

:hasChannel  a              owl:ObjectProperty ;
        rdfs:comment        "A person or spiritual entity (subject), e.g. a dead person, spirit, angel etc. has as a channel or medium a person or spiritual entity (object). I.e. the subject transmits messages to the object."^^xsd:string ;
        rdfs:label          "ha sensitivo(a)"@it , "tiene médium"@es , "has channel"@en , "hat Medium"@de ;
        rdfs:subPropertyOf  :hasSpiritualContact ;
        :correspondsTo      :HasIsChannel .

:HasRelative  a          owl:Class ;
        rdfs:comment     "This is the n-ary concept for the property hasRelative"^^xsd:string ;
        rdfs:label       "ha parente"@it , "tiene pariente"@es , "has relative"@en , "hat Verwandte(n)"@de ;
        rdfs:seeAlso     :hasRelative ;
        rdfs:subClassOf  :RelatedAgent .

rdfs:label  a   owl:AnnotationProperty .

:hasStepParent  a              owl:ObjectProperty ;
        rdfs:comment           "A person's (subject) biological parent is married with or cohabits with a person (object)."^^xsd:string ;
        rdfs:label             "ha padrigno o madrigna"@it , "tiene padre o madre adoptivo(a)"@es , "has stepparent"@en , "hat Stiefelter"@de ;
        rdfs:subPropertyOf     :hasParent ;
        :correspondsToInverse  :HasStepChildParent ;
        owl:inverseOf          :hasStepChild .

:HasCohabitee  a         owl:Class ;
        rdfs:comment     "This is the n-ary concept for the property hasCohabitee"^^xsd:string ;
        rdfs:label       "ha compagno(a) di vita"@it , "tiene cohabitante"@es , "has cohabitee"@en , "hat Lebensgefährte"@de ;
        rdfs:seeAlso     :hasCohabitee ;
        rdfs:subClassOf  :HasAcquaintance .

:hasSibling  a              owl:SymmetricProperty ;
        rdfs:comment        "A person has as some kind of sibling a person (object)."^^xsd:string ;
        rdfs:label          "ha fratello o sorella"@it , "tiene hermano(a)"@es , "has sibling"@en , "hat Geschwister"@de ;
        rdfs:subPropertyOf  :hasRelative ;
        :correspondsTo      :HasSibling .

:hasEmployee  a             owl:ObjectProperty ;
        rdfs:comment        "A person or corporation (subject) for whom/which a person (object) works."^^xsd:string ;
        rdfs:label          "ha impiegato(a)"@it , "tiene empleado(a)"@es , "has employee"@en , "hat Arbeitnehmer"@de ;
        rdfs:subPropertyOf  :hasProfessionalContact ;
        :correspondsTo      :HasEmployeeEmployer .

:hasStepSibling  a          owl:SymmetricProperty ;
        rdfs:comment        "A person (subject) has as sibling a person (object), where at least one of the two siblings is step child of a joint parent."^^xsd:string ;
        rdfs:label          "ha fratellastro o sorellastra"@it , "tiene hermano(a) adoptivo(a)"@es , "has stepsibling"@en , "hat Stiefgeschwister"@de ;
        rdfs:subPropertyOf  :hasSibling ;
        :correspondsTo      :HasStepSibling .

:HasIsMember  a          owl:Class ;
        rdfs:comment     "This is the n-ary concept for the properties hasMember / isMemberOf"^^xsd:string ;
        rdfs:label       "ha membro / è membro di"@it , "tiene membrio / es miembro de"@es , "has member / is member of"@en , "hat Mitglied / ist Mitglied von"@de ;
        rdfs:seeAlso     :isMemberOf , :hasMember ;
        rdfs:subClassOf  :HasAssociate .

:hasSubject  a        owl:ObjectProperty ;
        rdfs:comment  "At an n-ary concept's instance (subject), something (object) takes the subject role of the asymmetric relationship meant by the n-ary concept. \nFor inverse relationsships, the subject and object role follow the naming of the n-ary concept when reading quasi just the first part of the n-ary concept name."^^xsd:string ;
        rdfs:domain   :NAries ;
        rdfs:label    "ha soggetto"@it , "tiene sujeto"@es , "has subject"@en , "hat Subjekt"@de .

:hasAdoptiveParent  a          owl:ObjectProperty ;
        rdfs:comment           "A person (subject) was adopted by a person (object)."^^xsd:string ;
        rdfs:label             "ha genitore adottivo"@it , "tiene padre o madre adoptivo(a)"@es , "has adoptive parent"@en , "hat Adoptivelter"@de ;
        rdfs:subPropertyOf     :hasParent ;
        :correspondsToInverse  :HasAdoptiveChildParent ;
        owl:inverseOf          :hasAdoptiveChild .

:HasLover  a             owl:Class ;
        rdfs:comment     "This is the n-ary concept for the property hasLover"^^xsd:string ;
        rdfs:label       "ha amante"@it , "tiene amante"@es , "has lover"@en , "hat Geliebte(n)"@de ;
        rdfs:seeAlso     :hasLover ;
        rdfs:subClassOf  :HasAcquaintance .

:HasNieceNephewAuntUncle
        a                owl:Class ;
        rdfs:comment     "This is the n-ary concept for the properties hasAuntUncle / hasNieceNephew"^^xsd:string ;
        rdfs:label       "ha zia o zio / nipote (di zii)"@it , "tiene tío o tía / sobrino(a)"@es , "has aunt or uncle / niece or nephew"@en , "hat Tante oder Onkel / Nichte oder Neffe"@de ;
        rdfs:seeAlso     :hasNieceNephew , :hasAuntUncle ;
        rdfs:subClassOf  :HasRelative .

:IsHasPatron  a          owl:Class ;
        rdfs:comment     "This is the n-ary concept for the properties hasPatron / isPatronOf"^^xsd:string ;
        rdfs:label       "ha mecenateè mecenate di"@it , "tiene mecenas / es mecenas de"@es , "has patron / is patron of"@en , "hat Mäzen / ist Mäzen von"@de ;
        rdfs:seeAlso     :isPatronOf , :hasPatron ;
        rdfs:subClassOf  :HasProfessionalContact .

:hasLover  a                owl:SymmetricProperty ;
        rdfs:comment        "A person (subject) has a liaison with a person (object), without being married."^^xsd:string ;
        rdfs:label          "ha amante"@it , "tiene amante"@es , "has lover"@en , "hat Geliebte(n)"@de ;
        rdfs:subPropertyOf  :hasAcquaintance ;
        :correspondsTo      :HasLover .

:HasCooperator  a        owl:Class ;
        rdfs:comment     "This is the n-ary concept for the property hasCooperator"^^xsd:string ;
        rdfs:label       "ha collaboratore o collaboratrice"@it , "tiene colaborador(a)"@es , "has collaborator"@en , "hat Kollaborator"@de ;
        rdfs:seeAlso     :hasCooperator ;
        rdfs:subClassOf  :HasProfessionalContact .

:isChiefOf  a                  owl:ObjectProperty ;
        rdfs:comment           "A person (subject) ist chief of a group (object)."^^xsd:string ;
        rdfs:label             "è capo di"@it , "es jefe de"@es , "is chief of"@en , "ist Chef von"@de ;
        rdfs:subPropertyOf     :hasAssociate ;
        :correspondsToInverse  :HasIsChief .

:hasSiblingInlaw  a         owl:SymmetricProperty ;
        rdfs:comment        "A person's (subject) spouse has a sibling (object)."^^xsd:string ;
        rdfs:label          "ha cognato(a)"@it , "tiene cuñado(a)"@es , "has sibling-in-law"@en , "hat Schwager oder Schwägerin"@de ;
        rdfs:subPropertyOf  :hasInlaw ;
        :correspondsTo      :HasSiblingInlaw .

:hasInfluenceDonor  a          owl:ObjectProperty ;
        rdfs:comment           "A person or corporation (subject) who is influenced by a person or corporation (object)."^^xsd:string ;
        rdfs:label             "è influenzato(a) da"@it , "es influenciado(a) por"@es , "is influenced by"@en , "ist beeinflusst durch"@de ;
        rdfs:subPropertyOf     :hasProfessionalContact ;
        :correspondsToInverse  :HasInfluenceDoneeDonor ;
        owl:inverseOf          :hasInfluenceDonee .

:hasAssociate  a            owl:ObjectProperty ;
        rdfs:comment        "A person (subject) is associated with a group (object), or a group (subject) is associated with a person (object)."^^xsd:string ;
        rdfs:label          "ha gruppo di appartenenza"@it , "tiene grupo de afiliación"@es , "has group affiliation"@en , "hat Gruppenzugehörigkeit"@de ;
        rdfs:subPropertyOf  :relatedAgent ;
        :correspondsTo      :HasAssociate ;
        :hasGndCode         "affi" .

:HasVitalLethalContact
        a                owl:Class ;
        rdfs:comment     "This is the n-ary concept for the property hasVitalLethalContact"^^xsd:string ;
        rdfs:label       "ha contatto vitale o letale"@it , "tiene contacto vital o letal"@es , "has vital or lethal contact"@en , "hat vitalen oder letalen Kontakt"@de ;
        rdfs:seeAlso     :hasVitalLethalContact ;
        rdfs:subClassOf  :RelatedAgent .

:IsHasPhysician  a       owl:Class ;
        rdfs:comment     "This is the n-ary concept for the properties hasPhysician / isPhysicianOf"^^xsd:string ;
        rdfs:label       "ha medico / è medico di"@it , "tiene médico / es médico de"@es , "has physician / is physician of"@en , "hat Arzt / ist Arzt von"@de ;
        rdfs:seeAlso     :isPhysicianOf , :hasPhysician ;
        rdfs:subClassOf  :HasVitalLethalContact .

:correspondsToInverse
        a             owl:SymmetricProperty ;
        rdfs:comment  "A normal property's (type rdf:Property) fro-direction matches an n-ary concept (type rdfs:Class). \n2 mutually inverse normal properties match only 1 n-ary concept, because the meta statements must be identical for both 'to-direction' and 'fro-direction' of the relationship. \nThe normal property's to-direction is related to the n-ary concept via correspondsTo."^^xsd:string ;
        rdfs:label    "corrisponde inversamente a"@it , "corresponde inversamente con"@es , "corresponds to inverse"@en , "korrespondiert invers mit"@de .

:HasFianceeFiance  a     owl:Class ;
        rdfs:comment     "This is the n-ary concept for the property hasFianceeFiance"^^xsd:string ;
        rdfs:label       "ha fidanzato(a)"@it , "tiene prometido(a)"@es , "has fiancee  or fiance"@en , "hat Verlobte(n)"@de ;
        rdfs:seeAlso     :hasFianceeFiance ;
        rdfs:subClassOf  :HasInlaw .

:metadataConfidence  a  owl:DatatypeProperty ;
        rdfs:comment  "A statement or fact (subject) has a value indicating the statement's confidence or trustworthiness."^^xsd:string ;
        rdfs:label    "ha valore di fiducia"@it , "valor de confianza"@es , "has confidence value"@en , "hat Konfidenzwert"@de ;
        rdfs:range    xsd:double .

:isMemberOf  a                 owl:ObjectProperty ;
        rdfs:comment           "A person (subject) ist member of a group (object)."^^xsd:string ;
        rdfs:label             "è membro di"@it , "es miembro de"@es , "is member of"@en , "ist Mitglied von"@de ;
        rdfs:subPropertyOf     :hasAssociate ;
        :correspondsToInverse  :HasIsMember .

:hasAdoptiveChild  a        owl:ObjectProperty ;
        rdfs:comment        "A person (subject) adopted a person (object)."^^xsd:string ;
        rdfs:label          "ha figlio(a) adottivo(a)"@it , "tiene hijo(a) adoptivo(a)"@es , "has adoptive child"@en , "hat Adoptivkind"@de ;
        rdfs:subPropertyOf  :hasChild ;
        :correspondsTo      :HasAdoptiveChildParent .

:HasCousin  a            owl:Class ;
        rdfs:comment     "This is the n-ary concept for the property hasCousin"^^xsd:string ;
        rdfs:label       "ha cugino(a)"@it , "tiene primo o prima"@es , "has cousin"@en , "hat Cousin"@de ;
        rdfs:seeAlso     :hasCousin ;
        rdfs:subClassOf  :HasRelative .

:isPatronOf  a              owl:ObjectProperty ;
        rdfs:comment        "A person or corporation (subject) sponsors/favours a person or corporation (object; e.g. an artist or group of artists)."^^xsd:string ;
        rdfs:label          "è mecenate di"@it , "es mecenas de"@es , "is patron of"@en , "ist Mäzen von"@de ;
        rdfs:subPropertyOf  :hasProfessionalContact ;
        :correspondsTo      :IsHasPatron .

:hasTeacher  a                 owl:ObjectProperty ;
        rdfs:comment           "A person (subject) who is trained by a person (object)."^^xsd:string ;
        rdfs:label             "ha insegnante"@it , "tiene maestro(a)"@es , "has teacher"@en , "hat Lehrer"@de ;
        rdfs:subPropertyOf     :hasProfessionalContact ;
        :correspondsToInverse  :HasStudentTeacher .

:hasBeginDate  a      owl:DatatypeProperty ;
        rdfs:comment  "A metadata period or phase (subject) has a temporal start (date). The phase might e.g. concern a relationship between agents."^^xsd:string ;
        rdfs:label    "ha data dinizio"@it , "tiene fecha inicial"@es , "has begin date"@en , "hat Anfangsdatum"@de .

:isPhysicianOf  a           owl:ObjectProperty ;
        rdfs:comment        "A person or corporate body (subject) is physician of a person or corporate body (object)."^^xsd:string ;
        rdfs:label          "è medico di"@it , "es médico de"@es , "is physician of"@en , "ist Arzt von"@de ;
        rdfs:subPropertyOf  :hasVitalLethalContact ;
        :correspondsTo      :IsHasPhysician ;
        owl:inverseOf       :hasPhysician .

:RelatedAgent  a         owl:Class ;
        rdfs:comment     "This is the n-ary concept for the property relatedAgent"^^xsd:string ;
        rdfs:label       "agente connesso"@it , "agente relacionado"@es , "related Agent"@en , "verknüpfter Agens"@de ;
        rdfs:seeAlso     :relatedAgent ;
        rdfs:subClassOf  :NAries .

:hasMurderee  a             owl:ObjectProperty ;
        rdfs:comment        "A person or corporate body (subject) murders a person (object)."^^xsd:string ;
        rdfs:label          "ha vittima domicidio"@it , "tiene víctima"@es , "has murder victim"@en , "hat Mordopfer"@de ;
        rdfs:subPropertyOf  :hasVitalLethalContact ;
        :correspondsTo      :HasMurdereeMurderer .

:HasGrandChildParent  a  owl:Class ;
        rdfs:comment     "This is the n-ary concept for the properties hasGrandChild and hasGrandParent"^^xsd:string ;
        rdfs:label       "ha nipote (di nonni) / nonno(a)"@it , "tiene nieto(a) / abuelo(a)"@es , "has grandchild / grandparent"@en , "hat Enkel / Großelter"@de ;
        rdfs:seeAlso     :hasGrandParent , :hasGrandChild ;
        rdfs:subClassOf  :HasOffspringAncestor .

:hasSpouse  a               owl:SymmetricProperty ;
        rdfs:comment        "A person (subject) is married with a person (object)."^^xsd:string ;
        rdfs:label          "ha coniuge"@it , "tiene esposo(a)"@es , "has spouse"@en , "hat Ehepartner"@de ;
        rdfs:subPropertyOf  :hasInlaw ;
        :correspondsTo      :HasSpouse .

:HasBiologicalSibling
        a                owl:Class ;
        rdfs:comment     "This is the n-ary concept for the property hasBiologicalSibling"^^xsd:string ;
        rdfs:label       "ha fratello biologico o sorella biologica"@it , "tiene hermano(a) biológico(a)"@es , "has biological sibling"@en , "hat biologisches Geschwister"@de ;
        rdfs:seeAlso     :hasBiologicalSibling ;
        rdfs:subClassOf  :HasSibling .

:hasChief  a                owl:ObjectProperty ;
        rdfs:comment        "A group (subject) has as a chief a person (object)."^^xsd:string ;
        rdfs:label          "ha capo"@it , "tiene jefe"@es , "has chief"@en , "hat Chef"@de ;
        rdfs:subPropertyOf  :hasAssociate ;
        :correspondsTo      :HasIsChief .

:HasBiologicalChildParent
        a                owl:Class ;
        rdfs:comment     "This is the n-ary concept for the properties hasBiologicalChild and hasBiologicalParent"^^xsd:string ;
        rdfs:label       "ha figlio(a) / genitore biologico(a)"@it , "tiene hijo(a) / padre / madre biológico(a)"@es , "has biological child / parent"@en , "hat biologisches Kind / biologischen Elter"@de ;
        rdfs:seeAlso     :hasBiologicalParent , :hasBiologicalChild ;
        rdfs:subClassOf  :HasChildParent .

:hasEndDate  a        owl:DatatypeProperty ;
        rdfs:comment  "A metadata period or phase (subject) has a temporal end (date). The phase might e.g. concern a relationship between agents."^^xsd:string ;
        rdfs:label    "ha data finale"@it , "tiene fecha final"@es , "has end date"@en , "hat Enddatum"@de .

:isMuseOf  a                   owl:ObjectProperty ;
        rdfs:comment           "A person (subject) inspires a person or corporation (object)."^^xsd:string ;
        rdfs:label             "è musa di"@it , "es musa de"@es , "is muse of"@en , "ist Muse von"@de ;
        rdfs:subPropertyOf     :hasProfessionalContact ;
        :correspondsToInverse  :HasIsMuse .

:hasGodParent  a               owl:ObjectProperty ;
        rdfs:comment           "A person (subject) obtains as godparent a person (object) at the godchild's christening."^^xsd:string ;
        rdfs:label             "ha padrino o padrina"@it , "tiene padrino o madrina"@es , "has godparent"@en , "hat Pate"@de ;
        rdfs:subPropertyOf     :hasAuntUncle ;
        :correspondsToInverse  :HasGodChildParent .

:hasAuntUncle  a               owl:ObjectProperty ;
        rdfs:comment           "A person (subject) has an aunt or uncle (object)."^^xsd:string ;
        rdfs:label             "ha zia o zio"@it , "tiene tío o tía"@es , "has aunt or uncle"@en , "hat Tante oder Onkel"@de ;
        rdfs:subPropertyOf     :hasRelative ;
        :correspondsToInverse  :HasNieceNephewAuntUncle .

:NAries  a            owl:Class ;
        rdfs:comment  "This is the top class for all n-ary classes"^^xsd:string ;
        rdfs:label    "n-ary classes"@en , "n-ary Klassen"@de .

:hasStepChild  a            owl:ObjectProperty ;
        rdfs:comment        "A person's (subject) spouse has a child (object)."^^xsd:string ;
        rdfs:label          "ha figliastro(a)"@it , "tiene hijo(a) adoptivo(a)"@es , "has stepchild"@en , "hat Stiefkind"@de ;
        rdfs:subPropertyOf  :hasChild ;
        :correspondsTo      :HasStepChildParent .

:HasSiblingInlaw  a      owl:Class ;
        rdfs:comment     "This is the n-ary concept for the property hasSiblingInlaw"^^xsd:string ;
        rdfs:label       "ha cognato(a)"@it , "tiene cuñado(a)"@es , "has sibling-in-law"@en , "hat Schwager oder Schwägerin"@de ;
        rdfs:seeAlso     :hasSiblingInlaw ;
        rdfs:subClassOf  :HasInlaw .

:HasChildParent  a       owl:Class ;
        rdfs:comment     "This is the n-ary concept for the properties hasChild and hasParent"^^xsd:string ;
        rdfs:label       "ha figlio(a) / genitore"@it , "tiene hijo(a) / padre o madre"@es , "has child / parent"@en , "hat Kind /Elter"@de ;
        rdfs:seeAlso     :hasParent , :hasChild ;
        rdfs:subClassOf  :HasOffspringAncestor .

:HasColleague  a         owl:Class ;
        rdfs:comment     "This is the n-ary concept for the property hasColleague"^^xsd:string ;
        rdfs:label       "ha collega"@it , "tiene colega"@es , "has colleague"@en , "hat Kollege"@de ;
        rdfs:seeAlso     :hasColleague ;
        rdfs:subClassOf  :HasProfessionalContact .

:HasMurdereeMurderer  a  owl:Class ;
        rdfs:comment     "This is the n-ary concept for the properties hasMurderee / hasMurderer"^^xsd:string ;
        rdfs:label       "ha vittima domicidio / assassino(a)"@it , "tiene víctima / asesino(a)"@es , "has murder victim / murderer"@en , "hat Mordopfer / Mörder"@de ;
        rdfs:seeAlso     :hasMurderer , :hasMurderee ;
        rdfs:subClassOf  :HasVitalLethalContact .

:isSubjectObject  a   owl:ObjectProperty ;
        rdfs:comment  "Something (subject) takes the subject or object role at an n-ary concept's instance (object) of the symmetric relationship meant by the n-ary concept. \nFor inverse relationsships, the subject and object role follow the naming of the n-ary concept when reading quasi just the first part of the n-ary concept name."^^xsd:string ;
        rdfs:label    "è soggetto o oggetto"@it , "es sujeto u objeto"@es , "is subject or object"@en , "ist Subjekt oder Objekt"@de .

:HasFriend  a            owl:Class ;
        rdfs:comment     "This is the n-ary concept for the property hasFriend"^^xsd:string ;
        rdfs:label       "ha amico(a)"@it , "tiene amigo(a)"@es , "has friend"@en , "hat Freund"@de ;
        rdfs:seeAlso     :hasFriend ;
        rdfs:subClassOf  :HasAcquaintance .

:HasFosterChildParent
        a                owl:Class ;
        rdfs:comment     "This is the n-ary concept for the properties hasFosterChild and hasFosterParent"^^xsd:string ;
        rdfs:label       "ha pupillo(a) / genitore"@it , "tiene hijo(a) / padre o madre de crianza"@es , "has foster child / parent"@en , "hat Pflegekind / -elter"@de ;
        rdfs:seeAlso     :hasFosterParent , :hasFosterChild ;
        rdfs:subClassOf  :HasChildParent .

:HasIsMuse  a            owl:Class ;
        rdfs:comment     "This is the n-ary concept for the properties hasMuse / isMuseOf"^^xsd:string ;
        rdfs:label       "ha musa / è musa di"@it , "tiene musa / es musa de"@es , "has muse / is muse of"@en , "hat Muse / ist Muse von"@de ;
        rdfs:seeAlso     :isMuseOf , :hasMuse ;
        rdfs:subClassOf  :HasProfessionalContact .

:isChannelOf  a                owl:ObjectProperty ;
        rdfs:comment           "A person or spiritual entity (subject) is a channel or medium of a person or spiritual entity (object), e.g. a dead person, spirit, angel etc. I.e. the subject receives messages from the object."^^xsd:string ;
        rdfs:label             "è sensitivo(a) di"@it , "es médium de"@es , "is channel of"@en , "ist Medium von"@de ;
        rdfs:subPropertyOf     :hasSpiritualContact ;
        :correspondsToInverse  :HasIsChannel ;
        owl:inverseOf          :hasChannel .

:hasGrandParent  a              owl:ObjectProperty ;
        rdfs:comment            "A person (subject) has as grandparent a person (object), where the two parent-relations might include adoptive, foster, illegitimate, step relations."^^xsd:string ;
        rdfs:label              "has grandparent"@en , "tiene abuelo(a)"@en , "ha nonno(a)"@it , "hat Großelter"@de ;
        rdfs:subPropertyOf      :hasAncestor ;
        :correspondsToInverse   :HasGrandChildParent ;
        owl:inverseOf           :hasGrandChild ;
        owl:propertyChainAxiom  ( :hasParent :hasParent ) .

:HasSibling  a           owl:Class ;
        rdfs:comment     "This is the n-ary concept for the property hasSibling"^^xsd:string ;
        rdfs:label       "ha fratello o sorella"@it , "tiene hermano(a)"@es , "has sibling"@en , "hat Geschwister"@de ;
        rdfs:seeAlso     :hasSibling ;
        rdfs:subClassOf  :HasRelative .

:hasFosterParent  a            owl:ObjectProperty ;
        rdfs:comment           "A person (subject) was fostered by a person (object), without being a biological child."^^xsd:string ;
        rdfs:label             "ha foster genitore"@it , "tiene padre o madre de crianza"@es , "has foster parent"@en , "hat Pflegeelter"@de ;
        rdfs:subPropertyOf     :hasParent ;
        :correspondsToInverse  :HasFosterChildParent ;
        owl:inverseOf          :hasFosterChild .

:HasProfessionalContact
        a                owl:Class ;
        rdfs:comment     "This is the n-ary concept for the property hasProfessionalContact"^^xsd:string ;
        rdfs:label       "ha contatto professionale"@it , "tiene relación profesional"@es , "has professional contact"@en , "hat Berufskontakt"@de ;
        rdfs:seeAlso     :hasProfessionalContact ;
        rdfs:subClassOf  :RelatedAgent .

:HasIsChannel  a         owl:Class ;
        rdfs:comment     "This is the n-ary concept for the properties hasChannel / isChannelOf"^^xsd:string ;
        rdfs:label       "ha sensitivo(a) / è sensitivo(a) di"@it , "tiene médium / es médium de"@es , "has channel / is channel of"@en , "hat Medium / ist Medium von"@de ;
        rdfs:seeAlso     :isChannelOf , :hasChannel ;
        rdfs:subClassOf  :HasSpiritualContact .

:hasMultipleBirthSibling
        a                   owl:SymmetricProperty ;
        rdfs:comment        "A person (subject) has as sibling a person (object), where both siblings where carried together in a joint pregnancy. This denotes not only twins, but also triplets etc.. Mostly, multiple birth siblings are biolological siblings, i.e. share both biological parents, but this doesn't have to be the case."^^xsd:string ;
        rdfs:label          "ha fratello o sorella plurigemellare"@it , "tiene hermano(a) gemelo(a)"@es , "has multiple birth sibling"@en , "hat Mehrlingsgeschwister"@de ;
        rdfs:subPropertyOf  :hasSibling ;
        :correspondsTo      :HasMultipleBirthSibling .

:hasHalfSibling  a          owl:ObjectProperty ;
        rdfs:comment        "A person (subject) has as sibling a person (object), where the two siblings share only one biological parent."^^xsd:string ;
        rdfs:label          "ha fratellastro a sorellastra"@it , "tiene medio hermano(a)"@es , "has half sibling"@en , "hat Halbgeschwister"@de ;
        rdfs:subPropertyOf  :hasSibling ;
        :correspondsTo      :HasHalfSibling .

:hasChild  a                owl:ObjectProperty ;
        rdfs:comment        "A person has as some kind of child a person (object)."^^xsd:string ;
        rdfs:label          "ha figlio(a)"@it , "tiene hijo(a)"@es , "has child"@en , "hat Kind"@de ;
        rdfs:subPropertyOf  :hasOffspring ;
        :correspondsTo      :HasChildParent .

:hasMuse  a                 owl:ObjectProperty ;
        rdfs:comment        "A person or corporation (subject; e.g. an artist or group of artists) who is inspired by a person (object)."^^xsd:string ;
        rdfs:label          "ha musa"@it , "tiene musa"@es , "has muse"@en , "hat Muse"@de ;
        rdfs:subPropertyOf  :hasProfessionalContact ;
        :correspondsTo      :HasIsMuse ;
        owl:inverseOf       :isMuseOf .

:HasFosterSibling  a     owl:Class ;
        rdfs:comment     "This is the n-ary concept for the property hasFosterSibling"^^xsd:string ;
        rdfs:label       "ha fratello o sorella di latte"@it , "tiene hermano(a) de crianza"@es , "has foster sibling"@en , "has Pflegegeschwister"@de ;
        rdfs:seeAlso     :hasFosterSibling ;
        rdfs:subClassOf  :HasSibling .

:correspondsTo  a     owl:SymmetricProperty ;
        rdfs:comment  "A normal property's (type rdf:Property) to-direction matches an n-ary concept (type rdfs:Class). \n2 mutually inverse normal properties match only 1 n-ary concept, because the meta statements must be identical for both 'to-direction' and 'fro-direction' of the relationship. \nThe normal property's fro-direction is related to the n-ary concept via correspondsToInverse."^^xsd:string ;
        rdfs:label    "corrisponde a"@it , "corresponde con"@es , "corresponds to"@en , "korrespondiert mit"@de .

:hasBiologicalSibling
        a                   owl:ObjectProperty ;
        rdfs:comment        "A person (subject) has as sibling a person (object), where the two siblings share both biological parents."^^xsd:string ;
        rdfs:label          "ha fratello biologico o sorella biologica"@it , "tiene hermano(a) biológico(a)"@es , "has biological sibling"@en , "hat biologisches Geschwister"@de ;
        rdfs:subPropertyOf  :hasSibling ;
        :correspondsTo      :HasBiologicalSibling .

:hasCohabitee  a            owl:SymmetricProperty ;
        rdfs:comment        "A person (subject) lives together with and/or is companion of a person (object), without being married."^^xsd:string ;
        rdfs:label          "ha compagno(a) di vita"@it , "tiene cohabitante"@es , "has cohabitee"@en , "hat Lebensgefährte"@de ;
        rdfs:subPropertyOf  :hasAcquaintance ;
        :correspondsTo      :HasCohabitee .

:HasStepSibling  a       owl:Class ;
        rdfs:comment     "This is the n-ary concept for the property hasStepSibling"^^xsd:string ;
        rdfs:label       "ha fratellastro o sorellastra"@it , "tiene hermano(a) adoptivo(a)"@es , "has stepsibling"@en , "hat Stiefgeschwister"@de ;
        rdfs:seeAlso     :hasStepSibling ;
        rdfs:subClassOf  :HasSibling .

:HasIllegitimateChildParent
        a                owl:Class ;
        rdfs:comment     "This is the n-ary concept for the properties hasIllegitimateChild / hasIllegitimateParent"^^xsd:string ;
        rdfs:label       "ha figlio(a) / genitore illegittimo(a)"@it , "tiene hijo(a) / padre o madre illegítimo(a)"@es , "has illegitimate child / parent"@en , "hat illegitimes Kind / illegitimen Elter"@de ;
        rdfs:seeAlso     :hasIllegitimateParent , :hasIllegitimateChild ;
        rdfs:subClassOf  :HasBiologicalChildParent .

:hasIllegitimateParent
        a                      owl:ObjectProperty ;
        rdfs:comment           "A person (subject) was begotten/conceived by a person (object), without the two biological parents being married at the child's day of birth."^^xsd:string ;
        rdfs:label             "ha genitore illegittimo"@it , "tiene padre o madre ilegítimo(a)"@es , "has illegitimate parent"@en , "hat illegitimen Elter"@de ;
        rdfs:subPropertyOf     :hasBiologicalParent ;
        :correspondsToInverse  :HasIllegitimateChildParent ;
        owl:inverseOf          :hasIllegitimateChild .

:hasCousin  a               owl:SymmetricProperty ;
        rdfs:comment        "A person (subject) has a cousin (object)."^^xsd:string ;
        rdfs:label          "ha cugino(a)"@it , "tiene primo o prima"@es , "has cousin"@en , "hat Cousin"@de ;
        rdfs:subPropertyOf  :hasRelative ;
        :correspondsTo      :HasCousin .

:hasNieceNephew  a          owl:ObjectProperty ;
        rdfs:comment        "A person (subject) has a niece or nephew (object)."^^xsd:string ;
        rdfs:label          "ha nipote (di zii)"@it , "tiene sobrino(a)"@es , "has niece or nephew"@en , "hat Nichte oder Neffe"@de ;
        rdfs:subPropertyOf  :hasRelative ;
        :correspondsTo      :HasNieceNephewAuntUncle ;
        owl:inverseOf       :hasAuntUncle .

:HasCorrespondent  a     owl:Class ;
        rdfs:comment     "This is the n-ary concept for the property hasCorrespondent"^^xsd:string ;
        rdfs:label       "ha corrispondente"@it , "tiene correspondente"@es , "has correspondent"@en , "hat Korrespondent"@de ;
        rdfs:seeAlso     :hasCorrespondent ;
        rdfs:subClassOf  :RelatedAgent .

:HasGodChildParent  a    owl:Class ;
        rdfs:comment     "This is the n-ary concept for the properties hasGodChild and hasGodParent"^^xsd:string ;
        rdfs:label       "ha figlioccio o figlioccia / padrino o padrina"@it , "tiene ahijado(a) / padrino o madrina"@es , "has godchild / godparent"@en , "hat Patenkind / Pate"@de ;
        rdfs:seeAlso     :hasGodParent , :hasGodChild ;
        rdfs:subClassOf  :HasNieceNephewAuntUncle .

:hasAncestor  a                owl:TransitiveProperty ;
        rdfs:comment           "A person (subject) has an ancestor (object), where the chain of parent-relations might include adoptive, foster, illegitimate, step relations."^^xsd:string ;
        rdfs:label             "ha antenato"@it , "tiene ancestro"@es , "has ancestor"@en , "hat Vorfahr"@de ;
        rdfs:subPropertyOf     :hasRelative ;
        :correspondsToInverse  :HasOffspringAncestor ;
        owl:inverseOf          :hasOffspring .

:hasBiologicalChild  a      owl:ObjectProperty ;
        rdfs:comment        "A person (subject) begot/conceived a person (object)."^^xsd:string ;
        rdfs:label          "ha figlio(a) biologico(a)"@it , "tiene hijo(a) biológico(a)"@es , "has biological child"@en , "hat biologisches Kind"@de ;
        rdfs:subPropertyOf  :hasChild ;
        :correspondsTo      :HasBiologicalChildParent .

:HasInlaw  a             owl:Class ;
        rdfs:comment     "This is the n-ary concept for the property hasInlaw"^^xsd:string ;
        rdfs:label       "ha parente per matrimonio"@it , "tiene pariente político"@es , "has in-law"@en , "hat angeheiratete(n) Verwandte(n)"@de ;
        rdfs:seeAlso     :hasInlaw ;
        rdfs:subClassOf  :HasRelative .

:hasInlaw  a                owl:SymmetricProperty ;
        rdfs:comment        "A person (subject) is related with a person (object) by a marriage between themselves or between relatives."^^xsd:string ;
        rdfs:label          "ha parente per matrimonio"@it , "tiene pariente político"@es , "has in-law"@en , "hat angeheiratete(n) Verwandte(n)"@de ;
        rdfs:subPropertyOf  :hasRelative ;
        :correspondsTo      :HasInlaw .

:hasFianceeFiance  a        owl:ObjectProperty ;
        rdfs:comment        "A person (subject) is engaged with a person (object)."^^xsd:string ;
        rdfs:label          "ha fidanzato(a)"@it , "tiene prometido(a)"@es , "has fiancee  or fiance"@en , "hat Verlobte(n)"@de ;
        rdfs:subPropertyOf  :hasInlaw ;
        :correspondsTo      :HasFianceeFiance .

:hasObject  a          owl:ObjectProperty ;
        rdfs:comment   "At an n-ary concept's instance (subject), something (object) takes the object role of the asymmetric relationship meant by the n-ary concept. \nFor inverse relationsships, the subject and object role follow the naming of the n-ary concept when reading quasi just the first part of the n-ary concept name."^^xsd:string ;
        rdfs:domain    :NAries ;
        rdfs:label     "ha oggetto"@it , "tiene objeto"@es , "has object"@en , "hat Objekt"@de ;
        owl:inverseOf  :isObject .

:HasIsFounder  a         owl:Class ;
        rdfs:comment     "This is the n-ary concept for the properties hasFounder / isFounderOf"^^xsd:string ;
        rdfs:label       "ha fondatore o fondatrice / è fondatore o fondatrice di"@it , "tiene fundador(a) / es fundador(a) de"@es , "has founder / is founder of"@en , "hat Gründer / ist Gründer von"@de ;
        rdfs:seeAlso     :isFounderOf , :hasFounder ;
        rdfs:subClassOf  :HasAssociate .

:hasOffspring  a            owl:ObjectProperty ;
        rdfs:comment        "A person (subject) has an offspring (object), where the chain of child-relations might include adoptive, foster, illegitimate, step relations."^^xsd:string ;
        rdfs:label          "ha discendente"@it , "tiene heredero(a)"@es , "has offspring"@en , "hat Nachkomme"@de ;
        rdfs:subPropertyOf  :hasRelative ;
        :correspondsTo      :HasOffspringAncestor .

:hasRelative  a             owl:SymmetricProperty ;
        rdfs:comment        "A person (subject) is kin to a person (object). This denotes not only biological kinship, but also inlaw, adoptive, step, foster relationships."^^xsd:string ;
        rdfs:label          "ha parente"@it , "tiene pariente"@es , "has relative"@en , "hat Verwandte(n)"@de ;
        rdfs:subPropertyOf  :relatedAgent ;
        :correspondsTo      :HasRelative ;
        :hasGndCode         "bezf" .

:HasEmployeeEmployer  a  owl:Class ;
        rdfs:comment     "This is the n-ary concept for the properties hasEmployee and hasEmployer"^^xsd:string ;
        rdfs:label       "ha impiegato(a) / datore di lavoro"@it , "tiene empleado(a) / empleador(a)"@es , "has employee / employer"@en , "hat Arbeitnehmer / Arbeitgeber"@de ;
        rdfs:seeAlso     :hasEmployer , :hasEmployee ;
        rdfs:subClassOf  :HasProfessionalContact .

:hasStudent  a              owl:ObjectProperty ;
        rdfs:comment        "A person (subject) trains a person (object)."^^xsd:string ;
        rdfs:label          "ha scolaro(a)"@it , "tiene estudiante"@es , "has Student"@en , "hat Schüler"@de ;
        rdfs:subPropertyOf  :hasProfessionalContact ;
        :correspondsTo      :HasStudentTeacher ;
        owl:inverseOf       :hasTeacher .

:HasSpiritualContact  a  owl:Class ;
        rdfs:comment     "This is the n-ary concept for the property hasSpiritualContact"^^xsd:string ;
        rdfs:label       "ha contatto spirituale"@it , "tiene guía espiritual"@es , "has spiritual contact"@en , "hat spirituellen Kontakt"@de ;
        rdfs:seeAlso     :hasSpiritualContact ;
        rdfs:subClassOf  :RelatedAgent .

:hasMember  a               owl:ObjectProperty ;
        rdfs:comment        "A goup (subject) has as a member a person (object)."^^xsd:string ;
        rdfs:label          "ha membro"@it , "tiene membrio"@es , "has member"@en , "hat Mitglied"@de ;
        rdfs:subPropertyOf  :hasAssociate ;
        :correspondsTo      :HasIsMember .

:hasPhysician  a               owl:ObjectProperty ;
        rdfs:comment           "A person or corporate body (subject) has as physician a person or corporate body (object)."^^xsd:string ;
        rdfs:label             "ha medico"@it , "tiene médico"@es , "has physician"@en , "hat Arzt"@de ;
        rdfs:subPropertyOf     :hasVitalLethalContact ;
        :correspondsToInverse  :IsHasPhysician .

:relatedAgent  a        owl:ObjectProperty ;
        rdfs:comment    "A person or corporation (subject) has some kind of relation with a person or corporation (object)."^^xsd:string ;
        rdfs:label      "agente connesso"@it , "agente relacionado"@es , "related Agent"@en , "verknüpfter Agens"@de ;
        :correspondsTo  :RelatedAgent .

:hasGodChild  a             owl:ObjectProperty ;
        rdfs:comment        "A person (subject) obtains as godchild a person (object) at the godchild's christening."^^xsd:string ;
        rdfs:label          "ha figlioccio o figlioccia"@it , "tiene ahijado(a)"@es , "has godchild"@en , "hat Patenkind"@de ;
        rdfs:subPropertyOf  :hasNieceNephew ;
        :correspondsTo      :HasGodChildParent ;
        owl:inverseOf       :hasGodParent .
