@prefix dc:    <http://purl.org/dc/elements/1.1/#> .
@prefix :      <http://www.lexinfo.net/ontology/2.0/lexinfo#> .
@prefix ns:    <http://creativecommons.org/ns#> .
@prefix lexinfo: <http://www.lexinfo.net/ontology/2.0/lexinfo#> .
@prefix terms: <http://purl.org/dc/terms/> .
@prefix vann:  <http://purl.org/vocab/vann/> .
@prefix dcr:   <http://www.isocat.org/ns/dcr.rdf#> .
@prefix rdfs:  <http://www.w3.org/2000/01/rdf-schema#> .
@prefix owl2xml: <http://www.w3.org/2006/12/owl2-xml#> .
@prefix xsd:   <http://www.w3.org/2001/XMLSchema#> .
@prefix owl:   <http://www.w3.org/2002/07/owl#> .
@prefix rdf:   <http://www.w3.org/1999/02/22-rdf-syntax-ns#> .
@prefix lemon: <http://lemon-model.net/lemon#> .

lexinfo:Numeral  a           owl:Class ;
        rdfs:isDefinedBy     <http://www.lexinfo.net/ontology/2.0/lexinfo> ;
        rdfs:subClassOf      lemon:Word ;
        owl:equivalentClass  [ a                   owl:Restriction ;
                               owl:onProperty      lexinfo:partOfSpeech ;
                               owl:someValuesFrom  lexinfo:NumeralPOS
                             ] .

lexinfo:numeral  a        owl:NamedIndividual , lexinfo:PartOfSpeech , lexinfo:NumeralPOS , owl:Thing ;
        rdfs:comment      "Part of speech that expresses a number or the relation to a number." ;
        rdfs:isDefinedBy  <http://www.lexinfo.net/ontology/2.0/lexinfo> ;
        rdfs:label        "numeral" ;
        dc:creator        "Francopoulo, Gil" ;
        dcr:datcat        <http://www.isocat.org/datcat/DC-1334> ;
        owl:versionInfo   "1:0" .

lexinfo:ImpersonalIntransitiveFrame
        a                    owl:Class ;
        rdfs:isDefinedBy     <http://www.lexinfo.net/ontology/2.0/lexinfo> ;
        rdfs:subClassOf      lexinfo:ImpersonalFrame ;
        owl:equivalentClass  [ a                   owl:Class ;
                               owl:intersectionOf  ( lexinfo:ImpersonalFrame [ a                owl:Restriction ;
                                                                               owl:cardinality  "0"^^xsd:nonNegativeInteger ;
                                                                               owl:onProperty   lexinfo:object
                                                                             ] )
                             ] .

lexinfo:DativeTransitiveFrame
        a                    owl:Class ;
        rdfs:isDefinedBy     <http://www.lexinfo.net/ontology/2.0/lexinfo> ;
        rdfs:subClassOf      lexinfo:VerbFrame ;
        lexinfo:example      "ich DANKE dir"@de ;
        owl:equivalentClass  [ a                   owl:Class ;
                               owl:intersectionOf  ( lexinfo:VerbFrame [ a                owl:Restriction ;
                                                                         owl:cardinality  "0"^^xsd:nonNegativeInteger ;
                                                                         owl:onProperty   lexinfo:directObject
                                                                       ] [ a                owl:Restriction ;
                                                                           owl:cardinality  "1"^^xsd:nonNegativeInteger ;
                                                                           owl:onProperty   lexinfo:indirectObject
                                                                         ] [ a                owl:Restriction ;
                                                                             owl:cardinality  "1"^^xsd:nonNegativeInteger ;
                                                                             owl:onProperty   lexinfo:subject
                                                                           ] )
                             ] .

lexinfo:interrogativeCardinalNumeral
        a                 lexinfo:PartOfSpeech , lexinfo:NumeralPOS , owl:Thing , owl:NamedIndividual ;
        rdfs:comment      "An interrogative/relative word used to ask about quantity." ;
        rdfs:isDefinedBy  <http://www.lexinfo.net/ontology/2.0/lexinfo> ;
        rdfs:label        "interrogative cardinal numeral" ;
        dc:creator        "Zeman, Dan" ;
        dcr:datcat        <http://www.isocat.org/datcat/DC-3018> ;
        owl:versionInfo   "1:0" .

lexinfo:affix  a          owl:NamedIndividual , lexinfo:TermElement , owl:Thing ;
        rdfs:isDefinedBy  <http://www.lexinfo.net/ontology/2.0/lexinfo> .

terms:modified  a  owl:AnnotationProperty .

lexinfo:cardinalNumeral
        a                 lexinfo:NumeralPOS , owl:Thing , owl:NamedIndividual , lexinfo:PartOfSpeech ;
        rdfs:comment      "A word denoting a number." ;
        rdfs:isDefinedBy  <http://www.lexinfo.net/ontology/2.0/lexinfo> ;
        rdfs:label        "cardinal numeral" ;
        dc:creator        "Zeman, Dan" ;
        dcr:datcat        <http://www.isocat.org/datcat/DC-3027> ;
        owl:versionInfo   "1:0" .

lexinfo:Dating  a         owl:Class ;
        rdfs:isDefinedBy  <http://www.lexinfo.net/ontology/2.0/lexinfo> ;
        rdfs:subClassOf   lemon:PropertyValue .

lexinfo:old  a            owl:NamedIndividual , lexinfo:Dating , owl:Thing ;
        rdfs:comment      "Used in the past." ;
        rdfs:isDefinedBy  <http://www.lexinfo.net/ontology/2.0/lexinfo> ;
        rdfs:label        "old" ;
        dc:creator        "Francopoulo, Gil" ;
        dcr:datcat        <http://www.isocat.org/datcat/DC-1961> ;
        owl:versionInfo   "1:0" .

lexinfo:termType  a         owl:ObjectProperty ;
        rdfs:comment        "An attribute assigned to a lexeme or a term." ;
        rdfs:isDefinedBy    <http://www.lexinfo.net/ontology/2.0/lexinfo> ;
        rdfs:label          "lexTermType" ;
        rdfs:range          lexinfo:TermType ;
        rdfs:subPropertyOf  lemon:property ;
        dc:creator          "Wright, Sue Ellen" ;
        dcr:datcat          <http://www.isocat.org/datcat/DC-315> ;
        owl:versionInfo     "1:0" .

ns:license  a   owl:AnnotationProperty .

lemon:synArg  a  owl:ObjectProperty .

lexinfo:commonGender  a   owl:NamedIndividual , lexinfo:Gender , owl:Thing ;
        rdfs:comment      "Indistinguished gender for epicenes." ;
        rdfs:isDefinedBy  <http://www.lexinfo.net/ontology/2.0/lexinfo> ;
        rdfs:label        "common gender" ;
        dc:creator        "Francopoulo, Gil" ;
        dcr:datcat        <http://www.isocat.org/datcat/DC-1558> ;
        owl:versionInfo   "1:0" .

lexinfo:formula  a        lexinfo:TermType , owl:Thing , owl:NamedIndividual ;
        rdfs:comment      "Figures, symbols or the like used to express a concept briefly, such as a mathematical or chemical formula." ;
        rdfs:isDefinedBy  <http://www.lexinfo.net/ontology/2.0/lexinfo> ;
        rdfs:label        "formula" ;
        dc:creator        "Francopoulo, Gil" , "Wright, Sue Ellen" ;
        dcr:datcat        <http://www.isocat.org/datcat/DC-1888> , <http://www.isocat.org/datcat/DC-325> ;
        owl:versionInfo   "1:0" .

lexinfo:firstPerson  a    owl:NamedIndividual , lexinfo:Person , owl:Thing ;
        rdfs:comment      "First person deixis is deictic reference that refers to the speaker, or both the speaker and referents grouped with the speaker" ;
        rdfs:isDefinedBy  <http://www.lexinfo.net/ontology/2.0/lexinfo> ;
        rdfs:label        "first person" ;
        dc:creator        "Francopoulo, Gil" ;
        dcr:datcat        <http://www.isocat.org/datcat/DC-1288> ;
        owl:versionInfo   "1:0" .

lexinfo:indefinite  a     owl:NamedIndividual , lexinfo:Definiteness , owl:Thing ;
        rdfs:comment      "Value related to an entity in a situation where the identification of this entity is not clear cut." ;
        rdfs:isDefinedBy  <http://www.lexinfo.net/ontology/2.0/lexinfo> ;
        rdfs:label        "indefinite" ;
        dc:creator        "Francopoulo, Gil" ;
        dcr:datcat        <http://www.isocat.org/datcat/DC-2005> ;
        owl:versionInfo   "1:0" .

lexinfo:irreflexivePersonalPronoun
        a                 lexinfo:PartOfSpeech , owl:NamedIndividual , lexinfo:PronounPOS , owl:Thing ;
        rdfs:comment      "personal pronoun which is not reflexive" ;
        rdfs:isDefinedBy  <http://www.lexinfo.net/ontology/2.0/lexinfo> ;
        rdfs:label        "irreflexive personal pronoun" ;
        dc:creator        "Francopoulo, Gil" ;
        dcr:datcat        <http://www.isocat.org/datcat/DC-3013> ;
        owl:versionInfo   "1:0" .

lexinfo:massNoun  a       owl:Thing , lexinfo:Number , owl:NamedIndividual ;
        rdfs:comment      "Designation of a term or word that is not countable and cannot generally be used with the indefinite article or in the plural." ;
        rdfs:isDefinedBy  <http://www.lexinfo.net/ontology/2.0/lexinfo> ;
        rdfs:label        "massNoun" , "mass noun" ;
        dc:creator        "Francopoulo, Gil" , "Wright, Sue Ellen" ;
        dcr:datcat        <http://www.isocat.org/datcat/DC-255> , <http://www.isocat.org/datcat/DC-2277> ;
        owl:versionInfo   "1:0" .

lexinfo:TransitivePPFrame
        a                    owl:Class ;
        rdfs:isDefinedBy     <http://www.lexinfo.net/ontology/2.0/lexinfo> ;
        rdfs:subClassOf      lexinfo:TransitiveFrame ;
        lexinfo:example      "she ADDED salt TO the stew"@en ;
        owl:equivalentClass  [ a                   owl:Class ;
                               owl:intersectionOf  ( lexinfo:PPFrame lexinfo:TransitiveFrame )
                             ] .

lexinfo:paucal  a         owl:NamedIndividual , lexinfo:Number , owl:Thing ;
        rdfs:comment      "Number that specifies 'a few' things." ;
        rdfs:isDefinedBy  <http://www.lexinfo.net/ontology/2.0/lexinfo> ;
        rdfs:label        "paucal" ;
        dc:creator        "Francopoulo, Gil" ;
        dcr:datcat        <http://www.isocat.org/datcat/DC-1350> ;
        owl:versionInfo   "1:0" .

lexinfo:aspect  a           owl:ObjectProperty ;
        rdfs:comment        "Category associated to verbs and referring to the way the grammar marks the duration or type of temporal activity." ;
        rdfs:isDefinedBy    <http://www.lexinfo.net/ontology/2.0/lexinfo> ;
        rdfs:label          "aspect" ;
        rdfs:range          lexinfo:Aspect ;
        rdfs:subPropertyOf  lexinfo:morphosyntacticProperty ;
        dc:creator          "Francopoulo, Gil" ;
        dcr:datcat          <http://www.isocat.org/datcat/DC-1242> ;
        owl:versionInfo     "1:0" .

lexinfo:initialism  a     owl:Thing , lexinfo:TermType , owl:NamedIndividual , lexinfo:AbbreviatedForm ;
        rdfs:comment      "An abbreviation made up of the initial letters of the components of the full form of the designation or from syllables of the full form and pronounced letter by letter." ;
        rdfs:isDefinedBy  <http://www.lexinfo.net/ontology/2.0/lexinfo> ;
        rdfs:label        "initialism" ;
        dc:creator        "Wright, Sue Ellen" ;
        dcr:datcat        <http://www.isocat.org/datcat/DC-333> ;
        owl:versionInfo   "1:0" .

lexinfo:inanimate  a      lexinfo:Animacy , owl:Thing , owl:NamedIndividual ;
        rdfs:comment      "Perceived as not living." ;
        rdfs:isDefinedBy  <http://www.lexinfo.net/ontology/2.0/lexinfo> ;
        rdfs:label        "inanimate" ;
        dc:creator        "Wright, Sue Ellen" , "Francopoulo, Gil" ;
        dcr:datcat        <http://www.isocat.org/datcat/DC-1952> , <http://www.isocat.org/datcat/DC-80> ;
        owl:versionInfo   "1:0" .

lexinfo:NounPossessiveFrame
        a                    owl:Class ;
        rdfs:isDefinedBy     <http://www.lexinfo.net/ontology/2.0/lexinfo> ;
        rdfs:subClassOf      lexinfo:NounFrame ;
        lexinfo:example      "the CAPITAL OF france is paris"@en ;
        owl:equivalentClass  [ a                   owl:Class ;
                               owl:intersectionOf  ( lexinfo:NounFrame [ a                   owl:Restriction ;
                                                                         owl:minCardinality  "1"^^xsd:nonNegativeInteger ;
                                                                         owl:onProperty      lexinfo:copulativeArg
                                                                       ] [ a                            owl:Restriction ;
                                                                           owl:minQualifiedCardinality  "1"^^xsd:nonNegativeInteger ;
                                                                           owl:onClass                  lexinfo:PossessiveAdjunct ;
                                                                           owl:onProperty               lexinfo:possessiveAdjunct
                                                                         ] )
                             ] .

lexinfo:Cliticness  a     owl:Class ;
        rdfs:isDefinedBy  <http://www.lexinfo.net/ontology/2.0/lexinfo> ;
        rdfs:subClassOf   lexinfo:MorphosyntacticProperty .

lexinfo:partitiveCase
        a                 owl:NamedIndividual , lexinfo:Case , owl:Thing ;
        rdfs:comment      "Case that expresses the partial nature of the referent of the noun it marks, as opposed to expressing the whole unit or class of which the referent is a part." ;
        rdfs:isDefinedBy  <http://www.lexinfo.net/ontology/2.0/lexinfo> ;
        rdfs:label        "partitive case" ;
        dc:creator        "Francopoulo, Gil" ;
        dcr:datcat        <http://www.isocat.org/datcat/DC-2003> ;
        owl:versionInfo   "1:0" .

lexinfo:causallyRelatedConcept
        a                   owl:ObjectProperty ;
        rdfs:comment        "A concept that is related to another concept by virtue of the fact that it plays a causative role with respect to that concept." ;
        rdfs:isDefinedBy    <http://www.lexinfo.net/ontology/2.0/lexinfo> ;
        rdfs:label          "causallyRelatedConcept" ;
        rdfs:subPropertyOf  lemon:senseRelation ;
        dc:creator          "Wright, Sue Ellen" ;
        dcr:datcat          <http://www.isocat.org/datcat/DC-123> ;
        owl:versionInfo     "1:0" .

lexinfo:AdjectiveFrame
        a                owl:Class ;
        rdfs:subClassOf  lemon:Frame .

lexinfo:subjunctiveClause
        a                   owl:ObjectProperty ;
        rdfs:isDefinedBy    <http://www.lexinfo.net/ontology/2.0/lexinfo> ;
        rdfs:subPropertyOf  lexinfo:clausalArg .

lexinfo:AttributiveArgument
        a                 owl:Class ;
        rdfs:isDefinedBy  <http://www.lexinfo.net/ontology/2.0/lexinfo> ;
        rdfs:subClassOf   lemon:Argument .

lexinfo:AdverbPOS  a      owl:Class ;
        rdfs:isDefinedBy  <http://www.lexinfo.net/ontology/2.0/lexinfo> ;
        rdfs:subClassOf   lexinfo:PartOfSpeech .

lexinfo:IntransitivePPFrame
        a                    owl:Class ;
        rdfs:isDefinedBy     <http://www.lexinfo.net/ontology/2.0/lexinfo> ;
        rdfs:subClassOf      lexinfo:IntransitiveFrame ;
        lexinfo:example      "he TOOK CARE OF her"@en ;
        owl:equivalentClass  [ a                   owl:Class ;
                               owl:intersectionOf  ( lexinfo:IntransitiveFrame lexinfo:PPFrame )
                             ] .

lexinfo:interjection  a   owl:NamedIndividual , lexinfo:PartOfSpeech , owl:Thing ;
        rdfs:comment      "Word or sound that expresses an emotion." ;
        rdfs:isDefinedBy  <http://www.lexinfo.net/ontology/2.0/lexinfo> ;
        rdfs:label        "interjection" ;
        dc:creator        "Francopoulo, Gil" ;
        dcr:datcat        <http://www.isocat.org/datcat/DC-1318> ;
        owl:versionInfo   "1:0" .

lexinfo:genitiveObject
        a                   owl:ObjectProperty ;
        rdfs:isDefinedBy    <http://www.lexinfo.net/ontology/2.0/lexinfo> ;
        rdfs:range          lexinfo:GenitiveObject ;
        rdfs:subPropertyOf  lexinfo:object .

lexinfo:abessiveCase  a   owl:NamedIndividual , lexinfo:Case , owl:Thing ;
        rdfs:comment      "Case that expresses the lack or absence of the referent of the noun it marks." ;
        rdfs:isDefinedBy  <http://www.lexinfo.net/ontology/2.0/lexinfo> ;
        rdfs:label        "abessive case" ;
        dc:creator        "Francopoulo, Gil" ;
        dcr:datcat        <http://www.isocat.org/datcat/DC-1223> ;
        owl:versionInfo   "1:0" .

lemon:optional  a  owl:DatatypeProperty .

lexinfo:fusedPrepositionDeterminer
        a                 lexinfo:FusedPrepositionPOS , lexinfo:PartOfSpeech , owl:NamedIndividual , owl:Thing ;
        rdfs:comment      "word resulting from the aggregation of a proposition and a determiner" ;
        rdfs:isDefinedBy  <http://www.lexinfo.net/ontology/2.0/lexinfo> ;
        rdfs:label        "fused preposition determiner" ;
        dc:creator        "Francopoulo, Gil" ;
        dcr:datcat        <http://www.isocat.org/datcat/DC-3010> ;
        owl:versionInfo   "1:0" .

lexinfo:subordinatingConjunction
        a                 owl:NamedIndividual , lexinfo:PartOfSpeech , lexinfo:ConjunctionPOS , owl:Thing ;
        rdfs:comment      "Conjunction that links constructions by making one of them a constituent of another. The subordinating conjunction typically marks the incorporated constituent." ;
        rdfs:isDefinedBy  <http://www.lexinfo.net/ontology/2.0/lexinfo> ;
        rdfs:label        "subordinating conjunction" ;
        dc:creator        "Francopoulo, Gil" ;
        dcr:datcat        <http://www.isocat.org/datcat/DC-1393> ;
        owl:versionInfo   "1:0" .

lexinfo:pronoun  a        owl:Thing , lexinfo:PronounPOS , lexinfo:PartOfSpeech , owl:NamedIndividual ;
        rdfs:comment      "Word used in place of a noun or a noun phrase." ;
        rdfs:isDefinedBy  <http://www.lexinfo.net/ontology/2.0/lexinfo> ;
        rdfs:label        "pronoun" ;
        dc:creator        "Francopoulo, Gil" ;
        dcr:datcat        <http://www.isocat.org/datcat/DC-1370> ;
        owl:versionInfo   "1:0" .

lexinfo:imperfectTenseForm
        a                   owl:ObjectProperty ;
        rdfs:isDefinedBy    <http://www.lexinfo.net/ontology/2.0/lexinfo> ;
        rdfs:subPropertyOf  lexinfo:formTenseVariant .

lexinfo:GenitivePostPositiveArgument
        a                    owl:Class ;
        rdfs:isDefinedBy     <http://www.lexinfo.net/ontology/2.0/lexinfo> ;
        rdfs:subClassOf      lexinfo:PostPositiveArgument ;
        owl:equivalentClass  [ a                   owl:Class ;
                               owl:intersectionOf  ( lexinfo:PostPositiveArgument [ a               owl:Restriction ;
                                                                                    owl:hasValue    lexinfo:genitiveCase ;
                                                                                    owl:onProperty  lemon:marker
                                                                                  ] )
                             ] .

lexinfo:indicative  a     lexinfo:VerbFormMood , lexinfo:Mood , owl:NamedIndividual , owl:Thing ;
        rdfs:comment      "Mood value used in the expression of statements and questions." , "..." ;
        rdfs:isDefinedBy  <http://www.lexinfo.net/ontology/2.0/lexinfo> ;
        rdfs:label        "indicative" ;
        dc:creator        "Wright, Sue Ellen" , "Francopoulo, Gil" ;
        dcr:datcat        <http://www.isocat.org/datcat/DC-367> , <http://www.isocat.org/datcat/DC-1885> ;
        owl:versionInfo   "1:0" .

lexinfo:commonNoun  a     lexinfo:PartOfSpeech , lexinfo:NounPOS , owl:Thing , owl:NamedIndividual ;
        rdfs:comment      "Noun that signifies a non-specific member of a group." , "A noun or adjective denoting a class of objects." ;
        rdfs:isDefinedBy  <http://www.lexinfo.net/ontology/2.0/lexinfo> ;
        rdfs:label        "commonNoun" , "common noun" ;
        dc:creator        "Francopoulo, Gil" , "Wright, Sue Ellen" ;
        dcr:datcat        <http://www.isocat.org/datcat/DC-1256> , <http://www.isocat.org/datcat/DC-385> ;
        owl:versionInfo   "1:0" .

lexinfo:substanceHolonym
        a                   owl:ObjectProperty ;
        rdfs:comment        "Indicates what this is composed of"@en ;
        rdfs:isDefinedBy    <http://www.lexinfo.net/ontology/2.0/lexinfo> ;
        rdfs:label          "substance holonym"@en ;
        rdfs:subPropertyOf  lexinfo:holonymTerm .

lexinfo:inHouseRegister
        a                 owl:NamedIndividual , owl:Thing , lexinfo:Register ;
        rdfs:comment      "The register of terms that are company-specific and not readily recognized outside this environment." , "Register of terms that are company-specific and not readily recognized outside this environment." ;
        rdfs:isDefinedBy  <http://www.lexinfo.net/ontology/2.0/lexinfo> ;
        rdfs:label        "in house register" ;
        dc:creator        "Francopoulo, Gil" , "Wright, Sue Ellen" ;
        dcr:datcat        <http://www.isocat.org/datcat/DC-426> , <http://www.isocat.org/datcat/DC-1993> ;
        owl:versionInfo   "1:0" .

lexinfo:PronounPOS  a     owl:Class ;
        rdfs:isDefinedBy  <http://www.lexinfo.net/ontology/2.0/lexinfo> ;
        rdfs:subClassOf   lexinfo:PartOfSpeech .

lexinfo:shortArticle  a   owl:NamedIndividual , lexinfo:Definiteness , owl:Thing ;
        rdfs:comment      "For definiteness, when a specific form is not the syntactic subject of the clause." ;
        rdfs:isDefinedBy  <http://www.lexinfo.net/ontology/2.0/lexinfo> ;
        rdfs:label        "short article" ;
        dc:creator        "Francopoulo, Gil" ;
        dcr:datcat        <http://www.isocat.org/datcat/DC-1927> ;
        owl:versionInfo   "1:0" .

lexinfo:possessiveRelativePronoun
        a                 owl:NamedIndividual , lexinfo:PartOfSpeech , owl:Thing , lexinfo:PronounPOS ;
        rdfs:comment      "A relative pronoun whose antecedent is the possessor of the subject or object in the relative clause." ;
        rdfs:isDefinedBy  <http://www.lexinfo.net/ontology/2.0/lexinfo> ;
        rdfs:label        "possessive relative pronoun" ;
        dc:creator        "Zeman, Dan" ;
        dcr:datcat        <http://www.isocat.org/datcat/DC-3005> ;
        owl:versionInfo   "1:0" .

lemon:Frame  a  owl:Class .

lexinfo:plural  a         owl:Thing , owl:NamedIndividual , lexinfo:Number ;
        rdfs:comment      "The form of a term or word (usually of a noun) used to designate more than one object." , "Value that expresses more than one element." ;
        rdfs:isDefinedBy  <http://www.lexinfo.net/ontology/2.0/lexinfo> ;
        rdfs:label        "plural" ;
        dc:creator        "Francopoulo, Gil" , "Wright, Sue Ellen" ;
        dcr:datcat        <http://www.isocat.org/datcat/DC-253> , <http://www.isocat.org/datcat/DC-1354> ;
        owl:versionInfo   "1:0" .

lexinfo:senseExample  a     owl:ObjectProperty ;
        rdfs:comment        "Descriptive material that provides a sample of an object or entity defined in the entry." ;
        rdfs:isDefinedBy    <http://www.lexinfo.net/ontology/2.0/lexinfo> ;
        rdfs:label          "sense example" ;
        rdfs:subPropertyOf  lemon:definition ;
        dc:creator          "Francopoulo, Gil" , "Wright, Sue Ellen" ;
        dcr:datcat          <http://www.isocat.org/datcat/DC-222> , <http://www.isocat.org/datcat/DC-1958> ;
        owl:versionInfo     "1:0" .

lexinfo:semiColon  a      lexinfo:SymbolPOS , owl:NamedIndividual , owl:Thing , lexinfo:PartOfSpeech ;
        rdfs:comment      "Sign (;) usually used to separate phrases." ;
        rdfs:isDefinedBy  <http://www.lexinfo.net/ontology/2.0/lexinfo> ;
        rdfs:label        "semi-colon" ;
        dc:creator        "Francopoulo, Gil" ;
        dcr:datcat        <http://www.isocat.org/datcat/DC-1446> ;
        owl:versionInfo   "1:0" .

lexinfo:reflexiveDeterminer
        a                 lexinfo:PartOfSpeech , lexinfo:DeterminerPOS , owl:Thing , owl:NamedIndividual ;
        rdfs:comment      "Determiner that refers to the same entity." ;
        rdfs:isDefinedBy  <http://www.lexinfo.net/ontology/2.0/lexinfo> ;
        rdfs:label        "reflexive adjective" ;
        dc:creator        "Francopoulo, Gil" ;
        dcr:datcat        <http://www.isocat.org/datcat/DC-1377> ;
        owl:versionInfo   "1:0" .

lexinfo:negativeParticle
        a                 lexinfo:PartOfSpeech , owl:Thing , lexinfo:ParticlePOS , owl:NamedIndividual ;
        rdfs:comment      "Particle used to express negation." ;
        rdfs:isDefinedBy  <http://www.lexinfo.net/ontology/2.0/lexinfo> ;
        rdfs:label        "negative particle" ;
        dc:creator        "Francopoulo, Gil" ;
        dcr:datcat        <http://www.isocat.org/datcat/DC-1894> ;
        owl:versionInfo   "1:0" .

lexinfo:indefiniteCardinalNumeral
        a                 owl:NamedIndividual , lexinfo:NumeralPOS , lexinfo:PartOfSpeech , owl:Thing ;
        rdfs:comment      "A word used to express imprecise quantity." ;
        rdfs:isDefinedBy  <http://www.lexinfo.net/ontology/2.0/lexinfo> ;
        rdfs:label        "indefinite cardinal numeral" ;
        dc:creator        "Zeman, Dan" ;
        dcr:datcat        <http://www.isocat.org/datcat/DC-3023> ;
        owl:versionInfo   "1:0" .

lexinfo:gerundClause  a     owl:ObjectProperty ;
        rdfs:isDefinedBy    <http://www.lexinfo.net/ontology/2.0/lexinfo> ;
        rdfs:subPropertyOf  lexinfo:clausalArg .

lexinfo:AdpositionalObject
        a                    owl:Class ;
        rdfs:isDefinedBy     <http://www.lexinfo.net/ontology/2.0/lexinfo> ;
        rdfs:subClassOf      lexinfo:Object ;
        rdfs:subClassOf      [ a                   owl:Restriction ;
                               owl:onProperty      lemon:marker ;
                               owl:someValuesFrom  lexinfo:Adposition
                             ] ;
        owl:equivalentClass  [ a                   owl:Class ;
                               owl:intersectionOf  ( lexinfo:Object [ a                   owl:Restriction ;
                                                                      owl:onProperty      lemon:marker ;
                                                                      owl:someValuesFrom  lexinfo:Adposition
                                                                    ] )
                             ] .

lexinfo:root  a             owl:ObjectProperty ;
        rdfs:comment        "base of a word" ;
        rdfs:isDefinedBy    <http://www.lexinfo.net/ontology/2.0/lexinfo> ;
        rdfs:label          "root" ;
        rdfs:subPropertyOf  lemon:lexicalVariant ;
        dc:creator          "Francopoulo, Gil" ;
        dcr:datcat          <http://www.isocat.org/datcat/DC-2231> ;
        owl:versionInfo     "1:0" .

lexinfo:IntransitiveInfinitiveACFrame
        a                    owl:Class ;
        rdfs:isDefinedBy     <http://www.lexinfo.net/ontology/2.0/lexinfo> ;
        rdfs:subClassOf      lexinfo:InfinitiveFrame ;
        lexinfo:example      "I HELPED [to save the child]"@en ;
        owl:equivalentClass  [ a                   owl:Class ;
                               owl:intersectionOf  ( lexinfo:ArbitraryControl lexinfo:InfinitiveFrame lexinfo:IntransitiveFrame )
                             ] .

lexinfo:standardText  a   owl:NamedIndividual , lexinfo:TermType , owl:Thing ;
        rdfs:comment      "A fixed chunk of recurring text." ;
        rdfs:isDefinedBy  <http://www.lexinfo.net/ontology/2.0/lexinfo> ;
        rdfs:label        "standard text" ;
        dc:creator        "Wright, Sue Ellen" ;
        dcr:datcat        <http://www.isocat.org/datcat/DC-343> ;
        owl:versionInfo   "1:0" .

lexinfo:preterite  a  lexinfo:Tense , owl:NamedIndividual ;
        rdfs:comment  "The simple past or preterite as distinct from the perfect form, e.g,, \"showed\" not \"shown\""@en .

lexinfo:partMeronym  a      owl:ObjectProperty ;
        rdfs:comment        "Indicates this a component of the other concept"@en ;
        rdfs:isDefinedBy    <http://www.lexinfo.net/ontology/2.0/lexinfo> ;
        rdfs:label          "part meronym"@en ;
        rdfs:subPropertyOf  lexinfo:meronymTerm .

lexinfo:accusativeCaseForm
        a                   owl:ObjectProperty ;
        rdfs:isDefinedBy    <http://www.lexinfo.net/ontology/2.0/lexinfo> ;
        rdfs:subPropertyOf  lexinfo:formCaseVariant .

lexinfo:gender  a           owl:ObjectProperty ;
        rdfs:comment        "A grammatical category that indicates grammatical relationships between words in sentences." ;
        rdfs:isDefinedBy    <http://www.lexinfo.net/ontology/2.0/lexinfo> ;
        rdfs:label          "grammatical gender" ;
        rdfs:range          lexinfo:Gender ;
        rdfs:subPropertyOf  lexinfo:morphosyntacticProperty ;
        dcr:datcat          <http://www.isocat.org/datcat/DC-245> , <http://www.isocat.org/datcat/DC-1297> .

lexinfo:Particle  a          owl:Class ;
        rdfs:isDefinedBy     <http://www.lexinfo.net/ontology/2.0/lexinfo> ;
        rdfs:subClassOf      lemon:Word ;
        owl:equivalentClass  [ a                   owl:Restriction ;
                               owl:onProperty      lexinfo:partOfSpeech ;
                               owl:someValuesFrom  lexinfo:ParticlePOS
                             ] .

lexinfo:transliteration
        a                   owl:DatatypeProperty ;
        rdfs:comment        "Form resulting from the conversion of one writing system into another" ;
        rdfs:isDefinedBy    <http://www.lexinfo.net/ontology/2.0/lexinfo> ;
        rdfs:label          "transliteration" ;
        rdfs:range          xsd:string ;
        rdfs:subPropertyOf  lemon:representation ;
        dc:creator          "Francopoulo, Gil" ;
        dcr:datcat          <http://www.isocat.org/datcat/DC-1848> ;
        owl:versionInfo     "1:0" .

lexinfo:explanation  a      owl:ObjectProperty ;
        rdfs:comment        "A statement that describes and clarifies a concept and makes it understandable, but does not necessarily differentiate it from other concepts." ;
        rdfs:isDefinedBy    <http://www.lexinfo.net/ontology/2.0/lexinfo> ;
        rdfs:label          "explanation" ;
        rdfs:subPropertyOf  lemon:definition ;
        dc:creator          "Wright, Sue Ellen" ;
        dcr:datcat          <http://www.isocat.org/datcat/DC-223> ;
        owl:versionInfo     "1:0" .

lexinfo:past  a           owl:NamedIndividual , lexinfo:Tense , owl:Thing ;
        rdfs:comment      "Past tense is an absolute tense that refers to a time before the moment of utterance." ;
        rdfs:isDefinedBy  <http://www.lexinfo.net/ontology/2.0/lexinfo> ;
        rdfs:label        "past" ;
        dc:creator        "Francopoulo, Gil" ;
        dcr:datcat        <http://www.isocat.org/datcat/DC-1347> ;
        owl:versionInfo   "1:0" .

lexinfo:essiveCase  a     owl:NamedIndividual , lexinfo:Case , owl:Thing ;
        rdfs:comment      "Case which expresses a state of being." ;
        rdfs:isDefinedBy  <http://www.lexinfo.net/ontology/2.0/lexinfo> ;
        rdfs:label        "essive case" ;
        dc:creator        "Francopoulo, Gil" ;
        dcr:datcat        <http://www.isocat.org/datcat/DC-1281> ;
        owl:versionInfo   "1:0" .

lexinfo:adjunct  a          owl:ObjectProperty ;
        rdfs:isDefinedBy    <http://www.lexinfo.net/ontology/2.0/lexinfo> ;
        rdfs:range          lexinfo:Adjunct ;
        rdfs:subPropertyOf  lemon:synArg .

lemon:Argument  a  owl:Class .

lexinfo:GerundFrame  a       owl:Class ;
        rdfs:comment         "Indicates one of the arguments is a gerund clause"@en ;
        rdfs:isDefinedBy     <http://www.lexinfo.net/ontology/2.0/lexinfo> ;
        rdfs:subClassOf      lexinfo:VerbFrame ;
        owl:equivalentClass  [ a                   owl:Class ;
                               owl:intersectionOf  ( lexinfo:VerbFrame [ a                   owl:Restriction ;
                                                                         owl:onProperty      lemon:synArg ;
                                                                         owl:someValuesFrom  lexinfo:Gerund
                                                                       ] )
                             ] .

lexinfo:finite  a         owl:NamedIndividual , lexinfo:Finiteness , owl:Thing ;
        rdfs:comment      "Property applied to a verb form that can occur on its own in an independent sentence." ;
        rdfs:isDefinedBy  <http://www.lexinfo.net/ontology/2.0/lexinfo> ;
        rdfs:label        "finite" ;
        dc:creator        "Francopoulo, Gil" ;
        dcr:datcat        <http://www.isocat.org/datcat/DC-1287> ;
        owl:versionInfo   "1:0" .

lexinfo:singularNumberForm
        a                   owl:ObjectProperty ;
        rdfs:isDefinedBy    <http://www.lexinfo.net/ontology/2.0/lexinfo> ;
        rdfs:subPropertyOf  lexinfo:formNumberVariant .

lexinfo:memberMeronym
        a                   owl:ObjectProperty ;
        rdfs:comment        "Indicates this is an element of the other"@en ;
        rdfs:isDefinedBy    <http://www.lexinfo.net/ontology/2.0/lexinfo> ;
        rdfs:label          "member meronym"@en ;
        rdfs:subPropertyOf  lexinfo:meronymTerm .

lexinfo:string  a         owl:NamedIndividual , lexinfo:TermType , owl:Thing ;
        rdfs:comment      "A chunk of text used in a software interface, documentation, help file, or the like." ;
        rdfs:isDefinedBy  <http://www.lexinfo.net/ontology/2.0/lexinfo> ;
        rdfs:label        "string" ;
        dc:creator        "Wright, Sue Ellen" ;
        dcr:datcat        <http://www.isocat.org/datcat/DC-344> ;
        owl:versionInfo   "1:0" .

lexinfo:indefiniteMultiplicativeNumeral
        a                 lexinfo:NumeralPOS , owl:Thing , lexinfo:PartOfSpeech , owl:NamedIndividual ;
        rdfs:comment      "A word indicating imprecise number of times something happened." ;
        rdfs:isDefinedBy  <http://www.lexinfo.net/ontology/2.0/lexinfo> ;
        rdfs:label        "indefinite multiplicative numeral" ;
        dc:creator        "Zeman, Dan" ;
        dcr:datcat        <http://www.isocat.org/datcat/DC-3024> ;
        owl:versionInfo   "1:0" .

lexinfo:sociativeCase
        a                 owl:NamedIndividual , lexinfo:Case , owl:Thing ;
        rdfs:comment      "Case related to the person in whose company the action is carried out, or to any belongings of people which take part in the action." ;
        rdfs:isDefinedBy  <http://www.lexinfo.net/ontology/2.0/lexinfo> ;
        rdfs:label        "sociative case" ;
        dc:creator        "Francopoulo, Gil" ;
        dcr:datcat        <http://www.isocat.org/datcat/DC-1388> ;
        owl:versionInfo   "1:0" .

lexinfo:example  a    owl:AnnotationProperty ;
        rdfs:comment  "An example of the usage of a frame."@en ;
        rdfs:label    "example" .

lexinfo:superlativeDegreeForm
        a                   owl:ObjectProperty ;
        rdfs:isDefinedBy    <http://www.lexinfo.net/ontology/2.0/lexinfo> ;
        rdfs:subPropertyOf  lexinfo:formDegreeVariant .

lexinfo:slangRegister
        a                 owl:NamedIndividual , lexinfo:Register , owl:Thing ;
        rdfs:comment      "An extremely informal register of a word, term, or text that is used in spoken and everyday language and less commonly in documents." ;
        rdfs:isDefinedBy  <http://www.lexinfo.net/ontology/2.0/lexinfo> ;
        rdfs:label        "slang register" ;
        dc:creator        "Wright, Sue Ellen" , "Francopoulo, Gil" ;
        dcr:datcat        <http://www.isocat.org/datcat/DC-428> , <http://www.isocat.org/datcat/DC-1995> ;
        owl:versionInfo   "1:0" .

lexinfo:possessiveDeterminer
        a                 owl:Thing , lexinfo:PartOfSpeech , lexinfo:DeterminerPOS , owl:NamedIndividual ;
        rdfs:comment      "Determiner that expresses ownership." ;
        rdfs:isDefinedBy  <http://www.lexinfo.net/ontology/2.0/lexinfo> ;
        rdfs:label        "possessive determiner" ;
        dc:creator        "Francopoulo, Gil" ;
        dcr:datcat        <http://www.isocat.org/datcat/DC-1357> ;
        owl:versionInfo   "1:0" .

lexinfo:point  a          owl:NamedIndividual , lexinfo:PartOfSpeech , owl:Thing , lexinfo:SymbolPOS ;
        rdfs:comment      "Sign (.) used to expresses the end of a sentence or an abbreviation." ;
        rdfs:isDefinedBy  <http://www.lexinfo.net/ontology/2.0/lexinfo> ;
        rdfs:label        "point" ;
        dc:creator        "Francopoulo, Gil" ;
        dcr:datcat        <http://www.isocat.org/datcat/DC-1445> ;
        owl:versionInfo   "1:0" .

lexinfo:complement  a       owl:ObjectProperty ;
        rdfs:comment        "A noun phrase that follows a copula or similar verb, as for example an idiot in the sentence He is an idiot. - A clause that serves as the subject or direct object of a verb or the direct object of a preposition, as for example that he would be early in the sentence I hoped that he would be early" ;
        rdfs:isDefinedBy    <http://www.lexinfo.net/ontology/2.0/lexinfo> ;
        rdfs:label          "complement" ;
        rdfs:range          lexinfo:Complement ;
        rdfs:subPropertyOf  lemon:synArg ;
        dcr:datcat          <http://www.isocat.org/datcat/DC-1257> .

lexinfo:pronunciation
        a                   owl:DatatypeProperty ;
        rdfs:comment        "The representation of the manner by which a term or word is articulated." ;
        rdfs:isDefinedBy    <http://www.lexinfo.net/ontology/2.0/lexinfo> ;
        rdfs:label          "pronunciation" ;
        rdfs:range          xsd:string ;
        rdfs:subPropertyOf  lemon:representation ;
        dc:creator          "Wright, Sue Ellen" ;
        dcr:datcat          <http://www.isocat.org/datcat/DC-407> ;
        owl:versionInfo     "1:0" .

lexinfo:negativePronoun
        a                 lexinfo:PartOfSpeech , owl:Thing , owl:NamedIndividual , lexinfo:PronounPOS ;
        rdfs:comment      "Pronoun used in a context of a negation or for expressing a negation." ;
        rdfs:isDefinedBy  <http://www.lexinfo.net/ontology/2.0/lexinfo> ;
        rdfs:label        "negative pronoun" ;
        dc:creator        "Francopoulo, Gil" ;
        dcr:datcat        <http://www.isocat.org/datcat/DC-1925> ;
        owl:versionInfo   "1:0" .

lexinfo:TransitiveInfinitiveACFrame
        a                    owl:Class ;
        rdfs:isDefinedBy     <http://www.lexinfo.net/ontology/2.0/lexinfo> ;
        rdfs:subClassOf      lexinfo:InfinitiveFrame ;
        lexinfo:example      "they CONVINCED him [to go]"@en ;
        owl:equivalentClass  [ a                   owl:Class ;
                               owl:intersectionOf  ( lexinfo:ArbitraryControl lexinfo:InfinitiveFrame lexinfo:TransitiveFrame )
                             ] .

lexinfo:ProperNoun  a        owl:Class ;
        rdfs:isDefinedBy     <http://www.lexinfo.net/ontology/2.0/lexinfo> ;
        rdfs:subClassOf      lexinfo:Noun ;
        owl:equivalentClass  [ a               owl:Restriction ;
                               owl:hasValue    lexinfo:properNoun ;
                               owl:onProperty  lexinfo:partOfSpeech
                             ] .

lexinfo:passiveVoice  a   owl:NamedIndividual , lexinfo:Voice , owl:Thing ;
        rdfs:comment      "Term referring to a situation where the grammatical subject is typically the recipient or goal of the action denoted by the verb." ;
        rdfs:isDefinedBy  <http://www.lexinfo.net/ontology/2.0/lexinfo> ;
        rdfs:label        "passive voice" ;
        dc:creator        "Francopoulo, Gil" ;
        dcr:datcat        <http://www.isocat.org/datcat/DC-1346> ;
        owl:versionInfo   "1:0" .

lexinfo:comma  a          lexinfo:SymbolPOS , owl:Thing , lexinfo:PartOfSpeech , owl:NamedIndividual ;
        rdfs:comment      "Mark (,) used in writing to show a short pause or to separate items in a list." ;
        rdfs:isDefinedBy  <http://www.lexinfo.net/ontology/2.0/lexinfo> ;
        rdfs:label        "comma" ;
        dc:creator        "Francopoulo, Gil" ;
        dcr:datcat        <http://www.isocat.org/datcat/DC-1448> ;
        owl:versionInfo   "1:0" .

lexinfo:ParticlePOS  a    owl:Class ;
        rdfs:isDefinedBy  <http://www.lexinfo.net/ontology/2.0/lexinfo> ;
        rdfs:subClassOf   lexinfo:PartOfSpeech .

lexinfo:adessiveCase  a   owl:NamedIndividual , lexinfo:Case , owl:Thing ;
        rdfs:comment      "Case which expresses the meaning of presence 'at' or 'near' a place." ;
        rdfs:isDefinedBy  <http://www.lexinfo.net/ontology/2.0/lexinfo> ;
        rdfs:label        "adessive case" ;
        dc:creator        "Francopoulo, Gil" ;
        dcr:datcat        <http://www.isocat.org/datcat/DC-1228> ;
        owl:versionInfo   "1:0" .

lexinfo:singular  a       lexinfo:Number , owl:Thing , owl:NamedIndividual ;
        rdfs:comment      "Value that expresses one element." , "The form of a term or word (usually of a noun) used to designate one object." ;
        rdfs:isDefinedBy  <http://www.lexinfo.net/ontology/2.0/lexinfo> ;
        rdfs:label        "singular" ;
        dc:creator        "Francopoulo, Gil" , "Wright, Sue Ellen" ;
        dcr:datcat        <http://www.isocat.org/datcat/DC-1387> , <http://www.isocat.org/datcat/DC-252> ;
        owl:versionInfo   "1:0" .

lexinfo:setPhrase  a      owl:NamedIndividual , lexinfo:TermType , owl:Thing ;
        rdfs:comment      "A fixed, lexicalized phrase." ;
        rdfs:isDefinedBy  <http://www.lexinfo.net/ontology/2.0/lexinfo> ;
        rdfs:label        "set phrase" ;
        dc:creator        "Wright, Sue Ellen" ;
        dcr:datcat        <http://www.isocat.org/datcat/DC-341> ;
        owl:versionInfo   "1:0" .

lexinfo:degree  a           owl:ObjectProperty ;
        rdfs:comment        "Property concerning comparison." ;
        rdfs:isDefinedBy    <http://www.lexinfo.net/ontology/2.0/lexinfo> ;
        rdfs:label          "degree" ;
        rdfs:range          lexinfo:Degree ;
        rdfs:subPropertyOf  lexinfo:morphosyntacticProperty ;
        dc:creator          "Francopoulo, Gil" ;
        dcr:datcat          <http://www.isocat.org/datcat/DC-1419> ;
        owl:versionInfo     "1:0" .

lexinfo:collectivePronoun
        a                 owl:Thing , lexinfo:PronounPOS , owl:NamedIndividual , lexinfo:PartOfSpeech ;
        rdfs:comment      "A pronoun that refers to all elements of a set." ;
        rdfs:isDefinedBy  <http://www.lexinfo.net/ontology/2.0/lexinfo> ;
        rdfs:label        "collective pronoun" ;
        dc:creator        "Zeman, Dan" ;
        dcr:datcat        <http://www.isocat.org/datcat/DC-3006> ;
        owl:versionInfo   "1:0" .

lexinfo:InterrogativeInfinitiveFrame
        a                    owl:Class ;
        rdfs:comment         "Indicates the frame has an argument that is a clause with both an interrogative and the clause is in the infinitive form"@en ;
        rdfs:isDefinedBy     <http://www.lexinfo.net/ontology/2.0/lexinfo> ;
        rdfs:subClassOf      lexinfo:VerbFrame ;
        owl:equivalentClass  [ a                   owl:Class ;
                               owl:intersectionOf  ( lexinfo:VerbFrame [ a                   owl:Restriction ;
                                                                         owl:minCardinality  "1"^^xsd:nonNegativeInteger ;
                                                                         owl:onProperty      lexinfo:interrogativeInfinitiveClause
                                                                       ] )
                             ] .

lexinfo:punctuation  a    lexinfo:PartOfSpeech , owl:Thing , owl:NamedIndividual , lexinfo:SymbolPOS ;
        rdfs:comment      "Graphical mark used either at word level to indicate an abbreviation or at a text level to separate phrases or sentences." ;
        rdfs:isDefinedBy  <http://www.lexinfo.net/ontology/2.0/lexinfo> ;
        rdfs:label        "punctuation" ;
        dc:creator        "Francopoulo, Gil" ;
        dcr:datcat        <http://www.isocat.org/datcat/DC-1372> ;
        owl:versionInfo   "1:0" .

lexinfo:archaicForm  a    owl:NamedIndividual , lexinfo:TemporalQualifier , owl:Thing ;
        rdfs:comment      "A term or lexeme no longer in ordinary use, though retained for special purposes." ;
        rdfs:isDefinedBy  <http://www.lexinfo.net/ontology/2.0/lexinfo> ;
        rdfs:label        "archaic form" ;
        dc:creator        "Wright, Sue Ellen" ;
        dcr:datcat        <http://www.isocat.org/datcat/DC-504> ;
        owl:versionInfo   "1:0" .

lexinfo:temporalQualifier
        a                   owl:ObjectProperty ;
        rdfs:comment        "An attribution of a term or lexeme with respect to its use over time." ;
        rdfs:isDefinedBy    <http://www.lexinfo.net/ontology/2.0/lexinfo> ;
        rdfs:label          "temporal qualifier" ;
        rdfs:range          lexinfo:TemporalQualifier ;
        rdfs:subPropertyOf  lemon:context ;
        dc:creator          "Wright, Sue Ellen" ;
        dcr:datcat          <http://www.isocat.org/datcat/DC-503> ;
        owl:versionInfo     "1:0" .

lexinfo:PartOfSpeech  a   owl:Class ;
        rdfs:isDefinedBy  <http://www.lexinfo.net/ontology/2.0/lexinfo> ;
        rdfs:subClassOf   lexinfo:MorphosyntacticProperty .

lexinfo:PrepositionalFrame
        a                    owl:Class ;
        rdfs:comment         "Abstract frame for words that take a prepositional phrase as an argument"@en ;
        rdfs:isDefinedBy     <http://www.lexinfo.net/ontology/2.0/lexinfo> ;
        rdfs:subClassOf      lemon:Frame ;
        owl:equivalentClass  [ a                   owl:Restriction ;
                               owl:minCardinality  "1"^^xsd:nonNegativeInteger ;
                               owl:onProperty      lexinfo:prepositionalAdjunct
                             ] .

lexinfo:adjective-na  a           lexinfo:AdjectivePOS , owl:NamedIndividual ;
        rdfs:comment              "Denominal adjectives in Japanese formed from a noun plus the particle 'na'"@en ;
        lexinfo:languageSpecific  "ja" .

lexinfo:diminutiveNoun
        a                 lexinfo:NounPOS , owl:NamedIndividual , owl:Thing , lexinfo:PartOfSpeech ;
        rdfs:comment      "diminutive noun" ;
        rdfs:isDefinedBy  <http://www.lexinfo.net/ontology/2.0/lexinfo> ;
        rdfs:label        "diminutive noun" ;
        dc:creator        "Francopoulo, Gil" ;
        dcr:datcat        <http://www.isocat.org/datcat/DC-2225> ;
        owl:versionInfo   "1:0" .

lexinfo:definiteness  a     owl:ObjectProperty ;
        rdfs:comment        "Property about the possiblity to identify an entity." ;
        rdfs:isDefinedBy    <http://www.lexinfo.net/ontology/2.0/lexinfo> ;
        rdfs:label          "definiteness" ;
        rdfs:range          lexinfo:Definiteness ;
        rdfs:subPropertyOf  lexinfo:morphosyntacticProperty ;
        dc:creator          "Francopoulo, Gil" ;
        dcr:datcat          <http://www.isocat.org/datcat/DC-1926> ;
        owl:versionInfo     "1:0" .

lexinfo:NumeralPOS  a     owl:Class ;
        rdfs:isDefinedBy  <http://www.lexinfo.net/ontology/2.0/lexinfo> ;
        rdfs:subClassOf   lexinfo:PartOfSpeech .

lexinfo:aditiveCase  a    owl:NamedIndividual , lexinfo:Case , owl:Thing ;
        rdfs:comment      "Case expressing &quot;to&quot; in Basque studies." ;
        rdfs:isDefinedBy  <http://www.lexinfo.net/ontology/2.0/lexinfo> ;
        rdfs:label        "aditive case" ;
        dc:creator        "Francopoulo, Gil" ;
        dcr:datcat        <http://www.isocat.org/datcat/DC-1229> ;
        owl:versionInfo   "1:0" .

lexinfo:Adposition  a        owl:Class ;
        rdfs:isDefinedBy     <http://www.lexinfo.net/ontology/2.0/lexinfo> ;
        rdfs:subClassOf      lemon:Word ;
        owl:equivalentClass  [ a                   owl:Restriction ;
                               owl:onProperty      lexinfo:partOfSpeech ;
                               owl:someValuesFrom  lexinfo:AdpositionPOS
                             ] .

lexinfo:Definiteness  a   owl:Class ;
        rdfs:isDefinedBy  <http://www.lexinfo.net/ontology/2.0/lexinfo> ;
        rdfs:subClassOf   lexinfo:MorphosyntacticProperty .

lexinfo:formPersonVariant
        a                   owl:ObjectProperty ;
        rdfs:isDefinedBy    <http://www.lexinfo.net/ontology/2.0/lexinfo> ;
        rdfs:subPropertyOf  lemon:formVariant .

lexinfo:preposition  a    owl:NamedIndividual , owl:Thing , lexinfo:AdpositionPOS , lexinfo:PartOfSpeech ;
        rdfs:comment      "Adposition placed at the beginning of a noun phrase." ;
        rdfs:isDefinedBy  <http://www.lexinfo.net/ontology/2.0/lexinfo> ;
        rdfs:label        "preposition" ;
        dc:creator        "Francopoulo, Gil" ;
        dcr:datcat        <http://www.isocat.org/datcat/DC-1366> ;
        owl:versionInfo   "1:0" .

lexinfo:homograph  a        owl:ObjectProperty ;
        rdfs:comment        "A word that is spelled like another, but that has a different pronunciation, meaning, and/or origin." , "Word that is written like another, but that has a different pronunciation, meaning, and/or origin." ;
        rdfs:isDefinedBy    <http://www.lexinfo.net/ontology/2.0/lexinfo> ;
        rdfs:label          "homograph" ;
        rdfs:subPropertyOf  lemon:lexicalVariant ;
        dc:creator          "Wright, Sue Ellen" , "Francopoulo, Gil" ;
        dcr:datcat          <http://www.isocat.org/datcat/DC-1300> , <http://www.isocat.org/datcat/DC-260> ;
        owl:versionInfo     "1:0" .

lexinfo:conditional  a    owl:NamedIndividual , lexinfo:VerbFormMood , owl:Thing ;
        rdfs:comment      "A conditional relation is a logical relation in which the illocutionary act employing one of a pair of propositions is expressed or implied to be true or in force if the other proposition is true." ;
        rdfs:isDefinedBy  <http://www.lexinfo.net/ontology/2.0/lexinfo> ;
        rdfs:label        "conditional" ;
        dc:creator        "Francopoulo, Gil" ;
        dcr:datcat        <http://www.isocat.org/datcat/DC-1258> ;
        owl:versionInfo   "1:0" .

lexinfo:multiplicativeNumeral
        a                 owl:Thing , owl:NamedIndividual , lexinfo:PartOfSpeech , lexinfo:NumeralPOS ;
        rdfs:comment      "A word that expresses the number of times something happened." ;
        rdfs:isDefinedBy  <http://www.lexinfo.net/ontology/2.0/lexinfo> ;
        rdfs:label        "multiplicative numeral" ;
        dc:creator        "Zeman, Dan" ;
        dcr:datcat        <http://www.isocat.org/datcat/DC-3020> ;
        owl:versionInfo   "1:0" .

lexinfo:reflexivePossessivePronoun
        a                 owl:NamedIndividual , lexinfo:PronounPOS , owl:Thing , lexinfo:PartOfSpeech ;
        rdfs:comment      "A possessive pronoun that refers to the subject as the possessor." ;
        rdfs:isDefinedBy  <http://www.lexinfo.net/ontology/2.0/lexinfo> ;
        rdfs:label        "reflexive possessive pronoun" ;
        dc:creator        "Zeman, Dan" ;
        dcr:datcat        <http://www.isocat.org/datcat/DC-3001> ;
        owl:versionInfo   "1:0" .

lexinfo:directObject  a     owl:ObjectProperty ;
        rdfs:comment        "relation between a phrase and a verb, in which the relation is central to the verb" ;
        rdfs:isDefinedBy    <http://www.lexinfo.net/ontology/2.0/lexinfo> ;
        rdfs:label          "direct object" ;
        rdfs:range          lexinfo:DirectObject ;
        rdfs:subPropertyOf  lexinfo:object ;
        dcr:datcat          <http://www.isocat.org/datacat/DC-2263> .

lexinfo:superessiveCase
        a                 owl:NamedIndividual , lexinfo:Case , owl:Thing ;
        rdfs:comment      "Case indicating location on top of something or on the surface of something." ;
        rdfs:isDefinedBy  <http://www.lexinfo.net/ontology/2.0/lexinfo> ;
        rdfs:label        "superessive case" ;
        dc:creator        "Francopoulo, Gil" ;
        dcr:datcat        <http://www.isocat.org/datcat/DC-1396> ;
        owl:versionInfo   "1:0" .

lexinfo:secondPersonForm
        a                   owl:ObjectProperty ;
        rdfs:isDefinedBy    <http://www.lexinfo.net/ontology/2.0/lexinfo> ;
        rdfs:subPropertyOf  lexinfo:formPersonVariant .

lexinfo:finiteness  a       owl:ObjectProperty ;
        rdfs:comment        "Property referring to finite and non-finite status of a verbal form." ;
        rdfs:isDefinedBy    <http://www.lexinfo.net/ontology/2.0/lexinfo> ;
        rdfs:label          "finitness" ;
        rdfs:range          lexinfo:Finiteness ;
        rdfs:subPropertyOf  lexinfo:morphosyntacticProperty ;
        dc:creator          "Francopoulo, Gil" ;
        dcr:datcat          <http://www.isocat.org/datcat/DC-1893> ;
        owl:versionInfo     "1:0" .

lexinfo:instrumentalCase
        a                 owl:NamedIndividual , lexinfo:Case , owl:Thing ;
        rdfs:comment      "Case indicating that the referent of the noun it marks is the means of the accomplishment of the action expressed by the clause." ;
        rdfs:isDefinedBy  <http://www.lexinfo.net/ontology/2.0/lexinfo> ;
        rdfs:label        "instrumental case" ;
        dc:creator        "Francopoulo, Gil" ;
        dcr:datcat        <http://www.isocat.org/datcat/DC-1316> ;
        owl:versionInfo   "1:0" .

lexinfo:SubjunctiveClause
        a                 owl:Class ;
        rdfs:comment      "A subclause that is in the subjunctive mood"@en ;
        rdfs:isDefinedBy  <http://www.lexinfo.net/ontology/2.0/lexinfo> ;
        rdfs:subClassOf   lexinfo:ClausalArgument .

lexinfo:mood  a             owl:ObjectProperty ;
        rdfs:comment        "In TEI: contains information about the grammatical mood of verbs (e.g. indicative, subjunctive, imperative)." ;
        rdfs:isDefinedBy    <http://www.lexinfo.net/ontology/2.0/lexinfo> ;
        rdfs:label          "mood" ;
        rdfs:range          lexinfo:Mood ;
        rdfs:subPropertyOf  lexinfo:morphosyntacticProperty ;
        dc:creator          "Wright, Sue Ellen" ;
        dcr:datcat          <http://www.isocat.org/datcat/DC-366> ;
        owl:versionInfo     "1:0" .

lexinfo:indefiniteArticle
        a                 owl:Thing , lexinfo:PartOfSpeech , lexinfo:DeterminerPOS , owl:NamedIndividual ;
        rdfs:comment      "Article not capable of expressing identification." ;
        rdfs:isDefinedBy  <http://www.lexinfo.net/ontology/2.0/lexinfo> ;
        rdfs:label        "indefinite article" ;
        dc:creator        "Francopoulo, Gil" ;
        dcr:datcat        <http://www.isocat.org/datcat/DC-1308> ;
        owl:versionInfo   "1:0" .

lexinfo:DirectObject  a   owl:Class ;
        rdfs:isDefinedBy  <http://www.lexinfo.net/ontology/2.0/lexinfo> ;
        rdfs:subClassOf   lexinfo:Object .

lexinfo:relativeParticle
        a                 lexinfo:ParticlePOS , owl:NamedIndividual , lexinfo:PartOfSpeech , owl:Thing ;
        rdfs:comment      "relative particle" ;
        rdfs:isDefinedBy  <http://www.lexinfo.net/ontology/2.0/lexinfo> ;
        rdfs:label        "relative particle" ;
        dc:creator        "Francopoulo, Gil" ;
        dcr:datcat        <http://www.isocat.org/datcat/DC-2229> ;
        owl:versionInfo   "1:0" .

lexinfo:partitiveArticle
        a                 lexinfo:PartOfSpeech , lexinfo:ArticlePOS , owl:Thing , owl:NamedIndividual ;
        rdfs:comment      "Article expressing a part or quantity." ;
        rdfs:isDefinedBy  <http://www.lexinfo.net/ontology/2.0/lexinfo> ;
        rdfs:label        "partitive article" ;
        dc:creator        "Francopoulo, Gil" ;
        dcr:datcat        <http://www.isocat.org/datcat/DC-1898> ;
        owl:versionInfo   "1:0" .

lexinfo:pertainsTo  a       owl:ObjectProperty ;
        rdfs:isDefinedBy    <http://www.lexinfo.net/ontology/2.0/lexinfo> ;
        rdfs:subPropertyOf  lemon:senseRelation .

lemon:SenseContext  a  owl:Class .

lexinfo:InterrogativeClause
        a                 owl:Class ;
        rdfs:comment      "A subclause that begins interrogative construction (\"wh\"-word in English)"@en ;
        rdfs:isDefinedBy  <http://www.lexinfo.net/ontology/2.0/lexinfo> ;
        rdfs:subClassOf   lexinfo:ClausalArgument .

lexinfo:TransitiveDeclarativeFrame
        a                    owl:Class ;
        rdfs:isDefinedBy     <http://www.lexinfo.net/ontology/2.0/lexinfo> ;
        rdfs:subClassOf      lexinfo:DeclarativeFrame ;
        lexinfo:example      "he CONVINCED her [that she should go]"@en ;
        owl:equivalentClass  [ a                   owl:Class ;
                               owl:intersectionOf  ( lexinfo:DeclarativeFrame lexinfo:TransitiveFrame )
                             ] .

lexinfo:trial  a          owl:NamedIndividual , lexinfo:Number , owl:Thing ;
        rdfs:comment      "Grammatical number referring to 'three things', as opposed to 'singular' and 'plural'." ;
        rdfs:isDefinedBy  <http://www.lexinfo.net/ontology/2.0/lexinfo> ;
        rdfs:label        "trial" ;
        dc:creator        "Francopoulo, Gil" ;
        dcr:datcat        <http://www.isocat.org/datcat/DC-1407> ;
        owl:versionInfo   "1:0" .

lexinfo:Aspect  a         owl:Class ;
        rdfs:isDefinedBy  <http://www.lexinfo.net/ontology/2.0/lexinfo> ;
        rdfs:subClassOf   lexinfo:MorphosyntacticProperty .

lexinfo:questionMark  a   lexinfo:SymbolPOS , lexinfo:PartOfSpeech , owl:NamedIndividual , owl:Thing ;
        rdfs:comment      "Sign used to express a question." ;
        rdfs:isDefinedBy  <http://www.lexinfo.net/ontology/2.0/lexinfo> ;
        rdfs:label        "question mark" ;
        dc:creator        "Francopoulo, Gil" ;
        dcr:datcat        <http://www.isocat.org/datcat/DC-1444> ;
        owl:versionInfo   "1:0" .

lexinfo:generalizationWord
        a                 owl:NamedIndividual , lexinfo:PartOfSpeech , owl:Thing ;
        rdfs:comment      "A word that does not carry its own meaning but generalizes the meaning of a neighboring word, adding the &quot;etc.&quot; sense." ;
        rdfs:isDefinedBy  <http://www.lexinfo.net/ontology/2.0/lexinfo> ;
        rdfs:label        "generalization word" ;
        dc:creator        "Zeman, Dan" ;
        dcr:datcat        <http://www.isocat.org/datcat/DC-3033> ;
        owl:versionInfo   "1:0" .

lexinfo:normativeAuthorization
        a                   owl:ObjectProperty ;
        rdfs:comment        "A term status qualifier assigned by an authoritative body, such as a standards body or a governmental entity with a regulatory function." ;
        rdfs:isDefinedBy    <http://www.lexinfo.net/ontology/2.0/lexinfo> ;
        rdfs:label          "normative authorization" ;
        rdfs:range          lexinfo:NormativeAuthorization ;
        rdfs:subPropertyOf  lemon:context ;
        dc:creator          "Wright, Sue Ellen" ;
        dcr:datcat          <http://www.isocat.org/datcat/DC-374> ;
        owl:versionInfo     "1:0" .

lexinfo:NominalComplementFrame
        a                    owl:Class ;
        rdfs:isDefinedBy     <http://www.lexinfo.net/ontology/2.0/lexinfo> ;
        rdfs:subClassOf      lexinfo:VerbFrame ;
        owl:equivalentClass  [ a                   owl:Class ;
                               owl:intersectionOf  ( lexinfo:VerbFrame [ a                   owl:Restriction ;
                                                                         owl:minCardinality  "1"^^xsd:nonNegativeInteger ;
                                                                         owl:onProperty      lexinfo:predicativeNominative
                                                                       ] )
                             ] .

lexinfo:noun  a           lexinfo:PartOfSpeech , owl:Thing , owl:NamedIndividual , lexinfo:NounPOS ;
        rdfs:comment      "Part of speech used to express the name of a person, place, action or thing." ;
        rdfs:isDefinedBy  <http://www.lexinfo.net/ontology/2.0/lexinfo> ;
        rdfs:label        "noun" ;
        dc:creator        "Francopoulo, Gil" ;
        dcr:datcat        <http://www.isocat.org/datcat/DC-1333> ;
        owl:versionInfo   "1:0" .

lexinfo:ReflexiveTransitivePPFrame
        a                    owl:Class ;
        rdfs:isDefinedBy     <http://www.lexinfo.net/ontology/2.0/lexinfo> ;
        rdfs:subClassOf      lexinfo:ReflexiveFrame ;
        lexinfo:example      "elle se APPROCHE DE la gare"@fr , "ich ERRINERE mich AN seinen vater"@de ;
        owl:equivalentClass  [ a                   owl:Class ;
                               owl:intersectionOf  ( lexinfo:ReflexiveFrame lexinfo:TransitivePPFrame )
                             ] .

lexinfo:formTenseVariant
        a                   owl:ObjectProperty ;
        rdfs:isDefinedBy    <http://www.lexinfo.net/ontology/2.0/lexinfo> ;
        rdfs:subPropertyOf  lemon:formVariant .

lexinfo:suffix  a         owl:NamedIndividual , lexinfo:TermElement , owl:Thing ;
        rdfs:isDefinedBy  <http://www.lexinfo.net/ontology/2.0/lexinfo> .

lexinfo:feminine  a       lexinfo:Gender , owl:NamedIndividual , owl:Thing ;
        rdfs:comment      "Of, relating to, or constituting the gender that ordinarily includes most words or grammatical forms referring to females." ;
        rdfs:isDefinedBy  <http://www.lexinfo.net/ontology/2.0/lexinfo> ;
        rdfs:label        "feminine" ;
        dc:creator        "Francopoulo, Gil" , "Wright, Sue Ellen" ;
        dcr:datcat        <http://www.isocat.org/datcat/DC-1880> , <http://www.isocat.org/datcat/DC-247> ;
        owl:versionInfo   "1:0" .

lexinfo:negative  a         owl:ObjectProperty ;
        rdfs:comment        "denotes the negation or the absence" ;
        rdfs:isDefinedBy    <http://www.lexinfo.net/ontology/2.0/lexinfo> ;
        rdfs:label          "negative" ;
        rdfs:range          lexinfo:Negative ;
        rdfs:subPropertyOf  lexinfo:morphosyntacticProperty ;
        dc:creator          "Francopoulo, Gil" ;
        dcr:datcat          <http://www.isocat.org/datcat/DC-1839> ;
        owl:versionInfo     "1:0" .

lexinfo:DitransitiveFrame_To
        a                         owl:Class ;
        rdfs:isDefinedBy          <http://www.lexinfo.net/ontology/2.0/lexinfo> ;
        rdfs:subClassOf           lexinfo:DitransitiveFrame ;
        lexinfo:example           "he GAVE his mother a present\nhe GAVE a present TO his mother"@en ;
        lexinfo:languageSpecific  "en" .

lexinfo:FusedPrepositionPOS
        a                 owl:Class ;
        rdfs:isDefinedBy  <http://www.lexinfo.net/ontology/2.0/lexinfo> ;
        rdfs:subClassOf   lexinfo:PartOfSpeech .

lexinfo:AdjectivePostPositiveFrame
        a                    owl:Class ;
        rdfs:isDefinedBy     <http://www.lexinfo.net/ontology/2.0/lexinfo> ;
        rdfs:subClassOf      lexinfo:AdjectiveFrame ;
        lexinfo:example      "that is something INTERESTING"@en ;
        owl:equivalentClass  [ a                   owl:Class ;
                               owl:intersectionOf  ( lexinfo:AdjectiveFrame [ a                owl:Restriction ;
                                                                              owl:cardinality  "1"^^xsd:nonNegativeInteger ;
                                                                              owl:onProperty   lexinfo:copulativeArg
                                                                            ] [ a                owl:Restriction ;
                                                                                owl:cardinality  "1"^^xsd:nonNegativeInteger ;
                                                                                owl:onProperty   lexinfo:postPositiveArg
                                                                              ] )
                             ] .

lexinfo:ReferentType  a   owl:Class ;
        rdfs:isDefinedBy  <http://www.lexinfo.net/ontology/2.0/lexinfo> ;
        rdfs:subClassOf   lexinfo:MorphosyntacticProperty .

lexinfo:AccusativePostPositiveArgument
        a                    owl:Class ;
        rdfs:isDefinedBy     <http://www.lexinfo.net/ontology/2.0/lexinfo> ;
        rdfs:subClassOf      lexinfo:PostPositiveArgument ;
        owl:equivalentClass  [ a                   owl:Class ;
                               owl:intersectionOf  ( lexinfo:PostPositiveArgument [ a               owl:Restriction ;
                                                                                    owl:hasValue    lexinfo:accusativeCase ;
                                                                                    owl:onProperty  lemon:marker
                                                                                  ] )
                             ] .

lexinfo:interrogativeInfinitiveClause
        a                   owl:ObjectProperty ;
        rdfs:isDefinedBy    <http://www.lexinfo.net/ontology/2.0/lexinfo> ;
        rdfs:subPropertyOf  lexinfo:clausalArg .

lexinfo:wordElement  a    owl:NamedIndividual , lexinfo:TermElement , owl:Thing ;
        rdfs:comment      "Any lexeme element in a compound lexical unit that is itself a word." ;
        rdfs:isDefinedBy  <http://www.lexinfo.net/ontology/2.0/lexinfo> ;
        rdfs:label        "wordElement" ;
        dc:creator        "Wright, Sue Ellen" ;
        dcr:datcat        <http://www.isocat.org/datcat/DC-298> ;
        owl:versionInfo   "1:0" .

lexinfo:perfective  a     owl:NamedIndividual , lexinfo:Aspect , owl:Thing ;
        rdfs:comment      "Perfective aspect is an aspect that expresses a temporal view of an event or state as a simple whole, apart from the consideration of the internal structure of the time in which it occurs." ;
        rdfs:isDefinedBy  <http://www.lexinfo.net/ontology/2.0/lexinfo> ;
        rdfs:label        "perfective" ;
        dc:creator        "Francopoulo, Gil" ;
        dcr:datcat        <http://www.isocat.org/datcat/DC-1352> ;
        owl:versionInfo   "1:0" .

lexinfo:existentialPronoun
        a                 owl:NamedIndividual , owl:Thing , lexinfo:PronounPOS , lexinfo:PartOfSpeech ;
        rdfs:comment      "pronoun that indicates the existence of something or someone" ;
        rdfs:isDefinedBy  <http://www.lexinfo.net/ontology/2.0/lexinfo> ;
        rdfs:label        "existential pronoun" ;
        dc:creator        "Francopoulo, Gil" ;
        dcr:datcat        <http://www.isocat.org/datcat/DC-3012> ;
        owl:versionInfo   "1:0" .

lexinfo:animate  a        owl:Thing , owl:NamedIndividual , lexinfo:Animacy ;
        rdfs:comment      "Perceived as alive." ;
        rdfs:isDefinedBy  <http://www.lexinfo.net/ontology/2.0/lexinfo> ;
        rdfs:label        "animate" ;
        dc:creator        "Wright, Sue Ellen" , "Francopoulo, Gil" ;
        dcr:datcat        <http://www.isocat.org/datcat/DC-79> , <http://www.isocat.org/datcat/DC-1911> ;
        owl:versionInfo   "1:0" .

lexinfo:TransitiveInfinitiveSCFrame
        a                    owl:Class ;
        rdfs:isDefinedBy     <http://www.lexinfo.net/ontology/2.0/lexinfo> ;
        rdfs:subClassOf      lexinfo:InfinitiveFrame ;
        lexinfo:example      "john PROMISED mary [to resign]"@en ;
        owl:equivalentClass  [ a                   owl:Class ;
                               owl:intersectionOf  ( lexinfo:InfinitiveFrame lexinfo:SubjectControl lexinfo:TransitiveFrame )
                             ] .

lexinfo:interrogativeClause
        a                   owl:ObjectProperty ;
        rdfs:isDefinedBy    <http://www.lexinfo.net/ontology/2.0/lexinfo> ;
        rdfs:subPropertyOf  lexinfo:clausalArg .

lexinfo:IntransitiveSententialFrame
        a                    owl:Class ;
        rdfs:isDefinedBy     <http://www.lexinfo.net/ontology/2.0/lexinfo> ;
        rdfs:subClassOf      lexinfo:SententialFrame ;
        lexinfo:example      "they THOUGHT he was always late"@en ;
        owl:equivalentClass  [ a                   owl:Class ;
                               owl:intersectionOf  ( lexinfo:IntransitiveFrame lexinfo:SententialFrame )
                             ] .

lexinfo:Tense  a          owl:Class ;
        rdfs:isDefinedBy  <http://www.lexinfo.net/ontology/2.0/lexinfo> ;
        rdfs:subClassOf   lexinfo:MorphosyntacticProperty .

lexinfo:benchLevelRegister
        a                 owl:NamedIndividual , lexinfo:Register , owl:Thing ;
        rdfs:comment      "Register of terms used in applications-oriented as opposed to theoretical or academic levels of language." , "The register of terms used in applications-oriented as opposed to theoretical or academic levels of language." ;
        rdfs:isDefinedBy  <http://www.lexinfo.net/ontology/2.0/lexinfo> ;
        rdfs:label        "bench-level register" ;
        dc:creator        "Francopoulo, Gil" , "Wright, Sue Ellen" ;
        dcr:datcat        <http://www.isocat.org/datcat/DC-1989> , <http://www.isocat.org/datcat/DC-427> ;
        owl:versionInfo   "1:0" .

lexinfo:inessiveCase  a   owl:NamedIndividual , lexinfo:Case , owl:Thing ;
        rdfs:comment      "Case which expresses the meaning of location or position within a place." ;
        rdfs:isDefinedBy  <http://www.lexinfo.net/ontology/2.0/lexinfo> ;
        rdfs:label        "inessive case" ;
        dc:creator        "Francopoulo, Gil" ;
        dcr:datcat        <http://www.isocat.org/datcat/DC-1311> ;
        owl:versionInfo   "1:0" .

lexinfo:slash  a          lexinfo:PartOfSpeech , owl:Thing , owl:NamedIndividual , lexinfo:SymbolPOS ;
        rdfs:comment      "The punctuation sign /" ;
        rdfs:isDefinedBy  <http://www.lexinfo.net/ontology/2.0/lexinfo> ;
        rdfs:label        "slash" ;
        dc:creator        "Francopoulo, Gil" ;
        dcr:datcat        <http://www.isocat.org/datcat/DC-1437> ;
        owl:versionInfo   "1:0" .

lexinfo:relatedTerm  a      owl:ObjectProperty ;
        rdfs:comment        "A term connected to another term by a coordinate or associative relation." ;
        rdfs:isDefinedBy    <http://www.lexinfo.net/ontology/2.0/lexinfo> ;
        rdfs:label          "relatedTerm" ;
        rdfs:subPropertyOf  lemon:senseRelation ;
        dc:creator          "Wright, Sue Ellen" ;
        dcr:datcat          <http://www.isocat.org/datcat/DC-438> ;
        owl:versionInfo     "1:0" .

lexinfo:NounPOS  a        owl:Class ;
        rdfs:isDefinedBy  <http://www.lexinfo.net/ontology/2.0/lexinfo> ;
        rdfs:subClassOf   lexinfo:PartOfSpeech .

lexinfo:ReflexiveDativeTransitiveFrame
        a                    owl:Class ;
        rdfs:comment         "ist diese frame echt?"@de ;
        rdfs:isDefinedBy     <http://www.lexinfo.net/ontology/2.0/lexinfo> ;
        rdfs:subClassOf      lexinfo:ReflexiveFrame ;
        lexinfo:example      "ich TUE mir WEH"@de ;
        owl:equivalentClass  [ a                   owl:Class ;
                               owl:intersectionOf  ( lexinfo:DativeTransitiveFrame lexinfo:ReflexiveFrame )
                             ] .

lexinfo:adverbialPronoun
        a                 lexinfo:PartOfSpeech , owl:NamedIndividual , owl:Thing , lexinfo:PronounPOS ;
        rdfs:comment      "()" ;
        rdfs:isDefinedBy  <http://www.lexinfo.net/ontology/2.0/lexinfo> ;
        rdfs:label        "adverbial pronoun" ;
        dc:creator        "Francopoulo, Gil" ;
        dcr:datcat        <http://www.isocat.org/datcat/DC-3011> ;
        owl:versionInfo   "1:0" .

lexinfo:SubjectControl
        a                 owl:Class ;
        rdfs:comment      "Indicates the subject of the main clause is the (omitted) subject of the subclause"@en ;
        rdfs:isDefinedBy  <http://www.lexinfo.net/ontology/2.0/lexinfo> ;
        rdfs:subClassOf   lexinfo:Control .

lemon:context  a  owl:ObjectProperty .

lexinfo:AdjectivalComplementFrame
        a                    owl:Class ;
        rdfs:isDefinedBy     <http://www.lexinfo.net/ontology/2.0/lexinfo> ;
        rdfs:subClassOf      lexinfo:VerbFrame ;
        owl:equivalentClass  [ a                   owl:Class ;
                               owl:intersectionOf  ( lexinfo:VerbFrame [ a                   owl:Restriction ;
                                                                         owl:minCardinality  "1"^^xsd:nonNegativeInteger ;
                                                                         owl:onProperty      lexinfo:predicativeAdjective
                                                                       ] )
                             ] .

lexinfo:formNumberVariant
        a                   owl:ObjectProperty ;
        rdfs:isDefinedBy    <http://www.lexinfo.net/ontology/2.0/lexinfo> ;
        rdfs:subPropertyOf  lemon:formVariant .

lexinfo:objectComplement
        a                   owl:ObjectProperty ;
        rdfs:isDefinedBy    <http://www.lexinfo.net/ontology/2.0/lexinfo> ;
        rdfs:range          lexinfo:ObjectComplement ;
        rdfs:subPropertyOf  lexinfo:complement .

lexinfo:NounPredicateFrame
        a                    owl:Class ;
        rdfs:isDefinedBy     <http://www.lexinfo.net/ontology/2.0/lexinfo> ;
        rdfs:subClassOf      lexinfo:NounFrame ;
        lexinfo:example      "he is a MAN"@en ;
        owl:equivalentClass  [ a                   owl:Class ;
                               owl:intersectionOf  ( lexinfo:NounFrame [ a                   owl:Restriction ;
                                                                         owl:minCardinality  "1"^^xsd:nonNegativeInteger ;
                                                                         owl:onProperty      lexinfo:copulativeArg
                                                                       ] )
                             ] .

lexinfo:deprecatedTerm
        a                 owl:NamedIndividual , lexinfo:NormativeAuthorization , owl:Thing ;
        rdfs:comment      "A term rated according to the scale of a term acceptability rating as undesired." ;
        rdfs:isDefinedBy  <http://www.lexinfo.net/ontology/2.0/lexinfo> ;
        rdfs:label        "deprecated term" ;
        dc:creator        "Wright, Sue Ellen" ;
        dcr:datcat        <http://www.isocat.org/datcat/DC-378> ;
        owl:versionInfo   "1:0" .

lemon:RaisableArgument
        a                owl:Class ;
        rdfs:subClassOf  lemon:Argument .

lexinfo:lightVerb  a      lexinfo:VerbPOS , owl:Thing , owl:NamedIndividual , lexinfo:PartOfSpeech ;
        rdfs:comment      "verb participating in a complex predication that has little semantic content of its own." ;
        rdfs:isDefinedBy  <http://www.lexinfo.net/ontology/2.0/lexinfo> ;
        rdfs:label        "light verb" ;
        dc:creator        "Francopoulo, Gil" ;
        dcr:datcat        <http://www.isocat.org/datcat/DC-3003> ;
        owl:versionInfo   "1:0" .

lexinfo:interrogativeDeterminer
        a                 owl:NamedIndividual , owl:Thing , lexinfo:DeterminerPOS , lexinfo:PartOfSpeech ;
        rdfs:comment      "Determiner used to express a question." ;
        rdfs:isDefinedBy  <http://www.lexinfo.net/ontology/2.0/lexinfo> ;
        rdfs:label        "interrogative determiner" ;
        dc:creator        "Francopoulo, Gil" ;
        dcr:datcat        <http://www.isocat.org/datcat/DC-1320> ;
        owl:versionInfo   "1:0" .

lexinfo:entryTerm  a      owl:NamedIndividual , lexinfo:TermType , owl:Thing ;
        rdfs:comment      "A term that heads a terminological entry." ;
        rdfs:isDefinedBy  <http://www.lexinfo.net/ontology/2.0/lexinfo> ;
        rdfs:label        "entry term" ;
        dc:creator        "Wright, Sue Ellen" ;
        dcr:datcat        <http://www.isocat.org/datcat/DC-316> ;
        owl:versionInfo   "1:0" .

lexinfo:PrepositionalPhraseFrame
        a                    owl:Class ;
        rdfs:isDefinedBy     <http://www.lexinfo.net/ontology/2.0/lexinfo> ;
        rdfs:subClassOf      lexinfo:PrepositionFrame ;
        lexinfo:example      "he is IN london"@en ;
        owl:equivalentClass  [ a                   owl:Class ;
                               owl:intersectionOf  ( lexinfo:PrepositionFrame [ a                            owl:Restriction ;
                                                                                owl:minQualifiedCardinality  "1"^^xsd:nonNegativeInteger ;
                                                                                owl:onClass                  lexinfo:PrepositionalAdjunct ;
                                                                                owl:onProperty               lexinfo:complement
                                                                              ] [ a                   owl:Restriction ;
                                                                                  owl:minCardinality  "1"^^xsd:nonNegativeInteger ;
                                                                                  owl:onProperty      lexinfo:copulativeSubject
                                                                                ] )
                             ] .

lexinfo:circumposition
        a                 owl:NamedIndividual , owl:Thing , lexinfo:AdpositionPOS , lexinfo:PartOfSpeech ;
        rdfs:comment      "Adposition which consists of two parts which are positioned ahead and after the adpositional foci." ;
        rdfs:isDefinedBy  <http://www.lexinfo.net/ontology/2.0/lexinfo> ;
        rdfs:label        "circumposition" ;
        dc:creator        "Francopoulo, Gil" ;
        dcr:datcat        <http://www.isocat.org/datcat/DC-1906> ;
        owl:versionInfo   "1:0" .

lexinfo:quasiEquivalent
        a                   owl:ObjectProperty ;
        rdfs:isDefinedBy    <http://www.lexinfo.net/ontology/2.0/lexinfo> ;
        rdfs:subPropertyOf  lemon:senseRelation ;
        dcr:datcat          <http://www.isocat.org/datcat/DC-177> .

lexinfo:abbreviatedForm
        a                 lexinfo:AbbreviatedForm , lexinfo:TermType , owl:NamedIndividual , owl:Thing ;
        rdfs:comment      "A term or lexeme resulting from the omission of any part of the full term or lexeme while designating the same concept." ;
        rdfs:isDefinedBy  <http://www.lexinfo.net/ontology/2.0/lexinfo> ;
        rdfs:label        "abbreviated form" ;
        dc:creator        "Wright, Sue Ellen" ;
        dcr:datcat        <http://www.isocat.org/datcat/DC-329> ;
        owl:versionInfo   "1:0" .

lexinfo:Gerund  a         owl:Class ;
        rdfs:comment      "A clause, whose head is a non-finite verb form, which is used in place of an argument. In English these use the \"-ing\" suffix"@en ;
        rdfs:isDefinedBy  <http://www.lexinfo.net/ontology/2.0/lexinfo> ;
        rdfs:subClassOf   lexinfo:ClausalArgument .

lexinfo:interrogativeOrdinalNumeral
        a                 lexinfo:NumeralPOS , lexinfo:PartOfSpeech , owl:NamedIndividual , owl:Thing ;
        rdfs:comment      "An interrogative/relative word used to ask about numeric ranking." ;
        rdfs:isDefinedBy  <http://www.lexinfo.net/ontology/2.0/lexinfo> ;
        rdfs:label        "interrogative ordinal numeral" ;
        dc:creator        "Zeman, Dan" ;
        dcr:datcat        <http://www.isocat.org/datcat/DC-3019> ;
        owl:versionInfo   "1:0" .

lexinfo:strongPersonalPronoun
        a                 lexinfo:PronounPOS , lexinfo:PartOfSpeech , owl:Thing , owl:NamedIndividual ;
        rdfs:comment      "Personal pronoun that can occupy the position after a preposition and/or reinforce a weak personal pronoun." ;
        rdfs:isDefinedBy  <http://www.lexinfo.net/ontology/2.0/lexinfo> ;
        rdfs:label        "strong personal pronoun" ;
        dc:creator        "Francopoulo, Gil" ;
        dcr:datcat        <http://www.isocat.org/datcat/DC-1390> ;
        owl:versionInfo   "1:0" .

lexinfo:GerundACFrame
        a                    owl:Class ;
        rdfs:isDefinedBy     <http://www.lexinfo.net/ontology/2.0/lexinfo> ;
        rdfs:subClassOf      lexinfo:GerundFrame ;
        owl:equivalentClass  [ a                   owl:Class ;
                               owl:intersectionOf  ( lexinfo:ArbitraryControl lexinfo:GerundFrame )
                             ] .

lexinfo:locativeCase  a   owl:NamedIndividual , lexinfo:Case , owl:Thing ;
        rdfs:comment      "Case that indicates a final location of action or a time of the action." ;
        rdfs:isDefinedBy  <http://www.lexinfo.net/ontology/2.0/lexinfo> ;
        rdfs:label        "locative case" ;
        dc:creator        "Francopoulo, Gil" ;
        dcr:datcat        <http://www.isocat.org/datcat/DC-1326> ;
        owl:versionInfo   "1:0" .

lexinfo:comparativeAdjunct
        a                   owl:ObjectProperty ;
        rdfs:isDefinedBy    <http://www.lexinfo.net/ontology/2.0/lexinfo> ;
        rdfs:range          lexinfo:ComparativeAdjunct ;
        rdfs:subPropertyOf  lexinfo:predicativeAdjunct .

lexinfo:number  a           owl:ObjectProperty ;
        rdfs:comment        "Grammatical category for the variation in form of nouns, pronouns, and any words agreeing with them, depending on how many persons or things are referred to." , "In many languages, the grammatical distinction that indicates the number of objects referred to by the term or word." ;
        rdfs:isDefinedBy    <http://www.lexinfo.net/ontology/2.0/lexinfo> ;
        rdfs:label          "grammatical number" ;
        rdfs:range          lexinfo:Number ;
        rdfs:subPropertyOf  lexinfo:morphosyntacticProperty ;
        dc:creator          "Francopoulo, Gil" , "Wright, Sue Ellen" ;
        dcr:datcat          <http://www.isocat.org/datcat/DC-1298> , <http://www.isocat.org/datcat/DC-251> ;
        owl:versionInfo     "1:0" .

dc:creator  a   owl:AnnotationProperty .

lexinfo:Register  a       owl:Class ;
        rdfs:isDefinedBy  <http://www.lexinfo.net/ontology/2.0/lexinfo> ;
        rdfs:subClassOf   lemon:SenseContext .

lexinfo:GenitiveDitransitiveFrame
        a                    owl:Class ;
        rdfs:isDefinedBy     <http://www.lexinfo.net/ontology/2.0/lexinfo> ;
        rdfs:subClassOf      lexinfo:VerbFrame ;
        lexinfo:example      "man KLAGTE ihn des diebstahls AN"@de ;
        owl:equivalentClass  [ a                   owl:Class ;
                               owl:intersectionOf  ( lexinfo:VerbFrame [ a                owl:Restriction ;
                                                                         owl:cardinality  "1"^^xsd:nonNegativeInteger ;
                                                                         owl:onProperty   lexinfo:directObject
                                                                       ] [ a                owl:Restriction ;
                                                                           owl:cardinality  "1"^^xsd:nonNegativeInteger ;
                                                                           owl:onProperty   lexinfo:genitiveObject
                                                                         ] [ a                owl:Restriction ;
                                                                             owl:cardinality  "1"^^xsd:nonNegativeInteger ;
                                                                             owl:onProperty   lexinfo:subject
                                                                           ] )
                             ] .

lexinfo:AdjectivePOS  a   owl:Class ;
        rdfs:isDefinedBy  <http://www.lexinfo.net/ontology/2.0/lexinfo> ;
        rdfs:subClassOf   lexinfo:PartOfSpeech .

lexinfo:Gender  a         owl:Class ;
        rdfs:isDefinedBy  <http://www.lexinfo.net/ontology/2.0/lexinfo> ;
        rdfs:subClassOf   lexinfo:MorphosyntacticProperty .

lexinfo:dual  a           lexinfo:Number , owl:NamedIndividual , owl:Thing ;
        rdfs:comment      "Form used in some languages to designate two persons or things." , "The form used in some languages to designate two persons or things." ;
        rdfs:isDefinedBy  <http://www.lexinfo.net/ontology/2.0/lexinfo> ;
        rdfs:label        "dual" ;
        dc:creator        "Wright, Sue Ellen" , "Francopoulo, Gil" ;
        dcr:datcat        <http://www.isocat.org/datcat/DC-1879> , <http://www.isocat.org/datcat/DC-254> ;
        owl:versionInfo   "1:0" .

lexinfo:pluralNumberForm
        a                   owl:ObjectProperty ;
        rdfs:isDefinedBy    <http://www.lexinfo.net/ontology/2.0/lexinfo> ;
        rdfs:subPropertyOf  lexinfo:formNumberVariant .

lexinfo:modern  a         owl:NamedIndividual , lexinfo:Dating , owl:Thing ;
        rdfs:comment      "Currently in use." ;
        rdfs:isDefinedBy  <http://www.lexinfo.net/ontology/2.0/lexinfo> ;
        rdfs:label        "modern" ;
        dc:creator        "Francopoulo, Gil" ;
        dcr:datcat        <http://www.isocat.org/datcat/DC-1962> ;
        owl:versionInfo   "1:0" .

lexinfo:reflexivePersonalPronoun
        a                 owl:Thing , owl:NamedIndividual , lexinfo:PronounPOS , lexinfo:PartOfSpeech ;
        rdfs:comment      "personal pronoun which is reflexive" ;
        rdfs:isDefinedBy  <http://www.lexinfo.net/ontology/2.0/lexinfo> ;
        rdfs:label        "reflexive personal pronoun" ;
        dc:creator        "Francopoulo, Gil" ;
        dcr:datcat        <http://www.isocat.org/datcat/DC-3014> ;
        owl:versionInfo   "1:0" .

lexinfo:commonlyUsed  a   owl:NamedIndividual , lexinfo:Frequency , owl:Thing ;
        rdfs:comment      "Said of a term that appears frequently." ;
        rdfs:isDefinedBy  <http://www.lexinfo.net/ontology/2.0/lexinfo> ;
        rdfs:label        "commonly used" , "commonlyUsed" ;
        dc:creator        "Wright, Sue Ellen" , "Francopoulo, Gil" ;
        dcr:datcat        <http://www.isocat.org/datcat/DC-234> , <http://www.isocat.org/datcat/DC-1984> ;
        owl:versionInfo   "1:0" .

lexinfo:qualifierAdjective
        a                 owl:NamedIndividual , owl:Thing , lexinfo:AdjectivePOS , lexinfo:PartOfSpeech ;
        rdfs:comment      "Adjective used to qualify." ;
        rdfs:isDefinedBy  <http://www.lexinfo.net/ontology/2.0/lexinfo> ;
        rdfs:label        "qualifier adjective" ;
        dc:creator        "Francopoulo, Gil" ;
        dcr:datcat        <http://www.isocat.org/datcat/DC-1477> ;
        owl:versionInfo   "1:0" .

lemon:lexicalVariant  a  owl:ObjectProperty .

lexinfo:PrepositionFrame
        a                 owl:Class ;
        rdfs:isDefinedBy  <http://www.lexinfo.net/ontology/2.0/lexinfo> ;
        rdfs:subClassOf   lemon:Frame .

lexinfo:Case  a           owl:Class ;
        rdfs:isDefinedBy  <http://www.lexinfo.net/ontology/2.0/lexinfo> ;
        rdfs:subClassOf   lexinfo:MorphosyntacticProperty .

lexinfo:unclassifiedParticle
        a                 lexinfo:PartOfSpeech , owl:Thing , lexinfo:ParticlePOS , owl:NamedIndividual ;
        rdfs:comment      "Particle that is not covered by other sorts of particle definitions." ;
        rdfs:isDefinedBy  <http://www.lexinfo.net/ontology/2.0/lexinfo> ;
        rdfs:label        "unclassified particle" ;
        dc:creator        "Francopoulo, Gil" ;
        dcr:datcat        <http://www.isocat.org/datcat/DC-1897> ;
        owl:versionInfo   "1:0" .

lexinfo:IntransitiveAdjectivalComplementFrame
        a                    owl:Class ;
        rdfs:isDefinedBy     <http://www.lexinfo.net/ontology/2.0/lexinfo> ;
        rdfs:subClassOf      lexinfo:IntransitiveFrame ;
        lexinfo:example      "his reputation SANK low"@en ;
        owl:equivalentClass  [ a                   owl:Class ;
                               owl:intersectionOf  ( lexinfo:IntransitiveFrame [ a                   owl:Restriction ;
                                                                                 owl:minCardinality  "1"^^xsd:nonNegativeInteger ;
                                                                                 owl:onProperty      lexinfo:predicativeAdjective
                                                                               ] )
                             ] .

lexinfo:AdjectiveComparativeFrame
        a                    owl:Class ;
        rdfs:isDefinedBy     <http://www.lexinfo.net/ontology/2.0/lexinfo> ;
        rdfs:subClassOf      lexinfo:AdjectiveFrame ;
        lexinfo:example      "new york is BIGGER THAN berlin"@en ;
        owl:equivalentClass  [ a                   owl:Class ;
                               owl:intersectionOf  ( lexinfo:AdjectiveFrame [ a                owl:Restriction ;
                                                                              owl:cardinality  "1"^^xsd:nonNegativeInteger ;
                                                                              owl:onProperty   lexinfo:comparativeAdjunct
                                                                            ] [ a                owl:Restriction ;
                                                                                owl:cardinality  "1"^^xsd:nonNegativeInteger ;
                                                                                owl:onProperty   lexinfo:copulativeSubject
                                                                              ] )
                             ] .

lexinfo:copulativeSubject
        a                   owl:ObjectProperty ;
        rdfs:comment        "Indicates the subject of a copula construction. It is assumed that by using this the copula construction is not reversible e.g.,\n\nHe is happy/*happy is him"@en ;
        rdfs:isDefinedBy    <http://www.lexinfo.net/ontology/2.0/lexinfo> ;
        rdfs:subPropertyOf  lexinfo:subject , lexinfo:copulativeArg .

lexinfo:futureParticle
        a                 owl:Thing , lexinfo:PartOfSpeech , owl:NamedIndividual , lexinfo:ParticlePOS ;
        rdfs:comment      "Particle used in order to express future." ;
        rdfs:isDefinedBy  <http://www.lexinfo.net/ontology/2.0/lexinfo> ;
        rdfs:label        "future particle" ;
        dc:creator        "Francopoulo, Gil" ;
        dcr:datcat        <http://www.isocat.org/datcat/DC-1919> ;
        owl:versionInfo   "1:0" .

lexinfo:inflectionElement
        a                 owl:NamedIndividual , lexinfo:TermElement , owl:Thing ;
        rdfs:comment      "An element of language used to change the form of a word (noun, adjective) by declension, and (verbs) by conjugation." ;
        rdfs:isDefinedBy  <http://www.lexinfo.net/ontology/2.0/lexinfo> ;
        rdfs:label        "inflectionElement" ;
        dc:creator        "Wright, Sue Ellen" ;
        dcr:datcat        <http://www.isocat.org/datcat/DC-292> ;
        owl:versionInfo   "1:0" .

lexinfo:infinitiveClause
        a                   owl:ObjectProperty ;
        rdfs:isDefinedBy    <http://www.lexinfo.net/ontology/2.0/lexinfo> ;
        rdfs:subPropertyOf  lexinfo:clausalArg .

lexinfo:present  a        owl:NamedIndividual , lexinfo:Tense , owl:Thing ;
        rdfs:comment      "Verb tense that indicates action or state of being in the present." ;
        rdfs:isDefinedBy  <http://www.lexinfo.net/ontology/2.0/lexinfo> ;
        rdfs:label        "present" ;
        dc:creator        "Francopoulo, Gil" ;
        dcr:datcat        <http://www.isocat.org/datcat/DC-1367> ;
        owl:versionInfo   "1:0" .

lexinfo:ObjectComplement
        a                 owl:Class ;
        rdfs:isDefinedBy  <http://www.lexinfo.net/ontology/2.0/lexinfo> ;
        rdfs:subClassOf   lexinfo:Complement .

lexinfo:verb  a           lexinfo:PartOfSpeech , owl:NamedIndividual , lexinfo:VerbPOS , owl:Thing ;
        rdfs:comment      "Element which, singly or in combination with other verbs is used as the minimal predicate of a sentence, co-occurring with a subject. If the predicate contains other elements (e.g. object, complement), then it is the verb which more than any other is the unit which influences the choice and extent of these elements." ;
        rdfs:isDefinedBy  <http://www.lexinfo.net/ontology/2.0/lexinfo> ;
        rdfs:label        "verb" ;
        dc:creator        "Francopoulo, Gil" ;
        dcr:datcat        <http://www.isocat.org/datcat/DC-1424> ;
        owl:versionInfo   "1:0" .

lexinfo:NounPPFrame  a       owl:Class ;
        rdfs:isDefinedBy     <http://www.lexinfo.net/ontology/2.0/lexinfo> ;
        rdfs:subClassOf      lexinfo:NounFrame ;
        owl:equivalentClass  [ a                   owl:Class ;
                               owl:intersectionOf  ( lexinfo:NounPredicateFrame lexinfo:PrepositionalFrame )
                             ] .

lexinfo:fusedPronounAuxiliary
        a                 owl:NamedIndividual , lexinfo:PronounPOS , lexinfo:PartOfSpeech , owl:Thing ;
        rdfs:comment      "word resulting from the aggregation of a pronoun and an auxiliary" ;
        rdfs:isDefinedBy  <http://www.lexinfo.net/ontology/2.0/lexinfo> ;
        rdfs:label        "fused pronoun auxiliary" ;
        dc:creator        "Francopoulo, Gil" ;
        dcr:datcat        <http://www.isocat.org/datcat/DC-3008> ;
        owl:versionInfo   "1:0" .

lexinfo:TransitiveAdverbialComplementFrame
        a                    owl:Class ;
        rdfs:isDefinedBy     <http://www.lexinfo.net/ontology/2.0/lexinfo> ;
        rdfs:subClassOf      lexinfo:TransitiveFrame ;
        lexinfo:example      "she PUT the cheese back"@en ;
        owl:equivalentClass  [ a                   owl:Class ;
                               owl:intersectionOf  ( lexinfo:AdverbialComplementFrame lexinfo:TransitiveFrame )
                             ] .

lexinfo:AdjectiveGenitivePostPositiveFrame
        a                    owl:Class ;
        rdfs:isDefinedBy     <http://www.lexinfo.net/ontology/2.0/lexinfo> ;
        rdfs:subClassOf      lexinfo:AdjectivePostPositiveFrame ;
        lexinfo:example      "er ist des hochverrats SCHULDIG"@de ;
        owl:equivalentClass  [ a                   owl:Class ;
                               owl:intersectionOf  ( lexinfo:AdjectivePostPositiveFrame [ a                   owl:Restriction ;
                                                                                          owl:onProperty      lexinfo:postPositiveArg ;
                                                                                          owl:someValuesFrom  lexinfo:GenitivePostPositiveArgument
                                                                                        ] )
                             ] .

lexinfo:TemporalQualifier
        a                 owl:Class ;
        rdfs:isDefinedBy  <http://www.lexinfo.net/ontology/2.0/lexinfo> ;
        rdfs:subClassOf   lemon:SenseContext .

lexinfo:syllable  a       owl:NamedIndividual , lexinfo:TermElement , owl:Thing ;
        rdfs:comment      "A unit of spoken language that is next bigger than a speech sound and consists of one or more vowel sounds alone or of a syllabic consonant alone or of either with one or more consonant sounds preceding or following." ;
        rdfs:isDefinedBy  <http://www.lexinfo.net/ontology/2.0/lexinfo> ;
        rdfs:label        "syllable" ;
        dc:creator        "Wright, Sue Ellen" ;
        dcr:datcat        <http://www.isocat.org/datcat/DC-297> ;
        owl:versionInfo   "1:0" .

lexinfo:VerbPhrase  a        owl:Class ;
        rdfs:isDefinedBy     <http://www.lexinfo.net/ontology/2.0/lexinfo> ;
        rdfs:subClassOf      lemon:Phrase ;
        owl:equivalentClass  [ a                   owl:Class ;
                               owl:intersectionOf  ( lemon:Phrase [ a                   owl:Restriction ;
                                                                    owl:onProperty      lexinfo:head ;
                                                                    owl:someValuesFrom  lexinfo:Verb
                                                                  ] )
                             ] .

lemon:incompatible  a  owl:ObjectProperty .

lexinfo:future  a         owl:NamedIndividual , lexinfo:Tense , owl:Thing ;
        rdfs:comment      "Verb tense that indicates action or state of being in the future." ;
        rdfs:isDefinedBy  <http://www.lexinfo.net/ontology/2.0/lexinfo> ;
        rdfs:label        "future" ;
        dc:creator        "Francopoulo, Gil" ;
        dcr:datcat        <http://www.isocat.org/datcat/DC-1291> ;
        owl:versionInfo   "1:0" .

lexinfo:IntransitiveInfinitiveRSFrame
        a                    owl:Class ;
        rdfs:isDefinedBy     <http://www.lexinfo.net/ontology/2.0/lexinfo> ;
        rdfs:subClassOf      lexinfo:InfinitiveFrame ;
        lexinfo:example      "he SEEMED [to be happy]"@en ;
        owl:equivalentClass  [ a                   owl:Class ;
                               owl:intersectionOf  ( lexinfo:InfinitiveFrame lexinfo:IntransitiveFrame lexinfo:RaisingSubject )
                             ] .

lexinfo:benefactiveCase
        a                 owl:NamedIndividual , lexinfo:Case , owl:Thing ;
        rdfs:comment      "Case that expresses that the referent of the noun it marks receives the benefit of the situation expressed by the clause." ;
        rdfs:isDefinedBy  <http://www.lexinfo.net/ontology/2.0/lexinfo> ;
        rdfs:label        "benefactive case" ;
        dc:creator        "Francopoulo, Gil" ;
        dcr:datcat        <http://www.isocat.org/datcat/DC-1247> ;
        owl:versionInfo   "1:0" .

lexinfo:dialectRegister
        a                 owl:NamedIndividual , lexinfo:Register , owl:Thing ;
        rdfs:isDefinedBy  <http://www.lexinfo.net/ontology/2.0/lexinfo> .

terms:rights  a  owl:AnnotationProperty .

lexinfo:secondPerson  a   owl:NamedIndividual , lexinfo:Person , owl:Thing ;
        rdfs:comment      "Second person deixis is deictic reference to a person or persons identified as addressee." ;
        rdfs:isDefinedBy  <http://www.lexinfo.net/ontology/2.0/lexinfo> ;
        rdfs:label        "second person" ;
        dc:creator        "Francopoulo, Gil" ;
        dcr:datcat        <http://www.isocat.org/datcat/DC-1384> ;
        owl:versionInfo   "1:0" .

lexinfo:positiveDegreeForm
        a                   owl:ObjectProperty ;
        rdfs:isDefinedBy    <http://www.lexinfo.net/ontology/2.0/lexinfo> ;
        rdfs:subPropertyOf  lexinfo:formDegreeVariant .

terms:title  a  owl:AnnotationProperty .

lexinfo:AdjectivePredicateFrame
        a                    owl:Class ;
        rdfs:comment         "Note this frame should be used when both attributive and predicative use of the adjective is allowed"@en ;
        rdfs:isDefinedBy     <http://www.lexinfo.net/ontology/2.0/lexinfo> ;
        rdfs:subClassOf      lexinfo:AdjectiveFrame ;
        owl:equivalentClass  [ a                   owl:Class ;
                               owl:intersectionOf  ( lexinfo:AdjectiveAttributiveFrame lexinfo:AdjectivePredicativeFrame )
                             ] .

lexinfo:tense  a            owl:ObjectProperty ;
        rdfs:comment        "Property referring to the way the grammar marks the time at which the action denoted by the verb took place." ;
        rdfs:isDefinedBy    <http://www.lexinfo.net/ontology/2.0/lexinfo> ;
        rdfs:label          "tense" ;
        rdfs:range          lexinfo:Tense ;
        rdfs:subPropertyOf  lexinfo:morphosyntacticProperty ;
        dc:creator          "Francopoulo, Gil" ;
        dcr:datcat          <http://www.isocat.org/datcat/DC-1286> ;
        owl:versionInfo     "1:0" .

lexinfo:modificationType
        a                   owl:ObjectProperty ;
        rdfs:comment        "Refers to the prenominal or postnominal positions of determiners which distinguish different forms." ;
        rdfs:isDefinedBy    <http://www.lexinfo.net/ontology/2.0/lexinfo> ;
        rdfs:label          "modification type" ;
        rdfs:range          lexinfo:ModificationType ;
        rdfs:subPropertyOf  lexinfo:morphosyntacticProperty ;
        dc:creator          "Francopoulo, Gil" ;
        dcr:datcat          <http://www.isocat.org/datcat/DC-1931> ;
        owl:versionInfo     "1:0" .

lemon:marker  a  owl:ObjectProperty .

lexinfo:AdjectiveScaleFrame
        a                    owl:Class ;
        rdfs:isDefinedBy     <http://www.lexinfo.net/ontology/2.0/lexinfo> ;
        rdfs:subClassOf      lexinfo:AdjectiveFrame ;
        lexinfo:example      "Everest is 8,848m HIGH"@en ;
        owl:equivalentClass  [ a                   owl:Class ;
                               owl:intersectionOf  ( [ a                owl:Restriction ;
                                                       owl:cardinality  "1"^^xsd:nonNegativeInteger ;
                                                       owl:onProperty   lexinfo:adverbialComplement
                                                     ] [ a                owl:Restriction ;
                                                         owl:cardinality  "1"^^xsd:nonNegativeInteger ;
                                                         owl:onProperty   lexinfo:copulativeSubject
                                                       ] )
                             ] .

lexinfo:person  a           owl:ObjectProperty ;
        rdfs:comment        "Indication of grammatical person (1st, 2nd, 3rd, etc.) associated with a given inflected form." ;
        rdfs:isDefinedBy    <http://www.lexinfo.net/ontology/2.0/lexinfo> ;
        rdfs:label          "person" ;
        rdfs:range          lexinfo:Person ;
        rdfs:subPropertyOf  lexinfo:morphosyntacticProperty ;
        dc:creator          "Francopoulo, Gil" ;
        dcr:datcat          <http://www.isocat.org/datcat/DC-1328> ;
        owl:versionInfo     "1:0" .

lexinfo:Frequency  a      owl:Class ;
        rdfs:isDefinedBy  <http://www.lexinfo.net/ontology/2.0/lexinfo> ;
        rdfs:subClassOf   lemon:SenseContext .

lexinfo:impersonalPronoun
        a                 owl:Thing , lexinfo:PartOfSpeech , lexinfo:PronounPOS , owl:NamedIndividual ;
        rdfs:comment      "Pronoun lacking person referent." ;
        rdfs:isDefinedBy  <http://www.lexinfo.net/ontology/2.0/lexinfo> ;
        rdfs:label        "impersonal pronoun" ;
        dc:creator        "Francopoulo, Gil" ;
        dcr:datcat        <http://www.isocat.org/datcat/DC-1426> ;
        owl:versionInfo   "1:0" .

lexinfo:interrogativeRelativePronoun
        a                 owl:NamedIndividual , lexinfo:PartOfSpeech , owl:Thing ;
        rdfs:comment      "pronoun which may act as a relative pronoun or an interrogative one" ;
        rdfs:isDefinedBy  <http://www.lexinfo.net/ontology/2.0/lexinfo> ;
        rdfs:label        "interrogative relative pronoun" ;
        dc:creator        "Francopoulo, Gil" ;
        dcr:datcat        <http://www.isocat.org/datcat/DC-3016> ;
        owl:versionInfo   "1:0" .

lexinfo:NounPhrase  a        owl:Class ;
        rdfs:isDefinedBy     <http://www.lexinfo.net/ontology/2.0/lexinfo> ;
        rdfs:subClassOf      lemon:Phrase ;
        owl:equivalentClass  [ a                   owl:Class ;
                               owl:intersectionOf  ( lemon:Phrase [ a                   owl:Restriction ;
                                                                    owl:onProperty      lexinfo:head ;
                                                                    owl:someValuesFrom  lexinfo:Noun
                                                                  ] )
                             ] .

lexinfo:Finiteness  a     owl:Class ;
        rdfs:isDefinedBy  <http://www.lexinfo.net/ontology/2.0/lexinfo> ;
        rdfs:subClassOf   lexinfo:MorphosyntacticProperty .

lexinfo:languageSpecific
        a       owl:AnnotationProperty .

lexinfo:middleVoice  a    owl:NamedIndividual , lexinfo:Voice , owl:Thing ;
        rdfs:comment      "Value for middle voice that expresses that the subject is both the agent and object, or that the subject is separate from the agent or that the receiver is the agent him/herself." ;
        rdfs:isDefinedBy  <http://www.lexinfo.net/ontology/2.0/lexinfo> ;
        rdfs:label        "middle voice" ;
        dc:creator        "Francopoulo, Gil" ;
        dcr:datcat        <http://www.isocat.org/datcat/DC-1983> ;
        owl:versionInfo   "1:0" .

lexinfo:substanceMeronym
        a                   owl:ObjectProperty ;
        rdfs:comment        "Indicates this is a substance that composes the other"@en ;
        rdfs:isDefinedBy    <http://www.lexinfo.net/ontology/2.0/lexinfo> ;
        rdfs:label          "substance meronym"@en ;
        rdfs:subPropertyOf  lexinfo:meronymTerm .

lexinfo:interrogativeParticle
        a                 lexinfo:PartOfSpeech , owl:Thing , owl:NamedIndividual , lexinfo:ParticlePOS ;
        rdfs:comment      "Particle used to express a question." ;
        rdfs:isDefinedBy  <http://www.lexinfo.net/ontology/2.0/lexinfo> ;
        rdfs:label        "interrogative particle" ;
        dc:creator        "Francopoulo, Gil" ;
        dcr:datcat        <http://www.isocat.org/datcat/DC-1921> ;
        owl:versionInfo   "1:0" .

lexinfo:superlativeParticle
        a                 lexinfo:ParticlePOS , owl:NamedIndividual , lexinfo:PartOfSpeech , owl:Thing ;
        rdfs:comment      "Particle expressing superlative degree. Superlative is the comparison between more than two entities and contrasts with comparative where only two entities are involved and positive where no comparison is implied." ;
        rdfs:isDefinedBy  <http://www.lexinfo.net/ontology/2.0/lexinfo> ;
        rdfs:label        "superlative particle" ;
        dc:creator        "Francopoulo, Gil" ;
        dcr:datcat        <http://www.isocat.org/datcat/DC-1923> ;
        owl:versionInfo   "1:0" .

lexinfo:otherGender  a    owl:NamedIndividual , lexinfo:Gender , owl:Thing ;
        rdfs:comment      "A grammatical category that indicates grammatical relationships between words in sentences." ;
        rdfs:isDefinedBy  <http://www.lexinfo.net/ontology/2.0/lexinfo> ;
        rdfs:label        "otherGender" ;
        dc:creator        "Wright, Sue Ellen" ;
        dcr:datcat        <http://www.isocat.org/datcat/DC-249> ;
        owl:versionInfo   "1:0" .

lemon:broader  a  owl:ObjectProperty .

lexinfo:expression  a     owl:NamedIndividual , lexinfo:TermType , owl:Thing ;
        rdfs:comment      "A significant word or phrase." ;
        rdfs:isDefinedBy  <http://www.lexinfo.net/ontology/2.0/lexinfo> ;
        rdfs:label        "expression" ;
        dc:creator        "Wright, Sue Ellen" ;
        dcr:datcat        <http://www.isocat.org/datcat/DC-349> ;
        owl:versionInfo   "1:0" .

lexinfo:InfinitiveClause
        a                 owl:Class ;
        rdfs:comment      "A clause whose main verb is infinitive"@en ;
        rdfs:isDefinedBy  <http://www.lexinfo.net/ontology/2.0/lexinfo> ;
        rdfs:subClassOf   lexinfo:ClausalArgument .

lexinfo:shortFormFor  a     owl:ObjectProperty ;
        rdfs:comment        "A linking element used to identify a relation between a short form and its full or expanded form." ;
        rdfs:isDefinedBy    <http://www.lexinfo.net/ontology/2.0/lexinfo> ;
        rdfs:label          "short form for" ;
        rdfs:subPropertyOf  lexinfo:contractionFor ;
        dc:creator          "Wright, Sue Ellen" ;
        dcr:datcat          <http://www.isocat.org/datcat/DC-468> ;
        owl:versionInfo     "1:0" .

lexinfo:suspensionPoints
        a                 owl:Thing , owl:NamedIndividual , lexinfo:SymbolPOS , lexinfo:PartOfSpeech ;
        rdfs:comment      "Sequence of three dots having the same meaning as &quot;et cetera&quot; (full form) or &quot;etc&quot; (abbreviated form)." ;
        rdfs:isDefinedBy  <http://www.lexinfo.net/ontology/2.0/lexinfo> ;
        rdfs:label        "suspension points" ;
        dc:creator        "Francopoulo, Gil" ;
        dcr:datcat        <http://www.isocat.org/datcat/DC-1447> ;
        owl:versionInfo   "1:0" .

<http://purl.org/vocommons/voaf#Vocabulary>
        a       owl:Class .

lexinfo:postModifier  a   owl:NamedIndividual , lexinfo:ModificationType , owl:Thing ;
        rdfs:comment      "Situation where the modifier is after the modified." ;
        rdfs:isDefinedBy  <http://www.lexinfo.net/ontology/2.0/lexinfo> ;
        rdfs:label        "post modifier" ;
        dc:creator        "Francopoulo, Gil" ;
        dcr:datcat        <http://www.isocat.org/datcat/DC-1945> ;
        owl:versionInfo   "1:0" .

lexinfo:bullet  a         lexinfo:SymbolPOS , owl:NamedIndividual , lexinfo:PartOfSpeech , owl:Thing ;
        rdfs:comment      "Sign used to mark an item in a list." ;
        rdfs:isDefinedBy  <http://www.lexinfo.net/ontology/2.0/lexinfo> ;
        rdfs:label        "bullet" ;
        dc:creator        "Francopoulo, Gil" ;
        dcr:datcat        <http://www.isocat.org/datcat/DC-1438> ;
        owl:versionInfo   "1:0" .

lexinfo:conditionalParticle
        a                 lexinfo:PartOfSpeech , lexinfo:ParticlePOS , owl:Thing , owl:NamedIndividual ;
        rdfs:comment      "conditional particule" ;
        rdfs:isDefinedBy  <http://www.lexinfo.net/ontology/2.0/lexinfo> ;
        rdfs:label        "conditional particule" ;
        dc:creator        "Francopoulo, Gil" ;
        dcr:datcat        <http://www.isocat.org/datcat/DC-2230> ;
        owl:versionInfo   "1:0" .

lexinfo:GerundSCFrame
        a                    owl:Class ;
        rdfs:isDefinedBy     <http://www.lexinfo.net/ontology/2.0/lexinfo> ;
        rdfs:subClassOf      lexinfo:GerundFrame ;
        owl:equivalentClass  [ a                   owl:Class ;
                               owl:intersectionOf  ( lexinfo:GerundFrame lexinfo:SubjectControl )
                             ] .

lexinfo:IntransitiveFrame
        a                    owl:Class ;
        rdfs:isDefinedBy     <http://www.lexinfo.net/ontology/2.0/lexinfo> ;
        rdfs:subClassOf      lexinfo:VerbFrame ;
        lexinfo:example      "he LEFT"@en ;
        owl:equivalentClass  [ a                   owl:Class ;
                               owl:intersectionOf  ( lexinfo:VerbFrame [ a                owl:Restriction ;
                                                                         owl:cardinality  "0"^^xsd:nonNegativeInteger ;
                                                                         owl:onProperty   lexinfo:directObject
                                                                       ] [ a                owl:Restriction ;
                                                                           owl:cardinality  "1"^^xsd:nonNegativeInteger ;
                                                                           owl:onProperty   lexinfo:subject
                                                                         ] )
                             ] .

lexinfo:numeralFraction
        a                 lexinfo:NumeralPOS , owl:NamedIndividual , lexinfo:PartOfSpeech , owl:Thing ;
        rdfs:comment      "Word used to denote the denominator of a fraction." ;
        rdfs:isDefinedBy  <http://www.lexinfo.net/ontology/2.0/lexinfo> ;
        rdfs:label        "numeral fraction" ;
        dc:creator        "Zeman, Dan" ;
        dcr:datcat        <http://www.isocat.org/datcat/DC-3026> ;
        owl:versionInfo   "1:0" .

lexinfo:segmentation  a     owl:DatatypeProperty ;
        rdfs:comment        "Specification of the pointers in time or sequence that indicates the segmentation process." ;
        rdfs:isDefinedBy    <http://www.lexinfo.net/ontology/2.0/lexinfo> ;
        rdfs:label          "segmentation" ;
        rdfs:range          xsd:string ;
        rdfs:subPropertyOf  lemon:representation ;
        dc:creator          "Wittenburg, Peter" ;
        dcr:datcat          <http://www.isocat.org/datcat/DC-2578> ;
        owl:versionInfo     "1:0" .

lexinfo:participle  a     owl:NamedIndividual , lexinfo:VerbFormMood , owl:Thing ;
        rdfs:comment      "Term referring to a word derived from a verb and used as an adjective." ;
        rdfs:isDefinedBy  <http://www.lexinfo.net/ontology/2.0/lexinfo> ;
        rdfs:label        "participle" ;
        dc:creator        "Francopoulo, Gil" ;
        dcr:datcat        <http://www.isocat.org/datcat/DC-1341> ;
        owl:versionInfo   "1:0" .

lexinfo:ReflexiveTransitiveFrame
        a                    owl:Class ;
        rdfs:isDefinedBy     <http://www.lexinfo.net/ontology/2.0/lexinfo> ;
        rdfs:subClassOf      lexinfo:ReflexiveFrame ;
        lexinfo:example      "elle se COUCHE"@fr , "er ERHOLT sich"@de ;
        owl:equivalentClass  [ a                   owl:Class ;
                               owl:intersectionOf  ( lexinfo:ReflexiveFrame lexinfo:TransitiveFrame )
                             ] .

lexinfo:Animacy  a        owl:Class ;
        rdfs:isDefinedBy  <http://www.lexinfo.net/ontology/2.0/lexinfo> ;
        rdfs:subClassOf   lexinfo:MorphosyntacticProperty .

lexinfo:VerbFrame  a      owl:Class ;
        rdfs:isDefinedBy  <http://www.lexinfo.net/ontology/2.0/lexinfo> ;
        rdfs:subClassOf   lemon:Frame .

lexinfo:animacy  a          owl:ObjectProperty ;
        rdfs:comment        "The characteristic of a word indicating that in a given discourse community, its referent is considered to be alive or to possess a quality of volition or consciousness." ;
        rdfs:isDefinedBy    <http://www.lexinfo.net/ontology/2.0/lexinfo> ;
        rdfs:label          "animacy" ;
        rdfs:range          lexinfo:Animacy ;
        rdfs:subPropertyOf  lexinfo:morphosyntacticProperty ;
        dc:creator          "Wright, Sue Ellen" , "Francopoulo, Gil" ;
        dcr:datcat          <http://www.isocat.org/datcat/DC-1902> , <http://www.isocat.org/datcat/DC-78> ;
        owl:versionInfo     "1:0" .

lexinfo:indefiniteDeterminer
        a                 owl:Thing , owl:NamedIndividual , lexinfo:PartOfSpeech , lexinfo:DeterminerPOS ;
        rdfs:comment      "Determiner not capable of identification." ;
        rdfs:isDefinedBy  <http://www.lexinfo.net/ontology/2.0/lexinfo> ;
        rdfs:label        "indefinite determiner" ;
        dc:creator        "Francopoulo, Gil" ;
        dcr:datcat        <http://www.isocat.org/datcat/DC-1307> ;
        owl:versionInfo   "1:0" .

lexinfo:TransitiveSententialFrame
        a                    owl:Class ;
        rdfs:isDefinedBy     <http://www.lexinfo.net/ontology/2.0/lexinfo> ;
        rdfs:subClassOf      lexinfo:SententialFrame ;
        lexinfo:example      "he TOLD the audience he was leaving"@en ;
        owl:equivalentClass  [ a                   owl:Class ;
                               owl:intersectionOf  ( lexinfo:SententialFrame lexinfo:TransitiveFrame )
                             ] .

lexinfo:prefix  a         owl:NamedIndividual , lexinfo:TermElement , owl:Thing ;
        rdfs:isDefinedBy  <http://www.lexinfo.net/ontology/2.0/lexinfo> .

lexinfo:unaccomplished
        a                 owl:NamedIndividual , lexinfo:Aspect , owl:Thing ;
        rdfs:comment      "aspect that expresses an event or state that is not finished." ;
        rdfs:isDefinedBy  <http://www.lexinfo.net/ontology/2.0/lexinfo> ;
        rdfs:label        "unaccomplished" ;
        dc:creator        "Francopoulo, Gil" ;
        dcr:datcat        <http://www.isocat.org/datcat/DC-2217> ;
        owl:versionInfo   "1:0" .

lexinfo:TransitiveAdjectivalComplementFrame
        a                    owl:Class ;
        rdfs:isDefinedBy     <http://www.lexinfo.net/ontology/2.0/lexinfo> ;
        rdfs:subClassOf      lexinfo:TransitiveFrame ;
        lexinfo:example      "they PAINTED it red"@en ;
        owl:equivalentClass  [ a                   owl:Class ;
                               owl:intersectionOf  ( lexinfo:AdjectivalComplementFrame lexinfo:TransitiveFrame )
                             ] .

lexinfo:causativeCase
        a                 owl:NamedIndividual , lexinfo:Case , owl:Thing ;
        rdfs:comment      "Case which expresses that the referent of the noun it marks is the cause of the situation expressed by the clause." ;
        rdfs:isDefinedBy  <http://www.lexinfo.net/ontology/2.0/lexinfo> ;
        rdfs:label        "causative case" ;
        dc:creator        "Francopoulo, Gil" ;
        dcr:datcat        <http://www.isocat.org/datcat/DC-1253> ;
        owl:versionInfo   "1:0" .

lexinfo:neuter  a         lexinfo:Gender , owl:NamedIndividual , owl:Thing ;
        rdfs:comment      "Of, relating to, or constituting the gender that ordinarily includes most words or grammatical forms referring to objects that are not characterized as male or female." ;
        rdfs:isDefinedBy  <http://www.lexinfo.net/ontology/2.0/lexinfo> ;
        rdfs:label        "neuter" ;
        dc:creator        "Wright, Sue Ellen" , "Francopoulo, Gil" ;
        dcr:datcat        <http://www.isocat.org/datcat/DC-248> , <http://www.isocat.org/datcat/DC-1884> ;
        owl:versionInfo   "1:0" .

lexinfo:exclamativePoint
        a                 owl:Thing , owl:NamedIndividual , lexinfo:PartOfSpeech , lexinfo:SymbolPOS ;
        rdfs:comment      "Special sign (!) usually used in writing to mark exclamation." ;
        rdfs:isDefinedBy  <http://www.lexinfo.net/ontology/2.0/lexinfo> ;
        rdfs:label        "exclamative point" ;
        dc:creator        "Francopoulo, Gil" ;
        dcr:datcat        <http://www.isocat.org/datcat/DC-1441> ;
        owl:versionInfo   "1:0" .

lexinfo:ModificationType
        a                 owl:Class ;
        rdfs:isDefinedBy  <http://www.lexinfo.net/ontology/2.0/lexinfo> ;
        rdfs:subClassOf   lexinfo:MorphosyntacticProperty .

lexinfo:DativePostPositiveArgument
        a                    owl:Class ;
        rdfs:isDefinedBy     <http://www.lexinfo.net/ontology/2.0/lexinfo> ;
        rdfs:subClassOf      lexinfo:PostPositiveArgument ;
        owl:equivalentClass  [ a                   owl:Class ;
                               owl:intersectionOf  ( lexinfo:PostPositiveArgument [ a               owl:Restriction ;
                                                                                    owl:hasValue    lexinfo:dativeCase ;
                                                                                    owl:onProperty  lemon:marker
                                                                                  ] )
                             ] .

lexinfo:declarativeClause
        a                   owl:ObjectProperty ;
        rdfs:isDefinedBy    <http://www.lexinfo.net/ontology/2.0/lexinfo> ;
        rdfs:subPropertyOf  lexinfo:clausalArg .

lexinfo:ImpersonalFrame
        a                    owl:Class ;
        rdfs:isDefinedBy     <http://www.lexinfo.net/ontology/2.0/lexinfo> ;
        rdfs:subClassOf      lexinfo:VerbFrame ;
        owl:equivalentClass  [ a                   owl:Class ;
                               owl:intersectionOf  ( lexinfo:VerbFrame [ a                owl:Restriction ;
                                                                         owl:cardinality  "0"^^xsd:nonNegativeInteger ;
                                                                         owl:onProperty   lexinfo:subject
                                                                       ] )
                             ] .

lexinfo:infrequentlyUsed
        a                 owl:Thing , lexinfo:Frequency , owl:NamedIndividual ;
        rdfs:comment      "Said of a term that does not appear frequently." ;
        rdfs:isDefinedBy  <http://www.lexinfo.net/ontology/2.0/lexinfo> ;
        rdfs:label        "infrequentlyUsed" , "infrequently used" ;
        dc:creator        "Francopoulo, Gil" , "Wright, Sue Ellen" ;
        dcr:datcat        <http://www.isocat.org/datcat/DC-235> , <http://www.isocat.org/datcat/DC-1985> ;
        owl:versionInfo   "1:0" .

lexinfo:adjective  a      lexinfo:PartOfSpeech , owl:NamedIndividual , owl:Thing , lexinfo:AdjectivePOS ;
        rdfs:comment      "Part of speech related to attributes of noun." ;
        rdfs:isDefinedBy  <http://www.lexinfo.net/ontology/2.0/lexinfo> ;
        rdfs:label        "adjective" ;
        dc:creator        "Francopoulo, Gil" ;
        dcr:datcat        <http://www.isocat.org/datcat/DC-1230> ;
        owl:versionInfo   "1:0" .

lexinfo:TransitiveInfinitiveOCFrame
        a                    owl:Class ;
        rdfs:isDefinedBy     <http://www.lexinfo.net/ontology/2.0/lexinfo> ;
        rdfs:subClassOf      lexinfo:InfinitiveFrame ;
        lexinfo:example      "i WANT john [to go]"@en ;
        owl:equivalentClass  [ a                   owl:Class ;
                               owl:intersectionOf  ( lexinfo:InfinitiveFrame lexinfo:ObjectControl lexinfo:TransitiveFrame )
                             ] .

lexinfo:elativeCase  a    owl:NamedIndividual , lexinfo:Case , owl:Thing ;
        rdfs:comment      "Case which expresses the meaning of motion 'away from' from the referent of the noun it marks." ;
        rdfs:isDefinedBy  <http://www.lexinfo.net/ontology/2.0/lexinfo> ;
        rdfs:label        "elative case" ;
        dc:creator        "Francopoulo, Gil" ;
        dcr:datcat        <http://www.isocat.org/datcat/DC-1276> ;
        owl:versionInfo   "1:0" .

lexinfo:AdjectiveAttributiveFrame
        a                    owl:Class ;
        rdfs:isDefinedBy     <http://www.lexinfo.net/ontology/2.0/lexinfo> ;
        rdfs:subClassOf      lexinfo:AdjectiveFrame ;
        lexinfo:example      "the RED ball"@en ;
        owl:equivalentClass  [ a                   owl:Class ;
                               owl:intersectionOf  ( lexinfo:AdjectiveFrame [ a                   owl:Restriction ;
                                                                              owl:minCardinality  "1"^^xsd:nonNegativeInteger ;
                                                                              owl:onProperty      lexinfo:attributiveArg
                                                                            ] )
                             ] .

lexinfo:cessative  a      owl:NamedIndividual , lexinfo:Aspect , owl:Thing ;
        rdfs:comment      "Aspect that expresses the cessation of an event or state." ;
        rdfs:isDefinedBy  <http://www.lexinfo.net/ontology/2.0/lexinfo> ;
        rdfs:label        "cessative" ;
        dc:creator        "Francopoulo, Gil" ;
        dcr:datcat        <http://www.isocat.org/datcat/DC-2001> ;
        owl:versionInfo   "1:0" .

lexinfo:cliticness  a       owl:ObjectProperty ;
        rdfs:comment        "Categorization of the different types of clitics" ;
        rdfs:isDefinedBy    <http://www.lexinfo.net/ontology/2.0/lexinfo> ;
        rdfs:label          "cliticness" ;
        rdfs:range          lexinfo:Cliticness ;
        rdfs:subPropertyOf  lexinfo:morphosyntacticProperty ;
        dc:creator          "Francopoulo, Gil" ;
        dcr:datcat          <http://www.isocat.org/datcat/DC-1903> ;
        owl:versionInfo     "1:0" .

lexinfo:relativeDeterminer
        a                 owl:Thing , lexinfo:PartOfSpeech , lexinfo:DeterminerPOS , owl:NamedIndividual ;
        rdfs:comment      "Determiner related to a referent." ;
        rdfs:isDefinedBy  <http://www.lexinfo.net/ontology/2.0/lexinfo> ;
        rdfs:label        "relative determiner" ;
        dc:creator        "Francopoulo, Gil" ;
        dcr:datcat        <http://www.isocat.org/datcat/DC-1379> ;
        owl:versionInfo   "1:0" .

lexinfo:homophone  a        owl:ObjectProperty ;
        rdfs:comment        "A word that is pronounced in the same way as another word but that is spelled differently." , "Word that sounds like another word, but is different in writiing or meaning." ;
        rdfs:isDefinedBy    <http://www.lexinfo.net/ontology/2.0/lexinfo> ;
        rdfs:label          "homophone" ;
        rdfs:subPropertyOf  lemon:lexicalVariant ;
        dc:creator          "Francopoulo, Gil" , "Wright, Sue Ellen" ;
        dcr:datcat          <http://www.isocat.org/datcat/DC-263> , <http://www.isocat.org/datcat/DC-1302> ;
        owl:versionInfo     "1:0" .

lexinfo:collocation  a      owl:ObjectProperty ;
        rdfs:isDefinedBy    <http://www.lexinfo.net/ontology/2.0/lexinfo> ;
        rdfs:subPropertyOf  lemon:senseRelation .

vann:preferredNamespaceUri
        a       owl:AnnotationProperty .

lexinfo:DeterminerPOS
        a                 owl:Class ;
        rdfs:isDefinedBy  <http://www.lexinfo.net/ontology/2.0/lexinfo> ;
        rdfs:subClassOf   lexinfo:PartOfSpeech .

lexinfo:letter  a         owl:NamedIndividual , lexinfo:SymbolPOS , owl:Thing ;
        rdfs:isDefinedBy  <http://www.lexinfo.net/ontology/2.0/lexinfo> .

lexinfo:abbreviation  a   owl:NamedIndividual , lexinfo:TermType , lexinfo:AbbreviatedForm , owl:Thing ;
        rdfs:isDefinedBy  <http://www.lexinfo.net/ontology/2.0/lexinfo> .

lexinfo:etymologicalRoot
        a                   owl:ObjectProperty ;
        rdfs:comment        "Morpheme that has a particular status with regards to the word's etymology." ;
        rdfs:isDefinedBy    <http://www.lexinfo.net/ontology/2.0/lexinfo> ;
        rdfs:label          "etymological root" ;
        rdfs:subPropertyOf  lemon:lexicalVariant ;
        dc:creator          "Francopoulo, Gil" ;
        dcr:datcat          <http://www.isocat.org/datcat/DC-1987> ;
        owl:versionInfo     "1:0" .

lexinfo:allativeCase  a   owl:NamedIndividual , lexinfo:Case , owl:Thing ;
        rdfs:comment      "Case which expresses the meaning of motion 'to' or 'towards' the referent it marks." ;
        rdfs:isDefinedBy  <http://www.lexinfo.net/ontology/2.0/lexinfo> ;
        rdfs:label        "allative case" ;
        dc:creator        "Francopoulo, Gil" ;
        dcr:datcat        <http://www.isocat.org/datcat/DC-1236> ;
        owl:versionInfo   "1:0" .

lexinfo:closeParenthesis
        a                 lexinfo:PartOfSpeech , lexinfo:SymbolPOS , owl:Thing , owl:NamedIndividual ;
        rdfs:comment      "End of a parenthesis pair." ;
        rdfs:isDefinedBy  <http://www.lexinfo.net/ontology/2.0/lexinfo> ;
        rdfs:label        "close parenthesis" ;
        dc:creator        "Francopoulo, Gil" ;
        dcr:datcat        <http://www.isocat.org/datcat/DC-1440> ;
        owl:versionInfo   "1:0" .

lexinfo:case  a             owl:ObjectProperty ;
        rdfs:comment        "In a given sentence, the way in which the form of a word changes in order to express a relationship with one or several words of the sentence. The morphological modification may apply to nouns, pronouns noun phrase constituents, such as adjectives or numerals." ;
        rdfs:isDefinedBy    <http://www.lexinfo.net/ontology/2.0/lexinfo> ;
        rdfs:label          "case" ;
        rdfs:range          lexinfo:Case ;
        rdfs:subPropertyOf  lexinfo:morphosyntacticProperty ;
        dc:creator          "Francopoulo, Gil" ;
        dcr:datcat          <http://www.isocat.org/datcat/DC-1840> ;
        owl:versionInfo     "1:0" .

lexinfo:fusedPrepositionPronoun
        a                 owl:NamedIndividual , owl:Thing , lexinfo:PartOfSpeech , lexinfo:FusedPrepositionPOS ;
        rdfs:comment      "word resulting from the aggregation of a preposition and a pronoun" ;
        rdfs:isDefinedBy  <http://www.lexinfo.net/ontology/2.0/lexinfo> ;
        rdfs:label        "fused preposition pronoun" ;
        dc:creator        "Francopoulo, Gil" ;
        dcr:datcat        <http://www.isocat.org/datcat/DC-3009> ;
        owl:versionInfo   "1:0" .

terms:issued  a  owl:AnnotationProperty .

lexinfo:adverb  a         owl:NamedIndividual , lexinfo:AdverbPOS , owl:Thing , lexinfo:PartOfSpeech ;
        rdfs:comment      "Part of speech to refer to an heterogeneous group of words whose most frequent function is to specify the mode of action of the verb." ;
        rdfs:isDefinedBy  <http://www.lexinfo.net/ontology/2.0/lexinfo> ;
        rdfs:label        "adverb" ;
        dc:creator        "Francopoulo, Gil" ;
        dcr:datcat        <http://www.isocat.org/datcat/DC-1232> ;
        owl:versionInfo   "1:0" .

lexinfo:Determiner  a        owl:Class ;
        rdfs:isDefinedBy     <http://www.lexinfo.net/ontology/2.0/lexinfo> ;
        rdfs:subClassOf      lemon:Word ;
        owl:equivalentClass  [ a                   owl:Restriction ;
                               owl:onProperty      lexinfo:partOfSpeech ;
                               owl:someValuesFrom  lexinfo:DeterminerPOS
                             ] .

lexinfo:definiteArticle
        a                 lexinfo:PartOfSpeech , owl:NamedIndividual , lexinfo:ArticlePOS , owl:Thing , lexinfo:DeterminerPOS ;
        rdfs:comment      "Article that allows the reference to a specific, identifiable entity (or class of entities)." ;
        rdfs:isDefinedBy  <http://www.lexinfo.net/ontology/2.0/lexinfo> ;
        rdfs:label        "definite article" ;
        dc:creator        "Francopoulo, Gil" ;
        dcr:datcat        <http://www.isocat.org/datcat/DC-1430> ;
        owl:versionInfo   "1:0" .

lexinfo:IntransitiveInterrogativeFrame
        a                    owl:Class ;
        rdfs:comment         "he ASKED [what he should do]"@en ;
        rdfs:isDefinedBy     <http://www.lexinfo.net/ontology/2.0/lexinfo> ;
        rdfs:subClassOf      lexinfo:InterrogativeFrame ;
        owl:equivalentClass  [ a                   owl:Class ;
                               owl:intersectionOf  ( lexinfo:InterrogativeFrame lexinfo:IntransitiveFrame )
                             ] .

lexinfo:copulativeArg
        a                   owl:ObjectProperty ;
        rdfs:comment        "Used with copula constructions. This represents the subject/object in a copula construction. As such constructions are reversible this property is used instead of the usual verb subject/object. E,g.,\n\nBarack Obama is the president/The president is Barack Obama"@en ;
        rdfs:isDefinedBy    <http://www.lexinfo.net/ontology/2.0/lexinfo> ;
        rdfs:subPropertyOf  lemon:synArg .

lexinfo:masculine  a      owl:Thing , lexinfo:Gender , owl:NamedIndividual ;
        rdfs:comment      "Of, relating to, or constituting the gender that ordinarily includes most words or grammatical forms referring to males." ;
        rdfs:isDefinedBy  <http://www.lexinfo.net/ontology/2.0/lexinfo> ;
        rdfs:label        "masculine" ;
        dc:creator        "Wright, Sue Ellen" , "Francopoulo, Gil" ;
        dcr:datcat        <http://www.isocat.org/datcat/DC-246> , <http://www.isocat.org/datcat/DC-1883> ;
        owl:versionInfo   "1:0" .

lexinfo:CJK_compound  a   owl:NamedIndividual , lexinfo:TermType , owl:Thing ;
        rdfs:comment      "A lexical unit in a CJKV language that is represented by at least two CJKV characters." ;
        rdfs:isDefinedBy  <http://www.lexinfo.net/ontology/2.0/lexinfo> ;
        rdfs:label        "compound(cjkv)" ;
        dc:creator        "Wright, Sue Ellen" ;
        dcr:datcat        <http://www.isocat.org/datcat/DC-356> ;
        owl:versionInfo   "1:0" .

lexinfo:Article  a           owl:Class ;
        rdfs:isDefinedBy     <http://www.lexinfo.net/ontology/2.0/lexinfo> ;
        rdfs:subClassOf      lexinfo:Determiner ;
        owl:equivalentClass  [ a                   owl:Restriction ;
                               owl:onProperty      lexinfo:partOfSpeech ;
                               owl:someValuesFrom  lexinfo:ArticlePOS
                             ] .

lexinfo:preModifier  a    owl:NamedIndividual , lexinfo:ModificationType , owl:Thing ;
        rdfs:comment      "Situation where the modifier is before the modified." ;
        rdfs:isDefinedBy  <http://www.lexinfo.net/ontology/2.0/lexinfo> ;
        rdfs:label        "premodifier" ;
        dc:creator        "Francopoulo, Gil" ;
        dcr:datcat        <http://www.isocat.org/datcat/DC-1943> ;
        owl:versionInfo   "1:0" .

lexinfo:conditionalPronoun
        a                 owl:NamedIndividual , lexinfo:PronounPOS , lexinfo:PartOfSpeech , owl:Thing ;
        rdfs:comment      "conditional pronoun" ;
        rdfs:isDefinedBy  <http://www.lexinfo.net/ontology/2.0/lexinfo> ;
        rdfs:label        "conditional pronoun" ;
        dc:creator        "Francopoulo, Gil" ;
        dcr:datcat        <http://www.isocat.org/datcat/DC-2222> ;
        owl:versionInfo   "1:0" .

lexinfo:commonName  a     owl:NamedIndividual , lexinfo:TermType , owl:Thing ;
        rdfs:comment      "A synonym for an international scientific term that is used in general discourse in a given language." ;
        rdfs:isDefinedBy  <http://www.lexinfo.net/ontology/2.0/lexinfo> ;
        rdfs:label        "common name" ;
        dc:creator        "Wright, Sue Ellen" ;
        dcr:datcat        <http://www.isocat.org/datcat/DC-328> ;
        owl:versionInfo   "1:0" .

lexinfo:article  a        lexinfo:DeterminerPOS , owl:NamedIndividual , owl:Thing , lexinfo:PartOfSpeech , lexinfo:ArticlePOS ;
        rdfs:comment      "..." , "Term used in the grammatical classification of words referring to a subclass of determiners which displays a primary role in differentiating the uses of nouns." ;
        rdfs:isDefinedBy  <http://www.lexinfo.net/ontology/2.0/lexinfo> ;
        rdfs:label        "article" ;
        dc:creator        "Wright, Sue Ellen" , "Francopoulo, Gil" ;
        dcr:datcat        <http://www.isocat.org/datcat/DC-1892> , <http://www.isocat.org/datcat/DC-101> ;
        owl:versionInfo   "1:0" .

lexinfo:affixedPersonalPronoun
        a                 owl:NamedIndividual , lexinfo:PronounPOS , owl:Thing , lexinfo:PartOfSpeech ;
        rdfs:comment      "Personnal pronoun that is affixed, i.e. added as an affix to another word." ;
        rdfs:isDefinedBy  <http://www.lexinfo.net/ontology/2.0/lexinfo> ;
        rdfs:label        "affixed personal pronoun" ;
        dc:creator        "Francopoulo, Gil" ;
        dcr:datcat        <http://www.isocat.org/datcat/DC-2221> ;
        owl:versionInfo   "1:0" .

lexinfo:sku  a            owl:NamedIndividual , lexinfo:TermType , owl:Thing ;
        rdfs:comment      "An inventory item identified by a unique alphanumeric designation assigned to an object in an inventory control system." ;
        rdfs:isDefinedBy  <http://www.lexinfo.net/ontology/2.0/lexinfo> ;
        rdfs:label        "sku" ;
        dc:creator        "Wright, Sue Ellen" ;
        dcr:datcat        <http://www.isocat.org/datcat/DC-337> ;
        owl:versionInfo   "1:0" .

lexinfo:approximateSynonym
        a                   owl:ObjectProperty ;
        rdfs:isDefinedBy    <http://www.lexinfo.net/ontology/2.0/lexinfo> ;
        rdfs:subPropertyOf  lemon:senseRelation .

lexinfo:fullForm  a       owl:NamedIndividual , lexinfo:TermType , owl:Thing ;
        rdfs:comment      "The complete presentation of a term or lexeme for which there is an abbreviated form." ;
        rdfs:isDefinedBy  <http://www.lexinfo.net/ontology/2.0/lexinfo> ;
        rdfs:label        "full form" ;
        dc:creator        "Wright, Sue Ellen" ;
        dcr:datcat        <http://www.isocat.org/datcat/DC-321> ;
        owl:versionInfo   "1:0" .

lexinfo:holonymTerm  a      owl:ObjectProperty ;
        rdfs:comment        "Indicates that the referenced element is a part of this object"@en ;
        rdfs:isDefinedBy    <http://www.lexinfo.net/ontology/2.0/lexinfo> ;
        rdfs:label          "holonym"@en ;
        rdfs:subPropertyOf  lexinfo:partitiveRelation ;
        owl:inverseOf       lexinfo:meronymTerm .

lexinfo:synonym  a          owl:ObjectProperty ;
        rdfs:isDefinedBy    <http://www.lexinfo.net/ontology/2.0/lexinfo> ;
        rdfs:subPropertyOf  lemon:equivalent .

lexinfo:antonym  a          owl:ObjectProperty ;
        rdfs:comment        "A term or lexeme whose concept or sense constitutes the opposite of the concept represented by a second term or lexeme." ;
        rdfs:isDefinedBy    <http://www.lexinfo.net/ontology/2.0/lexinfo> ;
        rdfs:label          "antonym term" ;
        rdfs:subPropertyOf  lemon:incompatible ;
        dc:creator          "Wright, Sue Ellen" ;
        dcr:datcat          <http://www.isocat.org/datcat/DC-83> ;
        owl:versionInfo     "1:0" .

lexinfo:logicalExpression
        a                 owl:NamedIndividual , lexinfo:TermType , owl:Thing ;
        rdfs:comment      "An expression used to represent a concept based on mathematical or logical relations, such as statements of inequality, set relationships, boolean operations, and the like." ;
        rdfs:isDefinedBy  <http://www.lexinfo.net/ontology/2.0/lexinfo> ;
        rdfs:label        "logical expression" ;
        dc:creator        "Wright, Sue Ellen" ;
        dcr:datcat        <http://www.isocat.org/datcat/DC-327> ;
        owl:versionInfo   "1:0" .

lexinfo:TermElement  a    owl:Class ;
        rdfs:isDefinedBy  <http://www.lexinfo.net/ontology/2.0/lexinfo> ;
        rdfs:subClassOf   lemon:PropertyValue .

lexinfo:supersededTerm
        a                 owl:NamedIndividual , lexinfo:NormativeAuthorization , owl:Thing ;
        rdfs:comment      "A term that is no longer preferred or admitted." ;
        rdfs:isDefinedBy  <http://www.lexinfo.net/ontology/2.0/lexinfo> ;
        rdfs:label        "superseded term" ;
        dc:creator        "Wright, Sue Ellen" ;
        dcr:datcat        <http://www.isocat.org/datcat/DC-379> ;
        owl:versionInfo   "1:0" .

lexinfo:ImpersonalIntransitivePPFrame
        a                    owl:Class ;
        rdfs:isDefinedBy     <http://www.lexinfo.net/ontology/2.0/lexinfo> ;
        rdfs:subClassOf      lexinfo:PrepositionalFrame , lexinfo:ImpersonalTransitiveFrame ;
        lexinfo:example      "it REEKS OF tar"@en ;
        owl:equivalentClass  [ a                   owl:Class ;
                               owl:intersectionOf  ( lexinfo:ImpersonalIntransitiveFrame lexinfo:PrepositionalFrame )
                             ] .

lexinfo:ablativeCase  a   owl:NamedIndividual , lexinfo:Case , owl:Thing ;
        rdfs:comment      "Case used to typically indicate locative or instrumental function." ;
        rdfs:isDefinedBy  <http://www.lexinfo.net/ontology/2.0/lexinfo> ;
        rdfs:label        "ablative case" ;
        dc:creator        "Francopoulo, Gil" ;
        dcr:datcat        <http://www.isocat.org/datcat/DC-1224> ;
        owl:versionInfo   "1:0" .

lexinfo:subjunctive  a    lexinfo:Mood , owl:NamedIndividual , lexinfo:VerbFormMood , owl:Thing ;
        rdfs:comment      "..." , "Mood often used to express uncertainty, whishes or desires." ;
        rdfs:isDefinedBy  <http://www.lexinfo.net/ontology/2.0/lexinfo> ;
        rdfs:label        "subjunctive" ;
        dc:creator        "Wright, Sue Ellen" , "Francopoulo, Gil" ;
        dcr:datcat        <http://www.isocat.org/datcat/DC-1843> , <http://www.isocat.org/datcat/DC-368> ;
        owl:versionInfo   "1:0" .

lexinfo:DitransitiveFrame_For
        a                         owl:Class ;
        rdfs:isDefinedBy          <http://www.lexinfo.net/ontology/2.0/lexinfo> ;
        rdfs:subClassOf           lexinfo:DitransitiveFrame ;
        lexinfo:example           "she BOUGHT him it\nshe BOUGHT it FOR him"@en ;
        lexinfo:languageSpecific  "en" .

lexinfo:ArticlePOS  a     owl:Class ;
        rdfs:isDefinedBy  <http://www.lexinfo.net/ontology/2.0/lexinfo> ;
        rdfs:subClassOf   lexinfo:DeterminerPOS .

lexinfo:exclamativeDeterminer
        a                 owl:Thing , lexinfo:DeterminerPOS , owl:NamedIndividual , lexinfo:PartOfSpeech ;
        rdfs:comment      "Determiner expressing an emotional utterance and marked with a strong intonation." ;
        rdfs:isDefinedBy  <http://www.lexinfo.net/ontology/2.0/lexinfo> ;
        rdfs:label        "exclamative determiner" ;
        dc:creator        "Francopoulo, Gil" ;
        dcr:datcat        <http://www.isocat.org/datcat/DC-1284> ;
        owl:versionInfo   "1:0" .

lexinfo:GenitiveTransitiveFrame
        a                    owl:Class ;
        rdfs:isDefinedBy     <http://www.lexinfo.net/ontology/2.0/lexinfo> ;
        rdfs:subClassOf      lexinfo:VerbFrame ;
        lexinfo:example      "wir BEDENKEN jenes mannes"@de ;
        owl:equivalentClass  [ a                   owl:Class ;
                               owl:intersectionOf  ( lexinfo:VerbFrame [ a                owl:Restriction ;
                                                                         owl:cardinality  "1"^^xsd:nonNegativeInteger ;
                                                                         owl:onProperty   lexinfo:genitiveObject
                                                                       ] [ a                owl:Restriction ;
                                                                           owl:cardinality  "1"^^xsd:nonNegativeInteger ;
                                                                           owl:onProperty   lexinfo:subject
                                                                         ] )
                             ] .

lexinfo:imperfect  a      owl:NamedIndividual , lexinfo:Tense , owl:Thing ;
        rdfs:comment      "Verb tense that refers to action in the past that is incomplete or ongoing." ;
        rdfs:isDefinedBy  <http://www.lexinfo.net/ontology/2.0/lexinfo> ;
        rdfs:label        "imperfect" ;
        dc:creator        "Francopoulo, Gil" ;
        dcr:datcat        <http://www.isocat.org/datcat/DC-1304> ;
        owl:versionInfo   "1:0" .

lexinfo:comitativeCase
        a                 owl:NamedIndividual , lexinfo:Case , owl:Thing ;
        rdfs:comment      "Case which expresses a meaning similar to 'along with' or 'accompagnied by'." ;
        rdfs:isDefinedBy  <http://www.lexinfo.net/ontology/2.0/lexinfo> ;
        rdfs:label        "comitative case" ;
        dc:creator        "Francopoulo, Gil" ;
        dcr:datcat        <http://www.isocat.org/datcat/DC-1255> ;
        owl:versionInfo   "1:0" .

lexinfo:baseElement  a    owl:NamedIndividual , lexinfo:TermElement , owl:Thing ;
        rdfs:comment      "The root form of a word or term that is used as the formal dictionary entry for the term." ;
        rdfs:isDefinedBy  <http://www.lexinfo.net/ontology/2.0/lexinfo> ;
        rdfs:label        "baseElement" ;
        dc:creator        "Wright, Sue Ellen" ;
        dcr:datcat        <http://www.isocat.org/datcat/DC-290> ;
        owl:versionInfo   "1:0" .

lexinfo:relationNoun  a   lexinfo:NounPOS , owl:Thing , lexinfo:PartOfSpeech , owl:NamedIndividual ;
        rdfs:comment      "relation noun" ;
        rdfs:isDefinedBy  <http://www.lexinfo.net/ontology/2.0/lexinfo> ;
        rdfs:label        "relation noun" ;
        dc:creator        "Francopoulo, Gil" ;
        dcr:datcat        <http://www.isocat.org/datcat/DC-2226> ;
        owl:versionInfo   "1:0" .

lemon:synBehavior  a  owl:ObjectProperty .

lexinfo:positiveForm  a     owl:ObjectProperty ;
        rdfs:isDefinedBy    <http://www.lexinfo.net/ontology/2.0/lexinfo> ;
        rdfs:subPropertyOf  lexinfo:formPositivityVariant .

lexinfo:AdjectivePPFrame
        a                    owl:Class ;
        rdfs:isDefinedBy     <http://www.lexinfo.net/ontology/2.0/lexinfo> ;
        rdfs:subClassOf      lexinfo:AdjectiveFrame ;
        lexinfo:example      "he is RELATED TO her"@en ;
        owl:equivalentClass  [ a                   owl:Class ;
                               owl:intersectionOf  ( lexinfo:AdjectivePredicativeFrame lexinfo:PrepositionalFrame )
                             ] .

lexinfo:ReflexiveObject
        a                 owl:Class ;
        rdfs:isDefinedBy  <http://www.lexinfo.net/ontology/2.0/lexinfo> ;
        rdfs:subClassOf   lexinfo:Object .

lexinfo:clippedTermFor
        a                   owl:ObjectProperty ;
        rdfs:comment        "A linking element used to identify a relation between a clipped term and its full or expanded form." ;
        rdfs:isDefinedBy    <http://www.lexinfo.net/ontology/2.0/lexinfo> ;
        rdfs:label          "clippedTermFor" ;
        rdfs:subPropertyOf  lexinfo:derivedForm ;
        dc:creator          "Wright, Sue Ellen" ;
        dcr:datcat          <http://www.isocat.org/datcat/DC-130> ;
        owl:versionInfo     "1:0" .

lexinfo:etymology  a        owl:ObjectProperty ;
        rdfs:comment        "Information on the origin of a word and the development of its meaning." ;
        rdfs:isDefinedBy    <http://www.lexinfo.net/ontology/2.0/lexinfo> ;
        rdfs:label          "etymology" ;
        rdfs:subPropertyOf  lemon:definition ;
        dc:creator          "Wright, Sue Ellen" ;
        dcr:datcat          <http://www.isocat.org/datcat/DC-221> ;
        owl:versionInfo     "1:0" .

lexinfo:compound  a       owl:NamedIndividual , lexinfo:TermType , owl:Thing ;
        rdfs:comment      "A lexical unit that combines two or sometimes more different words, frequently such that the sense of the new lexical unit is not clearly derivable from the combination of its parts." ;
        rdfs:isDefinedBy  <http://www.lexinfo.net/ontology/2.0/lexinfo> ;
        rdfs:label        "compound" ;
        dc:creator        "Wright, Sue Ellen" ;
        dcr:datcat        <http://www.isocat.org/datcat/DC-352> ;
        owl:versionInfo   "1:0" .

lexinfo:prepositionalGerundClause
        a                   owl:ObjectProperty ;
        rdfs:isDefinedBy    <http://www.lexinfo.net/ontology/2.0/lexinfo> ;
        rdfs:subPropertyOf  lexinfo:clausalArg .

lexinfo:admittedTerm  a   owl:NamedIndividual , lexinfo:NormativeAuthorization , owl:Thing ;
        rdfs:comment      "A term rated according to the scale of a term acceptability rating as a synonym for a preferred term." ;
        rdfs:isDefinedBy  <http://www.lexinfo.net/ontology/2.0/lexinfo> ;
        rdfs:label        "admitted term" ;
        dc:creator        "Wright, Sue Ellen" ;
        dcr:datcat        <http://www.isocat.org/datcat/DC-377> ;
        owl:versionInfo   "1:0" .

lemon:representation  a  owl:DatatypeProperty .

lexinfo:properNoun  a     owl:NamedIndividual , lexinfo:NounPOS , lexinfo:PartOfSpeech , owl:Thing ;
        rdfs:comment      "Noun that is the name of a specific individual, place, or object." , "A noun or adjective denoting a single object." ;
        rdfs:isDefinedBy  <http://www.lexinfo.net/ontology/2.0/lexinfo> ;
        rdfs:label        "proper noun" , "properNoun" ;
        dc:creator        "Wright, Sue Ellen" , "Francopoulo, Gil" ;
        dcr:datcat        <http://www.isocat.org/datcat/DC-384> , <http://www.isocat.org/datcat/DC-1371> ;
        owl:versionInfo   "1:0" .

lexinfo:nominativeCase
        a                 owl:NamedIndividual , lexinfo:Case , owl:Thing ;
        rdfs:comment      "Case used to indicate the subject of a verb." ;
        rdfs:isDefinedBy  <http://www.lexinfo.net/ontology/2.0/lexinfo> ;
        rdfs:label        "nominative case" ;
        dc:creator        "Francopoulo, Gil" ;
        dcr:datcat        <http://www.isocat.org/datcat/DC-1331> ;
        owl:versionInfo   "1:0" .

lexinfo:TransitiveFrame
        a                    owl:Class ;
        rdfs:isDefinedBy     <http://www.lexinfo.net/ontology/2.0/lexinfo> ;
        rdfs:subClassOf      lexinfo:VerbFrame ;
        lexinfo:example      "the dog BIT the man"@en ;
        owl:equivalentClass  [ a                   owl:Class ;
                               owl:intersectionOf  ( lexinfo:VerbFrame [ a                owl:Restriction ;
                                                                         owl:cardinality  "1"^^xsd:nonNegativeInteger ;
                                                                         owl:onProperty   lexinfo:directObject
                                                                       ] [ a                owl:Restriction ;
                                                                           owl:cardinality  "1"^^xsd:nonNegativeInteger ;
                                                                           owl:onProperty   lexinfo:subject
                                                                         ] )
                             ] .

lexinfo:InfinitiveFrame
        a                    owl:Class ;
        rdfs:comment         "Infinitive frames take an infinitive clause as an argument"@en ;
        rdfs:isDefinedBy     <http://www.lexinfo.net/ontology/2.0/lexinfo> ;
        rdfs:subClassOf      lexinfo:VerbFrame ;
        owl:equivalentClass  [ a                   owl:Class ;
                               owl:intersectionOf  ( lexinfo:VerbFrame [ a                   owl:Restriction ;
                                                                         owl:minCardinality  "1"^^xsd:nonNegativeInteger ;
                                                                         owl:onProperty      lexinfo:infinitiveClause
                                                                       ] )
                             ] .

lexinfo:thirdPersonForm
        a                   owl:ObjectProperty ;
        rdfs:isDefinedBy    <http://www.lexinfo.net/ontology/2.0/lexinfo> ;
        rdfs:subPropertyOf  lexinfo:formPersonVariant .

lexinfo:Infix  a             owl:Class ;
        rdfs:isDefinedBy     <http://www.lexinfo.net/ontology/2.0/lexinfo> ;
        rdfs:subClassOf      lexinfo:Affix ;
        owl:equivalentClass  [ a                   owl:Restriction ;
                               owl:onProperty      lexinfo:termElement ;
                               owl:someValuesFrom  lexinfo:Infix
                             ] .

lexinfo:imperativeMoodForm
        a                   owl:ObjectProperty ;
        rdfs:isDefinedBy    <http://www.lexinfo.net/ontology/2.0/lexinfo> ;
        rdfs:subPropertyOf  lexinfo:formMoodVariant .

lexinfo:Object  a         owl:Class ;
        rdfs:isDefinedBy  <http://www.lexinfo.net/ontology/2.0/lexinfo> ;
        rdfs:subClassOf   lemon:Argument ;
        rdfs:subClassOf   [ a               owl:Restriction ;
                            owl:hasValue    false ;
                            owl:onProperty  lemon:optional
                          ] .

lexinfo:VerbFormMood  a   owl:Class ;
        rdfs:isDefinedBy  <http://www.lexinfo.net/ontology/2.0/lexinfo> ;
        rdfs:subClassOf   lexinfo:MorphosyntacticProperty .

terms:contributor  a  owl:AnnotationProperty .

lexinfo:Person  a         owl:Class ;
        rdfs:isDefinedBy  <http://www.lexinfo.net/ontology/2.0/lexinfo> ;
        rdfs:subClassOf   lexinfo:MorphosyntacticProperty .

lexinfo:ReflexiveFrame
        a                    owl:Class ;
        rdfs:isDefinedBy     <http://www.lexinfo.net/ontology/2.0/lexinfo> ;
        rdfs:subClassOf      lexinfo:VerbFrame ;
        owl:equivalentClass  [ a                   owl:Class ;
                               owl:intersectionOf  ( lexinfo:VerbFrame [ a                   owl:Restriction ;
                                                                         owl:onProperty      lexinfo:object ;
                                                                         owl:someValuesFrom  lexinfo:ReflexiveObject
                                                                       ] )
                             ] .

lexinfo:TransitiveInterrogativeInfinitiveFrame
        a                 owl:Class ;
        rdfs:isDefinedBy  <http://www.lexinfo.net/ontology/2.0/lexinfo> ;
        rdfs:subClassOf   lexinfo:InterrogativeInfinitiveFrame ;
        lexinfo:example   "he ASKED her [what to do]"@en .

lexinfo:abbreviationFor
        a                   owl:ObjectProperty ;
        rdfs:comment        "A linking element used to identify a relation between an abbreviation and its full or expanded form." ;
        rdfs:isDefinedBy    <http://www.lexinfo.net/ontology/2.0/lexinfo> ;
        rdfs:label          "abbreviationFor" ;
        rdfs:subPropertyOf  lexinfo:contractionFor ;
        dc:creator          "Wright, Sue Ellen" ;
        dcr:datcat          <http://www.isocat.org/datcat/DC-65> ;
        owl:versionInfo     "1:0" .

lexinfo:lativeCase  a     owl:NamedIndividual , lexinfo:Case , owl:Thing ;
        rdfs:comment      "Case which expresses motion to a location." ;
        rdfs:isDefinedBy  <http://www.lexinfo.net/ontology/2.0/lexinfo> ;
        rdfs:label        "lative case" ;
        dc:creator        "Francopoulo, Gil" ;
        dcr:datcat        <http://www.isocat.org/datcat/DC-1323> ;
        owl:versionInfo   "1:0" .

lexinfo:otherNumber  a    owl:NamedIndividual , lexinfo:Number , owl:Thing ;
        rdfs:comment      "Designation used to classify number-related grammatical information that can differ from the standard European classifications cited above." ;
        rdfs:isDefinedBy  <http://www.lexinfo.net/ontology/2.0/lexinfo> ;
        rdfs:label        "otherNumber" ;
        dc:creator        "Wright, Sue Ellen" ;
        dcr:datcat        <http://www.isocat.org/datcat/DC-256> ;
        owl:versionInfo   "1:0" .

lexinfo:partOfSpeech  a     owl:ObjectProperty ;
        rdfs:comment        "A category assigned to a word based on its grammatical and semantic properties." , "Term used to describe how a particular word is used in a sentence." ;
        rdfs:isDefinedBy    <http://www.lexinfo.net/ontology/2.0/lexinfo> ;
        rdfs:label          "part of speech" ;
        rdfs:range          lexinfo:PartOfSpeech ;
        rdfs:subPropertyOf  lexinfo:morphosyntacticProperty ;
        dc:creator          "Francopoulo, Gil" , "Wright, Sue Ellen" ;
        dcr:datcat          <http://www.isocat.org/datcat/DC-1345> , <http://www.isocat.org/datcat/DC-396> ;
        owl:versionInfo     "1:0" .

lexinfo:generalAdverb
        a                 owl:NamedIndividual , lexinfo:PartOfSpeech , lexinfo:AdverbPOS , owl:Thing ;
        rdfs:comment      "Adverb belonging to the general class of adverbs" ;
        rdfs:isDefinedBy  <http://www.lexinfo.net/ontology/2.0/lexinfo> ;
        rdfs:label        "general adverb" ;
        dc:creator        "Francopoulo, Gil" ;
        dcr:datcat        <http://www.isocat.org/datcat/DC-1435> ;
        owl:versionInfo   "1:0" .

lexinfo:infinitive  a     owl:NamedIndividual , lexinfo:VerbFormMood , owl:Thing ;
        rdfs:comment      "Mood cited as unmarked or base form." ;
        rdfs:isDefinedBy  <http://www.lexinfo.net/ontology/2.0/lexinfo> ;
        rdfs:label        "infinitive" ;
        dc:creator        "Francopoulo, Gil" ;
        dcr:datcat        <http://www.isocat.org/datcat/DC-1312> ;
        owl:versionInfo   "1:0" .

lexinfo:formDegreeVariant
        a                   owl:ObjectProperty ;
        rdfs:isDefinedBy    <http://www.lexinfo.net/ontology/2.0/lexinfo> ;
        rdfs:subPropertyOf  lemon:formVariant .

lexinfo:personalPronoun
        a                 lexinfo:PartOfSpeech , lexinfo:PronounPOS , owl:NamedIndividual , owl:Thing ;
        rdfs:comment      "Pronoun referring a person." ;
        rdfs:isDefinedBy  <http://www.lexinfo.net/ontology/2.0/lexinfo> ;
        rdfs:label        "personal pronoun" ;
        dc:creator        "Francopoulo, Gil" ;
        dcr:datcat        <http://www.isocat.org/datcat/DC-1463> ;
        owl:versionInfo   "1:0" .

dcr:datcat  a   owl:AnnotationProperty .

lexinfo:adposition  a     lexinfo:AdpositionPOS , owl:Thing , lexinfo:PartOfSpeech , owl:NamedIndividual ;
        rdfs:comment      "Part of speech that occurs before/inside/after a complement composed of a noun phrase, noun, pronoun or clause that functions as a noun phrase and form a single structure with the complement to express its grammatical and semantic relation to another unit." ;
        rdfs:isDefinedBy  <http://www.lexinfo.net/ontology/2.0/lexinfo> ;
        rdfs:label        "adposition" ;
        dc:creator        "Francopoulo, Gil" ;
        dcr:datcat        <http://www.isocat.org/datcat/DC-1231> ;
        owl:versionInfo   "1:0" .

lexinfo:gerundive  a      owl:NamedIndividual , lexinfo:VerbFormMood , owl:Thing ;
        rdfs:isDefinedBy  <http://www.lexinfo.net/ontology/2.0/lexinfo> .

lexinfo:possessive  a     owl:NamedIndividual , lexinfo:ReferentType , owl:Thing ;
        rdfs:comment      "Relative to the possession or association." ;
        rdfs:isDefinedBy  <http://www.lexinfo.net/ontology/2.0/lexinfo> ;
        rdfs:label        "possessive" ;
        dc:creator        "Francopoulo, Gil" ;
        dcr:datcat        <http://www.isocat.org/datcat/DC-1355> ;
        owl:versionInfo   "1:0" .

lexinfo:head  a             owl:ObjectProperty ;
        rdfs:isDefinedBy    <http://www.lexinfo.net/ontology/2.0/lexinfo> ;
        rdfs:subPropertyOf  lemon:lexicalVariant .

lexinfo:ReciprocalFrame
        a                    owl:Class ;
        rdfs:isDefinedBy     <http://www.lexinfo.net/ontology/2.0/lexinfo> ;
        rdfs:subClassOf      lexinfo:VerbFrame ;
        lexinfo:example      "mary and john MET"@en ;
        owl:equivalentClass  [ a                   owl:Class ;
                               owl:intersectionOf  ( lexinfo:VerbFrame [ a                   owl:Restriction ;
                                                                         owl:minCardinality  "2"^^xsd:nonNegativeInteger ;
                                                                         owl:onProperty      lexinfo:subject
                                                                       ] )
                             ] .

lexinfo:facetiousRegister
        a                 owl:NamedIndividual , lexinfo:Register , owl:Thing ;
        rdfs:isDefinedBy  <http://www.lexinfo.net/ontology/2.0/lexinfo> .

lexinfo:GerundOCFrame
        a                    owl:Class ;
        rdfs:isDefinedBy     <http://www.lexinfo.net/ontology/2.0/lexinfo> ;
        rdfs:subClassOf      lexinfo:GerundFrame ;
        owl:equivalentClass  [ a                   owl:Class ;
                               owl:intersectionOf  ( lexinfo:GerundFrame lexinfo:ObjectControl )
                             ] .

lexinfo:bound  a          owl:NamedIndividual , lexinfo:Cliticness , owl:Thing ;
        rdfs:comment      "Linked to a particular element." ;
        rdfs:isDefinedBy  <http://www.lexinfo.net/ontology/2.0/lexinfo> ;
        rdfs:label        "bound" ;
        dc:creator        "Francopoulo, Gil" ;
        dcr:datcat        <http://www.isocat.org/datcat/DC-1933> ;
        owl:versionInfo   "1:0" .

lexinfo:ArbitraryControl
        a                 owl:Class ;
        rdfs:comment      "Indicates either the subject or object of the main clause may be the omitted argument of the subclause"@en ;
        rdfs:isDefinedBy  <http://www.lexinfo.net/ontology/2.0/lexinfo> ;
        rdfs:subClassOf   lexinfo:Control .

lexinfo:AdverbialComplementFrame
        a                    owl:Class ;
        rdfs:isDefinedBy     <http://www.lexinfo.net/ontology/2.0/lexinfo> ;
        rdfs:subClassOf      lexinfo:VerbFrame ;
        owl:equivalentClass  [ a                   owl:Class ;
                               owl:intersectionOf  ( lexinfo:VerbFrame [ a                   owl:Restriction ;
                                                                         owl:minCardinality  "1"^^xsd:nonNegativeInteger ;
                                                                         owl:onProperty      lexinfo:predicativeAdverb
                                                                       ] )
                             ] .

lexinfo:standardizedTerm
        a                 owl:NamedIndividual , lexinfo:NormativeAuthorization , owl:Thing ;
        rdfs:comment      "A term that has been standardized by a standardizing body." ;
        rdfs:isDefinedBy  <http://www.lexinfo.net/ontology/2.0/lexinfo> ;
        rdfs:label        "standardized term" ;
        dc:creator        "Wright, Sue Ellen" ;
        dcr:datcat        <http://www.isocat.org/datcat/DC-375> ;
        owl:versionInfo   "1:0" .

lexinfo:Conjunction  a       owl:Class ;
        rdfs:isDefinedBy     <http://www.lexinfo.net/ontology/2.0/lexinfo> ;
        rdfs:subClassOf      lemon:Word ;
        owl:equivalentClass  [ a                   owl:Restriction ;
                               owl:onProperty      lexinfo:partOfSpeech ;
                               owl:someValuesFrom  lexinfo:ConjunctionPOS
                             ] .

lexinfo:meronymTerm  a      owl:ObjectProperty ;
        rdfs:comment        "Indicates this is a part of another concept"@en ;
        rdfs:isDefinedBy    <http://www.lexinfo.net/ontology/2.0/lexinfo> ;
        rdfs:label          "meronym"@en ;
        rdfs:subPropertyOf  lexinfo:partitiveRelation .

lemon:narrower  a  owl:ObjectProperty .

lexinfo:DeclarativeClause
        a                 owl:Class ;
        rdfs:comment      "A clause beginning with the declarative conjunction (\"that\" in English)"@en ;
        rdfs:isDefinedBy  <http://www.lexinfo.net/ontology/2.0/lexinfo> ;
        rdfs:subClassOf   lexinfo:ClausalArgument .

lexinfo:IndirectObject
        a                 owl:Class ;
        rdfs:isDefinedBy  <http://www.lexinfo.net/ontology/2.0/lexinfo> ;
        rdfs:subClassOf   lexinfo:Object .

lexinfo:interrogativeMultiplicativeNumeral
        a                 lexinfo:NumeralPOS , lexinfo:PartOfSpeech , owl:NamedIndividual , owl:Thing ;
        rdfs:comment      "An interrogative/relative word used to ask about the number of times something happened." ;
        rdfs:isDefinedBy  <http://www.lexinfo.net/ontology/2.0/lexinfo> ;
        rdfs:label        "interrogative multiplicative numeral" ;
        dc:creator        "Zeman, Dan" ;
        dcr:datcat        <http://www.isocat.org/datcat/DC-3021> ;
        owl:versionInfo   "1:0" .

lexinfo:PrepositionalObject
        a                    owl:Class ;
        rdfs:isDefinedBy     <http://www.lexinfo.net/ontology/2.0/lexinfo> ;
        rdfs:subClassOf      lexinfo:AdpositionalObject ;
        owl:equivalentClass  [ a                   owl:Class ;
                               owl:intersectionOf  ( lexinfo:AdpositionalObject [ a                   owl:Restriction ;
                                                                                  owl:onProperty      lemon:marker ;
                                                                                  owl:someValuesFrom  lexinfo:Preposition
                                                                                ] )
                             ] .

lexinfo:Negative  a       owl:Class ;
        rdfs:isDefinedBy  <http://www.lexinfo.net/ontology/2.0/lexinfo> ;
        rdfs:subClassOf   lexinfo:MorphosyntacticProperty .

lexinfo:preferredTerm
        a                 owl:NamedIndividual , lexinfo:NormativeAuthorization , owl:Thing ;
        rdfs:comment      "A term rated according to the scale of a term acceptability rating as the primary term for a given concept." ;
        rdfs:isDefinedBy  <http://www.lexinfo.net/ontology/2.0/lexinfo> ;
        rdfs:label        "preferred term" ;
        dc:creator        "Wright, Sue Ellen" ;
        dcr:datcat        <http://www.isocat.org/datcat/DC-376> ;
        owl:versionInfo   "1:0" .

lexinfo:AdjectiveAccusativePostPositiveFrame
        a                    owl:Class ;
        rdfs:isDefinedBy     <http://www.lexinfo.net/ontology/2.0/lexinfo> ;
        rdfs:subClassOf      lexinfo:AdjectivePostPositiveFrame ;
        lexinfo:example      "wird wurden unseren irrtum GEWAHR"@de ;
        owl:equivalentClass  [ a                   owl:Class ;
                               owl:intersectionOf  ( lexinfo:AdjectivePostPositiveFrame [ a                   owl:Restriction ;
                                                                                          owl:onProperty      lexinfo:postPositiveArg ;
                                                                                          owl:someValuesFrom  lexinfo:AccusativePostPositiveArgument
                                                                                        ] )
                             ] .

lexinfo:IntransitiveAdverbialComplementFrame
        a                    owl:Class ;
        rdfs:isDefinedBy     <http://www.lexinfo.net/ontology/2.0/lexinfo> ;
        rdfs:subClassOf      lexinfo:IntransitiveFrame ;
        lexinfo:example      "he SEEMED well"@en ;
        owl:equivalentClass  [ a                   owl:Class ;
                               owl:intersectionOf  ( lexinfo:IntransitiveFrame [ a                   owl:Restriction ;
                                                                                 owl:minCardinality  "1"^^xsd:nonNegativeInteger ;
                                                                                 owl:onProperty      lexinfo:predicativeAdverb
                                                                               ] )
                             ] .

lexinfo:genitiveCaseForm
        a                   owl:ObjectProperty ;
        rdfs:isDefinedBy    <http://www.lexinfo.net/ontology/2.0/lexinfo> ;
        rdfs:subPropertyOf  lexinfo:formCaseVariant .

lexinfo:Prefix  a            owl:Class ;
        rdfs:isDefinedBy     <http://www.lexinfo.net/ontology/2.0/lexinfo> ;
        rdfs:subClassOf      lexinfo:Affix ;
        owl:equivalentClass  [ a               owl:Restriction ;
                               owl:hasValue    lexinfo:prefix ;
                               owl:onProperty  lexinfo:termElement
                             ] .

lexinfo:illativeCase  a   owl:NamedIndividual , lexinfo:Case , owl:Thing ;
        rdfs:comment      "Case which expresses the meaning of 'motion into' or 'direction towards' the referent of the noun it marks." ;
        rdfs:isDefinedBy  <http://www.lexinfo.net/ontology/2.0/lexinfo> ;
        rdfs:label        "illative case" ;
        dc:creator        "Francopoulo, Gil" ;
        dcr:datcat        <http://www.isocat.org/datcat/DC-1303> ;
        owl:versionInfo   "1:0" .

lexinfo:technicalRegister
        a                 owl:NamedIndividual , owl:Thing , lexinfo:Register ;
        rdfs:comment      "The register appropriate to scientific texts or special languages." ;
        rdfs:isDefinedBy  <http://www.lexinfo.net/ontology/2.0/lexinfo> ;
        rdfs:label        "technical register" ;
        dc:creator        "Wright, Sue Ellen" , "Francopoulo, Gil" ;
        dcr:datcat        <http://www.isocat.org/datcat/DC-425> , <http://www.isocat.org/datcat/DC-1997> ;
        owl:versionInfo   "1:0" .

lexinfo:vocativeCase  a   owl:NamedIndividual , lexinfo:Case , owl:Thing ;
        rdfs:comment      "Case used to indicate direct address." ;
        rdfs:isDefinedBy  <http://www.lexinfo.net/ontology/2.0/lexinfo> ;
        rdfs:label        "vocative  case" ;
        dc:creator        "Francopoulo, Gil" ;
        dcr:datcat        <http://www.isocat.org/datcat/DC-1412> ;
        owl:versionInfo   "1:0" .

lexinfo:reciprocalPronoun
        a                 lexinfo:PronounPOS , owl:Thing , owl:NamedIndividual , lexinfo:PartOfSpeech ;
        rdfs:comment      "Pronoun expressing mutual relationship." ;
        rdfs:isDefinedBy  <http://www.lexinfo.net/ontology/2.0/lexinfo> ;
        rdfs:label        "reciprocal pronoun" ;
        dc:creator        "Francopoulo, Gil" ;
        dcr:datcat        <http://www.isocat.org/datcat/DC-1924> ;
        owl:versionInfo   "1:0" .

lexinfo:plainVerb  a      owl:NamedIndividual , lexinfo:PartOfSpeech , lexinfo:VerbPOS , owl:Thing ;
        rdfs:comment      "verb which has its own semantics" ;
        rdfs:isDefinedBy  <http://www.lexinfo.net/ontology/2.0/lexinfo> ;
        rdfs:label        "plain verb" ;
        dc:creator        "Francopoulo, Gil" ;
        dcr:datcat        <http://www.isocat.org/datcat/DC-3004> ;
        owl:versionInfo   "1:0" .

lexinfo:associativeRelation
        a                   owl:ObjectProperty ;
        rdfs:comment        "A relation between two concepts having a non-hierarchical thematic connection by virtue of experience." ;
        rdfs:isDefinedBy    <http://www.lexinfo.net/ontology/2.0/lexinfo> ;
        rdfs:label          "concept relation" ;
        rdfs:subPropertyOf  lexinfo:relatedTerm ;
        dc:creator          "Wright, Sue Ellen" ;
        dcr:datcat          <http://www.isocat.org/datcat/DC-88> ;
        owl:versionInfo     "1:0" .

lexinfo:PrepositionalAdjunct
        a                 owl:Class ;
        rdfs:isDefinedBy  <http://www.lexinfo.net/ontology/2.0/lexinfo> ;
        rdfs:subClassOf   lexinfo:Adjunct ;
        rdfs:subClassOf   [ a                   owl:Restriction ;
                            owl:onProperty      lemon:marker ;
                            owl:someValuesFrom  lexinfo:Preposition
                          ] .

lexinfo:rarelyUsed  a     lexinfo:Frequency , owl:Thing , owl:NamedIndividual ;
        rdfs:comment      "Said of a term that is almost never used." ;
        rdfs:isDefinedBy  <http://www.lexinfo.net/ontology/2.0/lexinfo> ;
        rdfs:label        "rarelyUsed" , "rarely used" ;
        dc:creator        "Wright, Sue Ellen" , "Francopoulo, Gil" ;
        dcr:datcat        <http://www.isocat.org/datcat/DC-1986> , <http://www.isocat.org/datcat/DC-236> ;
        owl:versionInfo   "1:0" .

lexinfo:translation  a      owl:ObjectProperty ;
        rdfs:isDefinedBy    <http://www.lexinfo.net/ontology/2.0/lexinfo> ;
        rdfs:subPropertyOf  lemon:senseRelation .

lexinfo:imperfective  a   owl:NamedIndividual , lexinfo:Aspect , owl:Thing ;
        rdfs:comment      "Imperfective aspect is an aspect that expresses an event or state, with respect to its internal structure, instead of expressing it as a simple whole." ;
        rdfs:isDefinedBy  <http://www.lexinfo.net/ontology/2.0/lexinfo> ;
        rdfs:label        "imperfective" ;
        dc:creator        "Francopoulo, Gil" ;
        dcr:datcat        <http://www.isocat.org/datcat/DC-1305> ;
        owl:versionInfo   "1:0" .

lexinfo:attributiveArg
        a                   owl:ObjectProperty ;
        rdfs:isDefinedBy    <http://www.lexinfo.net/ontology/2.0/lexinfo> ;
        rdfs:range          lexinfo:AttributiveArgument ;
        rdfs:subPropertyOf  lemon:synArg .

lexinfo:Interjection  a      owl:Class ;
        rdfs:isDefinedBy     <http://www.lexinfo.net/ontology/2.0/lexinfo> ;
        rdfs:subClassOf      lemon:Word ;
        owl:equivalentClass  [ a               owl:Restriction ;
                               owl:hasValue    lexinfo:interjection ;
                               owl:onProperty  lexinfo:partOfSpeech
                             ] .

lexinfo:Pronoun  a           owl:Class ;
        rdfs:isDefinedBy     <http://www.lexinfo.net/ontology/2.0/lexinfo> ;
        rdfs:subClassOf      lemon:Word ;
        owl:equivalentClass  [ a                   owl:Restriction ;
                               owl:onProperty      lexinfo:partOfSpeech ;
                               owl:someValuesFrom  lexinfo:PronounPOS
                             ] .

lexinfo:fullFormFor  a      owl:ObjectProperty ;
        rdfs:comment        "A linking element used to identify a relation between any full form of a term or lexical unit and its abbreviated form." ;
        rdfs:isDefinedBy    <http://www.lexinfo.net/ontology/2.0/lexinfo> ;
        rdfs:label          "fullFormFor" ;
        rdfs:subPropertyOf  lemon:lexicalVariant ;
        dc:creator          "Wright, Sue Ellen" ;
        dcr:datcat          <http://www.isocat.org/datcat/DC-241> ;
        owl:versionInfo     "1:0" .

lexinfo:openParenthesis
        a                 owl:Thing , lexinfo:PartOfSpeech , owl:NamedIndividual , lexinfo:SymbolPOS ;
        rdfs:comment      "Beginning of a pair of parenthesis." ;
        rdfs:isDefinedBy  <http://www.lexinfo.net/ontology/2.0/lexinfo> ;
        rdfs:label        "open parenthesis" ;
        dc:creator        "Francopoulo, Gil" ;
        dcr:datcat        <http://www.isocat.org/datcat/DC-1442> ;
        owl:versionInfo   "1:0" .

lexinfo:SententialFrame
        a                    owl:Class ;
        rdfs:comment         "Sentential frames take a clause as argument, no conjunction is used and the syntax of the clause is the same as a main clause"@en ;
        rdfs:isDefinedBy     <http://www.lexinfo.net/ontology/2.0/lexinfo> ;
        rdfs:subClassOf      lexinfo:VerbFrame ;
        owl:equivalentClass  [ a                   owl:Class ;
                               owl:intersectionOf  ( lexinfo:VerbFrame [ a                   owl:Restriction ;
                                                                         owl:minCardinality  "1"^^xsd:nonNegativeInteger ;
                                                                         owl:onProperty      lexinfo:sententialClause
                                                                       ] )
                             ] .

lexinfo:participleAdjective
        a                 lexinfo:PartOfSpeech , owl:NamedIndividual , lexinfo:AdjectivePOS , owl:Thing ;
        rdfs:comment      "Adjective based on a verb." ;
        rdfs:isDefinedBy  <http://www.lexinfo.net/ontology/2.0/lexinfo> ;
        rdfs:label        "participle adjective" ;
        dc:creator        "Francopoulo, Gil" ;
        dcr:datcat        <http://www.isocat.org/datcat/DC-1598> ;
        owl:versionInfo   "1:0" .

lexinfo:invertedComma
        a                 owl:NamedIndividual , owl:Thing , lexinfo:SymbolPOS , lexinfo:PartOfSpeech ;
        rdfs:comment      "Inverted comma." ;
        rdfs:isDefinedBy  <http://www.lexinfo.net/ontology/2.0/lexinfo> ;
        rdfs:label        "inverted comma" ;
        dc:creator        "Francopoulo, Gil" ;
        dcr:datcat        <http://www.isocat.org/datcat/DC-1443> ;
        owl:versionInfo   "1:0" .

lexinfo:definite  a       owl:NamedIndividual , lexinfo:Definiteness , owl:Thing ;
        rdfs:comment      "Value referring to the capacity of identification of an entity." ;
        rdfs:isDefinedBy  <http://www.lexinfo.net/ontology/2.0/lexinfo> ;
        rdfs:label        "definite" ;
        dc:creator        "Francopoulo, Gil" ;
        dcr:datcat        <http://www.isocat.org/datcat/DC-2004> ;
        owl:versionInfo   "1:0" .

lexinfo:PredicativeAdverb
        a                 owl:Class ;
        rdfs:isDefinedBy  <http://www.lexinfo.net/ontology/2.0/lexinfo> ;
        rdfs:subClassOf   lexinfo:Complement .

lexinfo:prepositionalObject
        a                   owl:ObjectProperty ;
        rdfs:isDefinedBy    <http://www.lexinfo.net/ontology/2.0/lexinfo> ;
        rdfs:range          lexinfo:PrepositionalObject ;
        rdfs:subPropertyOf  lexinfo:adpositionalObject .

lexinfo:formMoodVariant
        a                   owl:ObjectProperty ;
        rdfs:isDefinedBy    <http://www.lexinfo.net/ontology/2.0/lexinfo> ;
        rdfs:subPropertyOf  lemon:formVariant .

lexinfo:description  a      owl:ObjectProperty ;
        rdfs:comment        "A description in general prose text of the issues that are indicated by the context. The description field can occur at many different places in a component and profile." ;
        rdfs:isDefinedBy    <http://www.lexinfo.net/ontology/2.0/lexinfo> ;
        rdfs:label          "description" ;
        rdfs:subPropertyOf  lemon:definition ;
        dc:creator          "Wittenburg, Peter" ;
        dcr:datcat          <http://www.isocat.org/datcat/DC-2520> ;
        owl:versionInfo     "1:0" .

lexinfo:Mood  a           owl:Class ;
        rdfs:isDefinedBy  <http://www.lexinfo.net/ontology/2.0/lexinfo> ;
        rdfs:subClassOf   lexinfo:MorphosyntacticProperty .

lexinfo:IntransitiveDeclarativeFrame
        a                    owl:Class ;
        rdfs:isDefinedBy     <http://www.lexinfo.net/ontology/2.0/lexinfo> ;
        rdfs:subClassOf      lexinfo:DeclarativeFrame ;
        lexinfo:example      "i KNOW [that is a bad idea]"@en ;
        owl:equivalentClass  [ a                   owl:Class ;
                               owl:intersectionOf  ( lexinfo:DeclarativeFrame lexinfo:IntransitiveFrame )
                             ] .

lexinfo:ObjectControl
        a                 owl:Class ;
        rdfs:comment      "Indicates the object of the main clause is also the (omitted) object of the subclause"@en ;
        rdfs:isDefinedBy  <http://www.lexinfo.net/ontology/2.0/lexinfo> ;
        rdfs:subClassOf   lexinfo:Control .

lexinfo:usageNote  a        owl:ObjectProperty ;
        rdfs:comment        "A note containing information on the usage of the associated word or term." ;
        rdfs:isDefinedBy    <http://www.lexinfo.net/ontology/2.0/lexinfo> ;
        rdfs:label          "usage note" ;
        rdfs:subPropertyOf  lemon:definition ;
        dc:creator          "Wright, Sue Ellen" ;
        dcr:datcat          <http://www.isocat.org/datcat/DC-526> ;
        owl:versionInfo     "1:0" .

lexinfo:referentType  a     owl:ObjectProperty ;
        rdfs:comment        "Type of concrete object or concept (the referent) that an expression represents (the reference)." ;
        rdfs:isDefinedBy    <http://www.lexinfo.net/ontology/2.0/lexinfo> ;
        rdfs:label          "referent type" ;
        rdfs:range          lexinfo:ReferentType ;
        rdfs:subPropertyOf  lexinfo:morphosyntacticProperty ;
        dc:creator          "Francopoulo, Gil" ;
        dcr:datcat          <http://www.isocat.org/datcat/DC-1376> ;
        owl:versionInfo     "1:0" .

lexinfo:note  a             owl:ObjectProperty ;
        rdfs:comment        "A statement that provides further information on any part of a language resource entry." ;
        rdfs:isDefinedBy    <http://www.lexinfo.net/ontology/2.0/lexinfo> ;
        rdfs:label          "note" ;
        rdfs:subPropertyOf  lemon:definition ;
        dc:creator          "Wright, Sue Ellen" ;
        dcr:datcat          <http://www.isocat.org/datcat/DC-382> ;
        owl:versionInfo     "1:0" .

lexinfo:gloss  a            owl:ObjectProperty ;
        rdfs:comment        "In TEI: A phrase or word used to provide a gloss or definition for some other word or phrase.\nIn 1951: Any editorial comment." ;
        rdfs:isDefinedBy    <http://www.lexinfo.net/ontology/2.0/lexinfo> ;
        rdfs:label          "gloss" ;
        rdfs:subPropertyOf  lemon:definition ;
        dc:creator          "Wright, Sue Ellen" ;
        dcr:datcat          <http://www.isocat.org/datcat/DC-244> ;
        owl:versionInfo     "1:0" .

lexinfo:thirdPerson  a    owl:NamedIndividual , lexinfo:Person , owl:Thing ;
        rdfs:comment      "Third person deixis is deictic reference to a referent(s) not identified as the speaker or addressee." ;
        rdfs:isDefinedBy  <http://www.lexinfo.net/ontology/2.0/lexinfo> ;
        rdfs:label        "third person" ;
        dc:creator        "Francopoulo, Gil" ;
        dcr:datcat        <http://www.isocat.org/datcat/DC-1402> ;
        owl:versionInfo   "1:0" .

lexinfo:derivedForm  a      owl:ObjectProperty ;
        rdfs:isDefinedBy    <http://www.lexinfo.net/ontology/2.0/lexinfo> ;
        rdfs:subPropertyOf  lemon:lexicalVariant .

lexinfo:CommonNoun  a        owl:Class ;
        rdfs:isDefinedBy     <http://www.lexinfo.net/ontology/2.0/lexinfo> ;
        rdfs:subClassOf      lexinfo:Noun ;
        owl:equivalentClass  [ a               owl:Restriction ;
                               owl:hasValue    lexinfo:commonNoun ;
                               owl:onProperty  lexinfo:partOfSpeech
                             ] .

lexinfo:deficientVerb
        a                 owl:NamedIndividual , owl:Thing , lexinfo:VerbPOS , lexinfo:PartOfSpeech ;
        rdfs:comment      "verb lacking certain morphosyntactic properties" ;
        rdfs:isDefinedBy  <http://www.lexinfo.net/ontology/2.0/lexinfo> ;
        rdfs:label        "deficient verb" ;
        dc:creator        "Francopoulo, Gil" ;
        dcr:datcat        <http://www.isocat.org/datcat/DC-3007> ;
        owl:versionInfo   "1:0" .

lexinfo:translativeCase
        a                 owl:NamedIndividual , lexinfo:Case , owl:Thing ;
        rdfs:comment      "Case indicating that the referent of the noun, or the quality of the adjective, that it marks is the result of a process of change." ;
        rdfs:isDefinedBy  <http://www.lexinfo.net/ontology/2.0/lexinfo> ;
        rdfs:label        "translative case" ;
        dc:creator        "Francopoulo, Gil" ;
        dcr:datcat        <http://www.isocat.org/datcat/DC-1406> ;
        owl:versionInfo   "1:0" .

lexinfo:RaisableSubject
        a                    owl:Class ;
        rdfs:isDefinedBy     <http://www.lexinfo.net/ontology/2.0/lexinfo> ;
        rdfs:subClassOf      lexinfo:Subject ;
        owl:equivalentClass  [ a                   owl:Class ;
                               owl:intersectionOf  ( lemon:RaisableArgument lexinfo:Subject )
                             ] .

lexinfo:PPFrame  a           owl:Class ;
        rdfs:isDefinedBy     <http://www.lexinfo.net/ontology/2.0/lexinfo> ;
        rdfs:subClassOf      lexinfo:VerbFrame ;
        owl:equivalentClass  [ a                   owl:Class ;
                               owl:intersectionOf  ( lexinfo:PrepositionalFrame lexinfo:VerbFrame )
                             ] .

lexinfo:acronymFor  a       owl:ObjectProperty ;
        rdfs:comment        "A linking element used to identify a relation between an acronym and its full or expanded form." ;
        rdfs:isDefinedBy    <http://www.lexinfo.net/ontology/2.0/lexinfo> ;
        rdfs:label          "acronymFor" ;
        rdfs:subPropertyOf  lexinfo:contractionFor ;
        dc:creator          "Wright, Sue Ellen" ;
        dcr:datcat          <http://www.isocat.org/datcat/DC-66> ;
        owl:versionInfo     "1:0" .

lexinfo:Adverb  a            owl:Class ;
        rdfs:isDefinedBy     <http://www.lexinfo.net/ontology/2.0/lexinfo> ;
        rdfs:subClassOf      lemon:Word ;
        owl:equivalentClass  [ a                   owl:Restriction ;
                               owl:onProperty      lexinfo:partOfSpeech ;
                               owl:someValuesFrom  lexinfo:AdverbPOS
                             ] .

lemon:PropertyValue  a  owl:Class .

lexinfo:AdjectivePhrase
        a                    owl:Class ;
        rdfs:isDefinedBy     <http://www.lexinfo.net/ontology/2.0/lexinfo> ;
        rdfs:subClassOf      lemon:Phrase ;
        owl:equivalentClass  [ a                   owl:Class ;
                               owl:intersectionOf  ( lemon:Phrase [ a                   owl:Restriction ;
                                                                    owl:onProperty      lexinfo:head ;
                                                                    owl:someValuesFrom  lexinfo:Adjective
                                                                  ] )
                             ] .

lexinfo:Noun  a              owl:Class ;
        rdfs:isDefinedBy     <http://www.lexinfo.net/ontology/2.0/lexinfo> ;
        rdfs:subClassOf      lemon:Word ;
        rdfs:subClassOf      [ a                  owl:Restriction ;
                               owl:allValuesFrom  lexinfo:NounFrame ;
                               owl:onProperty     lemon:synBehavior
                             ] ;
        owl:equivalentClass  [ a                   owl:Restriction ;
                               owl:onProperty      lexinfo:partOfSpeech ;
                               owl:someValuesFrom  lexinfo:NounPOS
                             ] .

lexinfo:GenitiveObject
        a                    owl:Class ;
        rdfs:isDefinedBy     <http://www.lexinfo.net/ontology/2.0/lexinfo> ;
        rdfs:subClassOf      lexinfo:Object ;
        owl:equivalentClass  [ a               owl:Restriction ;
                               owl:hasValue    lexinfo:genitiveCase ;
                               owl:onProperty  lemon:marker
                             ] .

lemon:equivalent  a  owl:ObjectProperty .

lemon:Part  a   owl:Class .

lexinfo:infix  a          owl:NamedIndividual , lexinfo:TermElement , owl:Thing ;
        rdfs:isDefinedBy  <http://www.lexinfo.net/ontology/2.0/lexinfo> .

lexinfo:AdjectiveImpersonalFrame
        a                    owl:Class ;
        rdfs:isDefinedBy     <http://www.lexinfo.net/ontology/2.0/lexinfo> ;
        rdfs:subClassOf      lexinfo:AdjectiveFrame ;
        lexinfo:example      "es ist mir HEISS"@de ;
        owl:equivalentClass  [ a                   owl:Class ;
                               owl:intersectionOf  ( lexinfo:AdjectiveFrame [ a                   owl:Restriction ;
                                                                              owl:minCardinality  "1"^^xsd:nonNegativeInteger ;
                                                                              owl:onProperty      lexinfo:object
                                                                            ] [ a                owl:Restriction ;
                                                                                owl:cardinality  "0"^^xsd:nonNegativeInteger ;
                                                                                owl:onProperty   lexinfo:copulativeSubject
                                                                              ] )
                             ] .

lexinfo:romanization  a     owl:DatatypeProperty ;
        rdfs:comment        "Transcription or transliteration from non-Latin script into Latin script." ;
        rdfs:isDefinedBy    <http://www.lexinfo.net/ontology/2.0/lexinfo> ;
        rdfs:label          "romanization" ;
        rdfs:range          xsd:string ;
        rdfs:subPropertyOf  lemon:representation ;
        dc:creator          "Francopoulo, Gil" ;
        dcr:datcat          <http://www.isocat.org/datcat/DC-1873> ;
        owl:versionInfo     "1:0" .

lexinfo:transcribedForm
        a                 owl:NamedIndividual , lexinfo:TermType , owl:Thing ;
        rdfs:comment      "A form of a term or lexeme resulting from an operation whereby the characters of one writing system are represented by characters from another writing system, taking into account the pronunciation of the characters converted." ;
        rdfs:isDefinedBy  <http://www.lexinfo.net/ontology/2.0/lexinfo> ;
        rdfs:label        "transcribed form" ;
        dc:creator        "Wright, Sue Ellen" ;
        dcr:datcat        <http://www.isocat.org/datcat/DC-322> ;
        owl:versionInfo   "1:0" .

lexinfo:contractionFor
        a                   owl:ObjectProperty ;
        rdfs:comment        "The full form that corresponds to a contracted form." ;
        rdfs:isDefinedBy    <http://www.lexinfo.net/ontology/2.0/lexinfo> ;
        rdfs:label          "contractionFor" ;
        rdfs:subPropertyOf  lexinfo:derivedForm ;
        dc:creator          "Wright, Sue Ellen" ;
        dcr:datcat          <http://www.isocat.org/datcat/DC-157> ;
        owl:versionInfo     "1:0" .

lexinfo:TransitiveNominalComplementFrame
        a                    owl:Class ;
        rdfs:isDefinedBy     <http://www.lexinfo.net/ontology/2.0/lexinfo> ;
        rdfs:subClassOf      lexinfo:TransitiveFrame ;
        lexinfo:example      "they ELECTED him president"@en ;
        owl:equivalentClass  [ a                   owl:Class ;
                               owl:intersectionOf  ( lexinfo:NominalComplementFrame lexinfo:TransitiveFrame )
                             ] .

lexinfo:postposition  a   owl:NamedIndividual , owl:Thing , lexinfo:AdpositionPOS , lexinfo:PartOfSpeech ;
        rdfs:comment      "Adposition that appears at the end of the noun phrase." ;
        rdfs:isDefinedBy  <http://www.lexinfo.net/ontology/2.0/lexinfo> ;
        rdfs:label        "postposition" ;
        dc:creator        "Francopoulo, Gil" ;
        dcr:datcat        <http://www.isocat.org/datcat/DC-1360> ;
        owl:versionInfo   "1:0" .

lexinfo:ironicRegister
        a                 owl:NamedIndividual , lexinfo:Register , owl:Thing ;
        rdfs:isDefinedBy  <http://www.lexinfo.net/ontology/2.0/lexinfo> .

lexinfo:Subject  a        owl:Class ;
        rdfs:isDefinedBy  <http://www.lexinfo.net/ontology/2.0/lexinfo> ;
        rdfs:subClassOf   lemon:Argument ;
        rdfs:subClassOf   [ a               owl:Restriction ;
                            owl:hasValue    false ;
                            owl:onProperty  lemon:optional
                          ] .

lexinfo:AdpositionPOS
        a                 owl:Class ;
        rdfs:isDefinedBy  <http://www.lexinfo.net/ontology/2.0/lexinfo> ;
        rdfs:subClassOf   lexinfo:PartOfSpeech .

lexinfo:Adjunct  a        owl:Class ;
        rdfs:isDefinedBy  <http://www.lexinfo.net/ontology/2.0/lexinfo> ;
        rdfs:subClassOf   lemon:Argument ;
        rdfs:subClassOf   [ a               owl:Restriction ;
                            owl:hasValue    true ;
                            owl:onProperty  lemon:optional
                          ] .

terms:creator  a  owl:AnnotationProperty .

lexinfo:subject  a          owl:ObjectProperty ;
        rdfs:comment        "relation between a phrase and a verb, that represents the person or thing that performs the action or about which something is stated" ;
        rdfs:isDefinedBy    <http://www.lexinfo.net/ontology/2.0/lexinfo> ;
        rdfs:label          "subject" ;
        rdfs:range          lexinfo:Subject ;
        rdfs:subPropertyOf  lemon:synArg ;
        dcr:datcat          <http://www.isocat.org/datcat/DC-2261> .

lexinfo:otherAnimacy  a   owl:NamedIndividual , lexinfo:Animacy , owl:Thing ;
        rdfs:comment      "Perceived as related to animacy, but without specific reference to the previous items." ;
        rdfs:isDefinedBy  <http://www.lexinfo.net/ontology/2.0/lexinfo> ;
        rdfs:label        "otherAnimacy" , "other animacy" ;
        dc:creator        "Wright, Sue Ellen" , "Francopoulo, Gil" ;
        dcr:datcat        <http://www.isocat.org/datcat/DC-1953> , <http://www.isocat.org/datcat/DC-81> ;
        owl:versionInfo   "1:0" .

lexinfo:compoundPreposition
        a                 owl:Thing , lexinfo:AdpositionPOS , owl:NamedIndividual , lexinfo:PartOfSpeech ;
        rdfs:comment      "Preposition that is a aggregation of words" ;
        rdfs:isDefinedBy  <http://www.lexinfo.net/ontology/2.0/lexinfo> ;
        rdfs:label        "compound preposition" ;
        dc:creator        "Francopoulo, Gil" ;
        dcr:datcat        <http://www.isocat.org/datcat/DC-1934> ;
        owl:versionInfo   "1:0" .

lexinfo:infinitiveParticle
        a                 owl:Thing , owl:NamedIndividual , lexinfo:PartOfSpeech , lexinfo:ParticlePOS ;
        rdfs:comment      "Particle used to express infinitive." ;
        rdfs:isDefinedBy  <http://www.lexinfo.net/ontology/2.0/lexinfo> ;
        rdfs:label        "infinitive particle" ;
        dc:creator        "Francopoulo, Gil" ;
        dcr:datcat        <http://www.isocat.org/datcat/DC-1896> ;
        owl:versionInfo   "1:0" .

lexinfo:participleFormOf
        a                   owl:ObjectProperty ;
        rdfs:comment        "Indicates that one lexical entry is the participle form of another, e.g., the adjective 'reassuring' is the participle of 'to reassure'"@en ;
        rdfs:isDefinedBy    <http://www.lexinfo.net/ontology/2.0/lexinfo> ;
        rdfs:subPropertyOf  lexinfo:derivedForm .

lexinfo:predicativeAdjunct
        a                   owl:ObjectProperty ;
        rdfs:isDefinedBy    <http://www.lexinfo.net/ontology/2.0/lexinfo> ;
        rdfs:range          lexinfo:Adjunct ;
        rdfs:subPropertyOf  lexinfo:adjunct .

lexinfo:positive  a       owl:NamedIndividual , lexinfo:Degree , owl:Thing ;
        rdfs:comment      "Value used in a comparison relationship when no comparison is involved." ;
        rdfs:isDefinedBy  <http://www.lexinfo.net/ontology/2.0/lexinfo> ;
        rdfs:label        "positive" ;
        dc:creator        "Francopoulo, Gil" ;
        dcr:datcat        <http://www.isocat.org/datcat/DC-1420> ;
        owl:versionInfo   "1:0" .

lexinfo:Postposition  a      owl:Class ;
        rdfs:isDefinedBy     <http://www.lexinfo.net/ontology/2.0/lexinfo> ;
        rdfs:subClassOf      lexinfo:Adposition ;
        owl:equivalentClass  [ a               owl:Restriction ;
                               owl:hasValue    lexinfo:postposition ;
                               owl:onProperty  lexinfo:partOfSpeech
                             ] .

lexinfo:weakPersonalPronoun
        a                 lexinfo:PartOfSpeech , lexinfo:PronounPOS , owl:Thing , owl:NamedIndividual ;
        rdfs:comment      "Personal pronoun that cannot occupy the position after a preposition and/or reinforce a strong personal pronoun." ;
        rdfs:isDefinedBy  <http://www.lexinfo.net/ontology/2.0/lexinfo> ;
        rdfs:label        "weak personal pronoun" ;
        dc:creator        "Francopoulo, Gil" ;
        dcr:datcat        <http://www.isocat.org/datcat/DC-1414> ;
        owl:versionInfo   "1:0" .

lexinfo:tabooRegister
        a                 owl:NamedIndividual , lexinfo:Register , owl:Thing ;
        rdfs:isDefinedBy  <http://www.lexinfo.net/ontology/2.0/lexinfo> .

lexinfo:NounFrame  a      owl:Class ;
        rdfs:isDefinedBy  <http://www.lexinfo.net/ontology/2.0/lexinfo> ;
        rdfs:subClassOf   lemon:Frame .

lexinfo:formCaseVariant
        a                   owl:ObjectProperty ;
        rdfs:isDefinedBy    <http://www.lexinfo.net/ontology/2.0/lexinfo> ;
        rdfs:subPropertyOf  lemon:formVariant .

lexinfo:terminativeCase
        a                 owl:NamedIndividual , lexinfo:Case , owl:Thing ;
        rdfs:comment      "Case that indicates to what or where something ends." ;
        rdfs:isDefinedBy  <http://www.lexinfo.net/ontology/2.0/lexinfo> ;
        rdfs:label        "terminative case" ;
        dc:creator        "Francopoulo, Gil" ;
        dcr:datcat        <http://www.isocat.org/datcat/DC-1401> ;
        owl:versionInfo   "1:0" .

lexinfo:possessiveInfinitiveClause
        a                   owl:ObjectProperty ;
        rdfs:isDefinedBy    <http://www.lexinfo.net/ontology/2.0/lexinfo> ;
        rdfs:subPropertyOf  lexinfo:clausalArg .

lexinfo:SubjectlessIntransitiveFrame
        a                    owl:Class ;
        rdfs:isDefinedBy     <http://www.lexinfo.net/ontology/2.0/lexinfo> ;
        rdfs:subClassOf      lexinfo:SubjectlessFrame ;
        lexinfo:example      "mir SCHWINDELT"@de ;
        owl:equivalentClass  [ a                   owl:Class ;
                               owl:intersectionOf  ( lexinfo:SubjectlessFrame [ a                owl:Restriction ;
                                                                                owl:cardinality  "1"^^xsd:nonNegativeInteger ;
                                                                                owl:onProperty   lexinfo:indirectObject
                                                                              ] )
                             ] .

lexinfo:indefiniteOrdinalNumeral
        a                 lexinfo:NumeralPOS , owl:NamedIndividual , owl:Thing , lexinfo:PartOfSpeech ;
        rdfs:comment      "A word used to indicate imprecise rank of an object in a sequence." ;
        rdfs:isDefinedBy  <http://www.lexinfo.net/ontology/2.0/lexinfo> ;
        rdfs:label        "indefinite ordinal numeral" ;
        dc:creator        "Zeman, Dan" ;
        dcr:datcat        <http://www.isocat.org/datcat/DC-3025> ;
        owl:versionInfo   "1:0" .

lexinfo:yes  a            lexinfo:Negative , owl:NamedIndividual , owl:Thing , lexinfo:Cliticness ;
        rdfs:comment      "Positive value" ;
        rdfs:isDefinedBy  <http://www.lexinfo.net/ontology/2.0/lexinfo> ;
        rdfs:label        "yes" ;
        dc:creator        "Francopoulo, Gil" ;
        dcr:datcat        <http://www.isocat.org/datcat/DC-1904> ;
        owl:versionInfo   "1:0" .

lemon:property  a  owl:ObjectProperty .

lexinfo:Complement  a     owl:Class ;
        rdfs:isDefinedBy  <http://www.lexinfo.net/ontology/2.0/lexinfo> ;
        rdfs:subClassOf   lemon:Argument .

lexinfo:prolativeCase
        a                 owl:NamedIndividual , lexinfo:Case , owl:Thing ;
        rdfs:comment      "Case for a noun or a pronoun that expresses motion within a place or a period of time needed for an event." ;
        rdfs:isDefinedBy  <http://www.lexinfo.net/ontology/2.0/lexinfo> ;
        rdfs:label        "prolative case" ;
        dc:creator        "Francopoulo, Gil" ;
        dcr:datcat        <http://www.isocat.org/datcat/DC-1368> ;
        owl:versionInfo   "1:0" .

lexinfo:outdatedForm  a   owl:NamedIndividual , lexinfo:TemporalQualifier , owl:Thing ;
        rdfs:comment      "A term or lexeme that has fallen from fashion, but the meaning of which is readily recognizable." ;
        rdfs:isDefinedBy  <http://www.lexinfo.net/ontology/2.0/lexinfo> ;
        rdfs:label        "outdated form" ;
        dc:creator        "Wright, Sue Ellen" ;
        dcr:datcat        <http://www.isocat.org/datcat/DC-505> ;
        owl:versionInfo   "1:0" .

lexinfo:NormativeAuthorization
        a                 owl:Class ;
        rdfs:isDefinedBy  <http://www.lexinfo.net/ontology/2.0/lexinfo> ;
        rdfs:subClassOf   lemon:SenseContext .

lexinfo:adjective-i  a            lexinfo:AdjectivePOS , owl:NamedIndividual ;
        rdfs:comment              "Deverbal adjective in Japanese ending with the '-i' suffix in dictionary form"@en ;
        lexinfo:languageSpecific  "ja" .

lexinfo:possessivePronoun
        a                 owl:Thing , owl:NamedIndividual , lexinfo:PronounPOS , lexinfo:PartOfSpeech ;
        rdfs:comment      "Pronoun that expresses ownership and relationships like ownership, such as kinship, and other forms of association." ;
        rdfs:isDefinedBy  <http://www.lexinfo.net/ontology/2.0/lexinfo> ;
        rdfs:label        "possessive pronoun" ;
        dc:creator        "Francopoulo, Gil" ;
        dcr:datcat        <http://www.isocat.org/datcat/DC-1359> ;
        owl:versionInfo   "1:0" .

lexinfo:particle  a       lexinfo:PartOfSpeech , lexinfo:ParticlePOS , owl:NamedIndividual , owl:Thing ;
        rdfs:comment      "Word that does not belong to one of the main classes of words, is invariable in form, and typically has grammatical or pragmatic meaning." ;
        rdfs:isDefinedBy  <http://www.lexinfo.net/ontology/2.0/lexinfo> ;
        rdfs:label        "particle" ;
        dc:creator        "Francopoulo, Gil" ;
        dcr:datcat        <http://www.isocat.org/datcat/DC-1342> ;
        owl:versionInfo   "1:0" .

lexinfo:sublativeCase
        a                 owl:NamedIndividual , lexinfo:Case , owl:Thing ;
        rdfs:comment      "Case for a move of something to the surface of another object." ;
        rdfs:isDefinedBy  <http://www.lexinfo.net/ontology/2.0/lexinfo> ;
        rdfs:label        "sublative case" ;
        dc:creator        "Francopoulo, Gil" ;
        dcr:datcat        <http://www.isocat.org/datcat/DC-1392> ;
        owl:versionInfo   "1:0" .

lexinfo:fullArticle  a    owl:NamedIndividual , lexinfo:Definiteness , owl:Thing ;
        rdfs:comment      "For definiteness, when a specific form is the syntactic subject of the clause." ;
        rdfs:isDefinedBy  <http://www.lexinfo.net/ontology/2.0/lexinfo> ;
        rdfs:label        "full article" ;
        dc:creator        "Francopoulo, Gil" ;
        dcr:datcat        <http://www.isocat.org/datcat/DC-1928> ;
        owl:versionInfo   "1:0" .

lexinfo:approximate  a      owl:ObjectProperty ;
        rdfs:comment        "Property used to qualify something similar but not exactly the same" ;
        rdfs:isDefinedBy    <http://www.lexinfo.net/ontology/2.0/lexinfo> ;
        rdfs:label          "approximate" ;
        rdfs:subPropertyOf  lemon:senseRelation ;
        dc:creator          "Francopoulo, Gil" ;
        dcr:datcat          <http://www.isocat.org/datcat/DC-2206> ;
        owl:versionInfo     "1:0" .

lexinfo:homonym  a          owl:ObjectProperty ;
        rdfs:comment        "A word that is pronounced like another word and that can be spelled the same way (homograph) or can merely sound the same (homophone)." , "Word that sounds the same and is written the same as another word but is different in meaning." ;
        rdfs:isDefinedBy    <http://www.lexinfo.net/ontology/2.0/lexinfo> ;
        rdfs:label          "homonym" ;
        rdfs:subPropertyOf  lemon:lexicalVariant ;
        dc:creator          "Francopoulo, Gil" , "Wright, Sue Ellen" ;
        dcr:datcat          <http://www.isocat.org/datcat/DC-262> , <http://www.isocat.org/datcat/DC-1301> ;
        owl:versionInfo     "1:0" .

lexinfo:DitransitiveFrame
        a                    owl:Class ;
        rdfs:isDefinedBy     <http://www.lexinfo.net/ontology/2.0/lexinfo> ;
        rdfs:subClassOf      lexinfo:VerbFrame ;
        lexinfo:example      "i GAVE him it"@en , "mein vater SCHREIBT ihr einen brief"@de ;
        owl:equivalentClass  [ a                   owl:Class ;
                               owl:intersectionOf  ( lexinfo:VerbFrame [ a                owl:Restriction ;
                                                                         owl:cardinality  "1"^^xsd:nonNegativeInteger ;
                                                                         owl:onProperty   lexinfo:directObject
                                                                       ] [ a                owl:Restriction ;
                                                                           owl:cardinality  "1"^^xsd:nonNegativeInteger ;
                                                                           owl:onProperty   lexinfo:indirectObject
                                                                         ] [ a                owl:Restriction ;
                                                                             owl:cardinality  "1"^^xsd:nonNegativeInteger ;
                                                                             owl:onProperty   lexinfo:subject
                                                                           ] )
                             ] .

lexinfo:morphologicalElement
        a                 owl:NamedIndividual , lexinfo:TermElement , owl:Thing ;
        rdfs:comment      "Unit resulting from the division of words into their smallest meaningful parts.\nNote: moved to lexeme element from being an independent element; note that this is currently an independent element in 12620" ;
        rdfs:isDefinedBy  <http://www.lexinfo.net/ontology/2.0/lexinfo> ;
        rdfs:label        "morphological element" ;
        dc:creator        "Wright, Sue Ellen" ;
        dcr:datcat        <http://www.isocat.org/datcat/DC-300> ;
        owl:versionInfo   "1:0" .

lexinfo:IntransitivePPDeclarativeFrame
        a                    owl:Class ;
        rdfs:isDefinedBy     <http://www.lexinfo.net/ontology/2.0/lexinfo> ;
        rdfs:subClassOf      lexinfo:DeclarativeFrame ;
        lexinfo:example      "the SUGGESTED to him [that he should go]"@en ;
        owl:equivalentClass  [ a                   owl:Class ;
                               owl:intersectionOf  ( lexinfo:DeclarativeFrame lexinfo:IntransitivePPFrame )
                             ] .

lexinfo:prepositionalAdverb
        a                 lexinfo:AdverbPOS , owl:Thing , lexinfo:PartOfSpeech , owl:NamedIndividual ;
        rdfs:comment      "adverb which is very similar in its form to a preposition" ;
        rdfs:isDefinedBy  <http://www.lexinfo.net/ontology/2.0/lexinfo> ;
        rdfs:label        "prepositional adverb" ;
        dc:creator        "Francopoulo, Gil" ;
        dcr:datcat        <http://www.isocat.org/datcat/DC-3000> ;
        owl:versionInfo   "1:0" .

lemon:separator  a        owl:DatatypeProperty ;
        rdfs:isDefinedBy  <http://www.lexinfo.net/ontology/2.0/lexinfo> ;
        dcr:datcat        <http://www.isocat.org/datcat/DC-1863> .

lexinfo:coordinatingConjunction
        a                 owl:NamedIndividual , owl:Thing , lexinfo:PartOfSpeech , lexinfo:ConjunctionPOS ;
        rdfs:comment      "Conjunction that links constituents." ;
        rdfs:isDefinedBy  <http://www.lexinfo.net/ontology/2.0/lexinfo> ;
        rdfs:label        "coordinating conjunction" ;
        dc:creator        "Francopoulo, Gil" ;
        dcr:datcat        <http://www.isocat.org/datcat/DC-1262> ;
        owl:versionInfo   "1:0" .

lexinfo:demonstrativeDeterminer
        a                 lexinfo:PartOfSpeech , owl:Thing , lexinfo:DeterminerPOS , owl:NamedIndividual ;
        rdfs:comment      "Determiner used to point to an entity in the situation or elsewhere in a sentence." ;
        rdfs:isDefinedBy  <http://www.lexinfo.net/ontology/2.0/lexinfo> ;
        rdfs:label        "demonstrative determiner" ;
        dc:creator        "Francopoulo, Gil" ;
        dcr:datcat        <http://www.isocat.org/datcat/DC-1269> ;
        owl:versionInfo   "1:0" .

lexinfo:proverb  a        owl:NamedIndividual , lexinfo:TermType , owl:Thing ;
        rdfs:comment      "A brief popular axiom or saying." ;
        rdfs:isDefinedBy  <http://www.lexinfo.net/ontology/2.0/lexinfo> ;
        rdfs:label        "proverb" ;
        dc:creator        "Wright, Sue Ellen" ;
        dcr:datcat        <http://www.isocat.org/datcat/DC-353> ;
        owl:versionInfo   "1:0" .

lexinfo:PredicativeAdjective
        a                 owl:Class ;
        rdfs:isDefinedBy  <http://www.lexinfo.net/ontology/2.0/lexinfo> ;
        rdfs:subClassOf   lexinfo:Complement .

lexinfo:obsoleteForm  a   owl:NamedIndividual , lexinfo:TemporalQualifier , owl:Thing ;
        rdfs:comment      "A term or lexeme which is no longer in common use." ;
        rdfs:isDefinedBy  <http://www.lexinfo.net/ontology/2.0/lexinfo> ;
        rdfs:label        "obsolete form" ;
        dc:creator        "Wright, Sue Ellen" ;
        dcr:datcat        <http://www.isocat.org/datcat/DC-506> ;
        owl:versionInfo   "1:0" .

lexinfo:mainVerb  a       owl:Thing , lexinfo:VerbPOS , owl:NamedIndividual , lexinfo:PartOfSpeech ;
        rdfs:comment      "Main verb in contrast to a modal or an auxiliary." ;
        rdfs:isDefinedBy  <http://www.lexinfo.net/ontology/2.0/lexinfo> ;
        rdfs:label        "main verb" ;
        dc:creator        "Francopoulo, Gil" ;
        dcr:datcat        <http://www.isocat.org/datcat/DC-1400> ;
        owl:versionInfo   "1:0" .

lexinfo:sententialClause
        a                   owl:ObjectProperty ;
        rdfs:isDefinedBy    <http://www.lexinfo.net/ontology/2.0/lexinfo> ;
        rdfs:subPropertyOf  lexinfo:clausalArg .

lexinfo:dualNumberForm
        a                   owl:ObjectProperty ;
        rdfs:isDefinedBy    <http://www.lexinfo.net/ontology/2.0/lexinfo> ;
        rdfs:subPropertyOf  lexinfo:formNumberVariant .

lemon:formVariant  a  owl:ObjectProperty .

lexinfo:ConjunctionPOS
        a                 owl:Class ;
        rdfs:isDefinedBy  <http://www.lexinfo.net/ontology/2.0/lexinfo> ;
        rdfs:subClassOf   lexinfo:PartOfSpeech .

lexinfo:AdjectiveSuperlativeFrame
        a                    owl:Class ;
        rdfs:isDefinedBy     <http://www.lexinfo.net/ontology/2.0/lexinfo> ;
        rdfs:subClassOf      lexinfo:AdjectiveFrame ;
        lexinfo:example      "tokyo is the BIGGEST of all metropoles"@en ;
        owl:equivalentClass  [ a                   owl:Class ;
                               owl:intersectionOf  ( lexinfo:AdjectiveFrame [ a                   owl:Restriction ;
                                                                              owl:minCardinality  "1"^^xsd:nonNegativeInteger ;
                                                                              owl:onProperty      lexinfo:superlativeAdjunct
                                                                            ] [ a                owl:Restriction ;
                                                                                owl:cardinality  "1"^^xsd:nonNegativeInteger ;
                                                                                owl:onProperty   lexinfo:copulativeSubject
                                                                              ] )
                             ] .

lexinfo:clippedTerm  a    lexinfo:AbbreviatedForm , owl:NamedIndividual , lexinfo:TermType , owl:Thing ;
        rdfs:comment      "An abbreviation formed by truncating a part of a simple term." ;
        rdfs:isDefinedBy  <http://www.lexinfo.net/ontology/2.0/lexinfo> ;
        rdfs:label        "clipped term" ;
        dc:creator        "Wright, Sue Ellen" ;
        dcr:datcat        <http://www.isocat.org/datcat/DC-335> ;
        owl:versionInfo   "1:0" .

lexinfo:AdjectivePredicativeFrame
        a                    owl:Class ;
        rdfs:isDefinedBy     <http://www.lexinfo.net/ontology/2.0/lexinfo> ;
        rdfs:subClassOf      lexinfo:AdjectiveFrame ;
        lexinfo:example      "he is HAPPY"@en ;
        owl:equivalentClass  [ a                   owl:Class ;
                               owl:intersectionOf  ( lexinfo:AdjectiveFrame [ a                owl:Restriction ;
                                                                              owl:cardinality  "1"^^xsd:nonNegativeInteger ;
                                                                              owl:onProperty   lexinfo:copulativeSubject
                                                                            ] )
                             ] .

lexinfo:IntransitiveInterrogativeInfinitiveFrame
        a                    owl:Class ;
        rdfs:isDefinedBy     <http://www.lexinfo.net/ontology/2.0/lexinfo> ;
        rdfs:subClassOf      lexinfo:InterrogativeInfinitiveFrame ;
        lexinfo:example      "he ASKED [what to do]"@en ;
        owl:equivalentClass  [ a                   owl:Class ;
                               owl:intersectionOf  ( lexinfo:InterrogativeInfinitiveFrame lexinfo:IntransitiveFrame )
                             ] .

lemon:Word  a   owl:Class .

lexinfo:superlative  a    owl:NamedIndividual , lexinfo:Degree , owl:Thing ;
        rdfs:comment      "Value used in a comparison between more than two entities." ;
        rdfs:isDefinedBy  <http://www.lexinfo.net/ontology/2.0/lexinfo> ;
        rdfs:label        "superlative" ;
        dc:creator        "Francopoulo, Gil" ;
        dcr:datcat        <http://www.isocat.org/datcat/DC-1422> ;
        owl:versionInfo   "1:0" .

lexinfo:Degree  a         owl:Class ;
        rdfs:isDefinedBy  <http://www.lexinfo.net/ontology/2.0/lexinfo> ;
        rdfs:subClassOf   lexinfo:MorphosyntacticProperty .

lexinfo:morphosyntacticProperty
        a                   owl:ObjectProperty ;
        rdfs:isDefinedBy    <http://www.lexinfo.net/ontology/2.0/lexinfo> ;
        rdfs:range          lexinfo:MorphosyntacticProperty ;
        rdfs:subPropertyOf  lemon:property .

lexinfo:comparative  a    owl:NamedIndividual , lexinfo:Degree , owl:Thing ;
        rdfs:comment      "Comparative is the comparison where only two entites are involved." ;
        rdfs:isDefinedBy  <http://www.lexinfo.net/ontology/2.0/lexinfo> ;
        rdfs:label        "comparative" ;
        dc:creator        "Francopoulo, Gil" ;
        dcr:datcat        <http://www.isocat.org/datcat/DC-1421> ;
        owl:versionInfo   "1:0" .

lexinfo:Verb  a              owl:Class ;
        rdfs:isDefinedBy     <http://www.lexinfo.net/ontology/2.0/lexinfo> ;
        rdfs:subClassOf      lemon:Word ;
        rdfs:subClassOf      [ a                  owl:Restriction ;
                               owl:allValuesFrom  lexinfo:VerbFrame ;
                               owl:onProperty     lemon:synBehavior
                             ] ;
        owl:equivalentClass  [ a                   owl:Restriction ;
                               owl:onProperty      lexinfo:partOfSpeech ;
                               owl:someValuesFrom  lexinfo:VerbPOS
                             ] .

lexinfo:SubjectlessFrame
        a                    owl:Class ;
        rdfs:isDefinedBy     <http://www.lexinfo.net/ontology/2.0/lexinfo> ;
        rdfs:subClassOf      lexinfo:VerbFrame ;
        owl:equivalentClass  [ a                   owl:Class ;
                               owl:intersectionOf  ( lexinfo:VerbFrame [ a                owl:Restriction ;
                                                                         owl:cardinality  "0"^^xsd:nonNegativeInteger ;
                                                                         owl:onProperty   lexinfo:subject
                                                                       ] )
                             ] .

lexinfo:indefinitePronoun
        a                 owl:NamedIndividual , lexinfo:PartOfSpeech , lexinfo:PronounPOS , owl:Thing ;
        rdfs:comment      "Pronoun that does not allow reference." ;
        rdfs:isDefinedBy  <http://www.lexinfo.net/ontology/2.0/lexinfo> ;
        rdfs:label        "indefinite pronoun" ;
        dc:creator        "Francopoulo, Gil" ;
        dcr:datcat        <http://www.isocat.org/datcat/DC-1309> ;
        owl:versionInfo   "1:0" .

lexinfo:symbol  a         owl:NamedIndividual , lexinfo:TermType , owl:Thing ;
        rdfs:isDefinedBy  <http://www.lexinfo.net/ontology/2.0/lexinfo> .

lexinfo:equativeCase  a   owl:NamedIndividual , lexinfo:Case , owl:Thing ;
        rdfs:comment      "Case that expresses likeness or identity to the referent of the noun it marks. It can have meaning, such as: 'as', 'like', or 'in the capacity of'." ;
        rdfs:isDefinedBy  <http://www.lexinfo.net/ontology/2.0/lexinfo> ;
        rdfs:label        "equative case" ;
        dc:creator        "Francopoulo, Gil" ;
        dcr:datcat        <http://www.isocat.org/datcat/DC-1279> ;
        owl:versionInfo   "1:0" .

lexinfo:Voice  a          owl:Class ;
        rdfs:isDefinedBy  <http://www.lexinfo.net/ontology/2.0/lexinfo> ;
        rdfs:subClassOf   lexinfo:MorphosyntacticProperty .

lexinfo:possessiveAdjunct
        a                   owl:ObjectProperty ;
        rdfs:isDefinedBy    <http://www.lexinfo.net/ontology/2.0/lexinfo> ;
        rdfs:range          lexinfo:PossessiveAdjunct ;
        rdfs:subPropertyOf  lexinfo:adjunct .

lexinfo:InterrogativeFrame
        a                    owl:Class ;
        rdfs:comment         "Indicates the frame has a subframe indicated with the appropriate interrogative (e.g., \"who\", \"where\", \"how\")"@en ;
        rdfs:isDefinedBy     <http://www.lexinfo.net/ontology/2.0/lexinfo> ;
        rdfs:subClassOf      lexinfo:VerbFrame ;
        owl:equivalentClass  [ a                   owl:Class ;
                               owl:intersectionOf  ( lexinfo:VerbFrame [ a                   owl:Restriction ;
                                                                         owl:minCardinality  "1"^^xsd:nonNegativeInteger ;
                                                                         owl:onProperty      lexinfo:interrogativeClause
                                                                       ] )
                             ] .

lexinfo:partHolonym  a      owl:ObjectProperty ;
        rdfs:comment        "Indicates a part of this object"@en ;
        rdfs:isDefinedBy    <http://www.lexinfo.net/ontology/2.0/lexinfo> ;
        rdfs:label          "part holonym"@en ;
        rdfs:subPropertyOf  lexinfo:holonymTerm .

lexinfo:indicativeMoodForm
        a                   owl:ObjectProperty ;
        rdfs:isDefinedBy    <http://www.lexinfo.net/ontology/2.0/lexinfo> ;
        rdfs:subPropertyOf  lexinfo:formMoodVariant .

lexinfo:idiom  a          owl:NamedIndividual , lexinfo:TermType , owl:Thing ;
        rdfs:comment      "A group of words in a fixed order that have a particular meaning that is different from the meanings of each word understood on its own." ;
        rdfs:isDefinedBy  <http://www.lexinfo.net/ontology/2.0/lexinfo> ;
        rdfs:label        "idiom" ;
        dc:creator        "Wright, Sue Ellen" ;
        dcr:datcat        <http://www.isocat.org/datcat/DC-351> ;
        owl:versionInfo   "1:0" .

lexinfo:ImpersonalTransitiveFrame
        a                    owl:Class ;
        rdfs:isDefinedBy     <http://www.lexinfo.net/ontology/2.0/lexinfo> ;
        rdfs:subClassOf      lexinfo:ImpersonalFrame ;
        lexinfo:example      "es JUCKT mich"@de ;
        owl:equivalentClass  [ a                   owl:Class ;
                               owl:intersectionOf  ( lexinfo:ImpersonalFrame [ a                   owl:Restriction ;
                                                                               owl:minCardinality  "1"^^xsd:nonNegativeInteger ;
                                                                               owl:onProperty      lexinfo:directObject
                                                                             ] )
                             ] .

lexinfo:comparativeDegreeForm
        a                   owl:ObjectProperty ;
        rdfs:isDefinedBy    <http://www.lexinfo.net/ontology/2.0/lexinfo> ;
        rdfs:subPropertyOf  lexinfo:formDegreeVariant .

lexinfo:allusivePronoun
        a                 lexinfo:PartOfSpeech , owl:NamedIndividual , owl:Thing , lexinfo:PronounPOS ;
        rdfs:comment      "Pronoun that refers to something characterized by allusions." ;
        rdfs:isDefinedBy  <http://www.lexinfo.net/ontology/2.0/lexinfo> ;
        rdfs:label        "allusive pronoun" ;
        dc:creator        "Francopoulo, Gil" ;
        dcr:datcat        <http://www.isocat.org/datcat/DC-2223> ;
        owl:versionInfo   "1:0" .

terms:description  a  owl:AnnotationProperty .

lexinfo:relativePronoun
        a                 owl:Thing , lexinfo:PartOfSpeech , lexinfo:PronounPOS , owl:NamedIndividual ;
        rdfs:comment      "Pronoun which introduces a relative clause and refers to something that has been said before." ;
        rdfs:isDefinedBy  <http://www.lexinfo.net/ontology/2.0/lexinfo> ;
        rdfs:label        "relative pronoun" ;
        dc:creator        "Francopoulo, Gil" ;
        dcr:datcat        <http://www.isocat.org/datcat/DC-1380> ;
        owl:versionInfo   "1:0" .

lexinfo:PrepositionalInterrogativeFrame
        a                    owl:Class ;
        rdfs:isDefinedBy     <http://www.lexinfo.net/ontology/2.0/lexinfo> ;
        rdfs:subClassOf      lexinfo:VerbFrame ;
        owl:equivalentClass  [ a                   owl:Class ;
                               owl:intersectionOf  ( lexinfo:VerbFrame [ a                   owl:Restriction ;
                                                                         owl:minCardinality  "1"^^xsd:nonNegativeInteger ;
                                                                         owl:onProperty      lexinfo:prepositionalInterrogativeClause
                                                                       ] )
                             ] .

lexinfo:ClausalArgument
        a                 owl:Class ;
        rdfs:isDefinedBy  <http://www.lexinfo.net/ontology/2.0/lexinfo> ;
        rdfs:subClassOf   lemon:Argument .

lexinfo:IntransitiveInfinitiveSCFrame
        a                    owl:Class ;
        rdfs:isDefinedBy     <http://www.lexinfo.net/ontology/2.0/lexinfo> ;
        rdfs:subClassOf      lexinfo:InfinitiveFrame ;
        lexinfo:example      "I WANTED [to come]"@en ;
        owl:equivalentClass  [ a                   owl:Class ;
                               owl:intersectionOf  ( lexinfo:InfinitiveFrame lexinfo:IntransitiveFrame lexinfo:SubjectControl )
                             ] .

lexinfo:fusedPreposition
        a                 lexinfo:PartOfSpeech , lexinfo:FusedPrepositionPOS , owl:Thing , owl:NamedIndividual ;
        rdfs:comment      "Preposition that is the result of a morphological merge from at least two words." ;
        rdfs:isDefinedBy  <http://www.lexinfo.net/ontology/2.0/lexinfo> ;
        rdfs:label        "fused preposition" ;
        dc:creator        "Francopoulo, Gil" ;
        dcr:datcat        <http://www.isocat.org/datcat/DC-1901> ;
        owl:versionInfo   "1:0" .

lexinfo:negativeForm  a     owl:ObjectProperty ;
        rdfs:isDefinedBy    <http://www.lexinfo.net/ontology/2.0/lexinfo> ;
        rdfs:subPropertyOf  lexinfo:formPositivityVariant .

lexinfo:distinctiveParticle
        a                 lexinfo:PartOfSpeech , lexinfo:ParticlePOS , owl:Thing , owl:NamedIndividual ;
        rdfs:comment      "distinctive particle" ;
        rdfs:isDefinedBy  <http://www.lexinfo.net/ontology/2.0/lexinfo> ;
        rdfs:label        "distinctive particle" ;
        dc:creator        "Francopoulo, Gil" ;
        dcr:datcat        <http://www.isocat.org/datcat/DC-2228> ;
        owl:versionInfo   "1:0" .

lexinfo:TermType  a       owl:Class ;
        rdfs:isDefinedBy  <http://www.lexinfo.net/ontology/2.0/lexinfo> ;
        rdfs:subClassOf   lemon:PropertyValue .

lexinfo:memberHolonym
        a                   owl:ObjectProperty ;
        rdfs:comment        "Indicates the object is a member of this"@en ;
        rdfs:isDefinedBy    <http://www.lexinfo.net/ontology/2.0/lexinfo> ;
        rdfs:label          "member holonym"@en ;
        rdfs:subPropertyOf  lexinfo:holonymTerm .

lexinfo:adverbialComplement
        a                   owl:ObjectProperty ;
        rdfs:isDefinedBy    <http://www.lexinfo.net/ontology/2.0/lexinfo> ;
        rdfs:subPropertyOf  lexinfo:complement .

lexinfo:regulatedTerm
        a                 owl:NamedIndividual , lexinfo:NormativeAuthorization , owl:Thing ;
        rdfs:comment      "A term defined by law or government regulation." ;
        rdfs:isDefinedBy  <http://www.lexinfo.net/ontology/2.0/lexinfo> ;
        rdfs:label        "regulated term" ;
        dc:creator        "Wright, Sue Ellen" ;
        dcr:datcat        <http://www.isocat.org/datcat/DC-381> ;
        owl:versionInfo   "1:0" .

lexinfo:geographicalVariant
        a                   owl:ObjectProperty ;
        rdfs:comment        "Description of a specific form used in a certain region as opposed to another form used in another region" ;
        rdfs:isDefinedBy    <http://www.lexinfo.net/ontology/2.0/lexinfo> ;
        rdfs:label          "geographical variant" ;
        rdfs:subPropertyOf  lemon:lexicalVariant ;
        dc:creator          "Francopoulo, Gil" ;
        dcr:datcat          <http://www.isocat.org/datcat/DC-1851> ;
        owl:versionInfo     "1:0" .

lexinfo:dating  a           owl:ObjectProperty ;
        rdfs:comment        "Indication specifying whether the usage is old or modern." ;
        rdfs:isDefinedBy    <http://www.lexinfo.net/ontology/2.0/lexinfo> ;
        rdfs:label          "dating" ;
        rdfs:range          lexinfo:Dating ;
        rdfs:subPropertyOf  lemon:property ;
        dc:creator          "Francopoulo, Gil" ;
        dcr:datcat          <http://www.isocat.org/datcat/DC-1959> ;
        owl:versionInfo     "1:0" .

lexinfo:interrogativePronoun
        a                 owl:NamedIndividual , lexinfo:PartOfSpeech , owl:Thing , lexinfo:PronounPOS ;
        rdfs:comment      "Pronoun used to express a question." ;
        rdfs:isDefinedBy  <http://www.lexinfo.net/ontology/2.0/lexinfo> ;
        rdfs:label        "interrogative pronoun" ;
        dc:creator        "Francopoulo, Gil" ;
        dcr:datcat        <http://www.isocat.org/datcat/DC-1321> ;
        owl:versionInfo   "1:0" .

lexinfo:coordinationParticle
        a                 owl:Thing , lexinfo:PartOfSpeech , owl:NamedIndividual , lexinfo:ParticlePOS ;
        rdfs:comment      "particle for coordination" ;
        rdfs:isDefinedBy  <http://www.lexinfo.net/ontology/2.0/lexinfo> ;
        rdfs:label        "coordination particle" ;
        dc:creator        "Francopoulo, Gil" ;
        dcr:datcat        <http://www.isocat.org/datcat/DC-2227> ;
        owl:versionInfo   "1:0" .

vann:preferredNamespacePrefix
        a       owl:AnnotationProperty .

lexinfo:partitiveRelation
        a                   owl:ObjectProperty ;
        rdfs:comment        "A relation between two concepts where one of the concepts constitutes the whole and the other concept a part of that whole." ;
        rdfs:isDefinedBy    <http://www.lexinfo.net/ontology/2.0/lexinfo> ;
        rdfs:label          "partitive relation" ;
        rdfs:subPropertyOf  lemon:senseRelation ;
        dc:creator          "Wright, Sue Ellen" ;
        dcr:datcat          <http://www.isocat.org/datcat/DC-397> ;
        owl:versionInfo     "1:0" .

lemon:senseRelation  a  owl:ObjectProperty .

lexinfo:superlativeAdjunct
        a                   owl:ObjectProperty ;
        rdfs:isDefinedBy    <http://www.lexinfo.net/ontology/2.0/lexinfo> ;
        rdfs:range          lexinfo:SuperlativeAdjunct ;
        rdfs:subPropertyOf  lexinfo:predicativeAdjunct .

lexinfo:obliqueCase  a    owl:NamedIndividual , lexinfo:Case , owl:Thing ;
        rdfs:comment      "Case that is used when a noun is the object of a verb or a proposition, except for nominative and vocative case." ;
        rdfs:isDefinedBy  <http://www.lexinfo.net/ontology/2.0/lexinfo> ;
        rdfs:label        "oblique case" ;
        dc:creator        "Francopoulo, Gil" ;
        dcr:datcat        <http://www.isocat.org/datcat/DC-1336> ;
        owl:versionInfo   "1:0" .

lexinfo:Adjective  a         owl:Class ;
        rdfs:isDefinedBy     <http://www.lexinfo.net/ontology/2.0/lexinfo> ;
        rdfs:subClassOf      lemon:Word ;
        rdfs:subClassOf      [ a                  owl:Restriction ;
                               owl:allValuesFrom  lexinfo:AdjectiveFrame ;
                               owl:onProperty     lemon:synBehavior
                             ] ;
        owl:equivalentClass  [ a                   owl:Restriction ;
                               owl:onProperty      lexinfo:partOfSpeech ;
                               owl:someValuesFrom  lexinfo:AdjectivePOS
                             ] .

lexinfo:postPositiveArg
        a                   owl:ObjectProperty ;
        rdfs:comment        "Indicates an argument of an adjective indicated by post-positive modification. An example in english would be that \"that is something interesting\", where the adjective interesting post-postively modifies something"@en ;
        rdfs:isDefinedBy    <http://www.lexinfo.net/ontology/2.0/lexinfo> ;
        rdfs:range          lexinfo:PostPositiveArgument ;
        rdfs:subPropertyOf  lemon:synArg .

lexinfo:phraseologicalUnit
        a                 owl:NamedIndividual , lexinfo:TermType , owl:Thing ;
        rdfs:comment      "Any group of two or more words that form a unit, the meaning of which frequently cannot be deduced based on the combined sense of the words making up the phrase." ;
        rdfs:isDefinedBy  <http://www.lexinfo.net/ontology/2.0/lexinfo> ;
        rdfs:label        "phraseological unit" ;
        dc:creator        "Wright, Sue Ellen" ;
        dcr:datcat        <http://www.isocat.org/datcat/DC-339> ;
        owl:versionInfo   "1:0" .

lexinfo:predicativeNominative
        a                   owl:ObjectProperty ;
        rdfs:isDefinedBy    <http://www.lexinfo.net/ontology/2.0/lexinfo> ;
        rdfs:range          lexinfo:PredicativeNominative ;
        rdfs:subPropertyOf  lexinfo:complement .

lexinfo:MorphosyntacticProperty
        a                 owl:Class ;
        rdfs:isDefinedBy  <http://www.lexinfo.net/ontology/2.0/lexinfo> ;
        rdfs:subClassOf   lemon:PropertyValue .

lexinfo:prepositionalAdjunct
        a                   owl:ObjectProperty ;
        rdfs:isDefinedBy    <http://www.lexinfo.net/ontology/2.0/lexinfo> ;
        rdfs:range          lexinfo:PrepositionalAdjunct ;
        rdfs:subPropertyOf  lexinfo:adjunct .

lexinfo:ComparativeAdjunct
        a                 owl:Class ;
        rdfs:isDefinedBy  <http://www.lexinfo.net/ontology/2.0/lexinfo> ;
        rdfs:subClassOf   lexinfo:Adjunct .

lexinfo:formalRegister
        a                 owl:NamedIndividual , lexinfo:Register , owl:Thing ;
        rdfs:isDefinedBy  <http://www.lexinfo.net/ontology/2.0/lexinfo> .

lexinfo:activeVoice  a    owl:NamedIndividual , lexinfo:Voice , owl:Thing ;
        rdfs:comment      "Value that expresses the situation where the grammatical subject is also the semantic actor of the verb." ;
        rdfs:isDefinedBy  <http://www.lexinfo.net/ontology/2.0/lexinfo> ;
        rdfs:label        "active voice" ;
        dc:creator        "Francopoulo, Gil" ;
        dcr:datcat        <http://www.isocat.org/datcat/DC-1227> ;
        owl:versionInfo   "1:0" .

lexinfo:internationalScientificTerm
        a                 owl:NamedIndividual , lexinfo:TermType , owl:Thing ;
        rdfs:comment      "A term that is part of an international scientific nomenclature as adopted by an appropriate scientific body." ;
        rdfs:isDefinedBy  <http://www.lexinfo.net/ontology/2.0/lexinfo> ;
        rdfs:label        "international scientific term" ;
        dc:creator        "Wright, Sue Ellen" ;
        dcr:datcat        <http://www.isocat.org/datcat/DC-319> ;
        owl:versionInfo   "1:0" .

lexinfo:imperative  a     lexinfo:VerbFormMood , owl:Thing , owl:NamedIndividual , lexinfo:Mood ;
        rdfs:comment      "Mood used to express an order." , "..." ;
        rdfs:isDefinedBy  <http://www.lexinfo.net/ontology/2.0/lexinfo> ;
        rdfs:label        "imperative" ;
        dc:creator        "Wright, Sue Ellen" , "Francopoulo, Gil" ;
        dcr:datcat        <http://www.isocat.org/datcat/DC-1844> , <http://www.isocat.org/datcat/DC-369> ;
        owl:versionInfo   "1:0" .

lexinfo:comparativeParticle
        a                 lexinfo:ParticlePOS , owl:NamedIndividual , lexinfo:PartOfSpeech , owl:Thing ;
        rdfs:comment      "Particle used to compare." ;
        rdfs:isDefinedBy  <http://www.lexinfo.net/ontology/2.0/lexinfo> ;
        rdfs:label        "comparative particle" ;
        dc:creator        "Francopoulo, Gil" ;
        dcr:datcat        <http://www.isocat.org/datcat/DC-1922> ;
        owl:versionInfo   "1:0" .

lexinfo:Preposition  a       owl:Class ;
        rdfs:isDefinedBy     <http://www.lexinfo.net/ontology/2.0/lexinfo> ;
        rdfs:subClassOf      lexinfo:Adposition ;
        owl:equivalentClass  [ a               owl:Restriction ;
                               owl:hasValue    lexinfo:preposition ;
                               owl:onProperty  lexinfo:partOfSpeech
                             ] .

lexinfo:presentTenseForm
        a                   owl:ObjectProperty ;
        rdfs:isDefinedBy    <http://www.lexinfo.net/ontology/2.0/lexinfo> ;
        rdfs:subPropertyOf  lexinfo:formTenseVariant .

lexinfo:ergativeCase  a   owl:NamedIndividual , lexinfo:Case , owl:Thing ;
        rdfs:comment      "Case assigned to the subject of a transitive verb as opposed to absolutive case." ;
        rdfs:isDefinedBy  <http://www.lexinfo.net/ontology/2.0/lexinfo> ;
        rdfs:label        "ergative case" ;
        dc:creator        "Francopoulo, Gil" ;
        dcr:datcat        <http://www.isocat.org/datcat/DC-1280> ;
        owl:versionInfo   "1:0" .

lexinfo:ordinalAdjective
        a                 owl:NamedIndividual , lexinfo:PartOfSpeech , lexinfo:AdjectivePOS , owl:Thing ;
        rdfs:comment      "Adjective/numeral/number expressing a numeric ranking." ;
        rdfs:isDefinedBy  <http://www.lexinfo.net/ontology/2.0/lexinfo> ;
        rdfs:label        "ordinal adjective" ;
        dc:creator        "Francopoulo, Gil" ;
        dcr:datcat        <http://www.isocat.org/datcat/DC-1338> ;
        owl:versionInfo   "1:0" .

lexinfo:no  a             lexinfo:Cliticness , lexinfo:Negative , owl:NamedIndividual , owl:Thing ;
        rdfs:comment      "Value for negation." ;
        rdfs:isDefinedBy  <http://www.lexinfo.net/ontology/2.0/lexinfo> ;
        rdfs:label        "no" ;
        dc:creator        "Francopoulo, Gil" ;
        dcr:datcat        <http://www.isocat.org/datcat/DC-1905> ;
        owl:versionInfo   "1:0" .

lexinfo:termElement  a      owl:ObjectProperty ;
        rdfs:comment        "Any logically significant portion of a larger term or lexeme." ;
        rdfs:isDefinedBy    <http://www.lexinfo.net/ontology/2.0/lexinfo> ;
        rdfs:label          "lexTermElement" ;
        rdfs:range          lexinfo:TermElement ;
        rdfs:subPropertyOf  lemon:property ;
        dc:creator          "Wright, Sue Ellen" ;
        dcr:datcat          <http://www.isocat.org/datcat/DC-289> ;
        owl:versionInfo     "1:0" .

lexinfo:Suffix  a            owl:Class ;
        rdfs:isDefinedBy     <http://www.lexinfo.net/ontology/2.0/lexinfo> ;
        rdfs:subClassOf      lexinfo:Affix ;
        owl:equivalentClass  [ a               owl:Restriction ;
                               owl:hasValue    lexinfo:suffix ;
                               owl:onProperty  lexinfo:termElement
                             ] .

lexinfo:AdjectiveDativePostPositiveFrame
        a                    owl:Class ;
        rdfs:isDefinedBy     <http://www.lexinfo.net/ontology/2.0/lexinfo> ;
        rdfs:subClassOf      lexinfo:AdjectivePostPositiveFrame ;
        lexinfo:example      "er ist seinem bruder ÄHNLICH"@de ;
        owl:equivalentClass  [ a                   owl:Class ;
                               owl:intersectionOf  ( lexinfo:AdjectivePostPositiveFrame [ a                   owl:Restriction ;
                                                                                          owl:onProperty      lexinfo:postPositiveArg ;
                                                                                          owl:someValuesFrom  lexinfo:DativePostPositiveArgument
                                                                                        ] )
                             ] .

lexinfo:clausalArg  a       owl:ObjectProperty ;
        rdfs:isDefinedBy    <http://www.lexinfo.net/ontology/2.0/lexinfo> ;
        rdfs:range          lexinfo:ClausalArgument ;
        rdfs:subPropertyOf  lemon:synArg .

lexinfo:neutralRegister
        a                 lexinfo:Register , owl:Thing , owl:NamedIndividual ;
        rdfs:comment      "The register appropriate to general texts or discourse." ;
        rdfs:isDefinedBy  <http://www.lexinfo.net/ontology/2.0/lexinfo> ;
        rdfs:label        "neutral register" ;
        dc:creator        "Wright, Sue Ellen" , "Francopoulo, Gil" ;
        dcr:datcat        <http://www.isocat.org/datcat/DC-1999> , <http://www.isocat.org/datcat/DC-424> ;
        owl:versionInfo   "1:0" .

owl:Thing  a    owl:Class .

lexinfo:emphaticPronoun
        a                 owl:Thing , lexinfo:PronounPOS , lexinfo:PartOfSpeech , owl:NamedIndividual ;
        rdfs:comment      "An emphatic pronoun is a personal pronoun that is used to emphasize its referent." ;
        rdfs:isDefinedBy  <http://www.lexinfo.net/ontology/2.0/lexinfo> ;
        rdfs:label        "emphatic pronoun" ;
        dc:creator        "Francopoulo, Gil" ;
        dcr:datcat        <http://www.isocat.org/datcat/DC-1941> ;
        owl:versionInfo   "1:0" .

lexinfo:copula  a         lexinfo:VerbPOS , owl:NamedIndividual , lexinfo:PartOfSpeech , owl:Thing ;
        rdfs:comment      "Special word that combines the subject of a sentence and its description." ;
        rdfs:isDefinedBy  <http://www.lexinfo.net/ontology/2.0/lexinfo> ;
        rdfs:label        "copula" ;
        dc:creator        "Francopoulo, Gil" ;
        dcr:datcat        <http://www.isocat.org/datcat/DC-1263> ;
        owl:versionInfo   "1:0" .

lexinfo:vulgarRegister
        a                 owl:Thing , lexinfo:Register , owl:NamedIndividual ;
        rdfs:comment      "The register of a term or text type that can be characterized as profane or socially unacceptable." , "Register of a term or text type that can be characterized as profane or socially unacceptable." ;
        rdfs:isDefinedBy  <http://www.lexinfo.net/ontology/2.0/lexinfo> ;
        rdfs:label        "vulgar register" ;
        dc:creator        "Wright, Sue Ellen" , "Francopoulo, Gil" ;
        dcr:datcat        <http://www.isocat.org/datcat/DC-429> , <http://www.isocat.org/datcat/DC-1998> ;
        owl:versionInfo   "1:0" .

lexinfo:subjunctiveMoodForm
        a                   owl:ObjectProperty ;
        rdfs:isDefinedBy    <http://www.lexinfo.net/ontology/2.0/lexinfo> ;
        rdfs:subPropertyOf  lexinfo:formMoodVariant .

lexinfo:indifferent  a    owl:NamedIndividual , lexinfo:ModificationType , owl:Thing ;
        rdfs:comment      "Markup to express that there is not any pertinence." ;
        rdfs:isDefinedBy  <http://www.lexinfo.net/ontology/2.0/lexinfo> ;
        rdfs:label        "indifferent" ;
        dc:creator        "Francopoulo, Gil" ;
        dcr:datcat        <http://www.isocat.org/datcat/DC-1944> ;
        owl:versionInfo   "1:0" .

lexinfo:PostPositiveArgument
        a                 owl:Class ;
        rdfs:isDefinedBy  <http://www.lexinfo.net/ontology/2.0/lexinfo> ;
        rdfs:subClassOf   lemon:Argument .

lexinfo:pastParticipleAdjective
        a                 lexinfo:PartOfSpeech , lexinfo:AdjectivePOS , owl:Thing , owl:NamedIndividual ;
        rdfs:comment      "Adjective based on a past participle." ;
        rdfs:isDefinedBy  <http://www.lexinfo.net/ontology/2.0/lexinfo> ;
        rdfs:label        "past participle adjective" ;
        dc:creator        "Francopoulo, Gil" ;
        dcr:datcat        <http://www.isocat.org/datcat/DC-1596> ;
        owl:versionInfo   "1:0" .

lexinfo:hypernym  a         owl:ObjectProperty ;
        rdfs:isDefinedBy    <http://www.lexinfo.net/ontology/2.0/lexinfo> ;
        rdfs:subPropertyOf  lemon:broader .

lemon:definition  a  owl:ObjectProperty .

lexinfo:FusedPreposition
        a                    owl:Class ;
        rdfs:comment         "A word that is a fusion of a preposition and some other word... examples include the German words \"zum\" and \"daran\""@en ;
        rdfs:isDefinedBy     <http://www.lexinfo.net/ontology/2.0/lexinfo> ;
        rdfs:subClassOf      lemon:Word ;
        owl:equivalentClass  [ a                   owl:Restriction ;
                               owl:onProperty      lexinfo:partOfSpeech ;
                               owl:someValuesFrom  lexinfo:FusedPrepositionPOS
                             ] .

lexinfo:nonFinite  a      owl:NamedIndividual , lexinfo:Finiteness , owl:Thing ;
        rdfs:comment      "Property related for verb forms occurring on their own only in dependent clauses and lacking tense and mood contrasts." ;
        rdfs:isDefinedBy  <http://www.lexinfo.net/ontology/2.0/lexinfo> ;
        rdfs:label        "non-finite" ;
        dc:creator        "Francopoulo, Gil" ;
        dcr:datcat        <http://www.isocat.org/datcat/DC-1332> ;
        owl:versionInfo   "1:0" .

lexinfo:ReflexiveReciprocalFrame
        a                    owl:Class ;
        rdfs:isDefinedBy     <http://www.lexinfo.net/ontology/2.0/lexinfo> ;
        rdfs:subClassOf      lexinfo:ReflexiveFrame ;
        lexinfo:example      "hans und marie TREFFEN sich"@de ;
        owl:equivalentClass  [ a                   owl:Class ;
                               owl:intersectionOf  ( lexinfo:ReciprocalFrame lexinfo:ReflexiveFrame )
                             ] .

lexinfo:partNumber  a     owl:NamedIndividual , lexinfo:TermType , owl:Thing ;
        rdfs:comment      "A unique alphanumeric designation assigned to an object in a manufacturing system." ;
        rdfs:isDefinedBy  <http://www.lexinfo.net/ontology/2.0/lexinfo> ;
        rdfs:label        "part number" ;
        dc:creator        "Wright, Sue Ellen" ;
        dcr:datcat        <http://www.isocat.org/datcat/DC-338> ;
        owl:versionInfo   "1:0" .

lexinfo:dativeCase  a     owl:NamedIndividual , lexinfo:Case , owl:Thing ;
        rdfs:comment      "Case that expresses an indirect object relationship or a range of meaning similar to that covered by 'to' or 'for' in English; but there is a great deal of variation between languages in the way this case is used." ;
        rdfs:isDefinedBy  <http://www.lexinfo.net/ontology/2.0/lexinfo> ;
        rdfs:label        "dative case" ;
        dc:creator        "Francopoulo, Gil" ;
        dcr:datcat        <http://www.isocat.org/datcat/DC-1265> ;
        owl:versionInfo   "1:0" .

lexinfo:optionalElement
        a                 owl:NamedIndividual , lexinfo:TermElement , owl:Thing ;
        rdfs:comment      "1951: An optional part of a headword.\n1951; examples? The question arises whether these are true options or whether the options reflect synonyms or hyponyms (e.g., barrage, barrage de retenue). The question is not whether 1951 should use this markup, but rather how to map this markup in a global environment." ;
        rdfs:isDefinedBy  <http://www.lexinfo.net/ontology/2.0/lexinfo> ;
        rdfs:label        "optionalElement" ;
        dc:creator        "Wright, Sue Ellen" ;
        dcr:datcat        <http://www.isocat.org/datcat/DC-299> ;
        owl:versionInfo   "1:0" .

lexinfo:determiner  a     lexinfo:PartOfSpeech , owl:Thing , owl:NamedIndividual , lexinfo:DeterminerPOS ;
        rdfs:comment      "Word or affix that belongs to a class of noun modifiers that expresses the reference, including quantity, of a noun." ;
        rdfs:isDefinedBy  <http://www.lexinfo.net/ontology/2.0/lexinfo> ;
        rdfs:label        "determiner" ;
        dc:creator        "Francopoulo, Gil" ;
        dcr:datcat        <http://www.isocat.org/datcat/DC-1272> ;
        owl:versionInfo   "1:0" .

lexinfo:SubjectlessIntransitivePPFrame
        a                    owl:Class ;
        rdfs:isDefinedBy     <http://www.lexinfo.net/ontology/2.0/lexinfo> ;
        rdfs:subClassOf      lexinfo:SubjectlessIntransitiveFrame ;
        lexinfo:example      "mir TRÄUMT VON jener zeit"@de ;
        owl:equivalentClass  [ a                   owl:Class ;
                               owl:intersectionOf  ( lexinfo:PPFrame lexinfo:SubjectlessIntransitiveFrame )
                             ] .

lexinfo:accusativeCase
        a                 owl:NamedIndividual , lexinfo:Case , owl:Thing ;
        rdfs:comment      "Case used to indicate direct object." ;
        rdfs:isDefinedBy  <http://www.lexinfo.net/ontology/2.0/lexinfo> ;
        rdfs:label        "accusative case" ;
        dc:creator        "Francopoulo, Gil" ;
        dcr:datcat        <http://www.isocat.org/datcat/DC-1226> ;
        owl:versionInfo   "1:0" .

lexinfo:genericNumeral
        a                 owl:Thing , lexinfo:PartOfSpeech , lexinfo:NumeralPOS , owl:NamedIndividual ;
        rdfs:comment      "A numeral used to indicate the number of sets/kinds of objects." ;
        rdfs:isDefinedBy  <http://www.lexinfo.net/ontology/2.0/lexinfo> ;
        rdfs:label        "generic numeral" ;
        dc:creator        "Zeman, Dan" ;
        dcr:datcat        <http://www.isocat.org/datcat/DC-3022> ;
        owl:versionInfo   "1:0" .

lexinfo:formPositivityVariant
        a                   owl:ObjectProperty ;
        rdfs:isDefinedBy    <http://www.lexinfo.net/ontology/2.0/lexinfo> ;
        rdfs:subPropertyOf  lemon:formVariant .

lexinfo:nucleus  a        owl:NamedIndividual , lexinfo:TermType , owl:Thing ;
        rdfs:comment      "The component of a multiword or multi-morphemic compound term that is determined or modified by the other components making up the term." ;
        rdfs:isDefinedBy  <http://www.lexinfo.net/ontology/2.0/lexinfo> ;
        rdfs:label        "nucleus" ;
        dc:creator        "Wright, Sue Ellen" ;
        dcr:datcat        <http://www.isocat.org/datcat/DC-357> ;
        owl:versionInfo   "1:0" .

lexinfo:acronym  a        owl:NamedIndividual , lexinfo:AbbreviatedForm , lexinfo:TermType , owl:Thing ;
        rdfs:comment      "An abbreviation made up of the initial letters of the components of the full form of the designation or from syllables of the full form and pronounced syllabically." ;
        rdfs:isDefinedBy  <http://www.lexinfo.net/ontology/2.0/lexinfo> ;
        rdfs:label        "acronym" ;
        dc:creator        "Wright, Sue Ellen" ;
        dcr:datcat        <http://www.isocat.org/datcat/DC-334> ;
        owl:versionInfo   "1:0" .

lexinfo:DitransitiveDoubleAccusativeFrame
        a                    owl:Class ;
        rdfs:isDefinedBy     <http://www.lexinfo.net/ontology/2.0/lexinfo> ;
        rdfs:subClassOf      lexinfo:VerbFrame ;
        lexinfo:example      "das KOSTET ihn sein leben"@de ;
        owl:equivalentClass  [ a                   owl:Class ;
                               owl:intersectionOf  ( lexinfo:VerbFrame [ a                owl:Restriction ;
                                                                         owl:cardinality  "2"^^xsd:nonNegativeInteger ;
                                                                         owl:onProperty   lexinfo:directObject
                                                                       ] [ a                owl:Restriction ;
                                                                           owl:cardinality  "1"^^xsd:nonNegativeInteger ;
                                                                           owl:onProperty   lexinfo:subject
                                                                         ] )
                             ] .

lexinfo:predicativeAdverb
        a                   owl:ObjectProperty ;
        rdfs:isDefinedBy    <http://www.lexinfo.net/ontology/2.0/lexinfo> ;
        rdfs:range          lexinfo:PredicativeAdverb ;
        rdfs:subPropertyOf  lexinfo:complement .

lexinfo:voice  a            owl:ObjectProperty ;
        rdfs:comment        "Way sentences may alter the relationship between the subject and object of a verb, without changing the meaning of the sentence." ;
        rdfs:isDefinedBy    <http://www.lexinfo.net/ontology/2.0/lexinfo> ;
        rdfs:label          "voice" ;
        rdfs:range          lexinfo:Voice ;
        rdfs:subPropertyOf  lexinfo:morphosyntacticProperty ;
        dc:creator          "Francopoulo, Gil" ;
        dcr:datcat          <http://www.isocat.org/datcat/DC-1413> ;
        owl:versionInfo     "1:0" .

lexinfo:possessiveParticle
        a                 lexinfo:PartOfSpeech , owl:Thing , lexinfo:ParticlePOS , owl:NamedIndividual ;
        rdfs:comment      "Particle expressing ownship." ;
        rdfs:isDefinedBy  <http://www.lexinfo.net/ontology/2.0/lexinfo> ;
        rdfs:label        "possessive particle" ;
        dc:creator        "Francopoulo, Gil" ;
        dcr:datcat        <http://www.isocat.org/datcat/DC-1895> ;
        owl:versionInfo   "1:0" .

lexinfo:affirmativeParticle
        a                 owl:NamedIndividual , owl:Thing , lexinfo:ParticlePOS , lexinfo:PartOfSpeech ;
        rdfs:comment      "Particle used to express affirmation." ;
        rdfs:isDefinedBy  <http://www.lexinfo.net/ontology/2.0/lexinfo> ;
        rdfs:label        "affirmative particule" ;
        dc:creator        "Francopoulo, Gil" ;
        dcr:datcat        <http://www.isocat.org/datcat/DC-1918> ;
        owl:versionInfo   "1:0" .

lexinfo:Affix  a             owl:Class ;
        rdfs:isDefinedBy     <http://www.lexinfo.net/ontology/2.0/lexinfo> ;
        rdfs:subClassOf      lemon:Part ;
        owl:equivalentClass  [ a               owl:Restriction ;
                               owl:hasValue    lexinfo:affix ;
                               owl:onProperty  lexinfo:termElement
                             ] .

lexinfo:presentParticipleAdjective
        a                 lexinfo:PartOfSpeech , owl:NamedIndividual , lexinfo:AdjectivePOS , owl:Thing ;
        rdfs:comment      "Adjective based on a present participle." ;
        rdfs:isDefinedBy  <http://www.lexinfo.net/ontology/2.0/lexinfo> ;
        rdfs:label        "present participle adjective" ;
        dc:creator        "Francopoulo, Gil" ;
        dcr:datcat        <http://www.isocat.org/datcat/DC-1597> ;
        owl:versionInfo   "1:0" .

lexinfo:coordinateConcept
        a                   owl:ObjectProperty ;
        rdfs:comment        "A subordinate concept having the same nearest superordinate concept and same criterion of subdivision as some other concept in a given concept system." ;
        rdfs:isDefinedBy    <http://www.lexinfo.net/ontology/2.0/lexinfo> ;
        rdfs:label          "coordinateConcept" ;
        rdfs:subPropertyOf  lexinfo:relatedTerm ;
        dc:creator          "Wright, Sue Ellen" ;
        dcr:datcat          <http://www.isocat.org/datcat/DC-158> ;
        owl:versionInfo     "1:0" .

lexinfo:pastTenseForm
        a                   owl:ObjectProperty ;
        rdfs:isDefinedBy    <http://www.lexinfo.net/ontology/2.0/lexinfo> ;
        rdfs:subPropertyOf  lexinfo:formTenseVariant .

lexinfo:IntransitiveNominalComplementFrame
        a                    owl:Class ;
        rdfs:isDefinedBy     <http://www.lexinfo.net/ontology/2.0/lexinfo> ;
        rdfs:subClassOf      lexinfo:IntransitiveFrame ;
        lexinfo:example      "he SEEMED a fool"@en ;
        owl:equivalentClass  [ a                   owl:Class ;
                               owl:intersectionOf  ( lexinfo:IntransitiveFrame [ a                   owl:Restriction ;
                                                                                 owl:minCardinality  "1"^^xsd:nonNegativeInteger ;
                                                                                 owl:onProperty      lexinfo:predicativeNominative
                                                                               ] )
                             ] .

lexinfo:SubjectlessTransitivePPFrame
        a                    owl:Class ;
        rdfs:isDefinedBy     <http://www.lexinfo.net/ontology/2.0/lexinfo> ;
        rdfs:subClassOf      lexinfo:SubjectlessTransitiveFrame , lexinfo:PPFrame ;
        lexinfo:example      "mich EKELT VOR fleisch"@de ;
        owl:equivalentClass  [ a                   owl:Class ;
                               owl:intersectionOf  ( lexinfo:PPFrame lexinfo:SubjectlessTransitiveFrame )
                             ] .

lexinfo:PredicativeNominative
        a                 owl:Class ;
        rdfs:isDefinedBy  <http://www.lexinfo.net/ontology/2.0/lexinfo> ;
        rdfs:subClassOf   lexinfo:Complement .

lexinfo:contraction  a    owl:Thing , lexinfo:AbbreviatedForm , lexinfo:TermType , owl:NamedIndividual ;
        rdfs:comment      "A lexical unit formed by a shortening of a word, syllable, or word group by omission of a sound or letter." ;
        rdfs:isDefinedBy  <http://www.lexinfo.net/ontology/2.0/lexinfo> ;
        rdfs:label        "contraction" ;
        dc:creator        "Wright, Sue Ellen" ;
        dcr:datcat        <http://www.isocat.org/datcat/DC-354> ;
        owl:versionInfo   "1:0" .

lexinfo:stringCategory
        a                 owl:NamedIndividual , lexinfo:TermType , owl:Thing ;
        rdfs:comment      "A type value assigned to a string." ;
        rdfs:isDefinedBy  <http://www.lexinfo.net/ontology/2.0/lexinfo> ;
        rdfs:label        "stringCategory" ;
        dc:creator        "Wright, Sue Ellen" ;
        dcr:datcat        <http://www.isocat.org/datcat/DC-345> ;
        owl:versionInfo   "1:0" .

lexinfo:prepositionalInterrogativeClause
        a                   owl:ObjectProperty ;
        rdfs:isDefinedBy    <http://www.lexinfo.net/ontology/2.0/lexinfo> ;
        rdfs:subPropertyOf  lexinfo:clausalArg .

lexinfo:modal  a          lexinfo:PartOfSpeech , owl:NamedIndividual , lexinfo:VerbPOS , owl:Thing ;
        rdfs:comment      "Verb form that is usually used with another verb to express ideas such as possibilities, permission, or intention." ;
        rdfs:isDefinedBy  <http://www.lexinfo.net/ontology/2.0/lexinfo> ;
        rdfs:label        "modal" ;
        dc:creator        "Francopoulo, Gil" ;
        dcr:datcat        <http://www.isocat.org/datcat/DC-1329> ;
        owl:versionInfo   "1:0" .

lexinfo:SymbolPOS  a      owl:Class ;
        rdfs:isDefinedBy  <http://www.lexinfo.net/ontology/2.0/lexinfo> ;
        rdfs:subClassOf   lexinfo:PartOfSpeech .

lexinfo:internationalism
        a                 owl:NamedIndividual , lexinfo:TermType , owl:Thing ;
        rdfs:comment      "A term that has the same or nearly identical orthographic or phonemic form in many languages." ;
        rdfs:isDefinedBy  <http://www.lexinfo.net/ontology/2.0/lexinfo> ;
        rdfs:label        "internationalism" ;
        dc:creator        "Wright, Sue Ellen" ;
        dcr:datcat        <http://www.isocat.org/datcat/DC-320> ;
        owl:versionInfo   "1:0" .

lexinfo:demonstrativePronoun
        a                 owl:NamedIndividual , lexinfo:PronounPOS , owl:Thing , lexinfo:PartOfSpeech ;
        rdfs:comment      "Pronoun used to point to an entity in the situation or elsewhere in a sentence." ;
        rdfs:isDefinedBy  <http://www.lexinfo.net/ontology/2.0/lexinfo> ;
        rdfs:label        "demonstrative pronoun" ;
        dc:creator        "Francopoulo, Gil" ;
        dcr:datcat        <http://www.isocat.org/datcat/DC-1270> ;
        owl:versionInfo   "1:0" .

lexinfo:Number  a         owl:Class ;
        rdfs:isDefinedBy  <http://www.lexinfo.net/ontology/2.0/lexinfo> ;
        rdfs:subClassOf   lexinfo:MorphosyntacticProperty .

lexinfo:genitiveCase  a   owl:NamedIndividual , lexinfo:Case , owl:Thing ;
        rdfs:comment      "Case which expresses a possessive relationship (e.g. the boy's book) or some other similarly close connection (e.g. a summer's day)." ;
        rdfs:isDefinedBy  <http://www.lexinfo.net/ontology/2.0/lexinfo> ;
        rdfs:label        "genitive case" ;
        dc:creator        "Francopoulo, Gil" ;
        dcr:datcat        <http://www.isocat.org/datcat/DC-1293> ;
        owl:versionInfo   "1:0" .

lexinfo:colon  a          lexinfo:PartOfSpeech , owl:NamedIndividual , owl:Thing , lexinfo:SymbolPOS ;
        rdfs:comment      "Sign with two vertical points that is used in writing and printing to introduce an explanation, example or quotation." ;
        rdfs:isDefinedBy  <http://www.lexinfo.net/ontology/2.0/lexinfo> ;
        rdfs:label        "colon" ;
        dc:creator        "Francopoulo, Gil" ;
        dcr:datcat        <http://www.isocat.org/datcat/DC-1439> ;
        owl:versionInfo   "1:0" .

lexinfo:presentativePronoun
        a                 owl:NamedIndividual , lexinfo:PartOfSpeech , lexinfo:PronounPOS , owl:Thing ;
        rdfs:comment      "pronoun that identify the current locative or temporal situation" ;
        rdfs:isDefinedBy  <http://www.lexinfo.net/ontology/2.0/lexinfo> ;
        rdfs:label        "presentative pronoun" ;
        dc:creator        "Francopoulo, Gil" ;
        dcr:datcat        <http://www.isocat.org/datcat/DC-3015> ;
        owl:versionInfo   "1:0" .

lexinfo:initialismFor
        a                   owl:ObjectProperty ;
        rdfs:comment        "A linking element used to identify a relation between an initialism and its full or expanded form." ;
        rdfs:isDefinedBy    <http://www.lexinfo.net/ontology/2.0/lexinfo> ;
        rdfs:label          "initialismFor" ;
        rdfs:subPropertyOf  lexinfo:contractionFor ;
        dc:creator          "Wright, Sue Ellen" ;
        dcr:datcat          <http://www.isocat.org/datcat/DC-272> ;
        owl:versionInfo     "1:0" .

lexinfo:VerbPOS  a        owl:Class ;
        rdfs:isDefinedBy  <http://www.lexinfo.net/ontology/2.0/lexinfo> ;
        rdfs:subClassOf   lexinfo:PartOfSpeech .

lexinfo:register  a         owl:ObjectProperty ;
        rdfs:comment        "Classification indicating the relative level of language individually assigned to a lexeme or term or to a text type." ;
        rdfs:isDefinedBy    <http://www.lexinfo.net/ontology/2.0/lexinfo> ;
        rdfs:label          "register" ;
        rdfs:range          lexinfo:Register ;
        rdfs:subPropertyOf  lemon:context ;
        dc:creator          "Wright, Sue Ellen" , "Francopoulo, Gil" ;
        dcr:datcat          <http://www.isocat.org/datcat/DC-1988> , <http://www.isocat.org/datcat/DC-423> ;
        owl:versionInfo     "1:0" .

lexinfo:possessiveAdjective
        a                 lexinfo:AdjectivePOS , owl:NamedIndividual , lexinfo:PartOfSpeech , owl:Thing ;
        rdfs:comment      "An adjective derived from a noun and denoting possession by the object described by the noun." ;
        rdfs:isDefinedBy  <http://www.lexinfo.net/ontology/2.0/lexinfo> ;
        rdfs:label        "possessive adjective" ;
        dc:creator        "Zeman, Dan" ;
        dcr:datcat        <http://www.isocat.org/datcat/DC-3017> ;
        owl:versionInfo   "1:0" .

lexinfo:personal  a       owl:NamedIndividual , lexinfo:ReferentType , owl:Thing ;
        rdfs:comment      "Property that refers to the person." ;
        rdfs:isDefinedBy  <http://www.lexinfo.net/ontology/2.0/lexinfo> ;
        rdfs:label        "personal" ;
        dc:creator        "Francopoulo, Gil" ;
        dcr:datcat        <http://www.isocat.org/datcat/DC-1946> ;
        owl:versionInfo   "1:0" .

lexinfo:equation  a       owl:NamedIndividual , lexinfo:TermType , owl:Thing ;
        rdfs:comment      "An expression used to represent a concept based on a statement that two mathematical expressions are, for instance, equal as identified by the equal sign (=), or assigned to one another by a similar sign." ;
        rdfs:isDefinedBy  <http://www.lexinfo.net/ontology/2.0/lexinfo> ;
        rdfs:label        "equation" ;
        dc:creator        "Wright, Sue Ellen" ;
        dcr:datcat        <http://www.isocat.org/datcat/DC-326> ;
        owl:versionInfo   "1:0" .

lexinfo:legalTerm  a      owl:NamedIndividual , lexinfo:NormativeAuthorization , owl:Thing ;
        rdfs:comment      "A term that is legally defined and used in legally binding documents." ;
        rdfs:isDefinedBy  <http://www.lexinfo.net/ontology/2.0/lexinfo> ;
        rdfs:label        "legal term" ;
        dc:creator        "Wright, Sue Ellen" ;
        dcr:datcat        <http://www.isocat.org/datcat/DC-380> ;
        owl:versionInfo   "1:0" .

lexinfo:AbbreviatedForm
        a                 owl:Class ;
        rdfs:isDefinedBy  <http://www.lexinfo.net/ontology/2.0/lexinfo> ;
        rdfs:subClassOf   lexinfo:TermType .

lexinfo:shortForm  a      owl:NamedIndividual , lexinfo:TermType , owl:Thing ;
        rdfs:comment      "A variant of a multiword term or lexeme that includes fewer words than the full form." ;
        rdfs:isDefinedBy  <http://www.lexinfo.net/ontology/2.0/lexinfo> ;
        rdfs:label        "short form" ;
        dc:creator        "Wright, Sue Ellen" ;
        dcr:datcat        <http://www.isocat.org/datcat/DC-332> ;
        owl:versionInfo   "1:0" .

<http://www.lexinfo.net/ontology/2.0/lexinfo>
        a                              owl:Ontology , <http://purl.org/vocommons/voaf#Vocabulary> , owl:NamedIndividual ;
        rdfs:comment                   "An ontology of types, values and properties to be used with the lemon model, partially derived from ISOcat."@en ;
        rdfs:label                     "LexInfo"@en ;
        ns:license                     <https://creativecommons.org/licenses/by/4.0/> ;
        terms:contributor              <http://www.cimiano.de/philipp> , <http://john.mccr.ae/> , <http://www.paulbuitelaar.net/> ;
        terms:creator                  <http://john.mccr.ae/> ;
        terms:description              "An ontology of types, values and properties to be used with the lemon model, partially derived from ISOcat."@en ;
        terms:issued                   "2010-11-22"^^xsd:date ;
        terms:modified                 "2014-06-14"^^xsd:date ;
        terms:publisher                <http://john.mccr.ae/> ;
        terms:rights                   "Copyright 2010 Monnet Project"@en ;
        terms:rights                   <https://creativecommons.org/licenses/by/4.0/> ;
        terms:title                    "LexInfo"@en ;
        vann:preferredNamespacePrefix  "lexinfo" ;
        vann:preferredNamespaceUri     "http://www.lexinfo.net/ontology/2.0/lexinfo#"^^xsd:anyURI ;
        owl:imports                    <http://lemon-model.net/lemon> ;
        owl:versionInfo                "2.0"@en .

lexinfo:SuperlativeAdjunct
        a                 owl:Class ;
        rdfs:isDefinedBy  <http://www.lexinfo.net/ontology/2.0/lexinfo> ;
        rdfs:subClassOf   lexinfo:Adjunct .

lexinfo:absolutiveCase
        a                 owl:NamedIndividual , lexinfo:Case , owl:Thing ;
        rdfs:comment      "Case for nouns in ergative-absolute languages that would generally be the subjects of intransitive verbs or the objects of transitive verbs in the translational equivalents of nominative-accusative languages such as English." ;
        rdfs:isDefinedBy  <http://www.lexinfo.net/ontology/2.0/lexinfo> ;
        rdfs:label        "absolutive case" ;
        dc:creator        "Francopoulo, Gil" ;
        dcr:datcat        <http://www.isocat.org/datcat/DC-1225> ;
        owl:versionInfo   "1:0" .

lexinfo:TransitiveInterrogativeFrame
        a                    owl:Class ;
        rdfs:isDefinedBy     <http://www.lexinfo.net/ontology/2.0/lexinfo> ;
        rdfs:subClassOf      lexinfo:InterrogativeFrame ;
        lexinfo:example      "he ASKED her [what he should do]"@en ;
        owl:equivalentClass  [ a                   owl:Class ;
                               owl:intersectionOf  ( lexinfo:InterrogativeFrame lexinfo:TransitiveFrame )
                             ] .

lexinfo:conjunction  a    owl:NamedIndividual , lexinfo:PartOfSpeech , lexinfo:ConjunctionPOS , owl:Thing ;
        rdfs:comment      "Word that syntactically links words or constituents, and expresses a semantic relationship between them." ;
        rdfs:isDefinedBy  <http://www.lexinfo.net/ontology/2.0/lexinfo> ;
        rdfs:label        "conjunction" ;
        dc:creator        "Francopoulo, Gil" ;
        dcr:datcat        <http://www.isocat.org/datcat/DC-1260> ;
        owl:versionInfo   "1:0" .

lexinfo:ReflexiveDitransitiveFrame
        a                    owl:Class ;
        rdfs:isDefinedBy     <http://www.lexinfo.net/ontology/2.0/lexinfo> ;
        rdfs:subClassOf      lexinfo:ReflexiveFrame ;
        lexinfo:example      "das habe ich mir EINGEBILDET"@de ;
        owl:equivalentClass  [ a                   owl:Class ;
                               owl:intersectionOf  ( lexinfo:DitransitiveFrame lexinfo:ReflexiveFrame [ a                   owl:Restriction ;
                                                                                                        owl:onProperty      lexinfo:directObject ;
                                                                                                        owl:someValuesFrom  lexinfo:ReflexiveObject
                                                                                                      ] )
                             ] .

lexinfo:object  a           owl:ObjectProperty ;
        rdfs:isDefinedBy    <http://www.lexinfo.net/ontology/2.0/lexinfo> ;
        rdfs:range          lexinfo:Object ;
        rdfs:subPropertyOf  lemon:synArg .

lexinfo:Control  a        owl:Class ;
        rdfs:comment      "Control indicates how a an argument from a main clause will be utilized in a subclause. This class includes both control structures and raising structures"@en ;
        rdfs:isDefinedBy  <http://www.lexinfo.net/ontology/2.0/lexinfo> ;
        rdfs:subClassOf   lemon:Frame .

lexinfo:nominativeCaseForm
        a                   owl:ObjectProperty ;
        rdfs:isDefinedBy    <http://www.lexinfo.net/ontology/2.0/lexinfo> ;
        rdfs:subPropertyOf  lexinfo:formCaseVariant .

lexinfo:predicativeAdjective
        a                   owl:ObjectProperty ;
        rdfs:isDefinedBy    <http://www.lexinfo.net/ontology/2.0/lexinfo> ;
        rdfs:range          lexinfo:PredicativeAdjective ;
        rdfs:subPropertyOf  lexinfo:complement .

lexinfo:firstPersonForm
        a                   owl:ObjectProperty ;
        rdfs:isDefinedBy    <http://www.lexinfo.net/ontology/2.0/lexinfo> ;
        rdfs:subPropertyOf  lexinfo:formPersonVariant .

lexinfo:futureTenseForm
        a                   owl:ObjectProperty ;
        rdfs:isDefinedBy    <http://www.lexinfo.net/ontology/2.0/lexinfo> ;
        rdfs:subPropertyOf  lexinfo:formTenseVariant .

lexinfo:dativeCaseForm
        a                   owl:ObjectProperty ;
        rdfs:isDefinedBy    <http://www.lexinfo.net/ontology/2.0/lexinfo> ;
        rdfs:subPropertyOf  lexinfo:formCaseVariant .

lexinfo:collective  a     owl:NamedIndividual , lexinfo:Number , owl:Thing ;
        rdfs:comment      "A collective number is a number referring to 'a set of things'. Languages that have this feature can use it to get a phrase like 'flock of sheeps' by using 'sheep' in collective number." ;
        rdfs:isDefinedBy  <http://www.lexinfo.net/ontology/2.0/lexinfo> ;
        rdfs:label        "collective" ;
        dc:creator        "Francopoulo, Gil" ;
        dcr:datcat        <http://www.isocat.org/datcat/DC-1254> ;
        owl:versionInfo   "1:0" .

lexinfo:PossessiveAdjunct
        a                 owl:Class ;
        rdfs:isDefinedBy  <http://www.lexinfo.net/ontology/2.0/lexinfo> ;
        rdfs:subClassOf   lexinfo:Adjunct .

lexinfo:quadrial  a       owl:NamedIndividual , lexinfo:Number , owl:Thing ;
        rdfs:comment      "Property related to four elements." ;
        rdfs:isDefinedBy  <http://www.lexinfo.net/ontology/2.0/lexinfo> ;
        rdfs:label        "quadrial" ;
        dc:creator        "Francopoulo, Gil" ;
        dcr:datcat        <http://www.isocat.org/datcat/DC-2000> ;
        owl:versionInfo   "1:0" .

lexinfo:delativeCase  a   owl:NamedIndividual , lexinfo:Case , owl:Thing ;
        rdfs:comment      "Case which expresses motion downward from the referent of the noun it marks." ;
        rdfs:isDefinedBy  <http://www.lexinfo.net/ontology/2.0/lexinfo> ;
        rdfs:label        "delative case" ;
        dc:creator        "Francopoulo, Gil" ;
        dcr:datcat        <http://www.isocat.org/datcat/DC-1268> ;
        owl:versionInfo   "1:0" .

lexinfo:appellation  a    owl:NamedIndividual , lexinfo:TermType , owl:Thing ;
        rdfs:comment      "A designation that represents an individual concept." ;
        rdfs:isDefinedBy  <http://www.lexinfo.net/ontology/2.0/lexinfo> ;
        rdfs:label        "appellation" ;
        dc:creator        "Wright, Sue Ellen" ;
        dcr:datcat        <http://www.isocat.org/datcat/DC-347> ;
        owl:versionInfo   "1:0" .

lexinfo:DeclarativeFrame
        a                    owl:Class ;
        rdfs:comment         "Declarative frames take a clause as an argument, this argument is marker with the declarative conjunction (\"that\" in English)"@en ;
        rdfs:isDefinedBy     <http://www.lexinfo.net/ontology/2.0/lexinfo> ;
        rdfs:subClassOf      lexinfo:VerbFrame ;
        owl:equivalentClass  [ a                   owl:Class ;
                               owl:intersectionOf  ( lexinfo:VerbFrame [ a                   owl:Restriction ;
                                                                         owl:minCardinality  "1"^^xsd:nonNegativeInteger ;
                                                                         owl:onProperty      lexinfo:declarativeClause
                                                                       ] )
                             ] .

lemon:Phrase  a  owl:Class .

lexinfo:productName  a    owl:NamedIndividual , lexinfo:TermType , owl:Thing ;
        rdfs:comment      "An attribute assigned to a term indicating that that term is the official designator for a product." ;
        rdfs:isDefinedBy  <http://www.lexinfo.net/ontology/2.0/lexinfo> ;
        rdfs:label        "productName" ;
        dc:creator        "Wright, Sue Ellen" ;
        dcr:datcat        <http://www.isocat.org/datcat/DC-346> ;
        owl:versionInfo   "1:0" .

lexinfo:exact  a            owl:ObjectProperty ;
        rdfs:comment        "Completely correct in every detail" ;
        rdfs:isDefinedBy    <http://www.lexinfo.net/ontology/2.0/lexinfo> ;
        rdfs:label          "exact" ;
        rdfs:subPropertyOf  lemon:equivalent ;
        dc:creator          "Francopoulo, Gil" ;
        dcr:datcat          <http://www.isocat.org/datcat/DC-2205> ;
        owl:versionInfo     "1:0" .

lexinfo:hyponym  a          owl:ObjectProperty ;
        rdfs:isDefinedBy    <http://www.lexinfo.net/ontology/2.0/lexinfo> ;
        rdfs:subPropertyOf  lemon:narrower .

lexinfo:SubjectlessTransitiveFrame
        a                    owl:Class ;
        rdfs:isDefinedBy     <http://www.lexinfo.net/ontology/2.0/lexinfo> ;
        rdfs:subClassOf      lexinfo:SubjectlessFrame ;
        lexinfo:example      "mich FRIERT"@de ;
        owl:equivalentClass  [ a                   owl:Class ;
                               owl:intersectionOf  ( lexinfo:SubjectlessFrame [ a                owl:Restriction ;
                                                                                owl:cardinality  "1"^^xsd:nonNegativeInteger ;
                                                                                owl:onProperty   lexinfo:directObject
                                                                              ] )
                             ] .

lexinfo:RaisingSubject
        a                    owl:Class ;
        rdfs:comment         "Indicates the syntactic subject of the main clause is in fact the subject of the subclause. The main clause should then be interpreted as being impersonal."@en ;
        rdfs:isDefinedBy     <http://www.lexinfo.net/ontology/2.0/lexinfo> ;
        rdfs:subClassOf      lexinfo:Control ;
        owl:equivalentClass  [ a                   owl:Restriction ;
                               owl:onProperty      lexinfo:subject ;
                               owl:someValuesFrom  lexinfo:RaisableSubject
                             ] .

lexinfo:Symbol  a            owl:Class ;
        rdfs:isDefinedBy     <http://www.lexinfo.net/ontology/2.0/lexinfo> ;
        rdfs:subClassOf      lemon:Word ;
        owl:equivalentClass  [ a                   owl:Restriction ;
                               owl:onProperty      lexinfo:partOfSpeech ;
                               owl:someValuesFrom  lexinfo:SymbolPOS
                             ] .

lexinfo:pronominalAdverb
        a                 lexinfo:AdverbPOS , lexinfo:PartOfSpeech , owl:NamedIndividual , owl:Thing ;
        rdfs:comment      "adverb formed in replacement of a preposition and a pronoun" ;
        rdfs:isDefinedBy  <http://www.lexinfo.net/ontology/2.0/lexinfo> ;
        rdfs:label        "pronominal adverb" ;
        dc:creator        "Francopoulo, Gil" ;
        dcr:datcat        <http://www.isocat.org/datcat/DC-2998> ;
        owl:versionInfo   "1:0" .

lexinfo:verbFormMood  a     owl:ObjectProperty ;
        rdfs:comment        "One of a set of distinctive forms that are used to signal modality. Modality is a facet of illocutionary point or general intent of a speaker, or a speaker's degree of commitment to the expressed proposition's believability, obligatoriness, desirability or reality." ;
        rdfs:isDefinedBy    <http://www.lexinfo.net/ontology/2.0/lexinfo> ;
        rdfs:label          "verb form mood" ;
        rdfs:range          lexinfo:VerbFormMood ;
        rdfs:subPropertyOf  lexinfo:morphosyntacticProperty ;
        dc:creator          "Francopoulo, Gil" ;
        dcr:datcat          <http://www.isocat.org/datcat/DC-1427> ;
        owl:versionInfo     "1:0" .

lexinfo:adpositionalObject
        a                   owl:ObjectProperty ;
        rdfs:isDefinedBy    <http://www.lexinfo.net/ontology/2.0/lexinfo> ;
        rdfs:range          lexinfo:AdpositionalObject ;
        rdfs:subPropertyOf  lexinfo:object .

lexinfo:exclamativePronoun
        a                 lexinfo:PronounPOS , lexinfo:PartOfSpeech , owl:Thing , owl:NamedIndividual ;
        rdfs:comment      "Pronoun marked with an emotional utterance and/or a strong intonation." ;
        rdfs:isDefinedBy  <http://www.lexinfo.net/ontology/2.0/lexinfo> ;
        rdfs:label        "exclamative pronoun" ;
        dc:creator        "Francopoulo, Gil" ;
        dcr:datcat        <http://www.isocat.org/datcat/DC-1285> ;
        owl:versionInfo   "1:0" .

lexinfo:indirectObject
        a                   owl:ObjectProperty ;
        rdfs:comment        "An indirect object is a grammatical relation that is one means of expressing the semantic role of goal and other similar roles. It is proposed for languages in which the role is distinct from the direct object and the oblique object on the basis of multiple independent syntactic or morphological criteria, such as the following: - Having a particular case marking, commonly dative - Governing an agreement affix on the verb, such as person or number - Being distinct from oblique relations in that it may be relativized" ;
        rdfs:isDefinedBy    <http://www.lexinfo.net/ontology/2.0/lexinfo> ;
        rdfs:label          "indirect object" ;
        rdfs:range          lexinfo:IndirectObject ;
        rdfs:subPropertyOf  lexinfo:object ;
        dcr:datcat          <http://www.isocat.org/datcat/DC-1310> .

lexinfo:radical  a        owl:NamedIndividual , lexinfo:TermElement , owl:Thing ;
        rdfs:comment      "A basic identifiable component of every CJKV character, often found on the left side of the character, that sometimes gives a rough indication of meaning and is used for collating lexical and terminological resources." ;
        rdfs:isDefinedBy  <http://www.lexinfo.net/ontology/2.0/lexinfo> ;
        rdfs:label        "radical" ;
        dc:creator        "Wright, Sue Ellen" ;
        dcr:datcat        <http://www.isocat.org/datcat/DC-296> ;
        owl:versionInfo   "1:0" .

lexinfo:inchoative  a     owl:NamedIndividual , lexinfo:Aspect , owl:Thing ;
        rdfs:comment      "Aspect that expresses the beginning of an event or state." ;
        rdfs:isDefinedBy  <http://www.lexinfo.net/ontology/2.0/lexinfo> ;
        rdfs:label        "inchoative" ;
        dc:creator        "Francopoulo, Gil" ;
        dcr:datcat        <http://www.isocat.org/datcat/DC-2002> ;
        owl:versionInfo   "1:0" .

lexinfo:frequency  a        owl:ObjectProperty ;
        rdfs:comment        "The relative commonness with which a term occurs." ;
        rdfs:isDefinedBy    <http://www.lexinfo.net/ontology/2.0/lexinfo> ;
        rdfs:label          "frequency" ;
        rdfs:range          lexinfo:Frequency ;
        rdfs:subPropertyOf  lemon:property ;
        dc:creator          "Wright, Sue Ellen" , "Francopoulo, Gil" ;
        dcr:datcat          <http://www.isocat.org/datcat/DC-1965> , <http://www.isocat.org/datcat/DC-233> ;
        owl:versionInfo     "1:0" .
