@prefix adms:  <http://www.w3.org/ns/adms#> .
@prefix dc:    <http://purl.org/dc/elements/1.1/> .
@prefix rdfs:  <http://www.w3.org/2000/01/rdf-schema#> .
@prefix cogs:  <http://vocab.deri.ie/cogs#> .
@prefix foaf:  <http://xmlns.com/foaf/0.1/> .
@prefix owl:   <http://www.w3.org/2002/07/owl#> .
@prefix xsd:   <http://www.w3.org/2001/XMLSchema#> .
@prefix rdf:   <http://www.w3.org/1999/02/22-rdf-syntax-ns#> .
@prefix vann:  <http://purl.org/vocab/vann/> .
@prefix dcterms: <http://purl.org/dc/terms/> .

cogs:Ceil  a             owl:Class , rdfs:Class ;
        rdfs:comment     "Returns the smallest integer greater than or equal to n. @en-us" ;
        rdfs:label       "Ceil" ;
        rdfs:subClassOf  cogs:NumericOperation .

cogs:KeyGeneration  a    owl:Class , rdfs:Class ;
        rdfs:comment     "Process of generating keys/indexes for tables. @en-us" ;
        rdfs:label       "KeyGeneration" ;
        rdfs:subClassOf  cogs:Operation .

cogs:Column  a        owl:Class , rdfs:Class ;
        rdfs:comment  "Database tables are composed of individual columns corresponding to the attributes of the object. @en-us" ;
        rdfs:label    "Column" .

cogs:Server  a        owl:Class , rdfs:Class ;
        rdfs:comment  "Software program, or the computer on which that program runs, that provides a specific kind of service to a client software. @en-us" ;
        rdfs:label    "Server" .

cogs:InsertTriple  a     owl:Class , rdfs:Class ;
        rdfs:comment     "Includes one or more triple into the store. @en-us" ;
        rdfs:label       "InsertTriple" ;
        rdfs:subClassOf  cogs:GraphOperation .

cogs:HumanValidation  a  owl:Class , rdfs:Class ;
        rdfs:comment     "Validation performed by a person:  an user or admin. @en-us" ;
        rdfs:label       "HumanValidation" ;
        rdfs:subClassOf  cogs:Validation .

cogs:Extraction  a    owl:Class , rdfs:Class ;
        rdfs:comment  "The first part of an ETL process which involves extracting the data from source systems. @en-us" ;
        rdfs:label    "Extraction" .

cogs:Cube  a          owl:Class , rdfs:Class ;
        rdfs:comment  "A multidimensional database that holds data. @en-us" ;
        rdfs:label    "Cube" .

cogs:Operation  a        owl:Class , rdfs:Class ;
        rdfs:comment     "Functional operations that can be done by a computer. " ;
        rdfs:label       "Operation" ;
        rdfs:subClassOf  cogs:Transformation .

cogs:FieldDecoding  a    owl:Class , rdfs:Class ;
        rdfs:comment     "Performs decoding operations when you specify field-encoding function. @en-us" ;
        rdfs:label       "FieldDecoding" ;
        rdfs:subClassOf  cogs:ValueOperation .

cogs:DatetimeConversion
        a                owl:Class , rdfs:Class ;
        rdfs:comment     "Conversion from a datetime format to a different one." ;
        rdfs:label       "DatetimeConversion" ;
        rdfs:subClassOf  cogs:ValueOperation .

cogs:TerminologicalMapping
        a                owl:Class , rdfs:Class ;
        rdfs:comment     "Maps terminological-level (schema-level) entities. @en-us" ;
        rdfs:label       "TerminologicalMapping" ;
        rdfs:subClassOf  cogs:Mapping .

cogs:StringOperation  a  owl:Class , rdfs:Class ;
        rdfs:comment     "Operations for manipulating strings. @en-us" ;
        rdfs:label       "StringOperation" ;
        rdfs:subClassOf  cogs:ValueOperation .

cogs:Filter  a           owl:Class , rdfs:Class ;
        rdfs:comment     "An operation that can be used to retain rows in a mapping that do not meet specific conditions. @en-us" ;
        rdfs:label       "Filter" ;
        rdfs:subClassOf  cogs:Operation .

cogs:isExpressedBy  a  rdf:Property ;
        rdfs:comment  "This property allows the association between an abstract representation of a Transformation and an encapsulated computational artifact artifact (e.g. code, binary)." ;
        rdfs:domain   cogs:Transformation ;
        rdfs:label    "isExpressedBy" .

cogs:RejectedData  a  owl:Class , rdfs:Class ;
        rdfs:comment  "Data that contain database violations and are forbidden to get inserted into a table. @en-us" ;
        rdfs:label    "RejectedData" .

cogs:Event  a         owl:Class , rdfs:Class ;
        rdfs:comment  "An action that is usually initiated outside the scope of a program and that is handled by a piece of code inside the program. @en-us" ;
        rdfs:label    "Event" .

<http://vocab.deri.ie/cogs#AIFB%2FKIT>
        a              dcterms:Agent ;
        foaf:homepage  <http://www.kit.edu/> ;
        foaf:member    cogs:benkam ;
        foaf:name      "AIFB/KIT" .

cogs:AutomatedValidation
        a                owl:Class , rdfs:Class ;
        rdfs:comment     "Validation performed by a computer. @en-us" ;
        rdfs:label       "AutomatedValidation" ;
        rdfs:subClassOf  cogs:Validation .

cogs:Parsing  a          owl:Class , rdfs:Class ;
        rdfs:comment     "Process of analyzing text or data, checking for correct syntax and building a representation based on the input tokens. @en-us" ;
        rdfs:label       "Parsing" ;
        rdfs:subClassOf  cogs:Extraction .

cogs:StringFilter  a     owl:Class , rdfs:Class ;
        rdfs:comment     "Provides means for matching strings of text, such as particular characters, words, or patterns of characters. @en-us" ;
        rdfs:label       "StringFilter" ;
        rdfs:subClassOf  cogs:Filter .

cogs:GraphOperation  a   owl:Class , rdfs:Class ;
        rdfs:comment     "Instructions performed on graphs. @en-us" ;
        rdfs:label       "GraphOperation" ;
        rdfs:subClassOf  cogs:Operation .

cogs:Log  a           owl:Class , rdfs:Class ;
        rdfs:comment  "A record of computer activity. @en-us" ;
        rdfs:label    "Log" .

cogs:dependsOn  a    rdf:Property ;
        rdfs:domain  cogs:Job ;
        rdfs:label   "dependsOn" ;
        rdfs:range   cogs:Job .

cogs:FormatRevision  a   owl:Class , rdfs:Class ;
        rdfs:comment     "Reviews the file format. @en-us" ;
        rdfs:label       "FormatRevision" ;
        rdfs:subClassOf  cogs:ValueOperation .

cogs:DeleteTriple  a     owl:Class , rdfs:Class ;
        rdfs:comment     "Deletes on or more triples into the store.@en-us" ;
        rdfs:label       "DeleteTriple" ;
        rdfs:subClassOf  cogs:GraphOperation .

cogs:Success  a          owl:Class , rdfs:Class ;
        rdfs:comment     "Status of a job that had successful  performance. @en-us" ;
        rdfs:label       "Success" ;
        rdfs:subClassOf  cogs:ExecutionStatus .

cogs:DeleteRow  a        owl:Class , rdfs:Class ;
        rdfs:comment     "Exclusion of a single or group of rows by a certain criteria on a table. @en-us" ;
        rdfs:label       "DeleteRow" ;
        rdfs:subClassOf  cogs:RowOperation .

cogs:MappingProcess  a   owl:Class , rdfs:Class ;
        rdfs:comment     "The process of mapping information from a source format to a destination format. @en-us" ;
        rdfs:label       "MappingProcess" ;
        rdfs:subClassOf  cogs:Mapping .

cogs:AggregateRows  a    owl:Class , rdfs:Class ;
        rdfs:comment     " Functions which return a single result row based on groups of rows. @en-us" ;
        rdfs:label       "AggregateRows" ;
        rdfs:subClassOf  cogs:RowOperation .

cogs:SelectQueryObject
        a                owl:Class , rdfs:Class ;
        rdfs:comment     "Query that locates and displays information requested. @en-us" ;
        rdfs:label       "SelectQuery" ;
        rdfs:subClassOf  cogs:QueryObject .

cogs:Device  a        owl:Class , rdfs:Class ;
        rdfs:comment  "A machine designed for a purpose. E.g.: Unit of hardware.  @en-us" ;
        rdfs:label    "Device" .

cogs:ApplyScript  a      owl:Class , rdfs:Class ;
        rdfs:comment     "Execution of a script. @en-us" ;
        rdfs:label       "ApplyScript" ;
        rdfs:subClassOf  cogs:Operation .

cogs:TableLookup  a      owl:Class , rdfs:Class ;
        rdfs:comment     "Process of using a known attribute to search for data on a table. @en-us" ;
        rdfs:label       "TableLookup" ;
        rdfs:subClassOf  cogs:Lookup .

cogs:Job  a              owl:Class , rdfs:Class ;
        rdfs:comment     "The instance of a process or group of processes (workflow)." ;
        rdfs:label       "Job" ;
        rdfs:subClassOf  cogs:Execution .

cogs:DataAccessLayer  a  owl:Class , rdfs:Class ;
        rdfs:comment     "Layer that controls access to data in a computer-based information system. @en-us" ;
        rdfs:label       "DataAccessLayer" ;
        rdfs:subClassOf  cogs:Layer .

cogs:InsertColumn  a     owl:Class , rdfs:Class ;
        rdfs:comment     "Inserts one or more columns according to a certain criteria to a table. @en-us" ;
        rdfs:label       "InsertColumn" ;
        rdfs:subClassOf  cogs:ColumnOperation .

cogs:RenameColumn  a     owl:Class , rdfs:Class ;
        rdfs:comment     "Changes the name of a certain column. @en-us" ;
        rdfs:label       "RenameColumn" ;
        rdfs:subClassOf  cogs:ColumnOperation .

cogs:Validation  a       owl:Class , rdfs:Class ;
        rdfs:comment     "The act of validating; finding or testing the truth of something. @en-us" ;
        rdfs:label       "Validation" ;
        rdfs:subClassOf  cogs:Transformation .

cogs:RDFNamedGraph  a  owl:Class , rdfs:Class ;
        rdfs:comment  "Multiple RDF graphs in a single document/repository and naming them with URIs. @en-us" ;
        rdfs:label    "RDFNamedGraph" .

cogs:Prefiltering  a     owl:Class , rdfs:Class ;
        rdfs:comment     "Preliminary filtering during the extraction phase." ;
        rdfs:label       "Prefiltering" ;
        rdfs:subClassOf  cogs:Extraction .

cogs:Trim  a             owl:Class , rdfs:Class ;
        rdfs:comment     "String operation for removing leading and trailing whitespace from a string. @en-us" ;
        rdfs:label       "Trim" ;
        rdfs:subClassOf  cogs:StringOperation .

cogs:Uppercase  a        owl:Class , rdfs:Class ;
        rdfs:comment     "String operation for converting a string to uppercase. @en-us" ;
        rdfs:label       "Uppercase" ;
        rdfs:subClassOf  cogs:StringOperation .

cogs:Transformation  a   owl:Class , rdfs:Class ;
        rdfs:comment     "The process of manipulating data. @en-us" ;
        rdfs:label       "Transformation" ;
        rdfs:subClassOf  owl:Thing .

cogs:SimilarityMatching
        a                owl:Class , rdfs:Class ;
        rdfs:comment     "The process of matching two objects by a similarity measure. @en-us" ;
        rdfs:label       "SimilarityMatching" ;
        rdfs:subClassOf  cogs:AutomatedMatching .

cogs:Loading  a       owl:Class , rdfs:Class ;
        rdfs:comment  "Stage that is responsible for loading data into the end target. @en-us" ;
        rdfs:label    "Loading" .

cogs:MappingFile  a   owl:Class , rdfs:Class ;
        rdfs:comment  "The specification of a mapping between source and target fields (e.g. RDB2RDF)." ;
        rdfs:label    "MappingFile" .

cogs:Trigger  a       owl:Class , rdfs:Class ;
        rdfs:comment  "A procedural code that is automatically executed in response to certain events on a particular table or view in a database.  @en-us" ;
        rdfs:label    "Trigger" .

cogs:KeyRestructuring
        a                owl:Class , rdfs:Class ;
        rdfs:comment     "Transformation of keys with built-in meanings into generic keys. @en-us" ;
        rdfs:label       "KeyRestructuring" ;
        rdfs:subClassOf  cogs:RowOperation .

cogs:DeleteQueryObject
        a                owl:Class , rdfs:Class ;
        rdfs:comment     "Query that does a delete operation on a row, column, table for example. @en-us" ;
        rdfs:label       "DeleteQuery" ;
        rdfs:subClassOf  cogs:QueryObject .

cogs:Formula  a       owl:Class , rdfs:Class ;
        rdfs:comment  "A rule or principle. @en-us" ;
        rdfs:label    "Formula" .

<http://vocab.deri.ie/cogs#DERI%2C%20NUI%20Galway>
        a              dcterms:Agent ;
        foaf:homepage  <http://www.deri.ie/> ;
        foaf:member    cogs:andfre ;
        foaf:name      "DERI, NUI Galway" .

<http://vocab.deri.ie/cogs>
        a                              adms:SemanticAsset , owl:Ontology ;
        dc:creator                     cogs:benkam , cogs:andfre , cogs:timleb ;
        dcterms:created                "2014-03-10"^^xsd:date ;
        dcterms:description            "COGS: Vocabulary for describing ETL and data transformation activities." ;
        dcterms:modified               "2014-03-10"^^xsd:date ;
        dcterms:partOf                 <http://vocab.deri.ie> ;
        dcterms:publisher              "http://vocab.deri.ie/cogs#DERI%2C%20NUI%20Galway" ;
        dcterms:status                 <http://purl.org/adms/status/UnderDevelopment> ;
        dcterms:title                  "COGS Vocabulary" ;
        dcterms:type                   <http://purl.org/adms/assettype/Ontology> ;
        vann:preferredNamespacePrefix  "cogs" ;
        vann:preferredNamespaceUri     "http://vocab.deri.ie/cogs#" ;
        foaf:homepage                  <http://vocab.deri.ie/cogs.html> .

cogs:StagingAreaArtifact
        a             owl:Class , rdfs:Class ;
        rdfs:comment  "The final product; what the end users see. @en-us" ;
        rdfs:label    "StagingAreaArtifact" .

cogs:Running  a          owl:Class , rdfs:Class ;
        rdfs:comment     "Status of a job that is in the state of being operated. @en-us" ;
        rdfs:label       "Running" ;
        rdfs:subClassOf  cogs:ExecutionStatus .

cogs:RDFGraph  a      owl:Class , rdfs:Class ;
        rdfs:comment  "A set of RDF triples. @en-us" ;
        rdfs:label    "RDFGraph" .

cogs:AutomatedMatching
        a                owl:Class , rdfs:Class ;
        rdfs:comment     "Task of finding entries that refer to the same entity across different data sources using computer resources. @en-us" ;
        rdfs:label       "AutomatedMatching" ;
        rdfs:subClassOf  cogs:MappingProcess .

cogs:Exception  a     owl:Class , rdfs:Class ;
        rdfs:comment  "An event, which occurs during the execution of a program, which disrupts the normal flow of the program's instructions. @en-us" ;
        rdfs:label    "Exception" .

cogs:Row  a           owl:Class , rdfs:Class ;
        rdfs:comment  "A serie of objects placed in line. @en-us" ;
        rdfs:label    "Row" .

cogs:ExecutionStatus  a  owl:Class , rdfs:Class ;
        rdfs:comment  "Provides the current execution status of a running process instance (a job). e.g. : fail, running, success. @en-us" ;
        rdfs:label    "ExecutionStatus" .

cogs:StringSimilarity
        a                owl:Class , rdfs:Class ;
        rdfs:comment     "Matching based on string similarity measures. @en-us" ;
        rdfs:label       "StringSimilarity" ;
        rdfs:subClassOf  cogs:SimilarityMatching .

cogs:Assignment  a       owl:Class , rdfs:Class ;
        rdfs:comment     "Sets or re-sets the value stored in the storage location(s) denoted by a variable name. @en-us" ;
        rdfs:label       "Assignment" ;
        rdfs:subClassOf  cogs:ValueOperation .

cogs:ManualAdHocProcess
        a                owl:Class , rdfs:Class ;
        rdfs:comment     "A non-recurrent, not-frequent manual process." ;
        rdfs:label       "ManualAdHocProcess" ;
        rdfs:subClassOf  cogs:AdHocProcess .

cogs:PerformanceIndicator
        a             owl:Class , rdfs:Class ;
        rdfs:comment  "Measures used to evaluate the success of a particular activity. " ;
        rdfs:label    "PerformanceIndicator" .

cogs:ValueOperation  a   owl:Class , rdfs:Class ;
        rdfs:comment     "Evaluate a selected function for a particular value of x. @en-us" ;
        rdfs:label       "ValueOperation" ;
        rdfs:subClassOf  cogs:Operation .

cogs:Rule  a          owl:Class , rdfs:Class ;
        rdfs:comment  "A principle or formula. @en-us" ;
        rdfs:label    "Rule" .

cogs:UpdateQueryObject
        a                owl:Class , rdfs:Class ;
        rdfs:comment     "Query that changes the data of one or more records in a table.  @en-us" ;
        rdfs:label       "UpdateQuery" ;
        rdfs:subClassOf  cogs:QueryObject .

cogs:ColumnOperation  a  owl:Class , rdfs:Class ;
        rdfs:comment     "Instructions applied on one or more columns. @en-us" ;
        rdfs:label       "ColumnOperation" ;
        rdfs:subClassOf  cogs:Operation .

cogs:Output  a        owl:Class , rdfs:Class ;
        rdfs:comment  "Information, resulting from computer processing, that is delivered to a user. @en-us" ;
        rdfs:label    "Output" .

cogs:JoinRows  a         owl:Class , rdfs:Class ;
        rdfs:comment     "Row Operation that allows combinations (Cartesian product) of all rows in the input streams.@en-us" ;
        rdfs:label       "JoinRows" ;
        rdfs:subClassOf  cogs:RowOperation .

cogs:IncrementalLoad  a  owl:Class , rdfs:Class ;
        rdfs:comment     "Applies ongoing changes to one or more tables based on a predefined schedule. @en-us" ;
        rdfs:label       "IncrementalLoad" ;
        rdfs:subClassOf  cogs:Loading .

cogs:ScheduledJob  a     owl:Class , rdfs:Class ;
        rdfs:comment     "Job that owns information on when and how often it has to execute operations. @en-us" ;
        rdfs:label       "ScheduledJob" ;
        rdfs:subClassOf  cogs:Job .

cogs:Program  a       owl:Class , rdfs:Class ;
        rdfs:comment  "A sequence of instructions written to perform a specified task for a computer. @en-us" ;
        rdfs:label    "Program" .

cogs:precededBy  a          rdf:Property ;
        rdfs:comment        "Defines the ordering among two processes" ;
        rdfs:label          "precededBy" ;
        rdfs:subPropertyOf  owl:topObjectProperty .

cogs:Sensor  a        owl:Class , rdfs:Class ;
        rdfs:comment  "Device that measures or detects a real-world condition and converts the condition into an analog or digital representation. @en-us" ;
        rdfs:label    "Sensor" .

cogs:InsertRow  a        owl:Class , rdfs:Class ;
        rdfs:comment     "Inclusion of a row on a table. @en-us" ;
        rdfs:label       "InsertRow" ;
        rdfs:subClassOf  cogs:RowOperation .

cogs:Layer  a         owl:Class , rdfs:Class ;
        rdfs:comment  "Each individual level. @en-us" ;
        rdfs:label    "Layer" .

cogs:AutomatedAdHocProcess
        a                owl:Class , rdfs:Class ;
        rdfs:comment     "A non-recurrent, not frequent automated process." ;
        rdfs:label       "AutomatedAdHocProcess" ;
        rdfs:subClassOf  cogs:AdHocProcess .

cogs:FillDown  a         owl:Class , rdfs:Class ;
        rdfs:comment     "Copy the contents of the topmost cells of a selected range into the cells below.@en-us" ;
        rdfs:label       "FillDown" ;
        rdfs:subClassOf  cogs:ColumnOperation .

cogs:Lowercase  a        owl:Class , rdfs:Class ;
        rdfs:comment     "String operation for converting a string to lowercase.@en-us" ;
        rdfs:label       "Lowercase" ;
        rdfs:subClassOf  cogs:StringOperation .

cogs:NumericCast  a      owl:Class , rdfs:Class ;
        rdfs:comment     "Converts an expression of one numeric data type to another. @en-us" ;
        rdfs:label       "NumericCast" ;
        rdfs:subClassOf  cogs:NumericOperation .

cogs:DimensionTable  a   owl:Class , rdfs:Class ;
        rdfs:comment     "One of the set of companion tables to a fact table. @en-us" ;
        rdfs:label       "DimensionTable" ;
        rdfs:subClassOf  cogs:Table .

cogs:Lookup  a           owl:Class , rdfs:Class ;
        rdfs:comment     "A process used to look up data in a relational table, view or dictionary. @en-us" ;
        rdfs:label       "Lookup" ;
        rdfs:subClassOf  cogs:Transformation .

cogs:RDFDataPropertyMapping
        a                owl:Class , rdfs:Class ;
        rdfs:comment     "Maps data properties from source to target." ;
        rdfs:label       "RDFDataPropertyMapping" ;
        rdfs:subClassOf  cogs:TerminologicalMapping .

cogs:RegexFilter  a      owl:Class , rdfs:Class ;
        rdfs:comment     "Filter written in a formal language that can be interpreted by a regular expression processor. @en-us" ;
        rdfs:label       "RegexFilter" ;
        rdfs:subClassOf  cogs:Filter .

cogs:Split  a            owl:Class , rdfs:Class ;
        rdfs:comment     "String operation that returns a zero-based, one-dimensional array containing a specified number of substrings. @en-us" ;
        rdfs:label       "Split" ;
        rdfs:subClassOf  cogs:StringOperation .

cogs:RESTLookup  a       owl:Class , rdfs:Class ;
        rdfs:comment     "Lookup on a REST service. @en-us" ;
        rdfs:label       "RESTLookup" ;
        rdfs:subClassOf  cogs:Lookup .

cogs:Script  a        owl:Class , rdfs:Class ;
        rdfs:comment  "A program or sequence of instructions that is interpreted or carried out by another program rather than by the computer processor. @en-us" ;
        rdfs:label    "Script" .

cogs:Order  a            owl:Class , rdfs:Class ;
        rdfs:comment     "Application of a specific order to a set of elemetns.  @en-us" ;
        rdfs:label       "Order" ;
        rdfs:subClassOf  cogs:Operation .

cogs:StoredProcedure  a  owl:Class , rdfs:Class ;
        rdfs:comment  "A transformation used to create unique primary key values or cycle through a sequential range of numbers to replace missing keys. @en-us" ;
        rdfs:label    "StoredProcedure" .

cogs:Metadata  a      owl:Class , rdfs:Class ;
        rdfs:comment  "Data that describe data and other structures, such as objects, business rules and processes. @en-us" ;
        rdfs:label    "Metadata" .

cogs:DataStream  a    owl:Class , rdfs:Class ;
        rdfs:comment  "A sequence of digitally encoded coherent signals (packets of data) used to transmit or receive information that is in the process of being transmitted. @en-us" ;
        rdfs:label    "DataStream" .

cogs:ApplyFormula  a     owl:Class , rdfs:Class ;
        rdfs:comment     "New data are computed based on the user-defined formula. @en-us" ;
        rdfs:label       "ApplyFormula" ;
        rdfs:subClassOf  cogs:NumericOperation .

cogs:DataMart  a      owl:Class , rdfs:Class ;
        rdfs:comment  "Data mart is a process-oriented subset of the overall organization’s data based on a foundation of atomic data, and that depends only on the structure of the data-measurement events, not on the anticipated user’s questions." ;
        rdfs:label    "DataMart" .

cogs:Execution  a     owl:Class , rdfs:Class ;
        rdfs:comment  "The instantiation of an activity or workflow. @en-us" ;
        rdfs:label    "Execution" .

cogs:DestructiveMerge
        a                owl:Class , rdfs:Class ;
        rdfs:comment     "Inputs the incoming data to the target data if the primary key of an incoming record matches with the key of an existing record, updating the matching target record. If the incoming record is a new record without a match with any existing record, it adds the incoming record to the target table. @en-us" ;
        rdfs:label       "DestructiveMerge" ;
        rdfs:subClassOf  cogs:Loading .

cogs:Move  a             owl:Class , rdfs:Class ;
        rdfs:comment     "To change in position from one point to another. @en-us" ;
        rdfs:label       "Move" ;
        rdfs:subClassOf  cogs:Operation .

cogs:FileLookup  a       owl:Class , rdfs:Class ;
        rdfs:comment     "The process of looking up for information on a file. @en-us" ;
        rdfs:label       "FileLookup" ;
        rdfs:subClassOf  cogs:Lookup .

cogs:Paste  a            owl:Class , rdfs:Class ;
        rdfs:comment     "To copy an object from a buffer  or clipboard to a file. @en-us" ;
        rdfs:label       "Paste" ;
        rdfs:subClassOf  cogs:Operation .

cogs:ObjectReference  a  owl:Class , rdfs:Class ;
        rdfs:comment  "Value that enables a program to indirectly access a particular object. @en-us" ;
        rdfs:label    "ObjectReference" .

cogs:Mapping  a          owl:Class , rdfs:Class ;
        rdfs:comment     "The definition of a semantic equivalence relationship between source and target objects. @en-us" ;
        rdfs:label       "Mapping" ;
        rdfs:subClassOf  cogs:Transformation .

cogs:andfre  a         foaf:Person ;
        foaf:homepage  <http://vocab.deri.ie/cogs> ;
        foaf:name      "André Freitas" .

cogs:RowOperation  a     owl:Class , rdfs:Class ;
        rdfs:comment     "Instructions executed on rows of a table or file. @en-us" ;
        rdfs:label       "RowOperation" ;
        rdfs:subClassOf  cogs:Operation .

cogs:SemanticSimilarity
        a                owl:Class , rdfs:Class ;
        rdfs:comment     "Matching by a measure of semantic similarity. @en-us" ;
        rdfs:label       "SemanticSimilarity" ;
        rdfs:subClassOf  cogs:SimilarityMatching .

cogs:rdf  a                 adms:SemanticDistribution ;
        dcterms:FileFormat  <http://vocab.deri.ie/cogs> ;
        adms:accessURL      "http://vocab.deri.ie/cogs.rdf" ;
        adms:status         <http://purl.org/adms/status/Completed> .

cogs:Service  a       owl:Class , rdfs:Class ;
        rdfs:comment  "Action done by a device or user with the function of giving good by providing usefulness. @en-us" ;
        rdfs:label    "Service" .

cogs:benkam  a         foaf:Person ;
        foaf:homepage  <http://vocab.deri.ie/cogs> ;
        foaf:name      "Benedikt Kämpgen" .

cogs:ManuallyStartedJob
        a                owl:Class , rdfs:Class ;
        rdfs:comment     "Job that was initialized by an user. @en-us" ;
        rdfs:label       "ManuallyStartedJob" ;
        rdfs:subClassOf  cogs:Job .

cogs:Method  a        owl:Class , rdfs:Class ;
        rdfs:comment  "A subroutine that is exclusively associated with a object. @en-us" ;
        rdfs:label    "Method" .

cogs:MergeRow  a         owl:Class , rdfs:Class ;
        rdfs:comment     "Row Operation that allows the comparison of two streams of rows. It is often used in situations where the source system of a data warehouse does not contain a date of last update. @en-us" ;
        rdfs:label       "MergeRow" ;
        rdfs:subClassOf  cogs:RowOperation .

cogs:DataManagementLayer
        a                owl:Class , rdfs:Class ;
        rdfs:comment     "Layer responsible for the development, execution and supervision of plans, policies, programs and practices that control, protect, deliver and enhance the value of data and information assets. @en-us" ;
        rdfs:label       "DataManagementLayer" ;
        rdfs:subClassOf  cogs:Layer .

cogs:PresentationArea
        a                owl:Class , rdfs:Class ;
        rdfs:comment     "What the user sees. @en-us" ;
        rdfs:label       "PresentationArea" ;
        rdfs:subClassOf  cogs:DataAccessLayer .

cogs:UnitConversion  a   owl:Class , rdfs:Class ;
        rdfs:comment     "Conversion on different units of measurement. @en-us" ;
        rdfs:label       "UnitConversion" ;
        rdfs:subClassOf  cogs:ValueOperation .

cogs:WebServiceLookup
        a                owl:Class , rdfs:Class ;
        rdfs:comment     "Allows the retrieving of data from a web service and uses this during the form filling process.  @en-us" ;
        rdfs:label       "WebServiceLookup" ;
        rdfs:subClassOf  cogs:Lookup .

cogs:RulesBasedMatching
        a                owl:Class , rdfs:Class ;
        rdfs:comment     "Matching of data based on a rule or group of rules. @en-us" ;
        rdfs:label       "RulesBasedMatching" ;
        rdfs:subClassOf  cogs:AutomatedMatching .

cogs:Endpoint  a      owl:Class , rdfs:Class ;
        rdfs:comment  "Database access point as a web service (SPARQL Endpoint) . @en-us" ;
        rdfs:label    "Endpoint" .

cogs:AdHocProcess  a     owl:Class , rdfs:Class ;
        rdfs:comment     "Process that seeks a solution designed for a specific problem or task, non-generalizable, and not intended to be able to be adapted to other purposes. @en-us" ;
        rdfs:label       "AdHocProcess" ;
        rdfs:subClassOf  cogs:Execution .

cogs:hasStartPoint  a  rdf:Property ;
        rdfs:comment  "First process in a transformation workflow." ;
        rdfs:domain   cogs:Transformation ;
        rdfs:label    "hasStartPoint" ;
        rdfs:range    cogs:Transformation .

cogs:InsertQueryObject
        a                owl:Class , rdfs:Class ;
        rdfs:comment     "Query that inserts data into the database. @en-us" ;
        rdfs:label       "InsertQuery" ;
        rdfs:subClassOf  cogs:QueryObject .

cogs:Operator  a      owl:Class , rdfs:Class ;
        rdfs:comment  "A symbol or function representing a mathematical operation. @en-us" ;
        rdfs:label    "Operator" .

cogs:Publication  a   owl:Class , rdfs:Class ;
        rdfs:comment  "The process of publishing the output of an ETL process. @en-us" ;
        rdfs:label    "Publication" .

cogs:InitialLoad  a      owl:Class , rdfs:Class ;
        rdfs:comment     "Populates the tables in the data warehouse schema and verifies if the data is ready for use. @en-us" ;
        rdfs:label       "InitialLoad" ;
        rdfs:subClassOf  cogs:Loading .

cogs:File  a          owl:Class , rdfs:Class ;
        rdfs:comment  "A block of arbitrary information, or resource for storing information, which is available to a computer program. @en-us" ;
        rdfs:label    "File" .

cogs:Schema  a        owl:Class , rdfs:Class ;
        rdfs:comment  "The structure of a database system described in a formal language supported by the database management system. Describes tables, for example. @en-us" ;
        rdfs:label    "Schema" .

cogs:Copy  a             owl:Class , rdfs:Class ;
        rdfs:comment     "A piece of data that was duplicated. @en-us" ;
        rdfs:label       "Copy" ;
        rdfs:subClassOf  cogs:Operation .

cogs:DSN  a           owl:Class , rdfs:Class ;
        rdfs:comment  "Data Source Name (DSN) is a data structure that contains the information about a specific database. @en-us" ;
        rdfs:label    "DSN" .

cogs:ValueCalculation
        a                owl:Class , rdfs:Class ;
        rdfs:comment     "A calculation performed on a specified input value. " ;
        rdfs:label       "ValueCalculation" ;
        rdfs:subClassOf  cogs:ValueOperation .

cogs:CharacterSetConversion
        a                owl:Class , rdfs:Class ;
        rdfs:comment     "Converts strings between different character sets. @en-us" ;
        rdfs:label       "CharacterSetConversion" ;
        rdfs:subClassOf  cogs:ValueOperation .

cogs:timleb  a         foaf:Person ;
        foaf:homepage  <http://vocab.deri.ie/cogs> ;
        foaf:mbox      <mailto:lebot@rpi.edu> ;
        foaf:name      "Timothy Lebo" .

cogs:Database  a      owl:Class , rdfs:Class ;
        rdfs:comment  "A database is a collection of information organized into interrelated tables of data and specifications of data objects. @en-us" ;
        rdfs:label    "Database" .

cogs:Class  a         owl:Class , rdfs:Class ;
        rdfs:comment  "A construct that is used as a blueprint to create instances of the class. @en-us" ;
        rdfs:label    "Class" .

cogs:NumericOperation
        a                owl:Class , rdfs:Class ;
        rdfs:comment     "Manipulate and manage numeric data. @en-us" ;
        rdfs:label       "NumericOperation" ;
        rdfs:subClassOf  cogs:ValueOperation .

cogs:DeleteColumn  a     owl:Class , rdfs:Class ;
        rdfs:comment     "Deletes one or more columns according to a certain criteria to a table. @en-us" ;
        rdfs:label       "DeleteColumn" ;
        rdfs:subClassOf  cogs:ColumnOperation .

cogs:HumanMatching  a    owl:Class , rdfs:Class ;
        rdfs:comment     "Matching based on a human decision." ;
        rdfs:label       "HumanMatching" ;
        rdfs:subClassOf  cogs:MappingProcess .

cogs:Round  a            owl:Class , rdfs:Class ;
        rdfs:comment     "Round a numeric value to a close number by following a specific rounding criteria. @en-us" ;
        rdfs:label       "Round" ;
        rdfs:subClassOf  cogs:NumericOperation .

cogs:QueryObject  a   owl:Class , rdfs:Class ;
        rdfs:comment  "A structured object which is used to request information or perform an action in a database. @en-us" ;
        rdfs:label    "Query" .

cogs:hasEndPoint  a   rdf:Property ;
        rdfs:comment  "Last process in a transformation workflow." ;
        rdfs:domain   cogs:Transformation ;
        rdfs:label    "hasEndPoint" ;
        rdfs:range    cogs:Transformation .

cogs:Input  a         owl:Class , rdfs:Class ;
        rdfs:comment  "Any data entered into a computer.@en-us" ;
        rdfs:label    "Input" .

cogs:Source  a           owl:Class , rdfs:Class ;
        rdfs:comment     "A database, application, file or other storage facility from which the data is derived. @en-us" ;
        rdfs:label       "Source" ;
        rdfs:subClassOf  cogs:DataManagementLayer .

cogs:Fail  a             owl:Class , rdfs:Class ;
        rdfs:comment     "Status of a job that stops operating or functioning. @en-us" ;
        rdfs:label       "Fail" ;
        rdfs:subClassOf  cogs:ExecutionStatus .

cogs:RDFObjectPropertyMapping
        a                owl:Class , rdfs:Class ;
        rdfs:comment     "Maps object properties from source to target." ;
        rdfs:label       "RDFObjectPropertyMapping" ;
        rdfs:subClassOf  cogs:TerminologicalMapping .

cogs:PredefinedMatching
        a                owl:Class , rdfs:Class ;
        rdfs:comment     "Forces a matching under a certain predefined criteria.  @en-us" ;
        rdfs:label       "PredefinedMatching" ;
        rdfs:subClassOf  cogs:MappingProcess .

cogs:ConstructiveMerge
        a                owl:Class , rdfs:Class ;
        rdfs:comment     "If the primary key of an incoming record matches with the key of an existing Record, leaves the existing Record, adds the incoming record and marks the added record as superseding the old record. @en-us" ;
        rdfs:label       "ConstructiveMerge" ;
        rdfs:subClassOf  cogs:Loading .

cogs:ttl  a                 adms:SemanticDistribution ;
        dcterms:FileFormat  <http://vocab.deri.ie/cogs> ;
        adms:accessURL      "http://vocab.deri.ie/cogs.ttl" ;
        adms:status         <http://purl.org/adms/status/Completed> .

cogs:Deduplication  a    owl:Class , rdfs:Class ;
        rdfs:comment     "Elimination of redundant data. @en-us" ;
        rdfs:label       "Deduplication" ;
        rdfs:subClassOf  cogs:RowOperation .

cogs:ObjectRepresentation
        a             owl:Class , rdfs:Class ;
        rdfs:comment  "Internal representation of an object suitable for matching its features. @en-us" ;
        rdfs:label    "ObjectRepresentation" .

cogs:Append  a           owl:Class , rdfs:Class ;
        rdfs:comment     "String operation for concatenating lists or arrays. @en-us" ;
        rdfs:label       "Append" ;
        rdfs:subClassOf  cogs:StringOperation .

cogs:View  a          owl:Class , rdfs:Class ;
        rdfs:comment  "Consists of a stored query accessible as a virtual table composed of the result set of a query. @en-us" ;
        rdfs:label    "View" .

cogs:TransformationProcess
        a                owl:Class , rdfs:Class ;
        rdfs:comment     "Process that applies a series of rules or functions to the extracted data from the source to derive the data for loading into the end target. @en-us" ;
        rdfs:label       "TransformationProcess" ;
        rdfs:subClassOf  cogs:Transformation .

cogs:Table  a         owl:Class , rdfs:Class ;
        rdfs:comment  "A predefined format of rows and columns that define a database entity. @en-us" ;
        rdfs:label    "Table" .

cogs:Replace  a          owl:Class , rdfs:Class ;
        rdfs:comment     "String operation for updating the content of a string. @en-us" ;
        rdfs:label       "Replace" ;
        rdfs:subClassOf  cogs:StringOperation .

cogs:associatedEndpoint
        a           rdf:Property ;
        rdfs:label  "associatedEndpoint" ;
        rdfs:range  cogs:Endpoint .

cogs:RDFInstanceMapping
        a                owl:Class , rdfs:Class ;
        rdfs:comment     "Maps an instance-level element from a source to an instance-level element in a target dataset. " ;
        rdfs:label       "RDFInstanceMapping" ;
        rdfs:subClassOf  cogs:Mapping .

cogs:SplitColumn  a      owl:Class , rdfs:Class ;
        rdfs:comment     "Divides a column in one or more other columns. @en-us" ;
        rdfs:label       "SplitColumn" ;
        rdfs:subClassOf  cogs:ColumnOperation .

cogs:FullRefresh  a      owl:Class , rdfs:Class ;
        rdfs:comment     "Truncates all the tables and data gets loaded again. @en-us" ;
        rdfs:label       "FullRefresh" ;
        rdfs:subClassOf  cogs:Loading .

cogs:StaggingArea  a     owl:Class , rdfs:Class ;
        rdfs:comment     "A place where data can be processed before entering the warehouse area. @en-us" ;
        rdfs:label       "StaggingArea" ;
        rdfs:subClassOf  cogs:DataManagementLayer .

cogs:Query  a            owl:Class , rdfs:Class ;
        rdfs:comment     "Query over a structured or semi-structured data source." ;
        rdfs:label       "Query" ;
        rdfs:subClassOf  cogs:Operation .

cogs:LastError  a     owl:Class , rdfs:Class ;
        rdfs:comment  "Final error on a execution workflow. @en-us" ;
        rdfs:label    "LastError" .

cogs:SortRow  a          owl:Class , rdfs:Class ;
        rdfs:comment     "Row Operation that sorts rows based on a specified fields and on whether they should be sorted in ascending or descending order. @en-us" ;
        rdfs:label       "SortRow" ;
        rdfs:subClassOf  cogs:RowOperation .

cogs:FactTable  a        owl:Class , rdfs:Class ;
        rdfs:comment     "A table that consists of the measurements, metrics or facts of a  process. @en-us" ;
        rdfs:label       "FactTable" ;
        rdfs:subClassOf  cogs:Table .

cogs:associatedGraph  a  rdf:Property ;
        rdfs:label  "associatedGraph" ;
        rdfs:range  cogs:RDFNamedGraph .
