@prefix : <http://rdf.muninn-project.org/ontologies/military#> .
@prefix dc: <http://purl.org/dc/elements/1.1/> .
@prefix person: <http://rdf.muninn-project.org/ontologies/person#> .
@prefix foaf: <http://xmlns.com/foaf/spec/> .
@prefix muninn: <http://rdf.muninn-project.org/ontologies/muninn#> .
@prefix vs: <http://www.w3.org/2003/06/sw-vocab-status/ns#> .
@prefix org: <http://rdf.muninn-project.org/ontologies/organization#> .
@prefix rdfs: <http://www.w3.org/2000/01/rdf-schema#> .
@prefix time: <http://www.w3.org/2006/time#> .
@prefix swrl: <http://www.w3.org/2003/11/swrl#> .
@prefix swrlb: <http://www.w3.org/2003/11/swrlb#> .
@prefix dbpedia: <http://dbpedia.org/resource/> .
@prefix owl: <http://www.w3.org/2002/07/owl#> .
@prefix xsd: <http://www.w3.org/2001/XMLSchema#> .
@prefix rdf: <http://www.w3.org/1999/02/22-rdf-syntax-ns#> .

<dbpedia:%C3%87orbac%C4%B1> muninn:wikipedia_version "482582155" .

<dbpedia:Able_seaman_%28rank%29> muninn:wikipedia_version "485001067" .

<dbpedia:Achaean_League> muninn:wikipedia_version "497254384" .

<dbpedia:Admiral> muninn:wikipedia_version "103794321" .

<dbpedia:Admiral_of_the_Fleet_%28Russia%29> muninn:wikipedia_version "474375587" .

<dbpedia:Agha_%28Ottoman_Empire%29> muninn:wikipedia_version "496783931" .

<dbpedia:Air_chief_marshal> muninn:wikipedia_version "495804436" .

<dbpedia:Air_vice-marshal> muninn:wikipedia_version "495806110" .

<dbpedia:Anthypolochagos> muninn:wikipedia_version "485272666" .

<dbpedia:Antisyntagmatarchis> muninn:wikipedia_version "485253360" .

<dbpedia:Army_General_%28Russia%29> muninn:wikipedia_version "474376394" .

<dbpedia:Aspirant> muninn:wikipedia_version "479973767" .

<dbpedia:Ataman> muninn:wikipedia_version "470073774" .

<dbpedia:Australia> muninn:wikipedia_version "498314417" .

<dbpedia:Austria> muninn:wikipedia_version "498078721" .

<dbpedia:Belarus> muninn:wikipedia_version "498368216" .

<dbpedia:Belgium> muninn:wikipedia_version "498001232" .

<dbpedia:Birinci_Ferik> muninn:wikipedia_version "478074487" .

<dbpedia:Bombardier_%28rank%29> muninn:wikipedia_version "492510161" .

<dbpedia:Bootsmann> muninn:wikipedia_version "339832695" .

<dbpedia:Brigade_General> muninn:wikipedia_version "488560485" .

<dbpedia:Brigadier> muninn:wikipedia_version "102695895" .

<dbpedia:Brigadier_general> muninn:wikipedia_version "498197413" .

<dbpedia:British_Indian_Army> muninn:wikipedia_version "502841968" .

<dbpedia:British_Raj> muninn:wikipedia_version "503927597" .

<dbpedia:Buffer_%28navy%29> muninn:wikipedia_version "332327992" .

<dbpedia:Byzantine_Empire> muninn:wikipedia_version "498328033" .

<dbpedia:Canada> muninn:wikipedia_version "498337533" .

<dbpedia:Captain_%28OF-2%29> muninn:wikipedia_version "495714124" .

<dbpedia:Captain_%28naval%29> muninn:wikipedia_version "494810123" .

<dbpedia:Captain_Lieutenant> muninn:wikipedia_version "469741486" .

<dbpedia:Captain_lieutenant> muninn:wikipedia_version "497303881" .

<dbpedia:Carrier_battle_group> muninn:wikipedia_version "496435661" .

<dbpedia:Chief_Marshal> muninn:wikipedia_version "489506259" .

<dbpedia:Chief_petty_officer> muninn:wikipedia_version "494987481" .

<dbpedia:Chiliarch> muninn:wikipedia_version "493968908" .

<dbpedia:Chor%C4%85%C5%BCy> muninn:wikipedia_version "493459036" .

<dbpedia:Colonel> muninn:wikipedia_version "88659726" .

<dbpedia:Comandarm> muninn:wikipedia_version "484165039" .

<dbpedia:Combat_%28military_rank%29> muninn:wikipedia_version "449517873" .

<dbpedia:Combrig> muninn:wikipedia_version "444403891" .

<dbpedia:Comcor> muninn:wikipedia_version "414282347" .

<dbpedia:Comdiv> muninn:wikipedia_version "466619272" .

<dbpedia:Commandant_%28rank%29> muninn:wikipedia_version "469176328" .

<dbpedia:Commander> muninn:wikipedia_version "92206694" .

<dbpedia:Commandeur> muninn:wikipedia_version "444183372" .

<dbpedia:Commonwealth_of_Nations> muninn:wikipedia_version "498034851" .

<dbpedia:Company_Quartermaster_Sergeant> muninn:wikipedia_version "469636323" .

<dbpedia:Company_sergeant_major> muninn:wikipedia_version "497899716" .

<dbpedia:Conductor_%28Army%29> muninn:wikipedia_version "495627480" .

<dbpedia:Cossack_Hetmanate> muninn:wikipedia_version "497147011" .

<dbpedia:Daejang> muninn:wikipedia_version "469177179" .

<dbpedia:Daffadar> muninn:wikipedia_version "474978288" .

<dbpedia:Denmark> muninn:wikipedia_version "498348760" .

<dbpedia:Divisional_Admiral> muninn:wikipedia_version "469675599" .

<dbpedia:Divisional_General> muninn:wikipedia_version "492101670" .

<dbpedia:Driver_%28rank%29> muninn:wikipedia_version "366534265" .

<dbpedia:Drum_Major_General> muninn:wikipedia_version "488221776" .

<dbpedia:Drum_major_%28rank%29> muninn:wikipedia_version "498071860" .

<dbpedia:England> muninn:wikipedia_version "497805822" .

<dbpedia:Epihipparch> muninn:wikipedia_version "444383081" .

<dbpedia:Estonia> muninn:wikipedia_version "498355716" .

<dbpedia:Ferik_%28rank%29> muninn:wikipedia_version "440865120" .

<dbpedia:Finland> muninn:wikipedia_version "498358269" .

<dbpedia:Fleet_Board> muninn:wikipedia_version "467663769" .

<dbpedia:Flight_(military_unit)> muninn:wikipedia_version "504477222" .

<dbpedia:Flight_sergeant> muninn:wikipedia_version "463753770" .

<dbpedia:Flotilla> muninn:wikipedia_version "502628506" .

<dbpedia:France> muninn:wikipedia_version "498318960" .

<dbpedia:Front_(military)> muninn:wikipedia_version "506004403" .

<dbpedia:Front_(military_formation)> muninn:wikipedia_version "492944457" .

<dbpedia:Garrison_Sergeant_Major> muninn:wikipedia_version "462244580" .

<dbpedia:Gefreiter> muninn:wikipedia_version "492036845" .

<dbpedia:General-in-Chief> muninn:wikipedia_version "469172883" .

<dbpedia:General_Admiral> muninn:wikipedia_version "491014584" .

<dbpedia:Germany> muninn:wikipedia_version "498342708" .

<dbpedia:Greece> muninn:wikipedia_version "498205865" .

<dbpedia:Group_(military_aviation_unit)> muninn:wikipedia_version "497782734" .

<dbpedia:Hasa_%28Korean_military%29> muninn:wikipedia_version "391617597" .

<dbpedia:Havildar> muninn:wikipedia_version "424862948" .

<dbpedia:Hetman> muninn:wikipedia_version "472297416" .

<dbpedia:Hipparchus_%28cavalry_officer%29> muninn:wikipedia_version "472932397" .

<dbpedia:Italy> muninn:wikipedia_version "498219654" .

<dbpedia:Jungsa> muninn:wikipedia_version "294619203" .

<dbpedia:Jungwi> muninn:wikipedia_version "342301621" .

<dbpedia:Junior_sergeant> muninn:wikipedia_version "481658126" .

<dbpedia:Junjang> muninn:wikipedia_version "450552760" .

<dbpedia:Kapudan_Pasha> muninn:wikipedia_version "481287970" .

<dbpedia:Kindral> muninn:wikipedia_version "350970761" .

<dbpedia:Kingdom_of_Denmark> muninn:wikipedia_version "472858436" .

<dbpedia:Kola%C4%9Fas%C4%B1> muninn:wikipedia_version "491860380" .

<dbpedia:Kolonel> muninn:wikipedia_version "439589790" .

<dbpedia:Lance-corporal_of_horse> muninn:wikipedia_version "450536613" .

<dbpedia:Lance_corporal> muninn:wikipedia_version "498208325" .

<dbpedia:Lance_sergeant> muninn:wikipedia_version "471580953" .

<dbpedia:Leading_aircraftman> muninn:wikipedia_version "460246691" .

<dbpedia:Lieutenant> muninn:wikipedia_version "81222307" .

<dbpedia:Lithuania> muninn:wikipedia_version "498142623" .

<dbpedia:Lochagos> muninn:wikipedia_version "485272515" .

<dbpedia:Lord_High_Admiral_of_the_Wash> muninn:wikipedia_version "462939912" .

<dbpedia:Macedonia_%28ancient_kingdom%29> muninn:wikipedia_version "495202996" .

<dbpedia:Major> muninn:wikipedia_version "103728073" .

<dbpedia:Major_general> muninn:wikipedia_version "498199972" .

<dbpedia:Marshal> muninn:wikipedia_version "103489138" .

<dbpedia:Marshal_of_the_Soviet_Union> muninn:wikipedia_version "497557208" .

<dbpedia:Master_warrant_officer> muninn:wikipedia_version "452828931" .

<dbpedia:Midshipman> muninn:wikipedia_version "104159410" .

<dbpedia:Mirliva> muninn:wikipedia_version "443324813" .

<dbpedia:Naval_fleet> muninn:wikipedia_version "490946787" .

<dbpedia:Navarch> muninn:wikipedia_version "493032839" .

<dbpedia:Netherlands> muninn:wikipedia_version "498374388" .

<dbpedia:North_Korea> muninn:wikipedia_version "498359658" .

<dbpedia:Norway> muninn:wikipedia_version "496844290" .

<dbpedia:Numbered_Air_Force> muninn:wikipedia_version "491557779" .

<dbpedia:Obergefreiter> muninn:wikipedia_version "482305142" .

<dbpedia:Oberst> muninn:wikipedia_version "485029855" .

<dbpedia:Ordinary_seaman_%28rating%29> muninn:wikipedia_version "450538267" .

<dbpedia:Ottoman_Empire> muninn:wikipedia_version "498292397" .

<dbpedia:Phrourarch> muninn:wikipedia_version "491704131" .

<dbpedia:Pipe_Major> muninn:wikipedia_version "484159324" .

<dbpedia:Podpolkovnik> muninn:wikipedia_version "476865824" .

<dbpedia:Podpraporshchik> muninn:wikipedia_version "481610330" .

<dbpedia:Poland> muninn:wikipedia_version "497868027" .

<dbpedia:Polemarch> muninn:wikipedia_version "480243861" .

<dbpedia:Polkovnik> muninn:wikipedia_version "493964196" .

<dbpedia:Poruchik> muninn:wikipedia_version "491662172" .

<dbpedia:Praporshchik> muninn:wikipedia_version "491581201" .

<dbpedia:Private_%28rank%29> muninn:wikipedia_version "497378634" .

<dbpedia:Rear_admiral> muninn:wikipedia_version "494693473" .

<dbpedia:Regimental_Quartermaster_Sergeant> muninn:wikipedia_version "495627637" .

<dbpedia:Regimental_sergeant_major> muninn:wikipedia_version "469660582" .

<dbpedia:Republic_of_Ireland> muninn:wikipedia_version "498350287" .

<dbpedia:Romania> muninn:wikipedia_version "498318250" .

<dbpedia:Royal_Air_Force_station> muninn:wikipedia_version "499356677" .

<dbpedia:Russia> muninn:wikipedia_version "498219998" , "498382883" , "498386672" .

<dbpedia:Sangsa> muninn:wikipedia_version "294619474" .

<dbpedia:Schout-bij-nacht> muninn:wikipedia_version "469920162" .

<dbpedia:Scotland> muninn:wikipedia_version "498376035" .

<dbpedia:Seaman> muninn:wikipedia_version "91409028" .

<dbpedia:Second_Corporal> muninn:wikipedia_version "332271219" .

<dbpedia:Septinsular_Republic> muninn:wikipedia_version "496530677" .

<dbpedia:Sergeant> muninn:wikipedia_version "102800259" .

<dbpedia:Sergeant_Major_Instructor> muninn:wikipedia_version "345897828" .

<dbpedia:Sergeant_Pilot> muninn:wikipedia_version "491338622" .

<dbpedia:Singapore> muninn:wikipedia_version "498300526" .

<dbpedia:Skeuophoros> muninn:wikipedia_version "488522679" .

<dbpedia:Somatophylakes> muninn:wikipedia_version "493685412" .

<dbpedia:Sotnik> muninn:wikipedia_version "472347025" .

<dbpedia:South_Korea> muninn:wikipedia_version "498171765" .

<dbpedia:Soviet_Union> muninn:wikipedia_version "498351053" .

<dbpedia:Sowi> muninn:wikipedia_version "354997832" .

<dbpedia:Squadron_(aviation)> muninn:wikipedia_version "497146873" .

<dbpedia:Squadron_(naval)> muninn:wikipedia_version "506073626" .

<dbpedia:Staabikapten> muninn:wikipedia_version "440079788" .

<dbpedia:Stabskapit%C3%A4n> muninn:wikipedia_version "493853501" .

<dbpedia:Staff_Corporal> muninn:wikipedia_version "409702884" .

<dbpedia:Staff_Sergeant_Major> muninn:wikipedia_version "335788405" .

<dbpedia:Staff_sergeant> muninn:wikipedia_version "497529431" .

<dbpedia:Starshina> muninn:wikipedia_version "492104942" .

<dbpedia:Stratarches> muninn:wikipedia_version "473387231" .

<dbpedia:Strategos> muninn:wikipedia_version "491977225" .

<dbpedia:Suba%C5%9Fi> muninn:wikipedia_version "490611693" .

<dbpedia:Subaltern> muninn:wikipedia_version "495224024" .

<dbpedia:Sweden> muninn:wikipedia_version "497805145" .

<dbpedia:Switzerland> muninn:wikipedia_version "498226943" .

<dbpedia:Syntagmatarchis> muninn:wikipedia_version "485256724" .

<dbpedia:Tagmatarchis> muninn:wikipedia_version "485265746" .

<dbpedia:Task_force> muninn:wikipedia_version "504995678" .

<dbpedia:Taxiarch> muninn:wikipedia_version "498203964" .

<dbpedia:Tetrarch> muninn:wikipedia_version "465320704" .

<dbpedia:Trierarch> muninn:wikipedia_version "492902890" .

<dbpedia:Trooper_%28rank%29> muninn:wikipedia_version "486616093" .

<dbpedia:Trumpet_Major> muninn:wikipedia_version "261772661" .

<dbpedia:Tysyatsky> muninn:wikipedia_version "484427552" .

<dbpedia:Ukraine> muninn:wikipedia_version "497889189" .

<dbpedia:Under_Officer> muninn:wikipedia_version "491386869" .

<dbpedia:V%C3%A4%C3%A4peli> muninn:wikipedia_version "476502911" .

<dbpedia:Veebel> muninn:wikipedia_version "404975154" .

<dbpedia:Vice-Admiral_of_the_Coast> muninn:wikipedia_version "449897542" .

<dbpedia:Vice-Admiral_of_the_West> muninn:wikipedia_version "459382951" .

<dbpedia:Vice_admiral> muninn:wikipedia_version "495831034" .

<dbpedia:Wachtmeister> muninn:wikipedia_version "437735728" .

<dbpedia:Wales> muninn:wikipedia_version "497995158" .

<dbpedia:Warrant_officer_%28United_Kingdom%29> muninn:wikipedia_version "496940079" .

<dbpedia:Wing_(military_aviation_unit)> muninn:wikipedia_version "500722310" .

<dbpedia:Wing_commander_%28rank%29> muninn:wikipedia_version "496628941" .

<dbpedia:Wojski> muninn:wikipedia_version "454605449" .

<dbpedia:Wonsu> muninn:wikipedia_version "492136047" .

<dbpedia:Yesaul> muninn:wikipedia_version "464140973" .

<dbpedia:Ypolochagos> muninn:wikipedia_version "496047552" .

<http://rdf.muninn-project.org/ontologies/Armor> a :ArmsType ;
	rdfs:comment "Armor as a weapon type and organizational unit." ;
	rdfs:label "Armor"@en ;
	foaf:name "Armor" .

<http://rdf.muninn-project.org/ontologies/HouseholdCavalryAppointments> a owl:Class ;
	owl:subClassOf <http://rdf.muninn-project.org/ontologies/Appointment> .

<http://rdf.muninn-project.org/ontologies/HouseholdCavalryRanks> a owl:Class ;
	owl:subClassOf <mil:Rank> .

<http://rdf.muninn-project.org/ontologies/military> dc:description "The Muninn Military Ontology marks up information about military people, organizations and events." ;
	dc:title "The Muninn Military Ontology" ;
	a :Spy , owl:Ontology ;
	rdfs:comment "The Muninn Military Ontology marks up information about military people, organizations and events."@en ;
	rdfs:label "The Muninn Military Ontology"@en ;
	owl:sameAs dbpedia:Howard_Burnham ;
	owl:versionInfo "0.2"^^xsd:decimal .

<http://rdf.muninn-project.org/ontologies/military##Rank_Buffer_Navy> a :MilitaryRank ;
	rdfs:comment "Buffer is the colloquial title for the senior seaman sailor in a Commonwealth of Nations Navy ship. The formal title is Chief Boatswain's Mate. This person is typically a Chief Petty Officer in frigates or destroyers, and in larger ships may be a Warrant Officer. In smaller ships, such as a patrol boat, the Buffer may be a Petty Officer."@en ;
	rdfs:label "Buffer (navy)"@en ;
	owl:sameAs <dbpedia:Buffer_%28navy%29> ;
	foaf:name "Buffer" .

<http://rdf.muninn-project.org/ontologies/military##Rank_Buffer_Navy_Australia> org:rankOf <dbpedia:Australia> ;
	a :MilitaryRank ;
	rdfs:comment "The specific instance of the Buffer (navy) rank in the context of country Australia."@en ;
	rdfs:label "Buffer (navy) (Australia)"@en , "Buffer (navy) (Australia)"@es , "Buffer (navy) (Australia)"@fi , "Buffer (navy) (Australia)"@it , "Buffer (navy) (Australia)"@no , "Buffer (navy) (Australia)"@pl , "Buffer (navy) (Australie)"@fr , "Buffer (navy) (Australien)"@de , "Buffer (navy) (Australien)"@sv , "Buffer (navy) (Australië (land))"@nl , "Buffer (navy) (Austrália)"@pt , "Buffer (navy) (Австралия)"@ru ;
	owl:subClass <http://rdf.muninn-project.org/ontologies/military##Rank_Buffer_Navy> ;
	foaf:name "Buffer"@en .

<http://rdf.muninn-project.org/ontologies/military##Rank_Buffer_Navy_Commonwealth_of_Nations> org:rankOf <dbpedia:Commonwealth_of_Nations> ;
	a :MilitaryRank ;
	rdfs:comment "The specific instance of the Buffer (navy) rank in the context of country Commonwealth of Nations."@en ;
	rdfs:label "Buffer (navy) (Commonwealth delle nazioni)"@it , "Buffer (navy) (Commonwealth of Nations)"@de , "Buffer (navy) (Commonwealth of Nations)"@en , "Buffer (navy) (Commonwealth of Nations)"@fr , "Buffer (navy) (Commonwealth)"@pt , "Buffer (navy) (Gemenebest van Naties)"@nl , "Buffer (navy) (Kansainyhteisö)"@fi , "Buffer (navy) (Mancomunidad de Naciones)"@es , "Buffer (navy) (Samveldet av nasjoner)"@no , "Buffer (navy) (Samväldet)"@sv , "Buffer (navy) (Wspólnota Narodów)"@pl , "Buffer (navy) (Содружество наций)"@ru ;
	owl:subClass <http://rdf.muninn-project.org/ontologies/military##Rank_Buffer_Navy> ;
	foaf:name "Buffer"@en .

:ActingRank a owl:Class ;
	rdfs:comment "An acting military rank."@en ;
	rdfs:label "Acting Rank (Military)"@en , "Grade Intérimaire (Militare)"@fr , "Handelnden Rang (Militärischen)"@de ;
	owl:subClassOf :MilitaryRank , <org:Acting_Rank> .

:AirDivision org:hasPart :NamedAirForceUnit ;
	org:isPartOf :AirForceServiceBranch ;
	a owl:Class ;
	rdfs:label "Air Division"@en ;
	foaf:name "Air Division" .

:AirForceCommand org:hasPart :TacticalAirForce ;
	org:isPartOf :AirForceServiceBranch ;
	a owl:Class ;
	rdfs:comment "An air force command. eg: Bomber Command."@en ;
	rdfs:label ""@de , ""@fr , "Command (Air Force)"@en .

:AirForceDetail a owl:Class ;
	rdfs:comment "A detail from an Air Force flight."@en ;
	rdfs:label ""@de , " "@fr , "Detail (Air Force)"@en .

:AirForceGroup org:hasPart :AirForceSquadron ;
	org:isPartOf :AirForceServiceBranch , :TacticalAirForce ;
	a owl:Class ;
	rdfs:comment "A group is a military aviation unit, a component of military organization and a military formation. Usage of the terms group and wing differ from one country to another, as well as different branches of a defence force, in some cases. Groups therefore vary considerably in size. In most air services and most countries, a group is made up of two to four squadrons and is commanded by a Lieutenant Colonel, Commander or similar ranks."@en ;
	rdfs:label "Group (military aviation unit)"@en , "Groupe (Force Aérienne)"@fr , "Gruppe (Luftfahrt)"@de ;
	owl:sameAs <dbpedia:Group_(military_aviation_unit)> ;
	foaf:name "Group" .

:AirForceServiceBranch a owl:Class ;
	rdfs:label "Air Force (Service Branch)"@en , "Force aérienne (Service Militare)"@fr , "Luftstreitkräfte (Service)"@de ;
	owl:subClassOf :FightsPrimarilyInAir , :MilitaryServiceBranch , <org:AirBasedOrganization> .

:AirForceSquadron org:hasPart :MilitaryFlightUnit ;
	org:isPartOf :AirForceWing ;
	a owl:Class ;
	rdfs:comment "A squadron in air force, army aviation or naval aviation is mainly a unit comprising a number of military aircraft, usually of the same type, typically with 12 to 24 aircraft, sometimes divided into three or four flights, depending on aircraft type and air force. In most air forces, two or more squadrons form a group or wing. Some air forces also use the term squadrons for non-flying ground units. An escadron is the equivalent unit in France's Armée de l'Air."@en ;
	rdfs:label "Escuadrilla"@es , "Esquadrilha"@pt , "Esquadrilla"@ca , "Laivue (ilmavoimat)"@fi , "Phi đoàn"@vi , "Skvadron"@no , "Squadron"@nl , "Squadron (aviation)"@en , "Staffel (Militär)"@de , "Эскадрилья"@ru ;
	owl:sameAs <dbpedia:Squadron_(aviation)> ;
	owl:subClass :Squadron ;
	foaf:name "Squadron" .

:AirForceStation a owl:Class ;
	rdfs:comment "An Air Force station."@en ;
	rdfs:label "Station (Air Force)"@en , "Station (Force Aérienne)"@fr , "Station (Luftfahrt)"@de .

:AirForceStationRAF org:isPartOf :AirForceGroup ;
	a owl:Class ;
	rdfs:comment "A Royal Air Force station is a permanent Royal Air Force operations location. Many RAF stations are aerodromes, or airbases, being the home to one or more flying squadrons. Other RAF stations are training units, administrative units, headquarters (HQ), or carry out ground-based operational tasks. Although many RAF units are often called stations, they can only be properly classified as an RAF station if they are self-accounting with their own station commander and headquarters."@en ;
	rdfs:label "Royal Air Force station"@en ;
	owl:sameAs <dbpedia:Royal_Air_Force_station> ;
	owl:subClass :AirForceStation ;
	foaf:name "Royal Air Force station" .

:AirForceWing org:hasPart :AirForceSquadron ;
	org:isPartOf :AirForceGroup ;
	a owl:Class ;
	rdfs:comment "Wing is a term used by different military aviation forces for a unit of command. The terms wing, group or Staffel are used for different-sized units from one country or service to another. In some military aviation services, a wing is a relatively large formation of two or more groups, which in turn control two or more squadrons. In other contexts a wing is a smaller unit, comprising two to four squadrons, with several wings forming a group."@en ;
	rdfs:label "Ala (militar)"@pt , "Flygflottilj"@sv , "Geschwader"@de , "Không đoàn"@vi , "Skrzydło (oddział lotnictwa)"@pl , "Stormo (unità militare)"@it , "Ving (militær enhet)"@no , "Wing (luchtmacht)"@nl , "Wing (military aviation unit)"@en , "Авиационное крыло"@ru ;
	owl:sameAs <dbpedia:Wing_(military_aviation_unit)> ;
	foaf:name "Wing" .

:ArmsType a owl:Class ;
	rdfs:comment "The category of arms in use"@en ;
	rdfs:label "?"@de , "Arms Type(Military)"@en , "Type Armes (Military)"@fr .

:ArmyCompany org:hasPart :Platoon ;
	org:isPartOf :ArmyServiceBranch , :Battalion ;
	org:nominalSize "100" ;
	a owl:Class ;
	rdfs:comment "A military company"@en ;
	rdfs:label "Compagnie (militaire)"@fr , "Company (Military Unit)"@en , "Kompanie (Militär)"@de ;
	owl:sameAs "dbpedia:Company_(military_unit)" ;
	foaf:logo <http://rdf.muninn-project.org/ww1/2011/11/11/Image/86f5d79432849d7059da6460a74ba7fe> .

:ArmyFront org:hasPart :FieldArmy ;
	org:isPartOf :ArmyServiceBranch ;
	a owl:Class ;
	rdfs:comment "A front was a major military formation. Appearing to originate with the Russian Empire, it has been used by the Polish Army, the Red Army and Soviet Army, and by Turkey. It was roughly equivalent to an army group in the militaries of most other countries. It should not to be confused with the more general usage of military front, describing a geographic area in wartime."@en ;
	rdfs:label "Front"@cs , "Front (Großverband)"@de , "Front (Röda armén)"@sv , "Front (forband)"@no , "Front (military formation)"@en , "Front (seregtest)"@hu , "Front (unité soviétique)"@fr , "Fronty radzieckie"@pl , "Phương diện quân (Liên Xô)"@vi , "Rintama (puna-armeija)"@fi , "Советские фронты во время Великой Отечественной войны"@ru ;
	owl:sameAs <dbpedia:Front_(military_formation)> ;
	foaf:name "Front" .

:ArmyGroup org:hasPart :FieldArmy ;
	org:isPartOf :ArmyServiceBranch ;
	a owl:Class ;
	rdfs:comment "A field army containing Corps, Brigades, Divisions, etc..."@en ;
	rdfs:label "Army Group"@en , "Groupe d'Armée"@fr , "Heeresgruppe"@de .

:ArmySection org:isPartOf :ArmyServiceBranch , :Platoon ;
	a owl:Class ;
	rdfs:label "Abschnitt (Militär)"@de , "Section (Militaire)"@fr , "Section (Military Unit)"@en ;
	owl:sameAs "dbpedia:Section_(military_unit)" ;
	foaf:logo <http://rdf.muninn-project.org/ww1/2011/11/11/image/32> .

:ArmyServiceBranch a owl:Class ;
	rdfs:label "Armee (Service)"@de , "Army (Service Branch)"@en , "Armée (Service)"@fr ;
	owl:subClassOf :FightsPrimarilyOnAndInLand , :GroundBasedOrganization , :MilitaryServiceBranch .

:ArmySquad org:isPartOf :ArmyServiceBranch , :Platoon ;
	a owl:Class ;
	rdfs:label "Gruppe (Militär)"@de , "Squad (Military Unit)"@en , "Équipe (Militaire)"@fr ;
	owl:sameAs "dbpedia:Section_(military_unit)" ;
	foaf:logo <http://rdf.muninn-project.org/ww1/2011/11/11/image/33> .

:ArmyTroop a owl:Class ;
	rdfs:comment "A generic class for an army troop in the Cavalry or a Corps."@en ;
	rdfs:label "Troop (Military)"@en , "Troupe (Militare)"@fr , "Truppe (Militär)"@de .

:Artillery a :ArmsType ;
	rdfs:comment "Artillery as a weapon type and organizational unit." ;
	rdfs:label "Artillery"@en ;
	foaf:name "Artillery" .

:ArtilleryBattery a owl:Class ;
	rdfs:label "Artillery Battery"@en , "Batterie (Militär)"@de , "Batterie (armement)"@fr ;
	owl:sameAs "dbpedia:Artillery_battery" ;
	owl:subClassOf :Artillery ;
	foaf:logo <http://rdf.muninn-project.org/ww1/2011/11/11/image/35> .

:ArtilleryBatteryDivision a owl:Class ;
	rdfs:label "Batterie Division (Militär)"@de , "Division de Batterie (armement)"@fr , "Divisional Artillery"@en ;
	owl:subClassOf :Artillery .

:AssaultGroupInfantry org:isPartOf :ArmySection , :ArmyServiceBranch , :ArmySquad ;
	a owl:Class ;
	rdfs:label "Assault Group (Infantry)"@en ;
	foaf:name "Assault Group" .

:Battalion org:isPartOf :ArmyServiceBranch , :Brigade ;
	org:nominalSize "1000" ;
	a owl:Class ;
	rdfs:label "Bataillon"@de , "Bataillon"@fr , "Battalion (Military)"@en ;
	owl:sameAs "dbpedia:Battalion" ;
	foaf:logo <http://rdf.muninn-project.org/ww1/2011/11/11/image/24> .

:BattleSpace a owl:Class ;
	rdfs:comment "A detail from an Air Force flight."@en ;
	rdfs:label ""@de , "Battle Space"@en , "Espace de Battaille"@fr ;
	owl:sameAs "dbpedia:Battlespace" .

:BattleStandard a owl:ObjectProperty ;
	rdfs:comment "Flag used to represent that unit on a battlefield."@en ;
	rdfs:domain :ArmyServiceBranch ;
	rdfs:label ""@de , "Battle Standard"@en , "Drapeau de combat(?)"@fr ;
	rdfs:subPropertyOf <org:flag> .

:BrevetRank a owl:Class ;
	rdfs:comment "A Brevet military rank."@en ;
	rdfs:label "Brevet Rang (Militärischen)"@de , "Brevet Rank (Military)"@en , "Grade Brevet (Militare)"@fr ;
	owl:subClassOf :MilitaryRank .

:Brigade org:hasPart :Battalion ;
	org:isPartOf :ArmyServiceBranch , :Division ;
	a owl:Class ;
	rdfs:label "Brigade"@de , "Brigade (Militare)"@fr , "Brigade (Military)"@en ;
	owl:sameAs "dbpedia:Brigade" ;
	foaf:logo <http://rdf.muninn-project.org/ww1/2011/11/11/image/27> .

:BrigadeAirCorps org:hasPart :AirForceWing ;
	org:isPartOf :AirForceStation , :ProtoAirForce ;
	org:leadBy :Rank_Brigadier_general ;
	a owl:Class ;
	rdfs:label "Brigade (Air Corps)"@en ;
	foaf:name "Brigade" .

:CarrierBattleGroup org:hasPart :Flotilla ;
	org:isPartOf :NavalTaskForce ;
	a owl:Class ;
	rdfs:comment "A carrier battle group (CVBG) consists of an aircraft carrier (designated CV) and its escorts, together comprising the group. The first naval task forces built around carriers appeared just prior to and during World War II. The Imperial Japanese Navy was the first to assemble a large number of carriers into a single task force, known as Kido Butai. This task force was used with devastating effect during the Pearl Harbor Attack."@en ;
	rdfs:label "Carrier Strike Group"@no , "Carrier battle group"@en , "Flugzeugträgerkampfgruppe"@de , "Groupe aéronaval"@fr , "Gruppo da battaglia di una portaerei"@it , "Авианосная ударная группа"@ru ;
	owl:isPartOf :Navy ;
	owl:sameAs <dbpedia:Carrier_battle_group> ;
	foaf:name "Carrier battle group" .

:Cavalry a owl:Class ;
	rdfs:label "Cavalerie"@fr , "Cavalry"@en , "Kavallerie"@de ;
	owl:sameAs "dbpedia:Cavalry" .

:CavalrySquadron a owl:Class ;
	rdfs:comment "A squadron of cavalry."@en ;
	rdfs:label "Cavalry Squadron"@en , "Escadron de Cavalerie"@fr , "Kavallerie Schwadron"@de ;
	owl:sameAs "dbpedia:Squadron_(army)" ;
	owl:subClass :Cavalry , :Squadron .

:CavalryTroop a owl:Class ;
	rdfs:comment "A troop of Cavalrymen."@en ;
	rdfs:label "Cavalry Troop"@en , "Kavallerie Truppe"@de , "Troupe de Cavalerie"@fr ;
	owl:subClass :ArmyTroop , :Cavalry .

:Civilian a owl:Class ;
	rdfs:comment "A person uninvolved with the conflict and not working for the conflicting powers."@en ;
	rdfs:label "Civil"@fr , "Civilian"@en , "Zivilist"@de ;
	owl:subClassOf :Non-Combatant ;
	foaf:name "Civilian" .

:Combatant a owl:Class ;
	rdfs:comment "A person engaging in combat and/or war."@en ;
	rdfs:label ""@de , "Combatant"@en , "Combatant"@fr ;
	owl:subClassOf :Person , <org:Role> ;
	foaf:name "Combatant" .

:CorpsFormation org:hasPart :Division ;
	org:isPartOf :ArmyServiceBranch , :FieldArmy ;
	a owl:Class ;
	rdfs:comment "A military formation containing Brigades, Divisions, etc..."@en ;
	rdfs:label "Corps (Formation)"@en , "Corps d'armée"@fr , "Korps (Großverband)"@de ;
	owl:sameAs "dbpedia:Corps" ;
	foaf:logo <http://rdf.muninn-project.org/ww1/2011/11/11/image/28> .

:CorpsUnit org:hasPart :Division ;
	org:isPartOf :ArmyServiceBranch , :FieldArmy ;
	a owl:Class ;
	rdfs:comment "A stand-alone administrative military unit with a specialized function, eg: Medical Corps."@en ;
	rdfs:label "Corps (Unit)"@en , "Corps (Unité d'armée)"@fr , "Korps (Unit)"@de ;
	owl:sameAs "dbpedia:Corps" .

:DemiBrigade org:isPartOf :ArmyServiceBranch , :Brigade , :Division ;
	a owl:Class ;
	rdfs:comment "An military organizational unit derived from French Regiments."@en ;
	rdfs:label "Demi-brigade"@fr , "Halbbrigade"@de , "Half-Brigade"@en ;
	owl:sameAs "dbpedia:Demi-brigade" ;
	owl:subClassOf :regiment .

:Depot a owl:Class ;
	rdfs:comment "A location where military supplies are stored."@en ;
	rdfs:label "Depot (Military)"@en , "Depot (Militär)"@de , "Dépot (Military)"@fr .

:Detachment a owl:Class ;
	rdfs:comment "A group of people detached from another larger group for a specific purpose."@en ;
	rdfs:label "Detachement"@de , "Detachment (military)"@en , "Détachement (Militare)"@fr ;
	owl:sameAs "dbpedia:Detachment_(military)" ;
	owl:subClassOf :MilitaryOrganization .

:Division org:hasPart :Brigade ;
	org:isPartOf :ArmyServiceBranch , :Brigade ;
	a owl:Class ;
	rdfs:label "Division (Militaire)"@fr , "Division (Military)"@en , "Division (Militär)"@de ;
	owl:sameAs "dbpedia:Division_(military)" ;
	foaf:logo <http://rdf.muninn-project.org/ww1/2011/11/11/image/25> .

:DivisionNavalEstablishment org:isPartOf :NavalSquadron ;
	a owl:Class ;
	rdfs:label "Division"@de , "Division (Marine)"@fr , "Division (Navy)"@en ;
	owl:subClass :Navy .

:DivisionNavalUnit a owl:Class ;
	rdfs:label "Division"@de , "Division de Navire (Marine)"@fr , "Ship's Division (Navy)"@en .

:DraftedSoldier a owl:Class ;
	rdfs:comment "A soldier which serves on a full-time basis."@en ;
	rdfs:label "Soldat (Rédigé)"@fr , "Soldat (eingezogen)"@de , "Soldier (Drafted)"@en ;
	owl:subClassOf :RegularForceSoldier ;
	foaf:name "Draftee" .

:Enlisted a owl:Class ;
	rdfs:comment "A soldier below the rank of Officer or non-commissioned Officer."@en ;
	rdfs:label "Enlisted Soldier"@en , "Hommes de Troupes"@fr , "angeworbenen Soldaten"@de ;
	owl:subClassOf :Soldier ;
	foaf:name "Enlisted" .

:ExchangeOfficer a owl:Class ;
	rdfs:comment "An officer exchanged for a set period of time."@en ;
	rdfs:label "Austausch-Offizier"@de , "Exchange Officer"@en , "Officier d'échange"@fr ;
	owl:sameAs <dbpedia:Exchange_officer> ;
	owl:subClassOf :Officer ;
	foaf:name "Exchange Officer" .

:FieldArmy org:hasPart :CorpsFormation ;
	org:isPartOf :ArmyFront , :ArmyGroup , :ArmyServiceBranch ;
	a owl:Class ;
	rdfs:comment "A field army containing Corps, Brigades, Divisions, etc..."@en ;
	rdfs:label "Armee (Großverband)"@de , "Armée (Unité)"@fr , "Field Army"@en ;
	owl:sameAs "dbpedia:Field_army" ;
	foaf:logo <http://rdf.muninn-project.org/ww1/2011/11/11/image/29> .

:FieldArtillery a owl:Class ;
	rdfs:comment "Field, or foot, artillery where the guns are pulled by horses but the gun crews are on foot."@en ;
	rdfs:label "Artillerie de campagne"@fr , "Berittene Kampagne"@de , "Field Artillery"@en ;
	owl:sameAs "dbpedia:Field_artillery" ;
	owl:subClassOf :Artillery .

:Fireteam org:isPartOf :ArmySection , :ArmyServiceBranch , :ArmySquad ;
	a owl:Class ;
	rdfs:label "Fireteam (Military Unit)"@en , "Fireteam?"@fr , "Trupp (Militär)"@de ;
	owl:sameAs "dbpedia:Section_(military_unit)" ;
	foaf:logo <http://rdf.muninn-project.org/ww1/2011/11/11/image/34> .

:FlagOfficer a owl:Class ;
	rdfs:comment "A Commissioned Officer serving in a political entity's Navy."@en ;
	rdfs:label "????"@fr , "Flag Officer"@en , "Flaggoffizier"@de ;
	owl:subClassOf :NavalOfficer .

:Flotilla org:hasPart :NavalSquadron ;
	org:isPartOf :CarrierBattleGroup ;
	a owl:Class ;
	rdfs:comment "A flotilla (from Spanish, meaning a small flota of ships, and this from French flotte), or naval flotilla, is a formation of small warships that may be part of a larger fleet. A flotilla is usually composed of a homogeneous group of the same class of warship, such as frigates, destroyers, torpedo boats, submarines, gunboats, or minesweepers."@en ;
	rdfs:label "Flotila"@cs , "Flotilha"@pt , "Flotilla"@ca , "Flotilla"@en , "Flotilla"@es , "Flottielje"@nl , "Flottilj"@sv , "Flottille"@de , "Flottille"@fr , "Flotylla okrętów"@pl , "Флотилия"@ru ;
	owl:isPartOf :Navy ;
	owl:sameAs <dbpedia:Flotilla> ;
	foaf:name "Flotilla" .

:Frigate a owl:Class ;
	rdfs:label ""@de , "Fregate"@fr , "Frigate"@en ;
	owl:subClassOf :Warship .

:FrontLine org:isPartOf :WarTheater ;
	a owl:Class ;
	rdfs:comment "A military front or battlefront is a contested armed frontier between opposing forces. This can be a local or tactical front, or it can range to a theater. A typical front was the Western Front in France and Belgium in World War I. The term \"home front\" has been used to denote conditions in the civilian sector of a country at war, including those involved in the production of matériel."@en ;
	rdfs:label "Frente (término militar)"@es , "Frente de batalha"@pt , "Front (militar)"@ca , "Front (military)"@en , "Front (oorlog)"@nl , "Front militaire"@fr , "Fronte (guerra)"@it , "Frontlinje"@sv , "Kampfront"@no , "Kriegsfront"@de , "Válečná fronta"@cs ;
	owl:sameAs <dbpedia:Front_(military)> ;
	foaf:name "Front" .

:Garrison a owl:Class ;
	rdfs:comment "A collection of military units housed and occuping a location."@en ;
	rdfs:label "Garnison (Militaire)"@fr , "Garnison (Militär)"@de , "Garrison (military)"@en ;
	owl:sameAs "dbpedia:Garrison" .

:GeneralOfficer a owl:Class ;
	rdfs:comment "General staff officers"@en ;
	rdfs:label "General Officer"@en , "Officiers Généraux"@fr , "allgemeinen Offizier"@de ;
	owl:subClassOf :Soldier ;
	foaf:name "General Officer" .

:GrandeBatterie a owl:Class ;
	rdfs:comment "Large unit of all available artillery batteries."@en ;
	rdfs:label "Grand Battery"@en , "Grand-Batterie"@de , "Grande Batterie"@fr ;
	owl:sameAs "dbpedia:Grand_Battery" ;
	owl:subClassOf :Artillery .

:HorseArtillery a owl:Class ;
	rdfs:comment "Field, or foot, artillery where the guns and the gun crewa are transported by horses."@en ;
	rdfs:label "Artillerie à cheval"@fr , "Berittene Artillerie"@de , "Horse Artillery"@en ;
	owl:sameAs "dbpedia:Horse_artillery" ;
	owl:subClassOf :Artillery .

:HouseholdCavalry a owl:Class ;
	rdfs:label "Household Cavalry"@en ;
	owl:sameAs "dbpedia:Household_Cavalry" ;
	foaf:membershipClass <http://rdf.muninn-project.org/ontologies/HouseholdCavalryAppointments> , <http://rdf.muninn-project.org/ontologies/HouseholdCavalryRanks> .

:Infantry a :ArmsType ;
	rdfs:label "Infantry"@en ;
	foaf:name "Infantry" .

:LiaisonOfficer a owl:Class ;
	rdfs:comment "An officer exchanged to another unit for a set purpose."@en ;
	rdfs:label "Liaison Officer"@en , "Officier de Liason"@fr , "Verbindungsoffizier"@de ;
	owl:sameAs <dbpedia:Liaison_officer> ;
	owl:subClassOf :Officer ;
	foaf:name "Liaison Officer" .

:MilitaryAction a owl:Class ;
	owl:subClassOf :WarEvent .

:MilitaryAirborneFlight a owl:Class ;
	rdfs:comment "An aviation airborne flight."@en ;
	rdfs:label "Aviation Flight (Military Unit)"@en , "Escadrille"@fr , "Schwarm (Luftfahrt)"@de ;
	owl:subClass :MilitaryFlightUnit .

:MilitaryAppointment a owl:Class ;
	rdfs:comment "An appointment / function in a Military Organization."@en ;
	rdfs:label "Appointment (Militare)"@fr , "Appointment (Military)"@en , "Appointment (Militärischen)"@de .

:MilitaryDecoration a owl:Class ;
	owl:subClassOf <org:Decoration> .

:MilitaryFlightUnit org:isPartOf :AirForceSquadron ;
	a owl:Class ;
	rdfs:comment "A flight is a military unit in an air force, naval air service, or army air corps. It usually comprises three to six aircraft, with their aircrews and ground staff; or, in the case of a non-flying ground flight, no aircraft and a roughly equivalent number of support personnel. In most usages, multiple flights make up a squadron. The \"flight\" is also a basic unit for intercontinental ballistic missiles."@en ;
	rdfs:label "Escadrille"@fr , "Flight (luchtmacht)"@nl , "Flight (military unit)"@en , "Phi đội"@vi , "Schwarm"@de ;
	owl:sameAs <dbpedia:Flight_(military_unit)> ;
	foaf:name "Flight (military unit)" .

:MilitaryGroundFlight a owl:Class ;
	rdfs:comment "Consists of ground personel for an Air Force."@en ;
	rdfs:label "Escadrille de terra"@fr , "Ground Flight (Military Unit)"@en , "Schwarm Boden(Luftfahrt)"@de .

:MilitaryIncident a owl:Class ;
	owl:subClassOf :WarEvent .

:MilitaryOrganization a owl:Class ;
	rdfs:comment "An organization that is military."@en ;
	rdfs:label ""@de , "A Military Organization"@en , "Une Organisation Militare"@fr ;
	owl:sameAs <dbpedia:MilitaryUnit> ;
	owl:subClassOf <org:Organization> .

:MilitaryRank a owl:Class ;
	rdfs:comment "A military rank."@en ;
	rdfs:label "Grade (Militare)"@fr , "Rang (Militärischen)"@de , "Rank (Military)"@en ;
	owl:subClassOf <org:Rank> ;
	foaf:name "Rank" .

:MilitaryServiceBranch a owl:Class ;
	rdfs:label "Branche du service militaire"@fr , "Service Branch (Military)"@en , "Teilstreitkraft"@de ;
	owl:sameAs <dbpedia:Military_branch> ;
	owl:subClassOf :MilitaryOrganization ;
	foaf:name "Service Branch" .

:MilitaryUniform a owl:Class ;
	rdfs:label "Military Uniform"@en .

:MountainArtillery a owl:Class ;
	rdfs:comment "Artillery units capable of disassembling and reassembling their guns for mountain transport."@en ;
	rdfs:label "Artillerie de Montagnecampagne"@fr , "Gebirgsgeschütz"@de , "Mountain Artillery"@en ;
	owl:subClassOf :Artillery .

:NamedAirForceUnit org:isPartOf :AirForceServiceBranch ;
	a owl:Class ;
	rdfs:comment "Use this for numbered / named air forces, eg: US 8th Air Force. Ambiguous useage over time within the command structure."@en ;
	rdfs:label "Força Aérea Numerada"@pt , "Không lực mang số"@vi , "Luftflotten der United States Air Force"@de , "Numbered Air Force"@en , "Numbered Air Force"@it ;
	owl:sameAs <dbpedia:Numbered_Air_Force> ;
	foaf:name "Named Air Force" .

:NatoRankOF-1 org:rankSeniorTo <http://rdf.muninn-project.org/ontologies/NatoRankOF-1> ;
	a owl:Class ;
	rdfs:label "NATO Officer Rank OF-1"@en ;
	owl:subClassOf :NatoRanks , :Officer .

:NatoRankOF-10 org:rankJuniorTo <http://rdf.muninn-project.org/ontologies/NatoRankOF-10> ;
	org:rankSeniorTo <http://rdf.muninn-project.org/ontologies/NatoRankWO-1> ;
	a owl:Class ;
	rdfs:label "NATO Officer Rank OF-10"@en ;
	owl:subClassOf :NatoRanks , :Officer .

:NatoRankOF-2 org:rankJuniorTo <http://rdf.muninn-project.org/ontologies/NatoRankOF-1> ;
	org:rankSeniorTo <http://rdf.muninn-project.org/ontologies/NatoRankOF-3> ;
	a owl:Class ;
	rdfs:label "NATO Officer Rank OF-2"@en ;
	owl:subClassOf :Nato_Ranks , :Officer .

:NatoRankOF-3 org:rankJuniorTo <http://rdf.muninn-project.org/ontologies/NatoRankOF-2> ;
	org:rankSeniorTo <http://rdf.muninn-project.org/ontologies/NatoRankOF-4> ;
	a owl:Class ;
	rdfs:label "NATO Officer Rank OF-3"@en ;
	owl:subClassOf :NatoRanks , :Officer .

:NatoRankOF-4 org:rankJuniorTo <http://rdf.muninn-project.org/ontologies/NatoRankOF-3> ;
	org:rankSeniorTo <http://rdf.muninn-project.org/ontologies/NatoRankOF-5> ;
	a owl:Class ;
	rdfs:label "NATO Officer Rank OF-4"@en ;
	owl:subClassOf :NatoRanks , :Officer .

:NatoRankOF-5 org:rankJuniorTo <http://rdf.muninn-project.org/ontologies/NatoRankOF-4> ;
	org:rankSeniorTo <http://rdf.muninn-project.org/ontologies/NatoRankOF-6> ;
	a owl:Class ;
	rdfs:label "NATO Officer Rank OF-5"@en ;
	owl:subClassOf :NatoRanks , :Officer .

:NatoRankOF-6 org:rankJuniorTo <http://rdf.muninn-project.org/ontologies/NatoRankOF-5> ;
	org:rankSeniorTo <http://rdf.muninn-project.org/ontologies/NatoRankOF-7> ;
	a owl:Class ;
	rdfs:label "NATO Officer Rank OF-6"@en ;
	owl:subClassOf :NatoRanks , :Officer .

:NatoRankOF-7 org:rankJuniorTo <http://rdf.muninn-project.org/ontologies/NatoRankOF-6> ;
	org:rankSeniorTo <http://rdf.muninn-project.org/ontologies/NatoRankOF-8> ;
	a owl:Class ;
	rdfs:label "NATO Officer Rank OF-7"@en ;
	owl:subClassOf :NatoRanks , :Officer .

:NatoRankOF-8 org:rankJuniorTo <http://rdf.muninn-project.org/ontologies/NatoRankOF-7> ;
	org:rankSeniorTo <http://rdf.muninn-project.org/ontologies/NatoRankOF-9> ;
	a owl:Class ;
	rdfs:label "NATO Officer Rank OF-8"@en ;
	owl:subClassOf :NatoRanks , :Officer .

:NatoRankOF-9 org:rankJuniorTo <http://rdf.muninn-project.org/ontologies/NatoRankOF-8> ;
	org:rankSeniorTo <http://rdf.muninn-project.org/ontologies/NatoRankOF-10> ;
	a owl:Class ;
	rdfs:label "NATO Officer Rank OF-9"@en ;
	owl:subClassOf :NatoRanks , :Officer .

:NatoRankOR-1 org:rankJuniorTo <http://rdf.muninn-project.org/ontologies/NatoRankWO-5> ;
	org:rankSeniorTo <http://rdf.muninn-project.org/ontologies/NatoRankOR-2> ;
	a owl:Class ;
	rdfs:label "NATO Other/Enlisted Rank OR-1"@en ;
	owl:subClassOf :Enlisted , :NatoRanks , :NonCommissionedOfficer .

:NatoRankOR-2 org:rankJuniorTo <http://rdf.muninn-project.org/ontologies/NatoRankOR-1> ;
	org:rankSeniorTo <http://rdf.muninn-project.org/ontologies/NatoRankOR-3> ;
	a owl:Class ;
	rdfs:label "NATO Other/Enlisted Rank OR-2"@en ;
	owl:subClassOf :Enlisted , :NatoRanks , :NonCommissionedOfficer .

:NatoRankOR-3 org:rankJuniorTo <http://rdf.muninn-project.org/ontologies/NatoRankOR-2> ;
	org:rankSeniorTo <http://rdf.muninn-project.org/ontologies/NatoRankOR-4> ;
	a owl:Class ;
	rdfs:label "NATO Other/Enlisted Rank OR-3"@en ;
	owl:subClassOf :Enlisted , :NatoRanks , :NonCommissionedOfficer .

:NatoRankOR-4 org:rankJuniorTo <http://rdf.muninn-project.org/ontologies/NatoRankOR-3> ;
	org:rankSeniorTo <http://rdf.muninn-project.org/ontologies/NatoRankOR-5> ;
	a owl:Class ;
	rdfs:label "NATO Other/Enlisted Rank OR-4"@en ;
	owl:subClassOf :Enlisted , :NatoRanks , :NonCommissionedOfficer .

:NatoRankOR-5 org:rankJuniorTo <http://rdf.muninn-project.org/ontologies/NatoRankOR-4> ;
	org:rankSeniorTo <http://rdf.muninn-project.org/ontologies/NatoRankOR-6> ;
	a owl:Class ;
	rdfs:label "NATO Other/Enlisted Rank OR-5"@en ;
	owl:subClassOf :Enlisted , :NatoRanks , :NonCommissionedOfficer .

:NatoRankOR-6 org:rankJuniorTo <http://rdf.muninn-project.org/ontologies/NatoRankOR-5> ;
	org:rankSeniorTo <http://rdf.muninn-project.org/ontologies/NatoRankOR-7> ;
	a owl:Class ;
	rdfs:label "NATO Other/Enlisted Rank OR-6"@en ;
	owl:subClassOf :Enlisted , :NatoRanks , :NonCommissionedOfficer .

:NatoRankOR-7 org:rankJuniorTo <http://rdf.muninn-project.org/ontologies/NatoRankOR-6> ;
	org:rankSeniorTo <http://rdf.muninn-project.org/ontologies/NatoRankOR-8> ;
	a owl:Class ;
	rdfs:label "NATO Other/Enlisted Rank OR-7"@en ;
	owl:subClassOf :Enlisted , :NatoRanks , :NonCommissionedOfficer .

:NatoRankOR-8 org:rankJuniorTo <http://rdf.muninn-project.org/ontologies/NatoRankOR-7> ;
	org:rankSeniorTo <http://rdf.muninn-project.org/ontologies/NatoRankOR-9> ;
	a owl:Class ;
	rdfs:label "NATO Other/Enlisted Rank OR-8"@en ;
	owl:subClassOf :Enlisted , :NatoRanks , :NonCommissionedOfficer .

:NatoRankOR-9 org:rankJuniorTo <http://rdf.muninn-project.org/ontologies/NatoRankOR-8> ;
	a owl:Class ;
	rdfs:label "NATO Other/Enlisted Rank OR-9"@en ;
	owl:subClassOf :Enlisted , :NatoRanks , :NonCommissionedOfficer .

:NatoRankWO-1 org:rankJuniorTo <http://rdf.muninn-project.org/ontologies/NatoRankOF-10> ;
	org:rankSeniorTo <http://rdf.muninn-project.org/ontologies/NatoRankWO-2> ;
	a owl:Class ;
	rdfs:label "NATO Warrant Officer Rank WO-1"@en ;
	owl:subClassOf :NatoRanks , :WarrantOfficer .

:NatoRankWO-2 org:rankJuniorTo <http://rdf.muninn-project.org/ontologies/NatoRankWO-1> ;
	org:rankSeniorTo <http://rdf.muninn-project.org/ontologies/NatoRankWO-3> ;
	a owl:Class ;
	rdfs:label "NATO Warrant Officer Rank WO-2"@en ;
	owl:subClassOf :NatoRanks , :WarrantOfficer .

:NatoRankWO-3 org:rankJuniorTo <http://rdf.muninn-project.org/ontologies/NatoRankWO-2> ;
	org:rankSeniorTo <http://rdf.muninn-project.org/ontologies/NatoRankWO-4> ;
	a owl:Class ;
	rdfs:label "NATO Warrant Officer Rank WO-3"@en ;
	owl:subClassOf :NatoRanks , :WarrantOfficer .

:NatoRankWO-4 org:rankJuniorTo <http://rdf.muninn-project.org/ontologies/NatoRankWO-3> ;
	org:rankSeniorTo <http://rdf.muninn-project.org/ontologies/NatoRankWO-5> ;
	a owl:Class ;
	rdfs:label "NATO Warrant Officer Rank WO-4"@en ;
	owl:subClassOf :NatoRanks , :WarrantOfficer .

:NatoRankWO-5 org:rankJuniorTo <http://rdf.muninn-project.org/ontologies/NatoRankWO-4> ;
	org:rankSeniorTo <http://rdf.muninn-project.org/ontologies/NatoRankOR-1> ;
	a owl:Class ;
	rdfs:label "NATO Warrant Officer Rank WO-5"@en ;
	owl:subClassOf :NatoRanks , :WarrantOfficer .

:NatoRanks a owl:Class ;
	rdfs:label "Grades de l'OTAN"@fr , "NATO Rangcode"@de , "Ranks of NATO"@en ;
	owl:subClassOf :MilitaryRank .

:NavalArtillery a owl:Class ;
	rdfs:comment "Naval artillery unit operating from the ship on land."@en ;
	rdfs:label "Artillerie Navale"@fr , "Navel Artillery"@en , "Schiffsartillerie"@de ;
	owl:isPartOf :Navy ;
	owl:subClassOf :Artillery .

:NavalFleet org:hasPart :NavalTaskForce ;
	org:isPartOf :NavyBigFleet ;
	a owl:Class ;
	rdfs:comment "A fleet, or naval fleet, is a large formation of warships, and the largest formation in any navy. A fleet at sea is the direct equivalent of an army on land. Fleets are usually, but not necessarily, permanent formations and are generally assigned to a particular ocean or sea. Most fleets are named after that ocean or sea, but the convention in the United States Navy is to use numbers."@en ;
	rdfs:label "Flota"@ca , "Flota"@es , "Flota"@pl , "Flotta"@it , "Flotta"@sv , "Flotte"@fr , "Flotte (Marine)"@de , "Flåte (marine)"@no , "Frota"@pt , "Hạm đội"@vi , "Laivasto (sotilasyksikkö)"@fi , "Loďstvo"@cs , "Naval fleet"@en , "Vloot"@nl , "Флот"@ru ;
	owl:isPartOf :Navy ;
	owl:sameAs <dbpedia:Naval_fleet> ;
	foaf:name "Naval fleet" .

:NavalOfficer a owl:Class ;
	rdfs:comment "A Commissioned Officer serving in a political entity's Navy."@en ;
	rdfs:label "Naval Officer"@en , "Officier (Marine)"@fr , "Offiziere (Deutsche Marine)"@de ;
	owl:subClassOf :SeamanMilitary .

:NavalRating a owl:Class ;
	rdfs:comment "A Seaman serving in a political entity's Navy."@en ;
	rdfs:label "Maître (Marine de Guerre)"@fr , "Naval Rating"@en , "Unteroffiziere (Deutsche Marine)"@de ;
	owl:subClassOf :SeamanMilitary .

:NavalSquadron org:hasPart :DivisionNavalEstablishment ;
	org:isPartOf :Flotilla ;
	org:nominalSize "4" ;
	a owl:Class ;
	rdfs:comment "A squadron, or naval squadron, is a unit of 3-4 major warships, transport ships, submarines, or sometimes small craft that may be part of a larger task force or a fleet. A squadron is usually composed of a homogeneous group of the same classification of ships, such as battleships, battlecruisers, cruisers, destroyers or frigates, or of various types tasked with a specific mission such as coastal patrol, blockade, or minesweeping. Smaller warships are usually grouped in flotillas."@en ;
	rdfs:label "Escadre"@fr , "Eskader"@nl , "Eskader"@sv , "Eskadra"@cs , "Eskadra (marynarka wojenna)"@pl , "Eskadre"@no , "Esquadra naval"@pt , "Geschwader (Marine)"@de , "Hải đoàn"@vi , "Laivue (laivasto)"@fi , "Squadron (naval)"@en , "Эскадра"@ru ;
	owl:sameAs <dbpedia:Squadron_(naval)> ;
	owl:subClass :Navy , :Squadron ;
	foaf:name "Squadron" .

:NavalTaskForce org:hasPart :CarrierBattleGroup ;
	org:isPartOf :NavalFleet ;
	a owl:Class ;
	rdfs:label "Force opérationnelle (Marine)"@fr , "Task Force (Marine)"@de , "Task Force (Naval)"@en ;
	owl:differentFrom <dbpedia:Task_force> ;
	owl:isPartOf :Navy .

:NavyAirStation a owl:Class ;
	rdfs:comment "An Naval air station."@en ;
	rdfs:label ""@de , ""@fr , "Station (Naval Aircraft)"@en .

:NavyBigFleet org:hasPart :NavalFleet ;
	a owl:Class ;
	rdfs:comment "A named or numbered Navy based on operating area or administrative grouping."@en ;
	rdfs:label "Marine (Boot-Gruppe)"@de , "Marine (Groupe de batiment naval)"@fr , "Navy (Named or Numbered)"@en ;
	owl:isPartOf :Navy ;
	foaf:name "Navy" .

:NavyMerchant a owl:Class ;
	owl:disjointWith :NavyServiceBranch ;
	owl:sameAs "dbpedia:Merchant_navy" ;
	owl:subClassOf <org:WaterBasedOrganization> .

:NavyServiceBranch :member :SeamanMilitary ;
	:membershipClass <http://rdf.muninn-project.org/ww1/2011/11/11/GroupMemberships/NavyAppointments> ;
	a owl:Class ;
	owl:sameAs "dbpedia:Navy" ;
	owl:subClassOf :FightsPrimarilyOnAndInWater , :MilitaryServiceBranch , :WaterBasedOrganization .

:Non-Combatant a owl:Class ;
	rdfs:comment "A person not engaged in combat and/or war, but which might be involved in a war. This includes nurses, chaplains, medics depending on the era."@en ;
	rdfs:label ""@de , "Non-Combatant"@en , "Non-Combatant"@fr ;
	owl:disjointWith :Combatant ;
	owl:subClassOf :Person , <org:Role> ;
	foaf:name "Non-Combatant" .

:NonCommissionedOfficer a owl:Class ;
	rdfs:comment "A soldier with a rank of Corporal or above."@en ;
	rdfs:label "Non Commissioned Officer"@en , "Soldatenlaufbahnverordnung"@de , "Sous-Officier Subalternes"@fr ;
	owl:subClassOf :Soldier ;
	foaf:name "Non Commissioned Officer" .

:Officer a owl:Class ;
	rdfs:comment "A commissioned officer, acting, breveted or confirmed."@en ;
	rdfs:label "Officer"@en , "Officier"@fr , "Offizier"@de ;
	owl:subClassOf :Soldier ;
	foaf:name "Officer" .

:Platoon org:hasPart :ArmySection , :ArmySquad ;
	org:isPartOf :ArmyCompany , :ArmyServiceBranch ;
	a owl:Class ;
	rdfs:comment "A platoon"@en ;
	rdfs:label "Peloton (militaire)"@de , "Platoon"@en , "Platoon"@fr ;
	owl:sameAs "dbpedia:Platoon" ;
	foaf:logo <http://rdf.muninn-project.org/ww1/2011/11/11/image/31> .

:PrivilegedCombatant a owl:Class ;
	rdfs:comment "A person engaging in combat and/or war as a privileged combatants under the rules of war, circa Great War."@en ;
	rdfs:label "Combatant privilégié"@fr , "Privileged Combatant"@en , "privilegierten Kämpfer"@de ;
	owl:disjointWith :UnprivilegedCombatant ;
	owl:subClassOf :Combatant ;
	foaf:name "Privileged Combatant" .

:ProtoAirForce org:hasPart :BrigadeAirCorps ;
	org:isPartOf :ArmyServiceBranch ;
	a :ArmsType , owl:Class ;
	rdfs:comment "Use this class for army air corps, naval aviation and army aviation."@en ;
	rdfs:label "Proto Air Force"@en , "Proto_air_force"@en ;
	owl:disjointWith :AirForceServiceBranch ;
	owl:subClassOf :FightsPrimarilyInAir ;
	foaf:name "Proto Air Force" .

:RankAbleSeaman a :MilitaryRank ;
	rdfs:label "Able Seaman"@en ;
	owl:sameAs <dbpedia:Able_seaman_%28rank%29> ;
	foaf:name "Able Seaman" .

:RankAbleSeaman_Canada org:rankOf <dbpedia:Canada> ;
	a :MilitaryRank ;
	rdfs:comment "The specific instance of the  rank in the context of country ."@en ;
	owl:subClass :RankAbleSeaman ;
	foaf:name ""@en .

:RankAbleSeaman_Commonwealth_of_Nations org:rankOf <dbpedia:Commonwealth_of_Nations> ;
	a :MilitaryRank ;
	rdfs:comment "The specific instance of the  rank in the context of country Commonwealth of Nations."@en ;
	rdfs:label " (Commonwealth delle nazioni)"@it , " (Commonwealth of Nations)"@de , " (Commonwealth of Nations)"@en , " (Commonwealth of Nations)"@fr , " (Commonwealth)"@pt , " (Gemenebest van Naties)"@nl , " (Kansainyhteisö)"@fi , " (Mancomunidad de Naciones)"@es , " (Samveldet av nasjoner)"@no , " (Samväldet)"@sv , " (Wspólnota Narodów)"@pl , " (Содружество наций)"@ru ;
	owl:subClass :RankAbleSeaman ;
	foaf:name ""@en .

:RankCaptainNaval a :MilitaryRank ;
	rdfs:comment "Captain is the name most often given in English-speaking navies to the rank corresponding to command of the largest ships. The NATO rank code is OF-5, equivalent to an army full colonel. The equivalent rank in some navies translates as \"ship captain\" (e.g. French - capitaine de vaisseau), \"captain of sea and war\" (Portuguese capitão de mar e guerra), \"captain at sea\" (e.g. German Kapitän zur See) or \"captain of the first rank\" (Russian - капитан 1-го ранга)."@en ;
	rdfs:label "Capitaine de vaisseau"@fr , "Capitano di vascello"@it , "Capitán de navío"@es , "Capitão de mar e guerra"@pt , "Captain (naval)"@en , "Kapitein-ter-zee"@nl , "Kapitän zur See"@de , "Komandor"@pl , "Kommandør"@no , "Kommendör"@sv , "Kommodori"@fi , "Капитан 1-го ранга"@ru ;
	owl:sameAs <dbpedia:Captain_%28naval%29> ;
	foaf:name "Captain" .

:RankCaptainNaval_Australia org:rankOf <dbpedia:Australia> ;
	a :MilitaryRank ;
	rdfs:comment "The specific instance of the Captain (naval) rank in the context of country Australia."@en ;
	rdfs:label "Capitaine de vaisseau (Australie)"@fr , "Capitano di vascello (Australia)"@it , "Capitán de navío (Australia)"@es , "Capitão de mar e guerra (Austrália)"@pt , "Captain (naval) (Australia)"@en , "Kapitein-ter-zee (Australië (land))"@nl , "Kapitän zur See (Australien)"@de , "Komandor (Australia)"@pl , "Kommandør (Australia)"@no , "Kommendör (Australien)"@sv , "Kommodori (Australia)"@fi , "Капитан 1-го ранга (Австралия)"@ru ;
	owl:subClass :RankCaptainNaval ;
	foaf:name "Captain"@en .

:RankCaptainNaval_Canada org:rankOf <dbpedia:Canada> ;
	a :MilitaryRank ;
	rdfs:comment "The specific instance of the Captain (naval) rank in the context of Canada."@en ;
	rdfs:label "Capitaine de vaisseau (Canada)"@fr , "Capitano di vascello (Canada)"@it , "Capitán de navío (Canada)"@es , "Capitão de mar e guerra (Canada)"@pt , "Captain (naval, Canada)"@en , "Kapitein-ter-zee (Canada)"@nl , "Kapitän zur See (Canada)"@de , "Komandor (Canada)"@pl , "Kommandør (Canada)"@no , "Kommendör (Canada)"@sv , "Kommodori (Canada)"@fi , "Капитан 1-го ранга (Canada)"@ru ;
	owl:subClass :RankCaptainNaval ;
	foaf:name "Capitaine de vaisseau"@fr .

:RankCombatMilitaryRank a :MilitaryRank ;
	rdfs:comment "Combat or Kombat, abbreviated from Командир батальона (\"Commander of a battalion\") was a military rank in the Red Army until the end of the 1930s. At that time it was roughly equivalent to the rank of Captain."@en ;
	rdfs:label "Combat (military rank)"@en ;
	owl:sameAs <dbpedia:Combat_%28military_rank%29> ;
	foaf:name "Combat" .

:RankCombatMilitaryRank_Russia org:rankOf <dbpedia:Russia> ;
	a :MilitaryRank ;
	rdfs:comment "The specific instance of the Combat (military rank) rank in the context of country Russia."@en ;
	rdfs:label "Combat (military rank) (Rosja)"@pl , "Combat (military rank) (Rusia)"@es , "Combat (military rank) (Rusland)"@nl , "Combat (military rank) (Russia)"@en , "Combat (military rank) (Russia)"@it , "Combat (military rank) (Russie)"@fr , "Combat (military rank) (Russland)"@de , "Combat (military rank) (Russland)"@no , "Combat (military rank) (Ryssland)"@sv , "Combat (military rank) (Rússia)"@pt , "Combat (military rank) (Venäjä)"@fi , "Combat (military rank) (Россия)"@ru ;
	owl:subClass :RankCombatMilitaryRank ;
	foaf:name "Combat"@en .

:RankCombatMilitaryRank_Soviet_Union org:rankOf <dbpedia:Soviet_Union> ;
	a :MilitaryRank ;
	rdfs:comment "The specific instance of the Combat (military rank) rank in the context of country Soviet Union."@en ;
	rdfs:label "Combat (military rank) (Neuvostoliitto)"@fi , "Combat (military rank) (Soviet Union)"@en , "Combat (military rank) (Sovjet-Unie)"@nl , "Combat (military rank) (Sovjetunionen)"@no , "Combat (military rank) (Sovjetunionen)"@sv , "Combat (military rank) (Sowjetunion)"@de , "Combat (military rank) (Union des républiques socialistes soviétiques)"@fr , "Combat (military rank) (Unione Sovietica)"@it , "Combat (military rank) (União Soviética)"@pt , "Combat (military rank) (Unión Soviética)"@es , "Combat (military rank) (Związek Socjalistycznych Republik Radzieckich)"@pl , "Combat (military rank) (Союз Советских Социалистических Республик)"@ru ;
	owl:subClass :RankCombatMilitaryRank ;
	foaf:name "Combat"@en .

:RankCommandant a :MilitaryRank ;
	rdfs:comment "Commandant is a military or police rank. In the French, Spanish and Irish armed forces it is a rank equivalent to major. In South Africa for most of the second half of the 20th century, commandant was a rank equivalent to lieutenant-colonel in other countries."@en ;
	rdfs:label "Commandant (rank)"@en ;
	owl:sameAs <dbpedia:Commandant_%28rank%29> ;
	foaf:name "Commandant" .

:RankCommandant_France org:rankOf <dbpedia:France> ;
	a :MilitaryRank ;
	rdfs:comment "The specific instance of the Commandant (rank) rank in the context of France."@en ;
	rdfs:label "Commandant (rank) (France)"@en ;
	owl:subClass :RankCommandant ;
	foaf:name "Commandant"@en .

:RankCommandant_Republic_of_Ireland org:rankOf <dbpedia:Republic_of_Ireland> ;
	a :MilitaryRank ;
	rdfs:comment "The specific instance of the Commandant (rank) rank in the context of country Republic of Ireland."@en ;
	rdfs:label "Commandant (rank) (Ierland (land))"@nl , "Commandant (rank) (Irland)"@de , "Commandant (rank) (Irland)"@no , "Commandant (rank) (Irland)"@sv , "Commandant (rank) (Irlanda)"@es , "Commandant (rank) (Irlanda)"@it , "Commandant (rank) (Irlande (pays))"@fr , "Commandant (rank) (Irlandia)"@pl , "Commandant (rank) (Irlanti)"@fi , "Commandant (rank) (Republic of Ireland)"@en , "Commandant (rank) (República da Irlanda)"@pt , "Commandant (rank) (Ирландия)"@ru ;
	owl:subClass :RankCommandant ;
	foaf:name "Commandant"@en .

:RankDriver a :MilitaryRank ;
	rdfs:comment "Driver (Dvr) was a military rank used in the British Army and the armies of other Commonwealth countries. It was equivalent to the rank of Private. The rank was initially used in the Royal Artillery for the men who drove the teams of horses which pulled the guns. It was phased out after the First World War (when all Royal Artillerymen of the lowest rank were redesignated as Gunners). It was also used in the Royal Australian Artillery and Royal Canadian Artillery."@en ;
	rdfs:label "Driver (rank)"@en ;
	owl:sameAs <dbpedia:Driver_%28rank%29> ;
	foaf:name "Driver" .

:RankDriver_Australia org:rankOf <dbpedia:Australia> ;
	a :MilitaryRank ;
	rdfs:comment "The specific instance of the Driver (rank) rank in the context of country Australia."@en ;
	rdfs:label "Driver (rank) (Australia)"@en , "Driver (rank) (Australia)"@es , "Driver (rank) (Australia)"@fi , "Driver (rank) (Australia)"@it , "Driver (rank) (Australia)"@no , "Driver (rank) (Australia)"@pl , "Driver (rank) (Australie)"@fr , "Driver (rank) (Australien)"@de , "Driver (rank) (Australien)"@sv , "Driver (rank) (Australië (land))"@nl , "Driver (rank) (Austrália)"@pt , "Driver (rank) (Австралия)"@ru ;
	owl:subClass :RankDriver ;
	foaf:name "Driver"@en .

:RankDriver_Canada org:rankOf <dbpedia:Canada> ;
	a :MilitaryRank ;
	rdfs:comment "The specific instance of the Driver (rank) rank in the context of Canada."@en ;
	rdfs:label "Driver (rank, Canada)"@en ;
	owl:subClass :RankDriver ;
	foaf:name "Driver"@en .

:Rank_Admiral_EnglishTradition org:rankEquivalentTo :Rank_Air_marshal_EnglishTradition , :Rank_General_officer_EnglishTradition ;
	org:rankJuniorToTransitive :Rank_Admiral_of_the_fleet_EnglishTradition ;
	org:rankOf :EnglishTradition , <mil:NavyServiceBranch> ;
	org:rankSeniorToTransitive <http://rdf.muninn-project.org/ontologies/military#Rank_Commodore_(rank)_EnglishTradition> ;
	a :MilitaryRank ;
	rdfs:comment "Admiral is the rank, or part of the name of the ranks, of the highest naval officers. It is usually considered a full admiral (equivalent to full general) and above vice admiral and below admiral of the fleet. It is usually abbreviated to \"Adm\" or \"ADM\". Where relevant, admiral has a NATO code of OF-9, and is a 4 star rank."@en ;
	rdfs:label "Admiral"@de , "Admiral"@en , "Amiral"@fr ;
	owl:sameAs <dbpedia:Admiral> .

:Rank_Admiral_of_the_Fleet_Russia a :MilitaryRank ;
	rdfs:comment "Admiral of the Fleet or Fleet Admiral (Адмирал флoта, Admiral flota) is the highest naval (deck) rank of the Russian Federation. It is the equivalent of the Soviet naval rank of Admiral of the Fleet and the present Russian rank of General of the Army. The rank is roughly equivalent to 4-stars Admiral ranks of other nations. There is only one rank higher than that of Admiral of the Fleet in the Russian armed forces, namely Marshal of the Russian Federation."@en ;
	rdfs:label "Admiral of the Fleet (Russia)"@en , "Ammiraglio della flotta (Russia)"@it ;
	owl:sameAs <dbpedia:Admiral_of_the_Fleet_%28Russia%29> ;
	foaf:name "Admiral of the Fleet" .

:Rank_Admiral_of_the_Fleet_Russia_Russia org:rankOf <dbpedia:Russia> ;
	a :MilitaryRank ;
	rdfs:comment "The specific instance of the Admiral of the Fleet (Russia) rank in the context of country Russia."@en ;
	rdfs:label "Admiral of the Fleet (Russia) (Rosja)"@pl , "Admiral of the Fleet (Russia) (Rusia)"@es , "Admiral of the Fleet (Russia) (Rusland)"@nl , "Admiral of the Fleet (Russia) (Russia)"@en , "Admiral of the Fleet (Russia) (Russie)"@fr , "Admiral of the Fleet (Russia) (Russland)"@de , "Admiral of the Fleet (Russia) (Russland)"@no , "Admiral of the Fleet (Russia) (Ryssland)"@sv , "Admiral of the Fleet (Russia) (Rússia)"@pt , "Admiral of the Fleet (Russia) (Venäjä)"@fi , "Admiral of the Fleet (Russia) (Россия)"@ru , "Ammiraglio della flotta (Russia) (Russia)"@it ;
	owl:subClass :Rank_Admiral_of_the_Fleet_Russia ;
	foaf:name "Admiral of the Fleet"@en .

:Rank_Admiral_of_the_Fleet_Russia_Soviet_Union org:rankOf <dbpedia:Soviet_Union> ;
	a :MilitaryRank ;
	rdfs:comment "The specific instance of the Admiral of the Fleet (Russia) rank in the context of country Soviet Union."@en ;
	rdfs:label "Admiral of the Fleet (Russia) (Neuvostoliitto)"@fi , "Admiral of the Fleet (Russia) (Soviet Union)"@en , "Admiral of the Fleet (Russia) (Sovjet-Unie)"@nl , "Admiral of the Fleet (Russia) (Sovjetunionen)"@no , "Admiral of the Fleet (Russia) (Sovjetunionen)"@sv , "Admiral of the Fleet (Russia) (Sowjetunion)"@de , "Admiral of the Fleet (Russia) (Union des républiques socialistes soviétiques)"@fr , "Admiral of the Fleet (Russia) (União Soviética)"@pt , "Admiral of the Fleet (Russia) (Unión Soviética)"@es , "Admiral of the Fleet (Russia) (Związek Socjalistycznych Republik Radzieckich)"@pl , "Admiral of the Fleet (Russia) (Союз Советских Социалистических Республик)"@ru , "Ammiraglio della flotta (Russia) (Unione Sovietica)"@it ;
	owl:subClass :Rank_Admiral_of_the_Fleet_Russia ;
	foaf:name "Admiral of the Fleet"@en .

:Rank_Admiral_of_the_fleet_EnglishTradition org:rankEquivalentTo :Rank_Field_marshal_EnglishTradition , :Rank_Marshal_EnglishTradition , :Rank_Marshal_of_the_air_force_EnglishTradition ;
	org:rankOf :EnglishTradition , <mil:NavyServiceBranch> ;
	org:rankSeniorToTransitive :Rank_Admiral_EnglishTradition ;
	a :MilitaryRank ;
	rdfs:label "Admiral of the fleet"@en ;
	owl:sameAs <dbpedia:Admiral_of_the_fleet> .

:Rank_Agha a :MilitaryRank ;
	rdfs:comment "For other uses of the term 'Aga', see Aga. For other uses of the term 'Agha', see Agha. Agha, also Aga, as a title for a civil or military officer, or often part of such title, was placed after the name of certain military functionaries in the Ottoman Empire. At the same time some court functionaries were entitled to the agha title."@en ;
	rdfs:label "Aga (wojsko)"@pl , "Agha"@fi , "Agha"@fr , "Agha"@it , "Agha"@no , "Agha"@sv , "Agha (Ottoman Empire)"@en , "Agha (Titel)"@de , "Ага (титул военачальников)"@ru ;
	owl:sameAs <dbpedia:Agha_%28Ottoman_Empire%29> ;
	foaf:name "Agha" .

:Rank_Agha_Cossack_Hetmanate org:rankOf <dbpedia:Cossack_Hetmanate> ;
	a :MilitaryRank ;
	rdfs:comment "The specific instance of the Agha (Ottoman Empire) rank in the context of country Cossack Hetmanate."@en ;
	rdfs:label "Aga (wojsko) (Hetmańszczyzna)"@pl , "Agha (Cossack Hetmanate)"@fi , "Agha (Cossack Hetmanate)"@it , "Agha (Cossack Hetmanate)"@no , "Agha (Cossack Hetmanate)"@sv , "Agha (Hetmanat cosaque)"@fr , "Agha (Ottoman Empire) (Cossack Hetmanate)"@en , "Agha (Ottoman Empire) (Hetmanato cosaco)"@es , "Agha (Titel) (Hetmanat)"@de , "Ага (титул военачальников) (Гетманщина)"@ru ;
	owl:subClass :Rank_Agha ;
	foaf:name "Agha"@en .

:Rank_Agha_Ottoman_Empire org:rankOf <dbpedia:Ottoman_Empire> ;
	a :MilitaryRank ;
	rdfs:comment "The specific instance of the Agha (Ottoman Empire) rank in the context of country Ottoman Empire."@en ;
	rdfs:label "Aga (wojsko) (Imperium osmańskie)"@pl , "Agha (Det osmanske rike)"@no , "Agha (Empire ottoman)"@fr , "Agha (Impero ottomano)"@it , "Agha (Osmanien valtakunta)"@fi , "Agha (Osmanska riket)"@sv , "Agha (Ottoman Empire) (Imperio otomano)"@es , "Agha (Ottoman Empire) (Império Otomano)"@pt , "Agha (Ottoman Empire) (Ottomaanse Rijk)"@nl , "Agha (Ottoman Empire) (Ottoman Empire)"@en , "Agha (Titel) (Osmanisches Reich)"@de , "Ага (титул военачальников) (Османская империя)"@ru ;
	owl:subClass :Rank_Agha ;
	foaf:name "Agha"@en .

:Rank_Agha_Septinsular_Republic org:rankOf <dbpedia:Septinsular_Republic> ;
	a :MilitaryRank ;
	rdfs:comment "The specific instance of the Agha (Ottoman Empire) rank in the context of country Septinsular Republic."@en ;
	rdfs:label "Aga (wojsko) (Republika Siedmiu Wysp)"@pl , "Agha (Ottoman Empire) (Republiek van de Zeven Eilanden)"@nl , "Agha (Ottoman Empire) (República de las Islas Jónicas)"@es , "Agha (Ottoman Empire) (Septinsular Republic)"@en , "Agha (Repubblica delle Sette Isole Unite)"@it , "Agha (République des Sept-Îles)"@fr , "Agha (Septinsular Republic)"@fi , "Agha (Septinsular Republic)"@no , "Agha (Septinsular Republic)"@sv , "Agha (Titel) (Septinsular Republic)"@de , "Ага (титул военачальников) (Республика Семи Островов)"@ru ;
	owl:subClass :Rank_Agha ;
	foaf:name "Agha"@en .

:Rank_Air_chief_marshal a :MilitaryRank ;
	rdfs:label "Air chief marshal"@en ;
	owl:sameAs <dbpedia:Air_chief_marshal> ;
	foaf:name "Air chief marshal" .

:Rank_Air_chief_marshal_Australia org:rankOf <dbpedia:Australia> ;
	a :MilitaryRank ;
	rdfs:comment "The specific instance of the Air chief marshal rank in the context of country Australia."@en ;
	rdfs:label "Air chief marshal (Australia)"@en , "Air chief marshal (Australia)"@es , "Air chief marshal (Australia)"@fi , "Air chief marshal (Australia)"@it , "Air chief marshal (Australia)"@no , "Air chief marshal (Australia)"@pl , "Air chief marshal (Australie)"@fr , "Air chief marshal (Australien)"@de , "Air chief marshal (Australien)"@sv , "Air chief marshal (Australië (land))"@nl , "Air chief marshal (Austrália)"@pt , "Air chief marshal (Австралия)"@ru ;
	owl:subClass :Rank_Air_chief_marshal ;
	foaf:name "Air chief marshal"@en .

:Rank_Air_chief_marshal_Australia_Australia org:rankOf <dbpedia:Australia> ;
	a :MilitaryRank ;
	rdfs:comment "The specific instance of the  rank in the context of country Australia."@en ;
	rdfs:label " (Australia)"@en , " (Australia)"@es , " (Australia)"@fi , " (Australia)"@it , " (Australia)"@no , " (Australia)"@pl , " (Australie)"@fr , " (Australien)"@de , " (Australien)"@sv , " (Australië (land))"@nl , " (Austrália)"@pt , " (Австралия)"@ru ;
	owl:subClass :Rank_Air_chief_marshal_Australia ;
	foaf:name ""@en .

:Rank_Air_chief_marshal_Canada org:rankOf <dbpedia:Canada> ;
	a :MilitaryRank ;
	rdfs:comment "The specific instance of the Air chief marshal rank in the context of Canada."@en ;
	rdfs:label "Air chief marshal (Canada)"@en ;
	owl:subClass :Rank_Air_chief_marshal ;
	foaf:name "Air chief marshal"@en .

:Rank_Air_chief_marshal_Commonwealth_of_Nations org:rankOf <dbpedia:Commonwealth_of_Nations> ;
	a :MilitaryRank ;
	rdfs:comment "The specific instance of the Air chief marshal rank in the context of country Commonwealth of Nations."@en ;
	rdfs:label "Air chief marshal (Commonwealth delle nazioni)"@it , "Air chief marshal (Commonwealth of Nations)"@de , "Air chief marshal (Commonwealth of Nations)"@en , "Air chief marshal (Commonwealth of Nations)"@fr , "Air chief marshal (Commonwealth)"@pt , "Air chief marshal (Gemenebest van Naties)"@nl , "Air chief marshal (Kansainyhteisö)"@fi , "Air chief marshal (Mancomunidad de Naciones)"@es , "Air chief marshal (Samveldet av nasjoner)"@no , "Air chief marshal (Samväldet)"@sv , "Air chief marshal (Wspólnota Narodów)"@pl , "Air chief marshal (Содружество наций)"@ru ;
	owl:subClass :Rank_Air_chief_marshal ;
	foaf:name "Air chief marshal"@en .

:Rank_Air_commodore_EnglishTradition org:rankEquivalentTo :Rank_Brigadier_EnglishTradition , <http://rdf.muninn-project.org/ontologies/military#Rank_Commodore_(rank)_EnglishTradition> ;
	org:rankJuniorToTransitive :Rank_Air_marshal_EnglishTradition ;
	org:rankOf :EnglishTradition , <mil:AirForceServiceBranch> ;
	org:rankSeniorToTransitive :Rank_Group_captain_EnglishTradition ;
	a :MilitaryRank ;
	rdfs:label "Air commodore"@en ;
	owl:sameAs <dbpedia:Air_commodore> .

:Rank_Air_marshal_EnglishTradition org:rankEquivalentTo :Rank_Admiral_EnglishTradition , :Rank_General_officer_EnglishTradition ;
	org:rankJuniorToTransitive :Rank_Marshal_of_the_air_force_EnglishTradition ;
	org:rankOf :EnglishTradition , <mil:AirForceServiceBranch> ;
	org:rankSeniorToTransitive :Rank_Air_commodore_EnglishTradition ;
	a :MilitaryRank ;
	rdfs:label "Air marshal"@en ;
	owl:sameAs <dbpedia:Air_marshal> .

:Rank_Air_vice-marshal a :MilitaryRank ;
	rdfs:label "Air vice-marshal"@en ;
	owl:sameAs <dbpedia:Air_vice-marshal> ;
	foaf:name "Air vice-marshal" .

:Rank_Air_vice-marshal_Australia org:rankOf <dbpedia:Australia> ;
	a :MilitaryRank ;
	rdfs:comment "The specific instance of the Air vice-marshal rank in the context of country Australia."@en ;
	rdfs:label "Air vice-marshal (Australia)"@en , "Air vice-marshal (Australia)"@es , "Air vice-marshal (Australia)"@fi , "Air vice-marshal (Australia)"@it , "Air vice-marshal (Australia)"@no , "Air vice-marshal (Australia)"@pl , "Air vice-marshal (Australie)"@fr , "Air vice-marshal (Australien)"@de , "Air vice-marshal (Australien)"@sv , "Air vice-marshal (Australië (land))"@nl , "Air vice-marshal (Austrália)"@pt , "Air vice-marshal (Австралия)"@ru ;
	owl:subClass :Rank_Air_vice-marshal ;
	foaf:name "Air vice-marshal"@en .

:Rank_Air_vice-marshal_Canada org:rankOf <dbpedia:Canada> ;
	a :MilitaryRank ;
	rdfs:comment "The specific instance of the Air vice-marshal rank in the context of Canada."@en ;
	rdfs:label "Air vice-marshal (Canada)"@en ;
	owl:subClass :Rank_Air_vice-marshal ;
	foaf:name "Air vice-marshal"@en .

:Rank_Air_vice-marshal_Commonwealth_of_Nations org:rankOf <dbpedia:Commonwealth_of_Nations> ;
	a :MilitaryRank ;
	rdfs:comment "The specific instance of the Air vice-marshal rank in the context of country Commonwealth of Nations."@en ;
	rdfs:label "Air vice-marshal (Commonwealth delle nazioni)"@it , "Air vice-marshal (Commonwealth of Nations)"@de , "Air vice-marshal (Commonwealth of Nations)"@en , "Air vice-marshal (Commonwealth of Nations)"@fr , "Air vice-marshal (Commonwealth)"@pt , "Air vice-marshal (Gemenebest van Naties)"@nl , "Air vice-marshal (Kansainyhteisö)"@fi , "Air vice-marshal (Mancomunidad de Naciones)"@es , "Air vice-marshal (Samveldet av nasjoner)"@no , "Air vice-marshal (Samväldet)"@sv , "Air vice-marshal (Wspólnota Narodów)"@pl , "Air vice-marshal (Содружество наций)"@ru ;
	owl:subClass :Rank_Air_vice-marshal ;
	foaf:name "Air vice-marshal"@en .

:Rank_Aircraftman_EnglishTradition org:rankEquivalentTo <http://rdf.muninn-project.org/ontologies/military#Rank_Private_(rank)_EnglishTradition> , :Rank_Seaman_EnglishTradition ;
	org:rankJuniorToTransitive :Rank_Corporal_EnglishTradition ;
	org:rankOf :EnglishTradition , <mil:AirForceServiceBranch> ;
	a :MilitaryRank ;
	rdfs:comment "Aircraftman (AC), or Aircraftwoman (ACW), is the lowest rank in the Royal Air Force and the air forces of several other Commonwealth countries. Aircraftman ranks below Leading Aircraftman and has a NATO rank code of OR-1. It is presently a training rank only and no airmen in productive service hold this rank. Aircraftman do not wear any rank insignia."@en ;
	rdfs:label "Aircraftman"@en ;
	owl:sameAs <dbpedia:Aircraftman> .

:Rank_Anthypolochagos a :MilitaryRank ;
	rdfs:comment "Anthypolochagos is used in the Greek language to mean \"Second Lieutenant\". In the modern Hellenic Army the rank is the lowest commissioned officer rank and is inferior to an Ypolochagos. The insignia consists of a single silver star (or a star and a bar for reserve officers). Officers holding this rank should be addressed as \"Kyrie Anthypolochage\" (Κύριε Ανθυπολοχαγέ) by their subordinates, or \"Anthypolochage + family name\" by their superior officers."@en ;
	rdfs:label "Anthypolochagos"@en ;
	owl:sameAs <dbpedia:Anthypolochagos> ;
	foaf:name "Anthypolochagos" .

:Rank_Anthypolochagos_Greece org:rankOf <dbpedia:Greece> ;
	a :MilitaryRank ;
	rdfs:comment "The specific instance of the Anthypolochagos rank in the context of country Greece."@en ;
	rdfs:label "Anthypolochagos (Grecia)"@es , "Anthypolochagos (Grecia)"@it , "Anthypolochagos (Grecja)"@pl , "Anthypolochagos (Greece)"@en , "Anthypolochagos (Grekland)"@sv , "Anthypolochagos (Griechenland)"@de , "Anthypolochagos (Griekenland)"@nl , "Anthypolochagos (Grèce)"@fr , "Anthypolochagos (Grécia)"@pt , "Anthypolochagos (Hellas)"@no , "Anthypolochagos (Kreikka)"@fi , "Anthypolochagos (Греция)"@ru ;
	owl:subClass :Rank_Anthypolochagos ;
	foaf:name "Anthypolochagos"@en .

:Rank_Anthypolochagos_Official_Timocracy_of_Sapinetia org:rankOf <dbpedia:Official_Timocracy_of_Sapinetia> ;
	a :MilitaryRank ;
	rdfs:comment "The specific instance of the Anthypolochagos rank in the context of the Timocracy_of_Sapinetia."@en ;
	rdfs:label "Anthypolochagos (Timocracy of Sapinetia)"@en ;
	owl:subClass :Rank_Anthypolochagos ;
	foaf:name "Anthypolochagos"@en .

:Rank_Antisyntagmatarchis a :MilitaryRank ;
	rdfs:comment "Antisyntagmatarchis is used in the Greek language to mean \"Lieutenant Colonel\". The typical responsibility of an Antisyntagmatarchis is to exercise command of a battalion. Officers holding this rank should be addressed as \"Kyrie Diikita\" (Κύριε διοικητά) (stressed on the last syllable), by their subordinates when they exercise battalion command or \"Kyrie Antisyntagmatarcha\" (Κύριε Αντισυνταγματάρχα) (stressed on the syllable before last) in other cases."@en ;
	rdfs:label "Antisyntagmatarchis"@en ;
	owl:sameAs <dbpedia:Antisyntagmatarchis> ;
	foaf:name "Antisyntagmatarchis" .

:Rank_Antisyntagmatarchis_Greece org:rankOf <dbpedia:Greece> ;
	a :MilitaryRank ;
	rdfs:comment "The specific instance of the Antisyntagmatarchis rank in the context of country Greece."@en ;
	rdfs:label "Antisyntagmatarchis (Grecia)"@es , "Antisyntagmatarchis (Grecia)"@it , "Antisyntagmatarchis (Grecja)"@pl , "Antisyntagmatarchis (Greece)"@en , "Antisyntagmatarchis (Grekland)"@sv , "Antisyntagmatarchis (Griechenland)"@de , "Antisyntagmatarchis (Griekenland)"@nl , "Antisyntagmatarchis (Grèce)"@fr , "Antisyntagmatarchis (Grécia)"@pt , "Antisyntagmatarchis (Hellas)"@no , "Antisyntagmatarchis (Kreikka)"@fi , "Antisyntagmatarchis (Греция)"@ru ;
	owl:subClass :Rank_Antisyntagmatarchis ;
	foaf:name "Antisyntagmatarchis"@en .

:Rank_Antisyntagmatarchis_Official_Timocracy_of_Sapinetia org:rankOf <dbpedia:Official_Timocracy_of_Sapinetia> ;
	a :MilitaryRank ;
	rdfs:comment "The specific instance of the Antisyntagmatarchis rank in the context of the Timocracy_of_Sapinetia."@en ;
	rdfs:label "Antisyntagmatarchis (Timocracy_of_Sapinetia)"@en ;
	owl:subClass :Rank_Antisyntagmatarchis ;
	foaf:name "Antisyntagmatarchis"@en .

:Rank_Appointee_Italy org:rankOf <dbpedia:Italy> ;
	a :MilitaryRank ;
	rdfs:comment "The specific instance of the Appointee rank in the context of country Italy."@en ;
	rdfs:label "Appointee (Italia)"@es , "Appointee (Italia)"@fi , "Appointee (Italia)"@no , "Appointee (Italien)"@de , "Appointee (Italien)"@sv , "Appointee (Italië)"@nl , "Appointee (Italy)"@en , "Appointee (Itália)"@pt , "Appointee (Włochy)"@pl , "Appointee (Италия)"@ru , "Appointé (Italie)"@fr , "Appuntato (Italia)"@it ;
	owl:subClass :Rank_Appointee ;
	foaf:name "Appuntato"@it .

:Rank_Appointee_Switzerland org:rankOf <dbpedia:Switzerland> ;
	a :MilitaryRank ;
	rdfs:comment "The specific instance of the Appointee rank in the context of country Switzerland."@en ;
	rdfs:label "Appointee (Schweiz)"@de , "Appointee (Schweiz)"@sv , "Appointee (Suiza)"@es , "Appointee (Suíça)"@pt , "Appointee (Sveits)"@no , "Appointee (Sveitsi)"@fi , "Appointee (Switzerland)"@en , "Appointee (Szwajcaria)"@pl , "Appointee (Zwitserland)"@nl , "Appointee (Швейцария)"@ru , "Appointé (Suisse)"@fr , "Appuntato (Svizzera)"@it ;
	owl:subClass :Rank_Appointee ;
	foaf:name "Appointé"@fr , "Appuntato"@it .

:Rank_Army_General_Russia a :MilitaryRank ;
	rdfs:comment "Please see \"Army General\" for other nations which use this rank Army General is the second highest military rank in the Russian Federation, inferior only to a Marshal and superior to a Colonel General. It is a direct counterpart of the Soviet rank, General of the Army (USSR)."@en ;
	rdfs:label "Army General (Russia)"@en , "Генерал армии (Россия)"@ru ;
	owl:sameAs <dbpedia:Army_General_%28Russia%29> ;
	foaf:name "Army General" .

:Rank_Army_General_Russia_Russia org:rankOf <dbpedia:Russia> ;
	a :MilitaryRank ;
	rdfs:comment "The specific instance of the Army General (Russia) rank in the context of country Russia."@en ;
	rdfs:label "Army General (Russia) (Rosja)"@pl , "Army General (Russia) (Rusia)"@es , "Army General (Russia) (Rusland)"@nl , "Army General (Russia) (Russia)"@en , "Army General (Russia) (Russia)"@it , "Army General (Russia) (Russie)"@fr , "Army General (Russia) (Russland)"@de , "Army General (Russia) (Russland)"@no , "Army General (Russia) (Ryssland)"@sv , "Army General (Russia) (Rússia)"@pt , "Army General (Russia) (Venäjä)"@fi , "Генерал армии (Россия) (Россия)"@ru ;
	owl:subClass :Rank_Army_General_Russia ;
	foaf:name "Генерал армии"@ru .

:Rank_Army_General_Russia_Soviet_Union org:rankOf <dbpedia:Soviet_Union> ;
	a :MilitaryRank ;
	rdfs:comment "The specific instance of the Army General (Russia) rank in the context of country Soviet Union."@en ;
	rdfs:label "Army General (Russia) (Neuvostoliitto)"@fi , "Army General (Russia) (Soviet Union)"@en , "Army General (Russia) (Sovjet-Unie)"@nl , "Army General (Russia) (Sovjetunionen)"@no , "Army General (Russia) (Sovjetunionen)"@sv , "Army General (Russia) (Sowjetunion)"@de , "Army General (Russia) (Union des républiques socialistes soviétiques)"@fr , "Army General (Russia) (Unione Sovietica)"@it , "Army General (Russia) (União Soviética)"@pt , "Army General (Russia) (Unión Soviética)"@es , "Army General (Russia) (Związek Socjalistycznych Republik Radzieckich)"@pl , "Генерал армии (Россия) (Союз Советских Социалистических Республик)"@ru ;
	owl:subClass :Rank_Army_General_Russia ;
	foaf:name "Army General"@en .

:Rank_Aspirant a :MilitaryRank ;
	rdfs:comment "Aspirant is a military rank in the Canadian Navy, French military, Brazilian military, Romanian Navy and Polish Police."@en ;
	rdfs:label "Aspirant"@en ;
	owl:sameAs <dbpedia:Aspirant> ;
	foaf:name "Aspirant" .

:Rank_Aspirant_France org:rankOf <dbpedia:France> ;
	a :MilitaryRank ;
	rdfs:comment "The specific instance of the Aspirant rank in the context of France."@en ;
	rdfs:label "Aspirant (France)"@en ;
	owl:subClass :Rank_Aspirant ;
	foaf:name "Aspirant"@en .

:Rank_Aspirant_Romania org:rankOf <dbpedia:Romania> ;
	a :MilitaryRank ;
	rdfs:comment "The specific instance of the Aspirant rank in the context of country Romania."@en ;
	rdfs:label "Aspirant (Roemenië)"@nl , "Aspirant (Romania)"@en , "Aspirant (Romania)"@fi , "Aspirant (Romania)"@it , "Aspirant (Romania)"@no , "Aspirant (Roménia)"@pt , "Aspirant (Roumanie)"@fr , "Aspirant (Rumania)"@es , "Aspirant (Rumunia)"@pl , "Aspirant (Rumänien)"@de , "Aspirant (Rumänien)"@sv , "Aspirant (Румыния)"@ru ;
	owl:subClass :Rank_Aspirant ;
	foaf:name "Aspirant"@en .

:Rank_Aspirant_Romania_Romania org:rankOf <dbpedia:Romania> ;
	a :MilitaryRank ;
	rdfs:comment "The specific instance of the Aspirant (Romania) rank in the context of country Romania."@en ;
	rdfs:label "Aspirant (Romania) (Roemenië)"@nl , "Aspirant (Romania) (Romania)"@en , "Aspirant (Romania) (Romania)"@fi , "Aspirant (Romania) (Romania)"@it , "Aspirant (Romania) (Romania)"@no , "Aspirant (Romania) (Roménia)"@pt , "Aspirant (Romania) (Roumanie)"@fr , "Aspirant (Romania) (Rumania)"@es , "Aspirant (Romania) (Rumunia)"@pl , "Aspirant (Romania) (Rumänien)"@de , "Aspirant (Romania) (Rumänien)"@sv , "Aspirant (Romania) (Румыния)"@ru ;
	owl:subClass :Rank_Aspirant_Romania ;
	foaf:name "Aspirant"@en .

:Rank_Ataman a :MilitaryRank ;
	rdfs:comment "Ataman was a commander title of the Ukrainian People's Army, Cossack, and haidamak leaders, who were in essence the Cossacks. In the Russia Empire, the term was the official title of the supreme military commanders of the Cossack armies. It had a derogatory suggestion and was also used for the leader of a fisherman artel, a band of robbers or thieves, or leaders of the opposition forces."@en ;
	rdfs:label "Atamaani"@fi , "Ataman"@de , "Ataman"@en , "Ataman"@pl , "Ataman / Otaman"@fr , "Atamano"@it , "Atamán"@es , "Атаман"@ru ;
	owl:sameAs <dbpedia:Ataman> ;
	foaf:name "Ataman" .

:Rank_Ataman_Russia org:rankOf <dbpedia:Russia> ;
	a :MilitaryRank ;
	rdfs:comment "The specific instance of the Ataman rank in the context of country Russia."@en ;
	rdfs:label "Atamaani (Venäjä)"@fi , "Ataman (Rosja)"@pl , "Ataman (Rusland)"@nl , "Ataman (Russia)"@en , "Ataman (Russland)"@de , "Ataman (Russland)"@no , "Ataman (Ryssland)"@sv , "Ataman (Rússia)"@pt , "Ataman / Otaman (Russie)"@fr , "Atamano (Russia)"@it , "Atamán (Rusia)"@es , "Атаман (Россия)"@ru ;
	owl:subClass :Rank_Ataman ;
	foaf:name "Атаман"@ru .

:Rank_Ataman_Soviet_Union org:rankOf <dbpedia:Soviet_Union> ;
	a :MilitaryRank ;
	rdfs:comment "The specific instance of the Ataman rank in the context of country Soviet Union."@en ;
	rdfs:label "Atamaani (Neuvostoliitto)"@fi , "Ataman (Soviet Union)"@en , "Ataman (Sovjet-Unie)"@nl , "Ataman (Sovjetunionen)"@no , "Ataman (Sovjetunionen)"@sv , "Ataman (Sowjetunion)"@de , "Ataman (União Soviética)"@pt , "Ataman (Związek Socjalistycznych Republik Radzieckich)"@pl , "Ataman / Otaman (Union des républiques socialistes soviétiques)"@fr , "Atamano (Unione Sovietica)"@it , "Atamán (Unión Soviética)"@es , "Атаман (Союз Советских Социалистических Республик)"@ru ;
	owl:subClass :Rank_Ataman ;
	foaf:name "Ataman"@en .

:Rank_Ataman_Ukraine org:rankOf <dbpedia:Ukraine> ;
	a :MilitaryRank ;
	rdfs:comment "The specific instance of the Ataman rank in the context of country Ukraine."@en ;
	rdfs:label "Atamaani (Ukraina)"@fi , "Ataman (Oekraïne)"@nl , "Ataman (Ucrânia)"@pt , "Ataman (Ukraina)"@no , "Ataman (Ukraina)"@pl , "Ataman (Ukraina)"@sv , "Ataman (Ukraine)"@de , "Ataman (Ukraine)"@en , "Ataman / Otaman (Ukraine)"@fr , "Atamano (Ucraina)"@it , "Atamán (Ucrania)"@es , "Атаман (Украина)"@ru ;
	owl:subClass :Rank_Ataman ;
	foaf:name "Атаман"@ru .

:Rank_Battery_sergeant_major org:rankOf :Artillery ;
	a :MilitaryAppointment , :MilitaryRank ;
	rdfs:label "Battery Sergeant Major"@en ;
	foaf:name "Battery sergeant major" .

:Rank_Birinci_Ferik a :MilitaryRank ;
	rdfs:comment "Birinci Ferik or Ferik-i evvel was a military rank of the Ottoman Army. It is translated as Lieutenant General or General (Orgeneral). The title means \"first Ferik\" and was superior to a Ferik and junior only to the Müşir. The title of Birinci Ferik was abolished with Act No. 2590 of 26 November 1934 on the Abolition of Titles and Appellations such as Efendi, Bey or Pasha."@en ;
	rdfs:label "Birinci Ferik"@en ;
	owl:sameAs <dbpedia:Birinci_Ferik> ;
	foaf:name "Birinci Ferik" .

:Rank_Birinci_Ferik_Cossack_Hetmanate org:rankOf <dbpedia:Cossack_Hetmanate> ;
	a :MilitaryRank ;
	rdfs:comment "The specific instance of the Birinci Ferik rank in the context of country Cossack Hetmanate."@en ;
	rdfs:label "Birinci Ferik (Cossack Hetmanate)"@en , "Birinci Ferik (Hetmanat cosaque)"@fr , "Birinci Ferik (Hetmanat)"@de , "Birinci Ferik (Hetmanato cosaco)"@es , "Birinci Ferik (Hetmańszczyzna)"@pl , "Birinci Ferik (Гетманщина)"@ru ;
	owl:subClass :Rank_Birinci_Ferik ;
	foaf:name "Birinci Ferik"@en .

:Rank_Birinci_Ferik_Ottoman_Empire org:rankOf <dbpedia:Ottoman_Empire> ;
	a :MilitaryRank ;
	rdfs:comment "The specific instance of the Birinci Ferik rank in the context of country Ottoman Empire."@en ;
	rdfs:label "Birinci Ferik (Det osmanske rike)"@no , "Birinci Ferik (Empire ottoman)"@fr , "Birinci Ferik (Imperio otomano)"@es , "Birinci Ferik (Imperium osmańskie)"@pl , "Birinci Ferik (Impero ottomano)"@it , "Birinci Ferik (Império Otomano)"@pt , "Birinci Ferik (Osmanien valtakunta)"@fi , "Birinci Ferik (Osmanisches Reich)"@de , "Birinci Ferik (Osmanska riket)"@sv , "Birinci Ferik (Ottomaanse Rijk)"@nl , "Birinci Ferik (Ottoman Empire)"@en , "Birinci Ferik (Османская империя)"@ru ;
	owl:subClass :Rank_Birinci_Ferik ;
	foaf:name "Birinci Ferik"@en .

:Rank_Birinci_Ferik_Septinsular_Republic org:rankOf <dbpedia:Septinsular_Republic> ;
	a :MilitaryRank ;
	rdfs:comment "The specific instance of the Birinci Ferik rank in the context of country Septinsular Republic."@en ;
	rdfs:label "Birinci Ferik (Repubblica delle Sette Isole Unite)"@it , "Birinci Ferik (Republiek van de Zeven Eilanden)"@nl , "Birinci Ferik (Republika Siedmiu Wysp)"@pl , "Birinci Ferik (República de las Islas Jónicas)"@es , "Birinci Ferik (République des Sept-Îles)"@fr , "Birinci Ferik (Septinsular Republic)"@en , "Birinci Ferik (Республика Семи Островов)"@ru ;
	owl:subClass :Rank_Birinci_Ferik ;
	foaf:name "Birinci Ferik"@en .

:Rank_Bombardier a :MilitaryRank ;
	rdfs:comment "Bombardier is a rank used in artillery units in the armies of Commonwealth countries instead of corporal. Lance-bombardier is used instead of lance-corporal. Bombardier (Bdr) and lance-bombardier (LBdr or L/Bdr) are used by the British Army in the Royal Artillery and Royal Horse Artillery. The same applies to the Royal Australian Artillery, the Royal New Zealand Artillery, the South African Army Artillery and the Armed Forces of Malta (AFM)."@en ;
	rdfs:label "Bombardier (rank)"@en , "Bombardier (stopień)"@pl , "Бомбардир (воинское звание)"@ru ;
	owl:sameAs <dbpedia:Bombardier_%28rank%29> ;
	foaf:name "Bombardier" .

:Rank_Bombardier_Australia org:rankOf <dbpedia:Australia> ;
	a :MilitaryRank ;
	rdfs:comment "The specific instance of the Bombardier (rank) rank in the context of country Australia."@en ;
	rdfs:label "Bombardier (rank) (Australia)"@en , "Bombardier (rank) (Australia)"@es , "Bombardier (rank) (Australia)"@fi , "Bombardier (rank) (Australia)"@it , "Bombardier (rank) (Australia)"@no , "Bombardier (rank) (Australie)"@fr , "Bombardier (rank) (Australien)"@de , "Bombardier (rank) (Australien)"@sv , "Bombardier (rank) (Australië (land))"@nl , "Bombardier (rank) (Austrália)"@pt , "Bombardier (stopień) (Australia)"@pl , "Бомбардир (воинское звание) (Австралия)"@ru ;
	owl:subClass :Rank_Bombardier_%28rank%29 ;
	foaf:name "Bombardier"@en .

:Rank_Bombardier_Canada org:rankOf <dbpedia:Canada> ;
	a :MilitaryRank ;
	rdfs:comment "The specific instance of the Bombardier (rank) rank in the context of Canada."@en ;
	rdfs:label "Bombardier (rank, Canada)"@en , "Bombardier (stopień, Canada)"@pl , "Бомбардир (воинское звание, Canada)"@ru ;
	owl:subClass :Rank_Bombardier_%28rank%29 ;
	foaf:name "Bombardier"@en .

:Rank_Bombardier_Commonwealth_of_Nations org:rankOf <dbpedia:Commonwealth_of_Nations> ;
	a :MilitaryRank ;
	rdfs:comment "The specific instance of the Bombardier (rank) rank in the context of country Commonwealth of Nations."@en ;
	rdfs:label "Bombardier (rank) (Commonwealth delle nazioni)"@it , "Bombardier (rank) (Commonwealth of Nations)"@de , "Bombardier (rank) (Commonwealth of Nations)"@en , "Bombardier (rank) (Commonwealth of Nations)"@fr , "Bombardier (rank) (Commonwealth)"@pt , "Bombardier (rank) (Gemenebest van Naties)"@nl , "Bombardier (rank) (Kansainyhteisö)"@fi , "Bombardier (rank) (Mancomunidad de Naciones)"@es , "Bombardier (rank) (Samveldet av nasjoner)"@no , "Bombardier (rank) (Samväldet)"@sv , "Bombardier (stopień) (Wspólnota Narodów)"@pl , "Бомбардир (воинское звание) (Содружество наций)"@ru ;
	owl:subClass :Rank_Bombardier ;
	foaf:name "Bombardier"@en .

:Rank_Bootsmann a :MilitaryRank ;
	rdfs:comment "Bootsmann was a highest-ranking Petty Officer position in German naval forces. A lower-ranking Bootsmann was called Bootsmannsmaat. These names were adopted for the Russian Navy as боцман and боцманмат by Peter the Great, among many other Prussian and Holland military ranks; they were initially treated as positions rather than ranks. The army and air force equivalent is a Feldwebel. In the modern German Navy, Bootsmann is a senior NCO rank."@en ;
	rdfs:label "Bootsmann"@de , "Bootsmann"@en , "Боцман"@ru ;
	owl:sameAs <dbpedia:Bootsmann> ;
	foaf:name "Bootsmann" .

:Rank_Bootsmann_Germany org:rankOf <dbpedia:Germany> ;
	a :MilitaryRank ;
	rdfs:comment "The specific instance of the Bootsmann rank in the context of Germany."@en ;
	rdfs:label "Bootsmann (Germany)"@de , "Bootsmann (Germany)"@en , "Боцман (Germany)"@ru ;
	owl:subClass :Rank_Bootsmann ;
	foaf:name "Bootsmann"@de .

:Rank_Bootsmann_Russia org:rankOf <dbpedia:Russia> ;
	a :MilitaryRank ;
	rdfs:comment "The specific instance of the Bootsmann rank in the context of country Russia."@en ;
	rdfs:label "Bootsmann (Rosja)"@pl , "Bootsmann (Rusia)"@es , "Bootsmann (Rusland)"@nl , "Bootsmann (Russia)"@en , "Bootsmann (Russia)"@it , "Bootsmann (Russie)"@fr , "Bootsmann (Russland)"@de , "Bootsmann (Russland)"@no , "Bootsmann (Ryssland)"@sv , "Bootsmann (Rússia)"@pt , "Bootsmann (Venäjä)"@fi , "Боцман (Россия)"@ru ;
	owl:subClass :Rank_Bootsmann ;
	foaf:name "Боцман"@ru .

:Rank_Bootsmann_Soviet_Union org:rankOf <dbpedia:Soviet_Union> ;
	a :MilitaryRank ;
	rdfs:comment "The specific instance of the Bootsmann rank in the context of country Soviet Union."@en ;
	rdfs:label "Bootsmann (Neuvostoliitto)"@fi , "Bootsmann (Soviet Union)"@en , "Bootsmann (Sovjet-Unie)"@nl , "Bootsmann (Sovjetunionen)"@no , "Bootsmann (Sovjetunionen)"@sv , "Bootsmann (Sowjetunion)"@de , "Bootsmann (Union des républiques socialistes soviétiques)"@fr , "Bootsmann (Unione Sovietica)"@it , "Bootsmann (União Soviética)"@pt , "Bootsmann (Unión Soviética)"@es , "Bootsmann (Związek Socjalistycznych Republik Radzieckich)"@pl , "Боцман (Союз Советских Социалистических Республик)"@ru ;
	owl:subClass :Rank_Bootsmann ;
	foaf:name "Bootsmann"@en .

:Rank_Brigade_General a :MilitaryRank ;
	rdfs:label "Brigade General"@en ;
	owl:sameAs <dbpedia:Brigade_General> ;
	foaf:name "Brigade General" .

:Rank_Brigade_General_Australia org:rankOf <dbpedia:Australia> ;
	a :MilitaryRank ;
	rdfs:comment "The specific instance of the Brigade General rank in the context of country Australia."@en ;
	rdfs:label "Brigade General (Australia)"@en , "Brigade General (Australia)"@es , "Brigade General (Australia)"@fi , "Brigade General (Australia)"@it , "Brigade General (Australia)"@no , "Brigade General (Australia)"@pl , "Brigade General (Australie)"@fr , "Brigade General (Australien)"@de , "Brigade General (Australien)"@sv , "Brigade General (Australië (land))"@nl , "Brigade General (Austrália)"@pt , "Brigade General (Австралия)"@ru ;
	owl:subClass :Rank_Brigade_General ;
	foaf:name "Brigade General"@en .

:Rank_Brigade_General_Canada org:rankOf <dbpedia:Canada> ;
	a :MilitaryRank ;
	rdfs:comment "The specific instance of the Brigade General rank in the context of Canada."@en ;
	rdfs:label "Brigade General (Canada)"@en ;
	owl:subClass :Rank_Brigade_General ;
	foaf:name "Brigade General"@en .

:Rank_Brigadier_EnglishTradition org:rankEquivalentTo :Rank_Air_commodore_EnglishTradition , <http://rdf.muninn-project.org/ontologies/military#Rank_Commodore_(rank)_EnglishTradition> ;
	org:rankJuniorToTransitive :Rank_General_officer_EnglishTradition ;
	org:rankOf :EnglishTradition , <mil:ArmyServiceBranch> ;
	org:rankSeniorToTransitive :Rank_Colonel_EnglishTradition ;
	a :MilitaryRank ;
	rdfs:comment "Brigadier is a senior military rank, the meaning of which is somewhat different in different military services. The brigadier rank is generally superior to the rank of colonel, and subordinate to major general. A brigadier typically commands a brigade consisting of three battalions (approximately 3,000 troops). Many countries use the rank Brigadier General rather than Brigadier, and prior to the 1920s, so did members of the Commonwealth."@en ;
	rdfs:label "Brigadier"@de , "Brigadier"@en , "Brigadier"@fr ;
	owl:sameAs <dbpedia:Brigadier> .

:Rank_Brigadier_general a :MilitaryRank ;
	rdfs:label "Brigadier general"@en ;
	owl:sameAs <dbpedia:Brigadier_general> ;
	foaf:name "Brigadier general" .

:Rank_Brigadier_general_Australia org:rankOf <dbpedia:Australia> ;
	a :MilitaryRank ;
	rdfs:comment "The specific instance of the Brigadier general rank in the context of country Australia."@en ;
	rdfs:label "Brigadier general (Australia)"@en , "Brigadier general (Australia)"@es , "Brigadier general (Australia)"@fi , "Brigadier general (Australia)"@it , "Brigadier general (Australia)"@no , "Brigadier general (Australia)"@pl , "Brigadier general (Australie)"@fr , "Brigadier general (Australien)"@de , "Brigadier general (Australien)"@sv , "Brigadier general (Australië (land))"@nl , "Brigadier general (Austrália)"@pt , "Brigadier general (Австралия)"@ru ;
	owl:subClass :Rank_Brigadier_general ;
	foaf:name "Brigadier general"@en .

:Rank_Brigadier_general_Canada org:rankOf <dbpedia:Canada> ;
	a :MilitaryRank ;
	rdfs:comment "The specific instance of the Brigadier general rank in the context of Canada."@en ;
	rdfs:label "Brigadier general (Canada)"@en ;
	owl:subClass :Rank_Brigadier_general ;
	foaf:name "Brigadier general"@en .

:Rank_Captain a :MilitaryRank ;
	rdfs:comment "The army rank of captain (from the French capitaine) is a commissioned officer rank historically corresponding to command of a company of soldiers. The rank is also used by some air forces and marine forces. Today a captain is typically either the commander or second-in-command of a company or artillery battery. In the Chinese People's Liberation Army, a captain may also command a platoon, or be the second-in-command of a battalion. Captain is one rank above a lieutenant and one below a major."@en ;
	rdfs:label "Capitaine"@fr , "Capitano"@it , "Capitán"@es , "Capitão (militar)"@pt , "Captain (OF-2)"@en , "Hauptmann (Offizier)"@de , "Kapitan (ranga)"@pl , "Kapitein (rang)"@nl , "Kapteeni (sotilasarvo)"@fi , "Kaptein (grad)"@no , "Kapten"@sv , "Капитан (воинское звание)"@ru ;
	owl:sameAs <dbpedia:Captain_%28OF-2%29> ;
	foaf:name "Captain" .

<http://rdf.muninn-project.org/ontologies/military#Rank_Captain_(naval)_EnglishTradition> org:rankEquivalentTo :Rank_Colonel_EnglishTradition , :Rank_Group_captain_EnglishTradition ;
	org:rankJuniorToTransitive <http://rdf.muninn-project.org/ontologies/military#Rank_Commodore_(rank)_EnglishTradition> ;
	org:rankOf :EnglishTradition , <mil:NavyServiceBranch> ;
	org:rankSeniorToTransitive :Rank_Commander_EnglishTradition ;
	a :MilitaryRank ;
	owl:sameAs <dbpedia:Captain_(naval)> .

:Rank_Captain_Australia org:rankOf <dbpedia:Australia> ;
	a :MilitaryRank ;
	rdfs:comment "The specific instance of the Captain (OF-2) rank in the context of country Australia."@en ;
	rdfs:label "Capitaine (Australie)"@fr , "Capitano (Australia)"@it , "Capitán (Australia)"@es , "Capitão (militar) (Austrália)"@pt , "Captain (OF-2) (Australia)"@en , "Hauptmann (Offizier) (Australien)"@de , "Kapitan (ranga) (Australia)"@pl , "Kapitein (rang) (Australië (land))"@nl , "Kapteeni (sotilasarvo) (Australia)"@fi , "Kaptein (grad) (Australia)"@no , "Kapten (Australien)"@sv , "Капитан (воинское звание) (Австралия)"@ru ;
	owl:subClass :Rank_Captain ;
	foaf:name "Captain"@en .

:Rank_Captain_Canada org:rankOf <dbpedia:Canada> ;
	a :MilitaryRank ;
	rdfs:comment "The specific instance of the Captain (OF-2) rank in the context of Canada."@en ;
	rdfs:label "Capitaine (Canada)"@fr , "Capitano (Canada)"@it , "Capitán (Canada)"@es , "Capitão (militar, Canada)"@pt , "Captain (OF-2, Canada)"@en , "Hauptmann (Offizier, Canada)"@de , "Kapitan (ranga, Canada)"@pl , "Kapitein (rang, Canada)"@nl , "Kapteeni (sotilasarvo, Canada)"@fi , "Kaptein (grad, Canada)"@no , "Kapten (Canada)"@sv , "Капитан (воинское звание, Canada)"@ru ;
	owl:subClass :Rank_Captain ;
	foaf:name "Capitaine"@fr .

:Rank_Captain_EnglishTradition org:rankEquivalentTo :Rank_Flight_lieutenant_EnglishTradition , <http://rdf.muninn-project.org/ontologies/military#Rank_Lieutenant_(navy)_EnglishTradition> ;
	org:rankJuniorToTransitive <http://rdf.muninn-project.org/ontologies/military#Rank_Commandant_(rank)_EnglishTradition> ;
	org:rankOf :EnglishTradition , <mil:ArmyServiceBranch> ;
	org:rankSeniorToTransitive :Rank_Lieutenant_EnglishTradition ;
	a :MilitaryRank ;
	owl:sameAs <dbpedia:Captain_(OF-2)> ;
	owl:subClass :NatoRankOF-2 .

:Rank_Captain_Lieutenant a :MilitaryRank ;
	rdfs:comment "Captain Lieutenant or Captain-Lieutenant is a military rank, used in a number of different navies worldwide. It is generally equivalent to the Commonwealth or US rank of Lieutenant, and has the NATO rank code of OF-2, though this can vary."@en ;
	rdfs:label "Capitaine-lieutenant"@fr , "Captain Lieutenant"@en , "Kapitänleutnant"@de , "Kapteeniluutnantti"@fi , "Kapteinløytnant"@no , "Kaptenlöjtnant"@sv , "Капитан-лейтенант"@ru ;
	owl:sameAs <dbpedia:Captain_Lieutenant> ;
	foaf:name "Captain Lieutenant" .

:Rank_Captain_Lieutenant_Germany org:rankOf <dbpedia:Germany> ;
	a :MilitaryRank ;
	rdfs:comment "The specific instance of the Captain Lieutenant rank in the context of Germany."@en ;
	rdfs:label "Capitaine-lieutenant (Germany)"@fr , "Captain Lieutenant (Germany)"@en , "Kapitänleutnant (Germany)"@de , "Kapteeniluutnantti (Germany)"@fi , "Kapteinløytnant (Germany)"@no , "Kaptenlöjtnant (Germany)"@sv , "Капитан-лейтенант (Germany)"@ru ;
	owl:subClass :Rank_Captain_Lieutenant ;
	foaf:name "Kapitänleutnant"@de .

:Rank_Captain_Lieutenant_Russia org:rankOf <dbpedia:Russia> ;
	a :MilitaryRank ;
	rdfs:comment "The specific instance of the Captain Lieutenant rank in the context of country Russia."@en ;
	rdfs:label "Capitaine-lieutenant (Russie)"@fr , "Captain Lieutenant (Rosja)"@pl , "Captain Lieutenant (Rusia)"@es , "Captain Lieutenant (Rusland)"@nl , "Captain Lieutenant (Russia)"@en , "Captain Lieutenant (Russia)"@it , "Captain Lieutenant (Rússia)"@pt , "Kapitänleutnant (Russland)"@de , "Kapteeniluutnantti (Venäjä)"@fi , "Kapteinløytnant (Russland)"@no , "Kaptenlöjtnant (Ryssland)"@sv , "Капитан-лейтенант (Россия)"@ru ;
	owl:subClass :Rank_Captain_Lieutenant ;
	foaf:name "Капитан-лейтенант"@ru .

:Rank_Captain_Lieutenant_Soviet_Union org:rankOf <dbpedia:Soviet_Union> ;
	a :MilitaryRank ;
	rdfs:comment "The specific instance of the Captain Lieutenant rank in the context of country Soviet Union."@en ;
	rdfs:label "Capitaine-lieutenant (Union des républiques socialistes soviétiques)"@fr , "Captain Lieutenant (Soviet Union)"@en , "Captain Lieutenant (Sovjet-Unie)"@nl , "Captain Lieutenant (Unione Sovietica)"@it , "Captain Lieutenant (União Soviética)"@pt , "Captain Lieutenant (Unión Soviética)"@es , "Captain Lieutenant (Związek Socjalistycznych Republik Radzieckich)"@pl , "Kapitänleutnant (Sowjetunion)"@de , "Kapteeniluutnantti (Neuvostoliitto)"@fi , "Kapteinløytnant (Sovjetunionen)"@no , "Kaptenlöjtnant (Sovjetunionen)"@sv , "Капитан-лейтенант (Союз Советских Социалистических Республик)"@ru ;
	owl:subClass :Rank_Captain_Lieutenant ;
	foaf:name "Captain Lieutenant"@en .

:Rank_Captain_Republic_of_Ireland org:rankOf <dbpedia:Republic_of_Ireland> ;
	a :MilitaryRank ;
	rdfs:comment "The specific instance of the Captain (OF-2) rank in the context of country Republic of Ireland."@en ;
	rdfs:label "Capitaine (Irlande (pays))"@fr , "Capitano (Irlanda)"@it , "Capitán (Irlanda)"@es , "Capitão (militar) (República da Irlanda)"@pt , "Captain (OF-2) (Republic of Ireland)"@en , "Hauptmann (Offizier) (Irland)"@de , "Kapitan (ranga) (Irlandia)"@pl , "Kapitein (rang) (Ierland (land))"@nl , "Kapteeni (sotilasarvo) (Irlanti)"@fi , "Kaptein (grad) (Irland)"@no , "Kapten (Irland)"@sv , "Капитан (воинское звание) (Ирландия)"@ru ;
	owl:subClass :Rank_Captain ;
	foaf:name "Captain"@en .

:Rank_Captain_Russia org:rankOf <dbpedia:Russia> ;
	a :MilitaryRank ;
	rdfs:comment "The specific instance of the Captain (OF-2) rank in the context of country Russia."@en ;
	rdfs:label "Capitaine (Russie)"@fr , "Capitano (Russia)"@it , "Capitán (Rusia)"@es , "Capitão (militar) (Rússia)"@pt , "Captain (OF-2) (Russia)"@en , "Hauptmann (Offizier) (Russland)"@de , "Kapitan (ranga) (Rosja)"@pl , "Kapitein (rang) (Rusland)"@nl , "Kapteeni (sotilasarvo) (Venäjä)"@fi , "Kaptein (grad) (Russland)"@no , "Kapten (Ryssland)"@sv , "Капитан (воинское звание) (Россия)"@ru ;
	owl:subClass :Rank_Captain ;
	foaf:name "Капитан"@ru .

:Rank_Captain_Singapore org:rankOf <dbpedia:Singapore> ;
	a :MilitaryRank ;
	rdfs:comment "The specific instance of the Captain (OF-2) rank in the context of country Singapore."@en ;
	rdfs:label "Capitaine (Singapour)"@fr , "Capitano (Singapore)"@it , "Capitán (Singapur)"@es , "Capitão (militar) (Singapura)"@pt , "Captain (OF-2) (Singapore)"@en , "Hauptmann (Offizier) (Singapur)"@de , "Kapitan (ranga) (Singapur)"@pl , "Kapitein (rang) (Singapore)"@nl , "Kapteeni (sotilasarvo) (Singapore)"@fi , "Kaptein (grad) (Singapore)"@no , "Kapten (Singapore)"@sv , "Капитан (воинское звание) (Сингапур)"@ru ;
	owl:subClass :Rank_Captain ;
	foaf:name "Captain"@en .

:Rank_Captain_Soviet_Union org:rankOf <dbpedia:Soviet_Union> ;
	a :MilitaryRank ;
	rdfs:comment "The specific instance of the Captain (OF-2) rank in the context of country Soviet Union."@en ;
	rdfs:label "Capitaine (Union des républiques socialistes soviétiques)"@fr , "Capitano (Unione Sovietica)"@it , "Capitán (Unión Soviética)"@es , "Capitão (militar) (União Soviética)"@pt , "Captain (OF-2) (Soviet Union)"@en , "Hauptmann (Offizier) (Sowjetunion)"@de , "Kapitan (ranga) (Związek Socjalistycznych Republik Radzieckich)"@pl , "Kapitein (rang) (Sovjet-Unie)"@nl , "Kapteeni (sotilasarvo) (Neuvostoliitto)"@fi , "Kaptein (grad) (Sovjetunionen)"@no , "Kapten (Sovjetunionen)"@sv , "Капитан (воинское звание) (Союз Советских Социалистических Республик)"@ru ;
	owl:subClass :Rank_Captain ;
	foaf:name "Captain"@en .

:Rank_Captain_Sweden org:rankOf <dbpedia:Sweden> ;
	a :MilitaryRank ;
	rdfs:comment "The specific instance of the Captain (OF-2) rank in the context of country Sweden."@en ;
	rdfs:label "Capitaine (Suède)"@fr , "Capitano (Svezia)"@it , "Capitán (Suecia)"@es , "Capitão (militar) (Suécia)"@pt , "Captain (OF-2) (Sweden)"@en , "Hauptmann (Offizier) (Schweden)"@de , "Kapitan (ranga) (Szwecja)"@pl , "Kapitein (rang) (Zweden)"@nl , "Kapteeni (sotilasarvo) (Ruotsi)"@fi , "Kaptein (grad) (Sverige)"@no , "Kapten (Sverige)"@sv , "Капитан (воинское звание) (Швеция)"@ru ;
	owl:subClass :Rank_Captain ;
	foaf:name "Kapten"@sv .

:Rank_Captain_lieutenant a :MilitaryRank ;
	rdfs:label "Captain lieutenant"@en ;
	owl:sameAs <dbpedia:Captain_lieutenant> ;
	foaf:name "Captain lieutenant" .

:Rank_Captain_lieutenant_Germany org:rankOf <dbpedia:Germany> ;
	a :MilitaryRank ;
	rdfs:comment "The specific instance of the Captain lieutenant rank in the context of Germany."@en ;
	rdfs:label "Captain lieutenant (Germany)"@en ;
	owl:subClass :Rank_Captain_lieutenant ;
	foaf:name "Captain lieutenant"@en .

:Rank_Captain_lieutenant_Russia org:rankOf <dbpedia:Russia> ;
	a :MilitaryRank ;
	rdfs:comment "The specific instance of the Captain lieutenant rank in the context of country Russia."@en ;
	rdfs:label "Captain lieutenant (Rosja)"@pl , "Captain lieutenant (Rusia)"@es , "Captain lieutenant (Rusland)"@nl , "Captain lieutenant (Russia)"@en , "Captain lieutenant (Russia)"@it , "Captain lieutenant (Russie)"@fr , "Captain lieutenant (Russland)"@de , "Captain lieutenant (Russland)"@no , "Captain lieutenant (Ryssland)"@sv , "Captain lieutenant (Rússia)"@pt , "Captain lieutenant (Venäjä)"@fi , "Captain lieutenant (Россия)"@ru ;
	owl:subClass :Rank_Captain_lieutenant ;
	foaf:name "Captain lieutenant"@en .

:Rank_Captain_lieutenant_Soviet_Union org:rankOf <dbpedia:Soviet_Union> ;
	a :MilitaryRank ;
	rdfs:comment "The specific instance of the Captain lieutenant rank in the context of country Soviet Union."@en ;
	rdfs:label "Captain lieutenant (Neuvostoliitto)"@fi , "Captain lieutenant (Soviet Union)"@en , "Captain lieutenant (Sovjet-Unie)"@nl , "Captain lieutenant (Sovjetunionen)"@no , "Captain lieutenant (Sovjetunionen)"@sv , "Captain lieutenant (Sowjetunion)"@de , "Captain lieutenant (Union des républiques socialistes soviétiques)"@fr , "Captain lieutenant (Unione Sovietica)"@it , "Captain lieutenant (União Soviética)"@pt , "Captain lieutenant (Unión Soviética)"@es , "Captain lieutenant (Związek Socjalistycznych Republik Radzieckich)"@pl , "Captain lieutenant (Союз Советских Социалистических Республик)"@ru ;
	owl:subClass :Rank_Captain_lieutenant ;
	foaf:name "Captain lieutenant"@en .

:Rank_Chief_Marshal a :MilitaryRank ;
	rdfs:comment "The ranks of Marshal of a branch and Chief Marshal of a branch were senior military ranks of the Soviet Armed Forces. Immediately above the rank \"Marshal of a branch\" is the rank \"Chief Marshal of a branch\". Both ranks are immediately above the rank \"Colonel General\" and equal to Soviet General of the Army. The ranks were created as an analog to Air Marshal and Air Chief Marshal, though they weren't used just in the Soviet Air Force but also in the several Soviet Army's branch commands."@en ;
	rdfs:label "Chief Marshal"@en , "Главный маршал рода войск"@ru ;
	owl:sameAs <dbpedia:Chief_Marshal> ;
	foaf:name "Chief Marshal" .

:Rank_Chief_Marshal_Russia org:rankOf <dbpedia:Russia> ;
	a :MilitaryRank ;
	rdfs:comment "The specific instance of the Chief Marshal rank in the context of country Russia."@en ;
	rdfs:label "Chief Marshal (Rosja)"@pl , "Chief Marshal (Rusia)"@es , "Chief Marshal (Rusland)"@nl , "Chief Marshal (Russia)"@en , "Chief Marshal (Russia)"@it , "Chief Marshal (Russie)"@fr , "Chief Marshal (Russland)"@de , "Chief Marshal (Russland)"@no , "Chief Marshal (Ryssland)"@sv , "Chief Marshal (Rússia)"@pt , "Chief Marshal (Venäjä)"@fi , "Главный маршал рода войск (Россия)"@ru ;
	owl:subClass :Rank_Chief_Marshal ;
	foaf:name "Главный маршал рода войск"@ru .

:Rank_Chief_Marshal_Soviet_Union org:rankOf <dbpedia:Soviet_Union> ;
	a :MilitaryRank ;
	rdfs:comment "The specific instance of the Chief Marshal rank in the context of country Soviet Union."@en ;
	rdfs:label "Chief Marshal (Neuvostoliitto)"@fi , "Chief Marshal (Soviet Union)"@en , "Chief Marshal (Sovjet-Unie)"@nl , "Chief Marshal (Sovjetunionen)"@no , "Chief Marshal (Sovjetunionen)"@sv , "Chief Marshal (Sowjetunion)"@de , "Chief Marshal (Union des républiques socialistes soviétiques)"@fr , "Chief Marshal (Unione Sovietica)"@it , "Chief Marshal (União Soviética)"@pt , "Chief Marshal (Unión Soviética)"@es , "Chief Marshal (Związek Socjalistycznych Republik Radzieckich)"@pl , "Главный маршал рода войск (Союз Советских Социалистических Республик)"@ru ;
	owl:subClass :Rank_Chief_Marshal ;
	foaf:name "Chief Marshal"@en .

:Rank_Chief_petty_officer a :MilitaryRank ;
	rdfs:label "Chief petty officer"@en ;
	owl:sameAs <dbpedia:Chief_petty_officer> ;
	foaf:name "Chief petty officer" .

<http://rdf.muninn-project.org/ontologies/military#Rank_Chief_petty_officer,_1st_class_Canada> org:rankOf <dbpedia:Canada> ;
	a :MilitaryRank ;
	rdfs:comment "The specific instance of the  rank in the context of Canada."@en ;
	rdfs:label " Chief petty officer, 1st Class (Canada)"@en ;
	owl:subClass <http://rdf.muninn-project.org/ontologies/military#Rank_Chief_petty_officer,_1st_class> ;
	foaf:name "Chief petty officer, 1st Class"@en .

<http://rdf.muninn-project.org/ontologies/military#Rank_Chief_petty_officer,_2nd_class_Canada> org:rankOf <dbpedia:Canada> ;
	a :MilitaryRank ;
	rdfs:comment "The specific instance of the  rank in the context of Canada."@en ;
	rdfs:label " Chief petty officer, 2nd Class (Canada)"@en ;
	owl:subClass <http://rdf.muninn-project.org/ontologies/military#Rank_Chief_petty_officer,_2nd_class> ;
	foaf:name "Chief petty officer, 2nd Class"@en .

:Rank_Chief_petty_officer_Australia org:rankOf <dbpedia:Australia> ;
	a :MilitaryRank ;
	rdfs:comment "The specific instance of the Chief petty officer rank in the context of country Australia."@en ;
	rdfs:label "Chief petty officer (Australia)"@en , "Chief petty officer (Australia)"@es , "Chief petty officer (Australia)"@fi , "Chief petty officer (Australia)"@it , "Chief petty officer (Australia)"@no , "Chief petty officer (Australia)"@pl , "Chief petty officer (Australie)"@fr , "Chief petty officer (Australien)"@de , "Chief petty officer (Australien)"@sv , "Chief petty officer (Australië (land))"@nl , "Chief petty officer (Austrália)"@pt , "Chief petty officer (Австралия)"@ru ;
	owl:subClass :Rank_Chief_petty_officer ;
	foaf:name "Chief petty officer"@en .

:Rank_Chief_petty_officer_Canada org:rankOf <dbpedia:Canada> ;
	a :MilitaryRank ;
	rdfs:comment "The specific instance of the Chief petty officer rank in the context of Canada."@en ;
	rdfs:label "Chief petty officer (Canada)"@en ;
	owl:subClass :Rank_Chief_petty_officer ;
	foaf:name "Chief petty officer"@en .

:Rank_Chief_petty_officer_Commonwealth_of_Nations org:rankOf <dbpedia:Commonwealth_of_Nations> ;
	a :MilitaryRank ;
	rdfs:comment "The specific instance of the Chief petty officer rank in the context of country Commonwealth of Nations."@en ;
	rdfs:label "Chief petty officer (Commonwealth delle nazioni)"@it , "Chief petty officer (Commonwealth of Nations)"@de , "Chief petty officer (Commonwealth of Nations)"@en , "Chief petty officer (Commonwealth of Nations)"@fr , "Chief petty officer (Commonwealth)"@pt , "Chief petty officer (Gemenebest van Naties)"@nl , "Chief petty officer (Kansainyhteisö)"@fi , "Chief petty officer (Mancomunidad de Naciones)"@es , "Chief petty officer (Samveldet av nasjoner)"@no , "Chief petty officer (Samväldet)"@sv , "Chief petty officer (Wspólnota Narodów)"@pl , "Chief petty officer (Содружество наций)"@ru ;
	owl:subClass :Rank_Chief_petty_officer ;
	foaf:name "Chief petty officer"@en .

:Rank_Chiliarch a :MilitaryRank ;
	rdfs:comment "Chiliarch, in the Greek army of the Hellenistic period, was a commander of a 1,000 men unit, roughly equivalent to a modern battalion. The office was an adaptation by Alexander the Great of the Persian Achaemenid empire's hazarapatish. A chiliarch held duties both martial and civil. Alexander the Great first awarded this rank to Hephaestion Amyntoros, but after Hephaestion's death it was awarded to Perdiccas."@en ;
	rdfs:label "Chiliarca"@it , "Chiliarch"@de , "Chiliarch"@en , "Chiliarcha"@pl , "Chiliarque"@fr , "Quiliarca"@es ;
	owl:sameAs <dbpedia:Chiliarch> ;
	foaf:name "Chiliarch" .

:Rank_Chiliarch_Achaean_League org:rankOf <dbpedia:Achaean_League> ;
	a :MilitaryRank ;
	rdfs:comment "The specific instance of the Chiliarch rank in the context of country Achaean League."@en ;
	rdfs:label "Chiliarca (Lega achea)"@it , "Chiliarch (Achaean League)"@en , "Chiliarch (Achaeïsche Bond)"@nl , "Chiliarch (Achaiischer Bund)"@de , "Chiliarch (Achaiska förbundet)"@sv , "Chiliarch (Akhaian liitto)"@fi , "Chiliarch (Det akhaiske forbund)"@no , "Chiliarch (Liga Aqueia)"@pt , "Chiliarch (Ахейский союз)"@ru , "Chiliarcha (Związek Achajski)"@pl , "Chiliarque (Ligue achéenne)"@fr , "Quiliarca (Liga Aquea)"@es ;
	owl:subClass :Rank_Chiliarch ;
	foaf:name "Chiliarch"@en .

:Rank_Chiliarch_Byzantine_Empire org:rankOf <dbpedia:Byzantine_Empire> ;
	a :MilitaryRank ;
	rdfs:comment "The specific instance of the Chiliarch rank in the context of country Byzantine Empire."@en ;
	rdfs:label "Chiliarca (Impero bizantino)"@it , "Chiliarch (Bysantin valtakunta)"@fi , "Chiliarch (Bysantinska riket)"@sv , "Chiliarch (Byzantijnse Rijk)"@nl , "Chiliarch (Byzantine Empire)"@en , "Chiliarch (Byzantinisches Reich)"@de , "Chiliarch (Império Bizantino)"@pt , "Chiliarch (Østromerriket)"@no , "Chiliarch (Византийская империя)"@ru , "Chiliarcha (Cesarstwo Bizantyńskie)"@pl , "Chiliarque (Empire byzantin)"@fr , "Quiliarca (Imperio bizantino)"@es ;
	owl:subClass :Rank_Chiliarch ;
	foaf:name "Chiliarch"@en .

:Rank_Chiliarch_Greece org:rankOf <dbpedia:Greece> ;
	a :MilitaryRank ;
	rdfs:comment "The specific instance of the Chiliarch rank in the context of country Greece."@en ;
	rdfs:label "Chiliarca (Grecia)"@it , "Chiliarch (Greece)"@en , "Chiliarch (Grekland)"@sv , "Chiliarch (Griechenland)"@de , "Chiliarch (Griekenland)"@nl , "Chiliarch (Grécia)"@pt , "Chiliarch (Hellas)"@no , "Chiliarch (Kreikka)"@fi , "Chiliarch (Греция)"@ru , "Chiliarcha (Grecja)"@pl , "Chiliarque (Grèce)"@fr , "Quiliarca (Grecia)"@es ;
	owl:subClass :Rank_Chiliarch ;
	foaf:name "Chiliarch"@en .

:Rank_Chiliarch_Macedonia org:rankOf <dbpedia:Macedonia_%28ancient_kingdom%29> ;
	a :MilitaryRank ;
	rdfs:comment "The specific instance of the Chiliarch rank in the context of country Macedonia (ancient kingdom)."@en ;
	rdfs:label "Chiliarca (Regno di Macedonia)"@it , "Chiliarch (Macedonia (ancient kingdom))"@de , "Chiliarch (Macedonia (ancient kingdom))"@en , "Chiliarch (Macedonië (oudheid))"@nl , "Chiliarch (Macedónia Antiga)"@pt , "Chiliarch (Makedonian valtakunta)"@fi , "Chiliarch (Oldtidens Makedonia)"@no , "Chiliarch (Древняя Македония)"@ru , "Chiliarcha (Starożytna Macedonia)"@pl , "Chiliarque (Royaume de Macédoine)"@fr , "Quiliarca (Reino de Macedonia)"@es ;
	owl:subClass :Rank_Chiliarch ;
	foaf:name "Chiliarch"@en .

:Rank_Chiliarch_Official_Timocracy_of_Sapinetia org:rankOf <dbpedia:Official_Timocracy_of_Sapinetia> ;
	a :MilitaryRank ;
	rdfs:comment "The specific instance of the Chiliarch rank in the context of the Timocracy of Sapinetia."@en ;
	rdfs:label "Chiliarca (Timocracy of Sapinetia)"@it , "Chiliarch (Timocracy of Sapinetia)"@de , "Chiliarch (Timocracy of Sapinetia)"@en , "Chiliarcha (Timocracy of Sapinetia)"@pl , "Chiliarque (Timocracy of Sapinetia)"@fr , "Quiliarca (Timocracy of Sapinetia)"@es ;
	owl:subClass :Rank_Chiliarch ;
	foaf:name "Chiliarch"@en .

:Rank_Chorbaji a :MilitaryRank ;
	rdfs:comment "Çorbacı (sometimes variously transliterated as chorbaji, chorbadzhi, tschorbadji) was a military rank of the corps of Janissaries in the Ottoman Empire, used for the commander of an orta, i.e. , approximately corresponding to the rank of colonel. The word is pronounced tʃoɾbaˈdʒɯ in Turkish and literally means \"soup server\", derived from çorba, \"soup\". However, this word could be connected to an old Turkic word korbashi (head of the unit/campfire)."@en ;
	rdfs:label "Çorbacı"@en , "Чорбаджи"@ru ;
	owl:sameAs <dbpedia:%C3%87orbac%C4%B1> ;
	foaf:name "Çorbacı" .

:Rank_Chorbaji_Cossack_Hetmanate org:rankOf <dbpedia:Cossack_Hetmanate> ;
	a :MilitaryRank ;
	rdfs:comment "The specific instance of the Çorbacı rank in the context of country Cossack Hetmanate."@en ;
	rdfs:label "Çorbacı (Cossack Hetmanate)"@en , "Çorbacı (Hetmanat cosaque)"@fr , "Çorbacı (Hetmanat)"@de , "Çorbacı (Hetmanato cosaco)"@es , "Çorbacı (Hetmańszczyzna)"@pl , "Чорбаджи (Гетманщина)"@ru ;
	owl:subClass :Rank_Chorbaji ;
	foaf:name "Çorbacı"@en .

:Rank_Chorbaji_Ottoman_Empire org:rankOf <dbpedia:Ottoman_Empire> ;
	a :MilitaryRank ;
	rdfs:comment "The specific instance of the Çorbacı rank in the context of country Ottoman Empire."@en ;
	rdfs:label "Çorbacı (Det osmanske rike)"@no , "Çorbacı (Empire ottoman)"@fr , "Çorbacı (Imperio otomano)"@es , "Çorbacı (Imperium osmańskie)"@pl , "Çorbacı (Impero ottomano)"@it , "Çorbacı (Império Otomano)"@pt , "Çorbacı (Osmanien valtakunta)"@fi , "Çorbacı (Osmanisches Reich)"@de , "Çorbacı (Osmanska riket)"@sv , "Çorbacı (Ottomaanse Rijk)"@nl , "Çorbacı (Ottoman Empire)"@en , "Чорбаджи (Османская империя)"@ru ;
	owl:subClass :Rank_Chorbaji ;
	foaf:name "Çorbacı"@en .

:Rank_Chorbaji_Septinsular_Republic org:rankOf <dbpedia:Septinsular_Republic> ;
	a :MilitaryRank ;
	rdfs:comment "The specific instance of the Çorbacı rank in the context of country Septinsular Republic."@en ;
	rdfs:label "Çorbacı (Repubblica delle Sette Isole Unite)"@it , "Çorbacı (Republiek van de Zeven Eilanden)"@nl , "Çorbacı (Republika Siedmiu Wysp)"@pl , "Çorbacı (República de las Islas Jónicas)"@es , "Çorbacı (République des Sept-Îles)"@fr , "Çorbacı (Septinsular Republic)"@en , "Чорбаджи (Республика Семи Островов)"@ru ;
	owl:subClass :Rank_Chorbaji ;
	foaf:name "Çorbacı"@en .

:Rank_Chowqzy a :MilitaryRank ;
	rdfs:comment "Chorąży is a military rank in Poland and neighboring countries. A chorąży was once a knight who bore a standard — the emblem of an armed troop, a province, a land, a duchy, or the kingdom. This function later evolved into a non-hereditary noble title."@en ;
	rdfs:label "Chorąży"@en , "Chorąży"@pl , "Хорунжий"@ru ;
	owl:sameAs <dbpedia:Chor%C4%85%C5%BCy> ;
	foaf:name "Chorąży" .

:Rank_Chowqzy_Poland org:rankOf <dbpedia:Poland> ;
	a :MilitaryRank ;
	rdfs:comment "The specific instance of the Chorąży rank in the context of Poland."@en ;
	rdfs:label "Chorąży (Poland)"@en , "Chorąży (Poland)"@pl , "Хорунжий (Poland)"@ru ;
	owl:subClass :Rank_Chowqzy ;
	foaf:name "Chorąży"@en .

:Rank_Chowqzy_Russia org:rankOf <dbpedia:Russia> ;
	a :MilitaryRank ;
	rdfs:comment "The specific instance of the Chorąży rank in the context of country Russia."@en ;
	rdfs:label "Chorąży (Rosja)"@pl , "Chorąży (Rusia)"@es , "Chorąży (Rusland)"@nl , "Chorąży (Russia)"@en , "Chorąży (Russia)"@it , "Chorąży (Russie)"@fr , "Chorąży (Russland)"@de , "Chorąży (Russland)"@no , "Chorąży (Ryssland)"@sv , "Chorąży (Rússia)"@pt , "Chorąży (Venäjä)"@fi , "Хорунжий (Россия)"@ru ;
	owl:subClass :Rank_Chowqzy ;
	foaf:name "Хорунжий"@ru .

:Rank_Chowqzy_Soviet_Union org:rankOf <dbpedia:Soviet_Union> ;
	a :MilitaryRank ;
	rdfs:comment "The specific instance of the Chorąży rank in the context of country Soviet Union."@en ;
	rdfs:label "Chorąży (Neuvostoliitto)"@fi , "Chorąży (Soviet Union)"@en , "Chorąży (Sovjet-Unie)"@nl , "Chorąży (Sovjetunionen)"@no , "Chorąży (Sovjetunionen)"@sv , "Chorąży (Sowjetunion)"@de , "Chorąży (Union des républiques socialistes soviétiques)"@fr , "Chorąży (Unione Sovietica)"@it , "Chorąży (União Soviética)"@pt , "Chorąży (Unión Soviética)"@es , "Chorąży (Związek Socjalistycznych Republik Radzieckich)"@pl , "Хорунжий (Союз Советских Социалистических Республик)"@ru ;
	owl:subClass :Rank_Chowqzy ;
	foaf:name "Chorąży"@en .

:Rank_Chowqzy_Ukraine org:rankOf <dbpedia:Ukraine> ;
	a :MilitaryRank ;
	rdfs:comment "The specific instance of the Chorąży rank in the context of country Ukraine."@en ;
	rdfs:label "Chorąży (Oekraïne)"@nl , "Chorąży (Ucraina)"@it , "Chorąży (Ucrania)"@es , "Chorąży (Ucrânia)"@pt , "Chorąży (Ukraina)"@fi , "Chorąży (Ukraina)"@no , "Chorąży (Ukraina)"@pl , "Chorąży (Ukraina)"@sv , "Chorąży (Ukraine)"@de , "Chorąży (Ukraine)"@en , "Chorąży (Ukraine)"@fr , "Хорунжий (Украина)"@ru ;
	owl:subClass :Rank_Chowqzy ;
	foaf:name "Хорунжий"@ru .

:Rank_Colonel_EnglishTradition org:rankEquivalentTo <http://rdf.muninn-project.org/ontologies/military#Rank_Captain_(naval)_EnglishTradition> , :Rank_Group_captain_EnglishTradition ;
	org:rankJuniorToTransitive :Rank_Brigadier_EnglishTradition ;
	org:rankOf :EnglishTradition , <mil:ArmyServiceBranch> ;
	org:rankSeniorToTransitive :Rank_Lieutenant_colonel_EnglishTradition ;
	a :MilitaryRank ;
	rdfs:comment "Colonel, abbreviated as Col or COL, is a military rank of a senior commissioned officer. It or a corresponding rank exists in most armies and in many air forces; the naval equivalent rank is generally \"Captain\". It is also used in some police forces and other paramilitary rank structures. A colonel is typically in charge of a regiment in an army. \"Colonel\" is usually the highest or second-highest field rank, and is below the general ranks."@en ;
	rdfs:label "Colonel"@en , "Colonel"@fr , "Oberst"@de ;
	owl:sameAs <dbpedia:Colonel> .

:Rank_Comandarm a :MilitaryRank ;
	rdfs:comment "Comandarm (also Komandarm, Commandarm, Russian \"командарм\" - abbreviated \"командующий армией\", Commander of the Army) was a military rank in the Red Army until the end of the 1930s. Comandarm 2nd rank, with the insignia of four rombs, is graded at 4 ranks above colonel. Comandarm 1st rank, with the insignia of four rombs and a star, is at 5 ranks above colonel."@en ;
	rdfs:label "Comandarm"@en , "Komandarm"@de , "Komandarm"@pl , "Komandarm av 1. klasse"@no , "Komandarm av 2. klasse"@no , "Sowjetische Generalsränge"@de ;
	owl:sameAs <dbpedia:Comandarm> ;
	foaf:name "Comandarm" .

:Rank_Comandarm_Russia org:rankOf <dbpedia:Russia> ;
	a :MilitaryRank ;
	rdfs:comment "The specific instance of the Comandarm rank in the context of country Russia."@en ;
	rdfs:label "Comandarm (Rusia)"@es , "Comandarm (Rusland)"@nl , "Comandarm (Russia)"@en , "Comandarm (Russia)"@it , "Comandarm (Russie)"@fr , "Comandarm (Ryssland)"@sv , "Comandarm (Rússia)"@pt , "Comandarm (Venäjä)"@fi , "Comandarm (Россия)"@ru , "Komandarm (Rosja)"@pl , "Komandarm av 1. klasseKomandarm av 2. klasse (Russland)"@no , "Sowjetische GeneralsrängeKomandarm (Russland)"@de ;
	owl:subClass :Rank_Comandarm ;
	foaf:name "Comandarm"@en .

:Rank_Comandarm_Soviet_Union org:rankOf <dbpedia:Soviet_Union> ;
	a :MilitaryRank ;
	rdfs:comment "The specific instance of the Comandarm rank in the context of country Soviet Union."@en ;
	rdfs:label "Comandarm (Neuvostoliitto)"@fi , "Comandarm (Soviet Union)"@en , "Comandarm (Sovjet-Unie)"@nl , "Comandarm (Sovjetunionen)"@sv , "Comandarm (Union des républiques socialistes soviétiques)"@fr , "Comandarm (Unione Sovietica)"@it , "Comandarm (União Soviética)"@pt , "Comandarm (Unión Soviética)"@es , "Comandarm (Союз Советских Социалистических Республик)"@ru , "Komandarm (Związek Socjalistycznych Republik Radzieckich)"@pl , "Komandarm av 1. klasseKomandarm av 2. klasse (Sovjetunionen)"@no , "Sowjetische GeneralsrängeKomandarm (Sowjetunion)"@de ;
	owl:subClass :Rank_Comandarm ;
	foaf:name "Comandarm"@en .

:Rank_Combrig a :MilitaryRank ;
	rdfs:comment "Combrig was a military rank used in the Red Army for commanders of brigades between 1935 and 1940 (with some individuals still holding the rank in 1941). Kombrigs were senior to polkovniks (colonels) and junior to comdivs (commander of the division). When general ranks were reintroduced in July 1940 most kombrigs were transferred to the junior rank of polkovnik, while some received the rank of major general."@en ;
	rdfs:label "Combrig"@en , "Kombrig"@de , "Kombrig"@es , "Kombrig"@it , "Kombrig"@pl , "Prikaatinkomentaja"@fi , "Комбриг"@ru ;
	owl:sameAs <dbpedia:Combrig> ;
	foaf:name "Combrig" .

:Rank_Combrig_Russia org:rankOf <dbpedia:Russia> ;
	a :MilitaryRank ;
	rdfs:comment "The specific instance of the Combrig rank in the context of country Russia."@en ;
	rdfs:label "Combrig (Rusland)"@nl , "Combrig (Russia)"@en , "Combrig (Russie)"@fr , "Combrig (Russland)"@no , "Combrig (Ryssland)"@sv , "Combrig (Rússia)"@pt , "Kombrig (Rosja)"@pl , "Kombrig (Rusia)"@es , "Kombrig (Russia)"@it , "Kombrig (Russland)"@de , "Prikaatinkomentaja (Venäjä)"@fi , "Комбриг (Россия)"@ru ;
	owl:subClass :Rank_Combrig ;
	foaf:name "Комбриг"@ru .

:Rank_Combrig_Soviet_Union org:rankOf <dbpedia:Soviet_Union> ;
	a :MilitaryRank ;
	rdfs:comment "The specific instance of the Combrig rank in the context of country Soviet Union."@en ;
	rdfs:label "Combrig (Soviet Union)"@en , "Combrig (Sovjet-Unie)"@nl , "Combrig (Sovjetunionen)"@no , "Combrig (Sovjetunionen)"@sv , "Combrig (Union des républiques socialistes soviétiques)"@fr , "Combrig (União Soviética)"@pt , "Kombrig (Sowjetunion)"@de , "Kombrig (Unione Sovietica)"@it , "Kombrig (Unión Soviética)"@es , "Kombrig (Związek Socjalistycznych Republik Radzieckich)"@pl , "Prikaatinkomentaja (Neuvostoliitto)"@fi , "Комбриг (Союз Советских Социалистических Республик)"@ru ;
	owl:subClass :Rank_Combrig ;
	foaf:name "Combrig"@en .

:Rank_Comcor a :MilitaryRank ;
	rdfs:comment "Comcor (or Comkor, Komkor, abbreviated from Commander of the Corps) was a military rank in the Red Army until the end of the 1930"@en ;
	rdfs:label "Armeijakunnankomentaja"@fi , "Comcor"@en , "Komkor"@de , "Komkor"@es , "Komkor"@no , "Komkor"@pl , "Комкор"@ru ;
	owl:sameAs <dbpedia:Comcor> ;
	foaf:name "Comcor" .

:Rank_Comcor_Russia org:rankOf <dbpedia:Russia> ;
	a :MilitaryRank ;
	rdfs:comment "The specific instance of the Comcor rank in the context of country Russia."@en ;
	rdfs:label "Armeijakunnankomentaja (Venäjä)"@fi , "Comcor (Rusland)"@nl , "Comcor (Russia)"@en , "Comcor (Russia)"@it , "Comcor (Russie)"@fr , "Comcor (Ryssland)"@sv , "Comcor (Rússia)"@pt , "Komkor (Rosja)"@pl , "Komkor (Rusia)"@es , "Komkor (Russland)"@de , "Komkor (Russland)"@no , "Комкор (Россия)"@ru ;
	owl:subClass :Rank_Comcor ;
	foaf:name "Комкор"@ru .

:Rank_Comcor_Soviet_Union org:rankOf <dbpedia:Soviet_Union> ;
	a :MilitaryRank ;
	rdfs:comment "The specific instance of the Comcor rank in the context of country Soviet Union."@en ;
	rdfs:label "Armeijakunnankomentaja (Neuvostoliitto)"@fi , "Comcor (Soviet Union)"@en , "Comcor (Sovjet-Unie)"@nl , "Comcor (Sovjetunionen)"@sv , "Comcor (Union des républiques socialistes soviétiques)"@fr , "Comcor (Unione Sovietica)"@it , "Comcor (União Soviética)"@pt , "Komkor (Sovjetunionen)"@no , "Komkor (Sowjetunion)"@de , "Komkor (Unión Soviética)"@es , "Komkor (Związek Socjalistycznych Republik Radzieckich)"@pl , "Комкор (Союз Советских Социалистических Республик)"@ru ;
	owl:subClass :Rank_Comcor ;
	foaf:name "Comcor"@en .

:Rank_Comdiv a :MilitaryRank ;
	rdfs:comment "Comdiv or Komdiv, abbreviated from (\"Commander of the division\") was a military rank in the Red Army until the end of the 1930s."@en ;
	rdfs:label "Comdiv"@en , "Divisioonankomentaja"@fi , "Komdiv"@de , "Komdiv"@es , "Komdiv"@no , "Komdiw"@pl , "Комдив"@ru ;
	owl:sameAs <dbpedia:Comdiv> ;
	foaf:name "Comdiv" .

:Rank_Comdiv_Russia org:rankOf <dbpedia:Russia> ;
	a :MilitaryRank ;
	rdfs:comment "The specific instance of the Comdiv rank in the context of country Russia."@en ;
	rdfs:label "Comdiv (Rusland)"@nl , "Comdiv (Russia)"@en , "Comdiv (Russia)"@it , "Comdiv (Russie)"@fr , "Comdiv (Ryssland)"@sv , "Comdiv (Rússia)"@pt , "Divisioonankomentaja (Venäjä)"@fi , "Komdiv (Rusia)"@es , "Komdiv (Russland)"@de , "Komdiv (Russland)"@no , "Komdiw (Rosja)"@pl , "Комдив (Россия)"@ru ;
	owl:subClass :Rank_Comdiv ;
	foaf:name "Комдив"@ru .

:Rank_Comdiv_Soviet_Union org:rankOf <dbpedia:Soviet_Union> ;
	a :MilitaryRank ;
	rdfs:comment "The specific instance of the Comdiv rank in the context of country Soviet Union."@en ;
	rdfs:label "Comdiv (Soviet Union)"@en , "Comdiv (Sovjet-Unie)"@nl , "Comdiv (Sovjetunionen)"@sv , "Comdiv (Union des républiques socialistes soviétiques)"@fr , "Comdiv (Unione Sovietica)"@it , "Comdiv (União Soviética)"@pt , "Divisioonankomentaja (Neuvostoliitto)"@fi , "Komdiv (Sovjetunionen)"@no , "Komdiv (Sowjetunion)"@de , "Komdiv (Unión Soviética)"@es , "Komdiw (Związek Socjalistycznych Republik Radzieckich)"@pl , "Комдив (Союз Советских Социалистических Республик)"@ru ;
	owl:subClass :Rank_Comdiv ;
	foaf:name "Comdiv"@en .

<http://rdf.muninn-project.org/ontologies/military#Rank_Commandant_(rank)_EnglishTradition> org:rankEquivalentTo :Rank_Lieutenant_commander_EnglishTradition , :Rank_Squadron_leader_EnglishTradition ;
	org:rankJuniorToTransitive :Rank_Lieutenant_colonel_EnglishTradition ;
	org:rankOf :EnglishTradition , <mil:ArmyServiceBranch> ;
	org:rankSeniorToTransitive :Rank_Captain_EnglishTradition ;
	a :MilitaryRank ;
	owl:sameAs <dbpedia:Commandant_(rank)> .

:Rank_Commander_EnglishTradition org:rankEquivalentTo :Rank_Lieutenant_colonel_EnglishTradition , <http://rdf.muninn-project.org/ontologies/military#Rank_Wing_commander_(rank)_EnglishTradition> ;
	org:rankJuniorToTransitive <http://rdf.muninn-project.org/ontologies/military#Rank_Captain_(naval)_EnglishTradition> ;
	org:rankOf :EnglishTradition , <mil:NavyServiceBranch> ;
	org:rankSeniorToTransitive :Rank_Lieutenant_commander_EnglishTradition ;
	a :MilitaryRank ;
	rdfs:comment "Commander is a naval rank which is also sometimes used as a military title depending on the individual customs of a given military service. Commander is also used as a rank or title in some organizations outside of the armed forces, particularly in police and law enforcement."@en ;
	rdfs:label "Capitaine de frégate"@fr , "Commander"@en , "Fregattenkapitän"@de ;
	owl:sameAs <dbpedia:Commander> .

:Rank_Commandeur a :MilitaryRank ;
	rdfs:comment "Commandeur is a title in French and Dutch (also, now a purism, Kommandeur), usually rendered in English as Commander, with different uses. The literal meaning is he who commands, parallel to Commandant. In most senses the German equivalent is Kommandeur."@en ;
	rdfs:label "Commandeur"@en , "Commandeur"@fr , "Commandeur (marine)"@nl ;
	owl:sameAs <dbpedia:Commandeur> ;
	foaf:name "Commandeur" .

:Rank_Commandeur_France org:rankOf <dbpedia:France> ;
	a :MilitaryRank ;
	rdfs:comment "The specific instance of the Commandeur rank in the context of France."@en ;
	rdfs:label "Commandeur (France)"@en , "Commandeur (France)"@fr , "Commandeur (marine, France)"@nl ;
	owl:subClass :Rank_Commandeur ;
	foaf:name "Commandeur"@fr .

:Rank_Commandeur_Netherlands org:rankOf <dbpedia:Netherlands> ;
	a :MilitaryRank ;
	rdfs:comment "The specific instance of the Commandeur rank in the context of country Netherlands."@en ;
	rdfs:label "Commandeur (Alankomaat)"@fi , "Commandeur (Holandia)"@pl , "Commandeur (Nederland)"@no , "Commandeur (Nederländerna)"@sv , "Commandeur (Netherlands)"@en , "Commandeur (Niederlande)"@de , "Commandeur (Paesi Bassi)"@it , "Commandeur (Pays-Bas)"@fr , "Commandeur (Países Baixos)"@pt , "Commandeur (Países Bajos)"@es , "Commandeur (marine) (Nederland)"@nl , "Commandeur (Нидерланды)"@ru ;
	owl:subClass :Rank_Commandeur ;
	foaf:name "Commandeur"@en , "Commandeur"@nl .

<http://rdf.muninn-project.org/ontologies/military#Rank_Commodore_(rank)_EnglishTradition> org:rankEquivalentTo :Rank_Air_commodore_EnglishTradition , :Rank_Brigadier_EnglishTradition ;
	org:rankJuniorToTransitive :Rank_Admiral_EnglishTradition ;
	org:rankOf :EnglishTradition , <mil:NavyServiceBranch> ;
	org:rankSeniorToTransitive <http://rdf.muninn-project.org/ontologies/military#Rank_Captain_(naval)_EnglishTradition> ;
	a :MilitaryRank ;
	owl:sameAs <dbpedia:Commodore_(rank)> .

:Rank_Company_Quartermaster_Sergeant a :MilitaryRank ;
	rdfs:comment "Company Quartermaster Sergeant is a military rank or appointment."@en ;
	rdfs:label "Company Quartermaster Sergeant"@en ;
	owl:sameAs <dbpedia:Company_Quartermaster_Sergeant> ;
	foaf:name "Company Quartermaster Sergeant" .

:Rank_Company_Quartermaster_Sergeant_Commonwealth_of_Nations org:rankOf <dbpedia:Commonwealth_of_Nations> ;
	a :MilitaryRank ;
	rdfs:comment "The specific instance of the Company Quartermaster Sergeant rank in the context of country Commonwealth of Nations."@en ;
	rdfs:label "Company Quartermaster Sergeant (Commonwealth delle nazioni)"@it , "Company Quartermaster Sergeant (Commonwealth of Nations)"@de , "Company Quartermaster Sergeant (Commonwealth of Nations)"@en , "Company Quartermaster Sergeant (Commonwealth of Nations)"@fr , "Company Quartermaster Sergeant (Commonwealth)"@pt , "Company Quartermaster Sergeant (Gemenebest van Naties)"@nl , "Company Quartermaster Sergeant (Kansainyhteisö)"@fi , "Company Quartermaster Sergeant (Mancomunidad de Naciones)"@es , "Company Quartermaster Sergeant (Samveldet av nasjoner)"@no , "Company Quartermaster Sergeant (Samväldet)"@sv , "Company Quartermaster Sergeant (Wspólnota Narodów)"@pl , "Company Quartermaster Sergeant (Содружество наций)"@ru ;
	owl:subClass :Rank_Company_Quartermaster_Sergeant ;
	foaf:name "Company Quartermaster Sergeant"@en .

:Rank_Company_Quartermaster_Sergeant_England org:rankOf <dbpedia:England> ;
	a :MilitaryRank ;
	rdfs:comment "The specific instance of the Company Quartermaster Sergeant rank in the context of England."@en ;
	rdfs:label "Company Quartermaster Sergeant (England)"@en ;
	owl:subClass :Rank_Company_Quartermaster_Sergeant ;
	foaf:name "Company Quartermaster Sergeant"@en .

:Rank_Company_Quartermaster_Sergeant_Republic_of_Ireland org:rankOf <dbpedia:Republic_of_Ireland> ;
	a :MilitaryRank ;
	rdfs:comment "The specific instance of the Company Quartermaster Sergeant rank in the context of country Republic of Ireland."@en ;
	rdfs:label "Company Quartermaster Sergeant (Ierland (land))"@nl , "Company Quartermaster Sergeant (Irland)"@de , "Company Quartermaster Sergeant (Irland)"@no , "Company Quartermaster Sergeant (Irland)"@sv , "Company Quartermaster Sergeant (Irlanda)"@es , "Company Quartermaster Sergeant (Irlanda)"@it , "Company Quartermaster Sergeant (Irlande (pays))"@fr , "Company Quartermaster Sergeant (Irlandia)"@pl , "Company Quartermaster Sergeant (Irlanti)"@fi , "Company Quartermaster Sergeant (Republic of Ireland)"@en , "Company Quartermaster Sergeant (República da Irlanda)"@pt , "Company Quartermaster Sergeant (Ирландия)"@ru ;
	owl:subClass :Rank_Company_Quartermaster_Sergeant ;
	foaf:name "Company Quartermaster Sergeant"@en .

:Rank_Company_Quartermaster_Sergeant_Scotland org:rankOf <dbpedia:Scotland> ;
	a :MilitaryRank ;
	rdfs:comment "The specific instance of the Company Quartermaster Sergeant rank in the context of country Scotland."@en ;
	rdfs:label "Company Quartermaster Sergeant (Escocia)"@es , "Company Quartermaster Sergeant (Escócia)"@pt , "Company Quartermaster Sergeant (Schotland)"@nl , "Company Quartermaster Sergeant (Schottland)"@de , "Company Quartermaster Sergeant (Scotland)"@en , "Company Quartermaster Sergeant (Scozia)"@it , "Company Quartermaster Sergeant (Skotlanti)"@fi , "Company Quartermaster Sergeant (Skottland)"@no , "Company Quartermaster Sergeant (Skottland)"@sv , "Company Quartermaster Sergeant (Szkocja)"@pl , "Company Quartermaster Sergeant (Écosse)"@fr , "Company Quartermaster Sergeant (Шотландия)"@ru ;
	owl:subClass :Rank_Company_Quartermaster_Sergeant ;
	foaf:name "Company Quartermaster Sergeant"@en .

:Rank_Company_Quartermaster_Sergeant_Wales org:rankOf <dbpedia:Wales> ;
	a :MilitaryRank ;
	rdfs:comment "The specific instance of the Company Quartermaster Sergeant rank in the context of country Wales."@en ;
	rdfs:label "Company Quartermaster Sergeant (Gales)"@es , "Company Quartermaster Sergeant (Galles)"@it , "Company Quartermaster Sergeant (Pays de Galles)"@fr , "Company Quartermaster Sergeant (País de Gales)"@pt , "Company Quartermaster Sergeant (Wales)"@de , "Company Quartermaster Sergeant (Wales)"@en , "Company Quartermaster Sergeant (Wales)"@fi , "Company Quartermaster Sergeant (Wales)"@nl , "Company Quartermaster Sergeant (Wales)"@no , "Company Quartermaster Sergeant (Wales)"@sv , "Company Quartermaster Sergeant (Walia)"@pl , "Company Quartermaster Sergeant (Уэльс)"@ru ;
	owl:subClass :Rank_Company_Quartermaster_Sergeant ;
	foaf:name "Company Quartermaster Sergeant"@en .

:Rank_Company_sergeant_major a :MilitaryRank ;
	rdfs:label "Company sergeant major"@en ;
	owl:sameAs <dbpedia:Company_sergeant_major> ;
	foaf:name "Company sergeant major" .

:Rank_Company_sergeant_major_Australia org:rankOf <dbpedia:Australia> ;
	a :MilitaryRank ;
	rdfs:comment "The specific instance of the Company sergeant major rank in the context of country Australia."@en ;
	rdfs:label "Company sergeant major (Australia)"@en , "Company sergeant major (Australia)"@es , "Company sergeant major (Australia)"@fi , "Company sergeant major (Australia)"@it , "Company sergeant major (Australia)"@no , "Company sergeant major (Australia)"@pl , "Company sergeant major (Australie)"@fr , "Company sergeant major (Australien)"@de , "Company sergeant major (Australien)"@sv , "Company sergeant major (Australië (land))"@nl , "Company sergeant major (Austrália)"@pt , "Company sergeant major (Австралия)"@ru ;
	owl:subClass :Rank_Company_sergeant_major ;
	foaf:name "Company sergeant major"@en .

:Rank_Company_sergeant_major_Canada org:rankOf <dbpedia:Canada> ;
	a :MilitaryRank ;
	rdfs:comment "The specific instance of the Company sergeant major rank in the context of Canada."@en ;
	rdfs:label "Company sergeant major (Canada)"@en ;
	owl:subClass :Rank_Company_sergeant_major ;
	foaf:name "Company sergeant major"@en .

:Rank_Company_sergeant_major_Commonwealth_of_Nations org:rankOf <dbpedia:Commonwealth_of_Nations> ;
	a :MilitaryRank ;
	rdfs:comment "The specific instance of the Company sergeant major rank in the context of country Commonwealth of Nations."@en ;
	rdfs:label "Company sergeant major (Commonwealth delle nazioni)"@it , "Company sergeant major (Commonwealth of Nations)"@de , "Company sergeant major (Commonwealth of Nations)"@en , "Company sergeant major (Commonwealth of Nations)"@fr , "Company sergeant major (Commonwealth)"@pt , "Company sergeant major (Gemenebest van Naties)"@nl , "Company sergeant major (Kansainyhteisö)"@fi , "Company sergeant major (Mancomunidad de Naciones)"@es , "Company sergeant major (Samveldet av nasjoner)"@no , "Company sergeant major (Samväldet)"@sv , "Company sergeant major (Wspólnota Narodów)"@pl , "Company sergeant major (Содружество наций)"@ru ;
	owl:subClass :Rank_Company_sergeant_major ;
	foaf:name "Company sergeant major"@en .

:Rank_Company_sergeant_major_England org:rankOf <dbpedia:England> ;
	a :MilitaryRank ;
	rdfs:comment "The specific instance of the Company sergeant major rank in the context of England."@en ;
	rdfs:label "Company sergeant major (England)"@en ;
	owl:subClass :Rank_Company_sergeant_major ;
	foaf:name "Company sergeant major"@en .

:Rank_Company_sergeant_major_Scotland org:rankOf <dbpedia:Scotland> ;
	a :MilitaryRank ;
	rdfs:comment "The specific instance of the Company sergeant major rank in the context of country Scotland."@en ;
	rdfs:label "Company sergeant major (Escocia)"@es , "Company sergeant major (Escócia)"@pt , "Company sergeant major (Schotland)"@nl , "Company sergeant major (Schottland)"@de , "Company sergeant major (Scotland)"@en , "Company sergeant major (Scozia)"@it , "Company sergeant major (Skotlanti)"@fi , "Company sergeant major (Skottland)"@no , "Company sergeant major (Skottland)"@sv , "Company sergeant major (Szkocja)"@pl , "Company sergeant major (Écosse)"@fr , "Company sergeant major (Шотландия)"@ru ;
	owl:subClass :Rank_Company_sergeant_major ;
	foaf:name "Company sergeant major"@en .

:Rank_Company_sergeant_major_Singapore org:rankOf <dbpedia:Singapore> ;
	a :MilitaryRank ;
	rdfs:comment "The specific instance of the Company sergeant major rank in the context of country Singapore."@en ;
	rdfs:label "Company sergeant major (Singapore)"@en , "Company sergeant major (Singapore)"@fi , "Company sergeant major (Singapore)"@it , "Company sergeant major (Singapore)"@nl , "Company sergeant major (Singapore)"@no , "Company sergeant major (Singapore)"@sv , "Company sergeant major (Singapour)"@fr , "Company sergeant major (Singapur)"@de , "Company sergeant major (Singapur)"@es , "Company sergeant major (Singapur)"@pl , "Company sergeant major (Singapura)"@pt , "Company sergeant major (Сингапур)"@ru ;
	owl:subClass :Rank_Company_sergeant_major ;
	foaf:name "Company sergeant major"@en .

:Rank_Company_sergeant_major_Wales org:rankOf <dbpedia:Wales> ;
	a :MilitaryRank ;
	rdfs:comment "The specific instance of the Company sergeant major rank in the context of country Wales."@en ;
	rdfs:label "Company sergeant major (Gales)"@es , "Company sergeant major (Galles)"@it , "Company sergeant major (Pays de Galles)"@fr , "Company sergeant major (País de Gales)"@pt , "Company sergeant major (Wales)"@de , "Company sergeant major (Wales)"@en , "Company sergeant major (Wales)"@fi , "Company sergeant major (Wales)"@nl , "Company sergeant major (Wales)"@no , "Company sergeant major (Wales)"@sv , "Company sergeant major (Walia)"@pl , "Company sergeant major (Уэльс)"@ru ;
	owl:subClass :Rank_Company_sergeant_major ;
	foaf:name "Company sergeant major"@en .

:Rank_Conductor_army a :MilitaryRank ;
	rdfs:comment "Conductor (Cdr) is an appointment held by a few selected Warrant Officers Class 1 in the Royal Logistic Corps and is the most senior appointment that can be held by a warrant officer in the British Army. The appointment was also reintroduced into the Royal Australian Army Ordnance Corps for selected Warrant Officers Class 1 in 2005."@en ;
	rdfs:label "Conductor (Army)"@en ;
	owl:sameAs <dbpedia:Conductor_%28Army%29> ;
	foaf:name "Conductor" .

:Rank_Conductor_army_Australia org:rankOf <dbpedia:Australia> ;
	a :MilitaryRank ;
	rdfs:comment "The specific instance of the Conductor (Army) rank in the context of country Australia."@en ;
	rdfs:label "Conductor (Army) (Australia)"@en , "Conductor (Army) (Australia)"@es , "Conductor (Army) (Australia)"@fi , "Conductor (Army) (Australia)"@it , "Conductor (Army) (Australia)"@no , "Conductor (Army) (Australia)"@pl , "Conductor (Army) (Australie)"@fr , "Conductor (Army) (Australien)"@de , "Conductor (Army) (Australien)"@sv , "Conductor (Army) (Australië (land))"@nl , "Conductor (Army) (Austrália)"@pt , "Conductor (Army) (Австралия)"@ru ;
	owl:subClass :Rank_Conductor_army ;
	foaf:name "Conductor"@en .

:Rank_Conductor_army_England org:rankOf <dbpedia:England> ;
	a :MilitaryRank ;
	rdfs:comment "The specific instance of the Conductor (Army) rank in the context of England."@en ;
	rdfs:label "Conductor (Army) (England)"@en ;
	owl:subClass :Rank_Conductor_army ;
	foaf:name "Conductor"@en .

:Rank_Conductor_army_Scotland org:rankOf <dbpedia:Scotland> ;
	a :MilitaryRank ;
	rdfs:comment "The specific instance of the Conductor (Army) rank in the context of country Scotland."@en ;
	rdfs:label "Conductor (Army) (Escocia)"@es , "Conductor (Army) (Escócia)"@pt , "Conductor (Army) (Schotland)"@nl , "Conductor (Army) (Schottland)"@de , "Conductor (Army) (Scotland)"@en , "Conductor (Army) (Scozia)"@it , "Conductor (Army) (Skotlanti)"@fi , "Conductor (Army) (Skottland)"@no , "Conductor (Army) (Skottland)"@sv , "Conductor (Army) (Szkocja)"@pl , "Conductor (Army) (Écosse)"@fr , "Conductor (Army) (Шотландия)"@ru ;
	owl:subClass :Rank_Conductor_army ;
	foaf:name "Conductor"@en .

:Rank_Conductor_army_Wales org:rankOf <dbpedia:Wales> ;
	a :MilitaryRank ;
	rdfs:comment "The specific instance of the Conductor (Army) rank in the context of country Wales."@en ;
	rdfs:label "Conductor (Army) (Gales)"@es , "Conductor (Army) (Galles)"@it , "Conductor (Army) (Pays de Galles)"@fr , "Conductor (Army) (País de Gales)"@pt , "Conductor (Army) (Wales)"@de , "Conductor (Army) (Wales)"@en , "Conductor (Army) (Wales)"@fi , "Conductor (Army) (Wales)"@nl , "Conductor (Army) (Wales)"@no , "Conductor (Army) (Wales)"@sv , "Conductor (Army) (Walia)"@pl , "Conductor (Army) (Уэльс)"@ru ;
	owl:subClass :Rank_Conductor_army ;
	foaf:name "Conductor"@en .

:Rank_Corporal_EnglishTradition org:rankEquivalentTo :Rank_Corporal_EnglishTradition , :Rank_Leading_seaman_EnglishTradition ;
	org:rankJuniorToTransitive :Rank_Sergeant_EnglishTradition ;
	org:rankOf :EnglishTradition , <mil:AirForceServiceBranch> , <mil:ArmyServiceBranch> ;
	org:rankSeniorToTransitive :Rank_Aircraftman_EnglishTradition , <http://rdf.muninn-project.org/ontologies/military#Rank_Private_(rank)_EnglishTradition> ;
	a :MilitaryRank ;
	rdfs:comment "Corporal is a rank in use in some form by most militaries and by some police forces or other uniformed organizations. It is usually equivalent to NATO Rank Code OR-4. The rank of corporal nominally corresponds to commanding a section or squad of soldiers. However, in the United States Army, but not the U.S. Marines, a corporal is usually a fire team leader or second-in-command of a squad of soldiers."@en ;
	rdfs:label "Caporal"@fr , "Corporal"@en , "Korporal"@de ;
	owl:sameAs <dbpedia:Corporal> .

:Rank_Daejang a :MilitaryRank ;
	rdfs:comment "Daejang is a senior military rank of the Korean Peninsula, used by both North and South Korea. It is considered the combined equivalent of a General and Admiral in other nations. The rank of Daejang is sometimes spelled as Taejang, depending on the transliteration system used (Taejang in McCune-Reischauer, Daejang in official ROK transliteration system)."@en ;
	rdfs:label "Daejang"@en ;
	owl:sameAs <dbpedia:Daejang> ;
	foaf:name "Daejang" .

:Rank_Daejang_North_Korea org:rankOf <dbpedia:North_Korea> ;
	a :MilitaryRank ;
	rdfs:comment "The specific instance of the Daejang rank in the context of country North Korea."@en ;
	rdfs:label "Daejang (Corea del Nord)"@it , "Daejang (Corea del Norte)"@es , "Daejang (Coreia do Norte)"@pt , "Daejang (Corée du Nord)"@fr , "Daejang (Korea Północna)"@pl , "Daejang (Korean demokraattinen kansantasavalta)"@fi , "Daejang (Noord-Korea)"@nl , "Daejang (Nord-Korea)"@no , "Daejang (Nordkorea)"@de , "Daejang (Nordkorea)"@sv , "Daejang (North Korea)"@en , "Daejang (Корейская Народно-Демократическая Республика)"@ru ;
	owl:subClass :Rank_Daejang ;
	foaf:name "Daejang"@en .

:Rank_Daejang_South_Korea org:rankOf <dbpedia:South_Korea> ;
	a :MilitaryRank ;
	rdfs:comment "The specific instance of the Daejang rank in the context of country South Korea."@en ;
	rdfs:label "Daejang (Corea del Sud)"@it , "Daejang (Corea del Sur)"@es , "Daejang (Coreia do Sul)"@pt , "Daejang (Corée du Sud)"@fr , "Daejang (Korea Południowa)"@pl , "Daejang (Korean tasavalta)"@fi , "Daejang (South Korea)"@en , "Daejang (Sydkorea)"@sv , "Daejang (Sør-Korea)"@no , "Daejang (Südkorea)"@de , "Daejang (Zuid-Korea)"@nl , "Daejang (Республика Корея)"@ru ;
	owl:subClass :Rank_Daejang ;
	foaf:name "Daejang"@en .

:Rank_Daffadar org:rankEquivalentTo :Rank_Havildar ;
	org:rankOf <mil:Cavalry> ;
	a :MilitaryRank ;
	rdfs:comment "Daffadar, roughly equivalent to a Sergeant"@en ;
	rdfs:label "Daffadar"@en ;
	owl:sameAs <dbpedia:Daffadar> ;
	foaf:name "Daffadar"@en .

:Rank_Daffadar_British_India org:rankJuniorTo <http://rdf.muninn-project.org/ontologies/military> ;
	org:rankOf <dbpedia:British_Indian_Army> , <dbpedia:British_Raj> , <mil:Cavalry> ;
	org:subClass <mil:Rank_Sergeant> ;
	a :MilitaryRank ;
	rdfs:comment "Daffadar, roughly equivalent to a Sergeant"@en ;
	rdfs:label "Daffadar"@en ;
	foaf:name "Daffadar"@en .

:Rank_Divisional_Admiral a :MilitaryRank ;
	rdfs:comment "Divisional Admiral or Division Admiral is a commissioned officer rank in several navies. It is a two-star flag rank, equivalent to the rank of Rear Admiral in the Royal Navy and the rank of Rear Admiral (Upper Half) in the United States Navy."@en ;
	rdfs:label "Amiral de division"@fr , "Ammiraglio di divisione"@it , "Divisieadmiraal"@nl , "Divisional Admiral"@en ;
	owl:sameAs <dbpedia:Divisional_Admiral> ;
	foaf:name "Divisional Admiral" .

:Rank_Divisional_Admiral_Belgium org:rankOf <dbpedia:Belgium> ;
	a :MilitaryRank ;
	rdfs:comment "The specific instance of the Divisional Admiral rank in the context of country Belgium."@en ;
	rdfs:label "Amiral de division (Belgique)"@fr , "Ammiraglio di divisione (Belgio)"@it , "Divisieadmiraal (België)"@nl , "Divisional Admiral (Belgia)"@fi , "Divisional Admiral (Belgia)"@no , "Divisional Admiral (Belgia)"@pl , "Divisional Admiral (Belgien)"@de , "Divisional Admiral (Belgien)"@sv , "Divisional Admiral (Belgium)"@en , "Divisional Admiral (Bélgica)"@es , "Divisional Admiral (Bélgica)"@pt , "Divisional Admiral (Бельгия)"@ru ;
	owl:subClass :Rank_Divisional_Admiral ;
	foaf:name "Amiral de division"@fr , "Divisieadmiraal"@nl .

:Rank_Divisional_Admiral_Italy org:rankOf <dbpedia:Italy> ;
	a :MilitaryRank ;
	rdfs:comment "The specific instance of the Divisional Admiral rank in the context of country Italy."@en ;
	rdfs:label "Amiral de division (Italie)"@fr , "Ammiraglio di divisione (Italia)"@it , "Divisieadmiraal (Italië)"@nl , "Divisional Admiral (Italia)"@es , "Divisional Admiral (Italia)"@fi , "Divisional Admiral (Italia)"@no , "Divisional Admiral (Italien)"@de , "Divisional Admiral (Italien)"@sv , "Divisional Admiral (Italy)"@en , "Divisional Admiral (Itália)"@pt , "Divisional Admiral (Włochy)"@pl , "Divisional Admiral (Италия)"@ru ;
	owl:subClass :Rank_Divisional_Admiral ;
	foaf:name "Ammiraglio di divisione"@it .

:Rank_Divisional_General a :MilitaryRank ;
	rdfs:comment "Divisional General is a rank used in many armies to denote a rank of general, corresponding to command of a division. For convenience Divisional General is almost always translated into English as Major-General, the equivalent rank used by the UK, USA, etc. , although this translation is, strictly speaking, incorrect. The rank is particularly common in western Europe and Latin America."@en ;
	rdfs:label "Divisional General"@en , "Divisioonakenraali"@fi , "General de divisão"@pt , "Generale di divisione"@it , "Général de division"@fr ;
	owl:sameAs <dbpedia:Divisional_General> ;
	foaf:name "Divisional General" .

:Rank_Divisional_General_France org:rankOf <dbpedia:France> ;
	a :MilitaryRank ;
	rdfs:comment "The specific instance of the Divisional General rank in the context of France."@en ;
	rdfs:label "Divisional General (France)"@en , "Divisioonakenraali (France)"@fi , "General de divisão (France)"@pt , "Generale di divisione (France)"@it , "Général de division (France)"@fr ;
	owl:subClass :Rank_Divisional_General ;
	foaf:name "Général de division"@fr .

:Rank_Divisional_General_Poland org:rankOf <dbpedia:Poland> ;
	a :MilitaryRank ;
	rdfs:comment "The specific instance of the Divisional General rank in the context of Poland."@en ;
	rdfs:label "Divisional General (Poland)"@en , "Divisioonakenraali (Poland)"@fi , "General de divisão (Poland)"@pt , "Generale di divisione (Poland)"@it , "Général de division (Poland)"@fr ;
	owl:subClass :Rank_Divisional_General ;
	foaf:name "Divisional General"@en .

:Rank_Drum_Major_General a :MilitaryRank ;
	rdfs:comment "[edit] Overview The Drum Major General was a royal appointment in the British Army used from the mid-17th century and into the 18th century. Under this appointment, all training and licensing of military drummers took place."@en ;
	rdfs:label "Drum Major General"@en ;
	owl:sameAs <dbpedia:Drum_Major_General> ;
	foaf:name "Drum Major General" .

:Rank_Drum_Major_General_Commonwealth_of_Nations org:rankOf <dbpedia:Commonwealth_of_Nations> ;
	a :MilitaryRank ;
	rdfs:comment "The specific instance of the Drum Major General rank in the context of country Commonwealth of Nations."@en ;
	rdfs:label "Drum Major General (Commonwealth delle nazioni)"@it , "Drum Major General (Commonwealth of Nations)"@de , "Drum Major General (Commonwealth of Nations)"@en , "Drum Major General (Commonwealth of Nations)"@fr , "Drum Major General (Commonwealth)"@pt , "Drum Major General (Gemenebest van Naties)"@nl , "Drum Major General (Kansainyhteisö)"@fi , "Drum Major General (Mancomunidad de Naciones)"@es , "Drum Major General (Samveldet av nasjoner)"@no , "Drum Major General (Samväldet)"@sv , "Drum Major General (Wspólnota Narodów)"@pl , "Drum Major General (Содружество наций)"@ru ;
	owl:subClass :Rank_Drum_Major_General ;
	foaf:name "Drum Major General"@en .

:Rank_Drum_Major_General_England org:rankOf <dbpedia:England> ;
	a :MilitaryRank ;
	rdfs:comment "The specific instance of the Drum Major General rank in the context of England."@en ;
	rdfs:label "Drum Major General (England)"@en ;
	owl:subClass :Rank_Drum_Major_General ;
	foaf:name "Drum Major General"@en .

:Rank_Drum_Major_General_Scotland org:rankOf <dbpedia:Scotland> ;
	a :MilitaryRank ;
	rdfs:comment "The specific instance of the Drum Major General rank in the context of country Scotland."@en ;
	rdfs:label "Drum Major General (Escocia)"@es , "Drum Major General (Escócia)"@pt , "Drum Major General (Schotland)"@nl , "Drum Major General (Schottland)"@de , "Drum Major General (Scotland)"@en , "Drum Major General (Scozia)"@it , "Drum Major General (Skotlanti)"@fi , "Drum Major General (Skottland)"@no , "Drum Major General (Skottland)"@sv , "Drum Major General (Szkocja)"@pl , "Drum Major General (Écosse)"@fr , "Drum Major General (Шотландия)"@ru ;
	owl:subClass :Rank_Drum_Major_General ;
	foaf:name "Drum Major General"@en .

:Rank_Drum_Major_General_Wales org:rankOf <dbpedia:Wales> ;
	a :MilitaryRank ;
	rdfs:comment "The specific instance of the Drum Major General rank in the context of country Wales."@en ;
	rdfs:label "Drum Major General (Gales)"@es , "Drum Major General (Galles)"@it , "Drum Major General (Pays de Galles)"@fr , "Drum Major General (País de Gales)"@pt , "Drum Major General (Wales)"@de , "Drum Major General (Wales)"@en , "Drum Major General (Wales)"@fi , "Drum Major General (Wales)"@nl , "Drum Major General (Wales)"@no , "Drum Major General (Wales)"@sv , "Drum Major General (Walia)"@pl , "Drum Major General (Уэльс)"@ru ;
	owl:subClass :Rank_Drum_Major_General ;
	foaf:name "Drum Major General"@en .

:Rank_Drum_major a :MilitaryRank ;
	rdfs:comment "The title Drum Major is an appointment, not a military rank."@en ;
	rdfs:label "Drum major (rank)"@en ;
	owl:sameAs <dbpedia:Drum_major_%28rank%29> ;
	foaf:name "Drum major" .

:Rank_Drum_major_Commonwealth_of_Nations org:rankOf <dbpedia:Commonwealth_of_Nations> ;
	a :MilitaryRank ;
	rdfs:comment "The specific instance of the Drum major (rank) rank in the context of country Commonwealth of Nations."@en ;
	rdfs:label "Drum major (rank) (Commonwealth delle nazioni)"@it , "Drum major (rank) (Commonwealth of Nations)"@de , "Drum major (rank) (Commonwealth of Nations)"@en , "Drum major (rank) (Commonwealth of Nations)"@fr , "Drum major (rank) (Commonwealth)"@pt , "Drum major (rank) (Gemenebest van Naties)"@nl , "Drum major (rank) (Kansainyhteisö)"@fi , "Drum major (rank) (Mancomunidad de Naciones)"@es , "Drum major (rank) (Samveldet av nasjoner)"@no , "Drum major (rank) (Samväldet)"@sv , "Drum major (rank) (Wspólnota Narodów)"@pl , "Drum major (rank) (Содружество наций)"@ru ;
	owl:subClass :Rank_Drum_major ;
	foaf:name "Drum major"@en .

:Rank_Drum_major_England org:rankOf <dbpedia:England> ;
	a :MilitaryRank ;
	rdfs:comment "The specific instance of the Drum major (rank) rank in the context of England."@en ;
	rdfs:label "Drum major (rank, England)"@en ;
	owl:subClass :Rank_Drum_major ;
	foaf:name "Drum major"@en .

:Rank_Drum_major_Scotland org:rankOf <dbpedia:Scotland> ;
	a :MilitaryRank ;
	rdfs:comment "The specific instance of the Drum major (rank) rank in the context of country Scotland."@en ;
	rdfs:label "Drum major (rank) (Escocia)"@es , "Drum major (rank) (Escócia)"@pt , "Drum major (rank) (Schotland)"@nl , "Drum major (rank) (Schottland)"@de , "Drum major (rank) (Scotland)"@en , "Drum major (rank) (Scozia)"@it , "Drum major (rank) (Skotlanti)"@fi , "Drum major (rank) (Skottland)"@no , "Drum major (rank) (Skottland)"@sv , "Drum major (rank) (Szkocja)"@pl , "Drum major (rank) (Écosse)"@fr , "Drum major (rank) (Шотландия)"@ru ;
	owl:subClass :Rank_Drum_major ;
	foaf:name "Drum major"@en .

:Rank_Drum_major_Wales org:rankOf <dbpedia:Wales> ;
	a :MilitaryRank ;
	rdfs:comment "The specific instance of the Drum major (rank) rank in the context of country Wales."@en ;
	rdfs:label "Drum major (rank) (Gales)"@es , "Drum major (rank) (Galles)"@it , "Drum major (rank) (Pays de Galles)"@fr , "Drum major (rank) (País de Gales)"@pt , "Drum major (rank) (Wales)"@de , "Drum major (rank) (Wales)"@en , "Drum major (rank) (Wales)"@fi , "Drum major (rank) (Wales)"@nl , "Drum major (rank) (Wales)"@no , "Drum major (rank) (Wales)"@sv , "Drum major (rank) (Walia)"@pl , "Drum major (rank) (Уэльс)"@ru ;
	owl:subClass :Rank_Drum_major ;
	foaf:name "Drum major"@en .

<http://rdf.muninn-project.org/ontologies/military#Rank_Ensign_(rank)_EnglishTradition> org:rankEquivalentTo :Rank_Pilot_officer_EnglishTradition , :Rank_Second_lieutenant_EnglishTradition ;
	org:rankJuniorToTransitive :Rank_Sub-lieutenant_EnglishTradition ;
	org:rankOf :EnglishTradition , <mil:NavyServiceBranch> ;
	org:rankSeniorToTransitive :Rank_Midshipman_EnglishTradition ;
	a :MilitaryRank ;
	owl:sameAs <dbpedia:Ensign_(rank)> .

:Rank_Epihipparch a :MilitaryRank ;
	rdfs:comment "Epihipparch is an Ancient Greek military title for a cavalry commander of 1,000 horse. This unit was divided into two hipparchiai of 500. Each of these was commanded by a hipparchos."@en ;
	rdfs:label "Epihipparch"@en ;
	owl:sameAs <dbpedia:Epihipparch> ;
	foaf:name "Epihipparch" .

:Rank_Epihipparch_Achaean_League org:rankOf <dbpedia:Achaean_League> ;
	a :MilitaryRank ;
	rdfs:comment "The specific instance of the Epihipparch rank in the context of country Achaean League."@en ;
	rdfs:label "Epihipparch (Achaean League)"@en , "Epihipparch (Achaeïsche Bond)"@nl , "Epihipparch (Achaiischer Bund)"@de , "Epihipparch (Achaiska förbundet)"@sv , "Epihipparch (Akhaian liitto)"@fi , "Epihipparch (Det akhaiske forbund)"@no , "Epihipparch (Lega achea)"@it , "Epihipparch (Liga Aquea)"@es , "Epihipparch (Liga Aqueia)"@pt , "Epihipparch (Ligue achéenne)"@fr , "Epihipparch (Związek Achajski)"@pl , "Epihipparch (Ахейский союз)"@ru ;
	owl:subClass :Rank_Epihipparch ;
	foaf:name "Epihipparch"@en .

:Rank_Epihipparch_Macedonia org:rankOf <dbpedia:Macedonia_%28ancient_kingdom%29> ;
	a :MilitaryRank ;
	rdfs:comment "The specific instance of the Epihipparch rank in the context of country Macedonia (ancient kingdom)."@en ;
	rdfs:label "Epihipparch (Macedonia (ancient kingdom))"@en , "Epihipparch (Macedonië (oudheid))"@nl , "Epihipparch (Macedónia Antiga)"@pt , "Epihipparch (Makedonian valtakunta)"@fi , "Epihipparch (Oldtidens Makedonia)"@no , "Epihipparch (Regno di Macedonia)"@it , "Epihipparch (Reino de Macedonia)"@es , "Epihipparch (Royaume de Macédoine)"@fr , "Epihipparch (Starożytna Macedonia)"@pl , "Epihipparch (Древняя Македония)"@ru ;
	owl:subClass :Rank_Epihipparch ;
	foaf:name "Epihipparch"@en .

:Rank_Ferik a :MilitaryRank ;
	rdfs:comment "Ferik was a military rank of the Ottoman Army. It is translated as Major General or Lieutenant General (Korgeneral). It was superior to a Mirliva (\"Brigadier\") and junior to a Birinci Ferik (\"First Ferik/General\"). The title of Ferik was abolished with Act No. 2590 of 26 November 1934 on the Abolition of Titles and Appellations such as Efendi, Bey or Pasha."@en ;
	rdfs:label "Ferik (rank)"@en ;
	owl:sameAs <dbpedia:Ferik_%28rank%29> ;
	foaf:name "Ferik" .

:Rank_Ferik_Cossack_Hetmanate org:rankOf <dbpedia:Cossack_Hetmanate> ;
	a :MilitaryRank ;
	rdfs:comment "The specific instance of the Ferik (rank) rank in the context of country Cossack Hetmanate."@en ;
	rdfs:label "Ferik (rank) (Cossack Hetmanate)"@en , "Ferik (rank) (Hetmanat cosaque)"@fr , "Ferik (rank) (Hetmanat)"@de , "Ferik (rank) (Hetmanato cosaco)"@es , "Ferik (rank) (Hetmańszczyzna)"@pl , "Ferik (rank) (Гетманщина)"@ru ;
	owl:subClass :Rank_Ferik ;
	foaf:name "Ferik"@en .

:Rank_Ferik_Ottoman_Empire org:rankOf <dbpedia:Ottoman_Empire> ;
	a :MilitaryRank ;
	rdfs:comment "The specific instance of the Ferik (rank) rank in the context of country Ottoman Empire."@en ;
	rdfs:label "Ferik (rank) (Det osmanske rike)"@no , "Ferik (rank) (Empire ottoman)"@fr , "Ferik (rank) (Imperio otomano)"@es , "Ferik (rank) (Imperium osmańskie)"@pl , "Ferik (rank) (Impero ottomano)"@it , "Ferik (rank) (Império Otomano)"@pt , "Ferik (rank) (Osmanien valtakunta)"@fi , "Ferik (rank) (Osmanisches Reich)"@de , "Ferik (rank) (Osmanska riket)"@sv , "Ferik (rank) (Ottomaanse Rijk)"@nl , "Ferik (rank) (Ottoman Empire)"@en , "Ferik (rank) (Османская империя)"@ru ;
	owl:subClass :Rank_Ferik ;
	foaf:name "Ferik"@en .

:Rank_Ferik_Septinsular_Republic org:rankOf <dbpedia:Septinsular_Republic> ;
	a :MilitaryRank ;
	rdfs:comment "The specific instance of the Ferik (rank) rank in the context of country Septinsular Republic."@en ;
	rdfs:label "Ferik (rank) (Repubblica delle Sette Isole Unite)"@it , "Ferik (rank) (Republiek van de Zeven Eilanden)"@nl , "Ferik (rank) (Republika Siedmiu Wysp)"@pl , "Ferik (rank) (República de las Islas Jónicas)"@es , "Ferik (rank) (République des Sept-Îles)"@fr , "Ferik (rank) (Septinsular Republic)"@en , "Ferik (rank) (Республика Семи Островов)"@ru ;
	owl:subClass :Rank_Ferik ;
	foaf:name "Ferik"@en .

:Rank_Field_marshal_EnglishTradition org:rankEquivalentTo :Rank_Admiral_of_the_fleet_EnglishTradition , :Rank_Marshal_of_the_air_force_EnglishTradition ;
	org:rankOf :EnglishTradition , <mil:ArmyServiceBranch> ;
	org:rankSeniorToTransitive :Rank_General_officer_EnglishTradition ;
	a :MilitaryRank ;
	rdfs:label "Field marshal"@en ;
	owl:sameAs <dbpedia:Field_marshal> .

:Rank_Fleet_Board a :MilitaryRank ;
	rdfs:comment "Fleet Board is a term in the Royal Navy for the examination cadet officers take which qualifies them to become commissioned officers. After passing the examination, officers who entered as sub-lieutenants have their commissions backdated to the date when they entered the Royal Navy. Midshipmen are also considered commissioned officers at this point, but are not immediately promoted to sub-lieutenant."@en ;
	rdfs:label "Fleet Board"@en ;
	owl:sameAs <dbpedia:Fleet_Board> ;
	foaf:name "Fleet Board" .

:Rank_Fleet_Board_England org:rankOf <dbpedia:England> ;
	a :MilitaryRank ;
	rdfs:comment "The specific instance of the Fleet Board rank in the context of England."@en ;
	rdfs:label "Fleet Board (England)"@en ;
	owl:subClass :Rank_Fleet_Board ;
	foaf:name "Fleet Board"@en .

:Rank_Fleet_Board_Scotland org:rankOf <dbpedia:Scotland> ;
	a :MilitaryRank ;
	rdfs:comment "The specific instance of the Fleet Board rank in the context of country Scotland."@en ;
	rdfs:label "Fleet Board (Escocia)"@es , "Fleet Board (Escócia)"@pt , "Fleet Board (Schotland)"@nl , "Fleet Board (Schottland)"@de , "Fleet Board (Scotland)"@en , "Fleet Board (Scozia)"@it , "Fleet Board (Skotlanti)"@fi , "Fleet Board (Skottland)"@no , "Fleet Board (Skottland)"@sv , "Fleet Board (Szkocja)"@pl , "Fleet Board (Écosse)"@fr , "Fleet Board (Шотландия)"@ru ;
	owl:subClass :Rank_Fleet_Board ;
	foaf:name "Fleet Board"@en .

:Rank_Fleet_Board_Wales org:rankOf <dbpedia:Wales> ;
	a :MilitaryRank ;
	rdfs:comment "The specific instance of the Fleet Board rank in the context of country Wales."@en ;
	rdfs:label "Fleet Board (Gales)"@es , "Fleet Board (Galles)"@it , "Fleet Board (Pays de Galles)"@fr , "Fleet Board (País de Gales)"@pt , "Fleet Board (Wales)"@de , "Fleet Board (Wales)"@en , "Fleet Board (Wales)"@fi , "Fleet Board (Wales)"@nl , "Fleet Board (Wales)"@no , "Fleet Board (Wales)"@sv , "Fleet Board (Walia)"@pl , "Fleet Board (Уэльс)"@ru ;
	owl:subClass :Rank_Fleet_Board ;
	foaf:name "Fleet Board"@en .

:Rank_Flight_lieutenant_EnglishTradition org:rankEquivalentTo :Rank_Captain_EnglishTradition , <http://rdf.muninn-project.org/ontologies/military#Rank_Lieutenant_(navy)_EnglishTradition> ;
	org:rankJuniorToTransitive :Rank_Squadron_leader_EnglishTradition ;
	org:rankOf :EnglishTradition , <mil:AirForceServiceBranch> ;
	org:rankSeniorToTransitive :Rank_Flying_officer_EnglishTradition ;
	a :MilitaryRank ;
	rdfs:label "Flight lieutenant"@en ;
	owl:sameAs <dbpedia:Flight_lieutenant> .

:Rank_Flight_sergeant a :MilitaryRank ;
	rdfs:label "Flight sergeant"@en ;
	owl:sameAs <dbpedia:Flight_sergeant> ;
	foaf:name "Flight sergeant" .

:Rank_Flight_sergeant_Australia org:rankOf <dbpedia:Australia> ;
	a :MilitaryRank ;
	rdfs:comment "The specific instance of the Flight sergeant rank in the context of country Australia."@en ;
	rdfs:label "Flight sergeant (Australia)"@en , "Flight sergeant (Australia)"@es , "Flight sergeant (Australia)"@fi , "Flight sergeant (Australia)"@it , "Flight sergeant (Australia)"@no , "Flight sergeant (Australia)"@pl , "Flight sergeant (Australie)"@fr , "Flight sergeant (Australien)"@de , "Flight sergeant (Australien)"@sv , "Flight sergeant (Australië (land))"@nl , "Flight sergeant (Austrália)"@pt , "Flight sergeant (Австралия)"@ru ;
	owl:subClass :Rank_Flight_sergeant ;
	foaf:name "Flight sergeant"@en .

:Rank_Flight_sergeant_Canada org:rankOf <dbpedia:Canada> ;
	a :MilitaryRank ;
	rdfs:comment "The specific instance of the Flight sergeant rank in the context of Canada."@en ;
	rdfs:label "Flight sergeant (Canada)"@en ;
	owl:subClass :Rank_Flight_sergeant ;
	foaf:name "Flight sergeant"@en .

:Rank_Flight_sergeant_Commonwealth_of_Nations org:rankOf <dbpedia:Commonwealth_of_Nations> ;
	a :MilitaryRank ;
	rdfs:comment "The specific instance of the Flight sergeant rank in the context of country Commonwealth of Nations."@en ;
	rdfs:label "Flight sergeant (Commonwealth delle nazioni)"@it , "Flight sergeant (Commonwealth of Nations)"@de , "Flight sergeant (Commonwealth of Nations)"@en , "Flight sergeant (Commonwealth of Nations)"@fr , "Flight sergeant (Commonwealth)"@pt , "Flight sergeant (Gemenebest van Naties)"@nl , "Flight sergeant (Kansainyhteisö)"@fi , "Flight sergeant (Mancomunidad de Naciones)"@es , "Flight sergeant (Samveldet av nasjoner)"@no , "Flight sergeant (Samväldet)"@sv , "Flight sergeant (Wspólnota Narodów)"@pl , "Flight sergeant (Содружество наций)"@ru ;
	owl:subClass :Rank_Flight_sergeant ;
	foaf:name "Flight sergeant"@en .

:Rank_Flight_sergeant_Republic_of_Ireland org:rankOf <dbpedia:Republic_of_Ireland> ;
	a :MilitaryRank ;
	rdfs:comment "The specific instance of the Flight sergeant rank in the context of country Republic of Ireland."@en ;
	rdfs:label "Flight sergeant (Ierland (land))"@nl , "Flight sergeant (Irland)"@de , "Flight sergeant (Irland)"@no , "Flight sergeant (Irland)"@sv , "Flight sergeant (Irlanda)"@es , "Flight sergeant (Irlanda)"@it , "Flight sergeant (Irlande (pays))"@fr , "Flight sergeant (Irlandia)"@pl , "Flight sergeant (Irlanti)"@fi , "Flight sergeant (Republic of Ireland)"@en , "Flight sergeant (República da Irlanda)"@pt , "Flight sergeant (Ирландия)"@ru ;
	owl:subClass :Rank_Flight_sergeant ;
	foaf:name "Flight sergeant"@en .

:Rank_Flying_officer_EnglishTradition org:rankEquivalentTo :Rank_Lieutenant_EnglishTradition , :Rank_Sub-lieutenant_EnglishTradition ;
	org:rankJuniorToTransitive :Rank_Flight_lieutenant_EnglishTradition ;
	org:rankOf :EnglishTradition , <mil:AirForceServiceBranch> ;
	org:rankSeniorToTransitive :Rank_Pilot_officer_EnglishTradition ;
	a :MilitaryRank ;
	rdfs:label "Flying officer"@en ;
	owl:sameAs <dbpedia:Flying_officer> .

:Rank_Garrison_Sergeant_Major a :MilitaryRank ;
	rdfs:comment "A Garrison Sergeant Major (GSM) in the British Army is the senior warrant officer of a garrison and holds the rank of Warrant Officer Class 1. The GSM London District, always a guardsman, holds one of the four most senior WO1 appointments in the British Army, and has military ceremonial responsibility for important state occasions such as Trooping the Colour."@en ;
	rdfs:label "Garrison Sergeant Major"@en ;
	owl:sameAs <dbpedia:Garrison_Sergeant_Major> ;
	foaf:name "Garrison Sergeant Major" .

:Rank_Garrison_Sergeant_Major_England org:rankOf <dbpedia:England> ;
	a :MilitaryAppointment , :MilitaryRank ;
	rdfs:comment "The specific instance of the Garrison Sergeant Major rank in the context of England."@en ;
	rdfs:label "Garrison Sergeant Major (England)"@en ;
	owl:subClass :Rank_Garrison_Sergeant_Major ;
	foaf:name "Garrison Sergeant Major"@en .

:Rank_Garrison_Sergeant_Major_Scotland org:rankOf <dbpedia:Scotland> ;
	a :MilitaryRank ;
	rdfs:comment "The specific instance of the Garrison Sergeant Major rank in the context of country Scotland."@en ;
	rdfs:label "Garrison Sergeant Major (Escocia)"@es , "Garrison Sergeant Major (Escócia)"@pt , "Garrison Sergeant Major (Schotland)"@nl , "Garrison Sergeant Major (Schottland)"@de , "Garrison Sergeant Major (Scotland)"@en , "Garrison Sergeant Major (Scozia)"@it , "Garrison Sergeant Major (Skotlanti)"@fi , "Garrison Sergeant Major (Skottland)"@no , "Garrison Sergeant Major (Skottland)"@sv , "Garrison Sergeant Major (Szkocja)"@pl , "Garrison Sergeant Major (Écosse)"@fr , "Garrison Sergeant Major (Шотландия)"@ru ;
	owl:subClass :Rank_Garrison_Sergeant_Major ;
	foaf:name "Garrison Sergeant Major"@en .

:Rank_Garrison_Sergeant_Major_Wales org:rankOf <dbpedia:Wales> ;
	a :MilitaryRank ;
	rdfs:comment "The specific instance of the Garrison Sergeant Major rank in the context of country Wales."@en ;
	rdfs:label "Garrison Sergeant Major (Gales)"@es , "Garrison Sergeant Major (Galles)"@it , "Garrison Sergeant Major (Pays de Galles)"@fr , "Garrison Sergeant Major (País de Gales)"@pt , "Garrison Sergeant Major (Wales)"@de , "Garrison Sergeant Major (Wales)"@en , "Garrison Sergeant Major (Wales)"@fi , "Garrison Sergeant Major (Wales)"@nl , "Garrison Sergeant Major (Wales)"@no , "Garrison Sergeant Major (Wales)"@sv , "Garrison Sergeant Major (Walia)"@pl , "Garrison Sergeant Major (Уэльс)"@ru ;
	owl:subClass :Rank_Garrison_Sergeant_Major ;
	foaf:name "Garrison Sergeant Major"@en .

:Rank_Gefreiter a :MilitaryRank ;
	rdfs:comment "Gefreiter is the German, Swiss and Austrian equivalent for the military rank Private (NATO Rank Code OR-2). Gefreiter was the lowest rank to which an ordinary soldier could be promoted. As a military rank it has existed since at least the 16th century. From the 1920s on Gefreiter has expanded into several additional ranks, those being Obergefreiter, Hauptgefreiter, Stabsgefreiter and Oberstabsgefreiter (NATO Rank Code OR-3 and OR-4). Gefreiter means \"the exempted\"."@en ;
	rdfs:label "Gefrajter"@pl , "Gefreiter"@de , "Gefreiter"@en , "Gefreiter"@no , "Ефрейтор"@ru ;
	owl:sameAs <dbpedia:Gefreiter> ;
	foaf:name "Gefreiter" .

:Rank_Gefreiter_Germany org:rankOf <dbpedia:Germany> ;
	a :MilitaryRank ;
	rdfs:comment "The specific instance of the Gefreiter rank in the context of Germany."@en ;
	rdfs:label "Gefrajter (Germany)"@pl , "Gefreiter (Germany)"@de , "Gefreiter (Germany)"@en , "Gefreiter (Germany)"@no , "Ефрейтор (Germany)"@ru ;
	owl:subClass :Rank_Gefreiter ;
	foaf:name "Gefreiter"@de .

:Rank_Gefreiter_Russia org:rankOf <dbpedia:Russia> ;
	a :MilitaryRank ;
	rdfs:comment "The specific instance of the Gefreiter rank in the context of country Russia."@en ;
	rdfs:label "Gefrajter (Rosja)"@pl , "Gefreiter (Rusia)"@es , "Gefreiter (Rusland)"@nl , "Gefreiter (Russia)"@en , "Gefreiter (Russia)"@it , "Gefreiter (Russie)"@fr , "Gefreiter (Russland)"@de , "Gefreiter (Russland)"@no , "Gefreiter (Ryssland)"@sv , "Gefreiter (Rússia)"@pt , "Gefreiter (Venäjä)"@fi , "Ефрейтор (Россия)"@ru ;
	owl:subClass :Rank_Gefreiter ;
	foaf:name "Ефрейтор"@ru .

:Rank_Gefreiter_Soviet_Union org:rankOf <dbpedia:Soviet_Union> ;
	a :MilitaryRank ;
	rdfs:comment "The specific instance of the Gefreiter rank in the context of country Soviet Union."@en ;
	rdfs:label "Gefrajter (Związek Socjalistycznych Republik Radzieckich)"@pl , "Gefreiter (Neuvostoliitto)"@fi , "Gefreiter (Soviet Union)"@en , "Gefreiter (Sovjet-Unie)"@nl , "Gefreiter (Sovjetunionen)"@no , "Gefreiter (Sovjetunionen)"@sv , "Gefreiter (Sowjetunion)"@de , "Gefreiter (Union des républiques socialistes soviétiques)"@fr , "Gefreiter (Unione Sovietica)"@it , "Gefreiter (União Soviética)"@pt , "Gefreiter (Unión Soviética)"@es , "Ефрейтор (Союз Советских Социалистических Республик)"@ru ;
	owl:subClass :Rank_Gefreiter ;
	foaf:name "Gefreiter"@en .

:Rank_General-in-Chief a :MilitaryRank ;
	rdfs:comment "General-in-Chief has been a military rank or title in various armed forces around the world."@en ;
	rdfs:label "General en chef"@sv , "General-in-Chief"@en , "Генерал-аншеф"@ru ;
	owl:sameAs <dbpedia:General-in-Chief> ;
	foaf:name "General-in-Chief" .

:Rank_General-in-Chief_Russia org:rankOf <dbpedia:Russia> ;
	a :MilitaryRank ;
	rdfs:comment "The specific instance of the General-in-Chief rank in the context of country Russia."@en ;
	rdfs:label "General en chef (Ryssland)"@sv , "General-in-Chief (Rosja)"@pl , "General-in-Chief (Rusia)"@es , "General-in-Chief (Rusland)"@nl , "General-in-Chief (Russia)"@en , "General-in-Chief (Russia)"@it , "General-in-Chief (Russie)"@fr , "General-in-Chief (Russland)"@de , "General-in-Chief (Russland)"@no , "General-in-Chief (Rússia)"@pt , "General-in-Chief (Venäjä)"@fi , "Генерал-аншеф (Россия)"@ru ;
	owl:subClass :Rank_General-in-Chief ;
	foaf:name "Генерал-аншеф"@ru .

:Rank_General-in-Chief_Soviet_Union org:rankOf <dbpedia:Soviet_Union> ;
	a :MilitaryRank ;
	rdfs:comment "The specific instance of the General-in-Chief rank in the context of country Soviet Union."@en ;
	rdfs:label "General en chef (Sovjetunionen)"@sv , "General-in-Chief (Neuvostoliitto)"@fi , "General-in-Chief (Soviet Union)"@en , "General-in-Chief (Sovjet-Unie)"@nl , "General-in-Chief (Sovjetunionen)"@no , "General-in-Chief (Sowjetunion)"@de , "General-in-Chief (Union des républiques socialistes soviétiques)"@fr , "General-in-Chief (Unione Sovietica)"@it , "General-in-Chief (União Soviética)"@pt , "General-in-Chief (Unión Soviética)"@es , "General-in-Chief (Związek Socjalistycznych Republik Radzieckich)"@pl , "Генерал-аншеф (Союз Советских Социалистических Республик)"@ru ;
	owl:subClass :Rank_General-in-Chief ;
	foaf:name "General-in-Chief"@en .

:Rank_General_Admiral a :MilitaryRank ;
	rdfs:comment "General Admiral was a Danish, Dutch, German, Russian, Portuguese, Spanish and Swedish naval rank. Its historic origin is a title high military or naval dignitaries of early modern Europe sometimes held, for example the (nominal) Commander-in-Chief of the Dutch Republic's navy."@en ;
	rdfs:label "Admiraal-generaal"@nl , "Almirante General"@es , "General Admiral"@en , "Generaladmiral"@de , "Kenraaliamiraali"@fi , "Генерал-адмирал"@ru ;
	owl:sameAs <dbpedia:General_Admiral> ;
	foaf:name "General Admiral" .

:Rank_General_Admiral_Germany org:rankOf <dbpedia:Germany> ;
	a :MilitaryRank ;
	rdfs:comment "The specific instance of the General Admiral rank in the context of Germany."@en ;
	rdfs:label "Admiraal-generaal (Germany)"@nl , "Almirante General (Germany)"@es , "General Admiral (Germany)"@en , "Generaladmiral (Germany)"@de , "Kenraaliamiraali (Germany)"@fi , "Генерал-адмирал (Germany)"@ru ;
	owl:subClass :Rank_General_Admiral ;
	foaf:name "Generaladmiral"@de .

:Rank_General_Admiral_Russia org:rankOf <dbpedia:Russia> ;
	a :MilitaryRank ;
	rdfs:comment "The specific instance of the General Admiral rank in the context of country Russia."@en ;
	rdfs:label "Admiraal-generaal (Rusland)"@nl , "Almirante General (Rusia)"@es , "General Admiral (Rosja)"@pl , "General Admiral (Russia)"@en , "General Admiral (Russia)"@it , "General Admiral (Russie)"@fr , "General Admiral (Russland)"@no , "General Admiral (Ryssland)"@sv , "General Admiral (Rússia)"@pt , "Generaladmiral (Russland)"@de , "Kenraaliamiraali (Venäjä)"@fi , "Генерал-адмирал (Россия)"@ru ;
	owl:subClass :Rank_General_Admiral ;
	foaf:name "Генерал-адмирал"@ru .

:Rank_General_Admiral_Soviet_Union org:rankOf <dbpedia:Soviet_Union> ;
	a :MilitaryRank ;
	rdfs:comment "The specific instance of the General Admiral rank in the context of country Soviet Union."@en ;
	rdfs:label "Admiraal-generaal (Sovjet-Unie)"@nl , "Almirante General (Unión Soviética)"@es , "General Admiral (Soviet Union)"@en , "General Admiral (Sovjetunionen)"@no , "General Admiral (Sovjetunionen)"@sv , "General Admiral (Union des républiques socialistes soviétiques)"@fr , "General Admiral (Unione Sovietica)"@it , "General Admiral (União Soviética)"@pt , "General Admiral (Związek Socjalistycznych Republik Radzieckich)"@pl , "Generaladmiral (Sowjetunion)"@de , "Kenraaliamiraali (Neuvostoliitto)"@fi , "Генерал-адмирал (Союз Советских Социалистических Республик)"@ru ;
	owl:subClass :Rank_General_Admiral ;
	foaf:name "General Admiral"@en .

:Rank_General_officer_EnglishTradition org:rankEquivalentTo :Rank_Admiral_EnglishTradition , :Rank_Air_marshal_EnglishTradition ;
	org:rankJuniorToTransitive :Rank_Field_marshal_EnglishTradition ;
	org:rankOf :EnglishTradition , <mil:ArmyServiceBranch> ;
	org:rankSeniorToTransitive :Rank_Brigadier_EnglishTradition ;
	a :MilitaryRank ;
	rdfs:comment "A general officer is an officer of high military rank, usually in the army, and in some nations, the air force. The term is widely used by many nations of the world, and when a country uses a different term, there is an equivalent title given. The term General is used in two ways: as the generic title for all grades of general officer; and as a specific rank. Since the late twentieth century, the rank of General is usually the highest active rank of a military not at war."@en ;
	rdfs:label "General"@de , "General officer"@en , "Général"@fr ;
	owl:sameAs <dbpedia:General_officer> .

:Rank_Group_captain_EnglishTradition org:rankEquivalentTo <http://rdf.muninn-project.org/ontologies/military#Rank_Captain_(naval)_EnglishTradition> , :Rank_Colonel_EnglishTradition ;
	org:rankJuniorToTransitive :Rank_Air_commodore_EnglishTradition ;
	org:rankOf :EnglishTradition , <mil:AirForceServiceBranch> ;
	org:rankSeniorToTransitive <http://rdf.muninn-project.org/ontologies/military#Rank_Wing_commander_(rank)_EnglishTradition> ;
	a :MilitaryRank ;
	rdfs:label "Group captain"@en ;
	owl:sameAs <dbpedia:Group_captain> .

:Rank_Hasa a :MilitaryRank ;
	rdfs:comment "Hasa is a Korean military rank which is used in both the armed forces of North and South Korea. In both countries, the rank is considered the first non-commissioned officer grade and is generally considered the equivalent of a Corporal or Sergeant in western militaries."@en ;
	rdfs:label "Hasa (Korean military)"@en ;
	owl:sameAs <dbpedia:Hasa_%28Korean_military%29> ;
	foaf:name "Hasa" .

:Rank_Hasa_North_Korea org:rankOf <dbpedia:North_Korea> ;
	a :MilitaryRank ;
	rdfs:comment "The specific instance of the Hasa (Korean military) rank in the context of country North Korea."@en ;
	rdfs:label "Hasa (Korean military) (Corea del Nord)"@it , "Hasa (Korean military) (Corea del Norte)"@es , "Hasa (Korean military) (Coreia do Norte)"@pt , "Hasa (Korean military) (Corée du Nord)"@fr , "Hasa (Korean military) (Korea Północna)"@pl , "Hasa (Korean military) (Korean demokraattinen kansantasavalta)"@fi , "Hasa (Korean military) (Noord-Korea)"@nl , "Hasa (Korean military) (Nord-Korea)"@no , "Hasa (Korean military) (Nordkorea)"@de , "Hasa (Korean military) (Nordkorea)"@sv , "Hasa (Korean military) (North Korea)"@en , "Hasa (Korean military) (Корейская Народно-Демократическая Республика)"@ru ;
	owl:subClass :Rank_Hasa ;
	foaf:name "Hasa"@en .

:Rank_Hasa_South_Korea org:rankOf <dbpedia:South_Korea> ;
	a :MilitaryRank ;
	rdfs:comment "The specific instance of the Hasa (Korean military) rank in the context of country South Korea."@en ;
	rdfs:label "Hasa (Korean military) (Corea del Sud)"@it , "Hasa (Korean military) (Corea del Sur)"@es , "Hasa (Korean military) (Coreia do Sul)"@pt , "Hasa (Korean military) (Corée du Sud)"@fr , "Hasa (Korean military) (Korea Południowa)"@pl , "Hasa (Korean military) (Korean tasavalta)"@fi , "Hasa (Korean military) (South Korea)"@en , "Hasa (Korean military) (Sydkorea)"@sv , "Hasa (Korean military) (Sør-Korea)"@no , "Hasa (Korean military) (Südkorea)"@de , "Hasa (Korean military) (Zuid-Korea)"@nl , "Hasa (Korean military) (Республика Корея)"@ru ;
	owl:subClass :Rank_Hasa ;
	foaf:name "Hasa"@en .

:Rank_Havildar org:rankOf <mil:Infantry> ;
	a :MilitaryRank ;
	rdfs:comment "Havildar, roughly equivalent to a Sergeant"@en ;
	rdfs:label "Havildar"@en , "हविलदार"@hi ;
	owl:sameAs <dbpedia:Havildar> ;
	foaf:name "Havildar"@en .

:Rank_Havildar_British_India org:rankOf <dbpedia:British_Indian_Army> , <dbpedia:British_Raj> , <mil:Infantry> ;
	a :MilitaryRank ;
	rdfs:comment "Havildar, roughly equivalent to a Sergeant"@en ;
	rdfs:label "Havildar"@en , "हविलदार"@hi ;
	foaf:name "Havildar"@en .

:Rank_Hetman a :MilitaryRank ;
	rdfs:comment "Hetman was the title of the second-highest military commander in 15th- to 18th-century Poland and the Grand Duchy of Lithuania, which together, from 1569 to 1795, comprised the Polish-Lithuanian Commonwealth, or Rzeczpospolita. \"Hetman\" was also the highest military office, and head of state, in Ukraine's Cossack Hetmanate. The title (гетьман) was used by Ukraine's Cossacks from the 16th century, and by the Czechs (hejtman) in Bohemia from the Hussite Wars (15th century) on."@en ;
	rdfs:label "Hetman"@de , "Hetman"@en , "Hetman"@es , "Hetman"@fr , "Hetman"@nl , "Hetman"@no , "Hetman"@pl , "Hetman"@pt , "Hetman"@sv , "Hetmani"@fi , "Гетман"@ru ;
	owl:sameAs <dbpedia:Hetman> ;
	foaf:name "Hetman" .

:Rank_Hetman_Belarus org:rankOf <dbpedia:Belarus> ;
	a :MilitaryRank ;
	rdfs:comment "The specific instance of the Hetman rank in the context of country Belarus."@en ;
	rdfs:label "Hetman (Belarus)"@en , "Hetman (Białoruś)"@pl , "Hetman (Bielorrusia)"@es , "Hetman (Bielorrússia)"@pt , "Hetman (Bielorussia)"@it , "Hetman (Biélorussie)"@fr , "Hetman (Hviterussland)"@no , "Hetman (Vitryssland)"@sv , "Hetman (Weißrussland)"@de , "Hetman (Wit-Rusland)"@nl , "Hetmani (Valko-Venäjä)"@fi , "Гетман (Белоруссия)"@ru ;
	owl:subClass :Rank_Hetman ;
	foaf:name "Гетман"@ru .

:Rank_Hetman_Lithuania org:rankOf <dbpedia:Lithuania> ;
	a :MilitaryRank ;
	rdfs:comment "The specific instance of the Hetman rank in the context of country Lithuania."@en ;
	rdfs:label "Hetman (Litauen)"@de , "Hetman (Litauen)"@no , "Hetman (Litauen)"@sv , "Hetman (Lithuania)"@en , "Hetman (Litouwen)"@nl , "Hetman (Lituania)"@es , "Hetman (Lituania)"@it , "Hetman (Lituanie)"@fr , "Hetman (Lituânia)"@pt , "Hetman (Litwa)"@pl , "Hetmani (Liettua)"@fi , "Гетман (Литва)"@ru ;
	owl:subClass :Rank_Hetman ;
	foaf:name "Hetman"@en .

:Rank_Hetman_Poland org:rankOf <dbpedia:Poland> ;
	a :MilitaryRank ;
	rdfs:comment "The specific instance of the Hetman rank in the context of Poland."@en ;
	rdfs:label "Hetman (Poland)"@de , "Hetman (Poland)"@en , "Hetman (Poland)"@es , "Hetman (Poland)"@fr , "Hetman (Poland)"@nl , "Hetman (Poland)"@no , "Hetman (Poland)"@pl , "Hetman (Poland)"@pt , "Hetman (Poland)"@sv , "Hetmani (Poland)"@fi , "Гетман (Poland)"@ru ;
	owl:subClass :Rank_Hetman ;
	foaf:name "Hetman"@en .

:Rank_Hetman_Ukraine org:rankOf <dbpedia:Ukraine> ;
	a :MilitaryRank ;
	rdfs:comment "The specific instance of the Hetman rank in the context of country Ukraine."@en ;
	rdfs:label "Hetman (Oekraïne)"@nl , "Hetman (Ucraina)"@it , "Hetman (Ucrania)"@es , "Hetman (Ucrânia)"@pt , "Hetman (Ukraina)"@no , "Hetman (Ukraina)"@pl , "Hetman (Ukraina)"@sv , "Hetman (Ukraine)"@de , "Hetman (Ukraine)"@en , "Hetman (Ukraine)"@fr , "Hetmani (Ukraina)"@fi , "Гетман (Украина)"@ru ;
	owl:subClass :Rank_Hetman ;
	foaf:name "Гетман"@ru .

:Rank_Hipparchus_Cavalry a :MilitaryRank ;
	rdfs:comment "A Hipparchus or Hipparch was the title of an ancient Greek cavalry officer, commanding a hipparchia (unit of about 500 horsemen); two such units were commanded by an Epihipparchos."@en ;
	rdfs:label "Hiparco (oficial de caballería)"@es , "Hipparchos"@nl , "Hipparchus (cavalry officer)"@en , "Гиппарх (военачальник)"@ru ;
	owl:sameAs <dbpedia:Hipparchus_%28cavalry_officer%29> ;
	foaf:name "Hipparchus" .

:Rank_Hipparchus_Cavalry_Achaean_League org:rankOf <dbpedia:Achaean_League> ;
	a :MilitaryRank ;
	rdfs:comment "The specific instance of the Hipparchus (cavalry officer) rank in the context of country Achaean League."@en ;
	rdfs:label "Hiparco (oficial de caballería) (Liga Aquea)"@es , "Hipparchos (Achaeïsche Bond)"@nl , "Hipparchus (cavalry officer) (Achaean League)"@en , "Hipparchus (cavalry officer) (Achaiischer Bund)"@de , "Hipparchus (cavalry officer) (Achaiska förbundet)"@sv , "Hipparchus (cavalry officer) (Akhaian liitto)"@fi , "Hipparchus (cavalry officer) (Det akhaiske forbund)"@no , "Hipparchus (cavalry officer) (Lega achea)"@it , "Hipparchus (cavalry officer) (Liga Aqueia)"@pt , "Hipparchus (cavalry officer) (Ligue achéenne)"@fr , "Hipparchus (cavalry officer) (Związek Achajski)"@pl , "Гиппарх (военачальник) (Ахейский союз)"@ru ;
	owl:subClass :Rank_Hipparchus_Cavalry ;
	foaf:name "Hipparchus"@en .

:Rank_Hipparchus_Cavalry_Macedonia org:rankOf <dbpedia:Macedonia_%28ancient_kingdom%29> ;
	a :MilitaryRank ;
	rdfs:comment "The specific instance of the Hipparchus (cavalry officer) rank in the context of country Macedonia (ancient kingdom)."@en ;
	rdfs:label "Hiparco (oficial de caballería) (Reino de Macedonia)"@es , "Hipparchos (Macedonië (oudheid))"@nl , "Hipparchus (cavalry officer) (Macedonia (ancient kingdom))"@en , "Hipparchus (cavalry officer) (Macedónia Antiga)"@pt , "Hipparchus (cavalry officer) (Makedonian valtakunta)"@fi , "Hipparchus (cavalry officer) (Oldtidens Makedonia)"@no , "Hipparchus (cavalry officer) (Regno di Macedonia)"@it , "Hipparchus (cavalry officer) (Royaume de Macédoine)"@fr , "Hipparchus (cavalry officer) (Starożytna Macedonia)"@pl , "Гиппарх (военачальник) (Древняя Македония)"@ru ;
	owl:subClass :Rank_Hipparchus_Cavalry ;
	foaf:name "Hipparchus"@en .

:Rank_Jungsa a :MilitaryRank ;
	rdfs:comment "Jungsa is a Korean military rank used by the armed forces of South and North Koreas. A Jungsa is the equivalent to a Sergeant First Class. The rank of Jungsa is junior to a Sangsa in North and South Korea."@en ;
	rdfs:label "Jungsa"@en ;
	owl:sameAs <dbpedia:Jungsa> ;
	foaf:name "Jungsa" .

:Rank_Jungsa_North_Korea org:rankOf <dbpedia:North_Korea> ;
	a :MilitaryRank ;
	rdfs:comment "The specific instance of the Jungsa rank in the context of country North Korea."@en ;
	rdfs:label "Jungsa (Corea del Nord)"@it , "Jungsa (Corea del Norte)"@es , "Jungsa (Coreia do Norte)"@pt , "Jungsa (Corée du Nord)"@fr , "Jungsa (Korea Północna)"@pl , "Jungsa (Korean demokraattinen kansantasavalta)"@fi , "Jungsa (Noord-Korea)"@nl , "Jungsa (Nord-Korea)"@no , "Jungsa (Nordkorea)"@de , "Jungsa (Nordkorea)"@sv , "Jungsa (North Korea)"@en , "Jungsa (Корейская Народно-Демократическая Республика)"@ru ;
	owl:subClass :Rank_Jungsa ;
	foaf:name "Jungsa"@en .

:Rank_Jungsa_South_Korea org:rankOf <dbpedia:South_Korea> ;
	a :MilitaryRank ;
	rdfs:comment "The specific instance of the Jungsa rank in the context of country South Korea."@en ;
	rdfs:label "Jungsa (Corea del Sud)"@it , "Jungsa (Corea del Sur)"@es , "Jungsa (Coreia do Sul)"@pt , "Jungsa (Corée du Sud)"@fr , "Jungsa (Korea Południowa)"@pl , "Jungsa (Korean tasavalta)"@fi , "Jungsa (South Korea)"@en , "Jungsa (Sydkorea)"@sv , "Jungsa (Sør-Korea)"@no , "Jungsa (Südkorea)"@de , "Jungsa (Zuid-Korea)"@nl , "Jungsa (Республика Корея)"@ru ;
	owl:subClass :Rank_Jungsa ;
	foaf:name "Jungsa"@en .

:Rank_Jungwi a :MilitaryRank ;
	rdfs:comment "Chungwi (중위) is the second most junior Korean officer rank in both the militaries of North and South Korea. It is considered the equivalent of a First Lieutenant in most other militaries."@en ;
	rdfs:label "Jungwi"@en , "Jungwi"@no ;
	owl:sameAs <dbpedia:Jungwi> ;
	foaf:name "Jungwi" .

:Rank_Jungwi_North_Korea org:rankOf <dbpedia:North_Korea> ;
	a :MilitaryRank ;
	rdfs:comment "The specific instance of the Jungwi rank in the context of country North Korea."@en ;
	rdfs:label "Jungwi (Corea del Nord)"@it , "Jungwi (Corea del Norte)"@es , "Jungwi (Coreia do Norte)"@pt , "Jungwi (Corée du Nord)"@fr , "Jungwi (Korea Północna)"@pl , "Jungwi (Korean demokraattinen kansantasavalta)"@fi , "Jungwi (Noord-Korea)"@nl , "Jungwi (Nord-Korea)"@no , "Jungwi (Nordkorea)"@de , "Jungwi (Nordkorea)"@sv , "Jungwi (North Korea)"@en , "Jungwi (Корейская Народно-Демократическая Республика)"@ru ;
	owl:subClass :Rank_Jungwi ;
	foaf:name "Jungwi"@en .

:Rank_Jungwi_South_Korea org:rankOf <dbpedia:South_Korea> ;
	a :MilitaryRank ;
	rdfs:comment "The specific instance of the Jungwi rank in the context of country South Korea."@en ;
	rdfs:label "Jungwi (Corea del Sud)"@it , "Jungwi (Corea del Sur)"@es , "Jungwi (Coreia do Sul)"@pt , "Jungwi (Corée du Sud)"@fr , "Jungwi (Korea Południowa)"@pl , "Jungwi (Korean tasavalta)"@fi , "Jungwi (South Korea)"@en , "Jungwi (Sydkorea)"@sv , "Jungwi (Sør-Korea)"@no , "Jungwi (Südkorea)"@de , "Jungwi (Zuid-Korea)"@nl , "Jungwi (Республика Корея)"@ru ;
	owl:subClass :Rank_Jungwi ;
	foaf:name "Jungwi"@en .

:Rank_Junior_sergeant a :MilitaryRank ;
	rdfs:label "Junior Sergeant"@en ;
	owl:sameAs <dbpedia:Junior_sergeant> ;
	foaf:name "Junior Sergeant" .

:Rank_Junior_sergeant_Estonia org:rankOf <dbpedia:Estonia> ;
	a :MilitaryRank ;
	rdfs:comment "The specific instance of the  rank in the context of country Estonia."@en ;
	rdfs:label " (Estland)"@de , " (Estland)"@nl , " (Estland)"@no , " (Estland)"@sv , " (Estonia)"@en , " (Estonia)"@es , " (Estonia)"@it , " (Estonia)"@pl , " (Estonie)"@fr , " (Estónia)"@pt , " (Viro)"@fi , " (Эстония)"@ru ;
	owl:subClass :Rank_Junior_sergeant ;
	foaf:name ""@en .

:Rank_Junior_sergeant_Republic_of_Estonia_1920-1940 org:rankOf <dbpedia:Republic_of_Estonia_%281920-1940%29> ;
	a :MilitaryRank ;
	rdfs:comment "The specific instance of the  rank in the context of country ."@en ;
	owl:subClass :Rank_Junior_sergeant ;
	foaf:name ""@en .

:Rank_Junjang a :MilitaryRank ;
	rdfs:label "Junjang"@en ;
	owl:sameAs <dbpedia:Junjang> ;
	foaf:name "Junjang" .

:Rank_Junjang_North_Korea org:rankOf <dbpedia:North_Korea> ;
	a :MilitaryRank ;
	rdfs:comment "The specific instance of the Junjang rank in the context of country North Korea."@en ;
	rdfs:label "Junjang (Corea del Nord)"@it , "Junjang (Corea del Norte)"@es , "Junjang (Coreia do Norte)"@pt , "Junjang (Corée du Nord)"@fr , "Junjang (Korea Północna)"@pl , "Junjang (Korean demokraattinen kansantasavalta)"@fi , "Junjang (Noord-Korea)"@nl , "Junjang (Nord-Korea)"@no , "Junjang (Nordkorea)"@de , "Junjang (Nordkorea)"@sv , "Junjang (North Korea)"@en , "Junjang (Корейская Народно-Демократическая Республика)"@ru ;
	owl:subClass :Rank_Junjang ;
	foaf:name "Junjang"@en .

:Rank_Junjang_South_Korea org:rankOf <dbpedia:South_Korea> ;
	a :MilitaryRank ;
	rdfs:comment "The specific instance of the Junjang rank in the context of country South Korea."@en ;
	rdfs:label "Junjang (Corea del Sud)"@it , "Junjang (Corea del Sur)"@es , "Junjang (Coreia do Sul)"@pt , "Junjang (Corée du Sud)"@fr , "Junjang (Korea Południowa)"@pl , "Junjang (Korean tasavalta)"@fi , "Junjang (South Korea)"@en , "Junjang (Sydkorea)"@sv , "Junjang (Sør-Korea)"@no , "Junjang (Südkorea)"@de , "Junjang (Zuid-Korea)"@nl , "Junjang (Республика Корея)"@ru ;
	owl:subClass :Rank_Junjang ;
	foaf:name "Junjang"@en .

:Rank_Kapudan_Pasha a :MilitaryRank ;
	rdfs:comment "Kapudan Pasha or Kapudan-i Derya were the titles given to the chief commander of the navy in the Ottoman Empire. The title Kapudan-i Derya was first granted during the reign of Bayezid I as an official rank within the state structure. Starting with the reign of Mehmed II, holders of the rank were accorded the status of viziers and held the title of Pasha, thus they were more often called Kapudan Pasha."@en ;
	rdfs:label "Capitan pacha"@fr , "Kapudan Pascha"@de , "Kapudan Pasha"@en , "Капудан-паша"@ru ;
	owl:sameAs <dbpedia:Kapudan_Pasha> ;
	foaf:name "Kapudan Pasha" .

:Rank_Kapudan_Pasha_Cossack_Hetmanate org:rankOf <dbpedia:Cossack_Hetmanate> ;
	a :MilitaryRank ;
	rdfs:comment "The specific instance of the Kapudan Pasha rank in the context of country Cossack Hetmanate."@en ;
	rdfs:label "Capitan pacha (Hetmanat cosaque)"@fr , "Kapudan Pascha (Hetmanat)"@de , "Kapudan Pasha (Cossack Hetmanate)"@en , "Kapudan Pasha (Hetmanato cosaco)"@es , "Kapudan Pasha (Hetmańszczyzna)"@pl , "Капудан-паша (Гетманщина)"@ru ;
	owl:subClass :Rank_Kapudan_Pasha ;
	foaf:name "Kapudan Pasha"@en .

:Rank_Kapudan_Pasha_Ottoman_Empire org:rankOf <dbpedia:Ottoman_Empire> ;
	a :MilitaryRank ;
	rdfs:comment "The specific instance of the Kapudan Pasha rank in the context of country Ottoman Empire."@en ;
	rdfs:label "Capitan pacha (Empire ottoman)"@fr , "Kapudan Pascha (Osmanisches Reich)"@de , "Kapudan Pasha (Det osmanske rike)"@no , "Kapudan Pasha (Imperio otomano)"@es , "Kapudan Pasha (Imperium osmańskie)"@pl , "Kapudan Pasha (Impero ottomano)"@it , "Kapudan Pasha (Império Otomano)"@pt , "Kapudan Pasha (Osmanien valtakunta)"@fi , "Kapudan Pasha (Osmanska riket)"@sv , "Kapudan Pasha (Ottomaanse Rijk)"@nl , "Kapudan Pasha (Ottoman Empire)"@en , "Капудан-паша (Османская империя)"@ru ;
	owl:subClass :Rank_Kapudan_Pasha ;
	foaf:name "Kapudan Pasha"@en .

:Rank_Kapudan_Pasha_Septinsular_Republic org:rankOf <dbpedia:Septinsular_Republic> ;
	a :MilitaryRank ;
	rdfs:comment "The specific instance of the Kapudan Pasha rank in the context of country Septinsular Republic."@en ;
	rdfs:label "Capitan pacha (République des Sept-Îles)"@fr , "Kapudan Pascha (Septinsular Republic)"@de , "Kapudan Pasha (Repubblica delle Sette Isole Unite)"@it , "Kapudan Pasha (Republiek van de Zeven Eilanden)"@nl , "Kapudan Pasha (Republika Siedmiu Wysp)"@pl , "Kapudan Pasha (República de las Islas Jónicas)"@es , "Kapudan Pasha (Septinsular Republic)"@en , "Капудан-паша (Республика Семи Островов)"@ru ;
	owl:subClass :Rank_Kapudan_Pasha ;
	foaf:name "Kapudan Pasha"@en .

:Rank_Kindral a :MilitaryRank ;
	rdfs:comment "Kindral is the Estonian word for General which is also the highest military position in the Republic of Estonia. Both Ground Force and Air Force superior officers ranks share the same names which have been combined with the military rank of general and other senior officer ranks. There are four types of generals in the Estonia Defence Forces."@en ;
	rdfs:label "Kindral"@en ;
	owl:sameAs <dbpedia:Kindral> ;
	foaf:name "Kindral" .

:Rank_Kindral_Estonia org:rankOf <dbpedia:Estonia> ;
	a :MilitaryRank ;
	rdfs:comment "The specific instance of the Kindral rank in the context of country Estonia."@en ;
	rdfs:label "Kindral (Estland)"@de , "Kindral (Estland)"@nl , "Kindral (Estland)"@no , "Kindral (Estland)"@sv , "Kindral (Estonia)"@en , "Kindral (Estonia)"@es , "Kindral (Estonia)"@it , "Kindral (Estonia)"@pl , "Kindral (Estonie)"@fr , "Kindral (Estónia)"@pt , "Kindral (Viro)"@fi , "Kindral (Эстония)"@ru ;
	owl:subClass :Rank_Kindral ;
	foaf:name "Kindral"@en .

:Rank_Kindral_Republic_of_Estonia_1920-1940 org:rankOf <dbpedia:Republic_of_Estonia_%281920-1940%29> ;
	a :MilitaryRank ;
	rdfs:comment "The specific instance of the Kindral rank in the context of the Republic of Estonia, 1920-1940."@en ;
	rdfs:label "Kindral (Republic of Estonia, 1920-1940)"@en ;
	owl:subClass :Rank_Kindral ;
	foaf:name "Kindral"@en .

:Rank_Kolagasi a :MilitaryRank ;
	rdfs:comment "Kolağası (also written as Kol Ağsı, Kol Aghasi) was a military rank of the Ottoman Army. It corresponds to a Senior Captain or an Adjutant Major. Kol Ağası is a compound word composed of Kol and Ağa. The rank was junior to the Binbaşı (Major) and superior to the Yüzbaşı (Captain). The rank of Kol Ağası was changed to Önyüzbaşı in Republican period."@en ;
	rdfs:label "Kolağası"@en ;
	owl:sameAs <dbpedia:Kola%C4%9Fas%C4%B1> ;
	foaf:name "Kolağası" .

:Rank_Kolagasi_Cossack_Hetmanate org:rankOf <dbpedia:Cossack_Hetmanate> ;
	a :MilitaryRank ;
	rdfs:comment "The specific instance of the Kolağası rank in the context of country Cossack Hetmanate."@en ;
	rdfs:label "Kolağası (Cossack Hetmanate)"@en , "Kolağası (Hetmanat cosaque)"@fr , "Kolağası (Hetmanat)"@de , "Kolağası (Hetmanato cosaco)"@es , "Kolağası (Hetmańszczyzna)"@pl , "Kolağası (Гетманщина)"@ru ;
	owl:subClass :Rank_Kolagasi ;
	foaf:name "Kolağası"@en .

:Rank_Kolagasi_Ottoman_Empire org:rankOf <dbpedia:Ottoman_Empire> ;
	a :MilitaryRank ;
	rdfs:comment "The specific instance of the Kolağası rank in the context of country Ottoman Empire."@en ;
	rdfs:label "Kolağası (Det osmanske rike)"@no , "Kolağası (Empire ottoman)"@fr , "Kolağası (Imperio otomano)"@es , "Kolağası (Imperium osmańskie)"@pl , "Kolağası (Impero ottomano)"@it , "Kolağası (Império Otomano)"@pt , "Kolağası (Osmanien valtakunta)"@fi , "Kolağası (Osmanisches Reich)"@de , "Kolağası (Osmanska riket)"@sv , "Kolağası (Ottomaanse Rijk)"@nl , "Kolağası (Ottoman Empire)"@en , "Kolağası (Османская империя)"@ru ;
	owl:subClass :Rank_Kolagasi ;
	foaf:name "Kolağası"@en .

:Rank_Kolagasi_Septinsular_Republic org:rankOf <dbpedia:Septinsular_Republic> ;
	a :MilitaryRank ;
	rdfs:comment "The specific instance of the Kolağası rank in the context of country Septinsular Republic."@en ;
	rdfs:label "Kolağası (Repubblica delle Sette Isole Unite)"@it , "Kolağası (Republiek van de Zeven Eilanden)"@nl , "Kolağası (Republika Siedmiu Wysp)"@pl , "Kolağası (República de las Islas Jónicas)"@es , "Kolağası (République des Sept-Îles)"@fr , "Kolağası (Septinsular Republic)"@en , "Kolağası (Республика Семи Островов)"@ru ;
	owl:subClass :Rank_Kolagasi ;
	foaf:name "Kolağası"@en .

:Rank_Kolonel a :MilitaryRank ;
	rdfs:comment "Kolonel is a rank of the Belgium, Malaysia, Estonia and Netherlands which corresponds to the rank of Colonel in other countries."@en ;
	rdfs:label "Kolonel"@en ;
	owl:sameAs <dbpedia:Kolonel> ;
	foaf:name "Kolonel" .

:Rank_Kolonel_Belgium org:rankOf <dbpedia:Belgium> ;
	a :MilitaryRank ;
	rdfs:comment "The specific instance of the Kolonel rank in the context of country Belgium."@en ;
	rdfs:label "Kolonel (Belgia)"@fi , "Kolonel (Belgia)"@no , "Kolonel (Belgia)"@pl , "Kolonel (Belgien)"@de , "Kolonel (Belgien)"@sv , "Kolonel (Belgio)"@it , "Kolonel (Belgique)"@fr , "Kolonel (Belgium)"@en , "Kolonel (België)"@nl , "Kolonel (Bélgica)"@es , "Kolonel (Bélgica)"@pt , "Kolonel (Бельгия)"@ru ;
	owl:subClass :Rank_Kolonel ;
	foaf:name "Kolonel"@en .

:Rank_Kolonel_Estonia org:rankOf <dbpedia:Estonia> ;
	a :MilitaryRank ;
	rdfs:comment "The specific instance of the Kolonel rank in the context of country Estonia."@en ;
	rdfs:label "Kolonel (Estland)"@de , "Kolonel (Estland)"@nl , "Kolonel (Estland)"@no , "Kolonel (Estland)"@sv , "Kolonel (Estonia)"@en , "Kolonel (Estonia)"@es , "Kolonel (Estonia)"@it , "Kolonel (Estonia)"@pl , "Kolonel (Estonie)"@fr , "Kolonel (Estónia)"@pt , "Kolonel (Viro)"@fi , "Kolonel (Эстония)"@ru ;
	owl:subClass :Rank_Kolonel ;
	foaf:name "Kolonel"@en .

:Rank_Kolonel_Netherlands org:rankOf <dbpedia:Netherlands> ;
	a :MilitaryRank ;
	rdfs:comment "The specific instance of the Kolonel rank in the context of country Netherlands."@en ;
	rdfs:label "Kolonel (Alankomaat)"@fi , "Kolonel (Holandia)"@pl , "Kolonel (Nederland)"@nl , "Kolonel (Nederland)"@no , "Kolonel (Nederländerna)"@sv , "Kolonel (Netherlands)"@en , "Kolonel (Niederlande)"@de , "Kolonel (Paesi Bassi)"@it , "Kolonel (Pays-Bas)"@fr , "Kolonel (Países Baixos)"@pt , "Kolonel (Países Bajos)"@es , "Kolonel (Нидерланды)"@ru ;
	owl:subClass :Rank_Kolonel ;
	foaf:name "Kolonel"@en .

:Rank_Kolonel_Republic_of_Estonia_1920-1940 org:rankOf <dbpedia:Republic_of_Estonia_%281920-1940%29> ;
	a :MilitaryRank ;
	rdfs:comment "The specific instance of the Kolonel rank in the context of the Republic of Estonia, 1920-1940."@en ;
	rdfs:label "Kolonel (Republic of Estonia, 1920-1940)"@en ;
	owl:subClass :Rank_Kolonel ;
	foaf:name "Kolonel"@en .

:Rank_Lance-corporal_of_horse org:rankOf <mil:HouseholdCavalry> ;
	a :MilitaryRank ;
	rdfs:label "Lance Corporal of Horse"@en ;
	owl:sameAs <dbpedia:Lance-corporal_of_horse> ;
	foaf:name "Lance Corporal of Horse" .

:Rank_Lance-corporal_of_horse_England org:rankOf <dbpedia:England> ;
	a :MilitaryRank ;
	rdfs:comment "The specific instance of the  rank in the context of England."@en ;
	rdfs:label "Lance Corporal of Horse (England)"@en ;
	owl:subClass :Rank_Lance-corporal_of_horse ;
	foaf:name "Lance Corporal of Horse"@en .

:Rank_Lance-corporal_of_horse_Scotland org:rankOf <dbpedia:Scotland> ;
	a :MilitaryRank ;
	rdfs:comment "The specific instance of the Lance Corporal of Horse rank in the context of country Scotland."@en ;
	rdfs:label "Lance Corporal of Horse (Escocia)"@es , "Lance Corporal of Horse (Escócia)"@pt , "Lance Corporal of Horse (Schotland)"@nl , "Lance Corporal of Horse (Schottland)"@de , "Lance Corporal of Horse (Scotland)"@en , "Lance Corporal of Horse (Scozia)"@it , "Lance Corporal of Horse (Skotlanti)"@fi , "Lance Corporal of Horse (Skottland)"@no , "Lance Corporal of Horse (Skottland)"@sv , "Lance Corporal of Horse (Szkocja)"@pl , "Lance Corporal of Horse (Écosse)"@fr , "Lance Corporal of Horse (Шотландия)"@ru ;
	owl:subClass :Rank_Lance-corporal_of_horse ;
	foaf:name "Lance Corporal of Horse"@en .

:Rank_Lance-corporal_of_horse_Wales org:rankOf <dbpedia:Wales> ;
	a :MilitaryRank ;
	rdfs:comment "The specific instance of the Lance Corporal of Horse  rank in the context of country Wales."@en ;
	rdfs:label "Lance Corporal of Horse (Gales)"@es , "Lance Corporal of Horse (Galles)"@it , "Lance Corporal of Horse (Pays de Galles)"@fr , "Lance Corporal of Horse (País de Gales)"@pt , "Lance Corporal of Horse (Wales)"@de , "Lance Corporal of Horse (Wales)"@en , "Lance Corporal of Horse (Wales)"@fi , "Lance Corporal of Horse (Wales)"@nl , "Lance Corporal of Horse (Wales)"@no , "Lance Corporal of Horse (Wales)"@sv , "Lance Corporal of Horse (Walia)"@pl , "Lance Corporal of Horse (Уэльс)"@ru ;
	owl:subClass :Rank_Lance-corporal_of_horse ;
	foaf:name "Lance Corporal of Horse"@en .

:Rank_Lance_corporal a :MilitaryRank ;
	rdfs:label "Lance corporal"@en ;
	owl:sameAs <dbpedia:Lance_corporal> ;
	foaf:name "Lance corporal" .

:Rank_Lance_corporal_Australia org:rankOf <dbpedia:Australia> ;
	a :MilitaryRank ;
	rdfs:comment "The specific instance of the Lance corporal rank in the context of country Australia."@en ;
	rdfs:label "Lance corporal (Australia)"@en , "Lance corporal (Australia)"@es , "Lance corporal (Australia)"@fi , "Lance corporal (Australia)"@it , "Lance corporal (Australia)"@no , "Lance corporal (Australia)"@pl , "Lance corporal (Australie)"@fr , "Lance corporal (Australien)"@de , "Lance corporal (Australien)"@sv , "Lance corporal (Australië (land))"@nl , "Lance corporal (Austrália)"@pt , "Lance corporal (Австралия)"@ru ;
	owl:subClass :Rank_Lance_corporal ;
	foaf:name "Lance corporal"@en .

:Rank_Lance_corporal_Commonwealth_of_Nations org:rankOf <dbpedia:Commonwealth_of_Nations> ;
	a :MilitaryRank ;
	rdfs:comment "The specific instance of the Lance corporal rank in the context of country Commonwealth of Nations."@en ;
	rdfs:label "Lance corporal (Commonwealth delle nazioni)"@it , "Lance corporal (Commonwealth of Nations)"@de , "Lance corporal (Commonwealth of Nations)"@en , "Lance corporal (Commonwealth of Nations)"@fr , "Lance corporal (Commonwealth)"@pt , "Lance corporal (Gemenebest van Naties)"@nl , "Lance corporal (Kansainyhteisö)"@fi , "Lance corporal (Mancomunidad de Naciones)"@es , "Lance corporal (Samveldet av nasjoner)"@no , "Lance corporal (Samväldet)"@sv , "Lance corporal (Wspólnota Narodów)"@pl , "Lance corporal (Содружество наций)"@ru ;
	owl:subClass :Rank_Lance_corporal ;
	foaf:name "Lance corporal"@en .

:Rank_Lance_corporal_England org:rankOf <dbpedia:England> ;
	a :MilitaryRank ;
	rdfs:comment "The specific instance of the Lance corporal rank in the context of England"@en ;
	rdfs:label "Lance corporal (England)"@en ;
	owl:subClass :Rank_Lance_corporal ;
	foaf:name "Lance corporal"@en .

:Rank_Lance_corporal_Scotland org:rankOf <dbpedia:Scotland> ;
	a :MilitaryRank ;
	rdfs:comment "The specific instance of the Lance corporal rank in the context of country Scotland."@en ;
	rdfs:label "Lance corporal (Escocia)"@es , "Lance corporal (Escócia)"@pt , "Lance corporal (Schotland)"@nl , "Lance corporal (Schottland)"@de , "Lance corporal (Scotland)"@en , "Lance corporal (Scozia)"@it , "Lance corporal (Skotlanti)"@fi , "Lance corporal (Skottland)"@no , "Lance corporal (Skottland)"@sv , "Lance corporal (Szkocja)"@pl , "Lance corporal (Écosse)"@fr , "Lance corporal (Шотландия)"@ru ;
	owl:subClass :Rank_Lance_corporal ;
	foaf:name "Lance corporal"@en .

:Rank_Lance_corporal_Singapore org:rankOf <dbpedia:Singapore> ;
	a :MilitaryRank ;
	rdfs:comment "The specific instance of the Lance corporal rank in the context of country Singapore."@en ;
	rdfs:label "Lance corporal (Singapore)"@en , "Lance corporal (Singapore)"@fi , "Lance corporal (Singapore)"@it , "Lance corporal (Singapore)"@nl , "Lance corporal (Singapore)"@no , "Lance corporal (Singapore)"@sv , "Lance corporal (Singapour)"@fr , "Lance corporal (Singapur)"@de , "Lance corporal (Singapur)"@es , "Lance corporal (Singapur)"@pl , "Lance corporal (Singapura)"@pt , "Lance corporal (Сингапур)"@ru ;
	owl:subClass :Rank_Lance_corporal ;
	foaf:name "Lance corporal"@en .

:Rank_Lance_corporal_Wales org:rankOf <dbpedia:Wales> ;
	a :MilitaryRank ;
	rdfs:comment "The specific instance of the Lance corporal rank in the context of country Wales."@en ;
	rdfs:label "Lance corporal (Gales)"@es , "Lance corporal (Galles)"@it , "Lance corporal (Pays de Galles)"@fr , "Lance corporal (País de Gales)"@pt , "Lance corporal (Wales)"@de , "Lance corporal (Wales)"@en , "Lance corporal (Wales)"@fi , "Lance corporal (Wales)"@nl , "Lance corporal (Wales)"@no , "Lance corporal (Wales)"@sv , "Lance corporal (Walia)"@pl , "Lance corporal (Уэльс)"@ru ;
	owl:subClass :Rank_Lance_corporal ;
	foaf:name "Lance corporal"@en .

:Rank_Lance_sergeant a :MilitaryRank ;
	rdfs:label "Lance Sergeant"@en ;
	owl:sameAs <dbpedia:Lance_sergeant> ;
	foaf:name "Lance Sergeant" .

:Rank_Lance_sergeant_Australia org:rankOf <dbpedia:Australia> ;
	a :MilitaryRank ;
	rdfs:comment "The specific instance of the  rank in the context of country Australia."@en ;
	rdfs:label " (Australia)"@en , " (Australia)"@es , " (Australia)"@fi , " (Australia)"@it , " (Australia)"@no , " (Australia)"@pl , " (Australie)"@fr , " (Australien)"@de , " (Australien)"@sv , " (Australië (land))"@nl , " (Austrália)"@pt , " (Австралия)"@ru ;
	owl:subClass :Rank_Lance_sergeant ;
	foaf:name ""@en .

:Rank_Lance_sergeant_Commonwealth_of_Nations org:rankOf <dbpedia:Commonwealth_of_Nations> ;
	a :MilitaryRank ;
	rdfs:comment "The specific instance of the Lance Sergeant  rank in the context of country Commonwealth of Nations."@en ;
	rdfs:label "Lance Sergeant (Commonwealth delle nazioni)"@it , "Lance Sergeant (Commonwealth of Nations)"@de , "Lance Sergeant (Commonwealth of Nations)"@en , "Lance Sergeant (Commonwealth of Nations)"@fr , "Lance Sergeant (Commonwealth)"@pt , "Lance Sergeant (Gemenebest van Naties)"@nl , "Lance Sergeant (Kansainyhteisö)"@fi , "Lance Sergeant (Mancomunidad de Naciones)"@es , "Lance Sergeant (Samveldet av nasjoner)"@no , "Lance Sergeant (Samväldet)"@sv , "Lance Sergeant (Wspólnota Narodów)"@pl , "Lance Sergeant (Содружество наций)"@ru ;
	owl:subClass :Rank_Lance_sergeant ;
	foaf:name "Lance Sergeant"@en .

:Rank_Lance_sergeant_England org:rankOf <dbpedia:England> ;
	a :MilitaryRank ;
	rdfs:comment "The specific instance of the  rank in the context of England."@en ;
	rdfs:label "Lance Sergeant (England)"@en ;
	owl:subClass :Rank_Lance_sergeant ;
	foaf:name "Lance Sergeant"@en .

:Rank_Lance_sergeant_Scotland org:rankOf <dbpedia:Scotland> ;
	a :MilitaryRank ;
	rdfs:comment "The specific instance of the Lance Sergeant rank in the context of country Scotland."@en ;
	rdfs:label "Lance Sergeant (Escocia)"@es , "Lance Sergeant (Escócia)"@pt , "Lance Sergeant (Schotland)"@nl , "Lance Sergeant (Schottland)"@de , "Lance Sergeant (Scotland)"@en , "Lance Sergeant (Scozia)"@it , "Lance Sergeant (Skotlanti)"@fi , "Lance Sergeant (Skottland)"@no , "Lance Sergeant (Skottland)"@sv , "Lance Sergeant (Szkocja)"@pl , "Lance Sergeant (Écosse)"@fr , "Lance Sergeant (Шотландия)"@ru ;
	owl:subClass :Rank_Lance_sergeant ;
	foaf:name "Lance Sergeant"@en .

:Rank_Lance_sergeant_Wales org:rankOf <dbpedia:Wales> ;
	a :MilitaryRank ;
	rdfs:comment "The specific instance of the Lance Sergeant rank in the context of country Wales."@en ;
	rdfs:label "Lance Sergeant (Gales)"@es , "Lance Sergeant (Galles)"@it , "Lance Sergeant (Pays de Galles)"@fr , "Lance Sergeant (País de Gales)"@pt , "Lance Sergeant (Wales)"@de , "Lance Sergeant (Wales)"@en , "Lance Sergeant (Wales)"@fi , "Lance Sergeant (Wales)"@nl , "Lance Sergeant (Wales)"@no , "Lance Sergeant (Wales)"@sv , "Lance Sergeant (Walia)"@pl , "Lance Sergeant (Уэльс)"@ru ;
	owl:subClass :Rank_Lance_sergeant ;
	foaf:name "Lance Sergeant"@en .

:Rank_Leading_aircraftman a :MilitaryRank ;
	rdfs:label "Leading aircraftman"@en ;
	owl:sameAs <dbpedia:Leading_aircraftman> ;
	foaf:name "Leading aircraftman" .

:Rank_Leading_aircraftman_Australia org:rankOf <dbpedia:Australia> ;
	a :MilitaryRank ;
	rdfs:comment "The specific instance of the Leading aircraftman rank in the context of country Australia."@en ;
	rdfs:label "Leading aircraftman (Australia)"@en , "Leading aircraftman (Australia)"@es , "Leading aircraftman (Australia)"@fi , "Leading aircraftman (Australia)"@it , "Leading aircraftman (Australia)"@no , "Leading aircraftman (Australia)"@pl , "Leading aircraftman (Australie)"@fr , "Leading aircraftman (Australien)"@de , "Leading aircraftman (Australien)"@sv , "Leading aircraftman (Australië (land))"@nl , "Leading aircraftman (Austrália)"@pt , "Leading aircraftman (Австралия)"@ru ;
	owl:subClass :Rank_Leading_aircraftman ;
	foaf:name "Leading aircraftman"@en .

:Rank_Leading_aircraftman_Canada org:rankOf <dbpedia:Canada> ;
	a :MilitaryRank ;
	rdfs:comment "The specific instance of the Leading aircraftman rank in the context of Canada."@en ;
	rdfs:label "Leading aircraftman (Canada)"@en ;
	owl:subClass :Rank_Leading_aircraftman ;
	foaf:name "Leading aircraftman"@en .

:Rank_Leading_aircraftman_Commonwealth_of_Nations org:rankOf <dbpedia:Commonwealth_of_Nations> ;
	a :MilitaryRank ;
	rdfs:comment "The specific instance of the Leading aircraftman rank in the context of country Commonwealth of Nations."@en ;
	rdfs:label "Leading aircraftman (Commonwealth delle nazioni)"@it , "Leading aircraftman (Commonwealth of Nations)"@de , "Leading aircraftman (Commonwealth of Nations)"@en , "Leading aircraftman (Commonwealth of Nations)"@fr , "Leading aircraftman (Commonwealth)"@pt , "Leading aircraftman (Gemenebest van Naties)"@nl , "Leading aircraftman (Kansainyhteisö)"@fi , "Leading aircraftman (Mancomunidad de Naciones)"@es , "Leading aircraftman (Samveldet av nasjoner)"@no , "Leading aircraftman (Samväldet)"@sv , "Leading aircraftman (Wspólnota Narodów)"@pl , "Leading aircraftman (Содружество наций)"@ru ;
	owl:subClass :Rank_Leading_aircraftman ;
	foaf:name "Leading aircraftman"@en .

:Rank_Leading_seaman_EnglishTradition org:rankEquivalentTo :Rank_Corporal_EnglishTradition ;
	org:rankJuniorToTransitive :Rank_Petty_officer_EnglishTradition ;
	org:rankOf :EnglishTradition , <mil:NavyServiceBranch> ;
	org:rankSeniorToTransitive :Rank_Seaman_EnglishTradition ;
	a :MilitaryRank ;
	rdfs:label "Leading seaman"@en ;
	owl:sameAs <dbpedia:Leading_seaman> .

<http://rdf.muninn-project.org/ontologies/military#Rank_Lieutenant_(navy)_EnglishTradition> org:rankEquivalentTo :Rank_Captain_EnglishTradition , :Rank_Flight_lieutenant_EnglishTradition ;
	org:rankJuniorToTransitive :Rank_Lieutenant_commander_EnglishTradition ;
	org:rankOf :EnglishTradition , <mil:NavyServiceBranch> ;
	org:rankSeniorToTransitive :Rank_Sub-lieutenant_EnglishTradition ;
	a :MilitaryRank ;
	owl:sameAs <dbpedia:Lieutenant_(navy)> .

:Rank_Lieutenant_EnglishTradition org:rankEquivalentTo :Rank_Flying_officer_EnglishTradition , :Rank_Sub-lieutenant_EnglishTradition ;
	org:rankJuniorToTransitive :Rank_Captain_EnglishTradition ;
	org:rankOf :EnglishTradition , <mil:ArmyServiceBranch> ;
	org:rankSeniorToTransitive :Rank_Second_lieutenant_EnglishTradition ;
	a :MilitaryRank ;
	rdfs:comment "A Lieutenant is a commissioned officer in many nations' armed forces. Typically, the rank of lieutenant in naval usage is senior to the army rank. It is also used in fire services, emergency medical services, security services and police forces as a rank. Lieutenant may also appear as part of a title used in various other organizations with a codified command structure. It often designates someone who is \"second-in-command,\" and as such, may precede the name of the rank directly above it."@en ;
	rdfs:label "Leutnant"@de , "Lieutenant"@de , "Lieutenant"@en , "Lieutenant (grade militaire)"@fr ;
	owl:sameAs <dbpedia:Lieutenant> .

:Rank_Lieutenant_colonel_EnglishTradition org:rankEquivalentTo :Rank_Commander_EnglishTradition , <http://rdf.muninn-project.org/ontologies/military#Rank_Wing_commander_(rank)_EnglishTradition> ;
	org:rankJuniorToTransitive :Rank_Colonel_EnglishTradition ;
	org:rankOf :EnglishTradition , <mil:ArmyServiceBranch> ;
	org:rankSeniorToTransitive <http://rdf.muninn-project.org/ontologies/military#Rank_Commandant_(rank)_EnglishTradition> , :Rank_Major_EnglishTradition ;
	a :MilitaryRank ;
	rdfs:label "Lieutenant colonel"@en ;
	owl:sameAs <dbpedia:Lieutenant_colonel> .

:Rank_Lieutenant_commander_EnglishTradition org:rankEquivalentTo <http://rdf.muninn-project.org/ontologies/military#Rank_Commandant_(rank)_EnglishTradition> , :Rank_Major_EnglishTradition , :Rank_Squadron_leader_EnglishTradition ;
	org:rankJuniorToTransitive :Rank_Commander_EnglishTradition ;
	org:rankOf :EnglishTradition , <mil:NavyServiceBranch> ;
	org:rankSeniorToTransitive <http://rdf.muninn-project.org/ontologies/military#Rank_Lieutenant_(navy)_EnglishTradition> ;
	a :MilitaryRank ;
	rdfs:label "Lieutenant commander"@en ;
	owl:sameAs <dbpedia:Lieutenant_commander> .

:Rank_Lochagos a :MilitaryRank ;
	rdfs:comment "Lochagos is used in the Greek language to mean \"Captain\". More precisely, it means \"leader of a lochos\"."@en ;
	rdfs:label "Lochagos"@en ;
	owl:sameAs <dbpedia:Lochagos> ;
	foaf:name "Lochagos" .

:Rank_Lochagos_Achaean_League org:rankOf <dbpedia:Achaean_League> ;
	a :MilitaryRank ;
	rdfs:comment "The specific instance of the Lochagos rank in the context of country Achaean League."@en ;
	rdfs:label "Lochagos (Achaean League)"@en , "Lochagos (Achaeïsche Bond)"@nl , "Lochagos (Achaiischer Bund)"@de , "Lochagos (Achaiska förbundet)"@sv , "Lochagos (Akhaian liitto)"@fi , "Lochagos (Det akhaiske forbund)"@no , "Lochagos (Lega achea)"@it , "Lochagos (Liga Aquea)"@es , "Lochagos (Liga Aqueia)"@pt , "Lochagos (Ligue achéenne)"@fr , "Lochagos (Związek Achajski)"@pl , "Lochagos (Ахейский союз)"@ru ;
	owl:subClass :Rank_Lochagos ;
	foaf:name "Lochagos"@en .

:Rank_Lochagos_Greece org:rankOf <dbpedia:Greece> ;
	a :MilitaryRank ;
	rdfs:comment "The specific instance of the Lochagos rank in the context of country Greece."@en ;
	rdfs:label "Lochagos (Grecia)"@es , "Lochagos (Grecia)"@it , "Lochagos (Grecja)"@pl , "Lochagos (Greece)"@en , "Lochagos (Grekland)"@sv , "Lochagos (Griechenland)"@de , "Lochagos (Griekenland)"@nl , "Lochagos (Grèce)"@fr , "Lochagos (Grécia)"@pt , "Lochagos (Hellas)"@no , "Lochagos (Kreikka)"@fi , "Lochagos (Греция)"@ru ;
	owl:subClass :Rank_Lochagos ;
	foaf:name "Lochagos"@en .

:Rank_Lochagos_Macedonia org:rankOf <dbpedia:Macedonia_%28ancient_kingdom%29> ;
	a :MilitaryRank ;
	rdfs:comment "The specific instance of the Lochagos rank in the context of country Macedonia (ancient kingdom)."@en ;
	rdfs:label "Lochagos (Macedonia (ancient kingdom))"@en , "Lochagos (Macedonië (oudheid))"@nl , "Lochagos (Macedónia Antiga)"@pt , "Lochagos (Makedonian valtakunta)"@fi , "Lochagos (Oldtidens Makedonia)"@no , "Lochagos (Regno di Macedonia)"@it , "Lochagos (Reino de Macedonia)"@es , "Lochagos (Royaume de Macédoine)"@fr , "Lochagos (Starożytna Macedonia)"@pl , "Lochagos (Древняя Македония)"@ru ;
	owl:subClass :Rank_Lochagos ;
	foaf:name "Lochagos"@en .

:Rank_Lochagos_Official_Timocracy_of_Sapinetia org:rankOf <dbpedia:Official_Timocracy_of_Sapinetia> ;
	a :MilitaryRank ;
	rdfs:comment "The specific instance of the Lochagos rank in the context of the Timocracy of Sapinetia."@en ;
	rdfs:label "Lochagos (Timocracy of Sapinetia)"@en ;
	owl:subClass :Rank_Lochagos ;
	foaf:name "Lochagos"@en .

:Rank_Lord_High_Admiral_of_the_Wash a :MilitaryRank ;
	rdfs:comment "The position of Lord High Admiral of the Wash is an ancient hereditary naval office of England. In mediaeval times, the Lord High Admiral of the Wash was a nobleman with responsibility for the defence and protection of The Wash coast in north East Anglia. The post was granted to the le Strange family after the Norman Conquest. In the 16th century the post became obsolete and the Royal Navy took over the defence of the area."@en ;
	rdfs:label "Lord High Admiral of the Wash"@en ;
	owl:sameAs <dbpedia:Lord_High_Admiral_of_the_Wash> ;
	foaf:name "Lord High Admiral of the Wash" .

:Rank_Lord_High_Admiral_of_the_Wash_England org:rankOf <dbpedia:England> ;
	a :MilitaryRank ;
	rdfs:comment "The specific instance of the Lord High Admiral of the Wash rank in the context of England."@en ;
	rdfs:label "Lord High Admiral of the Wash (England)"@en ;
	owl:subClass :Rank_Lord_High_Admiral_of_the_Wash ;
	foaf:name "Lord High Admiral of the Wash"@en .

:Rank_Lord_High_Admiral_of_the_Wash_Scotland org:rankOf <dbpedia:Scotland> ;
	a :MilitaryRank ;
	rdfs:comment "The specific instance of the Lord High Admiral of the Wash rank in the context of country Scotland."@en ;
	rdfs:label "Lord High Admiral of the Wash (Escocia)"@es , "Lord High Admiral of the Wash (Escócia)"@pt , "Lord High Admiral of the Wash (Schotland)"@nl , "Lord High Admiral of the Wash (Schottland)"@de , "Lord High Admiral of the Wash (Scotland)"@en , "Lord High Admiral of the Wash (Scozia)"@it , "Lord High Admiral of the Wash (Skotlanti)"@fi , "Lord High Admiral of the Wash (Skottland)"@no , "Lord High Admiral of the Wash (Skottland)"@sv , "Lord High Admiral of the Wash (Szkocja)"@pl , "Lord High Admiral of the Wash (Écosse)"@fr , "Lord High Admiral of the Wash (Шотландия)"@ru ;
	owl:subClass :Rank_Lord_High_Admiral_of_the_Wash ;
	foaf:name "Lord High Admiral of the Wash"@en .

:Rank_Lord_High_Admiral_of_the_Wash_Wales org:rankOf <dbpedia:Wales> ;
	a :MilitaryRank ;
	rdfs:comment "The specific instance of the Lord High Admiral of the Wash rank in the context of country Wales."@en ;
	rdfs:label "Lord High Admiral of the Wash (Gales)"@es , "Lord High Admiral of the Wash (Galles)"@it , "Lord High Admiral of the Wash (Pays de Galles)"@fr , "Lord High Admiral of the Wash (País de Gales)"@pt , "Lord High Admiral of the Wash (Wales)"@de , "Lord High Admiral of the Wash (Wales)"@en , "Lord High Admiral of the Wash (Wales)"@fi , "Lord High Admiral of the Wash (Wales)"@nl , "Lord High Admiral of the Wash (Wales)"@no , "Lord High Admiral of the Wash (Wales)"@sv , "Lord High Admiral of the Wash (Walia)"@pl , "Lord High Admiral of the Wash (Уэльс)"@ru ;
	owl:subClass :Rank_Lord_High_Admiral_of_the_Wash ;
	foaf:name "Lord High Admiral of the Wash"@en .

:Rank_Major_EnglishTradition org:rankEquivalentTo :Rank_Lieutenant_commander_EnglishTradition , :Rank_Squadron_leader_EnglishTradition ;
	org:rankJuniorToTransitive :Rank_Lieutenant_colonel_EnglishTradition ;
	org:rankOf :EnglishTradition , <mil:ArmyServiceBranch> ;
	a :MilitaryRank ;
	rdfs:comment "Major is a rank of commissioned officer, with corresponding ranks existing in almost every military in the world. When used unhyphenated, in conjunction with no other indicator of rank, the term refers to the rank just senior to that of an Army captain and just below the rank of lieutenant colonel. It is considered the most junior of the field ranks. In some militaries, notably France, the rank is referred to as commandant, while in others it is known as \"captain-major\"."@en ;
	rdfs:label "Major"@de , "Major"@en , "Major"@fr ;
	owl:sameAs <dbpedia:Major> .

:Rank_Major_general a :MilitaryRank ;
	rdfs:label "Major general"@en ;
	owl:sameAs <dbpedia:Major_general> ;
	foaf:name "Major general" .

:Rank_Major_general_Australia org:rankOf <dbpedia:Australia> ;
	a :MilitaryRank ;
	rdfs:comment "The specific instance of the Major general rank in the context of country Australia."@en ;
	rdfs:label "Major general (Australia)"@en , "Major general (Australia)"@es , "Major general (Australia)"@fi , "Major general (Australia)"@it , "Major general (Australia)"@no , "Major general (Australia)"@pl , "Major general (Australie)"@fr , "Major general (Australien)"@de , "Major general (Australien)"@sv , "Major general (Australië (land))"@nl , "Major general (Austrália)"@pt , "Major general (Австралия)"@ru ;
	owl:subClass :Rank_Major_general ;
	foaf:name "Major general"@en .

:Rank_Major_general_Canada org:rankOf <dbpedia:Canada> ;
	a :MilitaryRank ;
	rdfs:comment "The specific instance of the Major general rank in the context of Canada."@en ;
	rdfs:label "Major general (Canada)"@en ;
	owl:subClass :Rank_Major_general ;
	foaf:name "Major general"@en .

:Rank_Marshal_EnglishTradition org:rankEquivalentTo :Rank_Admiral_of_the_fleet_EnglishTradition , :Rank_Marshal_of_the_air_force_EnglishTradition ;
	org:rankOf :EnglishTradition , <mil:ArmyServiceBranch> ;
	a :MilitaryRank ;
	rdfs:comment "Marshal (also spelled marshall, more commonly in British English than American English), is a word used in several official titles of various branches of society. The word is an ancient loan word from Old (Norman) French, cf. modern French maréchal, which in turn is a borrowing from Old Frankish *marhskalk \"stable boy, keeper, servant\", still continued by Middle Dutch maerscalc, marscal \"id. \", modern Dutch maarschalk \"military commander\" (the meaning is under French influence)."@en ;
	rdfs:label "Marschall"@de , "Marshal"@en , "Marshal"@fr , "Maréchal (armée)"@fr ;
	owl:sameAs <dbpedia:Marshal> .

:Rank_Marshal_of_the_Soviet_Union a :MilitaryRank ;
	rdfs:comment "Marshal of the Soviet Union was the de facto highest military rank of the Soviet Union. (The highest rank de jure, Generalissimus of the Soviet Union, was created for Joseph Stalin and held by him alone). The rank of Marshal of the Soviet Union was created in 1935 and abolished in 1991. Forty-one people held the rank of Marshal of the Soviet Union. The equivalent naval rank was Admiral of the Fleet of the Soviet Union."@en ;
	rdfs:label "Maarschalk van de Sovjet-Unie"@nl , "Marechal da União Soviética"@pt , "Maresciallo dell'Unione Sovietica"@it , "Mariscal de la Unión Soviética"@es , "Marschall der Sowjetunion"@de , "Marshal of the Soviet Union"@en , "Marskalk av Sovjetunionen"@no , "Marskalk av Sovjetunionen"@sv , "Marszałkowie ZSRR"@pl , "Maréchal de l'Union soviétique"@fr , "Neuvostoliiton marsalkka"@fi , "Маршал Советского Союза"@ru ;
	owl:sameAs <dbpedia:Marshal_of_the_Soviet_Union> ;
	foaf:name "Marshal of the Soviet Union" .

:Rank_Marshal_of_the_Soviet_Union_Soviet_Union org:rankOf <dbpedia:Soviet_Union> ;
	a :MilitaryRank ;
	rdfs:comment "The specific instance of the Marshal of the Soviet Union rank in the context of country Soviet Union."@en ;
	rdfs:label "Maarschalk van de Sovjet-Unie (Sovjet-Unie)"@nl , "Marechal da União Soviética (União Soviética)"@pt , "Maresciallo dell'Unione Sovietica (Unione Sovietica)"@it , "Mariscal de la Unión Soviética (Unión Soviética)"@es , "Marschall der Sowjetunion (Sowjetunion)"@de , "Marshal of the Soviet Union (Soviet Union)"@en , "Marskalk av Sovjetunionen (Sovjetunionen)"@no , "Marskalk av Sovjetunionen (Sovjetunionen)"@sv , "Marszałkowie ZSRR (Związek Socjalistycznych Republik Radzieckich)"@pl , "Maréchal de l'Union soviétique (Union des républiques socialistes soviétiques)"@fr , "Neuvostoliiton marsalkka (Neuvostoliitto)"@fi , "Маршал Советского Союза (Союз Советских Социалистических Республик)"@ru ;
	owl:subClass :Rank_Marshal_of_the_Soviet_Union ;
	foaf:name "Marshal of the Soviet Union"@en .

:Rank_Marshal_of_the_air_force_EnglishTradition org:rankEquivalentTo :Rank_Admiral_of_the_fleet_EnglishTradition , :Rank_Field_marshal_EnglishTradition , :Rank_Marshal_EnglishTradition ;
	org:rankOf :EnglishTradition , <mil:AirForceServiceBranch> ;
	org:rankSeniorToTransitive :Rank_Air_marshal_EnglishTradition ;
	a :MilitaryRank ;
	rdfs:label "Marshal of the air force"@en ;
	owl:sameAs <dbpedia:Marshal_of_the_air_force> .

:Rank_Master_warrant_officer a :MilitaryRank ;
	rdfs:label "Master Warrant Officer"@en ;
	owl:sameAs <dbpedia:Master_warrant_officer> ;
	foaf:name "Master Warrant Officer" .

:Rank_Master_warrant_officer_Canada org:rankOf <dbpedia:Canada> ;
	a :MilitaryRank ;
	rdfs:comment "The specific instance of the  Master Warrant Officerrank in the context of country Canada."@en ;
	rdfs:label "Master Warrant Officer (Canada)"@en ;
	owl:subClass :Rank_Master_warrant_officer ;
	foaf:name "Master Warrant Officer"@en .

:Rank_Master_warrant_officer_Singapore org:rankOf <dbpedia:Singapore> ;
	a :MilitaryRank ;
	rdfs:comment "The specific instance of the Master Warrant Officer rank in the context of country Singapore."@en ;
	rdfs:label "Master Warrant Officer (Singapore)"@en , "Master Warrant Officer (Singapore)"@fi , "Master Warrant Officer (Singapore)"@it , "Master Warrant Officer (Singapore)"@nl , "Master Warrant Officer (Singapore)"@no , "Master Warrant Officer (Singapore)"@sv , "Master Warrant Officer (Singapour)"@fr , "Master Warrant Officer (Singapur)"@de , "Master Warrant Officer (Singapur)"@es , "Master Warrant Officer (Singapur)"@pl , "Master Warrant Officer (Singapura)"@pt , "Master Warrant Officer (Сингапур)"@ru ;
	owl:subClass :Rank_Master_warrant_officer ;
	foaf:name "Master Warrant Officer"@en .

:Rank_Midshipman_EnglishTradition org:rankEquivalentTo :Rank_Officer_cadet_EnglishTradition ;
	org:rankJuniorToTransitive <http://rdf.muninn-project.org/ontologies/military#Rank_Ensign_(rank)_EnglishTradition> ;
	org:rankOf :EnglishTradition , <mil:NavyServiceBranch> ;
	org:rankSeniorToTransitive :Rank_Warrant_officer_EnglishTradition ;
	a :MilitaryRank ;
	rdfs:comment "A midshipman is an officer cadet, or a commissioned officer of the lowest rank, in the Royal Navy, United States Navy, and many Commonwealth navies. Commonwealth countries which use the rank include Australia, New Zealand, South Africa, Pakistan, India, Singapore, Sri Lanka and Kenya. The rank was also used, prior to 1968, by the Royal Canadian Navy, but upon the creation of the Canadian Forces the rank of midshipman was replaced with the rank of naval cadet."@en ;
	rdfs:label "Midshipman"@de , "Midshipman"@en , "Seekadett"@de ;
	owl:sameAs <dbpedia:Midshipman> .

:Rank_Mirliva a :MilitaryRank ;
	rdfs:comment "Mirliva or Mîr-i livâ was a military rank of the Ottoman Army. It corresponds to a Brigadier General or Major General (Tümgeneral). Mirliva is a compound word composed of Mir and Liva. The rank was junior to the Ferik and superior to the Miralay (Colonel). The title of Mirliva was abolished with Act No. 2590 of 26 November 1934 on the Abolition of Titles and Appellations such as Efendi, Bey or Pasha."@en ;
	rdfs:label "Mirliva"@en ;
	owl:sameAs <dbpedia:Mirliva> ;
	foaf:name "Mirliva" .

:Rank_Mirliva_Cossack_Hetmanate org:rankOf <dbpedia:Cossack_Hetmanate> ;
	a :MilitaryRank ;
	rdfs:comment "The specific instance of the Mirliva rank in the context of country Cossack Hetmanate."@en ;
	rdfs:label "Mirliva (Cossack Hetmanate)"@en , "Mirliva (Hetmanat cosaque)"@fr , "Mirliva (Hetmanat)"@de , "Mirliva (Hetmanato cosaco)"@es , "Mirliva (Hetmańszczyzna)"@pl , "Mirliva (Гетманщина)"@ru ;
	owl:subClass :Rank_Mirliva ;
	foaf:name "Mirliva"@en .

:Rank_Mirliva_Ottoman_Empire org:rankOf <dbpedia:Ottoman_Empire> ;
	a :MilitaryRank ;
	rdfs:comment "The specific instance of the Mirliva rank in the context of country Ottoman Empire."@en ;
	rdfs:label "Mirliva (Det osmanske rike)"@no , "Mirliva (Empire ottoman)"@fr , "Mirliva (Imperio otomano)"@es , "Mirliva (Imperium osmańskie)"@pl , "Mirliva (Impero ottomano)"@it , "Mirliva (Império Otomano)"@pt , "Mirliva (Osmanien valtakunta)"@fi , "Mirliva (Osmanisches Reich)"@de , "Mirliva (Osmanska riket)"@sv , "Mirliva (Ottomaanse Rijk)"@nl , "Mirliva (Ottoman Empire)"@en , "Mirliva (Османская империя)"@ru ;
	owl:subClass :Rank_Mirliva ;
	foaf:name "Mirliva"@en .

:Rank_Mirliva_Septinsular_Republic org:rankOf <dbpedia:Septinsular_Republic> ;
	a :MilitaryRank ;
	rdfs:comment "The specific instance of the Mirliva rank in the context of country Septinsular Republic."@en ;
	rdfs:label "Mirliva (Repubblica delle Sette Isole Unite)"@it , "Mirliva (Republiek van de Zeven Eilanden)"@nl , "Mirliva (Republika Siedmiu Wysp)"@pl , "Mirliva (República de las Islas Jónicas)"@es , "Mirliva (République des Sept-Îles)"@fr , "Mirliva (Septinsular Republic)"@en , "Mirliva (Республика Семи Островов)"@ru ;
	owl:subClass :Rank_Mirliva ;
	foaf:name "Mirliva"@en .

:Rank_Musir a :MilitaryRank ;
	rdfs:label "Müşir"@en ;
	owl:sameAs <dbpedia:M%C3%BC%C5%9Fir> ;
	foaf:name "Müşir" .

:Rank_Musir_Cossack_Hetmanate org:rankOf <dbpedia:Cossack_Hetmanate> ;
	a :MilitaryRank ;
	rdfs:comment "The specific instance of the Müşir rank in the context of country Cossack Hetmanate."@en ;
	rdfs:label "Müşir (Cossack Hetmanate)"@en , "Müşir (Hetmanat cosaque)"@fr , "Müşir (Hetmanat)"@de , "Müşir (Hetmanato cosaco)"@es , "Müşir (Hetmańszczyzna)"@pl , "Müşir (Гетманщина)"@ru ;
	owl:subClass :Rank_Musir ;
	foaf:name "Müşir"@en .

:Rank_Musir_Ottoman_Empire org:rankOf <dbpedia:Ottoman_Empire> ;
	a :MilitaryRank ;
	rdfs:comment "The specific instance of the Müşir rank in the context of country Ottoman Empire."@en ;
	rdfs:label "Müşir (Det osmanske rike)"@no , "Müşir (Empire ottoman)"@fr , "Müşir (Imperio otomano)"@es , "Müşir (Imperium osmańskie)"@pl , "Müşir (Impero ottomano)"@it , "Müşir (Império Otomano)"@pt , "Müşir (Osmanien valtakunta)"@fi , "Müşir (Osmanisches Reich)"@de , "Müşir (Osmanska riket)"@sv , "Müşir (Ottomaanse Rijk)"@nl , "Müşir (Ottoman Empire)"@en , "Müşir (Османская империя)"@ru ;
	owl:subClass :Rank_Musir ;
	foaf:name "Müşir"@en .

:Rank_Musir_Septinsular_Republic org:rankOf <dbpedia:Septinsular_Republic> ;
	a :MilitaryRank ;
	rdfs:comment "The specific instance of the Müşir rank in the context of country Septinsular Republic."@en ;
	rdfs:label "Müşir (Repubblica delle Sette Isole Unite)"@it , "Müşir (Republiek van de Zeven Eilanden)"@nl , "Müşir (Republika Siedmiu Wysp)"@pl , "Müşir (República de las Islas Jónicas)"@es , "Müşir (République des Sept-Îles)"@fr , "Müşir (Septinsular Republic)"@en , "Müşir (Республика Семи Островов)"@ru ;
	owl:subClass :Rank_Musir ;
	foaf:name "Müşir"@en .

:Rank_Navarch a :MilitaryRank ;
	rdfs:comment "Navarch is a Greek word meaning \"leader of the ships\", which in some states became the title of an office equivalent to that of a modern admiral."@en ;
	rdfs:label "Nauarch"@de , "Nauarch"@pl , "Navarch"@en , "Navarco"@es , "Navarque"@fr , "Наварх"@ru ;
	owl:sameAs <dbpedia:Navarch> ;
	foaf:name "Navarch" .

:Rank_Navarch_Achaean_League org:rankOf <dbpedia:Achaean_League> ;
	a :MilitaryRank ;
	rdfs:comment "The specific instance of the Navarch rank in the context of country Achaean League."@en ;
	rdfs:label "Nauarch (Achaiischer Bund)"@de , "Nauarch (Związek Achajski)"@pl , "Navarch (Achaean League)"@en , "Navarch (Achaeïsche Bond)"@nl , "Navarch (Achaiska förbundet)"@sv , "Navarch (Akhaian liitto)"@fi , "Navarch (Det akhaiske forbund)"@no , "Navarch (Lega achea)"@it , "Navarch (Liga Aqueia)"@pt , "Navarco (Liga Aquea)"@es , "Navarque (Ligue achéenne)"@fr , "Наварх (Ахейский союз)"@ru ;
	owl:subClass :Rank_Navarch ;
	foaf:name "Navarch"@en .

:Rank_Navarch_Greece org:rankOf <dbpedia:Greece> ;
	a :MilitaryRank ;
	rdfs:comment "The specific instance of the Navarch rank in the context of country Greece."@en ;
	rdfs:label "Nauarch (Grecja)"@pl , "Nauarch (Griechenland)"@de , "Navarch (Grecia)"@it , "Navarch (Greece)"@en , "Navarch (Grekland)"@sv , "Navarch (Griekenland)"@nl , "Navarch (Grécia)"@pt , "Navarch (Hellas)"@no , "Navarch (Kreikka)"@fi , "Navarco (Grecia)"@es , "Navarque (Grèce)"@fr , "Наварх (Греция)"@ru ;
	owl:subClass :Rank_Navarch ;
	foaf:name "Navarch"@en .

:Rank_Navarch_Macedonia org:rankOf <dbpedia:Macedonia_%28ancient_kingdom%29> ;
	a :MilitaryRank ;
	rdfs:comment "The specific instance of the Navarch rank in the context of country Macedonia (ancient kingdom)."@en ;
	rdfs:label "Nauarch (Macedonia (ancient kingdom))"@de , "Nauarch (Starożytna Macedonia)"@pl , "Navarch (Macedonia (ancient kingdom))"@en , "Navarch (Macedonië (oudheid))"@nl , "Navarch (Macedónia Antiga)"@pt , "Navarch (Makedonian valtakunta)"@fi , "Navarch (Oldtidens Makedonia)"@no , "Navarch (Regno di Macedonia)"@it , "Navarco (Reino de Macedonia)"@es , "Navarque (Royaume de Macédoine)"@fr , "Наварх (Древняя Македония)"@ru ;
	owl:subClass :Rank_Navarch ;
	foaf:name "Navarch"@en .

:Rank_Navarch_Official_Timocracy_of_Sapinetia org:rankOf <dbpedia:Official_Timocracy_of_Sapinetia> ;
	a :MilitaryRank ;
	rdfs:comment "The specific instance of the Navarch rank in the context of the Timocracy of Sapinetia."@en ;
	rdfs:label "Nauarch (Timocracy of Sapinetia)"@de , "Nauarch (Timocracy of Sapinetia)"@pl , "Navarch (Timocracy of Sapinetia)"@en , "Navarco (Timocracy of Sapinetia)"@es , "Navarque (Timocracy of Sapinetia)"@fr , "Наварх (Timocracy of Sapinetia)"@ru ;
	owl:subClass :Rank_Navarch ;
	foaf:name "Navarch"@en .

:Rank_Obergefreiter a :MilitaryRank ;
	rdfs:comment """Obergefreiter is a rank of the German and Swiss militaries which dates from the 19th century. 	 		 			021-Obergefreiter. png 			 German Army rank insignia (shoulder tab) 			 		 		 			3 - ogefr. GIF 			 German Navy rank insignia (sleeve) 			 		 	 The rank was only used in the German army's heavy artillery branch (Fußartillerie) before 1919 and commonly established with the founding of the Reichswehr."""@en ;
	rdfs:label "Obergefreiter"@de , "Obergefreiter"@en , "Ylikorpraali"@fi ;
	owl:sameAs <dbpedia:Obergefreiter> ;
	foaf:name "Obergefreiter" .

:Rank_Obergefreiter_Germany org:rankOf <dbpedia:Germany> ;
	a :MilitaryRank ;
	rdfs:comment "The specific instance of the Obergefreiter rank in the context of Germany."@en ;
	rdfs:label "Obergefreiter (Germany)"@de , "Obergefreiter (Germany)"@en , "Ylikorpraali (Germany)"@fi ;
	owl:subClass :Rank_Obergefreiter ;
	foaf:name "Obergefreiter"@de .

:Rank_Obergefreiter_Switzerland org:rankOf <dbpedia:Switzerland> ;
	a :MilitaryRank ;
	rdfs:comment "The specific instance of the Obergefreiter rank in the context of country Switzerland."@en ;
	rdfs:label "Obergefreiter (Schweiz)"@de , "Obergefreiter (Schweiz)"@sv , "Obergefreiter (Suisse)"@fr , "Obergefreiter (Suiza)"@es , "Obergefreiter (Suíça)"@pt , "Obergefreiter (Sveits)"@no , "Obergefreiter (Svizzera)"@it , "Obergefreiter (Switzerland)"@en , "Obergefreiter (Szwajcaria)"@pl , "Obergefreiter (Zwitserland)"@nl , "Obergefreiter (Швейцария)"@ru , "Ylikorpraali (Sveitsi)"@fi ;
	owl:subClass :Rank_Obergefreiter ;
	foaf:name "Obergefreiter"@de .

:Rank_Oberst a :MilitaryRank ;
	rdfs:comment "Oberst is a military rank in several German-speaking and Scandinavian countries, equivalent to Colonel. It is currently used by both the ground and air forces of Austria, Germany, Switzerland, Denmark and Norway. The Swedish rank överste is a direct translation, as are the Finnish rank eversti and the Icelandic rank ofursti. In the Netherlands the rank overste is used as a synonym for a Lieutenant Colonel"@en ;
	rdfs:label "Oberst"@en , "Oberst"@pt ;
	owl:sameAs <dbpedia:Oberst> ;
	foaf:name "Oberst" .

:Rank_Oberst_Austria org:rankOf <dbpedia:Austria> ;
	a :MilitaryRank ;
	rdfs:comment "The specific instance of the Oberst rank in the context of country Austria."@en ;
	rdfs:label "Oberst (Austria)"@en , "Oberst (Austria)"@es , "Oberst (Austria)"@it , "Oberst (Austria)"@pl , "Oberst (Autriche)"@fr , "Oberst (Itävalta)"@fi , "Oberst (Oostenrijk)"@nl , "Oberst (Áustria)"@pt , "Oberst (Österreich)"@de , "Oberst (Österrike)"@sv , "Oberst (Østerrike)"@no , "Oberst (Австрия)"@ru ;
	owl:subClass :Rank_Oberst ;
	foaf:name "Oberst"@en .

:Rank_Oberst_Denmark org:rankOf <dbpedia:Denmark> ;
	a :MilitaryRank ;
	rdfs:comment "The specific instance of the Oberst rank in the context of country Denmark."@en ;
	rdfs:label "Oberst (Danemark)"@fr , "Oberst (Dania)"@pl , "Oberst (Danimarca)"@it , "Oberst (Danmark)"@no , "Oberst (Danmark)"@sv , "Oberst (Denemarken)"@nl , "Oberst (Denmark)"@en , "Oberst (Dinamarca)"@es , "Oberst (Dinamarca)"@pt , "Oberst (Dänemark)"@de , "Oberst (Tanska)"@fi , "Oberst (Дания)"@ru ;
	owl:subClass :Rank_Oberst ;
	foaf:name "Oberst"@en .

:Rank_Oberst_Finland org:rankOf <dbpedia:Finland> ;
	a :MilitaryRank ;
	rdfs:comment "The specific instance of the Oberst rank in the context of country Finland."@en ;
	rdfs:label "Oberst (Finland)"@en , "Oberst (Finland)"@nl , "Oberst (Finland)"@no , "Oberst (Finland)"@sv , "Oberst (Finlande)"@fr , "Oberst (Finlandia)"@es , "Oberst (Finlandia)"@it , "Oberst (Finlandia)"@pl , "Oberst (Finlândia)"@pt , "Oberst (Finnland)"@de , "Oberst (Suomi)"@fi , "Oberst (Финляндия)"@ru ;
	owl:subClass :Rank_Oberst ;
	foaf:name "Oberst"@en .

:Rank_Oberst_Germany org:rankOf <dbpedia:Germany> ;
	a :MilitaryRank ;
	rdfs:comment "The specific instance of the Oberst rank in the context of country ."@en , "The specific instance of the Oberst rank in the context of country Germany."@en ;
	rdfs:label "Oberst (Germany)"@en , "Oberst (Germany)"@pt ;
	owl:subClass :Rank_Oberst ;
	foaf:name "Oberst"@en .

:Rank_Oberst_Kingdom_of_Denmark org:rankOf <dbpedia:Kingdom_of_Denmark> ;
	a :MilitaryRank ;
	rdfs:comment "The specific instance of the Oberst rank in the context of country Kingdom of Denmark."@en ;
	rdfs:label "Oberst (Kingdom of Denmark)"@en , "Oberst (Kungariket Danmark)"@sv , "Oberst (Regno Unito di Danimarca)"@it , "Oberst (Reino da Dinamarca)"@pt , "Oberst (Reino de Dinamarca)"@es , "Oberst (Tanskan kuningaskunta)"@fi , "Oberst (Королевство Дания)"@ru ;
	owl:subClass :Rank_Oberst ;
	foaf:name "Oberst"@en .

:Rank_Oberst_Norway org:rankOf <dbpedia:Norway> ;
	a :MilitaryRank ;
	rdfs:comment "The specific instance of the Oberst rank in the context of country Norway."@en ;
	rdfs:label "Oberst (Noorwegen)"@nl , "Oberst (Norge)"@no , "Oberst (Norge)"@sv , "Oberst (Norja)"@fi , "Oberst (Noruega)"@es , "Oberst (Noruega)"@pt , "Oberst (Norvegia)"@it , "Oberst (Norvège)"@fr , "Oberst (Norway)"@en , "Oberst (Norwegen)"@de , "Oberst (Norwegia)"@pl , "Oberst (Норвегия)"@ru ;
	owl:subClass :Rank_Oberst ;
	foaf:name "Oberst"@en .

:Rank_Oberst_Sweden org:rankOf <dbpedia:Sweden> ;
	a :MilitaryRank ;
	rdfs:comment "The specific instance of the Oberst rank in the context of country Sweden."@en ;
	rdfs:label "Oberst (Ruotsi)"@fi , "Oberst (Schweden)"@de , "Oberst (Suecia)"@es , "Oberst (Suède)"@fr , "Oberst (Suécia)"@pt , "Oberst (Sverige)"@no , "Oberst (Sverige)"@sv , "Oberst (Svezia)"@it , "Oberst (Sweden)"@en , "Oberst (Szwecja)"@pl , "Oberst (Zweden)"@nl , "Oberst (Швеция)"@ru ;
	owl:subClass :Rank_Oberst ;
	foaf:name "Oberst"@en .

:Rank_Oberst_Switzerland org:rankOf <dbpedia:Switzerland> ;
	a :MilitaryRank ;
	rdfs:comment "The specific instance of the Oberst rank in the context of country Switzerland."@en ;
	rdfs:label "Oberst (Schweiz)"@de , "Oberst (Schweiz)"@sv , "Oberst (Suisse)"@fr , "Oberst (Suiza)"@es , "Oberst (Suíça)"@pt , "Oberst (Sveits)"@no , "Oberst (Sveitsi)"@fi , "Oberst (Svizzera)"@it , "Oberst (Switzerland)"@en , "Oberst (Szwajcaria)"@pl , "Oberst (Zwitserland)"@nl , "Oberst (Швейцария)"@ru ;
	owl:subClass :Rank_Oberst ;
	foaf:name "Oberst"@en .

:Rank_Oberstleutnant_Germany org:rankOf <dbpedia:Germany> ;
	a :MilitaryRank ;
	rdfs:comment "The specific instance of the Oberstleutnant rank in the context of Germany."@en , "The specific instance of the Oberstleutnant rank in the context of country Germany."@en ;
	rdfs:label "Oberstleutnant (Germany)"@en , "Oberstleutnant (Germany)"@pt ;
	owl:subClass :Rank_Oberstleutnant ;
	foaf:name "Oberstleutnant"@en .

:Rank_Officer_cadet_EnglishTradition org:rankEquivalentTo :Rank_Midshipman_EnglishTradition , :Rank_Officer_cadet_EnglishTradition ;
	org:rankJuniorToTransitive :Rank_Pilot_officer_EnglishTradition , :Rank_Second_lieutenant_EnglishTradition ;
	org:rankOf :EnglishTradition , <mil:AirForceServiceBranch> , <mil:ArmyServiceBranch> ;
	org:rankSeniorToTransitive :Rank_Sergeant_major_EnglishTradition , :Rank_Warrant_officer_EnglishTradition ;
	a :MilitaryRank ;
	rdfs:label "Officer cadet"@en ;
	owl:sameAs <dbpedia:Officer_cadet> .

:Rank_Ordinary_seaman_rating org:rankOf <mil:NavyServiceBranch> ;
	a :MilitaryRank ;
	rdfs:label "Ordinary Seaman"@en ;
	owl:sameAs <dbpedia:Ordinary_seaman_%28rating%29> ;
	foaf:name "Ordinary Seaman" .

:Rank_Ordinary_seaman_rating_Australia org:rankOf <dbpedia:Australia> ;
	a :MilitaryRank ;
	rdfs:comment "The specific instance of the  rank in the context of country Australia."@en ;
	rdfs:label " (Australia)"@en , " (Australia)"@es , " (Australia)"@fi , " (Australia)"@it , " (Australia)"@no , " (Australia)"@pl , " (Australie)"@fr , " (Australien)"@de , " (Australien)"@sv , " (Australië (land))"@nl , " (Austrália)"@pt , " (Австралия)"@ru ;
	owl:subClass :Rank_Ordinary_seaman_rating ;
	foaf:name ""@en .

:Rank_Ordinary_seaman_rating_Canada org:rankOf <dbpedia:Canada> ;
	a :MilitaryRank ;
	rdfs:comment "The specific instance of the  rank in the context of Canada."@en ;
	rdfs:label "Ordinary Seaman (Canada)"@en ;
	owl:subClass :Rank_Ordinary_seaman_rating ;
	foaf:name "Ordinary Seaman"@en .

:Rank_Ordinary_seaman_rating_Commonwealth_of_Nations org:rankOf <dbpedia:Commonwealth_of_Nations> ;
	a :MilitaryRank ;
	rdfs:comment "The specific instance of the  rank in the context of country Commonwealth of Nations."@en ;
	rdfs:label "Ordinary Seaman (Commonwealth delle nazioni)"@it , "Ordinary Seaman (Commonwealth of Nations)"@de , "Ordinary Seaman (Commonwealth of Nations)"@en , "Ordinary Seaman (Commonwealth of Nations)"@fr , "Ordinary Seaman (Commonwealth)"@pt , "Ordinary Seaman (Gemenebest van Naties)"@nl , "Ordinary Seaman (Kansainyhteisö)"@fi , "Ordinary Seaman (Mancomunidad de Naciones)"@es , "Ordinary Seaman (Samveldet av nasjoner)"@no , "Ordinary Seaman (Samväldet)"@sv , "Ordinary Seaman (Wspólnota Narodów)"@pl , "Ordinary Seaman (Содружество наций)"@ru ;
	owl:subClass :Rank_Ordinary_seaman_rating ;
	foaf:name "Ordinary Seaman"@en .

:Rank_Petty_officer_EnglishTradition org:rankEquivalentTo :Rank_Sergeant_EnglishTradition ;
	org:rankJuniorToTransitive :Rank_Warrant_officer_EnglishTradition ;
	org:rankOf :EnglishTradition , <mil:NavyServiceBranch> ;
	org:rankSeniorToTransitive :Rank_Leading_seaman_EnglishTradition ;
	a :MilitaryRank ;
	rdfs:comment "A petty officer is a non-commissioned officer in many navies and is given the NATO rank denotion OR-6. They are equal in rank to sergeant, British Army and Royal Air Force. A Petty Officer is superior in rank to Leading Rate and subordinate to Chief Petty Officer, in the case of the British Armed Forces. The modern petty officer dates back to the Age of Sail. Petty officers rank between naval officers and most enlisted sailors."@en ;
	rdfs:label "Maître (grade)"@fr , "Petty Officer"@de , "Petty officer"@en ;
	owl:sameAs <dbpedia:Petty_officer> .

:Rank_Phrourarch a :MilitaryRank ;
	rdfs:comment "Phrourarch or Phrourarchos is a Greek military title, meaning garrison commander. Athenians controlled their overseas empire with the episcopi and phrourarchs . The term was widely used by the Macedonian and later Hellenistic armies. Regarding the Spartans, it is not clear if phrourarch was the specific Spartan term. Phroura (garrison) is reported to be a Spartan term for 'a small mobile or expeditionary force'."@en ;
	rdfs:label "Phrourarch"@en ;
	owl:sameAs <dbpedia:Phrourarch> ;
	foaf:name "Phrourarch" .

:Rank_Phrourarch_Achaean_League org:rankOf <dbpedia:Achaean_League> ;
	a :MilitaryRank ;
	rdfs:comment "The specific instance of the Phrourarch rank in the context of country Achaean League."@en ;
	rdfs:label "Phrourarch (Achaean League)"@en , "Phrourarch (Achaeïsche Bond)"@nl , "Phrourarch (Achaiischer Bund)"@de , "Phrourarch (Achaiska förbundet)"@sv , "Phrourarch (Akhaian liitto)"@fi , "Phrourarch (Det akhaiske forbund)"@no , "Phrourarch (Lega achea)"@it , "Phrourarch (Liga Aquea)"@es , "Phrourarch (Liga Aqueia)"@pt , "Phrourarch (Ligue achéenne)"@fr , "Phrourarch (Związek Achajski)"@pl , "Phrourarch (Ахейский союз)"@ru ;
	owl:subClass :Rank_Phrourarch ;
	foaf:name "Phrourarch"@en .

:Rank_Phrourarch_Greece org:rankOf <dbpedia:Greece> ;
	a :MilitaryRank ;
	rdfs:comment "The specific instance of the Phrourarch rank in the context of country Greece."@en ;
	rdfs:label "Phrourarch (Grecia)"@es , "Phrourarch (Grecia)"@it , "Phrourarch (Grecja)"@pl , "Phrourarch (Greece)"@en , "Phrourarch (Grekland)"@sv , "Phrourarch (Griechenland)"@de , "Phrourarch (Griekenland)"@nl , "Phrourarch (Grèce)"@fr , "Phrourarch (Grécia)"@pt , "Phrourarch (Hellas)"@no , "Phrourarch (Kreikka)"@fi , "Phrourarch (Греция)"@ru ;
	owl:subClass :Rank_Phrourarch ;
	foaf:name "Phrourarch"@en .

:Rank_Phrourarch_Macedonia org:rankOf <dbpedia:Macedonia_%28ancient_kingdom%29> ;
	a :MilitaryRank ;
	rdfs:comment "The specific instance of the Phrourarch rank in the context of country Macedonia (ancient kingdom)."@en ;
	rdfs:label "Phrourarch (Macedonia (ancient kingdom))"@en , "Phrourarch (Macedonië (oudheid))"@nl , "Phrourarch (Macedónia Antiga)"@pt , "Phrourarch (Makedonian valtakunta)"@fi , "Phrourarch (Oldtidens Makedonia)"@no , "Phrourarch (Regno di Macedonia)"@it , "Phrourarch (Reino de Macedonia)"@es , "Phrourarch (Royaume de Macédoine)"@fr , "Phrourarch (Starożytna Macedonia)"@pl , "Phrourarch (Древняя Македония)"@ru ;
	owl:subClass :Rank_Phrourarch ;
	foaf:name "Phrourarch"@en .

:Rank_Phrourarch_Official_Timocracy_of_Sapinetia org:rankOf <dbpedia:Official_Timocracy_of_Sapinetia> ;
	a :MilitaryRank ;
	rdfs:comment "The specific instance of the Phrourarch rank in the context of the Timocracy of Sapinetia."@en ;
	rdfs:label "Phrourarch (Timocracy of Sapinetia)"@en ;
	owl:subClass :Rank_Phrourarch ;
	foaf:name "Phrourarch"@en .

:Rank_Pilot_officer_EnglishTradition org:rankEquivalentTo <http://rdf.muninn-project.org/ontologies/military#Rank_Ensign_(rank)_EnglishTradition> , :Rank_Second_lieutenant_EnglishTradition ;
	org:rankJuniorToTransitive :Rank_Flying_officer_EnglishTradition ;
	org:rankOf :EnglishTradition , <mil:AirForceServiceBranch> ;
	org:rankSeniorToTransitive :Rank_Officer_cadet_EnglishTradition ;
	a :MilitaryRank ;
	rdfs:label "Pilot officer"@en ;
	owl:sameAs <dbpedia:Pilot_officer> .

:Rank_Pipe_Major a :MilitaryRank ;
	rdfs:comment "The Pipe Major is the director of bagpipe music in a Scottish or Irish pipe band. Like Drum Major, the position of Pipe Major is derived from British Army traditions. During the early twentieth century, the term Sergeant Piper was used for the role in place of \"Pipe Major\". Civillian and military pipe bands usually assign a Pipe Major."@en ;
	rdfs:label "Pipe Major"@en ;
	owl:sameAs <dbpedia:Pipe_Major> ;
	foaf:name "Pipe Major" .

:Rank_Pipe_Major_Commonwealth_of_Nations org:rankOf <dbpedia:Commonwealth_of_Nations> ;
	a :MilitaryRank ;
	rdfs:comment "The specific instance of the Pipe Major rank in the context of country Commonwealth of Nations."@en ;
	rdfs:label "Pipe Major (Commonwealth delle nazioni)"@it , "Pipe Major (Commonwealth of Nations)"@de , "Pipe Major (Commonwealth of Nations)"@en , "Pipe Major (Commonwealth of Nations)"@fr , "Pipe Major (Commonwealth)"@pt , "Pipe Major (Gemenebest van Naties)"@nl , "Pipe Major (Kansainyhteisö)"@fi , "Pipe Major (Mancomunidad de Naciones)"@es , "Pipe Major (Samveldet av nasjoner)"@no , "Pipe Major (Samväldet)"@sv , "Pipe Major (Wspólnota Narodów)"@pl , "Pipe Major (Содружество наций)"@ru ;
	owl:subClass :Rank_Pipe_Major ;
	foaf:name "Pipe Major"@en .

:Rank_Pipe_Major_England org:rankOf <dbpedia:England> ;
	a :MilitaryRank ;
	rdfs:comment "The specific instance of the Pipe Major rank in the context of England."@en ;
	rdfs:label "Pipe Major (England)"@en ;
	owl:subClass :Rank_Pipe_Major ;
	foaf:name "Pipe Major"@en .

:Rank_Pipe_Major_Scotland org:rankOf <dbpedia:Scotland> ;
	a :MilitaryRank ;
	rdfs:comment "The specific instance of the Pipe Major rank in the context of country Scotland."@en ;
	rdfs:label "Pipe Major (Escocia)"@es , "Pipe Major (Escócia)"@pt , "Pipe Major (Schotland)"@nl , "Pipe Major (Schottland)"@de , "Pipe Major (Scotland)"@en , "Pipe Major (Scozia)"@it , "Pipe Major (Skotlanti)"@fi , "Pipe Major (Skottland)"@no , "Pipe Major (Skottland)"@sv , "Pipe Major (Szkocja)"@pl , "Pipe Major (Écosse)"@fr , "Pipe Major (Шотландия)"@ru ;
	owl:subClass :Rank_Pipe_Major ;
	foaf:name "Pipe Major"@en .

:Rank_Pipe_Major_Wales org:rankOf <dbpedia:Wales> ;
	a :MilitaryRank ;
	rdfs:comment "The specific instance of the Pipe Major rank in the context of country Wales."@en ;
	rdfs:label "Pipe Major (Gales)"@es , "Pipe Major (Galles)"@it , "Pipe Major (Pays de Galles)"@fr , "Pipe Major (País de Gales)"@pt , "Pipe Major (Wales)"@de , "Pipe Major (Wales)"@en , "Pipe Major (Wales)"@fi , "Pipe Major (Wales)"@nl , "Pipe Major (Wales)"@no , "Pipe Major (Wales)"@sv , "Pipe Major (Walia)"@pl , "Pipe Major (Уэльс)"@ru ;
	owl:subClass :Rank_Pipe_Major ;
	foaf:name "Pipe Major"@en .

:Rank_Podpolkovnik a :MilitaryRank ;
	rdfs:comment "Podpolkovnik is a military rank in Slavic countries which corresponds to a Lieutenant Colonel in English-speaking states. Usually this word is translated as Lieutenant Colonel, however the transliteration is also in common usage, for the sake of the historical context. The exact name of this rank maintains a variety of spellings in different languages: File:Flag of Bulgaria. svg Bulgaria — Подполковник File:Flag of the Czech Republic. svg Czech Republic — Podplukovník File:Flag of Georgia."@en ;
	rdfs:label "Podpolkovnik"@en , "Podpułkownik"@pl ;
	owl:sameAs <dbpedia:Podpolkovnik> ;
	foaf:name "Podpolkovnik" .

:Rank_Podpolkovnik_Poland org:rankOf <dbpedia:Poland> ;
	a :MilitaryRank ;
	rdfs:comment "The specific instance of the Podpolkovnik rank in the context of Poland."@en ;
	rdfs:label "Podpolkovnik (Poland)"@en , "Podpułkownik (Poland)"@pl ;
	owl:subClass :Rank_Podpolkovnik ;
	foaf:name "Podpolkovnik"@en .

:Rank_Podpolkovnik_Russia org:rankOf <dbpedia:Russia> ;
	a :MilitaryRank ;
	rdfs:comment "The specific instance of the Podpolkovnik rank in the context of country Russia."@en ;
	rdfs:label "Podpolkovnik (Rusia)"@es , "Podpolkovnik (Rusland)"@nl , "Podpolkovnik (Russia)"@en , "Podpolkovnik (Russia)"@it , "Podpolkovnik (Russie)"@fr , "Podpolkovnik (Russland)"@de , "Podpolkovnik (Russland)"@no , "Podpolkovnik (Ryssland)"@sv , "Podpolkovnik (Rússia)"@pt , "Podpolkovnik (Venäjä)"@fi , "Podpolkovnik (Россия)"@ru , "Podpułkownik (Rosja)"@pl ;
	owl:subClass :Rank_Podpolkovnik ;
	foaf:name "Podpolkovnik"@en .

:Rank_Podpolkovnik_Soviet_Union org:rankOf <dbpedia:Soviet_Union> ;
	a :MilitaryRank ;
	rdfs:comment "The specific instance of the Podpolkovnik rank in the context of country Soviet Union."@en ;
	rdfs:label "Podpolkovnik (Neuvostoliitto)"@fi , "Podpolkovnik (Soviet Union)"@en , "Podpolkovnik (Sovjet-Unie)"@nl , "Podpolkovnik (Sovjetunionen)"@no , "Podpolkovnik (Sovjetunionen)"@sv , "Podpolkovnik (Sowjetunion)"@de , "Podpolkovnik (Union des républiques socialistes soviétiques)"@fr , "Podpolkovnik (Unione Sovietica)"@it , "Podpolkovnik (União Soviética)"@pt , "Podpolkovnik (Unión Soviética)"@es , "Podpolkovnik (Союз Советских Социалистических Республик)"@ru , "Podpułkownik (Związek Socjalistycznych Republik Radzieckich)"@pl ;
	owl:subClass :Rank_Podpolkovnik ;
	foaf:name "Podpolkovnik"@en .

:Rank_Podpolkovnik_Ukraine org:rankOf <dbpedia:Ukraine> ;
	a :MilitaryRank ;
	rdfs:comment "The specific instance of the Podpolkovnik rank in the context of country Ukraine."@en ;
	rdfs:label "Podpolkovnik (Oekraïne)"@nl , "Podpolkovnik (Ucraina)"@it , "Podpolkovnik (Ucrania)"@es , "Podpolkovnik (Ucrânia)"@pt , "Podpolkovnik (Ukraina)"@fi , "Podpolkovnik (Ukraina)"@no , "Podpolkovnik (Ukraina)"@sv , "Podpolkovnik (Ukraine)"@de , "Podpolkovnik (Ukraine)"@en , "Podpolkovnik (Ukraine)"@fr , "Podpolkovnik (Украина)"@ru , "Podpułkownik (Ukraina)"@pl ;
	owl:subClass :Rank_Podpolkovnik ;
	foaf:name "Podpolkovnik"@en .

:Rank_Podpraporshchik a :MilitaryRank ;
	rdfs:comment "Podpraporshchik (Sub-Praporshchik) was one of the non-commissioned ranks, originally below the Sergeant and Feldwebel but since 1826 it became the highest non-commissioned rank of the infantry, cavalry and Leib Guard. In 1884, the podpraporshchik rank was renamed Zauryad-praporshchik (Ordinary Praporshchik)."@en ;
	rdfs:label "Podpraporshchik"@en , "Подпрапорщик"@ru ;
	owl:sameAs <dbpedia:Podpraporshchik> ;
	foaf:name "Podpraporshchik" .

:Rank_Podpraporshchik_Russia org:rankOf <dbpedia:Russia> ;
	a :MilitaryRank ;
	rdfs:comment "The specific instance of the Podpraporshchik rank in the context of country Russia."@en ;
	rdfs:label "Podpraporshchik (Rosja)"@pl , "Podpraporshchik (Rusia)"@es , "Podpraporshchik (Rusland)"@nl , "Podpraporshchik (Russia)"@en , "Podpraporshchik (Russia)"@it , "Podpraporshchik (Russie)"@fr , "Podpraporshchik (Russland)"@de , "Podpraporshchik (Russland)"@no , "Podpraporshchik (Ryssland)"@sv , "Podpraporshchik (Rússia)"@pt , "Podpraporshchik (Venäjä)"@fi , "Подпрапорщик (Россия)"@ru ;
	owl:subClass :Rank_Podpraporshchik ;
	foaf:name "Подпрапорщик"@ru .

:Rank_Podpraporshchik_Soviet_Union org:rankOf <dbpedia:Soviet_Union> ;
	a :MilitaryRank ;
	rdfs:comment "The specific instance of the Podpraporshchik rank in the context of country Soviet Union."@en ;
	rdfs:label "Podpraporshchik (Neuvostoliitto)"@fi , "Podpraporshchik (Soviet Union)"@en , "Podpraporshchik (Sovjet-Unie)"@nl , "Podpraporshchik (Sovjetunionen)"@no , "Podpraporshchik (Sovjetunionen)"@sv , "Podpraporshchik (Sowjetunion)"@de , "Podpraporshchik (Union des républiques socialistes soviétiques)"@fr , "Podpraporshchik (Unione Sovietica)"@it , "Podpraporshchik (União Soviética)"@pt , "Podpraporshchik (Unión Soviética)"@es , "Podpraporshchik (Związek Socjalistycznych Republik Radzieckich)"@pl , "Подпрапорщик (Союз Советских Социалистических Республик)"@ru ;
	owl:subClass :Rank_Podpraporshchik ;
	foaf:name "Podpraporshchik"@en .

:Rank_Polemarch a :MilitaryRank ;
	rdfs:comment "A polemarch was a senior military title in various ancient Greek city states (poleis). The title is composed out of the polemos (war) and archon (ruler/leader) and translates as \"warleader\" or \"warlord\", one of the nine archontes (ἄρχοντες) appointed annually in Athens. The name indicates that the polemarchos original function was to command the army; presumably the office was created to take over this function from the king."@en ;
	rdfs:label "Polemarca"@es , "Polemarch"@en , "Polemarchos"@nl , "Polemarco"@pt , "Polemark"@sv , "Polemarkos"@no , "Polémarque"@fr , "Полемарх"@ru ;
	owl:sameAs <dbpedia:Polemarch> ;
	foaf:name "Polemarch" .

:Rank_Polemarch_Achaean_League org:rankOf <dbpedia:Achaean_League> ;
	a :MilitaryRank ;
	rdfs:comment "The specific instance of the Polemarch rank in the context of country Achaean League."@en ;
	rdfs:label "Polemarca (Liga Aquea)"@es , "Polemarch (Achaean League)"@en , "Polemarch (Achaiischer Bund)"@de , "Polemarch (Akhaian liitto)"@fi , "Polemarch (Lega achea)"@it , "Polemarch (Związek Achajski)"@pl , "Polemarchos (Achaeïsche Bond)"@nl , "Polemarco (Liga Aqueia)"@pt , "Polemark (Achaiska förbundet)"@sv , "Polemarkos (Det akhaiske forbund)"@no , "Polémarque (Ligue achéenne)"@fr , "Полемарх (Ахейский союз)"@ru ;
	owl:subClass :Rank_Polemarch ;
	foaf:name "Polemarch"@en .

:Rank_Polemarch_Macedonia org:rankOf <dbpedia:Macedonia_%28ancient_kingdom%29> ;
	a :MilitaryRank ;
	rdfs:comment "The specific instance of the Polemarch rank in the context of country Macedonia (ancient kingdom)."@en ;
	rdfs:label "Polemarca (Reino de Macedonia)"@es , "Polemarch (Macedonia (ancient kingdom))"@en , "Polemarch (Makedonian valtakunta)"@fi , "Polemarch (Regno di Macedonia)"@it , "Polemarch (Starożytna Macedonia)"@pl , "Polemarchos (Macedonië (oudheid))"@nl , "Polemarco (Macedónia Antiga)"@pt , "Polemark (Macedonia (ancient kingdom))"@sv , "Polemarkos (Oldtidens Makedonia)"@no , "Polémarque (Royaume de Macédoine)"@fr , "Полемарх (Древняя Македония)"@ru ;
	owl:subClass :Rank_Polemarch ;
	foaf:name "Polemarch"@en .

:Rank_Polkovnik a :MilitaryRank ;
	rdfs:comment "Polkovnik is often a military rank in Slavic countries which corresponds to a Colonel in English-speaking states. However, in the History of Ukraine polkovnyk was an administrative rank similar to a governor as well. Usually this word is translated as Colonel, however the transliteration is also in common usage, for the sake of the historical and social context."@en ;
	rdfs:label "Polkovnik"@en ;
	owl:sameAs <dbpedia:Polkovnik> ;
	foaf:name "Polkovnik" .

:Rank_Polkovnik_Poland org:rankOf <dbpedia:Poland> ;
	a :MilitaryRank ;
	rdfs:comment "The specific instance of the Polkovnik rank in the context of Poland."@en ;
	rdfs:label "Polkovnik (Poland)"@en ;
	owl:subClass :Rank_Polkovnik ;
	foaf:name "Polkovnik"@en .

:Rank_Polkovnik_Russia org:rankOf <dbpedia:Russia> ;
	a :MilitaryRank ;
	rdfs:comment "The specific instance of the Polkovnik rank in the context of country Russia."@en ;
	rdfs:label "Polkovnik (Rosja)"@pl , "Polkovnik (Rusia)"@es , "Polkovnik (Rusland)"@nl , "Polkovnik (Russia)"@en , "Polkovnik (Russia)"@it , "Polkovnik (Russie)"@fr , "Polkovnik (Russland)"@de , "Polkovnik (Russland)"@no , "Polkovnik (Ryssland)"@sv , "Polkovnik (Rússia)"@pt , "Polkovnik (Venäjä)"@fi , "Polkovnik (Россия)"@ru ;
	owl:subClass :Rank_Polkovnik ;
	foaf:name "Polkovnik"@en .

:Rank_Polkovnik_Soviet_Union org:rankOf <dbpedia:Soviet_Union> ;
	a :MilitaryRank ;
	rdfs:comment "The specific instance of the Polkovnik rank in the context of country Soviet Union."@en ;
	rdfs:label "Polkovnik (Neuvostoliitto)"@fi , "Polkovnik (Soviet Union)"@en , "Polkovnik (Sovjet-Unie)"@nl , "Polkovnik (Sovjetunionen)"@no , "Polkovnik (Sovjetunionen)"@sv , "Polkovnik (Sowjetunion)"@de , "Polkovnik (Union des républiques socialistes soviétiques)"@fr , "Polkovnik (Unione Sovietica)"@it , "Polkovnik (União Soviética)"@pt , "Polkovnik (Unión Soviética)"@es , "Polkovnik (Związek Socjalistycznych Republik Radzieckich)"@pl , "Polkovnik (Союз Советских Социалистических Республик)"@ru ;
	owl:subClass :Rank_Polkovnik ;
	foaf:name "Polkovnik"@en .

:Rank_Polkovnik_Ukraine org:rankOf <dbpedia:Ukraine> ;
	a :MilitaryRank ;
	rdfs:comment "The specific instance of the Polkovnik rank in the context of country Ukraine."@en ;
	rdfs:label "Polkovnik (Oekraïne)"@nl , "Polkovnik (Ucraina)"@it , "Polkovnik (Ucrania)"@es , "Polkovnik (Ucrânia)"@pt , "Polkovnik (Ukraina)"@fi , "Polkovnik (Ukraina)"@no , "Polkovnik (Ukraina)"@pl , "Polkovnik (Ukraina)"@sv , "Polkovnik (Ukraine)"@de , "Polkovnik (Ukraine)"@en , "Polkovnik (Ukraine)"@fr , "Polkovnik (Украина)"@ru ;
	owl:subClass :Rank_Polkovnik ;
	foaf:name "Polkovnik"@en .

:Rank_Poruchik a :MilitaryRank ;
	rdfs:comment "Poruchik was a military rank in several Slavic countries, such as the Russian Empire and the Republic of Poland, equivalent to Lieutenant. \"Poruchik\" means \"messenger\", \"officer for orders\". This is a Slavic (Czech) copy of the term \"Lieutenant\" (locum tenens). In Russia this rank was first introduced in Strelets New Regiments, the rank legalised by the Table of Ranks. A podporuchik is simply a Sub-Poruchik."@en ;
	rdfs:label "Poroetsjik"@nl , "Poruchik"@en , "Porutschik"@de , "Poručik"@it , "Поручик"@ru ;
	owl:sameAs <dbpedia:Poruchik> ;
	foaf:name "Poruchik" .

:Rank_Poruchik_Poland org:rankOf <dbpedia:Poland> ;
	a :MilitaryRank ;
	rdfs:comment "The specific instance of the Poruchik rank in the context of Poland."@en ;
	rdfs:label "Poroetsjik (Poland)"@nl , "Poruchik (Poland)"@en , "Porutschik (Poland)"@de , "Poručik (Poland)"@it , "Поручик (Poland)"@ru ;
	owl:subClass :Rank_Poruchik ;
	foaf:name "Poruchik"@en .

:Rank_Poruchik_Russia org:rankOf <dbpedia:Russia> ;
	a :MilitaryRank ;
	rdfs:comment "The specific instance of the Poruchik rank in the context of country Russia."@en ;
	rdfs:label "Poroetsjik (Rusland)"@nl , "Poruchik (Rosja)"@pl , "Poruchik (Rusia)"@es , "Poruchik (Russia)"@en , "Poruchik (Russie)"@fr , "Poruchik (Russland)"@no , "Poruchik (Ryssland)"@sv , "Poruchik (Rússia)"@pt , "Poruchik (Venäjä)"@fi , "Porutschik (Russland)"@de , "Poručik (Russia)"@it , "Поручик (Россия)"@ru ;
	owl:subClass :Rank_Poruchik ;
	foaf:name "Поручик"@ru .

:Rank_Poruchik_Soviet_Union org:rankOf <dbpedia:Soviet_Union> ;
	a :MilitaryRank ;
	rdfs:comment "The specific instance of the Poruchik rank in the context of country Soviet Union."@en ;
	rdfs:label "Poroetsjik (Sovjet-Unie)"@nl , "Poruchik (Neuvostoliitto)"@fi , "Poruchik (Soviet Union)"@en , "Poruchik (Sovjetunionen)"@no , "Poruchik (Sovjetunionen)"@sv , "Poruchik (Union des républiques socialistes soviétiques)"@fr , "Poruchik (União Soviética)"@pt , "Poruchik (Unión Soviética)"@es , "Poruchik (Związek Socjalistycznych Republik Radzieckich)"@pl , "Porutschik (Sowjetunion)"@de , "Poručik (Unione Sovietica)"@it , "Поручик (Союз Советских Социалистических Республик)"@ru ;
	owl:subClass :Rank_Poruchik ;
	foaf:name "Poruchik"@en .

:Rank_Praporshchik a :MilitaryRank ;
	rdfs:comment "Praporshchik is a rank in the Russian military."@en ;
	rdfs:label "Praporshchik"@en , "Прапорщик"@ru ;
	owl:sameAs <dbpedia:Praporshchik> ;
	foaf:name "Praporshchik" .

:Rank_Praporshchik_Russia org:rankOf <dbpedia:Russia> ;
	a :MilitaryRank ;
	rdfs:comment "The specific instance of the Praporshchik rank in the context of country Russia."@en ;
	rdfs:label "Praporshchik (Rosja)"@pl , "Praporshchik (Rusia)"@es , "Praporshchik (Rusland)"@nl , "Praporshchik (Russia)"@en , "Praporshchik (Russia)"@it , "Praporshchik (Russie)"@fr , "Praporshchik (Russland)"@de , "Praporshchik (Russland)"@no , "Praporshchik (Ryssland)"@sv , "Praporshchik (Rússia)"@pt , "Praporshchik (Venäjä)"@fi , "Прапорщик (Россия)"@ru ;
	owl:subClass :Rank_Praporshchik ;
	foaf:name "Прапорщик"@ru .

:Rank_Praporshchik_Soviet_Union org:rankOf <dbpedia:Soviet_Union> ;
	a :MilitaryRank ;
	rdfs:comment "The specific instance of the Praporshchik rank in the context of country Soviet Union."@en ;
	rdfs:label "Praporshchik (Neuvostoliitto)"@fi , "Praporshchik (Soviet Union)"@en , "Praporshchik (Sovjet-Unie)"@nl , "Praporshchik (Sovjetunionen)"@no , "Praporshchik (Sovjetunionen)"@sv , "Praporshchik (Sowjetunion)"@de , "Praporshchik (Union des républiques socialistes soviétiques)"@fr , "Praporshchik (Unione Sovietica)"@it , "Praporshchik (União Soviética)"@pt , "Praporshchik (Unión Soviética)"@es , "Praporshchik (Związek Socjalistycznych Republik Radzieckich)"@pl , "Прапорщик (Союз Советских Социалистических Республик)"@ru ;
	owl:subClass :Rank_Praporshchik ;
	foaf:name "Praporshchik"@en .

:Rank_Private a :MilitaryRank ;
	rdfs:comment "A Private is a soldier of the lowest military rank (equivalent to NATO Rank Grades OR-1 to OR-3 depending on the force served in). In modern military parlance, 'Private' is shortened to 'Pte' in the United Kingdom and other Commonwealth countries and to 'Pvt. ' in the United States."@en ;
	rdfs:label "Deuxième classe"@fr , "Menig"@no , "Menig"@sv , "Menig (grad)"@no , "Menig 1kl"@sv , "Private (Dienstgrad)"@de , "Private (rank)"@en , "Soldado raso"@es , "Soldat (Dienstgrad)"@de , "Soldat (grade)"@fr , "Sotamies"@fi , "Szeregowy"@pl , "Рядовой"@ru ;
	owl:sameAs <dbpedia:Private_%28rank%29> ;
	foaf:name "Private" .

<http://rdf.muninn-project.org/ontologies/military#Rank_Private_(rank)_EnglishTradition> org:rankEquivalentTo :Rank_Aircraftman_EnglishTradition , :Rank_Seaman_EnglishTradition ;
	org:rankJuniorToTransitive :Rank_Corporal_EnglishTradition ;
	org:rankOf :EnglishTradition , <mil:ArmyServiceBranch> ;
	a :MilitaryRank ;
	owl:sameAs <dbpedia:Private_(rank)> .

:Rank_Private_Australia org:rankOf <dbpedia:Australia> ;
	a :MilitaryRank ;
	rdfs:comment "The specific instance of the Private (rank) rank in the context of country Australia."@en ;
	rdfs:label "Deuxième classeSoldat (grade) (Australie)"@fr , "Menig (grad)Menig (Australia)"@no , "Menig 1klMenig (Australien)"@sv , "Private (Dienstgrad)Soldat (Dienstgrad) (Australien)"@de , "Private (rank) (Australia)"@en , "Private (rank) (Australia)"@it , "Private (rank) (Australië (land))"@nl , "Private (rank) (Austrália)"@pt , "Soldado raso (Australia)"@es , "Sotamies (Australia)"@fi , "Szeregowy (Australia)"@pl , "Рядовой (Австралия)"@ru ;
	owl:subClass :Rank_Private ;
	foaf:name "Private"@en .

:Rank_Private_Canada org:rankOf <dbpedia:Canada> ;
	a :MilitaryRank ;
	rdfs:comment "The specific instance of the Private (rank) rank in the context of Canada."@en ;
	rdfs:label "Deuxième classeSoldat (grade, Canada)"@fr , "Menig (grad, Canada)"@no , "Menig 1klMenig (Canada)"@sv , "Private (rank, Canada)"@en , "Soldado raso (Canada)"@es , "Soldat (Dienstgrad, Canada)"@de , "Sotamies (Canada)"@fi , "Szeregowy (Canada)"@pl , "Рядовой (Canada)"@ru ;
	owl:subClass :Rank_Private ;
	foaf:name "Private"@en , "Soldat, Deuxième classe"@fr .

:Rank_Private_England org:rankOf <dbpedia:England> ;
	a :MilitaryRank ;
	rdfs:comment "The specific instance of the Private (rank) rank in the context of England."@en ;
	rdfs:label "Deuxième classeSoldat (grade) (England)"@fr , "Menig (grad, England)"@no , "Menig 1klMenig (England)"@sv , "Private (Dienstgrad)Soldat (Dienstgrad, England)"@de , "Private (rank, England)"@en , "Soldado raso (England)"@es , "Sotamies (England)"@fi , "Szeregowy (England)"@pl , "Рядовой (England)"@ru ;
	owl:subClass :Rank_Private ;
	foaf:name "Private"@en .

:Rank_Private_Republic_of_Ireland org:rankOf <dbpedia:Republic_of_Ireland> ;
	a :MilitaryRank ;
	rdfs:comment "The specific instance of the Private (rank) rank in the context of country Republic of Ireland."@en ;
	rdfs:label "Deuxième classeSoldat (grade) (Irlande (pays))"@fr , "Menig (grad)Menig (Irland)"@no , "Menig 1klMenig (Irland)"@sv , "Private (Dienstgrad)Soldat (Dienstgrad) (Irland)"@de , "Private (rank) (Ierland (land))"@nl , "Private (rank) (Irlanda)"@it , "Private (rank) (Republic of Ireland)"@en , "Private (rank) (República da Irlanda)"@pt , "Soldado raso (Irlanda)"@es , "Sotamies (Irlanti)"@fi , "Szeregowy (Irlandia)"@pl , "Рядовой (Ирландия)"@ru ;
	owl:subClass :Rank_Private ;
	foaf:name "Private"@en .

:Rank_Private_Scotland org:rankOf <dbpedia:Scotland> ;
	a :MilitaryRank ;
	rdfs:comment "The specific instance of the Private (rank) rank in the context of country Scotland."@en ;
	rdfs:label "Deuxième classeSoldat (grade) (Écosse)"@fr , "Menig (grad)Menig (Skottland)"@no , "Menig 1klMenig (Skottland)"@sv , "Private (Dienstgrad)Soldat (Dienstgrad) (Schottland)"@de , "Private (rank) (Escócia)"@pt , "Private (rank) (Schotland)"@nl , "Private (rank) (Scotland)"@en , "Private (rank) (Scozia)"@it , "Soldado raso (Escocia)"@es , "Sotamies (Skotlanti)"@fi , "Szeregowy (Szkocja)"@pl , "Рядовой (Шотландия)"@ru ;
	owl:subClass :Rank_Private ;
	foaf:name "Private"@en .

:Rank_Private_Wales org:rankOf <dbpedia:Wales> ;
	a :MilitaryRank ;
	rdfs:comment "The specific instance of the Private (rank) rank in the context of country Wales."@en ;
	rdfs:label "Deuxième classeSoldat (grade) (Pays de Galles)"@fr , "Menig (grad)Menig (Wales)"@no , "Menig 1klMenig (Wales)"@sv , "Private (Dienstgrad)Soldat (Dienstgrad) (Wales)"@de , "Private (rank) (Galles)"@it , "Private (rank) (País de Gales)"@pt , "Private (rank) (Wales)"@en , "Private (rank) (Wales)"@nl , "Soldado raso (Gales)"@es , "Sotamies (Wales)"@fi , "Szeregowy (Walia)"@pl , "Рядовой (Уэльс)"@ru ;
	owl:subClass :Rank_Private ;
	foaf:name "Private"@en .

:Rank_Rear_admiral a :MilitaryRank ;
	rdfs:comment "Rear admiral is a naval commissioned officer rank above that of a commodore and captain, and below that of a vice admiral. It is generally regarded as the lowest of the \"admiral\" ranks, which are also sometimes referred to as \"flag officers\" or \"flag ranks\". In many navies it is referred to as a two-star rank. It originated from the days of naval sailing squadrons and can trace its origins to the Royal Navy."@en ;
	rdfs:label "Rear admiral"@en ;
	owl:sameAs <dbpedia:Rear_admiral> ;
	foaf:name "Rear admiral" .

:Rank_Rear_admiral_Australia org:rankOf <dbpedia:Australia> ;
	a :MilitaryRank ;
	rdfs:comment "The specific instance of the Rear admiral rank in the context of country Australia."@en ;
	rdfs:label "Rear admiral (Australia)"@en , "Rear admiral (Australia)"@es , "Rear admiral (Australia)"@fi , "Rear admiral (Australia)"@it , "Rear admiral (Australia)"@no , "Rear admiral (Australia)"@pl , "Rear admiral (Australie)"@fr , "Rear admiral (Australien)"@de , "Rear admiral (Australien)"@sv , "Rear admiral (Australië (land))"@nl , "Rear admiral (Austrália)"@pt , "Rear admiral (Австралия)"@ru ;
	owl:subClass :Rank_Rear_admiral ;
	foaf:name "Rear admiral"@en .

:Rank_Rear_admiral_Canada org:rankOf <dbpedia:Canada> ;
	a :MilitaryRank ;
	rdfs:comment "The specific instance of the Rear admiral rank in the context of Canada."@en ;
	rdfs:label "Rear admiral (Canada)"@en ;
	owl:subClass :Rank_Rear_admiral ;
	foaf:name "Rear admiral"@en .

:Rank_Regimental_Quartermaster_Sergeant a :MilitaryRank ;
	rdfs:comment "Regimental Quartermaster Sergeant is a military rank in some militaries, and an appointment in others."@en ;
	rdfs:label "Regimental Quartermaster Sergeant"@en ;
	owl:sameAs <dbpedia:Regimental_Quartermaster_Sergeant> ;
	foaf:name "Regimental Quartermaster Sergeant" .

:Rank_Regimental_Quartermaster_Sergeant_Australia org:rankOf <dbpedia:Australia> ;
	a :MilitaryRank ;
	rdfs:comment "The specific instance of the Regimental Quartermaster Sergeant rank in the context of country Australia."@en ;
	rdfs:label "Regimental Quartermaster Sergeant (Australia)"@en , "Regimental Quartermaster Sergeant (Australia)"@es , "Regimental Quartermaster Sergeant (Australia)"@fi , "Regimental Quartermaster Sergeant (Australia)"@it , "Regimental Quartermaster Sergeant (Australia)"@no , "Regimental Quartermaster Sergeant (Australia)"@pl , "Regimental Quartermaster Sergeant (Australie)"@fr , "Regimental Quartermaster Sergeant (Australien)"@de , "Regimental Quartermaster Sergeant (Australien)"@sv , "Regimental Quartermaster Sergeant (Australië (land))"@nl , "Regimental Quartermaster Sergeant (Austrália)"@pt , "Regimental Quartermaster Sergeant (Австралия)"@ru ;
	owl:subClass :Rank_Regimental_Quartermaster_Sergeant ;
	foaf:name "Regimental Quartermaster Sergeant"@en .

:Rank_Regimental_Quartermaster_Sergeant_Canada org:rankOf <dbpedia:Canada> ;
	a :MilitaryRank ;
	rdfs:comment "The specific instance of the Regimental Quartermaster Sergeant rank in the context of Canada."@en ;
	rdfs:label "Regimental Quartermaster Sergeant (Canada)"@en ;
	owl:subClass :Rank_Regimental_Quartermaster_Sergeant ;
	foaf:name "Regimental Quartermaster Sergeant"@en .

:Rank_Regimental_Quartermaster_Sergeant_Commonwealth_of_Nations org:rankOf <dbpedia:Commonwealth_of_Nations> ;
	a :MilitaryRank ;
	rdfs:comment "The specific instance of the Regimental Quartermaster Sergeant rank in the context of country Commonwealth of Nations."@en ;
	rdfs:label "Regimental Quartermaster Sergeant (Commonwealth delle nazioni)"@it , "Regimental Quartermaster Sergeant (Commonwealth of Nations)"@de , "Regimental Quartermaster Sergeant (Commonwealth of Nations)"@en , "Regimental Quartermaster Sergeant (Commonwealth of Nations)"@fr , "Regimental Quartermaster Sergeant (Commonwealth)"@pt , "Regimental Quartermaster Sergeant (Gemenebest van Naties)"@nl , "Regimental Quartermaster Sergeant (Kansainyhteisö)"@fi , "Regimental Quartermaster Sergeant (Mancomunidad de Naciones)"@es , "Regimental Quartermaster Sergeant (Samveldet av nasjoner)"@no , "Regimental Quartermaster Sergeant (Samväldet)"@sv , "Regimental Quartermaster Sergeant (Wspólnota Narodów)"@pl , "Regimental Quartermaster Sergeant (Содружество наций)"@ru ;
	owl:subClass :Rank_Regimental_Quartermaster_Sergeant ;
	foaf:name "Regimental Quartermaster Sergeant"@en .

:Rank_Regimental_Quartermaster_Sergeant_England org:rankOf <dbpedia:England> ;
	a :MilitaryRank ;
	rdfs:comment "The specific instance of the Regimental Quartermaster Sergeant rank in the context of England."@en ;
	rdfs:label "Regimental Quartermaster Sergeant (England)"@en ;
	owl:subClass :Rank_Regimental_Quartermaster_Sergeant ;
	foaf:name "Regimental Quartermaster Sergeant"@en .

:Rank_Regimental_Quartermaster_Sergeant_Republic_of_Ireland org:rankOf <dbpedia:Republic_of_Ireland> ;
	a :MilitaryRank ;
	rdfs:comment "The specific instance of the Regimental Quartermaster Sergeant rank in the context of country Republic of Ireland."@en ;
	rdfs:label "Regimental Quartermaster Sergeant (Ierland (land))"@nl , "Regimental Quartermaster Sergeant (Irland)"@de , "Regimental Quartermaster Sergeant (Irland)"@no , "Regimental Quartermaster Sergeant (Irland)"@sv , "Regimental Quartermaster Sergeant (Irlanda)"@es , "Regimental Quartermaster Sergeant (Irlanda)"@it , "Regimental Quartermaster Sergeant (Irlande (pays))"@fr , "Regimental Quartermaster Sergeant (Irlandia)"@pl , "Regimental Quartermaster Sergeant (Irlanti)"@fi , "Regimental Quartermaster Sergeant (Republic of Ireland)"@en , "Regimental Quartermaster Sergeant (República da Irlanda)"@pt , "Regimental Quartermaster Sergeant (Ирландия)"@ru ;
	owl:subClass :Rank_Regimental_Quartermaster_Sergeant ;
	foaf:name "Regimental Quartermaster Sergeant"@en .

:Rank_Regimental_Quartermaster_Sergeant_Scotland org:rankOf <dbpedia:Scotland> ;
	a :MilitaryRank ;
	rdfs:comment "The specific instance of the Regimental Quartermaster Sergeant rank in the context of country Scotland."@en ;
	rdfs:label "Regimental Quartermaster Sergeant (Escocia)"@es , "Regimental Quartermaster Sergeant (Escócia)"@pt , "Regimental Quartermaster Sergeant (Schotland)"@nl , "Regimental Quartermaster Sergeant (Schottland)"@de , "Regimental Quartermaster Sergeant (Scotland)"@en , "Regimental Quartermaster Sergeant (Scozia)"@it , "Regimental Quartermaster Sergeant (Skotlanti)"@fi , "Regimental Quartermaster Sergeant (Skottland)"@no , "Regimental Quartermaster Sergeant (Skottland)"@sv , "Regimental Quartermaster Sergeant (Szkocja)"@pl , "Regimental Quartermaster Sergeant (Écosse)"@fr , "Regimental Quartermaster Sergeant (Шотландия)"@ru ;
	owl:subClass :Rank_Regimental_Quartermaster_Sergeant ;
	foaf:name "Regimental Quartermaster Sergeant"@en .

:Rank_Regimental_Quartermaster_Sergeant_Wales org:rankOf <dbpedia:Wales> ;
	a :MilitaryRank ;
	rdfs:comment "The specific instance of the Regimental Quartermaster Sergeant rank in the context of country Wales."@en ;
	rdfs:label "Regimental Quartermaster Sergeant (Gales)"@es , "Regimental Quartermaster Sergeant (Galles)"@it , "Regimental Quartermaster Sergeant (Pays de Galles)"@fr , "Regimental Quartermaster Sergeant (País de Gales)"@pt , "Regimental Quartermaster Sergeant (Wales)"@de , "Regimental Quartermaster Sergeant (Wales)"@en , "Regimental Quartermaster Sergeant (Wales)"@fi , "Regimental Quartermaster Sergeant (Wales)"@nl , "Regimental Quartermaster Sergeant (Wales)"@no , "Regimental Quartermaster Sergeant (Wales)"@sv , "Regimental Quartermaster Sergeant (Walia)"@pl , "Regimental Quartermaster Sergeant (Уэльс)"@ru ;
	owl:subClass :Rank_Regimental_Quartermaster_Sergeant ;
	foaf:name "Regimental Quartermaster Sergeant"@en .

:Rank_Regimental_sergeant_major a :MilitaryAppointment , :MilitaryRank ;
	rdfs:label "Regimental sergeant major"@en ;
	owl:sameAs <dbpedia:Regimental_sergeant_major> ;
	foaf:name "Regimental sergeant major" .

:Rank_Regimental_sergeant_major_Australia org:rankOf <dbpedia:Australia> ;
	a :MilitaryRank ;
	rdfs:comment "The specific instance of the Regimental sergeant major rank in the context of country Australia."@en ;
	rdfs:label "Regimental sergeant major (Australia)"@en , "Regimental sergeant major (Australia)"@es , "Regimental sergeant major (Australia)"@fi , "Regimental sergeant major (Australia)"@it , "Regimental sergeant major (Australia)"@no , "Regimental sergeant major (Australia)"@pl , "Regimental sergeant major (Australie)"@fr , "Regimental sergeant major (Australien)"@de , "Regimental sergeant major (Australien)"@sv , "Regimental sergeant major (Australië (land))"@nl , "Regimental sergeant major (Austrália)"@pt , "Regimental sergeant major (Австралия)"@ru ;
	owl:subClass :Rank_Regimental_sergeant_major ;
	foaf:name "Regimental sergeant major"@en .

:Rank_Regimental_sergeant_major_Commonwealth_of_Nations org:rankOf <dbpedia:Commonwealth_of_Nations> ;
	a :MilitaryRank ;
	rdfs:comment "The specific instance of the Regimental sergeant major rank in the context of country Commonwealth of Nations."@en ;
	rdfs:label "Regimental sergeant major (Commonwealth delle nazioni)"@it , "Regimental sergeant major (Commonwealth of Nations)"@de , "Regimental sergeant major (Commonwealth of Nations)"@en , "Regimental sergeant major (Commonwealth of Nations)"@fr , "Regimental sergeant major (Commonwealth)"@pt , "Regimental sergeant major (Gemenebest van Naties)"@nl , "Regimental sergeant major (Kansainyhteisö)"@fi , "Regimental sergeant major (Mancomunidad de Naciones)"@es , "Regimental sergeant major (Samveldet av nasjoner)"@no , "Regimental sergeant major (Samväldet)"@sv , "Regimental sergeant major (Wspólnota Narodów)"@pl , "Regimental sergeant major (Содружество наций)"@ru ;
	owl:subClass :Rank_Regimental_sergeant_major ;
	foaf:name "Regimental sergeant major"@en .

:Rank_Regimental_sergeant_major_Singapore org:rankOf <dbpedia:Singapore> ;
	a :MilitaryRank ;
	rdfs:comment "The specific instance of the Regimental sergeant major rank in the context of country Singapore."@en ;
	rdfs:label "Regimental sergeant major (Singapore)"@en , "Regimental sergeant major (Singapore)"@fi , "Regimental sergeant major (Singapore)"@it , "Regimental sergeant major (Singapore)"@nl , "Regimental sergeant major (Singapore)"@no , "Regimental sergeant major (Singapore)"@sv , "Regimental sergeant major (Singapour)"@fr , "Regimental sergeant major (Singapur)"@de , "Regimental sergeant major (Singapur)"@es , "Regimental sergeant major (Singapur)"@pl , "Regimental sergeant major (Singapura)"@pt , "Regimental sergeant major (Сингапур)"@ru ;
	owl:subClass :Rank_Regimental_sergeant_major ;
	foaf:name "Regimental sergeant major"@en .

:Rank_Sangsa a :MilitaryRank ;
	rdfs:comment "Sangsa is a Korean military rank used by both the armed forces of North and South Korea. A Sangsa is the equivalent to a First Sergeant in most other militaries. The rank of Sangsa is junior to a Wonsa in South Korea and to a Warrant Officer like rank in the North known as Teukmu Sangsa."@en ;
	rdfs:label "Sangsa"@en ;
	owl:sameAs <dbpedia:Sangsa> ;
	foaf:name "Sangsa" .

:Rank_Sangsa_North_Korea org:rankOf <dbpedia:North_Korea> ;
	a :MilitaryRank ;
	rdfs:comment "The specific instance of the Sangsa rank in the context of country North Korea."@en ;
	rdfs:label "Sangsa (Corea del Nord)"@it , "Sangsa (Corea del Norte)"@es , "Sangsa (Coreia do Norte)"@pt , "Sangsa (Corée du Nord)"@fr , "Sangsa (Korea Północna)"@pl , "Sangsa (Korean demokraattinen kansantasavalta)"@fi , "Sangsa (Noord-Korea)"@nl , "Sangsa (Nord-Korea)"@no , "Sangsa (Nordkorea)"@de , "Sangsa (Nordkorea)"@sv , "Sangsa (North Korea)"@en , "Sangsa (Корейская Народно-Демократическая Республика)"@ru ;
	owl:subClass :Rank_Sangsa ;
	foaf:name "Sangsa"@en .

:Rank_Sangsa_South_Korea org:rankOf <dbpedia:South_Korea> ;
	a :MilitaryRank ;
	rdfs:comment "The specific instance of the Sangsa rank in the context of country South Korea."@en ;
	rdfs:label "Sangsa (Corea del Sud)"@it , "Sangsa (Corea del Sur)"@es , "Sangsa (Coreia do Sul)"@pt , "Sangsa (Corée du Sud)"@fr , "Sangsa (Korea Południowa)"@pl , "Sangsa (Korean tasavalta)"@fi , "Sangsa (South Korea)"@en , "Sangsa (Sydkorea)"@sv , "Sangsa (Sør-Korea)"@no , "Sangsa (Südkorea)"@de , "Sangsa (Zuid-Korea)"@nl , "Sangsa (Республика Корея)"@ru ;
	owl:subClass :Rank_Sangsa ;
	foaf:name "Sangsa"@en .

:Rank_Schout-bij-nacht a :MilitaryRank ;
	rdfs:comment "Schout-bij-nacht is a Dutch Naval rank, equivalent to Rear Admiral in the US Navy and Royal Navy. It is the second most junior Admiral position of the Dutch Navy, ranking above Commandeur and below a Vice-admiraal. The rank of Schout-bij-nacht originated between the 15th and 16th century. Translated as Watch-at-night, the Schout-bij-Nacht was the officer who supervised the ship when the Captain was asleep."@en ;
	rdfs:label "Schout-bij-nacht"@en , "Schout-bij-nacht"@fr , "Schout-bij-nacht"@nl , "Schoutbynacht"@no , "Schoutbynacht"@sv , "Шаутбенахт"@ru ;
	owl:sameAs <dbpedia:Schout-bij-nacht> ;
	foaf:name "Schout-bij-nacht" .

:Rank_Schout-bij-nacht_Netherlands org:rankOf <dbpedia:Netherlands> ;
	a :MilitaryRank ;
	rdfs:comment "The specific instance of the Schout-bij-nacht rank in the context of country Netherlands."@en ;
	rdfs:label "Schout-bij-nacht (Alankomaat)"@fi , "Schout-bij-nacht (Holandia)"@pl , "Schout-bij-nacht (Nederland)"@nl , "Schout-bij-nacht (Netherlands)"@en , "Schout-bij-nacht (Niederlande)"@de , "Schout-bij-nacht (Paesi Bassi)"@it , "Schout-bij-nacht (Pays-Bas)"@fr , "Schout-bij-nacht (Países Baixos)"@pt , "Schout-bij-nacht (Países Bajos)"@es , "Schoutbynacht (Nederland)"@no , "Schoutbynacht (Nederländerna)"@sv , "Шаутбенахт (Нидерланды)"@ru ;
	owl:subClass :Rank_Schout-bij-nacht ;
	foaf:name "Schout-bij-nacht"@en , "Schout-bij-nacht"@nl .

:Rank_Schout-bij-nacht_Russia org:rankOf <dbpedia:Russia> ;
	a :MilitaryRank ;
	rdfs:comment "The specific instance of the Schout-bij-nacht rank in the context of country Russia."@en ;
	rdfs:label "Schout-bij-nacht (Rosja)"@pl , "Schout-bij-nacht (Rusia)"@es , "Schout-bij-nacht (Rusland)"@nl , "Schout-bij-nacht (Russia)"@en , "Schout-bij-nacht (Russia)"@it , "Schout-bij-nacht (Russie)"@fr , "Schout-bij-nacht (Russland)"@de , "Schout-bij-nacht (Rússia)"@pt , "Schout-bij-nacht (Venäjä)"@fi , "Schoutbynacht (Russland)"@no , "Schoutbynacht (Ryssland)"@sv , "Шаутбенахт (Россия)"@ru ;
	owl:subClass :Rank_Schout-bij-nacht ;
	foaf:name "Шаутбенахт"@ru .

:Rank_Schout-bij-nacht_Soviet_Union org:rankOf <dbpedia:Soviet_Union> ;
	a :MilitaryRank ;
	rdfs:comment "The specific instance of the Schout-bij-nacht rank in the context of country Soviet Union."@en ;
	rdfs:label "Schout-bij-nacht (Neuvostoliitto)"@fi , "Schout-bij-nacht (Soviet Union)"@en , "Schout-bij-nacht (Sovjet-Unie)"@nl , "Schout-bij-nacht (Sowjetunion)"@de , "Schout-bij-nacht (Union des républiques socialistes soviétiques)"@fr , "Schout-bij-nacht (Unione Sovietica)"@it , "Schout-bij-nacht (União Soviética)"@pt , "Schout-bij-nacht (Unión Soviética)"@es , "Schout-bij-nacht (Związek Socjalistycznych Republik Radzieckich)"@pl , "Schoutbynacht (Sovjetunionen)"@no , "Schoutbynacht (Sovjetunionen)"@sv , "Шаутбенахт (Союз Советских Социалистических Республик)"@ru ;
	owl:subClass :Rank_Schout-bij-nacht ;
	foaf:name "Schout-bij-nacht"@en .

:Rank_Seaman_EnglishTradition org:rankEquivalentTo :Rank_Aircraftman_EnglishTradition , <http://rdf.muninn-project.org/ontologies/military#Rank_Private_(rank)_EnglishTradition> ;
	org:rankJuniorToTransitive :Rank_Leading_seaman_EnglishTradition ;
	org:rankOf :EnglishTradition , <mil:NavyServiceBranch> ;
	a :MilitaryRank ;
	rdfs:comment "Seaman is one of the lowest ranks in a Navy. In the Commonwealth it is the lowest rank in the Navy, followed by Able Seaman and Leading Seaman, and followed by the Petty Officer ranks. In the United States, it means the lowest three enlisted rates of the U.S. Navy, followed by the higher Petty Officer ranks. The equivalent of the seaman, in French-speaking countries, is the Matelot."@en ;
	rdfs:label "Matelot"@fr , "Seaman"@en , "Seemann"@de ;
	owl:sameAs <dbpedia:Seaman> .

:Rank_Second_Corporal a :MilitaryRank ;
	rdfs:comment "Second Corporal was a rank in the Royal Engineers and Army Ordnance Corps of the British Army. Second Corporals wore one rank chevron, but unlike Lance-Corporals they held full non-commissioned officer rank. They were thus equivalent to Bombardiers in the Royal Artillery. The rank was abolished in 1920."@en ;
	rdfs:label "Second Corporal"@en ;
	owl:sameAs <dbpedia:Second_Corporal> ;
	foaf:name "Second Corporal" .

:Rank_Second_Corporal_England org:rankOf <dbpedia:England> ;
	a :MilitaryRank ;
	rdfs:comment "The specific instance of the Second Corporal rank in the context of England."@en ;
	rdfs:label "Second Corporal (England)"@en ;
	owl:subClass :Rank_Second_Corporal ;
	foaf:name "Second Corporal"@en .

:Rank_Second_Corporal_Scotland org:rankOf <dbpedia:Scotland> ;
	a :MilitaryRank ;
	rdfs:comment "The specific instance of the Second Corporal rank in the context of country Scotland."@en ;
	rdfs:label "Second Corporal (Escocia)"@es , "Second Corporal (Escócia)"@pt , "Second Corporal (Schotland)"@nl , "Second Corporal (Schottland)"@de , "Second Corporal (Scotland)"@en , "Second Corporal (Scozia)"@it , "Second Corporal (Skotlanti)"@fi , "Second Corporal (Skottland)"@no , "Second Corporal (Skottland)"@sv , "Second Corporal (Szkocja)"@pl , "Second Corporal (Écosse)"@fr , "Second Corporal (Шотландия)"@ru ;
	owl:subClass :Rank_Second_Corporal ;
	foaf:name "Second Corporal"@en .

:Rank_Second_Corporal_Wales org:rankOf <dbpedia:Wales> ;
	a :MilitaryRank ;
	rdfs:comment "The specific instance of the Second Corporal rank in the context of country Wales."@en ;
	rdfs:label "Second Corporal (Gales)"@es , "Second Corporal (Galles)"@it , "Second Corporal (Pays de Galles)"@fr , "Second Corporal (País de Gales)"@pt , "Second Corporal (Wales)"@de , "Second Corporal (Wales)"@en , "Second Corporal (Wales)"@fi , "Second Corporal (Wales)"@nl , "Second Corporal (Wales)"@no , "Second Corporal (Wales)"@sv , "Second Corporal (Walia)"@pl , "Second Corporal (Уэльс)"@ru ;
	owl:subClass :Rank_Second_Corporal ;
	foaf:name "Second Corporal"@en .

:Rank_Second_lieutenant_EnglishTradition org:rankEquivalentTo <http://rdf.muninn-project.org/ontologies/military#Rank_Ensign_(rank)_EnglishTradition> , :Rank_Pilot_officer_EnglishTradition ;
	org:rankJuniorToTransitive :Rank_Lieutenant_EnglishTradition ;
	org:rankOf :EnglishTradition , <mil:ArmyServiceBranch> ;
	org:rankSeniorToTransitive :Rank_Officer_cadet_EnglishTradition ;
	a :MilitaryRank ;
	rdfs:label "Second lieutenant"@en ;
	owl:sameAs <dbpedia:Second_lieutenant> .

:Rank_Sergeant_EnglishTradition org:rankEquivalentTo :Rank_Petty_officer_EnglishTradition , :Rank_Sergeant_EnglishTradition ;
	org:rankJuniorToTransitive :Rank_Sergeant_major_EnglishTradition , :Rank_Warrant_officer_EnglishTradition ;
	org:rankOf :EnglishTradition , <mil:AirForceServiceBranch> , <mil:ArmyServiceBranch> ;
	org:rankSeniorToTransitive :Rank_Corporal_EnglishTradition ;
	a :MilitaryRank ;
	rdfs:comment "Sergeant (normally abbreviated to Sgt) is a rank used in some form by most militaries, police forces, and other uniformed organizations around the world. Its origins are the Latin serviens, \"one who serves\", through the French term Sergent. In most armies the rank of sergeant corresponds to command of a squad. In Commonwealth armies it is a more senior rank, corresponding roughly to a platoon second-in-command."@en ;
	rdfs:label "Sergeant"@de , "Sergeant"@en , "Sergent"@fr ;
	owl:sameAs <dbpedia:Sergeant> .

:Rank_Sergeant_Major_Instructor a :MilitaryRank ;
	rdfs:comment "Sergeant Major Instructor (SMI) is a British Army appointment held by Warrant Officers Class 1 in the Small Arms School Corps and the Army Physical Training Corps and by some WO1s in the Royal Engineers."@en ;
	rdfs:label "Sergeant Major Instructor"@en ;
	owl:sameAs <dbpedia:Sergeant_Major_Instructor> ;
	foaf:name "Sergeant Major Instructor" .

:Rank_Sergeant_Major_Instructor_England org:rankOf <dbpedia:England> ;
	a :MilitaryRank ;
	rdfs:comment "The specific instance of the Sergeant Major Instructor rank in the context of England."@en ;
	rdfs:label "Sergeant Major Instructor (England)"@en ;
	owl:subClass :Rank_Sergeant_Major_Instructor ;
	foaf:name "Sergeant Major Instructor"@en .

:Rank_Sergeant_Major_Instructor_Scotland org:rankOf <dbpedia:Scotland> ;
	a :MilitaryRank ;
	rdfs:comment "The specific instance of the Sergeant Major Instructor rank in the context of country Scotland."@en ;
	rdfs:label "Sergeant Major Instructor (Escocia)"@es , "Sergeant Major Instructor (Escócia)"@pt , "Sergeant Major Instructor (Schotland)"@nl , "Sergeant Major Instructor (Schottland)"@de , "Sergeant Major Instructor (Scotland)"@en , "Sergeant Major Instructor (Scozia)"@it , "Sergeant Major Instructor (Skotlanti)"@fi , "Sergeant Major Instructor (Skottland)"@no , "Sergeant Major Instructor (Skottland)"@sv , "Sergeant Major Instructor (Szkocja)"@pl , "Sergeant Major Instructor (Écosse)"@fr , "Sergeant Major Instructor (Шотландия)"@ru ;
	owl:subClass :Rank_Sergeant_Major_Instructor ;
	foaf:name "Sergeant Major Instructor"@en .

:Rank_Sergeant_Major_Instructor_Wales org:rankOf <dbpedia:Wales> ;
	a :MilitaryRank ;
	rdfs:comment "The specific instance of the Sergeant Major Instructor rank in the context of country Wales."@en ;
	rdfs:label "Sergeant Major Instructor (Gales)"@es , "Sergeant Major Instructor (Galles)"@it , "Sergeant Major Instructor (Pays de Galles)"@fr , "Sergeant Major Instructor (País de Gales)"@pt , "Sergeant Major Instructor (Wales)"@de , "Sergeant Major Instructor (Wales)"@en , "Sergeant Major Instructor (Wales)"@fi , "Sergeant Major Instructor (Wales)"@nl , "Sergeant Major Instructor (Wales)"@no , "Sergeant Major Instructor (Wales)"@sv , "Sergeant Major Instructor (Walia)"@pl , "Sergeant Major Instructor (Уэльс)"@ru ;
	owl:subClass :Rank_Sergeant_Major_Instructor ;
	foaf:name "Sergeant Major Instructor"@en .

:Rank_Sergeant_Pilot a :MilitaryRank ;
	rdfs:comment "A Sergeant Pilot was a non-commissioned officer who had undergone flight training and was a qualified pilot in the air forces of several Commonwealth countries and in the United States Army Air Force before, during and after World War II. After World War II, non-commissioned pilots began to be phased out and today all air force pilots are commissioned officers. In the United States, the Flight Officer Act ended enlisted men's chances of undergoing flight training."@en ;
	rdfs:label "Fältflygare"@sv , "Sergeant Pilot"@en ;
	owl:sameAs <dbpedia:Sergeant_Pilot> ;
	foaf:name "Sergeant Pilot" .

:Rank_Sergeant_Pilot_Australia org:rankOf <dbpedia:Australia> ;
	a :MilitaryRank ;
	rdfs:comment "The specific instance of the Sergeant Pilot rank in the context of country Australia."@en ;
	rdfs:label "Fältflygare (Australien)"@sv , "Sergeant Pilot (Australia)"@en , "Sergeant Pilot (Australia)"@es , "Sergeant Pilot (Australia)"@fi , "Sergeant Pilot (Australia)"@it , "Sergeant Pilot (Australia)"@no , "Sergeant Pilot (Australia)"@pl , "Sergeant Pilot (Australie)"@fr , "Sergeant Pilot (Australien)"@de , "Sergeant Pilot (Australië (land))"@nl , "Sergeant Pilot (Austrália)"@pt , "Sergeant Pilot (Австралия)"@ru ;
	owl:subClass :Rank_Sergeant_Pilot ;
	foaf:name "Sergeant Pilot"@en .

:Rank_Sergeant_Pilot_Canada org:rankOf <dbpedia:Canada> ;
	a :MilitaryRank ;
	rdfs:comment "The specific instance of the Sergeant Pilot rank in the context of Canada."@en ;
	rdfs:label "Fältflygare (Canada)"@sv , "Sergeant Pilot (Canada)"@en ;
	owl:subClass :Rank_Sergeant_Pilot ;
	foaf:name "Sergeant Pilot"@en .

:Rank_Sergeant_Pilot_Commonwealth_of_Nations org:rankOf <dbpedia:Commonwealth_of_Nations> ;
	a :MilitaryRank ;
	rdfs:comment "The specific instance of the Sergeant Pilot rank in the context of country Commonwealth of Nations."@en ;
	rdfs:label "Fältflygare (Samväldet)"@sv , "Sergeant Pilot (Commonwealth delle nazioni)"@it , "Sergeant Pilot (Commonwealth of Nations)"@de , "Sergeant Pilot (Commonwealth of Nations)"@en , "Sergeant Pilot (Commonwealth of Nations)"@fr , "Sergeant Pilot (Commonwealth)"@pt , "Sergeant Pilot (Gemenebest van Naties)"@nl , "Sergeant Pilot (Kansainyhteisö)"@fi , "Sergeant Pilot (Mancomunidad de Naciones)"@es , "Sergeant Pilot (Samveldet av nasjoner)"@no , "Sergeant Pilot (Wspólnota Narodów)"@pl , "Sergeant Pilot (Содружество наций)"@ru ;
	owl:subClass :Rank_Sergeant_Pilot ;
	foaf:name "Sergeant Pilot"@en .

:Rank_Sergeant_Pilot_England org:rankOf <dbpedia:England> ;
	a :MilitaryRank ;
	rdfs:comment "The specific instance of the Sergeant Pilot rank in the context of England."@en ;
	rdfs:label "Fältflygare (England)"@sv , "Sergeant Pilot (England)"@en ;
	owl:subClass :Rank_Sergeant_Pilot ;
	foaf:name "Sergeant Pilot"@en .

:Rank_Sergeant_Pilot_Scotland org:rankOf <dbpedia:Scotland> ;
	a :MilitaryRank ;
	rdfs:comment "The specific instance of the Sergeant Pilot rank in the context of country Scotland."@en ;
	rdfs:label "Fältflygare (Skottland)"@sv , "Sergeant Pilot (Escocia)"@es , "Sergeant Pilot (Escócia)"@pt , "Sergeant Pilot (Schotland)"@nl , "Sergeant Pilot (Schottland)"@de , "Sergeant Pilot (Scotland)"@en , "Sergeant Pilot (Scozia)"@it , "Sergeant Pilot (Skotlanti)"@fi , "Sergeant Pilot (Skottland)"@no , "Sergeant Pilot (Szkocja)"@pl , "Sergeant Pilot (Écosse)"@fr , "Sergeant Pilot (Шотландия)"@ru ;
	owl:subClass :Rank_Sergeant_Pilot ;
	foaf:name "Sergeant Pilot"@en .

:Rank_Sergeant_Pilot_Wales org:rankOf <dbpedia:Wales> ;
	a :MilitaryRank ;
	rdfs:comment "The specific instance of the Sergeant Pilot rank in the context of country Wales."@en ;
	rdfs:label "Fältflygare (Wales)"@sv , "Sergeant Pilot (Gales)"@es , "Sergeant Pilot (Galles)"@it , "Sergeant Pilot (Pays de Galles)"@fr , "Sergeant Pilot (País de Gales)"@pt , "Sergeant Pilot (Wales)"@de , "Sergeant Pilot (Wales)"@en , "Sergeant Pilot (Wales)"@fi , "Sergeant Pilot (Wales)"@nl , "Sergeant Pilot (Wales)"@no , "Sergeant Pilot (Walia)"@pl , "Sergeant Pilot (Уэльс)"@ru ;
	owl:subClass :Rank_Sergeant_Pilot ;
	foaf:name "Sergeant Pilot"@en .

:Rank_Sergeant_major_EnglishTradition org:rankEquivalentTo :Rank_Warrant_officer_EnglishTradition ;
	org:rankJuniorToTransitive :Rank_Officer_cadet_EnglishTradition ;
	org:rankOf :EnglishTradition , <mil:ArmyServiceBranch> ;
	org:rankSeniorToTransitive :Rank_Sergeant_EnglishTradition ;
	a :MilitaryRank ;
	rdfs:label "Sergeant major"@en ;
	owl:sameAs <dbpedia:Sergeant_major> .

:Rank_Skeuophoros a :MilitaryRank ;
	rdfs:comment "A skeuophoros was a slave or servant who carried baggage in Ancient Greece. Herodotus records that every hoplite was followed on campaign by a servant as a skeuophoros. In Aristophanes' play The Frogs, Xanthias, the slave of Dionysus, acts as his skeuophoros: Διόνυσος ἴθι νυν ἐπειδὴ ληματίας κἀνδρεῖος εἶ,σὺ μὲν γενοῦ 'γὼ τὸ ῥόπαλον τουτὶ λαβὼνκαὶ τὴν λεοντῆν, εἴπερ ἀφοβόσπλαγχνος εἶ:ἐγὼ δ᾽ ἔσομαί σοι σκευοφόρος ἐν τῷ μέρει."@en ;
	rdfs:label "Skeuophoros"@en ;
	owl:sameAs <dbpedia:Skeuophoros> ;
	foaf:name "Skeuophoros" .

:Rank_Skeuophoros_Achaean_League org:rankOf <dbpedia:Achaean_League> ;
	a :MilitaryRank ;
	rdfs:comment "The specific instance of the Skeuophoros rank in the context of country Achaean League."@en ;
	rdfs:label "Skeuophoros (Achaean League)"@en , "Skeuophoros (Achaeïsche Bond)"@nl , "Skeuophoros (Achaiischer Bund)"@de , "Skeuophoros (Achaiska förbundet)"@sv , "Skeuophoros (Akhaian liitto)"@fi , "Skeuophoros (Det akhaiske forbund)"@no , "Skeuophoros (Lega achea)"@it , "Skeuophoros (Liga Aquea)"@es , "Skeuophoros (Liga Aqueia)"@pt , "Skeuophoros (Ligue achéenne)"@fr , "Skeuophoros (Związek Achajski)"@pl , "Skeuophoros (Ахейский союз)"@ru ;
	owl:subClass :Rank_Skeuophoros ;
	foaf:name "Skeuophoros"@en .

:Rank_Skeuophoros_Macedonia org:rankOf <dbpedia:Macedonia_%28ancient_kingdom%29> ;
	a :MilitaryRank ;
	rdfs:comment "The specific instance of the Skeuophoros rank in the context of country Macedonia (ancient kingdom)."@en ;
	rdfs:label "Skeuophoros (Macedonia (ancient kingdom))"@en , "Skeuophoros (Macedonië (oudheid))"@nl , "Skeuophoros (Macedónia Antiga)"@pt , "Skeuophoros (Makedonian valtakunta)"@fi , "Skeuophoros (Oldtidens Makedonia)"@no , "Skeuophoros (Regno di Macedonia)"@it , "Skeuophoros (Reino de Macedonia)"@es , "Skeuophoros (Royaume de Macédoine)"@fr , "Skeuophoros (Starożytna Macedonia)"@pl , "Skeuophoros (Древняя Македония)"@ru ;
	owl:subClass :Rank_Skeuophoros ;
	foaf:name "Skeuophoros"@en .

:Rank_Somatophylakes a :MilitaryRank ;
	rdfs:comment "Somatophylakes, in its literal English translation from Greek, means \"bodyguards\". The most famous body of somatophylakes were those of Philip of Macedon and Alexander the Great. They consisted of seven men, drawn from the Macedonian nobility, who also acted as high-ranking military officers, holding command positions such as general or chiliarch. Alexander the Great appointed Peucestas as eighth somatophylax after the siege of Malli."@en ;
	rdfs:label "Somatofilachie"@it , "Somatofylakes"@fi , "Somatophylakes"@de , "Somatophylakes"@en , "Somatophylakes"@es , "Somatophylax"@nl , "Sômatophylaques"@fr ;
	owl:sameAs <dbpedia:Somatophylakes> ;
	foaf:name "Somatophylakes" .

:Rank_Somatophylakes_Achaean_League org:rankOf <dbpedia:Achaean_League> ;
	a :MilitaryRank ;
	rdfs:comment "The specific instance of the Somatophylakes rank in the context of country Achaean League."@en ;
	rdfs:label "Somatofilachie (Lega achea)"@it , "Somatofylakes (Akhaian liitto)"@fi , "Somatophylakes (Achaean League)"@en , "Somatophylakes (Achaiischer Bund)"@de , "Somatophylakes (Achaiska förbundet)"@sv , "Somatophylakes (Det akhaiske forbund)"@no , "Somatophylakes (Liga Aquea)"@es , "Somatophylakes (Liga Aqueia)"@pt , "Somatophylakes (Związek Achajski)"@pl , "Somatophylakes (Ахейский союз)"@ru , "Somatophylax (Achaeïsche Bond)"@nl , "Sômatophylaques (Ligue achéenne)"@fr ;
	owl:subClass :Rank_Somatophylakes ;
	foaf:name "Somatophylakes"@en .

:Rank_Somatophylakes_Macedonia org:rankOf <dbpedia:Macedonia_%28ancient_kingdom%29> ;
	a :MilitaryRank ;
	rdfs:comment "The specific instance of the Somatophylakes rank in the context of country Macedonia (ancient kingdom)."@en ;
	rdfs:label "Somatofilachie (Regno di Macedonia)"@it , "Somatofylakes (Makedonian valtakunta)"@fi , "Somatophylakes (Macedonia (ancient kingdom))"@de , "Somatophylakes (Macedonia (ancient kingdom))"@en , "Somatophylakes (Macedónia Antiga)"@pt , "Somatophylakes (Oldtidens Makedonia)"@no , "Somatophylakes (Reino de Macedonia)"@es , "Somatophylakes (Starożytna Macedonia)"@pl , "Somatophylakes (Древняя Македония)"@ru , "Somatophylax (Macedonië (oudheid))"@nl , "Sômatophylaques (Royaume de Macédoine)"@fr ;
	owl:subClass :Rank_Somatophylakes ;
	foaf:name "Somatophylakes"@en .

:Rank_Sotnik a :MilitaryRank ;
	rdfs:comment "Sotnik or Sotnyk was a military rank among the Cossack starshyna (officers), Strelets Troops (17th century) in Muscovy and Imperial Cossack cavalry (since 1826), the Ukrainian Insurgent Army, the Ukrainian Galician Army, and the Ukrainian People's Army."@en ;
	rdfs:label "Sotnik"@en , "Sotnik"@fr , "Sotnik"@nl , "Sótnik"@pt , "Сотник"@ru ;
	owl:sameAs <dbpedia:Sotnik> ;
	foaf:name "Sotnik" .

:Rank_Sotnik_Russia org:rankOf <dbpedia:Russia> ;
	a :MilitaryRank ;
	rdfs:comment "The specific instance of the Sotnik rank in the context of country Russia."@en ;
	rdfs:label "Sotnik (Rosja)"@pl , "Sotnik (Rusia)"@es , "Sotnik (Rusland)"@nl , "Sotnik (Russia)"@en , "Sotnik (Russia)"@it , "Sotnik (Russie)"@fr , "Sotnik (Russland)"@de , "Sotnik (Russland)"@no , "Sotnik (Ryssland)"@sv , "Sotnik (Venäjä)"@fi , "Sótnik (Rússia)"@pt , "Сотник (Россия)"@ru ;
	owl:subClass :Rank_Sotnik ;
	foaf:name "Сотник"@ru .

:Rank_Sotnik_Soviet_Union org:rankOf <dbpedia:Soviet_Union> ;
	a :MilitaryRank ;
	rdfs:comment "The specific instance of the Sotnik rank in the context of country Soviet Union."@en ;
	rdfs:label "Sotnik (Neuvostoliitto)"@fi , "Sotnik (Soviet Union)"@en , "Sotnik (Sovjet-Unie)"@nl , "Sotnik (Sovjetunionen)"@no , "Sotnik (Sovjetunionen)"@sv , "Sotnik (Sowjetunion)"@de , "Sotnik (Union des républiques socialistes soviétiques)"@fr , "Sotnik (Unione Sovietica)"@it , "Sotnik (Unión Soviética)"@es , "Sotnik (Związek Socjalistycznych Republik Radzieckich)"@pl , "Sótnik (União Soviética)"@pt , "Сотник (Союз Советских Социалистических Республик)"@ru ;
	owl:subClass :Rank_Sotnik ;
	foaf:name "Sotnik"@en .

:Rank_Sotnik_Ukraine org:rankOf <dbpedia:Ukraine> ;
	a :MilitaryRank ;
	rdfs:comment "The specific instance of the Sotnik rank in the context of country Ukraine."@en ;
	rdfs:label "Sotnik (Oekraïne)"@nl , "Sotnik (Ucraina)"@it , "Sotnik (Ucrania)"@es , "Sotnik (Ukraina)"@fi , "Sotnik (Ukraina)"@no , "Sotnik (Ukraina)"@pl , "Sotnik (Ukraina)"@sv , "Sotnik (Ukraine)"@de , "Sotnik (Ukraine)"@en , "Sotnik (Ukraine)"@fr , "Sótnik (Ucrânia)"@pt , "Сотник (Украина)"@ru ;
	owl:subClass :Rank_Sotnik ;
	foaf:name "Сотник"@ru .

:Rank_Sowi a :MilitaryRank ;
	rdfs:comment "Sowi (소위) is the junior most Korean officer rank in both the militaries of North and South Korea. It is considered the equivalent of a Second Lieutenant in most other militaries."@en ;
	rdfs:label "Sowi"@en ;
	owl:sameAs <dbpedia:Sowi> ;
	foaf:name "Sowi" .

:Rank_Sowi_North_Korea org:rankOf <dbpedia:North_Korea> ;
	a :MilitaryRank ;
	rdfs:comment "The specific instance of the Sowi rank in the context of country North Korea."@en ;
	rdfs:label "Sowi (Corea del Nord)"@it , "Sowi (Corea del Norte)"@es , "Sowi (Coreia do Norte)"@pt , "Sowi (Corée du Nord)"@fr , "Sowi (Korea Północna)"@pl , "Sowi (Korean demokraattinen kansantasavalta)"@fi , "Sowi (Noord-Korea)"@nl , "Sowi (Nord-Korea)"@no , "Sowi (Nordkorea)"@de , "Sowi (Nordkorea)"@sv , "Sowi (North Korea)"@en , "Sowi (Корейская Народно-Демократическая Республика)"@ru ;
	owl:subClass :Rank_Sowi ;
	foaf:name "Sowi"@en .

:Rank_Sowi_South_Korea org:rankOf <dbpedia:South_Korea> ;
	a :MilitaryRank ;
	rdfs:comment "The specific instance of the Sowi rank in the context of country South Korea."@en ;
	rdfs:label "Sowi (Corea del Sud)"@it , "Sowi (Corea del Sur)"@es , "Sowi (Coreia do Sul)"@pt , "Sowi (Corée du Sud)"@fr , "Sowi (Korea Południowa)"@pl , "Sowi (Korean tasavalta)"@fi , "Sowi (South Korea)"@en , "Sowi (Sydkorea)"@sv , "Sowi (Sør-Korea)"@no , "Sowi (Südkorea)"@de , "Sowi (Zuid-Korea)"@nl , "Sowi (Республика Корея)"@ru ;
	owl:subClass :Rank_Sowi ;
	foaf:name "Sowi"@en .

:Rank_Squadron_leader_EnglishTradition org:rankEquivalentTo <http://rdf.muninn-project.org/ontologies/military#Rank_Commandant_(rank)_EnglishTradition> , :Rank_Lieutenant_commander_EnglishTradition , :Rank_Major_EnglishTradition ;
	org:rankJuniorToTransitive <http://rdf.muninn-project.org/ontologies/military#Rank_Wing_commander_(rank)_EnglishTradition> ;
	org:rankOf :EnglishTradition , <mil:AirForceServiceBranch> ;
	org:rankSeniorToTransitive :Rank_Flight_lieutenant_EnglishTradition ;
	a :MilitaryRank ;
	rdfs:label "Squadron leader"@en ;
	owl:sameAs <dbpedia:Squadron_leader> .

:Rank_Staabikapten a :MilitaryRank ;
	rdfs:comment "A Staff-Captain (staabikapten in Estonian language), was an Estonian military rank in the Naval forces of Estonia, which existed between 1918 in 1922."@en ;
	rdfs:label "Staabikapten"@en ;
	owl:sameAs <dbpedia:Staabikapten> ;
	foaf:name "Staabikapten" .

:Rank_Staabikapten_Estonia org:rankOf <dbpedia:Estonia> ;
	a :MilitaryRank ;
	rdfs:comment "The specific instance of the Staabikapten rank in the context of country Estonia."@en ;
	rdfs:label "Staabikapten (Estland)"@de , "Staabikapten (Estland)"@nl , "Staabikapten (Estland)"@no , "Staabikapten (Estland)"@sv , "Staabikapten (Estonia)"@en , "Staabikapten (Estonia)"@es , "Staabikapten (Estonia)"@it , "Staabikapten (Estonia)"@pl , "Staabikapten (Estonie)"@fr , "Staabikapten (Estónia)"@pt , "Staabikapten (Viro)"@fi , "Staabikapten (Эстония)"@ru ;
	owl:subClass :Rank_Staabikapten ;
	foaf:name "Staabikapten"@en .

:Rank_Staabikapten_Republic_of_Estonia_1920-1940 org:rankOf <dbpedia:Republic_of_Estonia_%281920-1940%29> ;
	a :MilitaryRank ;
	rdfs:comment "The specific instance of the Staabikapten rank in the context of the Republic of Estonia, 1920-1940."@en ;
	rdfs:label "Staabikapten (Republic of Estonia, 1920-1940)"@en ;
	owl:subClass :Rank_Staabikapten ;
	foaf:name "Staabikapten"@en .

:Rank_Stabskapitan a :MilitaryRank ;
	rdfs:comment "Stabskapitän (staff captain) is a historic military rank, used in the Prussian and Russian armies. It ranked between the Premierleutnant and Hauptmann/Rittmeister in the Prussian army, and between lieutenant and captain in the Russian army."@en ;
	rdfs:label "Alikapteeni"@fi , "Stabskapitän"@de , "Stabskapitän"@en , "Sztabskapitan"@pl , "Штабс-капитан"@ru ;
	owl:sameAs <dbpedia:Stabskapit%C3%A4n> ;
	foaf:name "Stabskapitän" .

:Rank_Stabskapitan_Germany org:rankOf <dbpedia:Germany> ;
	a :MilitaryRank ;
	rdfs:comment "The specific instance of the Stabskapitän rank in the context of Germany."@en ;
	rdfs:label "Alikapteeni (Germany)"@fi , "Stabskapitän (Germany)"@de , "Stabskapitän (Germany)"@en , "Sztabskapitan (Germany)"@pl , "Штабс-капитан (Germany)"@ru ;
	owl:subClass :Rank_Stabskapitan ;
	foaf:name "Stabskapitän"@de .

:Rank_Stabskapitan_Russia org:rankOf <dbpedia:Russia> ;
	a :MilitaryRank ;
	rdfs:comment "The specific instance of the Stabskapitän rank in the context of country Russia."@en ;
	rdfs:label "Alikapteeni (Venäjä)"@fi , "Stabskapitän (Rusia)"@es , "Stabskapitän (Rusland)"@nl , "Stabskapitän (Russia)"@en , "Stabskapitän (Russia)"@it , "Stabskapitän (Russie)"@fr , "Stabskapitän (Russland)"@de , "Stabskapitän (Russland)"@no , "Stabskapitän (Ryssland)"@sv , "Stabskapitän (Rússia)"@pt , "Sztabskapitan (Rosja)"@pl , "Штабс-капитан (Россия)"@ru ;
	owl:subClass :Rank_Stabskapitan ;
	foaf:name "Штабс-капитан"@ru .

:Rank_Stabskapitan_Soviet_Union org:rankOf <dbpedia:Soviet_Union> ;
	a :MilitaryRank ;
	rdfs:comment "The specific instance of the Stabskapitän rank in the context of country Soviet Union."@en ;
	rdfs:label "Alikapteeni (Neuvostoliitto)"@fi , "Stabskapitän (Soviet Union)"@en , "Stabskapitän (Sovjet-Unie)"@nl , "Stabskapitän (Sovjetunionen)"@no , "Stabskapitän (Sovjetunionen)"@sv , "Stabskapitän (Sowjetunion)"@de , "Stabskapitän (Union des républiques socialistes soviétiques)"@fr , "Stabskapitän (Unione Sovietica)"@it , "Stabskapitän (União Soviética)"@pt , "Stabskapitän (Unión Soviética)"@es , "Sztabskapitan (Związek Socjalistycznych Republik Radzieckich)"@pl , "Штабс-капитан (Союз Советских Социалистических Республик)"@ru ;
	owl:subClass :Rank_Stabskapitan ;
	foaf:name "Stabskapitän"@en .

:Rank_Stabskapitanleutnant_Germany org:rankOf <dbpedia:Germany> ;
	a :MilitaryRank ;
	rdfs:comment "The specific instance of the Stabskapitänleutnant rank in the context of Germany."@en ;
	rdfs:label "Stabskapitänleutnant (Germany)"@de , "Stabskapitänleutnant (Germany)"@en ;
	owl:subClass :Rank_Stabskapitanleutnant ;
	foaf:name "Stabskapitänleutnant"@de .

:Rank_Staff_Corporal a :MilitaryRank ;
	rdfs:comment "Staff Corporal (SCpl or S/Cpl) is the equivalent rank to Staff Sergeant in the Household Cavalry, ranking between Corporal of Horse and Warrant Officer Class 2. He may hold an appointment such as Squadron Quartermaster Corporal. A Staff Corporal wears four point-up rank chevrons on his cuff, surmounted by a crown."@en ;
	rdfs:label "Staff Corporal"@en ;
	owl:sameAs <dbpedia:Staff_Corporal> ;
	foaf:name "Staff Corporal" .

:Rank_Staff_Corporal_England org:rankOf <dbpedia:England> ;
	a :MilitaryRank ;
	rdfs:comment "The specific instance of the Staff Corporal rank in the context of England."@en ;
	rdfs:label "Staff Corporal (England)"@en ;
	owl:subClass :Rank_Staff_Corporal ;
	foaf:name "Staff Corporal"@en .

:Rank_Staff_Corporal_Scotland org:rankOf <dbpedia:Scotland> ;
	a :MilitaryRank ;
	rdfs:comment "The specific instance of the Staff Corporal rank in the context of country Scotland."@en ;
	rdfs:label "Staff Corporal (Escocia)"@es , "Staff Corporal (Escócia)"@pt , "Staff Corporal (Schotland)"@nl , "Staff Corporal (Schottland)"@de , "Staff Corporal (Scotland)"@en , "Staff Corporal (Scozia)"@it , "Staff Corporal (Skotlanti)"@fi , "Staff Corporal (Skottland)"@no , "Staff Corporal (Skottland)"@sv , "Staff Corporal (Szkocja)"@pl , "Staff Corporal (Écosse)"@fr , "Staff Corporal (Шотландия)"@ru ;
	owl:subClass :Rank_Staff_Corporal ;
	foaf:name "Staff Corporal"@en .

:Rank_Staff_Corporal_Wales org:rankOf <dbpedia:Wales> ;
	a :MilitaryRank ;
	rdfs:comment "The specific instance of the Staff Corporal rank in the context of country Wales."@en ;
	rdfs:label "Staff Corporal (Gales)"@es , "Staff Corporal (Galles)"@it , "Staff Corporal (Pays de Galles)"@fr , "Staff Corporal (País de Gales)"@pt , "Staff Corporal (Wales)"@de , "Staff Corporal (Wales)"@en , "Staff Corporal (Wales)"@fi , "Staff Corporal (Wales)"@nl , "Staff Corporal (Wales)"@no , "Staff Corporal (Wales)"@sv , "Staff Corporal (Walia)"@pl , "Staff Corporal (Уэльс)"@ru ;
	owl:subClass :Rank_Staff_Corporal ;
	foaf:name "Staff Corporal"@en .

:Rank_Staff_Sergeant_Major a :MilitaryRank ;
	rdfs:label "Staff Sergeant Major"@en ;
	owl:sameAs <dbpedia:Staff_Sergeant_Major> ;
	foaf:name "Staff Sergeant Major" .

:Rank_Staff_Sergeant_Major_England org:rankOf <dbpedia:England> ;
	a :MilitaryRank ;
	rdfs:comment "The specific instance of the Staff Sergeant Major rank in the context of England."@en ;
	rdfs:label "Staff Sergeant Major (England)"@en ;
	owl:subClass :Rank_Staff_Sergeant_Major ;
	foaf:name "Staff Sergeant Major"@en .

:Rank_Staff_Sergeant_Major_Scotland org:rankOf <dbpedia:Scotland> ;
	a :MilitaryRank ;
	rdfs:comment "The specific instance of the Staff Sergeant Major rank in the context of country Scotland."@en ;
	rdfs:label "Staff Sergeant Major (Escocia)"@es , "Staff Sergeant Major (Escócia)"@pt , "Staff Sergeant Major (Schotland)"@nl , "Staff Sergeant Major (Schottland)"@de , "Staff Sergeant Major (Scotland)"@en , "Staff Sergeant Major (Scozia)"@it , "Staff Sergeant Major (Skotlanti)"@fi , "Staff Sergeant Major (Skottland)"@no , "Staff Sergeant Major (Skottland)"@sv , "Staff Sergeant Major (Szkocja)"@pl , "Staff Sergeant Major (Écosse)"@fr , "Staff Sergeant Major (Шотландия)"@ru ;
	owl:subClass :Rank_Staff_Sergeant_Major ;
	foaf:name "Staff Sergeant Major"@en .

:Rank_Staff_Sergeant_Major_Wales org:rankOf <dbpedia:Wales> ;
	a :MilitaryRank ;
	rdfs:comment "The specific instance of the Staff Sergeant Major rank in the context of country Wales."@en ;
	rdfs:label "Staff Sergeant Major (Gales)"@es , "Staff Sergeant Major (Galles)"@it , "Staff Sergeant Major (Pays de Galles)"@fr , "Staff Sergeant Major (País de Gales)"@pt , "Staff Sergeant Major (Wales)"@de , "Staff Sergeant Major (Wales)"@en , "Staff Sergeant Major (Wales)"@fi , "Staff Sergeant Major (Wales)"@nl , "Staff Sergeant Major (Wales)"@no , "Staff Sergeant Major (Wales)"@sv , "Staff Sergeant Major (Walia)"@pl , "Staff Sergeant Major (Уэльс)"@ru ;
	owl:subClass :Rank_Staff_Sergeant_Major ;
	foaf:name "Staff Sergeant Major"@en .

:Rank_Staff_sergeant a :MilitaryRank ;
	rdfs:label "Staff sergeant"@en ;
	owl:sameAs <dbpedia:Staff_sergeant> ;
	foaf:name "Staff sergeant" .

:Rank_Staff_sergeant_Australia org:rankOf <dbpedia:Australia> ;
	a :MilitaryRank ;
	rdfs:comment "The specific instance of the Staff sergeant rank in the context of country Australia."@en ;
	rdfs:label "Staff sergeant (Australia)"@en , "Staff sergeant (Australia)"@es , "Staff sergeant (Australia)"@fi , "Staff sergeant (Australia)"@it , "Staff sergeant (Australia)"@no , "Staff sergeant (Australia)"@pl , "Staff sergeant (Australie)"@fr , "Staff sergeant (Australien)"@de , "Staff sergeant (Australien)"@sv , "Staff sergeant (Australië (land))"@nl , "Staff sergeant (Austrália)"@pt , "Staff sergeant (Австралия)"@ru ;
	owl:subClass :Rank_Staff_sergeant ;
	foaf:name "Staff sergeant"@en .

:Rank_Staff_sergeant_Canada org:rankOf <dbpedia:Canada> ;
	a :MilitaryRank ;
	rdfs:comment "The specific instance of the Staff sergeant rank in the context of Canada."@en ;
	rdfs:label "Staff sergeant (Canada)"@en ;
	owl:subClass :Rank_Staff_sergeant ;
	foaf:name "Staff sergeant"@en .

:Rank_Staff_sergeant_Commonwealth_of_Nations org:rankOf <dbpedia:Commonwealth_of_Nations> ;
	a :MilitaryRank ;
	rdfs:comment "The specific instance of the Staff sergeant rank in the context of country Commonwealth of Nations."@en ;
	rdfs:label "Staff sergeant (Commonwealth delle nazioni)"@it , "Staff sergeant (Commonwealth of Nations)"@de , "Staff sergeant (Commonwealth of Nations)"@en , "Staff sergeant (Commonwealth of Nations)"@fr , "Staff sergeant (Commonwealth)"@pt , "Staff sergeant (Gemenebest van Naties)"@nl , "Staff sergeant (Kansainyhteisö)"@fi , "Staff sergeant (Mancomunidad de Naciones)"@es , "Staff sergeant (Samveldet av nasjoner)"@no , "Staff sergeant (Samväldet)"@sv , "Staff sergeant (Wspólnota Narodów)"@pl , "Staff sergeant (Содружество наций)"@ru ;
	owl:subClass :Rank_Staff_sergeant ;
	foaf:name "Staff sergeant"@en .

:Rank_Staff_sergeant_Singapore org:rankOf <dbpedia:Singapore> ;
	a :MilitaryRank ;
	rdfs:comment "The specific instance of the Staff sergeant rank in the context of country Singapore."@en ;
	rdfs:label "Staff sergeant (Singapore)"@en , "Staff sergeant (Singapore)"@fi , "Staff sergeant (Singapore)"@it , "Staff sergeant (Singapore)"@nl , "Staff sergeant (Singapore)"@no , "Staff sergeant (Singapore)"@sv , "Staff sergeant (Singapour)"@fr , "Staff sergeant (Singapur)"@de , "Staff sergeant (Singapur)"@es , "Staff sergeant (Singapur)"@pl , "Staff sergeant (Singapura)"@pt , "Staff sergeant (Сингапур)"@ru ;
	owl:subClass :Rank_Staff_sergeant ;
	foaf:name "Staff sergeant"@en .

:Rank_Starshina a :MilitaryRank ;
	rdfs:comment "Starshina, or Starshyna, initially was a Cossacks officership, but in Soviet times was used as the top non-commissioned officer. Among Cossacks and in Ukraine, starshina was a collective noun for categories of officership or a military elite: junior starshina (Молодша старшина), general starshina (Генеральна старшина), military starshina (Військова старшина), substarshina (Підстаршина)."@en ;
	rdfs:label "Starshina"@en , "Starshiná"@es , "Старшина"@ru ;
	owl:sameAs <dbpedia:Starshina> ;
	foaf:name "Starshina" .

:Rank_Starshina_Russia org:rankOf <dbpedia:Russia> ;
	a :MilitaryRank ;
	rdfs:comment "The specific instance of the Starshina rank in the context of country Russia."@en ;
	rdfs:label "Starshina (Rosja)"@pl , "Starshina (Rusland)"@nl , "Starshina (Russia)"@en , "Starshina (Russia)"@it , "Starshina (Russie)"@fr , "Starshina (Russland)"@de , "Starshina (Russland)"@no , "Starshina (Ryssland)"@sv , "Starshina (Rússia)"@pt , "Starshina (Venäjä)"@fi , "Starshiná (Rusia)"@es , "Старшина (Россия)"@ru ;
	owl:subClass :Rank_Starshina ;
	foaf:name "Старшина"@ru .

:Rank_Starshina_Soviet_Union org:rankOf <dbpedia:Soviet_Union> ;
	a :MilitaryRank ;
	rdfs:comment "The specific instance of the Starshina rank in the context of country Soviet Union."@en ;
	rdfs:label "Starshina (Neuvostoliitto)"@fi , "Starshina (Soviet Union)"@en , "Starshina (Sovjet-Unie)"@nl , "Starshina (Sovjetunionen)"@no , "Starshina (Sovjetunionen)"@sv , "Starshina (Sowjetunion)"@de , "Starshina (Union des républiques socialistes soviétiques)"@fr , "Starshina (Unione Sovietica)"@it , "Starshina (União Soviética)"@pt , "Starshina (Związek Socjalistycznych Republik Radzieckich)"@pl , "Starshiná (Unión Soviética)"@es , "Старшина (Союз Советских Социалистических Республик)"@ru ;
	owl:subClass :Rank_Starshina ;
	foaf:name "Starshina"@en .

:Rank_Starshina_Ukraine org:rankOf <dbpedia:Ukraine> ;
	a :MilitaryRank ;
	rdfs:comment "The specific instance of the Starshina rank in the context of country Ukraine."@en ;
	rdfs:label "Starshina (Oekraïne)"@nl , "Starshina (Ucraina)"@it , "Starshina (Ucrânia)"@pt , "Starshina (Ukraina)"@fi , "Starshina (Ukraina)"@no , "Starshina (Ukraina)"@pl , "Starshina (Ukraina)"@sv , "Starshina (Ukraine)"@de , "Starshina (Ukraine)"@en , "Starshina (Ukraine)"@fr , "Starshiná (Ucrania)"@es , "Старшина (Украина)"@ru ;
	owl:subClass :Rank_Starshina ;
	foaf:name "Старшина"@ru .

:Rank_Stratarches a :MilitaryRank ;
	rdfs:comment "Stratarches, means \"master/ruler of the army\" in Greek, and is a title associated with successful generals. In modern Greek usage, it corresponds to the rank of Field Marshal."@en ;
	rdfs:label "Stratarches"@en ;
	owl:sameAs <dbpedia:Stratarches> ;
	foaf:name "Stratarches" .

:Rank_Stratarches_Byzantine_Empire org:rankOf <dbpedia:Byzantine_Empire> ;
	a :MilitaryRank ;
	rdfs:comment "The specific instance of the Stratarches rank in the context of country Byzantine Empire."@en ;
	rdfs:label "Stratarches (Bysantin valtakunta)"@fi , "Stratarches (Bysantinska riket)"@sv , "Stratarches (Byzantijnse Rijk)"@nl , "Stratarches (Byzantine Empire)"@en , "Stratarches (Byzantinisches Reich)"@de , "Stratarches (Cesarstwo Bizantyńskie)"@pl , "Stratarches (Empire byzantin)"@fr , "Stratarches (Imperio bizantino)"@es , "Stratarches (Impero bizantino)"@it , "Stratarches (Império Bizantino)"@pt , "Stratarches (Østromerriket)"@no , "Stratarches (Византийская империя)"@ru ;
	owl:subClass :Rank_Stratarches ;
	foaf:name "Stratarches"@en .

:Rank_Stratarches_Greece org:rankOf <dbpedia:Greece> ;
	a :MilitaryRank ;
	rdfs:comment "The specific instance of the Stratarches rank in the context of country Greece."@en ;
	rdfs:label "Stratarches (Grecia)"@es , "Stratarches (Grecia)"@it , "Stratarches (Grecja)"@pl , "Stratarches (Greece)"@en , "Stratarches (Grekland)"@sv , "Stratarches (Griechenland)"@de , "Stratarches (Griekenland)"@nl , "Stratarches (Grèce)"@fr , "Stratarches (Grécia)"@pt , "Stratarches (Hellas)"@no , "Stratarches (Kreikka)"@fi , "Stratarches (Греция)"@ru ;
	owl:subClass :Rank_Stratarches ;
	foaf:name "Stratarches"@en .

:Rank_Stratarches_Official_Timocracy_of_Sapinetia org:rankOf <dbpedia:Official_Timocracy_of_Sapinetia> ;
	a :MilitaryRank ;
	rdfs:comment "The specific instance of the Stratarches rank in the context of country the Timocracy of Sapinetia."@en ;
	rdfs:label "Stratarches (Timocracy of Sapinetia)"@en ;
	owl:subClass :Rank_Stratarches ;
	foaf:name "Stratarches"@en .

:Rank_Strategos a :MilitaryRank ;
	rdfs:comment "Strategos, plural strategoi, is used in Greek to mean \"general\". In the Hellenistic and Byzantine Empires the term was also used to describe a military governor. In the modern Hellenic Army, it is the highest officer rank."@en ;
	rdfs:label "Estratego"@pt , "Strateg (Grecja)"@pl , "Strategos"@de , "Strategos"@en , "Strategos"@es , "Strategos"@fi , "Strategos"@it , "Strategos"@nl , "Strategos"@no , "Stratège"@fr , "Стратег"@ru ;
	owl:sameAs <dbpedia:Strategos> ;
	foaf:name "Strategos" .

:Rank_Strategos_Achaean_League org:rankOf <dbpedia:Achaean_League> ;
	a :MilitaryRank ;
	rdfs:comment "The specific instance of the Strategos rank in the context of country Achaean League."@en ;
	rdfs:label "Estratego (Liga Aqueia)"@pt , "Strateg (Grecja) (Związek Achajski)"@pl , "Strategos (Achaean League)"@en , "Strategos (Achaeïsche Bond)"@nl , "Strategos (Achaiischer Bund)"@de , "Strategos (Achaiska förbundet)"@sv , "Strategos (Akhaian liitto)"@fi , "Strategos (Det akhaiske forbund)"@no , "Strategos (Lega achea)"@it , "Strategos (Liga Aquea)"@es , "Stratège (Ligue achéenne)"@fr , "Стратег (Ахейский союз)"@ru ;
	owl:subClass :Rank_Strategos ;
	foaf:name "Strategos"@en .

:Rank_Strategos_Byzantine_Empire org:rankOf <dbpedia:Byzantine_Empire> ;
	a :MilitaryRank ;
	rdfs:comment "The specific instance of the Strategos rank in the context of country Byzantine Empire."@en ;
	rdfs:label "Estratego (Império Bizantino)"@pt , "Strateg (Grecja) (Cesarstwo Bizantyńskie)"@pl , "Strategos (Bysantin valtakunta)"@fi , "Strategos (Bysantinska riket)"@sv , "Strategos (Byzantijnse Rijk)"@nl , "Strategos (Byzantine Empire)"@en , "Strategos (Byzantinisches Reich)"@de , "Strategos (Imperio bizantino)"@es , "Strategos (Impero bizantino)"@it , "Strategos (Østromerriket)"@no , "Stratège (Empire byzantin)"@fr , "Стратег (Византийская империя)"@ru ;
	owl:subClass :Rank_Strategos ;
	foaf:name "Strategos"@en .

:Rank_Strategos_Greece org:rankOf <dbpedia:Greece> ;
	a :MilitaryRank ;
	rdfs:comment "The specific instance of the Strategos rank in the context of country Greece."@en ;
	rdfs:label "Estratego (Grécia)"@pt , "Strateg (Grecja) (Grecja)"@pl , "Strategos (Grecia)"@es , "Strategos (Grecia)"@it , "Strategos (Greece)"@en , "Strategos (Grekland)"@sv , "Strategos (Griechenland)"@de , "Strategos (Griekenland)"@nl , "Strategos (Hellas)"@no , "Strategos (Kreikka)"@fi , "Stratège (Grèce)"@fr , "Стратег (Греция)"@ru ;
	owl:subClass :Rank_Strategos ;
	foaf:name "Strategos"@en .

:Rank_Strategos_Macedonia org:rankOf <dbpedia:Macedonia_%28ancient_kingdom%29> ;
	a :MilitaryRank ;
	rdfs:comment "The specific instance of the Strategos rank in the context of country Macedonia (ancient kingdom)."@en ;
	rdfs:label "Estratego (Macedónia Antiga)"@pt , "Strateg (Grecja) (Starożytna Macedonia)"@pl , "Strategos (Macedonia (ancient kingdom))"@de , "Strategos (Macedonia (ancient kingdom))"@en , "Strategos (Macedonië (oudheid))"@nl , "Strategos (Makedonian valtakunta)"@fi , "Strategos (Oldtidens Makedonia)"@no , "Strategos (Regno di Macedonia)"@it , "Strategos (Reino de Macedonia)"@es , "Stratège (Royaume de Macédoine)"@fr , "Стратег (Древняя Македония)"@ru ;
	owl:subClass :Rank_Strategos ;
	foaf:name "Strategos"@en .

:Rank_Strategos_Official_Timocracy_of_Sapinetia org:rankOf <dbpedia:Official_Timocracy_of_Sapinetia> ;
	a :MilitaryRank ;
	rdfs:comment "The specific instance of the Strategos rank in the context of the Timocracy of Sapinetia."@en ;
	rdfs:label "Estratego (Timocracy of Sapinetia)"@pt , "Strateg (Grecja) (Timocracy of Sapinetia)"@pl , "Strategos (Timocracy of Sapinetia)"@de , "Strategos (Timocracy of Sapinetia)"@en , "Strategos (Timocracy of Sapinetia)"@es , "Strategos (Timocracy of Sapinetia)"@fi , "Strategos (Timocracy of Sapinetia)"@it , "Strategos (Timocracy of Sapinetia)"@nl , "Strategos (Timocracy of Sapinetia)"@no , "Stratège (Timocracy of Sapinetia)"@fr , "Стратег (Timocracy of Sapinetia)"@ru ;
	owl:subClass :Rank_Strategos ;
	foaf:name "Strategos"@en .

:Rank_Strategos_autokrator_Byzantine_Empire org:rankOf <dbpedia:Byzantine_Empire> ;
	a :MilitaryRank ;
	rdfs:comment "The specific instance of the Strategos autokrator rank in the context of country Byzantine Empire."@en ;
	rdfs:label "Strategos autokrator (Bysantin valtakunta)"@fi , "Strategos autokrator (Bysantinska riket)"@sv , "Strategos autokrator (Byzantijnse Rijk)"@nl , "Strategos autokrator (Byzantine Empire)"@en , "Strategos autokrator (Byzantinisches Reich)"@de , "Strategos autokrator (Cesarstwo Bizantyńskie)"@pl , "Strategos autokrator (Empire byzantin)"@fr , "Strategos autokrator (Imperio bizantino)"@es , "Strategos autokrator (Impero bizantino)"@it , "Strategos autokrator (Império Bizantino)"@pt , "Strategos autokrator (Østromerriket)"@no , "Strategos autokrator (Византийская империя)"@ru ;
	owl:subClass :Rank_Strategos_autokrator ;
	foaf:name "Strategos autokrator"@en .

:Rank_Sub-lieutenant_EnglishTradition org:rankEquivalentTo :Rank_Flying_officer_EnglishTradition , :Rank_Lieutenant_EnglishTradition ;
	org:rankJuniorToTransitive <http://rdf.muninn-project.org/ontologies/military#Rank_Lieutenant_(navy)_EnglishTradition> ;
	org:rankOf :EnglishTradition , <mil:NavyServiceBranch> ;
	org:rankSeniorToTransitive <http://rdf.muninn-project.org/ontologies/military#Rank_Ensign_(rank)_EnglishTradition> ;
	a :MilitaryRank ;
	rdfs:label "Sub-lieutenant"@en ;
	owl:sameAs <dbpedia:Sub-lieutenant> .

:Rank_Suba%C5%9Fi a :MilitaryRank ;
	rdfs:comment "Subaşi was an Ottoman gubernatorial title used to describe different positions within Ottoman hierarchy, depending on the context. This title was given to sanjak-beys of Ottoman sanjaks which generated more than 15,000 aspers per annum or to the assistants of the sanjabey. The term was also used for commander of the town or castle in Ottoman Empire, an ancient version of chief of police. A surname found among Balkan families, Subaša or Subašić, is derived from the Subaşi title."@en ;
	rdfs:label "Subaşi"@en ;
	owl:sameAs <dbpedia:Suba%C5%9Fi> ;
	foaf:name "Subaşi" .

:Rank_Subaltern a :MilitaryRank ;
	rdfs:comment "A subaltern is a chiefly British military term for a junior officer. Literally meaning \"subordinate,\" subaltern is used to describe commissioned officers below the rank of captain and generally comprises the various grades of lieutenant. In the British Army the senior subaltern rank was captain-lieutenant, obsolete since the 18th century."@en ;
	rdfs:label "Subaltern"@en , "Subalternofficer"@sv , "Subalternoffiser"@no , "Субалтерн-офицер"@ru ;
	owl:sameAs <dbpedia:Subaltern> ;
	foaf:name "Subaltern" .

:Rank_Subaltern_England org:rankOf <dbpedia:England> ;
	a :MilitaryRank ;
	rdfs:comment "The specific instance of the Subaltern rank in the context of England."@en ;
	rdfs:label "Subaltern (England)"@en , "Subalternofficer (England)"@sv , "Subalternoffiser (England)"@no , "Субалтерн-офицер (England)"@ru ;
	owl:subClass :Rank_Subaltern ;
	foaf:name "Subaltern"@en .

:Rank_Subaltern_Scotland org:rankOf <dbpedia:Scotland> ;
	a :MilitaryRank ;
	rdfs:comment "The specific instance of the Subaltern rank in the context of country Scotland."@en ;
	rdfs:label "Subaltern (Escocia)"@es , "Subaltern (Escócia)"@pt , "Subaltern (Schotland)"@nl , "Subaltern (Schottland)"@de , "Subaltern (Scotland)"@en , "Subaltern (Scozia)"@it , "Subaltern (Skotlanti)"@fi , "Subaltern (Szkocja)"@pl , "Subaltern (Écosse)"@fr , "Subalternofficer (Skottland)"@sv , "Subalternoffiser (Skottland)"@no , "Субалтерн-офицер (Шотландия)"@ru ;
	owl:subClass :Rank_Subaltern ;
	foaf:name "Subaltern"@en .

:Rank_Subaltern_Wales org:rankOf <dbpedia:Wales> ;
	a :MilitaryRank ;
	rdfs:comment "The specific instance of the Subaltern rank in the context of country Wales."@en ;
	rdfs:label "Subaltern (Gales)"@es , "Subaltern (Galles)"@it , "Subaltern (Pays de Galles)"@fr , "Subaltern (País de Gales)"@pt , "Subaltern (Wales)"@de , "Subaltern (Wales)"@en , "Subaltern (Wales)"@fi , "Subaltern (Wales)"@nl , "Subaltern (Walia)"@pl , "Subalternofficer (Wales)"@sv , "Subalternoffiser (Wales)"@no , "Субалтерн-офицер (Уэльс)"@ru ;
	owl:subClass :Rank_Subaltern ;
	foaf:name "Subaltern"@en .

:Rank_Subasi_Cossack_Hetmanate org:rankOf <dbpedia:Cossack_Hetmanate> ;
	a :MilitaryRank ;
	rdfs:comment "The specific instance of the Subaşi rank in the context of country Cossack Hetmanate."@en ;
	rdfs:label "Subaşi (Cossack Hetmanate)"@en , "Subaşi (Hetmanat cosaque)"@fr , "Subaşi (Hetmanat)"@de , "Subaşi (Hetmanato cosaco)"@es , "Subaşi (Hetmańszczyzna)"@pl , "Subaşi (Гетманщина)"@ru ;
	owl:subClass :Rank_Subasi ;
	foaf:name "Subaşi"@en .

:Rank_Subasi_Ottoman_Empire org:rankOf <dbpedia:Ottoman_Empire> ;
	a :MilitaryRank ;
	rdfs:comment "The specific instance of the Subaşi rank in the context of country Ottoman Empire."@en ;
	rdfs:label "Subaşi (Det osmanske rike)"@no , "Subaşi (Empire ottoman)"@fr , "Subaşi (Imperio otomano)"@es , "Subaşi (Imperium osmańskie)"@pl , "Subaşi (Impero ottomano)"@it , "Subaşi (Império Otomano)"@pt , "Subaşi (Osmanien valtakunta)"@fi , "Subaşi (Osmanisches Reich)"@de , "Subaşi (Osmanska riket)"@sv , "Subaşi (Ottomaanse Rijk)"@nl , "Subaşi (Ottoman Empire)"@en , "Subaşi (Османская империя)"@ru ;
	owl:subClass :Rank_Subasi ;
	foaf:name "Subaşi"@en .

:Rank_Subasi_Septinsular_Republic org:rankOf <dbpedia:Septinsular_Republic> ;
	a :MilitaryRank ;
	rdfs:comment "The specific instance of the Subaşi rank in the context of country Septinsular Republic."@en ;
	rdfs:label "Subaşi (Repubblica delle Sette Isole Unite)"@it , "Subaşi (Republiek van de Zeven Eilanden)"@nl , "Subaşi (Republika Siedmiu Wysp)"@pl , "Subaşi (República de las Islas Jónicas)"@es , "Subaşi (République des Sept-Îles)"@fr , "Subaşi (Septinsular Republic)"@en , "Subaşi (Республика Семи Островов)"@ru ;
	owl:subClass :Rank_Subasi ;
	foaf:name "Subaşi"@en .

:Rank_Syntagmatarchis a :MilitaryRank ;
	rdfs:comment "Syntagmatarchis, sometimes anglicized as Syntagmatarch, is used in modern Greek to denote the rank of Colonel. It is translated as \"leader of a regiment (syntagma)\", and dates back to the Classical Age armies. However, the name is misleading in that the Hellenic Army retains very few regiments in its command structure. Thus, the typical responsibilities of Syntagmatarches are in staff positions, or as Executive Officers in brigades."@en ;
	rdfs:label "Syntagmatarchis"@en ;
	owl:sameAs <dbpedia:Syntagmatarchis> ;
	foaf:name "Syntagmatarchis" .

:Rank_Syntagmatarchis_Achaean_League org:rankOf <dbpedia:Achaean_League> ;
	a :MilitaryRank ;
	rdfs:comment "The specific instance of the Syntagmatarchis rank in the context of country Achaean League."@en ;
	rdfs:label "Syntagmatarchis (Achaean League)"@en , "Syntagmatarchis (Achaeïsche Bond)"@nl , "Syntagmatarchis (Achaiischer Bund)"@de , "Syntagmatarchis (Achaiska förbundet)"@sv , "Syntagmatarchis (Akhaian liitto)"@fi , "Syntagmatarchis (Det akhaiske forbund)"@no , "Syntagmatarchis (Lega achea)"@it , "Syntagmatarchis (Liga Aquea)"@es , "Syntagmatarchis (Liga Aqueia)"@pt , "Syntagmatarchis (Ligue achéenne)"@fr , "Syntagmatarchis (Związek Achajski)"@pl , "Syntagmatarchis (Ахейский союз)"@ru ;
	owl:subClass :Rank_Syntagmatarchis ;
	foaf:name "Syntagmatarchis"@en .

:Rank_Syntagmatarchis_Greece org:rankOf <dbpedia:Greece> ;
	a :MilitaryRank ;
	rdfs:comment "The specific instance of the Syntagmatarchis rank in the context of country Greece."@en ;
	rdfs:label "Syntagmatarchis (Grecia)"@es , "Syntagmatarchis (Grecia)"@it , "Syntagmatarchis (Grecja)"@pl , "Syntagmatarchis (Greece)"@en , "Syntagmatarchis (Grekland)"@sv , "Syntagmatarchis (Griechenland)"@de , "Syntagmatarchis (Griekenland)"@nl , "Syntagmatarchis (Grèce)"@fr , "Syntagmatarchis (Grécia)"@pt , "Syntagmatarchis (Hellas)"@no , "Syntagmatarchis (Kreikka)"@fi , "Syntagmatarchis (Греция)"@ru ;
	owl:subClass :Rank_Syntagmatarchis ;
	foaf:name "Syntagmatarchis"@en .

:Rank_Syntagmatarchis_Macedonia org:rankOf <dbpedia:Macedonia_%28ancient_kingdom%29> ;
	a :MilitaryRank ;
	rdfs:comment "The specific instance of the Syntagmatarchis rank in the context of country Macedonia (ancient kingdom)."@en ;
	rdfs:label "Syntagmatarchis (Macedonia (ancient kingdom))"@en , "Syntagmatarchis (Macedonië (oudheid))"@nl , "Syntagmatarchis (Macedónia Antiga)"@pt , "Syntagmatarchis (Makedonian valtakunta)"@fi , "Syntagmatarchis (Oldtidens Makedonia)"@no , "Syntagmatarchis (Regno di Macedonia)"@it , "Syntagmatarchis (Reino de Macedonia)"@es , "Syntagmatarchis (Royaume de Macédoine)"@fr , "Syntagmatarchis (Starożytna Macedonia)"@pl , "Syntagmatarchis (Древняя Македония)"@ru ;
	owl:subClass :Rank_Syntagmatarchis ;
	foaf:name "Syntagmatarchis"@en .

:Rank_Syntagmatarchis_Official_Timocracy_of_Sapinetia org:rankOf <dbpedia:Official_Timocracy_of_Sapinetia> ;
	a :MilitaryRank ;
	rdfs:comment "The specific instance of the Syntagmatarchis rank in the context of the Timocracy of Sapinetia."@en ;
	rdfs:label "Syntagmatarchis (Timocracy of Sapinetia)"@en ;
	owl:subClass :Rank_Syntagmatarchis ;
	foaf:name "Syntagmatarchis"@en .

:Rank_Tagmatarchis a :MilitaryRank ;
	rdfs:comment "Tagmatarchis, in more archaic context transliterated as Tagmatarches, anglicized as Tagmatarch, is used in the Greek language to mean \"Major\". More precisely, it means \"commander of a tagma\". The rank dates to Antiquity and was also used in the Byzantine Empire. In the modern Hellenic Army, the rank is superior to a Lokhagos and inferior to an Antisyntagmatarchis, and held either usually by battalion (tagma) executive officers (battalions are typically commanded by Lieutenant Colonels)."@en ;
	rdfs:label "Tagmatarchis"@en ;
	owl:sameAs <dbpedia:Tagmatarchis> ;
	foaf:name "Tagmatarchis" .

:Rank_Tagmatarchis_Achaean_League org:rankOf <dbpedia:Achaean_League> ;
	a :MilitaryRank ;
	rdfs:comment "The specific instance of the Tagmatarchis rank in the context of country Achaean League."@en ;
	rdfs:label "Tagmatarchis (Achaean League)"@en , "Tagmatarchis (Achaeïsche Bond)"@nl , "Tagmatarchis (Achaiischer Bund)"@de , "Tagmatarchis (Achaiska förbundet)"@sv , "Tagmatarchis (Akhaian liitto)"@fi , "Tagmatarchis (Det akhaiske forbund)"@no , "Tagmatarchis (Lega achea)"@it , "Tagmatarchis (Liga Aquea)"@es , "Tagmatarchis (Liga Aqueia)"@pt , "Tagmatarchis (Ligue achéenne)"@fr , "Tagmatarchis (Związek Achajski)"@pl , "Tagmatarchis (Ахейский союз)"@ru ;
	owl:subClass :Rank_Tagmatarchis ;
	foaf:name "Tagmatarchis"@en .

:Rank_Tagmatarchis_Greece org:rankOf <dbpedia:Greece> ;
	a :MilitaryRank ;
	rdfs:comment "The specific instance of the Tagmatarchis rank in the context of country Greece."@en ;
	rdfs:label "Tagmatarchis (Grecia)"@es , "Tagmatarchis (Grecia)"@it , "Tagmatarchis (Grecja)"@pl , "Tagmatarchis (Greece)"@en , "Tagmatarchis (Grekland)"@sv , "Tagmatarchis (Griechenland)"@de , "Tagmatarchis (Griekenland)"@nl , "Tagmatarchis (Grèce)"@fr , "Tagmatarchis (Grécia)"@pt , "Tagmatarchis (Hellas)"@no , "Tagmatarchis (Kreikka)"@fi , "Tagmatarchis (Греция)"@ru ;
	owl:subClass :Rank_Tagmatarchis ;
	foaf:name "Tagmatarchis"@en .

:Rank_Tagmatarchis_Macedonia org:rankOf <dbpedia:Macedonia_%28ancient_kingdom%29> ;
	a :MilitaryRank ;
	rdfs:comment "The specific instance of the Tagmatarchis rank in the context of country Macedonia (ancient kingdom)."@en ;
	rdfs:label "Tagmatarchis (Macedonia (ancient kingdom))"@en , "Tagmatarchis (Macedonië (oudheid))"@nl , "Tagmatarchis (Macedónia Antiga)"@pt , "Tagmatarchis (Makedonian valtakunta)"@fi , "Tagmatarchis (Oldtidens Makedonia)"@no , "Tagmatarchis (Regno di Macedonia)"@it , "Tagmatarchis (Reino de Macedonia)"@es , "Tagmatarchis (Royaume de Macédoine)"@fr , "Tagmatarchis (Starożytna Macedonia)"@pl , "Tagmatarchis (Древняя Македония)"@ru ;
	owl:subClass :Rank_Tagmatarchis ;
	foaf:name "Tagmatarchis"@en .

:Rank_Tagmatarchis_Official_Timocracy_of_Sapinetia org:rankOf <dbpedia:Official_Timocracy_of_Sapinetia> ;
	a :MilitaryRank ;
	rdfs:comment "The specific instance of the Tagmatarchis rank in the context of the Timocracy of Sapinetia."@en ;
	rdfs:label "Tagmatarchis (Timocracy of Sapinetia)"@en ;
	owl:subClass :Rank_Tagmatarchis ;
	foaf:name "Tagmatarchis"@en .

:Rank_Taxiarch a :MilitaryRank ;
	rdfs:comment "Taxiarch, the anglicized form of taxiarchos or taxiarchēs is used in the Greek language to mean \"brigadier\". The term derives from táxis, \"order\", in military context \"an ordered formation\". In turn, the rank has given rise to the Greek term for brigade, taxiarchia. In Greek Orthodox usage, the term is also applied to the Archangels Michael and Gabriel, as leaders of the heavenly host, and several locations in Greece are named after them."@en ;
	rdfs:label "Taxiarch"@en , "Таксиарх"@ru ;
	owl:sameAs <dbpedia:Taxiarch> ;
	foaf:name "Taxiarch" .

:Rank_Taxiarch_Achaean_League org:rankOf <dbpedia:Achaean_League> ;
	a :MilitaryRank ;
	rdfs:comment "The specific instance of the Taxiarch rank in the context of country Achaean League."@en ;
	rdfs:label "Taxiarch (Achaean League)"@en , "Taxiarch (Achaeïsche Bond)"@nl , "Taxiarch (Achaiischer Bund)"@de , "Taxiarch (Achaiska förbundet)"@sv , "Taxiarch (Akhaian liitto)"@fi , "Taxiarch (Det akhaiske forbund)"@no , "Taxiarch (Lega achea)"@it , "Taxiarch (Liga Aquea)"@es , "Taxiarch (Liga Aqueia)"@pt , "Taxiarch (Ligue achéenne)"@fr , "Taxiarch (Związek Achajski)"@pl , "Таксиарх (Ахейский союз)"@ru ;
	owl:subClass :Rank_Taxiarch ;
	foaf:name "Taxiarch"@en .

:Rank_Taxiarch_Byzantine_Empire org:rankOf <dbpedia:Byzantine_Empire> ;
	a :MilitaryRank ;
	rdfs:comment "The specific instance of the Taxiarch rank in the context of country Byzantine Empire."@en ;
	rdfs:label "Taxiarch (Bysantin valtakunta)"@fi , "Taxiarch (Bysantinska riket)"@sv , "Taxiarch (Byzantijnse Rijk)"@nl , "Taxiarch (Byzantine Empire)"@en , "Taxiarch (Byzantinisches Reich)"@de , "Taxiarch (Cesarstwo Bizantyńskie)"@pl , "Taxiarch (Empire byzantin)"@fr , "Taxiarch (Imperio bizantino)"@es , "Taxiarch (Impero bizantino)"@it , "Taxiarch (Império Bizantino)"@pt , "Taxiarch (Østromerriket)"@no , "Таксиарх (Византийская империя)"@ru ;
	owl:subClass :Rank_Taxiarch ;
	foaf:name "Taxiarch"@en .

:Rank_Taxiarch_Greece org:rankOf <dbpedia:Greece> ;
	a :MilitaryRank ;
	rdfs:comment "The specific instance of the Taxiarch rank in the context of country Greece."@en ;
	rdfs:label "Taxiarch (Grecia)"@es , "Taxiarch (Grecia)"@it , "Taxiarch (Grecja)"@pl , "Taxiarch (Greece)"@en , "Taxiarch (Grekland)"@sv , "Taxiarch (Griechenland)"@de , "Taxiarch (Griekenland)"@nl , "Taxiarch (Grèce)"@fr , "Taxiarch (Grécia)"@pt , "Taxiarch (Hellas)"@no , "Taxiarch (Kreikka)"@fi , "Таксиарх (Греция)"@ru ;
	owl:subClass :Rank_Taxiarch ;
	foaf:name "Taxiarch"@en .

:Rank_Taxiarch_Macedonia org:rankOf <dbpedia:Macedonia_%28ancient_kingdom%29> ;
	a :MilitaryRank ;
	rdfs:comment "The specific instance of the Taxiarch rank in the context of country Macedonia (ancient kingdom)."@en ;
	rdfs:label "Taxiarch (Macedonia (ancient kingdom))"@en , "Taxiarch (Macedonië (oudheid))"@nl , "Taxiarch (Macedónia Antiga)"@pt , "Taxiarch (Makedonian valtakunta)"@fi , "Taxiarch (Oldtidens Makedonia)"@no , "Taxiarch (Regno di Macedonia)"@it , "Taxiarch (Reino de Macedonia)"@es , "Taxiarch (Royaume de Macédoine)"@fr , "Taxiarch (Starożytna Macedonia)"@pl , "Таксиарх (Древняя Македония)"@ru ;
	owl:subClass :Rank_Taxiarch ;
	foaf:name "Taxiarch"@en .

:Rank_Taxiarch_Official_Timocracy_of_Sapinetia org:rankOf <dbpedia:Official_Timocracy_of_Sapinetia> ;
	a :MilitaryRank ;
	rdfs:comment "The specific instance of the Taxiarch rank in the context of the Timocracy of Sapinetia."@en ;
	rdfs:label "Taxiarch (Timocracy of Sapinetia)"@en , "Таксиарх (Timocracy of Sapinetia)"@ru ;
	owl:subClass :Rank_Taxiarch ;
	foaf:name "Taxiarch"@en .

:Rank_Tetrarch a :MilitaryRank ;
	rdfs:label "Tetrarca"@pt , "Tetrarch"@de , "Tetrarch"@en , "Tetrarch"@nl , "Tetrark"@sv , "Tetrarkki"@fi , "Тетрарх (значения)"@ru ;
	owl:sameAs <dbpedia:Tetrarch> ;
	foaf:name "Tetrarch" .

:Rank_Tetrarch_Achaean_League org:rankOf <dbpedia:Achaean_League> ;
	a :MilitaryRank ;
	rdfs:comment "The specific instance of the Tetrarch rank in the context of country Achaean League."@en ;
	rdfs:label "Tetrarca (Liga Aqueia)"@pt , "Tetrarch (Achaean League)"@en , "Tetrarch (Achaeïsche Bond)"@nl , "Tetrarch (Achaiischer Bund)"@de , "Tetrarch (Det akhaiske forbund)"@no , "Tetrarch (Lega achea)"@it , "Tetrarch (Liga Aquea)"@es , "Tetrarch (Ligue achéenne)"@fr , "Tetrarch (Związek Achajski)"@pl , "Tetrark (Achaiska förbundet)"@sv , "Tetrarkki (Akhaian liitto)"@fi , "Тетрарх (значения) (Ахейский союз)"@ru ;
	owl:subClass :Rank_Tetrarch ;
	foaf:name "Tetrarch"@en .

:Rank_Tetrarch_Macedonia org:rankOf <dbpedia:Macedonia_%28ancient_kingdom%29> ;
	a :MilitaryRank ;
	rdfs:comment "The specific instance of the Tetrarch rank in the context of country Macedonia (ancient kingdom)."@en ;
	rdfs:label "Tetrarca (Macedónia Antiga)"@pt , "Tetrarch (Macedonia (ancient kingdom))"@de , "Tetrarch (Macedonia (ancient kingdom))"@en , "Tetrarch (Macedonië (oudheid))"@nl , "Tetrarch (Oldtidens Makedonia)"@no , "Tetrarch (Regno di Macedonia)"@it , "Tetrarch (Reino de Macedonia)"@es , "Tetrarch (Royaume de Macédoine)"@fr , "Tetrarch (Starożytna Macedonia)"@pl , "Tetrark (Macedonia (ancient kingdom))"@sv , "Tetrarkki (Makedonian valtakunta)"@fi , "Тетрарх (значения) (Древняя Македония)"@ru ;
	owl:subClass :Rank_Tetrarch ;
	foaf:name "Tetrarch"@en .

:Rank_Trierarch a :MilitaryRank ;
	rdfs:comment "Trierarch was the title of officers who commanded a trireme (triēres) in the classical Greek world. In Athens and a few other states this officer was also required to pay for the outfitting and maintenance of the ship. Trierarchs thus had to be men of considerable means, since the expenses incurred could run as high as a talent in the course of a year."@en ;
	rdfs:label "Trierarca"@es , "Trierarch"@en , "Trierarchia"@it , "Trierarchie"@de , "Trierark"@no , "Triérarchie"@fr , "Триерархия"@ru ;
	owl:sameAs <dbpedia:Trierarch> ;
	foaf:name "Trierarch" .

:Rank_Trierarch_Achaean_League org:rankOf <dbpedia:Achaean_League> ;
	a :MilitaryRank ;
	rdfs:comment "The specific instance of the Trierarch rank in the context of country Achaean League."@en ;
	rdfs:label "Trierarca (Liga Aquea)"@es , "Trierarch (Achaean League)"@en , "Trierarch (Achaeïsche Bond)"@nl , "Trierarch (Achaiska förbundet)"@sv , "Trierarch (Akhaian liitto)"@fi , "Trierarch (Liga Aqueia)"@pt , "Trierarch (Związek Achajski)"@pl , "Trierarchia (Lega achea)"@it , "Trierarchie (Achaiischer Bund)"@de , "Trierark (Det akhaiske forbund)"@no , "Triérarchie (Ligue achéenne)"@fr , "Триерархия (Ахейский союз)"@ru ;
	owl:subClass :Rank_Trierarch ;
	foaf:name "Trierarch"@en .

:Rank_Trierarch_Macedonia org:rankOf <dbpedia:Macedonia_%28ancient_kingdom%29> ;
	a :MilitaryRank ;
	rdfs:comment "The specific instance of the Trierarch rank in the context of country Macedonia (ancient kingdom)."@en ;
	rdfs:label "Trierarca (Reino de Macedonia)"@es , "Trierarch (Macedonia (ancient kingdom))"@en , "Trierarch (Macedonië (oudheid))"@nl , "Trierarch (Macedónia Antiga)"@pt , "Trierarch (Makedonian valtakunta)"@fi , "Trierarch (Starożytna Macedonia)"@pl , "Trierarchia (Regno di Macedonia)"@it , "Trierarchie (Macedonia (ancient kingdom))"@de , "Trierark (Oldtidens Makedonia)"@no , "Triérarchie (Royaume de Macédoine)"@fr , "Триерархия (Древняя Македония)"@ru ;
	owl:subClass :Rank_Trierarch ;
	foaf:name "Trierarch"@en .

:Rank_Trooper a :MilitaryRank ;
	rdfs:comment "Trooper (abbr. Tpr) from the French \"troupier\" is the equivalent rank to private in a regiment with a cavalry tradition in the British Army and many other Commonwealth armies, including those of Australia, Canada, South Africa and New Zealand. Today, most cavalry units operate in the armoured role, equipped with tanks or other armoured fighting vehicles. Some armoured regiments without a cavalry tradition do not use the rank, although the British Royal Tank Regiment does."@en ;
	rdfs:label "Trooper (rank)"@en ;
	owl:sameAs <dbpedia:Trooper_%28rank%29> ;
	foaf:name "Trooper" .

:Rank_Trooper_Australia org:rankOf <dbpedia:Australia> ;
	a :MilitaryRank ;
	rdfs:comment "The specific instance of the Trooper (rank) rank in the context of country Australia."@en ;
	rdfs:label "Trooper (rank) (Australia)"@en , "Trooper (rank) (Australia)"@es , "Trooper (rank) (Australia)"@fi , "Trooper (rank) (Australia)"@it , "Trooper (rank) (Australia)"@no , "Trooper (rank) (Australia)"@pl , "Trooper (rank) (Australie)"@fr , "Trooper (rank) (Australien)"@de , "Trooper (rank) (Australien)"@sv , "Trooper (rank) (Australië (land))"@nl , "Trooper (rank) (Austrália)"@pt , "Trooper (rank) (Австралия)"@ru ;
	owl:subClass :Rank_Trooper ;
	foaf:name "Trooper"@en .

:Rank_Trooper_Canada org:rankOf <dbpedia:Canada> ;
	a :MilitaryRank ;
	rdfs:comment "The specific instance of the Trooper (rank) rank in the context of Canada."@en ;
	rdfs:label "Trooper (rank, Canada)"@en ;
	owl:subClass :Rank_Trooper ;
	foaf:name "Trooper"@en .

:Rank_Trooper_Commonwealth_of_Nations org:rankOf <dbpedia:Commonwealth_of_Nations> ;
	a :MilitaryRank ;
	rdfs:comment "The specific instance of the Trooper (rank) rank in the context of country Commonwealth of Nations."@en ;
	rdfs:label "Trooper (rank) (Commonwealth delle nazioni)"@it , "Trooper (rank) (Commonwealth of Nations)"@de , "Trooper (rank) (Commonwealth of Nations)"@en , "Trooper (rank) (Commonwealth of Nations)"@fr , "Trooper (rank) (Commonwealth)"@pt , "Trooper (rank) (Gemenebest van Naties)"@nl , "Trooper (rank) (Kansainyhteisö)"@fi , "Trooper (rank) (Mancomunidad de Naciones)"@es , "Trooper (rank) (Samveldet av nasjoner)"@no , "Trooper (rank) (Samväldet)"@sv , "Trooper (rank) (Wspólnota Narodów)"@pl , "Trooper (rank) (Содружество наций)"@ru ;
	owl:subClass :Rank_Trooper ;
	foaf:name "Trooper"@en .

:Rank_Trumpet_Major a :MilitaryRank ;
	rdfs:comment "Trumpet Major is an appointment in British Army cavalry regiments or the Royal Horse Artillery, held by a Sergeant or a more senior non-commissioned officer or Warrant Officer. His job is to supervise the training and deployment of trumpeters who blow daily duty and ceremonial calls. Trumpet Majors were first appointed to the establishment in 1811. The trumpet was originally a signalling instrument, but it has become purely ceremonial since the invention of radio."@en ;
	rdfs:label "Trumpet Major"@en ;
	owl:sameAs <dbpedia:Trumpet_Major> ;
	foaf:name "Trumpet Major" .

:Rank_Trumpet_Major_Commonwealth_of_Nations org:rankOf <dbpedia:Commonwealth_of_Nations> ;
	a :MilitaryRank ;
	rdfs:comment "The specific instance of the Trumpet Major rank in the context of country Commonwealth of Nations."@en ;
	rdfs:label "Trumpet Major (Commonwealth delle nazioni)"@it , "Trumpet Major (Commonwealth of Nations)"@de , "Trumpet Major (Commonwealth of Nations)"@en , "Trumpet Major (Commonwealth of Nations)"@fr , "Trumpet Major (Commonwealth)"@pt , "Trumpet Major (Gemenebest van Naties)"@nl , "Trumpet Major (Kansainyhteisö)"@fi , "Trumpet Major (Mancomunidad de Naciones)"@es , "Trumpet Major (Samveldet av nasjoner)"@no , "Trumpet Major (Samväldet)"@sv , "Trumpet Major (Wspólnota Narodów)"@pl , "Trumpet Major (Содружество наций)"@ru ;
	owl:subClass :Rank_Trumpet_Major ;
	foaf:name "Trumpet Major"@en .

:Rank_Trumpet_Major_England org:rankOf <dbpedia:England> ;
	a :MilitaryRank ;
	rdfs:comment "The specific instance of the Trumpet Major rank in the context of England."@en ;
	rdfs:label "Trumpet Major (England)"@en ;
	owl:subClass :Rank_Trumpet_Major ;
	foaf:name "Trumpet Major"@en .

:Rank_Trumpet_Major_Scotland org:rankOf <dbpedia:Scotland> ;
	a :MilitaryRank ;
	rdfs:comment "The specific instance of the Trumpet Major rank in the context of country Scotland."@en ;
	rdfs:label "Trumpet Major (Escocia)"@es , "Trumpet Major (Escócia)"@pt , "Trumpet Major (Schotland)"@nl , "Trumpet Major (Schottland)"@de , "Trumpet Major (Scotland)"@en , "Trumpet Major (Scozia)"@it , "Trumpet Major (Skotlanti)"@fi , "Trumpet Major (Skottland)"@no , "Trumpet Major (Skottland)"@sv , "Trumpet Major (Szkocja)"@pl , "Trumpet Major (Écosse)"@fr , "Trumpet Major (Шотландия)"@ru ;
	owl:subClass :Rank_Trumpet_Major ;
	foaf:name "Trumpet Major"@en .

:Rank_Trumpet_Major_Wales org:rankOf <dbpedia:Wales> ;
	a :MilitaryRank ;
	rdfs:comment "The specific instance of the Trumpet Major rank in the context of country Wales."@en ;
	rdfs:label "Trumpet Major (Gales)"@es , "Trumpet Major (Galles)"@it , "Trumpet Major (Pays de Galles)"@fr , "Trumpet Major (País de Gales)"@pt , "Trumpet Major (Wales)"@de , "Trumpet Major (Wales)"@en , "Trumpet Major (Wales)"@fi , "Trumpet Major (Wales)"@nl , "Trumpet Major (Wales)"@no , "Trumpet Major (Wales)"@sv , "Trumpet Major (Walia)"@pl , "Trumpet Major (Уэльс)"@ru ;
	owl:subClass :Rank_Trumpet_Major ;
	foaf:name "Trumpet Major"@en .

:Rank_Tysyatsky a :MilitaryRank ;
	rdfs:comment "Tysyatsky was a military leader in Ancient Rus, who commanded a people's volunteer army called тысяча (tysyacha, or a thousand). In the Novgorod Republic, the tysyatsky evolved into a judicial or commercial official and was elected from boyars at a veche for a period of one year posadnik."@en ;
	rdfs:label "Tysjackij"@it , "Tysjatski"@nl , "Tysyatsky"@en , "Тысяцкий"@ru ;
	owl:sameAs <dbpedia:Tysyatsky> ;
	foaf:name "Tysyatsky" .

:Rank_Tysyatsky_Russia org:rankOf <dbpedia:Russia> ;
	a :MilitaryRank ;
	rdfs:comment "The specific instance of the Tysyatsky rank in the context of country Russia."@en ;
	rdfs:label "Tysjackij (Russia)"@it , "Tysjatski (Rusland)"@nl , "Tysyatsky (Rosja)"@pl , "Tysyatsky (Rusia)"@es , "Tysyatsky (Russia)"@en , "Tysyatsky (Russie)"@fr , "Tysyatsky (Russland)"@de , "Tysyatsky (Russland)"@no , "Tysyatsky (Ryssland)"@sv , "Tysyatsky (Rússia)"@pt , "Tysyatsky (Venäjä)"@fi , "Тысяцкий (Россия)"@ru ;
	owl:subClass :Rank_Tysyatsky ;
	foaf:name "Тысяцкий"@ru .

:Rank_Tysyatsky_Soviet_Union org:rankOf <dbpedia:Soviet_Union> ;
	a :MilitaryRank ;
	rdfs:comment "The specific instance of the Tysyatsky rank in the context of country Soviet Union."@en ;
	rdfs:label "Tysjackij (Unione Sovietica)"@it , "Tysjatski (Sovjet-Unie)"@nl , "Tysyatsky (Neuvostoliitto)"@fi , "Tysyatsky (Soviet Union)"@en , "Tysyatsky (Sovjetunionen)"@no , "Tysyatsky (Sovjetunionen)"@sv , "Tysyatsky (Sowjetunion)"@de , "Tysyatsky (Union des républiques socialistes soviétiques)"@fr , "Tysyatsky (União Soviética)"@pt , "Tysyatsky (Unión Soviética)"@es , "Tysyatsky (Związek Socjalistycznych Republik Radzieckich)"@pl , "Тысяцкий (Союз Советских Социалистических Республик)"@ru ;
	owl:subClass :Rank_Tysyatsky ;
	foaf:name "Tysyatsky"@en .

:Rank_Under_Officer a :MilitaryRank ;
	rdfs:comment "\"Underofficer\" redirects here, although it can also mean non-commissioned officer when translated from certain other languages. Under Officer is an appointment held by senior cadets at some Commonwealth officer training establishments and in University Officers' Training Corps in the United Kingdom, and also a rank used in some Commonwealth cadet forces."@en ;
	rdfs:label "Under Officer"@en ;
	owl:sameAs <dbpedia:Under_Officer> ;
	foaf:name "Under Officer" .

:Rank_Under_Officer_Australia org:rankOf <dbpedia:Australia> ;
	a :MilitaryRank ;
	rdfs:comment "The specific instance of the Under Officer rank in the context of country Australia."@en ;
	rdfs:label "Under Officer (Australia)"@en , "Under Officer (Australia)"@es , "Under Officer (Australia)"@fi , "Under Officer (Australia)"@it , "Under Officer (Australia)"@no , "Under Officer (Australia)"@pl , "Under Officer (Australie)"@fr , "Under Officer (Australien)"@de , "Under Officer (Australien)"@sv , "Under Officer (Australië (land))"@nl , "Under Officer (Austrália)"@pt , "Under Officer (Австралия)"@ru ;
	owl:subClass :Rank_Under_Officer ;
	foaf:name "Under Officer"@en .

:Rank_Under_Officer_Commonwealth_of_Nations org:rankOf <dbpedia:Commonwealth_of_Nations> ;
	a :MilitaryRank ;
	rdfs:comment "The specific instance of the Under Officer rank in the context of country Commonwealth of Nations."@en ;
	rdfs:label "Under Officer (Commonwealth delle nazioni)"@it , "Under Officer (Commonwealth of Nations)"@de , "Under Officer (Commonwealth of Nations)"@en , "Under Officer (Commonwealth of Nations)"@fr , "Under Officer (Commonwealth)"@pt , "Under Officer (Gemenebest van Naties)"@nl , "Under Officer (Kansainyhteisö)"@fi , "Under Officer (Mancomunidad de Naciones)"@es , "Under Officer (Samveldet av nasjoner)"@no , "Under Officer (Samväldet)"@sv , "Under Officer (Wspólnota Narodów)"@pl , "Under Officer (Содружество наций)"@ru ;
	owl:subClass :Rank_Under_Officer ;
	foaf:name "Under Officer"@en .

:Rank_Under_Officer_England org:rankOf <dbpedia:England> ;
	a :MilitaryRank ;
	rdfs:comment "The specific instance of the Under Officer rank in the context of England."@en ;
	rdfs:label "Under Officer (England)"@en ;
	owl:subClass :Rank_Under_Officer ;
	foaf:name "Under Officer"@en .

:Rank_Under_Officer_Scotland org:rankOf <dbpedia:Scotland> ;
	a :MilitaryRank ;
	rdfs:comment "The specific instance of the Under Officer rank in the context of country Scotland."@en ;
	rdfs:label "Under Officer (Escocia)"@es , "Under Officer (Escócia)"@pt , "Under Officer (Schotland)"@nl , "Under Officer (Schottland)"@de , "Under Officer (Scotland)"@en , "Under Officer (Scozia)"@it , "Under Officer (Skotlanti)"@fi , "Under Officer (Skottland)"@no , "Under Officer (Skottland)"@sv , "Under Officer (Szkocja)"@pl , "Under Officer (Écosse)"@fr , "Under Officer (Шотландия)"@ru ;
	owl:subClass :Rank_Under_Officer ;
	foaf:name "Under Officer"@en .

:Rank_Under_Officer_Wales org:rankOf <dbpedia:Wales> ;
	a :MilitaryRank ;
	rdfs:comment "The specific instance of the Under Officer rank in the context of country Wales."@en ;
	rdfs:label "Under Officer (Gales)"@es , "Under Officer (Galles)"@it , "Under Officer (Pays de Galles)"@fr , "Under Officer (País de Gales)"@pt , "Under Officer (Wales)"@de , "Under Officer (Wales)"@en , "Under Officer (Wales)"@fi , "Under Officer (Wales)"@nl , "Under Officer (Wales)"@no , "Under Officer (Wales)"@sv , "Under Officer (Walia)"@pl , "Under Officer (Уэльс)"@ru ;
	owl:subClass :Rank_Under_Officer ;
	foaf:name "Under Officer"@en .

:Rank_Vaapeli a :MilitaryRank ;
	rdfs:label "Vääpeli"@en ;
	owl:sameAs <dbpedia:V%C3%A4%C3%A4peli> ;
	foaf:name "Vääpeli" .

:Rank_Vaapeli_Finland org:rankOf <dbpedia:Finland> ;
	a :MilitaryRank ;
	rdfs:comment "The specific instance of the Vääpeli rank in the context of country Finland."@en ;
	rdfs:label "Vääpeli (Finland)"@en , "Vääpeli (Finland)"@nl , "Vääpeli (Finland)"@no , "Vääpeli (Finland)"@sv , "Vääpeli (Finlande)"@fr , "Vääpeli (Finlandia)"@es , "Vääpeli (Finlandia)"@it , "Vääpeli (Finlandia)"@pl , "Vääpeli (Finlândia)"@pt , "Vääpeli (Finnland)"@de , "Vääpeli (Suomi)"@fi , "Vääpeli (Финляндия)"@ru ;
	owl:subClass :Rank_Vaapeli ;
	foaf:name "Vääpeli"@en .

:Rank_Vaapeli_Sweden org:rankOf <dbpedia:Sweden> ;
	a :MilitaryRank ;
	rdfs:comment "The specific instance of the Vääpeli rank in the context of country Sweden."@en ;
	rdfs:label "Vääpeli (Ruotsi)"@fi , "Vääpeli (Schweden)"@de , "Vääpeli (Suecia)"@es , "Vääpeli (Suède)"@fr , "Vääpeli (Suécia)"@pt , "Vääpeli (Sverige)"@no , "Vääpeli (Sverige)"@sv , "Vääpeli (Svezia)"@it , "Vääpeli (Sweden)"@en , "Vääpeli (Szwecja)"@pl , "Vääpeli (Zweden)"@nl , "Vääpeli (Швеция)"@ru ;
	owl:subClass :Rank_Vaapeli ;
	foaf:name "Vääpeli"@en .

:Rank_Veebel a :MilitaryRank ;
	rdfs:comment "Veebel is an Estonian military rank which has existed since the 20th century. The word veebel is usually, but incorrectly, translated in English as Sergeant. The correct equivalent is Warrant Officer."@en ;
	rdfs:label "Veebel"@en ;
	owl:sameAs <dbpedia:Veebel> ;
	foaf:name "Veebel" .

:Rank_Veebel_Estonia org:rankOf <dbpedia:Estonia> ;
	a :MilitaryRank ;
	rdfs:comment "The specific instance of the Veebel rank in the context of country Estonia."@en ;
	rdfs:label "Veebel (Estland)"@de , "Veebel (Estland)"@nl , "Veebel (Estland)"@no , "Veebel (Estland)"@sv , "Veebel (Estonia)"@en , "Veebel (Estonia)"@es , "Veebel (Estonia)"@it , "Veebel (Estonia)"@pl , "Veebel (Estonie)"@fr , "Veebel (Estónia)"@pt , "Veebel (Viro)"@fi , "Veebel (Эстония)"@ru ;
	owl:subClass :Rank_Veebel ;
	foaf:name "Veebel"@en .

:Rank_Veebel_Republic_of_Estonia_1920-1940 org:rankOf <dbpedia:Republic_of_Estonia_%281920-1940%29> ;
	a :MilitaryRank ;
	rdfs:comment "The specific instance of the Veebel rank in the context of the Republic of Estonia, 1920-1940."@en ;
	rdfs:label "Veebel (Republic of Estonia, 1920-1940)"@en ;
	owl:subClass :Rank_Veebel ;
	foaf:name "Veebel"@en .

:Rank_Vice-Admiral_of_the_Coast a :MilitaryRank ;
	rdfs:comment "The holder of the post Vice-Admiral of the Coast was responsible for the defence of one of the twenty maritime counties of England, the North and South of Wales, or the four provinces of Ireland. As a Vice-Admiral, the post holder was the chief of naval administration for his district. His responsibilities included pressing men for naval service, deciding the lawfulness of prizes (captured by pirate ships), dealing with salvage claims for wrecks and acting as a judge."@en ;
	rdfs:label "Vice-Admiral of the Coast"@en ;
	owl:sameAs <dbpedia:Vice-Admiral_of_the_Coast> ;
	foaf:name "Vice-Admiral of the Coast" .

:Rank_Vice-Admiral_of_the_Coast_England org:rankOf <dbpedia:England> ;
	a :MilitaryRank ;
	rdfs:comment "The specific instance of the Vice-Admiral of the Coast rank in the context of country England."@en ;
	rdfs:label "Vice-Admiral of the Coast (England)"@en ;
	owl:subClass :Rank_Vice-Admiral_of_the_Coast ;
	foaf:name "Vice-Admiral of the Coast"@en .

:Rank_Vice-Admiral_of_the_Coast_Scotland org:rankOf <dbpedia:Scotland> ;
	a :MilitaryRank ;
	rdfs:comment "The specific instance of the Vice-Admiral of the Coast rank in the context of country Scotland."@en ;
	rdfs:label "Vice-Admiral of the Coast (Escocia)"@es , "Vice-Admiral of the Coast (Escócia)"@pt , "Vice-Admiral of the Coast (Schotland)"@nl , "Vice-Admiral of the Coast (Schottland)"@de , "Vice-Admiral of the Coast (Scotland)"@en , "Vice-Admiral of the Coast (Scozia)"@it , "Vice-Admiral of the Coast (Skotlanti)"@fi , "Vice-Admiral of the Coast (Skottland)"@no , "Vice-Admiral of the Coast (Skottland)"@sv , "Vice-Admiral of the Coast (Szkocja)"@pl , "Vice-Admiral of the Coast (Écosse)"@fr , "Vice-Admiral of the Coast (Шотландия)"@ru ;
	owl:subClass :Rank_Vice-Admiral_of_the_Coast ;
	foaf:name "Vice-Admiral of the Coast"@en .

:Rank_Vice-Admiral_of_the_Coast_Wales org:rankOf <dbpedia:Wales> ;
	a :MilitaryRank ;
	rdfs:comment "The specific instance of the Vice-Admiral of the Coast rank in the context of country Wales."@en ;
	rdfs:label "Vice-Admiral of the Coast (Gales)"@es , "Vice-Admiral of the Coast (Galles)"@it , "Vice-Admiral of the Coast (Pays de Galles)"@fr , "Vice-Admiral of the Coast (País de Gales)"@pt , "Vice-Admiral of the Coast (Wales)"@de , "Vice-Admiral of the Coast (Wales)"@en , "Vice-Admiral of the Coast (Wales)"@fi , "Vice-Admiral of the Coast (Wales)"@nl , "Vice-Admiral of the Coast (Wales)"@no , "Vice-Admiral of the Coast (Wales)"@sv , "Vice-Admiral of the Coast (Walia)"@pl , "Vice-Admiral of the Coast (Уэльс)"@ru ;
	owl:subClass :Rank_Vice-Admiral_of_the_Coast ;
	foaf:name "Vice-Admiral of the Coast"@en .

:Rank_Vice-Admiral_of_the_West a :MilitaryRank ;
	rdfs:comment "The historical title Vice-Admiral of the West is sometimes applied to holders of the crown appointment Vice-Admiral of the Coast of counties in the South West of England. The duties of a Vice-Admiral of the coast were to control the shipping (especially piracy) around a maritime county's coast and organise defense on land and at sea. He also acted as a local judge to deal with maritime matters."@en ;
	rdfs:label "Vice-Admiral of the West"@en ;
	owl:sameAs <dbpedia:Vice-Admiral_of_the_West> ;
	foaf:name "Vice-Admiral of the West" .

:Rank_Vice-Admiral_of_the_West_England org:rankOf <dbpedia:England> ;
	a :MilitaryRank ;
	rdfs:comment "The specific instance of the Vice-Admiral of the West rank in the context of England."@en ;
	rdfs:label "Vice-Admiral of the West (England)"@en ;
	owl:subClass :Rank_Vice-Admiral_of_the_West ;
	foaf:name "Vice-Admiral of the West"@en .

:Rank_Vice-Admiral_of_the_West_Scotland org:rankOf <dbpedia:Scotland> ;
	a :MilitaryRank ;
	rdfs:comment "The specific instance of the Vice-Admiral of the West rank in the context of country Scotland."@en ;
	rdfs:label "Vice-Admiral of the West (Escocia)"@es , "Vice-Admiral of the West (Escócia)"@pt , "Vice-Admiral of the West (Schotland)"@nl , "Vice-Admiral of the West (Schottland)"@de , "Vice-Admiral of the West (Scotland)"@en , "Vice-Admiral of the West (Scozia)"@it , "Vice-Admiral of the West (Skotlanti)"@fi , "Vice-Admiral of the West (Skottland)"@no , "Vice-Admiral of the West (Skottland)"@sv , "Vice-Admiral of the West (Szkocja)"@pl , "Vice-Admiral of the West (Écosse)"@fr , "Vice-Admiral of the West (Шотландия)"@ru ;
	owl:subClass :Rank_Vice-Admiral_of_the_West ;
	foaf:name "Vice-Admiral of the West"@en .

:Rank_Vice-Admiral_of_the_West_Wales org:rankOf <dbpedia:Wales> ;
	a :MilitaryRank ;
	rdfs:comment "The specific instance of the Vice-Admiral of the West rank in the context of country Wales."@en ;
	rdfs:label "Vice-Admiral of the West (Gales)"@es , "Vice-Admiral of the West (Galles)"@it , "Vice-Admiral of the West (Pays de Galles)"@fr , "Vice-Admiral of the West (País de Gales)"@pt , "Vice-Admiral of the West (Wales)"@de , "Vice-Admiral of the West (Wales)"@en , "Vice-Admiral of the West (Wales)"@fi , "Vice-Admiral of the West (Wales)"@nl , "Vice-Admiral of the West (Wales)"@no , "Vice-Admiral of the West (Wales)"@sv , "Vice-Admiral of the West (Walia)"@pl , "Vice-Admiral of the West (Уэльс)"@ru ;
	owl:subClass :Rank_Vice-Admiral_of_the_West ;
	foaf:name "Vice-Admiral of the West"@en .

:Rank_Vice_admiral a :MilitaryRank ;
	rdfs:label "Vice admiral"@en ;
	owl:sameAs <dbpedia:Vice_admiral> ;
	foaf:name "Vice admiral" .

:Rank_Vice_admiral_Australia org:rankOf <dbpedia:Australia> ;
	a :MilitaryRank ;
	rdfs:comment "The specific instance of the Vice admiral rank in the context of country Australia."@en ;
	rdfs:label "Vice admiral (Australia)"@en , "Vice admiral (Australia)"@es , "Vice admiral (Australia)"@fi , "Vice admiral (Australia)"@it , "Vice admiral (Australia)"@no , "Vice admiral (Australia)"@pl , "Vice admiral (Australie)"@fr , "Vice admiral (Australien)"@de , "Vice admiral (Australien)"@sv , "Vice admiral (Australië (land))"@nl , "Vice admiral (Austrália)"@pt , "Vice admiral (Австралия)"@ru ;
	owl:subClass :Rank_Vice_admiral ;
	foaf:name "Vice admiral"@en .

:Rank_Vice_admiral_Australia_Australia org:rankOf <dbpedia:Australia> ;
	a :MilitaryRank ;
	rdfs:comment "The specific instance of the  rank in the context of country Australia."@en ;
	rdfs:label " (Australia)"@en , " (Australia)"@es , " (Australia)"@fi , " (Australia)"@it , " (Australia)"@no , " (Australia)"@pl , " (Australie)"@fr , " (Australien)"@de , " (Australien)"@sv , " (Australië (land))"@nl , " (Austrália)"@pt , " (Австралия)"@ru ;
	owl:subClass :Rank_Vice_admiral_Australia ;
	foaf:name ""@en .

:Rank_Vice_admiral_Canada org:rankOf <dbpedia:Canada> ;
	a :MilitaryRank ;
	rdfs:comment "The specific instance of the Vice admiral rank in the context of Canada."@en ;
	rdfs:label "Vice admiral (Canada)"@en ;
	owl:subClass :Rank_Vice_admiral ;
	foaf:name "Vice admiral"@en .

:Rank_Wachtmeister a :MilitaryRank ;
	rdfs:comment "Wachtmeister (German for master-sentinel; watch-master) was a German, Austrian and Swiss military rank of non-commissioned officers. It was also adopted into Russian Army vakhmistr and was used as Sergeant-grade rank in cavalry (until 1826), then Special Corps of Gendarmes and Cossack cavalry and Cossack Leib Guard units. Also, the Polish army used the rank Wachmistrz as a cavalry-specific title for Sergeant. This was similar to calling cavalry Captains Rittmeister."@en ;
	rdfs:label "Wachmistrz"@pl , "Wachtmeister"@de , "Wachtmeister"@en , "Вахмистр"@ru ;
	owl:sameAs <dbpedia:Wachtmeister> ;
	foaf:name "Wachtmeister" .

:Rank_Wachtmeister_Germany org:rankOf <dbpedia:Germany> ;
	a :MilitaryRank ;
	rdfs:comment "The specific instance of the Wachtmeister rank in the context of Germany."@en ;
	rdfs:label "Wachmistrz (Germany)"@pl , "Wachtmeister (Germany)"@de , "Wachtmeister (Germany)"@en , "Вахмистр (Germany)"@ru ;
	owl:subClass :Rank_Wachtmeister ;
	foaf:name "Wachtmeister"@de .

:Rank_Wachtmeister_Russia org:rankOf <dbpedia:Russia> ;
	a :MilitaryRank ;
	rdfs:comment "The specific instance of the Wachtmeister rank in the context of country Russia."@en ;
	rdfs:label "Wachmistrz (Rosja)"@pl , "Wachtmeister (Rusia)"@es , "Wachtmeister (Rusland)"@nl , "Wachtmeister (Russia)"@en , "Wachtmeister (Russia)"@it , "Wachtmeister (Russie)"@fr , "Wachtmeister (Russland)"@de , "Wachtmeister (Russland)"@no , "Wachtmeister (Ryssland)"@sv , "Wachtmeister (Rússia)"@pt , "Wachtmeister (Venäjä)"@fi , "Вахмистр (Россия)"@ru ;
	owl:subClass :Rank_Wachtmeister ;
	foaf:name "Вахмистр"@ru .

:Rank_Wachtmeister_Soviet_Union org:rankOf <dbpedia:Soviet_Union> ;
	a :MilitaryRank ;
	rdfs:comment "The specific instance of the Wachtmeister rank in the context of country Soviet Union."@en ;
	rdfs:label "Wachmistrz (Związek Socjalistycznych Republik Radzieckich)"@pl , "Wachtmeister (Neuvostoliitto)"@fi , "Wachtmeister (Soviet Union)"@en , "Wachtmeister (Sovjet-Unie)"@nl , "Wachtmeister (Sovjetunionen)"@no , "Wachtmeister (Sovjetunionen)"@sv , "Wachtmeister (Sowjetunion)"@de , "Wachtmeister (Union des républiques socialistes soviétiques)"@fr , "Wachtmeister (Unione Sovietica)"@it , "Wachtmeister (União Soviética)"@pt , "Wachtmeister (Unión Soviética)"@es , "Вахмистр (Союз Советских Социалистических Республик)"@ru ;
	owl:subClass :Rank_Wachtmeister ;
	foaf:name "Wachtmeister"@en .

:Rank_Warrant_officer_EnglishTradition org:rankEquivalentTo :Rank_Sergeant_major_EnglishTradition , :Rank_Warrant_officer_EnglishTradition ;
	org:rankJuniorToTransitive :Rank_Midshipman_EnglishTradition , :Rank_Officer_cadet_EnglishTradition ;
	org:rankOf :EnglishTradition , <mil:AirForceServiceBranch> , <mil:NavyServiceBranch> ;
	org:rankSeniorToTransitive :Rank_Petty_officer_EnglishTradition , :Rank_Sergeant_EnglishTradition ;
	a :MilitaryRank ;
	rdfs:label "Warrant officer"@en ;
	owl:sameAs <dbpedia:Warrant_officer> .

:Rank_Warrant_officer_United_Kingdom a :MilitaryRank ;
	rdfs:label "Warrant Officer"@en ;
	owl:sameAs <dbpedia:Warrant_officer_%28United_Kingdom%29> ;
	owl:subClassOf <mil:#Rank_Warrant_officer_EnglishTradition> ;
	foaf:name "Warrant Officer" .

:Rank_Warrant_officer_United_Kingdom_Australia org:rankOf <dbpedia:Australia> ;
	a :MilitaryRank ;
	rdfs:comment "The specific instance of the Warrant Officer rank in the context of country Australia."@en ;
	rdfs:label "Warrant Officer (Australia)"@en , "Warrant Officer (Australia)"@es , "Warrant Officer (Australia)"@fi , "Warrant Officer (Australia)"@it , "Warrant Officer (Australia)"@no , "Warrant Officer (Australia)"@pl , "Warrant Officer (Australie)"@fr , "Warrant Officer (Australien)"@de , "Warrant Officer (Australien)"@sv , "Warrant Officer (Australië (land))"@nl , "Warrant Officer (Austrália)"@pt , "Warrant Officer (Австралия)"@ru ;
	owl:subClass :Rank_Warrant_officer_United_Kingdom ;
	foaf:name "Warrant Officer"@en .

:Rank_Warrant_officer_United_Kingdom_Canada org:rankOf <dbpedia:Canada> ;
	a :MilitaryRank ;
	rdfs:comment "The specific instance of the  rank in the context of Canada"@en ;
	rdfs:label "Warrant Officer (Canada)"@en ;
	owl:subClass :Rank_Warrant_officer_United_Kingdom ;
	foaf:name "Warrant Officer"@en .

:Rank_Warrant_officer_United_Kingdom_Commonwealth_of_Nations org:rankOf <dbpedia:Commonwealth_of_Nations> ;
	a :MilitaryRank ;
	rdfs:comment "The specific instance of the  rank in the context of country Commonwealth of Nations."@en ;
	rdfs:label "Warrant Officer (Commonwealth delle nazioni)"@it , "Warrant Officer (Commonwealth of Nations)"@de , "Warrant Officer (Commonwealth of Nations)"@en , "Warrant Officer (Commonwealth of Nations)"@fr , "Warrant Officer (Commonwealth)"@pt , "Warrant Officer (Gemenebest van Naties)"@nl , "Warrant Officer (Kansainyhteisö)"@fi , "Warrant Officer (Mancomunidad de Naciones)"@es , "Warrant Officer (Samveldet av nasjoner)"@no , "Warrant Officer (Samväldet)"@sv , "Warrant Officer (Wspólnota Narodów)"@pl , "Warrant Officer (Содружество наций)"@ru ;
	owl:subClass :Rank_Warrant_officer_United_Kingdom ;
	foaf:name "Warrant Officer"@en .

:Rank_Warrant_officer_United_Kingdom_England org:rankOf <dbpedia:England> ;
	a :MilitaryRank ;
	rdfs:comment "The specific instance of the  rank in the context of England."@en ;
	rdfs:label "Warrant Officer (England)"@en ;
	owl:subClass :Rank_Warrant_officer_United_Kingdom ;
	foaf:name "Warrant Officer"@en .

:Rank_Warrant_officer_United_Kingdom_Scotland org:rankOf <dbpedia:Scotland> ;
	a :MilitaryRank ;
	rdfs:comment "The specific instance of the Warrant Officer rank in the context of country Scotland."@en ;
	rdfs:label "Warrant Officer (Escocia)"@es , "Warrant Officer (Escócia)"@pt , "Warrant Officer (Schotland)"@nl , "Warrant Officer (Schottland)"@de , "Warrant Officer (Scotland)"@en , "Warrant Officer (Scozia)"@it , "Warrant Officer (Skotlanti)"@fi , "Warrant Officer (Skottland)"@no , "Warrant Officer (Skottland)"@sv , "Warrant Officer (Szkocja)"@pl , "Warrant Officer (Écosse)"@fr , "Warrant Officer (Шотландия)"@ru ;
	owl:subClass :Rank_Warrant_officer_United_Kingdom ;
	foaf:name "Warrant Officer"@en .

:Rank_Warrant_officer_United_Kingdom_Wales org:rankOf <dbpedia:Wales> ;
	a :MilitaryRank ;
	rdfs:comment "The specific instance of the Warrant Officer rank in the context of country Wales."@en ;
	rdfs:label "Warrant Officer (Gales)"@es , "Warrant Officer (Galles)"@it , "Warrant Officer (Pays de Galles)"@fr , "Warrant Officer (País de Gales)"@pt , "Warrant Officer (Wales)"@de , "Warrant Officer (Wales)"@en , "Warrant Officer (Wales)"@fi , "Warrant Officer (Wales)"@nl , "Warrant Officer (Wales)"@no , "Warrant Officer (Wales)"@sv , "Warrant Officer (Walia)"@pl , "Warrant Officer (Уэльс)"@ru ;
	owl:subClass :Rank_Warrant_officer_United_Kingdom ;
	foaf:name "Warrant Officer"@en .

:Rank_Wing_commander a :MilitaryRank ;
	rdfs:label "Wing commander (rank)"@en ;
	owl:sameAs <dbpedia:Wing_commander_%28rank%29> ;
	foaf:name "Wing commander" .

<http://rdf.muninn-project.org/ontologies/military#Rank_Wing_commander_(rank)_EnglishTradition> org:rankEquivalentTo :Rank_Commander_EnglishTradition , :Rank_Lieutenant_colonel_EnglishTradition ;
	org:rankJuniorToTransitive :Rank_Group_captain_EnglishTradition ;
	org:rankOf :EnglishTradition , <mil:AirForceServiceBranch> ;
	org:rankSeniorToTransitive :Rank_Squadron_leader_EnglishTradition ;
	a :MilitaryRank ;
	owl:sameAs <dbpedia:Wing_commander_(rank)> .

:Rank_Wing_commander_Australia org:rankOf <dbpedia:Australia> ;
	a :MilitaryRank ;
	rdfs:comment "The specific instance of the Wing commander (rank) rank in the context of country Australia."@en ;
	rdfs:label "Wing commander (rank) (Australia)"@en , "Wing commander (rank) (Australia)"@es , "Wing commander (rank) (Australia)"@fi , "Wing commander (rank) (Australia)"@it , "Wing commander (rank) (Australia)"@no , "Wing commander (rank) (Australia)"@pl , "Wing commander (rank) (Australie)"@fr , "Wing commander (rank) (Australien)"@de , "Wing commander (rank) (Australien)"@sv , "Wing commander (rank) (Australië (land))"@nl , "Wing commander (rank) (Austrália)"@pt , "Wing commander (rank) (Австралия)"@ru ;
	owl:subClass :Rank_Wing_commander ;
	foaf:name "Wing commander"@en .

:Rank_Wing_commander_Canada org:rankOf <dbpedia:Canada> ;
	a :MilitaryRank ;
	rdfs:comment "The specific instance of the Wing commander (rank) rank in the context of Canada."@en ;
	rdfs:label "Wing commander (rank, Canada)"@en ;
	owl:subClass :Rank_Wing_commander ;
	foaf:name "Wing commander"@en .

:Rank_Wing_commander_Commonwealth_of_Nations org:rankOf <dbpedia:Commonwealth_of_Nations> ;
	a :MilitaryRank ;
	rdfs:comment "The specific instance of the Wing commander (rank) rank in the context of country Commonwealth of Nations."@en ;
	rdfs:label "Wing commander (rank) (Commonwealth delle nazioni)"@it , "Wing commander (rank) (Commonwealth of Nations)"@de , "Wing commander (rank) (Commonwealth of Nations)"@en , "Wing commander (rank) (Commonwealth of Nations)"@fr , "Wing commander (rank) (Commonwealth)"@pt , "Wing commander (rank) (Gemenebest van Naties)"@nl , "Wing commander (rank) (Kansainyhteisö)"@fi , "Wing commander (rank) (Mancomunidad de Naciones)"@es , "Wing commander (rank) (Samveldet av nasjoner)"@no , "Wing commander (rank) (Samväldet)"@sv , "Wing commander (rank) (Wspólnota Narodów)"@pl , "Wing commander (rank) (Содружество наций)"@ru ;
	owl:subClass :Rank_Wing_commander ;
	foaf:name "Wing commander"@en .

:Rank_Wojski a :MilitaryRank ;
	rdfs:comment "The Wojski was an officer in medieval Poland, responsible for the security of voivodships or districts at times when voivods and castellans had accompanied the szlachta (nobility) to war. With time, the wojski's responsibilities were take over by starostas, and \"wojski\" became an honorary district office in the Polish-Lithuanian Commonwealth."@en ;
	rdfs:label "Wojski"@en , "Wojski"@pl , "Войский"@ru ;
	owl:sameAs <dbpedia:Wojski> ;
	foaf:name "Wojski" .

:Rank_Wojski_Lithuania org:rankOf <dbpedia:Lithuania> ;
	a :MilitaryRank ;
	rdfs:comment "The specific instance of the Wojski rank in the context of country Lithuania."@en ;
	rdfs:label "Wojski (Liettua)"@fi , "Wojski (Litauen)"@de , "Wojski (Litauen)"@no , "Wojski (Litauen)"@sv , "Wojski (Lithuania)"@en , "Wojski (Litouwen)"@nl , "Wojski (Lituania)"@es , "Wojski (Lituania)"@it , "Wojski (Lituanie)"@fr , "Wojski (Lituânia)"@pt , "Wojski (Litwa)"@pl , "Войский (Литва)"@ru ;
	owl:subClass :Rank_Wojski ;
	foaf:name "Wojski"@en .

:Rank_Wojski_Poland org:rankOf <dbpedia:Poland> ;
	a :MilitaryRank ;
	rdfs:comment "The specific instance of the Wojski rank in the context of Poland."@en ;
	rdfs:label "Wojski (Poland)"@en , "Wojski (Poland)"@pl , "Войский (Poland)"@ru ;
	owl:subClass :Rank_Wojski ;
	foaf:name "Wojski"@en .

:Rank_Wonsu a :MilitaryRank ;
	rdfs:comment "Wonsu is a very high military rank of the armed forces of the Republic of Korea and of North Korea."@en ;
	rdfs:label "Wonsu"@en , "Вонсу"@ru ;
	owl:sameAs <dbpedia:Wonsu> ;
	foaf:name "Wonsu" .

:Rank_Wonsu_North_Korea org:rankOf <dbpedia:North_Korea> ;
	a :MilitaryRank ;
	rdfs:comment "The specific instance of the Wonsu rank in the context of country North Korea."@en ;
	rdfs:label "Wonsu (Corea del Nord)"@it , "Wonsu (Corea del Norte)"@es , "Wonsu (Coreia do Norte)"@pt , "Wonsu (Corée du Nord)"@fr , "Wonsu (Korea Północna)"@pl , "Wonsu (Korean demokraattinen kansantasavalta)"@fi , "Wonsu (Noord-Korea)"@nl , "Wonsu (Nord-Korea)"@no , "Wonsu (Nordkorea)"@de , "Wonsu (Nordkorea)"@sv , "Wonsu (North Korea)"@en , "Вонсу (Корейская Народно-Демократическая Республика)"@ru ;
	owl:subClass :Rank_Wonsu ;
	foaf:name "Wonsu"@en .

:Rank_Wonsu_South_Korea org:rankOf <dbpedia:South_Korea> ;
	a :MilitaryRank ;
	rdfs:comment "The specific instance of the Wonsu rank in the context of country South Korea."@en ;
	rdfs:label "Wonsu (Corea del Sud)"@it , "Wonsu (Corea del Sur)"@es , "Wonsu (Coreia do Sul)"@pt , "Wonsu (Corée du Sud)"@fr , "Wonsu (Korea Południowa)"@pl , "Wonsu (Korean tasavalta)"@fi , "Wonsu (South Korea)"@en , "Wonsu (Sydkorea)"@sv , "Wonsu (Sør-Korea)"@no , "Wonsu (Südkorea)"@de , "Wonsu (Zuid-Korea)"@nl , "Вонсу (Республика Корея)"@ru ;
	owl:subClass :Rank_Wonsu ;
	foaf:name "Wonsu"@en .

:Rank_Yesaul a :MilitaryRank ;
	rdfs:comment "For the town in Armenia, see Ovuni. Part of a series onCossacksFile:Repin Cossacks."@en ;
	rdfs:label "Esauł"@pl , "Jesaul"@sv , "Jessaul"@de , "Yesaul"@en , "Есаул"@ru ;
	owl:sameAs <dbpedia:Yesaul> ;
	foaf:name "Yesaul" .

:Rank_Yesaul_Russia org:rankOf <dbpedia:Russia> ;
	a :MilitaryRank ;
	rdfs:comment "The specific instance of the Yesaul rank in the context of country Russia."@en ;
	rdfs:label "Esauł (Rosja)"@pl , "Jesaul (Ryssland)"@sv , "Jessaul (Russland)"@de , "Yesaul (Rusia)"@es , "Yesaul (Rusland)"@nl , "Yesaul (Russia)"@en , "Yesaul (Russia)"@it , "Yesaul (Russie)"@fr , "Yesaul (Russland)"@no , "Yesaul (Rússia)"@pt , "Yesaul (Venäjä)"@fi , "Есаул (Россия)"@ru ;
	owl:subClass :Rank_Yesaul ;
	foaf:name "Есаул"@ru .

:Rank_Yesaul_Soviet_Union org:rankOf <dbpedia:Soviet_Union> ;
	a :MilitaryRank ;
	rdfs:comment "The specific instance of the Yesaul rank in the context of country Soviet Union."@en ;
	rdfs:label "Esauł (Związek Socjalistycznych Republik Radzieckich)"@pl , "Jesaul (Sovjetunionen)"@sv , "Jessaul (Sowjetunion)"@de , "Yesaul (Neuvostoliitto)"@fi , "Yesaul (Soviet Union)"@en , "Yesaul (Sovjet-Unie)"@nl , "Yesaul (Sovjetunionen)"@no , "Yesaul (Union des républiques socialistes soviétiques)"@fr , "Yesaul (Unione Sovietica)"@it , "Yesaul (União Soviética)"@pt , "Yesaul (Unión Soviética)"@es , "Есаул (Союз Советских Социалистических Республик)"@ru ;
	owl:subClass :Rank_Yesaul ;
	foaf:name "Yesaul"@en .

:Rank_Yesaul_Ukraine org:rankOf <dbpedia:Ukraine> ;
	a :MilitaryRank ;
	rdfs:comment "The specific instance of the Yesaul rank in the context of country Ukraine."@en ;
	rdfs:label "Esauł (Ukraina)"@pl , "Jesaul (Ukraina)"@sv , "Jessaul (Ukraine)"@de , "Yesaul (Oekraïne)"@nl , "Yesaul (Ucraina)"@it , "Yesaul (Ucrania)"@es , "Yesaul (Ucrânia)"@pt , "Yesaul (Ukraina)"@fi , "Yesaul (Ukraina)"@no , "Yesaul (Ukraine)"@en , "Yesaul (Ukraine)"@fr , "Есаул (Украина)"@ru ;
	owl:subClass :Rank_Yesaul ;
	foaf:name "Есаул"@ru .

:Rank_Ypolochagos a :MilitaryRank ;
	rdfs:comment "Ypolochagos is used in the modern Greek language to mean \"First Lieutenant\". In the modern Hellenic Army the rank is superior to that of Anthypolochagos and inferior to that of an Lochagos. The insignia consists of two silver stars. Officers holding this rank should be addressed as \"Kyrie Ypolochage\" (Κύριε Υπολοχαγέ) by their subordinates, or \"Ypolochage + family name\" by their superior officers."@en ;
	rdfs:label "Ypolochagos"@en ;
	owl:sameAs <dbpedia:Ypolochagos> ;
	foaf:name "Ypolochagos" .

:Rank_Ypolochagos_Greece org:rankOf <dbpedia:Greece> ;
	a :MilitaryRank ;
	rdfs:comment "The specific instance of the Ypolochagos rank in the context of country Greece."@en ;
	rdfs:label "Ypolochagos (Grecia)"@es , "Ypolochagos (Grecia)"@it , "Ypolochagos (Grecja)"@pl , "Ypolochagos (Greece)"@en , "Ypolochagos (Grekland)"@sv , "Ypolochagos (Griechenland)"@de , "Ypolochagos (Griekenland)"@nl , "Ypolochagos (Grèce)"@fr , "Ypolochagos (Grécia)"@pt , "Ypolochagos (Hellas)"@no , "Ypolochagos (Kreikka)"@fi , "Ypolochagos (Греция)"@ru ;
	owl:subClass :Rank_Ypolochagos ;
	foaf:name "Ypolochagos"@en .

:Rank_Ypolochagos_Official_Timocracy_of_Sapinetia org:rankOf <dbpedia:Official_Timocracy_of_Sapinetia> ;
	a :MilitaryRank ;
	rdfs:comment "The specific instance of the Ypolochagos rank in the context of the Timocracy_of_Sapinetia."@en ;
	rdfs:label "Ypolochagos (Timocracy_of_Sapinetia)"@en ;
	owl:subClass :Rank_Ypolochagos ;
	foaf:name "Ypolochagos"@en .

:Regiment org:hasPart :Battalion ;
	org:isPartOf :ArmyServiceBranch , :Brigade ;
	a owl:Class ;
	rdfs:comment "A regiment, be it administrative or historical."@en ;
	rdfs:label "Regiment"@de , "Regiment"@en , "Régiment"@fr ;
	owl:sameAs "dbpedia:Regiment" ;
	foaf:logo <http://rdf.muninn-project.org/ww1/2011/11/11/image/26> .

:RegimentalColours a owl:ObjectProperty ;
	rdfs:comment "Flag used by a regiment on a battlefield or on parade."@en ;
	rdfs:domain :Regiment ;
	rdfs:label ""@de , "Drapeau du Regiment"@fr , "Regimental Colours"@en ;
	rdfs:subPropertyOf <org:flag> .

:RegularForceSoldier a owl:Class ;
	rdfs:comment "A soldier who serves on a full-time basis."@en ;
	rdfs:label "Regular Soldier"@en , "Soldat Régulier"@fr , "regulärer Soldat"@de ;
	owl:subClassOf :Soldier ;
	foaf:name "Regular Soldier" .

:Reservist a owl:Class ;
	rdfs:comment "A soldier who serves on a part-time basis or when called up."@en ;
	rdfs:label "Reservist (Soldat)"@de , "Reservist (Soldier)"@en , "Soldat Réserviste"@fr ;
	owl:disjointWith :RegularForceSoldier ;
	owl:subClassOf :Soldier ;
	foaf:name "Reservist" .

:SeamanMilitary a owl:Class ;
	rdfs:comment "A Seaman serving in a political entity's Navy."@en ;
	rdfs:label "Matelot (Militare)"@fr , "Matrose (Militär)"@de , "Seaman (Military)"@en ;
	owl:subClassOf :PrivilegedCombatant .

:Ship a owl:Class ;
	rdfs:label ""@de , "Navire Militare"@fr , "Ship"@en .

:ShoreEstablishment a owl:Class ;
	rdfs:label "Etablishment de Terre (Marine)"@fr , "Shore Establishment (Navy)"@en , "Ufer Gründung (Kriegsmarine)"@de ;
	owl:disjointWith :warship ;
	owl:subClassOf :ship .

:Soldier a owl:Class ;
	rdfs:comment "A soldier serving in a political entity's Army."@en ;
	rdfs:label "Soldat"@de , "Soldat"@fr , "Soldier"@en ;
	owl:sameAs <dbpedia:Soldier> ;
	owl:subClassOf :PrivilegedCombatant ;
	foaf:name "Soldier" .

:Spy a owl:Class ;
	rdfs:comment "A person engaging in combat, war and/or espionage as an unprivileged combatant under the rules of war."@en ;
	rdfs:label "Espion"@fr , "Spion"@de , "Spy"@en ;
	owl:subClassOf :UnprivilegedCombatant ;
	foaf:name "Spy" .

:Squadron a owl:Class ;
	rdfs:label "Escadron"@fr , "Schwadron"@de , "Squadron (unit)"@en .

:SupplyTrain a owl:Class ;
	rdfs:comment "A supply organization moving military supplies."@en ;
	rdfs:label "Supply Train (Military)"@en , "Train D'alimentation (Military)"@fr , "liefern dem Zug (Militär)"@de .

:TacticalAirForce org:hasPart :AirForceGroup ;
	org:isPartOf :AirForceCommand , :AirForceServiceBranch ;
	a owl:Class ;
	rdfs:comment "Tactical Air Force."@en ;
	rdfs:label "Force Aérienne Tactique "@fr , "Luftstreitkräfte (taktisch)"@de , "Tactical Air Force"@en .

:UnprivilegedCombatant a owl:Class ;
	rdfs:comment "A person engaging in combat and/or war as an unprivileged combatants under the rules of war."@en ;
	rdfs:label "Combatant non-privilégié"@fr , "Unprivileged Combatant"@en , "unprivilegierten Kämpfer"@de ;
	owl:subClassOf :Combatant ;
	foaf:name "Unprivileged Combatant" .

:VolunteerSoldier a owl:Class ;
	rdfs:comment "A soldier which serves on a full-time basis."@en ;
	rdfs:label "Soldat (Volontaire)"@fr , "Soldat (freiwilliger)"@de , "Soldier (Volunteer)"@en ;
	owl:disjointWith :DraftedSoldier ;
	owl:subClassOf :RegularForceSoldier ;
	foaf:name "Volunteer" .

:War a owl:Class ;
	owl:subClassOf :WarEvent .

:WarTheater org:hasPart :FrontLine ;
	a owl:Class ;
	rdfs:comment "An army theater of war."@en ;
	rdfs:label "Kriegsschauplatz"@de , "Theater (warfare)"@en , "Théâtre militaire"@fr ;
	owl:sameAs "dbpedia:Theater_(warfare)" .

:WarrantOfficer a owl:Class ;
	rdfs:comment "A senior non-officer ."@en ;
	rdfs:label "?"@de , "Officiers Mariniers"@fr , "Warrant Officer"@en ;
	owl:subClassOf :Soldier ;
	foaf:name "Warrant Officer" .

:Warship a owl:Class ;
	rdfs:label ""@de , "Navire Militare"@fr , "Warship"@en ;
	owl:subClassOf :Ship .

:Weapon a owl:Class ;
	rdfs:comment "A weapon type but not a branch."@en ;
	rdfs:label "Arme (Military)"@fr , "Waffe (Militär)"@de , "Weapon (Military)"@en ;
	owl:sameAs <dbpedia:Weapon> .

:commanderInChiefOf a owl:ObjectProperty , <owl:FunctionalProperty> ;
	rdfs:label "Commander In Chief of"@en ;
	rdfs:range :MilitaryOrganization ;
	owl:inverseOf :hasCommanderInChief .

:epauletDepiction a owl:ObjectProperty ;
	rdfs:domain :MilitaryUniform ;
	rdfs:label "Epaulets"@en ;
	rdfs:subPropertyOf <foaf:depiction> .

:hasCommanderInChief a owl:ObjectProperty , <owl:FunctionalProperty> ;
	rdfs:domain :MilitaryOrganization ;
	rdfs:label "Commander In Chief"@en ;
	owl:inverseOf :CommanderInChiefOf .

:hasUniform a owl:ObjectProperty ;
	rdfs:domain <mil:MilitaryRank> ;
	rdfs:label "Has Uniform"@en ;
	rdfs:range <mil:MilitaryUniform> ;
	owl:inverseOf :CommanderInChiefOf .

:inUse a owl:ObjectProperty ;
	rdfs:domain :MilitaryUniform ;
	rdfs:label "In Use"@en ;
	rdfs:range <time:TemporalEntity> .

<http://rdf.muninn-project.org/ww1/2011/11/11/BattleSpace/FightsPrimarilyInAir> a :BattleSpace ;
	rdfs:comment "Fights primarily in Air."@en ;
	rdfs:label "Air (Battleground)"@en .

<http://rdf.muninn-project.org/ww1/2011/11/11/BattleSpace/FightsPrimarilyOnAndInLand> a :BattleSpace ;
	rdfs:comment "Fights primarily in and on Water."@en ;
	rdfs:label "Land (Battleground)"@en .

<http://rdf.muninn-project.org/ww1/2011/11/11/BattleSpace/FightsPrimarilyOnAndInWater> a :BattleSpace ;
	rdfs:comment "Fights primarily in and on Water."@en ;
	rdfs:label "Water (Battleground)"@en .

<http://rdf.muninn-project.org/ww1/2011/11/11/BattleSpace/information> a :BattleSpace ;
	rdfs:comment "Fights primarily with information, used for intelligence outfits."@en ;
	rdfs:label "Information"@en .

<http://rdf.muninn-project.org/ww1/2011/11/11/BattleSpace/spacethefinalfrontier> a :BattleSpace ;
	rdfs:comment "Fights primarily in space."@en ;
	rdfs:label "Space"@en .

<http://rdf.muninn-project.org/ww1/2011/11/11/GroupMemberships/NavyAppointments> a owl:Class ;
	owl:subClassOf <mil:Rank> .
