@prefix dc: <http://purl.org/dc/elements/1.1/> .
@prefix rdfs: <http://www.w3.org/2000/01/rdf-schema#> .
@prefix foaf: <http://xmlns.com/foaf/0.1/> .
@prefix status: <http://metadataregistry.org/uri/RegStatus/> .
@prefix reg: <http://metadataregistry.org/uri/profile/RegAp/> .
@prefix dct: <http://purl.org/dc/terms/> .
@prefix owl: <http://www.w3.org/2002/07/owl#> .
@prefix rdf: <http://www.w3.org/1999/02/22-rdf-syntax-ns#> .
@prefix skos: <http://www.w3.org/2004/02/skos/core#> .

status:1001 a skos:Concept ;
	skos:prefLabel "Published"@en .

<http://rdaregistry.info/Elements/a/> dc:title "RDA Agent properties"@en ;
	skos:note "Properties derived from RDA elements and relationship designators with the domain of RDA Agent."@en .

<http://rdaregistry.info/Elements/a/P50001> reg:name "respondentOf"@en ;
	reg:status status:1001 ;
	a rdf:Property ;
	rdfs:domain <http://rdaregistry.info/Elements/c/C10004> ;
	rdfs:isDefinedBy <http://rdaregistry.info/Elements/a/> ;
	rdfs:label "is respondent of"@en ;
	rdfs:range <http://rdaregistry.info/Elements/c/C10001> ;
	rdfs:subPropertyOf <http://rdaregistry.info/Elements/a/P50204> , <http://rdaregistry.info/Elements/u/P60001> ;
	owl:inverseOf <http://rdaregistry.info/Elements/w/P10001> ;
	owl:sameAs <http://rdaregistry.info/Elements/a/respondentOf> ;
	skos:definition "Relates a candidate for a degree who defends or opposes a thesis provided by the praeses in an academic disputation to the work."@en .

<http://rdaregistry.info/Elements/a/P50002> reg:name "appelleeCorporateBodyOf"@en ;
	reg:status status:1001 ;
	a rdf:Property ;
	rdfs:domain <http://rdaregistry.info/Elements/c/C10005> ;
	rdfs:isDefinedBy <http://rdaregistry.info/Elements/a/> ;
	rdfs:label "is appellee corporate body of"@en ;
	rdfs:range <http://rdaregistry.info/Elements/c/C10001> ;
	rdfs:subPropertyOf <http://rdaregistry.info/Elements/a/P50087> , <http://rdaregistry.info/Elements/u/P60601> ;
	owl:inverseOf <http://rdaregistry.info/Elements/w/P10005> ;
	owl:sameAs <http://rdaregistry.info/Elements/a/appelleeCorporateBodyOf> ;
	skos:definition "Relates a corporate body against whom an appeal is taken to the work."@en .

<http://rdaregistry.info/Elements/a/P50003> reg:name "degreeGrantingInstitutionOf"@en ;
	reg:status status:1001 ;
	a rdf:Property ;
	rdfs:domain <http://rdaregistry.info/Elements/c/C10005> ;
	rdfs:isDefinedBy <http://rdaregistry.info/Elements/a/> ;
	rdfs:label "is degree granting institution of"@en ;
	rdfs:range <http://rdaregistry.info/Elements/c/C10001> ;
	rdfs:subPropertyOf <http://rdaregistry.info/Elements/a/P50131> , <http://rdaregistry.info/Elements/u/P60002> ;
	owl:inverseOf <http://rdaregistry.info/Elements/w/P10006> ;
	owl:sameAs <http://rdaregistry.info/Elements/a/degreeGrantingInstitutionOf> ;
	skos:definition "Relates a corporate body granting an academic degree to the work."@en .

<http://rdaregistry.info/Elements/a/P50004> reg:name "hostInstitutionOf"@en ;
	reg:status status:1001 ;
	a rdf:Property ;
	rdfs:domain <http://rdaregistry.info/Elements/c/C10005> ;
	rdfs:isDefinedBy <http://rdaregistry.info/Elements/a/> ;
	rdfs:label "is host institution of"@en ;
	rdfs:range <http://rdaregistry.info/Elements/c/C10001> ;
	rdfs:subPropertyOf <http://rdaregistry.info/Elements/a/P50131> , <http://rdaregistry.info/Elements/u/P60003> ;
	owl:inverseOf <http://rdaregistry.info/Elements/w/P10007> ;
	owl:sameAs <http://rdaregistry.info/Elements/a/hostInstitutionOf> ;
	skos:definition "Relates a corporate body hosting the event, exhibit, conference, etc to the work."@en .

<http://rdaregistry.info/Elements/a/P50005> reg:name "productionCompanyOf"@en ;
	reg:status status:1001 ;
	a rdf:Property ;
	rdfs:domain <http://rdaregistry.info/Elements/c/C10005> ;
	rdfs:isDefinedBy <http://rdaregistry.info/Elements/a/> ;
	rdfs:label "is production company of"@en ;
	rdfs:range <http://rdaregistry.info/Elements/c/C10001> ;
	rdfs:subPropertyOf <http://rdaregistry.info/Elements/a/P50131> , <http://rdaregistry.info/Elements/u/P60004> ;
	owl:inverseOf <http://rdaregistry.info/Elements/w/P10008> ;
	owl:sameAs <http://rdaregistry.info/Elements/a/productionCompanyOf> ;
	skos:definition "Relates a corporate body that is responsible for financial, technical, and organizational management of a production for stage, screen, sound recording, television, webcast, etc to the work."@en .

<http://rdaregistry.info/Elements/a/P50006> reg:name "identifierForTheCorporateBody"@en ;
	reg:status status:1001 ;
	a rdf:Property ;
	rdfs:domain <http://rdaregistry.info/Elements/c/C10005> ;
	rdfs:isDefinedBy <http://rdaregistry.info/Elements/a/> ;
	rdfs:label "has identifier for the corporate body"@en ;
	rdfs:subPropertyOf <http://rdaregistry.info/Elements/u/P60053> ;
	owl:sameAs <http://rdaregistry.info/Elements/a/identifierForTheCorporateBody> ;
	skos:definition "Relates a corporate body to a character string uniquely associated with a corporate body, or with a surrogate for a corporate body (e.g., an authority record)."@en ;
	skos:scopeNote "The identifier serves to differentiate that corporate body from other corporate bodies."@en .

<http://rdaregistry.info/Elements/a/P50007> reg:name "foundingCorporateBody"@en ;
	reg:status status:1001 ;
	a rdf:Property ;
	rdfs:domain <http://rdaregistry.info/Elements/c/C10005> ;
	rdfs:isDefinedBy <http://rdaregistry.info/Elements/a/> ;
	rdfs:label "has founding corporate body"@en ;
	rdfs:range <http://rdaregistry.info/Elements/c/C10005> ;
	rdfs:subPropertyOf <http://rdaregistry.info/Elements/u/P60694> ;
	owl:inverseOf <http://rdaregistry.info/Elements/a/P50017> ;
	owl:sameAs <http://rdaregistry.info/Elements/a/foundingCorporateBody> ;
	skos:definition "Relates a corporate body to a corporate body that founded the other corporate body."@en .

<http://rdaregistry.info/Elements/a/P50008> reg:name "hierarchicalSuperior"@en ;
	reg:status status:1001 ;
	a rdf:Property ;
	rdfs:domain <http://rdaregistry.info/Elements/c/C10005> ;
	rdfs:isDefinedBy <http://rdaregistry.info/Elements/a/> ;
	rdfs:label "has hierarchical superior"@en ;
	rdfs:range <http://rdaregistry.info/Elements/c/C10005> ;
	rdfs:subPropertyOf <http://rdaregistry.info/Elements/u/P60680> ;
	owl:inverseOf <http://rdaregistry.info/Elements/a/P50010> ;
	owl:sameAs <http://rdaregistry.info/Elements/a/hierarchicalSuperior> ;
	skos:definition "Relates a corporate body to a corporate body that is hierarchically superior to the other corporate body."@en .

<http://rdaregistry.info/Elements/a/P50009> reg:name "sponsoredCorporateBodyOfCorporateBody"@en ;
	reg:status status:1001 ;
	a rdf:Property ;
	rdfs:domain <http://rdaregistry.info/Elements/c/C10005> ;
	rdfs:isDefinedBy <http://rdaregistry.info/Elements/a/> ;
	rdfs:label "has sponsored corporate body of corporate body"@en ;
	rdfs:range <http://rdaregistry.info/Elements/c/C10005> ;
	rdfs:subPropertyOf <http://rdaregistry.info/Elements/u/P60688> ;
	owl:inverseOf <http://rdaregistry.info/Elements/a/P50015> ;
	owl:sameAs <http://rdaregistry.info/Elements/a/sponsoredCorporateBodyOfCorporateBody> ;
	skos:definition "Relates a corporate body to a corporate body that is sponsored by the other corporate body."@en .

<http://rdaregistry.info/Elements/a/P50010> reg:name "hierarchicalSubordinate"@en ;
	reg:status status:1001 ;
	a rdf:Property ;
	rdfs:domain <http://rdaregistry.info/Elements/c/C10005> ;
	rdfs:isDefinedBy <http://rdaregistry.info/Elements/a/> ;
	rdfs:label "has hierarchical subordinate"@en ;
	rdfs:range <http://rdaregistry.info/Elements/c/C10005> ;
	rdfs:subPropertyOf <http://rdaregistry.info/Elements/u/P60681> ;
	owl:inverseOf <http://rdaregistry.info/Elements/a/P50008> ;
	owl:sameAs <http://rdaregistry.info/Elements/a/hierarchicalSubordinate> ;
	skos:definition "Relates a corporate body to a corporate body that is subordinate to the other corporate body."@en .

<http://rdaregistry.info/Elements/a/P50011> reg:name "mergee"@en ;
	reg:status status:1001 ;
	a rdf:Property ;
	rdfs:domain <http://rdaregistry.info/Elements/c/C10005> ;
	rdfs:isDefinedBy <http://rdaregistry.info/Elements/a/> ;
	rdfs:label "has mergee"@en ;
	rdfs:range <http://rdaregistry.info/Elements/c/C10005> ;
	rdfs:subPropertyOf <http://rdaregistry.info/Elements/u/P60682> ;
	owl:inverseOf <http://rdaregistry.info/Elements/a/P50011> ;
	owl:sameAs <http://rdaregistry.info/Elements/a/mergee> ;
	skos:definition "Relates a corporate body to a corporate body that merged with the other corporate body to form a third."@en .

<http://rdaregistry.info/Elements/a/P50012> reg:name "predecessor"@en ;
	reg:status status:1001 ;
	a rdf:Property ;
	rdfs:domain <http://rdaregistry.info/Elements/c/C10005> ;
	rdfs:isDefinedBy <http://rdaregistry.info/Elements/a/> ;
	rdfs:label "has predecessor"@en ;
	rdfs:range <http://rdaregistry.info/Elements/c/C10005> ;
	rdfs:subPropertyOf <http://rdaregistry.info/Elements/u/P60683> ;
	owl:inverseOf <http://rdaregistry.info/Elements/a/P50016> ;
	owl:sameAs <http://rdaregistry.info/Elements/a/predecessor> ;
	skos:definition "Relates a corporate body to a corporate body that precedes the other corporate body."@en .

<http://rdaregistry.info/Elements/a/P50013> reg:name "productOfAMerger"@en ;
	reg:status status:1001 ;
	a rdf:Property ;
	rdfs:domain <http://rdaregistry.info/Elements/c/C10005> ;
	rdfs:isDefinedBy <http://rdaregistry.info/Elements/a/> ;
	rdfs:label "has product of merger"@en ;
	rdfs:range <http://rdaregistry.info/Elements/c/C10005> ;
	rdfs:subPropertyOf <http://rdaregistry.info/Elements/u/P60684> ;
	owl:inverseOf <http://rdaregistry.info/Elements/a/P50232> ;
	owl:sameAs <http://rdaregistry.info/Elements/a/productOfAMerger> ;
	skos:definition "Relates a corporate body to a corporate body that resulted from a merger of two or more other corporate bodies."@en .

<http://rdaregistry.info/Elements/a/P50014> reg:name "productOfASplit"@en ;
	reg:status status:1001 ;
	a rdf:Property ;
	rdfs:domain <http://rdaregistry.info/Elements/c/C10005> ;
	rdfs:isDefinedBy <http://rdaregistry.info/Elements/a/> ;
	rdfs:label "has product of split"@en ;
	rdfs:range <http://rdaregistry.info/Elements/c/C10005> ;
	rdfs:subPropertyOf <http://rdaregistry.info/Elements/u/P60685> ;
	owl:inverseOf <http://rdaregistry.info/Elements/a/P50229> ;
	owl:sameAs <http://rdaregistry.info/Elements/a/productOfASplit> ;
	skos:definition "Relates a corporate body to a corporate body that resulted from a split or division of the other corporate body."@en .

<http://rdaregistry.info/Elements/a/P50015> reg:name "sponsoringCorporateBody"@en ;
	reg:status status:1001 ;
	a rdf:Property ;
	rdfs:domain <http://rdaregistry.info/Elements/c/C10005> ;
	rdfs:isDefinedBy <http://rdaregistry.info/Elements/a/> ;
	rdfs:label "has sponsoring corporate body"@en ;
	rdfs:range <http://rdaregistry.info/Elements/c/C10005> ;
	rdfs:subPropertyOf <http://rdaregistry.info/Elements/u/P60676> ;
	owl:inverseOf <http://rdaregistry.info/Elements/a/P50009> ;
	owl:sameAs <http://rdaregistry.info/Elements/a/sponsoringCorporateBody> ;
	skos:definition "Relates a corporate body to a corporate body that sponsors the other corporate body."@en .

<http://rdaregistry.info/Elements/a/P50016> reg:name "successor"@en ;
	reg:status status:1001 ;
	a rdf:Property ;
	rdfs:domain <http://rdaregistry.info/Elements/c/C10005> ;
	rdfs:isDefinedBy <http://rdaregistry.info/Elements/a/> ;
	rdfs:label "has successor"@en ;
	rdfs:range <http://rdaregistry.info/Elements/c/C10005> ;
	rdfs:subPropertyOf <http://rdaregistry.info/Elements/u/P60686> ;
	owl:inverseOf <http://rdaregistry.info/Elements/a/P50012> ;
	owl:sameAs <http://rdaregistry.info/Elements/a/successor> ;
	skos:definition "Relates a corporate body to a corporate body that succeeds or follows the other corporate body."@en .

<http://rdaregistry.info/Elements/a/P50017> reg:name "foundedCorporateBodyOfCorporateBody"@en ;
	reg:status status:1001 ;
	a rdf:Property ;
	rdfs:domain <http://rdaregistry.info/Elements/c/C10005> ;
	rdfs:isDefinedBy <http://rdaregistry.info/Elements/a/> ;
	rdfs:label "has founded corporate body of corporate body"@en ;
	rdfs:range <http://rdaregistry.info/Elements/c/C10005> ;
	rdfs:subPropertyOf <http://rdaregistry.info/Elements/u/P60687> ;
	owl:inverseOf <http://rdaregistry.info/Elements/a/P50007> ;
	owl:sameAs <http://rdaregistry.info/Elements/a/foundedCorporateBodyOfCorporateBody> ;
	skos:definition "Relates a corporate body to a corporate body that the other corporate body founded."@en .

<http://rdaregistry.info/Elements/a/P50018> reg:name "locationOfHeadquarters"@en ;
	reg:status status:1001 ;
	a rdf:Property ;
	rdfs:domain <http://rdaregistry.info/Elements/c/C10005> ;
	rdfs:isDefinedBy <http://rdaregistry.info/Elements/a/> ;
	rdfs:label "has location of headquarters"@en ;
	rdfs:subPropertyOf <http://rdaregistry.info/Elements/a/P50031> , <http://rdaregistry.info/Elements/u/P60064> ;
	owl:sameAs <http://rdaregistry.info/Elements/a/locationOfHeadquarters> ;
	skos:definition "Relates a corporate body to a country, state, province, etc., or local place in which an organization has its headquarters."@en .

<http://rdaregistry.info/Elements/a/P50019> reg:name "numberOfAConferenceEtc"@en ;
	reg:status status:1001 ;
	a rdf:Property ;
	rdfs:domain <http://rdaregistry.info/Elements/c/C10005> ;
	rdfs:isDefinedBy <http://rdaregistry.info/Elements/a/> ;
	rdfs:label "has number of a conference, etc."@en ;
	rdfs:subPropertyOf <http://rdaregistry.info/Elements/u/P60079> ;
	owl:sameAs <http://rdaregistry.info/Elements/a/numberOfAConferenceEtc> ;
	skos:definition "Relates a corporate body to a designation of the sequencing of a conference, etc., within a series of conferences, etc."@en .

<http://rdaregistry.info/Elements/a/P50020> reg:name "foundingFamily"@en ;
	reg:status status:1001 ;
	a rdf:Property ;
	rdfs:domain <http://rdaregistry.info/Elements/c/C10005> ;
	rdfs:isDefinedBy <http://rdaregistry.info/Elements/a/> ;
	rdfs:label "has founding family"@en ;
	rdfs:range <http://rdaregistry.info/Elements/c/C10008> ;
	rdfs:subPropertyOf <http://rdaregistry.info/Elements/u/P60694> ;
	owl:inverseOf <http://rdaregistry.info/Elements/a/P50062> ;
	owl:sameAs <http://rdaregistry.info/Elements/a/foundingFamily> ;
	skos:definition "Relates a corporate body to a family that founded the corporate body."@en .

<http://rdaregistry.info/Elements/a/P50021> reg:name "sponsoringFamily"@en ;
	reg:status status:1001 ;
	a rdf:Property ;
	rdfs:domain <http://rdaregistry.info/Elements/c/C10005> ;
	rdfs:isDefinedBy <http://rdaregistry.info/Elements/a/> ;
	rdfs:label "has sponsoring family"@en ;
	rdfs:range <http://rdaregistry.info/Elements/c/C10008> ;
	rdfs:subPropertyOf <http://rdaregistry.info/Elements/u/P60676> ;
	owl:inverseOf <http://rdaregistry.info/Elements/a/P50063> ;
	owl:sameAs <http://rdaregistry.info/Elements/a/sponsoringFamily> ;
	skos:definition "Relates a corporate body to a family that sponsors the corporate body."@en .

<http://rdaregistry.info/Elements/a/P50022> reg:name "fieldOfActivityOfTheCorporateBody"@en ;
	reg:status status:1001 ;
	a rdf:Property ;
	rdfs:domain <http://rdaregistry.info/Elements/c/C10005> ;
	rdfs:isDefinedBy <http://rdaregistry.info/Elements/a/> ;
	rdfs:label "has field of activity of the corporate body"@en ;
	rdfs:subPropertyOf <http://rdaregistry.info/Elements/u/P60089> ;
	owl:sameAs <http://rdaregistry.info/Elements/a/fieldOfActivityOfTheCorporateBody> ;
	skos:definition "Relates a corporate body to a field of business in which a corporate body is engaged and/or the body's area of competence, responsibility, jurisdiction, etc."@en .

<http://rdaregistry.info/Elements/a/P50023> reg:name "languageOfTheCorporateBody"@en ;
	reg:status status:1001 ;
	a rdf:Property ;
	rdfs:domain <http://rdaregistry.info/Elements/c/C10005> ;
	rdfs:isDefinedBy <http://rdaregistry.info/Elements/a/> ;
	rdfs:label "has language of the corporate body"@en ;
	rdfs:subPropertyOf <http://rdaregistry.info/Elements/u/P60098> ;
	owl:sameAs <http://rdaregistry.info/Elements/a/languageOfTheCorporateBody> ;
	skos:definition "Relates a corporate body to a language a corporate body uses in its communications."@en .

<http://rdaregistry.info/Elements/a/P50024> reg:name "locationOfConferenceEtc"@en ;
	reg:status status:1001 ;
	a rdf:Property ;
	rdfs:domain <http://rdaregistry.info/Elements/c/C10005> ;
	rdfs:isDefinedBy <http://rdaregistry.info/Elements/a/> ;
	rdfs:label "has location of conference, etc."@en ;
	rdfs:subPropertyOf <http://rdaregistry.info/Elements/a/P50031> , <http://rdaregistry.info/Elements/u/P60107> ;
	owl:sameAs <http://rdaregistry.info/Elements/a/locationOfConferenceEtc> ;
	skos:definition "Relates a corporate body to a local place in which a conference, congress, meeting, exhibition, fair, festival, etc., was held."@en .

<http://rdaregistry.info/Elements/a/P50025> reg:name "variantNameForTheCorporateBody"@en ;
	reg:status status:1001 ;
	a rdf:Property ;
	rdfs:domain <http://rdaregistry.info/Elements/c/C10005> ;
	rdfs:isDefinedBy <http://rdaregistry.info/Elements/a/> ;
	rdfs:label "has variant name for the corporate body"@en ;
	rdfs:subPropertyOf <http://rdaregistry.info/Elements/a/P50032> , <http://rdaregistry.info/Elements/u/P60119> ;
	owl:sameAs <http://rdaregistry.info/Elements/a/variantNameForTheCorporateBody> ;
	skos:definition "Relates a corporate body to a name or form of name by which a corporate body is known that differs from the name or form of name chosen as the preferred name."@en .

<http://rdaregistry.info/Elements/a/P50026> reg:name "employee"@en ;
	reg:status status:1001 ;
	a rdf:Property ;
	rdfs:domain <http://rdaregistry.info/Elements/c/C10005> ;
	rdfs:isDefinedBy <http://rdaregistry.info/Elements/a/> ;
	rdfs:label "has employee"@en ;
	rdfs:range <http://rdaregistry.info/Elements/c/C10004> ;
	rdfs:subPropertyOf <http://rdaregistry.info/Elements/u/P60629> ;
	owl:inverseOf <http://rdaregistry.info/Elements/a/P50096> ;
	owl:sameAs <http://rdaregistry.info/Elements/a/employee> ;
	skos:definition "Relates a corporate body to a person employed by the corporate body."@en .

<http://rdaregistry.info/Elements/a/P50027> reg:name "incumbent"@en ;
	reg:status status:1001 ;
	a rdf:Property ;
	rdfs:domain <http://rdaregistry.info/Elements/c/C10005> ;
	rdfs:isDefinedBy <http://rdaregistry.info/Elements/a/> ;
	rdfs:label "has incumbent"@en ;
	rdfs:range <http://rdaregistry.info/Elements/c/C10004> ;
	rdfs:subPropertyOf <http://rdaregistry.info/Elements/u/P60633> ;
	owl:inverseOf <http://rdaregistry.info/Elements/a/P50234> ;
	owl:sameAs <http://rdaregistry.info/Elements/a/incumbent> ;
	skos:definition "Relates a corporate body to a person holding an office in the corporate body."@en .

<http://rdaregistry.info/Elements/a/P50028> reg:name "sponsor"@en ;
	reg:status status:1001 ;
	a rdf:Property ;
	rdfs:domain <http://rdaregistry.info/Elements/c/C10005> ;
	rdfs:isDefinedBy <http://rdaregistry.info/Elements/a/> ;
	rdfs:label "has sponsor"@en ;
	rdfs:range <http://rdaregistry.info/Elements/c/C10004> ;
	rdfs:subPropertyOf <http://rdaregistry.info/Elements/u/P60676> ;
	owl:sameAs <http://rdaregistry.info/Elements/a/sponsor> ;
	skos:definition "Relates a corporate body to a person sponsoring the corporate body."@en .

<http://rdaregistry.info/Elements/a/P50029> reg:name "founder"@en ;
	reg:status status:1001 ;
	a rdf:Property ;
	rdfs:domain <http://rdaregistry.info/Elements/c/C10005> ;
	rdfs:isDefinedBy <http://rdaregistry.info/Elements/a/> ;
	rdfs:label "has founder"@en ;
	rdfs:range <http://rdaregistry.info/Elements/c/C10004> ;
	rdfs:subPropertyOf <http://rdaregistry.info/Elements/u/P60694> ;
	owl:inverseOf <http://rdaregistry.info/Elements/a/P50112> ;
	owl:sameAs <http://rdaregistry.info/Elements/a/founder> ;
	skos:definition "Relates a corporate body to a person who founded the corporate body."@en .

<http://rdaregistry.info/Elements/a/P50030> reg:name "groupMember"@en ;
	reg:status status:1001 ;
	a rdf:Property ;
	rdfs:domain <http://rdaregistry.info/Elements/c/C10005> ;
	rdfs:isDefinedBy <http://rdaregistry.info/Elements/a/> ;
	rdfs:label "has group member"@en ;
	rdfs:range <http://rdaregistry.info/Elements/c/C10004> ;
	rdfs:subPropertyOf <http://rdaregistry.info/Elements/u/P60697> ;
	owl:inverseOf <http://rdaregistry.info/Elements/a/P50095> ;
	owl:sameAs <http://rdaregistry.info/Elements/a/groupMember> ;
	skos:definition "Relates a corporate body to a person who is a member of the performing group, expedition, etc."@en .

<http://rdaregistry.info/Elements/a/P50031> reg:name "placeAssociatedWithTheCorporateBody"@en ;
	reg:status status:1001 ;
	a rdf:Property ;
	rdfs:domain <http://rdaregistry.info/Elements/c/C10005> ;
	rdfs:isDefinedBy <http://rdaregistry.info/Elements/a/> ;
	rdfs:label "has place associated with the corporate body"@en ;
	rdfs:subPropertyOf <http://rdaregistry.info/Elements/u/P60325> ;
	owl:sameAs <http://rdaregistry.info/Elements/a/placeAssociatedWithTheCorporateBody> ;
	skos:definition "Relates a corporate body to a significant location associated with a corporate body (e.g., location of a conference, etc., location of the headquarters of an organization)."@en .

<http://rdaregistry.info/Elements/a/P50032> reg:hasSubproperty <http://rdaregistry.info/Elements/a/P50041> ;
	reg:name "nameOfTheCorporateBody"@en ;
	reg:status status:1001 ;
	a rdf:Property ;
	rdfs:domain <http://rdaregistry.info/Elements/c/C10005> ;
	rdfs:isDefinedBy <http://rdaregistry.info/Elements/a/> ;
	rdfs:label "has name of the corporate body"@en ;
	rdfs:subPropertyOf <http://rdaregistry.info/Elements/u/P60368> ;
	owl:sameAs <http://rdaregistry.info/Elements/a/nameOfTheCorporateBody> ;
	skos:definition "Relates a corporate body to a word, character, or group of words and/or characters by which a corporate body is known."@en .

<http://rdaregistry.info/Elements/a/P50033> reg:name "otherDesignationAssociatedWithTheCorporateBody"@en ;
	reg:status status:1001 ;
	a rdf:Property ;
	rdfs:domain <http://rdaregistry.info/Elements/c/C10005> ;
	rdfs:isDefinedBy <http://rdaregistry.info/Elements/a/> ;
	rdfs:label "has other designation associated with the corporate body"@en ;
	rdfs:subPropertyOf <http://rdaregistry.info/Elements/u/P60370> ;
	owl:sameAs <http://rdaregistry.info/Elements/a/otherDesignationAssociatedWithTheCorporateBody> ;
	skos:definition "Relates a corporate body to a word, phrase, or abbreviation indicating incorporation or legal status of a corporate body, or any term serving to differentiate the body from other corporate bodies, persons, etc."@en .

<http://rdaregistry.info/Elements/a/P50034> reg:name "associatedInstitution"@en ;
	reg:status status:1001 ;
	a rdf:Property ;
	rdfs:domain <http://rdaregistry.info/Elements/c/C10005> ;
	rdfs:isDefinedBy <http://rdaregistry.info/Elements/a/> ;
	rdfs:label "has associated institution"@en ;
	rdfs:subPropertyOf <http://rdaregistry.info/Elements/u/P60482> ;
	owl:sameAs <http://rdaregistry.info/Elements/a/associatedInstitution> ;
	skos:definition "Relates a corporate body to an institution commonly associated with a corporate body."@en .

<http://rdaregistry.info/Elements/a/P50035> reg:name "corporateHistory"@en ;
	reg:status status:1001 ;
	a rdf:Property ;
	rdfs:domain <http://rdaregistry.info/Elements/c/C10005> ;
	rdfs:isDefinedBy <http://rdaregistry.info/Elements/a/> ;
	rdfs:label "has corporate history"@en ;
	rdfs:subPropertyOf <http://rdaregistry.info/Elements/u/P60484> ;
	owl:sameAs <http://rdaregistry.info/Elements/a/corporateHistory> ;
	skos:definition "Relates a corporate body to historical information about the corporate body."@en .

<http://rdaregistry.info/Elements/a/P50036> reg:name "addressOfTheCorporateBody"@en ;
	reg:status status:1001 ;
	a rdf:Property ;
	rdfs:domain <http://rdaregistry.info/Elements/c/C10005> ;
	rdfs:isDefinedBy <http://rdaregistry.info/Elements/a/> ;
	rdfs:label "has address of the corporate body"@en ;
	rdfs:subPropertyOf <http://rdaregistry.info/Elements/u/P60512> ;
	owl:sameAs <http://rdaregistry.info/Elements/a/addressOfTheCorporateBody> ;
	skos:definition "Relates a corporate body to the address of a corporate body’s headquarters or offices, or an e-mail or internet address for the body."@en .

<http://rdaregistry.info/Elements/a/P50037> reg:name "dateOfEstablishment"@en ;
	reg:status status:1001 ;
	a rdf:Property ;
	rdfs:domain <http://rdaregistry.info/Elements/c/C10005> ;
	rdfs:isDefinedBy <http://rdaregistry.info/Elements/a/> ;
	rdfs:label "has date of establishment"@en ;
	rdfs:subPropertyOf <http://rdaregistry.info/Elements/a/P50040> , <http://rdaregistry.info/Elements/u/P60524> ;
	owl:sameAs <http://rdaregistry.info/Elements/a/dateOfEstablishment> ;
	skos:definition "Relates a corporate body to the date on which a corporate body was established or founded."@en .

<http://rdaregistry.info/Elements/a/P50038> reg:name "dateOfTermination"@en ;
	reg:status status:1001 ;
	a rdf:Property ;
	rdfs:domain <http://rdaregistry.info/Elements/c/C10005> ;
	rdfs:isDefinedBy <http://rdaregistry.info/Elements/a/> ;
	rdfs:label "has date of termination"@en ;
	rdfs:subPropertyOf <http://rdaregistry.info/Elements/a/P50040> , <http://rdaregistry.info/Elements/u/P60525> ;
	owl:sameAs <http://rdaregistry.info/Elements/a/dateOfTermination> ;
	skos:definition "Relates a corporate body to the date on which a corporate body was terminated or dissolved."@en .

<http://rdaregistry.info/Elements/a/P50039> reg:name "dateOfConferenceEtc"@en ;
	reg:status status:1001 ;
	a rdf:Property ;
	rdfs:domain <http://rdaregistry.info/Elements/c/C10005> ;
	rdfs:isDefinedBy <http://rdaregistry.info/Elements/a/> ;
	rdfs:label "has date of conference, etc."@en ;
	rdfs:subPropertyOf <http://rdaregistry.info/Elements/a/P50040> , <http://rdaregistry.info/Elements/u/P60526> ;
	owl:sameAs <http://rdaregistry.info/Elements/a/dateOfConferenceEtc> ;
	skos:definition "Relates a corporate body to the date or range of dates on which a conference, congress, meeting, exhibition, fair, festival, etc., was held."@en .

<http://rdaregistry.info/Elements/a/P50040> reg:hasSubproperty <http://rdaregistry.info/Elements/a/P50037> , <http://rdaregistry.info/Elements/a/P50038> , <http://rdaregistry.info/Elements/a/P50039> ;
	reg:name "dateAssociatedWithTheCorporateBody"@en ;
	reg:status status:1001 ;
	a rdf:Property ;
	rdfs:domain <http://rdaregistry.info/Elements/c/C10005> ;
	rdfs:isDefinedBy <http://rdaregistry.info/Elements/a/> ;
	rdfs:label "has date associated with the corporate body"@en ;
	rdfs:subPropertyOf <http://rdaregistry.info/Elements/u/P60324> ;
	owl:sameAs <http://rdaregistry.info/Elements/a/dateAssociatedWithTheCorporateBody> ;
	skos:definition "Relates a corporate body to the date or range of dates on which a conference, etc., was held, or a date with which a corporate body is otherwise associated (e.g., date of founding)."@en .

<http://rdaregistry.info/Elements/a/P50041> reg:name "preferredNameForTheCorporateBody"@en ;
	reg:status status:1001 ;
	a rdf:Property ;
	rdfs:domain <http://rdaregistry.info/Elements/c/C10005> ;
	rdfs:isDefinedBy <http://rdaregistry.info/Elements/a/> ;
	rdfs:label "has preferred name for the corporate body"@en ;
	rdfs:subPropertyOf <http://rdaregistry.info/Elements/a/P50032> , <http://rdaregistry.info/Elements/u/P60549> ;
	owl:sameAs <http://rdaregistry.info/Elements/a/preferredNameForTheCorporateBody> ;
	skos:definition "Relates a corporate body to the name or form of name chosen to identify the corporate body. it is also the basis for the authorized access point representing that body."@en .

<http://rdaregistry.info/Elements/a/P50042> reg:name "appellantCorporateBodyOf"@en ;
	reg:status status:1001 ;
	a rdf:Property ;
	rdfs:domain <http://rdaregistry.info/Elements/c/C10005> ;
	rdfs:isDefinedBy <http://rdaregistry.info/Elements/a/> ;
	rdfs:label "is appellant corporate body of"@en ;
	rdfs:range <http://rdaregistry.info/Elements/c/C10001> ;
	rdfs:subPropertyOf <http://rdaregistry.info/Elements/a/P50088> , <http://rdaregistry.info/Elements/u/P60691> ;
	owl:inverseOf <http://rdaregistry.info/Elements/w/P10009> ;
	owl:sameAs <http://rdaregistry.info/Elements/a/appellantCorporateBodyOf> ;
	skos:definition "Relates a corporate body who appeals a lower court's decision to the work."@en .

<http://rdaregistry.info/Elements/a/P50043> reg:name "plaintiffCorporateBodyOf"@en ;
	reg:status status:1001 ;
	a rdf:Property ;
	rdfs:domain <http://rdaregistry.info/Elements/c/C10005> ;
	rdfs:isDefinedBy <http://rdaregistry.info/Elements/a/> ;
	rdfs:label "is plaintiff corporate body of"@en ;
	rdfs:range <http://rdaregistry.info/Elements/c/C10001> ;
	rdfs:subPropertyOf <http://rdaregistry.info/Elements/a/P50089> , <http://rdaregistry.info/Elements/u/P60693> ;
	owl:inverseOf <http://rdaregistry.info/Elements/w/P10010> ;
	owl:sameAs <http://rdaregistry.info/Elements/a/plaintiffCorporateBodyOf> ;
	skos:definition "Relates a corporate body who brings a suit in a civil proceeding to the work."@en .

<http://rdaregistry.info/Elements/a/P50044> reg:name "courtGovernedOf"@en ;
	reg:status status:1001 ;
	a rdf:Property ;
	rdfs:domain <http://rdaregistry.info/Elements/c/C10005> ;
	rdfs:isDefinedBy <http://rdaregistry.info/Elements/a/> ;
	rdfs:label "is court governed of"@en ;
	rdfs:range <http://rdaregistry.info/Elements/c/C10001> ;
	rdfs:subPropertyOf <http://rdaregistry.info/Elements/a/P50131> , <http://rdaregistry.info/Elements/u/P60005> ;
	owl:inverseOf <http://rdaregistry.info/Elements/w/P10011> ;
	owl:sameAs <http://rdaregistry.info/Elements/a/courtGovernedOf> ;
	skos:definition "Relates a court governed by court rules, regardless of their official nature (e.g., laws, administrative regulations) to the work."@en .

<http://rdaregistry.info/Elements/a/P50045> reg:name "collectorOf"@en ;
	reg:status status:1001 ;
	a rdf:Property ;
	rdfs:domain <http://rdaregistry.info/Elements/c/C10002> ;
	rdfs:isDefinedBy <http://rdaregistry.info/Elements/a/> ;
	rdfs:label "is collector of"@en ;
	rdfs:range <http://rdaregistry.info/Elements/c/C10003> ;
	rdfs:subPropertyOf <http://rdaregistry.info/Elements/a/P50133> , <http://rdaregistry.info/Elements/u/P60006> ;
	owl:inverseOf <http://rdaregistry.info/Elements/i/P40004> ;
	owl:sameAs <http://rdaregistry.info/Elements/a/collectorOf> ;
	skos:definition "Relates a curator who brings together items from various sources that are then arranged, described, and cataloged as a collection to the item."@en .

<http://rdaregistry.info/Elements/a/P50046> reg:name "collectionRegistrarOf"@en ;
	reg:status status:1001 ;
	a rdf:Property ;
	rdfs:domain <http://rdaregistry.info/Elements/c/C10002> ;
	rdfs:isDefinedBy <http://rdaregistry.info/Elements/a/> ;
	rdfs:label "is collection registrar of"@en ;
	rdfs:range <http://rdaregistry.info/Elements/c/C10003> ;
	rdfs:subPropertyOf <http://rdaregistry.info/Elements/a/P50133> , <http://rdaregistry.info/Elements/u/P60007> ;
	owl:inverseOf <http://rdaregistry.info/Elements/i/P40005> ;
	owl:sameAs <http://rdaregistry.info/Elements/a/collectionRegistrarOf> ;
	skos:definition "Relates a curator who lists or inventories the items in an aggregate work such as a collection of items or works to the item."@en .

<http://rdaregistry.info/Elements/a/P50047> reg:name "depositorOf"@en ;
	reg:status status:1001 ;
	a rdf:Property ;
	rdfs:domain <http://rdaregistry.info/Elements/c/C10002> ;
	rdfs:isDefinedBy <http://rdaregistry.info/Elements/a/> ;
	rdfs:label "is depositor of"@en ;
	rdfs:range <http://rdaregistry.info/Elements/c/C10003> ;
	rdfs:subPropertyOf <http://rdaregistry.info/Elements/a/P50162> , <http://rdaregistry.info/Elements/u/P60008> ;
	owl:inverseOf <http://rdaregistry.info/Elements/i/P40006> ;
	owl:sameAs <http://rdaregistry.info/Elements/a/depositorOf> ;
	skos:definition "Relates a current owner of an item who deposited the item into the custody of another person, family, or corporate body, while still retaining ownership to the item."@en .

<http://rdaregistry.info/Elements/a/P50048> reg:name "filmDirectorOf"@en ;
	reg:status status:1001 ;
	a rdf:Property ;
	rdfs:domain <http://rdaregistry.info/Elements/c/C10002> ;
	rdfs:isDefinedBy <http://rdaregistry.info/Elements/a/> ;
	rdfs:label "is film director of"@en ;
	rdfs:range <http://rdaregistry.info/Elements/c/C10001> ;
	rdfs:subPropertyOf <http://rdaregistry.info/Elements/a/P50205> , <http://rdaregistry.info/Elements/u/P60009> ;
	owl:inverseOf <http://rdaregistry.info/Elements/w/P10013> ;
	owl:sameAs <http://rdaregistry.info/Elements/a/filmDirectorOf> ;
	skos:definition "Relates a director responsible for the general management and supervision of a filmed performance to the work."@en .

<http://rdaregistry.info/Elements/a/P50049> reg:name "radioDirectorOf"@en ;
	reg:status status:1001 ;
	a rdf:Property ;
	rdfs:domain <http://rdaregistry.info/Elements/c/C10002> ;
	rdfs:isDefinedBy <http://rdaregistry.info/Elements/a/> ;
	rdfs:label "is radio director of"@en ;
	rdfs:range <http://rdaregistry.info/Elements/c/C10001> ;
	rdfs:subPropertyOf <http://rdaregistry.info/Elements/a/P50205> , <http://rdaregistry.info/Elements/u/P60010> ;
	owl:inverseOf <http://rdaregistry.info/Elements/w/P10014> ;
	owl:sameAs <http://rdaregistry.info/Elements/a/radioDirectorOf> ;
	skos:definition "Relates a director responsible for the general management and supervision of a radio program to the work."@en .

<http://rdaregistry.info/Elements/a/P50050> reg:name "televisionDirectorOf"@en ;
	reg:status status:1001 ;
	a rdf:Property ;
	rdfs:domain <http://rdaregistry.info/Elements/c/C10002> ;
	rdfs:isDefinedBy <http://rdaregistry.info/Elements/a/> ;
	rdfs:label "is television director of"@en ;
	rdfs:range <http://rdaregistry.info/Elements/c/C10001> ;
	rdfs:subPropertyOf <http://rdaregistry.info/Elements/a/P50205> , <http://rdaregistry.info/Elements/u/P60011> ;
	owl:inverseOf <http://rdaregistry.info/Elements/w/P10015> ;
	owl:sameAs <http://rdaregistry.info/Elements/a/televisionDirectorOf> ;
	skos:definition "Relates a director responsible for the general management and supervision of a television program to the work."@en .

<http://rdaregistry.info/Elements/a/P50051> reg:name "typeOfFamily"@en ;
	reg:status status:1001 ;
	a rdf:Property ;
	rdfs:domain <http://rdaregistry.info/Elements/c/C10008> ;
	rdfs:isDefinedBy <http://rdaregistry.info/Elements/a/> ;
	rdfs:label "has type of family"@en ;
	rdfs:subPropertyOf <http://rdaregistry.info/Elements/u/P60047> ;
	owl:sameAs <http://rdaregistry.info/Elements/a/typeOfFamily> ;
	skos:definition "Relates a family to a categorization or generic descriptor for the type of family."@en .

<http://rdaregistry.info/Elements/a/P50052> reg:name "identifierForTheFamily"@en ;
	reg:status status:1001 ;
	a rdf:Property ;
	rdfs:domain <http://rdaregistry.info/Elements/c/C10008> ;
	rdfs:isDefinedBy <http://rdaregistry.info/Elements/a/> ;
	rdfs:label "has identifier for the family"@en ;
	rdfs:subPropertyOf <http://rdaregistry.info/Elements/u/P60053> ;
	owl:sameAs <http://rdaregistry.info/Elements/a/identifierForTheFamily> ;
	skos:definition "Relates a family to a character string uniquely associated with a family, or with a surrogate for a family (e.g., an authority record)."@en ;
	skos:scopeNote "The identifier serves to differentiate that family from other families."@en .

<http://rdaregistry.info/Elements/a/P50053> reg:name "descendantFamily"@en ;
	reg:status status:1001 ;
	a rdf:Property ;
	rdfs:domain <http://rdaregistry.info/Elements/c/C10008> ;
	rdfs:isDefinedBy <http://rdaregistry.info/Elements/a/> ;
	rdfs:label "has descendant family"@en ;
	rdfs:range <http://rdaregistry.info/Elements/c/C10008> ;
	rdfs:subPropertyOf <http://rdaregistry.info/Elements/u/P60686> ;
	owl:sameAs <http://rdaregistry.info/Elements/a/descendantFamily> ;
	skos:definition "Relates a family to a family descended from the other family."@en .

<http://rdaregistry.info/Elements/a/P50054> reg:name "variantNameForTheFamily"@en ;
	reg:status status:1001 ;
	a rdf:Property ;
	rdfs:domain <http://rdaregistry.info/Elements/c/C10008> ;
	rdfs:isDefinedBy <http://rdaregistry.info/Elements/a/> ;
	rdfs:label "has variant name for the family"@en ;
	rdfs:subPropertyOf <http://rdaregistry.info/Elements/a/P50061> , <http://rdaregistry.info/Elements/u/P60119> ;
	owl:sameAs <http://rdaregistry.info/Elements/a/variantNameForTheFamily> ;
	skos:definition "Relates a family to a name or form of name by which a family is known that differs from the name or form of name chosen as the preferred name."@en .

<http://rdaregistry.info/Elements/a/P50055> reg:name "progenitor"@en ;
	reg:status status:1001 ;
	a rdf:Property ;
	rdfs:domain <http://rdaregistry.info/Elements/c/C10008> ;
	rdfs:isDefinedBy <http://rdaregistry.info/Elements/a/> ;
	rdfs:label "has progenitor"@en ;
	rdfs:range <http://rdaregistry.info/Elements/c/C10004> ;
	rdfs:subPropertyOf <http://rdaregistry.info/Elements/a/P50056> , <http://rdaregistry.info/Elements/u/P60683> ;
	owl:inverseOf <http://rdaregistry.info/Elements/a/P50099> ;
	owl:sameAs <http://rdaregistry.info/Elements/a/progenitor> ;
	skos:definition "Relates a family to a person from whom the family is descended."@en .

<http://rdaregistry.info/Elements/a/P50056> reg:hasSubproperty <http://rdaregistry.info/Elements/a/P50055> ;
	reg:name "familyMember"@en ;
	reg:status status:1001 ;
	a rdf:Property ;
	rdfs:domain <http://rdaregistry.info/Elements/c/C10008> ;
	rdfs:isDefinedBy <http://rdaregistry.info/Elements/a/> ;
	rdfs:label "has family member"@en ;
	rdfs:range <http://rdaregistry.info/Elements/c/C10004> ;
	rdfs:subPropertyOf <http://rdaregistry.info/Elements/u/P60648> ;
	owl:inverseOf <http://rdaregistry.info/Elements/a/P50233> ;
	owl:sameAs <http://rdaregistry.info/Elements/a/familyMember> ;
	skos:definition "Relates a family to a person who is a member of the family."@en .

<http://rdaregistry.info/Elements/a/P50057> reg:name "placeAssociatedWithTheFamily"@en ;
	reg:status status:1001 ;
	a rdf:Property ;
	rdfs:domain <http://rdaregistry.info/Elements/c/C10008> ;
	rdfs:isDefinedBy <http://rdaregistry.info/Elements/a/> ;
	rdfs:label "has place associated with the family"@en ;
	rdfs:subPropertyOf <http://rdaregistry.info/Elements/u/P60325> ;
	owl:sameAs <http://rdaregistry.info/Elements/a/placeAssociatedWithTheFamily> ;
	skos:definition "Relates a family to a place where a family resides or has resided or has some connection."@en .

<http://rdaregistry.info/Elements/a/P50058> reg:name "dateAssociatedWithTheFamily"@en ;
	reg:status status:1001 ;
	a rdf:Property ;
	rdfs:domain <http://rdaregistry.info/Elements/c/C10008> ;
	rdfs:isDefinedBy <http://rdaregistry.info/Elements/a/> ;
	rdfs:label "has date associated with the family"@en ;
	rdfs:subPropertyOf <http://rdaregistry.info/Elements/u/P60324> ;
	owl:sameAs <http://rdaregistry.info/Elements/a/dateAssociatedWithTheFamily> ;
	skos:definition "Relates a family to a significant date associated with a family."@en .

<http://rdaregistry.info/Elements/a/P50059> reg:name "hereditaryTitle"@en ;
	reg:status status:1001 ;
	a rdf:Property ;
	rdfs:domain <http://rdaregistry.info/Elements/c/C10008> ;
	rdfs:isDefinedBy <http://rdaregistry.info/Elements/a/> ;
	rdfs:label "has hereditary title"@en ;
	rdfs:subPropertyOf <http://rdaregistry.info/Elements/u/P60356> ;
	owl:sameAs <http://rdaregistry.info/Elements/a/hereditaryTitle> ;
	skos:definition "Relates a family to a title of nobility, etc., associated with a family."@en .

<http://rdaregistry.info/Elements/a/P50060> reg:name "prominentMemberOfTheFamily"@en ;
	reg:status status:1001 ;
	a rdf:Property ;
	rdfs:domain <http://rdaregistry.info/Elements/c/C10008> ;
	rdfs:isDefinedBy <http://rdaregistry.info/Elements/a/> ;
	rdfs:label "has prominent member of the family"@en ;
	rdfs:subPropertyOf <http://rdaregistry.info/Elements/u/P60362> ;
	owl:sameAs <http://rdaregistry.info/Elements/a/prominentMemberOfTheFamily> ;
	skos:definition "Relates a family to a well-known individual who is a member of a family."@en .

<http://rdaregistry.info/Elements/a/P50061> reg:hasSubproperty <http://rdaregistry.info/Elements/a/P50054> , <http://rdaregistry.info/Elements/a/P50065> ;
	reg:name "nameOfTheFamily"@en ;
	reg:status status:1001 ;
	a rdf:Property ;
	rdfs:domain <http://rdaregistry.info/Elements/c/C10008> ;
	rdfs:isDefinedBy <http://rdaregistry.info/Elements/a/> ;
	rdfs:label "has name of the family"@en ;
	rdfs:subPropertyOf <http://rdaregistry.info/Elements/u/P60368> ;
	owl:sameAs <http://rdaregistry.info/Elements/a/nameOfTheFamily> ;
	skos:definition "Relates a family to a word, character, or group of words and/or characters by which a family is known."@en .

<http://rdaregistry.info/Elements/a/P50062> reg:name "foundedCorporateBodyOfFamily"@en ;
	reg:status status:1001 ;
	a rdf:Property ;
	rdfs:domain <http://rdaregistry.info/Elements/c/C10008> ;
	rdfs:isDefinedBy <http://rdaregistry.info/Elements/a/> ;
	rdfs:label "has founded corporate body of family"@en ;
	rdfs:range <http://rdaregistry.info/Elements/c/C10005> ;
	rdfs:subPropertyOf <http://rdaregistry.info/Elements/u/P60687> ;
	owl:inverseOf <http://rdaregistry.info/Elements/a/P50020> ;
	owl:sameAs <http://rdaregistry.info/Elements/a/foundedCorporateBodyOfFamily> ;
	skos:definition "Relates a family to an organization that the family founded."@en .

<http://rdaregistry.info/Elements/a/P50063> reg:name "sponsoredCorporateBodyOfFamily"@en ;
	reg:status status:1001 ;
	a rdf:Property ;
	rdfs:domain <http://rdaregistry.info/Elements/c/C10008> ;
	rdfs:isDefinedBy <http://rdaregistry.info/Elements/a/> ;
	rdfs:label "has sponsored corporate body of family"@en ;
	rdfs:range <http://rdaregistry.info/Elements/c/C10005> ;
	rdfs:subPropertyOf <http://rdaregistry.info/Elements/u/P60688> ;
	owl:inverseOf <http://rdaregistry.info/Elements/a/P50021> ;
	owl:sameAs <http://rdaregistry.info/Elements/a/sponsoredCorporateBodyOfFamily> ;
	skos:definition "Relates a family to an organization that the family sponsors."@en .

<http://rdaregistry.info/Elements/a/P50064> reg:name "familyHistory"@en ;
	reg:status status:1001 ;
	a rdf:Property ;
	rdfs:domain <http://rdaregistry.info/Elements/c/C10008> ;
	rdfs:isDefinedBy <http://rdaregistry.info/Elements/a/> ;
	rdfs:label "has family history"@en ;
	rdfs:subPropertyOf <http://rdaregistry.info/Elements/u/P60484> ;
	owl:sameAs <http://rdaregistry.info/Elements/a/familyHistory> ;
	skos:definition "Relates a family to biographical information about the family and its members."@en .

<http://rdaregistry.info/Elements/a/P50065> reg:name "preferredNameForTheFamily"@en ;
	reg:status status:1001 ;
	a rdf:Property ;
	rdfs:domain <http://rdaregistry.info/Elements/c/C10008> ;
	rdfs:isDefinedBy <http://rdaregistry.info/Elements/a/> ;
	rdfs:label "has preferred name for the family"@en ;
	rdfs:subPropertyOf <http://rdaregistry.info/Elements/a/P50061> , <http://rdaregistry.info/Elements/u/P60549> ;
	owl:sameAs <http://rdaregistry.info/Elements/a/preferredNameForTheFamily> ;
	skos:definition "Relates a family to the name or form of name chosen to identify the family. it is also the basis for the authorized access point representing that family."@en .

<http://rdaregistry.info/Elements/a/P50066> reg:name "donorOf"@en ;
	reg:status status:1001 ;
	a rdf:Property ;
	rdfs:domain <http://rdaregistry.info/Elements/c/C10002> ;
	rdfs:isDefinedBy <http://rdaregistry.info/Elements/a/> ;
	rdfs:label "is donor of"@en ;
	rdfs:range <http://rdaregistry.info/Elements/c/C10003> ;
	rdfs:subPropertyOf <http://rdaregistry.info/Elements/a/P50163> , <http://rdaregistry.info/Elements/u/P60012> ;
	owl:inverseOf <http://rdaregistry.info/Elements/i/P40007> ;
	owl:sameAs <http://rdaregistry.info/Elements/a/donorOf> ;
	skos:definition "Relates a former owner of an item who donated that item to another owner to the item."@en .

<http://rdaregistry.info/Elements/a/P50067> reg:name "sellerOf"@en ;
	reg:status status:1001 ;
	a rdf:Property ;
	rdfs:domain <http://rdaregistry.info/Elements/c/C10002> ;
	rdfs:isDefinedBy <http://rdaregistry.info/Elements/a/> ;
	rdfs:label "is seller of"@en ;
	rdfs:range <http://rdaregistry.info/Elements/c/C10003> ;
	rdfs:subPropertyOf <http://rdaregistry.info/Elements/a/P50163> , <http://rdaregistry.info/Elements/u/P60013> ;
	owl:inverseOf <http://rdaregistry.info/Elements/i/P40008> ;
	owl:sameAs <http://rdaregistry.info/Elements/a/sellerOf> ;
	skos:definition "Relates a former owner of an item who sold that item to another owner to the item."@en .

<http://rdaregistry.info/Elements/a/P50068> reg:name "enactingJurisdictionOf"@en ;
	reg:status status:1001 ;
	a rdf:Property ;
	rdfs:domain <http://rdaregistry.info/Elements/c/C10005> ;
	rdfs:isDefinedBy <http://rdaregistry.info/Elements/a/> ;
	rdfs:label "is enacting jurisdiction of"@en ;
	rdfs:range <http://rdaregistry.info/Elements/c/C10001> ;
	rdfs:subPropertyOf <http://rdaregistry.info/Elements/a/P50204> , <http://rdaregistry.info/Elements/u/P60014> ;
	owl:inverseOf <http://rdaregistry.info/Elements/w/P10017> ;
	owl:sameAs <http://rdaregistry.info/Elements/a/enactingJurisdictionOf> ;
	skos:definition "Relates a jurisdiction enacting a law, regulation, constitution, court rule, etc. to the work."@en .

<http://rdaregistry.info/Elements/a/P50069> reg:name "jurisdictionGovernedOf"@en ;
	reg:status status:1001 ;
	a rdf:Property ;
	rdfs:domain <http://rdaregistry.info/Elements/c/C10005> ;
	rdfs:isDefinedBy <http://rdaregistry.info/Elements/a/> ;
	rdfs:label "is jurisdiction governed of"@en ;
	rdfs:range <http://rdaregistry.info/Elements/c/C10001> ;
	rdfs:subPropertyOf <http://rdaregistry.info/Elements/a/P50131> , <http://rdaregistry.info/Elements/u/P60015> ;
	owl:inverseOf <http://rdaregistry.info/Elements/w/P10018> ;
	owl:sameAs <http://rdaregistry.info/Elements/a/jurisdictionGovernedOf> ;
	skos:definition "Relates a jurisdiction governed by a law, regulation, etc., that was enacted by another jurisdiction to the work."@en .

<http://rdaregistry.info/Elements/a/P50070> reg:name "conductorOf"@en ;
	reg:status status:1001 ;
	a rdf:Property ;
	rdfs:domain <http://rdaregistry.info/Elements/c/C10002> ;
	rdfs:isDefinedBy <http://rdaregistry.info/Elements/a/> ;
	rdfs:label "is conductor of"@en ;
	rdfs:range <http://rdaregistry.info/Elements/c/C10006> ;
	rdfs:subPropertyOf <http://rdaregistry.info/Elements/a/P50147> , <http://rdaregistry.info/Elements/u/P60016> ;
	owl:inverseOf <http://rdaregistry.info/Elements/e/P20011> ;
	owl:sameAs <http://rdaregistry.info/Elements/a/conductorOf> ;
	skos:definition "Relates a performer contributing to an expression of a musical work by leading a performing group (orchestra, chorus, opera, etc.) in a musical or dramatic presentation, etc. to the expression."@en .

<http://rdaregistry.info/Elements/a/P50071> reg:hasSubproperty <http://rdaregistry.info/Elements/a/P50217> ;
	reg:name "actorOf"@en ;
	reg:status status:1001 ;
	a rdf:Property ;
	rdfs:domain <http://rdaregistry.info/Elements/c/C10002> ;
	rdfs:isDefinedBy <http://rdaregistry.info/Elements/a/> ;
	rdfs:label "is actor of"@en ;
	rdfs:range <http://rdaregistry.info/Elements/c/C10006> ;
	rdfs:subPropertyOf <http://rdaregistry.info/Elements/a/P50147> , <http://rdaregistry.info/Elements/u/P60017> ;
	owl:inverseOf <http://rdaregistry.info/Elements/e/P20012> ;
	owl:sameAs <http://rdaregistry.info/Elements/a/actorOf> ;
	skos:definition "Relates a performer contributing to an expression of a work by acting as a cast member or player in a musical or dramatic presentation, etc to the expression."@en .

<http://rdaregistry.info/Elements/a/P50072> reg:name "onScreenPresenterOf"@en ;
	reg:status status:1001 ;
	a rdf:Property ;
	rdfs:domain <http://rdaregistry.info/Elements/c/C10002> ;
	rdfs:isDefinedBy <http://rdaregistry.info/Elements/a/> ;
	rdfs:label "is on-screen presenter of"@en ;
	rdfs:range <http://rdaregistry.info/Elements/c/C10006> ;
	rdfs:subPropertyOf <http://rdaregistry.info/Elements/a/P50147> , <http://rdaregistry.info/Elements/u/P60018> ;
	owl:inverseOf <http://rdaregistry.info/Elements/e/P20013> ;
	owl:sameAs <http://rdaregistry.info/Elements/a/onScreenPresenterOf> ;
	skos:definition "Relates a performer contributing to an expression of a work by appearing on screen to provide contextual or background information to the expression."@en ;
	skos:scopeNote "An on-screen presenter may appear in nonfiction moving image materials or in introductions to fiction moving image materials."@en .

<http://rdaregistry.info/Elements/a/P50073> reg:name "dancerOf"@en ;
	reg:status status:1001 ;
	a rdf:Property ;
	rdfs:domain <http://rdaregistry.info/Elements/c/C10002> ;
	rdfs:isDefinedBy <http://rdaregistry.info/Elements/a/> ;
	rdfs:label "is dancer of"@en ;
	rdfs:range <http://rdaregistry.info/Elements/c/C10006> ;
	rdfs:subPropertyOf <http://rdaregistry.info/Elements/a/P50147> , <http://rdaregistry.info/Elements/u/P60019> ;
	owl:inverseOf <http://rdaregistry.info/Elements/e/P20014> ;
	owl:sameAs <http://rdaregistry.info/Elements/a/dancerOf> ;
	skos:definition "Relates a performer contributing to an expression of a work by dancing in a musical, dramatic, etc., presentation to the expression."@en .

<http://rdaregistry.info/Elements/a/P50074> reg:name "teacherOf"@en ;
	reg:status status:1001 ;
	a rdf:Property ;
	rdfs:domain <http://rdaregistry.info/Elements/c/C10002> ;
	rdfs:isDefinedBy <http://rdaregistry.info/Elements/a/> ;
	rdfs:label "is teacher of"@en ;
	rdfs:range <http://rdaregistry.info/Elements/c/C10006> ;
	rdfs:subPropertyOf <http://rdaregistry.info/Elements/a/P50147> , <http://rdaregistry.info/Elements/u/P60020> ;
	owl:inverseOf <http://rdaregistry.info/Elements/e/P20015> ;
	owl:sameAs <http://rdaregistry.info/Elements/a/teacherOf> ;
	skos:definition "Relates a performer contributing to an expression of a work by giving instruction or providing a demonstration to the expression."@en .

<http://rdaregistry.info/Elements/a/P50075> reg:name "hostOf"@en ;
	reg:status status:1001 ;
	a rdf:Property ;
	rdfs:domain <http://rdaregistry.info/Elements/c/C10002> ;
	rdfs:isDefinedBy <http://rdaregistry.info/Elements/a/> ;
	rdfs:label "is host of"@en ;
	rdfs:range <http://rdaregistry.info/Elements/c/C10006> ;
	rdfs:subPropertyOf <http://rdaregistry.info/Elements/a/P50147> , <http://rdaregistry.info/Elements/u/P60021> ;
	owl:inverseOf <http://rdaregistry.info/Elements/e/P20016> ;
	owl:sameAs <http://rdaregistry.info/Elements/a/hostOf> ;
	skos:definition "Relates a performer contributing to an expression of a work by leading a program (often broadcast) that includes other guests, performers, etc. (e.g., talk show host) to the expression."@en .

<http://rdaregistry.info/Elements/a/P50076> reg:name "moderatorOf"@en ;
	reg:status status:1001 ;
	a rdf:Property ;
	rdfs:domain <http://rdaregistry.info/Elements/c/C10002> ;
	rdfs:isDefinedBy <http://rdaregistry.info/Elements/a/> ;
	rdfs:label "is moderator of"@en ;
	rdfs:range <http://rdaregistry.info/Elements/c/C10006> ;
	rdfs:subPropertyOf <http://rdaregistry.info/Elements/a/P50147> , <http://rdaregistry.info/Elements/u/P60022> ;
	owl:inverseOf <http://rdaregistry.info/Elements/e/P20017> ;
	owl:sameAs <http://rdaregistry.info/Elements/a/moderatorOf> ;
	skos:definition "Relates a performer contributing to an expression of a work by leading a program (often broadcast) where topics are discussed, usually with participation of experts in fields related to the discussion to the expression."@en .

<http://rdaregistry.info/Elements/a/P50077> reg:name "puppeteerOf"@en ;
	reg:status status:1001 ;
	a rdf:Property ;
	rdfs:domain <http://rdaregistry.info/Elements/c/C10002> ;
	rdfs:isDefinedBy <http://rdaregistry.info/Elements/a/> ;
	rdfs:label "is puppeteer of"@en ;
	rdfs:range <http://rdaregistry.info/Elements/c/C10006> ;
	rdfs:subPropertyOf <http://rdaregistry.info/Elements/a/P50147> , <http://rdaregistry.info/Elements/u/P60023> ;
	owl:inverseOf <http://rdaregistry.info/Elements/e/P20018> ;
	owl:sameAs <http://rdaregistry.info/Elements/a/puppeteerOf> ;
	skos:definition "Relates a performer contributing to an expression of a work by manipulating, controlling, or directing puppets or marionettes in a moving image production or a musical or dramatic presentation or entertainment to the expression."@en .

<http://rdaregistry.info/Elements/a/P50078> reg:name "panelistOf"@en ;
	reg:status status:1001 ;
	a rdf:Property ;
	rdfs:domain <http://rdaregistry.info/Elements/c/C10002> ;
	rdfs:isDefinedBy <http://rdaregistry.info/Elements/a/> ;
	rdfs:label "is panelist of"@en ;
	rdfs:range <http://rdaregistry.info/Elements/c/C10006> ;
	rdfs:subPropertyOf <http://rdaregistry.info/Elements/a/P50147> , <http://rdaregistry.info/Elements/u/P60024> ;
	owl:inverseOf <http://rdaregistry.info/Elements/e/P20019> ;
	owl:sameAs <http://rdaregistry.info/Elements/a/panelistOf> ;
	skos:definition "Relates a performer contributing to an expression of a work by participating in a program (often broadcast) where topics are discussed, usually with participation of experts in fields related to the discussion to the expression."@en .

<http://rdaregistry.info/Elements/a/P50079> reg:name "instrumentalistOf"@en ;
	reg:status status:1001 ;
	a rdf:Property ;
	rdfs:domain <http://rdaregistry.info/Elements/c/C10002> ;
	rdfs:isDefinedBy <http://rdaregistry.info/Elements/a/> ;
	rdfs:label "is instrumentalist of"@en ;
	rdfs:range <http://rdaregistry.info/Elements/c/C10006> ;
	rdfs:subPropertyOf <http://rdaregistry.info/Elements/a/P50147> , <http://rdaregistry.info/Elements/u/P60025> ;
	owl:inverseOf <http://rdaregistry.info/Elements/e/P20020> ;
	owl:sameAs <http://rdaregistry.info/Elements/a/instrumentalistOf> ;
	skos:definition "Relates a performer contributing to an expression of a work by playing a musical instrument to the expression."@en .

<http://rdaregistry.info/Elements/a/P50080> reg:name "commentatorOf"@en ;
	reg:status status:1001 ;
	a rdf:Property ;
	rdfs:domain <http://rdaregistry.info/Elements/c/C10002> ;
	rdfs:isDefinedBy <http://rdaregistry.info/Elements/a/> ;
	rdfs:label "is commentator of"@en ;
	rdfs:range <http://rdaregistry.info/Elements/c/C10006> ;
	rdfs:subPropertyOf <http://rdaregistry.info/Elements/a/P50147> , <http://rdaregistry.info/Elements/u/P60026> ;
	owl:inverseOf <http://rdaregistry.info/Elements/e/P20021> ;
	owl:sameAs <http://rdaregistry.info/Elements/a/commentatorOf> ;
	skos:definition "Relates a performer contributing to an expression of a work by providing interpretation, analysis, or a discussion of the subject matter on a recording, film, or other audiovisual medium to the expression."@en .

<http://rdaregistry.info/Elements/a/P50081> reg:name "narratorOf"@en ;
	reg:status status:1001 ;
	a rdf:Property ;
	rdfs:domain <http://rdaregistry.info/Elements/c/C10002> ;
	rdfs:isDefinedBy <http://rdaregistry.info/Elements/a/> ;
	rdfs:label "is narrator of"@en ;
	rdfs:range <http://rdaregistry.info/Elements/c/C10006> ;
	rdfs:subPropertyOf <http://rdaregistry.info/Elements/a/P50147> , <http://rdaregistry.info/Elements/u/P60028> ;
	owl:inverseOf <http://rdaregistry.info/Elements/e/P20022> ;
	owl:sameAs <http://rdaregistry.info/Elements/a/narratorOf> ;
	skos:definition "Relates a performer contributing to an expression of a work by reading or speaking in order to give an account of an act, occurrence, course of events, etc to the expression."@en .

<http://rdaregistry.info/Elements/a/P50082> reg:name "storytellerOf"@en ;
	reg:status status:1001 ;
	a rdf:Property ;
	rdfs:domain <http://rdaregistry.info/Elements/c/C10002> ;
	rdfs:isDefinedBy <http://rdaregistry.info/Elements/a/> ;
	rdfs:label "is storyteller of"@en ;
	rdfs:range <http://rdaregistry.info/Elements/c/C10006> ;
	rdfs:subPropertyOf <http://rdaregistry.info/Elements/a/P50147> , <http://rdaregistry.info/Elements/u/P60029> ;
	owl:inverseOf <http://rdaregistry.info/Elements/e/P20023> ;
	owl:sameAs <http://rdaregistry.info/Elements/a/storytellerOf> ;
	skos:definition "Relates a performer contributing to an expression of a work by relaying a creator’s original story with dramatic or theatrical interpretation to the expression."@en .

<http://rdaregistry.info/Elements/a/P50083> reg:name "speakerOf"@en ;
	reg:status status:1001 ;
	a rdf:Property ;
	rdfs:domain <http://rdaregistry.info/Elements/c/C10002> ;
	rdfs:isDefinedBy <http://rdaregistry.info/Elements/a/> ;
	rdfs:label "is speaker of"@en ;
	rdfs:range <http://rdaregistry.info/Elements/c/C10006> ;
	rdfs:subPropertyOf <http://rdaregistry.info/Elements/a/P50147> , <http://rdaregistry.info/Elements/u/P60030> ;
	owl:inverseOf <http://rdaregistry.info/Elements/e/P20024> ;
	owl:sameAs <http://rdaregistry.info/Elements/a/speakerOf> ;
	skos:definition "Relates a performer contributing to an expression of a work by speaking words, such as a lecture, speech, etc to the expression."@en .

<http://rdaregistry.info/Elements/a/P50084> reg:name "singerOf"@en ;
	reg:status status:1001 ;
	a rdf:Property ;
	rdfs:domain <http://rdaregistry.info/Elements/c/C10002> ;
	rdfs:isDefinedBy <http://rdaregistry.info/Elements/a/> ;
	rdfs:label "is singer of"@en ;
	rdfs:range <http://rdaregistry.info/Elements/c/C10006> ;
	rdfs:subPropertyOf <http://rdaregistry.info/Elements/a/P50147> , <http://rdaregistry.info/Elements/u/P60031> ;
	owl:inverseOf <http://rdaregistry.info/Elements/e/P20025> ;
	owl:sameAs <http://rdaregistry.info/Elements/a/singerOf> ;
	skos:definition "Relates a performer contributing to an expression of a work by using his/her/their voice, with or without instrumental accompaniment, to produce music to the expression."@en ;
	skos:scopeNote "A singer’s performance may or may not include actual words."@en .

<http://rdaregistry.info/Elements/a/P50085> reg:name "appelleePersonOf"@en ;
	reg:status status:1001 ;
	a rdf:Property ;
	rdfs:domain <http://rdaregistry.info/Elements/c/C10004> ;
	rdfs:isDefinedBy <http://rdaregistry.info/Elements/a/> ;
	rdfs:label "is appellee person of"@en ;
	rdfs:range <http://rdaregistry.info/Elements/c/C10001> ;
	rdfs:subPropertyOf <http://rdaregistry.info/Elements/a/P50087> , <http://rdaregistry.info/Elements/u/P60601> ;
	owl:inverseOf <http://rdaregistry.info/Elements/w/P10035> ;
	owl:sameAs <http://rdaregistry.info/Elements/a/appelleePersonOf> ;
	skos:definition "Relates a person against whom an appeal is taken to the work."@en .

<http://rdaregistry.info/Elements/a/P50086> reg:name "mediumOf"@en ;
	reg:status status:1001 ;
	a rdf:Property ;
	rdfs:domain <http://rdaregistry.info/Elements/c/C10004> ;
	rdfs:isDefinedBy <http://rdaregistry.info/Elements/a/> ;
	rdfs:label "is medium of"@en ;
	rdfs:range <http://rdaregistry.info/Elements/c/C10001> ;
	rdfs:subPropertyOf <http://rdaregistry.info/Elements/a/P50131> , <http://rdaregistry.info/Elements/u/P60032> ;
	owl:inverseOf <http://rdaregistry.info/Elements/w/P10036> ;
	owl:sameAs <http://rdaregistry.info/Elements/a/mediumOf> ;
	skos:definition "Relates a person held to be a channel of communication between the earthly world and a world of spirits to the work."@en .

<http://rdaregistry.info/Elements/a/P50087> reg:hasSubproperty <http://rdaregistry.info/Elements/a/P50085> ;
	reg:name "appelleeOf"@en ;
	reg:status status:1001 ;
	a rdf:Property ;
	rdfs:isDefinedBy <http://rdaregistry.info/Elements/a/> ;
	rdfs:label "is appellee of"@en ;
	rdfs:range <http://rdaregistry.info/Elements/c/C10001> ;
	rdfs:subPropertyOf <http://rdaregistry.info/Elements/a/P50131> , <http://rdaregistry.info/Elements/u/P60601> ;
	owl:inverseOf <http://rdaregistry.info/Elements/w/P10037> ;
	owl:sameAs <http://rdaregistry.info/Elements/a/appelleeOf> ;
	skos:definition "Relates a person or corporate body against whom an appeal is taken to the work."@en .

<http://rdaregistry.info/Elements/a/P50088> reg:hasSubproperty <http://rdaregistry.info/Elements/a/P50042> ;
	reg:name "appellantOf"@en ;
	reg:status status:1001 ;
	a rdf:Property ;
	rdfs:isDefinedBy <http://rdaregistry.info/Elements/a/> ;
	rdfs:label "is appellant of"@en ;
	rdfs:range <http://rdaregistry.info/Elements/c/C10001> ;
	rdfs:subPropertyOf <http://rdaregistry.info/Elements/a/P50131> , <http://rdaregistry.info/Elements/u/P60691> ;
	owl:inverseOf <http://rdaregistry.info/Elements/w/P10038> ;
	owl:sameAs <http://rdaregistry.info/Elements/a/appellantOf> ;
	skos:definition "Relates a person or corporate body who appeals a lower court's decision to the work."@en .

<http://rdaregistry.info/Elements/a/P50089> reg:hasSubproperty <http://rdaregistry.info/Elements/a/P50043> , <http://rdaregistry.info/Elements/a/P50124> ;
	reg:name "plaintiffOf"@en ;
	reg:status status:1001 ;
	a rdf:Property ;
	rdfs:isDefinedBy <http://rdaregistry.info/Elements/a/> ;
	rdfs:label "is plaintiff of"@en ;
	rdfs:range <http://rdaregistry.info/Elements/c/C10001> ;
	rdfs:subPropertyOf <http://rdaregistry.info/Elements/a/P50131> , <http://rdaregistry.info/Elements/u/P60693> ;
	owl:inverseOf <http://rdaregistry.info/Elements/w/P10039> ;
	owl:sameAs <http://rdaregistry.info/Elements/a/plaintiffOf> ;
	skos:definition "Relates a person or corporate body who brings a suit in a civil proceeding to the work."@en .

<http://rdaregistry.info/Elements/a/P50090> reg:name "defendantOf"@en ;
	reg:status status:1001 ;
	a rdf:Property ;
	rdfs:domain <http://rdaregistry.info/Elements/c/C10002> ;
	rdfs:isDefinedBy <http://rdaregistry.info/Elements/a/> ;
	rdfs:label "is defendant of"@en ;
	rdfs:range <http://rdaregistry.info/Elements/c/C10001> ;
	rdfs:subPropertyOf <http://rdaregistry.info/Elements/a/P50131> , <http://rdaregistry.info/Elements/u/P60698> ;
	owl:inverseOf <http://rdaregistry.info/Elements/w/P10040> ;
	owl:sameAs <http://rdaregistry.info/Elements/a/defendantOf> ;
	skos:definition "Relates a person or corporate body who is accused in a criminal proceeding or sued in a civil proceeding to the work."@en .

<http://rdaregistry.info/Elements/a/P50091> reg:name "degreeSupervisorOf"@en ;
	reg:status status:1001 ;
	a rdf:Property ;
	rdfs:domain <http://rdaregistry.info/Elements/c/C10004> ;
	rdfs:isDefinedBy <http://rdaregistry.info/Elements/a/> ;
	rdfs:label "is degree supervisor of"@en ;
	rdfs:range <http://rdaregistry.info/Elements/c/C10001> ;
	rdfs:subPropertyOf <http://rdaregistry.info/Elements/a/P50131> , <http://rdaregistry.info/Elements/u/P60649> ;
	owl:inverseOf <http://rdaregistry.info/Elements/w/P10041> ;
	owl:sameAs <http://rdaregistry.info/Elements/a/degreeSupervisorOf> ;
	skos:definition "Relates a person overseeing a higher-level academic degree to the work."@en .

<http://rdaregistry.info/Elements/a/P50092> reg:name "illuminatorOf"@en ;
	reg:status status:1001 ;
	a rdf:Property ;
	rdfs:domain <http://rdaregistry.info/Elements/c/C10004> ;
	rdfs:isDefinedBy <http://rdaregistry.info/Elements/a/> ;
	rdfs:label "is illuminator of"@en ;
	rdfs:range <http://rdaregistry.info/Elements/c/C10003> ;
	rdfs:subPropertyOf <http://rdaregistry.info/Elements/a/P50182> , <http://rdaregistry.info/Elements/u/P60650> ;
	owl:inverseOf <http://rdaregistry.info/Elements/i/P40012> ;
	owl:sameAs <http://rdaregistry.info/Elements/a/illuminatorOf> ;
	skos:definition "Relates a person providing decoration to a specific item using precious metals or color, often with elaborate designs and motifs to the item."@en .

<http://rdaregistry.info/Elements/a/P50093> reg:name "undifferentiatedNameIndicator"@en ;
	reg:status status:1001 ;
	a rdf:Property ;
	rdfs:domain <http://rdaregistry.info/Elements/c/C10004> ;
	rdfs:isDefinedBy <http://rdaregistry.info/Elements/a/> ;
	rdfs:label "has undifferentiated name indicator"@en ;
	rdfs:subPropertyOf <http://rdaregistry.info/Elements/u/P60046> ;
	owl:sameAs <http://rdaregistry.info/Elements/a/undifferentiatedNameIndicator> ;
	skos:definition "Relates a person to a categorization indicating that the core elements recorded are insufficient to differentiate between two or more persons with the same name."@en .

<http://rdaregistry.info/Elements/a/P50094> reg:name "identifierForThePerson"@en ;
	reg:status status:1001 ;
	a rdf:Property ;
	rdfs:domain <http://rdaregistry.info/Elements/c/C10004> ;
	rdfs:isDefinedBy <http://rdaregistry.info/Elements/a/> ;
	rdfs:label "has identifier for the person"@en ;
	rdfs:subPropertyOf <http://rdaregistry.info/Elements/u/P60053> ;
	owl:sameAs <http://rdaregistry.info/Elements/a/identifierForThePerson> ;
	skos:definition "Relates a person to a character string uniquely associated with a person, or with a surrogate for a person (e.g., an authority record)."@en ;
	skos:scopeNote "The identifier serves to differentiate that person from other persons."@en .

<http://rdaregistry.info/Elements/a/P50095> reg:name "groupMemberOf"@en ;
	reg:status status:1001 ;
	a rdf:Property ;
	rdfs:domain <http://rdaregistry.info/Elements/c/C10004> ;
	rdfs:isDefinedBy <http://rdaregistry.info/Elements/a/> ;
	rdfs:label "has group member of"@en ;
	rdfs:range <http://rdaregistry.info/Elements/c/C10005> ;
	rdfs:subPropertyOf <http://rdaregistry.info/Elements/u/P60648> ;
	owl:inverseOf <http://rdaregistry.info/Elements/a/P50030> ;
	owl:sameAs <http://rdaregistry.info/Elements/a/groupMemberOf> ;
	skos:definition "Relates a person to a corporate body (performing group, expedition, etc.) of which the person is a member."@en .

<http://rdaregistry.info/Elements/a/P50096> reg:name "employer"@en ;
	reg:status status:1001 ;
	a rdf:Property ;
	rdfs:domain <http://rdaregistry.info/Elements/c/C10004> ;
	rdfs:isDefinedBy <http://rdaregistry.info/Elements/a/> ;
	rdfs:label "has employer"@en ;
	rdfs:range <http://rdaregistry.info/Elements/c/C10005> ;
	rdfs:subPropertyOf <http://rdaregistry.info/Elements/u/P60679> ;
	owl:inverseOf <http://rdaregistry.info/Elements/a/P50026> ;
	owl:sameAs <http://rdaregistry.info/Elements/a/employer> ;
	skos:definition "Relates a person to a corporate body that employs the person."@en .

<http://rdaregistry.info/Elements/a/P50097> reg:name "countryAssociatedWithThePerson"@en ;
	reg:status status:1001 ;
	a rdf:Property ;
	rdfs:domain <http://rdaregistry.info/Elements/c/C10004> ;
	rdfs:isDefinedBy <http://rdaregistry.info/Elements/a/> ;
	rdfs:label "has country associated with the person"@en ;
	rdfs:subPropertyOf <http://rdaregistry.info/Elements/u/P60063> ;
	owl:sameAs <http://rdaregistry.info/Elements/a/countryAssociatedWithThePerson> ;
	skos:definition "Relates a person to a country with which a person is identified."@en .

<http://rdaregistry.info/Elements/a/P50098> reg:name "periodOfActivityOfThePerson"@en ;
	reg:status status:1001 ;
	a rdf:Property ;
	rdfs:domain <http://rdaregistry.info/Elements/c/C10004> ;
	rdfs:isDefinedBy <http://rdaregistry.info/Elements/a/> ;
	rdfs:label "has period of activity of the person"@en ;
	rdfs:subPropertyOf <http://rdaregistry.info/Elements/a/P50107> , <http://rdaregistry.info/Elements/u/P60076> ;
	owl:sameAs <http://rdaregistry.info/Elements/a/periodOfActivityOfThePerson> ;
	skos:definition "Relates a person to a date or range of dates indicative of the period in which a person was active in his or her primary field of endeavour."@en .

<http://rdaregistry.info/Elements/a/P50099> reg:name "descendants"@en ;
	reg:status status:1001 ;
	a rdf:Property ;
	rdfs:domain <http://rdaregistry.info/Elements/c/C10004> ;
	rdfs:isDefinedBy <http://rdaregistry.info/Elements/a/> ;
	rdfs:label "has descendants"@en ;
	rdfs:range <http://rdaregistry.info/Elements/c/C10008> ;
	rdfs:subPropertyOf <http://rdaregistry.info/Elements/u/P60686> ;
	owl:inverseOf <http://rdaregistry.info/Elements/a/P50055> ;
	owl:sameAs <http://rdaregistry.info/Elements/a/descendants> ;
	skos:definition "Relates a person to a family descended from the particular person."@en .

<http://rdaregistry.info/Elements/a/P50100> reg:name "fieldOfActivityOfThePerson"@en ;
	reg:status status:1001 ;
	a rdf:Property ;
	rdfs:domain <http://rdaregistry.info/Elements/c/C10004> ;
	rdfs:isDefinedBy <http://rdaregistry.info/Elements/a/> ;
	rdfs:label "has field of activity of the person"@en ;
	rdfs:subPropertyOf <http://rdaregistry.info/Elements/u/P60089> ;
	owl:sameAs <http://rdaregistry.info/Elements/a/fieldOfActivityOfThePerson> ;
	skos:definition "Relates a person to a field of endeavour, area of expertise, etc., in which a person is engaged or was engaged."@en .

<http://rdaregistry.info/Elements/a/P50101> reg:name "affiliation"@en ;
	reg:status status:1001 ;
	a rdf:Property ;
	rdfs:domain <http://rdaregistry.info/Elements/c/C10004> ;
	rdfs:isDefinedBy <http://rdaregistry.info/Elements/a/> ;
	rdfs:label "has affiliation"@en ;
	rdfs:subPropertyOf <http://rdaregistry.info/Elements/u/P60095> ;
	owl:sameAs <http://rdaregistry.info/Elements/a/affiliation> ;
	skos:definition "Relates a person to a group with which a person is affiliated or has been affiliated through employment, membership, cultural identity, etc."@en .

<http://rdaregistry.info/Elements/a/P50102> reg:name "languageOfThePerson"@en ;
	reg:status status:1001 ;
	a rdf:Property ;
	rdfs:domain <http://rdaregistry.info/Elements/c/C10004> ;
	rdfs:isDefinedBy <http://rdaregistry.info/Elements/a/> ;
	rdfs:label "has language of the person"@en ;
	rdfs:subPropertyOf <http://rdaregistry.info/Elements/u/P60098> ;
	owl:sameAs <http://rdaregistry.info/Elements/a/languageOfThePerson> ;
	skos:definition "Relates a person to a language a person uses when writing for publication, broadcasting, etc."@en .

<http://rdaregistry.info/Elements/a/P50103> reg:name "variantNameForThePerson"@en ;
	reg:status status:1001 ;
	a rdf:Property ;
	rdfs:domain <http://rdaregistry.info/Elements/c/C10004> ;
	rdfs:isDefinedBy <http://rdaregistry.info/Elements/a/> ;
	rdfs:label "has variant name for the person"@en ;
	rdfs:subPropertyOf <http://rdaregistry.info/Elements/a/P50111> , <http://rdaregistry.info/Elements/u/P60119> ;
	owl:sameAs <http://rdaregistry.info/Elements/a/variantNameForThePerson> ;
	skos:definition "Relates a person to a name or form of name by which a person is known that differs from the name or form of name chosen as the preferred name."@en .

<http://rdaregistry.info/Elements/a/P50104> reg:name "professionOrOccupation"@en ;
	reg:status status:1001 ;
	a rdf:Property ;
	rdfs:domain <http://rdaregistry.info/Elements/c/C10004> ;
	rdfs:isDefinedBy <http://rdaregistry.info/Elements/a/> ;
	rdfs:label "has profession or occupation"@en ;
	rdfs:subPropertyOf <http://rdaregistry.info/Elements/u/P60468> ;
	owl:sameAs <http://rdaregistry.info/Elements/a/professionOrOccupation> ;
	skos:definition "Relates a person to a person’s vocation or avocation."@en .

<http://rdaregistry.info/Elements/a/P50105> reg:name "alternateIdentity"@en ;
	reg:status status:1001 ;
	a rdf:Property ;
	rdfs:domain <http://rdaregistry.info/Elements/c/C10004> ;
	rdfs:isDefinedBy <http://rdaregistry.info/Elements/a/> ;
	rdfs:label "has alternate identity"@en ;
	rdfs:range <http://rdaregistry.info/Elements/c/C10004> ;
	rdfs:subPropertyOf <http://rdaregistry.info/Elements/u/P60036> ;
	owl:inverseOf <http://rdaregistry.info/Elements/a/P50106> ;
	owl:sameAs <http://rdaregistry.info/Elements/a/alternateIdentity> ;
	skos:definition "Relates a person to a pseudonymous or other identity assumed by the person."@en .

<http://rdaregistry.info/Elements/a/P50106> reg:name "realIdentity"@en ;
	reg:status status:1001 ;
	a rdf:Property ;
	rdfs:domain <http://rdaregistry.info/Elements/c/C10004> ;
	rdfs:isDefinedBy <http://rdaregistry.info/Elements/a/> ;
	rdfs:label "has real identity"@en ;
	rdfs:range <http://rdaregistry.info/Elements/c/C10004> ;
	rdfs:subPropertyOf <http://rdaregistry.info/Elements/u/P60037> ;
	owl:inverseOf <http://rdaregistry.info/Elements/a/P50105> ;
	owl:sameAs <http://rdaregistry.info/Elements/a/realIdentity> ;
	skos:definition "Relates a person to a real person who assumes the alternate identity."@en .

<http://rdaregistry.info/Elements/a/P50107> reg:hasSubproperty <http://rdaregistry.info/Elements/a/P50098> , <http://rdaregistry.info/Elements/a/P50120> , <http://rdaregistry.info/Elements/a/P50121> ;
	reg:name "dateAssociatedWithThePerson"@en ;
	reg:status status:1001 ;
	a rdf:Property ;
	rdfs:domain <http://rdaregistry.info/Elements/c/C10004> ;
	rdfs:isDefinedBy <http://rdaregistry.info/Elements/a/> ;
	rdfs:label "has date associated with the person"@en ;
	rdfs:subPropertyOf <http://rdaregistry.info/Elements/u/P60324> ;
	owl:sameAs <http://rdaregistry.info/Elements/a/dateAssociatedWithThePerson> ;
	skos:definition "Relates a person to a significant date associated with a person (e.g., date of birth, date of death)."@en .

<http://rdaregistry.info/Elements/a/P50108> reg:name "otherDesignationAssociatedWithThePerson"@en ;
	reg:status status:1001 ;
	a rdf:Property ;
	rdfs:domain <http://rdaregistry.info/Elements/c/C10004> ;
	rdfs:isDefinedBy <http://rdaregistry.info/Elements/a/> ;
	rdfs:label "has other designation associated with the person"@en ;
	rdfs:subPropertyOf <http://rdaregistry.info/Elements/u/P60370> ;
	owl:sameAs <http://rdaregistry.info/Elements/a/otherDesignationAssociatedWithThePerson> ;
	skos:definition "Relates a person to a term other than a title that is associated with a person’s name."@en .

<http://rdaregistry.info/Elements/a/P50109> reg:name "placeOfResidenceEtc"@en ;
	reg:status status:1001 ;
	a rdf:Property ;
	rdfs:domain <http://rdaregistry.info/Elements/c/C10004> ;
	rdfs:isDefinedBy <http://rdaregistry.info/Elements/a/> ;
	rdfs:label "has place of residence, etc."@en ;
	rdfs:subPropertyOf <http://rdaregistry.info/Elements/u/P60360> ;
	owl:sameAs <http://rdaregistry.info/Elements/a/placeOfResidenceEtc> ;
	skos:definition "Relates a person to a town, city, province, state, and/or country in which a person resides or has resided, or another significant place associated with the person other than place of birth, place of death, or residence (e.g., a place where a person has worked or studied)."@en .

<http://rdaregistry.info/Elements/a/P50110> reg:name "titleOfThePerson"@en ;
	reg:status status:1001 ;
	a rdf:Property ;
	rdfs:domain <http://rdaregistry.info/Elements/c/C10004> ;
	rdfs:isDefinedBy <http://rdaregistry.info/Elements/a/> ;
	rdfs:label "has title of the person"@en ;
	rdfs:subPropertyOf <http://rdaregistry.info/Elements/u/P60363> ;
	owl:sameAs <http://rdaregistry.info/Elements/a/titleOfThePerson> ;
	skos:definition "Relates a person to a word or phrase indicative of royalty, nobility, or ecclesiastical rank or office, a term of address for a person of religious vocation, or another term indicative of rank, honour, or office."@en .

<http://rdaregistry.info/Elements/a/P50111> reg:hasSubproperty <http://rdaregistry.info/Elements/a/P50103> , <http://rdaregistry.info/Elements/a/P50117> ;
	reg:name "nameOfThePerson"@en ;
	reg:status status:1001 ;
	a rdf:Property ;
	rdfs:domain <http://rdaregistry.info/Elements/c/C10004> ;
	rdfs:isDefinedBy <http://rdaregistry.info/Elements/a/> ;
	rdfs:label "has name of the person"@en ;
	rdfs:subPropertyOf <http://rdaregistry.info/Elements/u/P60368> ;
	owl:sameAs <http://rdaregistry.info/Elements/a/nameOfThePerson> ;
	skos:definition "Relates a person to a word, character, or group of words and/or characters by which a person is known."@en .

<http://rdaregistry.info/Elements/a/P50112> reg:name "foundedCorporateBodyOfPerson"@en ;
	reg:status status:1001 ;
	a rdf:Property ;
	rdfs:domain <http://rdaregistry.info/Elements/c/C10004> ;
	rdfs:isDefinedBy <http://rdaregistry.info/Elements/a/> ;
	rdfs:label "has founded corporate body of person"@en ;
	rdfs:range <http://rdaregistry.info/Elements/c/C10005> ;
	rdfs:subPropertyOf <http://rdaregistry.info/Elements/u/P60687> ;
	owl:inverseOf <http://rdaregistry.info/Elements/a/P50029> ;
	owl:sameAs <http://rdaregistry.info/Elements/a/foundedCorporateBodyOfPerson> ;
	skos:definition "Relates a person to an organization that the person founded."@en .

<http://rdaregistry.info/Elements/a/P50113> reg:name "biographicalInformation"@en ;
	reg:status status:1001 ;
	a rdf:Property ;
	rdfs:domain <http://rdaregistry.info/Elements/c/C10004> ;
	rdfs:isDefinedBy <http://rdaregistry.info/Elements/a/> ;
	rdfs:label "has biographical information"@en ;
	rdfs:subPropertyOf <http://rdaregistry.info/Elements/u/P60492> ;
	owl:sameAs <http://rdaregistry.info/Elements/a/biographicalInformation> ;
	skos:definition "Relates a person to information about the life or history of a person."@en .

<http://rdaregistry.info/Elements/a/P50114> reg:name "addressOfThePerson"@en ;
	reg:status status:1001 ;
	a rdf:Property ;
	rdfs:domain <http://rdaregistry.info/Elements/c/C10004> ;
	rdfs:isDefinedBy <http://rdaregistry.info/Elements/a/> ;
	rdfs:label "has address of the person"@en ;
	rdfs:subPropertyOf <http://rdaregistry.info/Elements/u/P60512> ;
	owl:sameAs <http://rdaregistry.info/Elements/a/addressOfThePerson> ;
	skos:definition "Relates a person to the address of a person’s place of residence, business, or employer, and/or an e-mail or internet address."@en .

<http://rdaregistry.info/Elements/a/P50115> reg:name "fullerFormOfName"@en ;
	reg:status status:1001 ;
	a rdf:Property ;
	rdfs:domain <http://rdaregistry.info/Elements/c/C10004> ;
	rdfs:isDefinedBy <http://rdaregistry.info/Elements/a/> ;
	rdfs:label "has fuller form of name"@en ;
	rdfs:subPropertyOf <http://rdaregistry.info/Elements/u/P60530> ;
	owl:sameAs <http://rdaregistry.info/Elements/a/fullerFormOfName> ;
	skos:definition "Relates a person to the full form of a part of a name represented only by an initial or abbreviation in the form chosen as the preferred name, or a part of the name not included in the form chosen as the preferred name."@en .

<http://rdaregistry.info/Elements/a/P50116> reg:name "gender"@en ;
	reg:status status:1001 ;
	a rdf:Property ;
	rdfs:domain <http://rdaregistry.info/Elements/c/C10004> ;
	rdfs:isDefinedBy <http://rdaregistry.info/Elements/a/> ;
	rdfs:label "has gender"@en ;
	rdfs:subPropertyOf <http://rdaregistry.info/Elements/u/P60531> ;
	owl:sameAs <http://rdaregistry.info/Elements/a/gender> ;
	skos:definition "Relates a person to the gender with which a person identifies."@en .

<http://rdaregistry.info/Elements/a/P50117> reg:name "preferredNameForThePerson"@en ;
	reg:status status:1001 ;
	a rdf:Property ;
	rdfs:domain <http://rdaregistry.info/Elements/c/C10004> ;
	rdfs:isDefinedBy <http://rdaregistry.info/Elements/a/> ;
	rdfs:label "has preferred name for the person"@en ;
	rdfs:subPropertyOf <http://rdaregistry.info/Elements/a/P50111> , <http://rdaregistry.info/Elements/u/P60549> ;
	owl:sameAs <http://rdaregistry.info/Elements/a/preferredNameForThePerson> ;
	skos:definition "Relates a person to the name or form of name chosen to identify the person. it is also the basis for the authorized access point representing that person."@en .

<http://rdaregistry.info/Elements/a/P50118> reg:name "placeOfDeath"@en ;
	reg:status status:1001 ;
	a rdf:Property ;
	rdfs:domain <http://rdaregistry.info/Elements/c/C10004> ;
	rdfs:isDefinedBy <http://rdaregistry.info/Elements/a/> ;
	rdfs:label "has place of death"@en ;
	rdfs:subPropertyOf <http://rdaregistry.info/Elements/u/P60592> ;
	owl:sameAs <http://rdaregistry.info/Elements/a/placeOfDeath> ;
	skos:definition "Relates a person to the town, city, province, state, and/or country in which a person died."@en .

<http://rdaregistry.info/Elements/a/P50119> reg:name "placeOfBirth"@en ;
	reg:status status:1001 ;
	a rdf:Property ;
	rdfs:domain <http://rdaregistry.info/Elements/c/C10004> ;
	rdfs:isDefinedBy <http://rdaregistry.info/Elements/a/> ;
	rdfs:label "has place of birth"@en ;
	rdfs:subPropertyOf <http://rdaregistry.info/Elements/u/P60593> ;
	owl:sameAs <http://rdaregistry.info/Elements/a/placeOfBirth> ;
	skos:definition "Relates a person to the town, city, province, state, and/or country in which a person was born."@en .

<http://rdaregistry.info/Elements/a/P50120> reg:name "dateOfDeath"@en ;
	reg:status status:1001 ;
	a rdf:Property ;
	rdfs:domain <http://rdaregistry.info/Elements/c/C10004> ;
	rdfs:isDefinedBy <http://rdaregistry.info/Elements/a/> ;
	rdfs:label "has date of death"@en ;
	rdfs:subPropertyOf <http://rdaregistry.info/Elements/a/P50107> , <http://rdaregistry.info/Elements/u/P60598> ;
	owl:sameAs <http://rdaregistry.info/Elements/a/dateOfDeath> ;
	skos:definition "Relates a person to the year a person died."@en ;
	skos:scopeNote "Date of death may also include the month or month and day of the person’s death."@en .

<http://rdaregistry.info/Elements/a/P50121> reg:name "dateOfBirth"@en ;
	reg:status status:1001 ;
	a rdf:Property ;
	rdfs:domain <http://rdaregistry.info/Elements/c/C10004> ;
	rdfs:isDefinedBy <http://rdaregistry.info/Elements/a/> ;
	rdfs:label "has date of birth"@en ;
	rdfs:subPropertyOf <http://rdaregistry.info/Elements/a/P50107> , <http://rdaregistry.info/Elements/u/P60599> ;
	owl:sameAs <http://rdaregistry.info/Elements/a/dateOfBirth> ;
	skos:definition "Relates a person to the year a person was born."@en ;
	skos:scopeNote "Date of birth may also include the month or month and day of the person’s birth."@en .

<http://rdaregistry.info/Elements/a/P50122> reg:name "appellantPersonOf"@en ;
	reg:status status:1001 ;
	a rdf:Property ;
	rdfs:domain <http://rdaregistry.info/Elements/c/C10004> ;
	rdfs:isDefinedBy <http://rdaregistry.info/Elements/a/> ;
	rdfs:label "is appellant person of"@en ;
	rdfs:range <http://rdaregistry.info/Elements/c/C10001> ;
	rdfs:subPropertyOf <http://rdaregistry.info/Elements/u/P60691> ;
	owl:inverseOf <http://rdaregistry.info/Elements/w/P10042> ;
	owl:sameAs <http://rdaregistry.info/Elements/a/appellantPersonOf> ;
	skos:definition "Relates a person who appeals a lower court's decision to the work."@en .

<http://rdaregistry.info/Elements/a/P50123> reg:name "binderOf"@en ;
	reg:status status:1001 ;
	a rdf:Property ;
	rdfs:domain <http://rdaregistry.info/Elements/c/C10004> ;
	rdfs:isDefinedBy <http://rdaregistry.info/Elements/a/> ;
	rdfs:label "is binder of"@en ;
	rdfs:range <http://rdaregistry.info/Elements/c/C10003> ;
	rdfs:subPropertyOf <http://rdaregistry.info/Elements/a/P50182> , <http://rdaregistry.info/Elements/u/P60692> ;
	owl:inverseOf <http://rdaregistry.info/Elements/i/P40013> ;
	owl:sameAs <http://rdaregistry.info/Elements/a/binderOf> ;
	skos:definition "Relates a person who binds an item to the item."@en .

<http://rdaregistry.info/Elements/a/P50124> reg:name "plaintiffPersonOf"@en ;
	reg:status status:1001 ;
	a rdf:Property ;
	rdfs:domain <http://rdaregistry.info/Elements/c/C10004> ;
	rdfs:isDefinedBy <http://rdaregistry.info/Elements/a/> ;
	rdfs:label "is plaintiff person of"@en ;
	rdfs:range <http://rdaregistry.info/Elements/c/C10001> ;
	rdfs:subPropertyOf <http://rdaregistry.info/Elements/a/P50089> , <http://rdaregistry.info/Elements/u/P60693> ;
	owl:inverseOf <http://rdaregistry.info/Elements/w/P10043> ;
	owl:sameAs <http://rdaregistry.info/Elements/a/plaintiffPersonOf> ;
	skos:definition "Relates a person who brings a suit in a civil proceeding to the work."@en .

<http://rdaregistry.info/Elements/a/P50125> reg:name "inscriberOf"@en ;
	reg:status status:1001 ;
	a rdf:Property ;
	rdfs:domain <http://rdaregistry.info/Elements/c/C10004> ;
	rdfs:isDefinedBy <http://rdaregistry.info/Elements/a/> ;
	rdfs:label "is inscriber of"@en ;
	rdfs:range <http://rdaregistry.info/Elements/c/C10003> ;
	rdfs:subPropertyOf <http://rdaregistry.info/Elements/a/P50182> , <http://rdaregistry.info/Elements/u/P60695> ;
	owl:inverseOf <http://rdaregistry.info/Elements/i/P40014> ;
	owl:sameAs <http://rdaregistry.info/Elements/a/inscriberOf> ;
	skos:definition "Relates a person who has written a statement of dedication or gift on an item to the item."@en .

<http://rdaregistry.info/Elements/a/P50126> reg:name "judgeOf"@en ;
	reg:status status:1001 ;
	a rdf:Property ;
	rdfs:domain <http://rdaregistry.info/Elements/c/C10004> ;
	rdfs:isDefinedBy <http://rdaregistry.info/Elements/a/> ;
	rdfs:label "is judge of"@en ;
	rdfs:range <http://rdaregistry.info/Elements/c/C10001> ;
	rdfs:subPropertyOf <http://rdaregistry.info/Elements/a/P50131> , <http://rdaregistry.info/Elements/u/P60696> ;
	owl:inverseOf <http://rdaregistry.info/Elements/w/P10044> ;
	owl:sameAs <http://rdaregistry.info/Elements/a/judgeOf> ;
	skos:definition "Relates a person who hears and decides on legal matters in court to the work."@en .

<http://rdaregistry.info/Elements/a/P50127> reg:name "praesesOf"@en ;
	reg:status status:1001 ;
	a rdf:Property ;
	rdfs:domain <http://rdaregistry.info/Elements/c/C10004> ;
	rdfs:isDefinedBy <http://rdaregistry.info/Elements/a/> ;
	rdfs:label "is praeses of"@en ;
	rdfs:range <http://rdaregistry.info/Elements/c/C10001> ;
	rdfs:subPropertyOf <http://rdaregistry.info/Elements/a/P50204> , <http://rdaregistry.info/Elements/u/P60699> ;
	owl:inverseOf <http://rdaregistry.info/Elements/w/P10045> ;
	owl:sameAs <http://rdaregistry.info/Elements/a/praesesOf> ;
	skos:definition "Relates a person who is the faculty moderator of an academic disputation, normally proposing a thesis and participating in the ensuing disputation to the work."@en .

<http://rdaregistry.info/Elements/a/P50128> reg:name "annotatorOf"@en ;
	reg:status status:1001 ;
	a rdf:Property ;
	rdfs:domain <http://rdaregistry.info/Elements/c/C10004> ;
	rdfs:isDefinedBy <http://rdaregistry.info/Elements/a/> ;
	rdfs:label "is annotator of"@en ;
	rdfs:range <http://rdaregistry.info/Elements/c/C10003> ;
	rdfs:subPropertyOf <http://rdaregistry.info/Elements/a/P50182> , <http://rdaregistry.info/Elements/u/P60700> ;
	owl:inverseOf <http://rdaregistry.info/Elements/i/P40015> ;
	owl:sameAs <http://rdaregistry.info/Elements/a/annotatorOf> ;
	skos:definition "Relates a person who makes manuscript annotations on an item to the item."@en .

<http://rdaregistry.info/Elements/a/P50129> reg:name "autographerOf"@en ;
	reg:status status:1001 ;
	a rdf:Property ;
	rdfs:domain <http://rdaregistry.info/Elements/c/C10004> ;
	rdfs:isDefinedBy <http://rdaregistry.info/Elements/a/> ;
	rdfs:label "is autographer of"@en ;
	rdfs:range <http://rdaregistry.info/Elements/c/C10003> ;
	rdfs:subPropertyOf <http://rdaregistry.info/Elements/a/P50182> , <http://rdaregistry.info/Elements/u/P60702> ;
	owl:inverseOf <http://rdaregistry.info/Elements/i/P40016> ;
	owl:sameAs <http://rdaregistry.info/Elements/a/autographerOf> ;
	skos:definition "Relates a person whose manuscript signature appears on an item to the item."@en .

<http://rdaregistry.info/Elements/a/P50130> reg:name "issuingBodyOf"@en ;
	reg:status status:1001 ;
	a rdf:Property ;
	rdfs:domain <http://rdaregistry.info/Elements/c/C10002> ;
	rdfs:isDefinedBy <http://rdaregistry.info/Elements/a/> ;
	rdfs:label "is issuing body of"@en ;
	rdfs:range <http://rdaregistry.info/Elements/c/C10001> ;
	rdfs:subPropertyOf <http://rdaregistry.info/Elements/a/P50131> , <http://rdaregistry.info/Elements/u/P60703> ;
	owl:inverseOf <http://rdaregistry.info/Elements/w/P10046> ;
	owl:sameAs <http://rdaregistry.info/Elements/a/issuingBodyOf> ;
	skos:definition "Relates a person, family or corporate body issuing a work, such as an official organ of the body to the work."@en .

<http://rdaregistry.info/Elements/a/P50131> reg:hasSubproperty <http://rdaregistry.info/Elements/a/P50044> , <http://rdaregistry.info/Elements/a/P50069> , <http://rdaregistry.info/Elements/a/P50086> , <http://rdaregistry.info/Elements/a/P50087> , <http://rdaregistry.info/Elements/a/P50088> , <http://rdaregistry.info/Elements/a/P50089> , <http://rdaregistry.info/Elements/a/P50090> , <http://rdaregistry.info/Elements/a/P50091> , <http://rdaregistry.info/Elements/a/P50126> , <http://rdaregistry.info/Elements/a/P50130> , <http://rdaregistry.info/Elements/a/P50132> , <http://rdaregistry.info/Elements/a/P50166> , <http://rdaregistry.info/Elements/a/P50201> , <http://rdaregistry.info/Elements/a/P50205> , <http://rdaregistry.info/Elements/a/P50207> , <http://rdaregistry.info/Elements/a/P50208> , <http://rdaregistry.info/Elements/a/P50209> , <http://rdaregistry.info/Elements/a/P50211> , <http://rdaregistry.info/Elements/a/P50226> ;
	reg:name "otherPFCWorkOf"@en ;
	reg:status status:1001 ;
	a rdf:Property ;
	rdfs:domain <http://rdaregistry.info/Elements/c/C10002> ;
	rdfs:isDefinedBy <http://rdaregistry.info/Elements/a/> ;
	rdfs:label "is other person, family, or corporate body associated with a work of"@en ;
	rdfs:range <http://rdaregistry.info/Elements/c/C10001> ;
	rdfs:subPropertyOf <http://rdaregistry.info/Elements/u/P60374> ;
	owl:inverseOf <http://rdaregistry.info/Elements/w/P10047> ;
	owl:sameAs <http://rdaregistry.info/Elements/a/otherPFCWorkOf> ;
	skos:definition "Relates a person, family, or corporate body associated with a work other than as a creator to the work."@en ;
	skos:scopeNote "Includes persons, etc., to whom correspondence is addressed, persons, etc., honoured by a festschrift, directors, cinematographers, sponsoring bodies, production companies, institutions, etc., hosting an exhibition or event, etc"@en .

<http://rdaregistry.info/Elements/a/P50132> reg:name "dedicatorOf"@en ;
	reg:status status:1001 ;
	a rdf:Property ;
	rdfs:domain <http://rdaregistry.info/Elements/c/C10002> ;
	rdfs:isDefinedBy <http://rdaregistry.info/Elements/a/> ;
	rdfs:label "is dedicator of"@en ;
	rdfs:range <http://rdaregistry.info/Elements/c/C10001> ;
	rdfs:subPropertyOf <http://rdaregistry.info/Elements/a/P50131> , <http://rdaregistry.info/Elements/u/P60603> ;
	owl:inverseOf <http://rdaregistry.info/Elements/w/P10048> ;
	owl:sameAs <http://rdaregistry.info/Elements/a/dedicatorOf> ;
	skos:definition "Relates a person, family, or corporate body by whom a work is dedicated to the work."@en .

<http://rdaregistry.info/Elements/a/P50133> reg:hasSubproperty <http://rdaregistry.info/Elements/a/P50045> , <http://rdaregistry.info/Elements/a/P50046> ;
	reg:name "curatorOf"@en ;
	reg:status status:1001 ;
	a rdf:Property ;
	rdfs:domain <http://rdaregistry.info/Elements/c/C10002> ;
	rdfs:isDefinedBy <http://rdaregistry.info/Elements/a/> ;
	rdfs:label "is curator of"@en ;
	rdfs:range <http://rdaregistry.info/Elements/c/C10003> ;
	rdfs:subPropertyOf <http://rdaregistry.info/Elements/a/P50182> , <http://rdaregistry.info/Elements/u/P60604> ;
	owl:inverseOf <http://rdaregistry.info/Elements/i/P40017> ;
	owl:sameAs <http://rdaregistry.info/Elements/a/curatorOf> ;
	skos:definition "Relates a person, family, or corporate body conceiving, aggregating, and/or organizing an exhibition, collection, or other item to the item."@en .

<http://rdaregistry.info/Elements/a/P50134> reg:name "composerExpressionOf"@en ;
	reg:status status:1001 ;
	a rdf:Property ;
	rdfs:domain <http://rdaregistry.info/Elements/c/C10002> ;
	rdfs:isDefinedBy <http://rdaregistry.info/Elements/a/> ;
	rdfs:label "is composer (expression) of"@en ;
	rdfs:range <http://rdaregistry.info/Elements/c/C10006> ;
	rdfs:subPropertyOf <http://rdaregistry.info/Elements/a/P50161> , <http://rdaregistry.info/Elements/u/P60655> ;
	owl:inverseOf <http://rdaregistry.info/Elements/e/P20026> ;
	owl:sameAs <http://rdaregistry.info/Elements/a/composerExpressionOf> ;
	skos:definition "Relates a person, family, or corporate body contributing to an expression by adding music to a work that originally lacked it, by composing new music to substitute for the original music, or by composing new music to supplement the existing music to the expression."@en .

<http://rdaregistry.info/Elements/a/P50135> reg:name "surveyorOf"@en ;
	reg:status status:1001 ;
	a rdf:Property ;
	rdfs:domain <http://rdaregistry.info/Elements/c/C10002> ;
	rdfs:isDefinedBy <http://rdaregistry.info/Elements/a/> ;
	rdfs:label "is surveyor of"@en ;
	rdfs:range <http://rdaregistry.info/Elements/c/C10006> ;
	rdfs:subPropertyOf <http://rdaregistry.info/Elements/a/P50161> , <http://rdaregistry.info/Elements/u/P60605> ;
	owl:inverseOf <http://rdaregistry.info/Elements/e/P20027> ;
	owl:sameAs <http://rdaregistry.info/Elements/a/surveyorOf> ;
	skos:definition "Relates a person, family, or corporate body contributing to an expression of a cartographic work by providing measurements or dimensional relationships for the geographic area represented to the expression."@en .

<http://rdaregistry.info/Elements/a/P50136> reg:name "animatorOf"@en ;
	reg:status status:1001 ;
	a rdf:Property ;
	rdfs:domain <http://rdaregistry.info/Elements/c/C10002> ;
	rdfs:isDefinedBy <http://rdaregistry.info/Elements/a/> ;
	rdfs:label "is animator of"@en ;
	rdfs:range <http://rdaregistry.info/Elements/c/C10006> ;
	rdfs:subPropertyOf <http://rdaregistry.info/Elements/a/P50161> , <http://rdaregistry.info/Elements/u/P60606> ;
	owl:inverseOf <http://rdaregistry.info/Elements/e/P20028> ;
	owl:sameAs <http://rdaregistry.info/Elements/a/animatorOf> ;
	skos:definition "Relates a person, family, or corporate body contributing to an expression of a moving image work or computer program by giving apparent movement to inanimate objects or drawings to the expression."@en .

<http://rdaregistry.info/Elements/a/P50137> reg:name "arrangerOfMusicOf"@en ;
	reg:status status:1001 ;
	a rdf:Property ;
	rdfs:domain <http://rdaregistry.info/Elements/c/C10002> ;
	rdfs:isDefinedBy <http://rdaregistry.info/Elements/a/> ;
	rdfs:label "is arranger of music of"@en ;
	rdfs:range <http://rdaregistry.info/Elements/c/C10006> ;
	rdfs:subPropertyOf <http://rdaregistry.info/Elements/a/P50161> , <http://rdaregistry.info/Elements/u/P60607> ;
	owl:inverseOf <http://rdaregistry.info/Elements/e/P20029> ;
	owl:sameAs <http://rdaregistry.info/Elements/a/arrangerOfMusicOf> ;
	skos:definition "Relates a person, family, or corporate body contributing to an expression of a musical work by rewriting the composition for a medium of performance different from that for which the work was originally intended to the expression."@en ;
	skos:scopeNote "An arranger of music may also modify the work for the same medium of performance, etc., keeping the musical substance of the original composition essentially unchanged."@en .

<http://rdaregistry.info/Elements/a/P50138> reg:hasSubproperty <http://rdaregistry.info/Elements/a/P50216> ;
	reg:name "writerOfAddedTextOf"@en ;
	reg:status status:1001 ;
	a rdf:Property ;
	rdfs:domain <http://rdaregistry.info/Elements/c/C10002> ;
	rdfs:isDefinedBy <http://rdaregistry.info/Elements/a/> ;
	rdfs:label "is writer of added text of"@en ;
	rdfs:range <http://rdaregistry.info/Elements/c/C10006> ;
	rdfs:subPropertyOf <http://rdaregistry.info/Elements/a/P50154> , <http://rdaregistry.info/Elements/u/P60608> ;
	owl:inverseOf <http://rdaregistry.info/Elements/e/P20030> ;
	owl:sameAs <http://rdaregistry.info/Elements/a/writerOfAddedTextOf> ;
	skos:definition "Relates a person, family, or corporate body contributing to an expression of a work by providing supplementary textual content (e.g., an appendix, an introduction, a preface) to the original work to the expression."@en .

<http://rdaregistry.info/Elements/a/P50139> reg:name "stageDirectorOf"@en ;
	reg:status status:1001 ;
	a rdf:Property ;
	rdfs:domain <http://rdaregistry.info/Elements/c/C10002> ;
	rdfs:isDefinedBy <http://rdaregistry.info/Elements/a/> ;
	rdfs:label "is stage director of"@en ;
	rdfs:range <http://rdaregistry.info/Elements/c/C10006> ;
	rdfs:subPropertyOf <http://rdaregistry.info/Elements/a/P50161> , <http://rdaregistry.info/Elements/u/P60627> ;
	owl:inverseOf <http://rdaregistry.info/Elements/e/P20031> ;
	owl:sameAs <http://rdaregistry.info/Elements/a/stageDirectorOf> ;
	skos:definition "Relates a person, family, or corporate body contributing to an expression of a stage work through the general management and supervision of a performance to the expression."@en .

<http://rdaregistry.info/Elements/a/P50140> reg:name "interviewerExpressionOf"@en ;
	reg:status status:1001 ;
	a rdf:Property ;
	rdfs:domain <http://rdaregistry.info/Elements/c/C10002> ;
	rdfs:isDefinedBy <http://rdaregistry.info/Elements/a/> ;
	rdfs:label "is interviewer (expression) of"@en ;
	rdfs:range <http://rdaregistry.info/Elements/c/C10006> ;
	rdfs:subPropertyOf <http://rdaregistry.info/Elements/a/P50161> , <http://rdaregistry.info/Elements/u/P60659> ;
	owl:inverseOf <http://rdaregistry.info/Elements/e/P20032> ;
	owl:sameAs <http://rdaregistry.info/Elements/a/interviewerExpressionOf> ;
	skos:definition "Relates a person, family, or corporate body contributing to an expression of a work by acting as an interviewer, reporter, pollster, or some other information gathering agent to the expression."@en .

<http://rdaregistry.info/Elements/a/P50141> reg:name "draftsmanOf"@en ;
	reg:status status:1001 ;
	a rdf:Property ;
	rdfs:domain <http://rdaregistry.info/Elements/c/C10002> ;
	rdfs:isDefinedBy <http://rdaregistry.info/Elements/a/> ;
	rdfs:label "is draftsman of"@en ;
	rdfs:range <http://rdaregistry.info/Elements/c/C10006> ;
	rdfs:subPropertyOf <http://rdaregistry.info/Elements/a/P50161> , <http://rdaregistry.info/Elements/u/P60609> ;
	owl:inverseOf <http://rdaregistry.info/Elements/e/P20033> ;
	owl:sameAs <http://rdaregistry.info/Elements/a/draftsmanOf> ;
	skos:definition "Relates a person, family, or corporate body contributing to an expression of a work by an architect, inventor, etc., by making detailed plans or drawings for buildings, ships, aircraft, machines, objects, etc. to the expression."@en .

<http://rdaregistry.info/Elements/a/P50142> reg:name "transcriberOf"@en ;
	reg:status status:1001 ;
	a rdf:Property ;
	rdfs:domain <http://rdaregistry.info/Elements/c/C10002> ;
	rdfs:isDefinedBy <http://rdaregistry.info/Elements/a/> ;
	rdfs:label "is transcriber of"@en ;
	rdfs:range <http://rdaregistry.info/Elements/c/C10006> ;
	rdfs:subPropertyOf <http://rdaregistry.info/Elements/a/P50161> , <http://rdaregistry.info/Elements/u/P60610> ;
	owl:inverseOf <http://rdaregistry.info/Elements/e/P20034> ;
	owl:sameAs <http://rdaregistry.info/Elements/a/transcriberOf> ;
	skos:definition "Relates a person, family, or corporate body contributing to an expression of a work by changing it from one system of notation to another to the expression."@en .

<http://rdaregistry.info/Elements/a/P50143> reg:name "musicalDirectorOf"@en ;
	reg:status status:1001 ;
	a rdf:Property ;
	rdfs:domain <http://rdaregistry.info/Elements/c/C10002> ;
	rdfs:isDefinedBy <http://rdaregistry.info/Elements/a/> ;
	rdfs:label "is musical director of"@en ;
	rdfs:range <http://rdaregistry.info/Elements/c/C10006> ;
	rdfs:subPropertyOf <http://rdaregistry.info/Elements/a/P50161> , <http://rdaregistry.info/Elements/u/P60611> ;
	owl:inverseOf <http://rdaregistry.info/Elements/e/P20035> ;
	owl:sameAs <http://rdaregistry.info/Elements/a/musicalDirectorOf> ;
	skos:definition "Relates a person, family, or corporate body contributing to an expression of a work by coordinating the activities of the composer, the sound editor, and sound mixers for a moving image production or for a musical or dramatic presentation or entertainment to the expression."@en .

<http://rdaregistry.info/Elements/a/P50144> reg:name "costumeDesignerOf"@en ;
	reg:status status:1001 ;
	a rdf:Property ;
	rdfs:domain <http://rdaregistry.info/Elements/c/C10002> ;
	rdfs:isDefinedBy <http://rdaregistry.info/Elements/a/> ;
	rdfs:label "is costume designer of"@en ;
	rdfs:range <http://rdaregistry.info/Elements/c/C10006> ;
	rdfs:subPropertyOf <http://rdaregistry.info/Elements/a/P50161> , <http://rdaregistry.info/Elements/u/P60612> ;
	owl:inverseOf <http://rdaregistry.info/Elements/e/P20036> ;
	owl:sameAs <http://rdaregistry.info/Elements/a/costumeDesignerOf> ;
	skos:definition "Relates a person, family, or corporate body contributing to an expression of a work by designing the costumes for a moving image production or for a musical or dramatic presentation or entertainment to the expression."@en .

<http://rdaregistry.info/Elements/a/P50145> reg:name "translatorOf"@en ;
	reg:status status:1001 ;
	a rdf:Property ;
	rdfs:domain <http://rdaregistry.info/Elements/c/C10002> ;
	rdfs:isDefinedBy <http://rdaregistry.info/Elements/a/> ;
	rdfs:label "is translator of"@en ;
	rdfs:range <http://rdaregistry.info/Elements/c/C10006> ;
	rdfs:subPropertyOf <http://rdaregistry.info/Elements/a/P50161> , <http://rdaregistry.info/Elements/u/P60613> ;
	owl:inverseOf <http://rdaregistry.info/Elements/e/P20037> ;
	owl:sameAs <http://rdaregistry.info/Elements/a/translatorOf> ;
	skos:definition "Relates a person, family, or corporate body contributing to an expression of a work by expressing the original text of the work in a language different from that of the original work to the expression."@en ;
	skos:scopeNote "A translator may also translate a text from an older form of a language into the modern form."@en .

<http://rdaregistry.info/Elements/a/P50146> reg:name "artDirectorOf"@en ;
	reg:status status:1001 ;
	a rdf:Property ;
	rdfs:domain <http://rdaregistry.info/Elements/c/C10002> ;
	rdfs:isDefinedBy <http://rdaregistry.info/Elements/a/> ;
	rdfs:label "is art director of"@en ;
	rdfs:range <http://rdaregistry.info/Elements/c/C10006> ;
	rdfs:subPropertyOf <http://rdaregistry.info/Elements/a/P50161> , <http://rdaregistry.info/Elements/u/P60614> ;
	owl:inverseOf <http://rdaregistry.info/Elements/e/P20038> ;
	owl:sameAs <http://rdaregistry.info/Elements/a/artDirectorOf> ;
	skos:definition "Relates a person, family, or corporate body contributing to an expression of a work by overseeing the artists and craftspeople who build the sets for moving image productions to the expression."@en .

<http://rdaregistry.info/Elements/a/P50147> reg:hasSubproperty <http://rdaregistry.info/Elements/a/P50070> , <http://rdaregistry.info/Elements/a/P50071> , <http://rdaregistry.info/Elements/a/P50072> , <http://rdaregistry.info/Elements/a/P50073> , <http://rdaregistry.info/Elements/a/P50074> , <http://rdaregistry.info/Elements/a/P50075> , <http://rdaregistry.info/Elements/a/P50076> , <http://rdaregistry.info/Elements/a/P50077> , <http://rdaregistry.info/Elements/a/P50078> , <http://rdaregistry.info/Elements/a/P50079> , <http://rdaregistry.info/Elements/a/P50080> , <http://rdaregistry.info/Elements/a/P50081> , <http://rdaregistry.info/Elements/a/P50082> , <http://rdaregistry.info/Elements/a/P50083> , <http://rdaregistry.info/Elements/a/P50084> ;
	reg:name "performerOf"@en ;
	reg:status status:1001 ;
	a rdf:Property ;
	rdfs:domain <http://rdaregistry.info/Elements/c/C10002> ;
	rdfs:isDefinedBy <http://rdaregistry.info/Elements/a/> ;
	rdfs:label "is performer of"@en ;
	rdfs:range <http://rdaregistry.info/Elements/c/C10006> ;
	rdfs:subPropertyOf <http://rdaregistry.info/Elements/a/P50161> , <http://rdaregistry.info/Elements/u/P60615> ;
	owl:inverseOf <http://rdaregistry.info/Elements/e/P20039> ;
	owl:sameAs <http://rdaregistry.info/Elements/a/performerOf> ;
	skos:definition "Relates a person, family, or corporate body contributing to an expression of a work by performing music, acting, dancing, speaking, etc to the expression."@en .

<http://rdaregistry.info/Elements/a/P50148> reg:name "courtReporterOf"@en ;
	reg:status status:1001 ;
	a rdf:Property ;
	rdfs:domain <http://rdaregistry.info/Elements/c/C10002> ;
	rdfs:isDefinedBy <http://rdaregistry.info/Elements/a/> ;
	rdfs:label "is court reporter of"@en ;
	rdfs:range <http://rdaregistry.info/Elements/c/C10006> ;
	rdfs:subPropertyOf <http://rdaregistry.info/Elements/u/P60616> ;
	owl:inverseOf <http://rdaregistry.info/Elements/e/P20040> ;
	owl:sameAs <http://rdaregistry.info/Elements/a/courtReporterOf> ;
	skos:definition "Relates a person, family, or corporate body contributing to an expression of a work by preparing a court's opinions for publication to the expression."@en .

<http://rdaregistry.info/Elements/a/P50149> reg:name "writerOfPrefaceOf"@en ;
	reg:status status:1001 ;
	a rdf:Property ;
	rdfs:domain <http://rdaregistry.info/Elements/c/C10002> ;
	rdfs:isDefinedBy <http://rdaregistry.info/Elements/a/> ;
	rdfs:label "is writer of preface of"@en ;
	rdfs:range <http://rdaregistry.info/Elements/c/C10006> ;
	rdfs:subPropertyOf <http://rdaregistry.info/Elements/a/P50154> , <http://rdaregistry.info/Elements/u/P60617> ;
	owl:inverseOf <http://rdaregistry.info/Elements/e/P20041> ;
	owl:sameAs <http://rdaregistry.info/Elements/a/writerOfPrefaceOf> ;
	skos:definition "Relates a person, family, or corporate body contributing to an expression of a work by providing a preface to the original work to the expression."@en .

<http://rdaregistry.info/Elements/a/P50150> reg:name "cartographerExpressionOf"@en ;
	reg:status status:1001 ;
	a rdf:Property ;
	rdfs:domain <http://rdaregistry.info/Elements/c/C10002> ;
	rdfs:isDefinedBy <http://rdaregistry.info/Elements/a/> ;
	rdfs:label "is cartographer (expression) of"@en ;
	rdfs:range <http://rdaregistry.info/Elements/c/C10006> ;
	rdfs:subPropertyOf <http://rdaregistry.info/Elements/a/P50161> , <http://rdaregistry.info/Elements/u/P60654> ;
	owl:inverseOf <http://rdaregistry.info/Elements/e/P20042> ;
	owl:sameAs <http://rdaregistry.info/Elements/a/cartographerExpressionOf> ;
	skos:definition "Relates a person, family, or corporate body contributing to an expression of a work by providing additional cartography, or by modifying the previous cartography to the expression."@en .

<http://rdaregistry.info/Elements/a/P50151> reg:name "choreographerExpressionOf"@en ;
	reg:status status:1001 ;
	a rdf:Property ;
	rdfs:domain <http://rdaregistry.info/Elements/c/C10002> ;
	rdfs:isDefinedBy <http://rdaregistry.info/Elements/a/> ;
	rdfs:label "is choreographer (expression) of"@en ;
	rdfs:range <http://rdaregistry.info/Elements/c/C10006> ;
	rdfs:subPropertyOf <http://rdaregistry.info/Elements/a/P50161> , <http://rdaregistry.info/Elements/u/P60662> ;
	owl:inverseOf <http://rdaregistry.info/Elements/e/P20043> ;
	owl:sameAs <http://rdaregistry.info/Elements/a/choreographerExpressionOf> ;
	skos:definition "Relates a person, family, or corporate body contributing to an expression of a work by providing additional choreography, or by modifying the previous choreography to the expression."@en .

<http://rdaregistry.info/Elements/a/P50152> reg:name "writerOfAddedCommentaryOf"@en ;
	reg:status status:1001 ;
	a rdf:Property ;
	rdfs:domain <http://rdaregistry.info/Elements/c/C10002> ;
	rdfs:isDefinedBy <http://rdaregistry.info/Elements/a/> ;
	rdfs:label "is writer of added commentary of"@en ;
	rdfs:range <http://rdaregistry.info/Elements/c/C10006> ;
	rdfs:subPropertyOf <http://rdaregistry.info/Elements/a/P50154> , <http://rdaregistry.info/Elements/u/P60618> ;
	owl:inverseOf <http://rdaregistry.info/Elements/e/P20044> ;
	owl:sameAs <http://rdaregistry.info/Elements/a/writerOfAddedCommentaryOf> ;
	skos:definition "Relates a person, family, or corporate body contributing to an expression of a work by providing an interpretation or critical explanation of the original work to the expression."@en .

<http://rdaregistry.info/Elements/a/P50153> reg:name "writerOfIntroductionOf"@en ;
	reg:status status:1001 ;
	a rdf:Property ;
	rdfs:domain <http://rdaregistry.info/Elements/c/C10002> ;
	rdfs:isDefinedBy <http://rdaregistry.info/Elements/a/> ;
	rdfs:label "is writer of introduction of"@en ;
	rdfs:range <http://rdaregistry.info/Elements/c/C10006> ;
	rdfs:subPropertyOf <http://rdaregistry.info/Elements/a/P50154> , <http://rdaregistry.info/Elements/u/P60619> ;
	owl:inverseOf <http://rdaregistry.info/Elements/e/P20045> ;
	owl:sameAs <http://rdaregistry.info/Elements/a/writerOfIntroductionOf> ;
	skos:definition "Relates a person, family, or corporate body contributing to an expression of a work by providing an introduction to the original work to the expression."@en .

<http://rdaregistry.info/Elements/a/P50154> reg:hasSubproperty <http://rdaregistry.info/Elements/a/P50138> , <http://rdaregistry.info/Elements/a/P50149> , <http://rdaregistry.info/Elements/a/P50152> , <http://rdaregistry.info/Elements/a/P50153> ;
	reg:name "writerOfSupplementaryTextualContentOf"@en ;
	reg:status status:1001 ;
	a rdf:Property ;
	rdfs:domain <http://rdaregistry.info/Elements/c/C10002> ;
	rdfs:isDefinedBy <http://rdaregistry.info/Elements/a/> ;
	rdfs:label "is writer of supplementary textual content of"@en ;
	rdfs:range <http://rdaregistry.info/Elements/c/C10006> ;
	rdfs:subPropertyOf <http://rdaregistry.info/Elements/a/P50161> , <http://rdaregistry.info/Elements/u/P60620> ;
	owl:inverseOf <http://rdaregistry.info/Elements/e/P20046> ;
	owl:sameAs <http://rdaregistry.info/Elements/a/writerOfSupplementaryTextualContentOf> ;
	skos:definition "Relates a person, family, or corporate body contributing to an expression of a work by providing supplementary textual content (e to the expression."@en .

<http://rdaregistry.info/Elements/a/P50155> reg:name "intervieweeExpressionOf"@en ;
	reg:status status:1001 ;
	a rdf:Property ;
	rdfs:domain <http://rdaregistry.info/Elements/c/C10002> ;
	rdfs:isDefinedBy <http://rdaregistry.info/Elements/a/> ;
	rdfs:label "is interviewee (expression) of"@en ;
	rdfs:range <http://rdaregistry.info/Elements/c/C10006> ;
	rdfs:subPropertyOf <http://rdaregistry.info/Elements/a/P50161> , <http://rdaregistry.info/Elements/u/P60661> ;
	owl:inverseOf <http://rdaregistry.info/Elements/e/P20047> ;
	owl:sameAs <http://rdaregistry.info/Elements/a/intervieweeExpressionOf> ;
	skos:definition "Relates a person, family, or corporate body contributing to an expression of a work by responding to an interviewer, usually a reporter, pollster, or some other information gathering agent to the expression."@en .

<http://rdaregistry.info/Elements/a/P50156> reg:name "editorOf"@en ;
	reg:status status:1001 ;
	a rdf:Property ;
	rdfs:domain <http://rdaregistry.info/Elements/c/C10002> ;
	rdfs:isDefinedBy <http://rdaregistry.info/Elements/a/> ;
	rdfs:label "is editor of"@en ;
	rdfs:range <http://rdaregistry.info/Elements/c/C10006> ;
	rdfs:subPropertyOf <http://rdaregistry.info/Elements/a/P50161> , <http://rdaregistry.info/Elements/u/P60621> ;
	owl:inverseOf <http://rdaregistry.info/Elements/e/P20048> ;
	owl:sameAs <http://rdaregistry.info/Elements/a/editorOf> ;
	skos:definition "Relates a person, family, or corporate body contributing to an expression of a work by revising or clarifying the content, e to the expression."@en ;
	skos:scopeNote "An editor may also prepare an expression of a work for production, publication, or distribution."@en .

<http://rdaregistry.info/Elements/a/P50157> reg:name "abridgerOf"@en ;
	reg:status status:1001 ;
	a rdf:Property ;
	rdfs:domain <http://rdaregistry.info/Elements/c/C10002> ;
	rdfs:isDefinedBy <http://rdaregistry.info/Elements/a/> ;
	rdfs:label "is abridger of"@en ;
	rdfs:range <http://rdaregistry.info/Elements/c/C10006> ;
	rdfs:subPropertyOf <http://rdaregistry.info/Elements/a/P50161> , <http://rdaregistry.info/Elements/u/P60622> ;
	owl:inverseOf <http://rdaregistry.info/Elements/e/P20049> ;
	owl:sameAs <http://rdaregistry.info/Elements/a/abridgerOf> ;
	skos:definition "Relates a person, family, or corporate body contributing to an expression of a work by shortening or condensing the original work but leaving the nature and content of the original work substantially unchanged to the expression."@en .

<http://rdaregistry.info/Elements/a/P50158> reg:name "recordingEngineerOf"@en ;
	reg:status status:1001 ;
	a rdf:Property ;
	rdfs:domain <http://rdaregistry.info/Elements/c/C10002> ;
	rdfs:isDefinedBy <http://rdaregistry.info/Elements/a/> ;
	rdfs:label "is recording engineer of"@en ;
	rdfs:range <http://rdaregistry.info/Elements/c/C10006> ;
	rdfs:subPropertyOf <http://rdaregistry.info/Elements/a/P50161> , <http://rdaregistry.info/Elements/u/P60623> ;
	owl:inverseOf <http://rdaregistry.info/Elements/e/P20050> ;
	owl:sameAs <http://rdaregistry.info/Elements/a/recordingEngineerOf> ;
	skos:definition "Relates a person, family, or corporate body contributing to an expression of a work by supervising the technical aspects of a sound or video recording session to the expression."@en .

<http://rdaregistry.info/Elements/a/P50159> reg:name "illustratorOf"@en ;
	reg:status status:1001 ;
	a rdf:Property ;
	rdfs:domain <http://rdaregistry.info/Elements/c/C10002> ;
	rdfs:isDefinedBy <http://rdaregistry.info/Elements/a/> ;
	rdfs:label "is illustrator of"@en ;
	rdfs:range <http://rdaregistry.info/Elements/c/C10006> ;
	rdfs:subPropertyOf <http://rdaregistry.info/Elements/a/P50161> , <http://rdaregistry.info/Elements/u/P60624> ;
	owl:inverseOf <http://rdaregistry.info/Elements/e/P20051> ;
	owl:sameAs <http://rdaregistry.info/Elements/a/illustratorOf> ;
	skos:definition "Relates a person, family, or corporate body contributing to an expression of a work by supplementing the primary content with drawings, diagrams, photographs, etc to the expression."@en .

<http://rdaregistry.info/Elements/a/P50160> reg:name "recordistOf"@en ;
	reg:status status:1001 ;
	a rdf:Property ;
	rdfs:domain <http://rdaregistry.info/Elements/c/C10002> ;
	rdfs:isDefinedBy <http://rdaregistry.info/Elements/a/> ;
	rdfs:label "is recordist of"@en ;
	rdfs:range <http://rdaregistry.info/Elements/c/C10006> ;
	rdfs:subPropertyOf <http://rdaregistry.info/Elements/a/P50161> , <http://rdaregistry.info/Elements/u/P60625> ;
	owl:inverseOf <http://rdaregistry.info/Elements/e/P20052> ;
	owl:sameAs <http://rdaregistry.info/Elements/a/recordistOf> ;
	skos:definition "Relates a person, family, or corporate body contributing to an expression of a work by using a recording device to capture sound and/or video during a recording session, including field recordings of natural sounds, folkloric events, music, etc to the expression."@en .

<http://rdaregistry.info/Elements/a/P50161> reg:hasSubproperty <http://rdaregistry.info/Elements/a/P50134> , <http://rdaregistry.info/Elements/a/P50135> , <http://rdaregistry.info/Elements/a/P50136> , <http://rdaregistry.info/Elements/a/P50137> , <http://rdaregistry.info/Elements/a/P50139> , <http://rdaregistry.info/Elements/a/P50140> , <http://rdaregistry.info/Elements/a/P50141> , <http://rdaregistry.info/Elements/a/P50142> , <http://rdaregistry.info/Elements/a/P50143> , <http://rdaregistry.info/Elements/a/P50144> , <http://rdaregistry.info/Elements/a/P50145> , <http://rdaregistry.info/Elements/a/P50146> , <http://rdaregistry.info/Elements/a/P50147> , <http://rdaregistry.info/Elements/a/P50150> , <http://rdaregistry.info/Elements/a/P50151> , <http://rdaregistry.info/Elements/a/P50154> , <http://rdaregistry.info/Elements/a/P50155> , <http://rdaregistry.info/Elements/a/P50156> , <http://rdaregistry.info/Elements/a/P50157> , <http://rdaregistry.info/Elements/a/P50158> , <http://rdaregistry.info/Elements/a/P50159> , <http://rdaregistry.info/Elements/a/P50160> , <http://rdaregistry.info/Elements/a/P50183> , <http://rdaregistry.info/Elements/a/P50198> , <http://rdaregistry.info/Elements/a/P50212> ;
	reg:name "contributorOf"@en ;
	reg:status status:1001 ;
	a rdf:Property ;
	rdfs:domain <http://rdaregistry.info/Elements/c/C10002> ;
	rdfs:isDefinedBy <http://rdaregistry.info/Elements/a/> ;
	rdfs:label "is contributor of"@en ;
	rdfs:range <http://rdaregistry.info/Elements/c/C10006> ;
	rdfs:subPropertyOf <http://rdaregistry.info/Elements/u/P60626> ;
	owl:inverseOf <http://rdaregistry.info/Elements/e/P20053> ;
	owl:sameAs <http://rdaregistry.info/Elements/a/contributorOf> ;
	skos:definition "Relates a person, family, or corporate body contributing to an expression to the expression."@en ;
	skos:scopeNote "Contributors include editors, translators, arrangers of music, performers, etc."@en .

<http://rdaregistry.info/Elements/a/P50162> reg:hasSubproperty <http://rdaregistry.info/Elements/a/P50047> ;
	reg:name "currentOwnerOf"@en ;
	reg:status status:1001 ;
	a rdf:Property ;
	rdfs:domain <http://rdaregistry.info/Elements/c/C10002> ;
	rdfs:isDefinedBy <http://rdaregistry.info/Elements/a/> ;
	rdfs:label "is current owner of"@en ;
	rdfs:range <http://rdaregistry.info/Elements/c/C10003> ;
	rdfs:subPropertyOf <http://rdaregistry.info/Elements/a/P50165> , <http://rdaregistry.info/Elements/u/P60628> ;
	owl:inverseOf <http://rdaregistry.info/Elements/i/P40018> ;
	owl:sameAs <http://rdaregistry.info/Elements/a/currentOwnerOf> ;
	skos:definition "Relates a person, family, or corporate body currently having legal possession of an item to the item."@en .

<http://rdaregistry.info/Elements/a/P50163> reg:hasSubproperty <http://rdaregistry.info/Elements/a/P50066> , <http://rdaregistry.info/Elements/a/P50067> ;
	reg:name "formerOwnerOf"@en ;
	reg:status status:1001 ;
	a rdf:Property ;
	rdfs:domain <http://rdaregistry.info/Elements/c/C10002> ;
	rdfs:isDefinedBy <http://rdaregistry.info/Elements/a/> ;
	rdfs:label "is former owner of"@en ;
	rdfs:range <http://rdaregistry.info/Elements/c/C10003> ;
	rdfs:subPropertyOf <http://rdaregistry.info/Elements/a/P50165> , <http://rdaregistry.info/Elements/u/P60630> ;
	owl:inverseOf <http://rdaregistry.info/Elements/i/P40019> ;
	owl:sameAs <http://rdaregistry.info/Elements/a/formerOwnerOf> ;
	skos:definition "Relates a person, family, or corporate body formerly having legal possession of an item to the item."@en .

<http://rdaregistry.info/Elements/a/P50164> reg:name "custodianOf"@en ;
	reg:status status:1001 ;
	a rdf:Property ;
	rdfs:domain <http://rdaregistry.info/Elements/c/C10002> ;
	rdfs:isDefinedBy <http://rdaregistry.info/Elements/a/> ;
	rdfs:label "is custodian of"@en ;
	rdfs:range <http://rdaregistry.info/Elements/c/C10003> ;
	rdfs:subPropertyOf <http://rdaregistry.info/Elements/u/P60631> ;
	owl:inverseOf <http://rdaregistry.info/Elements/i/P40020> ;
	owl:sameAs <http://rdaregistry.info/Elements/a/custodianOf> ;
	skos:definition "Relates a person, family, or corporate body having legal custody of an item to the item."@en .

<http://rdaregistry.info/Elements/a/P50165> reg:hasSubproperty <http://rdaregistry.info/Elements/a/P50162> , <http://rdaregistry.info/Elements/a/P50163> ;
	reg:name "ownerOf"@en ;
	reg:status status:1001 ;
	a rdf:Property ;
	rdfs:domain <http://rdaregistry.info/Elements/c/C10002> ;
	rdfs:isDefinedBy <http://rdaregistry.info/Elements/a/> ;
	rdfs:label "is owner of"@en ;
	rdfs:range <http://rdaregistry.info/Elements/c/C10003> ;
	rdfs:subPropertyOf <http://rdaregistry.info/Elements/u/P60632> ;
	owl:inverseOf <http://rdaregistry.info/Elements/i/P40021> ;
	owl:sameAs <http://rdaregistry.info/Elements/a/ownerOf> ;
	skos:definition "Relates a person, family, or corporate body having legal possession of an item to the item."@en .

<http://rdaregistry.info/Elements/a/P50166> reg:name "honoureeOf"@en ;
	reg:status status:1001 ;
	a rdf:Property ;
	rdfs:domain <http://rdaregistry.info/Elements/c/C10002> ;
	rdfs:isDefinedBy <http://rdaregistry.info/Elements/a/> ;
	rdfs:label "is honouree of"@en ;
	rdfs:range <http://rdaregistry.info/Elements/c/C10001> ;
	rdfs:subPropertyOf <http://rdaregistry.info/Elements/a/P50131> , <http://rdaregistry.info/Elements/u/P60634> ;
	owl:inverseOf <http://rdaregistry.info/Elements/w/P10049> ;
	owl:sameAs <http://rdaregistry.info/Elements/a/honoureeOf> ;
	skos:definition "Relates a person, family, or corporate body honoured by a work (e.g., the honouree of a festschrift) to the work."@en .

<http://rdaregistry.info/Elements/a/P50167> reg:name "honoureeOfItemOf"@en ;
	reg:status status:1001 ;
	a rdf:Property ;
	rdfs:domain <http://rdaregistry.info/Elements/c/C10002> ;
	rdfs:isDefinedBy <http://rdaregistry.info/Elements/a/> ;
	rdfs:label "is honouree (item) of"@en ;
	rdfs:range <http://rdaregistry.info/Elements/c/C10003> ;
	rdfs:subPropertyOf <http://rdaregistry.info/Elements/a/P50182> , <http://rdaregistry.info/Elements/u/P60634> ;
	owl:inverseOf <http://rdaregistry.info/Elements/i/P40022> ;
	owl:sameAs <http://rdaregistry.info/Elements/a/honoureeOfItemOf> ;
	skos:definition "Relates a person, family, or corporate body honoured by an item, e.g., a person to whom a copy is presented, to the item."@en .

<http://rdaregistry.info/Elements/a/P50168> reg:name "broadcasterOf"@en ;
	reg:status status:1001 ;
	a rdf:Property ;
	rdfs:domain <http://rdaregistry.info/Elements/c/C10002> ;
	rdfs:isDefinedBy <http://rdaregistry.info/Elements/a/> ;
	rdfs:label "is broadcaster of"@en ;
	rdfs:range <http://rdaregistry.info/Elements/c/C10007> ;
	rdfs:subPropertyOf <http://rdaregistry.info/Elements/a/P50203> , <http://rdaregistry.info/Elements/u/P60635> ;
	owl:inverseOf <http://rdaregistry.info/Elements/m/P30067> ;
	owl:sameAs <http://rdaregistry.info/Elements/a/broadcasterOf> ;
	skos:definition "Relates a person, family, or corporate body involved in broadcasting a manifestation to an audience via radio, television, webcast, etc to the manifestation."@en .

<http://rdaregistry.info/Elements/a/P50169> reg:name "filmDistributorOf"@en ;
	reg:status status:1001 ;
	a rdf:Property ;
	rdfs:domain <http://rdaregistry.info/Elements/c/C10002> ;
	rdfs:isDefinedBy <http://rdaregistry.info/Elements/a/> ;
	rdfs:label "is film distributor of"@en ;
	rdfs:range <http://rdaregistry.info/Elements/c/C10007> ;
	rdfs:subPropertyOf <http://rdaregistry.info/Elements/a/P50199> , <http://rdaregistry.info/Elements/u/P60636> ;
	owl:inverseOf <http://rdaregistry.info/Elements/m/P30068> ;
	owl:sameAs <http://rdaregistry.info/Elements/a/filmDistributorOf> ;
	skos:definition "Relates a person, family, or corporate body involved in distributing a moving image manifestation to theatres or other distribution channels to the manifestation."@en .

<http://rdaregistry.info/Elements/a/P50170> reg:name "bookDesignerOf"@en ;
	reg:status status:1001 ;
	a rdf:Property ;
	rdfs:domain <http://rdaregistry.info/Elements/c/C10002> ;
	rdfs:isDefinedBy <http://rdaregistry.info/Elements/a/> ;
	rdfs:label "is book designer of"@en ;
	rdfs:range <http://rdaregistry.info/Elements/c/C10007> ;
	rdfs:subPropertyOf <http://rdaregistry.info/Elements/a/P50202> , <http://rdaregistry.info/Elements/u/P60637> ;
	owl:inverseOf <http://rdaregistry.info/Elements/m/P30069> ;
	owl:sameAs <http://rdaregistry.info/Elements/a/bookDesignerOf> ;
	skos:definition "Relates a person, family, or corporate body involved in manufacturing a manifestation by being responsible for the entire graphic design of a book, including arrangement of type and illustration, choice of materials, and process used to the manifestation."@en .

<http://rdaregistry.info/Elements/a/P50171> reg:name "engraverOf"@en ;
	reg:status status:1001 ;
	a rdf:Property ;
	rdfs:domain <http://rdaregistry.info/Elements/c/C10002> ;
	rdfs:isDefinedBy <http://rdaregistry.info/Elements/a/> ;
	rdfs:label "is engraver of"@en ;
	rdfs:range <http://rdaregistry.info/Elements/c/C10007> ;
	rdfs:subPropertyOf <http://rdaregistry.info/Elements/a/P50202> , <http://rdaregistry.info/Elements/u/P60638> ;
	owl:inverseOf <http://rdaregistry.info/Elements/m/P30070> ;
	owl:sameAs <http://rdaregistry.info/Elements/a/engraverOf> ;
	skos:definition "Relates a person, family, or corporate body involved in manufacturing a manifestation by cutting letters, figures, etc., on a surface such as a wooden or metal plate used for printing to the manifestation."@en .

<http://rdaregistry.info/Elements/a/P50172> reg:name "brailleEmbosserOf"@en ;
	reg:status status:1001 ;
	a rdf:Property ;
	rdfs:domain <http://rdaregistry.info/Elements/c/C10002> ;
	rdfs:isDefinedBy <http://rdaregistry.info/Elements/a/> ;
	rdfs:label "is braille embosser of"@en ;
	rdfs:range <http://rdaregistry.info/Elements/c/C10007> ;
	rdfs:subPropertyOf <http://rdaregistry.info/Elements/a/P50202> , <http://rdaregistry.info/Elements/u/P60639> ;
	owl:inverseOf <http://rdaregistry.info/Elements/m/P30071> ;
	owl:sameAs <http://rdaregistry.info/Elements/a/brailleEmbosserOf> ;
	skos:definition "Relates a person, family, or corporate body involved in manufacturing a manifestation by embossing braille cells using a stylus, special embossing printer, or other device to the manifestation."@en .

<http://rdaregistry.info/Elements/a/P50173> reg:name "printmakerOf"@en ;
	reg:status status:1001 ;
	a rdf:Property ;
	rdfs:domain <http://rdaregistry.info/Elements/c/C10002> ;
	rdfs:isDefinedBy <http://rdaregistry.info/Elements/a/> ;
	rdfs:label "is printmaker of"@en ;
	rdfs:range <http://rdaregistry.info/Elements/c/C10007> ;
	rdfs:subPropertyOf <http://rdaregistry.info/Elements/a/P50202> , <http://rdaregistry.info/Elements/u/P60640> ;
	owl:inverseOf <http://rdaregistry.info/Elements/m/P30072> ;
	owl:sameAs <http://rdaregistry.info/Elements/a/printmakerOf> ;
	skos:definition "Relates a person, family, or corporate body involved in manufacturing a manifestation by making a relief, intaglio, or planographic printing surface to the manifestation."@en .

<http://rdaregistry.info/Elements/a/P50174> reg:name "casterOf"@en ;
	reg:status status:1001 ;
	a rdf:Property ;
	rdfs:domain <http://rdaregistry.info/Elements/c/C10002> ;
	rdfs:isDefinedBy <http://rdaregistry.info/Elements/a/> ;
	rdfs:label "is caster of"@en ;
	rdfs:range <http://rdaregistry.info/Elements/c/C10007> ;
	rdfs:subPropertyOf <http://rdaregistry.info/Elements/a/P50202> , <http://rdaregistry.info/Elements/u/P60641> ;
	owl:inverseOf <http://rdaregistry.info/Elements/m/P30073> ;
	owl:sameAs <http://rdaregistry.info/Elements/a/casterOf> ;
	skos:definition "Relates a person, family, or corporate body involved in manufacturing a manifestation by pouring a liquid or molten substance into a mold and leaving it to solidify to take the shape of the mold to the manifestation."@en .

<http://rdaregistry.info/Elements/a/P50175> reg:name "lithographerOf"@en ;
	reg:status status:1001 ;
	a rdf:Property ;
	rdfs:domain <http://rdaregistry.info/Elements/c/C10002> ;
	rdfs:isDefinedBy <http://rdaregistry.info/Elements/a/> ;
	rdfs:label "is lithographer of"@en ;
	rdfs:range <http://rdaregistry.info/Elements/c/C10007> ;
	rdfs:subPropertyOf <http://rdaregistry.info/Elements/a/P50202> , <http://rdaregistry.info/Elements/u/P60642> ;
	owl:inverseOf <http://rdaregistry.info/Elements/m/P30074> ;
	owl:sameAs <http://rdaregistry.info/Elements/a/lithographerOf> ;
	skos:definition "Relates a person, family, or corporate body involved in manufacturing a manifestation by preparing a stone or plate for lithographic printing, including a graphic artist creating a design directly on the surface from which printing will be done to the manifestation."@en .

<http://rdaregistry.info/Elements/a/P50176> reg:name "platemakerOf"@en ;
	reg:status status:1001 ;
	a rdf:Property ;
	rdfs:domain <http://rdaregistry.info/Elements/c/C10002> ;
	rdfs:isDefinedBy <http://rdaregistry.info/Elements/a/> ;
	rdfs:label "is platemaker of"@en ;
	rdfs:range <http://rdaregistry.info/Elements/c/C10007> ;
	rdfs:subPropertyOf <http://rdaregistry.info/Elements/a/P50202> , <http://rdaregistry.info/Elements/u/P60643> ;
	owl:inverseOf <http://rdaregistry.info/Elements/m/P30075> ;
	owl:sameAs <http://rdaregistry.info/Elements/a/platemakerOf> ;
	skos:definition "Relates a person, family, or corporate body involved in manufacturing a manifestation by preparing plates used in the production of printed images and/or text to the manifestation."@en .

<http://rdaregistry.info/Elements/a/P50177> reg:name "etcherOf"@en ;
	reg:status status:1001 ;
	a rdf:Property ;
	rdfs:domain <http://rdaregistry.info/Elements/c/C10002> ;
	rdfs:isDefinedBy <http://rdaregistry.info/Elements/a/> ;
	rdfs:label "is etcher of"@en ;
	rdfs:range <http://rdaregistry.info/Elements/c/C10007> ;
	rdfs:subPropertyOf <http://rdaregistry.info/Elements/a/P50202> , <http://rdaregistry.info/Elements/u/P60644> ;
	owl:inverseOf <http://rdaregistry.info/Elements/m/P30076> ;
	owl:sameAs <http://rdaregistry.info/Elements/a/etcherOf> ;
	skos:definition "Relates a person, family, or corporate body involved in manufacturing a manifestation by subjecting metal, glass, or some other surface used for printing, to acid or another corrosive substance to the manifestation."@en .

<http://rdaregistry.info/Elements/a/P50178> reg:name "collotyperOf"@en ;
	reg:status status:1001 ;
	a rdf:Property ;
	rdfs:domain <http://rdaregistry.info/Elements/c/C10002> ;
	rdfs:isDefinedBy <http://rdaregistry.info/Elements/a/> ;
	rdfs:label "is collotyper of"@en ;
	rdfs:range <http://rdaregistry.info/Elements/c/C10007> ;
	rdfs:subPropertyOf <http://rdaregistry.info/Elements/a/P50202> , <http://rdaregistry.info/Elements/u/P60645> ;
	owl:inverseOf <http://rdaregistry.info/Elements/m/P30077> ;
	owl:sameAs <http://rdaregistry.info/Elements/a/collotyperOf> ;
	skos:definition "Relates a person, family, or corporate body involved in manufacturing a manifestation of photographic prints from film or other colloid that has ink-receptive and ink-repellent surfaces to the manifestation."@en .

<http://rdaregistry.info/Elements/a/P50179> reg:name "printerOf"@en ;
	reg:status status:1001 ;
	a rdf:Property ;
	rdfs:domain <http://rdaregistry.info/Elements/c/C10002> ;
	rdfs:isDefinedBy <http://rdaregistry.info/Elements/a/> ;
	rdfs:label "is printer of"@en ;
	rdfs:range <http://rdaregistry.info/Elements/c/C10007> ;
	rdfs:subPropertyOf <http://rdaregistry.info/Elements/a/P50202> , <http://rdaregistry.info/Elements/u/P60646> ;
	owl:inverseOf <http://rdaregistry.info/Elements/m/P30078> ;
	owl:sameAs <http://rdaregistry.info/Elements/a/printerOf> ;
	skos:definition "Relates a person, family, or corporate body involved in manufacturing a manifestation of printed text, notated music, etc., from type or plates, such as a book, newspaper, magazine, broadside, score, etc. to the manifestation."@en .

<http://rdaregistry.info/Elements/a/P50180> reg:name "presenterOf"@en ;
	reg:status status:1001 ;
	a rdf:Property ;
	rdfs:domain <http://rdaregistry.info/Elements/c/C10002> ;
	rdfs:isDefinedBy <http://rdaregistry.info/Elements/a/> ;
	rdfs:label "is presenter of"@en ;
	rdfs:range <http://rdaregistry.info/Elements/c/C10006> ;
	rdfs:subPropertyOf <http://rdaregistry.info/Elements/u/P60647> ;
	owl:inverseOf <http://rdaregistry.info/Elements/e/P20054> ;
	owl:sameAs <http://rdaregistry.info/Elements/a/presenterOf> ;
	skos:definition "Relates a person, family, or corporate body mentioned in an \"X presents\" credit for moving image materials and who is probably associated with production, finance, or distribution in some way to the expression."@en .

<http://rdaregistry.info/Elements/a/P50181> reg:name "otherPFCManifestationOf"@en ;
	reg:status status:1001 ;
	a rdf:Property ;
	rdfs:domain <http://rdaregistry.info/Elements/c/C10002> ;
	rdfs:isDefinedBy <http://rdaregistry.info/Elements/a/> ;
	rdfs:label "is other person, family, or corporate body associated with a manifestation of"@en ;
	rdfs:range <http://rdaregistry.info/Elements/c/C10007> ;
	rdfs:subPropertyOf <http://rdaregistry.info/Elements/u/P60374> ;
	owl:inverseOf <http://rdaregistry.info/Elements/m/P30079> ;
	owl:sameAs <http://rdaregistry.info/Elements/a/otherPFCManifestationOf> ;
	skos:definition "Relates a person, family, or corporate body other than a producer, publisher, distributor or manufacturer associated with a manifestation to the manifestation."@en ;
	skos:scopeNote "Includes book designers, platemakers, etc."@en .

<http://rdaregistry.info/Elements/a/P50182> reg:hasSubproperty <http://rdaregistry.info/Elements/a/P50092> , <http://rdaregistry.info/Elements/a/P50123> , <http://rdaregistry.info/Elements/a/P50125> , <http://rdaregistry.info/Elements/a/P50128> , <http://rdaregistry.info/Elements/a/P50129> , <http://rdaregistry.info/Elements/a/P50133> , <http://rdaregistry.info/Elements/a/P50167> , <http://rdaregistry.info/Elements/a/P50206> , <http://rdaregistry.info/Elements/a/P50210> ;
	reg:name "otherPFCItemOf"@en ;
	reg:status status:1001 ;
	a rdf:Property ;
	rdfs:domain <http://rdaregistry.info/Elements/c/C10002> ;
	rdfs:isDefinedBy <http://rdaregistry.info/Elements/a/> ;
	rdfs:label "is other person, family, or corporate body associated with an item of"@en ;
	rdfs:range <http://rdaregistry.info/Elements/c/C10003> ;
	rdfs:subPropertyOf <http://rdaregistry.info/Elements/u/P60374> ;
	owl:inverseOf <http://rdaregistry.info/Elements/i/P40023> ;
	owl:sameAs <http://rdaregistry.info/Elements/a/otherPFCItemOf> ;
	skos:definition "Relates a person, family, or corporate body other than an owner or custodian associated with an item to the item."@en ;
	skos:scopeNote "Includes curators, binders, restorationists, etc."@en .

<http://rdaregistry.info/Elements/a/P50183> reg:name "editorOfMovingImageWorkOf"@en ;
	reg:status status:1001 ;
	a rdf:Property ;
	rdfs:domain <http://rdaregistry.info/Elements/c/C10002> ;
	rdfs:isDefinedBy <http://rdaregistry.info/Elements/a/> ;
	rdfs:label "is editor of moving image work of"@en ;
	rdfs:range <http://rdaregistry.info/Elements/c/C10006> ;
	rdfs:subPropertyOf <http://rdaregistry.info/Elements/a/P50161> , <http://rdaregistry.info/Elements/u/P60651> ;
	owl:inverseOf <http://rdaregistry.info/Elements/e/P20055> ;
	owl:sameAs <http://rdaregistry.info/Elements/a/editorOfMovingImageWorkOf> ;
	skos:definition "Relates a person, family, or corporate body responsible for assembling, arranging, and trimming film, video, or other moving image formats, including both visual and audio aspects to the expression."@en .

<http://rdaregistry.info/Elements/a/P50184> reg:name "programmerOf"@en ;
	reg:status status:1001 ;
	a rdf:Property ;
	rdfs:domain <http://rdaregistry.info/Elements/c/C10002> ;
	rdfs:isDefinedBy <http://rdaregistry.info/Elements/a/> ;
	rdfs:label "is programmer of"@en ;
	rdfs:range <http://rdaregistry.info/Elements/c/C10001> ;
	rdfs:subPropertyOf <http://rdaregistry.info/Elements/a/P50204> , <http://rdaregistry.info/Elements/u/P60652> ;
	owl:inverseOf <http://rdaregistry.info/Elements/w/P10050> ;
	owl:sameAs <http://rdaregistry.info/Elements/a/programmerOf> ;
	skos:definition "Relates a person, family, or corporate body responsible for creating a computer program to the work."@en .

<http://rdaregistry.info/Elements/a/P50185> reg:name "designerOf"@en ;
	reg:status status:1001 ;
	a rdf:Property ;
	rdfs:domain <http://rdaregistry.info/Elements/c/C10002> ;
	rdfs:isDefinedBy <http://rdaregistry.info/Elements/a/> ;
	rdfs:label "is designer of"@en ;
	rdfs:range <http://rdaregistry.info/Elements/c/C10001> ;
	rdfs:subPropertyOf <http://rdaregistry.info/Elements/a/P50204> , <http://rdaregistry.info/Elements/u/P60653> ;
	owl:inverseOf <http://rdaregistry.info/Elements/w/P10051> ;
	owl:sameAs <http://rdaregistry.info/Elements/a/designerOf> ;
	skos:definition "Relates a person, family, or corporate body responsible for creating a design for an object to the work."@en .

<http://rdaregistry.info/Elements/a/P50186> reg:name "cartographerOf"@en ;
	reg:status status:1001 ;
	a rdf:Property ;
	rdfs:domain <http://rdaregistry.info/Elements/c/C10002> ;
	rdfs:isDefinedBy <http://rdaregistry.info/Elements/a/> ;
	rdfs:label "is cartographer of"@en ;
	rdfs:range <http://rdaregistry.info/Elements/c/C10001> ;
	rdfs:subPropertyOf <http://rdaregistry.info/Elements/a/P50204> , <http://rdaregistry.info/Elements/u/P60654> ;
	owl:inverseOf <http://rdaregistry.info/Elements/w/P10052> ;
	owl:sameAs <http://rdaregistry.info/Elements/a/cartographerOf> ;
	skos:definition "Relates a person, family, or corporate body responsible for creating a map, atlas, globe, or other cartographic work to the work."@en .

<http://rdaregistry.info/Elements/a/P50187> reg:name "composerOf"@en ;
	reg:status status:1001 ;
	a rdf:Property ;
	rdfs:domain <http://rdaregistry.info/Elements/c/C10002> ;
	rdfs:isDefinedBy <http://rdaregistry.info/Elements/a/> ;
	rdfs:label "is composer of"@en ;
	rdfs:range <http://rdaregistry.info/Elements/c/C10001> ;
	rdfs:subPropertyOf <http://rdaregistry.info/Elements/a/P50204> , <http://rdaregistry.info/Elements/u/P60655> ;
	owl:inverseOf <http://rdaregistry.info/Elements/w/P10053> ;
	owl:sameAs <http://rdaregistry.info/Elements/a/composerOf> ;
	skos:definition "Relates a person, family, or corporate body responsible for creating a musical work to the work."@en .

<http://rdaregistry.info/Elements/a/P50188> reg:name "inventorOf"@en ;
	reg:status status:1001 ;
	a rdf:Property ;
	rdfs:domain <http://rdaregistry.info/Elements/c/C10002> ;
	rdfs:isDefinedBy <http://rdaregistry.info/Elements/a/> ;
	rdfs:label "is inventor of"@en ;
	rdfs:range <http://rdaregistry.info/Elements/c/C10001> ;
	rdfs:subPropertyOf <http://rdaregistry.info/Elements/a/P50204> , <http://rdaregistry.info/Elements/u/P60656> ;
	owl:inverseOf <http://rdaregistry.info/Elements/w/P10054> ;
	owl:sameAs <http://rdaregistry.info/Elements/a/inventorOf> ;
	skos:definition "Relates a person, family, or corporate body responsible for creating a new device or process to the work."@en .

<http://rdaregistry.info/Elements/a/P50189> reg:name "compilerOf"@en ;
	reg:status status:1001 ;
	a rdf:Property ;
	rdfs:domain <http://rdaregistry.info/Elements/c/C10002> ;
	rdfs:isDefinedBy <http://rdaregistry.info/Elements/a/> ;
	rdfs:label "is compiler of"@en ;
	rdfs:range <http://rdaregistry.info/Elements/c/C10001> ;
	rdfs:subPropertyOf <http://rdaregistry.info/Elements/a/P50204> , <http://rdaregistry.info/Elements/u/P60657> ;
	owl:inverseOf <http://rdaregistry.info/Elements/w/P10055> ;
	owl:sameAs <http://rdaregistry.info/Elements/a/compilerOf> ;
	skos:definition "Relates a person, family, or corporate body responsible for creating a new work (e.g., a bibliography, a directory) by selecting, arranging, aggregating, and editing data, information, etc. to the work."@en .

<http://rdaregistry.info/Elements/a/P50190> reg:name "photographerOf"@en ;
	reg:status status:1001 ;
	a rdf:Property ;
	rdfs:domain <http://rdaregistry.info/Elements/c/C10002> ;
	rdfs:isDefinedBy <http://rdaregistry.info/Elements/a/> ;
	rdfs:label "is photographer of"@en ;
	rdfs:range <http://rdaregistry.info/Elements/c/C10001> ;
	rdfs:subPropertyOf <http://rdaregistry.info/Elements/a/P50204> , <http://rdaregistry.info/Elements/u/P60658> ;
	owl:inverseOf <http://rdaregistry.info/Elements/w/P10056> ;
	owl:sameAs <http://rdaregistry.info/Elements/a/photographerOf> ;
	skos:definition "Relates a person, family, or corporate body responsible for creating a photographic work to the work."@en .

<http://rdaregistry.info/Elements/a/P50191> reg:name "interviewerOf"@en ;
	reg:status status:1001 ;
	a rdf:Property ;
	rdfs:domain <http://rdaregistry.info/Elements/c/C10002> ;
	rdfs:isDefinedBy <http://rdaregistry.info/Elements/a/> ;
	rdfs:label "is interviewer of"@en ;
	rdfs:range <http://rdaregistry.info/Elements/c/C10001> ;
	rdfs:subPropertyOf <http://rdaregistry.info/Elements/a/P50204> , <http://rdaregistry.info/Elements/u/P60659> ;
	owl:inverseOf <http://rdaregistry.info/Elements/w/P10057> ;
	owl:sameAs <http://rdaregistry.info/Elements/a/interviewerOf> ;
	skos:definition "Relates a person, family, or corporate body responsible for creating a work by acting as an interviewer, reporter, pollster, or some other information gathering agent to the work."@en .

<http://rdaregistry.info/Elements/a/P50192> reg:hasSubproperty <http://rdaregistry.info/Elements/a/P50222> ;
	reg:name "artistOf"@en ;
	reg:status status:1001 ;
	a rdf:Property ;
	rdfs:domain <http://rdaregistry.info/Elements/c/C10002> ;
	rdfs:isDefinedBy <http://rdaregistry.info/Elements/a/> ;
	rdfs:label "is artist of"@en ;
	rdfs:range <http://rdaregistry.info/Elements/c/C10001> ;
	rdfs:subPropertyOf <http://rdaregistry.info/Elements/a/P50204> , <http://rdaregistry.info/Elements/u/P60660> ;
	owl:inverseOf <http://rdaregistry.info/Elements/w/P10058> ;
	owl:sameAs <http://rdaregistry.info/Elements/a/artistOf> ;
	skos:definition "Relates a person, family, or corporate body responsible for creating a work by conceiving, and often implementing, an original graphic design, drawing, painting, etc. to the work."@en .

<http://rdaregistry.info/Elements/a/P50193> reg:name "intervieweeOf"@en ;
	reg:status status:1001 ;
	a rdf:Property ;
	rdfs:domain <http://rdaregistry.info/Elements/c/C10002> ;
	rdfs:isDefinedBy <http://rdaregistry.info/Elements/a/> ;
	rdfs:label "is interviewee of"@en ;
	rdfs:range <http://rdaregistry.info/Elements/c/C10001> ;
	rdfs:subPropertyOf <http://rdaregistry.info/Elements/a/P50204> , <http://rdaregistry.info/Elements/u/P60661> ;
	owl:inverseOf <http://rdaregistry.info/Elements/w/P10059> ;
	owl:sameAs <http://rdaregistry.info/Elements/a/intervieweeOf> ;
	skos:definition "Relates a person, family, or corporate body responsible for creating a work by responding to an interviewer, usually a reporter, pollster, or some other information gathering agent to the work."@en .

<http://rdaregistry.info/Elements/a/P50194> reg:name "choreographerOf"@en ;
	reg:status status:1001 ;
	a rdf:Property ;
	rdfs:domain <http://rdaregistry.info/Elements/c/C10002> ;
	rdfs:isDefinedBy <http://rdaregistry.info/Elements/a/> ;
	rdfs:label "is choreographer of"@en ;
	rdfs:range <http://rdaregistry.info/Elements/c/C10001> ;
	rdfs:subPropertyOf <http://rdaregistry.info/Elements/a/P50204> , <http://rdaregistry.info/Elements/u/P60662> ;
	owl:inverseOf <http://rdaregistry.info/Elements/w/P10060> ;
	owl:sameAs <http://rdaregistry.info/Elements/a/choreographerOf> ;
	skos:definition "Relates a person, family, or corporate body responsible for creating a work of movement to the work."@en .

<http://rdaregistry.info/Elements/a/P50195> reg:hasSubproperty <http://rdaregistry.info/Elements/a/P50223> , <http://rdaregistry.info/Elements/a/P50224> , <http://rdaregistry.info/Elements/a/P50225> ;
	reg:name "authorOf"@en ;
	reg:status status:1001 ;
	a rdf:Property ;
	rdfs:domain <http://rdaregistry.info/Elements/c/C10002> ;
	rdfs:isDefinedBy <http://rdaregistry.info/Elements/a/> ;
	rdfs:label "is author of"@en ;
	rdfs:range <http://rdaregistry.info/Elements/c/C10001> ;
	rdfs:subPropertyOf <http://rdaregistry.info/Elements/a/P50204> , <http://rdaregistry.info/Elements/u/P60663> ;
	owl:inverseOf <http://rdaregistry.info/Elements/w/P10061> ;
	owl:sameAs <http://rdaregistry.info/Elements/a/authorOf> ;
	skos:definition "Relates a person, family, or corporate body responsible for creating a work that is primarily textual in content, regardless of media  type (e.g., printed text, spoken word, electronic text, tactile text) or genre (e.g., poems, novels, screenplays, blogs) to the work."@en .

<http://rdaregistry.info/Elements/a/P50196> reg:hasSubproperty <http://rdaregistry.info/Elements/a/P50221> ;
	reg:name "architectOf"@en ;
	reg:status status:1001 ;
	a rdf:Property ;
	rdfs:domain <http://rdaregistry.info/Elements/c/C10002> ;
	rdfs:isDefinedBy <http://rdaregistry.info/Elements/a/> ;
	rdfs:label "is architect of"@en ;
	rdfs:range <http://rdaregistry.info/Elements/c/C10001> ;
	rdfs:subPropertyOf <http://rdaregistry.info/Elements/a/P50204> , <http://rdaregistry.info/Elements/u/P60664> ;
	owl:inverseOf <http://rdaregistry.info/Elements/w/P10062> ;
	owl:sameAs <http://rdaregistry.info/Elements/a/architectOf> ;
	skos:definition "Relates a person, family, or corporate body responsible for creating an architectural design, including a pictorial representation intended to show how a building, etc. to the work."@en .

<http://rdaregistry.info/Elements/a/P50197> reg:name "filmmakerOf"@en ;
	reg:status status:1001 ;
	a rdf:Property ;
	rdfs:domain <http://rdaregistry.info/Elements/c/C10002> ;
	rdfs:isDefinedBy <http://rdaregistry.info/Elements/a/> ;
	rdfs:label "is filmmaker of"@en ;
	rdfs:range <http://rdaregistry.info/Elements/c/C10001> ;
	rdfs:subPropertyOf <http://rdaregistry.info/Elements/a/P50204> , <http://rdaregistry.info/Elements/u/P60665> ;
	owl:inverseOf <http://rdaregistry.info/Elements/w/P10063> ;
	owl:sameAs <http://rdaregistry.info/Elements/a/filmmakerOf> ;
	skos:definition "Relates a person, family, or corporate body responsible for creating an independent or personal film to the work."@en ;
	skos:scopeNote "A filmmaker is individually responsible for the conception and execution of all aspects of the film."@en .

<http://rdaregistry.info/Elements/a/P50198> reg:name "productionDesignerOf"@en ;
	reg:status status:1001 ;
	a rdf:Property ;
	rdfs:domain <http://rdaregistry.info/Elements/c/C10002> ;
	rdfs:isDefinedBy <http://rdaregistry.info/Elements/a/> ;
	rdfs:label "is production designer of"@en ;
	rdfs:range <http://rdaregistry.info/Elements/c/C10006> ;
	rdfs:subPropertyOf <http://rdaregistry.info/Elements/a/P50161> , <http://rdaregistry.info/Elements/u/P60666> ;
	owl:inverseOf <http://rdaregistry.info/Elements/e/P20056> ;
	owl:sameAs <http://rdaregistry.info/Elements/a/productionDesignerOf> ;
	skos:definition "Relates a person, family, or corporate body responsible for designing the overall visual appearance of a moving image production to the expression."@en .

<http://rdaregistry.info/Elements/a/P50199> reg:hasSubproperty <http://rdaregistry.info/Elements/a/P50169> ;
	reg:name "distributorOf"@en ;
	reg:status status:1001 ;
	a rdf:Property ;
	rdfs:domain <http://rdaregistry.info/Elements/c/C10002> ;
	rdfs:isDefinedBy <http://rdaregistry.info/Elements/a/> ;
	rdfs:label "is distributor of"@en ;
	rdfs:range <http://rdaregistry.info/Elements/c/C10007> ;
	rdfs:subPropertyOf <http://rdaregistry.info/Elements/u/P60667> ;
	owl:inverseOf <http://rdaregistry.info/Elements/m/P30080> ;
	owl:sameAs <http://rdaregistry.info/Elements/a/distributorOf> ;
	skos:definition "Relates a person, family, or corporate body responsible for distributing a resource to the manifestation."@en .

<http://rdaregistry.info/Elements/a/P50200> reg:name "producerOfAnUnpublishedResourceOf"@en ;
	reg:status status:1001 ;
	a rdf:Property ;
	rdfs:domain <http://rdaregistry.info/Elements/c/C10002> ;
	rdfs:isDefinedBy <http://rdaregistry.info/Elements/a/> ;
	rdfs:label "is producer of an unpublished resource of"@en ;
	rdfs:range <http://rdaregistry.info/Elements/c/C10007> ;
	owl:inverseOf <http://rdaregistry.info/Elements/m/P30081> ;
	owl:sameAs <http://rdaregistry.info/Elements/a/producerOfAnUnpublishedResourceOf> ;
	skos:definition "Relates a person, family, or corporate body responsible for inscribing, fabricating, constructing, etc to the manifestation."@en .

<http://rdaregistry.info/Elements/a/P50201> reg:hasSubproperty <http://rdaregistry.info/Elements/a/P50213> , <http://rdaregistry.info/Elements/a/P50214> , <http://rdaregistry.info/Elements/a/P50215> ;
	reg:name "producerOf"@en ;
	reg:status status:1001 ;
	a rdf:Property ;
	rdfs:domain <http://rdaregistry.info/Elements/c/C10002> ;
	rdfs:isDefinedBy <http://rdaregistry.info/Elements/a/> ;
	rdfs:label "is producer of"@en ;
	rdfs:range <http://rdaregistry.info/Elements/c/C10001> ;
	rdfs:subPropertyOf <http://rdaregistry.info/Elements/a/P50131> , <http://rdaregistry.info/Elements/u/P60668> ;
	owl:inverseOf <http://rdaregistry.info/Elements/w/P10064> ;
	owl:sameAs <http://rdaregistry.info/Elements/a/producerOf> ;
	skos:definition "Relates a person, family, or corporate body responsible for most of the business aspects of a production for screen, sound recording, television, webcast, etc to the work."@en ;
	skos:scopeNote "The producer is generally responsible for fund raising, managing the production, hiring key personnel, arranging for distributors, etc."@en .

<http://rdaregistry.info/Elements/a/P50202> reg:hasSubproperty <http://rdaregistry.info/Elements/a/P50170> , <http://rdaregistry.info/Elements/a/P50171> , <http://rdaregistry.info/Elements/a/P50172> , <http://rdaregistry.info/Elements/a/P50173> , <http://rdaregistry.info/Elements/a/P50174> , <http://rdaregistry.info/Elements/a/P50175> , <http://rdaregistry.info/Elements/a/P50176> , <http://rdaregistry.info/Elements/a/P50177> , <http://rdaregistry.info/Elements/a/P50178> , <http://rdaregistry.info/Elements/a/P50179> ;
	reg:name "manufacturerOf"@en ;
	reg:status status:1001 ;
	a rdf:Property ;
	rdfs:domain <http://rdaregistry.info/Elements/c/C10002> ;
	rdfs:isDefinedBy <http://rdaregistry.info/Elements/a/> ;
	rdfs:label "is manufacturer of"@en ;
	rdfs:range <http://rdaregistry.info/Elements/c/C10007> ;
	rdfs:subPropertyOf <http://rdaregistry.info/Elements/u/P60669> ;
	owl:inverseOf <http://rdaregistry.info/Elements/m/P30082> ;
	owl:sameAs <http://rdaregistry.info/Elements/a/manufacturerOf> ;
	skos:definition "Relates a person, family, or corporate body responsible for printing, duplicating, casting, etc to the manifestation."@en .

<http://rdaregistry.info/Elements/a/P50203> reg:hasSubproperty <http://rdaregistry.info/Elements/a/P50168> ;
	reg:name "publisherOf"@en ;
	reg:status status:1001 ;
	a rdf:Property ;
	rdfs:domain <http://rdaregistry.info/Elements/c/C10002> ;
	rdfs:isDefinedBy <http://rdaregistry.info/Elements/a/> ;
	rdfs:label "is publisher of"@en ;
	rdfs:range <http://rdaregistry.info/Elements/c/C10007> ;
	rdfs:subPropertyOf <http://rdaregistry.info/Elements/u/:P60670> ;
	owl:inverseOf <http://rdaregistry.info/Elements/m/P30083> ;
	owl:sameAs <http://rdaregistry.info/Elements/a/publisherOf> ;
	skos:definition "Relates a person, family, or corporate body responsible for publishing, releasing, or issuing a resource to the manifestation."@en .

<http://rdaregistry.info/Elements/a/P50204> reg:hasSubproperty <http://rdaregistry.info/Elements/a/P50068> , <http://rdaregistry.info/Elements/a/P50127> , <http://rdaregistry.info/Elements/a/P50184> , <http://rdaregistry.info/Elements/a/P50185> , <http://rdaregistry.info/Elements/a/P50186> , <http://rdaregistry.info/Elements/a/P50187> , <http://rdaregistry.info/Elements/a/P50188> , <http://rdaregistry.info/Elements/a/P50189> , <http://rdaregistry.info/Elements/a/P50190> , <http://rdaregistry.info/Elements/a/P50191> , <http://rdaregistry.info/Elements/a/P50192> , <http://rdaregistry.info/Elements/a/P50193> , <http://rdaregistry.info/Elements/a/P50194> , <http://rdaregistry.info/Elements/a/P50195> , <http://rdaregistry.info/Elements/a/P50196> , <http://rdaregistry.info/Elements/a/P50197> ;
	reg:name "creatorOf"@en ;
	reg:status status:1001 ;
	a rdf:Property ;
	rdfs:domain <http://rdaregistry.info/Elements/c/C10002> ;
	rdfs:isDefinedBy <http://rdaregistry.info/Elements/a/> ;
	rdfs:label "is creator of"@en ;
	rdfs:range <http://rdaregistry.info/Elements/c/C10001> ;
	rdfs:subPropertyOf <http://rdaregistry.info/Elements/u/P60672> ;
	owl:inverseOf <http://rdaregistry.info/Elements/w/P10065> ;
	owl:sameAs <http://rdaregistry.info/Elements/a/creatorOf> ;
	skos:definition "Relates a person, family, or corporate body responsible for the creation of a work to the work."@en .

<http://rdaregistry.info/Elements/a/P50205> reg:hasSubproperty <http://rdaregistry.info/Elements/a/P50048> , <http://rdaregistry.info/Elements/a/P50049> , <http://rdaregistry.info/Elements/a/P50050> ;
	reg:name "directorOf"@en ;
	reg:status status:1001 ;
	a rdf:Property ;
	rdfs:domain <http://rdaregistry.info/Elements/c/C10002> ;
	rdfs:isDefinedBy <http://rdaregistry.info/Elements/a/> ;
	rdfs:label "is director of"@en ;
	rdfs:range <http://rdaregistry.info/Elements/c/C10001> ;
	rdfs:subPropertyOf <http://rdaregistry.info/Elements/a/P50131> , <http://rdaregistry.info/Elements/u/P60673> ;
	owl:inverseOf <http://rdaregistry.info/Elements/w/P10066> ;
	owl:sameAs <http://rdaregistry.info/Elements/a/directorOf> ;
	skos:definition "Relates a person, family, or corporate body responsible for the general management and supervision of a filmed performance, a radio or television program, etc. to the work."@en .

<http://rdaregistry.info/Elements/a/P50206> reg:name "restorationistOf"@en ;
	reg:status status:1001 ;
	a rdf:Property ;
	rdfs:domain <http://rdaregistry.info/Elements/c/C10002> ;
	rdfs:isDefinedBy <http://rdaregistry.info/Elements/a/> ;
	rdfs:label "is restorationist of"@en ;
	rdfs:range <http://rdaregistry.info/Elements/c/C10003> ;
	rdfs:subPropertyOf <http://rdaregistry.info/Elements/a/P50182> , <http://rdaregistry.info/Elements/u/P60674> ;
	owl:inverseOf <http://rdaregistry.info/Elements/i/P40024> ;
	owl:sameAs <http://rdaregistry.info/Elements/a/restorationistOf> ;
	skos:definition "Relates a person, family, or corporate body responsible for the set of technical, editorial, and intellectual procedures aimed at compensating for the degradation of an item by bringing it back to a state as close as possible to its original condition to the item."@en .

<http://rdaregistry.info/Elements/a/P50207> reg:name "directorOfPhotographyOf"@en ;
	reg:status status:1001 ;
	a rdf:Property ;
	rdfs:domain <http://rdaregistry.info/Elements/c/C10002> ;
	rdfs:isDefinedBy <http://rdaregistry.info/Elements/a/> ;
	rdfs:label "is director of photography of"@en ;
	rdfs:range <http://rdaregistry.info/Elements/c/C10001> ;
	rdfs:subPropertyOf <http://rdaregistry.info/Elements/a/P50131> , <http://rdaregistry.info/Elements/u/P60678> ;
	owl:inverseOf <http://rdaregistry.info/Elements/w/P10068> ;
	owl:sameAs <http://rdaregistry.info/Elements/a/directorOfPhotographyOf> ;
	skos:definition "Relates a person, family, or corporate body that captures images, either electronically or on film or video stock, and often selects and arranges the lighting to the work."@en ;
	skos:scopeNote "The director of photography for a movie is also called the chief cinematographer."@en .

<http://rdaregistry.info/Elements/a/P50208> reg:name "dedicateeOf"@en ;
	reg:status status:1001 ;
	a rdf:Property ;
	rdfs:domain <http://rdaregistry.info/Elements/c/C10002> ;
	rdfs:isDefinedBy <http://rdaregistry.info/Elements/a/> ;
	rdfs:label "is dedicatee of"@en ;
	rdfs:range <http://rdaregistry.info/Elements/c/C10001> ;
	rdfs:subPropertyOf <http://rdaregistry.info/Elements/a/P50131> , <http://rdaregistry.info/Elements/u/P60689> ;
	owl:inverseOf <http://rdaregistry.info/Elements/w/P10069> ;
	owl:sameAs <http://rdaregistry.info/Elements/a/dedicateeOf> ;
	skos:definition "Relates a person, family, or corporate body to whom a work is dedicated to the work."@en .

<http://rdaregistry.info/Elements/a/P50209> reg:name "addresseeOf"@en ;
	reg:status status:1001 ;
	a rdf:Property ;
	rdfs:domain <http://rdaregistry.info/Elements/c/C10002> ;
	rdfs:isDefinedBy <http://rdaregistry.info/Elements/a/> ;
	rdfs:label "is addressee of"@en ;
	rdfs:range <http://rdaregistry.info/Elements/c/C10001> ;
	rdfs:subPropertyOf <http://rdaregistry.info/Elements/a/P50131> , <http://rdaregistry.info/Elements/u/P60690> ;
	owl:inverseOf <http://rdaregistry.info/Elements/w/P10070> ;
	owl:sameAs <http://rdaregistry.info/Elements/a/addresseeOf> ;
	skos:definition "Relates a person, family, or corporate body to whom a work or part of a work is addressed to the work."@en .

<http://rdaregistry.info/Elements/a/P50210> reg:name "dedicateeOfItemOf"@en ;
	reg:status status:1001 ;
	a rdf:Property ;
	rdfs:domain <http://rdaregistry.info/Elements/c/C10002> ;
	rdfs:isDefinedBy <http://rdaregistry.info/Elements/a/> ;
	rdfs:label "is dedicatee (item) of"@en ;
	rdfs:range <http://rdaregistry.info/Elements/c/C10003> ;
	rdfs:subPropertyOf <http://rdaregistry.info/Elements/a/P50182> , <http://rdaregistry.info/Elements/u/P60689> ;
	owl:inverseOf <http://rdaregistry.info/Elements/i/P40025> ;
	owl:sameAs <http://rdaregistry.info/Elements/a/dedicateeOfItemOf> ;
	skos:definition "Relates a person, family, or corporate body to whom an item is dedicated to the item."@en .

<http://rdaregistry.info/Elements/a/P50211> reg:name "consultantOf"@en ;
	reg:status status:1001 ;
	a rdf:Property ;
	rdfs:domain <http://rdaregistry.info/Elements/c/C10002> ;
	rdfs:isDefinedBy <http://rdaregistry.info/Elements/a/> ;
	rdfs:label "is consultant of"@en ;
	rdfs:range <http://rdaregistry.info/Elements/c/C10001> ;
	rdfs:subPropertyOf <http://rdaregistry.info/Elements/a/P50131> , <http://rdaregistry.info/Elements/u/P60701> ;
	owl:inverseOf <http://rdaregistry.info/Elements/w/P10071> ;
	owl:sameAs <http://rdaregistry.info/Elements/a/consultantOf> ;
	skos:definition "Relates a person, family, or corporate body who provides consultation services, and often makes recommendations, for another person, family or corporate body that is represented as the creator of a work to the work."@en .

<http://rdaregistry.info/Elements/a/P50212> reg:name "minuteTakerOf"@en ;
	reg:status status:1001 ;
	a rdf:Property ;
	rdfs:domain <http://rdaregistry.info/Elements/c/C10002> ;
	rdfs:isDefinedBy <http://rdaregistry.info/Elements/a/> ;
	rdfs:label "is minute taker of"@en ;
	rdfs:range <http://rdaregistry.info/Elements/c/C10006> ;
	rdfs:subPropertyOf <http://rdaregistry.info/Elements/a/P50161> , <http://rdaregistry.info/Elements/u/P60671> ;
	owl:inverseOf <http://rdaregistry.info/Elements/e/P20058> ;
	owl:sameAs <http://rdaregistry.info/Elements/a/minuteTakerOf> ;
	skos:definition "Relates a person, family, or corporate body, responsible for recording the minutes of a meeting to the expression."@en .

<http://rdaregistry.info/Elements/a/P50213> reg:name "filmProducerOf"@en ;
	reg:status status:1001 ;
	a rdf:Property ;
	rdfs:domain <http://rdaregistry.info/Elements/c/C10002> ;
	rdfs:isDefinedBy <http://rdaregistry.info/Elements/a/> ;
	rdfs:label "is film producer of"@en ;
	rdfs:range <http://rdaregistry.info/Elements/c/C10001> ;
	rdfs:subPropertyOf <http://rdaregistry.info/Elements/a/P50201> , <http://rdaregistry.info/Elements/u/P60033> ;
	owl:inverseOf <http://rdaregistry.info/Elements/w/P10073> ;
	owl:sameAs <http://rdaregistry.info/Elements/a/filmProducerOf> ;
	skos:definition "Relates a producer responsible for most of the business aspects of a film to the work."@en .

<http://rdaregistry.info/Elements/a/P50214> reg:name "radioProducerOf"@en ;
	reg:status status:1001 ;
	a rdf:Property ;
	rdfs:domain <http://rdaregistry.info/Elements/c/C10002> ;
	rdfs:isDefinedBy <http://rdaregistry.info/Elements/a/> ;
	rdfs:label "is radio producer of"@en ;
	rdfs:range <http://rdaregistry.info/Elements/c/C10001> ;
	rdfs:subPropertyOf <http://rdaregistry.info/Elements/a/P50201> , <http://rdaregistry.info/Elements/u/P60034> ;
	owl:inverseOf <http://rdaregistry.info/Elements/w/P10074> ;
	owl:sameAs <http://rdaregistry.info/Elements/a/radioProducerOf> ;
	skos:definition "Relates a producer responsible for most of the business aspects of a radio program to the work."@en .

<http://rdaregistry.info/Elements/a/P50215> reg:name "televisionProducerOf"@en ;
	reg:status status:1001 ;
	a rdf:Property ;
	rdfs:domain <http://rdaregistry.info/Elements/c/C10002> ;
	rdfs:isDefinedBy <http://rdaregistry.info/Elements/a/> ;
	rdfs:label "is television producer of"@en ;
	rdfs:range <http://rdaregistry.info/Elements/c/C10001> ;
	rdfs:subPropertyOf <http://rdaregistry.info/Elements/a/P50201> , <http://rdaregistry.info/Elements/u/P60035> ;
	owl:inverseOf <http://rdaregistry.info/Elements/w/P10075> ;
	owl:sameAs <http://rdaregistry.info/Elements/a/televisionProducerOf> ;
	skos:definition "Relates a producer responsible for most of the business aspects of a television program to the work."@en .

<http://rdaregistry.info/Elements/a/P50216> reg:name "writerOfAddedLyricsOf"@en ;
	reg:status status:1001 ;
	a rdf:Property ;
	rdfs:domain <http://rdaregistry.info/Elements/c/C10002> ;
	rdfs:isDefinedBy <http://rdaregistry.info/Elements/a/> ;
	rdfs:label "is writer of added lyrics of"@en ;
	rdfs:range <http://rdaregistry.info/Elements/c/C10006> ;
	rdfs:subPropertyOf <http://rdaregistry.info/Elements/a/P50138> , <http://rdaregistry.info/Elements/u/P60600> ;
	owl:inverseOf <http://rdaregistry.info/Elements/e/P20068> ;
	owl:sameAs <http://rdaregistry.info/Elements/a/writerOfAddedLyricsOf> ;
	skos:definition "Relates a writer of words added to an expression of a musical work to the expression."@en .

<http://rdaregistry.info/Elements/a/P50217> reg:name "voiceActorOf"@en ;
	reg:status status:1001 ;
	a rdf:Property ;
	rdfs:domain <http://rdaregistry.info/Elements/c/C10002> ;
	rdfs:isDefinedBy <http://rdaregistry.info/Elements/a/> ;
	rdfs:label "is voice actor of"@en ;
	rdfs:range <http://rdaregistry.info/Elements/c/C10006> ;
	rdfs:subPropertyOf <http://rdaregistry.info/Elements/a/P50071> , <http://rdaregistry.info/Elements/u/P60027> ;
	owl:inverseOf <http://rdaregistry.info/Elements/e/P20070> ;
	owl:sameAs <http://rdaregistry.info/Elements/a/voiceActorOf> ;
	skos:definition "Relates an actor contributing to an expression of a work by providing the voice for characters in radio and audio productions and for animated characters in moving image works, as well as by providing voice-overs in radio and television commercials, dubbed resources, etc to the expression."@en .

<http://rdaregistry.info/Elements/a/P50218> reg:name "relatedCorporateBody"@en ;
	reg:status status:1001 ;
	a rdf:Property ;
	rdfs:domain <http://rdaregistry.info/Elements/c/C10002> ;
	rdfs:isDefinedBy <http://rdaregistry.info/Elements/a/> ;
	rdfs:label "has related corporate body"@en ;
	rdfs:range <http://rdaregistry.info/Elements/c/C10005> ;
	rdfs:subPropertyOf <http://rdaregistry.info/Elements/u/P60454> ;
	owl:sameAs <http://rdaregistry.info/Elements/a/relatedCorporateBody> ;
	skos:definition "Relates an agent to a corporate body that is associated with the person, family, or corporate body being identified (e.g., a musical group to which a person belongs, a subsidiary company)."@en ;
	skos:scopeNote "Related corporate bodies include corporate bodies that precede or succeed the corporate body being identified as the result of a change of name."@en .

<http://rdaregistry.info/Elements/a/P50219> reg:name "relatedFamily"@en ;
	reg:status status:1001 ;
	a rdf:Property ;
	rdfs:domain <http://rdaregistry.info/Elements/c/C10002> ;
	rdfs:isDefinedBy <http://rdaregistry.info/Elements/a/> ;
	rdfs:label "has related family"@en ;
	rdfs:range <http://rdaregistry.info/Elements/c/C10008> ;
	rdfs:subPropertyOf <http://rdaregistry.info/Elements/u/P60454> ;
	owl:sameAs <http://rdaregistry.info/Elements/a/relatedFamily> ;
	skos:definition "Relates an agent to a family that is associated with the person, family, or corporate body being identified (e.g., a person's family, a family that owns the controlling interest in a corporate body)."@en .

<http://rdaregistry.info/Elements/a/P50220> reg:name "relatedPerson"@en ;
	reg:status status:1001 ;
	a rdf:Property ;
	rdfs:domain <http://rdaregistry.info/Elements/c/C10002> ;
	rdfs:isDefinedBy <http://rdaregistry.info/Elements/a/> ;
	rdfs:label "has related person"@en ;
	rdfs:range <http://rdaregistry.info/Elements/c/C10004> ;
	rdfs:subPropertyOf <http://rdaregistry.info/Elements/u/P60454> ;
	owl:sameAs <http://rdaregistry.info/Elements/a/relatedPerson> ;
	skos:definition "Relates an agent to a person who is associated with the person, family, or corporate body being identified (e.g., a collaborator, a member of a family, a founder of a corporate body)."@en ;
	skos:scopeNote "Related persons include separate identities established by an individual (either alone or in collaboration with one or more other individuals)."@en .

<http://rdaregistry.info/Elements/a/P50221> reg:name "landscapeArchitectOf"@en ;
	reg:status status:1001 ;
	a rdf:Property ;
	rdfs:domain <http://rdaregistry.info/Elements/c/C10002> ;
	rdfs:isDefinedBy <http://rdaregistry.info/Elements/a/> ;
	rdfs:label "is landscape architect of"@en ;
	rdfs:range <http://rdaregistry.info/Elements/c/C10001> ;
	rdfs:subPropertyOf <http://rdaregistry.info/Elements/a/P50196> , <http://rdaregistry.info/Elements/u/P60704> ;
	owl:inverseOf <http://rdaregistry.info/Elements/w/P10200> ;
	owl:sameAs <http://rdaregistry.info/Elements/a/landscapeArchitectOf> ;
	skos:definition "Relates an architect responsible for creating landscape works to the work."@en .

<http://rdaregistry.info/Elements/a/P50222> reg:name "sculptorOf"@en ;
	reg:status status:1001 ;
	a rdf:Property ;
	rdfs:domain <http://rdaregistry.info/Elements/c/C10002> ;
	rdfs:isDefinedBy <http://rdaregistry.info/Elements/a/> ;
	rdfs:label "is sculptor of"@en ;
	rdfs:range <http://rdaregistry.info/Elements/c/C10001> ;
	rdfs:subPropertyOf <http://rdaregistry.info/Elements/a/P50192> , <http://rdaregistry.info/Elements/u/P60705> ;
	owl:inverseOf <http://rdaregistry.info/Elements/w/P10202> ;
	owl:sameAs <http://rdaregistry.info/Elements/a/sculptorOf> ;
	skos:definition "Relates an artist responsible for creating a three-dimensional work by modeling, carving, or similar technique to the work."@en .

<http://rdaregistry.info/Elements/a/P50223> reg:name "screenwriterOf"@en ;
	reg:status status:1001 ;
	a rdf:Property ;
	rdfs:domain <http://rdaregistry.info/Elements/c/C10002> ;
	rdfs:isDefinedBy <http://rdaregistry.info/Elements/a/> ;
	rdfs:label "is screenwriter of"@en ;
	rdfs:range <http://rdaregistry.info/Elements/c/C10001> ;
	rdfs:subPropertyOf <http://rdaregistry.info/Elements/a/P50195> , <http://rdaregistry.info/Elements/u/P60706> ;
	owl:inverseOf <http://rdaregistry.info/Elements/w/P10203> ;
	owl:sameAs <http://rdaregistry.info/Elements/a/screenwriterOf> ;
	skos:definition "Relates an author of a screenplay, script, or scene to the work."@en .

<http://rdaregistry.info/Elements/a/P50224> reg:name "lyricistOf"@en ;
	reg:status status:1001 ;
	a rdf:Property ;
	rdfs:domain <http://rdaregistry.info/Elements/c/C10002> ;
	rdfs:isDefinedBy <http://rdaregistry.info/Elements/a/> ;
	rdfs:label "is lyricist of"@en ;
	rdfs:range <http://rdaregistry.info/Elements/c/C10001> ;
	rdfs:subPropertyOf <http://rdaregistry.info/Elements/a/P50195> , <http://rdaregistry.info/Elements/u/P60707> ;
	owl:inverseOf <http://rdaregistry.info/Elements/w/P10204> ;
	owl:sameAs <http://rdaregistry.info/Elements/a/lyricistOf> ;
	skos:definition "Relates an author of the words of a popular song, including a song or songs from a musical to the work."@en .

<http://rdaregistry.info/Elements/a/P50225> reg:name "librettistOf"@en ;
	reg:status status:1001 ;
	a rdf:Property ;
	rdfs:domain <http://rdaregistry.info/Elements/c/C10002> ;
	rdfs:isDefinedBy <http://rdaregistry.info/Elements/a/> ;
	rdfs:label "is librettist of"@en ;
	rdfs:range <http://rdaregistry.info/Elements/c/C10001> ;
	rdfs:subPropertyOf <http://rdaregistry.info/Elements/a/P50195> , <http://rdaregistry.info/Elements/u/P60708> ;
	owl:inverseOf <http://rdaregistry.info/Elements/w/P10205> ;
	owl:sameAs <http://rdaregistry.info/Elements/a/librettistOf> ;
	skos:definition "Relates an author of the words of an opera or other musical stage work, or an oratorio to the work."@en .

<http://rdaregistry.info/Elements/a/P50226> reg:name "sponsoringBodyOf"@en ;
	reg:status status:1001 ;
	a rdf:Property ;
	rdfs:domain <http://rdaregistry.info/Elements/c/C10002> ;
	rdfs:isDefinedBy <http://rdaregistry.info/Elements/a/> ;
	rdfs:label "is sponsoring body of"@en ;
	rdfs:range <http://rdaregistry.info/Elements/c/C10001> ;
	rdfs:subPropertyOf <http://rdaregistry.info/Elements/a/P50131> , <http://rdaregistry.info/Elements/u/P60675> ;
	owl:inverseOf <http://rdaregistry.info/Elements/w/P10067> ;
	owl:sameAs <http://rdaregistry.info/Elements/a/sponsoringBodyOf> ;
	skos:definition "Relates a person, family, or corporate body sponsoring some aspect of a work, e.g., funding research, sponsoring an event, to the work."@en .

<http://rdaregistry.info/Elements/a/P50227> reg:name "writerOfAfterwordOf"@en ;
	reg:status status:1001 ;
	a rdf:Property ;
	rdfs:domain <http://rdaregistry.info/Elements/c/C10002> ;
	rdfs:isDefinedBy <http://rdaregistry.info/Elements/a/> ;
	rdfs:label "is writer of afterword of"@en ;
	rdfs:range <http://rdaregistry.info/Elements/c/C10006> ;
	rdfs:subPropertyOf <http://rdaregistry.info/Elements/a/P50154> , <http://rdaregistry.info/Elements/u/P60717> ;
	owl:inverseOf <http://rdaregistry.info/Elements/e/P20237> ;
	owl:sameAs <http://rdaregistry.info/Elements/a/writerOfAfterwordOf> ;
	skos:definition "Relates a person, family, or corporate body contributing to an expression of a work by providing an afterword to the original work to the expression."@en .

<http://rdaregistry.info/Elements/a/P50228> reg:name "writerOfPostfaceOf"@en ;
	reg:status status:1001 ;
	a rdf:Property ;
	rdfs:domain <http://rdaregistry.info/Elements/c/C10002> ;
	rdfs:isDefinedBy <http://rdaregistry.info/Elements/a/> ;
	rdfs:label "is writer of postface of"@en ;
	rdfs:range <http://rdaregistry.info/Elements/c/C10006> ;
	rdfs:subPropertyOf <http://rdaregistry.info/Elements/a/P50154> , <http://rdaregistry.info/Elements/u/P60718> ;
	owl:inverseOf <http://rdaregistry.info/Elements/e/P20238> ;
	owl:sameAs <http://rdaregistry.info/Elements/a/writerOfPostfaceOf> ;
	skos:definition "Relates a person, family, or corporate body contributing to an expression of a work by providing a postface to the original work to the expression."@en .

<http://rdaregistry.info/Elements/a/P50229> reg:name "predecessorOfSplit"@en ;
	reg:status status:1001 ;
	a rdf:Property ;
	rdfs:domain <http://rdaregistry.info/Elements/c/C10005> ;
	rdfs:isDefinedBy <http://rdaregistry.info/Elements/a/> ;
	rdfs:label "has predecessor of split"@en ;
	rdfs:range <http://rdaregistry.info/Elements/c/C10005> ;
	rdfs:subPropertyOf <http://rdaregistry.info/Elements/u/P60733> ;
	owl:inverseOf <http://rdaregistry.info/Elements/a/P50014> ;
	owl:sameAs <http://rdaregistry.info/Elements/a/predecessorOfSplit> ;
	skos:definition "Relates a corporate body to a corporate body that split or divided into the other corporate body."@en .

<http://rdaregistry.info/Elements/a/P50230> reg:name "membershipCorporateBody"@en ;
	reg:status status:1001 ;
	a rdf:Property ;
	rdfs:domain <http://rdaregistry.info/Elements/c/C10005> ;
	rdfs:isDefinedBy <http://rdaregistry.info/Elements/a/> ;
	rdfs:label "has membership corporate body"@en ;
	rdfs:range <http://rdaregistry.info/Elements/c/C10005> ;
	rdfs:subPropertyOf <http://rdaregistry.info/Elements/u/P60648> ;
	owl:inverseOf <http://rdaregistry.info/Elements/a/P50231> ;
	owl:sameAs <http://rdaregistry.info/Elements/a/membershipCorporateBody> ;
	skos:definition "Relates a corporate body to a corporate body formed from the membership of other corporate bodies."@en .

<http://rdaregistry.info/Elements/a/P50231> reg:name "corporateMember"@en ;
	reg:status status:1001 ;
	a rdf:Property ;
	rdfs:domain <http://rdaregistry.info/Elements/c/C10005> ;
	rdfs:isDefinedBy <http://rdaregistry.info/Elements/a/> ;
	rdfs:label "has corporate member"@en ;
	rdfs:range <http://rdaregistry.info/Elements/c/C10005> ;
	rdfs:subPropertyOf <http://rdaregistry.info/Elements/u/P60697> ;
	owl:inverseOf <http://rdaregistry.info/Elements/a/P50230> ;
	owl:sameAs <http://rdaregistry.info/Elements/a/corporateMember> ;
	skos:definition "Relates a corporate body to a corporate body that is a member of the other corporate body."@en .

<http://rdaregistry.info/Elements/a/P50232> reg:name "componentOfAMerger"@en ;
	reg:status status:1001 ;
	a rdf:Property ;
	rdfs:domain <http://rdaregistry.info/Elements/c/C10005> ;
	rdfs:isDefinedBy <http://rdaregistry.info/Elements/a/> ;
	rdfs:label "has component of a merger"@en ;
	rdfs:range <http://rdaregistry.info/Elements/c/C10005> ;
	rdfs:subPropertyOf <http://rdaregistry.info/Elements/u/P60736> ;
	owl:inverseOf <http://rdaregistry.info/Elements/a/P50013> ;
	owl:sameAs <http://rdaregistry.info/Elements/a/componentOfAMerger> ;
	skos:definition "Relates a corporate body to a corporate body that formed the other corporate body by merging with one or more other corporate bodies."@en .

<http://rdaregistry.info/Elements/a/P50233> reg:name "family"@en ;
	reg:status status:1001 ;
	a rdf:Property ;
	rdfs:domain <http://rdaregistry.info/Elements/c/C10004> ;
	rdfs:isDefinedBy <http://rdaregistry.info/Elements/a/> ;
	rdfs:label "has family"@en ;
	rdfs:range <http://rdaregistry.info/Elements/c/C10008> ;
	rdfs:subPropertyOf <http://rdaregistry.info/Elements/u/P60697> ;
	owl:inverseOf <http://rdaregistry.info/Elements/a/P50056> ;
	owl:sameAs <http://rdaregistry.info/Elements/a/family> ;
	skos:definition "Relates a person to a family to which the person belongs."@en .

<http://rdaregistry.info/Elements/a/P50234> reg:name "officiatedCorporateBody"@en ;
	reg:status status:1001 ;
	a rdf:Property ;
	rdfs:domain <http://rdaregistry.info/Elements/c/C10004> ;
	rdfs:isDefinedBy <http://rdaregistry.info/Elements/a/> ;
	rdfs:label "has officiated corporate body"@en ;
	rdfs:range <http://rdaregistry.info/Elements/c/C10005> ;
	rdfs:subPropertyOf <http://rdaregistry.info/Elements/u/P60737> ;
	owl:inverseOf <http://rdaregistry.info/Elements/a/P50027> ;
	owl:sameAs <http://rdaregistry.info/Elements/a/officiatedCorporateBody> ;
	skos:definition "Relates a person to a corporate body in which the person holds an office."@en .

<http://rdaregistry.info/Elements/a/P50235> reg:name "languageOfTheFamily"@en ;
	reg:status status:1001 ;
	a rdf:Property ;
	rdfs:domain <http://rdaregistry.info/Elements/c/C10008> ;
	rdfs:isDefinedBy <http://rdaregistry.info/Elements/a/> ;
	rdfs:label "has language of the family"@en ;
	rdfs:subPropertyOf <http://rdaregistry.info/Elements/u/P60098> ;
	owl:sameAs <http://rdaregistry.info/Elements/a/languageOfTheFamily> ;
	skos:definition "Relates a family to a language a family uses in its communications."@en .

<http://rdaregistry.info/Elements/a/P50236> reg:name "periodOfActivityOfTheCorporateBody"@en ;
	reg:status status:1001 ;
	a rdf:Property ;
	rdfs:domain <http://rdaregistry.info/Elements/c/C10005> ;
	rdfs:isDefinedBy <http://rdaregistry.info/Elements/a/> ;
	rdfs:label "has period of activity of the corporate body"@en ;
	rdfs:subPropertyOf <http://rdaregistry.info/Elements/u/P60076> ;
	owl:sameAs <http://rdaregistry.info/Elements/a/periodOfActivityOfTheCorporateBody> ;
	skos:definition "Relates a corporate body to a date or range of dates indicative of the period in which a corporate body was active."@en .

<http://rdaregistry.info/Elements/a/P50237> reg:name "typeOfCorporateBody"@en ;
	reg:status status:1001 ;
	a rdf:Property ;
	rdfs:domain <http://rdaregistry.info/Elements/c/C10005> ;
	rdfs:isDefinedBy <http://rdaregistry.info/Elements/a/> ;
	rdfs:label "has type of corporate body"@en ;
	rdfs:subPropertyOf <http://rdaregistry.info/Elements/u/P60047> ;
	owl:sameAs <http://rdaregistry.info/Elements/a/typeOfCorporateBody> .

<http://rdaregistry.info/Elements/a/P50238> reg:name "typeOfJurisdiction"@en ;
	reg:status status:1001 ;
	a rdf:Property ;
	rdfs:domain <http://rdaregistry.info/Elements/c/C10005> ;
	rdfs:isDefinedBy <http://rdaregistry.info/Elements/a/> ;
	rdfs:label "has type of jurisdiction"@en ;
	rdfs:subPropertyOf <http://rdaregistry.info/Elements/u/P60047> ;
	owl:sameAs <http://rdaregistry.info/Elements/a/typeOfJurisdiction> .

<http://rdaregistry.info/Elements/a/P50239> reg:name "otherDesignation"@en ;
	reg:status status:1001 ;
	a rdf:Property ;
	rdfs:domain <http://rdaregistry.info/Elements/c/C10005> ;
	rdfs:isDefinedBy <http://rdaregistry.info/Elements/a/> ;
	rdfs:label "has other designation"@en ;
	rdfs:subPropertyOf <http://rdaregistry.info/Elements/u/P60370> ;
	owl:sameAs <http://rdaregistry.info/Elements/a/otherDesignation> .
