@prefix vaem: <http://www.linkedmodel.org/schema/vaem#> .
@prefix dc: <http://purl.org/dc/elements/1.1/> .
@prefix voag: <http://voag.linkedmodel.org/voag#> .
@prefix rdfs: <http://www.w3.org/2000/01/rdf-schema#> .
@prefix xsd: <http://www.w3.org/2001/XMLSchema#> .
@prefix owl: <http://www.w3.org/2002/07/owl#> .
@prefix rdf: <http://www.w3.org/1999/02/22-rdf-syntax-ns#> .

<http://www.linkedmodel.org/schema/vaem> a owl:Ontology ;
	vaem:usesNonImportedResource dc:author .

dc:author a owl:AnnotationProperty ;
	rdfs:label "author"^^xsd:string ;
	rdfs:range xsd:string .

<http://www.linkedmodel.org/schema/vaem> vaem:usesNonImportedResource dc:title .

dc:title a owl:AnnotationProperty ;
	rdfs:label "title"^^xsd:string ;
	rdfs:range xsd:string .

<http://www.linkedmodel.org/schema/vaem> dc:title "Vocabulary for Attaching Essential Metadata"^^xsd:string ;
	vaem:usesNonImportedResource voag:TopQuadrantAttribution .

voag:TopQuadrantAttribution a vaem:Attribution ;
	vaem:description "LinkedModel Ontologies and Vocabularies are issued under a Creative Commons Attribution Share Alike 3.0 United States License. Attribution should be made to TopQuadrant, Inc."^^xsd:string ;
	rdfs:label "TopQuadrant attribution"^^xsd:string .

<http://www.linkedmodel.org/schema/vaem> vaem:revision "1.2"^^xsd:string ;
	vaem:lastUpdated "2013-08-28"^^vaem:dateUnion ;
	vaem:withAttributionTo voag:TopQuadrantAttribution ;
	vaem:usesNonImportedResource dc:description .

dc:description a owl:AnnotationProperty ;
	rdfs:label "description"^^xsd:string ;
	rdfs:range xsd:string .

<http://www.linkedmodel.org/schema/vaem> vaem:description "VAEM stands for \"Vocabulary for Attaching Essential Metadata\". The purpose of VAEM is to provide, by import, a foundation for commonly needed resources when building an ontology. An effort has been made to restrict these resources to a minimal level.   What VAEM regards as 'essential metadata' is data about dates and times, confidentiality, and other characterisitic qualifiers of the ontology, but also references to where a ontology is documented and where to find ontology Governance, Attribution and Provenance. VAEM also defines classes for representing enumerations and enumerated values."^^xsd:string ;
	vaem:namespace "http://www.linkedmodel.org/schema/vaem#"^^xsd:anyURI ;
	vaem:hasCatalogEntry voag:VAEM-CatalogEntry .

voag:VAEM-CatalogEntry a vaem:CatalogEntry ;
	rdfs:label "VAEM catalog entry"^^xsd:string .

<http://www.linkedmodel.org/schema/vaem> rdfs:label "Vocabulary for Attaching Essential Metadata"^^xsd:string ;
	dc:contributor "Irene Polikoff"^^xsd:string ;
	vaem:namespacePrefix "vaem"^^xsd:string ;
	vaem:usesNonImportedResource dc:contributor .

dc:contributor a owl:AnnotationProperty ;
	rdfs:label "contributor"^^xsd:string ;
	rdfs:range xsd:string .

<http://www.linkedmodel.org/schema/vaem> owl:versionInfo "$Id$"^^xsd:string ;
	dc:author "Ralph Hodgson"^^xsd:string ;
	dc:subject "Metadata"^^xsd:string ;
	owl:versionIRI <http://www.linkedmodel.org/schema/vaem> ;
	vaem:usesNonImportedResource voag:VAEM-CatalogEntry ;
	vaem:name "VAEM"^^xsd:string ;
	vaem:dateCreated "2011-04-20"^^vaem:dateUnion ;
	vaem:hasGraphRole vaem:RulesGraph .

vaem:RulesGraph a vaem:GraphRole ;
	rdfs:label "Rules Graph"^^xsd:string .

<http://www.linkedmodel.org/schema/vaem> vaem:usesNonImportedResource dc:subject .

dc:subject a owl:AnnotationProperty ;
	rdfs:label "subject"^^xsd:string ;
	rdfs:range xsd:string .

vaem:dateUnion a rdfs:Datatype ;
	dc:description "A datatype that is the union of date xsd data types. 'dateUnion' is equivalent to the xsd specification that uses an xsd:union of memberTypes='xsd:date xsd:dateTime xsd:float xsd:gYear'."^^xsd:string ;
	rdfs:label "date union"^^xsd:string ;
	rdfs:subClassOf rdfs:Resource ;
	owl:equivalentClass _:node183724kisx42 .

_:node183724kisx42 a rdfs:Datatype ;
	owl:unionOf _:node183724kisx43 .

_:node183724kisx43 rdf:first xsd:date ;
	rdf:rest _:node183724kisx44 .

_:node183724kisx44 rdf:first xsd:dateTime ;
	rdf:rest _:node183724kisx45 .

_:node183724kisx45 rdf:first xsd:gYear ;
	rdf:rest rdf:nil .

vaem:numericUnion a rdfs:Datatype ;
	dc:description "A datatype that is the union of numeric xsd data types. 'numericUnion' is equivalent to the xsd specification that uses an xsd:union of memberTypes='xsd:decimal xsd:double xsd:float xsd:integer'."^^xsd:string ;
	rdfs:label "numeric union"^^xsd:string ;
	rdfs:subClassOf rdfs:Resource ;
	owl:equivalentClass _:node183724kisx46 .

_:node183724kisx46 a rdfs:Datatype ;
	owl:unionOf _:node183724kisx47 .

_:node183724kisx47 rdf:first xsd:float ;
	rdf:rest _:node183724kisx48 .

_:node183724kisx48 rdf:first xsd:decimal ;
	rdf:rest _:node183724kisx49 .

_:node183724kisx49 rdf:first xsd:integer ;
	rdf:rest _:node183724kisx50 .

_:node183724kisx50 rdf:first xsd:double ;
	rdf:rest rdf:nil .

vaem:Attribution a owl:Class ;
	dc:description "A mininal treatment of attribution. This serves as a placeholder class for voag:Attribution."^^xsd:string ;
	rdfs:label "Attribution"^^xsd:string ;
	rdfs:subClassOf owl:Thing , _:node183724kisx51 .

_:node183724kisx51 a owl:Restriction ;
	owl:cardinality "1"^^xsd:nonNegativeInteger ;
	owl:onProperty vaem:description .

vaem:description a owl:DatatypeProperty .

vaem:CatalogEntry a owl:Class ;
	dc:description "VAEM Governed Object class is a placeholder for concepts that are fully defined by the voag:GovernedObject concept hierarchy for building a catalog of ontologies and graphs."^^xsd:string ;
	rdfs:label "Governed object"^^xsd:string ;
	rdfs:subClassOf _:node183724kisx52 .

_:node183724kisx52 a owl:Restriction ;
	owl:minCardinality "1"^^xsd:nonNegativeInteger ;
	owl:onProperty vaem:description .

vaem:LicenseModel a owl:Class ;
	dc:description "The VAEM Licence Model class is a placeholder for concepts that are fully defined by VOAG."^^xsd:string ;
	rdfs:label "License model"^^xsd:string ;
	rdfs:subClassOf _:node183724kisx53 .

_:node183724kisx53 a owl:Restriction ;
	owl:maxCardinality "1"^^xsd:nonNegativeInteger ;
	owl:onProperty vaem:url .

vaem:url a owl:DatatypeProperty .

vaem:LicenseModel rdfs:subClassOf _:node183724kisx54 .

_:node183724kisx54 a owl:Restriction ;
	owl:minCardinality "1"^^xsd:nonNegativeInteger ;
	owl:onProperty vaem:description .

vaem:GraphRole a owl:Class ;
	rdfs:comment "GraphRole is used to characterize how a graph of resources participates in an ontology set.  For example, a graph can be a schema, vocabulary, dataset, script, or ruleset."^^xsd:string ;
	rdfs:label "Graph role"^^xsd:string ;
	rdfs:subClassOf owl:Thing ;
	owl:oneOf _:node183724kisx55 .

_:node183724kisx55 rdf:first vaem:AnnotationsGraph .

vaem:AnnotationsGraph a vaem:GraphRole ;
	rdfs:label "Annotations Graph"^^xsd:string .

_:node183724kisx55 rdf:rest _:node183724kisx56 .

_:node183724kisx56 rdf:first vaem:BridgeGraph .

vaem:BridgeGraph a vaem:GraphRole ;
	rdfs:label "Bridge graph"^^xsd:string .

_:node183724kisx56 rdf:rest _:node183724kisx57 .

_:node183724kisx57 rdf:first vaem:CollectionGraph .

vaem:CollectionGraph a vaem:GraphRole ;
	rdfs:label "Collection graph"^^xsd:string .

_:node183724kisx57 rdf:rest _:node183724kisx58 .

_:node183724kisx58 rdf:first vaem:CurationGraph .

vaem:CurationGraph a vaem:GraphRole ;
	dc:description "A curation graph is one whose purpose is to hold metadata that is needed to describe, govern and provision another graph. A curation graph will likely use VOAG and VAEM for this purpose. The property 'vaem:curationGraph' is used to link to the graph (or graphs) being curated."^^xsd:string ;
	rdfs:label "Curation graph"^^xsd:string .

_:node183724kisx58 rdf:rest _:node183724kisx59 .

_:node183724kisx59 rdf:first vaem:DataGraph .

vaem:DataGraph a vaem:GraphRole ;
	rdfs:label "Data graph"^^xsd:string .

_:node183724kisx59 rdf:rest _:node183724kisx60 .

_:node183724kisx60 rdf:first vaem:FunctionsGraph .

vaem:FunctionsGraph a vaem:GraphRole ;
	rdfs:label "Functions graph"^^xsd:string .

_:node183724kisx60 rdf:rest _:node183724kisx61 .

_:node183724kisx61 rdf:first vaem:MappingGraph .

vaem:MappingGraph a vaem:GraphRole ;
	vaem:description "A graph that specifies a transformation of a graph into another graph or graphs. Invariably this is a SPINMap graph using SPARQL Rules (SPIN) to express the transforms."^^xsd:string ;
	rdfs:label "Mapping graph"^^xsd:string .

_:node183724kisx61 rdf:rest _:node183724kisx62 .

_:node183724kisx62 rdf:first vaem:ProxyGraph .

vaem:ProxyGraph a vaem:GraphRole ;
	rdfs:label "Proxy graph"^^xsd:string .

_:node183724kisx62 rdf:rest _:node183724kisx63 .

_:node183724kisx63 rdf:first vaem:RulesGraph ;
	rdf:rest _:node183724kisx64 .

_:node183724kisx64 rdf:first vaem:SchemaGraph .

vaem:SchemaGraph a vaem:GraphRole ;
	rdfs:label "Schema graph"^^xsd:string .

_:node183724kisx64 rdf:rest _:node183724kisx65 .

_:node183724kisx65 rdf:first vaem:ScriptGraph .

vaem:ScriptGraph a vaem:GraphRole ;
	rdfs:label "Script graph"^^xsd:string .

_:node183724kisx65 rdf:rest _:node183724kisx66 .

_:node183724kisx66 rdf:first vaem:ViewGraph .

vaem:ViewGraph a vaem:GraphRole ;
	rdfs:label "View graph"^^xsd:string .

_:node183724kisx66 rdf:rest _:node183724kisx67 .

_:node183724kisx67 rdf:first vaem:VocabularyGraph .

vaem:VocabularyGraph a vaem:GraphRole ;
	vaem:description "An RDF/OWL Graph that is a controlled set of instances."^^xsd:string ;
	rdfs:label "Vocabulary graph"^^xsd:string .

_:node183724kisx67 rdf:rest rdf:nil .

vaem:withAttributionTo a owl:ObjectProperty ;
	rdfs:label "with attribution to"^^xsd:string .

vaem:reifiableBy a owl:ObjectProperty ;
	rdfs:comment "To express how statements in a model can be reifiable, this property is used to explicitly associate a property with a user-defined sub-class of 'rdf:Statement'. A recommended way of using this is to declare the properties that share the same reification constructs as sub-properties of a parent property that carries the 'vaem:reifiableBy' property. The parent property should be of type 'rdf:Property' so that it can have both datatype and object properties as sub-properties. By this means use and transformations of a model can be understood through a fully specified metamodel. 'vaem:reifiableBy' is rangeless in order to comply with OWL DL semantics. Its range would have been rdfs:Class in order to refer to 'rdf:Statement' sub-classes."^^xsd:string ;
	rdfs:label "reifiable by"^^xsd:string .

vaem:hasGraphRole a owl:ObjectProperty ;
	rdfs:comment "The property 'lms:hasGraphRole' is used to characterize how a resource participates in an ontology set.  The property is used to specify the role that a graph plays, for example, an ontology graph can be a schema, vocabulary, dataset, script, or ruleset."^^xsd:string ;
	rdfs:label "has graph role"^^xsd:string .

vaem:usesNonImportedResource a owl:ObjectProperty ;
	rdfs:comment "A property that is used to express dependencies on resources from graphs that are not imported."^^xsd:string ;
	rdfs:label "uses non-imported resource"^^xsd:string ;
	rdfs:range rdfs:Resource .

vaem:owningParty a owl:ObjectProperty ;
	rdfs:comment "The property 'vaem:owningParty' is used to refer to some concept of 'Party' and is a sub-property of 'vaem:ownedBy'."^^xsd:string ;
	rdfs:label "owning party"^^xsd:string ;
	rdfs:subPropertyOf vaem:ownedBy .

vaem:ownedBy a rdf:Property .

vaem:hasLicenseType a owl:ObjectProperty ;
	rdfs:label "has license type"@en-us .

vaem:hasCatalogEntry a owl:ObjectProperty ;
	rdfs:label "has catalog entry"^^xsd:string .

vaem:isRefinedBy a rdf:Property , owl:AnnotationProperty ;
	rdfs:comment "A refinement of the subject resource. Modelled after rdfs:isDefinedBy for the purpose of referring to layered graphs that further define a subject."^^xsd:string ;
	rdfs:domain rdfs:Resource ;
	rdfs:isDefinedBy <http://www.linkedmodel.org/schema/vaem> ;
	rdfs:label "isRefinedBy"^^xsd:string ;
	rdfs:range rdfs:Resource ;
	rdfs:subPropertyOf rdfs:isDefinedBy .

vaem:ownedBy rdfs:comment "The property 'vaem:ownedBy' is a general property that in some cases could have scalar values or may refer to some concept of 'Party'.  For this reason, the  type of this property is set as 'rdf:Property' and the property is rangeless. There are two sub-properties of 'vaem:ownedBy', namely 'vaem:owner' for string values and 'vaem:owningParty' for referencing a 'party'.  Ownership applies to thos ontologies that are proprietary. Other governance and provenance specifications are held in the VOAG ontology."^^xsd:string ;
	rdfs:label "owned by"^^xsd:string .

vaem:dateCreated a owl:DatatypeProperty ;
	rdfs:comment "The property 'vaem:dateCreated' is intended for general use as the name implies.  The range of the property is set as 'vaem:dateUnion' so as to allow a value to have a number of forms from a  year only to a full timestamp."^^xsd:string ;
	rdfs:label "date created"^^xsd:string ;
	rdfs:range vaem:dateUnion ;
	rdfs:subPropertyOf vaem:date .

vaem:date a owl:DatatypeProperty .

vaem:url dc:description "The property 'vaem:url' is intended for general use as the name implies.  The range of the property is set as an XSD URI."^^xsd:string ;
	rdfs:label "url"^^xsd:string ;
	rdfs:range xsd:anyURI .

vaem:owner a owl:DatatypeProperty ;
	rdfs:label "owner"^^xsd:string ;
	rdfs:range xsd:string ;
	rdfs:subPropertyOf vaem:ownedBy .

vaem:lastUpdated a owl:DatatypeProperty ;
	rdfs:comment "The property 'vaem:lastUpdated' is intended for general use as the name implies.  The range of the property is set as 'vaem:dateUnion' so as to allow a value to have a number of forms from a  year only to a full timestamp."^^xsd:string ;
	rdfs:label "last updated"^^xsd:string ;
	rdfs:range vaem:dateUnion ;
	rdfs:subPropertyOf vaem:date .

vaem:releaseDate a owl:DatatypeProperty ;
	rdfs:comment "The property 'vaem:releaseDate' is intended for general use as the name implies.  The range of the property is set as 'vaem:dateUnion' so as to allow a value to have a number of forms from a  year only to a full timestamp."^^xsd:string ;
	rdfs:label "release date"^^xsd:string ;
	rdfs:range vaem:dateUnion ;
	rdfs:subPropertyOf vaem:date .

vaem:namespace a owl:DatatypeProperty ;
	rdfs:comment "The property 'vaem:namespace' provides a means to specify the onotlogy URI with which a graph is primarily associated. The intent is to allow multiple graphs to define statements for resources in the same Ontology namespace. For example, a foundation level graph with the base URI of 'http://www.somesite.com/1.0/schema/OurOntology'  may define general  concepts for 'OurOntology'. Another graph with the base URI 'http://www.somesite.com/1.0/schema/level2/OurOntology'  may add more specific details to the same 'OurOntology'. Each of these two graphs would carry the same value for 'vaem:namespace', that is, 'http://www.somesite.com/schema/OurOntology'.    In other words, an ontology URI is the URI associated with the resources of a controlled namespace. On the other hand the graph URIs (the base URIs) identify the graphs that hold resources that make up an ontology."^^xsd:string ;
	rdfs:label "namespace"^^xsd:string ;
	rdfs:range xsd:anyURI .

vaem:name a owl:DatatypeProperty ;
	rdfs:comment "The property 'vaem:name' is intended for general use. In many cases 'rdfs:label' could be used give names to resources. In the case where compliance with a specific naming rule is needed,  'vaem:name' allows  a resource to carry a name that is used in more specific contexts. Making 'vaem:name' a sub-property of 'rdfs:label' allows 'vaem:name' to serve in the same way as an 'rdfs:label'."^^xsd:string ;
	rdfs:label "name"^^xsd:string ;
	rdfs:range xsd:string ;
	rdfs:subPropertyOf rdfs:label .

vaem:revision a owl:DatatypeProperty ;
	rdfs:comment "The property 'vaem:revision' is a property intended for general use as the name implies."^^xsd:string ;
	rdfs:label "revision"^^xsd:string ;
	rdfs:range xsd:string .

vaem:description rdfs:comment "The property 'vaem:description' is intended for general use as the name implies.  Unlike 'rdfs:comment',  'vaem:description' is an 'owl:DatatypeProperty'. As such it can play a stronger role in the model, for example, as a predicate in an axiom."^^xsd:string ;
	rdfs:label "description"^^xsd:string ;
	rdfs:range xsd:string .

vaem:namespacePrefix a owl:DatatypeProperty ;
	rdfs:comment "The property 'vaem:namespacePrefix' specifes a short handle or label for the URI of an Ontology.  Multiple graphs can define statements for resources in the same Ontololgy namespace. For example, a foundation level graph with the base URI of 'http://www.somesite.com/1.0/schema/OurOntology'  may define general  concepts for 'OurOntology'. Another graph with the base URI 'http://www.somesite.com/1.0/schema/level2/OurOntology'  may add more specific details to the same 'OurOntology'. Each of these two graphs would carry the same value for 'vaem:namespacePrefix', for this example, perhaps, 'ourOntology'."^^xsd:string ;
	rdfs:label "namespace prefix"^^xsd:string ;
	rdfs:range xsd:string .

vaem:title a owl:DatatypeProperty ;
	rdfs:label "title"^^xsd:string ;
	rdfs:range xsd:string .

vaem:date rdfs:comment "The property 'vaem:date' is intended for general use as the name implies.  The range of the property is set as 'vaem:dateUnion' so as to allow a value to have a number of forms from a  year only to a full timestamp. The property is also the parent of all dates so that queries can be made for any date on an ontology."^^xsd:string ;
	rdfs:label "date"^^xsd:string ;
	rdfs:range vaem:dateUnion .

vaem:comment a owl:AnnotationProperty ;
	rdfs:comment "An annotation property that can be freely used on any kind of resource. The range of the property is 'xsd:string'."^^xsd:string ;
	rdfs:label "definition"^^xsd:string ;
	rdfs:range xsd:string .

vaem:todo a owl:AnnotationProperty ;
	rdfs:comment "As it name implies, a way to attach an annotation about a 'todo' task"^^xsd:string ;
	rdfs:label "todo"^^xsd:string ;
	rdfs:range xsd:string .

voag:CC-SHAREALIKE_3PT0-US a vaem:LicenseModel ;
	rdfs:label "Creative Commons Attribution-Share Alike 3.0 United States License"^^xsd:string .

_:node183724kisx68 a owl:Restriction ;
	owl:maxCardinality "1"^^xsd:nonNegativeInteger ;
	owl:onProperty vaem:lastUpdated .

_:node183724kisx69 a owl:Restriction ;
	owl:maxCardinality "1"^^xsd:nonNegativeInteger ;
	owl:onProperty vaem:owningParty .

_:node183724kisx70 a owl:Restriction ;
	owl:maxCardinality "1"^^xsd:nonNegativeInteger ;
	owl:onProperty vaem:namespace .

_:node183724kisx71 a owl:Restriction ;
	owl:allValuesFrom vaem:Attribution ;
	owl:onProperty vaem:withAttributionTo .

_:node183724kisx72 a owl:Restriction ;
	owl:allValuesFrom vaem:GraphRole ;
	owl:onProperty vaem:hasGraphRole .

_:node183724kisx73 a owl:Restriction ;
	owl:maxCardinality "1"^^xsd:nonNegativeInteger ;
	owl:onProperty vaem:namespacePrefix .

_:node183724kisx74 a owl:Restriction ;
	owl:maxCardinality "1"^^xsd:nonNegativeInteger ;
	owl:onProperty vaem:name .

_:node183724kisx75 a owl:Restriction ;
	owl:maxCardinality "1"^^xsd:nonNegativeInteger ;
	owl:onProperty vaem:dateCreated .

_:node183724kisx76 a owl:Restriction ;
	owl:maxCardinality "1"^^xsd:nonNegativeInteger ;
	owl:onProperty vaem:hasLicenseType .

owl:Ontology rdfs:subClassOf _:node183724kisx73 , _:node183724kisx77 .

_:node183724kisx77 a owl:Restriction ;
	owl:maxCardinality "1"^^xsd:nonNegativeInteger ;
	owl:onProperty vaem:revision .

owl:Ontology rdfs:subClassOf _:node183724kisx76 , _:node183724kisx78 .

_:node183724kisx78 a owl:Restriction ;
	owl:maxCardinality "1"^^xsd:nonNegativeInteger ;
	owl:onProperty vaem:owner .

owl:Ontology rdfs:subClassOf _:node183724kisx79 .

_:node183724kisx79 a owl:Restriction ;
	owl:allValuesFrom rdfs:Resource ;
	owl:onProperty vaem:usesNonImportedResource .

owl:Ontology rdfs:subClassOf _:node183724kisx80 .

_:node183724kisx80 a owl:Restriction ;
	owl:maxCardinality "1"^^xsd:nonNegativeInteger ;
	owl:onProperty vaem:hasCatalogEntry .

owl:Ontology rdfs:subClassOf _:node183724kisx72 , _:node183724kisx74 , _:node183724kisx69 , _:node183724kisx70 , _:node183724kisx81 .

_:node183724kisx81 a owl:Restriction ;
	owl:allValuesFrom xsd:string ;
	owl:onProperty vaem:description .

owl:Ontology rdfs:subClassOf _:node183724kisx71 , _:node183724kisx75 , _:node183724kisx82 .

_:node183724kisx82 a owl:Restriction ;
	owl:allValuesFrom vaem:LicenseModel ;
	owl:onProperty vaem:hasLicenseType .

owl:Ontology rdfs:subClassOf _:node183724kisx68 .
