@prefix rdfs:  <http://www.w3.org/2000/01/rdf-schema#> .
@prefix ns4:   <http://linkeddata.finki.ukim.mk/lod/ontology/tao#> .
@prefix geo:   <http://www.w3.org/2003/01/geo/wgs84_pos#> .
@prefix owl:   <http://www.w3.org/2002/07/owl#> .
@prefix xsd:   <http://www.w3.org/2001/XMLSchema#> .
@prefix ns9:   <http://purl.org/vocab/vann/> .
@prefix rdf:   <http://www.w3.org/1999/02/22-rdf-syntax-ns#> .
@prefix ns5:   <http://purl.org/dc/terms/> .
@prefix skos:  <http://www.w3.org/2004/02/skos/core#> .
@prefix ns6:   <http://purl.org/ontology/places/> .
@prefix ns10:  <http://creativecommons.org/ns#> .

ns4:lane  a          owl:DatatypeProperty ;
        rdfs:domain  ns4:Road_Work ;
        rdfs:range   rdfs:Literal .

ns5:description  a   owl:DatatypeProperty ;
        rdfs:domain  ns4:Situation_Record ;
        rdfs:range   rdfs:Literal .

ns4:carriageway  a   owl:DatatypeProperty ;
        rdfs:domain  ns4:Road_Condition ;
        rdfs:range   rdfs:Literal .

ns4:speedLimit  a    owl:DatatypeProperty ;
        rdfs:domain  ns4:Road_Work ;
        rdfs:range   xsd:nonNegativeInteger .

ns4:distanceNearestCity
        a            owl:DatatypeProperty ;
        rdfs:domain  ns4:Rest_Area ;
        rdfs:range   xsd:nonNegativeInteger .

ns4:severity  a      owl:DatatypeProperty ;
        rdfs:domain  ns4:Situation_Record ;
        rdfs:range   rdfs:Literal .

ns4:ferryInfo  a     owl:DatatypeProperty ;
        rdfs:domain  ns4:Ferry_Service ;
        rdfs:range   rdfs:Literal .

skos:related  a      owl:ObjectProperty ;
        rdfs:domain  ns4:Rest_Area ;
        rdfs:range   ns4:Place_Info .

ns4:offsetDistance  a  owl:DatatypeProperty ;
        rdfs:domain  ns4:Accident_Service ;
        rdfs:range   xsd:nonNegativeInteger .

ns4:Road_Condition  a    owl:Class ;
        rdfs:comment     "Class that describe the conditions of the road surface which may affect driving conditions. These may be related to the weather (e.g. ice, snow etc.) or to other conditions (e.g. oil, mud, leaves etc. on the road)" ;
        rdfs:label       "Road_Condition" ;
        rdfs:subClassOf  ns4:Situation_Record .

ns4:preferredNamespaceUri
        a                   owl:AnnotationProperty ;
        rdfs:subPropertyOf  rdfs:isDefinedBy .

ns4:areaPlaceName  a  owl:DatatypeProperty ;
        rdfs:domain  ns4:Rest_Area ;
        rdfs:range   rdfs:Literal .

ns4:Place_Info  a  owl:Class .

ns4:situationRecordTime
        a            owl:DatatypeProperty ;
        rdfs:domain  ns4:Situation_Record ;
        rdfs:range   xsd:dateTime .

geo:latitude  a      owl:DatatypeProperty ;
        rdfs:domain  ns4:Location ;
        rdfs:range   xsd:decimal .

ns4:issued  a               owl:AnnotationProperty ;
        rdfs:subPropertyOf  rdfs:isDefinedBy .

ns6:road  a          owl:DatatypeProperty ;
        rdfs:domain  ns4:Location ;
        rdfs:range   rdfs:Literal .

ns4:Location  a       owl:Class ;
        rdfs:comment  "Information about location where the Situation Record was generated. It contains several properties describing the Location. It contains geo:longitude and geo:latitude for creataing external links to othe datasets." ;
        rdfs:label    "Location" .

ns4:title  a                owl:AnnotationProperty ;
        rdfs:subPropertyOf  rdfs:isDefinedBy .

ns4:lanesRestricted  a  owl:DatatypeProperty ;
        rdfs:domain  ns4:Accident_Service ;
        rdfs:range   xsd:nonNegativeInteger .

ns4:    a                             owl:Ontology ;
        rdfs:comment                  "Transport Administration Ontology (TAO) for describing data from Swedish Transport Administration Web site." ;
        rdfs:isDefinedBy              ns4: ;
        rdfs:label                    "Transport Administration Ontology" ;
        ns10:license                  <https://creativecommons.org/licenses/by/3.0/> ;
        ns5:contributor               <https://plus.google.com/+MilosJovanovik> ;
        ns5:creator                   <http://plus.google.com/+GoranPetkovski> ;
        ns5:description               "Transport Administration Ontology (TAO) for describing data from Swedish Transport Administration Web site." ;
        ns5:issued                    "2015-06-17" ;
        ns5:modified                  "2016-08-28" ;
        ns5:publisher                 <http://finki.ukim.mk/> ;
        ns5:rights                    "Copyright 2014, Goran Petkovski" ;
        ns5:title                     "Transport Administration Ontology" ;
        ns9:preferredNamespacePrefix  "tao" ;
        ns9:preferredNamespaceUri     "http://linkeddata.finki.ukim.mk/lod/ontology/tao#" ;
        owl:versionInfo               "1.1" .

ns4:textDescription  a  owl:DatatypeProperty ;
        rdfs:domain  ns4:Road_Condition ;
        rdfs:range   rdfs:Literal .

ns4:locaton_Descriptor
        a            owl:DatatypeProperty ;
        rdfs:domain  ns4:Rest_Area ;
        rdfs:range   rdfs:Literal .

ns4:lengthAffected  a  owl:DatatypeProperty ;
        rdfs:domain  ns4:Accident_Service ;
        rdfs:range   xsd:nonNegativeInteger .

ns4:contributor  a          owl:AnnotationProperty ;
        rdfs:subPropertyOf  rdfs:isDefinedBy .

geo:longitude  a     owl:DatatypeProperty ;
        rdfs:domain  ns4:Location ;
        rdfs:range   xsd:decimal .

ns4:preferredNamespacePrefix
        a                   owl:AnnotationProperty ;
        rdfs:subPropertyOf  rdfs:isDefinedBy .

ns4:location_Of_Situation
        a              owl:ObjectProperty ;
        rdfs:domain    ns4:Location ;
        rdfs:range     ns4:Situation_Record ;
        owl:inverseOf  ns4:has_Location .

ns4:information_Status
        a            owl:DatatypeProperty ;
        rdfs:domain  ns4:Situation_Record ;
        rdfs:range   rdfs:Literal .

ns4:has_Location  a  owl:ObjectProperty ;
        rdfs:domain  ns4:Situation_Record ;
        rdfs:range   ns4:Location .

ns4:countyNumber  a  owl:DatatypeProperty ;
        rdfs:domain  ns4:Location ;
        rdfs:range   xsd:nonNegativeInteger .

ns4:Accident_Service  a  owl:Class ;
        rdfs:comment     "Class that describe emergency information on traffic accidents, fallen trees and other obstructions that affect accessibility. Includes information on location, impact, causes and possible traffic restrictions." ;
        rdfs:label       "Accident_Service" ;
        rdfs:subClassOf  ns4:Situation_Record .

ns4:cityName  a      owl:DatatypeProperty ;
        rdfs:domain  ns4:Rest_Area ;
        rdfs:range   rdfs:Literal .

ns4:Road_Work  a         owl:Class ;
        rdfs:comment     "Class that describe information about ongoing, planned and completed roadworks. Includes information on location, type of road work, impact and restrictions like closures of lanes, width restrictions, rerouting and traffic and speed reductions." ;
        rdfs:label       "Road_Work" ;
        rdfs:subClassOf  ns4:Situation_Record .

ns4:Ferry_Service  a     owl:Class ;
        rdfs:comment     "Class that contains information about reports of deviations and cancellations of the SwedishTransport Administration ferry services. Contains information on ferry routes, estimated duration and possible restrictions." ;
        rdfs:label       "Ferry_Service" ;
        rdfs:subClassOf  ns4:Situation_Record .

ns4:Situation_Record  a  owl:Class ;
        rdfs:comment  "Class describing the basic information about Situation Record instances. It contains  information about time when it occured and information status." ;
        rdfs:label    "Situation_Record" .

ns4:Rest_Area  a         owl:Class ;
        rdfs:comment     "Class that describe rest areas with information on location, level of equipment, service and information functions." ;
        rdfs:label       "Rest_Area" ;
        rdfs:subClassOf  ns4:Situation_Record .
