@prefix :      <http://iais.fraunhofer.de/vocabs/rami#> .
@prefix dc:    <http://purl.org/dc/elements/1.1/> .
@prefix prov:  <http://www.w3.org/ns/prov#> .
@prefix DUL:   <http://www.loa-cnr.it/ontologies/DUL.owl#> .
@prefix foaf:  <http://xmlns.com/foaf/spec/> .
@prefix ssn:   <http://purl.oclc.org/NET/ssnx/ssn#> .
@prefix void:  <http://rdfs.org/ns/void#> .
@prefix vann:  <http://purl.org/vocab/vann/> .
@prefix sf:    <http://iais.fraunhofer.de/vocabs/sf#> .
@prefix vcard: <http://www.w3.org/2006/vcard/ns#> .
@prefix schema: <http://www.w3.org/2001/XMLSchema#> .
@prefix rdfs:  <http://www.w3.org/2000/01/rdf-schema#> .
@prefix dct:   <http://purl.org/dc/terms/> .
@prefix rami:  <http://iais.fraunhofer.de/vocabs/rami#> .
@prefix owl:   <http://www.w3.org/2002/07/owl#> .
@prefix om:    <http://www.wurvoc.org/vocabularies/om-1.8/> .
@prefix rdf:   <http://www.w3.org/1999/02/22-rdf-syntax-ns#> .
@prefix skos:  <http://www.w3.org/2004/02/skos/core#> .

rami:standardVersion  a  owl:DatatypeProperty ;
        rdfs:domain      rami:EngineeringData ;
        rdfs:range       schema:string ;
        skos:definition  "Version of the Standard that specifies the Engineering Data"@en ;
        skos:prefLabel   "Standard Version"@en .

rami:SafetyConfiguration
        a                owl:Class ;
        rdfs:subClassOf  rami:ApplicationData ;
        skos:definition  "Safety Configuration of the Object/Entity. It contains certificate of compliance that states that the object has fullfils the safety requirements according to a given standard"@en ;
        skos:prefLabel   "SafetyConfiguration"@en .

skos:definition  a  owl:AnnotationProperty .

om:volt  a      owl:Class .

rami:publishedURL  a     owl:DatatypeProperty , owl:ObjectProperty ;
        rdfs:domain      rami:Standard ;
        rdfs:range       schema:AnyURI ;
        skos:definition  "Published URL of the Standard"@en ;
        skos:prefLabel   "Published URL"@en .

rami:wraps  a            owl:ObjectProperty ;
        rdfs:domain      rami:AdminShell ;
        rdfs:range       rami:Object ;
        skos:definition  "Connect the Object with the Admin Shell"@en ;
        skos:prefLabel   "wraps"@en .

rami:Machine  a          owl:Class ;
        rdfs:subClassOf  rami:Object ;
        skos:definition  "A machine is ordered, designed, commissioned, operated, serviced, converted and recycled."@en ;
        skos:prefLabel   "Machine"@en .

rami:firmwareDate  a     owl:DatatypeProperty ;
        rdfs:domain      rami:Firmware ;
        rdfs:range       schema:date ;
        skos:definition  "Firmware date that belongs to the Object/Entity"@en ;
        skos:prefLabel   "firmware Date"@en .

rami:hasSensorId  a      owl:FunctionalProperty , owl:DatatypeProperty ;
        rdfs:domain      ssn:Sensor ;
        rdfs:range       schema:string ;
        skos:definition  "Unique Identification of the Sensor"@en ;
        skos:prefLabel   "hasSensorId"@en .

rami:certificateUrl  a   owl:FunctionalProperty , owl:DatatypeProperty ;
        rdfs:domain      rami:SafetyConfiguration ;
        rdfs:range       schema:anyURI ;
        skos:definition  "Certificate Safety Url of the Object/Entity"@en ;
        skos:prefLabel   "Certificate Url"@en .

rami:videoRecordingUrl
        a               owl:FunctionalProperty , owl:DatatypeProperty ;
        rdfs:domain     rami:VideoRecording ;
        rdfs:range      schema:anyURI ;
        skos:prefLabel  "Video Recording Url"@en .

rami:manual  a           owl:DatatypeProperty ;
        rdfs:domain      rami:ApplicationData ;
        rdfs:range       schema:anyURI ;
        skos:definition  "Points to the Manual document of a given Object/Entity"@en ;
        skos:prefLabel   "Manual"@en .

skos:hiddenLabel  a  owl:AnnotationProperty .

rami:certificateName  a  owl:FunctionalProperty , owl:DatatypeProperty ;
        rdfs:domain      rami:SafetyConfiguration ;
        rdfs:range       schema:string ;
        skos:definition  "Certificate Safety Name of the Object/Entity"@en ;
        skos:prefLabel   "Certificate Name"@en .

skos:note  a    owl:AnnotationProperty .

rami:Firmware  a         owl:Class ;
        rdfs:subClassOf  rami:ApplicationData ;
        skos:definition  "Used firmware, firmware modules"@en , "Eingesetzte Firmware, Firmware-Module"@de ;
        skos:prefLabel   "Firmware"@en , "Firmware"@de .

rami:isPartOf  a      owl:TransitiveProperty , owl:ObjectProperty ;
        rdfs:comment  "The Object can be part of of other Objects"@en ;
        rdfs:domain   rami:Object ;
        rdfs:label    "isPartOf"@en ;
        rdfs:range    rami:Object .

schema:AnyURI  a  owl:Class .

rami:isDescribedWith  a  owl:DatatypeProperty , owl:ObjectProperty ;
        rdfs:domain      rami:AdminShell ;
        rdfs:range       rami:Standard ;
        skos:definition  "Points to the Standard used to describe a given object"@en ;
        skos:prefLabel   "Is Described With"@en .

rami:blockUrl  a         owl:DatatypeProperty ;
        rdfs:domain      rami:Firmware ;
        rdfs:range       schema:anyURI ;
        skos:definition  "URL of the Firmware that belongs to the Object/Entity"@en ;
        skos:prefLabel   "Block Url"@en .

rami:VideoRecordings  a  owl:Class .

rami:ApplicationData  a  owl:Class ;
        rdfs:subClassOf  rami:BasicData ;
        skos:definition  "The object determines the format"@en , "Hier bestimmt der Gegenstand das Format"@de ;
        skos:prefLabel   "Application Data"@en , "Anwendungsdaten"@de .

rami:typeDescription  a  owl:DatatypeProperty ;
        rdfs:domain      rami:BasicData ;
        rdfs:range       schema:string ;
        rdfs:seeAlso     <https://www.w3.org/2005/Incubator/omm/XGR-omm-20111026/> ;
        skos:definition  "Describes the Entity/Object related data. It correspond to the Description concept of OMM"@en ;
        skos:prefLabel   "typeDescription"@en .

rami:brakingResistance
        a               owl:DatatypeProperty , owl:ObjectProperty ;
        rdfs:domain     rami:ElectricalData ;
        rdfs:range      om:hertz ;
        skos:prefLabel  "braking Resistance"@en .

rami:identification  a   owl:FunctionalProperty , owl:DatatypeProperty ;
        rdfs:domain      rami:BasicData ;
        rdfs:range       schema:string ;
        rdfs:seeAlso     <https://www.w3.org/2005/Incubator/omm/XGR-omm-20111026/> ;
        skos:definition  "Identification for the Entity/Object related data. It correspond to the ID concept of OMM"@en ;
        skos:prefLabel   "Identification"@en .

rami:CADFormat  a        owl:DatatypeProperty ;
        rdfs:domain      rami:MCAD ;
        rdfs:range       schema:string ;
        skos:definition  "Different types of format files for CAD Archive of the Object/Entity"@en ;
        skos:prefLabel   "CAD Format"@en .

rami:inputVoltage  a    owl:DatatypeProperty , owl:ObjectProperty ;
        rdfs:domain     rami:ElectricalData ;
        rdfs:range      om:volt ;
        skos:example    "230 V AC / 50-60 Hz" ;
        skos:prefLabel  "Input Voltage"@en .

rami:hasEnergyValue  a  owl:DatatypeProperty ;
        rdfs:domain     rami:CumulativeEnergyConsumption ;
        rdfs:range      schema:float ;
        skos:prefLabel  "hasEnergyValue"@en .

rami:CADSystem  a        owl:DatatypeProperty ;
        rdfs:domain      rami:MCAD ;
        rdfs:range       schema:string ;
        skos:definition  "Points to the different types of CAD systems of the Object/Entity"@en ;
        skos:example     "Neutral 2D, Neutral 3D, SolidWorks" ;
        skos:prefLabel   "CAD Format"@en .

skos:altLabel  a  owl:AnnotationProperty .

rami:Instance  a  owl:NamedIndividual .

rami:version  a          owl:DatatypeProperty ;
        rdfs:domain      rami:Standard , rami:Firmware ;
        rdfs:range       schema:string ;
        skos:definition  "Version of the Firmware that belongs to the Object/Entity"@en , "Current version of the Standard"@en ;
        skos:prefLabel   "has Version"@en , "Version"@en .

rami:   a                              owl:Ontology ;
        rdfs:isDefinedBy               rami: ;
        dct:created                    "2015-11-30"^^schema:date ;
        dct:creator                    "Irlan Grangel" , "Niklas Petersen" ;
        dct:publisher                  <http://de.dbpedia.org/resource/Fraunhofer-Gesellschaft> ;
        vann:preferredNamespacePrefix  "rami" ;
        vann:preferredNamespaceUri     "http://iais.fraunhofer.de/vocabs/rami#" ;
        void:vocabulary                dc: , <http://www.w3.org/XML/1998/namespace> , skos: , rdf: , schema: , sf: , foaf: , rdfs: , dct: ;
        owl:versionInfo                "SNAPSHOT" ;
        skos:definition                "A vocabulary which represents the Reference Architecture Model for Industry 4.0 (RAMI), including the concept of the Administration Shell I4.0 Component."@en ;
        skos:prefLabel                 "rami"@en .

dc:source  a    owl:AnnotationProperty .

rami:MCAD  a             owl:Class ;
        rdfs:subClassOf  rami:EngineeringData ;
        skos:definition  "Data that contain the files used for Mechanical Computer Aid Design of a given object"@en ;
        skos:prefLabel   "MCAD"@en , "MCAD"@de .

rami:logs  a            owl:DatatypeProperty ;
        rdfs:domain     rami:TraceRecordings ;
        rdfs:range      schema:string ;
        skos:prefLabel  "logs"@en .

rami:SensorMeasurementData
        a                    owl:Class ;
        rdfs:comment         "Data measured by a sensor"@en ;
        rdfs:label           "Sensor Data"@en ;
        rdfs:subClassOf      rami:BasicData ;
        owl:equivalentClass  ssn:SensorOutput .

rami:standardName  a     owl:DatatypeProperty ;
        rdfs:domain      rami:EngineeringData ;
        rdfs:range       schema:string ;
        skos:definition  "Name of the Standard that specifies the Engineering Data"@en ;
        skos:prefLabel   "Standard Name"@en .

rami:name  a             owl:FunctionalProperty , owl:DatatypeProperty ;
        rdfs:domain      rami:Object ;
        rdfs:range       schema:string ;
        skos:definition  "Name of the Object/Entity"@en ;
        skos:prefLabel   "has Name"@en .

rami:hasTechnicalFuncionality
        a                owl:ObjectProperty ;
        rdfs:domain      rami:AdminShell ;
        rdfs:range       rami:TechnicalFunctionality ;
        skos:definition  "The Administrative Shell has Technical Funcionalities"@en ;
        skos:prefLabel   "has Technical Funcionality"@en .

prov:Agent  a   owl:Class .

rami:ElectricalData  a   owl:Class ;
        rdfs:subClassOf  rami:BasicData ;
        skos:definition  "Electrical Data for the Object"@en ;
        skos:prefLabel   "Electrical Data"@en .

schema:date  a  rdfs:Datatype .

rami:FieldDevice  a      rami:RAMIHierarchyLevel , owl:NamedIndividual ;
        skos:definition  "Field Device hierarchy level of RAMI 4.0"@en ;
        skos:prefLabel   "Field Device"@en .

rami:Object  a               owl:Class ;
        owl:equivalentClass  [ a          owl:Class ;
                               owl:oneOf  ( rami:Instance rami:Type )
                             ] ;
        skos:altLabel        "Entität"@de , "Entity"@en ;
        skos:definition      "Eindeutig identifizierbarer Gegenstand, der aufgrund seiner Bedeutung in der Informationswelt verwaltet wird"@de , "Clearly identifiable object which is managed due to its importance in the world of information"@en ;
        skos:note            "Objects may be known in the form of a type or of an instance. An object in the planning phase is known as a type"@en ;
        skos:prefLabel       "Objekt"@de , "Object"@en .

rami:phasesNumber  a    owl:DatatypeProperty ;
        rdfs:domain     rami:ElectricalData ;
        rdfs:range      schema:string ;
        skos:example    "Single phase, three phase" ;
        skos:prefLabel  "Phases Number"@en .

rami:eClassClassification
        a                owl:FunctionalProperty , owl:DatatypeProperty ;
        rdfs:domain      rami:eClass ;
        rdfs:range       schema:integer ;
        skos:definition  "Identification of an object according to the eCl@ss Standard hierarchy level"@en ;
        skos:prefLabel   "eClassIRDI"@en .

rami:createdBy  a        owl:ObjectProperty ;
        rdfs:domain      rami:BasicData ;
        rdfs:range       prov:Agent ;
        skos:definition  "Agent(Person or Software) that creates to the Entity/Object related data. It correspond to the Creator concept of OMM"@en ;
        skos:prefLabel   "hasCreator"@en .

foaf:Image  a   owl:Class .

rami:CumulativeEnergyConsumption
        a       owl:Class .

rami:Station  a          rami:RAMIHierarchyLevel , owl:NamedIndividual ;
        skos:definition  "Station hierarchy level of RAMI 4.0"@en ;
        skos:prefLabel   "Station"@en .

skos:prefLabel  a  owl:AnnotationProperty .

rami:stdName  a          owl:DatatypeProperty ;
        rdfs:domain      rami:Standard ;
        rdfs:range       schema:string ;
        skos:definition  "Name of the Standard"@en ;
        skos:prefLabel   "Std Name"@en .

rami:contributes  a      owl:ObjectProperty ;
        rdfs:domain      rami:BasicData ;
        rdfs:range       prov:Agent ;
        skos:definition  "Agent(Person or Software) that contributes to the Entity/Object related data. It correspond to the Contributor concept of OMM"@en ;
        skos:prefLabel   "typeDescription"@en .

skos:example  a  owl:AnnotationProperty .

rami:WorkCenter  a       rami:RAMIHierarchyLevel , owl:NamedIndividual ;
        skos:definition  "Work Center hierarchy level of RAMI 4.0"@en ;
        skos:prefLabel   "Work Center"@en .

rami:releaseDate  a      owl:DatatypeProperty ;
        rdfs:domain      rami:Standard ;
        rdfs:range       schema:date ;
        skos:definition  "Release Date of the Standard"@en ;
        skos:prefLabel   "Release Date"@en .

rami:creationDate  a     owl:DatatypeProperty ;
        rdfs:domain      rami:BasicData ;
        rdfs:range       schema:dateTime ;
        skos:definition  "Date when an Agent(Person or Software) creates to the Entity/Object related data. It correspond to the Creator concept of OMM"@en ;
        skos:prefLabel   "hasCreator"@en .

rami:outputFrequency  a  owl:DatatypeProperty , owl:ObjectProperty ;
        rdfs:domain     rami:ElectricalData ;
        rdfs:range      om:hertz ;
        skos:prefLabel  "Output Frequency"@en .

rami:EngineeringData  a   owl:Class ;
        rdfs:isDefinedBy  <http://www.businessdictionary.com/definition/engineering-data.html#ixzz45Ydk71Su> ;
        rdfs:subClassOf   rami:BasicData ;
        skos:definition   "Documents such as drawings, manufacturer's specifications, standards, and other information relating to design, procurement, fabrication, test, and inspection of an item or structure."@en ;
        skos:prefLabel    "Engineering-Daten"@de , "Engineering Data"@en .

rami:Enterprise  a       rami:RAMIHierarchyLevel , owl:NamedIndividual ;
        skos:definition  "Enterprise hierarchy level of RAMI 4.0"@en ;
        skos:prefLabel   "Enterprise"@en .

om:hertz  a     owl:Class .

rami:inventoryNumber  a  owl:FunctionalProperty , owl:DatatypeProperty ;
        rdfs:domain      rami:BasicData ;
        rdfs:range       schema:string ;
        skos:definition  "Inventory number of the Entity/Object according to the identification nomenclature"@en ;
        skos:prefLabel   "Inventory Number"@en .

rami:eClassIRDI  a       owl:FunctionalProperty , owl:DatatypeProperty ;
        rdfs:domain      rami:eClass ;
        rdfs:range       schema:string ;
        skos:definition  "Unique Identification of an object according to eCl@ss Standard"@en ;
        skos:prefLabel   "eClassIRDI"@en .

rami:contributionDate
        a                owl:DatatypeProperty ;
        rdfs:domain      rami:BasicData ;
        rdfs:range       schema:dateTime ;
        skos:definition  "Date when an Agent(Person or Software) contributes to the Entity/Object related data. It correspond to the Contributor concept of OMM"@en ;
        skos:prefLabel   "hasCreator"@en .

rami:RAMIHierarchyLevel
        a                    owl:Class ;
        rdfs:seeAlso         <http://www.zvei.org/en/subjects/Industry-40/Pages/The-Reference-Architectural-Model-RAMI-40-and-the-Industrie-40-Component.aspx> ;
        owl:equivalentClass  [ a          owl:Class ;
                               owl:oneOf  ( rami:ConnectedWorld rami:ControlDevice rami:Enterprise rami:FieldDevice rami:Product rami:Station rami:WorkCenter )
                             ] ;
        skos:definition      "It describes the functional classification of various circumstances within Industrie 4.0. For classification within a factory, this axis of the reference architecture(layers) follows the IEC 62264 Standard."@en ;
        skos:prefLabel       "RAMI Hierarchy Level"@en .

rami:hasData  a          owl:ObjectProperty ;
        rdfs:domain      rami:AdminShell ;
        rdfs:range       rami:BasicData ;
        skos:definition  "Connects the AdminShell with the different types of Data for the Object/Entity"@en ;
        skos:prefLabel   "has Data"@en .

ssn:Sensor  a   owl:Class .

rami:TraceRecordings  a  owl:Class .

rami:description  a      owl:DatatypeProperty ;
        rdfs:domain      rami:Object ;
        rdfs:range       schema:string ;
        skos:definition  "Description of the Object/Entity"@en ;
        skos:prefLabel   "has Description"@en .

rami:videoUrl  a        owl:DatatypeProperty ;
        rdfs:domain     rami:VideoRecordings ;
        rdfs:range      schema:anyURI ;
        skos:prefLabel  "videoUrl"@en .

rami:VideoRecording  a  owl:Class .

rami:safetyName  a       owl:DatatypeProperty ;
        rdfs:domain      rami:SafetyConfiguration ;
        rdfs:range       schema:string ;
        skos:definition  "Name of the Safety Configuration of the Object/Entity"@en ;
        skos:prefLabel   "Safety Name"@en .

rami:Type  a    owl:NamedIndividual .

rami:standardURL  a      owl:DatatypeProperty ;
        rdfs:domain      rami:EngineeringData ;
        rdfs:range       schema:anyURI ;
        skos:definition  "Points to the URL of the Standard that specifies the Engineering Data"@en ;
        skos:prefLabel   "Standard URL"@en .

rami:livePicture  a   owl:ObjectProperty ;
        rdfs:comment  "Points to an Image for the Object/Entity"@en ;
        rdfs:domain   rami:Object ;
        rdfs:label    "Livebilder"@de , "LivePicture"@en ;
        rdfs:range    foaf:Image .

rami:ControlDevice  a    rami:RAMIHierarchyLevel , owl:NamedIndividual ;
        skos:definition  "Control Device hierarchy level of RAMI 4.0"@en ;
        skos:prefLabel   "Control Device"@en .

rami:hasRAMIHierarchyLevel
        a                owl:ObjectProperty ;
        rdfs:range       rami:RAMIHierarchyLevel ;
        skos:definition  "Connects the concepts with the correspondent layer in the RAMI Hierarchy Levels"@en ;
        skos:prefLabel   "has RAMI Hierarchy Level" .

rami:eClass  a           owl:Class ;
        rdfs:subClassOf  rami:Standard ;
        skos:definition  "Class to represent the connection of an I4.0 Entity/Object with the eCl@ss Standard"@en ;
        skos:prefLabel   "eClass"@en , "eClass"@de .

rami:Standard  a         owl:Class ;
        skos:definition  "Standards that are used to describe the actual I4.0 Entity/Object"@en ;
        skos:prefLabel   "Standard"@en , "Standard"@de .

rami:CADarchive  a       owl:DatatypeProperty ;
        rdfs:domain      rami:MCAD ;
        rdfs:range       schema:anyURI ;
        skos:definition  "Link(URL) to the CAD Archive of the Object/Entity"@en ;
        skos:prefLabel   "CAD Archive"@en .

rami:Order  a            owl:Class ;
        skos:definition  "Each order for manufacturing runs through a life cycle and its specifics necessarily have an impact on the production facility during performance of the order"@en ;
        skos:prefLabel   "Order"@en .

rami:TechnicalFunctionality
        a                owl:Class ;
        skos:definition  "Technical Functionality of the Administration Shell"@en ;
        skos:note        "Technical functionality takes place in the Functional Layer of the reference architecture model RAMI4.0"@en ;
        skos:prefLabel   "Technical Functionality"@en , "Fachliche Funktionalität"@de .

rami:AdminShell  a        owl:Class ;
        dc:source         "This definition comprises material from RAMI4.0."@en ;
        skos:altLabel     "Administration Shell"@en ;
        skos:definition   "Describe the Administration Shell for Products, Components, e.g. Machines"@en ;
        skos:hiddenLabel  "Administrative Shell"@en ;
        skos:prefLabel    "Verwaltungsschale"@de , "Admin Shell"@en .

rami:Product  a          rami:RAMIHierarchyLevel , owl:NamedIndividual ;
        skos:definition  "Product hierarchy level of RAMI 4.0"@en ;
        skos:prefLabel   "Product"@en .

rami:ConnectedWorld  a   rami:RAMIHierarchyLevel , owl:NamedIndividual ;
        skos:definition  "Connected World hierarchy level of RAMI 4.0.  Group of Factories, and the collaboration with external engineering firms, component suppliers and customers"@en ;
        skos:prefLabel   "Connected World"@en .

ssn:SensorOutput  a  owl:Class .

rami:objectId  a         owl:FunctionalProperty , owl:DatatypeProperty ;
        rdfs:domain      rami:Object ;
        rdfs:range       schema:string ;
        skos:definition  "Unique ID for the Object/Entity"@en ;
        skos:prefLabel   "has Object Id"@en .

rami:BasicData  a        owl:Class ;
        skos:definition  "Describe the different types of Data related to the I4.0 Entity/Object"@en ;
        skos:prefLabel   "Daten"@de , "Data"@en .
