@prefix : <http://purl.org/net/wf-invocation#> .
@prefix rdfs: <http://www.w3.org/2000/01/rdf-schema#> .
@prefix p-plan: <http://purl.org/net/p-plan#> .
@prefix terms: <http://purl.org/dc/terms/> .
@prefix owl: <http://www.w3.org/2002/07/owl#> .
@prefix xsd: <http://www.w3.org/2001/XMLSchema#> .
@prefix rdf: <http://www.w3.org/1999/02/22-rdf-syntax-ns#> .
@prefix vann: <http://purl.org/vocab/vann/> .

<http://purl.org/net/wf-invocation> a owl:Ontology ;
	rdfs:label "Workflow Invocation Ontology"@en ;
	terms:created "2013-05-17"^^xsd:date ;
	terms:creator "http://delicias.dia.fi.upm.es/members/DGarijo/#me"^^xsd:anyURI , "http://www.isi.edu/~varunr/resume.html"^^xsd:anyURI , "http://www.isi.edu/~gil/"^^xsd:anyURI ;
	terms:description "Wf-invoc is a simple profile of the P-plan ontology to describe how workflow steps are invoked within a workflow execution."@en ;
	terms:license "http://creativecommons.org/licenses/by-nc-sa/2.0/" ;
	terms:title "The Workflow Invocation Ontology"@en ;
	vann:preferredNamespaceUri "http://purl.org/net/wf-invocation#" ;
	vann:preferredNamespacePrefix "wf-invoc" ;
	owl:versionInfo "1.1"@en ;
	rdfs:comment "Workflow Invocation Ontology, an extension of P-Plan for representing the invocation of the workflow steps when submitting a template to an execution engine."@en ;
	owl:imports <http://purl.org/net/p-plan#> .

terms:creator a owl:AnnotationProperty .

:hasCodeBinding a owl:DatatypeProperty .

:hasCustomData a owl:DatatypeProperty ;
	rdfs:label "has Custom Data"@en ;
	rdfs:comment "Data property used to link a wf-invoc:Step with any particular metadata that will be used in the execution of the Step (e.g., environment requirements, memory, etc.)"@en ;
	rdfs:domain :Step ;
	rdfs:range rdfs:Literal .

:hasDataBinding a owl:DatatypeProperty ;
	rdfs:label "has Data Binding"@en ;
	rdfs:comment "Data property used to bind a wf-invoc:Variable with the path or URL where the data is available for the execution."@en ;
	rdfs:domain :Variable ;
	rdfs:range rdfs:Literal .

:hasInvocationLine a owl:DatatypeProperty ;
	rdfs:label "has Invocation Line"@en ;
	rdfs:comment "Data property used to link a wf-invoc:Step with the Literal representing the invocation line of the current Step."@en ;
	rdfs:domain :Step ;
	rdfs:range rdfs:Literal .

p-plan:Step a owl:Class .

p-plan:Variable a owl:Class .

:Step a owl:Class ;
	rdfs:label "Step"@en ;
	rdfs:subClassOf p-plan:Step ;
	rdfs:comment "Specialization of p-plan:Step in order to be able to assert domain specific properties. A wf-invoc:Step refers to those p-plan:Steps related to the scientific workflow invocation."@en .

:Variable a owl:Class ;
	rdfs:label "Variable"@en ;
	rdfs:subClassOf p-plan:Variable ;
	rdfs:comment "Specialization of p-plan:Variable in order to be able to assert specific properties. A wf-invoc:Variable refers to those p-plan:Variables related to the scientific workflow invocation."@en .
