@prefix adms:  <http://www.w3.org/ns/adms#> .
@prefix dc:    <http://purl.org/dc/elements/1.1/> .
@prefix rdfs:  <http://www.w3.org/2000/01/rdf-schema#> .
@prefix foaf:  <http://xmlns.com/foaf/0.1/> .
@prefix owl:   <http://www.w3.org/2002/07/owl#> .
@prefix xsd:   <http://www.w3.org/2001/XMLSchema#> .
@prefix rdf:   <http://www.w3.org/1999/02/22-rdf-syntax-ns#> .
@prefix vann:  <http://purl.org/vocab/vann/> .
@prefix dcterms: <http://purl.org/dc/terms/> .
@prefix incident: <http://vocab.resc.info/incident#> .

incident:Characteristic
        a             owl:Class , rdfs:Class ;
        rdfs:comment  "Holds characteristics of a Incident" ;
        rdfs:label    "Characteristic" .

incident:IncidentRecord
        a             owl:Class , rdfs:Class ;
        rdfs:comment  "A class to record the response to a incident by emergency response services." ;
        rdfs:label    "Incident Record" .

incident:arrivalTimestamp
        a             owl:DatatypeProperty , rdf:Property ;
        rdfs:comment  "The time the unit arrived at the incident location, this might not be automatically generated" ;
        rdfs:domain   incident:Deployment ;
        rdfs:label    "Arrival timestamp" ;
        rdfs:range    xsd:dateTime .

incident:incidentRecordStartTimestamp
        a             owl:DatatypeProperty , rdf:Property ;
        rdfs:comment  "The time the recordinf of the incident response begins" ;
        rdfs:domain   incident:IncidentRecord ;
        rdfs:label    "Incident Record timestamp" ;
        rdfs:range    xsd:dateTime .

<http://vocab.resc.info/incident>
        a                              owl:Ontology , adms:Asset ;
        dc:creator                     incident:bart ;
        dc:license                     "http://creativecommons.org/publicdomain/zero/1.0/" ;
        dcterms:created                "2014-12-19"^^xsd:date ;
        dcterms:description            "Vocabulary to describe the response to a incident by emergency services.\r\nThis is NOT intended to describe the incident itself, it describes the response" ;
        dcterms:isPartOf               <http://vocab.resc.info> ;
        dcterms:modified               "2015-06-22"^^xsd:date ;
        dcterms:title                  "Vocabulary to describe incident response by emergency respose services" ;
        dcterms:type                   <http://purl.org/adms/assettype/Ontology> ;
        vann:preferredNamespacePrefix  "incident" ;
        vann:preferredNamespaceUri     "http://vocab.resc.info/incident#" ;
        adms:status                    <http://purl.org/adms/status/UnderDevelopment> ;
        foaf:homepage                  <http://vocab.resc.info/incident.html> .

incident:Note  a      owl:Class , rdfs:Class ;
        rdfs:comment  "A text note for the incident, in general the CAD system log book. Should contain dcterms:modified instead of semtimestamp" ;
        rdfs:label    "Note" .

incident:deployedUnit
        a             rdf:Property ;
        rdfs:comment  "The unit deployed to a incident" ;
        rdfs:domain   incident:Deployment ;
        rdfs:label    "Unit deployed" ;
        rdfs:range    rdfs:Resource .

incident:bart  a   foaf:Person ;
        foaf:nick  "bart" .

incident:hasDeployment
        a             rdf:Property ;
        rdfs:comment  "a deployment of a unit to a incident" ;
        rdfs:domain   incident:IncidentRecord ;
        rdfs:label    "Has Deployment" ;
        rdfs:range    incident:Deployment .

incident:rdf  a             adms:AssetDistribution ;
        dcterms:FileFormat  <http://vocab.resc.info/incident> ;
        dcterms:license     <http://creativecommons.org/publicdomain/zero/1.0/> ;
        adms:status         <http://purl.org/adms/status/Completed> .

incident:deploymentStartTimestamp
        a             owl:DatatypeProperty , rdf:Property ;
        rdfs:comment  "The time that a unit is send out to a incident" ;
        rdfs:domain   incident:Deployment ;
        rdfs:label    "Deployment Start" ;
        rdfs:range    xsd:dateTime .

incident:deploymentEndTimestamp
        a             owl:DatatypeProperty , rdf:Property ;
        rdfs:comment  "The time the unit was no longer needed at the incident." ;
        rdfs:domain   incident:Deployment ;
        rdfs:label    "End of the deployment" ;
        rdfs:range    xsd:dateTime .

incident:ttl  a             adms:AssetDistribution ;
        dcterms:FileFormat  <http://vocab.resc.info/incident> ;
        dcterms:license     <http://creativecommons.org/publicdomain/zero/1.0/> ;
        adms:status         <http://purl.org/adms/status/Completed> .

incident:isDeploymentOf
        a             rdf:Property ;
        rdfs:comment  "This is a deployment to a specific incident" ;
        rdfs:domain   incident:Deployment ;
        rdfs:label    "is Deployment of" ;
        rdfs:range    incident:IncidentRecord .

incident:characteristicType
        a             rdf:Property ;
        rdfs:comment  "The type of the recorded characteristic, preferably points to a SKOS concept" ;
        rdfs:domain   incident:Characteristic ;
        rdfs:label    "Characteristic Type" .

incident:hasNote  a   rdf:Property ;
        rdfs:comment  "The relation between a incident and the text notes" ;
        rdfs:domain   incident:IncidentRecord ;
        rdfs:label    "hasNote" ;
        rdfs:range    incident:Note .

incident:location  a  rdf:Property ;
        rdfs:comment  "The location of the incident" ;
        rdfs:label    "Location" .

incident:Deployment  a  owl:Class , rdfs:Class ;
        rdfs:comment  "The actual sending of a responding unit to a Incident." ;
        rdfs:label    "Deployment" .

incident:incidentRecordEndTimestamp
        a             owl:DatatypeProperty , rdf:Property ;
        rdfs:comment  "the time the emergency response services are no longer involved in the incident." ;
        rdfs:domain   incident:IncidentRecord ;
        rdfs:label    "Incident Record end timestamp" ;
        rdfs:range    xsd:dateTime .

incident:hasCharacteristic
        a             rdf:Property ;
        rdfs:comment  "Relation between characteristics and incidents" ;
        rdfs:domain   incident:IncidentRecord ;
        rdfs:label    "has Characteristic" ;
        rdfs:range    incident:Characteristic .

incident:mobilizationTimestamp
        a             owl:DatatypeProperty , rdf:Property ;
        rdfs:comment  "The time the unit is mobilized, when it starts heading to the incident" ;
        rdfs:domain   incident:Deployment ;
        rdfs:label    "Mobilization timestamp" ;
        rdfs:range    xsd:dateTime .
