@prefix dc: <http://purl.org/dc/elements/1.1/> .
@prefix rdfs: <http://www.w3.org/2000/01/rdf-schema#> .
@prefix foaf: <http://xmlns.com/foaf/0.1/> .
@prefix status: <http://metadataregistry.org/uri/RegStatus/> .
@prefix reg: <http://metadataregistry.org/uri/profile/RegAp/> .
@prefix dct: <http://purl.org/dc/terms/> .
@prefix owl: <http://www.w3.org/2002/07/owl#> .
@prefix rdf: <http://www.w3.org/1999/02/22-rdf-syntax-ns#> .
@prefix skos: <http://www.w3.org/2004/02/skos/core#> .

status:1001 a skos:Concept ;
	skos:prefLabel "Published"@en .

status:1008 a skos:Concept ;
	skos:prefLabel "Deprecated"@en .

<http://rdaregistry.info/Elements/i/> dc:title "RDA Item properties"@en ;
	skos:note "Properties derived from RDA elements and relationship designators with the domain of RDA Item."@en .

<http://rdaregistry.info/Elements/i/P40001> reg:name "identifierForTheItem"@en ;
	reg:status status:1001 ;
	a rdf:Property ;
	rdfs:domain <http://rdaregistry.info/Elements/c/C10003> ;
	rdfs:isDefinedBy <http://rdaregistry.info/Elements/i/> ;
	rdfs:label "has identifier for the item"@en ;
	rdfs:subPropertyOf <http://rdaregistry.info/Elements/u/P60052> ;
	owl:sameAs <http://rdaregistry.info/Elements/i/identifierForTheItem> ;
	skos:definition "Relates an item to a character string associated with an item that serves to differentiate that item from other items."@en .

<http://rdaregistry.info/Elements/i/P40002> reg:status status:1008 ;
	rdfs:isDefinedBy <http://rdaregistry.info/Elements/i/> .

<http://rdaregistry.info/Elements/i/P40003> reg:name "noteOnItemSpecificCarrierCharacteristic"@en ;
	reg:status status:1001 ;
	a rdf:Property ;
	rdfs:domain <http://rdaregistry.info/Elements/c/C10003> ;
	rdfs:isDefinedBy <http://rdaregistry.info/Elements/i/> ;
	rdfs:label "has note on item-specific carrier characteristic"@en ;
	owl:sameAs <http://rdaregistry.info/Elements/i/itemSpecificCarrierCharacteristic> , <http://rdaregistry.info/Elements/i/noteOnItemSpecificCarrierCharacteristic> ;
	skos:definition "Relates an item to a note providing additional information about carrier characteristics that are specific to the item being described and are assumed not to apply to other items exemplifying the same manifestation."@en .

<http://rdaregistry.info/Elements/i/P40004> reg:name "collector"@en ;
	reg:status status:1001 ;
	a rdf:Property ;
	rdfs:domain <http://rdaregistry.info/Elements/c/C10003> ;
	rdfs:isDefinedBy <http://rdaregistry.info/Elements/i/> ;
	rdfs:label "has collector"@en ;
	rdfs:range <http://rdaregistry.info/Elements/c/C10002> ;
	rdfs:subPropertyOf <http://rdaregistry.info/Elements/i/P40017> , <http://rdaregistry.info/Elements/u/P60066> ;
	owl:inverseOf <http://rdaregistry.info/Elements/a/P50045> ;
	owl:sameAs <http://rdaregistry.info/Elements/i/collector> ;
	skos:definition "Relates an item to a curator who brings together items from various sources that are then arranged, described, and cataloged as a collection."@en .

<http://rdaregistry.info/Elements/i/P40005> reg:name "collectionRegistrar"@en ;
	reg:status status:1001 ;
	a rdf:Property ;
	rdfs:domain <http://rdaregistry.info/Elements/c/C10003> ;
	rdfs:isDefinedBy <http://rdaregistry.info/Elements/i/> ;
	rdfs:label "has collection registrar"@en ;
	rdfs:range <http://rdaregistry.info/Elements/c/C10002> ;
	rdfs:subPropertyOf <http://rdaregistry.info/Elements/i/P40017> , <http://rdaregistry.info/Elements/u/P60067> ;
	owl:inverseOf <http://rdaregistry.info/Elements/a/P50046> ;
	owl:sameAs <http://rdaregistry.info/Elements/i/collectionRegistrar> ;
	skos:definition "Relates an item to a curator who lists or inventories the items in an aggregate work such as a collection of items or works."@en .

<http://rdaregistry.info/Elements/i/P40006> reg:name "depositor"@en ;
	reg:status status:1001 ;
	a rdf:Property ;
	rdfs:domain <http://rdaregistry.info/Elements/c/C10003> ;
	rdfs:isDefinedBy <http://rdaregistry.info/Elements/i/> ;
	rdfs:label "has depositor"@en ;
	rdfs:range <http://rdaregistry.info/Elements/c/C10002> ;
	rdfs:subPropertyOf <http://rdaregistry.info/Elements/i/P40018> , <http://rdaregistry.info/Elements/u/P60068> ;
	owl:inverseOf <http://rdaregistry.info/Elements/a/P50047> ;
	owl:sameAs <http://rdaregistry.info/Elements/i/depositor> ;
	skos:definition "Relates an item to a current owner of an item who deposited the item into the custody of another person, family, or corporate body, while still retaining ownership."@en .

<http://rdaregistry.info/Elements/i/P40007> reg:name "donor"@en ;
	reg:status status:1001 ;
	a rdf:Property ;
	rdfs:domain <http://rdaregistry.info/Elements/c/C10003> ;
	rdfs:isDefinedBy <http://rdaregistry.info/Elements/i/> ;
	rdfs:label "has donor"@en ;
	rdfs:range <http://rdaregistry.info/Elements/c/C10002> ;
	rdfs:subPropertyOf <http://rdaregistry.info/Elements/i/P40019> , <http://rdaregistry.info/Elements/u/P60091> ;
	owl:inverseOf <http://rdaregistry.info/Elements/a/P50066> ;
	owl:sameAs <http://rdaregistry.info/Elements/i/donor> ;
	skos:definition "Relates an item to a former owner of an item who donated that item to another owner."@en .

<http://rdaregistry.info/Elements/i/P40008> reg:name "seller"@en ;
	reg:status status:1001 ;
	a rdf:Property ;
	rdfs:domain <http://rdaregistry.info/Elements/c/C10003> ;
	rdfs:isDefinedBy <http://rdaregistry.info/Elements/i/> ;
	rdfs:label "has seller"@en ;
	rdfs:range <http://rdaregistry.info/Elements/c/C10002> ;
	rdfs:subPropertyOf <http://rdaregistry.info/Elements/i/P40019> , <http://rdaregistry.info/Elements/u/P60092> ;
	owl:inverseOf <http://rdaregistry.info/Elements/a/P50067> ;
	owl:sameAs <http://rdaregistry.info/Elements/i/seller> ;
	skos:definition "Relates an item to a former owner of an item who sold that item to another owner."@en .

<http://rdaregistry.info/Elements/i/P40009> reg:name "containedInItem"@en ;
	reg:status status:1001 ;
	a rdf:Property ;
	rdfs:domain <http://rdaregistry.info/Elements/c/C10003> ;
	rdfs:isDefinedBy <http://rdaregistry.info/Elements/i/> ;
	rdfs:label "is contained in (item)"@en ;
	rdfs:range <http://rdaregistry.info/Elements/c/C10003> ;
	rdfs:subPropertyOf <http://rdaregistry.info/Elements/i/P40054> , <http://rdaregistry.info/Elements/u/P60101> ;
	owl:inverseOf <http://rdaregistry.info/Elements/i/P40034> ;
	owl:sameAs <http://rdaregistry.info/Elements/i/containedInItem> ;
	skos:definition "Relates an item to a larger item of which a part is a discrete component."@en .

<http://rdaregistry.info/Elements/i/P40010> reg:name "noteOnDimensionsOfItem"@en ;
	reg:status status:1001 ;
	a rdf:Property ;
	rdfs:domain <http://rdaregistry.info/Elements/c/C10003> ;
	rdfs:isDefinedBy <http://rdaregistry.info/Elements/i/> ;
	rdfs:label "has note on dimensions of item"@en ;
	rdfs:subPropertyOf <http://rdaregistry.info/Elements/i/P40003> , <http://rdaregistry.info/Elements/u/P60133> ;
	owl:sameAs <http://rdaregistry.info/Elements/i/noteOnDimensionsOfItem> ;
	skos:definition "Relates an item to a note providing information on the dimensions of the specific item being described that is not recorded as part of the dimensions element."@en .

<http://rdaregistry.info/Elements/i/P40011> reg:name "noteOnExtentOfItem"@en ;
	reg:status status:1001 ;
	a rdf:Property ;
	rdfs:domain <http://rdaregistry.info/Elements/c/C10003> ;
	rdfs:isDefinedBy <http://rdaregistry.info/Elements/i/> ;
	rdfs:label "has note on extent of item"@en ;
	rdfs:subPropertyOf <http://rdaregistry.info/Elements/i/P40003> , <http://rdaregistry.info/Elements/u/P60134> ;
	owl:sameAs <http://rdaregistry.info/Elements/i/noteOnExtentOfItem> ;
	skos:definition "Relates an item to a note providing information on the extent of the specific being described that is not recorded as part of the extent element."@en .

<http://rdaregistry.info/Elements/i/P40012> reg:name "illuminator"@en ;
	reg:status status:1001 ;
	a rdf:Property ;
	rdfs:domain <http://rdaregistry.info/Elements/c/C10003> ;
	rdfs:isDefinedBy <http://rdaregistry.info/Elements/i/> ;
	rdfs:label "has illuminator"@en ;
	rdfs:range <http://rdaregistry.info/Elements/c/C10004> ;
	rdfs:subPropertyOf <http://rdaregistry.info/Elements/i/P40023> , <http://rdaregistry.info/Elements/u/P60421> ;
	owl:inverseOf <http://rdaregistry.info/Elements/a/P50092> ;
	owl:sameAs <http://rdaregistry.info/Elements/i/illuminator> ;
	skos:definition "Relates an item to a person providing decoration to a specific item using precious metals or color, often with elaborate designs and motifs."@en .

<http://rdaregistry.info/Elements/i/P40013> reg:name "binder"@en ;
	reg:status status:1001 ;
	a rdf:Property ;
	rdfs:domain <http://rdaregistry.info/Elements/c/C10003> ;
	rdfs:isDefinedBy <http://rdaregistry.info/Elements/i/> ;
	rdfs:label "has binder"@en ;
	rdfs:range <http://rdaregistry.info/Elements/c/C10004> ;
	rdfs:subPropertyOf <http://rdaregistry.info/Elements/i/P40023> , <http://rdaregistry.info/Elements/u/P60458> ;
	owl:inverseOf <http://rdaregistry.info/Elements/a/P50123> ;
	owl:sameAs <http://rdaregistry.info/Elements/i/binder> ;
	skos:definition "Relates an item to a person who binds an item."@en .

<http://rdaregistry.info/Elements/i/P40014> reg:name "inscriber"@en ;
	reg:status status:1001 ;
	a rdf:Property ;
	rdfs:domain <http://rdaregistry.info/Elements/c/C10003> ;
	rdfs:isDefinedBy <http://rdaregistry.info/Elements/i/> ;
	rdfs:label "has inscriber"@en ;
	rdfs:range <http://rdaregistry.info/Elements/c/C10004> ;
	rdfs:subPropertyOf <http://rdaregistry.info/Elements/i/P40023> , <http://rdaregistry.info/Elements/u/P60460> ;
	owl:inverseOf <http://rdaregistry.info/Elements/a/P50125> ;
	owl:sameAs <http://rdaregistry.info/Elements/i/inscriber> ;
	skos:definition "Relates an item to a person who has written a statement of dedication or gift on an item."@en .

<http://rdaregistry.info/Elements/i/P40015> reg:name "annotator"@en ;
	reg:status status:1001 ;
	a rdf:Property ;
	rdfs:domain <http://rdaregistry.info/Elements/c/C10003> ;
	rdfs:isDefinedBy <http://rdaregistry.info/Elements/i/> ;
	rdfs:label "has annotator"@en ;
	rdfs:range <http://rdaregistry.info/Elements/c/C10004> ;
	rdfs:subPropertyOf <http://rdaregistry.info/Elements/i/P40023> , <http://rdaregistry.info/Elements/u/P60464> ;
	owl:inverseOf <http://rdaregistry.info/Elements/a/P50128> ;
	owl:sameAs <http://rdaregistry.info/Elements/i/annotator> ;
	skos:definition "Relates an item to a person who makes manuscript annotations on an item."@en .

<http://rdaregistry.info/Elements/i/P40016> reg:name "autographer"@en ;
	reg:status status:1001 ;
	a rdf:Property ;
	rdfs:domain <http://rdaregistry.info/Elements/c/C10003> ;
	rdfs:isDefinedBy <http://rdaregistry.info/Elements/i/> ;
	rdfs:label "has autographer"@en ;
	rdfs:range <http://rdaregistry.info/Elements/c/C10004> ;
	rdfs:subPropertyOf <http://rdaregistry.info/Elements/i/P40023> , <http://rdaregistry.info/Elements/u/P60466> ;
	owl:inverseOf <http://rdaregistry.info/Elements/a/P50129> ;
	owl:sameAs <http://rdaregistry.info/Elements/i/autographer> ;
	skos:definition "Relates an item to a person whose manuscript signature appears on an item."@en .

<http://rdaregistry.info/Elements/i/P40017> reg:hasSubproperty <http://rdaregistry.info/Elements/i/P40004> , <http://rdaregistry.info/Elements/i/P40005> ;
	reg:name "curator"@en ;
	reg:status status:1001 ;
	a rdf:Property ;
	rdfs:domain <http://rdaregistry.info/Elements/c/C10003> ;
	rdfs:isDefinedBy <http://rdaregistry.info/Elements/i/> ;
	rdfs:label "has curator"@en ;
	rdfs:range <http://rdaregistry.info/Elements/c/C10002> ;
	rdfs:subPropertyOf <http://rdaregistry.info/Elements/i/P40023> , <http://rdaregistry.info/Elements/u/P60376> ;
	owl:inverseOf <http://rdaregistry.info/Elements/a/P50133> ;
	owl:sameAs <http://rdaregistry.info/Elements/i/curator> ;
	skos:definition "Relates an item to a person, family, or corporate body conceiving, aggregating, and/or organizing an exhibition, collection, or other item."@en .

<http://rdaregistry.info/Elements/i/P40018> reg:hasSubproperty <http://rdaregistry.info/Elements/i/P40006> ;
	reg:name "currentOwner"@en ;
	reg:status status:1001 ;
	a rdf:Property ;
	rdfs:domain <http://rdaregistry.info/Elements/c/C10003> ;
	rdfs:isDefinedBy <http://rdaregistry.info/Elements/i/> ;
	rdfs:label "has current owner"@en ;
	rdfs:range <http://rdaregistry.info/Elements/c/C10002> ;
	rdfs:subPropertyOf <http://rdaregistry.info/Elements/i/P40021> , <http://rdaregistry.info/Elements/u/P60400> ;
	owl:inverseOf <http://rdaregistry.info/Elements/a/P50162> ;
	owl:sameAs <http://rdaregistry.info/Elements/i/currentOwner> ;
	skos:definition "Relates an item to a person, family, or corporate body currently having legal possession of an item."@en .

<http://rdaregistry.info/Elements/i/P40019> reg:hasSubproperty <http://rdaregistry.info/Elements/i/P40007> , <http://rdaregistry.info/Elements/i/P40008> ;
	reg:name "formerOwner"@en ;
	reg:status status:1001 ;
	a rdf:Property ;
	rdfs:domain <http://rdaregistry.info/Elements/c/C10003> ;
	rdfs:isDefinedBy <http://rdaregistry.info/Elements/i/> ;
	rdfs:label "has former owner"@en ;
	rdfs:range <http://rdaregistry.info/Elements/c/C10002> ;
	rdfs:subPropertyOf <http://rdaregistry.info/Elements/i/P40021> , <http://rdaregistry.info/Elements/u/P60401> ;
	owl:inverseOf <http://rdaregistry.info/Elements/a/P50163> ;
	owl:sameAs <http://rdaregistry.info/Elements/i/formerOwner> ;
	skos:definition "Relates an item to a person, family, or corporate body formerly having legal possession of an item."@en .

<http://rdaregistry.info/Elements/i/P40020> reg:name "custodian"@en ;
	reg:status status:1001 ;
	a rdf:Property ;
	rdfs:domain <http://rdaregistry.info/Elements/c/C10003> ;
	rdfs:isDefinedBy <http://rdaregistry.info/Elements/i/> ;
	rdfs:label "has custodian"@en ;
	rdfs:range <http://rdaregistry.info/Elements/c/C10002> ;
	rdfs:subPropertyOf <http://rdaregistry.info/Elements/u/P60402> ;
	owl:inverseOf <http://rdaregistry.info/Elements/a/P50164> ;
	owl:sameAs <http://rdaregistry.info/Elements/i/custodian> ;
	skos:definition "Relates an item to a person, family, or corporate body having legal custody of an item."@en .

<http://rdaregistry.info/Elements/i/P40021> reg:hasSubproperty <http://rdaregistry.info/Elements/i/P40018> , <http://rdaregistry.info/Elements/i/P40019> ;
	reg:name "owner"@en ;
	reg:status status:1001 ;
	a rdf:Property ;
	rdfs:domain <http://rdaregistry.info/Elements/c/C10003> ;
	rdfs:isDefinedBy <http://rdaregistry.info/Elements/i/> ;
	rdfs:label "has owner"@en ;
	rdfs:range <http://rdaregistry.info/Elements/c/C10002> ;
	rdfs:subPropertyOf <http://rdaregistry.info/Elements/u/P60404> ;
	owl:inverseOf <http://rdaregistry.info/Elements/a/P50165> ;
	owl:sameAs <http://rdaregistry.info/Elements/i/owner> ;
	skos:definition "Relates an item to a person, family, or corporate body having legal possession of an item."@en .

<http://rdaregistry.info/Elements/i/P40022> reg:name "honoureeOfItem"@en ;
	reg:status status:1001 ;
	a rdf:Property ;
	rdfs:domain <http://rdaregistry.info/Elements/c/C10003> ;
	rdfs:isDefinedBy <http://rdaregistry.info/Elements/i/> ;
	rdfs:label "has honouree (item)"@en ;
	rdfs:range <http://rdaregistry.info/Elements/c/C10002> ;
	rdfs:subPropertyOf <http://rdaregistry.info/Elements/i/P40023> , <http://rdaregistry.info/Elements/u/P60406> ;
	owl:inverseOf <http://rdaregistry.info/Elements/a/P50167> ;
	owl:sameAs <http://rdaregistry.info/Elements/i/honoureeOfItem> ;
	skos:definition "Relates an item to a person, family, or corporate body honoured by an item, e.g., a person to whom a copy is presented."@en .

<http://rdaregistry.info/Elements/i/P40023> reg:hasSubproperty <http://rdaregistry.info/Elements/i/P40012> , <http://rdaregistry.info/Elements/i/P40013> , <http://rdaregistry.info/Elements/i/P40014> , <http://rdaregistry.info/Elements/i/P40015> , <http://rdaregistry.info/Elements/i/P40016> , <http://rdaregistry.info/Elements/i/P40017> , <http://rdaregistry.info/Elements/i/P40022> , <http://rdaregistry.info/Elements/i/P40024> , <http://rdaregistry.info/Elements/i/P40025> ;
	reg:name "otherPFCItem"@en ;
	reg:status status:1001 ;
	a rdf:Property ;
	rdfs:domain <http://rdaregistry.info/Elements/c/C10003> ;
	rdfs:isDefinedBy <http://rdaregistry.info/Elements/i/> ;
	rdfs:label "has other person, family, or corporate body associated with an item"@en ;
	rdfs:range <http://rdaregistry.info/Elements/c/C10002> ;
	rdfs:subPropertyOf <http://rdaregistry.info/Elements/u/P60374> ;
	owl:inverseOf <http://rdaregistry.info/Elements/a/P50182> ;
	owl:sameAs <http://rdaregistry.info/Elements/i/otherPFCItem> ;
	skos:definition "Relates an item to a person, family, or corporate body other than an owner or custodian associated with an item."@en ;
	skos:scopeNote "Includes curators, binders, restorationists, etc."@en .

<http://rdaregistry.info/Elements/i/P40024> reg:name "restorationist"@en ;
	reg:status status:1001 ;
	a rdf:Property ;
	rdfs:domain <http://rdaregistry.info/Elements/c/C10003> ;
	rdfs:isDefinedBy <http://rdaregistry.info/Elements/i/> ;
	rdfs:label "has restorationist"@en ;
	rdfs:range <http://rdaregistry.info/Elements/c/C10002> ;
	rdfs:subPropertyOf <http://rdaregistry.info/Elements/i/P40023> , <http://rdaregistry.info/Elements/u/P60450> ;
	owl:inverseOf <http://rdaregistry.info/Elements/a/P50206> ;
	owl:sameAs <http://rdaregistry.info/Elements/i/restorationist> ;
	skos:definition "Relates an item to a person, family, or corporate body responsible for the set of technical, editorial, and intellectual procedures aimed at compensating for the degradation of an item by bringing it back to a state as close as possible to its original condition."@en .

<http://rdaregistry.info/Elements/i/P40025> reg:name "dedicateeOfItem"@en ;
	reg:status status:1001 ;
	a rdf:Property ;
	rdfs:domain <http://rdaregistry.info/Elements/c/C10003> ;
	rdfs:isDefinedBy <http://rdaregistry.info/Elements/i/> ;
	rdfs:label "has dedicatee (item)"@en ;
	rdfs:range <http://rdaregistry.info/Elements/c/C10002> ;
	rdfs:subPropertyOf <http://rdaregistry.info/Elements/i/P40023> , <http://rdaregistry.info/Elements/u/P60455> ;
	owl:inverseOf <http://rdaregistry.info/Elements/a/P50210> ;
	owl:sameAs <http://rdaregistry.info/Elements/i/dedicateeOfItem> ;
	skos:definition "Relates an item to a person, family, or corporate body to whom an item is dedicated."@en .

<http://rdaregistry.info/Elements/i/P40026> reg:name "custodialHistoryOfItem"@en ;
	reg:status status:1001 ;
	a rdf:Property ;
	rdfs:domain <http://rdaregistry.info/Elements/c/C10003> ;
	rdfs:isDefinedBy <http://rdaregistry.info/Elements/i/> ;
	rdfs:label "has custodial history of item"@en ;
	rdfs:subPropertyOf <http://rdaregistry.info/Elements/u/P60176> ;
	owl:sameAs <http://rdaregistry.info/Elements/i/custodialHistoryOfItem> ;
	skos:definition "Relates an item to a record of previous ownership or custodianship of an item."@en .

<http://rdaregistry.info/Elements/i/P40027> reg:name "electronicReproductionOfItem"@en ;
	reg:status status:1001 ;
	a rdf:Property ;
	rdfs:domain <http://rdaregistry.info/Elements/c/C10003> ;
	rdfs:isDefinedBy <http://rdaregistry.info/Elements/i/> ;
	rdfs:label "is electronic reproduction of (item)"@en ;
	rdfs:range <http://rdaregistry.info/Elements/c/C10003> ;
	rdfs:subPropertyOf <http://rdaregistry.info/Elements/i/P40042> , <http://rdaregistry.info/Elements/u/P60469> ;
	owl:sameAs <http://rdaregistry.info/Elements/i/electronicReproductionOfItem> ;
	skos:definition "Relates an item to an analog item used as the basis for an electronic reproduction."@en .

<http://rdaregistry.info/Elements/i/P40028> reg:name "noteOnItem"@en ;
	reg:status status:1001 ;
	a rdf:Property ;
	rdfs:domain <http://rdaregistry.info/Elements/c/C10003> ;
	rdfs:isDefinedBy <http://rdaregistry.info/Elements/i/> ;
	rdfs:label "has note on item"@en ;
	rdfs:subPropertyOf <http://rdaregistry.info/Elements/u/P60470> ;
	owl:sameAs <http://rdaregistry.info/Elements/i/noteOnItem> , <http://rdaregistry.info/Elements/i/noteOnManifestationOrItem> ;
	skos:definition "Relates an item to an annotation providing additional information about item attributes"@en .

<http://rdaregistry.info/Elements/i/P40029> reg:hasSubproperty <http://rdaregistry.info/Elements/i/P40032> , <http://rdaregistry.info/Elements/i/P40035> , <http://rdaregistry.info/Elements/i/P40036> ;
	reg:name "accompaniedByItem"@en ;
	reg:status status:1001 ;
	a rdf:Property ;
	rdfs:domain <http://rdaregistry.info/Elements/c/C10003> ;
	rdfs:isDefinedBy <http://rdaregistry.info/Elements/i/> ;
	rdfs:label "is accompanied by (item)"@en ;
	rdfs:range <http://rdaregistry.info/Elements/c/C10003> ;
	rdfs:subPropertyOf <http://rdaregistry.info/Elements/i/P40051> , <http://rdaregistry.info/Elements/u/P60196> ;
	owl:inverseOf <http://rdaregistry.info/Elements/i/P40029> ;
	owl:sameAs <http://rdaregistry.info/Elements/i/accompaniedByItem> ;
	skos:definition "Relates an item to an item brought together with another item after being issued."@en .

<http://rdaregistry.info/Elements/i/P40030> reg:hasSubproperty <http://rdaregistry.info/Elements/i/P40033> , <http://rdaregistry.info/Elements/i/P40037> , <http://rdaregistry.info/Elements/i/P40040> , <http://rdaregistry.info/Elements/i/P40041> , <http://rdaregistry.info/Elements/i/P40043> ;
	reg:name "descriptionOfItem"@en ;
	reg:status status:1001 ;
	a rdf:Property ;
	rdfs:domain <http://rdaregistry.info/Elements/c/C10003> ;
	rdfs:isDefinedBy <http://rdaregistry.info/Elements/i/> ;
	rdfs:label "is description of (item)"@en ;
	rdfs:range <http://rdaregistry.info/Elements/c/C10003> ;
	rdfs:subPropertyOf <http://rdaregistry.info/Elements/i/P40052> , <http://rdaregistry.info/Elements/u/P60190> ;
	owl:sameAs <http://rdaregistry.info/Elements/i/descriptionOfItem> ;
	skos:definition "Relates an item to an item described by a describing work."@en .

<http://rdaregistry.info/Elements/i/P40031> reg:hasSubproperty <http://rdaregistry.info/Elements/i/P40042> ;
	reg:name "equivalentItem"@en ;
	reg:status status:1001 ;
	a rdf:Property ;
	rdfs:domain <http://rdaregistry.info/Elements/c/C10003> ;
	rdfs:isDefinedBy <http://rdaregistry.info/Elements/i/> ;
	rdfs:label "is equivalent (item)"@en ;
	rdfs:range <http://rdaregistry.info/Elements/c/C10003> ;
	rdfs:subPropertyOf <http://rdaregistry.info/Elements/i/P40053> , <http://rdaregistry.info/Elements/u/P60191> ;
	owl:inverseOf <http://rdaregistry.info/Elements/i/P40031> ;
	owl:sameAs <http://rdaregistry.info/Elements/i/equivalentItem> ;
	skos:definition "Relates an item to an item embodying the same expression of a work."@en .

<http://rdaregistry.info/Elements/i/P40032> reg:name "boundWith"@en ;
	reg:status status:1001 ;
	a rdf:Property ;
	rdfs:domain <http://rdaregistry.info/Elements/c/C10003> ;
	rdfs:isDefinedBy <http://rdaregistry.info/Elements/i/> ;
	rdfs:label "is bound with"@en ;
	rdfs:range <http://rdaregistry.info/Elements/c/C10003> ;
	rdfs:subPropertyOf <http://rdaregistry.info/Elements/i/P40029> , <http://rdaregistry.info/Elements/u/P60237> ;
	owl:inverseOf <http://rdaregistry.info/Elements/i/P40032> ;
	owl:sameAs <http://rdaregistry.info/Elements/i/boundWith> ;
	skos:definition "Relates an item to an item that has been bound within the same binding as the item being described."@en .

<http://rdaregistry.info/Elements/i/P40033> reg:name "analysisOfItem"@en ;
	reg:status status:1001 ;
	a rdf:Property ;
	rdfs:domain <http://rdaregistry.info/Elements/c/C10003> ;
	rdfs:isDefinedBy <http://rdaregistry.info/Elements/i/> ;
	rdfs:label "is analysis of (item)"@en ;
	rdfs:range <http://rdaregistry.info/Elements/c/C10003> ;
	rdfs:subPropertyOf <http://rdaregistry.info/Elements/i/P40030> , <http://rdaregistry.info/Elements/u/P60239> ;
	owl:sameAs <http://rdaregistry.info/Elements/i/analysisOfItem> ;
	skos:definition "Relates an item to an item that has been examined to identify its components and their relations."@en .

<http://rdaregistry.info/Elements/i/P40034> reg:name "containerOfItem"@en ;
	reg:status status:1001 ;
	a rdf:Property ;
	rdfs:domain <http://rdaregistry.info/Elements/c/C10003> ;
	rdfs:isDefinedBy <http://rdaregistry.info/Elements/i/> ;
	rdfs:label "is container of (item)"@en ;
	rdfs:range <http://rdaregistry.info/Elements/c/C10003> ;
	rdfs:subPropertyOf <http://rdaregistry.info/Elements/i/P40054> , <http://rdaregistry.info/Elements/u/P60249> ;
	owl:inverseOf <http://rdaregistry.info/Elements/i/P40009> ;
	owl:sameAs <http://rdaregistry.info/Elements/i/containerOfItem> , <http://rdaregistry.info/Elements/i/containsItem> ;
	skos:definition "Relates an item to an item that is a discrete component of a larger item."@en .

<http://rdaregistry.info/Elements/i/P40035> reg:name "onDiscWithItem"@en ;
	reg:status status:1001 ;
	a rdf:Property ;
	rdfs:domain <http://rdaregistry.info/Elements/c/C10003> ;
	rdfs:isDefinedBy <http://rdaregistry.info/Elements/i/> ;
	rdfs:label "is on disc with (item)"@en ;
	rdfs:range <http://rdaregistry.info/Elements/c/C10003> ;
	rdfs:subPropertyOf <http://rdaregistry.info/Elements/i/P40029> , <http://rdaregistry.info/Elements/u/P60257> ;
	owl:inverseOf <http://rdaregistry.info/Elements/i/P40035> ;
	owl:sameAs <http://rdaregistry.info/Elements/i/onDiscWithItem> ;
	skos:definition "Relates an item to an item that is contained on the same disc with the item being described."@en .

<http://rdaregistry.info/Elements/i/P40036> reg:name "filmedWithItem"@en ;
	reg:status status:1001 ;
	a rdf:Property ;
	rdfs:domain <http://rdaregistry.info/Elements/c/C10003> ;
	rdfs:isDefinedBy <http://rdaregistry.info/Elements/i/> ;
	rdfs:label "is filmed with (item)"@en ;
	rdfs:range <http://rdaregistry.info/Elements/c/C10003> ;
	rdfs:subPropertyOf <http://rdaregistry.info/Elements/i/P40029> , <http://rdaregistry.info/Elements/u/P60258> ;
	owl:inverseOf <http://rdaregistry.info/Elements/i/P40036> ;
	owl:sameAs <http://rdaregistry.info/Elements/i/filmedWithItem> ;
	skos:definition "Relates an item to an item that is contained on the same microform with the item being described."@en .

<http://rdaregistry.info/Elements/i/P40037> reg:name "evaluationOfItem"@en ;
	reg:status status:1001 ;
	a rdf:Property ;
	rdfs:domain <http://rdaregistry.info/Elements/c/C10003> ;
	rdfs:isDefinedBy <http://rdaregistry.info/Elements/i/> ;
	rdfs:label "is evaluation of (item)"@en ;
	rdfs:range <http://rdaregistry.info/Elements/c/C10003> ;
	rdfs:subPropertyOf <http://rdaregistry.info/Elements/i/P40030> , <http://rdaregistry.info/Elements/u/P60255> ;
	owl:sameAs <http://rdaregistry.info/Elements/i/evaluationOfItem> ;
	skos:definition "Relates an item to an item that is examined or judged."@en .

<http://rdaregistry.info/Elements/i/P40038> reg:name "reprintOfItem"@en ;
	reg:status status:1001 ;
	a rdf:Property ;
	rdfs:domain <http://rdaregistry.info/Elements/c/C10003> ;
	rdfs:isDefinedBy <http://rdaregistry.info/Elements/i/> ;
	rdfs:label "is reprint of (item)"@en ;
	rdfs:range <http://rdaregistry.info/Elements/c/C10003> ;
	rdfs:subPropertyOf <http://rdaregistry.info/Elements/i/P40042> , <http://rdaregistry.info/Elements/u/P60168> ;
	owl:sameAs <http://rdaregistry.info/Elements/i/reprintOfItem> ;
	skos:definition "Relates an item to an item that is used as the basis for a reprint with the same content as the resource being described."@en .

<http://rdaregistry.info/Elements/i/P40039> reg:name "digitalTransferOfItem"@en ;
	reg:status status:1001 ;
	a rdf:Property ;
	rdfs:domain <http://rdaregistry.info/Elements/c/C10003> ;
	rdfs:isDefinedBy <http://rdaregistry.info/Elements/i/> ;
	rdfs:label "is digital transfer of (item)"@en ;
	rdfs:range <http://rdaregistry.info/Elements/c/C10003> ;
	rdfs:subPropertyOf <http://rdaregistry.info/Elements/i/P40042> , <http://rdaregistry.info/Elements/u/P60287> ;
	owl:sameAs <http://rdaregistry.info/Elements/i/digitalTransferOfItem> ;
	skos:definition "Relates an item to an item transferred from one digital format to another."@en .

<http://rdaregistry.info/Elements/i/P40040> reg:name "reviewOfItem"@en ;
	reg:status status:1001 ;
	a rdf:Property ;
	rdfs:domain <http://rdaregistry.info/Elements/c/C10003> ;
	rdfs:isDefinedBy <http://rdaregistry.info/Elements/i/> ;
	rdfs:label "is review of (item)"@en ;
	rdfs:range <http://rdaregistry.info/Elements/c/C10003> ;
	rdfs:subPropertyOf <http://rdaregistry.info/Elements/i/P40030> , <http://rdaregistry.info/Elements/u/P60288> ;
	owl:sameAs <http://rdaregistry.info/Elements/i/reviewOfItem> ;
	skos:definition "Relates an item to an item used as the basis for a brief evaluation."@en .

<http://rdaregistry.info/Elements/i/P40041> reg:name "critiqueOfItem"@en ;
	reg:status status:1001 ;
	a rdf:Property ;
	rdfs:domain <http://rdaregistry.info/Elements/c/C10003> ;
	rdfs:isDefinedBy <http://rdaregistry.info/Elements/i/> ;
	rdfs:label "is critique of (item)"@en ;
	rdfs:range <http://rdaregistry.info/Elements/c/C10003> ;
	rdfs:subPropertyOf <http://rdaregistry.info/Elements/i/P40030> , <http://rdaregistry.info/Elements/u/P60292> ;
	owl:sameAs <http://rdaregistry.info/Elements/i/critiqueOfItem> ;
	skos:definition "Relates an item to an item used as the basis for a critical evaluation."@en .

<http://rdaregistry.info/Elements/i/P40042> reg:hasSubproperty <http://rdaregistry.info/Elements/i/P40027> , <http://rdaregistry.info/Elements/i/P40038> , <http://rdaregistry.info/Elements/i/P40039> , <http://rdaregistry.info/Elements/i/P40045> ;
	reg:name "reproductionOfItem"@en ;
	reg:status status:1001 ;
	a rdf:Property ;
	rdfs:domain <http://rdaregistry.info/Elements/c/C10003> ;
	rdfs:isDefinedBy <http://rdaregistry.info/Elements/i/> ;
	rdfs:label "is reproduction of (item)"@en ;
	rdfs:range <http://rdaregistry.info/Elements/c/C10003> ;
	rdfs:subPropertyOf <http://rdaregistry.info/Elements/i/P40031> , <http://rdaregistry.info/Elements/u/P60297> ;
	owl:sameAs <http://rdaregistry.info/Elements/i/reproductionOfItem> ;
	skos:definition "Relates an item to an item used as the basis for a reproduction."@en .

<http://rdaregistry.info/Elements/i/P40043> reg:name "commentaryOnItem"@en ;
	reg:status status:1001 ;
	a rdf:Property ;
	rdfs:domain <http://rdaregistry.info/Elements/c/C10003> ;
	rdfs:isDefinedBy <http://rdaregistry.info/Elements/i/> ;
	rdfs:label "is commentary on (item)"@en ;
	rdfs:range <http://rdaregistry.info/Elements/c/C10003> ;
	rdfs:subPropertyOf <http://rdaregistry.info/Elements/i/P40030> , <http://rdaregistry.info/Elements/u/P60298> ;
	owl:sameAs <http://rdaregistry.info/Elements/i/commentaryOnItem> ;
	skos:definition "Relates an item to an item used as the basis for a set of explanatory or critical notes."@en .

<http://rdaregistry.info/Elements/i/P40044> reg:name "preservationFacsimileOfItem"@en ;
	reg:status status:1001 ;
	a rdf:Property ;
	rdfs:domain <http://rdaregistry.info/Elements/c/C10003> ;
	rdfs:isDefinedBy <http://rdaregistry.info/Elements/i/> ;
	rdfs:label "is preservation facsimile of (item)"@en ;
	rdfs:range <http://rdaregistry.info/Elements/c/C10003> ;
	rdfs:subPropertyOf <http://rdaregistry.info/Elements/i/P40045> , <http://rdaregistry.info/Elements/u/P60299> ;
	owl:sameAs <http://rdaregistry.info/Elements/i/preservationFacsimileOfItem> ;
	skos:definition "Relates an item to an item used as the basis for an exact reproduction on preservation-quality media, such as acid-free permanent or archival paper."@en .

<http://rdaregistry.info/Elements/i/P40045> reg:hasSubproperty <http://rdaregistry.info/Elements/i/P40044> ;
	reg:name "facsimileOfItem"@en ;
	reg:status status:1001 ;
	a rdf:Property ;
	rdfs:domain <http://rdaregistry.info/Elements/c/C10003> ;
	rdfs:isDefinedBy <http://rdaregistry.info/Elements/i/> ;
	rdfs:label "is facsimile of (item)"@en ;
	rdfs:range <http://rdaregistry.info/Elements/c/C10003> ;
	rdfs:subPropertyOf <http://rdaregistry.info/Elements/i/P40042> , <http://rdaregistry.info/Elements/u/P60301> ;
	owl:sameAs <http://rdaregistry.info/Elements/i/facsimileOfItem> ;
	skos:definition "Relates an item to an item used as the basis for an exact reproduction."@en .

<http://rdaregistry.info/Elements/i/P40046> reg:hasSubproperty <http://rdaregistry.info/Elements/i/P40052> , <http://rdaregistry.info/Elements/i/P40053> , <http://rdaregistry.info/Elements/i/P40054> ;
	reg:name "relatedItemOfItem"@en ;
	reg:status status:1001 ;
	a rdf:Property ;
	rdfs:domain <http://rdaregistry.info/Elements/c/C10003> ;
	rdfs:isDefinedBy <http://rdaregistry.info/Elements/i/> ;
	rdfs:label "has related item of item"@en ;
	rdfs:range <http://rdaregistry.info/Elements/c/C10003> ;
	owl:inverseOf <http://rdaregistry.info/Elements/i/P40046> ;
	owl:sameAs <http://rdaregistry.info/Elements/i/relatedItemOfItem> ;
	skos:definition "Relates an item to an item, represented by an identifier or a description, that is related to the item being described (e.g., an item used as the basis for a microform reproduction)."@en .

<http://rdaregistry.info/Elements/i/P40047> reg:name "restrictionsOnAccess"@en ;
	reg:status status:1001 ;
	a rdf:Property ;
	rdfs:domain <http://rdaregistry.info/Elements/c/C10003> ;
	rdfs:isDefinedBy <http://rdaregistry.info/Elements/i/> ;
	rdfs:label "has restrictions on access"@en ;
	rdfs:subPropertyOf <http://rdaregistry.info/Elements/u/P60496> ;
	owl:sameAs <http://rdaregistry.info/Elements/i/restrictionsOnAccess> ;
	skos:definition "Relates an item to limitations placed on access to a resource."@en .

<http://rdaregistry.info/Elements/i/P40048> reg:name "restrictionsOnUse"@en ;
	reg:status status:1001 ;
	a rdf:Property ;
	rdfs:domain <http://rdaregistry.info/Elements/c/C10003> ;
	rdfs:isDefinedBy <http://rdaregistry.info/Elements/i/> ;
	rdfs:label "has restrictions on use"@en ;
	rdfs:subPropertyOf <http://rdaregistry.info/Elements/u/P60497> ;
	owl:sameAs <http://rdaregistry.info/Elements/i/restrictionsOnUse> ;
	skos:definition "Relates an item to limitations placed on uses such as reproduction, publication, exhibition, etc."@en .

<http://rdaregistry.info/Elements/i/P40049> reg:name "manifestationExemplified"@en ;
	reg:status status:1001 ;
	a rdf:Property ;
	rdfs:domain <http://rdaregistry.info/Elements/c/C10003> ;
	rdfs:isDefinedBy <http://rdaregistry.info/Elements/i/> ;
	rdfs:label "has manifestation exemplified"@en ;
	rdfs:range <http://rdaregistry.info/Elements/c/C10007> ;
	owl:inverseOf <http://rdaregistry.info/Elements/m/P30103> ;
	owl:sameAs <http://rdaregistry.info/Elements/i/manifestationExemplified> ;
	skos:definition "Relates an item to the manifestation exemplified by an item."@en .

<http://rdaregistry.info/Elements/i/P40050> reg:name "immediateSourceOfAcquisitionOfItem"@en ;
	reg:status status:1001 ;
	a rdf:Property ;
	rdfs:domain <http://rdaregistry.info/Elements/c/C10003> ;
	rdfs:isDefinedBy <http://rdaregistry.info/Elements/i/> ;
	rdfs:label "has immediate source of acquisition of item"@en ;
	rdfs:subPropertyOf <http://rdaregistry.info/Elements/u/P60583> ;
	owl:sameAs <http://rdaregistry.info/Elements/i/immediateSourceOfAcquisitionOfItem> ;
	skos:definition "Relates an item to the source from which the agency directly acquired an item and the circumstances under which it was received."@en .

<http://rdaregistry.info/Elements/i/P40051> reg:hasSubproperty <http://rdaregistry.info/Elements/i/P40029> ;
	reg:name "accompanyingItemRelationship"@en ;
	reg:status status:1001 ;
	a rdf:Property ;
	rdfs:domain <http://rdaregistry.info/Elements/c/C10003> ;
	rdfs:isDefinedBy <http://rdaregistry.info/Elements/i/> ;
	rdfs:label "has accompanying item relationship with"@en ;
	rdfs:range <http://rdaregistry.info/Elements/c/C10003> ;
	rdfs:subPropertyOf <http://rdaregistry.info/Elements/u/P60709> ;
	owl:inverseOf <http://rdaregistry.info/Elements/i/P40051> ;
	owl:sameAs <http://rdaregistry.info/Elements/i/accompanyingItemRelationship> ;
	skos:definition "Relates an item to an item that accompanies or is accompanied by the item."@en .

<http://rdaregistry.info/Elements/i/P40052> reg:hasSubproperty <http://rdaregistry.info/Elements/i/P40030> ;
	reg:name "descriptiveItemRelationship"@en ;
	reg:status status:1001 ;
	a rdf:Property ;
	rdfs:domain <http://rdaregistry.info/Elements/c/C10003> ;
	rdfs:isDefinedBy <http://rdaregistry.info/Elements/i/> ;
	rdfs:label "has descriptive item relationship with"@en ;
	rdfs:range <http://rdaregistry.info/Elements/c/C10003> ;
	rdfs:subPropertyOf <http://rdaregistry.info/Elements/i/P40046> , <http://rdaregistry.info/Elements/u/P60711> ;
	owl:sameAs <http://rdaregistry.info/Elements/i/descriptiveItemRelationship> ;
	skos:definition "Relates an item to a work that is a description of the item."@en .

<http://rdaregistry.info/Elements/i/P40053> reg:hasSubproperty <http://rdaregistry.info/Elements/i/P40031> ;
	reg:name "equivalentItemRelationship"@en ;
	reg:status status:1001 ;
	a rdf:Property ;
	rdfs:domain <http://rdaregistry.info/Elements/c/C10003> ;
	rdfs:isDefinedBy <http://rdaregistry.info/Elements/i/> ;
	rdfs:label "has equivalent item relationship with"@en ;
	rdfs:range <http://rdaregistry.info/Elements/c/C10003> ;
	rdfs:subPropertyOf <http://rdaregistry.info/Elements/i/P40046> , <http://rdaregistry.info/Elements/u/P60712> ;
	owl:inverseOf <http://rdaregistry.info/Elements/i/P40053> ;
	owl:sameAs <http://rdaregistry.info/Elements/i/equivalentItemRelationship> ;
	skos:definition "Relates an item to an item that is equivalent to the item."@en .

<http://rdaregistry.info/Elements/i/P40054> reg:hasSubproperty <http://rdaregistry.info/Elements/i/P40009> , <http://rdaregistry.info/Elements/i/P40034> ;
	reg:name "wholePartItemRelationship"@en ;
	reg:status status:1001 ;
	a rdf:Property ;
	rdfs:domain <http://rdaregistry.info/Elements/c/C10003> ;
	rdfs:isDefinedBy <http://rdaregistry.info/Elements/i/> ;
	rdfs:label "has whole-part item relationship with"@en ;
	rdfs:range <http://rdaregistry.info/Elements/c/C10003> ;
	rdfs:subPropertyOf <http://rdaregistry.info/Elements/i/P40046> , <http://rdaregistry.info/Elements/u/P60714> ;
	owl:sameAs <http://rdaregistry.info/Elements/i/wholePartItemRelationship> ;
	skos:definition "Relates an item to an item that is contained in or contains the item."@en .
